@prefix cim    : <https://cim.ucaiug.io/ns#> .
@prefix nc     : <https://cim4.eu/ns/nc#> .
@prefix cims   : <http://iec.ch/TC57/1999/rdf-schema-extensions-19990926#> .
@prefix eu     : <https://cim.ucaiug.io/ns/eu#> .
@prefix profcim: <https://cim.ucaiug.io/ns/prof-cim#> .
@prefix er     : <https://ap-voc.cim4.eu/EquipmentReliability#> .
@prefix dcat   : <http://www.w3.org/ns/dcat#> .
@prefix dcterms: <http://purl.org/dc/terms/#> .
@prefix owl    : <http://www.w3.org/2002/07/owl#> .
@prefix rdf    : <http://www.w3.org/1999/02/22-rdf-syntax-ns#> .
@prefix rdfs   : <http://www.w3.org/2000/01/rdf-schema#> .

cim:ACDCConverter a rdfs:Class ;
  rdfs:label "ACDCConverter"@en ;
  rdfs:comment "A unit with valves for three phases, together with unit control equipment, essential protective and switching devices, DC storage capacitors, phase reactors and auxiliaries, if any, used for conversion." ;
  cims:belongsToCategory er:Package_EquipmentReliabilityProfile ;
  rdfs:subClassOf cim:ConductingEquipment .

cim:ACDCTerminal a rdfs:Class ;
  rdfs:label "ACDCTerminal"@en ;
  rdfs:comment "An electrical connection point (AC or DC) to a piece of conducting equipment. Terminals are connected at physical connection points called connectivity nodes." ;
  cims:belongsToCategory er:Package_EquipmentReliabilityProfile .

cim:ActivePower a rdfs:Class ;
  rdfs:label "ActivePower"@en ;
  rdfs:comment "Product of RMS value of the voltage and the RMS value of the in-phase component of the current." ;
  cims:belongsToCategory er:Package_EquipmentReliabilityProfile ;
  cims:stereotype "CIMDatatype" .

cim:ActivePowerChangeRate a rdfs:Class ;
  rdfs:label "ActivePowerChangeRate"@en ;
  rdfs:comment "Rate of change of active power per time." ;
  cims:belongsToCategory er:Package_EquipmentReliabilityProfile ;
  cims:stereotype "CIMDatatype" .

cim:AngleDegrees a rdfs:Class ;
  rdfs:label "AngleDegrees"@en ;
  rdfs:comment "Measurement of angle in degrees." ;
  cims:belongsToCategory er:Package_EquipmentReliabilityProfile ;
  cims:stereotype "CIMDatatype" .

cim:Boolean a rdfs:Class ;
  rdfs:label "Boolean"@en ;
  rdfs:comment "A type with the value space \"true\" and \"false\"." ;
  cims:belongsToCategory er:Package_EquipmentReliabilityProfile ;
  cims:stereotype "Primitive" .

cim:ConductingEquipment a rdfs:Class ;
  rdfs:label "ConductingEquipment"@en ;
  rdfs:comment "The parts of the AC power system that are designed to carry current or that are conductively connected through terminals." ;
  cims:belongsToCategory er:Package_EquipmentReliabilityProfile ;
  rdfs:subClassOf cim:Equipment .

cim:Conductor a rdfs:Class ;
  rdfs:label "Conductor"@en ;
  rdfs:comment "Combination of conducting material with consistent electrical characteristics, building a single electrical system, used to carry current between points in the power system.  " ;
  cims:belongsToCategory er:Package_EquipmentReliabilityProfile ;
  rdfs:subClassOf cim:ConductingEquipment .

cim:ConnectivityNode a rdfs:Class ;
  rdfs:label "ConnectivityNode"@en ;
  rdfs:comment "Connectivity nodes are points where terminals of AC conducting equipment are connected together with zero impedance." ;
  cims:belongsToCategory er:Package_EquipmentReliabilityProfile ;
  cims:stereotype <http://iec.ch/TC57/NonStandard/UML#concrete> ;
  rdfs:subClassOf cim:IdentifiedObject .

cim:ConnectivityNodeContainer a rdfs:Class ;
  rdfs:label "ConnectivityNodeContainer"@en ;
  rdfs:comment "A base class for all objects that may contain connectivity nodes or topological nodes." ;
  cims:belongsToCategory er:Package_EquipmentReliabilityProfile ;
  rdfs:subClassOf cim:PowerSystemResource .

cim:ControlArea a rdfs:Class ;
  rdfs:label "ControlArea"@en ;
  rdfs:comment """A control area is a grouping of generating units and/or loads and a cutset of tie lines (as terminals) which may be used for a variety of purposes including automatic generation control, power flow solution area interchange control specification, and input to load forecasting. All generation and load within the area defined by the terminals on the border are considered in the area interchange control. Note that any number of overlapping control area specifications can be superimposed on the physical model. The following general principles apply to ControlArea:
1.  The control area orientation for net interchange is positive for an import, negative for an export.
2.  The control area net interchange is determined by summing flows in Terminals. The Terminals are identified by creating a set of TieFlow objects associated with a ControlArea object. Each TieFlow object identifies one Terminal.
3.  In a single network model, a tie between two control areas must be modelled in both control area specifications, such that the two representations of the tie flow sum to zero.
4.  The normal orientation of Terminal flow is positive for flow into the conducting equipment that owns the Terminal. (i.e. flow from a bus into a device is positive.) However, the orientation of each flow in the control area specification must align with the control area convention, i.e. import is positive. If the orientation of the Terminal flow referenced by a TieFlow is positive into the control area, then this is confirmed by setting TieFlow.positiveFlowIn flag TRUE. If not, the orientation must be reversed by setting the TieFlow.positiveFlowIn flag FALSE.""" ;
  cims:belongsToCategory er:Package_EquipmentReliabilityProfile ;
  cims:stereotype "Description", <http://iec.ch/TC57/NonStandard/UML#concrete> ;
  rdfs:subClassOf cim:PowerSystemResource .

cim:Currency a rdfs:Class ;
  rdfs:label "Currency"@en ;
  rdfs:comment "Monetary currencies.  ISO 4217 standard including 3-character currency code." ;
  cims:belongsToCategory er:Package_EquipmentReliabilityProfile ;
  cims:stereotype <http://iec.ch/TC57/NonStandard/UML#enumeration> .

cim:CurrentFlow a rdfs:Class ;
  rdfs:label "CurrentFlow"@en ;
  rdfs:comment "Electrical current with sign convention: positive flow is out of the conducting equipment into the connectivity node. Can be both AC and DC." ;
  cims:belongsToCategory er:Package_EquipmentReliabilityProfile ;
  cims:stereotype "CIMDatatype" .

cim:Curve a rdfs:Class ;
  rdfs:label "Curve"@en ;
  rdfs:comment "A multi-purpose curve or functional relationship between an independent variable (X-axis) and dependent (Y-axis) variables. " ;
  cims:belongsToCategory er:Package_EquipmentReliabilityProfile ;
  rdfs:subClassOf cim:IdentifiedObject .

cim:CurveData a rdfs:Class ;
  rdfs:label "CurveData"@en ;
  rdfs:comment "Multi-purpose data points for defining a curve.  The use of this generic class is discouraged if a more specific class can be used to specify the X and Y axis values along with their specific data types." ;
  cims:belongsToCategory er:Package_EquipmentReliabilityProfile ;
  cims:stereotype <http://iec.ch/TC57/NonStandard/UML#concrete> .

cim:CurveStyle a rdfs:Class ;
  rdfs:label "CurveStyle"@en ;
  rdfs:comment "Style or shape of curve." ;
  cims:belongsToCategory er:Package_EquipmentReliabilityProfile ;
  cims:stereotype <http://iec.ch/TC57/NonStandard/UML#enumeration> .

cim:DCBreaker a rdfs:Class ;
  rdfs:label "DCBreaker"@en ;
  rdfs:comment "A breaker within a DC system. " ;
  cims:belongsToCategory er:Package_EquipmentReliabilityProfile ;
  cims:stereotype "Description", <http://iec.ch/TC57/NonStandard/UML#concrete> ;
  rdfs:subClassOf cim:DCSwitch .

cim:DCBusbar a rdfs:Class ;
  rdfs:label "DCBusbar"@en ;
  rdfs:comment "A busbar within a DC system." ;
  cims:belongsToCategory er:Package_EquipmentReliabilityProfile ;
  cims:stereotype "Description", <http://iec.ch/TC57/NonStandard/UML#concrete> ;
  rdfs:subClassOf cim:DCConductingEquipment .

cim:DCChopper a rdfs:Class ;
  rdfs:label "DCChopper"@en ;
  rdfs:comment "Low resistance equipment used in the internal DC circuit to balance voltages. It has typically positive and negative pole terminals and a ground." ;
  cims:belongsToCategory er:Package_EquipmentReliabilityProfile ;
  cims:stereotype "Description", <http://iec.ch/TC57/NonStandard/UML#concrete> ;
  rdfs:subClassOf cim:DCConductingEquipment .

cim:DCConductingEquipment a rdfs:Class ;
  rdfs:label "DCConductingEquipment"@en ;
  rdfs:comment "The parts of the DC power system that are designed to carry current or that are conductively connected through DC terminals." ;
  cims:belongsToCategory er:Package_EquipmentReliabilityProfile ;
  rdfs:subClassOf cim:Equipment .

cim:DCConverterUnit a rdfs:Class ;
  rdfs:label "DCConverterUnit"@en ;
  rdfs:comment "Indivisible operative unit comprising all equipment between the point of common coupling on the AC side and the point of common coupling – DC side, essentially one or more converters, together with one or more converter transformers, converter control equipment, essential protective and switching devices and auxiliaries, if any, used for conversion." ;
  cims:belongsToCategory er:Package_EquipmentReliabilityProfile ;
  cims:stereotype "Description", <http://iec.ch/TC57/NonStandard/UML#concrete> ;
  rdfs:subClassOf cim:DCEquipmentContainer .

cim:DCDisconnector a rdfs:Class ;
  rdfs:label "DCDisconnector"@en ;
  rdfs:comment "A disconnector within a DC system." ;
  cims:belongsToCategory er:Package_EquipmentReliabilityProfile ;
  cims:stereotype "Description", <http://iec.ch/TC57/NonStandard/UML#concrete> ;
  rdfs:subClassOf cim:DCSwitch .

cim:DCEquipmentContainer a rdfs:Class ;
  rdfs:label "DCEquipmentContainer"@en ;
  rdfs:comment "A modelling construct to provide a root class for containment of DC as well as AC equipment. The class differ from the EquipmentContaner for AC in that it may also contain DCNode-s. Hence it can contain both AC and DC equipment." ;
  cims:belongsToCategory er:Package_EquipmentReliabilityProfile ;
  rdfs:subClassOf cim:EquipmentContainer .

cim:DCGround a rdfs:Class ;
  rdfs:label "DCGround"@en ;
  rdfs:comment "A ground within a DC system." ;
  cims:belongsToCategory er:Package_EquipmentReliabilityProfile ;
  cims:stereotype "Description", <http://iec.ch/TC57/NonStandard/UML#concrete> ;
  rdfs:subClassOf cim:DCConductingEquipment .

cim:DCLine a rdfs:Class ;
  rdfs:label "DCLine"@en ;
  rdfs:comment "Overhead lines and/or cables connecting two or more HVDC substations." ;
  cims:belongsToCategory er:Package_EquipmentReliabilityProfile ;
  cims:stereotype "Description", <http://iec.ch/TC57/NonStandard/UML#concrete> .

cim:DCLineSegment a rdfs:Class ;
  rdfs:label "DCLineSegment"@en ;
  rdfs:comment "A wire or combination of wires not insulated from one another, with consistent electrical characteristics, used to carry direct current between points in the DC region of the power system." ;
  cims:belongsToCategory er:Package_EquipmentReliabilityProfile ;
  cims:stereotype "Description", <http://iec.ch/TC57/NonStandard/UML#concrete> ;
  rdfs:subClassOf cim:DCConductingEquipment .

cim:DCNode a rdfs:Class ;
  rdfs:label "DCNode"@en ;
  rdfs:comment "DC nodes are points where terminals of DC conducting equipment are connected together with zero impedance." ;
  cims:belongsToCategory er:Package_EquipmentReliabilityProfile ;
  cims:stereotype <http://iec.ch/TC57/NonStandard/UML#concrete> ;
  rdfs:subClassOf cim:IdentifiedObject .

cim:DCSeriesDevice a rdfs:Class ;
  rdfs:label "DCSeriesDevice"@en ;
  rdfs:comment "A series device within the DC system, typically a reactor used for filtering or smoothing.  Needed for transient and short circuit studies." ;
  cims:belongsToCategory er:Package_EquipmentReliabilityProfile ;
  cims:stereotype "Description", <http://iec.ch/TC57/NonStandard/UML#concrete> ;
  rdfs:subClassOf cim:DCConductingEquipment .

cim:DCShunt a rdfs:Class ;
  rdfs:label "DCShunt"@en ;
  rdfs:comment "A shunt device within the DC system, typically used for filtering.  Needed for transient and short circuit studies." ;
  cims:belongsToCategory er:Package_EquipmentReliabilityProfile ;
  cims:stereotype "Description", <http://iec.ch/TC57/NonStandard/UML#concrete> ;
  rdfs:subClassOf cim:DCConductingEquipment .

cim:DCSwitch a rdfs:Class ;
  rdfs:label "DCSwitch"@en ;
  rdfs:comment "A switch within the DC system." ;
  cims:belongsToCategory er:Package_EquipmentReliabilityProfile ;
  cims:stereotype "Description", <http://iec.ch/TC57/NonStandard/UML#concrete> ;
  rdfs:subClassOf cim:DCConductingEquipment .

cim:Date a rdfs:Class ;
  rdfs:label "Date"@en ;
  rdfs:comment "Date as \"yyyy-mm-dd\", which conforms with ISO 8601. UTC time zone is specified as \"yyyy-mm-ddZ\". A local timezone relative UTC is specified as \"yyyy-mm-dd(+/-)hh:mm\"." ;
  cims:belongsToCategory er:Package_DocEquipmentReliabilityProfile ;
  cims:stereotype "Primitive" .

cim:DateTime a rdfs:Class ;
  rdfs:label "DateTime"@en ;
  rdfs:comment "Date and time as \"yyyy-mm-ddThh:mm:ss.sss\", which conforms with ISO 8601. UTC time zone is specified as \"yyyy-mm-ddThh:mm:ss.sssZ\". A local timezone relative UTC is specified as \"yyyy-mm-ddThh:mm:ss.sss-hh:mm\". The second component (shown here as \"ss.sss\") could have any number of digits in its fractional part to allow any kind of precision beyond seconds." ;
  cims:belongsToCategory er:Package_DocEquipmentReliabilityProfile ;
  cims:stereotype "Primitive" .

cim:Decimal a rdfs:Class ;
  rdfs:label "Decimal"@en ;
  rdfs:comment "Decimal is the base-10 notational system for representing real numbers." ;
  cims:belongsToCategory er:Package_EquipmentReliabilityProfile ;
  cims:stereotype "Primitive" .

cim:Duration a rdfs:Class ;
  rdfs:label "Duration"@en ;
  rdfs:comment "Duration as \"PnYnMnDTnHnMnS\" which conforms to ISO 8601, where nY expresses a number of years, nM a number of months, nD a number of days. The letter T separates the date expression from the time expression and, after it, nH identifies a number of hours, nM a number of minutes and nS a number of seconds. The number of seconds could be expressed as a decimal number, but all other numbers are integers." ;
  cims:belongsToCategory er:Package_EquipmentReliabilityProfile ;
  cims:stereotype "Primitive" .

cim:EnergyConnection a rdfs:Class ;
  rdfs:label "EnergyConnection"@en ;
  rdfs:comment "A connection of energy generation or consumption on the power system model." ;
  cims:belongsToCategory er:Package_EquipmentReliabilityProfile ;
  rdfs:subClassOf cim:ConductingEquipment .

cim:EnergyConsumer a rdfs:Class ;
  rdfs:label "EnergyConsumer"@en ;
  rdfs:comment """Generic user of energy - a  point of consumption on the power system model.
EnergyConsumer.pfixed, .qfixed, .pfixedPct and .qfixedPct have meaning only if there is no LoadResponseCharacteristic associated with EnergyConsumer or if LoadResponseCharacteristic.exponentModel is set to False.""" ;
  cims:belongsToCategory er:Package_EquipmentReliabilityProfile ;
  cims:stereotype "Description", <http://iec.ch/TC57/NonStandard/UML#concrete> ;
  rdfs:subClassOf cim:EnergyConnection .

cim:Equipment a rdfs:Class ;
  rdfs:label "Equipment"@en ;
  rdfs:comment "The parts of a power system that are physical devices, electronic or mechanical." ;
  cims:belongsToCategory er:Package_EquipmentReliabilityProfile ;
  cims:stereotype "Description" ;
  rdfs:subClassOf cim:PowerSystemResource .

cim:EquipmentContainer a rdfs:Class ;
  rdfs:label "EquipmentContainer"@en ;
  rdfs:comment "A modelling construct to provide a root class for containing equipment. " ;
  cims:belongsToCategory er:Package_EquipmentReliabilityProfile ;
  rdfs:subClassOf cim:ConnectivityNodeContainer .

cim:EquivalentInjection a rdfs:Class ;
  rdfs:label "EquivalentInjection"@en ;
  rdfs:comment "This class represents equivalent injections (generation or load).  Voltage regulation is allowed only at the point of connection." ;
  cims:belongsToCategory er:Package_EquipmentReliabilityProfile ;
  cims:stereotype "Description", <http://iec.ch/TC57/NonStandard/UML#concrete> .

cim:Feeder a rdfs:Class ;
  rdfs:label "Feeder"@en ;
  rdfs:comment """A collection of equipment for organizational purposes, used for grouping distribution resources.
The organization a feeder does not necessarily reflect connectivity or current operation state.""" ;
  cims:belongsToCategory er:Package_EquipmentReliabilityProfile ;
  cims:stereotype <http://iec.ch/TC57/NonStandard/UML#concrete> ;
  rdfs:subClassOf cim:EquipmentContainer .

cim:Float a rdfs:Class ;
  rdfs:label "Float"@en ;
  rdfs:comment "A floating point number. The range is unspecified and not limited." ;
  cims:belongsToCategory er:Package_EquipmentReliabilityProfile ;
  cims:stereotype "Primitive" .

cim:FossilFuel a rdfs:Class ;
  rdfs:label "FossilFuel"@en ;
  rdfs:comment "The fossil fuel consumed by the non-nuclear thermal generating unit.   For example, coal, oil, gas, etc.   These are the specific fuels that the generating unit can consume." ;
  cims:belongsToCategory er:Package_EquipmentReliabilityProfile ;
  cims:stereotype "Description", <http://iec.ch/TC57/NonStandard/UML#concrete> .

cim:Frequency a rdfs:Class ;
  rdfs:label "Frequency"@en ;
  rdfs:comment "Cycles per second." ;
  cims:belongsToCategory er:Package_EquipmentReliabilityProfile ;
  cims:stereotype "CIMDatatype" .

cim:GeneratingUnit a rdfs:Class ;
  rdfs:label "GeneratingUnit"@en ;
  rdfs:comment "A single or set of synchronous machines for converting mechanical power into alternating-current power. For example, individual machines within a set may be defined for scheduling purposes while a single control signal is derived for the set. In this case there would be a GeneratingUnit for each member of the set and an additional GeneratingUnit corresponding to the set." ;
  cims:belongsToCategory er:Package_EquipmentReliabilityProfile ;
  cims:stereotype "Description", <http://iec.ch/TC57/NonStandard/UML#concrete> ;
  rdfs:subClassOf cim:Equipment .

cim:HydroPowerPlant a rdfs:Class ;
  rdfs:label "HydroPowerPlant"@en ;
  rdfs:comment "A hydro power station which can generate or pump. When generating, the generator turbines receive water from an upper reservoir. When pumping, the pumps receive their water from a lower reservoir." ;
  cims:belongsToCategory er:Package_EquipmentReliabilityProfile ;
  cims:stereotype "Description", <http://iec.ch/TC57/NonStandard/UML#concrete> .

cim:HydroPump a rdfs:Class ;
  rdfs:label "HydroPump"@en ;
  rdfs:comment "A synchronous motor-driven pump, typically associated with a pumped storage plant." ;
  cims:belongsToCategory er:Package_EquipmentReliabilityProfile ;
  cims:stereotype "Description", <http://iec.ch/TC57/NonStandard/UML#concrete> ;
  rdfs:subClassOf cim:Equipment .

cim:IdentifiedObject a rdfs:Class ;
  rdfs:label "IdentifiedObject"@en ;
  rdfs:comment "This is a root class to provide common identification for all classes needing identification and naming attributes." ;
  cims:belongsToCategory er:Package_EquipmentReliabilityProfile .

cim:Impedance a rdfs:Class ;
  rdfs:label "Impedance"@en ;
  rdfs:comment "Ratio of voltage to current." ;
  cims:belongsToCategory er:Package_EquipmentReliabilityProfile ;
  cims:stereotype "CIMDatatype" .

cim:Integer a rdfs:Class ;
  rdfs:label "Integer"@en ;
  rdfs:comment "An integer number. The range is unspecified and not limited." ;
  cims:belongsToCategory er:Package_EquipmentReliabilityProfile ;
  cims:stereotype "Primitive" .

cim:Line a rdfs:Class ;
  rdfs:label "Line"@en ;
  rdfs:comment "Contains equipment beyond a substation belonging to a power transmission line. " ;
  cims:belongsToCategory er:Package_EquipmentReliabilityProfile ;
  cims:stereotype "Description", <http://iec.ch/TC57/NonStandard/UML#concrete> ;
  rdfs:subClassOf cim:EquipmentContainer .

cim:Money a rdfs:Class ;
  rdfs:label "Money"@en ;
  rdfs:comment "Amount of money." ;
  cims:belongsToCategory er:Package_EquipmentReliabilityProfile ;
  cims:stereotype "CIMDatatype" .

cim:NuclearGeneratingUnit a rdfs:Class ;
  rdfs:label "NuclearGeneratingUnit"@en ;
  rdfs:comment "A nuclear generating unit." ;
  cims:belongsToCategory er:Package_EquipmentReliabilityProfile ;
  cims:stereotype "Description", <http://iec.ch/TC57/NonStandard/UML#concrete> ;
  rdfs:subClassOf cim:GeneratingUnit .

cim:OperationalLimit a rdfs:Class ;
  rdfs:label "OperationalLimit"@en ;
  rdfs:comment """A value and normal value associated with a specific kind of limit. 
The sub class value and normalValue attributes vary inversely to the associated OperationalLimitType.acceptableDuration (acceptableDuration for short).  
If a particular piece of equipment has multiple operational limits of the same kind (apparent power, current, etc.), the limit with the greatest acceptableDuration shall have the smallest limit value and the limit with the smallest acceptableDuration shall have the largest limit value.  Note: A large current can only be allowed to flow through a piece of equipment for a short duration without causing damage, but a lesser current can be allowed to flow for a longer duration. """ ;
  cims:belongsToCategory er:Package_EquipmentReliabilityProfile ;
  rdfs:subClassOf cim:IdentifiedObject .

cim:OperationalLimitDirectionKind a rdfs:Class ;
  rdfs:label "OperationalLimitDirectionKind"@en ;
  rdfs:comment "The direction attribute describes the side of  a limit that is a violation." ;
  cims:belongsToCategory er:Package_EquipmentReliabilityProfile ;
  cims:stereotype <http://iec.ch/TC57/NonStandard/UML#enumeration> .

cim:OperationalLimitSet a rdfs:Class ;
  rdfs:label "OperationalLimitSet"@en ;
  rdfs:comment "A set of limits associated with equipment.  Sets of limits might apply to a specific temperature, or season for example. A set of limits may contain different severities of limit levels that would apply to the same equipment. The set may contain limits of different types such as apparent power and current limits or high and low voltage limits  that are logically applied together as a set." ;
  cims:belongsToCategory er:Package_EquipmentReliabilityProfile ;
  cims:stereotype "Description", <http://iec.ch/TC57/NonStandard/UML#concrete> ;
  rdfs:subClassOf cim:IdentifiedObject .

cim:OperationalLimitType a rdfs:Class ;
  rdfs:label "OperationalLimitType"@en ;
  rdfs:comment "The operational meaning of a category of limits." ;
  cims:belongsToCategory er:Package_EquipmentReliabilityProfile ;
  cims:stereotype <http://iec.ch/TC57/NonStandard/UML#concrete> ;
  rdfs:subClassOf cim:IdentifiedObject .

cim:Organisation a rdfs:Class ;
  rdfs:label "Organisation"@en ;
  rdfs:comment "Organisation that might have roles as utility, contractor, supplier, manufacturer, customer, etc." ;
  cims:belongsToCategory er:Package_EquipmentReliabilityProfile ;
  cims:stereotype <http://iec.ch/TC57/NonStandard/UML#concrete> ;
  rdfs:subClassOf cim:IdentifiedObject .

cim:OrganisationRole a rdfs:Class ;
  rdfs:label "OrganisationRole"@en ;
  rdfs:comment "Identifies a way in which an organisation may participate in the utility enterprise (e.g., customer, manufacturer, etc)." ;
  cims:belongsToCategory er:Package_EquipmentReliabilityProfile ;
  rdfs:subClassOf cim:IdentifiedObject .

cim:PU a rdfs:Class ;
  rdfs:label "PU"@en ;
  rdfs:comment "Per Unit - a positive or negative value referred to a defined base. Values typically range from -10 to +10." ;
  cims:belongsToCategory er:Package_EquipmentReliabilityProfile ;
  cims:stereotype "CIMDatatype" .

cim:PerCent a rdfs:Class ;
  rdfs:label "PerCent"@en ;
  rdfs:comment "Percentage on a defined base.   For example, specify as 100 to indicate at the defined base." ;
  cims:belongsToCategory er:Package_EquipmentReliabilityProfile ;
  cims:stereotype "CIMDatatype" .

cim:PowerElectronicsUnit a rdfs:Class ;
  rdfs:label "PowerElectronicsUnit"@en ;
  rdfs:comment "A generating unit or battery or aggregation that connects to the AC network using power electronics rather than rotating machines." ;
  cims:belongsToCategory er:Package_EquipmentReliabilityProfile ;
  cims:stereotype "Description", <http://iec.ch/TC57/NonStandard/UML#concrete> ;
  rdfs:subClassOf cim:Equipment .

cim:PowerSystemResource a rdfs:Class ;
  rdfs:label "PowerSystemResource"@en ;
  rdfs:comment "A power system resource (PSR) can be an item of equipment such as a switch, an equipment container containing many individual items of equipment such as a substation, or an organisational entity such as sub-control area. Power system resources can have measurements associated." ;
  cims:belongsToCategory er:Package_EquipmentReliabilityProfile ;
  rdfs:subClassOf cim:IdentifiedObject .

cim:Pressure a rdfs:Class ;
  rdfs:label "Pressure"@en ;
  rdfs:comment "Pressure in pascals." ;
  cims:belongsToCategory er:Package_EquipmentReliabilityProfile ;
  cims:stereotype "CIMDatatype" .

cim:Reactance a rdfs:Class ;
  rdfs:label "Reactance"@en ;
  rdfs:comment "Reactance (imaginary part of impedance), at rated frequency." ;
  cims:belongsToCategory er:Package_EquipmentReliabilityProfile ;
  cims:stereotype "CIMDatatype" .

cim:ReactiveCapabilityCurve a rdfs:Class ;
  rdfs:label "ReactiveCapabilityCurve"@en ;
  rdfs:comment "Reactive power rating envelope versus the synchronous machine's active power, in both the generating and motoring modes. For each active power value there is a corresponding high and low reactive power limit  value. Typically there will be a separate curve for each coolant condition, such as hydrogen pressure.  The Y1 axis values represent reactive minimum and the Y2 axis values represent reactive maximum." ;
  cims:belongsToCategory er:Package_EquipmentReliabilityProfile ;
  cims:stereotype <http://iec.ch/TC57/NonStandard/UML#concrete> ;
  rdfs:subClassOf cim:Curve .

cim:ReactivePower a rdfs:Class ;
  rdfs:label "ReactivePower"@en ;
  rdfs:comment "Product of RMS value of the voltage and the RMS value of the quadrature component of the current." ;
  cims:belongsToCategory er:Package_EquipmentReliabilityProfile ;
  cims:stereotype "CIMDatatype" .

cim:RegulatingCondEq a rdfs:Class ;
  rdfs:label "RegulatingCondEq"@en ;
  rdfs:comment "A type of conducting equipment that can regulate a quantity (i.e. voltage or flow) at a specific point in the network. " ;
  cims:belongsToCategory er:Package_EquipmentReliabilityProfile ;
  rdfs:subClassOf cim:EnergyConnection .

cim:Reservoir a rdfs:Class ;
  rdfs:label "Reservoir"@en ;
  rdfs:comment "A water storage facility within a hydro system, including: ponds, lakes, lagoons, and rivers. The storage is usually behind some type of dam." ;
  cims:belongsToCategory er:Package_EquipmentReliabilityProfile ;
  cims:stereotype <http://iec.ch/TC57/NonStandard/UML#concrete> ;
  rdfs:subClassOf cim:PowerSystemResource .

cim:Resistance a rdfs:Class ;
  rdfs:label "Resistance"@en ;
  rdfs:comment "Resistance (real part of impedance)." ;
  cims:belongsToCategory er:Package_EquipmentReliabilityProfile ;
  cims:stereotype "CIMDatatype" .

cim:Seconds a rdfs:Class ;
  rdfs:label "Seconds"@en ;
  rdfs:comment "Time, in seconds." ;
  cims:belongsToCategory er:Package_EquipmentReliabilityProfile ;
  cims:stereotype "CIMDatatype" .

cim:String a rdfs:Class ;
  rdfs:label "String"@en ;
  rdfs:comment "A string consisting of a sequence of characters. The character encoding is UTF-8. The string length is unspecified and unlimited." ;
  cims:belongsToCategory er:Package_EquipmentReliabilityProfile ;
  cims:stereotype "Primitive" .

cim:Substation a rdfs:Class ;
  rdfs:label "Substation"@en ;
  rdfs:comment "A collection of equipment for purposes other than generation or utilization, through which electric energy in bulk is passed for the purposes of switching or modifying its characteristics. " ;
  cims:belongsToCategory er:Package_EquipmentReliabilityProfile ;
  cims:stereotype "Description", <http://iec.ch/TC57/NonStandard/UML#concrete> ;
  rdfs:subClassOf cim:EquipmentContainer .

cim:SynchronousMachine a rdfs:Class ;
  rdfs:label "SynchronousMachine"@en ;
  rdfs:comment "An electromechanical device that operates with shaft rotating synchronously with the network. It is a single machine operating either as a generator or synchronous condenser or pump." ;
  cims:belongsToCategory er:Package_EquipmentReliabilityProfile .

cim:TapChanger a rdfs:Class ;
  rdfs:label "TapChanger"@en ;
  rdfs:comment "Mechanism for changing transformer winding tap positions." ;
  cims:belongsToCategory er:Package_EquipmentReliabilityProfile ;
  cims:stereotype "Description" .

cim:Temperature a rdfs:Class ;
  rdfs:label "Temperature"@en ;
  rdfs:comment "Value of temperature in degrees Celsius." ;
  cims:belongsToCategory er:Package_EquipmentReliabilityProfile ;
  cims:stereotype "CIMDatatype" .

cim:Terminal a rdfs:Class ;
  rdfs:label "Terminal"@en ;
  rdfs:comment "An AC electrical connection point to a piece of conducting equipment. Terminals are connected at physical connection points called connectivity nodes." ;
  cims:belongsToCategory er:Package_EquipmentReliabilityProfile ;
  rdfs:subClassOf cim:ACDCTerminal .

cim:TieFlow a rdfs:Class ;
  rdfs:label "TieFlow"@en ;
  rdfs:comment "Defines the structure (in terms of location and direction) of the net interchange constraint for a control area. This constraint may be used by either AGC or power flow." ;
  cims:belongsToCategory er:Package_EquipmentReliabilityProfile ;
  cims:stereotype "Description", <http://iec.ch/TC57/NonStandard/UML#concrete> ;
  rdfs:subClassOf cim:IdentifiedObject .

cim:UnitMultiplier a rdfs:Class ;
  rdfs:label "UnitMultiplier"@en ;
  rdfs:comment """The unit multipliers defined for the CIM.  When applied to unit symbols, the unit symbol is treated as a derived unit. Regardless of the contents of the unit symbol text, the unit symbol shall be treated as if it were a single-character unit symbol. Unit symbols should not contain multipliers, and it should be left to the multiplier to define the multiple for an entire data type. 

For example, if a unit symbol is "m2Pers" and the multiplier is "k", then the value is k(m**2/s), and the multiplier applies to the entire final value, not to any individual part of the value. This can be conceptualized by substituting a derived unit symbol for the unit type. If one imagines that the symbol "Þ" represents the derived unit "m2Pers", then applying the multiplier "k" can be conceptualized simply as "kÞ".

For example, the SI unit for mass is "kg" and not "g".  If the unit symbol is defined as "kg", then the multiplier is applied to "kg" as a whole and does not replace the "k" in front of the "g". In this case, the multiplier of "m" would be used with the unit symbol of "kg" to represent one gram.  As a text string, this violates the instructions in IEC 80000-1. However, because the unit symbol in CIM is treated as a derived unit instead of as an SI unit, it makes more sense to conceptualize the "kg" as if it were replaced by one of the proposed replacements for the SI mass symbol. If one imagines that the "kg" were replaced by a symbol "Þ", then it is easier to conceptualize the multiplier "m" as creating the proper unit "mÞ", and not the forbidden unit "mkg".""" ;
  cims:belongsToCategory er:Package_EquipmentReliabilityProfile ;
  cims:stereotype <http://iec.ch/TC57/NonStandard/UML#enumeration> .

cim:UnitSymbol a rdfs:Class ;
  rdfs:label "UnitSymbol"@en ;
  rdfs:comment """The derived units defined for usage in the CIM. In some cases, the derived unit is equal to an SI unit. Whenever possible, the standard derived symbol is used instead of the formula for the derived unit. For example, the unit symbol Farad is defined as "F" instead of "CPerV". In cases where a standard symbol does not exist for a derived unit, the formula for the unit is used as the unit symbol. For example, density does not have a standard symbol and so it is represented as "kgPerm3". With the exception of the "kg", which is an SI unit, the unit symbols do not contain multipliers and therefore represent the base derived unit to which a multiplier can be applied as a whole. 
Every unit symbol is treated as an unparseable text as if it were a single-letter symbol. The meaning of each unit symbol is defined by the accompanying descriptive text and not by the text contents of the unit symbol.
To allow the widest possible range of serializations without requiring special character handling, several substitutions are made which deviate from the format described in IEC 80000-1. The division symbol "/" is replaced by the letters "Per". Exponents are written in plain text after the unit as "m3" instead of being formatted as "m" with a superscript of 3  or introducing a symbol as in "m^3". The degree symbol "°" is replaced with the letters "deg". Any clarification of the meaning for a substitution is included in the description for the unit symbol.
Non-SI units are included in list of unit symbols to allow sources of data to be correctly labelled with their non-SI units (for example, a GPS sensor that is reporting numbers that represent feet instead of meters). This allows software to use the unit symbol information correctly convert and scale the raw data of those sources into SI-based units. 
The integer values are used for harmonization with IEC 61850.""" ;
  cims:belongsToCategory er:Package_EquipmentReliabilityProfile ;
  cims:stereotype <http://iec.ch/TC57/NonStandard/UML#enumeration> .

cim:Voltage a rdfs:Class ;
  rdfs:label "Voltage"@en ;
  rdfs:comment "Electrical voltage, can be both AC and DC." ;
  cims:belongsToCategory er:Package_EquipmentReliabilityProfile ;
  cims:stereotype "CIMDatatype" .

cim:VoltagePerReactivePower a rdfs:Class ;
  rdfs:label "VoltagePerReactivePower"@en ;
  rdfs:comment "Voltage variation with reactive power." ;
  cims:belongsToCategory er:Package_EquipmentReliabilityProfile ;
  cims:stereotype "CIMDatatype" .

cim:VsCapabilityCurve a rdfs:Class ;
  rdfs:label "VsCapabilityCurve"@en ;
  rdfs:comment "The P-Q capability curve for a voltage source converter, with P on X-axis and Qmin and Qmax on Y1-axis and Y2-axis." ;
  cims:belongsToCategory er:Package_EquipmentReliabilityProfile ;
  cims:stereotype <http://iec.ch/TC57/NonStandard/UML#concrete> ;
  rdfs:subClassOf cim:Curve .

cim:VsConverter a rdfs:Class ;
  rdfs:label "VsConverter"@en ;
  rdfs:comment "DC side of the voltage source converter (VSC)." ;
  cims:belongsToCategory er:Package_EquipmentReliabilityProfile .

nc:ACDCConverterController a rdfs:Class ;
  rdfs:label "ACDCConverterController"@en ;
  rdfs:comment "ACDC converter unit control. According to IEC 60633, it is the control system used for the controlling, monitoring and protection of a single converter unit." ;
  cims:belongsToCategory er:Package_EquipmentReliabilityProfile ;
  cims:stereotype "NC", <http://iec.ch/TC57/NonStandard/UML#concrete> ;
  rdfs:subClassOf nc:DirectCurrentEquipmentController .

nc:ACEmulationControlFunction a rdfs:Class ;
  rdfs:label "ACEmulationControlFunction"@en ;
  rdfs:comment """The AC emulation control function is used when AC emulation model is activated for a DC system. It consists in computing the active power set point of the DC system as a function of the voltage angle difference between both points of common coupling with the AC network in order to mimic the behavior of an AC transmission line. This control mode enables the automatic adjustment of the active power reference following variations of the AC system operational point. 
The setpoint of the DC system is calculated by Psetpoint=Pref+Kdc*(angle1-angle2), where
- Pref is the existing active power setpoint; 
- Kdc is the control system gain and  
- angle1 and angle2 are the phase angle measurement (measured at points of common coupling with the AC network) respectively at the side 1 and 2 of the DC system.""" ;
  cims:belongsToCategory er:Package_EquipmentReliabilityProfile ;
  cims:stereotype "NC", <http://iec.ch/TC57/NonStandard/UML#concrete> ;
  rdfs:subClassOf nc:ControlFunctionBlock .

nc:ACPointOfCommonCoupling a rdfs:Class ;
  rdfs:label "ACPointOfCommonCoupling"@en ;
  rdfs:comment "Point of interconnection of the DC converter station to the adjacent AC system (IEC 60633)." ;
  cims:belongsToCategory er:Package_EquipmentReliabilityProfile ;
  cims:stereotype "NC", <http://iec.ch/TC57/NonStandard/UML#concrete> ;
  rdfs:subClassOf nc:PointOfCommonCoupling .

nc:ACTieCorridor a rdfs:Class ;
  rdfs:label "ACTieCorridor"@en ;
  rdfs:comment "A collection of one or more AC tie lines that connect two different control areas." ;
  cims:belongsToCategory er:Package_EquipmentReliabilityProfile ;
  cims:stereotype "NC", <http://iec.ch/TC57/NonStandard/UML#concrete> ;
  rdfs:subClassOf nc:TieCorridor .

nc:ActivePowerControlFunction a rdfs:Class ;
  rdfs:label "ActivePowerControlFunction"@en ;
  rdfs:comment "Active power control function is a function block that calculates operating point of the controlled equipment to achieve the target active power." ;
  cims:belongsToCategory er:Package_EquipmentReliabilityProfile ;
  cims:stereotype "NC", <http://iec.ch/TC57/NonStandard/UML#concrete> ;
  rdfs:subClassOf nc:ControlFunctionBlock .

nc:AmbientTemperatureDependencyCurve a rdfs:Class ;
  rdfs:label "AmbientTemperatureDependencyCurve"@en ;
  rdfs:comment "A curve or functional relationship between the ambient temperature independent variable (X-axis) and relative temperature dependent (Y-axis) variables." ;
  cims:belongsToCategory er:Package_EquipmentReliabilityProfile ;
  cims:stereotype "NC", <http://iec.ch/TC57/NonStandard/UML#concrete> ;
  rdfs:subClassOf nc:LimitDependencyCurve .

nc:AreaDispatchableUnit a rdfs:Class ;
  rdfs:label "AreaDispatchableUnit"@en ;
  rdfs:comment "Allocates a given producing or consuming unit, including direct current corridor and collection of units, to a given control area (through the scheduling area) for supporting the control of the given area through dispatch instruction. " ;
  cims:belongsToCategory er:Package_EquipmentReliabilityProfile ;
  cims:stereotype "NC", <http://iec.ch/TC57/NonStandard/UML#concrete> ;
  rdfs:subClassOf cim:PowerSystemResource .

nc:AreaInterchangeController a rdfs:Class ;
  rdfs:label "AreaInterchangeController"@en ;
  rdfs:comment "Area interchange control is set to control active power of an area." ;
  cims:belongsToCategory er:Package_EquipmentReliabilityProfile ;
  cims:stereotype "NC", <http://iec.ch/TC57/NonStandard/UML#concrete> ;
  rdfs:subClassOf nc:SystemControl .

nc:AutomationBlockGroup a rdfs:Class ;
  rdfs:label "AutomationBlockGroup"@en ;
  rdfs:comment "Grouping of function block that are operated with the same priority as settings." ;
  cims:belongsToCategory er:Package_EquipmentReliabilityProfile ;
  cims:stereotype "NC", <http://iec.ch/TC57/NonStandard/UML#concrete> .

nc:AutomationFunction a rdfs:Class ;
  rdfs:label "AutomationFunction"@en ;
  rdfs:comment "Automation function is a collection of functional block or other automation function that can be executed as a work cycle program as part of an automated system." ;
  cims:belongsToCategory er:Package_EquipmentReliabilityProfile ;
  cims:stereotype "NC" ;
  rdfs:subClassOf cim:PowerSystemResource .

nc:BaseOverloadLimitCurve a rdfs:Class ;
  rdfs:label "BaseOverloadLimitCurve"@en ;
  rdfs:comment """A curve or functional relationship between 
- the relative loading - current loading over permanent loading (PATL) independent variable (X-axis), and 
- temporary overloading (TATL) limiting dependent (Y-axis) variables.""" ;
  cims:belongsToCategory er:Package_EquipmentReliabilityProfile ;
  cims:stereotype "NC", <http://iec.ch/TC57/NonStandard/UML#concrete> ;
  rdfs:subClassOf nc:LimitDependencyCurve .

nc:BiddingZone a rdfs:Class ;
  rdfs:label "BiddingZone"@en ;
  rdfs:comment "A bidding zone is a market-based method for handling power transmission congestion. It consists of scheduling areas that include the relevant production (supply) and consumption (demand) to form an electrical area with the same market price without capacity allocation." ;
  cims:belongsToCategory er:Package_EquipmentReliabilityProfile ;
  cims:stereotype "NC", <http://iec.ch/TC57/NonStandard/UML#concrete> ;
  rdfs:subClassOf cim:PowerSystemResource .

nc:BiddingZoneBorder a rdfs:Class ;
  rdfs:label "BiddingZoneBorder"@en ;
  rdfs:comment "Defines the aggregated connection capacity between two Bidding Zones." ;
  cims:belongsToCategory er:Package_EquipmentReliabilityProfile ;
  cims:stereotype "NC", <http://iec.ch/TC57/NonStandard/UML#concrete> ;
  rdfs:subClassOf cim:PowerSystemResource .

nc:BipolarDCSystem a rdfs:Class ;
  rdfs:label "BipolarDCSystem"@en ;
  rdfs:comment "Bipolar DC system (IEC 60633) consists of two poles of opposite polarity with respect to earth. The overhead lines, if any, of the two poles may be carried on common or separate towers." ;
  cims:belongsToCategory er:Package_EquipmentReliabilityProfile ;
  cims:stereotype "NC", <http://iec.ch/TC57/NonStandard/UML#concrete> ;
  rdfs:subClassOf nc:DCSystem .

nc:CapacityCalculationRegion a rdfs:Class ;
  rdfs:label "CapacityCalculationRegion"@en ;
  rdfs:comment "Capacity calculation region is a coherent part of the interconnected system that is used for calculating the transmission capacity for a bidding zone or between bidding zones." ;
  cims:belongsToCategory er:Package_EquipmentReliabilityProfile ;
  cims:stereotype "NC", <http://iec.ch/TC57/NonStandard/UML#concrete> ;
  rdfs:subClassOf nc:Region .

nc:ChargingUnit a rdfs:Class ;
  rdfs:label "ChargingUnit"@en ;
  rdfs:comment "A unit that supplies electrical power for charging electrical non-stationary entities, e.g. electrical vehicle, trucks, buses, ferries, boats and airplanes. The characteristic is that the energy consumption is highly schedule dependent." ;
  cims:belongsToCategory er:Package_EquipmentReliabilityProfile ;
  cims:stereotype "NC", <http://iec.ch/TC57/NonStandard/UML#concrete> ;
  rdfs:subClassOf cim:PowerElectronicsUnit .

nc:Circuit a rdfs:Class ;
  rdfs:label "Circuit"@en ;
  rdfs:comment "A circuit is a collection of equipment in a network graph that provide common stability limits. The relevant equipment is in general given by the identifying terminal. A software application that can do topology processing shall calculate the equipment belonging to the circuit, if there are no stability limits associated to it. In case of stability limits, the containment reflects the equipments that were used in the calculation/analysis. " ;
  cims:belongsToCategory er:Package_EquipmentReliabilityProfile ;
  cims:stereotype "NC" ;
  rdfs:subClassOf cim:PowerSystemResource .

nc:CircuitShare a rdfs:Class ;
  rdfs:label "CircuitShare"@en ;
  rdfs:comment "Defines the share of the circuit which is part of an associated power transfer corridor." ;
  cims:belongsToCategory er:Package_EquipmentReliabilityProfile ;
  cims:stereotype "NC", <http://iec.ch/TC57/NonStandard/UML#concrete> ;
  rdfs:subClassOf cim:IdentifiedObject .

nc:ClosedDistributionSystemOperator a rdfs:Class ;
  rdfs:label "ClosedDistributionSystemOperator"@en ;
  rdfs:comment "A system operator which distributes electricity (or gas) within a geographically confined industrial, commercial or shared services and does not supply household customers." ;
  cims:belongsToCategory er:Package_EquipmentReliabilityProfile ;
  cims:stereotype "NC", <http://iec.ch/TC57/NonStandard/UML#concrete> ;
  rdfs:subClassOf nc:SystemOperator .

nc:CompensatorController a rdfs:Class ;
  rdfs:label "CompensatorController"@en ;
  rdfs:comment "Compensator controller is controlling the equipment to optimize the use of the compensators. " ;
  cims:belongsToCategory er:Package_EquipmentReliabilityProfile ;
  cims:stereotype "NC", <http://iec.ch/TC57/NonStandard/UML#concrete> ;
  rdfs:subClassOf nc:EquipmentController .

nc:ControlFunctionBlock a rdfs:Class ;
  rdfs:label "ControlFunctionBlock"@en ;
  rdfs:comment "Control function block is a function block that contains an algorithm for controlling the equipment." ;
  cims:belongsToCategory er:Package_EquipmentReliabilityProfile ;
  cims:stereotype "NC" ;
  rdfs:subClassOf nc:FunctionBlock .

nc:CoordinatedCapacityCalculator a rdfs:Class ;
  rdfs:label "CoordinatedCapacityCalculator"@en ;
  rdfs:comment "A role that coordinates and executes the task of calculating transmission capacity." ;
  cims:belongsToCategory er:Package_EquipmentReliabilityProfile ;
  cims:stereotype "NC", <http://iec.ch/TC57/NonStandard/UML#concrete> ;
  rdfs:subClassOf nc:SystemOperationCoordinator .

nc:CurrentControlFunction a rdfs:Class ;
  rdfs:label "CurrentControlFunction"@en ;
  rdfs:comment "Current control function is a function block that calculates the operating point of the controlled equipment  to achieve the target current." ;
  cims:belongsToCategory er:Package_EquipmentReliabilityProfile ;
  cims:stereotype "NC", <http://iec.ch/TC57/NonStandard/UML#concrete> ;
  rdfs:subClassOf nc:ControlFunctionBlock .

nc:CurrentDroopControlFunction a rdfs:Class ;
  rdfs:label "CurrentDroopControlFunction"@en ;
  rdfs:comment "Current droop control function is a function block that calculates the operating point of the controlled equipment to achieve the target current." ;
  cims:belongsToCategory er:Package_EquipmentReliabilityProfile ;
  cims:stereotype "NC", <http://iec.ch/TC57/NonStandard/UML#concrete> ;
  rdfs:subClassOf nc:ControlFunctionBlock .

nc:CurrentDroopOverride a rdfs:Class ;
  rdfs:label "CurrentDroopOverride"@en ;
  rdfs:comment """Current droop override uses the following logic:
- When the current exceeds a threshold the device executes the following transitions: 1) When injecting an inductive voltage or in monitoring mode the device tends to inject a voltage proportional to the difference between the line current and the aforementioned threshold. 2) When injecting a capacitive voltage the device transitions to monitoring mode. 
- If the aforementioned proportional voltage is lower than the initial one, the voltage injection remains unchanged. 
Current droop override is not applied when the device operates in currentDroop mode.""" ;
  cims:belongsToCategory er:Package_EquipmentReliabilityProfile ;
  cims:stereotype "NC", <http://iec.ch/TC57/NonStandard/UML#concrete> .

nc:DCBiPole a rdfs:Class ;
  rdfs:label "DCBiPole"@en ;
  rdfs:comment "DC system bipole (IEC 60633), which is part of an DC system consisting of two independently operable DC system poles, which during normal operation, exhibit opposite direct voltage polarities with respect to earth." ;
  cims:belongsToCategory er:Package_EquipmentReliabilityProfile ;
  cims:stereotype "NC", <http://iec.ch/TC57/NonStandard/UML#concrete> ;
  rdfs:subClassOf cim:PowerSystemResource .

nc:DCBypassSwitch a rdfs:Class ;
  rdfs:label "DCBypassSwitch"@en ;
  rdfs:comment "By-pass switch (IEC 60633) is a high-speed DC switch connected across each converter valve group in DC schemes using more than one independent converter per pole, designed to close rapidly to bypass a converter group that is being taken out of service and commutate the current back into a valve group that is being taken back in service. A by-pass switch may also be used for prolonged shunting of the bridge(s)." ;
  cims:belongsToCategory er:Package_EquipmentReliabilityProfile ;
  cims:stereotype "NC", <http://iec.ch/TC57/NonStandard/UML#concrete> ;
  rdfs:subClassOf nc:DCHighSpeedSwitch .

nc:DCCommutationSwitch a rdfs:Class ;
  rdfs:label "DCCommutationSwitch"@en ;
  rdfs:comment "DC commutation switch (IEC 60633) is a type of high-speed DC switch specifically designed to commutate load current into an alternative parallel current path." ;
  cims:belongsToCategory er:Package_EquipmentReliabilityProfile ;
  cims:stereotype "NC" ;
  rdfs:subClassOf nc:DCHighSpeedSwitch .

nc:DCConverterParallelingSwitch a rdfs:Class ;
  rdfs:label "DCConverterParallelingSwitch"@en ;
  rdfs:comment "Converter paralleling switch (IEC 60633) is a high-speed DC switch connected in series with each converter at the DC terminal in DC schemes where two or more converters are connected in parallel onto a common pole conductor, designed to allow additional converter(s) to be connected in parallel or disconnected without affecting the load current in the other converter." ;
  cims:belongsToCategory er:Package_EquipmentReliabilityProfile ;
  cims:stereotype "NC", <http://iec.ch/TC57/NonStandard/UML#concrete> ;
  rdfs:subClassOf nc:DCHighSpeedSwitch .

nc:DCCurrentControlFunction a rdfs:Class ;
  rdfs:label "DCCurrentControlFunction"@en ;
  rdfs:comment "DC current control function is a function block that calculates the operating point of the controlled equipment  to achieve the target current." ;
  cims:belongsToCategory er:Package_EquipmentReliabilityProfile ;
  cims:stereotype "NC", <http://iec.ch/TC57/NonStandard/UML#concrete> ;
  rdfs:subClassOf nc:ControlFunctionBlock .

nc:DCEarthReturnTransferSwitch a rdfs:Class ;
  rdfs:label "DCEarthReturnTransferSwitch"@en ;
  rdfs:comment "Earth return transfer switch (IEC 60633) DC commutation switch used to transfer DC current from a metallic return path to an earth return path. In some applications, this function is performed by a by-pass switch. Although the term \"earth return transfer breaker\" has been widely used in the industry for many years, it is misleading since such switches have no ability to interrupt fault current." ;
  cims:belongsToCategory er:Package_EquipmentReliabilityProfile ;
  cims:stereotype "NC", <http://iec.ch/TC57/NonStandard/UML#concrete> ;
  rdfs:subClassOf nc:DCCommutationSwitch .

nc:DCHarmonicFilter a rdfs:Class ;
  rdfs:label "DCHarmonicFilter"@en ;
  rdfs:comment "DC harmonic filter (IEC 60633) is a filter which, in conjunction with the DC reactor(s) and with the DC surge capacitor(s), if any, serves the primary function of reducing (current or voltage) ripple on the DC transmission line and/or earth electrode line." ;
  cims:belongsToCategory er:Package_EquipmentReliabilityProfile ;
  cims:stereotype "NC", <http://iec.ch/TC57/NonStandard/UML#concrete> ;
  rdfs:subClassOf cim:DCSeriesDevice .

nc:DCHighSpeedSwitch a rdfs:Class ;
  rdfs:label "DCHighSpeedSwitch"@en ;
  rdfs:comment "High-speed DC switch (IEC 60633) is a type of switchgear used on a DC scheme, required to open or close rapidly (&lt; 1 s), including in some cases the need to commutate load current into a parallel conducting path, but with no requirement to interrupt fault or load current. DC switchgear is usually based on a single-phase unit of an AC circuit-breaker, appropriately modified for their DC applications. Their capabilities to perform faster opening and closing than disconnect switches are used but the function of breaking short-circuit currents is not required." ;
  cims:belongsToCategory er:Package_EquipmentReliabilityProfile ;
  cims:stereotype "NC" ;
  rdfs:subClassOf cim:DCSwitch .

nc:DCLineParallelingSwitch a rdfs:Class ;
  rdfs:label "DCLineParallelingSwitch"@en ;
  rdfs:comment "Line paralleling switch (IEC 60633) DC commutation switch placed in series with one or more high-voltage pole conductors, allowing two or more lines to be connected in parallel or to revert to single-line operation while conducting load current." ;
  cims:belongsToCategory er:Package_EquipmentReliabilityProfile ;
  cims:stereotype "NC", <http://iec.ch/TC57/NonStandard/UML#concrete> ;
  rdfs:subClassOf nc:DCCommutationSwitch .

nc:DCMetalicReturnSwitch a rdfs:Class ;
  rdfs:label "DCMetalicReturnSwitch"@en ;
  rdfs:comment "Metallic return transfer switch (IEC 60633) is a DC commutation switch used to transfer DC current from an earth return path to a metallic return path. Although the term \"metallic return transfer breaker\" has been widely used in the industry for many years, it is misleading since such switches have no ability to interrupt fault current." ;
  cims:belongsToCategory er:Package_EquipmentReliabilityProfile ;
  cims:stereotype "NC", <http://iec.ch/TC57/NonStandard/UML#concrete> ;
  rdfs:subClassOf nc:DCCommutationSwitch .

nc:DCNeutralBusGroundingSwitch a rdfs:Class ;
  rdfs:label "DCNeutralBusGroundingSwitch"@en ;
  rdfs:comment "Neutral bus grounding switch (IEC 60633) or a neutral bus earthing switch is a DC commutation switch connected from the neutral bus to the station earth mat on a bipolar DC scheme, designed to provide a temporary earth connection in the event of an open circuit fault on the electrode line until the imbalance of current between the two poles can be reduced to a safe minimum level or the electrode line connection can be restored." ;
  cims:belongsToCategory er:Package_EquipmentReliabilityProfile ;
  cims:stereotype "NC", <http://iec.ch/TC57/NonStandard/UML#concrete> ;
  rdfs:subClassOf nc:DCCommutationSwitch .

nc:DCNeutralBusSwitch a rdfs:Class ;
  rdfs:label "DCNeutralBusSwitch"@en ;
  rdfs:comment "Neutral bus switch (IEC 60633) is a DC commutation switch connected in series with the neutral bus on a bipolar DC scheme, designed to commutate current out of the pole conductor or neutral bus and into the electrode line or dedicated metallic return conductor or earth in response to a fault in a converter or neutral bus." ;
  cims:belongsToCategory er:Package_EquipmentReliabilityProfile ;
  cims:stereotype "NC", <http://iec.ch/TC57/NonStandard/UML#concrete> ;
  rdfs:subClassOf nc:DCCommutationSwitch .

nc:DCPointOfCommonCoupling a rdfs:Class ;
  rdfs:label "DCPointOfCommonCoupling"@en ;
  rdfs:comment "Point of interconnection of the DC converter station to the DC transmission line (IEC 60633)." ;
  cims:belongsToCategory er:Package_EquipmentReliabilityProfile ;
  cims:stereotype "NC", <http://iec.ch/TC57/NonStandard/UML#concrete> ;
  rdfs:subClassOf nc:PointOfCommonCoupling .

nc:DCPole a rdfs:Class ;
  rdfs:label "DCPole"@en ;
  rdfs:comment "The direct current (DC) system pole (IEC 60633) is part of a DC system consisting of all the equipment in the DC substations and the interconnecting transmission lines, if any, which during normal operation exhibit a common direct voltage polarity with respect to earth." ;
  cims:belongsToCategory er:Package_EquipmentReliabilityProfile ;
  cims:stereotype "NC", <http://iec.ch/TC57/NonStandard/UML#concrete> ;
  rdfs:subClassOf cim:PowerSystemResource .

nc:DCSmoothingReactor a rdfs:Class ;
  rdfs:label "DCSmoothingReactor"@en ;
  rdfs:comment "Reactor (IEC 60633) connected in series with a converter unit or converter units on the DC side for the primary purpose of smoothing the direct current and reducing current transients." ;
  cims:belongsToCategory er:Package_EquipmentReliabilityProfile ;
  cims:stereotype "NC", <http://iec.ch/TC57/NonStandard/UML#concrete> ;
  rdfs:subClassOf cim:DCSeriesDevice .

nc:DCSmoothingReactorArrester a rdfs:Class ;
  rdfs:label "DCSmoothingReactorArrester"@en ;
  rdfs:comment "Arrester (IEC 60633) connected between the terminals of a smoothing reactor." ;
  cims:belongsToCategory er:Package_EquipmentReliabilityProfile ;
  cims:stereotype "NC", <http://iec.ch/TC57/NonStandard/UML#concrete> ;
  rdfs:subClassOf cim:DCSeriesDevice .

nc:DCSubstation a rdfs:Class ;
  rdfs:label "DCSubstation"@en ;
  rdfs:comment "DC substation or DC converter station (IEC 60633) is part of an DC system which consists of one or more converter units installed in a single location together with buildings, reactors, filters, reactive power supply, control, monitoring, protective, measuring and auxiliary equipment. A DC substation forming part of an DC transmission system may be referred to as an DC transmission substation." ;
  cims:belongsToCategory er:Package_EquipmentReliabilityProfile ;
  cims:stereotype "NC", <http://iec.ch/TC57/NonStandard/UML#concrete> ;
  rdfs:subClassOf cim:DCEquipmentContainer .

nc:DCSubstationBipole a rdfs:Class ;
  rdfs:label "DCSubstationBipole"@en ;
  rdfs:comment "Part of a bipolar DC system (IEC 60633) contained within a DC substation." ;
  cims:belongsToCategory er:Package_EquipmentReliabilityProfile ;
  cims:stereotype "NC", <http://iec.ch/TC57/NonStandard/UML#concrete> ;
  rdfs:subClassOf cim:DCEquipmentContainer .

nc:DCSubstationPole a rdfs:Class ;
  rdfs:label "DCSubstationPole"@en ;
  rdfs:comment "Part of an DC system pole (IEC 60633) which is contained within a DC substation." ;
  cims:belongsToCategory er:Package_EquipmentReliabilityProfile ;
  cims:stereotype "NC", <http://iec.ch/TC57/NonStandard/UML#concrete> ;
  rdfs:subClassOf cim:DCEquipmentContainer .

nc:DCSystem a rdfs:Class ;
  rdfs:label "DCSystem"@en ;
  rdfs:comment "Electrical power system which transfers energy in the form of direct current between two or more AC buses (defined in IEC 60633)." ;
  cims:belongsToCategory er:Package_EquipmentReliabilityProfile ;
  cims:stereotype "NC" ;
  rdfs:subClassOf cim:PowerSystemResource .

nc:DCSystemDirectionKind a rdfs:Class ;
  rdfs:label "DCSystemDirectionKind"@en ;
  rdfs:comment "Direction kinds of the DC system." ;
  cims:belongsToCategory er:Package_EquipmentReliabilityProfile ;
  cims:stereotype "NC", <http://iec.ch/TC57/NonStandard/UML#enumeration> .

nc:DCSystemTransmissionKind a rdfs:Class ;
  rdfs:label "DCSystemTransmissionKind"@en ;
  rdfs:comment "DC system transmission kind." ;
  cims:belongsToCategory er:Package_EquipmentReliabilityProfile ;
  cims:stereotype "NC", <http://iec.ch/TC57/NonStandard/UML#enumeration> .

nc:DCTieCorridor a rdfs:Class ;
  rdfs:label "DCTieCorridor"@en ;
  rdfs:comment "A collection of one or more direct current poles that connect two different control areas." ;
  cims:belongsToCategory er:Package_EquipmentReliabilityProfile ;
  cims:stereotype "NC", <http://iec.ch/TC57/NonStandard/UML#concrete> ;
  rdfs:subClassOf nc:TieCorridor .

nc:DCVoltageControlFunction a rdfs:Class ;
  rdfs:label "DCVoltageControlFunction"@en ;
  rdfs:comment "DC voltage control function is a function block that calculate the operating point of the controlled equipment to achieve the target voltage." ;
  cims:belongsToCategory er:Package_EquipmentReliabilityProfile ;
  cims:stereotype "NC", <http://iec.ch/TC57/NonStandard/UML#concrete> ;
  rdfs:subClassOf nc:ControlFunctionBlock .

nc:DirectCurrentBipoleController a rdfs:Class ;
  rdfs:label "DirectCurrentBipoleController"@en ;
  rdfs:comment "DC system bipole control that is the control system of a bipole in accordance with IEC 60633." ;
  cims:belongsToCategory er:Package_EquipmentReliabilityProfile ;
  cims:stereotype "NC", <http://iec.ch/TC57/NonStandard/UML#concrete> ;
  rdfs:subClassOf nc:DirectCurrentEquipmentController .

nc:DirectCurrentCircuit a rdfs:Class ;
  rdfs:label "DirectCurrentCircuit"@en ;
  rdfs:comment "A direct current circuit is a circuit consists of direct current equipment." ;
  cims:belongsToCategory er:Package_EquipmentReliabilityProfile ;
  cims:stereotype "NC", <http://iec.ch/TC57/NonStandard/UML#concrete> ;
  rdfs:subClassOf nc:Circuit .

nc:DirectCurrentEquipmentController a rdfs:Class ;
  rdfs:label "DirectCurrentEquipmentController"@en ;
  rdfs:comment "Direct current equipment controller used to control different parts of the hierarchical structure of the DC control system defined by IEC 60633." ;
  cims:belongsToCategory er:Package_EquipmentReliabilityProfile ;
  cims:stereotype "NC" ;
  rdfs:subClassOf nc:EquipmentController .

nc:DirectCurrentMasterController a rdfs:Class ;
  rdfs:label "DirectCurrentMasterController"@en ;
  rdfs:comment """Direct current system control is a control system which governs the operation of an entire DC system consisting of more than one DC substation and performs those functions of controlling, monitoring and protection which require information from more than one substation. This can also be a multiterminal control which is a DC system control for more that two DC substations or a DC master control, which is a general concept for control coordination of a DC system. The DC master control may be implemented at the bipole and/or pole level as defined in IEC 60633. 
The DC system control/multiterminal control/master control is part of the hierarchical structure of an HVDC control system that has an integrated AC/DC system control as the highest level of control which governs the integrated operation of AC and DC systems of a power system. This control system is under the responsibility of the system operator.""" ;
  cims:belongsToCategory er:Package_EquipmentReliabilityProfile ;
  cims:stereotype "NC", <http://iec.ch/TC57/NonStandard/UML#concrete> ;
  rdfs:subClassOf nc:DirectCurrentEquipmentController .

nc:DirectCurrentPoleController a rdfs:Class ;
  rdfs:label "DirectCurrentPoleController"@en ;
  rdfs:comment "DC system pole control, which is the control system of a pole in accordance with IEC 60633." ;
  cims:belongsToCategory er:Package_EquipmentReliabilityProfile ;
  cims:stereotype "NC", <http://iec.ch/TC57/NonStandard/UML#concrete> ;
  rdfs:subClassOf nc:DirectCurrentEquipmentController .

nc:DirectCurrentSubstationBipoleController a rdfs:Class ;
  rdfs:label "DirectCurrentSubstationBipoleController"@en ;
  rdfs:comment "Control system of a substation bipole (IEC 60633)." ;
  cims:belongsToCategory er:Package_EquipmentReliabilityProfile ;
  cims:stereotype "NC", <http://iec.ch/TC57/NonStandard/UML#concrete> ;
  rdfs:subClassOf nc:DirectCurrentSubstationController .

nc:DirectCurrentSubstationController a rdfs:Class ;
  rdfs:label "DirectCurrentSubstationController"@en ;
  rdfs:comment "Control system used for the controlling, monitoring and protection within a DC substation (IEC 60633). A DC substation control may be implemented at the bipole and/or pole level and may be referred to as local control." ;
  cims:belongsToCategory er:Package_EquipmentReliabilityProfile ;
  cims:stereotype "NC" ;
  rdfs:subClassOf nc:DirectCurrentEquipmentController .

nc:DirectCurrentSubstationPoleController a rdfs:Class ;
  rdfs:label "DirectCurrentSubstationPoleController"@en ;
  rdfs:comment "Control system of a substation pole (IEC 60633)." ;
  cims:belongsToCategory er:Package_EquipmentReliabilityProfile ;
  cims:stereotype "NC", <http://iec.ch/TC57/NonStandard/UML#concrete> ;
  rdfs:subClassOf nc:DirectCurrentSubstationController .

nc:DirectCurrentSystemOperator a rdfs:Class ;
  rdfs:label "DirectCurrentSystemOperator"@en ;
  rdfs:comment "System operator of the direct current pole. There are typically one or two system operators that are operating either the control area at one side or the control areas at both sides of the direct current pole. In some cases it is operated by an operator from the connected control areas." ;
  cims:belongsToCategory er:Package_EquipmentReliabilityProfile ;
  cims:stereotype "NC", <http://iec.ch/TC57/NonStandard/UML#concrete> ;
  rdfs:subClassOf nc:SystemOperator .

nc:DistributionSystemOperator a rdfs:Class ;
  rdfs:label "DistributionSystemOperator"@en ;
  rdfs:comment "A system operator that is responsible for operating of energy distribution network from transmission level down to low voltage levels including the connection to household." ;
  cims:belongsToCategory er:Package_EquipmentReliabilityProfile ;
  cims:stereotype "NC", <http://iec.ch/TC57/NonStandard/UML#concrete> ;
  rdfs:subClassOf nc:SystemOperator .

nc:DurationOverloadLimitCurve a rdfs:Class ;
  rdfs:label "DurationOverloadLimitCurve"@en ;
  rdfs:comment """A curve or functional relationship between
- the overload duration independent variable (X-axis), and 
- temporary overloading (TATL) limiting dependent (Y-axis) variables.""" ;
  cims:belongsToCategory er:Package_EquipmentReliabilityProfile ;
  cims:stereotype "NC", <http://iec.ch/TC57/NonStandard/UML#concrete> ;
  rdfs:subClassOf nc:LimitDependencyCurve .

nc:EnergyAlignmentCoordinator a rdfs:Class ;
  rdfs:label "EnergyAlignmentCoordinator"@en ;
  rdfs:comment "A role that is responsible for alignment of forecast and schedule energy to a given energy coordination region." ;
  cims:belongsToCategory er:Package_EquipmentReliabilityProfile ;
  cims:stereotype "NC", <http://iec.ch/TC57/NonStandard/UML#concrete> ;
  rdfs:subClassOf nc:SystemOperationCoordinator .

nc:EnergyBlockComponent a rdfs:Class ;
  rdfs:label "EnergyBlockComponent"@en ;
  rdfs:comment "Energy block component where the energy group is distributed according to the energy block order of each energy component in an energy group." ;
  cims:belongsToCategory er:Package_EquipmentReliabilityProfile ;
  cims:stereotype "NC", <http://iec.ch/TC57/NonStandard/UML#concrete> ;
  rdfs:subClassOf nc:EnergyComponent .

nc:EnergyBlockOrder a rdfs:Class ;
  rdfs:label "EnergyBlockOrder"@en ;
  rdfs:comment "The energy block order is a block (an amount) of energy that forms the sequence of orders that are going to be distributed to an energy block component." ;
  cims:belongsToCategory er:Package_EquipmentReliabilityProfile ;
  cims:stereotype "NC", <http://iec.ch/TC57/NonStandard/UML#concrete> ;
  rdfs:subClassOf cim:IdentifiedObject .

nc:EnergyComponent a rdfs:Class ;
  rdfs:label "EnergyComponent"@en ;
  rdfs:comment "The energy component for a producer or a consumer that has the same energy characteristic, e.g. fuel type and technology." ;
  cims:belongsToCategory er:Package_EquipmentReliabilityProfile ;
  cims:stereotype "NC" ;
  rdfs:subClassOf cim:IdentifiedObject .

nc:EnergyCoordinationRegion a rdfs:Class ;
  rdfs:label "EnergyCoordinationRegion"@en ;
  rdfs:comment "A region that has a common organisation or a service that is responsible for alignment of forecast and scheduling of energy." ;
  cims:belongsToCategory er:Package_EquipmentReliabilityProfile ;
  cims:stereotype "NC", <http://iec.ch/TC57/NonStandard/UML#concrete> ;
  rdfs:subClassOf nc:Region .

nc:EnergyGroup a rdfs:Class ;
  rdfs:label "EnergyGroup"@en ;
  rdfs:comment "An energy group is an aggregation of energy components which have the same energy characteristic, e.g. fuel type and technology. It can be used to allocate energy. " ;
  cims:belongsToCategory er:Package_EquipmentReliabilityProfile ;
  cims:stereotype "NC", <http://iec.ch/TC57/NonStandard/UML#concrete> ;
  rdfs:subClassOf cim:PowerSystemResource .

nc:EnergyKind a rdfs:Class ;
  rdfs:label "EnergyKind"@en ;
  rdfs:comment "Categories of energy used for energy groups." ;
  cims:belongsToCategory er:Package_EquipmentReliabilityProfile ;
  cims:stereotype "NC", <http://iec.ch/TC57/NonStandard/UML#enumeration> .

nc:EnergySourceReference a rdfs:Class ;
  rdfs:label "EnergySourceReference"@en ;
  rdfs:comment "An energy source reference refers to a set of  fuel types characteristic for reporting, e.g. European Energy Certificate System (EECS). The kind of energy should be possible to be linked with different type of energy forecast, e.g. wind production for a given area based on wind forecast." ;
  cims:belongsToCategory er:Package_EquipmentReliabilityProfile ;
  cims:stereotype "NC" .

nc:EnergyType a rdfs:Class ;
  rdfs:label "EnergyType"@en ;
  rdfs:comment """A source of the energy.

An energy type reference refers to an energy characteristic that is needed for reporting, e.g. European Energy Certificate System (EECS). The kind of energy should be possible to be linked with different type of energy forecast, e.g. wind production for a given area based on wind forecast.""" ;
  cims:belongsToCategory er:Package_EquipmentReliabilityProfile ;
  cims:stereotype "NC", <http://iec.ch/TC57/NonStandard/UML#concrete> ;
  rdfs:subClassOf cim:IdentifiedObject .

nc:EquipmentController a rdfs:Class ;
  rdfs:label "EquipmentController"@en ;
  rdfs:comment "Equipment controller is an automation function that can control one or multiple equipment function to achieve all the targets inside the given tolerance. " ;
  cims:belongsToCategory er:Package_EquipmentReliabilityProfile ;
  cims:stereotype "NC" ;
  rdfs:subClassOf nc:AutomationFunction .

nc:ExceptionalPowerTransferCorridor a rdfs:Class ;
  rdfs:label "ExceptionalPowerTransferCorridor"@en ;
  rdfs:comment "Potential power transfer corridor that can be triggered by equipment which changes its in service status or it is operating in an island.  " ;
  cims:belongsToCategory er:Package_EquipmentReliabilityProfile ;
  cims:stereotype "NC", <http://iec.ch/TC57/NonStandard/UML#concrete> ;
  rdfs:subClassOf nc:PowerTransferCorridor .

nc:FACTSEquipment a rdfs:Class ;
  rdfs:label "FACTSEquipment"@en ;
  rdfs:comment "Flexible Alternating Current Transmission System regulating equipment." ;
  cims:belongsToCategory er:Package_EquipmentReliabilityProfile ;
  cims:stereotype "NC" ;
  rdfs:subClassOf cim:RegulatingCondEq .

nc:FlexibleEnergyUnit a rdfs:Class ;
  rdfs:label "FlexibleEnergyUnit"@en ;
  rdfs:comment "Flexible consumer or embedded producer of energy. The unit cannot be a net producer." ;
  cims:belongsToCategory er:Package_EquipmentReliabilityProfile ;
  cims:stereotype "NC", <http://iec.ch/TC57/NonStandard/UML#concrete> ;
  rdfs:subClassOf cim:PowerElectronicsUnit .

nc:FrequencyControlFuntion a rdfs:Class ;
  rdfs:label "FrequencyControlFuntion"@en ;
  rdfs:comment "Frequency control function is a function block that calculate the operating point of the controlled equipment to achieve the target frequency." ;
  cims:belongsToCategory er:Package_EquipmentReliabilityProfile ;
  cims:stereotype "NC", <http://iec.ch/TC57/NonStandard/UML#concrete> ;
  rdfs:subClassOf nc:ControlFunctionBlock .

nc:FrequencyMonitoringTerminal a rdfs:Class ;
  rdfs:label "FrequencyMonitoringTerminal"@en ;
  rdfs:comment "Frequency monitoring terminal provides location in the model where the frequency is monitored for the purpose of power frequency control." ;
  cims:belongsToCategory er:Package_EquipmentReliabilityProfile ;
  cims:stereotype "NC", <http://iec.ch/TC57/NonStandard/UML#concrete> .

nc:FuelStorage a rdfs:Class ;
  rdfs:label "FuelStorage"@en ;
  rdfs:comment "Fuel storage. e.g. pile of coal that can be shared between multiple thermal generating units." ;
  cims:belongsToCategory er:Package_EquipmentReliabilityProfile ;
  cims:stereotype "NC", <http://iec.ch/TC57/NonStandard/UML#concrete> ;
  rdfs:subClassOf cim:PowerSystemResource .

nc:FunctionBlock a rdfs:Class ;
  rdfs:label "FunctionBlock"@en ;
  rdfs:comment "Function block is a function described as a set of elementary blocks. The blocks describe the function between input variables and output variables." ;
  cims:belongsToCategory er:Package_EquipmentReliabilityProfile ;
  cims:stereotype "NC" ;
  rdfs:subClassOf cim:IdentifiedObject .

nc:FunctionInputVariable a rdfs:Class ;
  rdfs:label "FunctionInputVariable"@en ;
  rdfs:comment "Functional input variable defines the domain of the function." ;
  cims:belongsToCategory er:Package_EquipmentReliabilityProfile ;
  cims:stereotype "NC" ;
  rdfs:subClassOf cim:IdentifiedObject .

nc:FunctionOutputVariable a rdfs:Class ;
  rdfs:label "FunctionOutputVariable"@en ;
  rdfs:comment "Functional output variable defines the codomain of the function." ;
  cims:belongsToCategory er:Package_EquipmentReliabilityProfile ;
  cims:stereotype "NC", <http://iec.ch/TC57/NonStandard/UML#concrete> ;
  rdfs:subClassOf cim:IdentifiedObject .

nc:GateInputPin a rdfs:Class ;
  rdfs:label "GateInputPin"@en ;
  rdfs:comment "Input pin for a logical gate. The condition described in the input pin gives a logical true or false. The result from measurement and calculation are converted to a true or false." ;
  cims:belongsToCategory er:Package_EquipmentReliabilityProfile ;
  cims:stereotype "NC", <http://iec.ch/TC57/NonStandard/UML#concrete> ;
  rdfs:subClassOf nc:FunctionInputVariable .

nc:GeothermalGeneratingUnit a rdfs:Class ;
  rdfs:label "GeothermalGeneratingUnit"@en ;
  rdfs:comment "Generating unit that is generating electrical power from geothermal energy." ;
  cims:belongsToCategory er:Package_EquipmentReliabilityProfile ;
  cims:stereotype "NC", <http://iec.ch/TC57/NonStandard/UML#concrete> ;
  rdfs:subClassOf cim:GeneratingUnit .

nc:GeothermalUnitKind a rdfs:Class ;
  rdfs:label "GeothermalUnitKind"@en ;
  rdfs:comment "Kind of geothermal." ;
  cims:belongsToCategory er:Package_EquipmentReliabilityProfile ;
  cims:stereotype "NC", <http://iec.ch/TC57/NonStandard/UML#enumeration> .

nc:ImpedanceControlFunction a rdfs:Class ;
  rdfs:label "ImpedanceControlFunction"@en ;
  rdfs:comment "Impedance control function is a function block that calculates the operating point of the controlled equipment to achieve the target impedance." ;
  cims:belongsToCategory er:Package_EquipmentReliabilityProfile ;
  cims:stereotype "NC", <http://iec.ch/TC57/NonStandard/UML#concrete> ;
  rdfs:subClassOf nc:ControlFunctionBlock .

nc:InfeedLimit a rdfs:Class ;
  rdfs:label "InfeedLimit"@en ;
  rdfs:comment "Infeed limit set constraints fed in to the network by two or more terminals." ;
  cims:belongsToCategory er:Package_EquipmentReliabilityProfile ;
  cims:stereotype "NC", <http://iec.ch/TC57/NonStandard/UML#concrete> ;
  rdfs:subClassOf cim:OperationalLimit .

nc:InfeedTerminal a rdfs:Class ;
  rdfs:label "InfeedTerminal"@en ;
  rdfs:comment "Infeed terminal defines the terminals that are linked to an infeed limit." ;
  cims:belongsToCategory er:Package_EquipmentReliabilityProfile ;
  cims:stereotype "NC", <http://iec.ch/TC57/NonStandard/UML#concrete> .

nc:InjectionController a rdfs:Class ;
  rdfs:label "InjectionController"@en ;
  rdfs:comment "Injection controller is controlling the equipment which represents an injection or an external network." ;
  cims:belongsToCategory er:Package_EquipmentReliabilityProfile ;
  cims:stereotype "NC", <http://iec.ch/TC57/NonStandard/UML#concrete> ;
  rdfs:subClassOf nc:EquipmentController .

nc:LimitDependencyCurve a rdfs:Class ;
  rdfs:label "LimitDependencyCurve"@en ;
  rdfs:comment "A curve or functional relationship between an independent variable (X-axis) and limiting dependent (Y-axis) variables." ;
  cims:belongsToCategory er:Package_EquipmentReliabilityProfile ;
  cims:stereotype "NC" ;
  rdfs:subClassOf cim:Curve .

nc:LineCircuit a rdfs:Class ;
  rdfs:label "LineCircuit"@en ;
  rdfs:comment "A line circuit is a circuit that has at least one ACLineSegment and may or may not include related switching and/or auxiliary equipment." ;
  cims:belongsToCategory er:Package_EquipmentReliabilityProfile ;
  cims:stereotype "NC", <http://iec.ch/TC57/NonStandard/UML#concrete> ;
  rdfs:subClassOf nc:Circuit .

nc:LoadFrequencyControlArea a rdfs:Class ;
  rdfs:label "LoadFrequencyControlArea"@en ;
  rdfs:comment "A part of a synchronous area or an entire synchronous area, physically demarcated by points of measurement at interconnectors to other load frequency control (LFC) areas, operated by one or more TSOs fulfilling the obligations of load-frequency control." ;
  cims:belongsToCategory er:Package_EquipmentReliabilityProfile ;
  cims:stereotype "NC", <http://iec.ch/TC57/NonStandard/UML#concrete> ;
  rdfs:subClassOf cim:PowerSystemResource .

nc:LoadFrequencyControlBlock a rdfs:Class ;
  rdfs:label "LoadFrequencyControlBlock"@en ;
  rdfs:comment "A part of a synchronous area or an entire synchronous area, physically demarcated by points of measurement at interconnectors to other load frequency control (LFC) blocks, consisting of one or more LFC areas, operated by one or more TSOs fulfilling the obligations of load-frequency control." ;
  cims:belongsToCategory er:Package_EquipmentReliabilityProfile ;
  cims:stereotype "NC", <http://iec.ch/TC57/NonStandard/UML#concrete> ;
  rdfs:subClassOf cim:PowerSystemResource .

nc:LoadFrequencyControlOperator a rdfs:Class ;
  rdfs:label "LoadFrequencyControlOperator"@en ;
  rdfs:comment "A role that is responsible for operational security by operating the load frequency control (LFC) mechanism." ;
  cims:belongsToCategory er:Package_EquipmentReliabilityProfile ;
  cims:stereotype "NC", <http://iec.ch/TC57/NonStandard/UML#concrete> ;
  rdfs:subClassOf nc:PowerSystemOrganisationRole .

nc:LogicalOperatorsKind a rdfs:Class ;
  rdfs:label "LogicalOperatorsKind"@en ;
  rdfs:comment "Kinds of logical operators for comparison." ;
  cims:belongsToCategory er:Package_EquipmentReliabilityProfile ;
  cims:stereotype "NC", <http://iec.ch/TC57/NonStandard/UML#enumeration> .

nc:LossCurve a rdfs:Class ;
  rdfs:label "LossCurve"@en ;
  rdfs:comment "Represents the losses in the equipment due to operation position." ;
  cims:belongsToCategory er:Package_EquipmentReliabilityProfile ;
  cims:stereotype "NC", <http://iec.ch/TC57/NonStandard/UML#concrete> ;
  rdfs:subClassOf cim:Curve .

nc:MarineUnitKind a rdfs:Class ;
  rdfs:label "MarineUnitKind"@en ;
  rdfs:comment "Kind of marine energy capture." ;
  cims:belongsToCategory er:Package_EquipmentReliabilityProfile ;
  cims:stereotype "NC", <http://iec.ch/TC57/NonStandard/UML#enumeration> .

nc:ModularStaticSynchronousSeriesCompensator a rdfs:Class ;
  rdfs:label "ModularStaticSynchronousSeriesCompensator"@en ;
  rdfs:comment "Modular static synchronous series compensator (MSSSC) is a type of flexible AC transmission system regulating equipment which consists of solid-state voltage source inverter connected in series with a transmission line. This is similar to static synchronous series compensator (SSSC), but without injection transformer. This enables the MSSSC to be truly modular with the ability to simply install a number of equipment in series to provide a desired maximum level of impedance. MSSSC can be dispersed into multiple location in a circuit working collectively under the same controller scheme." ;
  cims:belongsToCategory er:Package_EquipmentReliabilityProfile ;
  cims:stereotype "NC", <http://iec.ch/TC57/NonStandard/UML#concrete> ;
  rdfs:subClassOf nc:FACTSEquipment .

nc:MonitoringArea a rdfs:Class ;
  rdfs:label "MonitoringArea"@en ;
  rdfs:comment "A coherent part of the interconnected electrical power system, that includes the system operators' responsibility area and the surrounding parts of other system operators' responsibility area, that need to be monitored for security assessment." ;
  cims:belongsToCategory er:Package_EquipmentReliabilityProfile ;
  cims:stereotype "NC" ;
  rdfs:subClassOf cim:PowerSystemResource .

nc:MonopolarDCSystem a rdfs:Class ;
  rdfs:label "MonopolarDCSystem"@en ;
  rdfs:comment "Monopolar DC system (IEC 60633) is a DC system with only one pole." ;
  cims:belongsToCategory er:Package_EquipmentReliabilityProfile ;
  cims:stereotype "NC", <http://iec.ch/TC57/NonStandard/UML#concrete> ;
  rdfs:subClassOf nc:DCSystem .

nc:NuclearReactorKind a rdfs:Class ;
  rdfs:label "NuclearReactorKind"@en ;
  rdfs:comment "Kind of nuclear reactor." ;
  cims:belongsToCategory er:Package_EquipmentReliabilityProfile ;
  cims:stereotype "NC", <http://iec.ch/TC57/NonStandard/UML#enumeration> .

nc:OrdinaryPowerTransferCorridor a rdfs:Class ;
  rdfs:label "OrdinaryPowerTransferCorridor"@en ;
  rdfs:comment "Power transfer corridor defined for normal operating network." ;
  cims:belongsToCategory er:Package_EquipmentReliabilityProfile ;
  cims:stereotype "NC", <http://iec.ch/TC57/NonStandard/UML#concrete> ;
  rdfs:subClassOf nc:PowerTransferCorridor .

nc:OutageCoordinationRegion a rdfs:Class ;
  rdfs:label "OutageCoordinationRegion"@en ;
  rdfs:comment "A region that has a common organisation or service responsible for outage planning and coordination and its impact on grid operation." ;
  cims:belongsToCategory er:Package_EquipmentReliabilityProfile ;
  cims:stereotype "NC", <http://iec.ch/TC57/NonStandard/UML#concrete> ;
  rdfs:subClassOf nc:Region .

nc:OutageCoordinator a rdfs:Class ;
  rdfs:label "OutageCoordinator"@en ;
  rdfs:comment "A role that coordinates the planned availability status of relevant power system equipment to meet the need by the asset owner or operator and the security of the power system." ;
  cims:belongsToCategory er:Package_EquipmentReliabilityProfile ;
  cims:stereotype "NC", <http://iec.ch/TC57/NonStandard/UML#concrete> ;
  rdfs:subClassOf nc:SystemOperationCoordinator .

nc:OutagePlanningAgent a rdfs:Class ;
  rdfs:label "OutagePlanningAgent"@en ;
  rdfs:comment "An entity with the task of planning the availability status of a relevant power generating module, a relevant demand facility or a relevant grid element." ;
  cims:belongsToCategory er:Package_EquipmentReliabilityProfile ;
  cims:stereotype "NC", <http://iec.ch/TC57/NonStandard/UML#concrete> ;
  rdfs:subClassOf nc:PowerSystemOrganisationRole .

nc:OverlappingZone a rdfs:Class ;
  rdfs:label "OverlappingZone"@en ;
  rdfs:comment "A collection of all the overlapping cross border assessed elements which have the same sets of impacted and impacting regions." ;
  cims:belongsToCategory er:Package_EquipmentReliabilityProfile ;
  cims:stereotype "NC", <http://iec.ch/TC57/NonStandard/UML#concrete> ;
  rdfs:subClassOf cim:IdentifiedObject .

nc:PTCTriggeredEquipment a rdfs:Class ;
  rdfs:label "PTCTriggeredEquipment"@en ;
  rdfs:comment "Power Transfer Corridor triggered equipment connects the equipment that will create the exceptional power transfer corridor when taking out of service. e.g. A system with three lines gets an exceptional power transfer corridor when one of the lines is taken out of service." ;
  cims:belongsToCategory er:Package_EquipmentReliabilityProfile ;
  cims:stereotype "Description", "NC", <http://iec.ch/TC57/NonStandard/UML#concrete> ;
  rdfs:subClassOf cim:IdentifiedObject .

nc:PhaseControlFunction a rdfs:Class ;
  rdfs:label "PhaseControlFunction"@en ;
  rdfs:comment "Phase control function is a function block that calculate the operating point of the controlled equipment to achieve the target voltage." ;
  cims:belongsToCategory er:Package_EquipmentReliabilityProfile ;
  cims:stereotype "NC", <http://iec.ch/TC57/NonStandard/UML#concrete> ;
  rdfs:subClassOf nc:ControlFunctionBlock .

nc:PinTerminal a rdfs:Class ;
  rdfs:label "PinTerminal"@en ;
  rdfs:comment "Input pin associated with a Terminal. It is used for comparison." ;
  cims:belongsToCategory er:Package_EquipmentReliabilityProfile ;
  cims:stereotype "NC", <http://iec.ch/TC57/NonStandard/UML#concrete> ;
  rdfs:subClassOf nc:GateInputPin .

nc:PinTerminalKind a rdfs:Class ;
  rdfs:label "PinTerminalKind"@en ;
  rdfs:comment "The kind of quantities that can serve as an input value for the pin." ;
  cims:belongsToCategory er:Package_EquipmentReliabilityProfile ;
  cims:stereotype "NC", <http://iec.ch/TC57/NonStandard/UML#enumeration> .

nc:PointOfCommonCoupling a rdfs:Class ;
  rdfs:label "PointOfCommonCoupling"@en ;
  rdfs:comment "Point of Common Coupling (PCC) refers to the location where multiple electrical sources or loads are electrically connected and provide a reference point where the voltages and currents from different parts of the system are considered to be common. The PCC is used to support system analysis, control, and monitoring, as it provides a reference for understanding the interactions and power flow between various components within the system. It is also relevant to define the requirement and responsibility between different actors in operating a power system." ;
  cims:belongsToCategory er:Package_EquipmentReliabilityProfile ;
  cims:stereotype "NC" ;
  rdfs:subClassOf cim:IdentifiedObject .

nc:PowerBlockKind a rdfs:Class ;
  rdfs:label "PowerBlockKind"@en ;
  rdfs:comment "Power block kind describes the increase and/or decrease of power." ;
  cims:belongsToCategory er:Package_EquipmentReliabilityProfile ;
  cims:stereotype "NC", <http://iec.ch/TC57/NonStandard/UML#enumeration> .

nc:PowerCapacity a rdfs:Class ;
  rdfs:label "PowerCapacity"@en ;
  rdfs:comment "Power capacity defines the capacity in regard to generation, consumption and transmission (import and export) for a relevant power system resource, e.g. bidding zone, including maximum and minimum electrical power capacity and any capacity allocation." ;
  cims:belongsToCategory er:Package_EquipmentReliabilityProfile ;
  cims:stereotype "NC", <http://iec.ch/TC57/NonStandard/UML#concrete> .

nc:PowerElectricalChemicalUnit a rdfs:Class ;
  rdfs:label "PowerElectricalChemicalUnit"@en ;
  rdfs:comment "A unit capable of either generating electrical energy from chemical reactions or using electrical energy to cause chemical reactions." ;
  cims:belongsToCategory er:Package_EquipmentReliabilityProfile ;
  cims:stereotype "NC", <http://iec.ch/TC57/NonStandard/UML#concrete> ;
  rdfs:subClassOf cim:PowerElectronicsUnit .

nc:PowerElectricalChemicalUnitKind a rdfs:Class ;
  rdfs:label "PowerElectricalChemicalUnitKind"@en ;
  rdfs:comment "Kind of power electrical chemical unit." ;
  cims:belongsToCategory er:Package_EquipmentReliabilityProfile ;
  cims:stereotype "NC", <http://iec.ch/TC57/NonStandard/UML#enumeration> .

nc:PowerElectronicsConnectionController a rdfs:Class ;
  rdfs:label "PowerElectronicsConnectionController"@en ;
  rdfs:comment "Power electronics connection controller is controlling the equipment to optimize the power electronics connection. " ;
  cims:belongsToCategory er:Package_EquipmentReliabilityProfile ;
  cims:stereotype "NC", <http://iec.ch/TC57/NonStandard/UML#concrete> ;
  rdfs:subClassOf nc:EquipmentController .

nc:PowerElectronicsMarineUnit a rdfs:Class ;
  rdfs:label "PowerElectronicsMarineUnit"@en ;
  rdfs:comment "A unit that capture energy from marine sources, e.g. waves, for generating electrical power." ;
  cims:belongsToCategory er:Package_EquipmentReliabilityProfile ;
  cims:stereotype "NC", <http://iec.ch/TC57/NonStandard/UML#concrete> ;
  rdfs:subClassOf cim:PowerElectronicsUnit .

nc:PowerElectronicsUnitController a rdfs:Class ;
  rdfs:label "PowerElectronicsUnitController"@en ;
  rdfs:comment "Power electronics unit controller is controlling the equipment to optimize the power electronics unit. " ;
  cims:belongsToCategory er:Package_EquipmentReliabilityProfile ;
  cims:stereotype "NC", <http://iec.ch/TC57/NonStandard/UML#concrete> ;
  rdfs:subClassOf nc:EquipmentController .

nc:PowerFactorControlFunction a rdfs:Class ;
  rdfs:label "PowerFactorControlFunction"@en ;
  rdfs:comment "Power factor control function is a function block that calculates the operating point of the controlled equipment to achieve the target power factor." ;
  cims:belongsToCategory er:Package_EquipmentReliabilityProfile ;
  cims:stereotype "NC", <http://iec.ch/TC57/NonStandard/UML#concrete> ;
  rdfs:subClassOf nc:ControlFunctionBlock .

nc:PowerFrequencyControlKind a rdfs:Class ;
  rdfs:label "PowerFrequencyControlKind"@en ;
  rdfs:comment "Kinds of power frequency control modes." ;
  cims:belongsToCategory er:Package_EquipmentReliabilityProfile ;
  cims:stereotype "NC", <http://iec.ch/TC57/NonStandard/UML#enumeration> .

nc:PowerFrequencyController a rdfs:Class ;
  rdfs:label "PowerFrequencyController"@en ;
  rdfs:comment "Power frequency controller is controlling the active power balance as typically done by the secondary control. If an unbalance between the scheduled active power values of each generation unit and the loads plus losses occurs, primary control will adapt (increase/decrease) the active power production of each unit (depending on the power shift key strategy), leading to an over- or under-frequency situation. The secondary frequency controller will then control the frequency back to its nominal value, re- establishing a cost-efficient generation delivered by each unit." ;
  cims:belongsToCategory er:Package_EquipmentReliabilityProfile ;
  cims:stereotype "NC", <http://iec.ch/TC57/NonStandard/UML#concrete> ;
  rdfs:subClassOf nc:SystemControl .

nc:PowerPlantController a rdfs:Class ;
  rdfs:label "PowerPlantController"@en ;
  rdfs:comment "Power plant controller is controlling the equipment of a power plant. " ;
  cims:belongsToCategory er:Package_EquipmentReliabilityProfile ;
  cims:stereotype "NC", <http://iec.ch/TC57/NonStandard/UML#concrete> ;
  rdfs:subClassOf nc:EquipmentController .

nc:PowerShiftKeyKind a rdfs:Class ;
  rdfs:label "PowerShiftKeyKind"@en ;
  rdfs:comment "Kind of generating and load shift keys strategy." ;
  cims:belongsToCategory er:Package_EquipmentReliabilityProfile ;
  cims:stereotype "NC", <http://iec.ch/TC57/NonStandard/UML#enumeration> .

nc:PowerShiftKeyStrategy a rdfs:Class ;
  rdfs:label "PowerShiftKeyStrategy"@en ;
  rdfs:comment "Strategy of the power shift key." ;
  cims:belongsToCategory er:Package_EquipmentReliabilityProfile ;
  cims:stereotype "NC", <http://iec.ch/TC57/NonStandard/UML#concrete> ;
  rdfs:subClassOf cim:IdentifiedObject .

nc:PowerSystemOrganisationRole a rdfs:Class ;
  rdfs:label "PowerSystemOrganisationRole"@en ;
  rdfs:comment "A role that is responsible for the functional operational of a power system resource." ;
  cims:belongsToCategory er:Package_EquipmentReliabilityProfile ;
  cims:stereotype "NC" ;
  rdfs:subClassOf cim:OrganisationRole .

nc:PowerTransferCorridor a rdfs:Class ;
  rdfs:label "PowerTransferCorridor"@en ;
  rdfs:comment "A power transfer corridor is defined as a set of circuits (transmission lines or transformers) separating two portions of the power system, or a subset of circuits exposed to a substantial portion of the transmission exchange between two parts of the system." ;
  cims:belongsToCategory er:Package_EquipmentReliabilityProfile ;
  cims:stereotype "NC" ;
  rdfs:subClassOf cim:PowerSystemResource .

nc:PowerTransformerCircuit a rdfs:Class ;
  rdfs:label "PowerTransformerCircuit"@en ;
  rdfs:comment "A power transformer circuit is a circuit that has at least one PowerTransformer and may or may not include related switching and/or auxiliary equipment." ;
  cims:belongsToCategory er:Package_EquipmentReliabilityProfile ;
  cims:stereotype "NC", <http://iec.ch/TC57/NonStandard/UML#concrete> ;
  rdfs:subClassOf nc:Circuit .

nc:PropertyReference a rdfs:Class ;
  rdfs:label "PropertyReference"@en ;
  rdfs:comment "The reference to a class and one of its properties." ;
  cims:belongsToCategory er:Package_EquipmentReliabilityProfile ;
  cims:stereotype "NC" .

nc:ProportionalEnergyComponent a rdfs:Class ;
  rdfs:label "ProportionalEnergyComponent"@en ;
  rdfs:comment "Serves for grouping components within an energy group, with proportional energy allocation to all components." ;
  cims:belongsToCategory er:Package_EquipmentReliabilityProfile ;
  cims:stereotype "NC", <http://iec.ch/TC57/NonStandard/UML#concrete> ;
  rdfs:subClassOf nc:EnergyComponent .

nc:RampingPrincipleKind a rdfs:Class ;
  rdfs:label "RampingPrincipleKind"@en ;
  rdfs:comment "Kind of ramping principle." ;
  cims:belongsToCategory er:Package_EquipmentReliabilityProfile ;
  cims:stereotype "NC", <http://iec.ch/TC57/NonStandard/UML#enumeration> .

nc:ReactivePowerControlFunction a rdfs:Class ;
  rdfs:label "ReactivePowerControlFunction"@en ;
  rdfs:comment "Reactive power control function is a function block that calculate the operating point of the controlled equipment to achieve the target reactive power." ;
  cims:belongsToCategory er:Package_EquipmentReliabilityProfile ;
  cims:stereotype "NC", <http://iec.ch/TC57/NonStandard/UML#concrete> ;
  rdfs:subClassOf nc:ControlFunctionBlock .

nc:RecoveryOverloadLimitCurve a rdfs:Class ;
  rdfs:label "RecoveryOverloadLimitCurve"@en ;
  rdfs:comment "The relation between the recovery time and an overload limit." ;
  cims:belongsToCategory er:Package_EquipmentReliabilityProfile ;
  cims:stereotype "NC", <http://iec.ch/TC57/NonStandard/UML#concrete> ;
  rdfs:subClassOf nc:LimitDependencyCurve .

nc:Region a rdfs:Class ;
  rdfs:label "Region"@en ;
  rdfs:comment "A region where the system operator belongs to." ;
  cims:belongsToCategory er:Package_EquipmentReliabilityProfile ;
  cims:stereotype "NC" ;
  rdfs:subClassOf cim:PowerSystemResource .

nc:RotatingMachineController a rdfs:Class ;
  rdfs:label "RotatingMachineController"@en ;
  rdfs:comment "Rotating machine controller is controlling the equipment which may be used as a generator or motor." ;
  cims:belongsToCategory er:Package_EquipmentReliabilityProfile ;
  cims:stereotype "NC", <http://iec.ch/TC57/NonStandard/UML#concrete> ;
  rdfs:subClassOf nc:EquipmentController .

nc:SSSCController a rdfs:Class ;
  rdfs:label "SSSCController"@en ;
  rdfs:comment "The controller of a Static synchronous series compensator (SSSC)." ;
  cims:belongsToCategory er:Package_EquipmentReliabilityProfile ;
  cims:stereotype "NC", <http://iec.ch/TC57/NonStandard/UML#concrete> ;
  rdfs:subClassOf nc:EquipmentController .

nc:SSSCSimulationSettings a rdfs:Class ;
  rdfs:label "SSSCSimulationSettings"@en ;
  rdfs:comment "SSSC control simulation settings used by the algorithm for power flow calculations. " ;
  cims:belongsToCategory er:Package_EquipmentReliabilityProfile ;
  cims:stereotype "NC", <http://iec.ch/TC57/NonStandard/UML#concrete> .

nc:ScheduleResource a rdfs:Class ;
  rdfs:label "ScheduleResource"@en ;
  rdfs:comment "A schedule resource is a market-based method for handling participation of small units, particularly located on the lower voltage level that is controlled by a Distributed System Operator (DSO). It is a collection of units that can operate in the market by providing bids, offers and a resulting committed operational schedule for the collection." ;
  cims:belongsToCategory er:Package_EquipmentReliabilityProfile ;
  cims:stereotype "NC", <http://iec.ch/TC57/NonStandard/UML#concrete> ;
  rdfs:subClassOf cim:PowerSystemResource .

nc:ScheduleResourceController a rdfs:Class ;
  rdfs:label "ScheduleResourceController"@en ;
  rdfs:comment "Schedule resource controller is controlling the equipment to optimize the schedule resource. " ;
  cims:belongsToCategory er:Package_EquipmentReliabilityProfile ;
  cims:stereotype "NC", <http://iec.ch/TC57/NonStandard/UML#concrete> ;
  rdfs:subClassOf nc:EquipmentController .

nc:SchedulingArea a rdfs:Class ;
  rdfs:label "SchedulingArea"@en ;
  rdfs:comment "An area where production and/or consumption of energy can be forecasted, scheduled and measured. The area is operated by only one system operator, typically a Transmission System Operator (TSO). The area can consist of a sub area, which has the same definition as the main area, but it can be operated by another system operator (typically Distributed System Operator (DSO) or a Closed Distributed System Operator (CDSO)). This includes microgrid concept. A substation is the smallest grouping that can be included in the area. The area size should be considered in terms of the possibility of accumulated reading (settlement metering) and the capability of operating as an island." ;
  cims:belongsToCategory er:Package_EquipmentReliabilityProfile ;
  cims:stereotype "NC", <http://iec.ch/TC57/NonStandard/UML#concrete> ;
  rdfs:subClassOf cim:PowerSystemResource .

nc:SecurityCoordinator a rdfs:Class ;
  rdfs:label "SecurityCoordinator"@en ;
  rdfs:comment "A role that coordinates the relevant remedial actions and their optimisation to ensure efficient use to achieve required operational security of the power system." ;
  cims:belongsToCategory er:Package_EquipmentReliabilityProfile ;
  cims:stereotype "NC", <http://iec.ch/TC57/NonStandard/UML#concrete> ;
  rdfs:subClassOf nc:SystemOperationCoordinator .

nc:ShiftMethodKind a rdfs:Class ;
  rdfs:label "ShiftMethodKind"@en ;
  rdfs:comment "Kind of shift method. Describes the way a power schedule should be distributed amongst production and consumption. e.g. Type of generating and load shift key." ;
  cims:belongsToCategory er:Package_EquipmentReliabilityProfile ;
  cims:stereotype "NC", <http://iec.ch/TC57/NonStandard/UML#enumeration> .

nc:SolarRadiationDependencyCurve a rdfs:Class ;
  rdfs:label "SolarRadiationDependencyCurve"@en ;
  rdfs:comment """A curve or functional relationship between 
- the solar radiation independent variable (X-axis), and 
- relative dependent (Y-axis) variables.""" ;
  cims:belongsToCategory er:Package_EquipmentReliabilityProfile ;
  cims:stereotype "NC", <http://iec.ch/TC57/NonStandard/UML#concrete> ;
  rdfs:subClassOf nc:LimitDependencyCurve .

nc:StaticSynchronousCompensator a rdfs:Class ;
  rdfs:label "StaticSynchronousCompensator"@en ;
  rdfs:comment "Static synchronous compensator (STATCOM), also known as a static synchronous condenser (STATCON), is a type of flexible AC transmission system regulating equipment used on alternating current electricity transmission networks. It is based on a power electronics voltage-source converter and can act as either a source or sink of reactive AC power to an electricity network. If connected to a source of power it can also provide active AC power." ;
  cims:belongsToCategory er:Package_EquipmentReliabilityProfile ;
  cims:stereotype "NC", <http://iec.ch/TC57/NonStandard/UML#concrete> ;
  rdfs:subClassOf nc:FACTSEquipment .

nc:StaticSynchronousSeriesCompensator a rdfs:Class ;
  rdfs:label "StaticSynchronousSeriesCompensator"@en ;
  rdfs:comment "Static synchronous series compensator (SSSC) is a type of flexible AC transmission system which consists of a solid-state voltage source inverter coupled with a transformer that is connected in series with a transmission line. This device can inject an almost sinusoidal voltage in series with the line. This injected voltage could be considered as an inductive or capacitive reactance, which is connected in series with the transmission line. This feature can provide controllable voltage compensation. In addition, SSSC is able to reverse the power flow by injecting a sufficiently large series reactive compensating voltage. Moreover it can inject a voltage proportional to the difference between the line current and the pre-configured current threshold.<font color=\"#636671\"> </font>It shall have two Terminal-s associated with it. " ;
  cims:belongsToCategory er:Package_EquipmentReliabilityProfile ;
  cims:stereotype "NC", <http://iec.ch/TC57/NonStandard/UML#concrete> ;
  rdfs:subClassOf nc:FACTSEquipment .

nc:StaticVarCompensator a rdfs:Class ;
  rdfs:label "StaticVarCompensator"@en ;
  rdfs:comment """A facility for providing variable and controllable shunt reactive power. The SVC typically consists of a stepdown transformer, filter, thyristor-controlled reactor, and thyristor-switched capacitor arms.

The SVC may operate in fixed MVar output mode or in voltage control mode. When in voltage control mode, the output of the SVC will be proportional to the deviation of voltage at the controlled bus from the voltage setpoint.  The SVC characteristic slope defines the proportion.  If the voltage at the controlled bus is equal to the voltage setpoint, the SVC MVar output is zero.""" ;
  cims:belongsToCategory er:Package_EquipmentReliabilityProfile ;
  cims:stereotype "NC", <http://iec.ch/TC57/NonStandard/UML#concrete> ;
  rdfs:subClassOf nc:FACTSEquipment .

nc:SubSchedulingArea a rdfs:Class ;
  rdfs:label "SubSchedulingArea"@en ;
  rdfs:comment "An area that is a part of another scheduling area. Typically part of a Transmission System Operator (TSO) scheduling area operated by a Distributed System Operator (DSO) or a Close Distributed System Operator (CDSO). This includes microgrid concept. A sub scheduling area can contain other sub areas. A sub scheduling area leaf will form the smallest entity of any given energy area." ;
  cims:belongsToCategory er:Package_EquipmentReliabilityProfile ;
  cims:stereotype "NC", <http://iec.ch/TC57/NonStandard/UML#concrete> ;
  rdfs:subClassOf nc:SchedulingArea .

nc:SubstationController a rdfs:Class ;
  rdfs:label "SubstationController"@en ;
  rdfs:comment "Substation controller is controlling the equipment to optimize the use of the controlling equipment within a substation. " ;
  cims:belongsToCategory er:Package_EquipmentReliabilityProfile ;
  cims:stereotype "NC", <http://iec.ch/TC57/NonStandard/UML#concrete> ;
  rdfs:subClassOf nc:EquipmentController .

nc:SynchronousArea a rdfs:Class ;
  rdfs:label "SynchronousArea"@en ;
  rdfs:comment "A synchronous area is an electrical area covered by interconnect with a common system frequency in a steady-state. " ;
  cims:belongsToCategory er:Package_EquipmentReliabilityProfile ;
  cims:stereotype "NC", <http://iec.ch/TC57/NonStandard/UML#concrete> ;
  rdfs:subClassOf cim:PowerSystemResource .

nc:SystemControl a rdfs:Class ;
  rdfs:label "SystemControl"@en ;
  rdfs:comment """System control is the management and regulation of various parameters within the electrical grid to ensure its stable and reliable operation. The primary goal of system control is to maintain the balance between electricity generation and consumption, while also managing factors such as voltage, frequency, and power quality. This involves the use of control devices, automation, and monitoring systems to respond to changes in the grid and maintain its overall stability.
This serves as Integrated AC and DC control system (IEC 60633) which governs the integrated operation of AC and DC systems of a power system.""" ;
  cims:belongsToCategory er:Package_EquipmentReliabilityProfile ;
  cims:stereotype "NC" ;
  rdfs:subClassOf nc:AutomationFunction .

nc:SystemOperationCoordinator a rdfs:Class ;
  rdfs:label "SystemOperationCoordinator"@en ;
  rdfs:comment "A role that coordinates relevant information and impact in regards to operating the power system." ;
  cims:belongsToCategory er:Package_EquipmentReliabilityProfile ;
  cims:stereotype "NC" ;
  rdfs:subClassOf nc:PowerSystemOrganisationRole .

nc:SystemOperator a rdfs:Class ;
  rdfs:label "SystemOperator"@en ;
  rdfs:comment "System operator." ;
  cims:belongsToCategory er:Package_EquipmentReliabilityProfile ;
  cims:stereotype "NC" ;
  rdfs:subClassOf nc:PowerSystemOrganisationRole .

nc:TCSCCompensationPoint a rdfs:Class ;
  rdfs:label "TCSCCompensationPoint"@en ;
  rdfs:comment "Compensation point of a TCSC compensator." ;
  cims:belongsToCategory er:Package_EquipmentReliabilityProfile ;
  cims:stereotype "NC", <http://iec.ch/TC57/NonStandard/UML#concrete> .

nc:TCSCController a rdfs:Class ;
  rdfs:label "TCSCController"@en ;
  rdfs:comment "TCSC controller is controlling the equipment to optimize the performance of the TCSC. " ;
  cims:belongsToCategory er:Package_EquipmentReliabilityProfile ;
  cims:stereotype "NC", <http://iec.ch/TC57/NonStandard/UML#concrete> ;
  rdfs:subClassOf nc:EquipmentController .

nc:TapChangerController a rdfs:Class ;
  rdfs:label "TapChangerController"@en ;
  rdfs:comment "Tap changer controller is an equipment controller that controls a tap changer, e.g. how the voltage at the end of a line varies with the load level and compensation of the voltage drop by tap adjustment." ;
  cims:belongsToCategory er:Package_EquipmentReliabilityProfile ;
  cims:stereotype "NC", <http://iec.ch/TC57/NonStandard/UML#concrete> ;
  rdfs:subClassOf nc:EquipmentController .

nc:ThyristorControlledSeriesCompensator a rdfs:Class ;
  rdfs:label "ThyristorControlledSeriesCompensator"@en ;
  rdfs:comment "Thyristor-controlled series capacitors (TCSC) is a type of flexible AC transmission system regulating equipment that is configured with controlled reactors in parallel with sections of a capacitor bank. This combination allows smooth control of the fundamental frequency capacitive reactance over a wide range. The thyristor valve contains a string of series connected high power thyristors. TCSC can control power flows in order to achieve eliminating of line overloads, reducing loop flows and minimising system losses." ;
  cims:belongsToCategory er:Package_EquipmentReliabilityProfile ;
  cims:stereotype "NC", <http://iec.ch/TC57/NonStandard/UML#concrete> ;
  rdfs:subClassOf nc:FACTSEquipment .

nc:TieCorridor a rdfs:Class ;
  rdfs:label "TieCorridor"@en ;
  rdfs:comment "A collection of one or more tie-lines or direct current poles that connect two different control areas." ;
  cims:belongsToCategory er:Package_EquipmentReliabilityProfile ;
  cims:stereotype "NC", <http://iec.ch/TC57/NonStandard/UML#concrete> ;
  rdfs:subClassOf cim:PowerSystemResource .

nc:TransmissionSystemOperator a rdfs:Class ;
  rdfs:label "TransmissionSystemOperator"@en ;
  rdfs:comment "A system operator role that is responsible for operating of an energy transmission network." ;
  cims:belongsToCategory er:Package_EquipmentReliabilityProfile ;
  cims:stereotype "NC", <http://iec.ch/TC57/NonStandard/UML#concrete> ;
  rdfs:subClassOf nc:SystemOperator .

nc:UnifiedPowerFlowController a rdfs:Class ;
  rdfs:label "UnifiedPowerFlowController"@en ;
  rdfs:comment "Unified power flow controller (UPFC) is providing fast-acting reactive power compensation on high-voltage electricity transmission networks. " ;
  cims:belongsToCategory er:Package_EquipmentReliabilityProfile ;
  cims:stereotype "NC", <http://iec.ch/TC57/NonStandard/UML#concrete> ;
  rdfs:subClassOf nc:EquipmentController .

nc:VoltageAngleLimit a rdfs:Class ;
  rdfs:label "VoltageAngleLimit"@en ;
  rdfs:comment "Voltage angle limit between two terminals. The association end OperationalLimitSet.Terminal defines one end and the host of the limit. The association end VoltageAngleLimit.AngleReferenceTerminal defines the reference terminal." ;
  cims:belongsToCategory er:Package_EquipmentReliabilityProfile ;
  cims:stereotype "NC", <http://iec.ch/TC57/NonStandard/UML#concrete> ;
  rdfs:subClassOf cim:OperationalLimit .

nc:VoltageControlFunction a rdfs:Class ;
  rdfs:label "VoltageControlFunction"@en ;
  rdfs:comment "Voltage control function is a function block that calculate the operating point of the controlled equipment to achieve the target voltage." ;
  cims:belongsToCategory er:Package_EquipmentReliabilityProfile ;
  cims:stereotype "NC", <http://iec.ch/TC57/NonStandard/UML#concrete> ;
  rdfs:subClassOf nc:ControlFunctionBlock .

nc:VoltageInjectionControlFunction a rdfs:Class ;
  rdfs:label "VoltageInjectionControlFunction"@en ;
  rdfs:comment "Voltage injection control function is a function block that calculates the operating point of the controlled equipment to achieve the target voltage injection. The controlled point is the Terminal with sequenceNumber =1." ;
  cims:belongsToCategory er:Package_EquipmentReliabilityProfile ;
  cims:stereotype "NC", <http://iec.ch/TC57/NonStandard/UML#concrete> ;
  rdfs:subClassOf nc:ControlFunctionBlock .

profcim:IRI a rdfs:Class ;
  rdfs:label "IRI"@en ;
  rdfs:comment """An IRI (Internationalized Resource Identifier) within an RDF graph is a Unicode string that conforms to the syntax defined in RFC 3987.
The primitive is serialized as rdf:resource in RDFXML.
IRIs in the RDF abstract syntax must be absolute, and may contain a fragment identifier.
IRI equality: Two IRIs are equal if and only if they are equivalent under Simple String Comparison according to section 5.1 of [RFC3987]. Further normalization must not be performed when comparing IRIs for equality.
IRIs are a generalization of URIs [RFC3986] that permits a wider range of Unicode characters. Every absolute URI and URL is an IRI, but not every IRI is an URI. When IRIs are used in operations that are only defined for URIs, they must first be converted according to the mapping defined in section 3.1 of [RFC3987]. A notable example is retrieval over the HTTP protocol. The mapping involves UTF-8 encoding of non-ASCII characters, %-encoding of octets not allowed in URIs, and Punycode-encoding of domain names.""" ;
  cims:belongsToCategory er:Package_EquipmentReliabilityProfile ;
  cims:stereotype "Primitive", "profcim" .

profcim:StringFixedLanguage a rdfs:Class ;
  rdfs:label "StringFixedLanguage"@en ;
  rdfs:comment """A string consisting of a sequence of characters. The character encoding is UTF-8. The string length is unspecified and unlimited.
The primitive is serialized as literal without language support.""" ;
  cims:belongsToCategory er:Package_DocEquipmentReliabilityProfile ;
  cims:stereotype "Primitive", "profcim" .

profcim:StringIRI a rdfs:Class ;
  rdfs:label "StringIRI"@en ;
  rdfs:comment """An IRI (Internationalized Resource Identifier) within an RDF graph is a Unicode string that conforms to the syntax defined in RFC 3987.
The primitive is serialized as literal without language support.
IRIs in the RDF abstract syntax must be absolute, and may contain a fragment identifier.
IRI equality: Two IRIs are equal if and only if they are equivalent under Simple String Comparison according to section 5.1 of [RFC3987]. Further normalization must not be performed when comparing IRIs for equality.
IRIs are a generalization of URIs [RFC3986] that permits a wider range of Unicode characters. Every absolute URI and URL is an IRI, but not every IRI is an URI. When IRIs are used in operations that are only defined for URIs, they must first be converted according to the mapping defined in section 3.1 of [RFC3987]. A notable example is retrieval over the HTTP protocol. The mapping involves UTF-8 encoding of non-ASCII characters, %-encoding of octets not allowed in URIs, and Punycode-encoding of domain names.""" ;
  cims:belongsToCategory er:Package_DocEquipmentReliabilityProfile ;
  cims:stereotype "Primitive", "profcim" .

profcim:URL a rdfs:Class ;
  rdfs:label "URL"@en ;
  rdfs:comment "A Uniform Resource Locator (URL), colloquially termed a web address, is a reference to a web resource that specifies its location on a computer network and a mechanism for retrieving it. A URL is a specific type of Uniform Resource Identifier (URI), although many people use the two terms interchangeably.URLs occur most commonly to reference web pages (http), but are also used for file transfer (ftp), email (mailto), database access (JDBC), and many other applications." ;
  cims:belongsToCategory er:Package_DocEquipmentReliabilityProfile ;
  cims:stereotype "Primitive", "profcim" .

er:Ontology a owl:Ontology ;
  dcat:keyword "ER" ;
  dcat:theme "vocabulary"@en ;
  dcterms:conformsTo "file://CIM100_CGMES31v01_501-20v02_NC23v62_MM10v01.eap", "file://iec61970cim17v40_iec61968cim13v13a_iec62325cim03v17a.eap", "urn:iso:std:iec:61970-301:ed-7:amd1", "urn:iso:std:iec:61970-401:draft:ed-1", "urn:iso:std:iec:61970-501:draft:ed-2", "urn:iso:std:iec:61970-600-2:ed-1" ;
  dcterms:creator "ENTSO-E CIM WG NC project"@en ;
  dcterms:description "This vocabulary is describing the equipment reliability profile."@en ;
  dcterms:identifier "urn:uuid:5f727c5c-b49f-47be-b750-a00fefb7e806" ;
  dcterms:language "en-GB" ;
  dcterms:license "https://www.apache.org/licenses/LICENSE-2.0"@en ;
  dcterms:modified "2024-09-07"^^<http://www.w3.org/2001/XMLSchema#date> ;
  dcterms:publisher "ENTSO-E"@en ;
  dcterms:rightsHolder "ENTSO-E"@en ;
  dcterms:title "Equipment Reliability Vocabulary"@en ;
  owl:priorVersion <http://entsoe.eu/ns/CIM/EquipmentReliability-EU/2.2> ;
  owl:versionIRI <https://ap-voc.cim4.eu/EquipmentReliability/2.3> ;
  owl:versionInfo "2.3.1"@en .

cim:ACDCTerminal.OperationalLimitSet a rdf:Property ;
  rdfs:label "OperationalLimitSet"@en ;
  rdfs:comment "The operational limit sets at the terminal." ;
  cims:AssociationUsed "No" ;
  cims:inverseRoleName cim:OperationalLimitSet.Terminal ;
  cims:multiplicity cims:M:0..n ;
  rdfs:domain cim:ACDCTerminal ;
  rdfs:range cim:OperationalLimitSet .

cim:ActivePower.multiplier a rdf:Property ;
  rdfs:label "multiplier"@en ;
  cims:isFixed "M" ;
  cims:multiplicity cims:M:0..1 ;
  cims:stereotype <http://iec.ch/TC57/NonStandard/UML#attribute> ;
  rdfs:domain cim:ActivePower ;
  rdfs:range cim:UnitMultiplier .

cim:ActivePower.unit a rdf:Property ;
  rdfs:label "unit"@en ;
  cims:isFixed "W" ;
  cims:multiplicity cims:M:0..1 ;
  cims:stereotype <http://iec.ch/TC57/NonStandard/UML#attribute> ;
  rdfs:domain cim:ActivePower ;
  rdfs:range cim:UnitSymbol .

cim:ActivePower.value a rdf:Property ;
  rdfs:label "value"@en ;
  cims:dataType cim:Float ;
  cims:multiplicity cims:M:0..1 ;
  cims:stereotype <http://iec.ch/TC57/NonStandard/UML#attribute> ;
  rdfs:domain cim:ActivePower .

cim:ActivePowerChangeRate.multiplier a rdf:Property ;
  rdfs:label "multiplier"@en ;
  cims:isFixed "M" ;
  cims:multiplicity cims:M:0..1 ;
  cims:stereotype <http://iec.ch/TC57/NonStandard/UML#attribute> ;
  rdfs:domain cim:ActivePowerChangeRate ;
  rdfs:range cim:UnitMultiplier .

cim:ActivePowerChangeRate.unit a rdf:Property ;
  rdfs:label "unit"@en ;
  cims:isFixed "WPers" ;
  cims:multiplicity cims:M:0..1 ;
  cims:stereotype <http://iec.ch/TC57/NonStandard/UML#attribute> ;
  rdfs:domain cim:ActivePowerChangeRate ;
  rdfs:range cim:UnitSymbol .

cim:ActivePowerChangeRate.value a rdf:Property ;
  rdfs:label "value"@en ;
  cims:dataType cim:Float ;
  cims:multiplicity cims:M:0..1 ;
  cims:stereotype <http://iec.ch/TC57/NonStandard/UML#attribute> ;
  rdfs:domain cim:ActivePowerChangeRate .

cim:AngleDegrees.multiplier a rdf:Property ;
  rdfs:label "multiplier"@en ;
  cims:isFixed "none" ;
  cims:multiplicity cims:M:0..1 ;
  cims:stereotype <http://iec.ch/TC57/NonStandard/UML#attribute> ;
  rdfs:domain cim:AngleDegrees ;
  rdfs:range cim:UnitMultiplier .

cim:AngleDegrees.unit a rdf:Property ;
  rdfs:label "unit"@en ;
  cims:isFixed "deg" ;
  cims:multiplicity cims:M:0..1 ;
  cims:stereotype <http://iec.ch/TC57/NonStandard/UML#attribute> ;
  rdfs:domain cim:AngleDegrees ;
  rdfs:range cim:UnitSymbol .

cim:AngleDegrees.value a rdf:Property ;
  rdfs:label "value"@en ;
  cims:dataType cim:Float ;
  cims:multiplicity cims:M:0..1 ;
  cims:stereotype <http://iec.ch/TC57/NonStandard/UML#attribute> ;
  rdfs:domain cim:AngleDegrees .

cim:CurrentFlow.multiplier a rdf:Property ;
  rdfs:label "multiplier"@en ;
  cims:isFixed "none" ;
  cims:multiplicity cims:M:0..1 ;
  cims:stereotype <http://iec.ch/TC57/NonStandard/UML#attribute> ;
  rdfs:domain cim:CurrentFlow ;
  rdfs:range cim:UnitMultiplier .

cim:CurrentFlow.unit a rdf:Property ;
  rdfs:label "unit"@en ;
  cims:isFixed "A" ;
  cims:multiplicity cims:M:0..1 ;
  cims:stereotype <http://iec.ch/TC57/NonStandard/UML#attribute> ;
  rdfs:domain cim:CurrentFlow ;
  rdfs:range cim:UnitSymbol .

cim:CurrentFlow.value a rdf:Property ;
  rdfs:label "value"@en ;
  cims:dataType cim:Float ;
  cims:multiplicity cims:M:0..1 ;
  cims:stereotype <http://iec.ch/TC57/NonStandard/UML#attribute> ;
  rdfs:domain cim:CurrentFlow .

cim:Curve.CurveDatas a rdf:Property ;
  rdfs:label "CurveDatas"@en ;
  rdfs:comment "The point data values that define this curve." ;
  cims:AssociationUsed "No" ;
  cims:inverseRoleName cim:CurveData.Curve ;
  cims:multiplicity cims:M:1..n ;
  rdfs:domain cim:Curve ;
  rdfs:range cim:CurveData .

cim:Curve.curveStyle a rdf:Property ;
  rdfs:label "curveStyle"@en ;
  rdfs:comment "The style or shape of the curve." ;
  cims:multiplicity cims:M:1..1 ;
  cims:stereotype <http://iec.ch/TC57/NonStandard/UML#attribute> ;
  rdfs:domain cim:Curve ;
  rdfs:range cim:CurveStyle .

cim:Curve.xMultiplier a rdf:Property ;
  rdfs:label "xMultiplier"@en ;
  rdfs:comment "Multiplier for X-axis." ;
  cims:multiplicity cims:M:0..1 ;
  cims:stereotype <http://iec.ch/TC57/NonStandard/UML#attribute> ;
  rdfs:domain cim:Curve ;
  rdfs:range cim:UnitMultiplier .

cim:Curve.xUnit a rdf:Property ;
  rdfs:label "xUnit"@en ;
  rdfs:comment "The X-axis units of measure." ;
  cims:multiplicity cims:M:1..1 ;
  cims:stereotype <http://iec.ch/TC57/NonStandard/UML#attribute> ;
  rdfs:domain cim:Curve ;
  rdfs:range cim:UnitSymbol .

cim:Curve.y1Multiplier a rdf:Property ;
  rdfs:label "y1Multiplier"@en ;
  rdfs:comment "Multiplier for Y1-axis." ;
  cims:multiplicity cims:M:0..1 ;
  cims:stereotype <http://iec.ch/TC57/NonStandard/UML#attribute> ;
  rdfs:domain cim:Curve ;
  rdfs:range cim:UnitMultiplier .

cim:Curve.y1Unit a rdf:Property ;
  rdfs:label "y1Unit"@en ;
  rdfs:comment "The Y1-axis units of measure." ;
  cims:multiplicity cims:M:0..1 ;
  cims:stereotype <http://iec.ch/TC57/NonStandard/UML#attribute> ;
  rdfs:domain cim:Curve ;
  rdfs:range cim:UnitSymbol .

cim:Curve.y2Multiplier a rdf:Property ;
  rdfs:label "y2Multiplier"@en ;
  rdfs:comment "Multiplier for Y2-axis." ;
  cims:multiplicity cims:M:0..1 ;
  cims:stereotype <http://iec.ch/TC57/NonStandard/UML#attribute> ;
  rdfs:domain cim:Curve ;
  rdfs:range cim:UnitMultiplier .

cim:Curve.y2Unit a rdf:Property ;
  rdfs:label "y2Unit"@en ;
  rdfs:comment "The Y2-axis units of measure." ;
  cims:multiplicity cims:M:0..1 ;
  cims:stereotype <http://iec.ch/TC57/NonStandard/UML#attribute> ;
  rdfs:domain cim:Curve ;
  rdfs:range cim:UnitSymbol .

cim:CurveData.Curve a rdf:Property ;
  rdfs:label "Curve"@en ;
  rdfs:comment "The curve of  this curve data point." ;
  cims:AssociationUsed "Yes" ;
  cims:inverseRoleName cim:Curve.CurveDatas ;
  cims:multiplicity cims:M:1 ;
  rdfs:domain cim:CurveData ;
  rdfs:range cim:Curve .

cim:CurveData.xvalue a rdf:Property ;
  rdfs:label "xvalue"@en ;
  rdfs:comment "The data value of the X-axis variable,  depending on the X-axis units." ;
  cims:dataType cim:Float ;
  cims:multiplicity cims:M:1..1 ;
  cims:stereotype <http://iec.ch/TC57/NonStandard/UML#attribute> ;
  rdfs:domain cim:CurveData .

cim:CurveData.y1value a rdf:Property ;
  rdfs:label "y1value"@en ;
  rdfs:comment "The data value of the  first Y-axis variable, depending on the Y-axis units." ;
  cims:dataType cim:Float ;
  cims:multiplicity cims:M:1..1 ;
  cims:stereotype <http://iec.ch/TC57/NonStandard/UML#attribute> ;
  rdfs:domain cim:CurveData .

cim:CurveData.y2value a rdf:Property ;
  rdfs:label "y2value"@en ;
  rdfs:comment "The data value of the second Y-axis variable (if present), depending on the Y-axis units." ;
  cims:dataType cim:Float ;
  cims:multiplicity cims:M:0..1 ;
  cims:stereotype <http://iec.ch/TC57/NonStandard/UML#attribute> ;
  rdfs:domain cim:CurveData .

cim:DCConductingEquipment.ratedCurrent a rdf:Property ;
  rdfs:label "ratedCurrent"@en ;
  rdfs:comment """The maximum continuous current carrying capacity in amps governed by the device material and construction.
The attribute shall be a positive value.""" ;
  cims:dataType cim:CurrentFlow ;
  cims:multiplicity cims:M:0..1 ;
  cims:stereotype <http://iec.ch/TC57/NonStandard/UML#attribute> ;
  rdfs:domain cim:DCConductingEquipment .

cim:DCConverterUnit.Substation a rdf:Property ;
  rdfs:label "Substation"@en ;
  rdfs:comment "The containing substation of the DC converter unit." ;
  cims:AssociationUsed "Yes" ;
  cims:inverseRoleName cim:Substation.DCConverterUnit ;
  cims:multiplicity cims:M:0..1 ;
  rdfs:domain cim:DCConverterUnit ;
  rdfs:range cim:Substation .

cim:Equipment.AggregatedEquipment a rdf:Property ;
  rdfs:label "AggregatedEquipment"@en ;
  rdfs:comment "An aggregated representation of the detailed equipment." ;
  cims:AssociationUsed "Yes" ;
  cims:inverseRoleName cim:Equipment.DetailedEquipment ;
  cims:multiplicity cims:M:0..1 ;
  cims:stereotype "NC" ;
  rdfs:domain cim:Equipment ;
  rdfs:range cim:Equipment .

cim:Equipment.DetailedEquipment a rdf:Property ;
  rdfs:label "DetailedEquipment"@en ;
  rdfs:comment "A detailed representation of the aggregated equipment." ;
  cims:AssociationUsed "No" ;
  cims:inverseRoleName cim:Equipment.AggregatedEquipment ;
  cims:multiplicity cims:M:0..n ;
  cims:stereotype "NC" ;
  rdfs:domain cim:Equipment ;
  rdfs:range cim:Equipment .

cim:EquivalentInjection.ReactiveCapabilityCurve2 a rdf:Property ;
  rdfs:label "ReactiveCapabilityCurve2"@en ;
  rdfs:comment "The reactive capability curve used by this equivalent injection." ;
  cims:AssociationUsed "No" ;
  cims:inverseRoleName cim:ReactiveCapabilityCurve.EquivalentInjection2 ;
  cims:multiplicity cims:M:0..n ;
  cims:stereotype "NC" ;
  rdfs:domain cim:EquivalentInjection ;
  rdfs:range cim:ReactiveCapabilityCurve .

cim:Feeder.NamingSecondarySubstation a rdf:Property ;
  rdfs:label "NamingSecondarySubstation"@en ;
  rdfs:comment "The secondary substations that are normally energized from the feeder.  Used for naming purposes.   Should be consistent with the other associations for energizing terminal specification and the feeder energization specification." ;
  cims:AssociationUsed "Yes" ;
  cims:inverseRoleName cim:Substation.NamingFeeder ;
  cims:multiplicity cims:M:0..n ;
  rdfs:domain cim:Feeder ;
  rdfs:range cim:Substation .

cim:Feeder.NormalEnergizedSubstation a rdf:Property ;
  rdfs:label "NormalEnergizedSubstation"@en ;
  rdfs:comment "The substations that are normally energized by the feeder." ;
  cims:AssociationUsed "Yes" ;
  cims:inverseRoleName cim:Substation.NormalEnergizingFeeder ;
  cims:multiplicity cims:M:0..n ;
  rdfs:domain cim:Feeder ;
  rdfs:range cim:Substation .

cim:Feeder.NormalEnergizingSubstation a rdf:Property ;
  rdfs:label "NormalEnergizingSubstation"@en ;
  rdfs:comment "The substation that nominally energizes the feeder.  Also used for naming purposes." ;
  cims:AssociationUsed "Yes" ;
  cims:inverseRoleName cim:Substation.NormalEnergizedFeeder ;
  cims:multiplicity cims:M:0..1 ;
  rdfs:domain cim:Feeder ;
  rdfs:range cim:Substation .

cim:Frequency.multiplier a rdf:Property ;
  rdfs:label "multiplier"@en ;
  cims:isFixed "none" ;
  cims:multiplicity cims:M:0..1 ;
  cims:stereotype <http://iec.ch/TC57/NonStandard/UML#attribute> ;
  rdfs:domain cim:Frequency ;
  rdfs:range cim:UnitMultiplier .

cim:Frequency.unit a rdf:Property ;
  rdfs:label "unit"@en ;
  cims:isFixed "Hz" ;
  cims:multiplicity cims:M:0..1 ;
  cims:stereotype <http://iec.ch/TC57/NonStandard/UML#attribute> ;
  rdfs:domain cim:Frequency ;
  rdfs:range cim:UnitSymbol .

cim:Frequency.value a rdf:Property ;
  rdfs:label "value"@en ;
  cims:dataType cim:Float ;
  cims:multiplicity cims:M:0..1 ;
  cims:stereotype <http://iec.ch/TC57/NonStandard/UML#attribute> ;
  rdfs:domain cim:Frequency .

cim:GeneratingUnit.lowerRampRate a rdf:Property ;
  rdfs:label "lowerRampRate"@en ;
  rdfs:comment "The normal maximum rate the generating unit active power output can be lowered by control actions." ;
  cims:dataType cim:ActivePowerChangeRate ;
  cims:multiplicity cims:M:0..1 ;
  cims:stereotype <http://iec.ch/TC57/NonStandard/UML#attribute> ;
  rdfs:domain cim:GeneratingUnit .

cim:GeneratingUnit.maxEconomicP a rdf:Property ;
  rdfs:label "maxEconomicP"@en ;
  rdfs:comment "Maximum high economic active power limit, that should not exceed the maximum operating active power limit." ;
  cims:dataType cim:ActivePower ;
  cims:multiplicity cims:M:0..1 ;
  cims:stereotype <http://iec.ch/TC57/NonStandard/UML#attribute> ;
  rdfs:domain cim:GeneratingUnit .

cim:GeneratingUnit.minEconomicP a rdf:Property ;
  rdfs:label "minEconomicP"@en ;
  rdfs:comment "Low economic active power limit that shall be greater than or equal to the minimum operating active power limit." ;
  cims:dataType cim:ActivePower ;
  cims:multiplicity cims:M:0..1 ;
  cims:stereotype <http://iec.ch/TC57/NonStandard/UML#attribute> ;
  rdfs:domain cim:GeneratingUnit .

cim:GeneratingUnit.minimumOffTime a rdf:Property ;
  rdfs:label "minimumOffTime"@en ;
  rdfs:comment "Minimum time interval between unit shutdown and startup." ;
  cims:dataType cim:Seconds ;
  cims:multiplicity cims:M:0..1 ;
  cims:stereotype <http://iec.ch/TC57/NonStandard/UML#attribute> ;
  rdfs:domain cim:GeneratingUnit .

cim:GeneratingUnit.raiseRampRate a rdf:Property ;
  rdfs:label "raiseRampRate"@en ;
  rdfs:comment "The normal maximum rate the generating unit active power output can be raised by control actions." ;
  cims:dataType cim:ActivePowerChangeRate ;
  cims:multiplicity cims:M:0..1 ;
  cims:stereotype <http://iec.ch/TC57/NonStandard/UML#attribute> ;
  rdfs:domain cim:GeneratingUnit .

cim:HydroPowerPlant.Reservoir a rdf:Property ;
  rdfs:label "Reservoir"@en ;
  rdfs:comment "Generators discharge water to or pumps are supplied water from a downstream reservoir." ;
  cims:AssociationUsed "Yes" ;
  cims:inverseRoleName cim:Reservoir.HydroPowerPlants ;
  cims:multiplicity cims:M:0..1 ;
  rdfs:domain cim:HydroPowerPlant ;
  rdfs:range cim:Reservoir .

cim:IdentifiedObject.description a rdf:Property ;
  rdfs:label "description"@en ;
  rdfs:comment "The description is a free human readable text describing or naming the object. It may be non unique and may not correlate to a naming hierarchy." ;
  cims:dataType cim:String ;
  cims:multiplicity cims:M:0..1 ;
  cims:stereotype <http://iec.ch/TC57/NonStandard/UML#attribute> ;
  rdfs:domain cim:IdentifiedObject .

cim:IdentifiedObject.mRID a rdf:Property ;
  rdfs:label "mRID"@en ;
  rdfs:comment """Master resource identifier issued by a model authority. The mRID is unique within an exchange context. Global uniqueness is easily achieved by using a UUID, as specified in RFC 4122, for the mRID. The use of UUID is strongly recommended.
For CIMXML data files in RDF syntax conforming to IEC 61970-552, the mRID is mapped to rdf:ID or rdf:about attributes that identify CIM object elements.""" ;
  cims:dataType cim:String ;
  cims:multiplicity cims:M:1..1 ;
  cims:stereotype <http://iec.ch/TC57/NonStandard/UML#attribute> ;
  rdfs:domain cim:IdentifiedObject .

cim:IdentifiedObject.name a rdf:Property ;
  rdfs:label "name"@en ;
  rdfs:comment "The name is any free human readable and possibly non unique text naming the object." ;
  cims:dataType cim:String ;
  cims:multiplicity cims:M:0..1 ;
  cims:stereotype <http://iec.ch/TC57/NonStandard/UML#attribute> ;
  rdfs:domain cim:IdentifiedObject .

cim:Impedance.multiplier a rdf:Property ;
  rdfs:label "multiplier"@en ;
  cims:isFixed "none" ;
  cims:multiplicity cims:M:0..1 ;
  cims:stereotype <http://iec.ch/TC57/NonStandard/UML#attribute> ;
  rdfs:domain cim:Impedance ;
  rdfs:range cim:UnitMultiplier .

cim:Impedance.unit a rdf:Property ;
  rdfs:label "unit"@en ;
  cims:isFixed "ohm" ;
  cims:multiplicity cims:M:0..1 ;
  cims:stereotype <http://iec.ch/TC57/NonStandard/UML#attribute> ;
  rdfs:domain cim:Impedance ;
  rdfs:range cim:UnitSymbol .

cim:Impedance.value a rdf:Property ;
  rdfs:label "value"@en ;
  cims:dataType cim:Float ;
  cims:multiplicity cims:M:0..1 ;
  cims:stereotype <http://iec.ch/TC57/NonStandard/UML#attribute> ;
  rdfs:domain cim:Impedance .

cim:Money.multiplier a rdf:Property ;
  rdfs:label "multiplier"@en ;
  cims:isFixed "none" ;
  cims:multiplicity cims:M:0..1 ;
  cims:stereotype <http://iec.ch/TC57/NonStandard/UML#attribute> ;
  rdfs:domain cim:Money ;
  rdfs:range cim:UnitMultiplier .

cim:Money.unit a rdf:Property ;
  rdfs:label "unit"@en ;
  cims:multiplicity cims:M:0..1 ;
  cims:stereotype <http://iec.ch/TC57/NonStandard/UML#attribute> ;
  rdfs:domain cim:Money ;
  rdfs:range cim:Currency .

cim:Money.value a rdf:Property ;
  rdfs:label "value"@en ;
  cims:dataType cim:Decimal ;
  cims:multiplicity cims:M:0..1 ;
  cims:stereotype <http://iec.ch/TC57/NonStandard/UML#attribute> ;
  rdfs:domain cim:Money .

cim:OperationalLimit.OperationalLimitSet a rdf:Property ;
  rdfs:label "OperationalLimitSet"@en ;
  rdfs:comment "The limit set to which the limit values belong." ;
  cims:AssociationUsed "Yes" ;
  cims:inverseRoleName cim:OperationalLimitSet.OperationalLimitValue ;
  cims:multiplicity cims:M:1 ;
  rdfs:domain cim:OperationalLimit ;
  rdfs:range cim:OperationalLimitSet .

cim:OperationalLimit.OperationalLimitType a rdf:Property ;
  rdfs:label "OperationalLimitType"@en ;
  rdfs:comment "The limit type associated with this limit." ;
  cims:AssociationUsed "Yes" ;
  cims:inverseRoleName cim:OperationalLimitType.OperationalLimit ;
  cims:multiplicity cims:M:1 ;
  rdfs:domain cim:OperationalLimit ;
  rdfs:range cim:OperationalLimitType .

cim:OperationalLimitSet.OperationalLimitValue a rdf:Property ;
  rdfs:label "OperationalLimitValue"@en ;
  rdfs:comment "Values of equipment limits." ;
  cims:AssociationUsed "No" ;
  cims:inverseRoleName cim:OperationalLimit.OperationalLimitSet ;
  cims:multiplicity cims:M:1..n ;
  cims:stereotype <http://iec.ch/TC57/NonStandard/UML#ofAggregate> ;
  rdfs:domain cim:OperationalLimitSet ;
  rdfs:range cim:OperationalLimit .

cim:OperationalLimitSet.Terminal a rdf:Property ;
  rdfs:label "Terminal"@en ;
  rdfs:comment "The terminal where the operational limit set apply." ;
  cims:AssociationUsed "Yes" ;
  cims:inverseRoleName cim:ACDCTerminal.OperationalLimitSet ;
  cims:multiplicity cims:M:1 ;
  rdfs:domain cim:OperationalLimitSet ;
  rdfs:range cim:ACDCTerminal .

cim:OperationalLimitType.OperationalLimit a rdf:Property ;
  rdfs:label "OperationalLimit"@en ;
  rdfs:comment "The operational limits associated with this type of limit." ;
  cims:AssociationUsed "No" ;
  cims:inverseRoleName cim:OperationalLimit.OperationalLimitType ;
  cims:multiplicity cims:M:1..n ;
  rdfs:domain cim:OperationalLimitType ;
  rdfs:range cim:OperationalLimit .

cim:OperationalLimitType.direction a rdf:Property ;
  rdfs:label "direction"@en ;
  rdfs:comment "The direction of the limit." ;
  cims:multiplicity cims:M:1..1 ;
  cims:stereotype <http://iec.ch/TC57/NonStandard/UML#attribute> ;
  rdfs:domain cim:OperationalLimitType ;
  rdfs:range cim:OperationalLimitDirectionKind .

cim:Organisation.Roles a rdf:Property ;
  rdfs:label "Roles"@en ;
  rdfs:comment "All roles of this organisation." ;
  cims:AssociationUsed "No" ;
  cims:inverseRoleName cim:OrganisationRole.Organisation ;
  cims:multiplicity cims:M:0..n ;
  rdfs:domain cim:Organisation ;
  rdfs:range cim:OrganisationRole .

cim:OrganisationRole.Organisation a rdf:Property ;
  rdfs:label "Organisation"@en ;
  rdfs:comment "Organisation having this role." ;
  cims:AssociationUsed "Yes" ;
  cims:inverseRoleName cim:Organisation.Roles ;
  cims:multiplicity cims:M:0..1 ;
  rdfs:domain cim:OrganisationRole ;
  rdfs:range cim:Organisation .

cim:PU.multiplier a rdf:Property ;
  rdfs:label "multiplier"@en ;
  cims:isFixed "none" ;
  cims:multiplicity cims:M:0..1 ;
  cims:stereotype <http://iec.ch/TC57/NonStandard/UML#attribute> ;
  rdfs:domain cim:PU ;
  rdfs:range cim:UnitMultiplier .

cim:PU.unit a rdf:Property ;
  rdfs:label "unit"@en ;
  cims:isFixed "none" ;
  cims:multiplicity cims:M:0..1 ;
  cims:stereotype <http://iec.ch/TC57/NonStandard/UML#attribute> ;
  rdfs:domain cim:PU ;
  rdfs:range cim:UnitSymbol .

cim:PU.value a rdf:Property ;
  rdfs:label "value"@en ;
  cims:dataType cim:Float ;
  cims:multiplicity cims:M:0..1 ;
  cims:stereotype <http://iec.ch/TC57/NonStandard/UML#attribute> ;
  rdfs:domain cim:PU .

cim:PerCent.multiplier a rdf:Property ;
  rdfs:label "multiplier"@en ;
  cims:isFixed "none" ;
  cims:multiplicity cims:M:0..1 ;
  cims:stereotype <http://iec.ch/TC57/NonStandard/UML#attribute> ;
  rdfs:domain cim:PerCent ;
  rdfs:range cim:UnitMultiplier .

cim:PerCent.unit a rdf:Property ;
  rdfs:label "unit"@en ;
  cims:isFixed "none" ;
  cims:multiplicity cims:M:0..1 ;
  cims:stereotype <http://iec.ch/TC57/NonStandard/UML#attribute> ;
  rdfs:domain cim:PerCent ;
  rdfs:range cim:UnitSymbol .

cim:PerCent.value a rdf:Property ;
  rdfs:label "value"@en ;
  rdfs:comment "Normally 0 to 100 on a defined base." ;
  cims:dataType cim:Float ;
  cims:multiplicity cims:M:0..1 ;
  cims:stereotype <http://iec.ch/TC57/NonStandard/UML#attribute> ;
  rdfs:domain cim:PerCent .

cim:Pressure.multiplier a rdf:Property ;
  rdfs:label "multiplier"@en ;
  cims:isFixed "k" ;
  cims:multiplicity cims:M:0..1 ;
  cims:stereotype <http://iec.ch/TC57/NonStandard/UML#attribute> ;
  rdfs:domain cim:Pressure ;
  rdfs:range cim:UnitMultiplier .

cim:Pressure.unit a rdf:Property ;
  rdfs:label "unit"@en ;
  cims:isFixed "Pa" ;
  cims:multiplicity cims:M:0..1 ;
  cims:stereotype <http://iec.ch/TC57/NonStandard/UML#attribute> ;
  rdfs:domain cim:Pressure ;
  rdfs:range cim:UnitSymbol .

cim:Pressure.value a rdf:Property ;
  rdfs:label "value"@en ;
  cims:dataType cim:Float ;
  cims:multiplicity cims:M:0..1 ;
  cims:stereotype <http://iec.ch/TC57/NonStandard/UML#attribute> ;
  rdfs:domain cim:Pressure .

cim:Reactance.multiplier a rdf:Property ;
  rdfs:label "multiplier"@en ;
  cims:isFixed "none" ;
  cims:multiplicity cims:M:0..1 ;
  cims:stereotype <http://iec.ch/TC57/NonStandard/UML#attribute> ;
  rdfs:domain cim:Reactance ;
  rdfs:range cim:UnitMultiplier .

cim:Reactance.unit a rdf:Property ;
  rdfs:label "unit"@en ;
  cims:isFixed "ohm" ;
  cims:multiplicity cims:M:0..1 ;
  cims:stereotype <http://iec.ch/TC57/NonStandard/UML#attribute> ;
  rdfs:domain cim:Reactance ;
  rdfs:range cim:UnitSymbol .

cim:Reactance.value a rdf:Property ;
  rdfs:label "value"@en ;
  cims:dataType cim:Float ;
  cims:multiplicity cims:M:0..1 ;
  cims:stereotype <http://iec.ch/TC57/NonStandard/UML#attribute> ;
  rdfs:domain cim:Reactance .

cim:ReactiveCapabilityCurve.EquivalentInjection2 a rdf:Property ;
  rdfs:label "EquivalentInjection2"@en ;
  rdfs:comment "The equivalent injection using this reactive capability curve." ;
  cims:AssociationUsed "Yes" ;
  cims:inverseRoleName cim:EquivalentInjection.ReactiveCapabilityCurve2 ;
  cims:multiplicity cims:M:0..1 ;
  cims:stereotype "NC" ;
  rdfs:domain cim:ReactiveCapabilityCurve ;
  rdfs:range cim:EquivalentInjection .

cim:ReactiveCapabilityCurve.SynchronousMachine2 a rdf:Property ;
  rdfs:label "SynchronousMachine2"@en ;
  rdfs:comment "Synchronous machine using this curve." ;
  cims:AssociationUsed "Yes" ;
  cims:inverseRoleName cim:SynchronousMachine.ReactiveCapabilityCurve2 ;
  cims:multiplicity cims:M:0..1 ;
  cims:stereotype "NC" ;
  rdfs:domain cim:ReactiveCapabilityCurve ;
  rdfs:range cim:SynchronousMachine .

cim:ReactiveCapabilityCurve.coolantTemperature a rdf:Property ;
  rdfs:label "coolantTemperature"@en ;
  rdfs:comment "The machine's coolant temperature (e.g., ambient air or stator circulating water)." ;
  cims:dataType cim:Temperature ;
  cims:multiplicity cims:M:0..1 ;
  cims:stereotype <http://iec.ch/TC57/NonStandard/UML#attribute> ;
  rdfs:domain cim:ReactiveCapabilityCurve .

cim:ReactiveCapabilityCurve.hydrogenPressure a rdf:Property ;
  rdfs:label "hydrogenPressure"@en ;
  rdfs:comment "The hydrogen coolant pressure." ;
  cims:dataType cim:Pressure ;
  cims:multiplicity cims:M:0..1 ;
  cims:stereotype <http://iec.ch/TC57/NonStandard/UML#attribute> ;
  rdfs:domain cim:ReactiveCapabilityCurve .

cim:ReactivePower.multiplier a rdf:Property ;
  rdfs:label "multiplier"@en ;
  cims:multiplicity cims:M:0..1 ;
  cims:stereotype <http://iec.ch/TC57/NonStandard/UML#attribute> ;
  rdfs:domain cim:ReactivePower ;
  rdfs:range cim:UnitMultiplier .

cim:ReactivePower.unit a rdf:Property ;
  rdfs:label "unit"@en ;
  cims:isFixed "VAr" ;
  cims:multiplicity cims:M:0..1 ;
  cims:stereotype <http://iec.ch/TC57/NonStandard/UML#attribute> ;
  rdfs:domain cim:ReactivePower ;
  rdfs:range cim:UnitSymbol .

cim:ReactivePower.value a rdf:Property ;
  rdfs:label "value"@en ;
  cims:dataType cim:Float ;
  cims:multiplicity cims:M:0..1 ;
  cims:stereotype <http://iec.ch/TC57/NonStandard/UML#attribute> ;
  rdfs:domain cim:ReactivePower .

cim:Reservoir.HydroPowerPlants a rdf:Property ;
  rdfs:label "HydroPowerPlants"@en ;
  rdfs:comment "Generators discharge water to or pumps are supplied water from a downstream reservoir." ;
  cims:AssociationUsed "No" ;
  cims:inverseRoleName cim:HydroPowerPlant.Reservoir ;
  cims:multiplicity cims:M:0..n ;
  rdfs:domain cim:Reservoir ;
  rdfs:range cim:HydroPowerPlant .

cim:Resistance.multiplier a rdf:Property ;
  rdfs:label "multiplier"@en ;
  cims:isFixed "none" ;
  cims:multiplicity cims:M:0..1 ;
  cims:stereotype <http://iec.ch/TC57/NonStandard/UML#attribute> ;
  rdfs:domain cim:Resistance ;
  rdfs:range cim:UnitMultiplier .

cim:Resistance.unit a rdf:Property ;
  rdfs:label "unit"@en ;
  cims:isFixed "ohm" ;
  cims:multiplicity cims:M:0..1 ;
  cims:stereotype <http://iec.ch/TC57/NonStandard/UML#attribute> ;
  rdfs:domain cim:Resistance ;
  rdfs:range cim:UnitSymbol .

cim:Resistance.value a rdf:Property ;
  rdfs:label "value"@en ;
  cims:dataType cim:Float ;
  cims:multiplicity cims:M:0..1 ;
  cims:stereotype <http://iec.ch/TC57/NonStandard/UML#attribute> ;
  rdfs:domain cim:Resistance .

cim:Seconds.multiplier a rdf:Property ;
  rdfs:label "multiplier"@en ;
  cims:isFixed "none" ;
  cims:multiplicity cims:M:0..1 ;
  cims:stereotype <http://iec.ch/TC57/NonStandard/UML#attribute> ;
  rdfs:domain cim:Seconds ;
  rdfs:range cim:UnitMultiplier .

cim:Seconds.unit a rdf:Property ;
  rdfs:label "unit"@en ;
  cims:isFixed "s" ;
  cims:multiplicity cims:M:0..1 ;
  cims:stereotype <http://iec.ch/TC57/NonStandard/UML#attribute> ;
  rdfs:domain cim:Seconds ;
  rdfs:range cim:UnitSymbol .

cim:Seconds.value a rdf:Property ;
  rdfs:label "value"@en ;
  rdfs:comment "Time, in seconds" ;
  cims:dataType cim:Float ;
  cims:multiplicity cims:M:0..1 ;
  cims:stereotype <http://iec.ch/TC57/NonStandard/UML#attribute> ;
  rdfs:domain cim:Seconds .

cim:Substation.DCConverterUnit a rdf:Property ;
  rdfs:label "DCConverterUnit"@en ;
  rdfs:comment "The DC converter unit belonging of the substation." ;
  cims:AssociationUsed "No" ;
  cims:inverseRoleName cim:DCConverterUnit.Substation ;
  cims:multiplicity cims:M:0..n ;
  rdfs:domain cim:Substation ;
  rdfs:range cim:DCConverterUnit .

cim:Substation.NamingFeeder a rdf:Property ;
  rdfs:label "NamingFeeder"@en ;
  rdfs:comment "The primary feeder that normally energizes the secondary substation. Used for naming purposes.  Either this association or the substation to subgeographical region should be used for hierarchical containment specification." ;
  cims:AssociationUsed "No" ;
  cims:inverseRoleName cim:Feeder.NamingSecondarySubstation ;
  cims:multiplicity cims:M:0..1 ;
  rdfs:domain cim:Substation ;
  rdfs:range cim:Feeder .

cim:Substation.NormalEnergizedFeeder a rdf:Property ;
  rdfs:label "NormalEnergizedFeeder"@en ;
  rdfs:comment "The normal energized feeders of the substation. Also used for naming purposes." ;
  cims:AssociationUsed "No" ;
  cims:inverseRoleName cim:Feeder.NormalEnergizingSubstation ;
  cims:multiplicity cims:M:0..n ;
  rdfs:domain cim:Substation ;
  rdfs:range cim:Feeder .

cim:Substation.NormalEnergizingFeeder a rdf:Property ;
  rdfs:label "NormalEnergizingFeeder"@en ;
  rdfs:comment "The feeders that potentially energize  the downstream substation.  Should be consistent with the associations that describe the naming hierarchy." ;
  cims:AssociationUsed "No" ;
  cims:inverseRoleName cim:Feeder.NormalEnergizedSubstation ;
  cims:multiplicity cims:M:0..n ;
  rdfs:domain cim:Substation ;
  rdfs:range cim:Feeder .

cim:SynchronousMachine.ReactiveCapabilityCurve2 a rdf:Property ;
  rdfs:label "ReactiveCapabilityCurve2"@en ;
  rdfs:comment "Reactive capability curve for this synchronous machine." ;
  cims:AssociationUsed "No" ;
  cims:inverseRoleName cim:ReactiveCapabilityCurve.SynchronousMachine2 ;
  cims:multiplicity cims:M:0..n ;
  cims:stereotype "NC" ;
  rdfs:domain cim:SynchronousMachine ;
  rdfs:range cim:ReactiveCapabilityCurve .

cim:Temperature.multiplier a rdf:Property ;
  rdfs:label "multiplier"@en ;
  cims:isFixed "none" ;
  cims:multiplicity cims:M:0..1 ;
  cims:stereotype <http://iec.ch/TC57/NonStandard/UML#attribute> ;
  rdfs:domain cim:Temperature ;
  rdfs:range cim:UnitMultiplier .

cim:Temperature.unit a rdf:Property ;
  rdfs:label "unit"@en ;
  cims:isFixed "degC" ;
  cims:multiplicity cims:M:0..1 ;
  cims:stereotype <http://iec.ch/TC57/NonStandard/UML#attribute> ;
  rdfs:domain cim:Temperature ;
  rdfs:range cim:UnitSymbol .

cim:Temperature.value a rdf:Property ;
  rdfs:label "value"@en ;
  cims:dataType cim:Float ;
  cims:multiplicity cims:M:0..1 ;
  cims:stereotype <http://iec.ch/TC57/NonStandard/UML#attribute> ;
  rdfs:domain cim:Temperature .

cim:Voltage.multiplier a rdf:Property ;
  rdfs:label "multiplier"@en ;
  cims:isFixed "k" ;
  cims:multiplicity cims:M:0..1 ;
  cims:stereotype <http://iec.ch/TC57/NonStandard/UML#attribute> ;
  rdfs:domain cim:Voltage ;
  rdfs:range cim:UnitMultiplier .

cim:Voltage.unit a rdf:Property ;
  rdfs:label "unit"@en ;
  cims:isFixed "V" ;
  cims:multiplicity cims:M:0..1 ;
  cims:stereotype <http://iec.ch/TC57/NonStandard/UML#attribute> ;
  rdfs:domain cim:Voltage ;
  rdfs:range cim:UnitSymbol .

cim:Voltage.value a rdf:Property ;
  rdfs:label "value"@en ;
  cims:dataType cim:Float ;
  cims:multiplicity cims:M:0..1 ;
  cims:stereotype <http://iec.ch/TC57/NonStandard/UML#attribute> ;
  rdfs:domain cim:Voltage .

cim:VoltagePerReactivePower.multiplier a rdf:Property ;
  rdfs:label "multiplier"@en ;
  cims:isFixed "k" ;
  cims:multiplicity cims:M:0..1 ;
  cims:stereotype <http://iec.ch/TC57/NonStandard/UML#attribute> ;
  rdfs:domain cim:VoltagePerReactivePower ;
  rdfs:range cim:UnitMultiplier .

cim:VoltagePerReactivePower.unit a rdf:Property ;
  rdfs:label "unit"@en ;
  cims:isFixed "VPerVAr" ;
  cims:multiplicity cims:M:0..1 ;
  cims:stereotype <http://iec.ch/TC57/NonStandard/UML#attribute> ;
  rdfs:domain cim:VoltagePerReactivePower ;
  rdfs:range cim:UnitSymbol .

cim:VoltagePerReactivePower.value a rdf:Property ;
  rdfs:label "value"@en ;
  cims:dataType cim:Float ;
  cims:multiplicity cims:M:0..1 ;
  cims:stereotype <http://iec.ch/TC57/NonStandard/UML#attribute> ;
  rdfs:domain cim:VoltagePerReactivePower .

cim:VsCapabilityCurve.VsConverter a rdf:Property ;
  rdfs:label "VsConverter"@en ;
  rdfs:comment "Converter with this capability curve." ;
  cims:AssociationUsed "Yes" ;
  cims:inverseRoleName cim:VsConverter.CapabilityCurve2 ;
  cims:multiplicity cims:M:1 ;
  cims:stereotype "NC" ;
  rdfs:domain cim:VsCapabilityCurve ;
  rdfs:range cim:VsConverter .

cim:VsConverter.CapabilityCurve2 a rdf:Property ;
  rdfs:label "CapabilityCurve2"@en ;
  rdfs:comment "Capability curve of this converter." ;
  cims:AssociationUsed "No" ;
  cims:inverseRoleName cim:VsCapabilityCurve.VsConverter ;
  cims:multiplicity cims:M:0..n ;
  cims:stereotype "NC" ;
  rdfs:domain cim:VsConverter ;
  rdfs:range cim:VsCapabilityCurve .

eu:IdentifiedObject.energyIdentCodeEic a rdf:Property ;
  rdfs:label "energyIdentCodeEic"@en ;
  rdfs:comment "The attribute is used for an exchange of the EIC code (Energy identification Code). The length of the string is 16 characters as defined by the EIC code. For details on EIC scheme please refer to ENTSO-E web site." ;
  cims:dataType cim:String ;
  cims:multiplicity cims:M:0..1 ;
  cims:stereotype "European", "deprecated", <http://iec.ch/TC57/NonStandard/UML#attribute> ;
  rdfs:domain cim:IdentifiedObject .

nc:ACDCConverter.ACDCConverterController a rdf:Property ;
  rdfs:label "ACDCConverterController"@en ;
  rdfs:comment "Direct current controller which controls the ACDC converter." ;
  cims:AssociationUsed "No" ;
  cims:inverseRoleName nc:ACDCConverterController.ACDCConverter ;
  cims:multiplicity cims:M:0..1 ;
  cims:stereotype "NC" ;
  rdfs:domain cim:ACDCConverter ;
  rdfs:range nc:ACDCConverterController .

nc:ACDCConverterController.ACDCConverter a rdf:Property ;
  rdfs:label "ACDCConverter"@en ;
  rdfs:comment "ACDC converter controlled by the direct current controller." ;
  cims:AssociationUsed "Yes" ;
  cims:inverseRoleName nc:ACDCConverter.ACDCConverterController ;
  cims:multiplicity cims:M:1 ;
  cims:stereotype "NC" ;
  rdfs:domain nc:ACDCConverterController ;
  rdfs:range cim:ACDCConverter .

nc:ACDCConverterController.DirectCurrentPoleController a rdf:Property ;
  rdfs:label "DirectCurrentPoleController"@en ;
  rdfs:comment "DC pole controller that controls this ACDC controller." ;
  cims:AssociationUsed "Yes" ;
  cims:inverseRoleName nc:DirectCurrentPoleController.ACDCConverterController ;
  cims:multiplicity cims:M:0..1 ;
  cims:stereotype "NC" ;
  rdfs:domain nc:ACDCConverterController ;
  rdfs:range nc:DirectCurrentPoleController .

nc:ACDCTerminal.InfeedTerminal a rdf:Property ;
  rdfs:label "InfeedTerminal"@en ;
  rdfs:comment "Infeed terminal that is associated with an ACDCTerminal." ;
  cims:AssociationUsed "No" ;
  cims:inverseRoleName nc:InfeedTerminal.ACDCTerminal ;
  cims:multiplicity cims:M:0..n ;
  cims:stereotype "NC" ;
  rdfs:domain cim:ACDCTerminal ;
  rdfs:range nc:InfeedTerminal .

nc:ACPointOfCommonCoupling.ConnectivityNode a rdf:Property ;
  rdfs:label "ConnectivityNode"@en ;
  rdfs:comment "Connectivity node which is a point of common coupling AC." ;
  cims:AssociationUsed "Yes" ;
  cims:inverseRoleName nc:ConnectivityNode.ACPointOfCommonCoupling ;
  cims:multiplicity cims:M:1 ;
  cims:stereotype "NC" ;
  rdfs:domain nc:ACPointOfCommonCoupling ;
  rdfs:range cim:ConnectivityNode .

nc:ACPointOfCommonCoupling.DCConverterUnit a rdf:Property ;
  rdfs:label "DCConverterUnit"@en ;
  rdfs:comment "DC converter unit that has AC point of common coupling." ;
  cims:AssociationUsed "No" ;
  cims:inverseRoleName nc:DCConverterUnit.ACPointOfCommonCoupling ;
  cims:multiplicity cims:M:0..1 ;
  cims:stereotype "NC" ;
  rdfs:domain nc:ACPointOfCommonCoupling ;
  rdfs:range cim:DCConverterUnit .

nc:ACTieCorridor.Line a rdf:Property ;
  rdfs:label "Line"@en ;
  rdfs:comment "Line that is part of the ACTieCorridor." ;
  cims:AssociationUsed "No" ;
  cims:inverseRoleName nc:Line.ACTieCorridor ;
  cims:multiplicity cims:M:0..n ;
  cims:stereotype "NC" ;
  rdfs:domain nc:ACTieCorridor ;
  rdfs:range cim:Line .

nc:AmbientTemperatureDependencyCurve.OperationalLimitType a rdf:Property ;
  rdfs:label "OperationalLimitType"@en ;
  rdfs:comment "The operational limit type that has this permanent ambient temperature dependency curve." ;
  cims:AssociationUsed "No" ;
  cims:inverseRoleName nc:OperationalLimitType.PermanentAmbientTemperatureDependencyCurve ;
  cims:multiplicity cims:M:0..n ;
  cims:stereotype "NC" ;
  rdfs:domain nc:AmbientTemperatureDependencyCurve ;
  rdfs:range cim:OperationalLimitType .

nc:AreaDispatchableUnit.EnergyConsumer a rdf:Property ;
  rdfs:label "EnergyConsumer"@en ;
  rdfs:comment "Energy consumer for this area dispatchable unit." ;
  cims:AssociationUsed "Yes" ;
  cims:inverseRoleName nc:EnergyConsumer.AreaDispatchableUnit ;
  cims:multiplicity cims:M:0..1 ;
  rdfs:domain nc:AreaDispatchableUnit ;
  rdfs:range cim:EnergyConsumer .

nc:AreaDispatchableUnit.GeneratingUnit a rdf:Property ;
  rdfs:label "GeneratingUnit"@en ;
  rdfs:comment "The generating unit that belongs to area dispatchable unit." ;
  cims:AssociationUsed "Yes" ;
  cims:inverseRoleName nc:GeneratingUnit.AreaDispatchableUnit ;
  cims:multiplicity cims:M:0..1 ;
  cims:stereotype "NC" ;
  rdfs:domain nc:AreaDispatchableUnit ;
  rdfs:range cim:GeneratingUnit .

nc:AreaDispatchableUnit.HydroPump a rdf:Property ;
  rdfs:label "HydroPump"@en ;
  rdfs:comment "Hydro Pump which is associated with the area dispatchable unit." ;
  cims:AssociationUsed "Yes" ;
  cims:inverseRoleName nc:HydroPump.AreaDispatchableUnit ;
  cims:multiplicity cims:M:0..1 ;
  cims:stereotype "NC" ;
  rdfs:domain nc:AreaDispatchableUnit ;
  rdfs:range cim:HydroPump .

nc:AreaDispatchableUnit.PowerElectronicsUnit a rdf:Property ;
  rdfs:label "PowerElectronicsUnit"@en ;
  rdfs:comment "The power electronics unit that belongs to this area dispatchable unit." ;
  cims:AssociationUsed "Yes" ;
  cims:inverseRoleName nc:PowerElectronicsUnit.AreaDispatchableUnit ;
  cims:multiplicity cims:M:0..1 ;
  cims:stereotype "NC" ;
  rdfs:domain nc:AreaDispatchableUnit ;
  rdfs:range cim:PowerElectronicsUnit .

nc:AreaDispatchableUnit.ScheduleResource a rdf:Property ;
  rdfs:label "ScheduleResource"@en ;
  rdfs:comment "The resource which is mFRR for the EnergySchedulingArea to which the AreaDispatchableUnit is connected. Note that this can be different than the area for the energy schedule." ;
  cims:AssociationUsed "Yes" ;
  cims:inverseRoleName nc:ScheduleResource.AreaDispatchableUnit ;
  cims:multiplicity cims:M:0..1 ;
  cims:stereotype "NC" ;
  rdfs:domain nc:AreaDispatchableUnit ;
  rdfs:range nc:ScheduleResource .

nc:AreaDispatchableUnit.SchedulingArea a rdf:Property ;
  rdfs:label "SchedulingArea"@en ;
  rdfs:comment "The scheduling area that has this area dispatchable unit." ;
  cims:AssociationUsed "Yes" ;
  cims:inverseRoleName nc:SchedulingArea.AreaDispatchableUnit ;
  cims:multiplicity cims:M:0..1 ;
  cims:stereotype "NC" ;
  rdfs:domain nc:AreaDispatchableUnit ;
  rdfs:range nc:SchedulingArea .

nc:AreaDispatchableUnit.TieCorridor a rdf:Property ;
  rdfs:label "TieCorridor"@en ;
  rdfs:comment "Tie Corridor which belongs to the Area Dispatchable Unit." ;
  cims:AssociationUsed "Yes" ;
  cims:inverseRoleName nc:TieCorridor.AreaDispatchableUnit ;
  cims:multiplicity cims:M:0..1 ;
  cims:stereotype "NC" ;
  rdfs:domain nc:AreaDispatchableUnit ;
  rdfs:range nc:TieCorridor .

nc:AreaDispatchableUnit.normalEnabled a rdf:Property ;
  rdfs:label "normalEnabled"@en ;
  rdfs:comment "Identifies if the unit is normally enabled to accept a dispatch instruction. If true, the unit is enabled to accept a dispatch instruction. If false, the unit has the capability, but it is not enabled to receive a dispatch instruction." ;
  cims:dataType cim:Boolean ;
  cims:multiplicity cims:M:0..1 ;
  cims:stereotype "NC", <http://iec.ch/TC57/NonStandard/UML#attribute> ;
  rdfs:domain nc:AreaDispatchableUnit .

nc:AreaInterchangeController.BiddingZone a rdf:Property ;
  rdfs:label "BiddingZone"@en ;
  rdfs:comment "Bidding zone which has an area interchange controller." ;
  cims:AssociationUsed "Yes" ;
  cims:inverseRoleName nc:BiddingZone.AreaInterchangeController ;
  cims:multiplicity cims:M:0..1 ;
  cims:stereotype "NC" ;
  rdfs:domain nc:AreaInterchangeController ;
  rdfs:range nc:BiddingZone .

nc:AreaInterchangeController.BiddingZoneBorder a rdf:Property ;
  rdfs:label "BiddingZoneBorder"@en ;
  rdfs:comment "Bidding zone border that has an area interchange controller." ;
  cims:AssociationUsed "Yes" ;
  cims:inverseRoleName nc:BiddingZoneBorder.AreaInterchangeController ;
  cims:multiplicity cims:M:0..1 ;
  cims:stereotype "NC" ;
  rdfs:domain nc:AreaInterchangeController ;
  rdfs:range nc:BiddingZoneBorder .

nc:AreaInterchangeController.ControlArea a rdf:Property ;
  rdfs:label "ControlArea"@en ;
  rdfs:comment "Control area that has a area interchange controller." ;
  cims:AssociationUsed "Yes" ;
  cims:inverseRoleName nc:ControlArea.AreaInterchangeController ;
  cims:multiplicity cims:M:0..1 ;
  cims:stereotype "NC" ;
  rdfs:domain nc:AreaInterchangeController ;
  rdfs:range cim:ControlArea .

nc:AreaInterchangeController.pTolerance a rdf:Property ;
  rdfs:label "pTolerance"@en ;
  rdfs:comment "Active power net interchange tolerance. The attribute shall be a positive value or zero." ;
  cims:dataType cim:ActivePower ;
  cims:multiplicity cims:M:1..1 ;
  cims:stereotype "NC", <http://iec.ch/TC57/NonStandard/UML#attribute> ;
  rdfs:domain nc:AreaInterchangeController .

nc:AutomationBlockGroup.AutomationFunction a rdf:Property ;
  rdfs:label "AutomationFunction"@en ;
  rdfs:comment "Automation function which has automation block group." ;
  cims:AssociationUsed "Yes" ;
  cims:inverseRoleName nc:AutomationFunction.AutomationBlockGroup ;
  cims:multiplicity cims:M:1 ;
  cims:stereotype "NC" ;
  rdfs:domain nc:AutomationBlockGroup ;
  rdfs:range nc:AutomationFunction .

nc:AutomationBlockGroup.FunctionBlock a rdf:Property ;
  rdfs:label "FunctionBlock"@en ;
  rdfs:comment "Function block which belongs to an automation block group." ;
  cims:AssociationUsed "No" ;
  cims:inverseRoleName nc:FunctionBlock.AutomationBlockGroup ;
  cims:multiplicity cims:M:1..n ;
  cims:stereotype "NC" ;
  rdfs:domain nc:AutomationBlockGroup ;
  rdfs:range nc:FunctionBlock .

nc:AutomationBlockGroup.priority a rdf:Property ;
  rdfs:label "priority"@en ;
  rdfs:comment "Value 0 means ignore priority. 1 means the highest priority, 2 is the second highest priority." ;
  cims:dataType cim:Integer ;
  cims:multiplicity cims:M:0..1 ;
  cims:stereotype "NC", <http://iec.ch/TC57/NonStandard/UML#attribute> ;
  rdfs:domain nc:AutomationBlockGroup .

nc:AutomationFunction.AutomationBlockGroup a rdf:Property ;
  rdfs:label "AutomationBlockGroup"@en ;
  rdfs:comment "Automation block group which belongs to an automation function." ;
  cims:AssociationUsed "No" ;
  cims:inverseRoleName nc:AutomationBlockGroup.AutomationFunction ;
  cims:multiplicity cims:M:0..n ;
  cims:stereotype "NC", <http://iec.ch/TC57/NonStandard/UML#ofAggregate> ;
  rdfs:domain nc:AutomationFunction ;
  rdfs:range nc:AutomationBlockGroup .

nc:AutomationFunction.FunctionBlock a rdf:Property ;
  rdfs:label "FunctionBlock"@en ;
  rdfs:comment "Function block is part of this automation function." ;
  cims:AssociationUsed "No" ;
  cims:inverseRoleName nc:FunctionBlock.AutomationFunction ;
  cims:multiplicity cims:M:0..n ;
  cims:stereotype "NC" ;
  rdfs:domain nc:AutomationFunction ;
  rdfs:range nc:FunctionBlock .

nc:AutomationFunction.HasPart a rdf:Property ;
  rdfs:label "HasPart"@en ;
  rdfs:comment "Automation function has this automation function as a part." ;
  cims:AssociationUsed "No" ;
  cims:inverseRoleName nc:AutomationFunction.PartOf ;
  cims:multiplicity cims:M:0..n ;
  cims:stereotype "NC" ;
  rdfs:domain nc:AutomationFunction ;
  rdfs:range nc:AutomationFunction .

nc:AutomationFunction.PartOf a rdf:Property ;
  rdfs:label "PartOf"@en ;
  rdfs:comment "Automation function is part of this automation function." ;
  cims:AssociationUsed "Yes" ;
  cims:inverseRoleName nc:AutomationFunction.HasPart ;
  cims:multiplicity cims:M:0..1 ;
  cims:stereotype "NC" ;
  rdfs:domain nc:AutomationFunction ;
  rdfs:range nc:AutomationFunction .

nc:AutomationFunction.normalEnabled a rdf:Property ;
  rdfs:label "normalEnabled"@en ;
  rdfs:comment "True, if the automation function is enabled (active). Otherwise false." ;
  cims:dataType cim:Boolean ;
  cims:multiplicity cims:M:0..1 ;
  cims:stereotype "NC", <http://iec.ch/TC57/NonStandard/UML#attribute> ;
  rdfs:domain nc:AutomationFunction .

nc:AutomationFunction.type a rdf:Property ;
  rdfs:label "type"@en ;
  rdfs:comment "Type of automation function." ;
  cims:dataType cim:String ;
  cims:multiplicity cims:M:0..1 ;
  cims:stereotype "NC", <http://iec.ch/TC57/NonStandard/UML#attribute> ;
  rdfs:domain nc:AutomationFunction .

nc:BaseOverloadLimitCurve.OperationalLimitType a rdf:Property ;
  rdfs:label "OperationalLimitType"@en ;
  rdfs:comment "The operational limit type that has this temporary base overload limit curve." ;
  cims:AssociationUsed "No" ;
  cims:inverseRoleName nc:OperationalLimitType.TemporaryBaseOverloadLimitCurve ;
  cims:multiplicity cims:M:0..n ;
  cims:stereotype "NC" ;
  rdfs:domain nc:BaseOverloadLimitCurve ;
  rdfs:range cim:OperationalLimitType .

nc:BiddingZone.AreaInterchangeController a rdf:Property ;
  rdfs:label "AreaInterchangeController"@en ;
  rdfs:comment "Area interchange controller for this bidding zone." ;
  cims:AssociationUsed "No" ;
  cims:inverseRoleName nc:AreaInterchangeController.BiddingZone ;
  cims:multiplicity cims:M:0..1 ;
  cims:stereotype "NC" ;
  rdfs:domain nc:BiddingZone ;
  rdfs:range nc:AreaInterchangeController .

nc:BiddingZone.BiddingZoneBorderOne a rdf:Property ;
  rdfs:label "BiddingZoneBorderOne"@en ;
  rdfs:comment "The primary side of the border." ;
  cims:AssociationUsed "No" ;
  cims:inverseRoleName nc:BiddingZoneBorder.BiddingZoneOne ;
  cims:multiplicity cims:M:0..n ;
  cims:stereotype "NC" ;
  rdfs:domain nc:BiddingZone ;
  rdfs:range nc:BiddingZoneBorder .

nc:BiddingZone.BiddingZoneBorderTwo a rdf:Property ;
  rdfs:label "BiddingZoneBorderTwo"@en ;
  rdfs:comment "The secondary side of the border." ;
  cims:AssociationUsed "No" ;
  cims:inverseRoleName nc:BiddingZoneBorder.BiddingZoneTwo ;
  cims:multiplicity cims:M:0..n ;
  cims:stereotype "NC" ;
  rdfs:domain nc:BiddingZone ;
  rdfs:range nc:BiddingZoneBorder .

nc:BiddingZone.CapacityCalculationRegion a rdf:Property ;
  rdfs:label "CapacityCalculationRegion"@en ;
  rdfs:comment "The capacity calculation region related to this bidding zone." ;
  cims:AssociationUsed "Yes" ;
  cims:inverseRoleName nc:CapacityCalculationRegion.BiddingZone ;
  cims:multiplicity cims:M:0..1 ;
  cims:stereotype "NC" ;
  rdfs:domain nc:BiddingZone ;
  rdfs:range nc:CapacityCalculationRegion .

nc:BiddingZone.PowerCapacity a rdf:Property ;
  rdfs:label "PowerCapacity"@en ;
  rdfs:comment "Power capacity whidh is asocciated to the bidding zone." ;
  cims:AssociationUsed "Yes" ;
  cims:inverseRoleName nc:PowerCapacity.BiddingZone ;
  cims:multiplicity cims:M:0..1 ;
  cims:stereotype "NC" ;
  rdfs:domain nc:BiddingZone ;
  rdfs:range nc:PowerCapacity .

nc:BiddingZone.SchedulingArea a rdf:Property ;
  rdfs:label "SchedulingArea"@en ;
  rdfs:comment "The scheduling area that has bidding zone." ;
  cims:AssociationUsed "No" ;
  cims:inverseRoleName nc:SchedulingArea.BiddingZone ;
  cims:multiplicity cims:M:1..n ;
  cims:stereotype "NC" ;
  rdfs:domain nc:BiddingZone ;
  rdfs:range nc:SchedulingArea .

nc:BiddingZone.isTradeEnabled a rdf:Property ;
  rdfs:label "isTradeEnabled"@en ;
  rdfs:comment "Identifies the mechanism for determining the energy price for a given bidding zone. If true, the bid and the offer is expected to be provided for the bidding zone to create the market price. If false,  other mechanism determines the price of energy for a given bidding zone, e.g. virtual bidding zone." ;
  cims:dataType cim:Boolean ;
  cims:multiplicity cims:M:1..1 ;
  cims:stereotype "NC", <http://iec.ch/TC57/NonStandard/UML#attribute> ;
  rdfs:domain nc:BiddingZone .

nc:BiddingZoneBorder.AreaInterchangeController a rdf:Property ;
  rdfs:label "AreaInterchangeController"@en ;
  rdfs:comment "Area interchange controller that relates to this bidding zone border." ;
  cims:AssociationUsed "No" ;
  cims:inverseRoleName nc:AreaInterchangeController.BiddingZoneBorder ;
  cims:multiplicity cims:M:0..1 ;
  cims:stereotype "NC" ;
  rdfs:domain nc:BiddingZoneBorder ;
  rdfs:range nc:AreaInterchangeController .

nc:BiddingZoneBorder.BiddingZoneOne a rdf:Property ;
  rdfs:label "BiddingZoneOne"@en ;
  rdfs:comment "The bidding zone for the primary side." ;
  cims:AssociationUsed "Yes" ;
  cims:inverseRoleName nc:BiddingZone.BiddingZoneBorderOne ;
  cims:multiplicity cims:M:1 ;
  cims:stereotype "NC" ;
  rdfs:domain nc:BiddingZoneBorder ;
  rdfs:range nc:BiddingZone .

nc:BiddingZoneBorder.BiddingZoneTwo a rdf:Property ;
  rdfs:label "BiddingZoneTwo"@en ;
  rdfs:comment "The bidding zone for the secondary side." ;
  cims:AssociationUsed "Yes" ;
  cims:inverseRoleName nc:BiddingZone.BiddingZoneBorderTwo ;
  cims:multiplicity cims:M:1 ;
  cims:stereotype "NC" ;
  rdfs:domain nc:BiddingZoneBorder ;
  rdfs:range nc:BiddingZone .

nc:BiddingZoneBorder.CapacityCalculationRegion a rdf:Property ;
  rdfs:label "CapacityCalculationRegion"@en ;
  rdfs:comment "The capacity calculation region for which the capacity is derived from." ;
  cims:AssociationUsed "Yes" ;
  cims:inverseRoleName nc:CapacityCalculationRegion.BiddingZoneBorder ;
  cims:multiplicity cims:M:0..1 ;
  cims:stereotype "NC" ;
  rdfs:domain nc:BiddingZoneBorder ;
  rdfs:range nc:CapacityCalculationRegion .

nc:BiddingZoneBorder.TieCorridor a rdf:Property ;
  rdfs:label "TieCorridor"@en ;
  rdfs:comment "Tie corridor for a given bidding zone border." ;
  cims:AssociationUsed "No" ;
  cims:inverseRoleName nc:TieCorridor.BiddingZoneBorder ;
  cims:multiplicity cims:M:0..n ;
  cims:stereotype "NC" ;
  rdfs:domain nc:BiddingZoneBorder ;
  rdfs:range nc:TieCorridor .

nc:BipolarDCSystem.DCBiPole a rdf:Property ;
  rdfs:label "DCBiPole"@en ;
  rdfs:comment "DC bipole that belongs to a bipolar DC system." ;
  cims:AssociationUsed "No" ;
  cims:inverseRoleName nc:DCBiPole.BipolarDCSystem ;
  cims:multiplicity cims:M:0..1 ;
  cims:stereotype "NC" ;
  rdfs:domain nc:BipolarDCSystem ;
  rdfs:range nc:DCBiPole .

nc:BipolarDCSystem.isRigid a rdf:Property ;
  rdfs:label "isRigid"@en ;
  rdfs:comment "If true, the bipolar DC system is a rigid DC current bipolar system (IEC 60633). It is a bipolar DC system without neutral connection between both converter stations. Since only two (pole) conductors exist, no unbalance current between both poles is possible. In case of interruption of power transfer of one converter pole, the current of the other pole has to be interrupted as well (at least for a limited time to allow reconfiguration of the DC circuit)." ;
  cims:dataType cim:Boolean ;
  cims:multiplicity cims:M:1..1 ;
  cims:stereotype "NC", <http://iec.ch/TC57/NonStandard/UML#attribute> ;
  rdfs:domain nc:BipolarDCSystem .

nc:CapacityCalculationRegion.BiddingZone a rdf:Property ;
  rdfs:label "BiddingZone"@en ;
  rdfs:comment "The bidding zone for this capacity calculation region." ;
  cims:AssociationUsed "No" ;
  cims:inverseRoleName nc:BiddingZone.CapacityCalculationRegion ;
  cims:multiplicity cims:M:0..n ;
  cims:stereotype "NC" ;
  rdfs:domain nc:CapacityCalculationRegion ;
  rdfs:range nc:BiddingZone .

nc:CapacityCalculationRegion.BiddingZoneBorder a rdf:Property ;
  rdfs:label "BiddingZoneBorder"@en ;
  rdfs:comment "The bidding zone border on which the capacity is calculated. " ;
  cims:AssociationUsed "No" ;
  cims:inverseRoleName nc:BiddingZoneBorder.CapacityCalculationRegion ;
  cims:multiplicity cims:M:0..n ;
  cims:stereotype "NC" ;
  rdfs:domain nc:CapacityCalculationRegion ;
  rdfs:range nc:BiddingZoneBorder .

nc:CapacityCalculationRegion.CoordinatedCapacityCalculator a rdf:Property ;
  rdfs:label "CoordinatedCapacityCalculator"@en ;
  rdfs:comment "Coordinated capacity calculator responsible for the capacity calculation of the region." ;
  cims:AssociationUsed "Yes" ;
  cims:inverseRoleName nc:CoordinatedCapacityCalculator.CapacityCalculationRegion ;
  cims:multiplicity cims:M:0..1 ;
  cims:stereotype "NC" ;
  rdfs:domain nc:CapacityCalculationRegion ;
  rdfs:range nc:CoordinatedCapacityCalculator .

nc:CapacityCalculationRegion.SecurityCoordinator a rdf:Property ;
  rdfs:label "SecurityCoordinator"@en ;
  rdfs:comment "The security coordinator responsible for the capacity calculation region." ;
  cims:AssociationUsed "Yes" ;
  cims:inverseRoleName nc:SecurityCoordinator.CapacityCalculationRegion ;
  cims:multiplicity cims:M:0..1 ;
  cims:stereotype "NC" ;
  rdfs:domain nc:CapacityCalculationRegion ;
  rdfs:range nc:SecurityCoordinator .

nc:Circuit.CircuitShare a rdf:Property ;
  rdfs:label "CircuitShare"@en ;
  rdfs:comment "The circuit share of the given power transfer corridor." ;
  cims:AssociationUsed "No" ;
  cims:inverseRoleName nc:CircuitShare.Circuit ;
  cims:multiplicity cims:M:0..n ;
  cims:stereotype "NC" ;
  rdfs:domain nc:Circuit ;
  rdfs:range nc:CircuitShare .

nc:Circuit.Equipment a rdf:Property ;
  rdfs:label "Equipment"@en ;
  rdfs:comment "The equipment which is part of the circuit. This includes all equipment related to the circuit (e.g. If the circuit is a transformer, the equipment could be all switching and auxiliary equipments related to the transformer). A BusbarSection shall not be part of the circuit." ;
  cims:AssociationUsed "No" ;
  cims:inverseRoleName nc:Equipment.Circuit ;
  cims:multiplicity cims:M:0..n ;
  cims:stereotype "NC" ;
  rdfs:domain nc:Circuit ;
  rdfs:range cim:Equipment .

nc:Circuit.IdentifyingTerminal a rdf:Property ;
  rdfs:label "IdentifyingTerminal"@en ;
  rdfs:comment "Terminal that identifies the circuit." ;
  cims:AssociationUsed "Yes" ;
  cims:inverseRoleName nc:Terminal.Circuit ;
  cims:multiplicity cims:M:0..1 ;
  cims:stereotype "NC" ;
  rdfs:domain nc:Circuit ;
  rdfs:range cim:Terminal .

nc:Circuit.positiveFlowIn a rdf:Property ;
  rdfs:label "positiveFlowIn"@en ;
  rdfs:comment "True, if the positive value on the terminal shall be considered flow into the circuit. False, if the positive value on the terminal shall be considered flow out of the circuit." ;
  cims:dataType cim:Boolean ;
  cims:multiplicity cims:M:1..1 ;
  cims:stereotype "NC", <http://iec.ch/TC57/NonStandard/UML#attribute> ;
  rdfs:domain nc:Circuit .

nc:CircuitShare.Circuit a rdf:Property ;
  rdfs:label "Circuit"@en ;
  rdfs:comment "The circuit that has a share of the power system corridor." ;
  cims:AssociationUsed "Yes" ;
  cims:inverseRoleName nc:Circuit.CircuitShare ;
  cims:multiplicity cims:M:1 ;
  cims:stereotype "NC" ;
  rdfs:domain nc:CircuitShare ;
  rdfs:range nc:Circuit .

nc:CircuitShare.PowerTransferCorridor a rdf:Property ;
  rdfs:label "PowerTransferCorridor"@en ;
  rdfs:comment "The power transfer corridor that has this circuit share." ;
  cims:AssociationUsed "Yes" ;
  cims:inverseRoleName nc:PowerTransferCorridor.CircuitShare ;
  cims:multiplicity cims:M:1 ;
  cims:stereotype "NC" ;
  rdfs:domain nc:CircuitShare ;
  rdfs:range nc:PowerTransferCorridor .

nc:CircuitShare.normalContributionFactor a rdf:Property ;
  rdfs:label "normalContributionFactor"@en ;
  rdfs:comment """Normal contribution factor for the circuit which is part of a power transfer corridor.
The allowed value range is [0,100].""" ;
  cims:dataType cim:PerCent ;
  cims:multiplicity cims:M:0..1 ;
  cims:stereotype "NC", <http://iec.ch/TC57/NonStandard/UML#attribute> ;
  rdfs:domain nc:CircuitShare .

nc:ConnectivityNode.ACPointOfCommonCoupling a rdf:Property ;
  rdfs:label "ACPointOfCommonCoupling"@en ;
  rdfs:comment "Identifies this ConnectivityNode as a point of common coupling AC." ;
  cims:AssociationUsed "No" ;
  cims:inverseRoleName nc:ACPointOfCommonCoupling.ConnectivityNode ;
  cims:multiplicity cims:M:0..1 ;
  cims:stereotype "NC" ;
  rdfs:domain cim:ConnectivityNode ;
  rdfs:range nc:ACPointOfCommonCoupling .

nc:ControlArea.AreaInterchangeController a rdf:Property ;
  rdfs:label "AreaInterchangeController"@en ;
  rdfs:comment "Area interchange controller for this control area." ;
  cims:AssociationUsed "No" ;
  cims:inverseRoleName nc:AreaInterchangeController.ControlArea ;
  cims:multiplicity cims:M:0..1 ;
  cims:stereotype "NC" ;
  rdfs:domain cim:ControlArea ;
  rdfs:range nc:AreaInterchangeController .

nc:ControlArea.OutageCoordinationRegion a rdf:Property ;
  rdfs:label "OutageCoordinationRegion"@en ;
  rdfs:comment "The outage coordination region that has this control area." ;
  cims:AssociationUsed "Yes" ;
  cims:inverseRoleName nc:OutageCoordinationRegion.ControlArea ;
  cims:multiplicity cims:M:0..1 ;
  cims:stereotype "NC" ;
  rdfs:domain cim:ControlArea ;
  rdfs:range nc:OutageCoordinationRegion .

nc:ControlArea.PowerFrequencyController a rdf:Property ;
  rdfs:label "PowerFrequencyController"@en ;
  rdfs:comment "Power frequency controller for this control area." ;
  cims:AssociationUsed "No" ;
  cims:inverseRoleName nc:PowerFrequencyController.ControlArea ;
  cims:multiplicity cims:M:0..1 ;
  cims:stereotype "NC" ;
  rdfs:domain cim:ControlArea ;
  rdfs:range nc:PowerFrequencyController .

nc:ControlArea.SchedulingArea a rdf:Property ;
  rdfs:label "SchedulingArea"@en ;
  rdfs:comment "The scheduling area related to a control area." ;
  cims:AssociationUsed "No" ;
  cims:inverseRoleName nc:SchedulingArea.ControlArea ;
  cims:multiplicity cims:M:1..n ;
  cims:stereotype "NC" ;
  rdfs:domain cim:ControlArea ;
  rdfs:range nc:SchedulingArea .

nc:ControlArea.SystemOperator a rdf:Property ;
  rdfs:label "SystemOperator"@en ;
  rdfs:comment "The system operator that operates this control area." ;
  cims:AssociationUsed "Yes" ;
  cims:inverseRoleName nc:SystemOperator.ControlArea ;
  cims:multiplicity cims:M:0..1 ;
  cims:stereotype "NC" ;
  rdfs:domain cim:ControlArea ;
  rdfs:range nc:SystemOperator .

nc:ControlFunctionBlock.isDiscrete a rdf:Property ;
  rdfs:label "isDiscrete"@en ;
  rdfs:comment "True, if the control function is discrete. This applies to equipment with discrete controls, e.g. tap changers and shunt compensators." ;
  cims:dataType cim:Boolean ;
  cims:multiplicity cims:M:1..1 ;
  cims:stereotype "NC", <http://iec.ch/TC57/NonStandard/UML#attribute> ;
  rdfs:domain nc:ControlFunctionBlock .

nc:ControlFunctionBlock.maxAllowedTargetValue a rdf:Property ;
  rdfs:label "maxAllowedTargetValue"@en ;
  rdfs:comment """Maximum allowed target value given by the percent of target value.
The allowed value range is [0,100].""" ;
  cims:dataType cim:PerCent ;
  cims:multiplicity cims:M:0..1 ;
  cims:stereotype "NC", <http://iec.ch/TC57/NonStandard/UML#attribute> ;
  rdfs:domain nc:ControlFunctionBlock .

nc:ControlFunctionBlock.minAllowedTargetValue a rdf:Property ;
  rdfs:label "minAllowedTargetValue"@en ;
  rdfs:comment """Minimum allowed target value given by the percent of target value.
The allowed value range is [0,100].""" ;
  cims:dataType cim:PerCent ;
  cims:multiplicity cims:M:0..1 ;
  cims:stereotype "NC", <http://iec.ch/TC57/NonStandard/UML#attribute> ;
  rdfs:domain nc:ControlFunctionBlock .

nc:ControlFunctionBlock.targetDeadband a rdf:Property ;
  rdfs:label "targetDeadband"@en ;
  rdfs:comment """Target deadband is used with discrete control to avoid excessive update of controls like tap changers and shunt compensator banks while regulating.  The attribute shall be a positive value or zero. If isDiscrete is set to "false", the targetDeadband is to be ignored.
Note that for instance, if the targetValue is 100 kV and the targetDeadband is 2 kV the range is from 99 to 101 kV.""" ;
  cims:dataType cim:Float ;
  cims:multiplicity cims:M:0..1 ;
  cims:stereotype "NC", <http://iec.ch/TC57/NonStandard/UML#attribute> ;
  rdfs:domain nc:ControlFunctionBlock .

nc:CoordinatedCapacityCalculator.CapacityCalculationRegion a rdf:Property ;
  rdfs:label "CapacityCalculationRegion"@en ;
  rdfs:comment "Capacity calculation region in which the capacity is calculated by the coordinated capacity calculator." ;
  cims:AssociationUsed "No" ;
  cims:inverseRoleName nc:CapacityCalculationRegion.CoordinatedCapacityCalculator ;
  cims:multiplicity cims:M:0..n ;
  cims:stereotype "NC" ;
  rdfs:domain nc:CoordinatedCapacityCalculator ;
  rdfs:range nc:CapacityCalculationRegion .

nc:CurrentDroopControlFunction.droopCapacitive a rdf:Property ;
  rdfs:label "droopCapacitive"@en ;
  rdfs:comment "Droop in capacitive region. The unit is V/A." ;
  cims:dataType cim:Float ;
  cims:multiplicity cims:M:1..1 ;
  cims:stereotype "NC", <http://iec.ch/TC57/NonStandard/UML#attribute> ;
  rdfs:domain nc:CurrentDroopControlFunction .

nc:CurrentDroopControlFunction.droopInductive a rdf:Property ;
  rdfs:label "droopInductive"@en ;
  rdfs:comment "Droop in inductive region. The unit is V/A." ;
  cims:dataType cim:Float ;
  cims:multiplicity cims:M:1..1 ;
  cims:stereotype "NC", <http://iec.ch/TC57/NonStandard/UML#attribute> ;
  rdfs:domain nc:CurrentDroopControlFunction .

nc:CurrentDroopControlFunction.offsetCapacitive a rdf:Property ;
  rdfs:label "offsetCapacitive"@en ;
  rdfs:comment "Offset in capacitive region." ;
  cims:dataType cim:CurrentFlow ;
  cims:multiplicity cims:M:1..1 ;
  cims:stereotype "NC", <http://iec.ch/TC57/NonStandard/UML#attribute> ;
  rdfs:domain nc:CurrentDroopControlFunction .

nc:CurrentDroopControlFunction.offsetInductive a rdf:Property ;
  rdfs:label "offsetInductive"@en ;
  rdfs:comment "Offset in capacitive region." ;
  cims:dataType cim:CurrentFlow ;
  cims:multiplicity cims:M:1..1 ;
  cims:stereotype "NC", <http://iec.ch/TC57/NonStandard/UML#attribute> ;
  rdfs:domain nc:CurrentDroopControlFunction .

nc:CurrentDroopOverride.SSSCController a rdf:Property ;
  rdfs:label "SSSCController"@en ;
  rdfs:comment "The SSSC controller to which this CurrentDroopOverride applies to." ;
  cims:AssociationUsed "Yes" ;
  cims:inverseRoleName nc:SSSCController.CurrentDroopOverride ;
  cims:multiplicity cims:M:1 ;
  cims:stereotype "NC" ;
  rdfs:domain nc:CurrentDroopOverride ;
  rdfs:range nc:SSSCController .

nc:CurrentDroopOverride.droopCapacitive a rdf:Property ;
  rdfs:label "droopCapacitive"@en ;
  rdfs:comment "Droop in capacitive region. The unit is V/A." ;
  cims:dataType cim:Float ;
  cims:multiplicity cims:M:1..1 ;
  cims:stereotype "NC", <http://iec.ch/TC57/NonStandard/UML#attribute> ;
  rdfs:domain nc:CurrentDroopOverride .

nc:CurrentDroopOverride.droopInductive a rdf:Property ;
  rdfs:label "droopInductive"@en ;
  rdfs:comment "Droop in inductive region. The unit is V/A." ;
  cims:dataType cim:Float ;
  cims:multiplicity cims:M:1..1 ;
  cims:stereotype "NC", <http://iec.ch/TC57/NonStandard/UML#attribute> ;
  rdfs:domain nc:CurrentDroopOverride .

nc:CurrentDroopOverride.mRID a rdf:Property ;
  rdfs:label "mRID"@en ;
  rdfs:comment """Master resource identifier issued by a model authority. The mRID is unique within an exchange context. Global uniqueness is easily achieved by using a UUID, as specified in RFC 4122, for the mRID. The use of UUID is strongly recommended.
For CIMXML data files in RDF syntax conforming to IEC 61970-552, the mRID is mapped to rdf:ID or rdf:about attributes that identify CIM object elements.""" ;
  cims:dataType cim:String ;
  cims:multiplicity cims:M:1..1 ;
  cims:stereotype "NC", <http://iec.ch/TC57/NonStandard/UML#attribute> ;
  rdfs:domain nc:CurrentDroopOverride .

nc:CurrentDroopOverride.offsetCapacitiveI a rdf:Property ;
  rdfs:label "offsetCapacitiveI"@en ;
  rdfs:comment "Offset in capacitive region." ;
  cims:dataType cim:CurrentFlow ;
  cims:multiplicity cims:M:1..1 ;
  cims:stereotype "NC", <http://iec.ch/TC57/NonStandard/UML#attribute> ;
  rdfs:domain nc:CurrentDroopOverride .

nc:CurrentDroopOverride.offsetInductiveI a rdf:Property ;
  rdfs:label "offsetInductiveI"@en ;
  rdfs:comment "Offset in capacitive region." ;
  cims:dataType cim:CurrentFlow ;
  cims:multiplicity cims:M:1..1 ;
  cims:stereotype "NC", <http://iec.ch/TC57/NonStandard/UML#attribute> ;
  rdfs:domain nc:CurrentDroopOverride .

nc:DCBiPole.BipolarDCSystem a rdf:Property ;
  rdfs:label "BipolarDCSystem"@en ;
  rdfs:comment "Bipolar DC system that has this DC bipole." ;
  cims:AssociationUsed "Yes" ;
  cims:inverseRoleName nc:BipolarDCSystem.DCBiPole ;
  cims:multiplicity cims:M:0..1 ;
  cims:stereotype "NC" ;
  rdfs:domain nc:DCBiPole ;
  rdfs:range nc:BipolarDCSystem .

nc:DCBiPole.DCPole a rdf:Property ;
  rdfs:label "DCPole"@en ;
  rdfs:comment "DC pole part of the DC system bipole." ;
  cims:AssociationUsed "No" ;
  cims:inverseRoleName nc:DCPole.DCBiPole ;
  cims:multiplicity cims:M:1..2 ;
  cims:stereotype "NC" ;
  rdfs:domain nc:DCBiPole ;
  rdfs:range nc:DCPole .

nc:DCConverterUnit.ACPointOfCommonCoupling a rdf:Property ;
  rdfs:label "ACPointOfCommonCoupling"@en ;
  rdfs:comment "AC point of common coupling for this DC converter unit." ;
  cims:AssociationUsed "Yes" ;
  cims:inverseRoleName nc:ACPointOfCommonCoupling.DCConverterUnit ;
  cims:multiplicity cims:M:1 ;
  cims:stereotype "NC" ;
  rdfs:domain cim:DCConverterUnit ;
  rdfs:range nc:ACPointOfCommonCoupling .

nc:DCConverterUnit.DCPointOfCommonCoupling a rdf:Property ;
  rdfs:label "DCPointOfCommonCoupling"@en ;
  rdfs:comment "DCNode that is the point of common coupling at DC side of this DCConverterUnit." ;
  cims:AssociationUsed "Yes" ;
  cims:inverseRoleName nc:DCPointOfCommonCoupling.DCConverterUnit ;
  cims:multiplicity cims:M:1 ;
  cims:stereotype "NC" ;
  rdfs:domain cim:DCConverterUnit ;
  rdfs:range nc:DCPointOfCommonCoupling .

nc:DCConverterUnit.DCPole a rdf:Property ;
  rdfs:label "DCPole"@en ;
  rdfs:comment "The DC pole that has this DC converter unit." ;
  cims:AssociationUsed "Yes" ;
  cims:inverseRoleName nc:DCPole.DCConverterUnit ;
  cims:multiplicity cims:M:0..1 ;
  cims:stereotype "NC" ;
  rdfs:domain cim:DCConverterUnit ;
  rdfs:range nc:DCPole .

nc:DCConverterUnit.DCSubstation a rdf:Property ;
  rdfs:label "DCSubstation"@en ;
  rdfs:comment "DC substation that has one or more DC converter units." ;
  cims:AssociationUsed "Yes" ;
  cims:inverseRoleName nc:DCSubstation.DCConverterUnit ;
  cims:multiplicity cims:M:0..1 ;
  cims:stereotype "NC" ;
  rdfs:domain cim:DCConverterUnit ;
  rdfs:range nc:DCSubstation .

nc:DCCurrentControlFunction.droop a rdf:Property ;
  rdfs:label "droop"@en ;
  rdfs:comment "Droop constant. The pu value is obtained as D [kV/MW] x Sb / Ubdc. The attribute shall be a positive value." ;
  cims:dataType cim:PU ;
  cims:multiplicity cims:M:0..1 ;
  cims:stereotype "NC", <http://iec.ch/TC57/NonStandard/UML#attribute> ;
  rdfs:domain nc:DCCurrentControlFunction .

nc:DCCurrentControlFunction.droopCompensation a rdf:Property ;
  rdfs:label "droopCompensation"@en ;
  rdfs:comment "Compensation constant. Used to compensate for voltage drop when controlling voltage at a distant bus. The attribute shall be a positive value." ;
  cims:dataType cim:Resistance ;
  cims:multiplicity cims:M:0..1 ;
  cims:stereotype "NC", <http://iec.ch/TC57/NonStandard/UML#attribute> ;
  rdfs:domain nc:DCCurrentControlFunction .

nc:DCLine.DCPole a rdf:Property ;
  rdfs:label "DCPole"@en ;
  rdfs:comment "The DC pole that has this DC line." ;
  cims:AssociationUsed "Yes" ;
  cims:inverseRoleName nc:DCPole.DCLine ;
  cims:multiplicity cims:M:0..1 ;
  cims:stereotype "NC" ;
  rdfs:domain cim:DCLine ;
  rdfs:range nc:DCPole .

nc:DCNode.DCPointOfCommonCoupling a rdf:Property ;
  rdfs:label "DCPointOfCommonCoupling"@en ;
  rdfs:comment "Identifies that this DC node is a point of common coupling DC." ;
  cims:AssociationUsed "No" ;
  cims:inverseRoleName nc:DCPointOfCommonCoupling.DCNode ;
  cims:multiplicity cims:M:0..1 ;
  cims:stereotype "NC" ;
  rdfs:domain cim:DCNode ;
  rdfs:range nc:DCPointOfCommonCoupling .

nc:DCPointOfCommonCoupling.DCConverterUnit a rdf:Property ;
  rdfs:label "DCConverterUnit"@en ;
  rdfs:comment "DC converter unit that has DC point of common coupling." ;
  cims:AssociationUsed "No" ;
  cims:inverseRoleName nc:DCConverterUnit.DCPointOfCommonCoupling ;
  cims:multiplicity cims:M:0..1 ;
  cims:stereotype "NC" ;
  rdfs:domain nc:DCPointOfCommonCoupling ;
  rdfs:range cim:DCConverterUnit .

nc:DCPointOfCommonCoupling.DCNode a rdf:Property ;
  rdfs:label "DCNode"@en ;
  rdfs:comment "The DCNode that is a point of common coupling DC." ;
  cims:AssociationUsed "Yes" ;
  cims:inverseRoleName nc:DCNode.DCPointOfCommonCoupling ;
  cims:multiplicity cims:M:1 ;
  cims:stereotype "NC" ;
  rdfs:domain nc:DCPointOfCommonCoupling ;
  rdfs:range cim:DCNode .

nc:DCPole.AsymmetricMonopolarDCSystem a rdf:Property ;
  rdfs:label "AsymmetricMonopolarDCSystem"@en ;
  rdfs:comment "Asymmetric monopolar DC system that has this DC pole." ;
  cims:AssociationUsed "Yes" ;
  cims:inverseRoleName nc:MonopolarDCSystem.DCPole ;
  cims:multiplicity cims:M:0..1 ;
  cims:stereotype "NC" ;
  rdfs:domain nc:DCPole ;
  rdfs:range nc:MonopolarDCSystem .

nc:DCPole.DCBiPole a rdf:Property ;
  rdfs:label "DCBiPole"@en ;
  rdfs:comment "DC system bipole that has two independently operatable DC system poles." ;
  cims:AssociationUsed "Yes" ;
  cims:inverseRoleName nc:DCBiPole.DCPole ;
  cims:multiplicity cims:M:0..1 ;
  cims:stereotype "NC" ;
  rdfs:domain nc:DCPole ;
  rdfs:range nc:DCBiPole .

nc:DCPole.DCConverterUnit a rdf:Property ;
  rdfs:label "DCConverterUnit"@en ;
  rdfs:comment "The DC converter unit that relates to this DC pole." ;
  cims:AssociationUsed "No" ;
  cims:inverseRoleName nc:DCConverterUnit.DCPole ;
  cims:multiplicity cims:M:0..2 ;
  cims:stereotype "NC" ;
  rdfs:domain nc:DCPole ;
  rdfs:range cim:DCConverterUnit .

nc:DCPole.DCLine a rdf:Property ;
  rdfs:label "DCLine"@en ;
  rdfs:comment "The DC line that is related to this DC pole." ;
  cims:AssociationUsed "No" ;
  cims:inverseRoleName nc:DCLine.DCPole ;
  cims:multiplicity cims:M:0..1 ;
  cims:stereotype "NC" ;
  rdfs:domain nc:DCPole ;
  rdfs:range cim:DCLine .

nc:DCPole.DCTieCorridor a rdf:Property ;
  rdfs:label "DCTieCorridor"@en ;
  rdfs:comment "The DCTieCorridor that has this DC pole." ;
  cims:AssociationUsed "Yes" ;
  cims:inverseRoleName nc:DCTieCorridor.DCPole ;
  cims:multiplicity cims:M:0..1 ;
  cims:stereotype "NC" ;
  rdfs:domain nc:DCPole ;
  rdfs:range nc:DCTieCorridor .

nc:DCPole.DirectCurrentPoleController a rdf:Property ;
  rdfs:label "DirectCurrentPoleController"@en ;
  rdfs:comment "DC pole controller that controls this DC pole." ;
  cims:AssociationUsed "No" ;
  cims:inverseRoleName nc:DirectCurrentPoleController.DCPole ;
  cims:multiplicity cims:M:0..1 ;
  cims:stereotype "NC" ;
  rdfs:domain nc:DCPole ;
  rdfs:range nc:DirectCurrentPoleController .

nc:DCPole.normalParticipationFactor a rdf:Property ;
  rdfs:label "normalParticipationFactor"@en ;
  rdfs:comment """Normal participation factor describing the entity part of the active power provided by a collection of entities (e.g. an active power forecast to a collection of entities is divided to each of the member entity according to the participation factor). Must be a positive value.
In the case of a sharing strategy, the distribution is following entities value (V) equals aggregated value (T) divided by sum of participation factors (PF), i.e. V=T/sum(PF). 
In the case of priority strategy, the item with the lowest number gets allocated energy first.""" ;
  cims:dataType cim:Float ;
  cims:multiplicity cims:M:0..1 ;
  cims:stereotype "NC", <http://iec.ch/TC57/NonStandard/UML#attribute> ;
  rdfs:domain nc:DCPole .

nc:DCSubstation.DCConverterUnit a rdf:Property ;
  rdfs:label "DCConverterUnit"@en ;
  rdfs:comment "DC converter unit that belongs to this DC substation." ;
  cims:AssociationUsed "No" ;
  cims:inverseRoleName nc:DCConverterUnit.DCSubstation ;
  cims:multiplicity cims:M:0..n ;
  cims:stereotype "NC" ;
  rdfs:domain nc:DCSubstation ;
  rdfs:range cim:DCConverterUnit .

nc:DCSubstation.DCSubstationBipole a rdf:Property ;
  rdfs:label "DCSubstationBipole"@en ;
  rdfs:comment "DC substation bipole which is part of the DC substation. " ;
  cims:AssociationUsed "No" ;
  cims:inverseRoleName nc:DCSubstationBipole.DCSubstation ;
  cims:multiplicity cims:M:0..n ;
  cims:stereotype "NC" ;
  rdfs:domain nc:DCSubstation ;
  rdfs:range nc:DCSubstationBipole .

nc:DCSubstation.DCSubstationPole a rdf:Property ;
  rdfs:label "DCSubstationPole"@en ;
  rdfs:comment "DC substation pole which is part of the DC substation. " ;
  cims:AssociationUsed "No" ;
  cims:inverseRoleName nc:DCSubstationPole.DCSubstation ;
  cims:multiplicity cims:M:0..n ;
  cims:stereotype "NC" ;
  rdfs:domain nc:DCSubstation ;
  rdfs:range nc:DCSubstationPole .

nc:DCSubstation.Substation a rdf:Property ;
  rdfs:label "Substation"@en ;
  rdfs:comment "Substation that contains this DC susbstation." ;
  cims:AssociationUsed "Yes" ;
  cims:inverseRoleName nc:Substation.DCSubstation ;
  cims:multiplicity cims:M:0..1 ;
  cims:stereotype "NC" ;
  rdfs:domain nc:DCSubstation ;
  rdfs:range cim:Substation .

nc:DCSubstation.isTapping a rdf:Property ;
  rdfs:label "isTapping"@en ;
  rdfs:comment "DC tapping substation (IEC 60633) is a DC substation, mainly used for inversion, with a rating which is a small fraction of that of the rectifier(s) in the system." ;
  cims:dataType cim:Boolean ;
  cims:multiplicity cims:M:1..1 ;
  cims:stereotype "NC", <http://iec.ch/TC57/NonStandard/UML#attribute> ;
  rdfs:domain nc:DCSubstation .

nc:DCSubstationBipole.DCSubstation a rdf:Property ;
  rdfs:label "DCSubstation"@en ;
  rdfs:comment "DC substation that contains this DC substation bipole part." ;
  cims:AssociationUsed "Yes" ;
  cims:inverseRoleName nc:DCSubstation.DCSubstationBipole ;
  cims:multiplicity cims:M:0..1 ;
  cims:stereotype "NC" ;
  rdfs:domain nc:DCSubstationBipole ;
  rdfs:range nc:DCSubstation .

nc:DCSubstationBipole.DirectCurrentSubstationBipoleController a rdf:Property ;
  rdfs:label "DirectCurrentSubstationBipoleController"@en ;
  rdfs:comment "DC substation bipole controller controlling this DC substation bipole." ;
  cims:AssociationUsed "No" ;
  cims:inverseRoleName nc:DirectCurrentSubstationBipoleController.DCSubstationBipole ;
  cims:multiplicity cims:M:0..1 ;
  cims:stereotype "NC" ;
  rdfs:domain nc:DCSubstationBipole ;
  rdfs:range nc:DirectCurrentSubstationBipoleController .

nc:DCSubstationPole.DCSubstation a rdf:Property ;
  rdfs:label "DCSubstation"@en ;
  rdfs:comment "DC substation that contains this DC substation pole part." ;
  cims:AssociationUsed "Yes" ;
  cims:inverseRoleName nc:DCSubstation.DCSubstationPole ;
  cims:multiplicity cims:M:0..1 ;
  cims:stereotype "NC" ;
  rdfs:domain nc:DCSubstationPole ;
  rdfs:range nc:DCSubstation .

nc:DCSubstationPole.DirectCurrentSubstationPoleController a rdf:Property ;
  rdfs:label "DirectCurrentSubstationPoleController"@en ;
  rdfs:comment "DC substation pole controller controlling this DC substation pole." ;
  cims:AssociationUsed "No" ;
  cims:inverseRoleName nc:DirectCurrentSubstationPoleController.DCSubstationPole ;
  cims:multiplicity cims:M:0..1 ;
  cims:stereotype "NC" ;
  rdfs:domain nc:DCSubstationPole ;
  rdfs:range nc:DirectCurrentSubstationPoleController .

nc:DCSystem.directionKind a rdf:Property ;
  rdfs:label "directionKind"@en ;
  rdfs:comment "Direction kind of the DC system." ;
  cims:multiplicity cims:M:0..1 ;
  cims:stereotype "NC", <http://iec.ch/TC57/NonStandard/UML#attribute> ;
  rdfs:domain nc:DCSystem ;
  rdfs:range nc:DCSystemDirectionKind .

nc:DCSystem.transmissionKind a rdf:Property ;
  rdfs:label "transmissionKind"@en ;
  rdfs:comment "Transmission kind of the DC system." ;
  cims:multiplicity cims:M:0..1 ;
  cims:stereotype "NC", <http://iec.ch/TC57/NonStandard/UML#attribute> ;
  rdfs:domain nc:DCSystem ;
  rdfs:range nc:DCSystemTransmissionKind .

nc:DCTieCorridor.DCPole a rdf:Property ;
  rdfs:label "DCPole"@en ;
  rdfs:comment "The DCPole which is part of the DC corridor." ;
  cims:AssociationUsed "No" ;
  cims:inverseRoleName nc:DCPole.DCTieCorridor ;
  cims:multiplicity cims:M:0..n ;
  cims:stereotype "NC" ;
  rdfs:domain nc:DCTieCorridor ;
  rdfs:range nc:DCPole .

nc:DCTieCorridor.DirectCurrentMasterController a rdf:Property ;
  rdfs:label "DirectCurrentMasterController"@en ;
  rdfs:comment "Direct current master controller for this DCTieCorridor." ;
  cims:AssociationUsed "No" ;
  cims:inverseRoleName nc:DirectCurrentMasterController.DCTieCorridor ;
  cims:multiplicity cims:M:0..1 ;
  cims:stereotype "NC" ;
  rdfs:domain nc:DCTieCorridor ;
  rdfs:range nc:DirectCurrentMasterController .

nc:DCTieCorridor.SchedulingArea a rdf:Property ;
  rdfs:label "SchedulingArea"@en ;
  rdfs:comment "The scheduling area that has this DC tie corridor." ;
  cims:AssociationUsed "Yes" ;
  cims:inverseRoleName nc:SchedulingArea.DCTieCorridor ;
  cims:multiplicity cims:M:0..1 ;
  cims:stereotype "NC" ;
  rdfs:domain nc:DCTieCorridor ;
  rdfs:range nc:SchedulingArea .

nc:DCTieCorridor.maxRegulatingReserve a rdf:Property ;
  rdfs:label "maxRegulatingReserve"@en ;
  rdfs:comment "Maximum regulating reserve." ;
  cims:dataType cim:ActivePower ;
  cims:multiplicity cims:M:0..1 ;
  cims:stereotype "NC", <http://iec.ch/TC57/NonStandard/UML#attribute> ;
  rdfs:domain nc:DCTieCorridor .

nc:DCTieCorridor.minRegulatingReserve a rdf:Property ;
  rdfs:label "minRegulatingReserve"@en ;
  rdfs:comment "Minimum regulating reserve." ;
  cims:dataType cim:ActivePower ;
  cims:multiplicity cims:M:0..1 ;
  cims:stereotype "NC", <http://iec.ch/TC57/NonStandard/UML#attribute> ;
  rdfs:domain nc:DCTieCorridor .

nc:DCTieCorridor.rampingKind a rdf:Property ;
  rdfs:label "rampingKind"@en ;
  rdfs:comment "Ramping principle is used to define a transition from one scheduled value to next one." ;
  cims:multiplicity cims:M:0..1 ;
  cims:stereotype "NC", <http://iec.ch/TC57/NonStandard/UML#attribute> ;
  rdfs:domain nc:DCTieCorridor ;
  rdfs:range nc:RampingPrincipleKind .

nc:DirectCurrentBipoleController.DirectCurrentMasterController a rdf:Property ;
  rdfs:label "DirectCurrentMasterController"@en ;
  rdfs:comment "Direct current master controller which has direct current bipole controllers." ;
  cims:AssociationUsed "Yes" ;
  cims:inverseRoleName nc:DirectCurrentMasterController.DirectCurrentBipoleController ;
  cims:multiplicity cims:M:0..1 ;
  cims:stereotype "NC" ;
  rdfs:domain nc:DirectCurrentBipoleController ;
  rdfs:range nc:DirectCurrentMasterController .

nc:DirectCurrentBipoleController.DirectCurrentPoleController a rdf:Property ;
  rdfs:label "DirectCurrentPoleController"@en ;
  rdfs:comment "DC pole controller that is controlled by a DC bipole controller." ;
  cims:AssociationUsed "No" ;
  cims:inverseRoleName nc:DirectCurrentPoleController.DirectCurrentBipoleController ;
  cims:multiplicity cims:M:2..2 ;
  cims:stereotype "NC" ;
  rdfs:domain nc:DirectCurrentBipoleController ;
  rdfs:range nc:DirectCurrentPoleController .

nc:DirectCurrentMasterController.DCTieCorridor a rdf:Property ;
  rdfs:label "DCTieCorridor"@en ;
  rdfs:comment "DCTieCorridor controlled by this direct current master controller." ;
  cims:AssociationUsed "Yes" ;
  cims:inverseRoleName nc:DCTieCorridor.DirectCurrentMasterController ;
  cims:multiplicity cims:M:0..1 ;
  cims:stereotype "NC" ;
  rdfs:domain nc:DirectCurrentMasterController ;
  rdfs:range nc:DCTieCorridor .

nc:DirectCurrentMasterController.DirectCurrentBipoleController a rdf:Property ;
  rdfs:label "DirectCurrentBipoleController"@en ;
  rdfs:comment "Direct current bipole controller which belongs to a direct current master controller." ;
  cims:AssociationUsed "No" ;
  cims:inverseRoleName nc:DirectCurrentBipoleController.DirectCurrentMasterController ;
  cims:multiplicity cims:M:0..n ;
  cims:stereotype "NC" ;
  rdfs:domain nc:DirectCurrentMasterController ;
  rdfs:range nc:DirectCurrentBipoleController .

nc:DirectCurrentMasterController.DirectCurrentPoleController a rdf:Property ;
  rdfs:label "DirectCurrentPoleController"@en ;
  rdfs:comment "DC pole controller that is controlled by this DC master controller." ;
  cims:AssociationUsed "No" ;
  cims:inverseRoleName nc:DirectCurrentPoleController.DirectCurrentMasterController ;
  cims:multiplicity cims:M:0..n ;
  cims:stereotype "NC" ;
  rdfs:domain nc:DirectCurrentMasterController ;
  rdfs:range nc:DirectCurrentPoleController .

nc:DirectCurrentMasterController.DirectCurrentSubstationController a rdf:Property ;
  rdfs:label "DirectCurrentSubstationController"@en ;
  rdfs:comment "DC substation controller controlled by a multiterminal control." ;
  cims:AssociationUsed "No" ;
  cims:inverseRoleName nc:DirectCurrentSubstationController.MultiterminalControl ;
  cims:multiplicity cims:M:2..n ;
  cims:stereotype "NC" ;
  rdfs:domain nc:DirectCurrentMasterController ;
  rdfs:range nc:DirectCurrentSubstationController .

nc:DirectCurrentPoleController.ACDCConverterController a rdf:Property ;
  rdfs:label "ACDCConverterController"@en ;
  rdfs:comment "ACDC converter controller that is controlled by a DC pole controller." ;
  cims:AssociationUsed "No" ;
  cims:inverseRoleName nc:ACDCConverterController.DirectCurrentPoleController ;
  cims:multiplicity cims:M:2..2 ;
  cims:stereotype "NC" ;
  rdfs:domain nc:DirectCurrentPoleController ;
  rdfs:range nc:ACDCConverterController .

nc:DirectCurrentPoleController.DCPole a rdf:Property ;
  rdfs:label "DCPole"@en ;
  rdfs:comment "DC pole that is controlled by a DC pole controller." ;
  cims:AssociationUsed "Yes" ;
  cims:inverseRoleName nc:DCPole.DirectCurrentPoleController ;
  cims:multiplicity cims:M:1 ;
  cims:stereotype "NC" ;
  rdfs:domain nc:DirectCurrentPoleController ;
  rdfs:range nc:DCPole .

nc:DirectCurrentPoleController.DirectCurrentBipoleController a rdf:Property ;
  rdfs:label "DirectCurrentBipoleController"@en ;
  rdfs:comment "DC bipole controller that controls this DC pole controller." ;
  cims:AssociationUsed "Yes" ;
  cims:inverseRoleName nc:DirectCurrentBipoleController.DirectCurrentPoleController ;
  cims:multiplicity cims:M:0..1 ;
  cims:stereotype "NC" ;
  rdfs:domain nc:DirectCurrentPoleController ;
  rdfs:range nc:DirectCurrentBipoleController .

nc:DirectCurrentPoleController.DirectCurrentMasterController a rdf:Property ;
  rdfs:label "DirectCurrentMasterController"@en ;
  rdfs:comment "DC master controller that has a DC pole controller." ;
  cims:AssociationUsed "Yes" ;
  cims:inverseRoleName nc:DirectCurrentMasterController.DirectCurrentPoleController ;
  cims:multiplicity cims:M:0..1 ;
  cims:stereotype "NC" ;
  rdfs:domain nc:DirectCurrentPoleController ;
  rdfs:range nc:DirectCurrentMasterController .

nc:DirectCurrentSubstationBipoleController.DCSubstationBipole a rdf:Property ;
  rdfs:label "DCSubstationBipole"@en ;
  rdfs:comment "DC substation bipole that is controlled by a DC substation bipole controller." ;
  cims:AssociationUsed "Yes" ;
  cims:inverseRoleName nc:DCSubstationBipole.DirectCurrentSubstationBipoleController ;
  cims:multiplicity cims:M:1 ;
  cims:stereotype "NC" ;
  rdfs:domain nc:DirectCurrentSubstationBipoleController ;
  rdfs:range nc:DCSubstationBipole .

nc:DirectCurrentSubstationController.MultiterminalControl a rdf:Property ;
  rdfs:label "MultiterminalControl"@en ;
  rdfs:comment "Multiterminal control that controls more than two DC substation controllers." ;
  cims:AssociationUsed "Yes" ;
  cims:inverseRoleName nc:DirectCurrentMasterController.DirectCurrentSubstationController ;
  cims:multiplicity cims:M:0..1 ;
  cims:stereotype "NC" ;
  rdfs:domain nc:DirectCurrentSubstationController ;
  rdfs:range nc:DirectCurrentMasterController .

nc:DirectCurrentSubstationPoleController.DCSubstationPole a rdf:Property ;
  rdfs:label "DCSubstationPole"@en ;
  rdfs:comment "DC substation pole that is controlled by a DC substation pole controller." ;
  cims:AssociationUsed "Yes" ;
  cims:inverseRoleName nc:DCSubstationPole.DirectCurrentSubstationPoleController ;
  cims:multiplicity cims:M:1 ;
  cims:stereotype "NC" ;
  rdfs:domain nc:DirectCurrentSubstationPoleController ;
  rdfs:range nc:DCSubstationPole .

nc:DurationOverloadLimitCurve.OperationalLimitType a rdf:Property ;
  rdfs:label "OperationalLimitType"@en ;
  rdfs:comment "The operational limit type that has this temporary duration overload limit curve." ;
  cims:AssociationUsed "No" ;
  cims:inverseRoleName nc:OperationalLimitType.TemporaryDurationOverloadLimitCurve ;
  cims:multiplicity cims:M:0..n ;
  cims:stereotype "NC" ;
  rdfs:domain nc:DurationOverloadLimitCurve ;
  rdfs:range cim:OperationalLimitType .

nc:EnergyAlignmentCoordinator.EnergyCoordinationRegion a rdf:Property ;
  rdfs:label "EnergyCoordinationRegion"@en ;
  rdfs:comment "The energy coordination region that has this energy alignment coordinator." ;
  cims:AssociationUsed "No" ;
  cims:inverseRoleName nc:EnergyCoordinationRegion.EnergyAlignmentCoordinator ;
  cims:multiplicity cims:M:0..n ;
  cims:stereotype "NC" ;
  rdfs:domain nc:EnergyAlignmentCoordinator ;
  rdfs:range nc:EnergyCoordinationRegion .

nc:EnergyBlockComponent.EnergyBlockOrder a rdf:Property ;
  rdfs:label "EnergyBlockOrder"@en ;
  rdfs:comment "The energy block order for this energy block component." ;
  cims:AssociationUsed "No" ;
  cims:inverseRoleName nc:EnergyBlockOrder.EnergyBlockComponent ;
  cims:multiplicity cims:M:1..n ;
  cims:stereotype "NC" ;
  rdfs:domain nc:EnergyBlockComponent ;
  rdfs:range nc:EnergyBlockOrder .

nc:EnergyBlockOrder.EnergyBlockComponent a rdf:Property ;
  rdfs:label "EnergyBlockComponent"@en ;
  rdfs:comment "The energy block component that has this energy block order." ;
  cims:AssociationUsed "Yes" ;
  cims:inverseRoleName nc:EnergyBlockComponent.EnergyBlockOrder ;
  cims:multiplicity cims:M:1 ;
  cims:stereotype "NC" ;
  rdfs:domain nc:EnergyBlockOrder ;
  rdfs:range nc:EnergyBlockComponent .

nc:EnergyBlockOrder.normalParticipationFactor a rdf:Property ;
  rdfs:label "normalParticipationFactor"@en ;
  rdfs:comment "Normal participation factor." ;
  cims:dataType cim:Float ;
  cims:multiplicity cims:M:0..1 ;
  cims:stereotype "NC", <http://iec.ch/TC57/NonStandard/UML#attribute> ;
  rdfs:domain nc:EnergyBlockOrder .

nc:EnergyBlockOrder.normalSequence a rdf:Property ;
  rdfs:label "normalSequence"@en ;
  rdfs:comment """Normal sequence represents the local order of the power block order.

The sequence order for a given block dispatch instruction. The sequence number need to be unique for a given block dispatch instruction, e.g. two order in the same instruction cannot have the same sequence. """ ;
  cims:dataType cim:Integer ;
  cims:multiplicity cims:M:0..1 ;
  cims:stereotype "NC", <http://iec.ch/TC57/NonStandard/UML#attribute> ;
  rdfs:domain nc:EnergyBlockOrder .

nc:EnergyBlockOrder.powerDuration a rdf:Property ;
  rdfs:label "powerDuration"@en ;
  rdfs:comment "Duration for the active power." ;
  cims:dataType cim:Duration ;
  cims:multiplicity cims:M:0..1 ;
  cims:stereotype "NC", <http://iec.ch/TC57/NonStandard/UML#attribute> ;
  rdfs:domain nc:EnergyBlockOrder .

nc:EnergyComponent.EnergyConsumer a rdf:Property ;
  rdfs:label "EnergyConsumer"@en ;
  rdfs:comment "The energy consumer that relates to this energy component." ;
  cims:AssociationUsed "Yes" ;
  cims:inverseRoleName nc:EnergyConsumer.EnergyComponent ;
  cims:multiplicity cims:M:0..1 ;
  cims:stereotype "NC" ;
  rdfs:domain nc:EnergyComponent ;
  rdfs:range cim:EnergyConsumer .

nc:EnergyComponent.EnergyGroup a rdf:Property ;
  rdfs:label "EnergyGroup"@en ;
  rdfs:comment "The energy group that has this energy component." ;
  cims:AssociationUsed "Yes" ;
  cims:inverseRoleName nc:EnergyGroup.EnergyComponent ;
  cims:multiplicity cims:M:0..1 ;
  cims:stereotype "NC" ;
  rdfs:domain nc:EnergyComponent ;
  rdfs:range nc:EnergyGroup .

nc:EnergyComponent.GeneratingUnit a rdf:Property ;
  rdfs:label "GeneratingUnit"@en ;
  rdfs:comment "The generating unit that is part of this energy component." ;
  cims:AssociationUsed "Yes" ;
  cims:inverseRoleName nc:GeneratingUnit.EnergyComponent ;
  cims:multiplicity cims:M:0..1 ;
  cims:stereotype "NC" ;
  rdfs:domain nc:EnergyComponent ;
  rdfs:range cim:GeneratingUnit .

nc:EnergyComponent.HydroPump a rdf:Property ;
  rdfs:label "HydroPump"@en ;
  rdfs:comment "The hydro pump that relates to this energy component." ;
  cims:AssociationUsed "Yes" ;
  cims:inverseRoleName nc:HydroPump.EnergyComponent ;
  cims:multiplicity cims:M:0..1 ;
  cims:stereotype "NC" ;
  rdfs:domain nc:EnergyComponent ;
  rdfs:range cim:HydroPump .

nc:EnergyComponent.PowerElectronicsUnit a rdf:Property ;
  rdfs:label "PowerElectronicsUnit"@en ;
  rdfs:comment "The power electronics unit that relates to this energy component." ;
  cims:AssociationUsed "Yes" ;
  cims:inverseRoleName nc:PowerElectronicsUnit.EnergyComponent ;
  cims:multiplicity cims:M:0..1 ;
  cims:stereotype "NC" ;
  rdfs:domain nc:EnergyComponent ;
  rdfs:range cim:PowerElectronicsUnit .

nc:EnergyConsumer.AreaDispatchableUnit a rdf:Property ;
  rdfs:label "AreaDispatchableUnit"@en ;
  rdfs:comment "Area dispatchable unit that has this energy consumer." ;
  cims:AssociationUsed "No" ;
  cims:inverseRoleName nc:AreaDispatchableUnit.EnergyConsumer ;
  cims:multiplicity cims:M:0..1 ;
  rdfs:domain cim:EnergyConsumer ;
  rdfs:range nc:AreaDispatchableUnit .

nc:EnergyConsumer.EnergyComponent a rdf:Property ;
  rdfs:label "EnergyComponent"@en ;
  rdfs:comment "The energy component that has this energy consumer." ;
  cims:AssociationUsed "No" ;
  cims:inverseRoleName nc:EnergyComponent.EnergyConsumer ;
  cims:multiplicity cims:M:0..n ;
  cims:stereotype "NC" ;
  rdfs:domain cim:EnergyConsumer ;
  rdfs:range nc:EnergyComponent .

nc:EnergyConsumer.maxEconomicP a rdf:Property ;
  rdfs:label "maxEconomicP"@en ;
  rdfs:comment "Maximum high economic active power limit, that should not exceed the maximum operating active power limit." ;
  cims:dataType cim:ActivePower ;
  cims:multiplicity cims:M:0..1 ;
  cims:stereotype "NC", <http://iec.ch/TC57/NonStandard/UML#attribute> ;
  rdfs:domain cim:EnergyConsumer .

nc:EnergyConsumer.minEconomicP a rdf:Property ;
  rdfs:label "minEconomicP"@en ;
  rdfs:comment "Low economic active power limit that shall be greater than or equal to the minimum operating active power limit." ;
  cims:dataType cim:ActivePower ;
  cims:multiplicity cims:M:0..1 ;
  cims:stereotype "NC", <http://iec.ch/TC57/NonStandard/UML#attribute> ;
  rdfs:domain cim:EnergyConsumer .

nc:EnergyConsumer.normalParticipationFactor a rdf:Property ;
  rdfs:label "normalParticipationFactor"@en ;
  rdfs:comment """Participation factor describing the entity part of the active power provided by a collection of entities (e.g. an active power forecast to a collection of entities is divided to each of the member entity according to the participation factor). Must be a positive value.
In the case of a sharing strategy, the distribution is following entities value (V) equals aggregated value (T) divided by sum of participation factors (PF), i.e. V=T/sum(PF). 
In the case of priority strategy, the item with the lowest number gets allocated energy first.""" ;
  cims:dataType cim:Float ;
  cims:multiplicity cims:M:0..1 ;
  cims:stereotype "NC", <http://iec.ch/TC57/NonStandard/UML#attribute> ;
  rdfs:domain cim:EnergyConsumer .

nc:EnergyCoordinationRegion.EnergyAlignmentCoordinator a rdf:Property ;
  rdfs:label "EnergyAlignmentCoordinator"@en ;
  rdfs:comment "The energy alignment coordinator that operates this energy coordination region." ;
  cims:AssociationUsed "Yes" ;
  cims:inverseRoleName nc:EnergyAlignmentCoordinator.EnergyCoordinationRegion ;
  cims:multiplicity cims:M:0..1 ;
  cims:stereotype "NC" ;
  rdfs:domain nc:EnergyCoordinationRegion ;
  rdfs:range nc:EnergyAlignmentCoordinator .

nc:EnergyCoordinationRegion.SchedulingArea a rdf:Property ;
  rdfs:label "SchedulingArea"@en ;
  rdfs:comment "The scheduling area that is part of this energy coordination region." ;
  cims:AssociationUsed "No" ;
  cims:inverseRoleName nc:SchedulingArea.EnergyCoordinationRegion ;
  cims:multiplicity cims:M:0..n ;
  cims:stereotype "NC" ;
  rdfs:domain nc:EnergyCoordinationRegion ;
  rdfs:range nc:SchedulingArea .

nc:EnergyGroup.EnergyComponent a rdf:Property ;
  rdfs:label "EnergyComponent"@en ;
  rdfs:comment "The energy component that is part of this power group." ;
  cims:AssociationUsed "No" ;
  cims:inverseRoleName nc:EnergyComponent.EnergyGroup ;
  cims:multiplicity cims:M:0..n ;
  cims:stereotype "NC" ;
  rdfs:domain nc:EnergyGroup ;
  rdfs:range nc:EnergyComponent .

nc:EnergyGroup.EnergyType a rdf:Property ;
  rdfs:label "EnergyType"@en ;
  rdfs:comment "The energy type that the energy group are defined by." ;
  cims:AssociationUsed "Yes" ;
  cims:inverseRoleName nc:EnergyType.EnergyGroup ;
  cims:multiplicity cims:M:0..1 ;
  cims:stereotype "NC" ;
  rdfs:domain nc:EnergyGroup ;
  rdfs:range nc:EnergyType .

nc:EnergyGroup.SchedulingArea a rdf:Property ;
  rdfs:label "SchedulingArea"@en ;
  rdfs:comment "The scheduling area that has this energy group." ;
  cims:AssociationUsed "Yes" ;
  cims:inverseRoleName nc:SchedulingArea.EnergyGroup ;
  cims:multiplicity cims:M:1 ;
  cims:stereotype "NC" ;
  rdfs:domain nc:EnergyGroup ;
  rdfs:range nc:SchedulingArea .

nc:EnergyGroup.normalParticipationFactor a rdf:Property ;
  rdfs:label "normalParticipationFactor"@en ;
  rdfs:comment "Normal participation factor for the power group in relation to scheduling area. Must be a positive value." ;
  cims:dataType cim:Float ;
  cims:multiplicity cims:M:1..1 ;
  cims:stereotype "NC", <http://iec.ch/TC57/NonStandard/UML#attribute> ;
  rdfs:domain nc:EnergyGroup .

nc:EnergyGroup.powerDuration a rdf:Property ;
  rdfs:label "powerDuration"@en ;
  rdfs:comment "Duration for the active power." ;
  cims:dataType cim:Duration ;
  cims:multiplicity cims:M:0..1 ;
  cims:stereotype "NC", <http://iec.ch/TC57/NonStandard/UML#attribute> ;
  rdfs:domain nc:EnergyGroup .

nc:EnergySourceReference.EnergyTypeReference a rdf:Property ;
  rdfs:label "EnergyTypeReference"@en ;
  rdfs:comment "Energy type reference which belong to an energy source reference." ;
  cims:AssociationUsed "No" ;
  cims:inverseRoleName nc:EnergyType.EnergySourceReference ;
  cims:multiplicity cims:M:0..n ;
  cims:stereotype "NC" ;
  rdfs:domain nc:EnergySourceReference ;
  rdfs:range nc:EnergyType .

nc:EnergyType.EnergyGroup a rdf:Property ;
  rdfs:label "EnergyGroup"@en ;
  rdfs:comment "The energy group that has this energy type." ;
  cims:AssociationUsed "No" ;
  cims:inverseRoleName nc:EnergyGroup.EnergyType ;
  cims:multiplicity cims:M:0..n ;
  cims:stereotype "NC" ;
  rdfs:domain nc:EnergyType ;
  rdfs:range nc:EnergyGroup .

nc:EnergyType.EnergySourceReference a rdf:Property ;
  rdfs:label "EnergySourceReference"@en ;
  rdfs:comment "Energy source refrence which has energy type references." ;
  cims:AssociationUsed "Yes" ;
  cims:inverseRoleName nc:EnergySourceReference.EnergyTypeReference ;
  cims:multiplicity cims:M:0..1 ;
  cims:stereotype "NC" ;
  rdfs:domain nc:EnergyType ;
  rdfs:range nc:EnergySourceReference .

nc:EnergyType.ScheduleResource a rdf:Property ;
  rdfs:label "ScheduleResource"@en ;
  rdfs:comment "Schedule resource unit that has an energy reference type." ;
  cims:AssociationUsed "No" ;
  cims:inverseRoleName nc:ScheduleResource.PrimaryEnergySource ;
  cims:multiplicity cims:M:0..n ;
  cims:stereotype "NC" ;
  rdfs:domain nc:EnergyType ;
  rdfs:range nc:ScheduleResource .

nc:EnergyType.kind a rdf:Property ;
  rdfs:label "kind"@en ;
  rdfs:comment "The kind of energy type." ;
  cims:multiplicity cims:M:1..1 ;
  cims:stereotype "NC", <http://iec.ch/TC57/NonStandard/UML#attribute> ;
  rdfs:domain nc:EnergyType ;
  rdfs:range nc:EnergyKind .

nc:Equipment.Circuit a rdf:Property ;
  rdfs:label "Circuit"@en ;
  rdfs:comment "The circuit that containts its member equipment." ;
  cims:AssociationUsed "Yes" ;
  cims:inverseRoleName nc:Circuit.Equipment ;
  cims:multiplicity cims:M:0..1 ;
  cims:stereotype "NC" ;
  rdfs:domain cim:Equipment ;
  rdfs:range nc:Circuit .

nc:Equipment.PTCTriggeredEquipment a rdf:Property ;
  rdfs:label "PTCTriggeredEquipment"@en ;
  rdfs:comment "The equipment that can trigger the power transfer corridor." ;
  cims:AssociationUsed "No" ;
  cims:inverseRoleName nc:PTCTriggeredEquipment.Equipment ;
  cims:multiplicity cims:M:0..n ;
  cims:stereotype "NC" ;
  rdfs:domain cim:Equipment ;
  rdfs:range nc:PTCTriggeredEquipment .

nc:EquipmentController.RegulatingCondEq a rdf:Property ;
  rdfs:label "RegulatingCondEq"@en ;
  rdfs:comment "All regulating conducting equipment that belongs to this equipment controller." ;
  cims:AssociationUsed "No" ;
  cims:inverseRoleName nc:RegulatingCondEq.EquipmentController ;
  cims:multiplicity cims:M:0..n ;
  cims:stereotype "NC" ;
  rdfs:domain nc:EquipmentController ;
  rdfs:range cim:RegulatingCondEq .

nc:EquipmentController.SystemControl a rdf:Property ;
  rdfs:label "SystemControl"@en ;
  rdfs:comment "System control which controls this equipment controller." ;
  cims:AssociationUsed "No" ;
  cims:inverseRoleName nc:SystemControl.EquipmentController ;
  cims:multiplicity cims:M:0..1 ;
  cims:stereotype "NC" ;
  rdfs:domain nc:EquipmentController ;
  rdfs:range nc:SystemControl .

nc:EquivalentInjection.InjectionController a rdf:Property ;
  rdfs:label "InjectionController"@en ;
  rdfs:comment "Injection controller which controls the equivalent injection." ;
  cims:AssociationUsed "Yes" ;
  cims:inverseRoleName nc:InjectionController.EquivalentInjection ;
  cims:multiplicity cims:M:0..1 ;
  cims:stereotype "NC" ;
  rdfs:domain cim:EquivalentInjection ;
  rdfs:range nc:InjectionController .

nc:ExceptionalPowerTransferCorridor.PTCTriggeredEquipment a rdf:Property ;
  rdfs:label "PTCTriggeredEquipment"@en ;
  rdfs:comment "The equipment that triggers this exceptional power transfer corridor." ;
  cims:AssociationUsed "No" ;
  cims:inverseRoleName nc:PTCTriggeredEquipment.ExceptionalPowerTransferCorridor ;
  cims:multiplicity cims:M:1..n ;
  cims:stereotype "NC" ;
  rdfs:domain nc:ExceptionalPowerTransferCorridor ;
  rdfs:range nc:PTCTriggeredEquipment .

nc:FACTSEquipment.LossCurve a rdf:Property ;
  rdfs:label "LossCurve"@en ;
  rdfs:comment "The loss curve for the FACTS equipment." ;
  cims:AssociationUsed "No" ;
  cims:inverseRoleName nc:LossCurve.FACTSEquipment ;
  cims:multiplicity cims:M:0..n ;
  cims:stereotype "NC" ;
  rdfs:domain nc:FACTSEquipment ;
  rdfs:range nc:LossCurve .

nc:FACTSEquipment.maxC a rdf:Property ;
  rdfs:label "maxC"@en ;
  rdfs:comment "Capacitive reactance at maximum reactive power.  Shall always be positive." ;
  cims:dataType cim:Reactance ;
  cims:multiplicity cims:M:0..1 ;
  cims:stereotype "NC", <http://iec.ch/TC57/NonStandard/UML#attribute> ;
  rdfs:domain nc:FACTSEquipment .

nc:FACTSEquipment.maxL a rdf:Property ;
  rdfs:label "maxL"@en ;
  rdfs:comment "Inductive rating at maximum inductive reactive power.  Shall always be negative.  " ;
  cims:dataType cim:Reactance ;
  cims:multiplicity cims:M:0..1 ;
  cims:stereotype "NC", <http://iec.ch/TC57/NonStandard/UML#attribute> ;
  rdfs:domain nc:FACTSEquipment .

nc:FACTSEquipment.minC a rdf:Property ;
  rdfs:label "minC"@en ;
  rdfs:comment "Capacitive reactance at minimum reactive power.  Shall always be positive." ;
  cims:dataType cim:Reactance ;
  cims:multiplicity cims:M:0..1 ;
  cims:stereotype "NC", <http://iec.ch/TC57/NonStandard/UML#attribute> ;
  rdfs:domain nc:FACTSEquipment .

nc:FACTSEquipment.minL a rdf:Property ;
  rdfs:label "minL"@en ;
  rdfs:comment "Inductive rating at minimum inductive reactive power.  Shall always be negative.  " ;
  cims:dataType cim:Reactance ;
  cims:multiplicity cims:M:0..1 ;
  cims:stereotype "NC", <http://iec.ch/TC57/NonStandard/UML#attribute> ;
  rdfs:domain nc:FACTSEquipment .

nc:FACTSEquipment.ratedC a rdf:Property ;
  rdfs:label "ratedC"@en ;
  rdfs:comment "Capacitive reactance at maximum reactive power.  Shall always be positive." ;
  cims:dataType cim:Reactance ;
  cims:multiplicity cims:M:0..1 ;
  cims:stereotype "NC", <http://iec.ch/TC57/NonStandard/UML#attribute> ;
  rdfs:domain nc:FACTSEquipment .

nc:FACTSEquipment.ratedI a rdf:Property ;
  rdfs:label "ratedI"@en ;
  rdfs:comment "Rated current of the FACTS equipment." ;
  cims:dataType cim:CurrentFlow ;
  cims:multiplicity cims:M:0..1 ;
  cims:stereotype "NC", <http://iec.ch/TC57/NonStandard/UML#attribute> ;
  rdfs:domain nc:FACTSEquipment .

nc:FACTSEquipment.ratedL a rdf:Property ;
  rdfs:label "ratedL"@en ;
  rdfs:comment "Inductive rating at maximum inductive reactive power.  Shall always be negative.  " ;
  cims:dataType cim:Reactance ;
  cims:multiplicity cims:M:0..1 ;
  cims:stereotype "NC", <http://iec.ch/TC57/NonStandard/UML#attribute> ;
  rdfs:domain nc:FACTSEquipment .

nc:FACTSEquipment.ratedU a rdf:Property ;
  rdfs:label "ratedU"@en ;
  rdfs:comment "Rated voltage of the FACTS equipment." ;
  cims:dataType cim:Voltage ;
  cims:multiplicity cims:M:0..1 ;
  cims:stereotype "NC", <http://iec.ch/TC57/NonStandard/UML#attribute> ;
  rdfs:domain nc:FACTSEquipment .

nc:FACTSEquipment.slope a rdf:Property ;
  rdfs:label "slope"@en ;
  rdfs:comment """The characteristics slope which defines how the reactive power output changes in proportion to the difference between the regulated bus voltage and the voltage setpoint.
The attribute shall be a positive value or zero.""" ;
  cims:dataType cim:VoltagePerReactivePower ;
  cims:multiplicity cims:M:1..1 ;
  cims:stereotype "NC", <http://iec.ch/TC57/NonStandard/UML#attribute> ;
  rdfs:domain nc:FACTSEquipment .

nc:Feeder.SubSchedulingArea a rdf:Property ;
  rdfs:label "SubSchedulingArea"@en ;
  rdfs:comment "The subscheduling area that has this feeder." ;
  cims:AssociationUsed "Yes" ;
  cims:inverseRoleName nc:SubSchedulingArea.Feeder ;
  cims:multiplicity cims:M:0..1 ;
  cims:stereotype "NC" ;
  rdfs:domain cim:Feeder ;
  rdfs:range nc:SubSchedulingArea .

nc:FlexibleEnergyUnit.buffer a rdf:Property ;
  rdfs:label "buffer"@en ;
  rdfs:comment "The active power, that has the flexibility to operate as production and/or consumption. The buffer is bound. Example are heat pump, cooling system, embedded batteries including electric vehicle. Load sign convention is used, i.e. positive sign means flow out from a node." ;
  cims:dataType cim:ActivePower ;
  cims:multiplicity cims:M:0..1 ;
  cims:stereotype "NC", <http://iec.ch/TC57/NonStandard/UML#attribute> ;
  rdfs:domain nc:FlexibleEnergyUnit .

nc:FlexibleEnergyUnit.timeShift a rdf:Property ;
  rdfs:label "timeShift"@en ;
  rdfs:comment "The active power, that can be shifted from one pricing interval (market time unit) to another. It is expected to be a limited on the length of the shift. Example from household could be washing machine or dishwasher. Example from industry is the possible to shut down a machine for the relevant period. Load sign convention is used, i.e. positive sign means flow out from a node." ;
  cims:dataType cim:ActivePower ;
  cims:multiplicity cims:M:0..1 ;
  cims:stereotype "NC", <http://iec.ch/TC57/NonStandard/UML#attribute> ;
  rdfs:domain nc:FlexibleEnergyUnit .

nc:FlexibleEnergyUnit.unconstrained a rdf:Property ;
  rdfs:label "unconstrained"@en ;
  rdfs:comment "The active power, that has the flexibility to operate as production without any bound by a buffer. Example are alternative heating (wood, gas, diesel etc) or power generators. Load sign convention is used, i.e. positive sign means flow out from a node." ;
  cims:dataType cim:ActivePower ;
  cims:multiplicity cims:M:0..1 ;
  cims:stereotype "NC", <http://iec.ch/TC57/NonStandard/UML#attribute> ;
  rdfs:domain nc:FlexibleEnergyUnit .

nc:FlexibleEnergyUnit.uncontrollable a rdf:Property ;
  rdfs:label "uncontrollable"@en ;
  rdfs:comment "The active power, that forms the base consumption for the unit. This is measured and expected consumption. Load sign convention is used, i.e. positive sign means flow out from a node." ;
  cims:dataType cim:ActivePower ;
  cims:multiplicity cims:M:0..1 ;
  cims:stereotype "NC", <http://iec.ch/TC57/NonStandard/UML#attribute> ;
  rdfs:domain nc:FlexibleEnergyUnit .

nc:FossilFuel.FuelStorage a rdf:Property ;
  rdfs:label "FuelStorage"@en ;
  rdfs:comment "Fuel storage that store fossil fuels." ;
  cims:AssociationUsed "Yes" ;
  cims:inverseRoleName nc:FuelStorage.FossilFuel ;
  cims:multiplicity cims:M:0..1 ;
  cims:stereotype "NC" ;
  rdfs:domain cim:FossilFuel ;
  rdfs:range nc:FuelStorage .

nc:FrequencyMonitoringTerminal.PowerFrequencyController a rdf:Property ;
  rdfs:label "PowerFrequencyController"@en ;
  rdfs:comment "Power frequency controller that has this frequency monitoring terminal." ;
  cims:AssociationUsed "Yes" ;
  cims:inverseRoleName nc:PowerFrequencyController.FrequencyMonitoringTerminal ;
  cims:multiplicity cims:M:0..1 ;
  cims:stereotype "NC" ;
  rdfs:domain nc:FrequencyMonitoringTerminal ;
  rdfs:range nc:PowerFrequencyController .

nc:FrequencyMonitoringTerminal.Terminal a rdf:Property ;
  rdfs:label "Terminal"@en ;
  rdfs:comment "The terminal for this frequency monitoring terminal." ;
  cims:AssociationUsed "Yes" ;
  cims:inverseRoleName nc:Terminal.FrequencyMonitoringTerminal ;
  cims:multiplicity cims:M:0..1 ;
  cims:stereotype "NC" ;
  rdfs:domain nc:FrequencyMonitoringTerminal ;
  rdfs:range cim:Terminal .

nc:FrequencyMonitoringTerminal.mRID a rdf:Property ;
  rdfs:label "mRID"@en ;
  rdfs:comment """Master resource identifier issued by a model authority. The mRID is unique within an exchange context. Global uniqueness is easily achieved by using a UUID, as specified in RFC 4122, for the mRID. The use of UUID is strongly recommended.
For CIMXML data files in RDF syntax conforming to IEC 61970-552, the mRID is mapped to rdf:ID or rdf:about attributes that identify CIM object elements.""" ;
  cims:dataType cim:String ;
  cims:multiplicity cims:M:1..1 ;
  cims:stereotype "NC", <http://iec.ch/TC57/NonStandard/UML#attribute> ;
  rdfs:domain nc:FrequencyMonitoringTerminal .

nc:FrequencyMonitoringTerminal.priority a rdf:Property ;
  rdfs:label "priority"@en ;
  rdfs:comment "Value 0 means ignore priority. 1 means the highest priority, 2 is the second highest priority." ;
  cims:dataType cim:Integer ;
  cims:multiplicity cims:M:1..1 ;
  cims:stereotype "NC", <http://iec.ch/TC57/NonStandard/UML#attribute> ;
  rdfs:domain nc:FrequencyMonitoringTerminal .

nc:FuelStorage.FossilFuel a rdf:Property ;
  rdfs:label "FossilFuel"@en ;
  rdfs:comment "Fossil fuel stored in a fuel storage." ;
  cims:AssociationUsed "No" ;
  cims:inverseRoleName nc:FossilFuel.FuelStorage ;
  cims:multiplicity cims:M:0..n ;
  cims:stereotype "NC" ;
  rdfs:domain nc:FuelStorage ;
  rdfs:range cim:FossilFuel .

nc:FunctionBlock.AutomationBlockGroup a rdf:Property ;
  rdfs:label "AutomationBlockGroup"@en ;
  rdfs:comment "Automation block group which has function blocks." ;
  cims:AssociationUsed "Yes" ;
  cims:inverseRoleName nc:AutomationBlockGroup.FunctionBlock ;
  cims:multiplicity cims:M:0..1 ;
  cims:stereotype "NC" ;
  rdfs:domain nc:FunctionBlock ;
  rdfs:range nc:AutomationBlockGroup .

nc:FunctionBlock.AutomationFunction a rdf:Property ;
  rdfs:label "AutomationFunction"@en ;
  rdfs:comment "Automation function describe automation that this function block is part of." ;
  cims:AssociationUsed "Yes" ;
  cims:inverseRoleName nc:AutomationFunction.FunctionBlock ;
  cims:multiplicity cims:M:0..1 ;
  cims:stereotype "NC" ;
  rdfs:domain nc:FunctionBlock ;
  rdfs:range nc:AutomationFunction .

nc:FunctionBlock.FunctionOutputVariable a rdf:Property ;
  rdfs:label "FunctionOutputVariable"@en ;
  rdfs:comment "Function output variable describe the output or codomain to the function block." ;
  cims:AssociationUsed "No" ;
  cims:inverseRoleName nc:FunctionOutputVariable.FunctionBlock ;
  cims:multiplicity cims:M:1..n ;
  cims:stereotype "NC", <http://iec.ch/TC57/NonStandard/UML#ofAggregate> ;
  rdfs:domain nc:FunctionBlock ;
  rdfs:range nc:FunctionOutputVariable .

nc:FunctionBlock.Input a rdf:Property ;
  rdfs:label "Input"@en ;
  rdfs:comment "Function input variable describe the input or domain to the function block." ;
  cims:AssociationUsed "No" ;
  cims:inverseRoleName nc:FunctionInputVariable.Function ;
  cims:multiplicity cims:M:1..n ;
  cims:stereotype "NC", <http://iec.ch/TC57/NonStandard/UML#ofAggregate> ;
  rdfs:domain nc:FunctionBlock ;
  rdfs:range nc:FunctionInputVariable .

nc:FunctionBlock.normalEnabled a rdf:Property ;
  rdfs:label "normalEnabled"@en ;
  rdfs:comment "True, if the function block is enabled (active). Otherwise false." ;
  cims:dataType cim:Boolean ;
  cims:multiplicity cims:M:0..1 ;
  cims:stereotype "NC", <http://iec.ch/TC57/NonStandard/UML#attribute> ;
  rdfs:domain nc:FunctionBlock .

nc:FunctionInputVariable.Function a rdf:Property ;
  rdfs:label "Function"@en ;
  rdfs:comment "Function block describe the function that function input variable provides the domain for." ;
  cims:AssociationUsed "Yes" ;
  cims:inverseRoleName nc:FunctionBlock.Input ;
  cims:multiplicity cims:M:1 ;
  cims:stereotype "NC" ;
  rdfs:domain nc:FunctionInputVariable ;
  rdfs:range nc:FunctionBlock .

nc:FunctionOutputVariable.FunctionBlock a rdf:Property ;
  rdfs:label "FunctionBlock"@en ;
  rdfs:comment "Function block describe the function that function output variable provides the codomain for." ;
  cims:AssociationUsed "Yes" ;
  cims:inverseRoleName nc:FunctionBlock.FunctionOutputVariable ;
  cims:multiplicity cims:M:1 ;
  cims:stereotype "NC" ;
  rdfs:domain nc:FunctionOutputVariable ;
  rdfs:range nc:FunctionBlock .

nc:FunctionOutputVariable.PropertyReference a rdf:Property ;
  rdfs:label "PropertyReference"@en ;
  rdfs:comment "Property reference refers to a given class and property that is populated by the function output variable." ;
  cims:AssociationUsed "Yes" ;
  cims:inverseRoleName nc:PropertyReference.FunctionOutputVariable ;
  cims:multiplicity cims:M:1 ;
  cims:stereotype "NC" ;
  rdfs:domain nc:FunctionOutputVariable ;
  rdfs:range nc:PropertyReference .

nc:GateInputPin.absoluteValue a rdf:Property ;
  rdfs:label "absoluteValue"@en ;
  rdfs:comment "Indicates if the absolute value is used for comparison. If true, use the absolute value. If false, use the complex value (vector). " ;
  cims:dataType cim:Boolean ;
  cims:multiplicity cims:M:0..1 ;
  cims:stereotype "NC", <http://iec.ch/TC57/NonStandard/UML#attribute> ;
  rdfs:domain nc:GateInputPin .

nc:GateInputPin.duration a rdf:Property ;
  rdfs:label "duration"@en ;
  rdfs:comment "The time duration for which the condition is satisfied before acting. Default is 0 seconds." ;
  cims:dataType cim:Duration ;
  cims:multiplicity cims:M:0..1 ;
  cims:stereotype "NC", <http://iec.ch/TC57/NonStandard/UML#attribute> ;
  rdfs:domain nc:GateInputPin .

nc:GateInputPin.logicKind a rdf:Property ;
  rdfs:label "logicKind"@en ;
  rdfs:comment "The logical operator kind used for comparison." ;
  cims:multiplicity cims:M:0..1 ;
  cims:stereotype "NC", <http://iec.ch/TC57/NonStandard/UML#attribute> ;
  rdfs:domain nc:GateInputPin ;
  rdfs:range nc:LogicalOperatorsKind .

nc:GateInputPin.negate a rdf:Property ;
  rdfs:label "negate"@en ;
  rdfs:comment "Invert/negate the result of the comparison." ;
  cims:dataType cim:Boolean ;
  cims:multiplicity cims:M:0..1 ;
  cims:stereotype "NC", <http://iec.ch/TC57/NonStandard/UML#attribute> ;
  rdfs:domain nc:GateInputPin .

nc:GateInputPin.thresholdPercentage a rdf:Property ;
  rdfs:label "thresholdPercentage"@en ;
  rdfs:comment """The threshold percentage that should be used for compare with the percentage change between input value and threshold value.
The allowed value range is [0,100].""" ;
  cims:dataType cim:PerCent ;
  cims:multiplicity cims:M:0..1 ;
  cims:stereotype "NC", <http://iec.ch/TC57/NonStandard/UML#attribute> ;
  rdfs:domain nc:GateInputPin .

nc:GateInputPin.thresholdValue a rdf:Property ;
  rdfs:label "thresholdValue"@en ;
  rdfs:comment "The threshold value that should be used for compare with the input value." ;
  cims:dataType cim:Float ;
  cims:multiplicity cims:M:0..1 ;
  cims:stereotype "NC", <http://iec.ch/TC57/NonStandard/UML#attribute> ;
  rdfs:domain nc:GateInputPin .

nc:GeneratingUnit.AreaDispatchableUnit a rdf:Property ;
  rdfs:label "AreaDispatchableUnit"@en ;
  rdfs:comment "The area dispatchable unit for this generating unit. " ;
  cims:AssociationUsed "No" ;
  cims:inverseRoleName nc:AreaDispatchableUnit.GeneratingUnit ;
  cims:multiplicity cims:M:0..1 ;
  cims:stereotype "NC", <http://iec.ch/TC57/NonStandard/UML#ofAggregate> ;
  rdfs:domain cim:GeneratingUnit ;
  rdfs:range nc:AreaDispatchableUnit .

nc:GeneratingUnit.EnergyComponent a rdf:Property ;
  rdfs:label "EnergyComponent"@en ;
  rdfs:comment "The energy component that has this generating unit." ;
  cims:AssociationUsed "No" ;
  cims:inverseRoleName nc:EnergyComponent.GeneratingUnit ;
  cims:multiplicity cims:M:0..n ;
  cims:stereotype "NC" ;
  rdfs:domain cim:GeneratingUnit ;
  rdfs:range nc:EnergyComponent .

nc:GeneratingUnit.ScheduleResource a rdf:Property ;
  rdfs:label "ScheduleResource"@en ;
  rdfs:comment "The schedule resource that has this generating unit." ;
  cims:AssociationUsed "Yes" ;
  cims:inverseRoleName nc:ScheduleResource.GeneratingUnit ;
  cims:multiplicity cims:M:0..1 ;
  cims:stereotype "NC" ;
  rdfs:domain cim:GeneratingUnit ;
  rdfs:range nc:ScheduleResource .

nc:GeneratingUnit.coolDownTime a rdf:Property ;
  rdfs:label "coolDownTime"@en ;
  rdfs:comment "Time it takes from a unit shutdown until it is considered cold." ;
  cims:dataType cim:Duration ;
  cims:multiplicity cims:M:0..1 ;
  cims:stereotype "NC", <http://iec.ch/TC57/NonStandard/UML#attribute> ;
  rdfs:domain cim:GeneratingUnit .

nc:GeneratingUnit.maxStartupLoad a rdf:Property ;
  rdfs:label "maxStartupLoad"@en ;
  rdfs:comment "Maximum consumption by the generating unit as part of the startup process." ;
  cims:dataType cim:ActivePower ;
  cims:multiplicity cims:M:0..1 ;
  cims:stereotype "NC", <http://iec.ch/TC57/NonStandard/UML#attribute> ;
  rdfs:domain cim:GeneratingUnit .

nc:GeneratingUnit.minimumUpTime a rdf:Property ;
  rdfs:label "minimumUpTime"@en ;
  rdfs:comment "The time that a generating unit has to stay running after it has been switched on by the Remedial Action Optimizer." ;
  cims:dataType cim:Duration ;
  cims:multiplicity cims:M:0..1 ;
  cims:stereotype "NC", <http://iec.ch/TC57/NonStandard/UML#attribute> ;
  rdfs:domain cim:GeneratingUnit .

nc:GeneratingUnit.normalMustRunP a rdf:Property ;
  rdfs:label "normalMustRunP"@en ;
  rdfs:comment "Normal minimum active power injection that is needed to meet must-run requirement. This value can be higher or equal to minimum operational limit. Load sign convention is used, i.e. positive sign means flow out from a node." ;
  cims:dataType cim:ActivePower ;
  cims:multiplicity cims:M:0..1 ;
  cims:stereotype "NC", <http://iec.ch/TC57/NonStandard/UML#attribute> ;
  rdfs:domain cim:GeneratingUnit .

nc:GeneratingUnit.normalMustRunQ a rdf:Property ;
  rdfs:label "normalMustRunQ"@en ;
  rdfs:comment "Normal minimum reactive power injection that is needed to meet must-run requirement. This value can be higher or equal to minimum operational limit. Load sign convention is used, i.e. positive sign means flow out from a node." ;
  cims:dataType cim:ReactivePower ;
  cims:multiplicity cims:M:0..1 ;
  cims:stereotype "NC", <http://iec.ch/TC57/NonStandard/UML#attribute> ;
  rdfs:domain cim:GeneratingUnit .

nc:GeneratingUnit.normalStartupCost a rdf:Property ;
  rdfs:label "normalStartupCost"@en ;
  rdfs:comment "The normal initial startup cost incurred for each start of the GeneratingUnit." ;
  cims:dataType cim:Money ;
  cims:multiplicity cims:M:0..1 ;
  cims:stereotype "NC", <http://iec.ch/TC57/NonStandard/UML#attribute> ;
  rdfs:domain cim:GeneratingUnit .

nc:GeneratingUnit.normalWarmStartupCost a rdf:Property ;
  rdfs:label "normalWarmStartupCost"@en ;
  rdfs:comment "The normal warm startup cost incurred for each start of the GeneratingUnit." ;
  cims:dataType cim:Money ;
  cims:multiplicity cims:M:0..1 ;
  cims:stereotype "NC", <http://iec.ch/TC57/NonStandard/UML#attribute> ;
  rdfs:domain cim:GeneratingUnit .

nc:GeneratingUnit.runningLeadTime a rdf:Property ;
  rdfs:label "runningLeadTime"@en ;
  rdfs:comment "Time it takes to change the schedule when the unit is operating due to technical configuration of a supporting system, e.g. gas pipeline. " ;
  cims:dataType cim:Duration ;
  cims:multiplicity cims:M:0..1 ;
  cims:stereotype "NC", <http://iec.ch/TC57/NonStandard/UML#attribute> ;
  rdfs:domain cim:GeneratingUnit .

nc:GeneratingUnit.shutdownCost a rdf:Property ;
  rdfs:label "shutdownCost"@en ;
  rdfs:comment "The shutdown cost incurred for each shutdown of the GeneratingUnit." ;
  cims:dataType cim:Money ;
  cims:multiplicity cims:M:0..1 ;
  cims:stereotype "NC", <http://iec.ch/TC57/NonStandard/UML#attribute> ;
  rdfs:domain cim:GeneratingUnit .

nc:GeneratingUnit.shutdownTime a rdf:Property ;
  rdfs:label "shutdownTime"@en ;
  rdfs:comment "Time it takes to shutdown the unit." ;
  cims:dataType cim:Duration ;
  cims:multiplicity cims:M:0..1 ;
  cims:stereotype "NC", <http://iec.ch/TC57/NonStandard/UML#attribute> ;
  rdfs:domain cim:GeneratingUnit .

nc:GeneratingUnit.startupRampRate a rdf:Property ;
  rdfs:label "startupRampRate"@en ;
  rdfs:comment """The startup ramp rate of the generating unit which describes the speed of change of active power from zero to the minimum active power.
When the ramp is not provided, the optimisation process shall consider the change as an instant change of active power from zero to minimum active power.""" ;
  cims:dataType cim:ActivePowerChangeRate ;
  cims:multiplicity cims:M:0..1 ;
  cims:stereotype "NC", <http://iec.ch/TC57/NonStandard/UML#attribute> ;
  rdfs:domain cim:GeneratingUnit .

nc:GeneratingUnit.warmStartupTime a rdf:Property ;
  rdfs:label "warmStartupTime"@en ;
  rdfs:comment "Time it takes to startup the unit when it is warm." ;
  cims:dataType cim:Duration ;
  cims:multiplicity cims:M:0..1 ;
  cims:stereotype "NC", <http://iec.ch/TC57/NonStandard/UML#attribute> ;
  rdfs:domain cim:GeneratingUnit .

nc:GeothermalGeneratingUnit.kind a rdf:Property ;
  rdfs:label "kind"@en ;
  rdfs:comment "Kind of geothermal generating unit." ;
  cims:multiplicity cims:M:1..1 ;
  cims:stereotype "NC", <http://iec.ch/TC57/NonStandard/UML#attribute> ;
  rdfs:domain nc:GeothermalGeneratingUnit ;
  rdfs:range nc:GeothermalUnitKind .

nc:HydroPump.AreaDispatchableUnit a rdf:Property ;
  rdfs:label "AreaDispatchableUnit"@en ;
  rdfs:comment "Area dispatchable unit associated with a Hydro Pump." ;
  cims:AssociationUsed "No" ;
  cims:inverseRoleName nc:AreaDispatchableUnit.HydroPump ;
  cims:multiplicity cims:M:0..1 ;
  cims:stereotype "NC" ;
  rdfs:domain cim:HydroPump ;
  rdfs:range nc:AreaDispatchableUnit .

nc:HydroPump.EnergyComponent a rdf:Property ;
  rdfs:label "EnergyComponent"@en ;
  rdfs:comment "The energy component that has this hydro pump." ;
  cims:AssociationUsed "No" ;
  cims:inverseRoleName nc:EnergyComponent.HydroPump ;
  cims:multiplicity cims:M:0..n ;
  cims:stereotype "NC" ;
  rdfs:domain cim:HydroPump ;
  rdfs:range nc:EnergyComponent .

nc:HydroPump.ScheduleResource a rdf:Property ;
  rdfs:label "ScheduleResource"@en ;
  rdfs:comment "The schedule resource that has this hydro pump." ;
  cims:AssociationUsed "Yes" ;
  cims:inverseRoleName nc:ScheduleResource.HydroPump ;
  cims:multiplicity cims:M:0..1 ;
  cims:stereotype "NC" ;
  rdfs:domain cim:HydroPump ;
  rdfs:range nc:ScheduleResource .

nc:HydroPump.maxEconomicP a rdf:Property ;
  rdfs:label "maxEconomicP"@en ;
  rdfs:comment "Maximum high economic active power limit, that should not exceed the maximum operating active power limit." ;
  cims:dataType cim:ActivePower ;
  cims:multiplicity cims:M:0..1 ;
  cims:stereotype "NC", <http://iec.ch/TC57/NonStandard/UML#attribute> ;
  rdfs:domain cim:HydroPump .

nc:HydroPump.maxOperatingP a rdf:Property ;
  rdfs:label "maxOperatingP"@en ;
  rdfs:comment "This is the maximum operating active power limit the dispatcher can enter for this unit." ;
  cims:dataType cim:ActivePower ;
  cims:multiplicity cims:M:0..1 ;
  cims:stereotype "NC", <http://iec.ch/TC57/NonStandard/UML#attribute> ;
  rdfs:domain cim:HydroPump .

nc:HydroPump.minEconomicP a rdf:Property ;
  rdfs:label "minEconomicP"@en ;
  rdfs:comment "Low economic active power limit that shall be greater than or equal to the minimum operating active power limit." ;
  cims:dataType cim:ActivePower ;
  cims:multiplicity cims:M:0..1 ;
  cims:stereotype "NC", <http://iec.ch/TC57/NonStandard/UML#attribute> ;
  rdfs:domain cim:HydroPump .

nc:HydroPump.minOperatingP a rdf:Property ;
  rdfs:label "minOperatingP"@en ;
  rdfs:comment "This is the minimum operating active power limit the dispatcher can enter for this unit." ;
  cims:dataType cim:ActivePower ;
  cims:multiplicity cims:M:0..1 ;
  cims:stereotype "NC", <http://iec.ch/TC57/NonStandard/UML#attribute> ;
  rdfs:domain cim:HydroPump .

nc:HydroPump.normalParticipationFactor a rdf:Property ;
  rdfs:label "normalParticipationFactor"@en ;
  rdfs:comment """Participation factor describing the entity part of the active power provided by a collection of entities (e.g. an active power forecast to a collection of entities is divided to each of the member entity according to the participation factor). Must be a positive value.
In the case of a sharing strategy, the distribution is following entities value (V) equals aggregated value (T) divided by sum of participation factors (PF), i.e. V=T/sum(PF). 
In the case of priority strategy, the item with the lowest number gets allocated energy first.""" ;
  cims:dataType cim:Float ;
  cims:multiplicity cims:M:0..1 ;
  cims:stereotype "NC", <http://iec.ch/TC57/NonStandard/UML#attribute> ;
  rdfs:domain cim:HydroPump .

nc:InfeedLimit.InfeedTerminal a rdf:Property ;
  rdfs:label "InfeedTerminal"@en ;
  rdfs:comment "Infeed terminal that has infeed constraints." ;
  cims:AssociationUsed "No" ;
  cims:inverseRoleName nc:InfeedTerminal.InfeedConstraint ;
  cims:multiplicity cims:M:0..n ;
  cims:stereotype "NC" ;
  rdfs:domain nc:InfeedLimit ;
  rdfs:range nc:InfeedTerminal .

nc:InfeedLimit.normalValueA a rdf:Property ;
  rdfs:label "normalValueA"@en ;
  rdfs:comment "The normal current limit. The attribute shall be a positive value or zero." ;
  cims:dataType cim:CurrentFlow ;
  cims:multiplicity cims:M:0..1 ;
  cims:stereotype "NC", <http://iec.ch/TC57/NonStandard/UML#attribute> ;
  rdfs:domain nc:InfeedLimit .

nc:InfeedLimit.normalValueW a rdf:Property ;
  rdfs:label "normalValueW"@en ;
  rdfs:comment "The normal value of active power limit. The attribute shall be a positive value or zero." ;
  cims:dataType cim:ActivePower ;
  cims:multiplicity cims:M:0..1 ;
  cims:stereotype "NC", <http://iec.ch/TC57/NonStandard/UML#attribute> ;
  rdfs:domain nc:InfeedLimit .

nc:InfeedTerminal.ACDCTerminal a rdf:Property ;
  rdfs:label "ACDCTerminal"@en ;
  rdfs:comment "ACDCTerminal which is connected to an infeed terminal." ;
  cims:AssociationUsed "Yes" ;
  cims:inverseRoleName nc:ACDCTerminal.InfeedTerminal ;
  cims:multiplicity cims:M:1 ;
  cims:stereotype "NC" ;
  rdfs:domain nc:InfeedTerminal ;
  rdfs:range cim:ACDCTerminal .

nc:InfeedTerminal.InfeedConstraint a rdf:Property ;
  rdfs:label "InfeedConstraint"@en ;
  rdfs:comment "Infeed constraint which belongs to an infeed terminal." ;
  cims:AssociationUsed "Yes" ;
  cims:inverseRoleName nc:InfeedLimit.InfeedTerminal ;
  cims:multiplicity cims:M:1 ;
  cims:stereotype "NC" ;
  rdfs:domain nc:InfeedTerminal ;
  rdfs:range nc:InfeedLimit .

nc:InfeedTerminal.mRID a rdf:Property ;
  rdfs:label "mRID"@en ;
  rdfs:comment """Master resource identifier issued by a model authority. The mRID is unique within an exchange context. Global uniqueness is easily achieved by using a UUID, as specified in RFC 4122, for the mRID. The use of UUID is strongly recommended.
For CIMXML data files in RDF syntax conforming to IEC 61970-552, the mRID is mapped to rdf:ID or rdf:about attributes that identify CIM object elements.""" ;
  cims:dataType cim:String ;
  cims:multiplicity cims:M:1..1 ;
  cims:stereotype "NC", <http://iec.ch/TC57/NonStandard/UML#attribute> ;
  rdfs:domain nc:InfeedTerminal .

nc:InjectionController.EquivalentInjection a rdf:Property ;
  rdfs:label "EquivalentInjection"@en ;
  rdfs:comment "Equivalent injection controlled by the injection controller." ;
  cims:AssociationUsed "No" ;
  cims:inverseRoleName nc:EquivalentInjection.InjectionController ;
  cims:multiplicity cims:M:0..n ;
  cims:stereotype "NC" ;
  rdfs:domain nc:InjectionController ;
  rdfs:range cim:EquivalentInjection .

nc:Line.ACTieCorridor a rdf:Property ;
  rdfs:label "ACTieCorridor"@en ;
  rdfs:comment "ACTieCorridor that the line is part of." ;
  cims:AssociationUsed "Yes" ;
  cims:inverseRoleName nc:ACTieCorridor.Line ;
  cims:multiplicity cims:M:0..1 ;
  cims:stereotype "NC" ;
  rdfs:domain cim:Line ;
  rdfs:range nc:ACTieCorridor .

nc:Line.SchedulingArea a rdf:Property ;
  rdfs:label "SchedulingArea"@en ;
  rdfs:comment "The scheduling area that has this line." ;
  cims:AssociationUsed "Yes" ;
  cims:inverseRoleName nc:SchedulingArea.Line ;
  cims:multiplicity cims:M:0..1 ;
  cims:stereotype "NC" ;
  rdfs:domain cim:Line ;
  rdfs:range nc:SchedulingArea .

nc:LoadFrequencyControlArea.FrequencyControlOperator a rdf:Property ;
  rdfs:label "FrequencyControlOperator"@en ;
  rdfs:comment "The frequency control operator that operates this frequency control area." ;
  cims:AssociationUsed "Yes" ;
  cims:inverseRoleName nc:LoadFrequencyControlOperator.FrequencyControlArea ;
  cims:multiplicity cims:M:0..1 ;
  cims:stereotype "NC" ;
  rdfs:domain nc:LoadFrequencyControlArea ;
  rdfs:range nc:LoadFrequencyControlOperator .

nc:LoadFrequencyControlArea.LoadFrequencyControlBlock a rdf:Property ;
  rdfs:label "LoadFrequencyControlBlock"@en ;
  rdfs:comment "The load frequency control block that has this load frequency control area." ;
  cims:AssociationUsed "Yes" ;
  cims:inverseRoleName nc:LoadFrequencyControlBlock.LoadFrequencyControlArea ;
  cims:multiplicity cims:M:0..1 ;
  cims:stereotype "NC" ;
  rdfs:domain nc:LoadFrequencyControlArea ;
  rdfs:range nc:LoadFrequencyControlBlock .

nc:LoadFrequencyControlArea.SchedulingArea a rdf:Property ;
  rdfs:label "SchedulingArea"@en ;
  rdfs:comment "The scheduling area that is part of this load frequency control area." ;
  cims:AssociationUsed "No" ;
  cims:inverseRoleName nc:SchedulingArea.LoadFrequencyControlArea ;
  cims:multiplicity cims:M:0..n ;
  cims:stereotype "NC" ;
  rdfs:domain nc:LoadFrequencyControlArea ;
  rdfs:range nc:SchedulingArea .

nc:LoadFrequencyControlArea.TieCorridor a rdf:Property ;
  rdfs:label "TieCorridor"@en ;
  rdfs:comment "TieCorridor controlled by the LoadFrequencyControlArea." ;
  cims:AssociationUsed "No" ;
  cims:inverseRoleName nc:TieCorridor.LoadFrequencyControlArea ;
  cims:multiplicity cims:M:0..n ;
  cims:stereotype "NC" ;
  rdfs:domain nc:LoadFrequencyControlArea ;
  rdfs:range nc:TieCorridor .

nc:LoadFrequencyControlArea.deficientGenerationLimit a rdf:Property ;
  rdfs:label "deficientGenerationLimit"@en ;
  rdfs:comment "Percentage of average dispatch target plus average regulation used to calculate  Deficient Generation Limit. The value shall be a positive value between 0 and 100." ;
  cims:dataType cim:PerCent ;
  cims:multiplicity cims:M:0..1 ;
  cims:stereotype "NC", <http://iec.ch/TC57/NonStandard/UML#attribute> ;
  rdfs:domain nc:LoadFrequencyControlArea .

nc:LoadFrequencyControlArea.frequencyBiasFactor a rdf:Property ;
  rdfs:label "frequencyBiasFactor"@en ;
  rdfs:comment "Frequency bias in MW/Hz." ;
  cims:dataType cim:Float ;
  cims:multiplicity cims:M:0..1 ;
  cims:stereotype "NC", <http://iec.ch/TC57/NonStandard/UML#attribute> ;
  rdfs:domain nc:LoadFrequencyControlArea .

nc:LoadFrequencyControlArea.frequencyRestorationReserveDelay a rdf:Property ;
  rdfs:label "frequencyRestorationReserveDelay"@en ;
  rdfs:comment "FRR delay expressed in seconds. Must be a positive multiple of AGC's cycle duration." ;
  cims:dataType cim:Seconds ;
  cims:multiplicity cims:M:0..1 ;
  cims:stereotype "NC", <http://iec.ch/TC57/NonStandard/UML#attribute> ;
  rdfs:domain nc:LoadFrequencyControlArea .

nc:LoadFrequencyControlArea.frequencyRestorationReserveMaxRamp a rdf:Property ;
  rdfs:label "frequencyRestorationReserveMaxRamp"@en ;
  rdfs:comment "Maximum authorized ramp for both FRR dispatching and ramp to zero." ;
  cims:dataType cim:ActivePowerChangeRate ;
  cims:multiplicity cims:M:0..1 ;
  cims:stereotype "NC", <http://iec.ch/TC57/NonStandard/UML#attribute> ;
  rdfs:domain nc:LoadFrequencyControlArea .

nc:LoadFrequencyControlArea.frequencyRestorationReserveThreshold a rdf:Property ;
  rdfs:label "frequencyRestorationReserveThreshold"@en ;
  rdfs:comment "Authorized threshold for both FRR dispatching and ramp to zero." ;
  cims:dataType cim:ActivePower ;
  cims:multiplicity cims:M:0..1 ;
  cims:stereotype "NC", <http://iec.ch/TC57/NonStandard/UML#attribute> ;
  rdfs:domain nc:LoadFrequencyControlArea .

nc:LoadFrequencyControlArea.includeFrequencyBias a rdf:Property ;
  rdfs:label "includeFrequencyBias"@en ;
  rdfs:comment "True means the frequency bias that is taken into consideration in the frequency bias computation." ;
  cims:dataType cim:Boolean ;
  cims:multiplicity cims:M:1..1 ;
  cims:stereotype "NC", <http://iec.ch/TC57/NonStandard/UML#attribute> ;
  rdfs:domain nc:LoadFrequencyControlArea .

nc:LoadFrequencyControlBlock.LoadFrequencyControlArea a rdf:Property ;
  rdfs:label "LoadFrequencyControlArea"@en ;
  rdfs:comment "The load frequency control area that is part of this load frequency control block. " ;
  cims:AssociationUsed "No" ;
  cims:inverseRoleName nc:LoadFrequencyControlArea.LoadFrequencyControlBlock ;
  cims:multiplicity cims:M:0..n ;
  cims:stereotype "NC" ;
  rdfs:domain nc:LoadFrequencyControlBlock ;
  rdfs:range nc:LoadFrequencyControlArea .

nc:LoadFrequencyControlBlock.SynchronousArea a rdf:Property ;
  rdfs:label "SynchronousArea"@en ;
  rdfs:comment "The synchronous area that has this load frequency control block." ;
  cims:AssociationUsed "Yes" ;
  cims:inverseRoleName nc:SynchronousArea.LoadFrequencyControlBlock ;
  cims:multiplicity cims:M:0..1 ;
  cims:stereotype "NC" ;
  rdfs:domain nc:LoadFrequencyControlBlock ;
  rdfs:range nc:SynchronousArea .

nc:LoadFrequencyControlOperator.FrequencyControlArea a rdf:Property ;
  rdfs:label "FrequencyControlArea"@en ;
  rdfs:comment "The frequency control area that has this frequency control operator." ;
  cims:AssociationUsed "No" ;
  cims:inverseRoleName nc:LoadFrequencyControlArea.FrequencyControlOperator ;
  cims:multiplicity cims:M:0..n ;
  cims:stereotype "NC" ;
  rdfs:domain nc:LoadFrequencyControlOperator ;
  rdfs:range nc:LoadFrequencyControlArea .

nc:LossCurve.FACTSEquipment a rdf:Property ;
  rdfs:label "FACTSEquipment"@en ;
  rdfs:comment "The FACTS equipment which has a loss curve." ;
  cims:AssociationUsed "Yes" ;
  cims:inverseRoleName nc:FACTSEquipment.LossCurve ;
  cims:multiplicity cims:M:0..1 ;
  cims:stereotype "NC" ;
  rdfs:domain nc:LossCurve ;
  rdfs:range nc:FACTSEquipment .

nc:MonitoringArea.PowerFrequencyController a rdf:Property ;
  rdfs:label "PowerFrequencyController"@en ;
  rdfs:comment "Power frequency controller that applied to this monitoring area." ;
  cims:AssociationUsed "No" ;
  cims:inverseRoleName nc:PowerFrequencyController.MonitoringArea ;
  cims:multiplicity cims:M:0..1 ;
  cims:stereotype "NC" ;
  rdfs:domain nc:MonitoringArea ;
  rdfs:range nc:PowerFrequencyController .

nc:MonopolarDCSystem.DCPole a rdf:Property ;
  rdfs:label "DCPole"@en ;
  rdfs:comment "DC pole part of the asymmetric DC system." ;
  cims:AssociationUsed "No" ;
  cims:inverseRoleName nc:DCPole.AsymmetricMonopolarDCSystem ;
  cims:multiplicity cims:M:0..1 ;
  cims:stereotype "NC" ;
  rdfs:domain nc:MonopolarDCSystem ;
  rdfs:range nc:DCPole .

nc:MonopolarDCSystem.isSymmetrical a rdf:Property ;
  rdfs:label "isSymmetrical"@en ;
  rdfs:comment "if true, the monopolar DC system is symmetrical monopolar DC system (IEC 60633). It is a DC system with only one symmetrical monopole. A symmetrical monopole is part of an DC system consisting of all the equipment in the DC substations and the interconnecting transmission lines, if any, which during normal operation exhibits equal and opposite direct voltage polarities with respect to earth but without series connection of converters in each converter station. The term \"symmetrical monopole\" is used even though there are two polarities with DC voltages, because with only one converter it is not possible to provide the redundancy which is normally associated with the term \"bipole\"." ;
  cims:dataType cim:Boolean ;
  cims:multiplicity cims:M:1..1 ;
  cims:stereotype "NC", <http://iec.ch/TC57/NonStandard/UML#attribute> ;
  rdfs:domain nc:MonopolarDCSystem .

nc:NuclearGeneratingUnit.reactorKind a rdf:Property ;
  rdfs:label "reactorKind"@en ;
  rdfs:comment "Kind of nuclear reactor." ;
  cims:multiplicity cims:M:1..1 ;
  cims:stereotype "NC", <http://iec.ch/TC57/NonStandard/UML#attribute> ;
  rdfs:domain cim:NuclearGeneratingUnit ;
  rdfs:range nc:NuclearReactorKind .

nc:OperationalLimitSet.PowerTransferCorridor a rdf:Property ;
  rdfs:label "PowerTransferCorridor"@en ;
  rdfs:comment "The power transfer corridor that has this operational limit set." ;
  cims:AssociationUsed "Yes" ;
  cims:inverseRoleName nc:PowerTransferCorridor.OperationalLimitSet ;
  cims:multiplicity cims:M:0..1 ;
  cims:stereotype "NC" ;
  rdfs:domain cim:OperationalLimitSet ;
  rdfs:range nc:PowerTransferCorridor .

nc:OperationalLimitType.PermanentAmbientTemperatureDependencyCurve a rdf:Property ;
  rdfs:label "PermanentAmbientTemperatureDependencyCurve"@en ;
  rdfs:comment "The permanent ambient temperature dependency curve for this operational limit type." ;
  cims:AssociationUsed "Yes" ;
  cims:inverseRoleName nc:AmbientTemperatureDependencyCurve.OperationalLimitType ;
  cims:multiplicity cims:M:0..1 ;
  cims:stereotype "NC" ;
  rdfs:domain cim:OperationalLimitType ;
  rdfs:range nc:AmbientTemperatureDependencyCurve .

nc:OperationalLimitType.PermanentSolarRadiationCurve a rdf:Property ;
  rdfs:label "PermanentSolarRadiationCurve"@en ;
  rdfs:comment "The permanent solar radiation curve for this operational limit type." ;
  cims:AssociationUsed "Yes" ;
  cims:inverseRoleName nc:SolarRadiationDependencyCurve.OperationalLimitType ;
  cims:multiplicity cims:M:0..1 ;
  cims:stereotype "NC" ;
  rdfs:domain cim:OperationalLimitType ;
  rdfs:range nc:SolarRadiationDependencyCurve .

nc:OperationalLimitType.RecoveryOverloadLimitCurve a rdf:Property ;
  rdfs:label "RecoveryOverloadLimitCurve"@en ;
  rdfs:comment "This is the curve which provides the recovery time information for this limit type." ;
  cims:AssociationUsed "Yes" ;
  cims:inverseRoleName nc:RecoveryOverloadLimitCurve.OperationalLimitType ;
  cims:multiplicity cims:M:0..1 ;
  cims:stereotype "NC" ;
  rdfs:domain cim:OperationalLimitType ;
  rdfs:range nc:RecoveryOverloadLimitCurve .

nc:OperationalLimitType.TemporaryBaseOverloadLimitCurve a rdf:Property ;
  rdfs:label "TemporaryBaseOverloadLimitCurve"@en ;
  rdfs:comment "The temporary base overload limit curve for this operational limit type." ;
  cims:AssociationUsed "Yes" ;
  cims:inverseRoleName nc:BaseOverloadLimitCurve.OperationalLimitType ;
  cims:multiplicity cims:M:0..1 ;
  cims:stereotype "NC" ;
  rdfs:domain cim:OperationalLimitType ;
  rdfs:range nc:BaseOverloadLimitCurve .

nc:OperationalLimitType.TemporaryDurationOverloadLimitCurve a rdf:Property ;
  rdfs:label "TemporaryDurationOverloadLimitCurve"@en ;
  rdfs:comment "The temporary duration overload limit curve for this operational limit type." ;
  cims:AssociationUsed "Yes" ;
  cims:inverseRoleName nc:DurationOverloadLimitCurve.OperationalLimitType ;
  cims:multiplicity cims:M:0..1 ;
  cims:stereotype "NC" ;
  rdfs:domain cim:OperationalLimitType ;
  rdfs:range nc:DurationOverloadLimitCurve .

nc:OperationalLimitType.isMinimum a rdf:Property ;
  rdfs:label "isMinimum"@en ;
  rdfs:comment "Defines if the operational limit type is minimum. If true, the value is a minimum value of the same kind. This applies to stability and PATL. If false, the limit has the normal behaviour. OperationalLimitType.direction attribute shall be absoluteValue." ;
  cims:dataType cim:Boolean ;
  cims:multiplicity cims:M:0..1 ;
  cims:stereotype "NC", <http://iec.ch/TC57/NonStandard/UML#attribute> ;
  rdfs:domain cim:OperationalLimitType .

nc:OrganisationRole.globalLocationNumber a rdf:Property ;
  rdfs:label "globalLocationNumber"@en ;
  rdfs:comment """The Global Location Number (GLN) is part of the GS1 systems of standards. GLN is a 13-digit number structured that include GS1 Company Prefix, Location Reference (N1-N12) and Check Digit (N13).
GS1 is a neutral, not-for-profit, international organisation that develops and maintains standards for supply and demand chains across multiple sectors.""" ;
  cims:dataType cim:String ;
  cims:multiplicity cims:M:0..1 ;
  cims:stereotype "NC", <http://iec.ch/TC57/NonStandard/UML#attribute> ;
  rdfs:domain cim:OrganisationRole .

nc:OutageCoordinationRegion.ControlArea a rdf:Property ;
  rdfs:label "ControlArea"@en ;
  rdfs:comment "The control area that is part of this outage coordination region." ;
  cims:AssociationUsed "No" ;
  cims:inverseRoleName nc:ControlArea.OutageCoordinationRegion ;
  cims:multiplicity cims:M:0..n ;
  cims:stereotype "NC" ;
  rdfs:domain nc:OutageCoordinationRegion ;
  rdfs:range cim:ControlArea .

nc:OutageCoordinationRegion.OutageCoordinator a rdf:Property ;
  rdfs:label "OutageCoordinator"@en ;
  rdfs:comment "The outage coordinator responsible for this outage coordination region." ;
  cims:AssociationUsed "Yes" ;
  cims:inverseRoleName nc:OutageCoordinator.OutageCoordinationRegion ;
  cims:multiplicity cims:M:0..1 ;
  cims:stereotype "NC" ;
  rdfs:domain nc:OutageCoordinationRegion ;
  rdfs:range nc:OutageCoordinator .

nc:OutageCoordinationRegion.SecurityCoordinator a rdf:Property ;
  rdfs:label "SecurityCoordinator"@en ;
  rdfs:comment "The security coordinator that is responsible for this outage coordination region." ;
  cims:AssociationUsed "Yes" ;
  cims:inverseRoleName nc:SecurityCoordinator.OutageCoordinationRegion ;
  cims:multiplicity cims:M:0..1 ;
  cims:stereotype "NC" ;
  rdfs:domain nc:OutageCoordinationRegion ;
  rdfs:range nc:SecurityCoordinator .

nc:OutageCoordinator.OutageCoordinationRegion a rdf:Property ;
  rdfs:label "OutageCoordinationRegion"@en ;
  rdfs:comment "The outage coordination region that has this outage coordinator." ;
  cims:AssociationUsed "No" ;
  cims:inverseRoleName nc:OutageCoordinationRegion.OutageCoordinator ;
  cims:multiplicity cims:M:0..n ;
  cims:stereotype "NC" ;
  rdfs:domain nc:OutageCoordinator ;
  rdfs:range nc:OutageCoordinationRegion .

nc:OverlappingZone.ImpactedRegion a rdf:Property ;
  rdfs:label "ImpactedRegion"@en ;
  rdfs:comment "The region that is impacted by this overlapping zone." ;
  cims:AssociationUsed "No" ;
  cims:inverseRoleName nc:Region.OverlappingZone ;
  cims:multiplicity cims:M:0..n ;
  cims:stereotype "NC" ;
  rdfs:domain nc:OverlappingZone ;
  rdfs:range nc:Region .

nc:PTCTriggeredEquipment.Equipment a rdf:Property ;
  rdfs:label "Equipment"@en ;
  rdfs:comment "The equipment which is part of power transfer corridor triggering." ;
  cims:AssociationUsed "Yes" ;
  cims:inverseRoleName nc:Equipment.PTCTriggeredEquipment ;
  cims:multiplicity cims:M:1 ;
  cims:stereotype "NC" ;
  rdfs:domain nc:PTCTriggeredEquipment ;
  rdfs:range cim:Equipment .

nc:PTCTriggeredEquipment.ExceptionalPowerTransferCorridor a rdf:Property ;
  rdfs:label "ExceptionalPowerTransferCorridor"@en ;
  rdfs:comment "The power transfer corridor which is triggered by this equipment." ;
  cims:AssociationUsed "Yes" ;
  cims:inverseRoleName nc:ExceptionalPowerTransferCorridor.PTCTriggeredEquipment ;
  cims:multiplicity cims:M:1 ;
  cims:stereotype "NC" ;
  rdfs:domain nc:PTCTriggeredEquipment ;
  rdfs:range nc:ExceptionalPowerTransferCorridor .

nc:PinTerminal.Terminal a rdf:Property ;
  rdfs:label "Terminal"@en ;
  rdfs:comment "The Terminal that is used in the input pin." ;
  cims:AssociationUsed "Yes" ;
  cims:inverseRoleName nc:Terminal.PinTerminal ;
  cims:multiplicity cims:M:1 ;
  cims:stereotype "NC" ;
  rdfs:domain nc:PinTerminal ;
  rdfs:range cim:Terminal .

nc:PinTerminal.kind a rdf:Property ;
  rdfs:label "kind"@en ;
  rdfs:comment "The kind of quantity which is used as an input value." ;
  cims:multiplicity cims:M:1..1 ;
  cims:stereotype "NC", <http://iec.ch/TC57/NonStandard/UML#attribute> ;
  rdfs:domain nc:PinTerminal ;
  rdfs:range nc:PinTerminalKind .

nc:PowerCapacity.BiddingZone a rdf:Property ;
  rdfs:label "BiddingZone"@en ;
  rdfs:comment "Bidding zone which has a power capacity." ;
  cims:AssociationUsed "No" ;
  cims:inverseRoleName nc:BiddingZone.PowerCapacity ;
  cims:multiplicity cims:M:0..n ;
  cims:stereotype "NC" ;
  rdfs:domain nc:PowerCapacity ;
  rdfs:range nc:BiddingZone .

nc:PowerElectricalChemicalUnit.kind a rdf:Property ;
  rdfs:label "kind"@en ;
  rdfs:comment "Kind of power electrical chemical unit." ;
  cims:multiplicity cims:M:1..1 ;
  cims:stereotype "NC", <http://iec.ch/TC57/NonStandard/UML#attribute> ;
  rdfs:domain nc:PowerElectricalChemicalUnit ;
  rdfs:range nc:PowerElectricalChemicalUnitKind .

nc:PowerElectronicsConnectionController.PowerElectronicsUnitController a rdf:Property ;
  rdfs:label "PowerElectronicsUnitController"@en ;
  rdfs:comment "Power electronics unit controller that has this power electronics connection controller." ;
  cims:AssociationUsed "No" ;
  cims:inverseRoleName nc:PowerElectronicsUnitController.PowerElectronicsConnectionController ;
  cims:multiplicity cims:M:0..n ;
  cims:stereotype "NC" ;
  rdfs:domain nc:PowerElectronicsConnectionController ;
  rdfs:range nc:PowerElectronicsUnitController .

nc:PowerElectronicsMarineUnit.kind a rdf:Property ;
  rdfs:label "kind"@en ;
  rdfs:comment "Kind of marine unit." ;
  cims:multiplicity cims:M:1..1 ;
  cims:stereotype "NC", <http://iec.ch/TC57/NonStandard/UML#attribute> ;
  rdfs:domain nc:PowerElectronicsMarineUnit ;
  rdfs:range nc:MarineUnitKind .

nc:PowerElectronicsUnit.AreaDispatchableUnit a rdf:Property ;
  rdfs:label "AreaDispatchableUnit"@en ;
  rdfs:comment "The area dispatchable unit for this power electronics unit." ;
  cims:AssociationUsed "No" ;
  cims:inverseRoleName nc:AreaDispatchableUnit.PowerElectronicsUnit ;
  cims:multiplicity cims:M:0..1 ;
  cims:stereotype "NC", <http://iec.ch/TC57/NonStandard/UML#ofAggregate> ;
  rdfs:domain cim:PowerElectronicsUnit ;
  rdfs:range nc:AreaDispatchableUnit .

nc:PowerElectronicsUnit.EnergyComponent a rdf:Property ;
  rdfs:label "EnergyComponent"@en ;
  rdfs:comment "The energy component that has this power electronics unit." ;
  cims:AssociationUsed "No" ;
  cims:inverseRoleName nc:EnergyComponent.PowerElectronicsUnit ;
  cims:multiplicity cims:M:0..n ;
  cims:stereotype "NC" ;
  rdfs:domain cim:PowerElectronicsUnit ;
  rdfs:range nc:EnergyComponent .

nc:PowerElectronicsUnit.PowerElectronicsUnitController a rdf:Property ;
  rdfs:label "PowerElectronicsUnitController"@en ;
  rdfs:comment "Power electronics unit controller for this power electronics unit." ;
  cims:AssociationUsed "Yes" ;
  cims:inverseRoleName nc:PowerElectronicsUnitController.PowerElectronicsUnit ;
  cims:multiplicity cims:M:0..1 ;
  cims:stereotype "NC" ;
  rdfs:domain cim:PowerElectronicsUnit ;
  rdfs:range nc:PowerElectronicsUnitController .

nc:PowerElectronicsUnit.ScheduleResource a rdf:Property ;
  rdfs:label "ScheduleResource"@en ;
  rdfs:comment "The schedule resource that has this power electronics unit." ;
  cims:AssociationUsed "Yes" ;
  cims:inverseRoleName nc:ScheduleResource.PowerElectronicsUnit ;
  cims:multiplicity cims:M:0..1 ;
  cims:stereotype "NC" ;
  rdfs:domain cim:PowerElectronicsUnit ;
  rdfs:range nc:ScheduleResource .

nc:PowerElectronicsUnit.maxEconomicP a rdf:Property ;
  rdfs:label "maxEconomicP"@en ;
  rdfs:comment "Maximum high economic active power limit, that should not exceed the maximum operating active power limit." ;
  cims:dataType cim:ActivePower ;
  cims:multiplicity cims:M:0..1 ;
  cims:stereotype "NC", <http://iec.ch/TC57/NonStandard/UML#attribute> ;
  rdfs:domain cim:PowerElectronicsUnit .

nc:PowerElectronicsUnit.minEconomicP a rdf:Property ;
  rdfs:label "minEconomicP"@en ;
  rdfs:comment "Low economic active power limit that shall be greater than or equal to the minimum operating active power limit." ;
  cims:dataType cim:ActivePower ;
  cims:multiplicity cims:M:0..1 ;
  cims:stereotype "NC", <http://iec.ch/TC57/NonStandard/UML#attribute> ;
  rdfs:domain cim:PowerElectronicsUnit .

nc:PowerElectronicsUnit.normalParticipationFactor a rdf:Property ;
  rdfs:label "normalParticipationFactor"@en ;
  rdfs:comment """Participation factor describing the entity part of the active power provided by a collection of entities (e.g. an active power forecast to a collection of entities is divided to each of the member entity according to the participation factor). Must be a positive value.
In the case of a sharing strategy, the distribution is following entities value (V) equals aggregated value (T) divided by sum of participation factors (PF), i.e. V=T/sum(PF). 
In the case of priority strategy, the item with the lowest number gets allocated energy first.""" ;
  cims:dataType cim:Float ;
  cims:multiplicity cims:M:0..1 ;
  cims:stereotype "NC", <http://iec.ch/TC57/NonStandard/UML#attribute> ;
  rdfs:domain cim:PowerElectronicsUnit .

nc:PowerElectronicsUnitController.PowerElectronicsConnectionController a rdf:Property ;
  rdfs:label "PowerElectronicsConnectionController"@en ;
  rdfs:comment "Power electronics connection controller for the power electronics unit controller." ;
  cims:AssociationUsed "Yes" ;
  cims:inverseRoleName nc:PowerElectronicsConnectionController.PowerElectronicsUnitController ;
  cims:multiplicity cims:M:0..1 ;
  cims:stereotype "NC" ;
  rdfs:domain nc:PowerElectronicsUnitController ;
  rdfs:range nc:PowerElectronicsConnectionController .

nc:PowerElectronicsUnitController.PowerElectronicsUnit a rdf:Property ;
  rdfs:label "PowerElectronicsUnit"@en ;
  rdfs:comment "Power electronics unit that has this power electronics unit controller." ;
  cims:AssociationUsed "No" ;
  cims:inverseRoleName nc:PowerElectronicsUnit.PowerElectronicsUnitController ;
  cims:multiplicity cims:M:0..n ;
  cims:stereotype "NC" ;
  rdfs:domain nc:PowerElectronicsUnitController ;
  rdfs:range cim:PowerElectronicsUnit .

nc:PowerFrequencyController.ControlArea a rdf:Property ;
  rdfs:label "ControlArea"@en ;
  rdfs:comment "Control area which has a power frequency controller." ;
  cims:AssociationUsed "Yes" ;
  cims:inverseRoleName nc:ControlArea.PowerFrequencyController ;
  cims:multiplicity cims:M:0..1 ;
  cims:stereotype "NC" ;
  rdfs:domain nc:PowerFrequencyController ;
  rdfs:range cim:ControlArea .

nc:PowerFrequencyController.FrequencyMonitoringTerminal a rdf:Property ;
  rdfs:label "FrequencyMonitoringTerminal"@en ;
  rdfs:comment "Frequency monitoring terminal for this power frequency controller." ;
  cims:AssociationUsed "No" ;
  cims:inverseRoleName nc:FrequencyMonitoringTerminal.PowerFrequencyController ;
  cims:multiplicity cims:M:0..n ;
  cims:stereotype "NC" ;
  rdfs:domain nc:PowerFrequencyController ;
  rdfs:range nc:FrequencyMonitoringTerminal .

nc:PowerFrequencyController.MonitoringArea a rdf:Property ;
  rdfs:label "MonitoringArea"@en ;
  rdfs:comment "Monitoring area that has this power frequency controller." ;
  cims:AssociationUsed "Yes" ;
  cims:inverseRoleName nc:MonitoringArea.PowerFrequencyController ;
  cims:multiplicity cims:M:0..1 ;
  cims:stereotype "NC" ;
  rdfs:domain nc:PowerFrequencyController ;
  rdfs:range nc:MonitoringArea .

nc:PowerFrequencyController.PowerShiftKeyStrategy a rdf:Property ;
  rdfs:label "PowerShiftKeyStrategy"@en ;
  rdfs:comment "Power shift key strategy for this power frequency controller." ;
  cims:AssociationUsed "Yes" ;
  cims:inverseRoleName nc:PowerShiftKeyStrategy.PowerFrequencyController ;
  cims:multiplicity cims:M:0..1 ;
  cims:stereotype "NC" ;
  rdfs:domain nc:PowerFrequencyController ;
  rdfs:range nc:PowerShiftKeyStrategy .

nc:PowerFrequencyController.mode a rdf:Property ;
  rdfs:label "mode"@en ;
  rdfs:comment "Mode of the power frequency controller." ;
  cims:multiplicity cims:M:1..1 ;
  cims:stereotype "NC", <http://iec.ch/TC57/NonStandard/UML#attribute> ;
  rdfs:domain nc:PowerFrequencyController ;
  rdfs:range nc:PowerFrequencyControlKind .

nc:PowerShiftKeyStrategy.PowerFrequencyController a rdf:Property ;
  rdfs:label "PowerFrequencyController"@en ;
  rdfs:comment "Power frequency controller that has power shift key strategy." ;
  cims:AssociationUsed "No" ;
  cims:inverseRoleName nc:PowerFrequencyController.PowerShiftKeyStrategy ;
  cims:multiplicity cims:M:0..n ;
  cims:stereotype "NC" ;
  rdfs:domain nc:PowerShiftKeyStrategy ;
  rdfs:range nc:PowerFrequencyController .

nc:PowerShiftKeyStrategy.SchedulingArea a rdf:Property ;
  rdfs:label "SchedulingArea"@en ;
  rdfs:comment "Scheduling area associated with power shift key strategy." ;
  cims:AssociationUsed "Yes" ;
  cims:inverseRoleName nc:SchedulingArea.PowerShiftKeyStrategy ;
  cims:multiplicity cims:M:0..1 ;
  cims:stereotype "NC" ;
  rdfs:domain nc:PowerShiftKeyStrategy ;
  rdfs:range nc:SchedulingArea .

nc:PowerShiftKeyStrategy.dispatchableUnitOnly a rdf:Property ;
  rdfs:label "dispatchableUnitOnly"@en ;
  rdfs:comment """If true, only dispatchable units are included in the power shift key strategy. A unit is considered dispatchable if it is associated with an area dispatchable unit that is linked to the same scheduling area as the power shift key strategy.
Exceptions are done for units that are included in explicit or distributed strategies.""" ;
  cims:dataType cim:Boolean ;
  cims:multiplicity cims:M:0..1 ;
  cims:stereotype "NC", <http://iec.ch/TC57/NonStandard/UML#attribute> ;
  rdfs:domain nc:PowerShiftKeyStrategy .

nc:PowerShiftKeyStrategy.method a rdf:Property ;
  rdfs:label "method"@en ;
  rdfs:comment "Shift method used for the power shift strategy." ;
  cims:multiplicity cims:M:0..1 ;
  cims:stereotype "NC", <http://iec.ch/TC57/NonStandard/UML#attribute> ;
  rdfs:domain nc:PowerShiftKeyStrategy ;
  rdfs:range nc:ShiftMethodKind .

nc:PowerShiftKeyStrategy.normalEnabled a rdf:Property ;
  rdfs:label "normalEnabled"@en ;
  rdfs:comment "If true, the assessed element shall be considered under normal operating conditions." ;
  cims:dataType cim:Boolean ;
  cims:multiplicity cims:M:0..1 ;
  cims:stereotype "NC", <http://iec.ch/TC57/NonStandard/UML#attribute> ;
  rdfs:domain nc:PowerShiftKeyStrategy .

nc:PowerShiftKeyStrategy.normalParticipationFactor a rdf:Property ;
  rdfs:label "normalParticipationFactor"@en ;
  rdfs:comment "Normal participation factor describing the entities part of the power shift strategy. Must be a positive value." ;
  cims:dataType cim:Float ;
  cims:multiplicity cims:M:0..1 ;
  cims:stereotype "NC", <http://iec.ch/TC57/NonStandard/UML#attribute> ;
  rdfs:domain nc:PowerShiftKeyStrategy .

nc:PowerShiftKeyStrategy.powerBlockKind a rdf:Property ;
  rdfs:label "powerBlockKind"@en ;
  rdfs:comment "Power block kind creates block (one or more) of power shift key strategy to address increase and/or decrease of power for a given scheduling area." ;
  cims:multiplicity cims:M:0..1 ;
  cims:stereotype "NC", <http://iec.ch/TC57/NonStandard/UML#attribute> ;
  rdfs:domain nc:PowerShiftKeyStrategy ;
  rdfs:range nc:PowerBlockKind .

nc:PowerShiftKeyStrategy.powerShiftKey a rdf:Property ;
  rdfs:label "powerShiftKey"@en ;
  rdfs:comment "Power shift keys strategy gives instruction on how the value (Active power) is going to be distributed inside the relevant bidding zone." ;
  cims:multiplicity cims:M:0..1 ;
  cims:stereotype "NC", <http://iec.ch/TC57/NonStandard/UML#attribute> ;
  rdfs:domain nc:PowerShiftKeyStrategy ;
  rdfs:range nc:PowerShiftKeyKind .

nc:PowerTransferCorridor.CircuitShare a rdf:Property ;
  rdfs:label "CircuitShare"@en ;
  rdfs:comment "The circuit share for this power transfer corridor." ;
  cims:AssociationUsed "No" ;
  cims:inverseRoleName nc:CircuitShare.PowerTransferCorridor ;
  cims:multiplicity cims:M:0..n ;
  cims:stereotype "NC" ;
  rdfs:domain nc:PowerTransferCorridor ;
  rdfs:range nc:CircuitShare .

nc:PowerTransferCorridor.OperationalLimitSet a rdf:Property ;
  rdfs:label "OperationalLimitSet"@en ;
  rdfs:comment "The operational limit set relevant for this power transfer corridor." ;
  cims:AssociationUsed "No" ;
  cims:inverseRoleName nc:OperationalLimitSet.PowerTransferCorridor ;
  cims:multiplicity cims:M:0..n ;
  cims:stereotype "NC" ;
  rdfs:domain nc:PowerTransferCorridor ;
  rdfs:range cim:OperationalLimitSet .

nc:PowerTransferCorridor.normalEnabled a rdf:Property ;
  rdfs:label "normalEnabled"@en ;
  rdfs:comment "It is the normal enable/disable the monitoring/assessment of a power transfer corridor. True means that the monitoring of the power transfer corridor is assessed. False means the power transfer corridor is not assessed. " ;
  cims:dataType cim:Boolean ;
  cims:multiplicity cims:M:0..1 ;
  cims:stereotype "NC", <http://iec.ch/TC57/NonStandard/UML#attribute> ;
  rdfs:domain nc:PowerTransferCorridor .

nc:PropertyReference.FunctionOutputVariable a rdf:Property ;
  rdfs:label "FunctionOutputVariable"@en ;
  rdfs:comment "Function output variable is the function output this property reference is used in." ;
  cims:AssociationUsed "No" ;
  cims:inverseRoleName nc:FunctionOutputVariable.PropertyReference ;
  cims:multiplicity cims:M:0..n ;
  cims:stereotype "NC" ;
  rdfs:domain nc:PropertyReference ;
  rdfs:range nc:FunctionOutputVariable .

nc:ProportionalEnergyComponent.normalParticipationFactor a rdf:Property ;
  rdfs:label "normalParticipationFactor"@en ;
  rdfs:comment "Normal participation factor." ;
  cims:dataType cim:Float ;
  cims:multiplicity cims:M:0..1 ;
  cims:stereotype "NC", <http://iec.ch/TC57/NonStandard/UML#attribute> ;
  rdfs:domain nc:ProportionalEnergyComponent .

nc:ProportionalEnergyComponent.powerDuration a rdf:Property ;
  rdfs:label "powerDuration"@en ;
  rdfs:comment "Duration for the active power." ;
  cims:dataType cim:Duration ;
  cims:multiplicity cims:M:0..1 ;
  cims:stereotype "NC", <http://iec.ch/TC57/NonStandard/UML#attribute> ;
  rdfs:domain nc:ProportionalEnergyComponent .

nc:ReactiveCapabilityCurve.referenceVoltage a rdf:Property ;
  rdfs:label "referenceVoltage"@en ;
  rdfs:comment "The reference voltage for which the capability curve is valid." ;
  cims:dataType cim:Voltage ;
  cims:multiplicity cims:M:1..1 ;
  cims:stereotype "NC", <http://iec.ch/TC57/NonStandard/UML#attribute> ;
  rdfs:domain cim:ReactiveCapabilityCurve .

nc:RecoveryOverloadLimitCurve.OperationalLimitType a rdf:Property ;
  rdfs:label "OperationalLimitType"@en ;
  rdfs:comment "The operational limit type which has recovery time characteristic." ;
  cims:AssociationUsed "No" ;
  cims:inverseRoleName nc:OperationalLimitType.RecoveryOverloadLimitCurve ;
  cims:multiplicity cims:M:0..n ;
  cims:stereotype "NC" ;
  rdfs:domain nc:RecoveryOverloadLimitCurve ;
  rdfs:range cim:OperationalLimitType .

nc:Region.OverlappingZone a rdf:Property ;
  rdfs:label "OverlappingZone"@en ;
  rdfs:comment "The overlapping zone which is impacted by this  region." ;
  cims:AssociationUsed "Yes" ;
  cims:inverseRoleName nc:OverlappingZone.ImpactedRegion ;
  cims:multiplicity cims:M:0..1 ;
  cims:stereotype "NC" ;
  rdfs:domain nc:Region ;
  rdfs:range nc:OverlappingZone .

nc:RegulatingCondEq.EquipmentController a rdf:Property ;
  rdfs:label "EquipmentController"@en ;
  rdfs:comment "The equipment controller for this regulating conducting equipment." ;
  cims:AssociationUsed "Yes" ;
  cims:inverseRoleName nc:EquipmentController.RegulatingCondEq ;
  cims:multiplicity cims:M:0..1 ;
  cims:stereotype "NC" ;
  rdfs:domain cim:RegulatingCondEq ;
  rdfs:range nc:EquipmentController .

nc:SSSCController.CurrentDroopOverride a rdf:Property ;
  rdfs:label "CurrentDroopOverride"@en ;
  rdfs:comment "The current droop override for this SSSC controller. It is not used when the SSSC controller is in mode currentDroop." ;
  cims:AssociationUsed "No" ;
  cims:inverseRoleName nc:CurrentDroopOverride.SSSCController ;
  cims:multiplicity cims:M:0..1 ;
  cims:stereotype "NC" ;
  rdfs:domain nc:SSSCController ;
  rdfs:range nc:CurrentDroopOverride .

nc:SSSCController.SSSCSimulationSettings a rdf:Property ;
  rdfs:label "SSSCSimulationSettings"@en ;
  rdfs:comment "The simulation setings that apply for this controller." ;
  cims:AssociationUsed "Yes" ;
  cims:inverseRoleName nc:SSSCSimulationSettings.SSSCController ;
  cims:multiplicity cims:M:0..1 ;
  cims:stereotype "NC" ;
  rdfs:domain nc:SSSCController ;
  rdfs:range nc:SSSCSimulationSettings .

nc:SSSCController.maxInjectionU a rdf:Property ;
  rdfs:label "maxInjectionU"@en ;
  rdfs:comment "Maximum voltage that the device can inject." ;
  cims:dataType cim:Voltage ;
  cims:multiplicity cims:M:1..1 ;
  cims:stereotype "NC", <http://iec.ch/TC57/NonStandard/UML#attribute> ;
  rdfs:domain nc:SSSCController .

nc:SSSCController.maxLimitI a rdf:Property ;
  rdfs:label "maxLimitI"@en ;
  rdfs:comment "Maximum operating current limit applied for the controller and used by any of the available control functions." ;
  cims:dataType cim:CurrentFlow ;
  cims:multiplicity cims:M:0..1 ;
  cims:stereotype "NC", <http://iec.ch/TC57/NonStandard/UML#attribute> ;
  rdfs:domain nc:SSSCController .

nc:SSSCController.minInjectionU a rdf:Property ;
  rdfs:label "minInjectionU"@en ;
  rdfs:comment "Minimum voltage that the device can inject." ;
  cims:dataType cim:Voltage ;
  cims:multiplicity cims:M:1..1 ;
  cims:stereotype "NC", <http://iec.ch/TC57/NonStandard/UML#attribute> ;
  rdfs:domain nc:SSSCController .

nc:SSSCController.minLimitI a rdf:Property ;
  rdfs:label "minLimitI"@en ;
  rdfs:comment "Minimum operating current limit applied for the controller and used by any of the available control functions." ;
  cims:dataType cim:CurrentFlow ;
  cims:multiplicity cims:M:0..1 ;
  cims:stereotype "NC", <http://iec.ch/TC57/NonStandard/UML#attribute> ;
  rdfs:domain nc:SSSCController .

nc:SSSCSimulationSettings.SSSCController a rdf:Property ;
  rdfs:label "SSSCController"@en ;
  rdfs:comment "The controller that uses these simulation settings." ;
  cims:AssociationUsed "No" ;
  cims:inverseRoleName nc:SSSCController.SSSCSimulationSettings ;
  cims:multiplicity cims:M:0..n ;
  cims:stereotype "NC" ;
  rdfs:domain nc:SSSCSimulationSettings ;
  rdfs:range nc:SSSCController .

nc:SSSCSimulationSettings.deltaX a rdf:Property ;
  rdfs:label "deltaX"@en ;
  rdfs:comment "Reactance delta for the solution algorithm. The solution “outer-loop” algorithm is based on a secant method which needs two initial points. The second point is calculated from the first one by either adding or subtracting this “delta”. The “seed” is assumed to be 0 ohms." ;
  cims:dataType cim:Reactance ;
  cims:multiplicity cims:M:1..1 ;
  cims:stereotype "NC", <http://iec.ch/TC57/NonStandard/UML#attribute> ;
  rdfs:domain nc:SSSCSimulationSettings .

nc:SSSCSimulationSettings.isEstimateDLDVSensitive a rdf:Property ;
  rdfs:label "isEstimateDLDVSensitive"@en ;
  rdfs:comment "Defines if the estimate is considering the dI/dV sensitivity (true) instead of the secant algorithm (false). " ;
  cims:dataType cim:Boolean ;
  cims:multiplicity cims:M:1..1 ;
  cims:stereotype "NC", <http://iec.ch/TC57/NonStandard/UML#attribute> ;
  rdfs:domain nc:SSSCSimulationSettings .

nc:SSSCSimulationSettings.mRID a rdf:Property ;
  rdfs:label "mRID"@en ;
  rdfs:comment """Master resource identifier issued by a model authority. The mRID is unique within an exchange context. Global uniqueness is easily achieved by using a UUID, as specified in RFC 4122, for the mRID. The use of UUID is strongly recommended.
For CIMXML data files in RDF syntax conforming to IEC 61970-552, the mRID is mapped to rdf:ID or rdf:about attributes that identify CIM object elements.""" ;
  cims:dataType cim:String ;
  cims:multiplicity cims:M:1..1 ;
  cims:stereotype "NC", <http://iec.ch/TC57/NonStandard/UML#attribute> ;
  rdfs:domain nc:SSSCSimulationSettings .

nc:SSSCSimulationSettings.maxCorrectionX a rdf:Property ;
  rdfs:label "maxCorrectionX"@en ;
  rdfs:comment "Maximum value of the reactance correction applied between Iterations of the power flow calculation algorithm for the purpose of achieving control target value." ;
  cims:dataType cim:Reactance ;
  cims:multiplicity cims:M:1..1 ;
  cims:stereotype "NC", <http://iec.ch/TC57/NonStandard/UML#attribute> ;
  rdfs:domain nc:SSSCSimulationSettings .

nc:SSSCSimulationSettings.maxIterations a rdf:Property ;
  rdfs:label "maxIterations"@en ;
  rdfs:comment "Maximum number of iterations before claiming an open line condition. The algorithm uses it to assess if a line is really open by making sure low-currents are observed on various consecutive iterations. " ;
  cims:dataType cim:Integer ;
  cims:multiplicity cims:M:1..1 ;
  cims:stereotype "NC", <http://iec.ch/TC57/NonStandard/UML#attribute> ;
  rdfs:domain nc:SSSCSimulationSettings .

nc:SSSCSimulationSettings.maxMismatch a rdf:Property ;
  rdfs:label "maxMismatch"@en ;
  rdfs:comment "Maximum mismatch tolerance of voltage target value. If mismatch is lower, convergence is claimed. It is only used for voltageInjection and currentDroop control modes. " ;
  cims:dataType cim:Voltage ;
  cims:multiplicity cims:M:1..1 ;
  cims:stereotype "NC", <http://iec.ch/TC57/NonStandard/UML#attribute> ;
  rdfs:domain nc:SSSCSimulationSettings .

nc:ScheduleResource.AreaDispatchableUnit a rdf:Property ;
  rdfs:label "AreaDispatchableUnit"@en ;
  rdfs:comment "The dispatchable unit for this scheduled resource." ;
  cims:AssociationUsed "No" ;
  cims:inverseRoleName nc:AreaDispatchableUnit.ScheduleResource ;
  cims:multiplicity cims:M:0..1 ;
  cims:stereotype "NC", <http://iec.ch/TC57/NonStandard/UML#ofAggregate> ;
  rdfs:domain nc:ScheduleResource ;
  rdfs:range nc:AreaDispatchableUnit .

nc:ScheduleResource.GeneratingUnit a rdf:Property ;
  rdfs:label "GeneratingUnit"@en ;
  rdfs:comment "The generating unit that relates to this schedule resource." ;
  cims:AssociationUsed "No" ;
  cims:inverseRoleName nc:GeneratingUnit.ScheduleResource ;
  cims:multiplicity cims:M:0..n ;
  cims:stereotype "NC" ;
  rdfs:domain nc:ScheduleResource ;
  rdfs:range cim:GeneratingUnit .

nc:ScheduleResource.HydroPump a rdf:Property ;
  rdfs:label "HydroPump"@en ;
  rdfs:comment "The hydro pump that relates to this schedule resource." ;
  cims:AssociationUsed "No" ;
  cims:inverseRoleName nc:HydroPump.ScheduleResource ;
  cims:multiplicity cims:M:0..n ;
  cims:stereotype "NC" ;
  rdfs:domain nc:ScheduleResource ;
  rdfs:range cim:HydroPump .

nc:ScheduleResource.PowerElectronicsUnit a rdf:Property ;
  rdfs:label "PowerElectronicsUnit"@en ;
  rdfs:comment "The power electronics unit that relates to this schedule resource." ;
  cims:AssociationUsed "No" ;
  cims:inverseRoleName nc:PowerElectronicsUnit.ScheduleResource ;
  cims:multiplicity cims:M:0..n ;
  cims:stereotype "NC" ;
  rdfs:domain nc:ScheduleResource ;
  rdfs:range cim:PowerElectronicsUnit .

nc:ScheduleResource.PrimaryEnergySource a rdf:Property ;
  rdfs:label "PrimaryEnergySource"@en ;
  rdfs:comment "Primary energy reference type for this schedule resource." ;
  cims:AssociationUsed "Yes" ;
  cims:inverseRoleName nc:EnergyType.ScheduleResource ;
  cims:multiplicity cims:M:0..1 ;
  cims:stereotype "NC" ;
  rdfs:domain nc:ScheduleResource ;
  rdfs:range nc:EnergyType .

nc:ScheduleResource.ResourceOf a rdf:Property ;
  rdfs:label "ResourceOf"@en ;
  rdfs:comment "The schedule resource that has this subschedule resource." ;
  cims:AssociationUsed "Yes" ;
  cims:inverseRoleName nc:ScheduleResource.SubScheduleResource ;
  cims:multiplicity cims:M:0..1 ;
  cims:stereotype "NC" ;
  rdfs:domain nc:ScheduleResource ;
  rdfs:range nc:ScheduleResource .

nc:ScheduleResource.ScheduleResourceController a rdf:Property ;
  rdfs:label "ScheduleResourceController"@en ;
  rdfs:comment "Schedule resource controller for this schedule resource." ;
  cims:AssociationUsed "Yes" ;
  cims:inverseRoleName nc:ScheduleResourceController.ScheduleResource ;
  cims:multiplicity cims:M:0..1 ;
  cims:stereotype "NC" ;
  rdfs:domain nc:ScheduleResource ;
  rdfs:range nc:ScheduleResourceController .

nc:ScheduleResource.SchedulingArea a rdf:Property ;
  rdfs:label "SchedulingArea"@en ;
  rdfs:comment "The scheduling area that has this schedule resource." ;
  cims:AssociationUsed "Yes" ;
  cims:inverseRoleName nc:SchedulingArea.ScheduleResource ;
  cims:multiplicity cims:M:0..1 ;
  cims:stereotype "NC" ;
  rdfs:domain nc:ScheduleResource ;
  rdfs:range nc:SchedulingArea .

nc:ScheduleResource.SubScheduleResource a rdf:Property ;
  rdfs:label "SubScheduleResource"@en ;
  rdfs:comment "The subschedule resource that relates to the schedule resource." ;
  cims:AssociationUsed "No" ;
  cims:inverseRoleName nc:ScheduleResource.ResourceOf ;
  cims:multiplicity cims:M:0..n ;
  cims:stereotype "NC" ;
  rdfs:domain nc:ScheduleResource ;
  rdfs:range nc:ScheduleResource .

nc:ScheduleResourceController.ScheduleResource a rdf:Property ;
  rdfs:label "ScheduleResource"@en ;
  rdfs:comment "Schedule resource that has a schedule resource controller." ;
  cims:AssociationUsed "No" ;
  cims:inverseRoleName nc:ScheduleResource.ScheduleResourceController ;
  cims:multiplicity cims:M:0..1 ;
  cims:stereotype "NC" ;
  rdfs:domain nc:ScheduleResourceController ;
  rdfs:range nc:ScheduleResource .

nc:SchedulingArea.AreaDispatchableUnit a rdf:Property ;
  rdfs:label "AreaDispatchableUnit"@en ;
  rdfs:comment "The area dispatchable unit related to a scheduling area." ;
  cims:AssociationUsed "No" ;
  cims:inverseRoleName nc:AreaDispatchableUnit.SchedulingArea ;
  cims:multiplicity cims:M:0..n ;
  cims:stereotype "NC" ;
  rdfs:domain nc:SchedulingArea ;
  rdfs:range nc:AreaDispatchableUnit .

nc:SchedulingArea.BiddingZone a rdf:Property ;
  rdfs:label "BiddingZone"@en ;
  rdfs:comment "The bidding zone related to this scheduling area." ;
  cims:AssociationUsed "Yes" ;
  cims:inverseRoleName nc:BiddingZone.SchedulingArea ;
  cims:multiplicity cims:M:1 ;
  cims:stereotype "NC" ;
  rdfs:domain nc:SchedulingArea ;
  rdfs:range nc:BiddingZone .

nc:SchedulingArea.ControlArea a rdf:Property ;
  rdfs:label "ControlArea"@en ;
  rdfs:comment "The control area for this scheduling area." ;
  cims:AssociationUsed "Yes" ;
  cims:inverseRoleName nc:ControlArea.SchedulingArea ;
  cims:multiplicity cims:M:0..1 ;
  cims:stereotype "NC" ;
  rdfs:domain nc:SchedulingArea ;
  rdfs:range cim:ControlArea .

nc:SchedulingArea.DCTieCorridor a rdf:Property ;
  rdfs:label "DCTieCorridor"@en ;
  rdfs:comment "The DC tie corridor that is part of this scheduling area." ;
  cims:AssociationUsed "No" ;
  cims:inverseRoleName nc:DCTieCorridor.SchedulingArea ;
  cims:multiplicity cims:M:0..1 ;
  cims:stereotype "NC" ;
  rdfs:domain nc:SchedulingArea ;
  rdfs:range nc:DCTieCorridor .

nc:SchedulingArea.EnergyCoordinationRegion a rdf:Property ;
  rdfs:label "EnergyCoordinationRegion"@en ;
  rdfs:comment "The energy coordination region that has this scheduling area." ;
  cims:AssociationUsed "Yes" ;
  cims:inverseRoleName nc:EnergyCoordinationRegion.SchedulingArea ;
  cims:multiplicity cims:M:0..1 ;
  cims:stereotype "NC" ;
  rdfs:domain nc:SchedulingArea ;
  rdfs:range nc:EnergyCoordinationRegion .

nc:SchedulingArea.EnergyGroup a rdf:Property ;
  rdfs:label "EnergyGroup"@en ;
  rdfs:comment "The energy group belonging to a given energy scheduling area." ;
  cims:AssociationUsed "No" ;
  cims:inverseRoleName nc:EnergyGroup.SchedulingArea ;
  cims:multiplicity cims:M:0..n ;
  cims:stereotype "NC" ;
  rdfs:domain nc:SchedulingArea ;
  rdfs:range nc:EnergyGroup .

nc:SchedulingArea.Line a rdf:Property ;
  rdfs:label "Line"@en ;
  rdfs:comment "The line that is part of this scheduling area." ;
  cims:AssociationUsed "No" ;
  cims:inverseRoleName nc:Line.SchedulingArea ;
  cims:multiplicity cims:M:0..n ;
  cims:stereotype "NC" ;
  rdfs:domain nc:SchedulingArea ;
  rdfs:range cim:Line .

nc:SchedulingArea.LoadFrequencyControlArea a rdf:Property ;
  rdfs:label "LoadFrequencyControlArea"@en ;
  rdfs:comment "The load frequency control area which has this scheduling area." ;
  cims:AssociationUsed "Yes" ;
  cims:inverseRoleName nc:LoadFrequencyControlArea.SchedulingArea ;
  cims:multiplicity cims:M:0..1 ;
  cims:stereotype "NC" ;
  rdfs:domain nc:SchedulingArea ;
  rdfs:range nc:LoadFrequencyControlArea .

nc:SchedulingArea.PowerShiftKeyStrategy a rdf:Property ;
  rdfs:label "PowerShiftKeyStrategy"@en ;
  rdfs:comment "Power Shift Key Strategy which has a scheduling area." ;
  cims:AssociationUsed "No" ;
  cims:inverseRoleName nc:PowerShiftKeyStrategy.SchedulingArea ;
  cims:multiplicity cims:M:0..n ;
  cims:stereotype "NC" ;
  rdfs:domain nc:SchedulingArea ;
  rdfs:range nc:PowerShiftKeyStrategy .

nc:SchedulingArea.ScheduleResource a rdf:Property ;
  rdfs:label "ScheduleResource"@en ;
  rdfs:comment "The schedule resource that belongs to this scheduled area." ;
  cims:AssociationUsed "No" ;
  cims:inverseRoleName nc:ScheduleResource.SchedulingArea ;
  cims:multiplicity cims:M:0..n ;
  cims:stereotype "NC" ;
  rdfs:domain nc:SchedulingArea ;
  rdfs:range nc:ScheduleResource .

nc:SchedulingArea.SubSchedulingArea a rdf:Property ;
  rdfs:label "SubSchedulingArea"@en ;
  rdfs:comment "The subscheduling are that belongs to this scheduling area." ;
  cims:AssociationUsed "No" ;
  cims:inverseRoleName nc:SubSchedulingArea.SchedulingArea ;
  cims:multiplicity cims:M:0..n ;
  cims:stereotype "NC" ;
  rdfs:domain nc:SchedulingArea ;
  rdfs:range nc:SubSchedulingArea .

nc:SchedulingArea.Substation a rdf:Property ;
  rdfs:label "Substation"@en ;
  rdfs:comment "The substation that is part of this scheduling area." ;
  cims:AssociationUsed "No" ;
  cims:inverseRoleName nc:Substation.SchedulingArea ;
  cims:multiplicity cims:M:0..n ;
  cims:stereotype "NC" ;
  rdfs:domain nc:SchedulingArea ;
  rdfs:range cim:Substation .

nc:SchedulingArea.SynchronousArea a rdf:Property ;
  rdfs:label "SynchronousArea"@en ;
  rdfs:comment "The synchronous are that has this scheduling area." ;
  cims:AssociationUsed "Yes" ;
  cims:inverseRoleName nc:SynchronousArea.SchedulingArea ;
  cims:multiplicity cims:M:0..1 ;
  cims:stereotype "NC" ;
  rdfs:domain nc:SchedulingArea ;
  rdfs:range nc:SynchronousArea .

nc:SchedulingArea.SystemOperator a rdf:Property ;
  rdfs:label "SystemOperator"@en ;
  rdfs:comment "The system operator for this scheduling area." ;
  cims:AssociationUsed "Yes" ;
  cims:inverseRoleName nc:SystemOperator.SchedulingArea ;
  cims:multiplicity cims:M:0..1 ;
  cims:stereotype "NC" ;
  rdfs:domain nc:SchedulingArea ;
  rdfs:range nc:SystemOperator .

nc:SchedulingArea.isIslandingEnabled a rdf:Property ;
  rdfs:label "isIslandingEnabled"@en ;
  rdfs:comment "Identifies if the area can operate in island operation. If true, the area is enabled (capable) of operating as an electrical island. If false, the area does not have the capability or it is not enabled to operate as an electrical island." ;
  cims:dataType cim:Boolean ;
  cims:multiplicity cims:M:0..1 ;
  cims:stereotype "NC", <http://iec.ch/TC57/NonStandard/UML#attribute> ;
  rdfs:domain nc:SchedulingArea .

nc:SchedulingArea.isMeteringGridArea a rdf:Property ;
  rdfs:label "isMeteringGridArea"@en ;
  rdfs:comment "Identifies if the area is settlement metered for all import and export to the area. If true, the area is metered area. If false, it is not." ;
  cims:dataType cim:Boolean ;
  cims:multiplicity cims:M:0..1 ;
  cims:stereotype "NC", <http://iec.ch/TC57/NonStandard/UML#attribute> ;
  rdfs:domain nc:SchedulingArea .

nc:SchedulingArea.normalParticipationFactor a rdf:Property ;
  rdfs:label "normalParticipationFactor"@en ;
  rdfs:comment """Normal participation factor describing the entity part of the active power provided by a collection of entities (e.g. an active power forecast to a collection of entities is divided to each of the member entity according to the participation factor). Must be a positive value.
In the case of a sharing strategy, the distribution is following entities value (V) equals aggregated value (T) divided by sum of participation factors (PF), i.e. V=T/sum(PF). 
In the case of priority strategy, the item with the lowest number gets allocated energy first.""" ;
  cims:dataType cim:Float ;
  cims:multiplicity cims:M:0..1 ;
  cims:stereotype "NC", <http://iec.ch/TC57/NonStandard/UML#attribute> ;
  rdfs:domain nc:SchedulingArea .

nc:SecurityCoordinator.CapacityCalculationRegion a rdf:Property ;
  rdfs:label "CapacityCalculationRegion"@en ;
  rdfs:comment "The capacity calculation region operated by this security coordinator." ;
  cims:AssociationUsed "No" ;
  cims:inverseRoleName nc:CapacityCalculationRegion.SecurityCoordinator ;
  cims:multiplicity cims:M:0..n ;
  cims:stereotype "NC" ;
  rdfs:domain nc:SecurityCoordinator ;
  rdfs:range nc:CapacityCalculationRegion .

nc:SecurityCoordinator.OutageCoordinationRegion a rdf:Property ;
  rdfs:label "OutageCoordinationRegion"@en ;
  rdfs:comment "The outage coordination region that has this security coordinator." ;
  cims:AssociationUsed "No" ;
  cims:inverseRoleName nc:OutageCoordinationRegion.SecurityCoordinator ;
  cims:multiplicity cims:M:0..n ;
  cims:stereotype "NC" ;
  rdfs:domain nc:SecurityCoordinator ;
  rdfs:range nc:OutageCoordinationRegion .

nc:SolarRadiationDependencyCurve.OperationalLimitType a rdf:Property ;
  rdfs:label "OperationalLimitType"@en ;
  rdfs:comment "The operational limit type that has this permanent solar radiation curve." ;
  cims:AssociationUsed "No" ;
  cims:inverseRoleName nc:OperationalLimitType.PermanentSolarRadiationCurve ;
  cims:multiplicity cims:M:0..n ;
  cims:stereotype "NC" ;
  rdfs:domain nc:SolarRadiationDependencyCurve ;
  rdfs:range cim:OperationalLimitType .

nc:SubSchedulingArea.Feeder a rdf:Property ;
  rdfs:label "Feeder"@en ;
  rdfs:comment "The feeder that is part of this subscheduling area." ;
  cims:AssociationUsed "No" ;
  cims:inverseRoleName nc:Feeder.SubSchedulingArea ;
  cims:multiplicity cims:M:0..n ;
  cims:stereotype "NC" ;
  rdfs:domain nc:SubSchedulingArea ;
  rdfs:range cim:Feeder .

nc:SubSchedulingArea.SchedulingArea a rdf:Property ;
  rdfs:label "SchedulingArea"@en ;
  rdfs:comment "The scheduling area that has this subscheduling area." ;
  cims:AssociationUsed "Yes" ;
  cims:inverseRoleName nc:SchedulingArea.SubSchedulingArea ;
  cims:multiplicity cims:M:1 ;
  cims:stereotype "NC" ;
  rdfs:domain nc:SubSchedulingArea ;
  rdfs:range nc:SchedulingArea .

nc:Substation.DCSubstation a rdf:Property ;
  rdfs:label "DCSubstation"@en ;
  rdfs:comment "DC substation that is part of AC and DC substation." ;
  cims:AssociationUsed "No" ;
  cims:inverseRoleName nc:DCSubstation.Substation ;
  cims:multiplicity cims:M:0..n ;
  cims:stereotype "NC" ;
  rdfs:domain cim:Substation ;
  rdfs:range nc:DCSubstation .

nc:Substation.SchedulingArea a rdf:Property ;
  rdfs:label "SchedulingArea"@en ;
  rdfs:comment "The scheduling area that has this substation." ;
  cims:AssociationUsed "Yes" ;
  cims:inverseRoleName nc:SchedulingArea.Substation ;
  cims:multiplicity cims:M:0..1 ;
  cims:stereotype "NC" ;
  rdfs:domain cim:Substation ;
  rdfs:range nc:SchedulingArea .

nc:SynchronousArea.LoadFrequencyControlBlock a rdf:Property ;
  rdfs:label "LoadFrequencyControlBlock"@en ;
  rdfs:comment "The load frequency control block that is part of this synchronous area." ;
  cims:AssociationUsed "No" ;
  cims:inverseRoleName nc:LoadFrequencyControlBlock.SynchronousArea ;
  cims:multiplicity cims:M:0..n ;
  cims:stereotype "NC" ;
  rdfs:domain nc:SynchronousArea ;
  rdfs:range nc:LoadFrequencyControlBlock .

nc:SynchronousArea.SchedulingArea a rdf:Property ;
  rdfs:label "SchedulingArea"@en ;
  rdfs:comment "The scheduling area that is part of this synchronous area." ;
  cims:AssociationUsed "No" ;
  cims:inverseRoleName nc:SchedulingArea.SynchronousArea ;
  cims:multiplicity cims:M:0..n ;
  cims:stereotype "NC" ;
  rdfs:domain nc:SynchronousArea ;
  rdfs:range nc:SchedulingArea .

nc:SynchronousArea.nominalFrequency a rdf:Property ;
  rdfs:label "nominalFrequency"@en ;
  rdfs:comment "The nominal frequency for the Synchronous Area, e.g. 50 Hz for Europe." ;
  cims:dataType cim:Frequency ;
  cims:multiplicity cims:M:1..1 ;
  cims:stereotype "NC", <http://iec.ch/TC57/NonStandard/UML#attribute> ;
  rdfs:domain nc:SynchronousArea .

nc:SystemControl.EquipmentController a rdf:Property ;
  rdfs:label "EquipmentController"@en ;
  rdfs:comment "Equipment controller controlles by this system control" ;
  cims:AssociationUsed "Yes" ;
  cims:inverseRoleName nc:EquipmentController.SystemControl ;
  cims:multiplicity cims:M:1..n ;
  cims:stereotype "NC" ;
  rdfs:domain nc:SystemControl ;
  rdfs:range nc:EquipmentController .

nc:SystemOperator.ControlArea a rdf:Property ;
  rdfs:label "ControlArea"@en ;
  rdfs:comment "The control area that is related to this system operator." ;
  cims:AssociationUsed "No" ;
  cims:inverseRoleName nc:ControlArea.SystemOperator ;
  cims:multiplicity cims:M:0..n ;
  cims:stereotype "NC" ;
  rdfs:domain nc:SystemOperator ;
  rdfs:range cim:ControlArea .

nc:SystemOperator.SchedulingArea a rdf:Property ;
  rdfs:label "SchedulingArea"@en ;
  rdfs:comment "The scheduling area that is operated by this system operator." ;
  cims:AssociationUsed "No" ;
  cims:inverseRoleName nc:SchedulingArea.SystemOperator ;
  cims:multiplicity cims:M:0..n ;
  cims:stereotype "NC" ;
  rdfs:domain nc:SystemOperator ;
  rdfs:range nc:SchedulingArea .

nc:TCSCCompensationPoint.ThyristorControlledSeriesCompensator a rdf:Property ;
  rdfs:label "ThyristorControlledSeriesCompensator"@en ;
  rdfs:comment "TCSC that has different compensation points." ;
  cims:AssociationUsed "Yes" ;
  cims:inverseRoleName nc:ThyristorControlledSeriesCompensator.TCSCCompensationPoint ;
  cims:multiplicity cims:M:1 ;
  cims:stereotype "NC" ;
  rdfs:domain nc:TCSCCompensationPoint ;
  rdfs:range nc:ThyristorControlledSeriesCompensator .

nc:TCSCCompensationPoint.compensationZ a rdf:Property ;
  rdfs:label "compensationZ"@en ;
  rdfs:comment "The compensation impedance for this compensation point." ;
  cims:dataType cim:Impedance ;
  cims:multiplicity cims:M:1..1 ;
  cims:stereotype "NC", <http://iec.ch/TC57/NonStandard/UML#attribute> ;
  rdfs:domain nc:TCSCCompensationPoint .

nc:TCSCCompensationPoint.mRID a rdf:Property ;
  rdfs:label "mRID"@en ;
  rdfs:comment """Master resource identifier issued by a model authority. The mRID is unique within an exchange context. Global uniqueness is easily achieved by using a UUID, as specified in RFC 4122, for the mRID. The use of UUID is strongly recommended.
For CIMXML data files in RDF syntax conforming to IEC 61970-552, the mRID is mapped to rdf:ID or rdf:about attributes that identify CIM object elements.""" ;
  cims:dataType cim:String ;
  cims:multiplicity cims:M:1..1 ;
  cims:stereotype "NC", <http://iec.ch/TC57/NonStandard/UML#attribute> ;
  rdfs:domain nc:TCSCCompensationPoint .

nc:TCSCCompensationPoint.section a rdf:Property ;
  rdfs:label "section"@en ;
  rdfs:comment "The number of the section." ;
  cims:dataType cim:Integer ;
  cims:multiplicity cims:M:1..1 ;
  cims:stereotype "NC", <http://iec.ch/TC57/NonStandard/UML#attribute> ;
  rdfs:domain nc:TCSCCompensationPoint .

nc:TapChanger.TapChangeController a rdf:Property ;
  rdfs:label "TapChangeController"@en ;
  rdfs:comment "The tap changer controller that controls this TapChanger." ;
  cims:AssociationUsed "Yes" ;
  cims:inverseRoleName nc:TapChangerController.TapChanger ;
  cims:multiplicity cims:M:0..1 ;
  cims:stereotype "NC" ;
  rdfs:domain cim:TapChanger ;
  rdfs:range nc:TapChangerController .

nc:TapChangerController.TapChanger a rdf:Property ;
  rdfs:label "TapChanger"@en ;
  rdfs:comment "All tap changers controlled by this controller." ;
  cims:AssociationUsed "No" ;
  cims:inverseRoleName nc:TapChanger.TapChangeController ;
  cims:multiplicity cims:M:0..n ;
  cims:stereotype "NC" ;
  rdfs:domain nc:TapChangerController ;
  rdfs:range cim:TapChanger .

nc:Terminal.Circuit a rdf:Property ;
  rdfs:label "Circuit"@en ;
  rdfs:comment "Circuit that is identified by the given Terminal." ;
  cims:AssociationUsed "No" ;
  cims:inverseRoleName nc:Circuit.IdentifyingTerminal ;
  cims:multiplicity cims:M:0..1 ;
  cims:stereotype "NC" ;
  rdfs:domain cim:Terminal ;
  rdfs:range nc:Circuit .

nc:Terminal.FrequencyMonitoringTerminal a rdf:Property ;
  rdfs:label "FrequencyMonitoringTerminal"@en ;
  rdfs:comment "Frequency monitoring terminal that has a terminal." ;
  cims:AssociationUsed "No" ;
  cims:inverseRoleName nc:FrequencyMonitoringTerminal.Terminal ;
  cims:multiplicity cims:M:0..n ;
  cims:stereotype "NC" ;
  rdfs:domain cim:Terminal ;
  rdfs:range nc:FrequencyMonitoringTerminal .

nc:Terminal.PinTerminal a rdf:Property ;
  rdfs:label "PinTerminal"@en ;
  rdfs:comment "The pin that uses this input." ;
  cims:AssociationUsed "No" ;
  cims:inverseRoleName nc:PinTerminal.Terminal ;
  cims:multiplicity cims:M:0..n ;
  cims:stereotype "NC" ;
  rdfs:domain cim:Terminal ;
  rdfs:range nc:PinTerminal .

nc:Terminal.VoltageAngleLimit a rdf:Property ;
  rdfs:label "VoltageAngleLimit"@en ;
  rdfs:comment "The voltage angle limit which has this reference angle terminal." ;
  cims:AssociationUsed "No" ;
  cims:inverseRoleName nc:VoltageAngleLimit.AngleReferenceTerminal ;
  cims:multiplicity cims:M:0..n ;
  cims:stereotype "NC" ;
  rdfs:domain cim:Terminal ;
  rdfs:range nc:VoltageAngleLimit .

nc:ThyristorControlledSeriesCompensator.TCSCCompensationPoint a rdf:Property ;
  rdfs:label "TCSCCompensationPoint"@en ;
  rdfs:comment "Compensation point for this TCSC." ;
  cims:AssociationUsed "No" ;
  cims:inverseRoleName nc:TCSCCompensationPoint.ThyristorControlledSeriesCompensator ;
  cims:multiplicity cims:M:0..n ;
  cims:stereotype "NC" ;
  rdfs:domain nc:ThyristorControlledSeriesCompensator ;
  rdfs:range nc:TCSCCompensationPoint .

nc:ThyristorControlledSeriesCompensator.flexibleCapacitiveZ a rdf:Property ;
  rdfs:label "flexibleCapacitiveZ"@en ;
  rdfs:comment "Flexible impedance that can be controlled by the compensator when operating in the capacitive range.  Shall always be positive." ;
  cims:dataType cim:Impedance ;
  cims:multiplicity cims:M:1..1 ;
  cims:stereotype "NC", <http://iec.ch/TC57/NonStandard/UML#attribute> ;
  rdfs:domain nc:ThyristorControlledSeriesCompensator .

nc:ThyristorControlledSeriesCompensator.flexibleInductiveZ a rdf:Property ;
  rdfs:label "flexibleInductiveZ"@en ;
  rdfs:comment "Flexible impedance that can be controlled by the compensator when operating in the inductive range.  Shall always be negative." ;
  cims:dataType cim:Impedance ;
  cims:multiplicity cims:M:1..1 ;
  cims:stereotype "NC", <http://iec.ch/TC57/NonStandard/UML#attribute> ;
  rdfs:domain nc:ThyristorControlledSeriesCompensator .

nc:ThyristorControlledSeriesCompensator.minI a rdf:Property ;
  rdfs:label "minI"@en ;
  rdfs:comment "Minimum current below which the device bypassed." ;
  cims:dataType cim:CurrentFlow ;
  cims:multiplicity cims:M:1..1 ;
  cims:stereotype "NC", <http://iec.ch/TC57/NonStandard/UML#attribute> ;
  rdfs:domain nc:ThyristorControlledSeriesCompensator .

nc:ThyristorControlledSeriesCompensator.reconnectionI a rdf:Property ;
  rdfs:label "reconnectionI"@en ;
  rdfs:comment "The current for which the TCSC returns back to operation after bypass." ;
  cims:dataType cim:CurrentFlow ;
  cims:multiplicity cims:M:1..1 ;
  cims:stereotype "NC", <http://iec.ch/TC57/NonStandard/UML#attribute> ;
  rdfs:domain nc:ThyristorControlledSeriesCompensator .

nc:TieCorridor.AreaDispatchableUnit a rdf:Property ;
  rdfs:label "AreaDispatchableUnit"@en ;
  rdfs:comment "AreaDispatchableUnit for the Tie Corridor." ;
  cims:AssociationUsed "No" ;
  cims:inverseRoleName nc:AreaDispatchableUnit.TieCorridor ;
  cims:multiplicity cims:M:0..n ;
  cims:stereotype "NC" ;
  rdfs:domain nc:TieCorridor ;
  rdfs:range nc:AreaDispatchableUnit .

nc:TieCorridor.BiddingZoneBorder a rdf:Property ;
  rdfs:label "BiddingZoneBorder"@en ;
  rdfs:comment "Bidding zone border in which the tie corridor is located." ;
  cims:AssociationUsed "Yes" ;
  cims:inverseRoleName nc:BiddingZoneBorder.TieCorridor ;
  cims:multiplicity cims:M:0..1 ;
  cims:stereotype "NC" ;
  rdfs:domain nc:TieCorridor ;
  rdfs:range nc:BiddingZoneBorder .

nc:TieCorridor.LoadFrequencyControlArea a rdf:Property ;
  rdfs:label "LoadFrequencyControlArea"@en ;
  rdfs:comment "LoadFrequencyControlArea controlling the TieCorridor." ;
  cims:AssociationUsed "Yes" ;
  cims:inverseRoleName nc:LoadFrequencyControlArea.TieCorridor ;
  cims:multiplicity cims:M:0..1 ;
  cims:stereotype "NC" ;
  rdfs:domain nc:TieCorridor ;
  rdfs:range nc:LoadFrequencyControlArea .

nc:TieCorridor.TieFlow a rdf:Property ;
  rdfs:label "TieFlow"@en ;
  rdfs:comment "Tie flow which belongs to the tie corridor." ;
  cims:AssociationUsed "No" ;
  cims:inverseRoleName nc:TieFlow.TieCorridor ;
  cims:multiplicity cims:M:0..n ;
  cims:stereotype "NC" ;
  rdfs:domain nc:TieCorridor ;
  rdfs:range cim:TieFlow .

nc:TieCorridor.delayRegulatingReserve a rdf:Property ;
  rdfs:label "delayRegulatingReserve"@en ;
  rdfs:comment "A positive number that is a multiple of Automatic Generation Control (AGC) run cycles that describes the delay in adapting imbalance of the tie corridor." ;
  cims:dataType cim:Seconds ;
  cims:multiplicity cims:M:0..1 ;
  cims:stereotype "NC", <http://iec.ch/TC57/NonStandard/UML#attribute> ;
  rdfs:domain nc:TieCorridor .

nc:TieCorridor.maxRegulatingReserveRamp a rdf:Property ;
  rdfs:label "maxRegulatingReserveRamp"@en ;
  rdfs:comment "Maximum authorized ramp for regulating reserve." ;
  cims:dataType cim:Float ;
  cims:multiplicity cims:M:0..1 ;
  cims:stereotype "NC", <http://iec.ch/TC57/NonStandard/UML#attribute> ;
  rdfs:domain nc:TieCorridor .

nc:TieCorridor.thresholdRegulatingReserve a rdf:Property ;
  rdfs:label "thresholdRegulatingReserve"@en ;
  rdfs:comment "Regulating reserve threshold." ;
  cims:dataType cim:ActivePower ;
  cims:multiplicity cims:M:0..1 ;
  cims:stereotype "NC", <http://iec.ch/TC57/NonStandard/UML#attribute> ;
  rdfs:domain nc:TieCorridor .

nc:TieFlow.TieCorridor a rdf:Property ;
  rdfs:label "TieCorridor"@en ;
  rdfs:comment "Tie corridor which has the tie flow." ;
  cims:AssociationUsed "Yes" ;
  cims:inverseRoleName nc:TieCorridor.TieFlow ;
  cims:multiplicity cims:M:0..1 ;
  cims:stereotype "NC" ;
  rdfs:domain cim:TieFlow ;
  rdfs:range nc:TieCorridor .

nc:VoltageAngleLimit.AngleReferenceTerminal a rdf:Property ;
  rdfs:label "AngleReferenceTerminal"@en ;
  rdfs:comment "The angle reference terminal for the voltage angle limit." ;
  cims:AssociationUsed "Yes" ;
  cims:inverseRoleName nc:Terminal.VoltageAngleLimit ;
  cims:multiplicity cims:M:1 ;
  cims:stereotype "NC" ;
  rdfs:domain nc:VoltageAngleLimit ;
  rdfs:range cim:Terminal .

nc:VoltageAngleLimit.isFlowToRefTerminal a rdf:Property ;
  rdfs:label "isFlowToRefTerminal"@en ;
  rdfs:comment "True if the flow is from the operating limit terminal to the angle reference terminal. False means that the flow is the other direction. When it is not given, the limit is the same for both directions." ;
  cims:dataType cim:Boolean ;
  cims:multiplicity cims:M:0..1 ;
  cims:stereotype "NC", <http://iec.ch/TC57/NonStandard/UML#attribute> ;
  rdfs:domain nc:VoltageAngleLimit .

nc:VoltageAngleLimit.normalValue a rdf:Property ;
  rdfs:label "normalValue"@en ;
  rdfs:comment "The difference in angle degrees between referenced by the association end OperationalLimitSet.Terminal and the Terminal referenced by the association end VoltageAngleLimit.AngleReferenceTerminal. The value shall be positive (greater than zero)." ;
  cims:dataType cim:AngleDegrees ;
  cims:multiplicity cims:M:1..1 ;
  cims:stereotype "NC", <http://iec.ch/TC57/NonStandard/UML#attribute> ;
  rdfs:domain nc:VoltageAngleLimit .

nc:VsCapabilityCurve.referenceVoltage a rdf:Property ;
  rdfs:label "referenceVoltage"@en ;
  rdfs:comment "The reference voltage for which the capability curve is valid." ;
  cims:dataType cim:Voltage ;
  cims:multiplicity cims:M:1..1 ;
  cims:stereotype "NC", <http://iec.ch/TC57/NonStandard/UML#attribute> ;
  rdfs:domain cim:VsCapabilityCurve .

cim:Currency.AED a cim:Currency ;
  rdfs:label "AED"@en ;
  rdfs:comment "United Arab Emirates dirham." ;
  cims:stereotype "enum" .

cim:Currency.AFN a cim:Currency ;
  rdfs:label "AFN"@en ;
  rdfs:comment "Afghan afghani." ;
  cims:stereotype "enum" .

cim:Currency.ALL a cim:Currency ;
  rdfs:label "ALL"@en ;
  rdfs:comment "Albanian lek." ;
  cims:stereotype "enum" .

cim:Currency.AMD a cim:Currency ;
  rdfs:label "AMD"@en ;
  rdfs:comment "Armenian dram." ;
  cims:stereotype "enum" .

cim:Currency.ANG a cim:Currency ;
  rdfs:label "ANG"@en ;
  rdfs:comment "Netherlands Antillean guilder." ;
  cims:stereotype "enum" .

cim:Currency.AOA a cim:Currency ;
  rdfs:label "AOA"@en ;
  rdfs:comment "Angolan kwanza." ;
  cims:stereotype "enum" .

cim:Currency.ARS a cim:Currency ;
  rdfs:label "ARS"@en ;
  rdfs:comment "Argentine peso." ;
  cims:stereotype "enum" .

cim:Currency.AUD a cim:Currency ;
  rdfs:label "AUD"@en ;
  rdfs:comment "Australian dollar." ;
  cims:stereotype "enum" .

cim:Currency.AWG a cim:Currency ;
  rdfs:label "AWG"@en ;
  rdfs:comment "Aruban florin." ;
  cims:stereotype "enum" .

cim:Currency.AZN a cim:Currency ;
  rdfs:label "AZN"@en ;
  rdfs:comment "Azerbaijani manat." ;
  cims:stereotype "enum" .

cim:Currency.BAM a cim:Currency ;
  rdfs:label "BAM"@en ;
  rdfs:comment "Bosnia and Herzegovina convertible mark." ;
  cims:stereotype "enum" .

cim:Currency.BBD a cim:Currency ;
  rdfs:label "BBD"@en ;
  rdfs:comment "Barbados dollar." ;
  cims:stereotype "enum" .

cim:Currency.BDT a cim:Currency ;
  rdfs:label "BDT"@en ;
  rdfs:comment "Bangladeshi taka." ;
  cims:stereotype "enum" .

cim:Currency.BGN a cim:Currency ;
  rdfs:label "BGN"@en ;
  rdfs:comment "Bulgarian lev." ;
  cims:stereotype "enum" .

cim:Currency.BHD a cim:Currency ;
  rdfs:label "BHD"@en ;
  rdfs:comment "Bahraini dinar." ;
  cims:stereotype "enum" .

cim:Currency.BIF a cim:Currency ;
  rdfs:label "BIF"@en ;
  rdfs:comment "Burundian franc." ;
  cims:stereotype "enum" .

cim:Currency.BMD a cim:Currency ;
  rdfs:label "BMD"@en ;
  rdfs:comment "Bermudian dollar (customarily known as Bermuda dollar)." ;
  cims:stereotype "enum" .

cim:Currency.BND a cim:Currency ;
  rdfs:label "BND"@en ;
  rdfs:comment "Brunei dollar." ;
  cims:stereotype "enum" .

cim:Currency.BOB a cim:Currency ;
  rdfs:label "BOB"@en ;
  rdfs:comment "Boliviano." ;
  cims:stereotype "enum" .

cim:Currency.BOV a cim:Currency ;
  rdfs:label "BOV"@en ;
  rdfs:comment "Bolivian Mvdol (funds code)." ;
  cims:stereotype "enum" .

cim:Currency.BRL a cim:Currency ;
  rdfs:label "BRL"@en ;
  rdfs:comment "Brazilian real." ;
  cims:stereotype "enum" .

cim:Currency.BSD a cim:Currency ;
  rdfs:label "BSD"@en ;
  rdfs:comment "Bahamian dollar." ;
  cims:stereotype "enum" .

cim:Currency.BTN a cim:Currency ;
  rdfs:label "BTN"@en ;
  rdfs:comment "Bhutanese ngultrum." ;
  cims:stereotype "enum" .

cim:Currency.BWP a cim:Currency ;
  rdfs:label "BWP"@en ;
  rdfs:comment "Botswana pula." ;
  cims:stereotype "enum" .

cim:Currency.BYR a cim:Currency ;
  rdfs:label "BYR"@en ;
  rdfs:comment "Belarusian ruble." ;
  cims:stereotype "enum" .

cim:Currency.BZD a cim:Currency ;
  rdfs:label "BZD"@en ;
  rdfs:comment "Belize dollar." ;
  cims:stereotype "enum" .

cim:Currency.CAD a cim:Currency ;
  rdfs:label "CAD"@en ;
  rdfs:comment "Canadian dollar." ;
  cims:stereotype "enum" .

cim:Currency.CDF a cim:Currency ;
  rdfs:label "CDF"@en ;
  rdfs:comment "Congolese franc." ;
  cims:stereotype "enum" .

cim:Currency.CHF a cim:Currency ;
  rdfs:label "CHF"@en ;
  rdfs:comment "Swiss franc." ;
  cims:stereotype "enum" .

cim:Currency.CLF a cim:Currency ;
  rdfs:label "CLF"@en ;
  rdfs:comment "Unidad de Fomento (funds code), Chile." ;
  cims:stereotype "enum" .

cim:Currency.CLP a cim:Currency ;
  rdfs:label "CLP"@en ;
  rdfs:comment "Chilean peso." ;
  cims:stereotype "enum" .

cim:Currency.CNY a cim:Currency ;
  rdfs:label "CNY"@en ;
  rdfs:comment "Chinese yuan." ;
  cims:stereotype "enum" .

cim:Currency.COP a cim:Currency ;
  rdfs:label "COP"@en ;
  rdfs:comment "Colombian peso." ;
  cims:stereotype "enum" .

cim:Currency.COU a cim:Currency ;
  rdfs:label "COU"@en ;
  rdfs:comment "Unidad de Valor Real." ;
  cims:stereotype "enum" .

cim:Currency.CRC a cim:Currency ;
  rdfs:label "CRC"@en ;
  rdfs:comment "Costa Rican colon." ;
  cims:stereotype "enum" .

cim:Currency.CUC a cim:Currency ;
  rdfs:label "CUC"@en ;
  rdfs:comment "Cuban convertible peso." ;
  cims:stereotype "enum" .

cim:Currency.CUP a cim:Currency ;
  rdfs:label "CUP"@en ;
  rdfs:comment "Cuban peso." ;
  cims:stereotype "enum" .

cim:Currency.CVE a cim:Currency ;
  rdfs:label "CVE"@en ;
  rdfs:comment "Cape Verde escudo." ;
  cims:stereotype "enum" .

cim:Currency.CZK a cim:Currency ;
  rdfs:label "CZK"@en ;
  rdfs:comment "Czech koruna." ;
  cims:stereotype "enum" .

cim:Currency.DJF a cim:Currency ;
  rdfs:label "DJF"@en ;
  rdfs:comment "Djiboutian franc." ;
  cims:stereotype "enum" .

cim:Currency.DKK a cim:Currency ;
  rdfs:label "DKK"@en ;
  rdfs:comment "Danish krone." ;
  cims:stereotype "enum" .

cim:Currency.DOP a cim:Currency ;
  rdfs:label "DOP"@en ;
  rdfs:comment "Dominican peso." ;
  cims:stereotype "enum" .

cim:Currency.DZD a cim:Currency ;
  rdfs:label "DZD"@en ;
  rdfs:comment "Algerian dinar." ;
  cims:stereotype "enum" .

cim:Currency.EEK a cim:Currency ;
  rdfs:label "EEK"@en ;
  rdfs:comment "Estonian kroon." ;
  cims:stereotype "enum" .

cim:Currency.EGP a cim:Currency ;
  rdfs:label "EGP"@en ;
  rdfs:comment "Egyptian pound." ;
  cims:stereotype "enum" .

cim:Currency.ERN a cim:Currency ;
  rdfs:label "ERN"@en ;
  rdfs:comment "Eritrean nakfa." ;
  cims:stereotype "enum" .

cim:Currency.ETB a cim:Currency ;
  rdfs:label "ETB"@en ;
  rdfs:comment "Ethiopian birr." ;
  cims:stereotype "enum" .

cim:Currency.EUR a cim:Currency ;
  rdfs:label "EUR"@en ;
  rdfs:comment "Euro." ;
  cims:stereotype "enum" .

cim:Currency.FJD a cim:Currency ;
  rdfs:label "FJD"@en ;
  rdfs:comment "Fiji dollar." ;
  cims:stereotype "enum" .

cim:Currency.FKP a cim:Currency ;
  rdfs:label "FKP"@en ;
  rdfs:comment "Falkland Islands pound." ;
  cims:stereotype "enum" .

cim:Currency.GBP a cim:Currency ;
  rdfs:label "GBP"@en ;
  rdfs:comment "Pound sterling." ;
  cims:stereotype "enum" .

cim:Currency.GEL a cim:Currency ;
  rdfs:label "GEL"@en ;
  rdfs:comment "Georgian lari." ;
  cims:stereotype "enum" .

cim:Currency.GHS a cim:Currency ;
  rdfs:label "GHS"@en ;
  rdfs:comment "Ghanaian cedi." ;
  cims:stereotype "enum" .

cim:Currency.GIP a cim:Currency ;
  rdfs:label "GIP"@en ;
  rdfs:comment "Gibraltar pound." ;
  cims:stereotype "enum" .

cim:Currency.GMD a cim:Currency ;
  rdfs:label "GMD"@en ;
  rdfs:comment "Gambian dalasi." ;
  cims:stereotype "enum" .

cim:Currency.GNF a cim:Currency ;
  rdfs:label "GNF"@en ;
  rdfs:comment "Guinean franc." ;
  cims:stereotype "enum" .

cim:Currency.GTQ a cim:Currency ;
  rdfs:label "GTQ"@en ;
  rdfs:comment "Guatemalan quetzal." ;
  cims:stereotype "enum" .

cim:Currency.GYD a cim:Currency ;
  rdfs:label "GYD"@en ;
  rdfs:comment "Guyanese dollar." ;
  cims:stereotype "enum" .

cim:Currency.HKD a cim:Currency ;
  rdfs:label "HKD"@en ;
  rdfs:comment "Hong Kong dollar." ;
  cims:stereotype "enum" .

cim:Currency.HNL a cim:Currency ;
  rdfs:label "HNL"@en ;
  rdfs:comment "Honduran lempira." ;
  cims:stereotype "enum" .

cim:Currency.HRK a cim:Currency ;
  rdfs:label "HRK"@en ;
  rdfs:comment "Croatian kuna." ;
  cims:stereotype "enum" .

cim:Currency.HTG a cim:Currency ;
  rdfs:label "HTG"@en ;
  rdfs:comment "Haitian gourde." ;
  cims:stereotype "enum" .

cim:Currency.HUF a cim:Currency ;
  rdfs:label "HUF"@en ;
  rdfs:comment "Hungarian forint." ;
  cims:stereotype "enum" .

cim:Currency.IDR a cim:Currency ;
  rdfs:label "IDR"@en ;
  rdfs:comment "Indonesian rupiah." ;
  cims:stereotype "enum" .

cim:Currency.ILS a cim:Currency ;
  rdfs:label "ILS"@en ;
  rdfs:comment "Israeli new sheqel." ;
  cims:stereotype "enum" .

cim:Currency.INR a cim:Currency ;
  rdfs:label "INR"@en ;
  rdfs:comment "Indian rupee." ;
  cims:stereotype "enum" .

cim:Currency.IQD a cim:Currency ;
  rdfs:label "IQD"@en ;
  rdfs:comment "Iraqi dinar." ;
  cims:stereotype "enum" .

cim:Currency.IRR a cim:Currency ;
  rdfs:label "IRR"@en ;
  rdfs:comment "Iranian rial." ;
  cims:stereotype "enum" .

cim:Currency.ISK a cim:Currency ;
  rdfs:label "ISK"@en ;
  rdfs:comment "Icelandic króna." ;
  cims:stereotype "enum" .

cim:Currency.JMD a cim:Currency ;
  rdfs:label "JMD"@en ;
  rdfs:comment "Jamaican dollar." ;
  cims:stereotype "enum" .

cim:Currency.JOD a cim:Currency ;
  rdfs:label "JOD"@en ;
  rdfs:comment "Jordanian dinar." ;
  cims:stereotype "enum" .

cim:Currency.JPY a cim:Currency ;
  rdfs:label "JPY"@en ;
  rdfs:comment "Japanese yen." ;
  cims:stereotype "enum" .

cim:Currency.KES a cim:Currency ;
  rdfs:label "KES"@en ;
  rdfs:comment "Kenyan shilling." ;
  cims:stereotype "enum" .

cim:Currency.KGS a cim:Currency ;
  rdfs:label "KGS"@en ;
  rdfs:comment "Kyrgyzstani som." ;
  cims:stereotype "enum" .

cim:Currency.KHR a cim:Currency ;
  rdfs:label "KHR"@en ;
  rdfs:comment "Cambodian riel." ;
  cims:stereotype "enum" .

cim:Currency.KMF a cim:Currency ;
  rdfs:label "KMF"@en ;
  rdfs:comment "Comoro franc." ;
  cims:stereotype "enum" .

cim:Currency.KPW a cim:Currency ;
  rdfs:label "KPW"@en ;
  rdfs:comment "North Korean won." ;
  cims:stereotype "enum" .

cim:Currency.KRW a cim:Currency ;
  rdfs:label "KRW"@en ;
  rdfs:comment "South Korean won." ;
  cims:stereotype "enum" .

cim:Currency.KWD a cim:Currency ;
  rdfs:label "KWD"@en ;
  rdfs:comment "Kuwaiti dinar." ;
  cims:stereotype "enum" .

cim:Currency.KYD a cim:Currency ;
  rdfs:label "KYD"@en ;
  rdfs:comment "Cayman Islands dollar." ;
  cims:stereotype "enum" .

cim:Currency.KZT a cim:Currency ;
  rdfs:label "KZT"@en ;
  rdfs:comment "Kazakhstani tenge." ;
  cims:stereotype "enum" .

cim:Currency.LAK a cim:Currency ;
  rdfs:label "LAK"@en ;
  rdfs:comment "Lao kip." ;
  cims:stereotype "enum" .

cim:Currency.LBP a cim:Currency ;
  rdfs:label "LBP"@en ;
  rdfs:comment "Lebanese pound." ;
  cims:stereotype "enum" .

cim:Currency.LKR a cim:Currency ;
  rdfs:label "LKR"@en ;
  rdfs:comment "Sri Lanka rupee." ;
  cims:stereotype "enum" .

cim:Currency.LRD a cim:Currency ;
  rdfs:label "LRD"@en ;
  rdfs:comment "Liberian dollar." ;
  cims:stereotype "enum" .

cim:Currency.LSL a cim:Currency ;
  rdfs:label "LSL"@en ;
  rdfs:comment "Lesotho loti." ;
  cims:stereotype "enum" .

cim:Currency.LTL a cim:Currency ;
  rdfs:label "LTL"@en ;
  rdfs:comment "Lithuanian litas." ;
  cims:stereotype "enum" .

cim:Currency.LVL a cim:Currency ;
  rdfs:label "LVL"@en ;
  rdfs:comment "Latvian lats." ;
  cims:stereotype "enum" .

cim:Currency.LYD a cim:Currency ;
  rdfs:label "LYD"@en ;
  rdfs:comment "Libyan dinar." ;
  cims:stereotype "enum" .

cim:Currency.MAD a cim:Currency ;
  rdfs:label "MAD"@en ;
  rdfs:comment "Moroccan dirham." ;
  cims:stereotype "enum" .

cim:Currency.MDL a cim:Currency ;
  rdfs:label "MDL"@en ;
  rdfs:comment "Moldovan leu." ;
  cims:stereotype "enum" .

cim:Currency.MGA a cim:Currency ;
  rdfs:label "MGA"@en ;
  rdfs:comment "Malagasy ariary." ;
  cims:stereotype "enum" .

cim:Currency.MKD a cim:Currency ;
  rdfs:label "MKD"@en ;
  rdfs:comment "Macedonian denar." ;
  cims:stereotype "enum" .

cim:Currency.MMK a cim:Currency ;
  rdfs:label "MMK"@en ;
  rdfs:comment "Myanma kyat." ;
  cims:stereotype "enum" .

cim:Currency.MNT a cim:Currency ;
  rdfs:label "MNT"@en ;
  rdfs:comment "Mongolian tugrik." ;
  cims:stereotype "enum" .

cim:Currency.MOP a cim:Currency ;
  rdfs:label "MOP"@en ;
  rdfs:comment "Macanese pataca." ;
  cims:stereotype "enum" .

cim:Currency.MRO a cim:Currency ;
  rdfs:label "MRO"@en ;
  rdfs:comment "Mauritanian ouguiya." ;
  cims:stereotype "enum" .

cim:Currency.MUR a cim:Currency ;
  rdfs:label "MUR"@en ;
  rdfs:comment "Mauritian rupee." ;
  cims:stereotype "enum" .

cim:Currency.MVR a cim:Currency ;
  rdfs:label "MVR"@en ;
  rdfs:comment "Maldivian rufiyaa." ;
  cims:stereotype "enum" .

cim:Currency.MWK a cim:Currency ;
  rdfs:label "MWK"@en ;
  rdfs:comment "Malawian kwacha." ;
  cims:stereotype "enum" .

cim:Currency.MXN a cim:Currency ;
  rdfs:label "MXN"@en ;
  rdfs:comment "Mexican peso." ;
  cims:stereotype "enum" .

cim:Currency.MYR a cim:Currency ;
  rdfs:label "MYR"@en ;
  rdfs:comment "Malaysian ringgit." ;
  cims:stereotype "enum" .

cim:Currency.MZN a cim:Currency ;
  rdfs:label "MZN"@en ;
  rdfs:comment "Mozambican metical." ;
  cims:stereotype "enum" .

cim:Currency.NAD a cim:Currency ;
  rdfs:label "NAD"@en ;
  rdfs:comment "Namibian dollar." ;
  cims:stereotype "enum" .

cim:Currency.NGN a cim:Currency ;
  rdfs:label "NGN"@en ;
  rdfs:comment "Nigerian naira." ;
  cims:stereotype "enum" .

cim:Currency.NIO a cim:Currency ;
  rdfs:label "NIO"@en ;
  rdfs:comment "Cordoba oro." ;
  cims:stereotype "enum" .

cim:Currency.NOK a cim:Currency ;
  rdfs:label "NOK"@en ;
  rdfs:comment "Norwegian krone." ;
  cims:stereotype "enum" .

cim:Currency.NPR a cim:Currency ;
  rdfs:label "NPR"@en ;
  rdfs:comment "Nepalese rupee." ;
  cims:stereotype "enum" .

cim:Currency.NZD a cim:Currency ;
  rdfs:label "NZD"@en ;
  rdfs:comment "New Zealand dollar." ;
  cims:stereotype "enum" .

cim:Currency.OMR a cim:Currency ;
  rdfs:label "OMR"@en ;
  rdfs:comment "Omani rial." ;
  cims:stereotype "enum" .

cim:Currency.PAB a cim:Currency ;
  rdfs:label "PAB"@en ;
  rdfs:comment "Panamanian balboa." ;
  cims:stereotype "enum" .

cim:Currency.PEN a cim:Currency ;
  rdfs:label "PEN"@en ;
  rdfs:comment "Peruvian nuevo sol." ;
  cims:stereotype "enum" .

cim:Currency.PGK a cim:Currency ;
  rdfs:label "PGK"@en ;
  rdfs:comment "Papua New Guinean kina." ;
  cims:stereotype "enum" .

cim:Currency.PHP a cim:Currency ;
  rdfs:label "PHP"@en ;
  rdfs:comment "Philippine peso." ;
  cims:stereotype "enum" .

cim:Currency.PKR a cim:Currency ;
  rdfs:label "PKR"@en ;
  rdfs:comment "Pakistani rupee." ;
  cims:stereotype "enum" .

cim:Currency.PLN a cim:Currency ;
  rdfs:label "PLN"@en ;
  rdfs:comment "Polish zloty." ;
  cims:stereotype "enum" .

cim:Currency.PYG a cim:Currency ;
  rdfs:label "PYG"@en ;
  rdfs:comment "Paraguayan guaraní." ;
  cims:stereotype "enum" .

cim:Currency.QAR a cim:Currency ;
  rdfs:label "QAR"@en ;
  rdfs:comment "Qatari rial." ;
  cims:stereotype "enum" .

cim:Currency.RON a cim:Currency ;
  rdfs:label "RON"@en ;
  rdfs:comment "Romanian new leu." ;
  cims:stereotype "enum" .

cim:Currency.RSD a cim:Currency ;
  rdfs:label "RSD"@en ;
  rdfs:comment "Serbian dinar." ;
  cims:stereotype "enum" .

cim:Currency.RUB a cim:Currency ;
  rdfs:label "RUB"@en ;
  rdfs:comment "Russian rouble." ;
  cims:stereotype "enum" .

cim:Currency.RWF a cim:Currency ;
  rdfs:label "RWF"@en ;
  rdfs:comment "Rwandan franc." ;
  cims:stereotype "enum" .

cim:Currency.SAR a cim:Currency ;
  rdfs:label "SAR"@en ;
  rdfs:comment "Saudi riyal." ;
  cims:stereotype "enum" .

cim:Currency.SBD a cim:Currency ;
  rdfs:label "SBD"@en ;
  rdfs:comment "Solomon Islands dollar." ;
  cims:stereotype "enum" .

cim:Currency.SCR a cim:Currency ;
  rdfs:label "SCR"@en ;
  rdfs:comment "Seychelles rupee." ;
  cims:stereotype "enum" .

cim:Currency.SDG a cim:Currency ;
  rdfs:label "SDG"@en ;
  rdfs:comment "Sudanese pound." ;
  cims:stereotype "enum" .

cim:Currency.SEK a cim:Currency ;
  rdfs:label "SEK"@en ;
  rdfs:comment "Swedish krona/kronor." ;
  cims:stereotype "enum" .

cim:Currency.SGD a cim:Currency ;
  rdfs:label "SGD"@en ;
  rdfs:comment "Singapore dollar." ;
  cims:stereotype "enum" .

cim:Currency.SHP a cim:Currency ;
  rdfs:label "SHP"@en ;
  rdfs:comment "Saint Helena pound." ;
  cims:stereotype "enum" .

cim:Currency.SLL a cim:Currency ;
  rdfs:label "SLL"@en ;
  rdfs:comment "Sierra Leonean leone." ;
  cims:stereotype "enum" .

cim:Currency.SOS a cim:Currency ;
  rdfs:label "SOS"@en ;
  rdfs:comment "Somali shilling." ;
  cims:stereotype "enum" .

cim:Currency.SRD a cim:Currency ;
  rdfs:label "SRD"@en ;
  rdfs:comment "Surinamese dollar." ;
  cims:stereotype "enum" .

cim:Currency.STD a cim:Currency ;
  rdfs:label "STD"@en ;
  rdfs:comment "São Tomé and Príncipe dobra." ;
  cims:stereotype "enum" .

cim:Currency.SYP a cim:Currency ;
  rdfs:label "SYP"@en ;
  rdfs:comment "Syrian pound." ;
  cims:stereotype "enum" .

cim:Currency.SZL a cim:Currency ;
  rdfs:label "SZL"@en ;
  rdfs:comment "Lilangeni." ;
  cims:stereotype "enum" .

cim:Currency.THB a cim:Currency ;
  rdfs:label "THB"@en ;
  rdfs:comment "Thai baht." ;
  cims:stereotype "enum" .

cim:Currency.TJS a cim:Currency ;
  rdfs:label "TJS"@en ;
  rdfs:comment "Tajikistani somoni." ;
  cims:stereotype "enum" .

cim:Currency.TMT a cim:Currency ;
  rdfs:label "TMT"@en ;
  rdfs:comment "Turkmenistani manat." ;
  cims:stereotype "enum" .

cim:Currency.TND a cim:Currency ;
  rdfs:label "TND"@en ;
  rdfs:comment "Tunisian dinar." ;
  cims:stereotype "enum" .

cim:Currency.TOP a cim:Currency ;
  rdfs:label "TOP"@en ;
  rdfs:comment "Tongan pa'anga." ;
  cims:stereotype "enum" .

cim:Currency.TRY a cim:Currency ;
  rdfs:label "TRY"@en ;
  rdfs:comment "Turkish lira." ;
  cims:stereotype "enum" .

cim:Currency.TTD a cim:Currency ;
  rdfs:label "TTD"@en ;
  rdfs:comment "Trinidad and Tobago dollar." ;
  cims:stereotype "enum" .

cim:Currency.TWD a cim:Currency ;
  rdfs:label "TWD"@en ;
  rdfs:comment "New Taiwan dollar." ;
  cims:stereotype "enum" .

cim:Currency.TZS a cim:Currency ;
  rdfs:label "TZS"@en ;
  rdfs:comment "Tanzanian shilling." ;
  cims:stereotype "enum" .

cim:Currency.UAH a cim:Currency ;
  rdfs:label "UAH"@en ;
  rdfs:comment "Ukrainian hryvnia." ;
  cims:stereotype "enum" .

cim:Currency.UGX a cim:Currency ;
  rdfs:label "UGX"@en ;
  rdfs:comment "Ugandan shilling." ;
  cims:stereotype "enum" .

cim:Currency.USD a cim:Currency ;
  rdfs:label "USD"@en ;
  rdfs:comment "United States dollar." ;
  cims:stereotype "enum" .

cim:Currency.UYU a cim:Currency ;
  rdfs:label "UYU"@en ;
  rdfs:comment "Uruguayan peso." ;
  cims:stereotype "enum" .

cim:Currency.UZS a cim:Currency ;
  rdfs:label "UZS"@en ;
  rdfs:comment "Uzbekistan som." ;
  cims:stereotype "enum" .

cim:Currency.VEF a cim:Currency ;
  rdfs:label "VEF"@en ;
  rdfs:comment "Venezuelan bolívar fuerte." ;
  cims:stereotype "enum" .

cim:Currency.VND a cim:Currency ;
  rdfs:label "VND"@en ;
  rdfs:comment "Vietnamese Dong." ;
  cims:stereotype "enum" .

cim:Currency.VUV a cim:Currency ;
  rdfs:label "VUV"@en ;
  rdfs:comment "Vanuatu vatu." ;
  cims:stereotype "enum" .

cim:Currency.WST a cim:Currency ;
  rdfs:label "WST"@en ;
  rdfs:comment "Samoan tala." ;
  cims:stereotype "enum" .

cim:Currency.XAF a cim:Currency ;
  rdfs:label "XAF"@en ;
  rdfs:comment "CFA franc BEAC." ;
  cims:stereotype "enum" .

cim:Currency.XCD a cim:Currency ;
  rdfs:label "XCD"@en ;
  rdfs:comment "East Caribbean dollar." ;
  cims:stereotype "enum" .

cim:Currency.XOF a cim:Currency ;
  rdfs:label "XOF"@en ;
  rdfs:comment "CFA Franc BCEAO." ;
  cims:stereotype "enum" .

cim:Currency.XPF a cim:Currency ;
  rdfs:label "XPF"@en ;
  rdfs:comment "CFP franc." ;
  cims:stereotype "enum" .

cim:Currency.YER a cim:Currency ;
  rdfs:label "YER"@en ;
  rdfs:comment "Yemeni rial." ;
  cims:stereotype "enum" .

cim:Currency.ZAR a cim:Currency ;
  rdfs:label "ZAR"@en ;
  rdfs:comment "South African rand." ;
  cims:stereotype "enum" .

cim:Currency.ZMK a cim:Currency ;
  rdfs:label "ZMK"@en ;
  rdfs:comment "Zambian kwacha." ;
  cims:stereotype "enum" .

cim:Currency.ZWL a cim:Currency ;
  rdfs:label "ZWL"@en ;
  rdfs:comment "Zimbabwe dollar." ;
  cims:stereotype "enum" .

cim:CurveStyle.constantYValue a cim:CurveStyle ;
  rdfs:label "constantYValue"@en ;
  rdfs:comment "The Y-axis values are assumed constant until the next curve point and prior to the first curve point." ;
  cims:stereotype "enum" .

cim:CurveStyle.straightLineYValues a cim:CurveStyle ;
  rdfs:label "straightLineYValues"@en ;
  rdfs:comment "The Y-axis values are assumed to be a straight line between values.  Also known as linear interpolation." ;
  cims:stereotype "enum" .

cim:OperationalLimitDirectionKind.absoluteValue a cim:OperationalLimitDirectionKind ;
  rdfs:label "absoluteValue"@en ;
  rdfs:comment "An absoluteValue limit means that a monitored absolute value above the limit value is a violation." ;
  cims:stereotype "enum" .

cim:OperationalLimitDirectionKind.high a cim:OperationalLimitDirectionKind ;
  rdfs:label "high"@en ;
  rdfs:comment "High means that a monitored value above the limit value is a violation.   If applied to a terminal flow, the positive direction is into the terminal." ;
  cims:stereotype "enum" .

cim:OperationalLimitDirectionKind.low a cim:OperationalLimitDirectionKind ;
  rdfs:label "low"@en ;
  rdfs:comment "Low means a monitored value below the limit is a violation.  If applied to a terminal flow, the positive direction is into the terminal." ;
  cims:stereotype "enum" .

cim:UnitMultiplier.M a cim:UnitMultiplier ;
  rdfs:label "M"@en ;
  rdfs:comment "Mega 10**6." ;
  cims:stereotype "enum" .

cim:UnitMultiplier.k a cim:UnitMultiplier ;
  rdfs:label "k"@en ;
  rdfs:comment "Kilo 10**3." ;
  cims:stereotype "enum" .

cim:UnitMultiplier.none a cim:UnitMultiplier ;
  rdfs:label "none"@en ;
  rdfs:comment "No multiplier or equivalently multiply by 1." ;
  cims:stereotype "enum" .

cim:UnitSymbol.A a cim:UnitSymbol ;
  rdfs:label "A"@en ;
  rdfs:comment "Current in amperes." ;
  cims:stereotype "enum" .

cim:UnitSymbol.Hz a cim:UnitSymbol ;
  rdfs:label "Hz"@en ;
  rdfs:comment "Frequency in hertz (1/s)." ;
  cims:stereotype "enum" .

cim:UnitSymbol.Pa a cim:UnitSymbol ;
  rdfs:label "Pa"@en ;
  rdfs:comment "Pressure in pascals (N/m²). Note: the absolute or relative measurement of pressure is implied with this entry. See below for more explicit forms." ;
  cims:stereotype "enum" .

cim:UnitSymbol.V a cim:UnitSymbol ;
  rdfs:label "V"@en ;
  rdfs:comment "Electric potential in volts (W/A)." ;
  cims:stereotype "enum" .

cim:UnitSymbol.VAr a cim:UnitSymbol ;
  rdfs:label "VAr"@en ;
  rdfs:comment """Reactive power in volt amperes reactive. The “reactive” or “imaginary” component of electrical power (VIsin(phi)). (See also real power and apparent power).
Note: Different meter designs use different methods to arrive at their results. Some meters may compute reactive power as an arithmetic value, while others compute the value vectorially. The data consumer should determine the method in use and the suitability of the measurement for the intended purpose.""" ;
  cims:stereotype "enum" .

cim:UnitSymbol.VPerVAr a cim:UnitSymbol ;
  rdfs:label "VPerVAr"@en ;
  rdfs:comment "Power factor, PF, the ratio of the active power to the apparent power. Note: The sign convention used for power factor will differ between IEC meters and EEI (ANSI) meters. It is assumed that the data consumers understand the type of meter being used and agree on the sign convention in use at any given utility." ;
  cims:stereotype "enum" .

cim:UnitSymbol.W a cim:UnitSymbol ;
  rdfs:label "W"@en ;
  rdfs:comment "Real power in watts (J/s). Electrical power may have real and reactive components. The real portion of electrical power (I&#178;R or VIcos(phi)), is expressed in Watts. See also apparent power and reactive power." ;
  cims:stereotype "enum" .

cim:UnitSymbol.WPerm2 a cim:UnitSymbol ;
  rdfs:label "WPerm2"@en ;
  rdfs:comment "Heat flux density, irradiance, watts per square metre." ;
  cims:stereotype "enum" .

cim:UnitSymbol.WPers a cim:UnitSymbol ;
  rdfs:label "WPers"@en ;
  rdfs:comment "Ramp rate in watts per second." ;
  cims:stereotype "enum" .

cim:UnitSymbol.deg a cim:UnitSymbol ;
  rdfs:label "deg"@en ;
  rdfs:comment "Plane angle in degrees." ;
  cims:stereotype "enum" .

cim:UnitSymbol.degC a cim:UnitSymbol ;
  rdfs:label "degC"@en ;
  rdfs:comment """Relative temperature in degrees Celsius.
In the SI unit system the symbol is °C. Electric charge is measured in coulomb that has the unit symbol C. To distinguish degree Celsius from coulomb the symbol used in the UML is degC. The reason for not using °C is that the special character ° is difficult to manage in software.""" ;
  cims:stereotype "enum" .

cim:UnitSymbol.none a cim:UnitSymbol ;
  rdfs:label "none"@en ;
  rdfs:comment "Dimension less quantity, e.g. count, per unit, etc." ;
  cims:stereotype "enum" .

cim:UnitSymbol.ohm a cim:UnitSymbol ;
  rdfs:label "ohm"@en ;
  rdfs:comment "Electric resistance in ohms (V/A)." ;
  cims:stereotype "enum" .

cim:UnitSymbol.s a cim:UnitSymbol ;
  rdfs:label "s"@en ;
  rdfs:comment "Time in seconds." ;
  cims:stereotype "enum" .

er:Package_DocEquipmentReliabilityProfile a cims:ClassCategory ;
  rdfs:label "DocEquipmentReliabilityProfile"@en ;
  rdfs:comment "This package contains datatypes used only in the RDFS header." .

er:Package_EquipmentReliabilityProfile a cims:ClassCategory ;
  rdfs:label "EquipmentReliabilityProfile"@en ;
  rdfs:comment "This package contains equipment reliability profile." .

nc:DCSystemDirectionKind.bidirectional a nc:DCSystemDirectionKind ;
  rdfs:label "bidirectional"@en ;
  rdfs:comment "Bidirectional DC system used for the transfer of energy in either direction. According to IEC 60633 a multiterminal DC system is bidirectional if one or more substations are bidirectional." ;
  cims:stereotype "enum" .

nc:DCSystemDirectionKind.unidirectional a nc:DCSystemDirectionKind ;
  rdfs:label "unidirectional"@en ;
  rdfs:comment "Unidirectional DC system used for the transfer of energy in only one direction. According to IEC 60633, most DC systems are inherently bidirectional. However, some systems may be optimized to transmit power in only one preferred direction. Such systems may still be considered as \"bidirectional\"." ;
  cims:stereotype "enum" .

nc:DCSystemTransmissionKind.backToBack a nc:DCSystemTransmissionKind ;
  rdfs:label "backToBack"@en ;
  rdfs:comment "DC back-to-back system (IEC 60633) is a DC system which transfers energy between AC buses at the same location." ;
  cims:stereotype "enum" .

nc:DCSystemTransmissionKind.multiTerminal a nc:DCSystemTransmissionKind ;
  rdfs:label "multiTerminal"@en ;
  rdfs:comment "Multiterminal DC transmission system (IEC 60633) consisting of more than two separated DC substations and the interconnecting DC transmission lines." ;
  cims:stereotype "enum" .

nc:DCSystemTransmissionKind.twoTerminal a nc:DCSystemTransmissionKind ;
  rdfs:label "twoTerminal"@en ;
  rdfs:comment "Two-terminal DC transmission system (IEC 60633), consisting of two DC substations and the connecting DC transmission line(s)." ;
  cims:stereotype "enum" .

nc:EnergyKind.battery a nc:EnergyKind ;
  rdfs:label "battery"@en ;
  rdfs:comment "Battery storage." ;
  cims:stereotype "enum" .

nc:EnergyKind.biomass a nc:EnergyKind ;
  rdfs:label "biomass"@en ;
  rdfs:comment "Biomass." ;
  cims:stereotype "enum" .

nc:EnergyKind.bufferConsumption a nc:EnergyKind ;
  rdfs:label "bufferConsumption"@en ;
  rdfs:comment "Flexibility in operation but bound to some buffering capability e.g. battery, electrical vehicle, cooling system, freezer." ;
  cims:stereotype "enum" .

nc:EnergyKind.fossil a nc:EnergyKind ;
  rdfs:label "fossil"@en ;
  rdfs:comment "Fossil." ;
  cims:stereotype "enum" .

nc:EnergyKind.geothermal a nc:EnergyKind ;
  rdfs:label "geothermal"@en ;
  rdfs:comment "Geothermal." ;
  cims:stereotype "enum" .

nc:EnergyKind.hydroPump a nc:EnergyKind ;
  rdfs:label "hydroPump"@en ;
  rdfs:comment "Hydro pump." ;
  cims:stereotype "enum" .

nc:EnergyKind.hydroRunOfRiver a nc:EnergyKind ;
  rdfs:label "hydroRunOfRiver"@en ;
  rdfs:comment "Hydro run of river." ;
  cims:stereotype "enum" .

nc:EnergyKind.hydroWaterReservoir a nc:EnergyKind ;
  rdfs:label "hydroWaterReservoir"@en ;
  rdfs:comment "Hydro water reservoir." ;
  cims:stereotype "enum" .

nc:EnergyKind.marine a nc:EnergyKind ;
  rdfs:label "marine"@en ;
  rdfs:comment "Marine." ;
  cims:stereotype "enum" .

nc:EnergyKind.nuclear a nc:EnergyKind ;
  rdfs:label "nuclear"@en ;
  rdfs:comment "Nuclear." ;
  cims:stereotype "enum" .

nc:EnergyKind.other a nc:EnergyKind ;
  rdfs:label "other"@en ;
  rdfs:comment "Other." ;
  cims:stereotype "enum" .

nc:EnergyKind.solar a nc:EnergyKind ;
  rdfs:label "solar"@en ;
  rdfs:comment "Solar." ;
  cims:stereotype "enum" .

nc:EnergyKind.timeShiftConsumption a nc:EnergyKind ;
  rdfs:label "timeShiftConsumption"@en ;
  rdfs:comment "Operation can be shifted in time but can have a deadline e.g. washing machine, dishwasher." ;
  cims:stereotype "enum" .

nc:EnergyKind.unconstrainedConsumption a nc:EnergyKind ;
  rdfs:label "unconstrainedConsumption"@en ;
  rdfs:comment "Consumption is not constrained by any buffer and provides full flexibility. It is difficult to measure and to provide forecast. The consumption can be provided by local production. e.g. gas generator, diesel generator wood fire, etc." ;
  cims:stereotype "enum" .

nc:EnergyKind.uncontrollableConsumption a nc:EnergyKind ;
  rdfs:label "uncontrollableConsumption"@en ;
  rdfs:comment "Consumption where there is no flexibility and it is measurable and under possibility to provide a forecast. e.g. TV, indoor lightning." ;
  cims:stereotype "enum" .

nc:EnergyKind.waste a nc:EnergyKind ;
  rdfs:label "waste"@en ;
  rdfs:comment "Waste." ;
  cims:stereotype "enum" .

nc:EnergyKind.wind a nc:EnergyKind ;
  rdfs:label "wind"@en ;
  rdfs:comment "Wind." ;
  cims:stereotype "enum" .

nc:GeothermalUnitKind.binaryCycle a nc:GeothermalUnitKind ;
  rdfs:label "binaryCycle"@en ;
  rdfs:comment "The moderately hot geothermal water is passed by a secondary fluid with a much lower boiling point than water. " ;
  cims:stereotype "enum" .

nc:GeothermalUnitKind.drySteam a nc:GeothermalUnitKind ;
  rdfs:label "drySteam"@en ;
  rdfs:comment "Uses geothermal steam of 150 degree Celsius or greater to turn turbines." ;
  cims:stereotype "enum" .

nc:GeothermalUnitKind.flashSteam a nc:GeothermalUnitKind ;
  rdfs:label "flashSteam"@en ;
  rdfs:comment "Pull deep, high-pressure hot water into lower-pressure tanks and use the resulting flashed steam to drive turbines." ;
  cims:stereotype "enum" .

nc:GeothermalUnitKind.other a nc:GeothermalUnitKind ;
  rdfs:label "other"@en ;
  rdfs:comment "Other type of geothermal generating unit." ;
  cims:stereotype "enum" .

nc:LogicalOperatorsKind.equals a nc:LogicalOperatorsKind ;
  rdfs:label "equals"@en ;
  rdfs:comment "Equals (like) comparison operation." ;
  cims:stereotype "enum" .

nc:LogicalOperatorsKind.greaterThan a nc:LogicalOperatorsKind ;
  rdfs:label "greaterThan"@en ;
  rdfs:comment "Greater than comparison operation." ;
  cims:stereotype "enum" .

nc:LogicalOperatorsKind.greaterThanOrEquals a nc:LogicalOperatorsKind ;
  rdfs:label "greaterThanOrEquals"@en ;
  rdfs:comment "Greater than or equals comparison operation." ;
  cims:stereotype "enum" .

nc:LogicalOperatorsKind.lessThan a nc:LogicalOperatorsKind ;
  rdfs:label "lessThan"@en ;
  rdfs:comment "Less than comparison operation." ;
  cims:stereotype "enum" .

nc:LogicalOperatorsKind.lessThanOrEquals a nc:LogicalOperatorsKind ;
  rdfs:label "lessThanOrEquals"@en ;
  rdfs:comment "Less than or equals comparison operation." ;
  cims:stereotype "enum" .

nc:LogicalOperatorsKind.notEqual a nc:LogicalOperatorsKind ;
  rdfs:label "notEqual"@en ;
  rdfs:comment "Not equal (unlike) comparison operation." ;
  cims:stereotype "enum" .

nc:MarineUnitKind.currents a nc:MarineUnitKind ;
  rdfs:label "currents"@en ;
  rdfs:comment "Capture energy from ocean current which are caused by forces like breaking waves, wind, coriolis effect etc." ;
  cims:stereotype "enum" .

nc:MarineUnitKind.other a nc:MarineUnitKind ;
  rdfs:label "other"@en ;
  rdfs:comment "Other way of capture energy from marine elements." ;
  cims:stereotype "enum" .

nc:MarineUnitKind.pressure a nc:MarineUnitKind ;
  rdfs:label "pressure"@en ;
  rdfs:comment "Capture energy from pressure." ;
  cims:stereotype "enum" .

nc:MarineUnitKind.tidal a nc:MarineUnitKind ;
  rdfs:label "tidal"@en ;
  rdfs:comment "Capture energy from tidal power, which captures the energy of the current caused by the gravitational pull of the Sun and Moon." ;
  cims:stereotype "enum" .

nc:MarineUnitKind.wave a nc:MarineUnitKind ;
  rdfs:label "wave"@en ;
  rdfs:comment "Capture energy from wind waves." ;
  cims:stereotype "enum" .

nc:NuclearReactorKind.breeder a nc:NuclearReactorKind ;
  rdfs:label "breeder"@en ;
  rdfs:comment "Reactor whose heat source is a nuclear reactor that generates more fissile material than it consumes." ;
  cims:stereotype "enum" .

nc:NuclearReactorKind.graphite a nc:NuclearReactorKind ;
  rdfs:label "graphite"@en ;
  rdfs:comment "Reactor whose heat source is a graphite-moderated reactor that is a nuclear reactor that uses carbon as a neutron moderator, which allows natural uranium to be used as nuclear fuel." ;
  cims:stereotype "enum" .

nc:NuclearReactorKind.heavyWater a nc:NuclearReactorKind ;
  rdfs:label "heavyWater"@en ;
  rdfs:comment "Reactor whose heat source is a pressurized heavy-water reactor (PHWR) that uses heavy water (deuterium oxide D2O) as its coolant and neutron moderator." ;
  cims:stereotype "enum" .

nc:NuclearReactorKind.lightWater a nc:NuclearReactorKind ;
  rdfs:label "lightWater"@en ;
  rdfs:comment "Reactor whose heat source is a light-water reactor (LWR) that is a type of thermal-neutron reactor that uses normal water, as both its coolant and neutron moderator – furthermore a solid form of fissile elements is used as fuel. " ;
  cims:stereotype "enum" .

nc:NuclearReactorKind.liquidMetal a nc:NuclearReactorKind ;
  rdfs:label "liquidMetal"@en ;
  rdfs:comment "Reactor whose liquid metal cooled nuclear reactor, liquid metal fast reactor or LMFR is an advanced type of nuclear reactor where the primary coolant is a liquid metal." ;
  cims:stereotype "enum" .

nc:NuclearReactorKind.other a nc:NuclearReactorKind ;
  rdfs:label "other"@en ;
  rdfs:comment "Other type of nuclear reactors." ;
  cims:stereotype "enum" .

nc:PinTerminalKind.activePower a nc:PinTerminalKind ;
  rdfs:label "activePower"@en ;
  rdfs:comment "Active power on the Terminal." ;
  cims:stereotype "enum" .

nc:PinTerminalKind.apparentPower a nc:PinTerminalKind ;
  rdfs:label "apparentPower"@en ;
  rdfs:comment "Apparent power on the Terminal." ;
  cims:stereotype "enum" .

nc:PinTerminalKind.current a nc:PinTerminalKind ;
  rdfs:label "current"@en ;
  rdfs:comment "Current on the Terminal." ;
  cims:stereotype "enum" .

nc:PinTerminalKind.reactivePower a nc:PinTerminalKind ;
  rdfs:label "reactivePower"@en ;
  rdfs:comment "Reactive power on the Terminal." ;
  cims:stereotype "enum" .

nc:PinTerminalKind.voltageAngle a nc:PinTerminalKind ;
  rdfs:label "voltageAngle"@en ;
  rdfs:comment "Voltage angle on the Terminal." ;
  cims:stereotype "enum" .

nc:PinTerminalKind.voltageMagnitude a nc:PinTerminalKind ;
  rdfs:label "voltageMagnitude"@en ;
  rdfs:comment "Voltage magnitude on the Terminal." ;
  cims:stereotype "enum" .

nc:PowerBlockKind.powerDecrease a nc:PowerBlockKind ;
  rdfs:label "powerDecrease"@en ;
  rdfs:comment "Decrease in the power. The block represents action for decreased power." ;
  cims:stereotype "enum" .

nc:PowerBlockKind.powerIncrease a nc:PowerBlockKind ;
  rdfs:label "powerIncrease"@en ;
  rdfs:comment "Increase in the power. The block represents action for increased power." ;
  cims:stereotype "enum" .

nc:PowerBlockKind.powerIncreaseAndDecrease a nc:PowerBlockKind ;
  rdfs:label "powerIncreaseAndDecrease"@en ;
  rdfs:comment "Increase and decrease in the power. The block represents action for increased and decreased power." ;
  cims:stereotype "enum" .

nc:PowerElectricalChemicalUnitKind.electrolyticCell a nc:PowerElectricalChemicalUnitKind ;
  rdfs:label "electrolyticCell"@en ;
  rdfs:comment "An electrolytic cell is an electrochemical cell that drives a non-spontaneous redox reaction through the application of electrical energy. Example are the decomposition of water into hydrogen and oxygen. " ;
  cims:stereotype "enum" .

nc:PowerElectricalChemicalUnitKind.fuelCell a nc:PowerElectricalChemicalUnitKind ;
  rdfs:label "fuelCell"@en ;
  rdfs:comment "A fuel cell is an electrochemical cell that converts the chemical energy from a fuel into electricity through an electrochemical reaction of hydrogen fuel with oxygen or another oxidizing agent." ;
  cims:stereotype "enum" .

nc:PowerElectricalChemicalUnitKind.other a nc:PowerElectricalChemicalUnitKind ;
  rdfs:label "other"@en ;
  rdfs:comment "Other type of cell used in chemical reactions." ;
  cims:stereotype "enum" .

nc:PowerFrequencyControlKind.activePower a nc:PowerFrequencyControlKind ;
  rdfs:label "activePower"@en ;
  rdfs:comment "Active power control mode." ;
  cims:stereotype "enum" .

nc:PowerFrequencyControlKind.activePowerAndFrequency a nc:PowerFrequencyControlKind ;
  rdfs:label "activePowerAndFrequency"@en ;
  rdfs:comment "Active power and frequency control mode." ;
  cims:stereotype "enum" .

nc:PowerFrequencyControlKind.frequency a nc:PowerFrequencyControlKind ;
  rdfs:label "frequency"@en ;
  rdfs:comment "Frequency control mode." ;
  cims:stereotype "enum" .

nc:PowerShiftKeyKind.consumptionsFlat a nc:PowerShiftKeyKind ;
  rdfs:label "consumptionsFlat"@en ;
  rdfs:comment "Flat adjustment, equal amount of power, on all active consumption units (Energy Consumers and Power Electronics like FlexibleEnergyUnit). e.g. 100 MW decrease adjustment on 4 loads, it means that each of them get reduced 25 MW, as long as no other constraints are violated." ;
  cims:stereotype "enum" .

nc:PowerShiftKeyKind.consumptionsP a nc:PowerShiftKeyKind ;
  rdfs:label "consumptionsP"@en ;
  rdfs:comment "The distribution is based on the consumptions active power in the given case." ;
  cims:stereotype "enum" .

nc:PowerShiftKeyKind.explicitDistribution a nc:PowerShiftKeyKind ;
  rdfs:label "explicitDistribution"@en ;
  rdfs:comment "The distribution is explicitly done according to the power shift key  distribution in the power bid Schedule." ;
  cims:stereotype "enum" .

nc:PowerShiftKeyKind.explicitInstruction a nc:PowerShiftKeyKind ;
  rdfs:label "explicitInstruction"@en ;
  rdfs:comment "The distribution is done according to the individual participation factor on the unit." ;
  cims:stereotype "enum" .

nc:PowerShiftKeyKind.generatorsAndConsumptionsP a nc:PowerShiftKeyKind ;
  rdfs:label "generatorsAndConsumptionsP"@en ;
  rdfs:comment "The distribution is based on the generator and consumption active power in the given case." ;
  cims:stereotype "enum" .

nc:PowerShiftKeyKind.generatorsFlat a nc:PowerShiftKeyKind ;
  rdfs:label "generatorsFlat"@en ;
  rdfs:comment "Flat adjustment, equal amount of power, on all active generators. e.g. 100 MW increase adjustment on 4 generators, it means that each of them get increased 25 MW, as long as no other constraints are violated." ;
  cims:stereotype "enum" .

nc:PowerShiftKeyKind.generatorsP a nc:PowerShiftKeyKind ;
  rdfs:label "generatorsP"@en ;
  rdfs:comment "The distribution is based on the generators active power in the given case." ;
  cims:stereotype "enum" .

nc:PowerShiftKeyKind.generatorsPmax a nc:PowerShiftKeyKind ;
  rdfs:label "generatorsPmax"@en ;
  rdfs:comment "The distribution is relative to the maximum p of the generator." ;
  cims:stereotype "enum" .

nc:PowerShiftKeyKind.generatorsPmin a nc:PowerShiftKeyKind ;
  rdfs:label "generatorsPmin"@en ;
  rdfs:comment "The distribution is relative to the minimum p of the generator." ;
  cims:stereotype "enum" .

nc:PowerShiftKeyKind.generatorsRemainingCapacity a nc:PowerShiftKeyKind ;
  rdfs:label "generatorsRemainingCapacity"@en ;
  rdfs:comment "The distribution is based on the remaining capacity for generators in the given case." ;
  cims:stereotype "enum" .

nc:PowerShiftKeyKind.generatorsUsedCapacity a nc:PowerShiftKeyKind ;
  rdfs:label "generatorsUsedCapacity"@en ;
  rdfs:comment "The distribution is based on the used capacity, the difference between the minimum operation and operating p (GeneratingUnit.minOperatingP)" ;
  cims:stereotype "enum" .

nc:PowerShiftKeyKind.nonConformLoadP a nc:PowerShiftKeyKind ;
  rdfs:label "nonConformLoadP"@en ;
  rdfs:comment "The distribution is based on the non conform load active power in the given case." ;
  cims:stereotype "enum" .

nc:PowerShiftKeyKind.storageFlat a nc:PowerShiftKeyKind ;
  rdfs:label "storageFlat"@en ;
  rdfs:comment "Flat adjustment, equal amount of power, on all the batteries and any operating hydro pumps. e.g. 100 MW increase or decrease adjustment on 4 batteries, it means that each of them get increased or reduced 25 MW, as long as no other constraints are violated." ;
  cims:stereotype "enum" .

nc:PowerShiftKeyKind.storageP a nc:PowerShiftKeyKind ;
  rdfs:label "storageP"@en ;
  rdfs:comment "The distribution is based on the batteries and any operating hydro pumps active power in the given case." ;
  cims:stereotype "enum" .

nc:RampingPrincipleKind.continuous a nc:RampingPrincipleKind ;
  rdfs:label "continuous"@en ;
  rdfs:comment "Continuous ramping principle is applied between two scheduled time point. For instance, from 10 MW to 70 MW over one hour the change is 1 MW/min." ;
  cims:stereotype "enum" .

nc:RampingPrincipleKind.fifteenMinutes a nc:RampingPrincipleKind ;
  rdfs:label "fifteenMinutes"@en ;
  rdfs:comment "Fifteen minutes ramping principle. Ramping starts 15 minutes before the schedule time point and ends 15 minutes after. For instance, if the schedule time point is 19:30h it starts at 19:15h and ends at 19:45h. " ;
  cims:stereotype "enum" .

nc:RampingPrincipleKind.fiveMinutes a nc:RampingPrincipleKind ;
  rdfs:label "fiveMinutes"@en ;
  rdfs:comment "Five minutes ramping principle. Ramping starts five minutes before the schedule time point and ends five minutes after. For instance, if the schedule time point is 19:30h it starts at 19:25h and ends at 19:35h. " ;
  cims:stereotype "enum" .

nc:RampingPrincipleKind.maxContinuous a nc:RampingPrincipleKind ;
  rdfs:label "maxContinuous"@en ;
  rdfs:comment "Maximum continuous ramping principle. The schedule is kept as long as possible and the maximum ramping rate is used to get from one point to another, symmetrically around the schedule time points. For example, there is 40 MW change in the schedule the maximum ramp rate is 20 MW/min the ramping starts 1 min before (e.g. 19:29h) and finishes 1 min after (e.g. 19:31h).  " ;
  cims:stereotype "enum" .

nc:RampingPrincipleKind.tenMinutes a nc:RampingPrincipleKind ;
  rdfs:label "tenMinutes"@en ;
  rdfs:comment "Ten minutes ramping principle. Ramping starts 10 minutes before the schedule time point and ends 10 minutes after. For instance, if the schedule time point is 19:30h it starts at 19:20h and ends at 19:40h. " ;
  cims:stereotype "enum" .

nc:ShiftMethodKind.priority a nc:ShiftMethodKind ;
  rdfs:label "priority"@en ;
  rdfs:comment "Power schedule shift (distribution) is done by a shared fraction prioritizing the unit e.g. A two unit with the participation factor 60 and 40 will distribute a 10 MW increased schedule by first filling the highest participation factor (priority) until max economy power or maximum power allowed by the unit before it starts filling the next on the list. e.g. The unit with 60 will be getting its maximum shared first. The same logic applies with reducing the schedule. e.g. The 60 participation factor unit will be reduced to its min economy factor or minimum power." ;
  cims:stereotype "enum" .

nc:ShiftMethodKind.shared a nc:ShiftMethodKind ;
  rdfs:label "shared"@en ;
  rdfs:comment "Power schedule shift (distribution) is done by a shared fraction e.g. A two unit with the participation factor 60 and 40 will distribute a 10 MW schedule by 6 and 4 MW." ;
  cims:stereotype "enum" .


