@prefix cim    : <https://cim.ucaiug.io/ns#> .
@prefix nc     : <https://cim4.eu/ns/nc#> .
@prefix cims   : <http://iec.ch/TC57/1999/rdf-schema-extensions-19990926#> .
@prefix profcim: <https://cim.ucaiug.io/ns/prof-cim#> .
@prefix sis    : <https://ap-voc.cim4.eu/StateInstructionSchedule#> .
@prefix dcat   : <http://www.w3.org/ns/dcat#> .
@prefix dcterms: <http://purl.org/dc/terms/#> .
@prefix owl    : <http://www.w3.org/2002/07/owl#> .
@prefix rdf    : <http://www.w3.org/1999/02/22-rdf-syntax-ns#> .
@prefix rdfs   : <http://www.w3.org/2000/01/rdf-schema#> .

cim:ActivePower a rdfs:Class ;
  rdfs:label "ActivePower"@en ;
  rdfs:comment "Product of RMS value of the voltage and the RMS value of the in-phase component of the current." ;
  cims:belongsToCategory sis:Package_StateInstructionScheduleProfile ;
  cims:stereotype "CIMDatatype" .

cim:AngleDegrees a rdfs:Class ;
  rdfs:label "AngleDegrees"@en ;
  rdfs:comment "Measurement of angle in degrees." ;
  cims:belongsToCategory sis:Package_StateInstructionScheduleProfile ;
  cims:stereotype "CIMDatatype" .

cim:Boolean a rdfs:Class ;
  rdfs:label "Boolean"@en ;
  rdfs:comment "A type with the value space \"true\" and \"false\"." ;
  cims:belongsToCategory sis:Package_StateInstructionScheduleProfile ;
  cims:stereotype "Primitive" .

cim:ConductingEquipment a rdfs:Class ;
  rdfs:label "ConductingEquipment"@en ;
  rdfs:comment "The parts of the AC power system that are designed to carry current or that are conductively connected through terminals." ;
  cims:belongsToCategory sis:Package_StateInstructionScheduleProfile ;
  rdfs:subClassOf cim:Equipment .

cim:Contingency a rdfs:Class ;
  rdfs:label "Contingency"@en ;
  rdfs:comment "An event threatening system reliability, consisting of one or more contingency elements." ;
  cims:belongsToCategory sis:Package_StateInstructionScheduleProfile .

cim:Currency a rdfs:Class ;
  rdfs:label "Currency"@en ;
  rdfs:comment "Monetary currencies.  ISO 4217 standard including 3-character currency code." ;
  cims:belongsToCategory sis:Package_StateInstructionScheduleProfile ;
  cims:stereotype <http://iec.ch/TC57/NonStandard/UML#enumeration> .

cim:CurrentFlow a rdfs:Class ;
  rdfs:label "CurrentFlow"@en ;
  rdfs:comment "Electrical current with sign convention: positive flow is out of the conducting equipment into the connectivity node. Can be both AC and DC." ;
  cims:belongsToCategory sis:Package_StateInstructionScheduleProfile ;
  cims:stereotype "CIMDatatype" .

cim:Date a rdfs:Class ;
  rdfs:label "Date"@en ;
  rdfs:comment "Date as \"yyyy-mm-dd\", which conforms with ISO 8601. UTC time zone is specified as \"yyyy-mm-ddZ\". A local timezone relative UTC is specified as \"yyyy-mm-dd(+/-)hh:mm\"." ;
  cims:belongsToCategory sis:Package_DocStateInstructionScheduleProfile ;
  cims:stereotype "Primitive" .

cim:DateTime a rdfs:Class ;
  rdfs:label "DateTime"@en ;
  rdfs:comment "Date and time as \"yyyy-mm-ddThh:mm:ss.sss\", which conforms with ISO 8601. UTC time zone is specified as \"yyyy-mm-ddThh:mm:ss.sssZ\". A local timezone relative UTC is specified as \"yyyy-mm-ddThh:mm:ss.sss-hh:mm\". The second component (shown here as \"ss.sss\") could have any number of digits in its fractional part to allow any kind of precision beyond seconds." ;
  cims:belongsToCategory sis:Package_StateInstructionScheduleProfile ;
  cims:stereotype "Primitive" .

cim:Decimal a rdfs:Class ;
  rdfs:label "Decimal"@en ;
  rdfs:comment "Decimal is the base-10 notational system for representing real numbers." ;
  cims:belongsToCategory sis:Package_StateInstructionScheduleProfile ;
  cims:stereotype "Primitive" .

cim:Duration a rdfs:Class ;
  rdfs:label "Duration"@en ;
  rdfs:comment "Duration as \"PnYnMnDTnHnMnS\" which conforms to ISO 8601, where nY expresses a number of years, nM a number of months, nD a number of days. The letter T separates the date expression from the time expression and, after it, nH identifies a number of hours, nM a number of minutes and nS a number of seconds. The number of seconds could be expressed as a decimal number, but all other numbers are integers." ;
  cims:belongsToCategory sis:Package_StateInstructionScheduleProfile ;
  cims:stereotype "Primitive" .

cim:EnergyConnection a rdfs:Class ;
  rdfs:label "EnergyConnection"@en ;
  rdfs:comment "A connection of energy generation or consumption on the power system model." ;
  cims:belongsToCategory sis:Package_StateInstructionScheduleProfile ;
  rdfs:subClassOf cim:ConductingEquipment .

cim:EnergyConsumer a rdfs:Class ;
  rdfs:label "EnergyConsumer"@en ;
  rdfs:comment """Generic user of energy - a  point of consumption on the power system model.
EnergyConsumer.pfixed, .qfixed, .pfixedPct and .qfixedPct have meaning only if there is no LoadResponseCharacteristic associated with EnergyConsumer or if LoadResponseCharacteristic.exponentModel is set to False.""" ;
  cims:belongsToCategory sis:Package_StateInstructionScheduleProfile .

cim:EnergySource a rdfs:Class ;
  rdfs:label "EnergySource"@en ;
  rdfs:comment "A generic equivalent for an energy supplier on a transmission or distribution voltage level." ;
  cims:belongsToCategory sis:Package_StateInstructionScheduleProfile .

cim:Equipment a rdfs:Class ;
  rdfs:label "Equipment"@en ;
  rdfs:comment "The parts of a power system that are physical devices, electronic or mechanical." ;
  cims:belongsToCategory sis:Package_StateInstructionScheduleProfile ;
  rdfs:subClassOf cim:PowerSystemResource .

cim:EquivalentInjection a rdfs:Class ;
  rdfs:label "EquivalentInjection"@en ;
  rdfs:comment "This class represents equivalent injections (generation or load).  Voltage regulation is allowed only at the point of connection." ;
  cims:belongsToCategory sis:Package_StateInstructionScheduleProfile .

cim:ExternalNetworkInjection a rdfs:Class ;
  rdfs:label "ExternalNetworkInjection"@en ;
  rdfs:comment "This class represents the external network and it is used for IEC 60909 calculations." ;
  cims:belongsToCategory sis:Package_StateInstructionScheduleProfile .

cim:Float a rdfs:Class ;
  rdfs:label "Float"@en ;
  rdfs:comment "A floating point number. The range is unspecified and not limited." ;
  cims:belongsToCategory sis:Package_StateInstructionScheduleProfile ;
  cims:stereotype "Primitive" .

cim:GeneratingUnit a rdfs:Class ;
  rdfs:label "GeneratingUnit"@en ;
  rdfs:comment "A single or set of synchronous machines for converting mechanical power into alternating-current power. For example, individual machines within a set may be defined for scheduling purposes while a single control signal is derived for the set. In this case there would be a GeneratingUnit for each member of the set and an additional GeneratingUnit corresponding to the set." ;
  cims:belongsToCategory sis:Package_StateInstructionScheduleProfile .

cim:HydroPump a rdfs:Class ;
  rdfs:label "HydroPump"@en ;
  rdfs:comment "A synchronous motor-driven pump, typically associated with a pumped storage plant." ;
  cims:belongsToCategory sis:Package_StateInstructionScheduleProfile .

cim:IdentifiedObject a rdfs:Class ;
  rdfs:label "IdentifiedObject"@en ;
  rdfs:comment "This is a root class to provide common identification for all classes needing identification and naming attributes." ;
  cims:belongsToCategory sis:Package_StateInstructionScheduleProfile .

cim:Integer a rdfs:Class ;
  rdfs:label "Integer"@en ;
  rdfs:comment "An integer number. The range is unspecified and not limited." ;
  cims:belongsToCategory sis:Package_StateInstructionScheduleProfile ;
  cims:stereotype "Primitive" .

cim:Money a rdfs:Class ;
  rdfs:label "Money"@en ;
  rdfs:comment "Amount of money." ;
  cims:belongsToCategory sis:Package_StateInstructionScheduleProfile ;
  cims:stereotype "CIMDatatype" .

cim:MonthDay a rdfs:Class ;
  rdfs:label "MonthDay"@en ;
  rdfs:comment "MonthDay format as \"--mm-dd\", which conforms with XSD data type gMonthDay." ;
  cims:belongsToCategory sis:Package_StateInstructionScheduleProfile ;
  cims:stereotype "Primitive" .

cim:PerCent a rdfs:Class ;
  rdfs:label "PerCent"@en ;
  rdfs:comment "Percentage on a defined base.   For example, specify as 100 to indicate at the defined base." ;
  cims:belongsToCategory sis:Package_StateInstructionScheduleProfile ;
  cims:stereotype "CIMDatatype" .

cim:PowerElectronicsUnit a rdfs:Class ;
  rdfs:label "PowerElectronicsUnit"@en ;
  rdfs:comment "A generating unit or battery or aggregation that connects to the AC network using power electronics rather than rotating machines." ;
  cims:belongsToCategory sis:Package_StateInstructionScheduleProfile .

cim:PowerSystemResource a rdfs:Class ;
  rdfs:label "PowerSystemResource"@en ;
  rdfs:comment "A power system resource (PSR) can be an item of equipment such as a switch, an equipment container containing many individual items of equipment such as a substation, or an organisational entity such as sub-control area. Power system resources can have measurements associated." ;
  cims:belongsToCategory sis:Package_StateInstructionScheduleProfile ;
  rdfs:subClassOf cim:IdentifiedObject .

cim:RealEnergy a rdfs:Class ;
  rdfs:label "RealEnergy"@en ;
  rdfs:comment "Real electrical energy." ;
  cims:belongsToCategory sis:Package_StateInstructionScheduleProfile ;
  cims:stereotype "CIMDatatype" .

cim:Season a rdfs:Class ;
  rdfs:label "Season"@en ;
  rdfs:comment "A specified time period of the year." ;
  cims:belongsToCategory sis:Package_StateInstructionScheduleProfile ;
  cims:stereotype <http://iec.ch/TC57/NonStandard/UML#concrete> ;
  rdfs:subClassOf cim:IdentifiedObject .

cim:Seconds a rdfs:Class ;
  rdfs:label "Seconds"@en ;
  rdfs:comment "Time, in seconds." ;
  cims:belongsToCategory sis:Package_StateInstructionScheduleProfile ;
  cims:stereotype "CIMDatatype" .

cim:String a rdfs:Class ;
  rdfs:label "String"@en ;
  rdfs:comment "A string consisting of a sequence of characters. The character encoding is UTF-8. The string length is unspecified and unlimited." ;
  cims:belongsToCategory sis:Package_StateInstructionScheduleProfile ;
  cims:stereotype "Primitive" .

cim:Time a rdfs:Class ;
  rdfs:label "Time"@en ;
  rdfs:comment "Time as \"hh:mm:ss.sss\", which conforms with ISO 8601. UTC time zone is specified as \"hh:mm:ss.sssZ\". A local timezone relative UTC is specified as \"hh:mm:ss.sss±hh:mm\". The second component (shown here as \"ss.sss\") could have any number of digits in its fractional part to allow any kind of precision beyond seconds." ;
  cims:belongsToCategory sis:Package_StateInstructionScheduleProfile ;
  cims:stereotype "Primitive" .

cim:UnitMultiplier a rdfs:Class ;
  rdfs:label "UnitMultiplier"@en ;
  rdfs:comment """The unit multipliers defined for the CIM.  When applied to unit symbols, the unit symbol is treated as a derived unit. Regardless of the contents of the unit symbol text, the unit symbol shall be treated as if it were a single-character unit symbol. Unit symbols should not contain multipliers, and it should be left to the multiplier to define the multiple for an entire data type. 

For example, if a unit symbol is "m2Pers" and the multiplier is "k", then the value is k(m**2/s), and the multiplier applies to the entire final value, not to any individual part of the value. This can be conceptualized by substituting a derived unit symbol for the unit type. If one imagines that the symbol "Þ" represents the derived unit "m2Pers", then applying the multiplier "k" can be conceptualized simply as "kÞ".

For example, the SI unit for mass is "kg" and not "g".  If the unit symbol is defined as "kg", then the multiplier is applied to "kg" as a whole and does not replace the "k" in front of the "g". In this case, the multiplier of "m" would be used with the unit symbol of "kg" to represent one gram.  As a text string, this violates the instructions in IEC 80000-1. However, because the unit symbol in CIM is treated as a derived unit instead of as an SI unit, it makes more sense to conceptualize the "kg" as if it were replaced by one of the proposed replacements for the SI mass symbol. If one imagines that the "kg" were replaced by a symbol "Þ", then it is easier to conceptualize the multiplier "m" as creating the proper unit "mÞ", and not the forbidden unit "mkg".""" ;
  cims:belongsToCategory sis:Package_StateInstructionScheduleProfile ;
  cims:stereotype <http://iec.ch/TC57/NonStandard/UML#enumeration> .

cim:UnitSymbol a rdfs:Class ;
  rdfs:label "UnitSymbol"@en ;
  rdfs:comment """The derived units defined for usage in the CIM. In some cases, the derived unit is equal to an SI unit. Whenever possible, the standard derived symbol is used instead of the formula for the derived unit. For example, the unit symbol Farad is defined as "F" instead of "CPerV". In cases where a standard symbol does not exist for a derived unit, the formula for the unit is used as the unit symbol. For example, density does not have a standard symbol and so it is represented as "kgPerm3". With the exception of the "kg", which is an SI unit, the unit symbols do not contain multipliers and therefore represent the base derived unit to which a multiplier can be applied as a whole. 
Every unit symbol is treated as an unparseable text as if it were a single-letter symbol. The meaning of each unit symbol is defined by the accompanying descriptive text and not by the text contents of the unit symbol.
To allow the widest possible range of serializations without requiring special character handling, several substitutions are made which deviate from the format described in IEC 80000-1. The division symbol "/" is replaced by the letters "Per". Exponents are written in plain text after the unit as "m3" instead of being formatted as "m" with a superscript of 3  or introducing a symbol as in "m^3". The degree symbol "°" is replaced with the letters "deg". Any clarification of the meaning for a substitution is included in the description for the unit symbol.
Non-SI units are included in list of unit symbols to allow sources of data to be correctly labelled with their non-SI units (for example, a GPS sensor that is reporting numbers that represent feet instead of meters). This allows software to use the unit symbol information correctly convert and scale the raw data of those sources into SI-based units. 
The integer values are used for harmonization with IEC 61850.""" ;
  cims:belongsToCategory sis:Package_StateInstructionScheduleProfile ;
  cims:stereotype <http://iec.ch/TC57/NonStandard/UML#enumeration> .

nc:AssessedElement a rdfs:Class ;
  rdfs:label "AssessedElement"@en ;
  rdfs:comment """Assessed element is a network element for which the electrical state is evaluated in the regional or cross-regional process and which value is expected to fulfil regional rules function of the operational security limits.
The measurements and limits are as defined in the steady state hypothesis.""" ;
  cims:belongsToCategory sis:Package_StateInstructionScheduleProfile ;
  cims:stereotype "NC" ;
  rdfs:subClassOf cim:IdentifiedObject .

nc:AssessedElementRegularSchedule a rdfs:Class ;
  rdfs:label "AssessedElementRegularSchedule"@en ;
  rdfs:comment "Regular schedule for assessed element." ;
  cims:belongsToCategory sis:Package_StateInstructionScheduleProfile ;
  cims:stereotype "NC", <http://iec.ch/TC57/NonStandard/UML#concrete> ;
  rdfs:subClassOf nc:BaseRegularIntervalSchedule .

nc:AssessedElementRegularTimePoint a rdfs:Class ;
  rdfs:label "AssessedElementRegularTimePoint"@en ;
  rdfs:comment "Assessed element instruction value at a given point in time." ;
  cims:belongsToCategory sis:Package_StateInstructionScheduleProfile ;
  cims:stereotype "NC", <http://iec.ch/TC57/NonStandard/UML#concrete> .

nc:AssessedElementSchedule a rdfs:Class ;
  rdfs:label "AssessedElementSchedule"@en ;
  rdfs:comment "Schedule for assessed element." ;
  cims:belongsToCategory sis:Package_StateInstructionScheduleProfile ;
  cims:stereotype "NC", <http://iec.ch/TC57/NonStandard/UML#concrete> ;
  rdfs:subClassOf nc:BaseIrregularTimeSeries .

nc:AssessedElementTimePoint a rdfs:Class ;
  rdfs:label "AssessedElementTimePoint"@en ;
  rdfs:comment "Assessed element instruction value at a given point in time." ;
  cims:belongsToCategory sis:Package_StateInstructionScheduleProfile ;
  cims:stereotype "NC", <http://iec.ch/TC57/NonStandard/UML#concrete> .

nc:AssessedElementWithContingency a rdfs:Class ;
  rdfs:label "AssessedElementWithContingency"@en ;
  rdfs:comment "Combination of an assessed element and a contingency." ;
  cims:belongsToCategory sis:Package_StateInstructionScheduleProfile ;
  cims:stereotype "NC" .

nc:AssessedElementWithRemedialAction a rdfs:Class ;
  rdfs:label "AssessedElementWithRemedialAction"@en ;
  rdfs:comment "Combination of an assessed element and a remedial action" ;
  cims:belongsToCategory sis:Package_StateInstructionScheduleProfile ;
  cims:stereotype "NC" .

nc:AutomationFunction a rdfs:Class ;
  rdfs:label "AutomationFunction"@en ;
  rdfs:comment "Automation function is a collection of functional block or other automation function that can be executed as a work cycle program as part of an automated system." ;
  cims:belongsToCategory sis:Package_StateInstructionScheduleProfile ;
  cims:stereotype "NC" .

nc:AvailabilityTimePoint a rdfs:Class ;
  rdfs:label "AvailabilityTimePoint"@en ;
  rdfs:comment "Availability instruction value at a given point in time." ;
  cims:belongsToCategory sis:Package_StateInstructionScheduleProfile ;
  cims:stereotype "NC", <http://iec.ch/TC57/NonStandard/UML#concrete> .

nc:BaseIrregularTimeSeries a rdfs:Class ;
  rdfs:label "BaseIrregularTimeSeries"@en ;
  rdfs:comment "Time series that has irregular points in time." ;
  cims:belongsToCategory sis:Package_StateInstructionScheduleProfile ;
  cims:stereotype "NC" ;
  rdfs:subClassOf nc:BaseTimeSeries .

nc:BaseRegularIntervalSchedule a rdfs:Class ;
  rdfs:label "BaseRegularIntervalSchedule"@en ;
  rdfs:comment "Time series that has regular points in time." ;
  cims:belongsToCategory sis:Package_StateInstructionScheduleProfile ;
  cims:stereotype "NC" ;
  rdfs:subClassOf nc:BaseTimeSeries .

nc:BaseTimeSeries a rdfs:Class ;
  rdfs:label "BaseTimeSeries"@en ;
  rdfs:comment "Time series of values at points in time." ;
  cims:belongsToCategory sis:Package_StateInstructionScheduleProfile ;
  cims:stereotype "NC" ;
  rdfs:subClassOf cim:IdentifiedObject .

nc:BaseTimeSeriesKind a rdfs:Class ;
  rdfs:label "BaseTimeSeriesKind"@en ;
  rdfs:comment "Kind of time series. " ;
  cims:belongsToCategory sis:Package_StateInstructionScheduleProfile ;
  cims:stereotype "NC", <http://iec.ch/TC57/NonStandard/UML#enumeration> .

nc:BidDirectionKind a rdfs:Class ;
  rdfs:label "BidDirectionKind"@en ;
  rdfs:comment "Kind of direction of the bid." ;
  cims:belongsToCategory sis:Package_StateInstructionScheduleProfile ;
  cims:stereotype "NC", <http://iec.ch/TC57/NonStandard/UML#enumeration> .

nc:ContingencySchedule a rdfs:Class ;
  rdfs:label "ContingencySchedule"@en ;
  rdfs:comment "The schedule for Contingency." ;
  cims:belongsToCategory sis:Package_StateInstructionScheduleProfile ;
  cims:stereotype "NC", <http://iec.ch/TC57/NonStandard/UML#concrete> ;
  rdfs:subClassOf nc:BaseIrregularTimeSeries .

nc:ContingencyTimePoint a rdfs:Class ;
  rdfs:label "ContingencyTimePoint"@en ;
  rdfs:comment "Contingency instruction value at a given point in time." ;
  cims:belongsToCategory sis:Package_StateInstructionScheduleProfile ;
  cims:stereotype "NC", <http://iec.ch/TC57/NonStandard/UML#concrete> .

nc:ContingencyWithRemedialAction a rdfs:Class ;
  rdfs:label "ContingencyWithRemedialAction"@en ;
  rdfs:comment "Combination of a contingency and a remedial action. ContingencyWithRemedialAction shall not be instantiated for preventive RemedialAction (RemedialAction.kind equals RemedialActionKind.preventive)." ;
  cims:belongsToCategory sis:Package_StateInstructionScheduleProfile ;
  cims:stereotype "NC" .

nc:CrossBorderRelevance a rdfs:Class ;
  rdfs:label "CrossBorderRelevance"@en ;
  rdfs:comment "Combination of an assessed element and one or more bidding zone border that are affected by the assessment." ;
  cims:belongsToCategory sis:Package_StateInstructionScheduleProfile ;
  cims:stereotype "NC" .

nc:DCPole a rdfs:Class ;
  rdfs:label "DCPole"@en ;
  rdfs:comment "The direct current (DC) system pole (IEC 60633) is part of a DC system consisting of all the equipment in the DC substations and the interconnecting transmission lines, if any, which during normal operation exhibit a common direct voltage polarity with respect to earth." ;
  cims:belongsToCategory sis:Package_StateInstructionScheduleProfile ;
  cims:stereotype "NC" .

nc:DayOfWeekKind a rdfs:Class ;
  rdfs:label "DayOfWeekKind"@en ;
  rdfs:comment "The kind of day to be included in a regular schedule." ;
  cims:belongsToCategory sis:Package_StateInstructionScheduleProfile ;
  cims:stereotype "NC", <http://iec.ch/TC57/NonStandard/UML#enumeration> .

nc:EnablingTimePoint a rdfs:Class ;
  rdfs:label "EnablingTimePoint"@en ;
  rdfs:comment "Enabling instruction value at a given point in time." ;
  cims:belongsToCategory sis:Package_StateInstructionScheduleProfile ;
  cims:stereotype "NC", <http://iec.ch/TC57/NonStandard/UML#concrete> .

nc:EnergyBlockOrder a rdfs:Class ;
  rdfs:label "EnergyBlockOrder"@en ;
  rdfs:comment "The energy block order is a block (an amount) of energy that forms the sequence of orders that are going to be distributed to an energy block component." ;
  cims:belongsToCategory sis:Package_StateInstructionScheduleProfile ;
  cims:stereotype "NC" .

nc:EnergyDemandKind a rdfs:Class ;
  rdfs:label "EnergyDemandKind"@en ;
  rdfs:comment "Kind of energy demand." ;
  cims:belongsToCategory sis:Package_StateInstructionScheduleProfile ;
  cims:stereotype "NC", <http://iec.ch/TC57/NonStandard/UML#enumeration> .

nc:EnergyGroup a rdfs:Class ;
  rdfs:label "EnergyGroup"@en ;
  rdfs:comment "An energy group is an aggregation of energy components which have the same energy characteristic, e.g. fuel type and technology. It can be used to allocate energy. " ;
  cims:belongsToCategory sis:Package_StateInstructionScheduleProfile ;
  cims:stereotype "NC" .

nc:FunctionBlock a rdfs:Class ;
  rdfs:label "FunctionBlock"@en ;
  rdfs:comment "Function block is a function described as a set of elementary blocks. The blocks describe the function between input variables and output variables." ;
  cims:belongsToCategory sis:Package_StateInstructionScheduleProfile ;
  cims:stereotype "NC" .

nc:GenericAvailableSchedule a rdfs:Class ;
  rdfs:label "GenericAvailableSchedule"@en ;
  rdfs:comment "The schedule for the availability of elements." ;
  cims:belongsToCategory sis:Package_StateInstructionScheduleProfile ;
  cims:stereotype "NC", <http://iec.ch/TC57/NonStandard/UML#concrete> ;
  rdfs:subClassOf nc:BaseIrregularTimeSeries .

nc:GenericEnablingSchedule a rdfs:Class ;
  rdfs:label "GenericEnablingSchedule"@en ;
  rdfs:comment "The schedule for the enabling of elements." ;
  cims:belongsToCategory sis:Package_StateInstructionScheduleProfile ;
  cims:stereotype "NC", <http://iec.ch/TC57/NonStandard/UML#concrete> ;
  rdfs:subClassOf nc:BaseIrregularTimeSeries .

nc:GenericSequenceSchedule a rdfs:Class ;
  rdfs:label "GenericSequenceSchedule"@en ;
  rdfs:comment "Schedule for sequence." ;
  cims:belongsToCategory sis:Package_StateInstructionScheduleProfile ;
  cims:stereotype "NC", <http://iec.ch/TC57/NonStandard/UML#concrete> ;
  rdfs:subClassOf nc:BaseIrregularTimeSeries .

nc:GenericValueSchedule a rdfs:Class ;
  rdfs:label "GenericValueSchedule"@en ;
  rdfs:comment "Time series represent irregular generic value at given points in time. The type of value is given by the reference association.  " ;
  cims:belongsToCategory sis:Package_StateInstructionScheduleProfile ;
  cims:stereotype "NC", <http://iec.ch/TC57/NonStandard/UML#concrete> ;
  rdfs:subClassOf nc:BaseIrregularTimeSeries .

nc:GenericValueTimePoint a rdfs:Class ;
  rdfs:label "GenericValueTimePoint"@en ;
  rdfs:comment "Generic value for a given point in time." ;
  cims:belongsToCategory sis:Package_StateInstructionScheduleProfile ;
  cims:stereotype "NC", <http://iec.ch/TC57/NonStandard/UML#concrete> .

nc:GridStateAlteration a rdfs:Class ;
  rdfs:label "GridStateAlteration"@en ;
  rdfs:comment "Grid state alteration is a change of values describing state (operating point) of one element in the grid model compared to the base case." ;
  cims:belongsToCategory sis:Package_StateInstructionScheduleProfile ;
  cims:stereotype "NC" .

nc:GridStateAlterationSchedule a rdfs:Class ;
  rdfs:label "GridStateAlterationSchedule"@en ;
  rdfs:comment "Schedule for a grid state alteration." ;
  cims:belongsToCategory sis:Package_StateInstructionScheduleProfile ;
  cims:stereotype "NC", <http://iec.ch/TC57/NonStandard/UML#concrete> ;
  rdfs:subClassOf nc:BaseIrregularTimeSeries .

nc:GridStateAlterationTimePoint a rdfs:Class ;
  rdfs:label "GridStateAlterationTimePoint"@en ;
  rdfs:comment "Grid state alteration at a given point in time." ;
  cims:belongsToCategory sis:Package_StateInstructionScheduleProfile ;
  cims:stereotype "NC", <http://iec.ch/TC57/NonStandard/UML#concrete> .

nc:GridStateIntensitySchedule a rdfs:Class ;
  rdfs:label "GridStateIntensitySchedule"@en ;
  rdfs:comment "Defines the intensity applied for a given grid state alteration. It is primarily used in exchanges related to the remedial action schedule. The value provided by the schedule replaces the value of the attribute to which the schedule refers to." ;
  cims:belongsToCategory sis:Package_StateInstructionScheduleProfile ;
  cims:stereotype "NC", <http://iec.ch/TC57/NonStandard/UML#concrete> ;
  rdfs:subClassOf nc:GenericValueSchedule .

nc:HourPattern a rdfs:Class ;
  rdfs:label "HourPattern"@en ;
  rdfs:comment "Pattern of hourly period in a day with the same kind of intensity." ;
  cims:belongsToCategory sis:Package_StateInstructionScheduleProfile ;
  cims:stereotype "NC", <http://iec.ch/TC57/NonStandard/UML#concrete> ;
  rdfs:subClassOf cim:IdentifiedObject .

nc:HourPeriod a rdfs:Class ;
  rdfs:label "HourPeriod"@en ;
  rdfs:comment "Period of hours in a day." ;
  cims:belongsToCategory sis:Package_StateInstructionScheduleProfile ;
  cims:stereotype "NC", <http://iec.ch/TC57/NonStandard/UML#concrete> .

nc:InfeedLimit a rdfs:Class ;
  rdfs:label "InfeedLimit"@en ;
  rdfs:comment "Infeed limit set constraints fed in to the network by two or more terminals." ;
  cims:belongsToCategory sis:Package_StateInstructionScheduleProfile ;
  cims:stereotype "NC" .

nc:InfeedLimitSchedule a rdfs:Class ;
  rdfs:label "InfeedLimitSchedule"@en ;
  rdfs:comment "The schedule for an infeed limit." ;
  cims:belongsToCategory sis:Package_StateInstructionScheduleProfile ;
  cims:stereotype "NC", <http://iec.ch/TC57/NonStandard/UML#concrete> ;
  rdfs:subClassOf nc:BaseIrregularTimeSeries .

nc:InfeedLimitTimePoint a rdfs:Class ;
  rdfs:label "InfeedLimitTimePoint"@en ;
  rdfs:comment "Infeed limit at a given point in time." ;
  cims:belongsToCategory sis:Package_StateInstructionScheduleProfile ;
  cims:stereotype "NC", <http://iec.ch/TC57/NonStandard/UML#concrete> .

nc:ParticipationFactorTimePoint a rdfs:Class ;
  rdfs:label "ParticipationFactorTimePoint"@en ;
  rdfs:comment "Participation factor for a given point in time." ;
  cims:belongsToCategory sis:Package_StateInstructionScheduleProfile ;
  cims:stereotype "NC", <http://iec.ch/TC57/NonStandard/UML#concrete> .

nc:PeakKind a rdfs:Class ;
  rdfs:label "PeakKind"@en ;
  rdfs:comment "Kind of time period with similar intensity." ;
  cims:belongsToCategory sis:Package_StateInstructionScheduleProfile ;
  cims:stereotype "NC", <http://iec.ch/TC57/NonStandard/UML#enumeration> .

nc:PowerBidDependency a rdfs:Class ;
  rdfs:label "PowerBidDependency"@en ;
  rdfs:comment "Dependency between the related power bids." ;
  cims:belongsToCategory sis:Package_StateInstructionScheduleProfile ;
  cims:stereotype "NC", <http://iec.ch/TC57/NonStandard/UML#concrete> .

nc:PowerBidDependencyKind a rdfs:Class ;
  rdfs:label "PowerBidDependencyKind"@en ;
  rdfs:comment "Kind of power bid dependency." ;
  cims:belongsToCategory sis:Package_StateInstructionScheduleProfile ;
  cims:stereotype "NC", <http://iec.ch/TC57/NonStandard/UML#enumeration> .

nc:PowerBidSchedule a rdfs:Class ;
  rdfs:label "PowerBidSchedule"@en ;
  rdfs:comment "Power bid or offer related to a redispatch or countertrading measures. In the case of market place for economic efficiency of the bids and offers, this is equivalent to BidTimeSeries class in 62325 package." ;
  cims:belongsToCategory sis:Package_StateInstructionScheduleProfile ;
  cims:stereotype "NC", <http://iec.ch/TC57/NonStandard/UML#concrete> ;
  rdfs:subClassOf nc:BaseIrregularTimeSeries .

nc:PowerBidScheduleTimePoint a rdfs:Class ;
  rdfs:label "PowerBidScheduleTimePoint"@en ;
  rdfs:comment "Time series represent irregular power, active and reactive, values at given points in time." ;
  cims:belongsToCategory sis:Package_StateInstructionScheduleProfile ;
  cims:stereotype "NC", <http://iec.ch/TC57/NonStandard/UML#concrete> .

nc:PowerRemedialAction a rdfs:Class ;
  rdfs:label "PowerRemedialAction"@en ;
  rdfs:comment "Energy remedial action describes actions to rearrange power schedules." ;
  cims:belongsToCategory sis:Package_StateInstructionScheduleProfile ;
  cims:stereotype "NC" .

nc:PowerRemedialActionSchedule a rdfs:Class ;
  rdfs:label "PowerRemedialActionSchedule"@en ;
  rdfs:comment "The schedule for a power remedial action." ;
  cims:belongsToCategory sis:Package_StateInstructionScheduleProfile ;
  cims:stereotype "NC", <http://iec.ch/TC57/NonStandard/UML#concrete> ;
  rdfs:subClassOf nc:BaseIrregularTimeSeries .

nc:PowerRemedialActionTimePoint a rdfs:Class ;
  rdfs:label "PowerRemedialActionTimePoint"@en ;
  rdfs:comment "Regulating values at a given point in time." ;
  cims:belongsToCategory sis:Package_StateInstructionScheduleProfile ;
  cims:stereotype "NC", <http://iec.ch/TC57/NonStandard/UML#concrete> .

nc:PowerShiftKeyDistribution a rdfs:Class ;
  rdfs:label "PowerShiftKeyDistribution"@en ;
  rdfs:comment "Distribution of the bid action on the power shift keys." ;
  cims:belongsToCategory sis:Package_StateInstructionScheduleProfile ;
  cims:stereotype "NC", <http://iec.ch/TC57/NonStandard/UML#concrete> ;
  rdfs:subClassOf cim:IdentifiedObject .

nc:PowerShiftKeySchedule a rdfs:Class ;
  rdfs:label "PowerShiftKeySchedule"@en ;
  rdfs:comment "The schedule for Power Shift Keys." ;
  cims:belongsToCategory sis:Package_StateInstructionScheduleProfile ;
  cims:stereotype "NC", <http://iec.ch/TC57/NonStandard/UML#concrete> ;
  rdfs:subClassOf nc:BaseIrregularTimeSeries .

nc:PowerShiftKeyStrategy a rdfs:Class ;
  rdfs:label "PowerShiftKeyStrategy"@en ;
  rdfs:comment "Strategy of the power shift key." ;
  cims:belongsToCategory sis:Package_StateInstructionScheduleProfile ;
  cims:stereotype "NC" .

nc:PowerTransferCorridor a rdfs:Class ;
  rdfs:label "PowerTransferCorridor"@en ;
  rdfs:comment "A power transfer corridor is defined as a set of circuits (transmission lines or transformers) separating two portions of the power system, or a subset of circuits exposed to a substantial portion of the transmission exchange between two parts of the system." ;
  cims:belongsToCategory sis:Package_StateInstructionScheduleProfile ;
  cims:stereotype "NC" .

nc:RangeConstraint a rdfs:Class ;
  rdfs:label "RangeConstraint"@en ;
  rdfs:comment "Defines the rage constraint." ;
  cims:belongsToCategory sis:Package_StateInstructionScheduleProfile ;
  cims:stereotype "NC" ;
  rdfs:subClassOf cim:IdentifiedObject .

nc:RemedialAction a rdfs:Class ;
  rdfs:label "RemedialAction"@en ;
  rdfs:comment "Remedial action describes one or more actions that can be performed on a given power system model situation to eliminate one or more identified breaches of constraints. The remedial action can be costly, and have a cost characteristic, or non costly. " ;
  cims:belongsToCategory sis:Package_StateInstructionScheduleProfile ;
  cims:stereotype "NC" ;
  rdfs:subClassOf cim:IdentifiedObject .

nc:RemedialActionDependency a rdfs:Class ;
  rdfs:label "RemedialActionDependency"@en ;
  rdfs:comment """Remedial action dependency is making two remedial actions depending on each other. Multiple dependency is done by multiple instances of this class. The dependency can arrive by having one of the following examples.
<ul>
\t<li>The dependent remedial action is controlled by different system operator (Modeling Authority)  (e.g. SIPS that goes across control area).</li>
\t<li>The dependent remedial action is representing  two or more remedial action that represent the same grid state alteration but with different modeling resolution (e.g. detail direct current model versus a simplified model).</li>
\t<li>The remedial action can be combined with other remedial action without the need to create multiple remedial action with the same grid alteration for enabling dependency.</li>
</ul>""" ;
  cims:belongsToCategory sis:Package_StateInstructionScheduleProfile ;
  cims:stereotype "NC" .

nc:RemedialActionGroup a rdfs:Class ;
  rdfs:label "RemedialActionGroup"@en ;
  rdfs:comment "Grouping of remedial actions that can be operated together." ;
  cims:belongsToCategory sis:Package_StateInstructionScheduleProfile ;
  cims:stereotype "NC" .

nc:RemedialActionGroupSchedule a rdfs:Class ;
  rdfs:label "RemedialActionGroupSchedule"@en ;
  rdfs:comment "The schedule for a remedial action group." ;
  cims:belongsToCategory sis:Package_StateInstructionScheduleProfile ;
  cims:stereotype "NC", <http://iec.ch/TC57/NonStandard/UML#concrete> ;
  rdfs:subClassOf nc:BaseIrregularTimeSeries .

nc:RemedialActionGroupTimePoint a rdfs:Class ;
  rdfs:label "RemedialActionGroupTimePoint"@en ;
  rdfs:comment "Remedial action group at a given point in time." ;
  cims:belongsToCategory sis:Package_StateInstructionScheduleProfile ;
  cims:stereotype "NC", <http://iec.ch/TC57/NonStandard/UML#concrete> .

nc:RemedialActionScheme a rdfs:Class ;
  rdfs:label "RemedialActionScheme"@en ;
  rdfs:comment """Remedial Action Scheme (RAS), Special Protection Schemes (SPS), System Protection Schemes (SPS) or System Integrity Protection Schemes (SIPS).
A Remedial Action Scheme consists of one or more stages that can trigger and execute a protection action.""" ;
  cims:belongsToCategory sis:Package_StateInstructionScheduleProfile ;
  cims:stereotype "NC" .

nc:RemedialActionSchemeSchedule a rdfs:Class ;
  rdfs:label "RemedialActionSchemeSchedule"@en ;
  rdfs:comment "The schedule for a remedial action scheme." ;
  cims:belongsToCategory sis:Package_StateInstructionScheduleProfile ;
  cims:stereotype "NC", <http://iec.ch/TC57/NonStandard/UML#concrete> ;
  rdfs:subClassOf nc:BaseIrregularTimeSeries .

nc:RemedialActionSchemeTimePoint a rdfs:Class ;
  rdfs:label "RemedialActionSchemeTimePoint"@en ;
  rdfs:comment "Remedial action scheme at a given point in time." ;
  cims:belongsToCategory sis:Package_StateInstructionScheduleProfile ;
  cims:stereotype "NC", <http://iec.ch/TC57/NonStandard/UML#concrete> .

nc:ScheduleResource a rdfs:Class ;
  rdfs:label "ScheduleResource"@en ;
  rdfs:comment "A schedule resource is a market-based method for handling participation of small units, particularly located on the lower voltage level that is controlled by a Distributed System Operator (DSO). It is a collection of units that can operate in the market by providing bids, offers and a resulting committed operational schedule for the collection." ;
  cims:belongsToCategory sis:Package_StateInstructionScheduleProfile ;
  cims:stereotype "NC" .

nc:SecuredExclusionReasonKind a rdfs:Class ;
  rdfs:label "SecuredExclusionReasonKind"@en ;
  rdfs:comment "The kind of secured exclusion reason." ;
  cims:belongsToCategory sis:Package_StateInstructionScheduleProfile ;
  cims:stereotype "NC", <http://iec.ch/TC57/NonStandard/UML#enumeration> .

nc:SequenceTimePoint a rdfs:Class ;
  rdfs:label "SequenceTimePoint"@en ;
  rdfs:comment "Sequence at a given point in time." ;
  cims:belongsToCategory sis:Package_StateInstructionScheduleProfile ;
  cims:stereotype "NC", <http://iec.ch/TC57/NonStandard/UML#concrete> .

nc:StageTrigger a rdfs:Class ;
  rdfs:label "StageTrigger"@en ;
  rdfs:comment "Stage that is triggered either by TriggerCondition or by gate condition within a stage." ;
  cims:belongsToCategory sis:Package_StateInstructionScheduleProfile ;
  cims:stereotype "NC" .

nc:StageTriggerSchedule a rdfs:Class ;
  rdfs:label "StageTriggerSchedule"@en ;
  rdfs:comment "Schedule for a stage trigger." ;
  cims:belongsToCategory sis:Package_StateInstructionScheduleProfile ;
  cims:stereotype "NC", <http://iec.ch/TC57/NonStandard/UML#concrete> ;
  rdfs:subClassOf nc:BaseIrregularTimeSeries .

nc:StageTriggerTimePoint a rdfs:Class ;
  rdfs:label "StageTriggerTimePoint"@en ;
  rdfs:comment "Stage trigger values at a given point in time." ;
  cims:belongsToCategory sis:Package_StateInstructionScheduleProfile ;
  cims:stereotype "NC", <http://iec.ch/TC57/NonStandard/UML#concrete> .

nc:TimeSeriesInterpolationKind a rdfs:Class ;
  rdfs:label "TimeSeriesInterpolationKind"@en ;
  rdfs:comment "Kinds of interpolation of values between two time point. " ;
  cims:belongsToCategory sis:Package_StateInstructionScheduleProfile ;
  cims:stereotype "NC", <http://iec.ch/TC57/NonStandard/UML#enumeration> .

nc:UnitCostSchedule a rdfs:Class ;
  rdfs:label "UnitCostSchedule"@en ;
  rdfs:comment "The schedule for a unit cost." ;
  cims:belongsToCategory sis:Package_StateInstructionScheduleProfile ;
  cims:stereotype "NC", <http://iec.ch/TC57/NonStandard/UML#concrete> ;
  rdfs:subClassOf nc:BaseIrregularTimeSeries .

nc:UnitCostTimePoint a rdfs:Class ;
  rdfs:label "UnitCostTimePoint"@en ;
  rdfs:comment "Unit cost at a given point in time." ;
  cims:belongsToCategory sis:Package_StateInstructionScheduleProfile ;
  cims:stereotype "NC", <http://iec.ch/TC57/NonStandard/UML#concrete> .

nc:ValueOffsetKind a rdfs:Class ;
  rdfs:label "ValueOffsetKind"@en ;
  rdfs:comment "The kind of the value offset." ;
  cims:belongsToCategory sis:Package_StateInstructionScheduleProfile ;
  cims:stereotype "NC", <http://iec.ch/TC57/NonStandard/UML#enumeration> .

nc:VoltageAngleLimit a rdfs:Class ;
  rdfs:label "VoltageAngleLimit"@en ;
  rdfs:comment "Voltage angle limit between two terminals. The association end OperationalLimitSet.Terminal defines one end and the host of the limit. The association end VoltageAngleLimit.AngleReferenceTerminal defines the reference terminal." ;
  cims:belongsToCategory sis:Package_StateInstructionScheduleProfile ;
  cims:stereotype "NC" .

nc:VoltageAngleSchedule a rdfs:Class ;
  rdfs:label "VoltageAngleSchedule"@en ;
  rdfs:comment "The schedule for a voltage angle." ;
  cims:belongsToCategory sis:Package_StateInstructionScheduleProfile ;
  cims:stereotype "NC", <http://iec.ch/TC57/NonStandard/UML#concrete> ;
  rdfs:subClassOf nc:BaseIrregularTimeSeries .

nc:VoltageAngleTimePoint a rdfs:Class ;
  rdfs:label "VoltageAngleTimePoint"@en ;
  rdfs:comment "Voltage angle at a given point in time." ;
  cims:belongsToCategory sis:Package_StateInstructionScheduleProfile ;
  cims:stereotype "NC", <http://iec.ch/TC57/NonStandard/UML#concrete> .

profcim:IRI a rdfs:Class ;
  rdfs:label "IRI"@en ;
  rdfs:comment """An IRI (Internationalized Resource Identifier) within an RDF graph is a Unicode string that conforms to the syntax defined in RFC 3987.
The primitive is serialized as rdf:resource in RDFXML.
IRIs in the RDF abstract syntax must be absolute, and may contain a fragment identifier.
IRI equality: Two IRIs are equal if and only if they are equivalent under Simple String Comparison according to section 5.1 of [RFC3987]. Further normalization must not be performed when comparing IRIs for equality.
IRIs are a generalization of URIs [RFC3986] that permits a wider range of Unicode characters. Every absolute URI and URL is an IRI, but not every IRI is an URI. When IRIs are used in operations that are only defined for URIs, they must first be converted according to the mapping defined in section 3.1 of [RFC3987]. A notable example is retrieval over the HTTP protocol. The mapping involves UTF-8 encoding of non-ASCII characters, %-encoding of octets not allowed in URIs, and Punycode-encoding of domain names.""" ;
  cims:belongsToCategory sis:Package_DocStateInstructionScheduleProfile ;
  cims:stereotype "Primitive", "profcim" .

profcim:StringFixedLanguage a rdfs:Class ;
  rdfs:label "StringFixedLanguage"@en ;
  rdfs:comment """A string consisting of a sequence of characters. The character encoding is UTF-8. The string length is unspecified and unlimited.
The primitive is serialized as literal without language support.""" ;
  cims:belongsToCategory sis:Package_DocStateInstructionScheduleProfile ;
  cims:stereotype "Primitive", "profcim" .

profcim:StringIRI a rdfs:Class ;
  rdfs:label "StringIRI"@en ;
  rdfs:comment """An IRI (Internationalized Resource Identifier) within an RDF graph is a Unicode string that conforms to the syntax defined in RFC 3987.
The primitive is serialized as literal without language support.
IRIs in the RDF abstract syntax must be absolute, and may contain a fragment identifier.
IRI equality: Two IRIs are equal if and only if they are equivalent under Simple String Comparison according to section 5.1 of [RFC3987]. Further normalization must not be performed when comparing IRIs for equality.
IRIs are a generalization of URIs [RFC3986] that permits a wider range of Unicode characters. Every absolute URI and URL is an IRI, but not every IRI is an URI. When IRIs are used in operations that are only defined for URIs, they must first be converted according to the mapping defined in section 3.1 of [RFC3987]. A notable example is retrieval over the HTTP protocol. The mapping involves UTF-8 encoding of non-ASCII characters, %-encoding of octets not allowed in URIs, and Punycode-encoding of domain names.""" ;
  cims:belongsToCategory sis:Package_DocStateInstructionScheduleProfile ;
  cims:stereotype "Primitive", "profcim" .

profcim:URL a rdfs:Class ;
  rdfs:label "URL"@en ;
  rdfs:comment "A Uniform Resource Locator (URL), colloquially termed a web address, is a reference to a web resource that specifies its location on a computer network and a mechanism for retrieving it. A URL is a specific type of Uniform Resource Identifier (URI), although many people use the two terms interchangeably.URLs occur most commonly to reference web pages (http), but are also used for file transfer (ftp), email (mailto), database access (JDBC), and many other applications." ;
  cims:belongsToCategory sis:Package_DocStateInstructionScheduleProfile ;
  cims:stereotype "Primitive", "profcim" .

sis:Ontology a owl:Ontology ;
  dcat:keyword "SIS" ;
  dcat:theme "vocabulary"@en ;
  dcterms:conformsTo "file://CIM100_CGMES31v01_501-20v02_NC23v62_MM10v01.eap", "file://iec61970cim17v40_iec61968cim13v13a_iec62325cim03v17a.eap", "urn:iso:std:iec:61970-301:ed-7:amd1", "urn:iso:std:iec:61970-401:draft:ed-1", "urn:iso:std:iec:61970-501:draft:ed-2", "urn:iso:std:iec:61970-600-2:ed-1" ;
  dcterms:creator "ENTSO-E CIM WG NC project"@en ;
  dcterms:description "This vocabulary is describing the state instruction schedule profile."@en ;
  dcterms:identifier "urn:uuid:af884936-ea95-416b-b4c9-1214caa68658" ;
  dcterms:language "en-GB" ;
  dcterms:license "https://www.apache.org/licenses/LICENSE-2.0"@en ;
  dcterms:modified "2024-09-07"^^<http://www.w3.org/2001/XMLSchema#date> ;
  dcterms:publisher "ENTSO-E"@en ;
  dcterms:rightsHolder "ENTSO-E"@en ;
  dcterms:title "State instruction schedule vocabulary"@en ;
  owl:priorVersion <http://entsoe.eu/ns/CIM/StateInstructionSchedule-EU/2.2> ;
  owl:versionIRI <https://ap-voc.cim4.eu/StateInstructionSchedule/2.3> ;
  owl:versionInfo "2.3.1"@en .

cim:ActivePower.multiplier a rdf:Property ;
  rdfs:label "multiplier"@en ;
  cims:isFixed "M" ;
  cims:multiplicity cims:M:0..1 ;
  cims:stereotype <http://iec.ch/TC57/NonStandard/UML#attribute> ;
  rdfs:domain cim:ActivePower ;
  rdfs:range cim:UnitMultiplier .

cim:ActivePower.unit a rdf:Property ;
  rdfs:label "unit"@en ;
  cims:isFixed "W" ;
  cims:multiplicity cims:M:0..1 ;
  cims:stereotype <http://iec.ch/TC57/NonStandard/UML#attribute> ;
  rdfs:domain cim:ActivePower ;
  rdfs:range cim:UnitSymbol .

cim:ActivePower.value a rdf:Property ;
  rdfs:label "value"@en ;
  cims:dataType cim:Float ;
  cims:multiplicity cims:M:0..1 ;
  cims:stereotype <http://iec.ch/TC57/NonStandard/UML#attribute> ;
  rdfs:domain cim:ActivePower .

cim:AngleDegrees.multiplier a rdf:Property ;
  rdfs:label "multiplier"@en ;
  cims:isFixed "none" ;
  cims:multiplicity cims:M:0..1 ;
  cims:stereotype <http://iec.ch/TC57/NonStandard/UML#attribute> ;
  rdfs:domain cim:AngleDegrees ;
  rdfs:range cim:UnitMultiplier .

cim:AngleDegrees.unit a rdf:Property ;
  rdfs:label "unit"@en ;
  cims:isFixed "deg" ;
  cims:multiplicity cims:M:0..1 ;
  cims:stereotype <http://iec.ch/TC57/NonStandard/UML#attribute> ;
  rdfs:domain cim:AngleDegrees ;
  rdfs:range cim:UnitSymbol .

cim:AngleDegrees.value a rdf:Property ;
  rdfs:label "value"@en ;
  cims:dataType cim:Float ;
  cims:multiplicity cims:M:0..1 ;
  cims:stereotype <http://iec.ch/TC57/NonStandard/UML#attribute> ;
  rdfs:domain cim:AngleDegrees .

cim:CurrentFlow.multiplier a rdf:Property ;
  rdfs:label "multiplier"@en ;
  cims:multiplicity cims:M:0..1 ;
  cims:stereotype <http://iec.ch/TC57/NonStandard/UML#attribute> ;
  rdfs:domain cim:CurrentFlow ;
  rdfs:range cim:UnitMultiplier .

cim:CurrentFlow.unit a rdf:Property ;
  rdfs:label "unit"@en ;
  cims:isFixed "A" ;
  cims:multiplicity cims:M:0..1 ;
  cims:stereotype <http://iec.ch/TC57/NonStandard/UML#attribute> ;
  rdfs:domain cim:CurrentFlow ;
  rdfs:range cim:UnitSymbol .

cim:CurrentFlow.value a rdf:Property ;
  rdfs:label "value"@en ;
  cims:dataType cim:Float ;
  cims:multiplicity cims:M:0..1 ;
  cims:stereotype <http://iec.ch/TC57/NonStandard/UML#attribute> ;
  rdfs:domain cim:CurrentFlow .

cim:IdentifiedObject.description a rdf:Property ;
  rdfs:label "description"@en ;
  rdfs:comment "The description is a free human readable text describing or naming the object. It may be non unique and may not correlate to a naming hierarchy." ;
  cims:dataType cim:String ;
  cims:multiplicity cims:M:0..1 ;
  cims:stereotype <http://iec.ch/TC57/NonStandard/UML#attribute> ;
  rdfs:domain cim:IdentifiedObject .

cim:IdentifiedObject.mRID a rdf:Property ;
  rdfs:label "mRID"@en ;
  rdfs:comment """Master resource identifier issued by a model authority. The mRID is unique within an exchange context. Global uniqueness is easily achieved by using a UUID, as specified in RFC 4122, for the mRID. The use of UUID is strongly recommended.
For CIMXML data files in RDF syntax conforming to IEC 61970-552, the mRID is mapped to rdf:ID or rdf:about attributes that identify CIM object elements.""" ;
  cims:dataType cim:String ;
  cims:multiplicity cims:M:1..1 ;
  cims:stereotype <http://iec.ch/TC57/NonStandard/UML#attribute> ;
  rdfs:domain cim:IdentifiedObject .

cim:IdentifiedObject.name a rdf:Property ;
  rdfs:label "name"@en ;
  rdfs:comment "The name is any free human readable and possibly non unique text naming the object." ;
  cims:dataType cim:String ;
  cims:multiplicity cims:M:0..1 ;
  cims:stereotype <http://iec.ch/TC57/NonStandard/UML#attribute> ;
  rdfs:domain cim:IdentifiedObject .

cim:Money.multiplier a rdf:Property ;
  rdfs:label "multiplier"@en ;
  cims:multiplicity cims:M:0..1 ;
  cims:stereotype <http://iec.ch/TC57/NonStandard/UML#attribute> ;
  rdfs:domain cim:Money ;
  rdfs:range cim:UnitMultiplier .

cim:Money.unit a rdf:Property ;
  rdfs:label "unit"@en ;
  cims:multiplicity cims:M:0..1 ;
  cims:stereotype <http://iec.ch/TC57/NonStandard/UML#attribute> ;
  rdfs:domain cim:Money ;
  rdfs:range cim:Currency .

cim:Money.value a rdf:Property ;
  rdfs:label "value"@en ;
  cims:dataType cim:Decimal ;
  cims:multiplicity cims:M:0..1 ;
  cims:stereotype <http://iec.ch/TC57/NonStandard/UML#attribute> ;
  rdfs:domain cim:Money .

cim:PerCent.multiplier a rdf:Property ;
  rdfs:label "multiplier"@en ;
  cims:isFixed "none" ;
  cims:multiplicity cims:M:0..1 ;
  cims:stereotype <http://iec.ch/TC57/NonStandard/UML#attribute> ;
  rdfs:domain cim:PerCent ;
  rdfs:range cim:UnitMultiplier .

cim:PerCent.unit a rdf:Property ;
  rdfs:label "unit"@en ;
  cims:isFixed "none" ;
  cims:multiplicity cims:M:0..1 ;
  cims:stereotype <http://iec.ch/TC57/NonStandard/UML#attribute> ;
  rdfs:domain cim:PerCent ;
  rdfs:range cim:UnitSymbol .

cim:PerCent.value a rdf:Property ;
  rdfs:label "value"@en ;
  rdfs:comment "Normally 0 to 100 on a defined base." ;
  cims:dataType cim:Float ;
  cims:multiplicity cims:M:0..1 ;
  cims:stereotype <http://iec.ch/TC57/NonStandard/UML#attribute> ;
  rdfs:domain cim:PerCent .

cim:RealEnergy.multiplier a rdf:Property ;
  rdfs:label "multiplier"@en ;
  cims:isFixed "M" ;
  cims:multiplicity cims:M:0..1 ;
  cims:stereotype <http://iec.ch/TC57/NonStandard/UML#attribute> ;
  rdfs:domain cim:RealEnergy ;
  rdfs:range cim:UnitMultiplier .

cim:RealEnergy.unit a rdf:Property ;
  rdfs:label "unit"@en ;
  cims:isFixed "Wh" ;
  cims:multiplicity cims:M:0..1 ;
  cims:stereotype <http://iec.ch/TC57/NonStandard/UML#attribute> ;
  rdfs:domain cim:RealEnergy ;
  rdfs:range cim:UnitSymbol .

cim:RealEnergy.value a rdf:Property ;
  rdfs:label "value"@en ;
  cims:dataType cim:Float ;
  cims:multiplicity cims:M:0..1 ;
  cims:stereotype <http://iec.ch/TC57/NonStandard/UML#attribute> ;
  rdfs:domain cim:RealEnergy .

cim:Season.endDate a rdf:Property ;
  rdfs:label "endDate"@en ;
  rdfs:comment "Date season ends." ;
  cims:dataType cim:MonthDay ;
  cims:multiplicity cims:M:1..1 ;
  cims:stereotype <http://iec.ch/TC57/NonStandard/UML#attribute> ;
  rdfs:domain cim:Season .

cim:Season.startDate a rdf:Property ;
  rdfs:label "startDate"@en ;
  rdfs:comment "Date season starts." ;
  cims:dataType cim:MonthDay ;
  cims:multiplicity cims:M:1..1 ;
  cims:stereotype <http://iec.ch/TC57/NonStandard/UML#attribute> ;
  rdfs:domain cim:Season .

cim:Seconds.multiplier a rdf:Property ;
  rdfs:label "multiplier"@en ;
  cims:isFixed "none" ;
  cims:multiplicity cims:M:0..1 ;
  cims:stereotype <http://iec.ch/TC57/NonStandard/UML#attribute> ;
  rdfs:domain cim:Seconds ;
  rdfs:range cim:UnitMultiplier .

cim:Seconds.unit a rdf:Property ;
  rdfs:label "unit"@en ;
  cims:isFixed "s" ;
  cims:multiplicity cims:M:0..1 ;
  cims:stereotype <http://iec.ch/TC57/NonStandard/UML#attribute> ;
  rdfs:domain cim:Seconds ;
  rdfs:range cim:UnitSymbol .

cim:Seconds.value a rdf:Property ;
  rdfs:label "value"@en ;
  rdfs:comment "Time, in seconds" ;
  cims:dataType cim:Float ;
  cims:multiplicity cims:M:0..1 ;
  cims:stereotype <http://iec.ch/TC57/NonStandard/UML#attribute> ;
  rdfs:domain cim:Seconds .

nc:AssessedElement.AssessedElementRegularSchedule a rdf:Property ;
  rdfs:label "AssessedElementRegularSchedule"@en ;
  rdfs:comment "Regular schedule that belongs to an assessed element." ;
  cims:AssociationUsed "No" ;
  cims:inverseRoleName nc:AssessedElementRegularSchedule.AssessedElement ;
  cims:multiplicity cims:M:0..n ;
  cims:stereotype "NC" ;
  rdfs:domain nc:AssessedElement ;
  rdfs:range nc:AssessedElementRegularSchedule .

nc:AssessedElement.AssessedElementSchedule a rdf:Property ;
  rdfs:label "AssessedElementSchedule"@en ;
  rdfs:comment "Assessed element schedule for an assessed element." ;
  cims:AssociationUsed "No" ;
  cims:inverseRoleName nc:AssessedElementSchedule.AssessedElement ;
  cims:multiplicity cims:M:0..n ;
  cims:stereotype "NC" ;
  rdfs:domain nc:AssessedElement ;
  rdfs:range nc:AssessedElementSchedule .

nc:AssessedElementRegularSchedule.AssessedElement a rdf:Property ;
  rdfs:label "AssessedElement"@en ;
  rdfs:comment "Assessed Element that has regular schedules." ;
  cims:AssociationUsed "Yes" ;
  cims:inverseRoleName nc:AssessedElement.AssessedElementRegularSchedule ;
  cims:multiplicity cims:M:0..1 ;
  cims:stereotype "NC" ;
  rdfs:domain nc:AssessedElementRegularSchedule ;
  rdfs:range nc:AssessedElement .

nc:AssessedElementRegularSchedule.AssessedElementRegularTimePoint a rdf:Property ;
  rdfs:label "AssessedElementRegularTimePoint"@en ;
  rdfs:comment "Assessed element regular time point which belong to an assessed element regular schedule." ;
  cims:AssociationUsed "No" ;
  cims:inverseRoleName nc:AssessedElementRegularTimePoint.AssessedElementRegularSchedule ;
  cims:multiplicity cims:M:0..n ;
  cims:stereotype "NC", <http://iec.ch/TC57/NonStandard/UML#ofAggregate> ;
  rdfs:domain nc:AssessedElementRegularSchedule ;
  rdfs:range nc:AssessedElementRegularTimePoint .

nc:AssessedElementRegularTimePoint.AssessedElementRegularSchedule a rdf:Property ;
  rdfs:label "AssessedElementRegularSchedule"@en ;
  rdfs:comment "Assessed element regular schedule which has assessed element regular time points." ;
  cims:AssociationUsed "Yes" ;
  cims:inverseRoleName nc:AssessedElementRegularSchedule.AssessedElementRegularTimePoint ;
  cims:multiplicity cims:M:0..1 ;
  cims:stereotype "NC" ;
  rdfs:domain nc:AssessedElementRegularTimePoint ;
  rdfs:range nc:AssessedElementRegularSchedule .

nc:AssessedElementRegularTimePoint.appointedMargin a rdf:Property ;
  rdfs:label "appointedMargin"@en ;
  rdfs:comment """The percentage (appointed to a region) of the remaining margin obtained in the grid model to reach its current limit. The maximum percentage shall by default be 10% of the remaining margin.
It is only used when an assessed element is considered conservative for a region.
The allowed value range is [0,100].""" ;
  cims:dataType cim:PerCent ;
  cims:multiplicity cims:M:0..1 ;
  cims:stereotype "NC", <http://iec.ch/TC57/NonStandard/UML#attribute> ;
  rdfs:domain nc:AssessedElementRegularTimePoint .

nc:AssessedElementRegularTimePoint.enabled a rdf:Property ;
  rdfs:label "enabled"@en ;
  rdfs:comment "It identifies if the assessed element is enabled. True means enabled, False means disabled." ;
  cims:dataType cim:Boolean ;
  cims:multiplicity cims:M:0..1 ;
  cims:stereotype "NC", <http://iec.ch/TC57/NonStandard/UML#attribute> ;
  rdfs:domain nc:AssessedElementRegularTimePoint .

nc:AssessedElementRegularTimePoint.maxFlow a rdf:Property ;
  rdfs:label "maxFlow"@en ;
  rdfs:comment "Maximum flow on an a conducting equipment or a collection of conducting equipment forming a power transfer corridor. For assessed elements that is becomes critical due to contingency, this value represents the maximum flow with remedial action taken into consideration." ;
  cims:dataType cim:ActivePower ;
  cims:multiplicity cims:M:0..1 ;
  cims:stereotype "NC", <http://iec.ch/TC57/NonStandard/UML#attribute> ;
  rdfs:domain nc:AssessedElementRegularTimePoint .

nc:AssessedElementRegularTimePoint.scannedThresholdMargin a rdf:Property ;
  rdfs:label "scannedThresholdMargin"@en ;
  rdfs:comment """Threshold percentage that a scanned element can be overloaded, on a given element, on top of any overload prior to optimisation (default= 5%). e.g. Initial loading of the element is 110%, with a 5% scanned threshold margin, the new maximum is 115% of the limit (e.g. PATL, TATL, etc).
The allowed value range is [0,100].""" ;
  cims:dataType cim:PerCent ;
  cims:multiplicity cims:M:0..1 ;
  cims:stereotype "NC", <http://iec.ch/TC57/NonStandard/UML#attribute> ;
  rdfs:domain nc:AssessedElementRegularTimePoint .

nc:AssessedElementRegularTimePoint.virtualPositiveMargin a rdf:Property ;
  rdfs:label "virtualPositiveMargin"@en ;
  rdfs:comment """A margin defined only for scanned AssessedElement (If AssessedElement.ScannedForRegion is present) in order to represent the influence of available remedial action which is not cross-border relevant remedial action.
The margin is modifying the limits used for the assessment whatever the limit it is (e.g. PATL, TATL).This symbolizes a remedial action that can be applied internally by the System Operator. It will be resolved by the System Operator and not by the optimization of remedial actions. The attribute shall be a positive value.
The allowed value range is [0,100].""" ;
  cims:dataType cim:PerCent ;
  cims:multiplicity cims:M:0..1 ;
  cims:stereotype "NC", <http://iec.ch/TC57/NonStandard/UML#attribute> ;
  rdfs:domain nc:AssessedElementRegularTimePoint .

nc:AssessedElementSchedule.AssessedElement a rdf:Property ;
  rdfs:label "AssessedElement"@en ;
  rdfs:comment "Assessed element which has an assessed element schedule." ;
  cims:AssociationUsed "Yes" ;
  cims:inverseRoleName nc:AssessedElement.AssessedElementSchedule ;
  cims:multiplicity cims:M:1 ;
  cims:stereotype "NC" ;
  rdfs:domain nc:AssessedElementSchedule ;
  rdfs:range nc:AssessedElement .

nc:AssessedElementSchedule.AssessedElementTimePoint a rdf:Property ;
  rdfs:label "AssessedElementTimePoint"@en ;
  rdfs:comment "The time point that relates to this assessed element schedule." ;
  cims:AssociationUsed "No" ;
  cims:inverseRoleName nc:AssessedElementTimePoint.AssessedElementSchedule ;
  cims:multiplicity cims:M:1..n ;
  cims:stereotype "NC", <http://iec.ch/TC57/NonStandard/UML#ofAggregate> ;
  rdfs:domain nc:AssessedElementSchedule ;
  rdfs:range nc:AssessedElementTimePoint .

nc:AssessedElementTimePoint.AssessedElementSchedule a rdf:Property ;
  rdfs:label "AssessedElementSchedule"@en ;
  rdfs:comment "The assessed element schedule that has this time point." ;
  cims:AssociationUsed "Yes" ;
  cims:inverseRoleName nc:AssessedElementSchedule.AssessedElementTimePoint ;
  cims:multiplicity cims:M:1 ;
  cims:stereotype "NC" ;
  rdfs:domain nc:AssessedElementTimePoint ;
  rdfs:range nc:AssessedElementSchedule .

nc:AssessedElementTimePoint.appointedMargin a rdf:Property ;
  rdfs:label "appointedMargin"@en ;
  rdfs:comment """The percentage (appointed to a region) of the remaining margin obtained in the grid model to reach its current limit. The maximum percentage shall by default be 10% of the remaining margin.
It is only used when an assessed element is considered conservative for a region.
The allowed value range is [0,100].""" ;
  cims:dataType cim:PerCent ;
  cims:multiplicity cims:M:0..1 ;
  cims:stereotype "NC", <http://iec.ch/TC57/NonStandard/UML#attribute> ;
  rdfs:domain nc:AssessedElementTimePoint .

nc:AssessedElementTimePoint.atTime a rdf:Property ;
  rdfs:label "atTime"@en ;
  rdfs:comment "The time the data is valid for." ;
  cims:dataType cim:DateTime ;
  cims:multiplicity cims:M:1..1 ;
  cims:stereotype "NC", <http://iec.ch/TC57/NonStandard/UML#attribute> ;
  rdfs:domain nc:AssessedElementTimePoint .

nc:AssessedElementTimePoint.coordinatedValidationAdjustment a rdf:Property ;
  rdfs:label "coordinatedValidationAdjustment"@en ;
  rdfs:comment "A positive value expressed in MW, calculated and provided by the coordinated capacity calculator (CCC) for the reduction of Remaining Available Margin (RAM) in order to ensure grid security." ;
  cims:dataType cim:ActivePower ;
  cims:multiplicity cims:M:0..1 ;
  cims:stereotype "NC", <http://iec.ch/TC57/NonStandard/UML#attribute> ;
  rdfs:domain nc:AssessedElementTimePoint .

nc:AssessedElementTimePoint.coordinatedValidationAdjustmentJustification a rdf:Property ;
  rdfs:label "coordinatedValidationAdjustmentJustification"@en ;
  rdfs:comment "A text description provided by the coordinated capacity calculator (CCC) for justifying the reduction of Remaining Available Margin (RAM) by means of Coordinated Validation Adjustment (CVA). This justification is not intended for any application processing purpose, it should only be used for reporting." ;
  cims:dataType cim:String ;
  cims:multiplicity cims:M:0..1 ;
  cims:stereotype "NC", <http://iec.ch/TC57/NonStandard/UML#attribute> ;
  rdfs:domain nc:AssessedElementTimePoint .

nc:AssessedElementTimePoint.criticalElementContingencyJustification a rdf:Property ;
  rdfs:label "criticalElementContingencyJustification"@en ;
  rdfs:comment "Justification indicating the kind of critical element contingency. This justification is not intended for any application processing purpose, it should only be used for reporting." ;
  cims:dataType cim:String ;
  cims:multiplicity cims:M:0..1 ;
  cims:stereotype "NC", <http://iec.ch/TC57/NonStandard/UML#attribute> ;
  rdfs:domain nc:AssessedElementTimePoint .

nc:AssessedElementTimePoint.enabled a rdf:Property ;
  rdfs:label "enabled"@en ;
  rdfs:comment "It identifies if the assessed element is enabled. True means enabled, False means disabled." ;
  cims:dataType cim:Boolean ;
  cims:multiplicity cims:M:0..1 ;
  cims:stereotype "NC", <http://iec.ch/TC57/NonStandard/UML#attribute> ;
  rdfs:domain nc:AssessedElementTimePoint .

nc:AssessedElementTimePoint.exclusionReason a rdf:Property ;
  rdfs:label "exclusionReason"@en ;
  rdfs:comment "Reason for not associating this assessed element with a secured region." ;
  cims:multiplicity cims:M:0..1 ;
  cims:stereotype "NC", <http://iec.ch/TC57/NonStandard/UML#attribute> ;
  rdfs:domain nc:AssessedElementTimePoint ;
  rdfs:range nc:SecuredExclusionReasonKind .

nc:AssessedElementTimePoint.individualValidationAdjustment a rdf:Property ;
  rdfs:label "individualValidationAdjustment"@en ;
  rdfs:comment "A positive value expressed in MW, calculated and provided by System Operators from their individual validation process for the reduction of Remaining Available Margin in order to ensure grid security." ;
  cims:dataType cim:ActivePower ;
  cims:multiplicity cims:M:0..1 ;
  cims:stereotype "NC", <http://iec.ch/TC57/NonStandard/UML#attribute> ;
  rdfs:domain nc:AssessedElementTimePoint .

nc:AssessedElementTimePoint.individualValidationAdjustmentJustification a rdf:Property ;
  rdfs:label "individualValidationAdjustmentJustification"@en ;
  rdfs:comment "A text description provided by System Operators for justifying the reduction of Remaining Available Margin (RAM) by means of Individual Validation Adjustment (IVA). This justification is not intended for any application processing purpose, it should only be used for reporting." ;
  cims:dataType cim:String ;
  cims:multiplicity cims:M:0..1 ;
  cims:stereotype "NC", <http://iec.ch/TC57/NonStandard/UML#attribute> ;
  rdfs:domain nc:AssessedElementTimePoint .

nc:AssessedElementTimePoint.individualValidationAdjustmentShare a rdf:Property ;
  rdfs:label "individualValidationAdjustmentShare"@en ;
  rdfs:comment "A positive value expressed in MW, calculated by the coordinated capacity calculator (CCC) based on the provided Individual Validation Adjustment (IVA) by System Operators in order to show the actual reduction of Remaining Available Margin (RAM). Individual Validation Adjustment Share is a positive non-zero value. It is equal or less than the Individual Validation Adjustment value. " ;
  cims:dataType cim:ActivePower ;
  cims:multiplicity cims:M:0..1 ;
  cims:stereotype "NC", <http://iec.ch/TC57/NonStandard/UML#attribute> ;
  rdfs:domain nc:AssessedElementTimePoint .

nc:AssessedElementTimePoint.maxFlow a rdf:Property ;
  rdfs:label "maxFlow"@en ;
  rdfs:comment "Maximum flow on an a conducting equipment or a collection of conducting equipment forming a power transfer corridor. For assessed elements that is becomes critical due to contingency, this value represents the maximum flow with remedial action taken into consideration." ;
  cims:dataType cim:ActivePower ;
  cims:multiplicity cims:M:0..1 ;
  cims:stereotype "NC", <http://iec.ch/TC57/NonStandard/UML#attribute> ;
  rdfs:domain nc:AssessedElementTimePoint .

nc:AssessedElementTimePoint.scannedThresholdMargin a rdf:Property ;
  rdfs:label "scannedThresholdMargin"@en ;
  rdfs:comment """Threshold percentage that a scanned element can be overloaded, on a given element, on top of any overload prior to optimisation (default= 5%). e.g. Initial loading of the element is 110%, with a 5% scanned threshold margin, the new maximum is 115% of the limit (e.g. PATL, TATL, etc).
The allowed value range is [0,100].""" ;
  cims:dataType cim:PerCent ;
  cims:multiplicity cims:M:0..1 ;
  cims:stereotype "NC", <http://iec.ch/TC57/NonStandard/UML#attribute> ;
  rdfs:domain nc:AssessedElementTimePoint .

nc:AssessedElementTimePoint.targetRemainingAvailableMarginJustification a rdf:Property ;
  rdfs:label "targetRemainingAvailableMarginJustification"@en ;
  rdfs:comment "Justification indicating the target remaining available margin. This justification is not intended for any application processing purpose, it should only be used for reporting." ;
  cims:dataType cim:String ;
  cims:multiplicity cims:M:0..1 ;
  cims:stereotype "NC", <http://iec.ch/TC57/NonStandard/UML#attribute> ;
  rdfs:domain nc:AssessedElementTimePoint .

nc:AssessedElementTimePoint.virtualPositiveMargin a rdf:Property ;
  rdfs:label "virtualPositiveMargin"@en ;
  rdfs:comment """A margin defined only for scanned AssessedElement (If AssessedElement.ScannedForRegion is present) in order to represent the influence of available remedial action which is not cross-border relevant remedial action.
The margin is modifying the limits used for the assessment whatever the limit it is (e.g. PATL, TATL).This symbolizes a remedial action that can be applied internally by the System Operator. It will be resolved by the System Operator and not by the optimization of remedial actions. The attribute shall be a positive value.
The allowed value range is [0,100].""" ;
  cims:dataType cim:PerCent ;
  cims:multiplicity cims:M:0..1 ;
  cims:stereotype "NC", <http://iec.ch/TC57/NonStandard/UML#attribute> ;
  rdfs:domain nc:AssessedElementTimePoint .

nc:AssessedElementWithContingency.GenericEnablingSchedule a rdf:Property ;
  rdfs:label "GenericEnablingSchedule"@en ;
  rdfs:comment "Enabling schedule which belongs to the assessed element with contingency." ;
  cims:AssociationUsed "No" ;
  cims:inverseRoleName nc:GenericEnablingSchedule.AssessedElementWithContingency ;
  cims:multiplicity cims:M:0..n ;
  cims:stereotype "NC" ;
  rdfs:domain nc:AssessedElementWithContingency ;
  rdfs:range nc:GenericEnablingSchedule .

nc:AssessedElementWithRemedialAction.GenericEnablingSchedule a rdf:Property ;
  rdfs:label "GenericEnablingSchedule"@en ;
  rdfs:comment "Enabling schedule which belongs to the assessed element with remedial action." ;
  cims:AssociationUsed "No" ;
  cims:inverseRoleName nc:GenericEnablingSchedule.AssessedElementWithRemedialAction ;
  cims:multiplicity cims:M:0..n ;
  cims:stereotype "NC" ;
  rdfs:domain nc:AssessedElementWithRemedialAction ;
  rdfs:range nc:GenericEnablingSchedule .

nc:AutomationFunction.GenericEnablingSchedule a rdf:Property ;
  rdfs:label "GenericEnablingSchedule"@en ;
  rdfs:comment "Enabling schedule associated to an automation function." ;
  cims:AssociationUsed "No" ;
  cims:inverseRoleName nc:GenericEnablingSchedule.AutomationFunction ;
  cims:multiplicity cims:M:0..n ;
  cims:stereotype "NC" ;
  rdfs:domain nc:AutomationFunction ;
  rdfs:range nc:GenericEnablingSchedule .

nc:AvailabilityTimePoint.GenericAvailabilitySchedule a rdf:Property ;
  rdfs:label "GenericAvailabilitySchedule"@en ;
  rdfs:comment "The availability schedule which belongs to the availability timepoint." ;
  cims:AssociationUsed "Yes" ;
  cims:inverseRoleName nc:GenericAvailableSchedule.AvailabilityTimePoint ;
  cims:multiplicity cims:M:1 ;
  cims:stereotype "NC" ;
  rdfs:domain nc:AvailabilityTimePoint ;
  rdfs:range nc:GenericAvailableSchedule .

nc:AvailabilityTimePoint.atTime a rdf:Property ;
  rdfs:label "atTime"@en ;
  rdfs:comment "The time the data is valid for." ;
  cims:dataType cim:DateTime ;
  cims:multiplicity cims:M:1..1 ;
  cims:stereotype "NC", <http://iec.ch/TC57/NonStandard/UML#attribute> ;
  rdfs:domain nc:AvailabilityTimePoint .

nc:AvailabilityTimePoint.available a rdf:Property ;
  rdfs:label "available"@en ;
  rdfs:comment "It identifies if the element is available. True means available, False means unavailable." ;
  cims:dataType cim:Boolean ;
  cims:multiplicity cims:M:1..1 ;
  cims:stereotype "NC", <http://iec.ch/TC57/NonStandard/UML#attribute> ;
  rdfs:domain nc:AvailabilityTimePoint .

nc:BaseRegularIntervalSchedule.HourPattern a rdf:Property ;
  rdfs:label "HourPattern"@en ;
  rdfs:comment "HourPattern that has base regular interval schedule." ;
  cims:AssociationUsed "Yes" ;
  cims:inverseRoleName nc:HourPattern.BaseRegularIntervalSchedule ;
  cims:multiplicity cims:M:0..1 ;
  cims:stereotype "NC" ;
  rdfs:domain nc:BaseRegularIntervalSchedule ;
  rdfs:range nc:HourPattern .

nc:BaseRegularIntervalSchedule.Season a rdf:Property ;
  rdfs:label "Season"@en ;
  rdfs:comment "Season associated with a base regular interval schedule." ;
  cims:AssociationUsed "Yes" ;
  cims:inverseRoleName nc:Season.BaseRegularIntervalSchedule ;
  cims:multiplicity cims:M:0..1 ;
  cims:stereotype "NC" ;
  rdfs:domain nc:BaseRegularIntervalSchedule ;
  rdfs:range cim:Season .

nc:BaseRegularIntervalSchedule.dayOfWeek a rdf:Property ;
  rdfs:label "dayOfWeek"@en ;
  rdfs:comment "Day of the week for which the schedule is valid for." ;
  cims:multiplicity cims:M:0..1 ;
  cims:stereotype "NC", <http://iec.ch/TC57/NonStandard/UML#attribute> ;
  rdfs:domain nc:BaseRegularIntervalSchedule ;
  rdfs:range nc:DayOfWeekKind .

nc:BaseRegularIntervalSchedule.intervalEndTime a rdf:Property ;
  rdfs:label "intervalEndTime"@en ;
  rdfs:comment "Interval end time for which the schedule is valid for." ;
  cims:dataType cim:DateTime ;
  cims:multiplicity cims:M:0..1 ;
  cims:stereotype "NC", <http://iec.ch/TC57/NonStandard/UML#attribute> ;
  rdfs:domain nc:BaseRegularIntervalSchedule .

nc:BaseRegularIntervalSchedule.intervalStartTime a rdf:Property ;
  rdfs:label "intervalStartTime"@en ;
  rdfs:comment "Interval start time for which the schedule is valid for." ;
  cims:dataType cim:DateTime ;
  cims:multiplicity cims:M:0..1 ;
  cims:stereotype "NC", <http://iec.ch/TC57/NonStandard/UML#attribute> ;
  rdfs:domain nc:BaseRegularIntervalSchedule .

nc:BaseTimeSeries.actionMethod a rdf:Property ;
  rdfs:label "actionMethod"@en ;
  rdfs:comment "Action method used to create the value. This is used for identification in the case where there is multiple time series for the same validity period and kind. " ;
  cims:dataType cim:String ;
  cims:multiplicity cims:M:0..1 ;
  cims:stereotype "NC", <http://iec.ch/TC57/NonStandard/UML#attribute> ;
  rdfs:domain nc:BaseTimeSeries .

nc:BaseTimeSeries.interpolationKind a rdf:Property ;
  rdfs:label "interpolationKind"@en ;
  rdfs:comment "Kind of interpolation done between time point." ;
  cims:multiplicity cims:M:1..1 ;
  cims:stereotype "NC", <http://iec.ch/TC57/NonStandard/UML#attribute> ;
  rdfs:domain nc:BaseTimeSeries ;
  rdfs:range nc:TimeSeriesInterpolationKind .

nc:BaseTimeSeries.timeSeriesKind a rdf:Property ;
  rdfs:label "timeSeriesKind"@en ;
  rdfs:comment "Kind of base time series." ;
  cims:multiplicity cims:M:0..1 ;
  cims:stereotype "NC", <http://iec.ch/TC57/NonStandard/UML#attribute> ;
  rdfs:domain nc:BaseTimeSeries ;
  rdfs:range nc:BaseTimeSeriesKind .

nc:Contingency.ContingencySchedule a rdf:Property ;
  rdfs:label "ContingencySchedule"@en ;
  rdfs:comment "Contingency schedule for a contingecy." ;
  cims:AssociationUsed "No" ;
  cims:inverseRoleName nc:ContingencySchedule.Contingency ;
  cims:multiplicity cims:M:0..n ;
  cims:stereotype "NC" ;
  rdfs:domain cim:Contingency ;
  rdfs:range nc:ContingencySchedule .

nc:ContingencySchedule.Contingency a rdf:Property ;
  rdfs:label "Contingency"@en ;
  rdfs:comment "Contingency which has a contingency schedule." ;
  cims:AssociationUsed "Yes" ;
  cims:inverseRoleName nc:Contingency.ContingencySchedule ;
  cims:multiplicity cims:M:1 ;
  cims:stereotype "NC" ;
  rdfs:domain nc:ContingencySchedule ;
  rdfs:range cim:Contingency .

nc:ContingencySchedule.ContingencyTimePoint a rdf:Property ;
  rdfs:label "ContingencyTimePoint"@en ;
  rdfs:comment "The time point that relates to this contingency schedule." ;
  cims:AssociationUsed "No" ;
  cims:inverseRoleName nc:ContingencyTimePoint.ContingencySchedule ;
  cims:multiplicity cims:M:1..n ;
  cims:stereotype "NC", <http://iec.ch/TC57/NonStandard/UML#ofAggregate> ;
  rdfs:domain nc:ContingencySchedule ;
  rdfs:range nc:ContingencyTimePoint .

nc:ContingencyTimePoint.ContingencySchedule a rdf:Property ;
  rdfs:label "ContingencySchedule"@en ;
  rdfs:comment "The contingency schedule that has this time point." ;
  cims:AssociationUsed "Yes" ;
  cims:inverseRoleName nc:ContingencySchedule.ContingencyTimePoint ;
  cims:multiplicity cims:M:1 ;
  cims:stereotype "NC" ;
  rdfs:domain nc:ContingencyTimePoint ;
  rdfs:range nc:ContingencySchedule .

nc:ContingencyTimePoint.atTime a rdf:Property ;
  rdfs:label "atTime"@en ;
  rdfs:comment "The time the data is valid for." ;
  cims:dataType cim:DateTime ;
  cims:multiplicity cims:M:1..1 ;
  cims:stereotype "NC", <http://iec.ch/TC57/NonStandard/UML#attribute> ;
  rdfs:domain nc:ContingencyTimePoint .

nc:ContingencyTimePoint.mustStudy a rdf:Property ;
  rdfs:label "mustStudy"@en ;
  rdfs:comment "Set true if must study this contingency." ;
  cims:dataType cim:Boolean ;
  cims:multiplicity cims:M:0..1 ;
  cims:stereotype "NC", <http://iec.ch/TC57/NonStandard/UML#attribute> ;
  rdfs:domain nc:ContingencyTimePoint .

nc:ContingencyTimePoint.probability a rdf:Property ;
  rdfs:label "probability"@en ;
  rdfs:comment "Probability of occurrence. The allowed value range is [0,100]." ;
  cims:dataType cim:PerCent ;
  cims:multiplicity cims:M:0..1 ;
  cims:stereotype "NC", <http://iec.ch/TC57/NonStandard/UML#attribute> ;
  rdfs:domain nc:ContingencyTimePoint .

nc:ContingencyWithRemedialAction.GenericEnablingSchedule a rdf:Property ;
  rdfs:label "GenericEnablingSchedule"@en ;
  rdfs:comment "Enabling schedule associated to a contingency with remedial action." ;
  cims:AssociationUsed "No" ;
  cims:inverseRoleName nc:GenericEnablingSchedule.ContingencyWithRemedialAction ;
  cims:multiplicity cims:M:0..n ;
  cims:stereotype "NC" ;
  rdfs:domain nc:ContingencyWithRemedialAction ;
  rdfs:range nc:GenericEnablingSchedule .

nc:CrossBorderRelevance.GenericEnablingSchedule a rdf:Property ;
  rdfs:label "GenericEnablingSchedule"@en ;
  rdfs:comment "Enabling schedule which belongs to the cross border relevant." ;
  cims:AssociationUsed "No" ;
  cims:inverseRoleName nc:GenericEnablingSchedule.CrossBorderRelevance ;
  cims:multiplicity cims:M:0..n ;
  cims:stereotype "NC" ;
  rdfs:domain nc:CrossBorderRelevance ;
  rdfs:range nc:GenericEnablingSchedule .

nc:DCPole.PowerShiftKeySchedule a rdf:Property ;
  rdfs:label "PowerShiftKeySchedule"@en ;
  rdfs:comment "The Power Shift Key schedule for a DCPole." ;
  cims:AssociationUsed "No" ;
  cims:inverseRoleName nc:PowerShiftKeySchedule.DCPole ;
  cims:multiplicity cims:M:0..n ;
  cims:stereotype "NC" ;
  rdfs:domain nc:DCPole ;
  rdfs:range nc:PowerShiftKeySchedule .

nc:EnablingTimePoint.GenericEnablingSchedule a rdf:Property ;
  rdfs:label "GenericEnablingSchedule"@en ;
  rdfs:comment "The enabling schedule which belongs to the enabling timepoint." ;
  cims:AssociationUsed "Yes" ;
  cims:inverseRoleName nc:GenericEnablingSchedule.EnablingTimePoint ;
  cims:multiplicity cims:M:1 ;
  cims:stereotype "NC" ;
  rdfs:domain nc:EnablingTimePoint ;
  rdfs:range nc:GenericEnablingSchedule .

nc:EnablingTimePoint.atTime a rdf:Property ;
  rdfs:label "atTime"@en ;
  rdfs:comment "The time the data is valid for." ;
  cims:dataType cim:DateTime ;
  cims:multiplicity cims:M:1..1 ;
  cims:stereotype "NC", <http://iec.ch/TC57/NonStandard/UML#attribute> ;
  rdfs:domain nc:EnablingTimePoint .

nc:EnablingTimePoint.enabled a rdf:Property ;
  rdfs:label "enabled"@en ;
  rdfs:comment "It identifies if the element is enabled. True means enabled, False means not enabled." ;
  cims:dataType cim:Boolean ;
  cims:multiplicity cims:M:1..1 ;
  cims:stereotype "NC", <http://iec.ch/TC57/NonStandard/UML#attribute> ;
  rdfs:domain nc:EnablingTimePoint .

nc:EnergyBlockOrder.GenericSequenceSchedule a rdf:Property ;
  rdfs:label "GenericSequenceSchedule"@en ;
  rdfs:comment "Generic sequence schedule associated with an energy block order." ;
  cims:AssociationUsed "No" ;
  cims:inverseRoleName nc:GenericSequenceSchedule.EnergyBlockOrder ;
  cims:multiplicity cims:M:0..n ;
  cims:stereotype "NC" ;
  rdfs:domain nc:EnergyBlockOrder ;
  rdfs:range nc:GenericSequenceSchedule .

nc:EnergyBlockOrder.PowerShiftKeySchedule a rdf:Property ;
  rdfs:label "PowerShiftKeySchedule"@en ;
  rdfs:comment "The Power Shift Key schedule for an energy block order." ;
  cims:AssociationUsed "No" ;
  cims:inverseRoleName nc:PowerShiftKeySchedule.EnergyBlockOrder ;
  cims:multiplicity cims:M:0..n ;
  cims:stereotype "NC" ;
  rdfs:domain nc:EnergyBlockOrder ;
  rdfs:range nc:PowerShiftKeySchedule .

nc:EnergyConsumer.PowerShiftKeySchedule a rdf:Property ;
  rdfs:label "PowerShiftKeySchedule"@en ;
  rdfs:comment "The Power Shift Key schedule for an Energy Consumer." ;
  cims:AssociationUsed "No" ;
  cims:inverseRoleName nc:PowerShiftKeySchedule.EnergyConsumer ;
  cims:multiplicity cims:M:0..n ;
  cims:stereotype "NC" ;
  rdfs:domain cim:EnergyConsumer ;
  rdfs:range nc:PowerShiftKeySchedule .

nc:EnergyGroup.PowerShiftKeySchedule a rdf:Property ;
  rdfs:label "PowerShiftKeySchedule"@en ;
  rdfs:comment "The Power Shift Key schedule for an energy group." ;
  cims:AssociationUsed "No" ;
  cims:inverseRoleName nc:PowerShiftKeySchedule.EnergyGroup ;
  cims:multiplicity cims:M:0..n ;
  cims:stereotype "NC" ;
  rdfs:domain nc:EnergyGroup ;
  rdfs:range nc:PowerShiftKeySchedule .

nc:EnergySource.PowerShiftKeySchedule a rdf:Property ;
  rdfs:label "PowerShiftKeySchedule"@en ;
  rdfs:comment "The power shift key schedule for an energy source." ;
  cims:AssociationUsed "No" ;
  cims:inverseRoleName nc:PowerShiftKeySchedule.EnergySource ;
  cims:multiplicity cims:M:0..n ;
  cims:stereotype "NC" ;
  rdfs:domain cim:EnergySource ;
  rdfs:range nc:PowerShiftKeySchedule .

nc:EquivalentInjection.PowerShiftKeySchedule a rdf:Property ;
  rdfs:label "PowerShiftKeySchedule"@en ;
  rdfs:comment "Power shift key schedule associated with an equivalent injection." ;
  cims:AssociationUsed "No" ;
  cims:inverseRoleName nc:PowerShiftKeySchedule.EquivalentInjection ;
  cims:multiplicity cims:M:0..n ;
  cims:stereotype "NC" ;
  rdfs:domain cim:EquivalentInjection ;
  rdfs:range nc:PowerShiftKeySchedule .

nc:ExternalNetworkInjection.PowerShiftKeySchedule a rdf:Property ;
  rdfs:label "PowerShiftKeySchedule"@en ;
  rdfs:comment "The power shift key schedule for an external network injection." ;
  cims:AssociationUsed "No" ;
  cims:inverseRoleName nc:PowerShiftKeySchedule.ExternalNetworkInjection ;
  cims:multiplicity cims:M:0..n ;
  cims:stereotype "NC" ;
  rdfs:domain cim:ExternalNetworkInjection ;
  rdfs:range nc:PowerShiftKeySchedule .

nc:FunctionBlock.GenericEnablingSchedule a rdf:Property ;
  rdfs:label "GenericEnablingSchedule"@en ;
  rdfs:comment "Enabling schedule associated to a function block." ;
  cims:AssociationUsed "No" ;
  cims:inverseRoleName nc:GenericEnablingSchedule.FunctionBlock ;
  cims:multiplicity cims:M:0..n ;
  cims:stereotype "NC" ;
  rdfs:domain nc:FunctionBlock ;
  rdfs:range nc:GenericEnablingSchedule .

nc:GeneratingUnit.PowerShiftKeySchedule a rdf:Property ;
  rdfs:label "PowerShiftKeySchedule"@en ;
  rdfs:comment "The Power Shift Key schedule for a Generating Unit." ;
  cims:AssociationUsed "No" ;
  cims:inverseRoleName nc:PowerShiftKeySchedule.GeneratingUnit ;
  cims:multiplicity cims:M:0..n ;
  cims:stereotype "NC" ;
  rdfs:domain cim:GeneratingUnit ;
  rdfs:range nc:PowerShiftKeySchedule .

nc:GeneratingUnit.UnitCostSchedule a rdf:Property ;
  rdfs:label "UnitCostSchedule"@en ;
  rdfs:comment "Unit cost schedule associated with a generating unit." ;
  cims:AssociationUsed "No" ;
  cims:inverseRoleName nc:UnitCostSchedule.GeneratingUnit ;
  cims:multiplicity cims:M:0..n ;
  cims:stereotype "NC" ;
  rdfs:domain cim:GeneratingUnit ;
  rdfs:range nc:UnitCostSchedule .

nc:GenericAvailableSchedule.AvailabilityTimePoint a rdf:Property ;
  rdfs:label "AvailabilityTimePoint"@en ;
  rdfs:comment "The availability timepoint for an available schedule." ;
  cims:AssociationUsed "No" ;
  cims:inverseRoleName nc:AvailabilityTimePoint.GenericAvailabilitySchedule ;
  cims:multiplicity cims:M:1..n ;
  cims:stereotype "NC", <http://iec.ch/TC57/NonStandard/UML#ofAggregate> ;
  rdfs:domain nc:GenericAvailableSchedule ;
  rdfs:range nc:AvailabilityTimePoint .

nc:GenericAvailableSchedule.RemedialAction a rdf:Property ;
  rdfs:label "RemedialAction"@en ;
  rdfs:comment "Remedial action which has available schedules." ;
  cims:AssociationUsed "Yes" ;
  cims:inverseRoleName nc:RemedialAction.GenericAvailableSchedule ;
  cims:multiplicity cims:M:0..1 ;
  cims:stereotype "NC" ;
  rdfs:domain nc:GenericAvailableSchedule ;
  rdfs:range nc:RemedialAction .

nc:GenericEnablingSchedule.AssessedElementWithContingency a rdf:Property ;
  rdfs:label "AssessedElementWithContingency"@en ;
  rdfs:comment "Assessed element with contingency that has enabling schedules." ;
  cims:AssociationUsed "Yes" ;
  cims:inverseRoleName nc:AssessedElementWithContingency.GenericEnablingSchedule ;
  cims:multiplicity cims:M:0..1 ;
  cims:stereotype "NC" ;
  rdfs:domain nc:GenericEnablingSchedule ;
  rdfs:range nc:AssessedElementWithContingency .

nc:GenericEnablingSchedule.AssessedElementWithRemedialAction a rdf:Property ;
  rdfs:label "AssessedElementWithRemedialAction"@en ;
  rdfs:comment "Assessed element with remedial action that has enabling schedules." ;
  cims:AssociationUsed "Yes" ;
  cims:inverseRoleName nc:AssessedElementWithRemedialAction.GenericEnablingSchedule ;
  cims:multiplicity cims:M:0..1 ;
  cims:stereotype "NC" ;
  rdfs:domain nc:GenericEnablingSchedule ;
  rdfs:range nc:AssessedElementWithRemedialAction .

nc:GenericEnablingSchedule.AutomationFunction a rdf:Property ;
  rdfs:label "AutomationFunction"@en ;
  rdfs:comment "Automation function which has enabling schedules." ;
  cims:AssociationUsed "Yes" ;
  cims:inverseRoleName nc:AutomationFunction.GenericEnablingSchedule ;
  cims:multiplicity cims:M:0..1 ;
  cims:stereotype "NC" ;
  rdfs:domain nc:GenericEnablingSchedule ;
  rdfs:range nc:AutomationFunction .

nc:GenericEnablingSchedule.ContingencyWithRemedialAction a rdf:Property ;
  rdfs:label "ContingencyWithRemedialAction"@en ;
  rdfs:comment "Contingency with remedial action which has enabling schedules." ;
  cims:AssociationUsed "Yes" ;
  cims:inverseRoleName nc:ContingencyWithRemedialAction.GenericEnablingSchedule ;
  cims:multiplicity cims:M:0..1 ;
  cims:stereotype "NC" ;
  rdfs:domain nc:GenericEnablingSchedule ;
  rdfs:range nc:ContingencyWithRemedialAction .

nc:GenericEnablingSchedule.CrossBorderRelevance a rdf:Property ;
  rdfs:label "CrossBorderRelevance"@en ;
  rdfs:comment "Cross border relevant that has enabling schedules." ;
  cims:AssociationUsed "Yes" ;
  cims:inverseRoleName nc:CrossBorderRelevance.GenericEnablingSchedule ;
  cims:multiplicity cims:M:0..1 ;
  cims:stereotype "NC" ;
  rdfs:domain nc:GenericEnablingSchedule ;
  rdfs:range nc:CrossBorderRelevance .

nc:GenericEnablingSchedule.EnablingTimePoint a rdf:Property ;
  rdfs:label "EnablingTimePoint"@en ;
  rdfs:comment "The enabling timepoint for a assessed element with enabling schedule." ;
  cims:AssociationUsed "No" ;
  cims:inverseRoleName nc:EnablingTimePoint.GenericEnablingSchedule ;
  cims:multiplicity cims:M:1..n ;
  cims:stereotype "NC", <http://iec.ch/TC57/NonStandard/UML#ofAggregate> ;
  rdfs:domain nc:GenericEnablingSchedule ;
  rdfs:range nc:EnablingTimePoint .

nc:GenericEnablingSchedule.FunctionBlock a rdf:Property ;
  rdfs:label "FunctionBlock"@en ;
  rdfs:comment "Function block which has enabling schedules." ;
  cims:AssociationUsed "Yes" ;
  cims:inverseRoleName nc:FunctionBlock.GenericEnablingSchedule ;
  cims:multiplicity cims:M:0..1 ;
  cims:stereotype "NC" ;
  rdfs:domain nc:GenericEnablingSchedule ;
  rdfs:range nc:FunctionBlock .

nc:GenericEnablingSchedule.PowerTransferCorridor a rdf:Property ;
  rdfs:label "PowerTransferCorridor"@en ;
  rdfs:comment "Power transfer corridor which has generic enabling schedules." ;
  cims:AssociationUsed "Yes" ;
  cims:inverseRoleName nc:PowerTransferCorridor.GenericEnablingSchedule ;
  cims:multiplicity cims:M:0..1 ;
  cims:stereotype "NC" ;
  rdfs:domain nc:GenericEnablingSchedule ;
  rdfs:range nc:PowerTransferCorridor .

nc:GenericEnablingSchedule.RemedialActionDependency a rdf:Property ;
  rdfs:label "RemedialActionDependency"@en ;
  rdfs:comment "Remedial action dependency which has enabling schedules." ;
  cims:AssociationUsed "Yes" ;
  cims:inverseRoleName nc:RemedialActionDependency.GenericEnablingSchedule ;
  cims:multiplicity cims:M:0..1 ;
  cims:stereotype "NC" ;
  rdfs:domain nc:GenericEnablingSchedule ;
  rdfs:range nc:RemedialActionDependency .

nc:GenericSequenceSchedule.EnergyBlockOrder a rdf:Property ;
  rdfs:label "EnergyBlockOrder"@en ;
  rdfs:comment "Energy block order which has generic sequence schedules." ;
  cims:AssociationUsed "Yes" ;
  cims:inverseRoleName nc:EnergyBlockOrder.GenericSequenceSchedule ;
  cims:multiplicity cims:M:0..1 ;
  cims:stereotype "NC" ;
  rdfs:domain nc:GenericSequenceSchedule ;
  rdfs:range nc:EnergyBlockOrder .

nc:GenericSequenceSchedule.SequenceTimePoint a rdf:Property ;
  rdfs:label "SequenceTimePoint"@en ;
  rdfs:comment "The sequence timepoint for a sequence schedule." ;
  cims:AssociationUsed "No" ;
  cims:inverseRoleName nc:SequenceTimePoint.GenericSequenceSchedule ;
  cims:multiplicity cims:M:1..n ;
  cims:stereotype "NC" ;
  rdfs:domain nc:GenericSequenceSchedule ;
  rdfs:range nc:SequenceTimePoint .

nc:GenericValueSchedule.GenericValueTimePoint a rdf:Property ;
  rdfs:label "GenericValueTimePoint"@en ;
  rdfs:comment "Value for the point in time." ;
  cims:AssociationUsed "No" ;
  cims:inverseRoleName nc:GenericValueTimePoint.GenericValueSchedule ;
  cims:multiplicity cims:M:1..n ;
  cims:stereotype "NC", <http://iec.ch/TC57/NonStandard/UML#ofAggregate> ;
  rdfs:domain nc:GenericValueSchedule ;
  rdfs:range nc:GenericValueTimePoint .

nc:GenericValueSchedule.RangeConstraint a rdf:Property ;
  rdfs:label "RangeConstraint"@en ;
  rdfs:comment "Range constraint for the generic value schedule." ;
  cims:AssociationUsed "Yes" ;
  cims:inverseRoleName nc:RangeConstraint.GenericValueSchedule ;
  cims:multiplicity cims:M:0..1 ;
  cims:stereotype "NC" ;
  rdfs:domain nc:GenericValueSchedule ;
  rdfs:range nc:RangeConstraint .

nc:GenericValueTimePoint.GenericValueSchedule a rdf:Property ;
  rdfs:label "GenericValueSchedule"@en ;
  rdfs:comment "Time series the time point values belongs to." ;
  cims:AssociationUsed "Yes" ;
  cims:inverseRoleName nc:GenericValueSchedule.GenericValueTimePoint ;
  cims:multiplicity cims:M:1 ;
  cims:stereotype "NC" ;
  rdfs:domain nc:GenericValueTimePoint ;
  rdfs:range nc:GenericValueSchedule .

nc:GenericValueTimePoint.atTime a rdf:Property ;
  rdfs:label "atTime"@en ;
  rdfs:comment "The time the data is valid for." ;
  cims:dataType cim:DateTime ;
  cims:multiplicity cims:M:1..1 ;
  cims:stereotype "NC", <http://iec.ch/TC57/NonStandard/UML#attribute> ;
  rdfs:domain nc:GenericValueTimePoint .

nc:GenericValueTimePoint.value a rdf:Property ;
  rdfs:label "value"@en ;
  rdfs:comment "The value at the time. The meaning of the value is defined by the derived type of the associated schedule. The value can be integer, float or boolean. In case of boolean 1 equals true and 0 equals false." ;
  cims:dataType cim:Float ;
  cims:multiplicity cims:M:1..1 ;
  cims:stereotype "NC", <http://iec.ch/TC57/NonStandard/UML#attribute> ;
  rdfs:domain nc:GenericValueTimePoint .

nc:GridStateAlteration.GridStateAlterationSchedule a rdf:Property ;
  rdfs:label "GridStateAlterationSchedule"@en ;
  rdfs:comment "Grid state alteration schedule associated with a grid state alteration." ;
  cims:AssociationUsed "No" ;
  cims:inverseRoleName nc:GridStateAlterationSchedule.GridStateAlteration ;
  cims:multiplicity cims:M:0..n ;
  cims:stereotype "NC" ;
  rdfs:domain nc:GridStateAlteration ;
  rdfs:range nc:GridStateAlterationSchedule .

nc:GridStateAlterationSchedule.GridStateAlteration a rdf:Property ;
  rdfs:label "GridStateAlteration"@en ;
  rdfs:comment "Grid state alteration which has grid state alteration schedules." ;
  cims:AssociationUsed "Yes" ;
  cims:inverseRoleName nc:GridStateAlteration.GridStateAlterationSchedule ;
  cims:multiplicity cims:M:1 ;
  cims:stereotype "NC" ;
  rdfs:domain nc:GridStateAlterationSchedule ;
  rdfs:range nc:GridStateAlteration .

nc:GridStateAlterationSchedule.GridStateAlterationTimePoint a rdf:Property ;
  rdfs:label "GridStateAlterationTimePoint"@en ;
  rdfs:comment "Grid state alteration time point that relates to this grid state alteration schedule." ;
  cims:AssociationUsed "No" ;
  cims:inverseRoleName nc:GridStateAlterationTimePoint.GridStateAlterationSchedule ;
  cims:multiplicity cims:M:1..n ;
  cims:stereotype "NC" ;
  rdfs:domain nc:GridStateAlterationSchedule ;
  rdfs:range nc:GridStateAlterationTimePoint .

nc:GridStateAlterationTimePoint.GridStateAlterationSchedule a rdf:Property ;
  rdfs:label "GridStateAlterationSchedule"@en ;
  rdfs:comment "Grid state alteration schedule that has time point." ;
  cims:AssociationUsed "Yes" ;
  cims:inverseRoleName nc:GridStateAlterationSchedule.GridStateAlterationTimePoint ;
  cims:multiplicity cims:M:1 ;
  cims:stereotype "NC" ;
  rdfs:domain nc:GridStateAlterationTimePoint ;
  rdfs:range nc:GridStateAlterationSchedule .

nc:GridStateAlterationTimePoint.atTime a rdf:Property ;
  rdfs:label "atTime"@en ;
  rdfs:comment "The time the data is valid for." ;
  cims:dataType cim:DateTime ;
  cims:multiplicity cims:M:1..1 ;
  cims:stereotype "NC", <http://iec.ch/TC57/NonStandard/UML#attribute> ;
  rdfs:domain nc:GridStateAlterationTimePoint .

nc:GridStateAlterationTimePoint.enabled a rdf:Property ;
  rdfs:label "enabled"@en ;
  rdfs:comment "The status of the GridStateAlteration set by an operation or by a signal resulting from a control action." ;
  cims:dataType cim:Boolean ;
  cims:multiplicity cims:M:0..1 ;
  cims:stereotype "NC", <http://iec.ch/TC57/NonStandard/UML#attribute> ;
  rdfs:domain nc:GridStateAlterationTimePoint .

nc:GridStateAlterationTimePoint.participationFactor a rdf:Property ;
  rdfs:label "participationFactor"@en ;
  rdfs:comment """Participation factor describing the entity part of the active power provided by a collection of entities (e.g. an active power forecast to a collection of entities is divided to each of the member entity according to the participation factor). Must be a positive value.
In the case of a sharing strategy, the distribution is following entities value (V) equals aggregated value (T) divided by sum of participation factors (PF), i.e. V=T/sum(PF). 
In the case of priority strategy, the item with the lowest number gets allocated energy first.
e.g. If 0 this grid alteration does not participate. The sum of all participation factors for all grid state alterations associated with same remedial action shall be equal to 100%.""" ;
  cims:dataType cim:PerCent ;
  cims:multiplicity cims:M:0..1 ;
  cims:stereotype "NC", <http://iec.ch/TC57/NonStandard/UML#attribute> ;
  rdfs:domain nc:GridStateAlterationTimePoint .

nc:GridStateIntensitySchedule.valueKind a rdf:Property ;
  rdfs:label "valueKind"@en ;
  rdfs:comment "The kind of value1 and value2 of the associated IrregularIntervalSchedule." ;
  cims:multiplicity cims:M:0..1 ;
  cims:stereotype "NC", <http://iec.ch/TC57/NonStandard/UML#attribute> ;
  rdfs:domain nc:GridStateIntensitySchedule ;
  rdfs:range nc:ValueOffsetKind .

nc:HourPattern.BaseRegularIntervalSchedule a rdf:Property ;
  rdfs:label "BaseRegularIntervalSchedule"@en ;
  rdfs:comment "Base regulat interval schedule which belongs to an hour pattern." ;
  cims:AssociationUsed "No" ;
  cims:inverseRoleName nc:BaseRegularIntervalSchedule.HourPattern ;
  cims:multiplicity cims:M:0..n ;
  cims:stereotype "NC" ;
  rdfs:domain nc:HourPattern ;
  rdfs:range nc:BaseRegularIntervalSchedule .

nc:HourPattern.HourPeriod a rdf:Property ;
  rdfs:label "HourPeriod"@en ;
  rdfs:comment "Hour period which belongs to an hour pattern." ;
  cims:AssociationUsed "No" ;
  cims:inverseRoleName nc:HourPeriod.HourPattern ;
  cims:multiplicity cims:M:1..n ;
  cims:stereotype "NC" ;
  rdfs:domain nc:HourPattern ;
  rdfs:range nc:HourPeriod .

nc:HourPattern.energyDemandKind a rdf:Property ;
  rdfs:label "energyDemandKind"@en ;
  rdfs:comment "Type of energy demand that the pattern is valid for." ;
  cims:multiplicity cims:M:0..1 ;
  cims:stereotype "NC", <http://iec.ch/TC57/NonStandard/UML#attribute> ;
  rdfs:domain nc:HourPattern ;
  rdfs:range nc:EnergyDemandKind .

nc:HourPattern.peakKind a rdf:Property ;
  rdfs:label "peakKind"@en ;
  rdfs:comment "Type of peak or intensity that the pattern is valid for." ;
  cims:multiplicity cims:M:0..1 ;
  cims:stereotype "NC", <http://iec.ch/TC57/NonStandard/UML#attribute> ;
  rdfs:domain nc:HourPattern ;
  rdfs:range nc:PeakKind .

nc:HourPeriod.HourPattern a rdf:Property ;
  rdfs:label "HourPattern"@en ;
  rdfs:comment "HourPattern which has some hour periods." ;
  cims:AssociationUsed "Yes" ;
  cims:inverseRoleName nc:HourPattern.HourPeriod ;
  cims:multiplicity cims:M:1 ;
  cims:stereotype "NC" ;
  rdfs:domain nc:HourPeriod ;
  rdfs:range nc:HourPattern .

nc:HourPeriod.endTime a rdf:Property ;
  rdfs:label "endTime"@en ;
  rdfs:comment "Time the period end and not including, e.g. 13:00 which means it does not include the time of 13:00 but 12:59." ;
  cims:dataType cim:Time ;
  cims:multiplicity cims:M:1..1 ;
  cims:stereotype "NC", <http://iec.ch/TC57/NonStandard/UML#attribute> ;
  rdfs:domain nc:HourPeriod .

nc:HourPeriod.mRID a rdf:Property ;
  rdfs:label "mRID"@en ;
  rdfs:comment """Master resource identifier issued by a model authority. The mRID is unique within an exchange context. Global uniqueness is easily achieved by using a UUID, as specified in RFC 4122, for the mRID. The use of UUID is strongly recommended.
For CIMXML data files in RDF syntax conforming to IEC 61970-552, the mRID is mapped to rdf:ID or rdf:about attributes that identify CIM object elements.""" ;
  cims:dataType cim:String ;
  cims:multiplicity cims:M:1..1 ;
  cims:stereotype "NC", <http://iec.ch/TC57/NonStandard/UML#attribute> ;
  rdfs:domain nc:HourPeriod .

nc:HourPeriod.startTime a rdf:Property ;
  rdfs:label "startTime"@en ;
  rdfs:comment "Time the period start and including, e.g. 12:00 which means it include the time of 12:00." ;
  cims:dataType cim:Time ;
  cims:multiplicity cims:M:1..1 ;
  cims:stereotype "NC", <http://iec.ch/TC57/NonStandard/UML#attribute> ;
  rdfs:domain nc:HourPeriod .

nc:HydroPump.PowerShiftKeySchedule a rdf:Property ;
  rdfs:label "PowerShiftKeySchedule"@en ;
  rdfs:comment "The Power Shift Key schedule for a Hydro Pump." ;
  cims:AssociationUsed "No" ;
  cims:inverseRoleName nc:PowerShiftKeySchedule.HydroPump ;
  cims:multiplicity cims:M:0..n ;
  cims:stereotype "NC" ;
  rdfs:domain cim:HydroPump ;
  rdfs:range nc:PowerShiftKeySchedule .

nc:InfeedLimit.InfeedLimitSchedule a rdf:Property ;
  rdfs:label "InfeedLimitSchedule"@en ;
  rdfs:comment "Infeed limit schedule associated with an infeed  limit." ;
  cims:AssociationUsed "No" ;
  cims:inverseRoleName nc:InfeedLimitSchedule.InfeedLimit ;
  cims:multiplicity cims:M:0..n ;
  cims:stereotype "NC" ;
  rdfs:domain nc:InfeedLimit ;
  rdfs:range nc:InfeedLimitSchedule .

nc:InfeedLimitSchedule.InfeedLimit a rdf:Property ;
  rdfs:label "InfeedLimit"@en ;
  rdfs:comment "Infeed limit which has infeed limit schedules." ;
  cims:AssociationUsed "Yes" ;
  cims:inverseRoleName nc:InfeedLimit.InfeedLimitSchedule ;
  cims:multiplicity cims:M:1 ;
  cims:stereotype "NC" ;
  rdfs:domain nc:InfeedLimitSchedule ;
  rdfs:range nc:InfeedLimit .

nc:InfeedLimitSchedule.InfeedLimitTimePoint a rdf:Property ;
  rdfs:label "InfeedLimitTimePoint"@en ;
  rdfs:comment "Infeed limit time point that relates to this voltage angle schedule." ;
  cims:AssociationUsed "No" ;
  cims:inverseRoleName nc:InfeedLimitTimePoint.InfeedLimitSchedule ;
  cims:multiplicity cims:M:1..n ;
  cims:stereotype "NC", <http://iec.ch/TC57/NonStandard/UML#ofAggregate> ;
  rdfs:domain nc:InfeedLimitSchedule ;
  rdfs:range nc:InfeedLimitTimePoint .

nc:InfeedLimitTimePoint.InfeedLimitSchedule a rdf:Property ;
  rdfs:label "InfeedLimitSchedule"@en ;
  rdfs:comment "Infeed limit schedule that has time point." ;
  cims:AssociationUsed "Yes" ;
  cims:inverseRoleName nc:InfeedLimitSchedule.InfeedLimitTimePoint ;
  cims:multiplicity cims:M:1 ;
  cims:stereotype "NC" ;
  rdfs:domain nc:InfeedLimitTimePoint ;
  rdfs:range nc:InfeedLimitSchedule .

nc:InfeedLimitTimePoint.atTime a rdf:Property ;
  rdfs:label "atTime"@en ;
  rdfs:comment "The time the data is valid for." ;
  cims:dataType cim:DateTime ;
  cims:multiplicity cims:M:1..1 ;
  cims:stereotype "NC", <http://iec.ch/TC57/NonStandard/UML#attribute> ;
  rdfs:domain nc:InfeedLimitTimePoint .

nc:InfeedLimitTimePoint.valueA a rdf:Property ;
  rdfs:label "valueA"@en ;
  rdfs:comment "Value of current limit. The attribute shall be a positive value or zero." ;
  cims:dataType cim:CurrentFlow ;
  cims:multiplicity cims:M:0..1 ;
  cims:stereotype "NC", <http://iec.ch/TC57/NonStandard/UML#attribute> ;
  rdfs:domain nc:InfeedLimitTimePoint .

nc:InfeedLimitTimePoint.valueW a rdf:Property ;
  rdfs:label "valueW"@en ;
  rdfs:comment "Value of active power limit. The attribute shall be a positive value or zero." ;
  cims:dataType cim:ActivePower ;
  cims:multiplicity cims:M:0..1 ;
  cims:stereotype "NC", <http://iec.ch/TC57/NonStandard/UML#attribute> ;
  rdfs:domain nc:InfeedLimitTimePoint .

nc:ParticipationFactorTimePoint.PowerShiftKeySchedule a rdf:Property ;
  rdfs:label "PowerShiftKeySchedule"@en ;
  rdfs:comment "The Power Shift Key schedule which belongs to the participation factor timepoint." ;
  cims:AssociationUsed "Yes" ;
  cims:inverseRoleName nc:PowerShiftKeySchedule.ParticipationFactorTimePoint ;
  cims:multiplicity cims:M:1 ;
  cims:stereotype "NC" ;
  rdfs:domain nc:ParticipationFactorTimePoint ;
  rdfs:range nc:PowerShiftKeySchedule .

nc:ParticipationFactorTimePoint.atTime a rdf:Property ;
  rdfs:label "atTime"@en ;
  rdfs:comment "The time the data is valid for." ;
  cims:dataType cim:DateTime ;
  cims:multiplicity cims:M:0..1 ;
  cims:stereotype "NC", <http://iec.ch/TC57/NonStandard/UML#attribute> ;
  rdfs:domain nc:ParticipationFactorTimePoint .

nc:ParticipationFactorTimePoint.participationFactor a rdf:Property ;
  rdfs:label "participationFactor"@en ;
  rdfs:comment """Participation factor describing the entity part of the active power provided by a collection of entities (e.g. an active power forecast to a collection of entities is divided to each of the member entity according to the participation factor). Must be a positive value.
In the case of a sharing strategy, the distribution is following entities value (V) equals aggregated value (T) divided by sum of participation factors (PF), i.e. V=T/sum(PF). 
In the case of priority strategy, the item with the lowest number gets allocated energy first.""" ;
  cims:dataType cim:Float ;
  cims:multiplicity cims:M:0..1 ;
  cims:stereotype "NC", <http://iec.ch/TC57/NonStandard/UML#attribute> ;
  rdfs:domain nc:ParticipationFactorTimePoint .

nc:PowerBidDependency.DependentPowerBidSchedule a rdf:Property ;
  rdfs:label "DependentPowerBidSchedule"@en ;
  rdfs:comment "Dependent power bid which has some dependent bid delays." ;
  cims:AssociationUsed "Yes" ;
  cims:inverseRoleName nc:PowerBidSchedule.DependentBidDelay ;
  cims:multiplicity cims:M:1 ;
  cims:stereotype "NC" ;
  rdfs:domain nc:PowerBidDependency ;
  rdfs:range nc:PowerBidSchedule .

nc:PowerBidDependency.MainPowerBidSchedule a rdf:Property ;
  rdfs:label "MainPowerBidSchedule"@en ;
  rdfs:comment "Main power bid which some dependent power bids." ;
  cims:AssociationUsed "Yes" ;
  cims:inverseRoleName nc:PowerBidSchedule.PowerBidDependency ;
  cims:multiplicity cims:M:1 ;
  cims:stereotype "NC" ;
  rdfs:domain nc:PowerBidDependency ;
  rdfs:range nc:PowerBidSchedule .

nc:PowerBidDependency.delay a rdf:Property ;
  rdfs:label "delay"@en ;
  rdfs:comment "Time delay between activation of the parents until the dependent offer will be available." ;
  cims:dataType cim:Duration ;
  cims:multiplicity cims:M:0..1 ;
  cims:stereotype "NC", <http://iec.ch/TC57/NonStandard/UML#attribute> ;
  rdfs:domain nc:PowerBidDependency .

nc:PowerBidDependency.kind a rdf:Property ;
  rdfs:label "kind"@en ;
  rdfs:comment "Type of dependency between bids." ;
  cims:multiplicity cims:M:1..1 ;
  cims:stereotype "NC", <http://iec.ch/TC57/NonStandard/UML#attribute> ;
  rdfs:domain nc:PowerBidDependency ;
  rdfs:range nc:PowerBidDependencyKind .

nc:PowerBidDependency.mRID a rdf:Property ;
  rdfs:label "mRID"@en ;
  rdfs:comment """Master resource identifier issued by a model authority. The mRID is unique within an exchange context. Global uniqueness is easily achieved by using a UUID, as specified in RFC 4122, for the mRID. The use of UUID is strongly recommended.
For CIMXML data files in RDF syntax conforming to IEC 61970-552, the mRID is mapped to rdf:ID or rdf:about attributes that identify CIM object elements.""" ;
  cims:dataType cim:String ;
  cims:multiplicity cims:M:1..1 ;
  cims:stereotype "NC", <http://iec.ch/TC57/NonStandard/UML#attribute> ;
  rdfs:domain nc:PowerBidDependency .

nc:PowerBidSchedule.DependentBidDelay a rdf:Property ;
  rdfs:label "DependentBidDelay"@en ;
  rdfs:comment "Bid delay which depends on a main power bid." ;
  cims:AssociationUsed "No" ;
  cims:inverseRoleName nc:PowerBidDependency.DependentPowerBidSchedule ;
  cims:multiplicity cims:M:0..n ;
  cims:stereotype "NC" ;
  rdfs:domain nc:PowerBidSchedule ;
  rdfs:range nc:PowerBidDependency .

nc:PowerBidSchedule.PowerBidDependency a rdf:Property ;
  rdfs:label "PowerBidDependency"@en ;
  rdfs:comment "Power bids which depends on main bid." ;
  cims:AssociationUsed "No" ;
  cims:inverseRoleName nc:PowerBidDependency.MainPowerBidSchedule ;
  cims:multiplicity cims:M:0..n ;
  cims:stereotype "NC", <http://iec.ch/TC57/NonStandard/UML#ofAggregate> ;
  rdfs:domain nc:PowerBidSchedule ;
  rdfs:range nc:PowerBidDependency .

nc:PowerBidSchedule.PowerBidScheduleTimePoint a rdf:Property ;
  rdfs:label "PowerBidScheduleTimePoint"@en ;
  rdfs:comment "Power bid schedule time points which belong to a power bid schedule." ;
  cims:AssociationUsed "No" ;
  cims:inverseRoleName nc:PowerBidScheduleTimePoint.PowerBidSchedule ;
  cims:multiplicity cims:M:1..n ;
  cims:stereotype "NC", <http://iec.ch/TC57/NonStandard/UML#ofAggregate> ;
  rdfs:domain nc:PowerBidSchedule ;
  rdfs:range nc:PowerBidScheduleTimePoint .

nc:PowerBidSchedule.PowerRemedialAction a rdf:Property ;
  rdfs:label "PowerRemedialAction"@en ;
  rdfs:comment "Power remedial action for which the bid is given." ;
  cims:AssociationUsed "Yes" ;
  cims:inverseRoleName nc:PowerRemedialAction.PowerBidSchedule ;
  cims:multiplicity cims:M:0..1 ;
  cims:stereotype "NC" ;
  rdfs:domain nc:PowerBidSchedule ;
  rdfs:range nc:PowerRemedialAction .

nc:PowerBidSchedule.PowerShiftKeyDistribution a rdf:Property ;
  rdfs:label "PowerShiftKeyDistribution"@en ;
  rdfs:comment "Distribution of the power bid amongst the power shift keys." ;
  cims:AssociationUsed "No" ;
  cims:inverseRoleName nc:PowerShiftKeyDistribution.PowerBidSchedule ;
  cims:multiplicity cims:M:0..n ;
  cims:stereotype "NC" ;
  rdfs:domain nc:PowerBidSchedule ;
  rdfs:range nc:PowerShiftKeyDistribution .

nc:PowerBidSchedule.ScheduleResource a rdf:Property ;
  rdfs:label "ScheduleResource"@en ;
  rdfs:comment "Schedule resource which has several power bid schedules." ;
  cims:AssociationUsed "No" ;
  cims:inverseRoleName nc:ScheduleResource.PowerBidSchedule ;
  cims:multiplicity cims:M:0..1 ;
  cims:stereotype "NC" ;
  rdfs:domain nc:PowerBidSchedule ;
  rdfs:range nc:ScheduleResource .

nc:PowerBidSchedule.activationCost a rdf:Property ;
  rdfs:label "activationCost"@en ;
  rdfs:comment "Cost to activate the bid." ;
  cims:dataType cim:Decimal ;
  cims:multiplicity cims:M:0..1 ;
  cims:stereotype "NC", <http://iec.ch/TC57/NonStandard/UML#attribute> ;
  rdfs:domain nc:PowerBidSchedule .

nc:PowerBidSchedule.currency a rdf:Property ;
  rdfs:label "currency"@en ;
  rdfs:comment "Currency of the bid." ;
  cims:multiplicity cims:M:0..1 ;
  cims:stereotype "NC", <http://iec.ch/TC57/NonStandard/UML#attribute> ;
  rdfs:domain nc:PowerBidSchedule ;
  rdfs:range cim:Currency .

nc:PowerBidSchedule.direction a rdf:Property ;
  rdfs:label "direction"@en ;
  rdfs:comment "Define the direction of the energy adjustment." ;
  cims:multiplicity cims:M:0..1 ;
  cims:stereotype "NC", <http://iec.ch/TC57/NonStandard/UML#attribute> ;
  rdfs:domain nc:PowerBidSchedule ;
  rdfs:range nc:BidDirectionKind .

nc:PowerBidSchedule.isFixed a rdf:Property ;
  rdfs:label "isFixed"@en ;
  rdfs:comment "Indicates if the power bid schedule is fixed, meaning that all the different power bid schedule values need to be taken without changes. e.g. It is a take-it-or-leave-it bid offer." ;
  cims:dataType cim:Boolean ;
  cims:multiplicity cims:M:0..1 ;
  cims:stereotype "NC", <http://iec.ch/TC57/NonStandard/UML#attribute> ;
  rdfs:domain nc:PowerBidSchedule .

nc:PowerBidSchedule.isOffer a rdf:Property ;
  rdfs:label "isOffer"@en ;
  rdfs:comment "Indicates if the power bid is an offer or not. True, means that the bid is an offer. False, means that the bid is not an offer." ;
  cims:dataType cim:Boolean ;
  cims:multiplicity cims:M:0..1 ;
  cims:stereotype "NC", <http://iec.ch/TC57/NonStandard/UML#attribute> ;
  rdfs:domain nc:PowerBidSchedule .

nc:PowerBidSchedule.leadTime a rdf:Property ;
  rdfs:label "leadTime"@en ;
  rdfs:comment "Time it takes for the bid to be called upon until it is active." ;
  cims:dataType cim:Duration ;
  cims:multiplicity cims:M:0..1 ;
  cims:stereotype "NC", <http://iec.ch/TC57/NonStandard/UML#attribute> ;
  rdfs:domain nc:PowerBidSchedule .

nc:PowerBidSchedule.maxRampDownP a rdf:Property ;
  rdfs:label "maxRampDownP"@en ;
  rdfs:comment "Maximum decrease of the active power change from one time point to the next." ;
  cims:dataType cim:ActivePower ;
  cims:multiplicity cims:M:0..1 ;
  cims:stereotype "NC", <http://iec.ch/TC57/NonStandard/UML#attribute> ;
  rdfs:domain nc:PowerBidSchedule .

nc:PowerBidSchedule.maxRampUpP a rdf:Property ;
  rdfs:label "maxRampUpP"@en ;
  rdfs:comment "Maximum increase of the active power change from one time point to the next." ;
  cims:dataType cim:ActivePower ;
  cims:multiplicity cims:M:0..1 ;
  cims:stereotype "NC", <http://iec.ch/TC57/NonStandard/UML#attribute> ;
  rdfs:domain nc:PowerBidSchedule .

nc:PowerBidSchedule.maximumUptime a rdf:Property ;
  rdfs:label "maximumUptime"@en ;
  rdfs:comment "Maximum duration the action needs to be remain active after startup. " ;
  cims:dataType cim:Duration ;
  cims:multiplicity cims:M:0..1 ;
  cims:stereotype "NC", <http://iec.ch/TC57/NonStandard/UML#attribute> ;
  rdfs:domain nc:PowerBidSchedule .

nc:PowerBidSchedule.minimumOffTime a rdf:Property ;
  rdfs:label "minimumOffTime"@en ;
  rdfs:comment "Minimum time interval between activation of the bid involving startup and shutdown. This value overrides any value on the unit." ;
  cims:dataType cim:Duration ;
  cims:multiplicity cims:M:0..1 ;
  cims:stereotype "NC", <http://iec.ch/TC57/NonStandard/UML#attribute> ;
  rdfs:domain nc:PowerBidSchedule .

nc:PowerBidSchedule.minimumUptime a rdf:Property ;
  rdfs:label "minimumUptime"@en ;
  rdfs:comment "Minimum duration the action needs to be remain active after startup. " ;
  cims:dataType cim:Duration ;
  cims:multiplicity cims:M:0..1 ;
  cims:stereotype "NC", <http://iec.ch/TC57/NonStandard/UML#attribute> ;
  rdfs:domain nc:PowerBidSchedule .

nc:PowerBidSchedule.priority a rdf:Property ;
  rdfs:label "priority"@en ;
  rdfs:comment "The numeric local priority given to a bid. Lower numeric values will have higher priority." ;
  cims:dataType cim:Integer ;
  cims:multiplicity cims:M:0..1 ;
  cims:stereotype "NC", <http://iec.ch/TC57/NonStandard/UML#attribute> ;
  rdfs:domain nc:PowerBidSchedule .

nc:PowerBidSchedule.shutdownCost a rdf:Property ;
  rdfs:label "shutdownCost"@en ;
  rdfs:comment "Total shutdown cost incurred for all the units involved in the bid. This overrides any cost on the specific unit." ;
  cims:dataType cim:Decimal ;
  cims:multiplicity cims:M:0..1 ;
  cims:stereotype "NC", <http://iec.ch/TC57/NonStandard/UML#attribute> ;
  rdfs:domain nc:PowerBidSchedule .

nc:PowerBidSchedule.totalMaximumEnergy a rdf:Property ;
  rdfs:label "totalMaximumEnergy"@en ;
  rdfs:comment "Maximum total energy that can be activated by the bid." ;
  cims:dataType cim:RealEnergy ;
  cims:multiplicity cims:M:0..1 ;
  cims:stereotype "NC", <http://iec.ch/TC57/NonStandard/UML#attribute> ;
  rdfs:domain nc:PowerBidSchedule .

nc:PowerBidSchedule.totalMinimumEnergy a rdf:Property ;
  rdfs:label "totalMinimumEnergy"@en ;
  rdfs:comment "Minimum total energy that has to be activated by the bid." ;
  cims:dataType cim:RealEnergy ;
  cims:multiplicity cims:M:0..1 ;
  cims:stereotype "NC", <http://iec.ch/TC57/NonStandard/UML#attribute> ;
  rdfs:domain nc:PowerBidSchedule .

nc:PowerBidScheduleTimePoint.PowerBidSchedule a rdf:Property ;
  rdfs:label "PowerBidSchedule"@en ;
  rdfs:comment "Power bid schedule that has many power bid schedule time points." ;
  cims:AssociationUsed "Yes" ;
  cims:inverseRoleName nc:PowerBidSchedule.PowerBidScheduleTimePoint ;
  cims:multiplicity cims:M:1 ;
  cims:stereotype "NC" ;
  rdfs:domain nc:PowerBidScheduleTimePoint ;
  rdfs:range nc:PowerBidSchedule .

nc:PowerBidScheduleTimePoint.atTime a rdf:Property ;
  rdfs:label "atTime"@en ;
  rdfs:comment "The time the data is valid for." ;
  cims:dataType cim:DateTime ;
  cims:multiplicity cims:M:1..1 ;
  cims:stereotype "NC", <http://iec.ch/TC57/NonStandard/UML#attribute> ;
  rdfs:domain nc:PowerBidScheduleTimePoint .

nc:PowerBidScheduleTimePoint.minimumActivationP a rdf:Property ;
  rdfs:label "minimumActivationP"@en ;
  rdfs:comment "Minimum active power given in the time point." ;
  cims:dataType cim:ActivePower ;
  cims:multiplicity cims:M:0..1 ;
  cims:stereotype "NC", <http://iec.ch/TC57/NonStandard/UML#attribute> ;
  rdfs:domain nc:PowerBidScheduleTimePoint .

nc:PowerBidScheduleTimePoint.p a rdf:Property ;
  rdfs:label "p"@en ;
  rdfs:comment "Active power given in the time point." ;
  cims:dataType cim:ActivePower ;
  cims:multiplicity cims:M:1..1 ;
  cims:stereotype "NC", <http://iec.ch/TC57/NonStandard/UML#attribute> ;
  rdfs:domain nc:PowerBidScheduleTimePoint .

nc:PowerBidScheduleTimePoint.price a rdf:Property ;
  rdfs:label "price"@en ;
  rdfs:comment "Quantity given in the time points." ;
  cims:dataType cim:Decimal ;
  cims:multiplicity cims:M:0..1 ;
  cims:stereotype "NC", <http://iec.ch/TC57/NonStandard/UML#attribute> ;
  rdfs:domain nc:PowerBidScheduleTimePoint .

nc:PowerBidScheduleTimePoint.reservePrice a rdf:Property ;
  rdfs:label "reservePrice"@en ;
  rdfs:comment "Price for reserving the step increment active power." ;
  cims:dataType cim:Decimal ;
  cims:multiplicity cims:M:0..1 ;
  cims:stereotype "NC", <http://iec.ch/TC57/NonStandard/UML#attribute> ;
  rdfs:domain nc:PowerBidScheduleTimePoint .

nc:PowerBidScheduleTimePoint.stepIncrementP a rdf:Property ;
  rdfs:label "stepIncrementP"@en ;
  rdfs:comment "The minimum increment that can be applied for an increase in an activation request." ;
  cims:dataType cim:ActivePower ;
  cims:multiplicity cims:M:0..1 ;
  cims:stereotype "NC", <http://iec.ch/TC57/NonStandard/UML#attribute> ;
  rdfs:domain nc:PowerBidScheduleTimePoint .

nc:PowerElectronicsUnit.PowerShiftKeySchedule a rdf:Property ;
  rdfs:label "PowerShiftKeySchedule"@en ;
  rdfs:comment "The Power Shift Key schedule for a Power Electronics Unit." ;
  cims:AssociationUsed "No" ;
  cims:inverseRoleName nc:PowerShiftKeySchedule.PowerElectronicsUnit ;
  cims:multiplicity cims:M:0..n ;
  cims:stereotype "NC" ;
  rdfs:domain cim:PowerElectronicsUnit ;
  rdfs:range nc:PowerShiftKeySchedule .

nc:PowerRemedialAction.PowerBidSchedule a rdf:Property ;
  rdfs:label "PowerBidSchedule"@en ;
  rdfs:comment "Power bid schedule addressing the power remedial action." ;
  cims:AssociationUsed "No" ;
  cims:inverseRoleName nc:PowerBidSchedule.PowerRemedialAction ;
  cims:multiplicity cims:M:0..n ;
  cims:stereotype "NC" ;
  rdfs:domain nc:PowerRemedialAction ;
  rdfs:range nc:PowerBidSchedule .

nc:PowerRemedialAction.PowerRemedialActionSchedule a rdf:Property ;
  rdfs:label "PowerRemedialActionSchedule"@en ;
  rdfs:comment "Power remedial action schedule which has a power remedial action." ;
  cims:AssociationUsed "No" ;
  cims:inverseRoleName nc:PowerRemedialActionSchedule.PowerRemedialAction ;
  cims:multiplicity cims:M:0..n ;
  cims:stereotype "NC" ;
  rdfs:domain nc:PowerRemedialAction ;
  rdfs:range nc:PowerRemedialActionSchedule .

nc:PowerRemedialActionSchedule.PowerRemedialAction a rdf:Property ;
  rdfs:label "PowerRemedialAction"@en ;
  rdfs:comment "Power remedial action for the power remedial action schedule." ;
  cims:AssociationUsed "Yes" ;
  cims:inverseRoleName nc:PowerRemedialAction.PowerRemedialActionSchedule ;
  cims:multiplicity cims:M:1 ;
  cims:stereotype "NC" ;
  rdfs:domain nc:PowerRemedialActionSchedule ;
  rdfs:range nc:PowerRemedialAction .

nc:PowerRemedialActionSchedule.PowerRemedialActionTimePoint a rdf:Property ;
  rdfs:label "PowerRemedialActionTimePoint"@en ;
  rdfs:comment "The time point that relates to this power remedial action schedule." ;
  cims:AssociationUsed "No" ;
  cims:inverseRoleName nc:PowerRemedialActionTimePoint.PowerRemedialActionSchedule ;
  cims:multiplicity cims:M:1..n ;
  cims:stereotype "NC", <http://iec.ch/TC57/NonStandard/UML#ofAggregate> ;
  rdfs:domain nc:PowerRemedialActionSchedule ;
  rdfs:range nc:PowerRemedialActionTimePoint .

nc:PowerRemedialActionTimePoint.PowerRemedialActionSchedule a rdf:Property ;
  rdfs:label "PowerRemedialActionSchedule"@en ;
  rdfs:comment "The power remedial action schedule that has this time point." ;
  cims:AssociationUsed "Yes" ;
  cims:inverseRoleName nc:PowerRemedialActionSchedule.PowerRemedialActionTimePoint ;
  cims:multiplicity cims:M:1 ;
  cims:stereotype "NC" ;
  rdfs:domain nc:PowerRemedialActionTimePoint ;
  rdfs:range nc:PowerRemedialActionSchedule .

nc:PowerRemedialActionTimePoint.atTime a rdf:Property ;
  rdfs:label "atTime"@en ;
  rdfs:comment "The time the data is valid for." ;
  cims:dataType cim:DateTime ;
  cims:multiplicity cims:M:1..1 ;
  cims:stereotype "NC", <http://iec.ch/TC57/NonStandard/UML#attribute> ;
  rdfs:domain nc:PowerRemedialActionTimePoint .

nc:PowerRemedialActionTimePoint.maxRegulatingDown a rdf:Property ;
  rdfs:label "maxRegulatingDown"@en ;
  rdfs:comment "Maximum net amount of active power that the remedial action can regulate down." ;
  cims:dataType cim:ActivePower ;
  cims:multiplicity cims:M:0..1 ;
  cims:stereotype "NC", <http://iec.ch/TC57/NonStandard/UML#attribute> ;
  rdfs:domain nc:PowerRemedialActionTimePoint .

nc:PowerRemedialActionTimePoint.maxRegulatingUp a rdf:Property ;
  rdfs:label "maxRegulatingUp"@en ;
  rdfs:comment "Maximum net amount of active power that the remedial action can regulate up." ;
  cims:dataType cim:ActivePower ;
  cims:multiplicity cims:M:0..1 ;
  cims:stereotype "NC", <http://iec.ch/TC57/NonStandard/UML#attribute> ;
  rdfs:domain nc:PowerRemedialActionTimePoint .

nc:PowerShiftKeyDistribution.PowerBidSchedule a rdf:Property ;
  rdfs:label "PowerBidSchedule"@en ;
  rdfs:comment "Power bid schedule for the given distribution." ;
  cims:AssociationUsed "Yes" ;
  cims:inverseRoleName nc:PowerBidSchedule.PowerShiftKeyDistribution ;
  cims:multiplicity cims:M:0..1 ;
  cims:stereotype "NC" ;
  rdfs:domain nc:PowerShiftKeyDistribution ;
  rdfs:range nc:PowerBidSchedule .

nc:PowerShiftKeyDistribution.PowerShiftKeySchedule a rdf:Property ;
  rdfs:label "PowerShiftKeySchedule"@en ;
  rdfs:comment "Power Shift Key schedule in power shift key distribution." ;
  cims:AssociationUsed "Yes" ;
  cims:inverseRoleName nc:PowerShiftKeySchedule.PowerShiftKeyDistribution ;
  cims:multiplicity cims:M:1 ;
  cims:stereotype "NC" ;
  rdfs:domain nc:PowerShiftKeyDistribution ;
  rdfs:range nc:PowerShiftKeySchedule .

nc:PowerShiftKeyDistribution.PowerShiftKeyStrategy a rdf:Property ;
  rdfs:label "PowerShiftKeyStrategy"@en ;
  rdfs:comment "Power Shift Key Strategy which has a Power Shift Key Distribution." ;
  cims:AssociationUsed "Yes" ;
  cims:inverseRoleName nc:PowerShiftKeyStrategy.PowerShiftKeyDistribution ;
  cims:multiplicity cims:M:0..1 ;
  cims:stereotype "NC" ;
  rdfs:domain nc:PowerShiftKeyDistribution ;
  rdfs:range nc:PowerShiftKeyStrategy .

nc:PowerShiftKeySchedule.DCPole a rdf:Property ;
  rdfs:label "DCPole"@en ;
  rdfs:comment "A DC Pole which has a Power Shift Key Schedule." ;
  cims:AssociationUsed "Yes" ;
  cims:inverseRoleName nc:DCPole.PowerShiftKeySchedule ;
  cims:multiplicity cims:M:0..1 ;
  cims:stereotype "NC" ;
  rdfs:domain nc:PowerShiftKeySchedule ;
  rdfs:range nc:DCPole .

nc:PowerShiftKeySchedule.EnergyBlockOrder a rdf:Property ;
  rdfs:label "EnergyBlockOrder"@en ;
  rdfs:comment "An energy block order which has a Power Shift Key Schedule." ;
  cims:AssociationUsed "Yes" ;
  cims:inverseRoleName nc:EnergyBlockOrder.PowerShiftKeySchedule ;
  cims:multiplicity cims:M:0..1 ;
  cims:stereotype "NC" ;
  rdfs:domain nc:PowerShiftKeySchedule ;
  rdfs:range nc:EnergyBlockOrder .

nc:PowerShiftKeySchedule.EnergyConsumer a rdf:Property ;
  rdfs:label "EnergyConsumer"@en ;
  rdfs:comment "The EnergyConsumer that has a Power Shift Key schedule." ;
  cims:AssociationUsed "Yes" ;
  cims:inverseRoleName nc:EnergyConsumer.PowerShiftKeySchedule ;
  cims:multiplicity cims:M:0..1 ;
  cims:stereotype "NC" ;
  rdfs:domain nc:PowerShiftKeySchedule ;
  rdfs:range cim:EnergyConsumer .

nc:PowerShiftKeySchedule.EnergyGroup a rdf:Property ;
  rdfs:label "EnergyGroup"@en ;
  rdfs:comment "The energy group which has a Power Shift Key Schedule." ;
  cims:AssociationUsed "Yes" ;
  cims:inverseRoleName nc:EnergyGroup.PowerShiftKeySchedule ;
  cims:multiplicity cims:M:0..1 ;
  cims:stereotype "NC" ;
  rdfs:domain nc:PowerShiftKeySchedule ;
  rdfs:range nc:EnergyGroup .

nc:PowerShiftKeySchedule.EnergySource a rdf:Property ;
  rdfs:label "EnergySource"@en ;
  rdfs:comment "The energy source which has a power shift key schedule. The renewable resources should be modelled as PowerElecronicsUnit." ;
  cims:AssociationUsed "Yes" ;
  cims:inverseRoleName nc:EnergySource.PowerShiftKeySchedule ;
  cims:multiplicity cims:M:0..1 ;
  cims:stereotype "NC" ;
  rdfs:domain nc:PowerShiftKeySchedule ;
  rdfs:range cim:EnergySource .

nc:PowerShiftKeySchedule.EquivalentInjection a rdf:Property ;
  rdfs:label "EquivalentInjection"@en ;
  rdfs:comment "Equivalent injection which is part of a powoer shift key schedule." ;
  cims:AssociationUsed "Yes" ;
  cims:inverseRoleName nc:EquivalentInjection.PowerShiftKeySchedule ;
  cims:multiplicity cims:M:0..1 ;
  cims:stereotype "NC" ;
  rdfs:domain nc:PowerShiftKeySchedule ;
  rdfs:range cim:EquivalentInjection .

nc:PowerShiftKeySchedule.ExternalNetworkInjection a rdf:Property ;
  rdfs:label "ExternalNetworkInjection"@en ;
  rdfs:comment "The energy source which has a power shift key schedule." ;
  cims:AssociationUsed "Yes" ;
  cims:inverseRoleName nc:ExternalNetworkInjection.PowerShiftKeySchedule ;
  cims:multiplicity cims:M:0..1 ;
  cims:stereotype "NC" ;
  rdfs:domain nc:PowerShiftKeySchedule ;
  rdfs:range cim:ExternalNetworkInjection .

nc:PowerShiftKeySchedule.GeneratingUnit a rdf:Property ;
  rdfs:label "GeneratingUnit"@en ;
  rdfs:comment "The Generating Unit which has a Power Shift Key Schedule." ;
  cims:AssociationUsed "Yes" ;
  cims:inverseRoleName nc:GeneratingUnit.PowerShiftKeySchedule ;
  cims:multiplicity cims:M:0..1 ;
  cims:stereotype "NC" ;
  rdfs:domain nc:PowerShiftKeySchedule ;
  rdfs:range cim:GeneratingUnit .

nc:PowerShiftKeySchedule.HydroPump a rdf:Property ;
  rdfs:label "HydroPump"@en ;
  rdfs:comment "The Hydro Pump which has a Power Shift Key schedule." ;
  cims:AssociationUsed "Yes" ;
  cims:inverseRoleName nc:HydroPump.PowerShiftKeySchedule ;
  cims:multiplicity cims:M:0..1 ;
  cims:stereotype "NC" ;
  rdfs:domain nc:PowerShiftKeySchedule ;
  rdfs:range cim:HydroPump .

nc:PowerShiftKeySchedule.ParticipationFactorTimePoint a rdf:Property ;
  rdfs:label "ParticipationFactorTimePoint"@en ;
  rdfs:comment "The participation factor timepoint for a Power Shift Key schedule." ;
  cims:AssociationUsed "No" ;
  cims:inverseRoleName nc:ParticipationFactorTimePoint.PowerShiftKeySchedule ;
  cims:multiplicity cims:M:0..n ;
  cims:stereotype "NC", <http://iec.ch/TC57/NonStandard/UML#ofAggregate> ;
  rdfs:domain nc:PowerShiftKeySchedule ;
  rdfs:range nc:ParticipationFactorTimePoint .

nc:PowerShiftKeySchedule.PowerElectronicsUnit a rdf:Property ;
  rdfs:label "PowerElectronicsUnit"@en ;
  rdfs:comment "The Power Electronics Unit which has a  Power Shift Key schedule." ;
  cims:AssociationUsed "Yes" ;
  cims:inverseRoleName nc:PowerElectronicsUnit.PowerShiftKeySchedule ;
  cims:multiplicity cims:M:0..1 ;
  cims:stereotype "NC" ;
  rdfs:domain nc:PowerShiftKeySchedule ;
  rdfs:range cim:PowerElectronicsUnit .

nc:PowerShiftKeySchedule.PowerShiftKeyDistribution a rdf:Property ;
  rdfs:label "PowerShiftKeyDistribution"@en ;
  rdfs:comment "Power Shift Key distribution for the Power Shift Key schedule." ;
  cims:AssociationUsed "No" ;
  cims:inverseRoleName nc:PowerShiftKeyDistribution.PowerShiftKeySchedule ;
  cims:multiplicity cims:M:0..1 ;
  cims:stereotype "NC" ;
  rdfs:domain nc:PowerShiftKeySchedule ;
  rdfs:range nc:PowerShiftKeyDistribution .

nc:PowerShiftKeySchedule.ScheduleResource a rdf:Property ;
  rdfs:label "ScheduleResource"@en ;
  rdfs:comment "The Schedule Resource which has a  Power Shift Key schedule." ;
  cims:AssociationUsed "Yes" ;
  cims:inverseRoleName nc:ScheduleResource.PowerShiftKeySchedule ;
  cims:multiplicity cims:M:0..1 ;
  cims:stereotype "NC" ;
  rdfs:domain nc:PowerShiftKeySchedule ;
  rdfs:range nc:ScheduleResource .

nc:PowerShiftKeyStrategy.PowerShiftKeyDistribution a rdf:Property ;
  rdfs:label "PowerShiftKeyDistribution"@en ;
  rdfs:comment "Power Shift Key Distribution associated to this power shift key strategy." ;
  cims:AssociationUsed "No" ;
  cims:inverseRoleName nc:PowerShiftKeyDistribution.PowerShiftKeyStrategy ;
  cims:multiplicity cims:M:0..n ;
  cims:stereotype "NC" ;
  rdfs:domain nc:PowerShiftKeyStrategy ;
  rdfs:range nc:PowerShiftKeyDistribution .

nc:PowerTransferCorridor.GenericEnablingSchedule a rdf:Property ;
  rdfs:label "GenericEnablingSchedule"@en ;
  rdfs:comment "Generic enabling schedule associated with a power transfer corridor." ;
  cims:AssociationUsed "No" ;
  cims:inverseRoleName nc:GenericEnablingSchedule.PowerTransferCorridor ;
  cims:multiplicity cims:M:0..n ;
  cims:stereotype "NC" ;
  rdfs:domain nc:PowerTransferCorridor ;
  rdfs:range nc:GenericEnablingSchedule .

nc:RangeConstraint.GenericValueSchedule a rdf:Property ;
  rdfs:label "GenericValueSchedule"@en ;
  rdfs:comment "Generic value schedule which has a range constraint." ;
  cims:AssociationUsed "No" ;
  cims:inverseRoleName nc:GenericValueSchedule.RangeConstraint ;
  cims:multiplicity cims:M:0..n ;
  cims:stereotype "NC" ;
  rdfs:domain nc:RangeConstraint ;
  rdfs:range nc:GenericValueSchedule .

nc:RemedialAction.GenericAvailableSchedule a rdf:Property ;
  rdfs:label "GenericAvailableSchedule"@en ;
  rdfs:comment "Available schedule associated to a remedial action." ;
  cims:AssociationUsed "No" ;
  cims:inverseRoleName nc:GenericAvailableSchedule.RemedialAction ;
  cims:multiplicity cims:M:0..n ;
  cims:stereotype "NC" ;
  rdfs:domain nc:RemedialAction ;
  rdfs:range nc:GenericAvailableSchedule .

nc:RemedialActionDependency.GenericEnablingSchedule a rdf:Property ;
  rdfs:label "GenericEnablingSchedule"@en ;
  rdfs:comment "Enabling schedule associated to a remedial action dependency." ;
  cims:AssociationUsed "No" ;
  cims:inverseRoleName nc:GenericEnablingSchedule.RemedialActionDependency ;
  cims:multiplicity cims:M:0..n ;
  cims:stereotype "NC" ;
  rdfs:domain nc:RemedialActionDependency ;
  rdfs:range nc:GenericEnablingSchedule .

nc:RemedialActionGroup.RemedialActionGroupSchedule a rdf:Property ;
  rdfs:label "RemedialActionGroupSchedule"@en ;
  rdfs:comment "Remedial action group schedule associated with a remedial action group." ;
  cims:AssociationUsed "No" ;
  cims:inverseRoleName nc:RemedialActionGroupSchedule.RemedialActionGroup ;
  cims:multiplicity cims:M:0..n ;
  cims:stereotype "NC" ;
  rdfs:domain nc:RemedialActionGroup ;
  rdfs:range nc:RemedialActionGroupSchedule .

nc:RemedialActionGroupSchedule.RemedialActionGroup a rdf:Property ;
  rdfs:label "RemedialActionGroup"@en ;
  rdfs:comment "Remedial action group which has remedial action group schedules." ;
  cims:AssociationUsed "Yes" ;
  cims:inverseRoleName nc:RemedialActionGroup.RemedialActionGroupSchedule ;
  cims:multiplicity cims:M:1 ;
  cims:stereotype "NC" ;
  rdfs:domain nc:RemedialActionGroupSchedule ;
  rdfs:range nc:RemedialActionGroup .

nc:RemedialActionGroupSchedule.RemedialActionGroupTimePoint a rdf:Property ;
  rdfs:label "RemedialActionGroupTimePoint"@en ;
  rdfs:comment "Remedial action group time point that relates to this remedial action group schedule." ;
  cims:AssociationUsed "No" ;
  cims:inverseRoleName nc:RemedialActionGroupTimePoint.RemedialActionGroupSchedule ;
  cims:multiplicity cims:M:1..n ;
  cims:stereotype "NC" ;
  rdfs:domain nc:RemedialActionGroupSchedule ;
  rdfs:range nc:RemedialActionGroupTimePoint .

nc:RemedialActionGroupTimePoint.RemedialActionGroupSchedule a rdf:Property ;
  rdfs:label "RemedialActionGroupSchedule"@en ;
  rdfs:comment "Remedial action group schedule that has time point." ;
  cims:AssociationUsed "Yes" ;
  cims:inverseRoleName nc:RemedialActionGroupSchedule.RemedialActionGroupTimePoint ;
  cims:multiplicity cims:M:1 ;
  cims:stereotype "NC" ;
  rdfs:domain nc:RemedialActionGroupTimePoint ;
  rdfs:range nc:RemedialActionGroupSchedule .

nc:RemedialActionGroupTimePoint.atTime a rdf:Property ;
  rdfs:label "atTime"@en ;
  rdfs:comment "The time the data is valid for." ;
  cims:dataType cim:DateTime ;
  cims:multiplicity cims:M:1..1 ;
  cims:stereotype "NC", <http://iec.ch/TC57/NonStandard/UML#attribute> ;
  rdfs:domain nc:RemedialActionGroupTimePoint .

nc:RemedialActionGroupTimePoint.maxRegulatingDown a rdf:Property ;
  rdfs:label "maxRegulatingDown"@en ;
  rdfs:comment "Maximum net amount of active power that the group of remedial actions can regulate down." ;
  cims:dataType cim:ActivePower ;
  cims:multiplicity cims:M:0..1 ;
  cims:stereotype "NC", <http://iec.ch/TC57/NonStandard/UML#attribute> ;
  rdfs:domain nc:RemedialActionGroupTimePoint .

nc:RemedialActionGroupTimePoint.maxRegulatingUp a rdf:Property ;
  rdfs:label "maxRegulatingUp"@en ;
  rdfs:comment "Maximum net amount of active power that the group of remedial actions can regulate up." ;
  cims:dataType cim:ActivePower ;
  cims:multiplicity cims:M:0..1 ;
  cims:stereotype "NC", <http://iec.ch/TC57/NonStandard/UML#attribute> ;
  rdfs:domain nc:RemedialActionGroupTimePoint .

nc:RemedialActionScheme.RemedialActionSchemeSchedule a rdf:Property ;
  rdfs:label "RemedialActionSchemeSchedule"@en ;
  rdfs:comment "Remedial action scheme schedule that has this armed remedial action." ;
  cims:AssociationUsed "No" ;
  cims:inverseRoleName nc:RemedialActionSchemeSchedule.ArmedRemedialAction ;
  cims:multiplicity cims:M:0..n ;
  cims:stereotype "NC" ;
  rdfs:domain nc:RemedialActionScheme ;
  rdfs:range nc:RemedialActionSchemeSchedule .

nc:RemedialActionSchemeSchedule.ArmedRemedialAction a rdf:Property ;
  rdfs:label "ArmedRemedialAction"@en ;
  rdfs:comment "Armed remedial action for a remedial action scheme." ;
  cims:AssociationUsed "Yes" ;
  cims:inverseRoleName nc:RemedialActionScheme.RemedialActionSchemeSchedule ;
  cims:multiplicity cims:M:1 ;
  cims:stereotype "NC" ;
  rdfs:domain nc:RemedialActionSchemeSchedule ;
  rdfs:range nc:RemedialActionScheme .

nc:RemedialActionSchemeSchedule.RemedialActionSchemeTimePoint a rdf:Property ;
  rdfs:label "RemedialActionSchemeTimePoint"@en ;
  rdfs:comment "Remedial action scheme time point that relates to this remedial action scheme schedule." ;
  cims:AssociationUsed "No" ;
  cims:inverseRoleName nc:RemedialActionSchemeTimePoint.RemedialActionSchemeSchedule ;
  cims:multiplicity cims:M:1..n ;
  cims:stereotype "NC", <http://iec.ch/TC57/NonStandard/UML#ofAggregate> ;
  rdfs:domain nc:RemedialActionSchemeSchedule ;
  rdfs:range nc:RemedialActionSchemeTimePoint .

nc:RemedialActionSchemeTimePoint.RemedialActionSchemeSchedule a rdf:Property ;
  rdfs:label "RemedialActionSchemeSchedule"@en ;
  rdfs:comment "Remedial action scheme schedule that has time point." ;
  cims:AssociationUsed "Yes" ;
  cims:inverseRoleName nc:RemedialActionSchemeSchedule.RemedialActionSchemeTimePoint ;
  cims:multiplicity cims:M:1 ;
  cims:stereotype "NC" ;
  rdfs:domain nc:RemedialActionSchemeTimePoint ;
  rdfs:range nc:RemedialActionSchemeSchedule .

nc:RemedialActionSchemeTimePoint.armed a rdf:Property ;
  rdfs:label "armed"@en ;
  rdfs:comment "Defines the arming status of the remedial action scheme. It is set by operation or by signal." ;
  cims:dataType cim:Boolean ;
  cims:multiplicity cims:M:0..1 ;
  cims:stereotype "NC", <http://iec.ch/TC57/NonStandard/UML#attribute> ;
  rdfs:domain nc:RemedialActionSchemeTimePoint .

nc:RemedialActionSchemeTimePoint.atTime a rdf:Property ;
  rdfs:label "atTime"@en ;
  rdfs:comment "The time the data is valid for." ;
  cims:dataType cim:DateTime ;
  cims:multiplicity cims:M:1..1 ;
  cims:stereotype "NC", <http://iec.ch/TC57/NonStandard/UML#attribute> ;
  rdfs:domain nc:RemedialActionSchemeTimePoint .

nc:RemedialActionSchemeTimePoint.inService a rdf:Property ;
  rdfs:label "inService"@en ;
  rdfs:comment "Specifies the availability of the Remedial Action Scheme (RAS). If true, the RAS is available for contingency processing. If false, the RAS is treated by contingency processing as if it is not in the model." ;
  cims:dataType cim:Boolean ;
  cims:multiplicity cims:M:0..1 ;
  cims:stereotype "NC", <http://iec.ch/TC57/NonStandard/UML#attribute> ;
  rdfs:domain nc:RemedialActionSchemeTimePoint .

nc:ScheduleResource.PowerBidSchedule a rdf:Property ;
  rdfs:label "PowerBidSchedule"@en ;
  rdfs:comment "Power bid schedule which belongs to a schedule resource." ;
  cims:AssociationUsed "No" ;
  cims:inverseRoleName nc:PowerBidSchedule.ScheduleResource ;
  cims:multiplicity cims:M:0..n ;
  cims:stereotype "NC" ;
  rdfs:domain nc:ScheduleResource ;
  rdfs:range nc:PowerBidSchedule .

nc:ScheduleResource.PowerShiftKeySchedule a rdf:Property ;
  rdfs:label "PowerShiftKeySchedule"@en ;
  rdfs:comment "The  Power Shift Key schedule for a schedule resource." ;
  cims:AssociationUsed "No" ;
  cims:inverseRoleName nc:PowerShiftKeySchedule.ScheduleResource ;
  cims:multiplicity cims:M:0..n ;
  cims:stereotype "NC" ;
  rdfs:domain nc:ScheduleResource ;
  rdfs:range nc:PowerShiftKeySchedule .

nc:Season.BaseRegularIntervalSchedule a rdf:Property ;
  rdfs:label "BaseRegularIntervalSchedule"@en ;
  rdfs:comment "Base regular interval schedule which has seasons." ;
  cims:AssociationUsed "No" ;
  cims:inverseRoleName nc:BaseRegularIntervalSchedule.Season ;
  cims:multiplicity cims:M:0..n ;
  cims:stereotype "NC" ;
  rdfs:domain cim:Season ;
  rdfs:range nc:BaseRegularIntervalSchedule .

nc:SequenceTimePoint.GenericSequenceSchedule a rdf:Property ;
  rdfs:label "GenericSequenceSchedule"@en ;
  rdfs:comment "The sequence schedule which belongs to the sequence timepoint." ;
  cims:AssociationUsed "Yes" ;
  cims:inverseRoleName nc:GenericSequenceSchedule.SequenceTimePoint ;
  cims:multiplicity cims:M:1 ;
  cims:stereotype "NC" ;
  rdfs:domain nc:SequenceTimePoint ;
  rdfs:range nc:GenericSequenceSchedule .

nc:SequenceTimePoint.atTime a rdf:Property ;
  rdfs:label "atTime"@en ;
  rdfs:comment "The time the data is valid for." ;
  cims:dataType cim:DateTime ;
  cims:multiplicity cims:M:1..1 ;
  cims:stereotype "NC", <http://iec.ch/TC57/NonStandard/UML#attribute> ;
  rdfs:domain nc:SequenceTimePoint .

nc:SequenceTimePoint.sequence a rdf:Property ;
  rdfs:label "sequence"@en ;
  rdfs:comment "Sequence needs to be ordered by the scheduling area. It has to be unique by the scheduling area." ;
  cims:dataType cim:Integer ;
  cims:multiplicity cims:M:1..1 ;
  cims:stereotype "NC", <http://iec.ch/TC57/NonStandard/UML#attribute> ;
  rdfs:domain nc:SequenceTimePoint .

nc:StageTrigger.StageTriggerSchedule a rdf:Property ;
  rdfs:label "StageTriggerSchedule"@en ;
  rdfs:comment "Stage trigger schedule associated with a stage trigger." ;
  cims:AssociationUsed "No" ;
  cims:inverseRoleName nc:StageTriggerSchedule.StageTrigger ;
  cims:multiplicity cims:M:0..n ;
  cims:stereotype "NC" ;
  rdfs:domain nc:StageTrigger ;
  rdfs:range nc:StageTriggerSchedule .

nc:StageTriggerSchedule.StageTrigger a rdf:Property ;
  rdfs:label "StageTrigger"@en ;
  rdfs:comment "Stage trigger which has stage trigger schedules." ;
  cims:AssociationUsed "Yes" ;
  cims:inverseRoleName nc:StageTrigger.StageTriggerSchedule ;
  cims:multiplicity cims:M:1 ;
  cims:stereotype "NC" ;
  rdfs:domain nc:StageTriggerSchedule ;
  rdfs:range nc:StageTrigger .

nc:StageTriggerSchedule.StageTriggerTimePoint a rdf:Property ;
  rdfs:label "StageTriggerTimePoint"@en ;
  rdfs:comment "Stage trigger time point that relates to this remedial action scheme schedule." ;
  cims:AssociationUsed "No" ;
  cims:inverseRoleName nc:StageTriggerTimePoint.StageTriggerSchedule ;
  cims:multiplicity cims:M:1..n ;
  cims:stereotype "NC" ;
  rdfs:domain nc:StageTriggerSchedule ;
  rdfs:range nc:StageTriggerTimePoint .

nc:StageTriggerTimePoint.StageTriggerSchedule a rdf:Property ;
  rdfs:label "StageTriggerSchedule"@en ;
  rdfs:comment "Stage trigger schedule that has time point." ;
  cims:AssociationUsed "Yes" ;
  cims:inverseRoleName nc:StageTriggerSchedule.StageTriggerTimePoint ;
  cims:multiplicity cims:M:1 ;
  cims:stereotype "NC" ;
  rdfs:domain nc:StageTriggerTimePoint ;
  rdfs:range nc:StageTriggerSchedule .

nc:StageTriggerTimePoint.armed a rdf:Property ;
  rdfs:label "armed"@en ;
  rdfs:comment "Defines the arming status of the remedial action scheme. It is set by operation or by signal." ;
  cims:dataType cim:Boolean ;
  cims:multiplicity cims:M:0..1 ;
  cims:stereotype "NC", <http://iec.ch/TC57/NonStandard/UML#attribute> ;
  rdfs:domain nc:StageTriggerTimePoint .

nc:StageTriggerTimePoint.atTime a rdf:Property ;
  rdfs:label "atTime"@en ;
  rdfs:comment "The time the data is valid for." ;
  cims:dataType cim:DateTime ;
  cims:multiplicity cims:M:1..1 ;
  cims:stereotype "NC", <http://iec.ch/TC57/NonStandard/UML#attribute> ;
  rdfs:domain nc:StageTriggerTimePoint .

nc:StageTriggerTimePoint.inService a rdf:Property ;
  rdfs:label "inService"@en ;
  rdfs:comment "Specifies the availability of the Remedial Action Scheme (RAS). If true, the RAS is available for contingency processing. If false, the RAS is treated by contingency processing as if it is not in the model." ;
  cims:dataType cim:Boolean ;
  cims:multiplicity cims:M:0..1 ;
  cims:stereotype "NC", <http://iec.ch/TC57/NonStandard/UML#attribute> ;
  rdfs:domain nc:StageTriggerTimePoint .

nc:UnitCostSchedule.GeneratingUnit a rdf:Property ;
  rdfs:label "GeneratingUnit"@en ;
  rdfs:comment "GeneratingUnit which has unit cost schedules." ;
  cims:AssociationUsed "Yes" ;
  cims:inverseRoleName nc:GeneratingUnit.UnitCostSchedule ;
  cims:multiplicity cims:M:1 ;
  cims:stereotype "NC" ;
  rdfs:domain nc:UnitCostSchedule ;
  rdfs:range cim:GeneratingUnit .

nc:UnitCostSchedule.UnitCostTimePoint a rdf:Property ;
  rdfs:label "UnitCostTimePoint"@en ;
  rdfs:comment "The unit cost time point that relates to this unit cost schedule." ;
  cims:AssociationUsed "No" ;
  cims:inverseRoleName nc:UnitCostTimePoint.UnitCostSchedule ;
  cims:multiplicity cims:M:1..n ;
  cims:stereotype "NC", <http://iec.ch/TC57/NonStandard/UML#ofAggregate> ;
  rdfs:domain nc:UnitCostSchedule ;
  rdfs:range nc:UnitCostTimePoint .

nc:UnitCostTimePoint.UnitCostSchedule a rdf:Property ;
  rdfs:label "UnitCostSchedule"@en ;
  rdfs:comment "The unit cost schedule that has time point." ;
  cims:AssociationUsed "Yes" ;
  cims:inverseRoleName nc:UnitCostSchedule.UnitCostTimePoint ;
  cims:multiplicity cims:M:1 ;
  cims:stereotype "NC" ;
  rdfs:domain nc:UnitCostTimePoint ;
  rdfs:range nc:UnitCostSchedule .

nc:UnitCostTimePoint.atTime a rdf:Property ;
  rdfs:label "atTime"@en ;
  rdfs:comment "The time the data is valid for." ;
  cims:dataType cim:DateTime ;
  cims:multiplicity cims:M:1..1 ;
  cims:stereotype "NC", <http://iec.ch/TC57/NonStandard/UML#attribute> ;
  rdfs:domain nc:UnitCostTimePoint .

nc:UnitCostTimePoint.startupCost a rdf:Property ;
  rdfs:label "startupCost"@en ;
  rdfs:comment "The initial startup cost incurred for each start of the GeneratingUnit." ;
  cims:dataType cim:Money ;
  cims:multiplicity cims:M:0..1 ;
  cims:stereotype "NC", <http://iec.ch/TC57/NonStandard/UML#attribute> ;
  rdfs:domain nc:UnitCostTimePoint .

nc:UnitCostTimePoint.warmStartupCost a rdf:Property ;
  rdfs:label "warmStartupCost"@en ;
  rdfs:comment "The warm startup cost incurred for each start of the GeneratingUnit." ;
  cims:dataType cim:Money ;
  cims:multiplicity cims:M:0..1 ;
  cims:stereotype "NC", <http://iec.ch/TC57/NonStandard/UML#attribute> ;
  rdfs:domain nc:UnitCostTimePoint .

nc:VoltageAngleLimit.VoltageAngleSchedule a rdf:Property ;
  rdfs:label "VoltageAngleSchedule"@en ;
  rdfs:comment "Voltage angle schedule associated with a voltage angle limit." ;
  cims:AssociationUsed "No" ;
  cims:inverseRoleName nc:VoltageAngleSchedule.VoltageAngleLimit ;
  cims:multiplicity cims:M:0..n ;
  cims:stereotype "NC" ;
  rdfs:domain nc:VoltageAngleLimit ;
  rdfs:range nc:VoltageAngleSchedule .

nc:VoltageAngleSchedule.VoltageAngleLimit a rdf:Property ;
  rdfs:label "VoltageAngleLimit"@en ;
  rdfs:comment "Voltage angle limit which has voltage angle schedules." ;
  cims:AssociationUsed "Yes" ;
  cims:inverseRoleName nc:VoltageAngleLimit.VoltageAngleSchedule ;
  cims:multiplicity cims:M:1 ;
  cims:stereotype "NC" ;
  rdfs:domain nc:VoltageAngleSchedule ;
  rdfs:range nc:VoltageAngleLimit .

nc:VoltageAngleSchedule.VoltageAngletimePoint a rdf:Property ;
  rdfs:label "VoltageAngletimePoint"@en ;
  rdfs:comment "The voltage angle time point that relates to this voltage angle schedule." ;
  cims:AssociationUsed "No" ;
  cims:inverseRoleName nc:VoltageAngleTimePoint.VoltageAngleSchedule ;
  cims:multiplicity cims:M:1..n ;
  cims:stereotype "NC", <http://iec.ch/TC57/NonStandard/UML#ofAggregate> ;
  rdfs:domain nc:VoltageAngleSchedule ;
  rdfs:range nc:VoltageAngleTimePoint .

nc:VoltageAngleTimePoint.VoltageAngleSchedule a rdf:Property ;
  rdfs:label "VoltageAngleSchedule"@en ;
  rdfs:comment "The voltage angle schedule that has time point." ;
  cims:AssociationUsed "Yes" ;
  cims:inverseRoleName nc:VoltageAngleSchedule.VoltageAngletimePoint ;
  cims:multiplicity cims:M:1 ;
  cims:stereotype "NC" ;
  rdfs:domain nc:VoltageAngleTimePoint ;
  rdfs:range nc:VoltageAngleSchedule .

nc:VoltageAngleTimePoint.atTime a rdf:Property ;
  rdfs:label "atTime"@en ;
  rdfs:comment "The time the data is valid for." ;
  cims:dataType cim:DateTime ;
  cims:multiplicity cims:M:1..1 ;
  cims:stereotype "NC", <http://iec.ch/TC57/NonStandard/UML#attribute> ;
  rdfs:domain nc:VoltageAngleTimePoint .

nc:VoltageAngleTimePoint.value a rdf:Property ;
  rdfs:label "value"@en ;
  rdfs:comment "The difference in angle degrees between referenced by the association end OperationalLimitSet.Terminal and the Terminal referenced by the association end VoltageAngleLimit.AngleReferenceTerminal. The value shall be positive (greater than zero)." ;
  cims:dataType cim:AngleDegrees ;
  cims:multiplicity cims:M:1..1 ;
  cims:stereotype "NC", <http://iec.ch/TC57/NonStandard/UML#attribute> ;
  rdfs:domain nc:VoltageAngleTimePoint .

cim:Currency.AED a cim:Currency ;
  rdfs:label "AED"@en ;
  rdfs:comment "United Arab Emirates dirham." ;
  cims:stereotype "enum" .

cim:Currency.AFN a cim:Currency ;
  rdfs:label "AFN"@en ;
  rdfs:comment "Afghan afghani." ;
  cims:stereotype "enum" .

cim:Currency.ALL a cim:Currency ;
  rdfs:label "ALL"@en ;
  rdfs:comment "Albanian lek." ;
  cims:stereotype "enum" .

cim:Currency.AMD a cim:Currency ;
  rdfs:label "AMD"@en ;
  rdfs:comment "Armenian dram." ;
  cims:stereotype "enum" .

cim:Currency.ANG a cim:Currency ;
  rdfs:label "ANG"@en ;
  rdfs:comment "Netherlands Antillean guilder." ;
  cims:stereotype "enum" .

cim:Currency.AOA a cim:Currency ;
  rdfs:label "AOA"@en ;
  rdfs:comment "Angolan kwanza." ;
  cims:stereotype "enum" .

cim:Currency.ARS a cim:Currency ;
  rdfs:label "ARS"@en ;
  rdfs:comment "Argentine peso." ;
  cims:stereotype "enum" .

cim:Currency.AUD a cim:Currency ;
  rdfs:label "AUD"@en ;
  rdfs:comment "Australian dollar." ;
  cims:stereotype "enum" .

cim:Currency.AWG a cim:Currency ;
  rdfs:label "AWG"@en ;
  rdfs:comment "Aruban florin." ;
  cims:stereotype "enum" .

cim:Currency.AZN a cim:Currency ;
  rdfs:label "AZN"@en ;
  rdfs:comment "Azerbaijani manat." ;
  cims:stereotype "enum" .

cim:Currency.BAM a cim:Currency ;
  rdfs:label "BAM"@en ;
  rdfs:comment "Bosnia and Herzegovina convertible mark." ;
  cims:stereotype "enum" .

cim:Currency.BBD a cim:Currency ;
  rdfs:label "BBD"@en ;
  rdfs:comment "Barbados dollar." ;
  cims:stereotype "enum" .

cim:Currency.BDT a cim:Currency ;
  rdfs:label "BDT"@en ;
  rdfs:comment "Bangladeshi taka." ;
  cims:stereotype "enum" .

cim:Currency.BGN a cim:Currency ;
  rdfs:label "BGN"@en ;
  rdfs:comment "Bulgarian lev." ;
  cims:stereotype "enum" .

cim:Currency.BHD a cim:Currency ;
  rdfs:label "BHD"@en ;
  rdfs:comment "Bahraini dinar." ;
  cims:stereotype "enum" .

cim:Currency.BIF a cim:Currency ;
  rdfs:label "BIF"@en ;
  rdfs:comment "Burundian franc." ;
  cims:stereotype "enum" .

cim:Currency.BMD a cim:Currency ;
  rdfs:label "BMD"@en ;
  rdfs:comment "Bermudian dollar (customarily known as Bermuda dollar)." ;
  cims:stereotype "enum" .

cim:Currency.BND a cim:Currency ;
  rdfs:label "BND"@en ;
  rdfs:comment "Brunei dollar." ;
  cims:stereotype "enum" .

cim:Currency.BOB a cim:Currency ;
  rdfs:label "BOB"@en ;
  rdfs:comment "Boliviano." ;
  cims:stereotype "enum" .

cim:Currency.BOV a cim:Currency ;
  rdfs:label "BOV"@en ;
  rdfs:comment "Bolivian Mvdol (funds code)." ;
  cims:stereotype "enum" .

cim:Currency.BRL a cim:Currency ;
  rdfs:label "BRL"@en ;
  rdfs:comment "Brazilian real." ;
  cims:stereotype "enum" .

cim:Currency.BSD a cim:Currency ;
  rdfs:label "BSD"@en ;
  rdfs:comment "Bahamian dollar." ;
  cims:stereotype "enum" .

cim:Currency.BTN a cim:Currency ;
  rdfs:label "BTN"@en ;
  rdfs:comment "Bhutanese ngultrum." ;
  cims:stereotype "enum" .

cim:Currency.BWP a cim:Currency ;
  rdfs:label "BWP"@en ;
  rdfs:comment "Botswana pula." ;
  cims:stereotype "enum" .

cim:Currency.BYR a cim:Currency ;
  rdfs:label "BYR"@en ;
  rdfs:comment "Belarusian ruble." ;
  cims:stereotype "enum" .

cim:Currency.BZD a cim:Currency ;
  rdfs:label "BZD"@en ;
  rdfs:comment "Belize dollar." ;
  cims:stereotype "enum" .

cim:Currency.CAD a cim:Currency ;
  rdfs:label "CAD"@en ;
  rdfs:comment "Canadian dollar." ;
  cims:stereotype "enum" .

cim:Currency.CDF a cim:Currency ;
  rdfs:label "CDF"@en ;
  rdfs:comment "Congolese franc." ;
  cims:stereotype "enum" .

cim:Currency.CHF a cim:Currency ;
  rdfs:label "CHF"@en ;
  rdfs:comment "Swiss franc." ;
  cims:stereotype "enum" .

cim:Currency.CLF a cim:Currency ;
  rdfs:label "CLF"@en ;
  rdfs:comment "Unidad de Fomento (funds code), Chile." ;
  cims:stereotype "enum" .

cim:Currency.CLP a cim:Currency ;
  rdfs:label "CLP"@en ;
  rdfs:comment "Chilean peso." ;
  cims:stereotype "enum" .

cim:Currency.CNY a cim:Currency ;
  rdfs:label "CNY"@en ;
  rdfs:comment "Chinese yuan." ;
  cims:stereotype "enum" .

cim:Currency.COP a cim:Currency ;
  rdfs:label "COP"@en ;
  rdfs:comment "Colombian peso." ;
  cims:stereotype "enum" .

cim:Currency.COU a cim:Currency ;
  rdfs:label "COU"@en ;
  rdfs:comment "Unidad de Valor Real." ;
  cims:stereotype "enum" .

cim:Currency.CRC a cim:Currency ;
  rdfs:label "CRC"@en ;
  rdfs:comment "Costa Rican colon." ;
  cims:stereotype "enum" .

cim:Currency.CUC a cim:Currency ;
  rdfs:label "CUC"@en ;
  rdfs:comment "Cuban convertible peso." ;
  cims:stereotype "enum" .

cim:Currency.CUP a cim:Currency ;
  rdfs:label "CUP"@en ;
  rdfs:comment "Cuban peso." ;
  cims:stereotype "enum" .

cim:Currency.CVE a cim:Currency ;
  rdfs:label "CVE"@en ;
  rdfs:comment "Cape Verde escudo." ;
  cims:stereotype "enum" .

cim:Currency.CZK a cim:Currency ;
  rdfs:label "CZK"@en ;
  rdfs:comment "Czech koruna." ;
  cims:stereotype "enum" .

cim:Currency.DJF a cim:Currency ;
  rdfs:label "DJF"@en ;
  rdfs:comment "Djiboutian franc." ;
  cims:stereotype "enum" .

cim:Currency.DKK a cim:Currency ;
  rdfs:label "DKK"@en ;
  rdfs:comment "Danish krone." ;
  cims:stereotype "enum" .

cim:Currency.DOP a cim:Currency ;
  rdfs:label "DOP"@en ;
  rdfs:comment "Dominican peso." ;
  cims:stereotype "enum" .

cim:Currency.DZD a cim:Currency ;
  rdfs:label "DZD"@en ;
  rdfs:comment "Algerian dinar." ;
  cims:stereotype "enum" .

cim:Currency.EEK a cim:Currency ;
  rdfs:label "EEK"@en ;
  rdfs:comment "Estonian kroon." ;
  cims:stereotype "enum" .

cim:Currency.EGP a cim:Currency ;
  rdfs:label "EGP"@en ;
  rdfs:comment "Egyptian pound." ;
  cims:stereotype "enum" .

cim:Currency.ERN a cim:Currency ;
  rdfs:label "ERN"@en ;
  rdfs:comment "Eritrean nakfa." ;
  cims:stereotype "enum" .

cim:Currency.ETB a cim:Currency ;
  rdfs:label "ETB"@en ;
  rdfs:comment "Ethiopian birr." ;
  cims:stereotype "enum" .

cim:Currency.EUR a cim:Currency ;
  rdfs:label "EUR"@en ;
  rdfs:comment "Euro." ;
  cims:stereotype "enum" .

cim:Currency.FJD a cim:Currency ;
  rdfs:label "FJD"@en ;
  rdfs:comment "Fiji dollar." ;
  cims:stereotype "enum" .

cim:Currency.FKP a cim:Currency ;
  rdfs:label "FKP"@en ;
  rdfs:comment "Falkland Islands pound." ;
  cims:stereotype "enum" .

cim:Currency.GBP a cim:Currency ;
  rdfs:label "GBP"@en ;
  rdfs:comment "Pound sterling." ;
  cims:stereotype "enum" .

cim:Currency.GEL a cim:Currency ;
  rdfs:label "GEL"@en ;
  rdfs:comment "Georgian lari." ;
  cims:stereotype "enum" .

cim:Currency.GHS a cim:Currency ;
  rdfs:label "GHS"@en ;
  rdfs:comment "Ghanaian cedi." ;
  cims:stereotype "enum" .

cim:Currency.GIP a cim:Currency ;
  rdfs:label "GIP"@en ;
  rdfs:comment "Gibraltar pound." ;
  cims:stereotype "enum" .

cim:Currency.GMD a cim:Currency ;
  rdfs:label "GMD"@en ;
  rdfs:comment "Gambian dalasi." ;
  cims:stereotype "enum" .

cim:Currency.GNF a cim:Currency ;
  rdfs:label "GNF"@en ;
  rdfs:comment "Guinean franc." ;
  cims:stereotype "enum" .

cim:Currency.GTQ a cim:Currency ;
  rdfs:label "GTQ"@en ;
  rdfs:comment "Guatemalan quetzal." ;
  cims:stereotype "enum" .

cim:Currency.GYD a cim:Currency ;
  rdfs:label "GYD"@en ;
  rdfs:comment "Guyanese dollar." ;
  cims:stereotype "enum" .

cim:Currency.HKD a cim:Currency ;
  rdfs:label "HKD"@en ;
  rdfs:comment "Hong Kong dollar." ;
  cims:stereotype "enum" .

cim:Currency.HNL a cim:Currency ;
  rdfs:label "HNL"@en ;
  rdfs:comment "Honduran lempira." ;
  cims:stereotype "enum" .

cim:Currency.HRK a cim:Currency ;
  rdfs:label "HRK"@en ;
  rdfs:comment "Croatian kuna." ;
  cims:stereotype "enum" .

cim:Currency.HTG a cim:Currency ;
  rdfs:label "HTG"@en ;
  rdfs:comment "Haitian gourde." ;
  cims:stereotype "enum" .

cim:Currency.HUF a cim:Currency ;
  rdfs:label "HUF"@en ;
  rdfs:comment "Hungarian forint." ;
  cims:stereotype "enum" .

cim:Currency.IDR a cim:Currency ;
  rdfs:label "IDR"@en ;
  rdfs:comment "Indonesian rupiah." ;
  cims:stereotype "enum" .

cim:Currency.ILS a cim:Currency ;
  rdfs:label "ILS"@en ;
  rdfs:comment "Israeli new sheqel." ;
  cims:stereotype "enum" .

cim:Currency.INR a cim:Currency ;
  rdfs:label "INR"@en ;
  rdfs:comment "Indian rupee." ;
  cims:stereotype "enum" .

cim:Currency.IQD a cim:Currency ;
  rdfs:label "IQD"@en ;
  rdfs:comment "Iraqi dinar." ;
  cims:stereotype "enum" .

cim:Currency.IRR a cim:Currency ;
  rdfs:label "IRR"@en ;
  rdfs:comment "Iranian rial." ;
  cims:stereotype "enum" .

cim:Currency.ISK a cim:Currency ;
  rdfs:label "ISK"@en ;
  rdfs:comment "Icelandic króna." ;
  cims:stereotype "enum" .

cim:Currency.JMD a cim:Currency ;
  rdfs:label "JMD"@en ;
  rdfs:comment "Jamaican dollar." ;
  cims:stereotype "enum" .

cim:Currency.JOD a cim:Currency ;
  rdfs:label "JOD"@en ;
  rdfs:comment "Jordanian dinar." ;
  cims:stereotype "enum" .

cim:Currency.JPY a cim:Currency ;
  rdfs:label "JPY"@en ;
  rdfs:comment "Japanese yen." ;
  cims:stereotype "enum" .

cim:Currency.KES a cim:Currency ;
  rdfs:label "KES"@en ;
  rdfs:comment "Kenyan shilling." ;
  cims:stereotype "enum" .

cim:Currency.KGS a cim:Currency ;
  rdfs:label "KGS"@en ;
  rdfs:comment "Kyrgyzstani som." ;
  cims:stereotype "enum" .

cim:Currency.KHR a cim:Currency ;
  rdfs:label "KHR"@en ;
  rdfs:comment "Cambodian riel." ;
  cims:stereotype "enum" .

cim:Currency.KMF a cim:Currency ;
  rdfs:label "KMF"@en ;
  rdfs:comment "Comoro franc." ;
  cims:stereotype "enum" .

cim:Currency.KPW a cim:Currency ;
  rdfs:label "KPW"@en ;
  rdfs:comment "North Korean won." ;
  cims:stereotype "enum" .

cim:Currency.KRW a cim:Currency ;
  rdfs:label "KRW"@en ;
  rdfs:comment "South Korean won." ;
  cims:stereotype "enum" .

cim:Currency.KWD a cim:Currency ;
  rdfs:label "KWD"@en ;
  rdfs:comment "Kuwaiti dinar." ;
  cims:stereotype "enum" .

cim:Currency.KYD a cim:Currency ;
  rdfs:label "KYD"@en ;
  rdfs:comment "Cayman Islands dollar." ;
  cims:stereotype "enum" .

cim:Currency.KZT a cim:Currency ;
  rdfs:label "KZT"@en ;
  rdfs:comment "Kazakhstani tenge." ;
  cims:stereotype "enum" .

cim:Currency.LAK a cim:Currency ;
  rdfs:label "LAK"@en ;
  rdfs:comment "Lao kip." ;
  cims:stereotype "enum" .

cim:Currency.LBP a cim:Currency ;
  rdfs:label "LBP"@en ;
  rdfs:comment "Lebanese pound." ;
  cims:stereotype "enum" .

cim:Currency.LKR a cim:Currency ;
  rdfs:label "LKR"@en ;
  rdfs:comment "Sri Lanka rupee." ;
  cims:stereotype "enum" .

cim:Currency.LRD a cim:Currency ;
  rdfs:label "LRD"@en ;
  rdfs:comment "Liberian dollar." ;
  cims:stereotype "enum" .

cim:Currency.LSL a cim:Currency ;
  rdfs:label "LSL"@en ;
  rdfs:comment "Lesotho loti." ;
  cims:stereotype "enum" .

cim:Currency.LTL a cim:Currency ;
  rdfs:label "LTL"@en ;
  rdfs:comment "Lithuanian litas." ;
  cims:stereotype "enum" .

cim:Currency.LVL a cim:Currency ;
  rdfs:label "LVL"@en ;
  rdfs:comment "Latvian lats." ;
  cims:stereotype "enum" .

cim:Currency.LYD a cim:Currency ;
  rdfs:label "LYD"@en ;
  rdfs:comment "Libyan dinar." ;
  cims:stereotype "enum" .

cim:Currency.MAD a cim:Currency ;
  rdfs:label "MAD"@en ;
  rdfs:comment "Moroccan dirham." ;
  cims:stereotype "enum" .

cim:Currency.MDL a cim:Currency ;
  rdfs:label "MDL"@en ;
  rdfs:comment "Moldovan leu." ;
  cims:stereotype "enum" .

cim:Currency.MGA a cim:Currency ;
  rdfs:label "MGA"@en ;
  rdfs:comment "Malagasy ariary." ;
  cims:stereotype "enum" .

cim:Currency.MKD a cim:Currency ;
  rdfs:label "MKD"@en ;
  rdfs:comment "Macedonian denar." ;
  cims:stereotype "enum" .

cim:Currency.MMK a cim:Currency ;
  rdfs:label "MMK"@en ;
  rdfs:comment "Myanma kyat." ;
  cims:stereotype "enum" .

cim:Currency.MNT a cim:Currency ;
  rdfs:label "MNT"@en ;
  rdfs:comment "Mongolian tugrik." ;
  cims:stereotype "enum" .

cim:Currency.MOP a cim:Currency ;
  rdfs:label "MOP"@en ;
  rdfs:comment "Macanese pataca." ;
  cims:stereotype "enum" .

cim:Currency.MRO a cim:Currency ;
  rdfs:label "MRO"@en ;
  rdfs:comment "Mauritanian ouguiya." ;
  cims:stereotype "enum" .

cim:Currency.MUR a cim:Currency ;
  rdfs:label "MUR"@en ;
  rdfs:comment "Mauritian rupee." ;
  cims:stereotype "enum" .

cim:Currency.MVR a cim:Currency ;
  rdfs:label "MVR"@en ;
  rdfs:comment "Maldivian rufiyaa." ;
  cims:stereotype "enum" .

cim:Currency.MWK a cim:Currency ;
  rdfs:label "MWK"@en ;
  rdfs:comment "Malawian kwacha." ;
  cims:stereotype "enum" .

cim:Currency.MXN a cim:Currency ;
  rdfs:label "MXN"@en ;
  rdfs:comment "Mexican peso." ;
  cims:stereotype "enum" .

cim:Currency.MYR a cim:Currency ;
  rdfs:label "MYR"@en ;
  rdfs:comment "Malaysian ringgit." ;
  cims:stereotype "enum" .

cim:Currency.MZN a cim:Currency ;
  rdfs:label "MZN"@en ;
  rdfs:comment "Mozambican metical." ;
  cims:stereotype "enum" .

cim:Currency.NAD a cim:Currency ;
  rdfs:label "NAD"@en ;
  rdfs:comment "Namibian dollar." ;
  cims:stereotype "enum" .

cim:Currency.NGN a cim:Currency ;
  rdfs:label "NGN"@en ;
  rdfs:comment "Nigerian naira." ;
  cims:stereotype "enum" .

cim:Currency.NIO a cim:Currency ;
  rdfs:label "NIO"@en ;
  rdfs:comment "Cordoba oro." ;
  cims:stereotype "enum" .

cim:Currency.NOK a cim:Currency ;
  rdfs:label "NOK"@en ;
  rdfs:comment "Norwegian krone." ;
  cims:stereotype "enum" .

cim:Currency.NPR a cim:Currency ;
  rdfs:label "NPR"@en ;
  rdfs:comment "Nepalese rupee." ;
  cims:stereotype "enum" .

cim:Currency.NZD a cim:Currency ;
  rdfs:label "NZD"@en ;
  rdfs:comment "New Zealand dollar." ;
  cims:stereotype "enum" .

cim:Currency.OMR a cim:Currency ;
  rdfs:label "OMR"@en ;
  rdfs:comment "Omani rial." ;
  cims:stereotype "enum" .

cim:Currency.PAB a cim:Currency ;
  rdfs:label "PAB"@en ;
  rdfs:comment "Panamanian balboa." ;
  cims:stereotype "enum" .

cim:Currency.PEN a cim:Currency ;
  rdfs:label "PEN"@en ;
  rdfs:comment "Peruvian nuevo sol." ;
  cims:stereotype "enum" .

cim:Currency.PGK a cim:Currency ;
  rdfs:label "PGK"@en ;
  rdfs:comment "Papua New Guinean kina." ;
  cims:stereotype "enum" .

cim:Currency.PHP a cim:Currency ;
  rdfs:label "PHP"@en ;
  rdfs:comment "Philippine peso." ;
  cims:stereotype "enum" .

cim:Currency.PKR a cim:Currency ;
  rdfs:label "PKR"@en ;
  rdfs:comment "Pakistani rupee." ;
  cims:stereotype "enum" .

cim:Currency.PLN a cim:Currency ;
  rdfs:label "PLN"@en ;
  rdfs:comment "Polish zloty." ;
  cims:stereotype "enum" .

cim:Currency.PYG a cim:Currency ;
  rdfs:label "PYG"@en ;
  rdfs:comment "Paraguayan guaraní." ;
  cims:stereotype "enum" .

cim:Currency.QAR a cim:Currency ;
  rdfs:label "QAR"@en ;
  rdfs:comment "Qatari rial." ;
  cims:stereotype "enum" .

cim:Currency.RON a cim:Currency ;
  rdfs:label "RON"@en ;
  rdfs:comment "Romanian new leu." ;
  cims:stereotype "enum" .

cim:Currency.RSD a cim:Currency ;
  rdfs:label "RSD"@en ;
  rdfs:comment "Serbian dinar." ;
  cims:stereotype "enum" .

cim:Currency.RUB a cim:Currency ;
  rdfs:label "RUB"@en ;
  rdfs:comment "Russian rouble." ;
  cims:stereotype "enum" .

cim:Currency.RWF a cim:Currency ;
  rdfs:label "RWF"@en ;
  rdfs:comment "Rwandan franc." ;
  cims:stereotype "enum" .

cim:Currency.SAR a cim:Currency ;
  rdfs:label "SAR"@en ;
  rdfs:comment "Saudi riyal." ;
  cims:stereotype "enum" .

cim:Currency.SBD a cim:Currency ;
  rdfs:label "SBD"@en ;
  rdfs:comment "Solomon Islands dollar." ;
  cims:stereotype "enum" .

cim:Currency.SCR a cim:Currency ;
  rdfs:label "SCR"@en ;
  rdfs:comment "Seychelles rupee." ;
  cims:stereotype "enum" .

cim:Currency.SDG a cim:Currency ;
  rdfs:label "SDG"@en ;
  rdfs:comment "Sudanese pound." ;
  cims:stereotype "enum" .

cim:Currency.SEK a cim:Currency ;
  rdfs:label "SEK"@en ;
  rdfs:comment "Swedish krona/kronor." ;
  cims:stereotype "enum" .

cim:Currency.SGD a cim:Currency ;
  rdfs:label "SGD"@en ;
  rdfs:comment "Singapore dollar." ;
  cims:stereotype "enum" .

cim:Currency.SHP a cim:Currency ;
  rdfs:label "SHP"@en ;
  rdfs:comment "Saint Helena pound." ;
  cims:stereotype "enum" .

cim:Currency.SLL a cim:Currency ;
  rdfs:label "SLL"@en ;
  rdfs:comment "Sierra Leonean leone." ;
  cims:stereotype "enum" .

cim:Currency.SOS a cim:Currency ;
  rdfs:label "SOS"@en ;
  rdfs:comment "Somali shilling." ;
  cims:stereotype "enum" .

cim:Currency.SRD a cim:Currency ;
  rdfs:label "SRD"@en ;
  rdfs:comment "Surinamese dollar." ;
  cims:stereotype "enum" .

cim:Currency.STD a cim:Currency ;
  rdfs:label "STD"@en ;
  rdfs:comment "São Tomé and Príncipe dobra." ;
  cims:stereotype "enum" .

cim:Currency.SYP a cim:Currency ;
  rdfs:label "SYP"@en ;
  rdfs:comment "Syrian pound." ;
  cims:stereotype "enum" .

cim:Currency.SZL a cim:Currency ;
  rdfs:label "SZL"@en ;
  rdfs:comment "Lilangeni." ;
  cims:stereotype "enum" .

cim:Currency.THB a cim:Currency ;
  rdfs:label "THB"@en ;
  rdfs:comment "Thai baht." ;
  cims:stereotype "enum" .

cim:Currency.TJS a cim:Currency ;
  rdfs:label "TJS"@en ;
  rdfs:comment "Tajikistani somoni." ;
  cims:stereotype "enum" .

cim:Currency.TMT a cim:Currency ;
  rdfs:label "TMT"@en ;
  rdfs:comment "Turkmenistani manat." ;
  cims:stereotype "enum" .

cim:Currency.TND a cim:Currency ;
  rdfs:label "TND"@en ;
  rdfs:comment "Tunisian dinar." ;
  cims:stereotype "enum" .

cim:Currency.TOP a cim:Currency ;
  rdfs:label "TOP"@en ;
  rdfs:comment "Tongan pa'anga." ;
  cims:stereotype "enum" .

cim:Currency.TRY a cim:Currency ;
  rdfs:label "TRY"@en ;
  rdfs:comment "Turkish lira." ;
  cims:stereotype "enum" .

cim:Currency.TTD a cim:Currency ;
  rdfs:label "TTD"@en ;
  rdfs:comment "Trinidad and Tobago dollar." ;
  cims:stereotype "enum" .

cim:Currency.TWD a cim:Currency ;
  rdfs:label "TWD"@en ;
  rdfs:comment "New Taiwan dollar." ;
  cims:stereotype "enum" .

cim:Currency.TZS a cim:Currency ;
  rdfs:label "TZS"@en ;
  rdfs:comment "Tanzanian shilling." ;
  cims:stereotype "enum" .

cim:Currency.UAH a cim:Currency ;
  rdfs:label "UAH"@en ;
  rdfs:comment "Ukrainian hryvnia." ;
  cims:stereotype "enum" .

cim:Currency.UGX a cim:Currency ;
  rdfs:label "UGX"@en ;
  rdfs:comment "Ugandan shilling." ;
  cims:stereotype "enum" .

cim:Currency.USD a cim:Currency ;
  rdfs:label "USD"@en ;
  rdfs:comment "United States dollar." ;
  cims:stereotype "enum" .

cim:Currency.UYU a cim:Currency ;
  rdfs:label "UYU"@en ;
  rdfs:comment "Uruguayan peso." ;
  cims:stereotype "enum" .

cim:Currency.UZS a cim:Currency ;
  rdfs:label "UZS"@en ;
  rdfs:comment "Uzbekistan som." ;
  cims:stereotype "enum" .

cim:Currency.VEF a cim:Currency ;
  rdfs:label "VEF"@en ;
  rdfs:comment "Venezuelan bolívar fuerte." ;
  cims:stereotype "enum" .

cim:Currency.VND a cim:Currency ;
  rdfs:label "VND"@en ;
  rdfs:comment "Vietnamese Dong." ;
  cims:stereotype "enum" .

cim:Currency.VUV a cim:Currency ;
  rdfs:label "VUV"@en ;
  rdfs:comment "Vanuatu vatu." ;
  cims:stereotype "enum" .

cim:Currency.WST a cim:Currency ;
  rdfs:label "WST"@en ;
  rdfs:comment "Samoan tala." ;
  cims:stereotype "enum" .

cim:Currency.XAF a cim:Currency ;
  rdfs:label "XAF"@en ;
  rdfs:comment "CFA franc BEAC." ;
  cims:stereotype "enum" .

cim:Currency.XCD a cim:Currency ;
  rdfs:label "XCD"@en ;
  rdfs:comment "East Caribbean dollar." ;
  cims:stereotype "enum" .

cim:Currency.XOF a cim:Currency ;
  rdfs:label "XOF"@en ;
  rdfs:comment "CFA Franc BCEAO." ;
  cims:stereotype "enum" .

cim:Currency.XPF a cim:Currency ;
  rdfs:label "XPF"@en ;
  rdfs:comment "CFP franc." ;
  cims:stereotype "enum" .

cim:Currency.YER a cim:Currency ;
  rdfs:label "YER"@en ;
  rdfs:comment "Yemeni rial." ;
  cims:stereotype "enum" .

cim:Currency.ZAR a cim:Currency ;
  rdfs:label "ZAR"@en ;
  rdfs:comment "South African rand." ;
  cims:stereotype "enum" .

cim:Currency.ZMK a cim:Currency ;
  rdfs:label "ZMK"@en ;
  rdfs:comment "Zambian kwacha." ;
  cims:stereotype "enum" .

cim:Currency.ZWL a cim:Currency ;
  rdfs:label "ZWL"@en ;
  rdfs:comment "Zimbabwe dollar." ;
  cims:stereotype "enum" .

cim:UnitMultiplier.M a cim:UnitMultiplier ;
  rdfs:label "M"@en ;
  rdfs:comment "Mega 10**6." ;
  cims:stereotype "enum" .

cim:UnitMultiplier.none a cim:UnitMultiplier ;
  rdfs:label "none"@en ;
  rdfs:comment "No multiplier or equivalently multiply by 1." ;
  cims:stereotype "enum" .

cim:UnitSymbol.W a cim:UnitSymbol ;
  rdfs:label "W"@en ;
  rdfs:comment "Real power in watts (J/s). Electrical power may have real and reactive components. The real portion of electrical power (I&#178;R or VIcos(phi)), is expressed in Watts. See also apparent power and reactive power." ;
  cims:stereotype "enum" .

cim:UnitSymbol.Wh a cim:UnitSymbol ;
  rdfs:label "Wh"@en ;
  rdfs:comment "Real energy in watt hours." ;
  cims:stereotype "enum" .

cim:UnitSymbol.none a cim:UnitSymbol ;
  rdfs:label "none"@en ;
  rdfs:comment "Dimension less quantity, e.g. count, per unit, etc." ;
  cims:stereotype "enum" .

cim:UnitSymbol.s a cim:UnitSymbol ;
  rdfs:label "s"@en ;
  rdfs:comment "Time in seconds." ;
  cims:stereotype "enum" .

nc:BaseTimeSeriesKind.actual a nc:BaseTimeSeriesKind ;
  rdfs:label "actual"@en ;
  rdfs:comment "Time series is actual data. The values represent measured or calculated values that represent the actual behaviour. " ;
  cims:stereotype "enum" .

nc:BaseTimeSeriesKind.forecast a nc:BaseTimeSeriesKind ;
  rdfs:label "forecast"@en ;
  rdfs:comment "Time series is forecast data. The values represent the result of scientific predictions based on historical time stamped data." ;
  cims:stereotype "enum" .

nc:BaseTimeSeriesKind.hindcast a nc:BaseTimeSeriesKind ;
  rdfs:label "hindcast"@en ;
  rdfs:comment "Time series is hindcast data. The value represent probable past (historic) condition given by calculation done using actual values. For instance, determine the among of wind based on the energy produced by wind. However, hindcast is typical the result of a simulated forecasts for historical periods." ;
  cims:stereotype "enum" .

nc:BaseTimeSeriesKind.schedule a nc:BaseTimeSeriesKind ;
  rdfs:label "schedule"@en ;
  rdfs:comment "Time series is schedule data. The values represent the result of a committed and plan forecast data that has been through a quality control and could incur penalty when not followed." ;
  cims:stereotype "enum" .

nc:BidDirectionKind.down a nc:BidDirectionKind ;
  rdfs:label "down"@en ;
  rdfs:comment "Down signifies that the available power can be used by the purchasing area to decrease energy." ;
  cims:stereotype "enum" .

nc:BidDirectionKind.stable a nc:BidDirectionKind ;
  rdfs:label "stable"@en ;
  rdfs:comment "The direction at a given instant in time is considered to be stable." ;
  cims:stereotype "enum" .

nc:BidDirectionKind.up a nc:BidDirectionKind ;
  rdfs:label "up"@en ;
  rdfs:comment "Up signifies that the available power can be used by the purchasing area to increase energy." ;
  cims:stereotype "enum" .

nc:BidDirectionKind.upAndDown a nc:BidDirectionKind ;
  rdfs:label "upAndDown"@en ;
  rdfs:comment "Up and down signifies that both up and down values are equal." ;
  cims:stereotype "enum" .

nc:DayOfWeekKind.all a nc:DayOfWeekKind ;
  rdfs:label "all"@en ;
  rdfs:comment "All days of the week." ;
  cims:stereotype "enum" .

nc:DayOfWeekKind.bridgeDay a nc:DayOfWeekKind ;
  rdfs:label "bridgeDay"@en ;
  rdfs:comment "A day that is a gap between two distinguished days e.g holiday and weekend that leads to an abnormal scheduling behavior. e.g. if Ascension day falls on a Thursday, then Friday would be a bridge day due to the schedule will not have a normal Friday consumption and production." ;
  cims:stereotype "enum" .

nc:DayOfWeekKind.friday a nc:DayOfWeekKind ;
  rdfs:label "friday"@en ;
  rdfs:comment "Friday as the day of the week." ;
  cims:stereotype "enum" .

nc:DayOfWeekKind.holiday a nc:DayOfWeekKind ;
  rdfs:label "holiday"@en ;
  cims:stereotype "enum" .

nc:DayOfWeekKind.monday a nc:DayOfWeekKind ;
  rdfs:label "monday"@en ;
  rdfs:comment "Monday as the day of the week." ;
  cims:stereotype "enum" .

nc:DayOfWeekKind.saturday a nc:DayOfWeekKind ;
  rdfs:label "saturday"@en ;
  rdfs:comment "Saturday as the day of the week." ;
  cims:stereotype "enum" .

nc:DayOfWeekKind.sunday a nc:DayOfWeekKind ;
  rdfs:label "sunday"@en ;
  rdfs:comment "Sunday as the day of the week." ;
  cims:stereotype "enum" .

nc:DayOfWeekKind.thursday a nc:DayOfWeekKind ;
  rdfs:label "thursday"@en ;
  rdfs:comment "Thursday as the day of the week." ;
  cims:stereotype "enum" .

nc:DayOfWeekKind.tuesday a nc:DayOfWeekKind ;
  rdfs:label "tuesday"@en ;
  rdfs:comment "Tuesday as the day of the week." ;
  cims:stereotype "enum" .

nc:DayOfWeekKind.wednesday a nc:DayOfWeekKind ;
  rdfs:label "wednesday"@en ;
  rdfs:comment "Wednesday as the day of the week." ;
  cims:stereotype "enum" .

nc:DayOfWeekKind.weekday a nc:DayOfWeekKind ;
  rdfs:label "weekday"@en ;
  rdfs:comment "A day of the week other than Sunday or Saturday." ;
  cims:stereotype "enum" .

nc:DayOfWeekKind.weekend a nc:DayOfWeekKind ;
  rdfs:label "weekend"@en ;
  rdfs:comment "A day of the week which is Sunday or Saturday." ;
  cims:stereotype "enum" .

nc:EnergyDemandKind.consumption a nc:EnergyDemandKind ;
  rdfs:label "consumption"@en ;
  cims:stereotype "enum" .

nc:EnergyDemandKind.export a nc:EnergyDemandKind ;
  rdfs:label "export"@en ;
  cims:stereotype "enum" .

nc:EnergyDemandKind.import a nc:EnergyDemandKind ;
  rdfs:label "import"@en ;
  cims:stereotype "enum" .

nc:EnergyDemandKind.production a nc:EnergyDemandKind ;
  rdfs:label "production"@en ;
  cims:stereotype "enum" .

nc:EnergyDemandKind.storage a nc:EnergyDemandKind ;
  rdfs:label "storage"@en ;
  cims:stereotype "enum" .

nc:PeakKind.offPeak a nc:PeakKind ;
  rdfs:label "offPeak"@en ;
  rdfs:comment "Off-peak refer to periods of lower demand for a particular service or commodity." ;
  cims:stereotype "enum" .

nc:PeakKind.onPeak a nc:PeakKind ;
  rdfs:label "onPeak"@en ;
  rdfs:comment "Off-peak refer to periods of higher demand for a particular service or commodity." ;
  cims:stereotype "enum" .

nc:PowerBidDependencyKind.exclusive a nc:PowerBidDependencyKind ;
  rdfs:label "exclusive"@en ;
  rdfs:comment "Bids are exclusive depending on each other. e.g. Only one of the bids can be activated at the same time." ;
  cims:stereotype "enum" .

nc:PowerBidDependencyKind.inclusive a nc:PowerBidDependencyKind ;
  rdfs:label "inclusive"@en ;
  rdfs:comment "Bids are inclusive depending on each other. e.g. Both bids need to be activated if one of them is activated." ;
  cims:stereotype "enum" .

nc:PowerBidDependencyKind.restrictive a nc:PowerBidDependencyKind ;
  rdfs:label "restrictive"@en ;
  rdfs:comment "Bids are restrictive depending on each other. e.g. You have to take the father bid before you might take the child bid." ;
  cims:stereotype "enum" .

nc:SecuredExclusionReasonKind.capacityCalculationRegion a nc:SecuredExclusionReasonKind ;
  rdfs:label "capacityCalculationRegion"@en ;
  rdfs:comment "The network element that is going to be assessed is excluded for being secured by the capacity calculation region." ;
  cims:stereotype "enum" .

nc:SecuredExclusionReasonKind.nonNativeCapacityCalculationRegion a nc:SecuredExclusionReasonKind ;
  rdfs:label "nonNativeCapacityCalculationRegion"@en ;
  rdfs:comment "The network element that is going to be assessed is excluded for being secured for the native capacity calculation region since it would be secured for a non native capacity calculation region." ;
  cims:stereotype "enum" .

nc:SecuredExclusionReasonKind.systemOperator a nc:SecuredExclusionReasonKind ;
  rdfs:label "systemOperator"@en ;
  rdfs:comment "The network element that is going to be assessed is excluded for being secured by the system operator." ;
  cims:stereotype "enum" .

nc:TimeSeriesInterpolationKind.linear a nc:TimeSeriesInterpolationKind ;
  rdfs:label "linear"@en ;
  rdfs:comment "Linear interpolation is applied for values between two time points." ;
  cims:stereotype "enum" .

nc:TimeSeriesInterpolationKind.next a nc:TimeSeriesInterpolationKind ;
  rdfs:label "next"@en ;
  rdfs:comment "The value between two time points is set to next value." ;
  cims:stereotype "enum" .

nc:TimeSeriesInterpolationKind.none a nc:TimeSeriesInterpolationKind ;
  rdfs:label "none"@en ;
  rdfs:comment "No interpolation is applied." ;
  cims:stereotype "enum" .

nc:TimeSeriesInterpolationKind.previous a nc:TimeSeriesInterpolationKind ;
  rdfs:label "previous"@en ;
  rdfs:comment "The value between two time points is set to previous value." ;
  cims:stereotype "enum" .

nc:ValueOffsetKind.absolute a nc:ValueOffsetKind ;
  rdfs:label "absolute"@en ;
  rdfs:comment "Value of the range constraint is replacing the attribute value referenced by the PropertyReference in a determined operational scenario." ;
  cims:stereotype "enum" .

nc:ValueOffsetKind.incremental a nc:ValueOffsetKind ;
  rdfs:label "incremental"@en ;
  rdfs:comment "Value of the range constraint is incrementing the attribute value referenced by the PropertyReference in a determined operational scenario." ;
  cims:stereotype "enum" .

nc:ValueOffsetKind.incrementalPercentage a nc:ValueOffsetKind ;
  rdfs:label "incrementalPercentage"@en ;
  rdfs:comment "Value of the range constraint is incrementing in percentage the attribute value referenced by the PropertyReference in a determined operational scenario. " ;
  cims:stereotype "enum" .

sis:Package_DocStateInstructionScheduleProfile a cims:ClassCategory ;
  rdfs:label "DocStateInstructionScheduleProfile"@en ;
  rdfs:comment "This package contains datatypes used only in the RDFS header." .

sis:Package_StateInstructionScheduleProfile a cims:ClassCategory ;
  rdfs:label "StateInstructionScheduleProfile"@en ;
  rdfs:comment "This package contains the state instruction schedule profile." .


