@prefix     cim: <https://cim.ucaiug.io/ns#> .
@prefix    cims: <http://iec.ch/TC57/1999/rdf-schema-extensions-19990926#> .
@prefix      eu: <https://cim.ucaiug.io/ns/eu#> .
@prefix      eq: <http://iec.ch/TC57/ns/CIM/CoreEquipment-EU#> .
@prefix    dcat: <http://www.w3.org/ns/dcat#> .
@prefix     dct: <http://purl.org/dc/terms/> .
@prefix     owl: <http://www.w3.org/2002/07/owl#> .
@prefix     rdf: <http://www.w3.org/1999/02/22-rdf-syntax-ns#> .
@prefix    rdfs: <http://www.w3.org/2000/01/rdf-schema#> .
@prefix     xsd: <http://www.w3.org/2001/XMLSchema#> .

cim:ACDCConverter a rdfs:Class ;
  rdfs:label "ACDCConverter"@en ;
  rdfs:comment "A unit with valves for three phases, together with unit control equipment, essential protective and switching devices, DC storage capacitors, phase reactors and auxiliaries, if any, used for conversion." ;
  cims:belongsToCategory eq:Package_CoreEquipmentProfile ;
  rdfs:subClassOf cim:ConductingEquipment .

cim:ACDCConverterDCTerminal a rdfs:Class ;
  rdfs:label "ACDCConverterDCTerminal"@en ;
  rdfs:comment "A DC electrical connection point at the AC/DC converter. The AC/DC converter is electrically connected also to the AC side. The AC connection is inherited from the AC conducting equipment in the same way as any other AC equipment. The AC/DC converter DC terminal is separate from generic DC terminal to restrict the connection with the AC side to AC/DC converter and so that no other DC conducting equipment can be connected to the AC side." ;
  cims:belongsToCategory eq:Package_CoreEquipmentProfile ;
  cims:stereotype <http://iec.ch/TC57/NonStandard/UML#concrete> ;
  rdfs:subClassOf cim:DCBaseTerminal .

cim:ACDCTerminal a rdfs:Class ;
  rdfs:label "ACDCTerminal"@en ;
  rdfs:comment "An electrical connection point (AC or DC) to a piece of conducting equipment. Terminals are connected at physical connection points called connectivity nodes." ;
  cims:belongsToCategory eq:Package_CoreEquipmentProfile ;
  rdfs:subClassOf cim:IdentifiedObject .

cim:ACLineSegment a rdfs:Class ;
  rdfs:label "ACLineSegment"@en ;
  rdfs:comment """A wire or combination of wires, with consistent electrical characteristics, building a single electrical system, used to carry alternating current between points in the power system.
For symmetrical, transposed three phase lines, it is sufficient to use attributes of the line segment, which describe impedances and admittances for the entire length of the segment.  Additionally impedances can be computed by using length and associated per length impedances.
The BaseVoltage at the two ends of ACLineSegments in a Line shall have the same BaseVoltage.nominalVoltage. However, boundary lines may have slightly different BaseVoltage.nominalVoltages and variation is allowed. Larger voltage difference in general requires use of an equivalent branch.""" ;
  cims:belongsToCategory eq:Package_CoreEquipmentProfile ;
  cims:stereotype <http://iec.ch/TC57/NonStandard/UML#concrete> ;
  rdfs:subClassOf cim:Conductor .

cim:ActivePower a rdfs:Class ;
  rdfs:label "ActivePower"@en ;
  rdfs:comment "Product of RMS value of the voltage and the RMS value of the in-phase component of the current." ;
  cims:belongsToCategory eq:Package_CoreEquipmentProfile ;
  cims:stereotype "CIMDatatype" .

cim:ActivePowerLimit a rdfs:Class ;
  rdfs:label "ActivePowerLimit"@en ;
  rdfs:comment "Limit on active power flow." ;
  cims:belongsToCategory eq:Package_CoreEquipmentProfile ;
  cims:stereotype <http://iec.ch/TC57/NonStandard/UML#concrete> ;
  rdfs:subClassOf cim:OperationalLimit .

cim:ActivePowerPerCurrentFlow a rdfs:Class ;
  rdfs:label "ActivePowerPerCurrentFlow"@en ;
  rdfs:comment "Active power variation with current flow." ;
  cims:belongsToCategory eq:Package_CoreEquipmentProfile ;
  cims:stereotype "CIMDatatype" .

cim:ActivePowerPerFrequency a rdfs:Class ;
  rdfs:label "ActivePowerPerFrequency"@en ;
  rdfs:comment "Active power variation with frequency." ;
  cims:belongsToCategory eq:Package_CoreEquipmentProfile ;
  cims:stereotype "CIMDatatype" .

cim:AngleDegrees a rdfs:Class ;
  rdfs:label "AngleDegrees"@en ;
  rdfs:comment "Measurement of angle in degrees." ;
  cims:belongsToCategory eq:Package_CoreEquipmentProfile ;
  cims:stereotype "CIMDatatype" .

cim:ApparentPower a rdfs:Class ;
  rdfs:label "ApparentPower"@en ;
  rdfs:comment "Product of the RMS value of the voltage and the RMS value of the current." ;
  cims:belongsToCategory eq:Package_CoreEquipmentProfile ;
  cims:stereotype "CIMDatatype" .

cim:ApparentPowerLimit a rdfs:Class ;
  rdfs:label "ApparentPowerLimit"@en ;
  rdfs:comment "Apparent power limit." ;
  cims:belongsToCategory eq:Package_CoreEquipmentProfile ;
  cims:stereotype <http://iec.ch/TC57/NonStandard/UML#concrete> ;
  rdfs:subClassOf cim:OperationalLimit .

cim:AsynchronousMachine a rdfs:Class ;
  rdfs:label "AsynchronousMachine"@en ;
  rdfs:comment "A rotating machine whose shaft rotates asynchronously with the electrical field.  Also known as an induction machine with no external connection to the rotor windings, e.g. squirrel-cage induction machine." ;
  cims:belongsToCategory eq:Package_CoreEquipmentProfile ;
  cims:stereotype <http://iec.ch/TC57/NonStandard/UML#concrete> ;
  rdfs:subClassOf cim:RotatingMachine .

cim:AuxiliaryEquipment a rdfs:Class ;
  rdfs:label "AuxiliaryEquipment"@en ;
  rdfs:comment """AuxiliaryEquipment describe equipment that is not performing any primary functions but support for the equipment performing the primary function.
AuxiliaryEquipment is attached to primary equipment via an association with Terminal.""" ;
  cims:belongsToCategory eq:Package_CoreEquipmentProfile ;
  rdfs:subClassOf cim:Equipment .

cim:BaseVoltage a rdfs:Class ;
  rdfs:label "BaseVoltage"@en ;
  rdfs:comment "Defines a system base voltage which is referenced. " ;
  cims:belongsToCategory eq:Package_CoreEquipmentProfile ;
  cims:stereotype <http://iec.ch/TC57/NonStandard/UML#concrete> ;
  rdfs:subClassOf cim:IdentifiedObject .

cim:BasicIntervalSchedule a rdfs:Class ;
  rdfs:label "BasicIntervalSchedule"@en ;
  rdfs:comment "Schedule of values at points in time." ;
  cims:belongsToCategory eq:Package_CoreEquipmentProfile ;
  rdfs:subClassOf cim:IdentifiedObject .

cim:BatteryUnit a rdfs:Class ;
  rdfs:label "BatteryUnit"@en ;
  rdfs:comment "An electrochemical energy storage device." ;
  cims:belongsToCategory eq:Package_CoreEquipmentProfile ;
  cims:stereotype <http://iec.ch/TC57/NonStandard/UML#concrete> ;
  rdfs:subClassOf cim:PowerElectronicsUnit .

cim:Bay a rdfs:Class ;
  rdfs:label "Bay"@en ;
  rdfs:comment "A collection of power system resources (within a given substation) including conducting equipment, protection relays, measurements, and telemetry.  A bay typically represents a physical grouping related to modularization of equipment." ;
  cims:belongsToCategory eq:Package_CoreEquipmentProfile ;
  cims:stereotype <http://iec.ch/TC57/NonStandard/UML#concrete> ;
  rdfs:subClassOf cim:EquipmentContainer .

cim:Boolean a rdfs:Class ;
  rdfs:label "Boolean"@en ;
  rdfs:comment "A type with the value space \"true\" and \"false\"." ;
  cims:belongsToCategory eq:Package_CoreEquipmentProfile ;
  cims:stereotype "Primitive" .

cim:Breaker a rdfs:Class ;
  rdfs:label "Breaker"@en ;
  rdfs:comment "A mechanical switching device capable of making, carrying, and breaking currents under normal circuit conditions and also making, carrying for a specified time, and breaking currents under specified abnormal circuit conditions e.g.  those of short circuit." ;
  cims:belongsToCategory eq:Package_CoreEquipmentProfile ;
  cims:stereotype <http://iec.ch/TC57/NonStandard/UML#concrete> ;
  rdfs:subClassOf cim:ProtectedSwitch .

cim:BusNameMarker a rdfs:Class ;
  rdfs:label "BusNameMarker"@en ;
  rdfs:comment "Used to apply user standard names to TopologicalNodes. Associated with one or more terminals that are normally connected with the bus name.    The associated terminals are normally connected by non-retained switches. For a ring bus station configuration, all BusbarSection terminals in the ring are typically associated.   For a breaker and a half scheme, both BusbarSections would normally be associated.  For a ring bus, all BusbarSections would normally be associated.  For a \"straight\" busbar configuration, normally only the main terminal at the BusbarSection would be associated.  " ;
  cims:belongsToCategory eq:Package_CoreEquipmentProfile ;
  cims:stereotype <http://iec.ch/TC57/NonStandard/UML#concrete> ;
  rdfs:subClassOf cim:IdentifiedObject .

cim:BusbarSection a rdfs:Class ;
  rdfs:label "BusbarSection"@en ;
  rdfs:comment """A conductor, or group of conductors, with negligible impedance, that serve to connect other conducting equipment within a single substation. 
Voltage measurements are typically obtained from voltage transformers that are connected to busbar sections. A bus bar section may have many physical terminals but for analysis is modelled with exactly one logical terminal.""" ;
  cims:belongsToCategory eq:Package_CoreEquipmentProfile ;
  cims:stereotype <http://iec.ch/TC57/NonStandard/UML#concrete> ;
  rdfs:subClassOf cim:Connector .

cim:CAESPlant a rdfs:Class ;
  rdfs:label "CAESPlant"@en ;
  rdfs:comment "Compressed air energy storage plant." ;
  cims:belongsToCategory eq:Package_CoreEquipmentProfile ;
  cims:stereotype <http://iec.ch/TC57/NonStandard/UML#concrete> ;
  rdfs:subClassOf cim:PowerSystemResource .

cim:Capacitance a rdfs:Class ;
  rdfs:label "Capacitance"@en ;
  rdfs:comment "Capacitive part of reactance (imaginary part of impedance), at rated frequency." ;
  cims:belongsToCategory eq:Package_CoreEquipmentProfile ;
  cims:stereotype "CIMDatatype" .

cim:Clamp a rdfs:Class ;
  rdfs:label "Clamp"@en ;
  rdfs:comment """A Clamp is a galvanic connection at a line segment where other equipment is connected. A Clamp does not cut the line segment. 
A Clamp is ConductingEquipment and has one Terminal with an associated ConnectivityNode. Any other ConductingEquipment can be connected to the Clamp ConnectivityNode.""" ;
  cims:belongsToCategory eq:Package_CoreEquipmentProfile ;
  cims:stereotype <http://iec.ch/TC57/NonStandard/UML#concrete> ;
  rdfs:subClassOf cim:ConductingEquipment .

cim:CogenerationPlant a rdfs:Class ;
  rdfs:label "CogenerationPlant"@en ;
  rdfs:comment "A set of thermal generating units for the production of electrical energy and process steam (usually from the output of the steam turbines). The steam sendout is typically used for industrial purposes or for municipal heating and cooling." ;
  cims:belongsToCategory eq:Package_CoreEquipmentProfile ;
  cims:stereotype <http://iec.ch/TC57/NonStandard/UML#concrete> ;
  rdfs:subClassOf cim:PowerSystemResource .

cim:CombinedCyclePlant a rdfs:Class ;
  rdfs:label "CombinedCyclePlant"@en ;
  rdfs:comment "A set of combustion turbines and steam turbines where the exhaust heat from the combustion turbines is recovered to make steam for the steam turbines, resulting in greater overall plant efficiency." ;
  cims:belongsToCategory eq:Package_CoreEquipmentProfile ;
  cims:stereotype <http://iec.ch/TC57/NonStandard/UML#concrete> ;
  rdfs:subClassOf cim:PowerSystemResource .

cim:Conductance a rdfs:Class ;
  rdfs:label "Conductance"@en ;
  rdfs:comment "Factor by which voltage must be multiplied to give corresponding power lost from a circuit. Real part of admittance." ;
  cims:belongsToCategory eq:Package_CoreEquipmentProfile ;
  cims:stereotype "CIMDatatype" .

cim:ConductingEquipment a rdfs:Class ;
  rdfs:label "ConductingEquipment"@en ;
  rdfs:comment "The parts of the AC power system that are designed to carry current or that are conductively connected through terminals." ;
  cims:belongsToCategory eq:Package_CoreEquipmentProfile ;
  rdfs:subClassOf cim:Equipment .

cim:Conductor a rdfs:Class ;
  rdfs:label "Conductor"@en ;
  rdfs:comment "Combination of conducting material with consistent electrical characteristics, building a single electrical system, used to carry current between points in the power system.  " ;
  cims:belongsToCategory eq:Package_CoreEquipmentProfile ;
  rdfs:subClassOf cim:ConductingEquipment .

cim:ConformLoad a rdfs:Class ;
  rdfs:label "ConformLoad"@en ;
  rdfs:comment "ConformLoad represent loads that follow a daily load change pattern where the pattern can be used to scale the load with a system load." ;
  cims:belongsToCategory eq:Package_CoreEquipmentProfile ;
  cims:stereotype <http://iec.ch/TC57/NonStandard/UML#concrete> ;
  rdfs:subClassOf cim:EnergyConsumer .

cim:ConformLoadGroup a rdfs:Class ;
  rdfs:label "ConformLoadGroup"@en ;
  rdfs:comment "A group of loads conforming to an allocation pattern. " ;
  cims:belongsToCategory eq:Package_CoreEquipmentProfile ;
  cims:stereotype <http://iec.ch/TC57/NonStandard/UML#concrete> ;
  rdfs:subClassOf cim:LoadGroup .

cim:ConformLoadSchedule a rdfs:Class ;
  rdfs:label "ConformLoadSchedule"@en ;
  rdfs:comment "A curve of load  versus time (X-axis) showing the active power values (Y1-axis) and reactive power (Y2-axis) for each unit of the period covered. This curve represents a typical pattern of load over the time period for a given day type and season." ;
  cims:belongsToCategory eq:Package_CoreEquipmentProfile ;
  cims:stereotype <http://iec.ch/TC57/NonStandard/UML#concrete> ;
  rdfs:subClassOf cim:SeasonDayTypeSchedule .

cim:ConnectivityNode a rdfs:Class ;
  rdfs:label "ConnectivityNode"@en ;
  rdfs:comment "Connectivity nodes are points where terminals of AC conducting equipment are connected together with zero impedance." ;
  cims:belongsToCategory eq:Package_CoreEquipmentProfile ;
  cims:stereotype <http://iec.ch/TC57/NonStandard/UML#concrete> ;
  rdfs:subClassOf cim:IdentifiedObject .

cim:ConnectivityNodeContainer a rdfs:Class ;
  rdfs:label "ConnectivityNodeContainer"@en ;
  rdfs:comment "A base class for all objects that may contain connectivity nodes or topological nodes." ;
  cims:belongsToCategory eq:Package_CoreEquipmentProfile ;
  rdfs:subClassOf cim:PowerSystemResource .

cim:Connector a rdfs:Class ;
  rdfs:label "Connector"@en ;
  rdfs:comment "A conductor, or group of conductors, with negligible impedance, that serve to connect other conducting equipment within a single substation and are modelled with a single logical terminal." ;
  cims:belongsToCategory eq:Package_CoreEquipmentProfile ;
  rdfs:subClassOf cim:ConductingEquipment .

cim:ControlArea a rdfs:Class ;
  rdfs:label "ControlArea"@en ;
  rdfs:comment """A control area is a grouping of generating units and/or loads and a cutset of tie lines (as terminals) which may be used for a variety of purposes including automatic generation control, power flow solution area interchange control specification, and input to load forecasting. All generation and load within the area defined by the terminals on the border are considered in the area interchange control. Note that any number of overlapping control area specifications can be superimposed on the physical model. The following general principles apply to ControlArea:
1.  The control area orientation for net interchange is positive for an import, negative for an export.
2.  The control area net interchange is determined by summing flows in Terminals. The Terminals are identified by creating a set of TieFlow objects associated with a ControlArea object. Each TieFlow object identifies one Terminal.
3.  In a single network model, a tie between two control areas must be modelled in both control area specifications, such that the two representations of the tie flow sum to zero.
4.  The normal orientation of Terminal flow is positive for flow into the conducting equipment that owns the Terminal. (i.e. flow from a bus into a device is positive.) However, the orientation of each flow in the control area specification must align with the control area convention, i.e. import is positive. If the orientation of the Terminal flow referenced by a TieFlow is positive into the control area, then this is confirmed by setting TieFlow.positiveFlowIn flag TRUE. If not, the orientation must be reversed by setting the TieFlow.positiveFlowIn flag FALSE.""" ;
  cims:belongsToCategory eq:Package_CoreEquipmentProfile ;
  cims:stereotype <http://iec.ch/TC57/NonStandard/UML#concrete> ;
  rdfs:subClassOf cim:PowerSystemResource .

cim:ControlAreaGeneratingUnit a rdfs:Class ;
  rdfs:label "ControlAreaGeneratingUnit"@en ;
  rdfs:comment "A control area generating unit. This class is needed so that alternate control area definitions may include the same generating unit.   It should be noted that only one instance within a control area should reference a specific generating unit." ;
  cims:belongsToCategory eq:Package_CoreEquipmentProfile ;
  cims:stereotype <http://iec.ch/TC57/NonStandard/UML#concrete> ;
  rdfs:subClassOf cim:IdentifiedObject .

cim:ControlAreaTypeKind a rdfs:Class ;
  rdfs:label "ControlAreaTypeKind"@en ;
  rdfs:comment "The type of control area." ;
  cims:belongsToCategory eq:Package_CoreEquipmentProfile ;
  cims:stereotype <http://iec.ch/TC57/NonStandard/UML#enumeration> .

cim:CsConverter a rdfs:Class ;
  rdfs:label "CsConverter"@en ;
  rdfs:comment """DC side of the current source converter (CSC).
The firing angle controls the dc voltage at the converter, both for rectifier and inverter. The difference between the dc voltages of the rectifier and inverter determines the dc current. The extinction angle is used to limit the dc voltage at the inverter, if needed, and is not used in active power control. The firing angle, transformer tap position and number of connected filters are the primary means to control a current source dc line. Higher level controls are built on top, e.g. dc voltage, dc current and active power. From a steady state perspective it is sufficient to specify the wanted active power transfer (ACDCConverter.targetPpcc) and the control functions will set the dc voltage, dc current, firing angle, transformer tap position and number of connected filters to meet this. Therefore attributes targetAlpha and targetGamma are not applicable in this case.
The reactive power consumed by the converter is a function of the firing angle, transformer tap position and number of connected filter, which can be approximated with half of the active power. The losses is a function of the dc voltage and dc current.
The attributes minAlpha and maxAlpha define the range of firing angles for rectifier operation between which no discrete tap changer action takes place. The range is typically 10-18 degrees.
The attributes minGamma and maxGamma define the range of extinction angles for inverter operation between which no discrete tap changer action takes place. The range is typically 17-20 degrees.""" ;
  cims:belongsToCategory eq:Package_CoreEquipmentProfile ;
  cims:stereotype <http://iec.ch/TC57/NonStandard/UML#concrete> ;
  rdfs:subClassOf cim:ACDCConverter .

cim:Currency a rdfs:Class ;
  rdfs:label "Currency"@en ;
  rdfs:comment "Monetary currencies.  ISO 4217 standard including 3-character currency code." ;
  cims:belongsToCategory eq:Package_CoreEquipmentProfile ;
  cims:stereotype <http://iec.ch/TC57/NonStandard/UML#enumeration> .

cim:CurrentFlow a rdfs:Class ;
  rdfs:label "CurrentFlow"@en ;
  rdfs:comment "Electrical current with sign convention: positive flow is out of the conducting equipment into the connectivity node. Can be both AC and DC." ;
  cims:belongsToCategory eq:Package_CoreEquipmentProfile ;
  cims:stereotype "CIMDatatype" .

cim:CurrentLimit a rdfs:Class ;
  rdfs:label "CurrentLimit"@en ;
  rdfs:comment "Operational limit on current. " ;
  cims:belongsToCategory eq:Package_CoreEquipmentProfile ;
  cims:stereotype <http://iec.ch/TC57/NonStandard/UML#concrete> ;
  rdfs:subClassOf cim:OperationalLimit .

cim:CurrentTransformer a rdfs:Class ;
  rdfs:label "CurrentTransformer"@en ;
  rdfs:comment "Instrument transformer used to measure electrical qualities of the circuit that is being protected and/or monitored. Typically used as current transducer for the purpose of metering or protection. A typical secondary current rating would be 5A." ;
  cims:belongsToCategory eq:Package_CoreEquipmentProfile ;
  cims:stereotype <http://iec.ch/TC57/NonStandard/UML#concrete> ;
  rdfs:subClassOf cim:Sensor .

cim:Curve a rdfs:Class ;
  rdfs:label "Curve"@en ;
  rdfs:comment "A multi-purpose curve or functional relationship between an independent variable (X-axis) and dependent (Y-axis) variables. " ;
  cims:belongsToCategory eq:Package_CoreEquipmentProfile ;
  rdfs:subClassOf cim:IdentifiedObject .

cim:CurveData a rdfs:Class ;
  rdfs:label "CurveData"@en ;
  rdfs:comment "Multi-purpose data points for defining a curve.  The use of this generic class is discouraged if a more specific class can be used to specify the X and Y axis values along with their specific data types." ;
  cims:belongsToCategory eq:Package_CoreEquipmentProfile ;
  cims:stereotype <http://iec.ch/TC57/NonStandard/UML#concrete> .

cim:CurveStyle a rdfs:Class ;
  rdfs:label "CurveStyle"@en ;
  rdfs:comment "Style or shape of curve." ;
  cims:belongsToCategory eq:Package_CoreEquipmentProfile ;
  cims:stereotype <http://iec.ch/TC57/NonStandard/UML#enumeration> .

cim:Cut a rdfs:Class ;
  rdfs:label "Cut"@en ;
  rdfs:comment """A cut separates a line segment into two parts. The cut appears as a switch inserted between these two parts and connects them together. As the cut is normally open there is no galvanic connection between the two line segment parts. But it is possible to close the cut to get galvanic connection.
The cut terminals are oriented towards the line segment terminals with the same sequence number. Hence the cut terminal with sequence number equal to 1 is oriented to the line segment's terminal with sequence number equal to 1.
The cut terminals also act as connection points for jumpers and other equipment, e.g. a mobile generator. To enable this, connectivity nodes are placed at the cut terminals. Once the connectivity nodes are in place any conducting equipment can be connected at them.""" ;
  cims:belongsToCategory eq:Package_CoreEquipmentProfile ;
  cims:stereotype <http://iec.ch/TC57/NonStandard/UML#concrete> ;
  rdfs:subClassOf cim:Switch .

cim:DCBaseTerminal a rdfs:Class ;
  rdfs:label "DCBaseTerminal"@en ;
  rdfs:comment "An electrical connection point at a piece of DC conducting equipment. DC terminals are connected at one physical DC node that may have multiple DC terminals connected. A DC node is similar to an AC connectivity node. The model requires that DC connections are distinct from AC connections. " ;
  cims:belongsToCategory eq:Package_CoreEquipmentProfile ;
  rdfs:subClassOf cim:ACDCTerminal .

cim:DCBreaker a rdfs:Class ;
  rdfs:label "DCBreaker"@en ;
  rdfs:comment "A breaker within a DC system. " ;
  cims:belongsToCategory eq:Package_CoreEquipmentProfile ;
  cims:stereotype <http://iec.ch/TC57/NonStandard/UML#concrete> ;
  rdfs:subClassOf cim:DCSwitch .

cim:DCBusbar a rdfs:Class ;
  rdfs:label "DCBusbar"@en ;
  rdfs:comment "A busbar within a DC system." ;
  cims:belongsToCategory eq:Package_CoreEquipmentProfile ;
  cims:stereotype <http://iec.ch/TC57/NonStandard/UML#concrete> ;
  rdfs:subClassOf cim:DCConductingEquipment .

cim:DCChopper a rdfs:Class ;
  rdfs:label "DCChopper"@en ;
  rdfs:comment "Low resistance equipment used in the internal DC circuit to balance voltages. It has typically positive and negative pole terminals and a ground." ;
  cims:belongsToCategory eq:Package_CoreEquipmentProfile ;
  cims:stereotype <http://iec.ch/TC57/NonStandard/UML#concrete> ;
  rdfs:subClassOf cim:DCConductingEquipment .

cim:DCConductingEquipment a rdfs:Class ;
  rdfs:label "DCConductingEquipment"@en ;
  rdfs:comment "The parts of the DC power system that are designed to carry current or that are conductively connected through DC terminals." ;
  cims:belongsToCategory eq:Package_CoreEquipmentProfile ;
  rdfs:subClassOf cim:Equipment .

cim:DCConverterOperatingModeKind a rdfs:Class ;
  rdfs:label "DCConverterOperatingModeKind"@en ;
  rdfs:comment "The operating mode of an HVDC bipole." ;
  cims:belongsToCategory eq:Package_CoreEquipmentProfile ;
  cims:stereotype <http://iec.ch/TC57/NonStandard/UML#enumeration> .

cim:DCConverterUnit a rdfs:Class ;
  rdfs:label "DCConverterUnit"@en ;
  rdfs:comment "Indivisible operative unit comprising all equipment between the point of common coupling on the AC side and the point of common coupling – DC side, essentially one or more converters, together with one or more converter transformers, converter control equipment, essential protective and switching devices and auxiliaries, if any, used for conversion." ;
  cims:belongsToCategory eq:Package_CoreEquipmentProfile ;
  cims:stereotype <http://iec.ch/TC57/NonStandard/UML#concrete> ;
  rdfs:subClassOf cim:DCEquipmentContainer .

cim:DCDisconnector a rdfs:Class ;
  rdfs:label "DCDisconnector"@en ;
  rdfs:comment "A disconnector within a DC system." ;
  cims:belongsToCategory eq:Package_CoreEquipmentProfile ;
  cims:stereotype <http://iec.ch/TC57/NonStandard/UML#concrete> ;
  rdfs:subClassOf cim:DCSwitch .

cim:DCEquipmentContainer a rdfs:Class ;
  rdfs:label "DCEquipmentContainer"@en ;
  rdfs:comment "A modelling construct to provide a root class for containment of DC as well as AC equipment. The class differ from the EquipmentContaner for AC in that it may also contain DCNode-s. Hence it can contain both AC and DC equipment." ;
  cims:belongsToCategory eq:Package_CoreEquipmentProfile ;
  rdfs:subClassOf cim:EquipmentContainer .

cim:DCGround a rdfs:Class ;
  rdfs:label "DCGround"@en ;
  rdfs:comment "A ground within a DC system." ;
  cims:belongsToCategory eq:Package_CoreEquipmentProfile ;
  cims:stereotype <http://iec.ch/TC57/NonStandard/UML#concrete> ;
  rdfs:subClassOf cim:DCConductingEquipment .

cim:DCLine a rdfs:Class ;
  rdfs:label "DCLine"@en ;
  rdfs:comment "Overhead lines and/or cables connecting two or more HVDC substations." ;
  cims:belongsToCategory eq:Package_CoreEquipmentProfile ;
  cims:stereotype <http://iec.ch/TC57/NonStandard/UML#concrete> ;
  rdfs:subClassOf cim:DCEquipmentContainer .

cim:DCLineSegment a rdfs:Class ;
  rdfs:label "DCLineSegment"@en ;
  rdfs:comment "A wire or combination of wires not insulated from one another, with consistent electrical characteristics, used to carry direct current between points in the DC region of the power system." ;
  cims:belongsToCategory eq:Package_CoreEquipmentProfile ;
  cims:stereotype <http://iec.ch/TC57/NonStandard/UML#concrete> ;
  rdfs:subClassOf cim:DCConductingEquipment .

cim:DCNode a rdfs:Class ;
  rdfs:label "DCNode"@en ;
  rdfs:comment "DC nodes are points where terminals of DC conducting equipment are connected together with zero impedance." ;
  cims:belongsToCategory eq:Package_CoreEquipmentProfile ;
  cims:stereotype <http://iec.ch/TC57/NonStandard/UML#concrete> ;
  rdfs:subClassOf cim:IdentifiedObject .

cim:DCPolarityKind a rdfs:Class ;
  rdfs:label "DCPolarityKind"@en ;
  rdfs:comment "Polarity for DC circuits." ;
  cims:belongsToCategory eq:Package_CoreEquipmentProfile ;
  cims:stereotype <http://iec.ch/TC57/NonStandard/UML#enumeration> .

cim:DCSeriesDevice a rdfs:Class ;
  rdfs:label "DCSeriesDevice"@en ;
  rdfs:comment "A series device within the DC system, typically a reactor used for filtering or smoothing.  Needed for transient and short circuit studies." ;
  cims:belongsToCategory eq:Package_CoreEquipmentProfile ;
  cims:stereotype <http://iec.ch/TC57/NonStandard/UML#concrete> ;
  rdfs:subClassOf cim:DCConductingEquipment .

cim:DCShunt a rdfs:Class ;
  rdfs:label "DCShunt"@en ;
  rdfs:comment "A shunt device within the DC system, typically used for filtering.  Needed for transient and short circuit studies." ;
  cims:belongsToCategory eq:Package_CoreEquipmentProfile ;
  cims:stereotype <http://iec.ch/TC57/NonStandard/UML#concrete> ;
  rdfs:subClassOf cim:DCConductingEquipment .

cim:DCSwitch a rdfs:Class ;
  rdfs:label "DCSwitch"@en ;
  rdfs:comment "A switch within the DC system." ;
  cims:belongsToCategory eq:Package_CoreEquipmentProfile ;
  cims:stereotype <http://iec.ch/TC57/NonStandard/UML#concrete> ;
  rdfs:subClassOf cim:DCConductingEquipment .

cim:DCTerminal a rdfs:Class ;
  rdfs:label "DCTerminal"@en ;
  rdfs:comment "An electrical connection point to generic DC conducting equipment." ;
  cims:belongsToCategory eq:Package_CoreEquipmentProfile ;
  cims:stereotype <http://iec.ch/TC57/NonStandard/UML#concrete> ;
  rdfs:subClassOf cim:DCBaseTerminal .

cim:Date a rdfs:Class ;
  rdfs:label "Date"@en ;
  rdfs:comment "Date as \"yyyy-mm-dd\", which conforms with ISO 8601. UTC time zone is specified as \"yyyy-mm-ddZ\". A local timezone relative UTC is specified as \"yyyy-mm-dd(+/-)hh:mm\"." ;
  cims:belongsToCategory eq:Package_CoreEquipmentProfile ;
  cims:stereotype "Primitive" .

cim:DateTime a rdfs:Class ;
  rdfs:label "DateTime"@en ;
  rdfs:comment "Date and time as \"yyyy-mm-ddThh:mm:ss.sss\", which conforms with ISO 8601. UTC time zone is specified as \"yyyy-mm-ddThh:mm:ss.sssZ\". A local timezone relative UTC is specified as \"yyyy-mm-ddThh:mm:ss.sss-hh:mm\". The second component (shown here as \"ss.sss\") could have any number of digits in its fractional part to allow any kind of precision beyond seconds." ;
  cims:belongsToCategory eq:Package_CoreEquipmentProfile ;
  cims:stereotype "Primitive" .

cim:DayType a rdfs:Class ;
  rdfs:label "DayType"@en ;
  rdfs:comment "Group of similar days.   For example it could be used to represent weekdays, weekend, or holidays." ;
  cims:belongsToCategory eq:Package_CoreEquipmentProfile ;
  cims:stereotype <http://iec.ch/TC57/NonStandard/UML#concrete> ;
  rdfs:subClassOf cim:IdentifiedObject .

cim:Decimal a rdfs:Class ;
  rdfs:label "Decimal"@en ;
  rdfs:comment "Decimal is the base-10 notational system for representing real numbers." ;
  cims:belongsToCategory eq:Package_CoreEquipmentProfile ;
  cims:stereotype "Primitive" .

cim:DisconnectingCircuitBreaker a rdfs:Class ;
  rdfs:label "DisconnectingCircuitBreaker"@en ;
  rdfs:comment "A circuit breaking device including disconnecting function, eliminating the need for separate disconnectors." ;
  cims:belongsToCategory eq:Package_CoreEquipmentProfile ;
  cims:stereotype <http://iec.ch/TC57/NonStandard/UML#concrete> ;
  rdfs:subClassOf cim:Breaker .

cim:Disconnector a rdfs:Class ;
  rdfs:label "Disconnector"@en ;
  rdfs:comment "A manually operated or motor operated mechanical switching device used for changing the connections in a circuit, or for isolating a circuit or equipment from a source of power. It is required to open or close circuits when negligible current is broken or made. " ;
  cims:belongsToCategory eq:Package_CoreEquipmentProfile ;
  cims:stereotype <http://iec.ch/TC57/NonStandard/UML#concrete> ;
  rdfs:subClassOf cim:Switch .

cim:EarthFaultCompensator a rdfs:Class ;
  rdfs:label "EarthFaultCompensator"@en ;
  rdfs:comment "A conducting equipment used to represent a connection to ground which is typically used to compensate earth faults.   An earth fault compensator device modelled with a single terminal implies a second terminal solidly connected to ground.  If two terminals are modelled, the ground is not assumed and normal connection rules apply." ;
  cims:belongsToCategory eq:Package_CoreEquipmentProfile ;
  rdfs:subClassOf cim:ConductingEquipment .

cim:EnergyArea a rdfs:Class ;
  rdfs:label "EnergyArea"@en ;
  rdfs:comment "Describes an area having energy production or consumption.  Specializations are intended to support the load allocation function as typically required in energy management systems or planning studies to allocate hypothesized load levels to individual load points for power flow analysis.  Often the energy area can be linked to both measured and forecast load levels." ;
  cims:belongsToCategory eq:Package_CoreEquipmentProfile ;
  rdfs:subClassOf cim:IdentifiedObject .

cim:EnergyConnection a rdfs:Class ;
  rdfs:label "EnergyConnection"@en ;
  rdfs:comment "A connection of energy generation or consumption on the power system model." ;
  cims:belongsToCategory eq:Package_CoreEquipmentProfile ;
  rdfs:subClassOf cim:ConductingEquipment .

cim:EnergyConsumer a rdfs:Class ;
  rdfs:label "EnergyConsumer"@en ;
  rdfs:comment """Generic user of energy - a  point of consumption on the power system model.
EnergyConsumer.pfixed, .qfixed, .pfixedPct and .qfixedPct have meaning only if there is no LoadResponseCharacteristic associated with EnergyConsumer or if LoadResponseCharacteristic.exponentModel is set to False.""" ;
  cims:belongsToCategory eq:Package_CoreEquipmentProfile ;
  cims:stereotype <http://iec.ch/TC57/NonStandard/UML#concrete> ;
  rdfs:subClassOf cim:EnergyConnection .

cim:EnergySchedulingType a rdfs:Class ;
  rdfs:label "EnergySchedulingType"@en ;
  rdfs:comment "Used to define the type of generation for scheduling purposes." ;
  cims:belongsToCategory eq:Package_CoreEquipmentProfile ;
  cims:stereotype <http://iec.ch/TC57/NonStandard/UML#concrete> ;
  rdfs:subClassOf cim:IdentifiedObject .

cim:EnergySource a rdfs:Class ;
  rdfs:label "EnergySource"@en ;
  rdfs:comment "A generic equivalent for an energy supplier on a transmission or distribution voltage level." ;
  cims:belongsToCategory eq:Package_CoreEquipmentProfile ;
  cims:stereotype <http://iec.ch/TC57/NonStandard/UML#concrete> ;
  rdfs:subClassOf cim:EnergyConnection .

cim:Equipment a rdfs:Class ;
  rdfs:label "Equipment"@en ;
  rdfs:comment "The parts of a power system that are physical devices, electronic or mechanical." ;
  cims:belongsToCategory eq:Package_CoreEquipmentProfile ;
  rdfs:subClassOf cim:PowerSystemResource .

cim:EquipmentContainer a rdfs:Class ;
  rdfs:label "EquipmentContainer"@en ;
  rdfs:comment "A modelling construct to provide a root class for containing equipment. " ;
  cims:belongsToCategory eq:Package_CoreEquipmentProfile ;
  rdfs:subClassOf cim:ConnectivityNodeContainer .

cim:EquivalentBranch a rdfs:Class ;
  rdfs:label "EquivalentBranch"@en ;
  rdfs:comment "The class represents equivalent branches. In cases where a transformer phase shift is modelled and the EquivalentBranch is spanning the same nodes, the impedance quantities for the EquivalentBranch shall consider the needed phase shift." ;
  cims:belongsToCategory eq:Package_CoreEquipmentProfile ;
  cims:stereotype <http://iec.ch/TC57/NonStandard/UML#concrete> ;
  rdfs:subClassOf cim:EquivalentEquipment .

cim:EquivalentEquipment a rdfs:Class ;
  rdfs:label "EquivalentEquipment"@en ;
  rdfs:comment "The class represents equivalent objects that are the result of a network reduction. The class is the base for equivalent objects of different types." ;
  cims:belongsToCategory eq:Package_CoreEquipmentProfile ;
  rdfs:subClassOf cim:ConductingEquipment .

cim:EquivalentInjection a rdfs:Class ;
  rdfs:label "EquivalentInjection"@en ;
  rdfs:comment "This class represents equivalent injections (generation or load).  Voltage regulation is allowed only at the point of connection." ;
  cims:belongsToCategory eq:Package_CoreEquipmentProfile ;
  cims:stereotype <http://iec.ch/TC57/NonStandard/UML#concrete> ;
  rdfs:subClassOf cim:EquivalentEquipment .

cim:EquivalentNetwork a rdfs:Class ;
  rdfs:label "EquivalentNetwork"@en ;
  rdfs:comment "A class that groups electrical equivalents, including internal nodes, of a network that has been reduced. The ConnectivityNodes contained in the equivalent are intended to reflect internal nodes of the equivalent. The boundary Connectivity nodes where the equivalent connects outside itself are not contained by the equivalent." ;
  cims:belongsToCategory eq:Package_CoreEquipmentProfile ;
  cims:stereotype <http://iec.ch/TC57/NonStandard/UML#concrete> ;
  rdfs:subClassOf cim:ConnectivityNodeContainer .

cim:EquivalentShunt a rdfs:Class ;
  rdfs:label "EquivalentShunt"@en ;
  rdfs:comment "The class represents equivalent shunts." ;
  cims:belongsToCategory eq:Package_CoreEquipmentProfile ;
  cims:stereotype <http://iec.ch/TC57/NonStandard/UML#concrete> ;
  rdfs:subClassOf cim:EquivalentEquipment .

cim:ExternalNetworkInjection a rdfs:Class ;
  rdfs:label "ExternalNetworkInjection"@en ;
  rdfs:comment "This class represents the external network and it is used for IEC 60909 calculations." ;
  cims:belongsToCategory eq:Package_CoreEquipmentProfile ;
  cims:stereotype <http://iec.ch/TC57/NonStandard/UML#concrete> ;
  rdfs:subClassOf cim:RegulatingCondEq .

cim:FaultIndicator a rdfs:Class ;
  rdfs:label "FaultIndicator"@en ;
  rdfs:comment "A FaultIndicator is typically only an indicator (which may or may not be remotely monitored), and not a piece of equipment that actually initiates a protection event. It is used for FLISR (Fault Location, Isolation and Restoration) purposes, assisting with the dispatch of crews to \"most likely\" part of the network (i.e. assists with determining circuit section where the fault most likely happened)." ;
  cims:belongsToCategory eq:Package_CoreEquipmentProfile ;
  cims:stereotype <http://iec.ch/TC57/NonStandard/UML#concrete> ;
  rdfs:subClassOf cim:AuxiliaryEquipment .

cim:Float a rdfs:Class ;
  rdfs:label "Float"@en ;
  rdfs:comment "A floating point number. The range is unspecified and not limited." ;
  cims:belongsToCategory eq:Package_CoreEquipmentProfile ;
  cims:stereotype "Primitive" .

cim:FossilFuel a rdfs:Class ;
  rdfs:label "FossilFuel"@en ;
  rdfs:comment "The fossil fuel consumed by the non-nuclear thermal generating unit.   For example, coal, oil, gas, etc.   These are the specific fuels that the generating unit can consume." ;
  cims:belongsToCategory eq:Package_CoreEquipmentProfile ;
  cims:stereotype <http://iec.ch/TC57/NonStandard/UML#concrete> ;
  rdfs:subClassOf cim:IdentifiedObject .

cim:Frequency a rdfs:Class ;
  rdfs:label "Frequency"@en ;
  rdfs:comment "Cycles per second." ;
  cims:belongsToCategory eq:Package_CoreEquipmentProfile ;
  cims:stereotype "CIMDatatype" .

cim:FuelType a rdfs:Class ;
  rdfs:label "FuelType"@en ;
  rdfs:comment "Type of fuel." ;
  cims:belongsToCategory eq:Package_CoreEquipmentProfile ;
  cims:stereotype <http://iec.ch/TC57/NonStandard/UML#enumeration> .

cim:Fuse a rdfs:Class ;
  rdfs:label "Fuse"@en ;
  rdfs:comment "An overcurrent protective device with a circuit opening fusible part that is heated and severed by the passage of overcurrent through it. A fuse is considered a switching device because it breaks current." ;
  cims:belongsToCategory eq:Package_CoreEquipmentProfile ;
  cims:stereotype <http://iec.ch/TC57/NonStandard/UML#concrete> ;
  rdfs:subClassOf cim:Switch .

cim:GeneratingUnit a rdfs:Class ;
  rdfs:label "GeneratingUnit"@en ;
  rdfs:comment "A single or set of synchronous machines for converting mechanical power into alternating-current power. For example, individual machines within a set may be defined for scheduling purposes while a single control signal is derived for the set. In this case there would be a GeneratingUnit for each member of the set and an additional GeneratingUnit corresponding to the set." ;
  cims:belongsToCategory eq:Package_CoreEquipmentProfile ;
  cims:stereotype <http://iec.ch/TC57/NonStandard/UML#concrete> ;
  rdfs:subClassOf cim:Equipment .

cim:GeneratorControlSource a rdfs:Class ;
  rdfs:label "GeneratorControlSource"@en ;
  rdfs:comment "The source of controls for a generating unit." ;
  cims:belongsToCategory eq:Package_CoreEquipmentProfile ;
  cims:stereotype <http://iec.ch/TC57/NonStandard/UML#enumeration> .

cim:GeographicalRegion a rdfs:Class ;
  rdfs:label "GeographicalRegion"@en ;
  rdfs:comment "A geographical region of a power system network model." ;
  cims:belongsToCategory eq:Package_CoreEquipmentProfile ;
  cims:stereotype <http://iec.ch/TC57/NonStandard/UML#concrete> ;
  rdfs:subClassOf cim:IdentifiedObject .

cim:GrossToNetActivePowerCurve a rdfs:Class ;
  rdfs:label "GrossToNetActivePowerCurve"@en ;
  rdfs:comment "Relationship between the generating unit's gross active power output on the X-axis (measured at the terminals of the machine(s)) and the generating unit's net active power output on the Y-axis (based on utility-defined measurements at the power station). Station service loads, when modelled, should be treated as non-conforming bus loads. There may be more than one curve, depending on the auxiliary equipment that is in service." ;
  cims:belongsToCategory eq:Package_CoreEquipmentProfile ;
  cims:stereotype <http://iec.ch/TC57/NonStandard/UML#concrete> ;
  rdfs:subClassOf cim:Curve .

cim:Ground a rdfs:Class ;
  rdfs:label "Ground"@en ;
  rdfs:comment "A point where the system is grounded used for connecting conducting equipment to ground. The power system model can have any number of grounds." ;
  cims:belongsToCategory eq:Package_CoreEquipmentProfile ;
  cims:stereotype <http://iec.ch/TC57/NonStandard/UML#concrete> ;
  rdfs:subClassOf cim:ConductingEquipment .

cim:GroundDisconnector a rdfs:Class ;
  rdfs:label "GroundDisconnector"@en ;
  rdfs:comment "A manually operated or motor operated mechanical switching device used for isolating a circuit or equipment from ground." ;
  cims:belongsToCategory eq:Package_CoreEquipmentProfile ;
  cims:stereotype <http://iec.ch/TC57/NonStandard/UML#concrete> ;
  rdfs:subClassOf cim:Switch .

cim:GroundingImpedance a rdfs:Class ;
  rdfs:label "GroundingImpedance"@en ;
  rdfs:comment "A fixed impedance device used for grounding." ;
  cims:belongsToCategory eq:Package_CoreEquipmentProfile ;
  cims:stereotype <http://iec.ch/TC57/NonStandard/UML#concrete> ;
  rdfs:subClassOf cim:EarthFaultCompensator .

cim:HydroEnergyConversionKind a rdfs:Class ;
  rdfs:label "HydroEnergyConversionKind"@en ;
  rdfs:comment "Specifies the capability of the hydro generating unit to convert energy as a generator or pump." ;
  cims:belongsToCategory eq:Package_CoreEquipmentProfile ;
  cims:stereotype <http://iec.ch/TC57/NonStandard/UML#enumeration> .

cim:HydroGeneratingUnit a rdfs:Class ;
  rdfs:label "HydroGeneratingUnit"@en ;
  rdfs:comment "A generating unit whose prime mover is a hydraulic turbine (e.g., Francis, Pelton, Kaplan)." ;
  cims:belongsToCategory eq:Package_CoreEquipmentProfile ;
  cims:stereotype <http://iec.ch/TC57/NonStandard/UML#concrete> ;
  rdfs:subClassOf cim:GeneratingUnit .

cim:HydroPlantStorageKind a rdfs:Class ;
  rdfs:label "HydroPlantStorageKind"@en ;
  rdfs:comment "The type of hydro power plant." ;
  cims:belongsToCategory eq:Package_CoreEquipmentProfile ;
  cims:stereotype <http://iec.ch/TC57/NonStandard/UML#enumeration> .

cim:HydroPowerPlant a rdfs:Class ;
  rdfs:label "HydroPowerPlant"@en ;
  rdfs:comment "A hydro power station which can generate or pump. When generating, the generator turbines receive water from an upper reservoir. When pumping, the pumps receive their water from a lower reservoir." ;
  cims:belongsToCategory eq:Package_CoreEquipmentProfile ;
  cims:stereotype <http://iec.ch/TC57/NonStandard/UML#concrete> ;
  rdfs:subClassOf cim:PowerSystemResource .

cim:HydroPump a rdfs:Class ;
  rdfs:label "HydroPump"@en ;
  rdfs:comment "A synchronous motor-driven pump, typically associated with a pumped storage plant." ;
  cims:belongsToCategory eq:Package_CoreEquipmentProfile ;
  cims:stereotype <http://iec.ch/TC57/NonStandard/UML#concrete> ;
  rdfs:subClassOf cim:Equipment .

cim:HydroTurbineKind a rdfs:Class ;
  rdfs:label "HydroTurbineKind"@en ;
  rdfs:comment "Type of turbine." ;
  cims:belongsToCategory eq:Package_CoreEquipmentProfile ;
  cims:stereotype <http://iec.ch/TC57/NonStandard/UML#enumeration> .

cim:IdentifiedObject a rdfs:Class ;
  rdfs:label "IdentifiedObject"@en ;
  rdfs:comment "This is a root class to provide common identification for all classes needing identification and naming attributes." ;
  cims:belongsToCategory eq:Package_CoreEquipmentProfile .

cim:Inductance a rdfs:Class ;
  rdfs:label "Inductance"@en ;
  rdfs:comment "Inductive part of reactance (imaginary part of impedance), at rated frequency." ;
  cims:belongsToCategory eq:Package_CoreEquipmentProfile ;
  cims:stereotype "CIMDatatype" .

cim:Integer a rdfs:Class ;
  rdfs:label "Integer"@en ;
  rdfs:comment "An integer number. The range is unspecified and not limited." ;
  cims:belongsToCategory eq:Package_CoreEquipmentProfile ;
  cims:stereotype "Primitive" .

cim:Jumper a rdfs:Class ;
  rdfs:label "Jumper"@en ;
  rdfs:comment "A short section of conductor with negligible impedance which can be manually removed and replaced if the circuit is de-energized. Note that zero-impedance branches can potentially be modelled by other equipment types." ;
  cims:belongsToCategory eq:Package_CoreEquipmentProfile ;
  cims:stereotype <http://iec.ch/TC57/NonStandard/UML#concrete> ;
  rdfs:subClassOf cim:Switch .

cim:Junction a rdfs:Class ;
  rdfs:label "Junction"@en ;
  rdfs:comment "A point where one or more conducting equipments are connected with zero resistance." ;
  cims:belongsToCategory eq:Package_CoreEquipmentProfile ;
  cims:stereotype <http://iec.ch/TC57/NonStandard/UML#concrete> ;
  rdfs:subClassOf cim:Connector .

cim:Length a rdfs:Class ;
  rdfs:label "Length"@en ;
  rdfs:comment "Unit of length. It shall be a positive value or zero." ;
  cims:belongsToCategory eq:Package_CoreEquipmentProfile ;
  cims:stereotype "CIMDatatype" .

cim:Line a rdfs:Class ;
  rdfs:label "Line"@en ;
  rdfs:comment "Contains equipment beyond a substation belonging to a power transmission line. " ;
  cims:belongsToCategory eq:Package_CoreEquipmentProfile ;
  cims:stereotype <http://iec.ch/TC57/NonStandard/UML#concrete> ;
  rdfs:subClassOf cim:EquipmentContainer .

cim:LinearShuntCompensator a rdfs:Class ;
  rdfs:label "LinearShuntCompensator"@en ;
  rdfs:comment "A linear shunt compensator has banks or sections with equal admittance values." ;
  cims:belongsToCategory eq:Package_CoreEquipmentProfile ;
  cims:stereotype <http://iec.ch/TC57/NonStandard/UML#concrete> ;
  rdfs:subClassOf cim:ShuntCompensator .

cim:LoadArea a rdfs:Class ;
  rdfs:label "LoadArea"@en ;
  rdfs:comment "The class is the root or first level in a hierarchical structure for grouping of loads for the purpose of load flow load scaling." ;
  cims:belongsToCategory eq:Package_CoreEquipmentProfile ;
  cims:stereotype <http://iec.ch/TC57/NonStandard/UML#concrete> ;
  rdfs:subClassOf cim:EnergyArea .

cim:LoadBreakSwitch a rdfs:Class ;
  rdfs:label "LoadBreakSwitch"@en ;
  rdfs:comment "A mechanical switching device capable of making, carrying, and breaking currents under normal operating conditions." ;
  cims:belongsToCategory eq:Package_CoreEquipmentProfile ;
  cims:stereotype <http://iec.ch/TC57/NonStandard/UML#concrete> ;
  rdfs:subClassOf cim:ProtectedSwitch .

cim:LoadGroup a rdfs:Class ;
  rdfs:label "LoadGroup"@en ;
  rdfs:comment "The class is the third level in a hierarchical structure for grouping of loads for the purpose of load flow load scaling." ;
  cims:belongsToCategory eq:Package_CoreEquipmentProfile ;
  rdfs:subClassOf cim:IdentifiedObject .

cim:LoadResponseCharacteristic a rdfs:Class ;
  rdfs:label "LoadResponseCharacteristic"@en ;
  rdfs:comment """Models the characteristic response of the load demand due to changes in system conditions such as voltage and frequency. It is not related to demand response.
If LoadResponseCharacteristic.exponentModel is True, the exponential voltage or frequency dependent models are specified and used as to calculate active and reactive power components of the load model.
The equations to calculate active and reactive power components of the load model are internal to the power flow calculation, hence they use different quantities depending on the use case of the data exchange. 
The equations for exponential voltage dependent load model injected power are: 
pInjection= Pnominal* (Voltage/cim:BaseVoltage.nominalVoltage) ** cim:LoadResponseCharacteristic.pVoltageExponent
qInjection= Qnominal* (Voltage/cim:BaseVoltage.nominalVoltage) ** cim:LoadResponseCharacteristic.qVoltageExponent
Where: 
1) * means "multiply" and ** is "raised to power of";
2) Pnominal and Qnominal represent the active power and reactive power at nominal voltage as any load described by the voltage exponential model shall be given at nominal voltage.  This means that EnergyConsumer.p and EnergyConsumer.q  are at nominal voltage.
3) After power flow is solved: 
-pInjection and qInjection correspond to SvPowerflow.p and SvPowerflow.q respectively.  
- Voltage corresponds to SvVoltage.v at the TopologicalNode where the load is connected.""" ;
  cims:belongsToCategory eq:Package_CoreEquipmentProfile ;
  cims:stereotype <http://iec.ch/TC57/NonStandard/UML#concrete> ;
  rdfs:subClassOf cim:IdentifiedObject .

cim:Money a rdfs:Class ;
  rdfs:label "Money"@en ;
  rdfs:comment "Amount of money." ;
  cims:belongsToCategory eq:Package_CoreEquipmentProfile ;
  cims:stereotype "CIMDatatype" .

cim:MonthDay a rdfs:Class ;
  rdfs:label "MonthDay"@en ;
  rdfs:comment "MonthDay format as \"--mm-dd\", which conforms with XSD data type gMonthDay." ;
  cims:belongsToCategory eq:Package_CoreEquipmentProfile ;
  cims:stereotype "Primitive" .

cim:NonConformLoad a rdfs:Class ;
  rdfs:label "NonConformLoad"@en ;
  rdfs:comment "NonConformLoad represents loads that do not follow a daily load change pattern and whose changes are not correlated with the daily load change pattern." ;
  cims:belongsToCategory eq:Package_CoreEquipmentProfile ;
  cims:stereotype <http://iec.ch/TC57/NonStandard/UML#concrete> ;
  rdfs:subClassOf cim:EnergyConsumer .

cim:NonConformLoadGroup a rdfs:Class ;
  rdfs:label "NonConformLoadGroup"@en ;
  rdfs:comment "Loads that do not follow a daily and seasonal load variation pattern." ;
  cims:belongsToCategory eq:Package_CoreEquipmentProfile ;
  cims:stereotype <http://iec.ch/TC57/NonStandard/UML#concrete> ;
  rdfs:subClassOf cim:LoadGroup .

cim:NonConformLoadSchedule a rdfs:Class ;
  rdfs:label "NonConformLoadSchedule"@en ;
  rdfs:comment "An active power (Y1-axis) and reactive power (Y2-axis) schedule (curves) versus time (X-axis) for non-conforming loads, e.g., large industrial load or power station service (where modelled)." ;
  cims:belongsToCategory eq:Package_CoreEquipmentProfile ;
  cims:stereotype <http://iec.ch/TC57/NonStandard/UML#concrete> ;
  rdfs:subClassOf cim:SeasonDayTypeSchedule .

cim:NonlinearShuntCompensator a rdfs:Class ;
  rdfs:label "NonlinearShuntCompensator"@en ;
  rdfs:comment "A non linear shunt compensator has bank or section admittance values that differ. The attributes g, b, g0 and b0 of the associated NonlinearShuntCompensatorPoint describe the total conductance and admittance of a NonlinearShuntCompensatorPoint at a section number specified by NonlinearShuntCompensatorPoint.sectionNumber." ;
  cims:belongsToCategory eq:Package_CoreEquipmentProfile ;
  cims:stereotype <http://iec.ch/TC57/NonStandard/UML#concrete> ;
  rdfs:subClassOf cim:ShuntCompensator .

cim:NonlinearShuntCompensatorPoint a rdfs:Class ;
  rdfs:label "NonlinearShuntCompensatorPoint"@en ;
  rdfs:comment "A non linear shunt compensator bank or section admittance value. The number of NonlinearShuntCompenstorPoint instances associated with a NonlinearShuntCompensator shall be equal to ShuntCompensator.maximumSections. ShuntCompensator.sections shall only be set to one of the NonlinearShuntCompenstorPoint.sectionNumber. There is no interpolation between NonlinearShuntCompenstorPoint-s." ;
  cims:belongsToCategory eq:Package_CoreEquipmentProfile ;
  cims:stereotype <http://iec.ch/TC57/NonStandard/UML#concrete> .

cim:NuclearGeneratingUnit a rdfs:Class ;
  rdfs:label "NuclearGeneratingUnit"@en ;
  rdfs:comment "A nuclear generating unit." ;
  cims:belongsToCategory eq:Package_CoreEquipmentProfile ;
  cims:stereotype <http://iec.ch/TC57/NonStandard/UML#concrete> ;
  rdfs:subClassOf cim:GeneratingUnit .

cim:OperationalLimit a rdfs:Class ;
  rdfs:label "OperationalLimit"@en ;
  rdfs:comment """A value and normal value associated with a specific kind of limit. 
The sub class value and normalValue attributes vary inversely to the associated OperationalLimitType.acceptableDuration (acceptableDuration for short).  
If a particular piece of equipment has multiple operational limits of the same kind (apparent power, current, etc.), the limit with the greatest acceptableDuration shall have the smallest limit value and the limit with the smallest acceptableDuration shall have the largest limit value.  Note: A large current can only be allowed to flow through a piece of equipment for a short duration without causing damage, but a lesser current can be allowed to flow for a longer duration. """ ;
  cims:belongsToCategory eq:Package_CoreEquipmentProfile ;
  rdfs:subClassOf cim:IdentifiedObject .

cim:OperationalLimitDirectionKind a rdfs:Class ;
  rdfs:label "OperationalLimitDirectionKind"@en ;
  rdfs:comment "The direction attribute describes the side of  a limit that is a violation." ;
  cims:belongsToCategory eq:Package_CoreEquipmentProfile ;
  cims:stereotype <http://iec.ch/TC57/NonStandard/UML#enumeration> .

cim:OperationalLimitSet a rdfs:Class ;
  rdfs:label "OperationalLimitSet"@en ;
  rdfs:comment "A set of limits associated with equipment.  Sets of limits might apply to a specific temperature, or season for example. A set of limits may contain different severities of limit levels that would apply to the same equipment. The set may contain limits of different types such as apparent power and current limits or high and low voltage limits  that are logically applied together as a set." ;
  cims:belongsToCategory eq:Package_CoreEquipmentProfile ;
  cims:stereotype <http://iec.ch/TC57/NonStandard/UML#concrete> ;
  rdfs:subClassOf cim:IdentifiedObject .

cim:OperationalLimitType a rdfs:Class ;
  rdfs:label "OperationalLimitType"@en ;
  rdfs:comment "The operational meaning of a category of limits." ;
  cims:belongsToCategory eq:Package_CoreEquipmentProfile ;
  cims:stereotype <http://iec.ch/TC57/NonStandard/UML#concrete> ;
  rdfs:subClassOf cim:IdentifiedObject .

cim:PerCent a rdfs:Class ;
  rdfs:label "PerCent"@en ;
  rdfs:comment "Percentage on a defined base.   For example, specify as 100 to indicate at the defined base." ;
  cims:belongsToCategory eq:Package_CoreEquipmentProfile ;
  cims:stereotype "CIMDatatype" .

cim:PetersenCoil a rdfs:Class ;
  rdfs:label "PetersenCoil"@en ;
  rdfs:comment "A variable impedance device normally used to offset line charging during single line faults in an ungrounded section of network." ;
  cims:belongsToCategory eq:Package_CoreEquipmentProfile ;
  cims:stereotype <http://iec.ch/TC57/NonStandard/UML#concrete> ;
  rdfs:subClassOf cim:EarthFaultCompensator .

cim:PhaseCode a rdfs:Class ;
  rdfs:label "PhaseCode"@en ;
  rdfs:comment """An unordered enumeration of phase identifiers.  Allows designation of phases for both transmission and distribution equipment, circuits and loads.   The enumeration, by itself, does not describe how the phases are connected together or connected to ground.  Ground is not explicitly denoted as a phase.
Residential and small commercial loads are often served from single-phase, or split-phase, secondary circuits. For the example of s12N, phases 1 and 2 refer to hot wires that are 180 degrees out of phase, while N refers to the neutral wire. Through single-phase transformer connections, these secondary circuits may be served from one or two of the primary phases A, B, and C. For three-phase loads, use the A, B, C phase codes instead of s12N.
The integer values are from IEC 61968-9 to support revenue metering applications.""" ;
  cims:belongsToCategory eq:Package_CoreEquipmentProfile ;
  cims:stereotype <http://iec.ch/TC57/NonStandard/UML#enumeration> .

cim:PhaseTapChanger a rdfs:Class ;
  rdfs:label "PhaseTapChanger"@en ;
  rdfs:comment "A transformer phase shifting tap model that controls the phase angle difference across the power transformer and potentially the active power flow through the power transformer.  This phase tap model may also impact the voltage magnitude." ;
  cims:belongsToCategory eq:Package_CoreEquipmentProfile ;
  rdfs:subClassOf cim:TapChanger .

cim:PhaseTapChangerAsymmetrical a rdfs:Class ;
  rdfs:label "PhaseTapChangerAsymmetrical"@en ;
  rdfs:comment "Describes the tap model for an asymmetrical phase shifting transformer in which the difference voltage vector adds to the in-phase winding. The out-of-phase winding is the transformer end where the tap changer is located.  The angle between the in-phase and out-of-phase windings is named the winding connection angle. The phase shift depends on both the difference voltage magnitude and the winding connection angle." ;
  cims:belongsToCategory eq:Package_CoreEquipmentProfile ;
  cims:stereotype <http://iec.ch/TC57/NonStandard/UML#concrete> ;
  rdfs:subClassOf cim:PhaseTapChangerNonLinear .

cim:PhaseTapChangerLinear a rdfs:Class ;
  rdfs:label "PhaseTapChangerLinear"@en ;
  rdfs:comment """Describes a tap changer with a linear relation between the tap step and the phase angle difference across the transformer. This is a mathematical model that is an approximation of a real phase tap changer.
The phase angle is computed as stepPhaseShiftIncrement times the tap position.
The voltage magnitude of both sides is the same.""" ;
  cims:belongsToCategory eq:Package_CoreEquipmentProfile ;
  cims:stereotype <http://iec.ch/TC57/NonStandard/UML#concrete> ;
  rdfs:subClassOf cim:PhaseTapChanger .

cim:PhaseTapChangerNonLinear a rdfs:Class ;
  rdfs:label "PhaseTapChangerNonLinear"@en ;
  rdfs:comment "The non-linear phase tap changer describes the non-linear behaviour of a phase tap changer. This is a base class for the symmetrical and asymmetrical phase tap changer models. The details of these models can be found in IEC 61970-301." ;
  cims:belongsToCategory eq:Package_CoreEquipmentProfile ;
  rdfs:subClassOf cim:PhaseTapChanger .

cim:PhaseTapChangerSymmetrical a rdfs:Class ;
  rdfs:label "PhaseTapChangerSymmetrical"@en ;
  rdfs:comment "Describes a symmetrical phase shifting transformer tap model in which the voltage magnitude of both sides is the same. The difference voltage magnitude is the base in an equal-sided triangle where the sides corresponds to the primary and secondary voltages. The phase angle difference corresponds to the top angle and can be expressed as twice the arctangent of half the total difference voltage." ;
  cims:belongsToCategory eq:Package_CoreEquipmentProfile ;
  cims:stereotype <http://iec.ch/TC57/NonStandard/UML#concrete> ;
  rdfs:subClassOf cim:PhaseTapChangerNonLinear .

cim:PhaseTapChangerTable a rdfs:Class ;
  rdfs:label "PhaseTapChangerTable"@en ;
  rdfs:comment "Describes a tabular curve for how the phase angle difference and impedance varies with the tap step." ;
  cims:belongsToCategory eq:Package_CoreEquipmentProfile ;
  cims:stereotype <http://iec.ch/TC57/NonStandard/UML#concrete> ;
  rdfs:subClassOf cim:IdentifiedObject .

cim:PhaseTapChangerTablePoint a rdfs:Class ;
  rdfs:label "PhaseTapChangerTablePoint"@en ;
  rdfs:comment "Describes each tap step in the phase tap changer tabular curve." ;
  cims:belongsToCategory eq:Package_CoreEquipmentProfile ;
  cims:stereotype <http://iec.ch/TC57/NonStandard/UML#concrete> ;
  rdfs:subClassOf cim:TapChangerTablePoint .

cim:PhaseTapChangerTabular a rdfs:Class ;
  rdfs:label "PhaseTapChangerTabular"@en ;
  rdfs:comment "Describes a tap changer with a table defining the relation between the tap step and the phase angle difference across the transformer. " ;
  cims:belongsToCategory eq:Package_CoreEquipmentProfile ;
  cims:stereotype <http://iec.ch/TC57/NonStandard/UML#concrete> ;
  rdfs:subClassOf cim:PhaseTapChanger .

cim:PhotoVoltaicUnit a rdfs:Class ;
  rdfs:label "PhotoVoltaicUnit"@en ;
  rdfs:comment "A photovoltaic device or an aggregation of such devices." ;
  cims:belongsToCategory eq:Package_CoreEquipmentProfile ;
  cims:stereotype <http://iec.ch/TC57/NonStandard/UML#concrete> ;
  rdfs:subClassOf cim:PowerElectronicsUnit .

cim:PostLineSensor a rdfs:Class ;
  rdfs:label "PostLineSensor"@en ;
  rdfs:comment " A sensor used mainly in overhead distribution networks as the source of both current and voltage measurements." ;
  cims:belongsToCategory eq:Package_CoreEquipmentProfile ;
  cims:stereotype <http://iec.ch/TC57/NonStandard/UML#concrete> ;
  rdfs:subClassOf cim:Sensor .

cim:PotentialTransformer a rdfs:Class ;
  rdfs:label "PotentialTransformer"@en ;
  rdfs:comment "Instrument transformer (also known as Voltage Transformer) used to measure electrical qualities of the circuit that is being protected and/or monitored. Typically used as voltage transducer for the purpose of metering, protection, or sometimes auxiliary substation supply. A typical secondary voltage rating would be 120V." ;
  cims:belongsToCategory eq:Package_CoreEquipmentProfile ;
  cims:stereotype <http://iec.ch/TC57/NonStandard/UML#concrete> ;
  rdfs:subClassOf cim:Sensor .

cim:PowerElectronicsConnection a rdfs:Class ;
  rdfs:label "PowerElectronicsConnection"@en ;
  rdfs:comment "A connection to the AC network for energy production or consumption that uses power electronics rather than rotating machines." ;
  cims:belongsToCategory eq:Package_CoreEquipmentProfile ;
  cims:stereotype <http://iec.ch/TC57/NonStandard/UML#concrete> ;
  rdfs:subClassOf cim:RegulatingCondEq .

cim:PowerElectronicsUnit a rdfs:Class ;
  rdfs:label "PowerElectronicsUnit"@en ;
  rdfs:comment "A generating unit or battery or aggregation that connects to the AC network using power electronics rather than rotating machines." ;
  cims:belongsToCategory eq:Package_CoreEquipmentProfile ;
  rdfs:subClassOf cim:Equipment .

cim:PowerElectronicsWindUnit a rdfs:Class ;
  rdfs:label "PowerElectronicsWindUnit"@en ;
  rdfs:comment "A wind generating unit that connects to the AC network with power electronics rather than rotating machines or an aggregation of such units." ;
  cims:belongsToCategory eq:Package_CoreEquipmentProfile ;
  cims:stereotype <http://iec.ch/TC57/NonStandard/UML#concrete> ;
  rdfs:subClassOf cim:PowerElectronicsUnit .

cim:PowerSystemResource a rdfs:Class ;
  rdfs:label "PowerSystemResource"@en ;
  rdfs:comment "A power system resource (PSR) can be an item of equipment such as a switch, an equipment container containing many individual items of equipment such as a substation, or an organisational entity such as sub-control area. Power system resources can have measurements associated." ;
  cims:belongsToCategory eq:Package_CoreEquipmentProfile ;
  rdfs:subClassOf cim:IdentifiedObject .

cim:PowerTransformer a rdfs:Class ;
  rdfs:label "PowerTransformer"@en ;
  rdfs:comment """An electrical device consisting of  two or more coupled windings, with or without a magnetic core, for introducing mutual coupling between electric circuits. Transformers can be used to control voltage and phase shift (active power flow).
A power transformer may be composed of separate transformer tanks that need not be identical.
A power transformer can be modelled with or without tanks and is intended for use in both balanced and unbalanced representations.   A power transformer typically has two terminals, but may have one (grounding), three or more terminals.
The inherited association ConductingEquipment.BaseVoltage should not be used.  The association from TransformerEnd to BaseVoltage should be used instead.""" ;
  cims:belongsToCategory eq:Package_CoreEquipmentProfile ;
  cims:stereotype <http://iec.ch/TC57/NonStandard/UML#concrete> ;
  rdfs:subClassOf cim:ConductingEquipment .

cim:PowerTransformerEnd a rdfs:Class ;
  rdfs:label "PowerTransformerEnd"@en ;
  rdfs:comment """A PowerTransformerEnd is associated with each Terminal of a PowerTransformer.
The impedance values r, r0, x, and x0 of a PowerTransformerEnd represents a star equivalent as follows.
1) for a two Terminal PowerTransformer the high voltage (TransformerEnd.endNumber=1) PowerTransformerEnd has non zero values on r, r0, x, and x0 while the low voltage (TransformerEnd.endNumber=2) PowerTransformerEnd has zero values for r, r0, x, and x0.  Parameters are always provided, even if the PowerTransformerEnds have the same rated voltage.  In this case, the parameters are provided at the PowerTransformerEnd which has TransformerEnd.endNumber equal to 1.
2) for a three Terminal PowerTransformer the three PowerTransformerEnds represent a star equivalent with each leg in the star represented by r, r0, x, and x0 values.
3) For a three Terminal transformer each PowerTransformerEnd shall have g, g0, b and b0 values corresponding to the no load losses distributed on the three PowerTransformerEnds. The total no load loss shunt impedances may also be placed at one of the PowerTransformerEnds, preferably the end numbered 1, having the shunt values on end 1.  This is the preferred way.
4) for a PowerTransformer with more than three Terminals the PowerTransformerEnd impedance values cannot be used. Instead use the TransformerMeshImpedance or split the transformer into multiple PowerTransformers.
Each PowerTransformerEnd must be contained by a PowerTransformer. Because a PowerTransformerEnd (or any other object) can not be contained by more than one parent, a PowerTransformerEnd can not have an association to an EquipmentContainer (Substation, VoltageLevel, etc).""" ;
  cims:belongsToCategory eq:Package_CoreEquipmentProfile ;
  cims:stereotype <http://iec.ch/TC57/NonStandard/UML#concrete> ;
  rdfs:subClassOf cim:TransformerEnd .

cim:ProtectedSwitch a rdfs:Class ;
  rdfs:label "ProtectedSwitch"@en ;
  rdfs:comment "A ProtectedSwitch is a switching device that can be operated by ProtectionEquipment." ;
  cims:belongsToCategory eq:Package_CoreEquipmentProfile ;
  rdfs:subClassOf cim:Switch .

cim:RatioTapChanger a rdfs:Class ;
  rdfs:label "RatioTapChanger"@en ;
  rdfs:comment """A tap changer that changes the voltage ratio impacting the voltage magnitude but not the phase angle across the transformer.

Angle sign convention (general): Positive value indicates a positive phase shift from the winding where the tap is located to the other winding (for a two-winding transformer).""" ;
  cims:belongsToCategory eq:Package_CoreEquipmentProfile ;
  cims:stereotype <http://iec.ch/TC57/NonStandard/UML#concrete> ;
  rdfs:subClassOf cim:TapChanger .

cim:RatioTapChangerTable a rdfs:Class ;
  rdfs:label "RatioTapChangerTable"@en ;
  rdfs:comment "Describes a curve for how the voltage magnitude and impedance varies with the tap step. " ;
  cims:belongsToCategory eq:Package_CoreEquipmentProfile ;
  cims:stereotype <http://iec.ch/TC57/NonStandard/UML#concrete> ;
  rdfs:subClassOf cim:IdentifiedObject .

cim:RatioTapChangerTablePoint a rdfs:Class ;
  rdfs:label "RatioTapChangerTablePoint"@en ;
  rdfs:comment "Describes each tap step in the ratio tap changer tabular curve." ;
  cims:belongsToCategory eq:Package_CoreEquipmentProfile ;
  cims:stereotype <http://iec.ch/TC57/NonStandard/UML#concrete> ;
  rdfs:subClassOf cim:TapChangerTablePoint .

cim:Reactance a rdfs:Class ;
  rdfs:label "Reactance"@en ;
  rdfs:comment "Reactance (imaginary part of impedance), at rated frequency." ;
  cims:belongsToCategory eq:Package_CoreEquipmentProfile ;
  cims:stereotype "CIMDatatype" .

cim:ReactiveCapabilityCurve a rdfs:Class ;
  rdfs:label "ReactiveCapabilityCurve"@en ;
  rdfs:comment "Reactive power rating envelope versus the synchronous machine's active power, in both the generating and motoring modes. For each active power value there is a corresponding high and low reactive power limit  value. Typically there will be a separate curve for each coolant condition, such as hydrogen pressure.  The Y1 axis values represent reactive minimum and the Y2 axis values represent reactive maximum." ;
  cims:belongsToCategory eq:Package_CoreEquipmentProfile ;
  cims:stereotype <http://iec.ch/TC57/NonStandard/UML#concrete> ;
  rdfs:subClassOf cim:Curve .

cim:ReactivePower a rdfs:Class ;
  rdfs:label "ReactivePower"@en ;
  rdfs:comment "Product of RMS value of the voltage and the RMS value of the quadrature component of the current." ;
  cims:belongsToCategory eq:Package_CoreEquipmentProfile ;
  cims:stereotype "CIMDatatype" .

cim:RealEnergy a rdfs:Class ;
  rdfs:label "RealEnergy"@en ;
  rdfs:comment "Real electrical energy." ;
  cims:belongsToCategory eq:Package_CoreEquipmentProfile ;
  cims:stereotype "CIMDatatype" .

cim:RegularIntervalSchedule a rdfs:Class ;
  rdfs:label "RegularIntervalSchedule"@en ;
  rdfs:comment "The schedule has time points where the time between them is constant." ;
  cims:belongsToCategory eq:Package_CoreEquipmentProfile ;
  rdfs:subClassOf cim:BasicIntervalSchedule .

cim:RegularTimePoint a rdfs:Class ;
  rdfs:label "RegularTimePoint"@en ;
  rdfs:comment "Time point for a schedule where the time between the consecutive points is constant." ;
  cims:belongsToCategory eq:Package_CoreEquipmentProfile ;
  cims:stereotype <http://iec.ch/TC57/NonStandard/UML#concrete> .

cim:RegulatingCondEq a rdfs:Class ;
  rdfs:label "RegulatingCondEq"@en ;
  rdfs:comment "A type of conducting equipment that can regulate a quantity (i.e. voltage or flow) at a specific point in the network. " ;
  cims:belongsToCategory eq:Package_CoreEquipmentProfile ;
  rdfs:subClassOf cim:EnergyConnection .

cim:RegulatingControl a rdfs:Class ;
  rdfs:label "RegulatingControl"@en ;
  rdfs:comment """Specifies a set of equipment that works together to control a power system quantity such as voltage or flow. 
Remote bus voltage control is possible by specifying the controlled terminal located at some place remote from the controlling equipment.
The specified terminal shall be associated with the connectivity node of the controlled point.  The most specific subtype of RegulatingControl shall be used in case such equipment participate in the control, e.g. TapChangerControl for tap changers.
For flow control, load sign convention is used, i.e. positive sign means flow out from a TopologicalNode (bus) into the conducting equipment.
The attribute minAllowedTargetValue and maxAllowedTargetValue are required in the following cases:
- For a power generating module operated in power factor control mode to specify maximum and minimum power factor values;
- Whenever it is necessary to have an off center target voltage for the tap changer regulator. For instance, due to long cables to off shore wind farms and the need to have a simpler setup at the off shore transformer platform, the voltage is controlled from the land at the connection point for the off shore wind farm. Since there usually is a voltage rise along the cable, there is typical and overvoltage of up 3-4 kV compared to the on shore station. Thus in normal operation the tap changer on the on shore station is operated with a target set point, which is in the lower parts of the dead band.
The attributes minAllowedTargetValue and maxAllowedTargetValue are not related to the attribute targetDeadband and thus they are not treated as an alternative of the targetDeadband. They are needed due to limitations in the local substation controller. The attribute targetDeadband is used to prevent the power flow from move the tap position in circles (hunting) that is to be used regardless of the attributes minAllowedTargetValue and maxAllowedTargetValue.""" ;
  cims:belongsToCategory eq:Package_CoreEquipmentProfile ;
  cims:stereotype <http://iec.ch/TC57/NonStandard/UML#concrete> ;
  rdfs:subClassOf cim:PowerSystemResource .

cim:RegulatingControlModeKind a rdfs:Class ;
  rdfs:label "RegulatingControlModeKind"@en ;
  rdfs:comment "The kind of regulation model.   For example regulating voltage, reactive power, active power, etc." ;
  cims:belongsToCategory eq:Package_CoreEquipmentProfile ;
  cims:stereotype <http://iec.ch/TC57/NonStandard/UML#enumeration> .

cim:RegulationSchedule a rdfs:Class ;
  rdfs:label "RegulationSchedule"@en ;
  rdfs:comment "A pre-established pattern over time for a controlled variable, e.g., busbar voltage." ;
  cims:belongsToCategory eq:Package_CoreEquipmentProfile ;
  cims:stereotype <http://iec.ch/TC57/NonStandard/UML#concrete> ;
  rdfs:subClassOf cim:SeasonDayTypeSchedule .

cim:ReportingGroup a rdfs:Class ;
  rdfs:label "ReportingGroup"@en ;
  rdfs:comment "A reporting group is used for various ad-hoc groupings used for reporting." ;
  cims:belongsToCategory eq:Package_CoreEquipmentProfile ;
  cims:stereotype <http://iec.ch/TC57/NonStandard/UML#concrete> ;
  rdfs:subClassOf cim:IdentifiedObject .

cim:Resistance a rdfs:Class ;
  rdfs:label "Resistance"@en ;
  rdfs:comment "Resistance (real part of impedance)." ;
  cims:belongsToCategory eq:Package_CoreEquipmentProfile ;
  cims:stereotype "CIMDatatype" .

cim:RotatingMachine a rdfs:Class ;
  rdfs:label "RotatingMachine"@en ;
  rdfs:comment "A rotating machine which may be used as a generator or motor." ;
  cims:belongsToCategory eq:Package_CoreEquipmentProfile ;
  rdfs:subClassOf cim:RegulatingCondEq .

cim:RotationSpeed a rdfs:Class ;
  rdfs:label "RotationSpeed"@en ;
  rdfs:comment "Number of revolutions per second." ;
  cims:belongsToCategory eq:Package_CoreEquipmentProfile ;
  cims:stereotype "CIMDatatype" .

cim:SVCControlMode a rdfs:Class ;
  rdfs:label "SVCControlMode"@en ;
  rdfs:comment "Static VAr Compensator control mode." ;
  cims:belongsToCategory eq:Package_CoreEquipmentProfile ;
  cims:stereotype "deprecated", <http://iec.ch/TC57/NonStandard/UML#enumeration> .

cim:Season a rdfs:Class ;
  rdfs:label "Season"@en ;
  rdfs:comment "A specified time period of the year." ;
  cims:belongsToCategory eq:Package_CoreEquipmentProfile ;
  cims:stereotype <http://iec.ch/TC57/NonStandard/UML#concrete> ;
  rdfs:subClassOf cim:IdentifiedObject .

cim:SeasonDayTypeSchedule a rdfs:Class ;
  rdfs:label "SeasonDayTypeSchedule"@en ;
  rdfs:comment "A time schedule covering a 24 hour period, with curve data for a specific type of season and day." ;
  cims:belongsToCategory eq:Package_CoreEquipmentProfile ;
  rdfs:subClassOf cim:RegularIntervalSchedule .

cim:Seconds a rdfs:Class ;
  rdfs:label "Seconds"@en ;
  rdfs:comment "Time, in seconds." ;
  cims:belongsToCategory eq:Package_CoreEquipmentProfile ;
  cims:stereotype "CIMDatatype" .

cim:Sensor a rdfs:Class ;
  rdfs:label "Sensor"@en ;
  rdfs:comment "This class describe devices that transform a measured quantity into signals that can be presented at displays, used in control or be recorded." ;
  cims:belongsToCategory eq:Package_CoreEquipmentProfile ;
  rdfs:subClassOf cim:AuxiliaryEquipment .

cim:SeriesCompensator a rdfs:Class ;
  rdfs:label "SeriesCompensator"@en ;
  rdfs:comment "A Series Compensator is a series capacitor or reactor or an AC transmission line without charging susceptance.  It is a two terminal device." ;
  cims:belongsToCategory eq:Package_CoreEquipmentProfile ;
  cims:stereotype <http://iec.ch/TC57/NonStandard/UML#concrete> ;
  rdfs:subClassOf cim:ConductingEquipment .

cim:ShuntCompensator a rdfs:Class ;
  rdfs:label "ShuntCompensator"@en ;
  rdfs:comment "A shunt capacitor or reactor or switchable bank of shunt capacitors or reactors. A section of a shunt compensator is an individual capacitor or reactor. A negative value for bPerSection indicates that the compensator is a reactor. ShuntCompensator is a single terminal device.  Ground is implied." ;
  cims:belongsToCategory eq:Package_CoreEquipmentProfile ;
  rdfs:subClassOf cim:RegulatingCondEq .

cim:SolarGeneratingUnit a rdfs:Class ;
  rdfs:label "SolarGeneratingUnit"@en ;
  rdfs:comment "A solar thermal generating unit, connected to the grid by means of a rotating machine.  This class does not represent photovoltaic (PV) generation." ;
  cims:belongsToCategory eq:Package_CoreEquipmentProfile ;
  cims:stereotype <http://iec.ch/TC57/NonStandard/UML#concrete> ;
  rdfs:subClassOf cim:GeneratingUnit .

cim:StaticVarCompensator a rdfs:Class ;
  rdfs:label "StaticVarCompensator"@en ;
  rdfs:comment """A facility for providing variable and controllable shunt reactive power. The SVC typically consists of a stepdown transformer, filter, thyristor-controlled reactor, and thyristor-switched capacitor arms.

The SVC may operate in fixed MVar output mode or in voltage control mode. When in voltage control mode, the output of the SVC will be proportional to the deviation of voltage at the controlled bus from the voltage setpoint.  The SVC characteristic slope defines the proportion.  If the voltage at the controlled bus is equal to the voltage setpoint, the SVC MVar output is zero.""" ;
  cims:belongsToCategory eq:Package_CoreEquipmentProfile ;
  cims:stereotype <http://iec.ch/TC57/NonStandard/UML#concrete> ;
  rdfs:subClassOf cim:RegulatingCondEq .

cim:StationSupply a rdfs:Class ;
  rdfs:label "StationSupply"@en ;
  rdfs:comment "Station supply with load derived from the station output." ;
  cims:belongsToCategory eq:Package_CoreEquipmentProfile ;
  cims:stereotype <http://iec.ch/TC57/NonStandard/UML#concrete> ;
  rdfs:subClassOf cim:EnergyConsumer .

cim:String a rdfs:Class ;
  rdfs:label "String"@en ;
  rdfs:comment "A string consisting of a sequence of characters. The character encoding is UTF-8. The string length is unspecified and unlimited." ;
  cims:belongsToCategory eq:Package_CoreEquipmentProfile ;
  cims:stereotype "Primitive" .

cim:SubGeographicalRegion a rdfs:Class ;
  rdfs:label "SubGeographicalRegion"@en ;
  rdfs:comment "A subset of a geographical region of a power system network model." ;
  cims:belongsToCategory eq:Package_CoreEquipmentProfile ;
  cims:stereotype <http://iec.ch/TC57/NonStandard/UML#concrete> ;
  rdfs:subClassOf cim:IdentifiedObject .

cim:SubLoadArea a rdfs:Class ;
  rdfs:label "SubLoadArea"@en ;
  rdfs:comment "The class is the second level in a hierarchical structure for grouping of loads for the purpose of load flow load scaling." ;
  cims:belongsToCategory eq:Package_CoreEquipmentProfile ;
  cims:stereotype <http://iec.ch/TC57/NonStandard/UML#concrete> ;
  rdfs:subClassOf cim:EnergyArea .

cim:Substation a rdfs:Class ;
  rdfs:label "Substation"@en ;
  rdfs:comment "A collection of equipment for purposes other than generation or utilization, through which electric energy in bulk is passed for the purposes of switching or modifying its characteristics. " ;
  cims:belongsToCategory eq:Package_CoreEquipmentProfile ;
  cims:stereotype <http://iec.ch/TC57/NonStandard/UML#concrete> ;
  rdfs:subClassOf cim:EquipmentContainer .

cim:SurgeArrester a rdfs:Class ;
  rdfs:label "SurgeArrester"@en ;
  rdfs:comment "Shunt device, installed on the network, usually in the proximity of electrical equipment in order to protect the said equipment against transient voltage transients caused by lightning or switching activity." ;
  cims:belongsToCategory eq:Package_CoreEquipmentProfile ;
  cims:stereotype <http://iec.ch/TC57/NonStandard/UML#concrete> ;
  rdfs:subClassOf cim:AuxiliaryEquipment .

cim:Susceptance a rdfs:Class ;
  rdfs:label "Susceptance"@en ;
  rdfs:comment "Imaginary part of admittance." ;
  cims:belongsToCategory eq:Package_CoreEquipmentProfile ;
  cims:stereotype "CIMDatatype" .

cim:Switch a rdfs:Class ;
  rdfs:label "Switch"@en ;
  rdfs:comment "A generic device designed to close, or open, or both, one or more electric circuits.  All switches are two terminal devices including grounding switches. The ACDCTerminal.connected at the two sides of the switch shall not be considered for assessing switch connectivity, i.e. only Switch.open, .normalOpen and .locked are relevant." ;
  cims:belongsToCategory eq:Package_CoreEquipmentProfile ;
  cims:stereotype <http://iec.ch/TC57/NonStandard/UML#concrete> ;
  rdfs:subClassOf cim:ConductingEquipment .

cim:SwitchSchedule a rdfs:Class ;
  rdfs:label "SwitchSchedule"@en ;
  rdfs:comment "A schedule of switch positions.  If RegularTimePoint.value1 is 0, the switch is open.  If 1, the switch is closed.  " ;
  cims:belongsToCategory eq:Package_CoreEquipmentProfile ;
  cims:stereotype <http://iec.ch/TC57/NonStandard/UML#concrete> ;
  rdfs:subClassOf cim:SeasonDayTypeSchedule .

cim:SynchronousMachine a rdfs:Class ;
  rdfs:label "SynchronousMachine"@en ;
  rdfs:comment "An electromechanical device that operates with shaft rotating synchronously with the network. It is a single machine operating either as a generator or synchronous condenser or pump." ;
  cims:belongsToCategory eq:Package_CoreEquipmentProfile ;
  cims:stereotype <http://iec.ch/TC57/NonStandard/UML#concrete> ;
  rdfs:subClassOf cim:RotatingMachine .

cim:SynchronousMachineKind a rdfs:Class ;
  rdfs:label "SynchronousMachineKind"@en ;
  rdfs:comment "Synchronous machine type." ;
  cims:belongsToCategory eq:Package_CoreEquipmentProfile ;
  cims:stereotype <http://iec.ch/TC57/NonStandard/UML#enumeration> .

cim:TapChanger a rdfs:Class ;
  rdfs:label "TapChanger"@en ;
  rdfs:comment "Mechanism for changing transformer winding tap positions." ;
  cims:belongsToCategory eq:Package_CoreEquipmentProfile ;
  rdfs:subClassOf cim:PowerSystemResource .

cim:TapChangerControl a rdfs:Class ;
  rdfs:label "TapChangerControl"@en ;
  rdfs:comment "Describes behaviour specific to tap changers, e.g. how the voltage at the end of a line varies with the load level and compensation of the voltage drop by tap adjustment." ;
  cims:belongsToCategory eq:Package_CoreEquipmentProfile ;
  cims:stereotype <http://iec.ch/TC57/NonStandard/UML#concrete> ;
  rdfs:subClassOf cim:RegulatingControl .

cim:TapChangerTablePoint a rdfs:Class ;
  rdfs:label "TapChangerTablePoint"@en ;
  rdfs:comment "Describes each tap step in the tabular curve." ;
  cims:belongsToCategory eq:Package_CoreEquipmentProfile .

cim:TapSchedule a rdfs:Class ;
  rdfs:label "TapSchedule"@en ;
  rdfs:comment "A pre-established pattern over time for a tap step." ;
  cims:belongsToCategory eq:Package_CoreEquipmentProfile ;
  cims:stereotype <http://iec.ch/TC57/NonStandard/UML#concrete> ;
  rdfs:subClassOf cim:SeasonDayTypeSchedule .

cim:Terminal a rdfs:Class ;
  rdfs:label "Terminal"@en ;
  rdfs:comment "An AC electrical connection point to a piece of conducting equipment. Terminals are connected at physical connection points called connectivity nodes." ;
  cims:belongsToCategory eq:Package_CoreEquipmentProfile ;
  cims:stereotype <http://iec.ch/TC57/NonStandard/UML#concrete> ;
  rdfs:subClassOf cim:ACDCTerminal .

cim:ThermalGeneratingUnit a rdfs:Class ;
  rdfs:label "ThermalGeneratingUnit"@en ;
  rdfs:comment "A generating unit whose prime mover could be a steam turbine, combustion turbine, or diesel engine." ;
  cims:belongsToCategory eq:Package_CoreEquipmentProfile ;
  cims:stereotype <http://iec.ch/TC57/NonStandard/UML#concrete> ;
  rdfs:subClassOf cim:GeneratingUnit .

cim:TieFlow a rdfs:Class ;
  rdfs:label "TieFlow"@en ;
  rdfs:comment "Defines the structure (in terms of location and direction) of the net interchange constraint for a control area. This constraint may be used by either AGC or power flow." ;
  cims:belongsToCategory eq:Package_CoreEquipmentProfile ;
  cims:stereotype <http://iec.ch/TC57/NonStandard/UML#concrete> ;
  rdfs:subClassOf cim:IdentifiedObject .

cim:TransformerEnd a rdfs:Class ;
  rdfs:label "TransformerEnd"@en ;
  rdfs:comment "A conducting connection point of a power transformer. It corresponds to a physical transformer winding terminal.  In earlier CIM versions, the TransformerWinding class served a similar purpose, but this class is more flexible because it associates to terminal but is not a specialization of ConductingEquipment." ;
  cims:belongsToCategory eq:Package_CoreEquipmentProfile ;
  rdfs:subClassOf cim:IdentifiedObject .

cim:UnitMultiplier a rdfs:Class ;
  rdfs:label "UnitMultiplier"@en ;
  rdfs:comment """The unit multipliers defined for the CIM.  When applied to unit symbols, the unit symbol is treated as a derived unit. Regardless of the contents of the unit symbol text, the unit symbol shall be treated as if it were a single-character unit symbol. Unit symbols should not contain multipliers, and it should be left to the multiplier to define the multiple for an entire data type. 

For example, if a unit symbol is "m2Pers" and the multiplier is "k", then the value is k(m**2/s), and the multiplier applies to the entire final value, not to any individual part of the value. This can be conceptualized by substituting a derived unit symbol for the unit type. If one imagines that the symbol "Þ" represents the derived unit "m2Pers", then applying the multiplier "k" can be conceptualized simply as "kÞ".

For example, the SI unit for mass is "kg" and not "g".  If the unit symbol is defined as "kg", then the multiplier is applied to "kg" as a whole and does not replace the "k" in front of the "g". In this case, the multiplier of "m" would be used with the unit symbol of "kg" to represent one gram.  As a text string, this violates the instructions in IEC 80000-1. However, because the unit symbol in CIM is treated as a derived unit instead of as an SI unit, it makes more sense to conceptualize the "kg" as if it were replaced by one of the proposed replacements for the SI mass symbol. If one imagines that the "kg" were replaced by a symbol "Þ", then it is easier to conceptualize the multiplier "m" as creating the proper unit "mÞ", and not the forbidden unit "mkg".""" ;
  cims:belongsToCategory eq:Package_CoreEquipmentProfile ;
  cims:stereotype <http://iec.ch/TC57/NonStandard/UML#enumeration> .

cim:UnitSymbol a rdfs:Class ;
  rdfs:label "UnitSymbol"@en ;
  rdfs:comment """The derived units defined for usage in the CIM. In some cases, the derived unit is equal to an SI unit. Whenever possible, the standard derived symbol is used instead of the formula for the derived unit. For example, the unit symbol Farad is defined as "F" instead of "CPerV". In cases where a standard symbol does not exist for a derived unit, the formula for the unit is used as the unit symbol. For example, density does not have a standard symbol and so it is represented as "kgPerm3". With the exception of the "kg", which is an SI unit, the unit symbols do not contain multipliers and therefore represent the base derived unit to which a multiplier can be applied as a whole. 
Every unit symbol is treated as an unparseable text as if it were a single-letter symbol. The meaning of each unit symbol is defined by the accompanying descriptive text and not by the text contents of the unit symbol.
To allow the widest possible range of serializations without requiring special character handling, several substitutions are made which deviate from the format described in IEC 80000-1. The division symbol "/" is replaced by the letters "Per". Exponents are written in plain text after the unit as "m3" instead of being formatted as "m" with a superscript of 3  or introducing a symbol as in "m^3". The degree symbol "°" is replaced with the letters "deg". Any clarification of the meaning for a substitution is included in the description for the unit symbol.
Non-SI units are included in list of unit symbols to allow sources of data to be correctly labelled with their non-SI units (for example, a GPS sensor that is reporting numbers that represent feet instead of meters). This allows software to use the unit symbol information correctly convert and scale the raw data of those sources into SI-based units. 
The integer values are used for harmonization with IEC 61850.""" ;
  cims:belongsToCategory eq:Package_CoreEquipmentProfile ;
  cims:stereotype <http://iec.ch/TC57/NonStandard/UML#enumeration> .

cim:Voltage a rdfs:Class ;
  rdfs:label "Voltage"@en ;
  rdfs:comment "Electrical voltage, can be both AC and DC." ;
  cims:belongsToCategory eq:Package_CoreEquipmentProfile ;
  cims:stereotype "CIMDatatype" .

cim:VoltageLevel a rdfs:Class ;
  rdfs:label "VoltageLevel"@en ;
  rdfs:comment "A collection of equipment at one common system voltage forming a switchgear. The equipment typically consists of breakers, busbars, instrumentation, control, regulation and protection devices as well as assemblies of all these." ;
  cims:belongsToCategory eq:Package_CoreEquipmentProfile ;
  cims:stereotype <http://iec.ch/TC57/NonStandard/UML#concrete> ;
  rdfs:subClassOf cim:EquipmentContainer .

cim:VoltageLimit a rdfs:Class ;
  rdfs:label "VoltageLimit"@en ;
  rdfs:comment """Operational limit applied to voltage.
The use of operational VoltageLimit is preferred instead of limits defined at VoltageLevel. The operational VoltageLimits are used, if present.""" ;
  cims:belongsToCategory eq:Package_CoreEquipmentProfile ;
  cims:stereotype <http://iec.ch/TC57/NonStandard/UML#concrete> ;
  rdfs:subClassOf cim:OperationalLimit .

cim:VoltagePerReactivePower a rdfs:Class ;
  rdfs:label "VoltagePerReactivePower"@en ;
  rdfs:comment "Voltage variation with reactive power." ;
  cims:belongsToCategory eq:Package_CoreEquipmentProfile ;
  cims:stereotype "CIMDatatype" .

cim:VsCapabilityCurve a rdfs:Class ;
  rdfs:label "VsCapabilityCurve"@en ;
  rdfs:comment "The P-Q capability curve for a voltage source converter, with P on X-axis and Qmin and Qmax on Y1-axis and Y2-axis." ;
  cims:belongsToCategory eq:Package_CoreEquipmentProfile ;
  cims:stereotype <http://iec.ch/TC57/NonStandard/UML#concrete> ;
  rdfs:subClassOf cim:Curve .

cim:VsConverter a rdfs:Class ;
  rdfs:label "VsConverter"@en ;
  rdfs:comment "DC side of the voltage source converter (VSC)." ;
  cims:belongsToCategory eq:Package_CoreEquipmentProfile ;
  cims:stereotype <http://iec.ch/TC57/NonStandard/UML#concrete> ;
  rdfs:subClassOf cim:ACDCConverter .

cim:WaveTrap a rdfs:Class ;
  rdfs:label "WaveTrap"@en ;
  rdfs:comment "Line traps are devices that impede high frequency power line carrier signals yet present a negligible impedance at the main power frequency." ;
  cims:belongsToCategory eq:Package_CoreEquipmentProfile ;
  cims:stereotype <http://iec.ch/TC57/NonStandard/UML#concrete> ;
  rdfs:subClassOf cim:AuxiliaryEquipment .

cim:WindGenUnitKind a rdfs:Class ;
  rdfs:label "WindGenUnitKind"@en ;
  rdfs:comment "Kind of wind generating unit." ;
  cims:belongsToCategory eq:Package_CoreEquipmentProfile ;
  cims:stereotype <http://iec.ch/TC57/NonStandard/UML#enumeration> .

cim:WindGeneratingUnit a rdfs:Class ;
  rdfs:label "WindGeneratingUnit"@en ;
  rdfs:comment "A wind driven generating unit, connected to the grid by means of a rotating machine.  May be used to represent a single turbine or an aggregation.    " ;
  cims:belongsToCategory eq:Package_CoreEquipmentProfile ;
  cims:stereotype <http://iec.ch/TC57/NonStandard/UML#concrete> ;
  rdfs:subClassOf cim:GeneratingUnit .

cim:WindingConnection a rdfs:Class ;
  rdfs:label "WindingConnection"@en ;
  rdfs:comment "Winding connection type." ;
  cims:belongsToCategory eq:Package_CoreEquipmentProfile ;
  cims:stereotype <http://iec.ch/TC57/NonStandard/UML#enumeration> .

eu:BoundaryPoint a rdfs:Class ;
  rdfs:label "BoundaryPoint"@en ;
  rdfs:comment "Designates a connection point at which one or more model authority sets shall connect to. The location of the connection point as well as other properties are agreed between organisations responsible for the interconnection, hence all attributes of the class represent this agreement.  It is primarily used in a boundary model authority set which can contain one or many BoundaryPoint-s among other Equipment-s and their connections." ;
  cims:belongsToCategory eq:Package_CoreEquipmentProfile ;
  cims:stereotype "European", <http://iec.ch/TC57/NonStandard/UML#concrete> ;
  rdfs:subClassOf cim:PowerSystemResource .

eu:LimitKind a rdfs:Class ;
  rdfs:label "LimitKind"@en ;
  rdfs:comment "Limit kinds." ;
  cims:belongsToCategory eq:Package_CoreEquipmentProfile ;
  cims:stereotype "European", <http://iec.ch/TC57/NonStandard/UML#enumeration> .

eu:SolarPowerPlant a rdfs:Class ;
  rdfs:label "SolarPowerPlant"@en ;
  rdfs:comment "Solar power plant." ;
  cims:belongsToCategory eq:Package_CoreEquipmentProfile ;
  cims:stereotype "European", <http://iec.ch/TC57/NonStandard/UML#concrete> ;
  rdfs:subClassOf cim:PowerSystemResource .

eu:WindPowerPlant a rdfs:Class ;
  rdfs:label "WindPowerPlant"@en ;
  rdfs:comment "Wind power plant." ;
  cims:belongsToCategory eq:Package_CoreEquipmentProfile ;
  cims:stereotype "European", <http://iec.ch/TC57/NonStandard/UML#concrete> ;
  rdfs:subClassOf cim:PowerSystemResource .

eq:Ontology a owl:Ontology ;
  dct:description "This vocabulary is describing the core equipment profile from IEC 61970-600-2."@en ;
  dcat:keyword "EQ" ;
  dcat:landingPage "https://www.entsoe.eu/digital/cim/cim-for-grid-models-exchange/" ;
  dcat:theme "vocabulary"@en ;
  dct:conformsTo "file://iec61970cim17v40_iec61968cim13v13a_iec62325cim03v17a.eap", "urn:iso:std:iec:61970-301:ed-7:amd1", "urn:iso:std:iec:61970-501:draft:ed-2", "urn:iso:std:iec:61970-600-2:ed-1" ;
  dct:creator "ENTSO-E CIM EG"@en ;
  dct:identifier "urn:uuid:9fd00587-84d4-4910-bbd4-e003ed7e0821" ;
  dct:issued "2021-01-27T12:09:21Z"^^xsd:dateTime ;
  dct:language "en-GB" ;
  dct:modified "2020-10-12"^^xsd:date ;
  dct:publisher "ENTSO-E"@en ;
  dct:rights "Copyright"@en ;
  dct:rightsHolder "ENTSO-E"@en ;
  dct:title "Core Equipment Vocabulary"@en ;
  owl:incompatibleWith <http://entsoe.eu/2009/profile1> ;
  owl:priorVersion <http://entsoe.eu/CIM/EquipmentCore/3/1> ;
  owl:versionIRI <http://iec.ch/TC57/ns/CIM/CoreEquipment-EU/3.0> ;
  owl:versionInfo "3.0.0"@en .

cim:ACDCConverter.DCTerminals a rdf:Property ;
  rdfs:label "DCTerminals"@en ;
  rdfs:comment "A DC converter have DC converter terminals. A converter has two DC converter terminals." ;
  cims:AssociationUsed "No" ;
  cims:inverseRoleName cim:ACDCConverterDCTerminal.DCConductingEquipment ;
  cims:multiplicity cims:M:0..n ;
  rdfs:domain cim:ACDCConverter ;
  rdfs:range cim:ACDCConverterDCTerminal .

cim:ACDCConverter.PccTerminal a rdf:Property ;
  rdfs:label "PccTerminal"@en ;
  rdfs:comment "Point of common coupling terminal for this converter DC side. It is typically the terminal on the power transformer (or switch) closest to the AC network." ;
  cims:AssociationUsed "Yes" ;
  cims:inverseRoleName cim:Terminal.ConverterDCSides ;
  cims:multiplicity cims:M:0..1 ;
  rdfs:domain cim:ACDCConverter ;
  rdfs:range cim:Terminal .

cim:ACDCConverter.baseS a rdf:Property ;
  rdfs:label "baseS"@en ;
  rdfs:comment "Base apparent power of the converter pole. The attribute shall be a positive value." ;
  cims:dataType cim:ApparentPower ;
  cims:multiplicity cims:M:0..1 ;
  cims:stereotype <http://iec.ch/TC57/NonStandard/UML#attribute> ;
  rdfs:domain cim:ACDCConverter .

cim:ACDCConverter.idleLoss a rdf:Property ;
  rdfs:label "idleLoss"@en ;
  rdfs:comment "Active power loss in pole at no power transfer. It is converter’s configuration data used in power flow. The attribute shall be a positive value." ;
  cims:dataType cim:ActivePower ;
  cims:multiplicity cims:M:0..1 ;
  cims:stereotype <http://iec.ch/TC57/NonStandard/UML#attribute> ;
  rdfs:domain cim:ACDCConverter .

cim:ACDCConverter.maxP a rdf:Property ;
  rdfs:label "maxP"@en ;
  rdfs:comment "Maximum active power limit. The value is overwritten by values of VsCapabilityCurve, if present." ;
  cims:dataType cim:ActivePower ;
  cims:multiplicity cims:M:0..1 ;
  cims:stereotype <http://iec.ch/TC57/NonStandard/UML#attribute> ;
  rdfs:domain cim:ACDCConverter .

cim:ACDCConverter.maxUdc a rdf:Property ;
  rdfs:label "maxUdc"@en ;
  rdfs:comment "The maximum voltage on the DC side at which the converter should operate. It is converter’s configuration data used in power flow. The attribute shall be a positive value." ;
  cims:dataType cim:Voltage ;
  cims:multiplicity cims:M:0..1 ;
  cims:stereotype <http://iec.ch/TC57/NonStandard/UML#attribute> ;
  rdfs:domain cim:ACDCConverter .

cim:ACDCConverter.minP a rdf:Property ;
  rdfs:label "minP"@en ;
  rdfs:comment "Minimum active power limit. The value is overwritten by values of VsCapabilityCurve, if present." ;
  cims:dataType cim:ActivePower ;
  cims:multiplicity cims:M:0..1 ;
  cims:stereotype <http://iec.ch/TC57/NonStandard/UML#attribute> ;
  rdfs:domain cim:ACDCConverter .

cim:ACDCConverter.minUdc a rdf:Property ;
  rdfs:label "minUdc"@en ;
  rdfs:comment "The minimum voltage on the DC side at which the converter should operate. It is converter’s configuration data used in power flow. The attribute shall be a positive value." ;
  cims:dataType cim:Voltage ;
  cims:multiplicity cims:M:0..1 ;
  cims:stereotype <http://iec.ch/TC57/NonStandard/UML#attribute> ;
  rdfs:domain cim:ACDCConverter .

cim:ACDCConverter.numberOfValves a rdf:Property ;
  rdfs:label "numberOfValves"@en ;
  rdfs:comment "Number of valves in the converter. Used in loss calculations." ;
  cims:dataType cim:Integer ;
  cims:multiplicity cims:M:0..1 ;
  cims:stereotype <http://iec.ch/TC57/NonStandard/UML#attribute> ;
  rdfs:domain cim:ACDCConverter .

cim:ACDCConverter.ratedUdc a rdf:Property ;
  rdfs:label "ratedUdc"@en ;
  rdfs:comment "Rated converter DC voltage, also called UdN. The attribute shall be a positive value. It is converter’s configuration data used in power flow. For instance a bipolar HVDC link with value  200 kV has a 400kV difference between the dc lines." ;
  cims:dataType cim:Voltage ;
  cims:multiplicity cims:M:0..1 ;
  cims:stereotype <http://iec.ch/TC57/NonStandard/UML#attribute> ;
  rdfs:domain cim:ACDCConverter .

cim:ACDCConverter.resistiveLoss a rdf:Property ;
  rdfs:label "resistiveLoss"@en ;
  rdfs:comment "It is converter’s configuration data used in power flow. Refer to poleLossP. The attribute shall be a positive value." ;
  cims:dataType cim:Resistance ;
  cims:multiplicity cims:M:0..1 ;
  cims:stereotype <http://iec.ch/TC57/NonStandard/UML#attribute> ;
  rdfs:domain cim:ACDCConverter .

cim:ACDCConverter.switchingLoss a rdf:Property ;
  rdfs:label "switchingLoss"@en ;
  rdfs:comment "Switching losses, relative to the base apparent power 'baseS'. Refer to poleLossP. The attribute shall be a positive value." ;
  cims:dataType cim:ActivePowerPerCurrentFlow ;
  cims:multiplicity cims:M:0..1 ;
  cims:stereotype <http://iec.ch/TC57/NonStandard/UML#attribute> ;
  rdfs:domain cim:ACDCConverter .

cim:ACDCConverter.valveU0 a rdf:Property ;
  rdfs:label "valveU0"@en ;
  rdfs:comment "Valve threshold voltage, also called Uvalve. Forward voltage drop when the valve is conducting. Used in loss calculations, i.e. the switchLoss depend on numberOfValves * valveU0." ;
  cims:dataType cim:Voltage ;
  cims:multiplicity cims:M:0..1 ;
  cims:stereotype <http://iec.ch/TC57/NonStandard/UML#attribute> ;
  rdfs:domain cim:ACDCConverter .

cim:ACDCConverterDCTerminal.DCConductingEquipment a rdf:Property ;
  rdfs:label "DCConductingEquipment"@en ;
  rdfs:comment "A DC converter terminal belong to an DC converter." ;
  cims:AssociationUsed "Yes" ;
  cims:inverseRoleName cim:ACDCConverter.DCTerminals ;
  cims:multiplicity cims:M:1 ;
  rdfs:domain cim:ACDCConverterDCTerminal ;
  rdfs:range cim:ACDCConverter .

cim:ACDCConverterDCTerminal.polarity a rdf:Property ;
  rdfs:label "polarity"@en ;
  rdfs:comment """Represents the normal network polarity condition. Depending on the converter configuration the value shall be set as follows:
- For a monopole with two converter terminals use DCPolarityKind “positive” and “negative”.
- For a bi-pole or symmetric monopole with three converter terminals use DCPolarityKind “positive”, “middle” and “negative”.""" ;
  cims:multiplicity cims:M:1..1 ;
  cims:stereotype <http://iec.ch/TC57/NonStandard/UML#attribute> ;
  rdfs:domain cim:ACDCConverterDCTerminal ;
  rdfs:range cim:DCPolarityKind .

cim:ACDCTerminal.BusNameMarker a rdf:Property ;
  rdfs:label "BusNameMarker"@en ;
  rdfs:comment "The bus name marker used to name the bus (topological node)." ;
  cims:AssociationUsed "Yes" ;
  cims:inverseRoleName cim:BusNameMarker.Terminal ;
  cims:multiplicity cims:M:0..1 ;
  rdfs:domain cim:ACDCTerminal ;
  rdfs:range cim:BusNameMarker .

cim:ACDCTerminal.OperationalLimitSet a rdf:Property ;
  rdfs:label "OperationalLimitSet"@en ;
  rdfs:comment "The operational limit sets at the terminal." ;
  cims:AssociationUsed "No" ;
  cims:inverseRoleName cim:OperationalLimitSet.Terminal ;
  cims:multiplicity cims:M:0..n ;
  rdfs:domain cim:ACDCTerminal ;
  rdfs:range cim:OperationalLimitSet .

cim:ACDCTerminal.sequenceNumber a rdf:Property ;
  rdfs:label "sequenceNumber"@en ;
  rdfs:comment "The orientation of the terminal connections for a multiple terminal conducting equipment.  The sequence numbering starts with 1 and additional terminals should follow in increasing order.   The first terminal is the \"starting point\" for a two terminal branch." ;
  cims:dataType cim:Integer ;
  cims:multiplicity cims:M:1..1 ;
  cims:stereotype <http://iec.ch/TC57/NonStandard/UML#attribute> ;
  rdfs:domain cim:ACDCTerminal .

cim:ACLineSegment.Clamp a rdf:Property ;
  rdfs:label "Clamp"@en ;
  rdfs:comment "The clamps connected to the line segment." ;
  cims:AssociationUsed "No" ;
  cims:inverseRoleName cim:Clamp.ACLineSegment ;
  cims:multiplicity cims:M:0..n ;
  rdfs:domain cim:ACLineSegment ;
  rdfs:range cim:Clamp .

cim:ACLineSegment.Cut a rdf:Property ;
  rdfs:label "Cut"@en ;
  rdfs:comment "Cuts applied to the line segment." ;
  cims:AssociationUsed "No" ;
  cims:inverseRoleName cim:Cut.ACLineSegment ;
  cims:multiplicity cims:M:0..n ;
  rdfs:domain cim:ACLineSegment ;
  rdfs:range cim:Cut .

cim:ACLineSegment.bch a rdf:Property ;
  rdfs:label "bch"@en ;
  rdfs:comment "Positive sequence shunt (charging) susceptance, uniformly distributed, of the entire line section.  This value represents the full charging over the full length of the line." ;
  cims:dataType cim:Susceptance ;
  cims:multiplicity cims:M:1..1 ;
  cims:stereotype <http://iec.ch/TC57/NonStandard/UML#attribute> ;
  rdfs:domain cim:ACLineSegment .

cim:ACLineSegment.gch a rdf:Property ;
  rdfs:label "gch"@en ;
  rdfs:comment "Positive sequence shunt (charging) conductance, uniformly distributed, of the entire line section." ;
  cims:dataType cim:Conductance ;
  cims:multiplicity cims:M:0..1 ;
  cims:stereotype <http://iec.ch/TC57/NonStandard/UML#attribute> ;
  rdfs:domain cim:ACLineSegment .

cim:ACLineSegment.r a rdf:Property ;
  rdfs:label "r"@en ;
  rdfs:comment "Positive sequence series resistance of the entire line section." ;
  cims:dataType cim:Resistance ;
  cims:multiplicity cims:M:1..1 ;
  cims:stereotype <http://iec.ch/TC57/NonStandard/UML#attribute> ;
  rdfs:domain cim:ACLineSegment .

cim:ACLineSegment.x a rdf:Property ;
  rdfs:label "x"@en ;
  rdfs:comment "Positive sequence series reactance of the entire line section." ;
  cims:dataType cim:Reactance ;
  cims:multiplicity cims:M:1..1 ;
  cims:stereotype <http://iec.ch/TC57/NonStandard/UML#attribute> ;
  rdfs:domain cim:ACLineSegment .

cim:ActivePower.multiplier a rdf:Property ;
  rdfs:label "multiplier"@en ;
  cims:isFixed "M" ;
  cims:multiplicity cims:M:0..1 ;
  cims:stereotype <http://iec.ch/TC57/NonStandard/UML#attribute> ;
  rdfs:domain cim:ActivePower ;
  rdfs:range cim:UnitMultiplier .

cim:ActivePower.unit a rdf:Property ;
  rdfs:label "unit"@en ;
  cims:isFixed "W" ;
  cims:multiplicity cims:M:0..1 ;
  cims:stereotype <http://iec.ch/TC57/NonStandard/UML#attribute> ;
  rdfs:domain cim:ActivePower ;
  rdfs:range cim:UnitSymbol .

cim:ActivePower.value a rdf:Property ;
  rdfs:label "value"@en ;
  cims:dataType cim:Float ;
  cims:multiplicity cims:M:0..1 ;
  cims:stereotype <http://iec.ch/TC57/NonStandard/UML#attribute> ;
  rdfs:domain cim:ActivePower .

cim:ActivePowerLimit.normalValue a rdf:Property ;
  rdfs:label "normalValue"@en ;
  rdfs:comment "The normal value of active power limit. The attribute shall be a positive value or zero." ;
  cims:dataType cim:ActivePower ;
  cims:multiplicity cims:M:1..1 ;
  cims:stereotype <http://iec.ch/TC57/NonStandard/UML#attribute> ;
  rdfs:domain cim:ActivePowerLimit .

cim:ActivePowerPerCurrentFlow.multiplier a rdf:Property ;
  rdfs:label "multiplier"@en ;
  cims:isFixed "M" ;
  cims:multiplicity cims:M:0..1 ;
  cims:stereotype <http://iec.ch/TC57/NonStandard/UML#attribute> ;
  rdfs:domain cim:ActivePowerPerCurrentFlow ;
  rdfs:range cim:UnitMultiplier .

cim:ActivePowerPerCurrentFlow.unit a rdf:Property ;
  rdfs:label "unit"@en ;
  cims:isFixed "WPerA" ;
  cims:multiplicity cims:M:0..1 ;
  cims:stereotype <http://iec.ch/TC57/NonStandard/UML#attribute> ;
  rdfs:domain cim:ActivePowerPerCurrentFlow ;
  rdfs:range cim:UnitSymbol .

cim:ActivePowerPerCurrentFlow.value a rdf:Property ;
  rdfs:label "value"@en ;
  cims:dataType cim:Float ;
  cims:multiplicity cims:M:0..1 ;
  cims:stereotype <http://iec.ch/TC57/NonStandard/UML#attribute> ;
  rdfs:domain cim:ActivePowerPerCurrentFlow .

cim:ActivePowerPerFrequency.multiplier a rdf:Property ;
  rdfs:label "multiplier"@en ;
  cims:isFixed "M" ;
  cims:multiplicity cims:M:0..1 ;
  cims:stereotype <http://iec.ch/TC57/NonStandard/UML#attribute> ;
  rdfs:domain cim:ActivePowerPerFrequency ;
  rdfs:range cim:UnitMultiplier .

cim:ActivePowerPerFrequency.unit a rdf:Property ;
  rdfs:label "unit"@en ;
  cims:isFixed "WPers" ;
  cims:multiplicity cims:M:0..1 ;
  cims:stereotype <http://iec.ch/TC57/NonStandard/UML#attribute> ;
  rdfs:domain cim:ActivePowerPerFrequency ;
  rdfs:range cim:UnitSymbol .

cim:ActivePowerPerFrequency.value a rdf:Property ;
  rdfs:label "value"@en ;
  cims:dataType cim:Float ;
  cims:multiplicity cims:M:0..1 ;
  cims:stereotype <http://iec.ch/TC57/NonStandard/UML#attribute> ;
  rdfs:domain cim:ActivePowerPerFrequency .

cim:AngleDegrees.multiplier a rdf:Property ;
  rdfs:label "multiplier"@en ;
  cims:isFixed "none" ;
  cims:multiplicity cims:M:0..1 ;
  cims:stereotype <http://iec.ch/TC57/NonStandard/UML#attribute> ;
  rdfs:domain cim:AngleDegrees ;
  rdfs:range cim:UnitMultiplier .

cim:AngleDegrees.unit a rdf:Property ;
  rdfs:label "unit"@en ;
  cims:isFixed "deg" ;
  cims:multiplicity cims:M:0..1 ;
  cims:stereotype <http://iec.ch/TC57/NonStandard/UML#attribute> ;
  rdfs:domain cim:AngleDegrees ;
  rdfs:range cim:UnitSymbol .

cim:AngleDegrees.value a rdf:Property ;
  rdfs:label "value"@en ;
  cims:dataType cim:Float ;
  cims:multiplicity cims:M:0..1 ;
  cims:stereotype <http://iec.ch/TC57/NonStandard/UML#attribute> ;
  rdfs:domain cim:AngleDegrees .

cim:ApparentPower.multiplier a rdf:Property ;
  rdfs:label "multiplier"@en ;
  cims:isFixed "M" ;
  cims:multiplicity cims:M:0..1 ;
  cims:stereotype <http://iec.ch/TC57/NonStandard/UML#attribute> ;
  rdfs:domain cim:ApparentPower ;
  rdfs:range cim:UnitMultiplier .

cim:ApparentPower.unit a rdf:Property ;
  rdfs:label "unit"@en ;
  cims:isFixed "VA" ;
  cims:multiplicity cims:M:0..1 ;
  cims:stereotype <http://iec.ch/TC57/NonStandard/UML#attribute> ;
  rdfs:domain cim:ApparentPower ;
  rdfs:range cim:UnitSymbol .

cim:ApparentPower.value a rdf:Property ;
  rdfs:label "value"@en ;
  cims:dataType cim:Float ;
  cims:multiplicity cims:M:0..1 ;
  cims:stereotype <http://iec.ch/TC57/NonStandard/UML#attribute> ;
  rdfs:domain cim:ApparentPower .

cim:ApparentPowerLimit.normalValue a rdf:Property ;
  rdfs:label "normalValue"@en ;
  rdfs:comment "The normal apparent power limit. The attribute shall be a positive value or zero." ;
  cims:dataType cim:ApparentPower ;
  cims:multiplicity cims:M:1..1 ;
  cims:stereotype <http://iec.ch/TC57/NonStandard/UML#attribute> ;
  rdfs:domain cim:ApparentPowerLimit .

cim:AsynchronousMachine.nominalFrequency a rdf:Property ;
  rdfs:label "nominalFrequency"@en ;
  rdfs:comment "Nameplate data indicates if the machine is 50 Hz or 60 Hz." ;
  cims:dataType cim:Frequency ;
  cims:multiplicity cims:M:0..1 ;
  cims:stereotype <http://iec.ch/TC57/NonStandard/UML#attribute> ;
  rdfs:domain cim:AsynchronousMachine .

cim:AsynchronousMachine.nominalSpeed a rdf:Property ;
  rdfs:label "nominalSpeed"@en ;
  rdfs:comment "Nameplate data.  Depends on the slip and number of pole pairs." ;
  cims:dataType cim:RotationSpeed ;
  cims:multiplicity cims:M:0..1 ;
  cims:stereotype <http://iec.ch/TC57/NonStandard/UML#attribute> ;
  rdfs:domain cim:AsynchronousMachine .

cim:AuxiliaryEquipment.Terminal a rdf:Property ;
  rdfs:label "Terminal"@en ;
  rdfs:comment "The Terminal at the equipment where the AuxiliaryEquipment is attached." ;
  cims:AssociationUsed "Yes" ;
  cims:inverseRoleName cim:Terminal.AuxiliaryEquipment ;
  cims:multiplicity cims:M:1 ;
  rdfs:domain cim:AuxiliaryEquipment ;
  rdfs:range cim:Terminal .

cim:BaseVoltage.ConductingEquipment a rdf:Property ;
  rdfs:label "ConductingEquipment"@en ;
  rdfs:comment "All conducting equipment with this base voltage.  Use only when there is no voltage level container used and only one base voltage applies.  For example, not used for transformers." ;
  cims:AssociationUsed "No" ;
  cims:inverseRoleName cim:ConductingEquipment.BaseVoltage ;
  cims:multiplicity cims:M:0..n ;
  rdfs:domain cim:BaseVoltage ;
  rdfs:range cim:ConductingEquipment .

cim:BaseVoltage.TransformerEnds a rdf:Property ;
  rdfs:label "TransformerEnds"@en ;
  rdfs:comment "Transformer ends at the base voltage.  This is essential for PU calculation." ;
  cims:AssociationUsed "No" ;
  cims:inverseRoleName cim:TransformerEnd.BaseVoltage ;
  cims:multiplicity cims:M:0..n ;
  rdfs:domain cim:BaseVoltage ;
  rdfs:range cim:TransformerEnd .

cim:BaseVoltage.VoltageLevel a rdf:Property ;
  rdfs:label "VoltageLevel"@en ;
  rdfs:comment "The voltage levels having this base voltage." ;
  cims:AssociationUsed "No" ;
  cims:inverseRoleName cim:VoltageLevel.BaseVoltage ;
  cims:multiplicity cims:M:0..n ;
  rdfs:domain cim:BaseVoltage ;
  rdfs:range cim:VoltageLevel .

cim:BaseVoltage.nominalVoltage a rdf:Property ;
  rdfs:label "nominalVoltage"@en ;
  rdfs:comment "The power system resource's base voltage.  Shall be a positive value and not zero." ;
  cims:dataType cim:Voltage ;
  cims:multiplicity cims:M:1..1 ;
  cims:stereotype <http://iec.ch/TC57/NonStandard/UML#attribute> ;
  rdfs:domain cim:BaseVoltage .

cim:BasicIntervalSchedule.startTime a rdf:Property ;
  rdfs:label "startTime"@en ;
  rdfs:comment "The time for the first time point.  The value can be a time of day, not a specific date." ;
  cims:dataType cim:DateTime ;
  cims:multiplicity cims:M:1..1 ;
  cims:stereotype <http://iec.ch/TC57/NonStandard/UML#attribute> ;
  rdfs:domain cim:BasicIntervalSchedule .

cim:BasicIntervalSchedule.value1Unit a rdf:Property ;
  rdfs:label "value1Unit"@en ;
  rdfs:comment "Value1 units of measure." ;
  cims:multiplicity cims:M:1..1 ;
  cims:stereotype <http://iec.ch/TC57/NonStandard/UML#attribute> ;
  rdfs:domain cim:BasicIntervalSchedule ;
  rdfs:range cim:UnitSymbol .

cim:BasicIntervalSchedule.value2Unit a rdf:Property ;
  rdfs:label "value2Unit"@en ;
  rdfs:comment "Value2 units of measure." ;
  cims:multiplicity cims:M:0..1 ;
  cims:stereotype <http://iec.ch/TC57/NonStandard/UML#attribute> ;
  rdfs:domain cim:BasicIntervalSchedule ;
  rdfs:range cim:UnitSymbol .

cim:BatteryUnit.ratedE a rdf:Property ;
  rdfs:label "ratedE"@en ;
  rdfs:comment "Full energy storage capacity of the battery. The attribute shall be a positive value." ;
  cims:dataType cim:RealEnergy ;
  cims:multiplicity cims:M:1..1 ;
  cims:stereotype <http://iec.ch/TC57/NonStandard/UML#attribute> ;
  rdfs:domain cim:BatteryUnit .

cim:Bay.VoltageLevel a rdf:Property ;
  rdfs:label "VoltageLevel"@en ;
  rdfs:comment "The voltage level containing this bay." ;
  cims:AssociationUsed "Yes" ;
  cims:inverseRoleName cim:VoltageLevel.Bays ;
  cims:multiplicity cims:M:1 ;
  rdfs:domain cim:Bay ;
  rdfs:range cim:VoltageLevel .

cim:BusNameMarker.ReportingGroup a rdf:Property ;
  rdfs:label "ReportingGroup"@en ;
  rdfs:comment "The reporting group to which this bus name marker belongs." ;
  cims:AssociationUsed "Yes" ;
  cims:inverseRoleName cim:ReportingGroup.BusNameMarker ;
  cims:multiplicity cims:M:0..1 ;
  rdfs:domain cim:BusNameMarker ;
  rdfs:range cim:ReportingGroup .

cim:BusNameMarker.Terminal a rdf:Property ;
  rdfs:label "Terminal"@en ;
  rdfs:comment "The terminals associated with this bus name marker." ;
  cims:AssociationUsed "No" ;
  cims:inverseRoleName cim:ACDCTerminal.BusNameMarker ;
  cims:multiplicity cims:M:1..n ;
  rdfs:domain cim:BusNameMarker ;
  rdfs:range cim:ACDCTerminal .

cim:BusNameMarker.priority a rdf:Property ;
  rdfs:label "priority"@en ;
  rdfs:comment "Priority of bus name marker for use as topology bus name.  Use 0 for do not care.  Use 1 for highest priority.  Use 2 as priority is less than 1 and so on." ;
  cims:dataType cim:Integer ;
  cims:multiplicity cims:M:0..1 ;
  cims:stereotype <http://iec.ch/TC57/NonStandard/UML#attribute> ;
  rdfs:domain cim:BusNameMarker .

cim:CAESPlant.ThermalGeneratingUnit a rdf:Property ;
  rdfs:label "ThermalGeneratingUnit"@en ;
  rdfs:comment "A thermal generating unit may be a member of a compressed air energy storage plant." ;
  cims:AssociationUsed "No" ;
  cims:inverseRoleName cim:ThermalGeneratingUnit.CAESPlant ;
  cims:multiplicity cims:M:0..1 ;
  rdfs:domain cim:CAESPlant ;
  rdfs:range cim:ThermalGeneratingUnit .

cim:Capacitance.multiplier a rdf:Property ;
  rdfs:label "multiplier"@en ;
  cims:isFixed "none" ;
  cims:multiplicity cims:M:0..1 ;
  cims:stereotype <http://iec.ch/TC57/NonStandard/UML#attribute> ;
  rdfs:domain cim:Capacitance ;
  rdfs:range cim:UnitMultiplier .

cim:Capacitance.unit a rdf:Property ;
  rdfs:label "unit"@en ;
  cims:isFixed "F" ;
  cims:multiplicity cims:M:0..1 ;
  cims:stereotype <http://iec.ch/TC57/NonStandard/UML#attribute> ;
  rdfs:domain cim:Capacitance ;
  rdfs:range cim:UnitSymbol .

cim:Capacitance.value a rdf:Property ;
  rdfs:label "value"@en ;
  cims:dataType cim:Float ;
  cims:multiplicity cims:M:0..1 ;
  cims:stereotype <http://iec.ch/TC57/NonStandard/UML#attribute> ;
  rdfs:domain cim:Capacitance .

cim:Clamp.ACLineSegment a rdf:Property ;
  rdfs:label "ACLineSegment"@en ;
  rdfs:comment "The line segment to which the clamp is connected." ;
  cims:AssociationUsed "Yes" ;
  cims:inverseRoleName cim:ACLineSegment.Clamp ;
  cims:multiplicity cims:M:1 ;
  rdfs:domain cim:Clamp ;
  rdfs:range cim:ACLineSegment .

cim:Clamp.lengthFromTerminal1 a rdf:Property ;
  rdfs:label "lengthFromTerminal1"@en ;
  rdfs:comment "The length to the place where the clamp is located starting from side one of the line segment, i.e. the line segment terminal with sequence number equal to 1." ;
  cims:dataType cim:Length ;
  cims:multiplicity cims:M:0..1 ;
  cims:stereotype <http://iec.ch/TC57/NonStandard/UML#attribute> ;
  rdfs:domain cim:Clamp .

cim:CogenerationPlant.ThermalGeneratingUnits a rdf:Property ;
  rdfs:label "ThermalGeneratingUnits"@en ;
  rdfs:comment "A thermal generating unit may be a member of a cogeneration plant." ;
  cims:AssociationUsed "No" ;
  cims:inverseRoleName cim:ThermalGeneratingUnit.CogenerationPlant ;
  cims:multiplicity cims:M:0..n ;
  rdfs:domain cim:CogenerationPlant ;
  rdfs:range cim:ThermalGeneratingUnit .

cim:CombinedCyclePlant.ThermalGeneratingUnits a rdf:Property ;
  rdfs:label "ThermalGeneratingUnits"@en ;
  rdfs:comment "A thermal generating unit may be a member of a combined cycle plant." ;
  cims:AssociationUsed "No" ;
  cims:inverseRoleName cim:ThermalGeneratingUnit.CombinedCyclePlant ;
  cims:multiplicity cims:M:0..n ;
  rdfs:domain cim:CombinedCyclePlant ;
  rdfs:range cim:ThermalGeneratingUnit .

cim:Conductance.multiplier a rdf:Property ;
  rdfs:label "multiplier"@en ;
  cims:isFixed "none" ;
  cims:multiplicity cims:M:0..1 ;
  cims:stereotype <http://iec.ch/TC57/NonStandard/UML#attribute> ;
  rdfs:domain cim:Conductance ;
  rdfs:range cim:UnitMultiplier .

cim:Conductance.unit a rdf:Property ;
  rdfs:label "unit"@en ;
  cims:isFixed "S" ;
  cims:multiplicity cims:M:0..1 ;
  cims:stereotype <http://iec.ch/TC57/NonStandard/UML#attribute> ;
  rdfs:domain cim:Conductance ;
  rdfs:range cim:UnitSymbol .

cim:Conductance.value a rdf:Property ;
  rdfs:label "value"@en ;
  cims:dataType cim:Float ;
  cims:multiplicity cims:M:0..1 ;
  cims:stereotype <http://iec.ch/TC57/NonStandard/UML#attribute> ;
  rdfs:domain cim:Conductance .

cim:ConductingEquipment.BaseVoltage a rdf:Property ;
  rdfs:label "BaseVoltage"@en ;
  rdfs:comment "Base voltage of this conducting equipment.  Use only when there is no voltage level container used and only one base voltage applies.  For example, not used for transformers." ;
  cims:AssociationUsed "Yes" ;
  cims:inverseRoleName cim:BaseVoltage.ConductingEquipment ;
  cims:multiplicity cims:M:0..1 ;
  rdfs:domain cim:ConductingEquipment ;
  rdfs:range cim:BaseVoltage .

cim:ConductingEquipment.Terminals a rdf:Property ;
  rdfs:label "Terminals"@en ;
  rdfs:comment "Conducting equipment have terminals that may be connected to other conducting equipment terminals via connectivity nodes or topological nodes." ;
  cims:AssociationUsed "No" ;
  cims:inverseRoleName cim:Terminal.ConductingEquipment ;
  cims:multiplicity cims:M:0..n ;
  rdfs:domain cim:ConductingEquipment ;
  rdfs:range cim:Terminal .

cim:Conductor.length a rdf:Property ;
  rdfs:label "length"@en ;
  rdfs:comment "Segment length for calculating line section capabilities." ;
  cims:dataType cim:Length ;
  cims:multiplicity cims:M:0..1 ;
  cims:stereotype <http://iec.ch/TC57/NonStandard/UML#attribute> ;
  rdfs:domain cim:Conductor .

cim:ConformLoad.LoadGroup a rdf:Property ;
  rdfs:label "LoadGroup"@en ;
  rdfs:comment "Group of this ConformLoad." ;
  cims:AssociationUsed "Yes" ;
  cims:inverseRoleName cim:ConformLoadGroup.EnergyConsumers ;
  cims:multiplicity cims:M:1 ;
  rdfs:domain cim:ConformLoad ;
  rdfs:range cim:ConformLoadGroup .

cim:ConformLoadGroup.ConformLoadSchedules a rdf:Property ;
  rdfs:label "ConformLoadSchedules"@en ;
  rdfs:comment "The ConformLoadSchedules in the ConformLoadGroup." ;
  cims:AssociationUsed "No" ;
  cims:inverseRoleName cim:ConformLoadSchedule.ConformLoadGroup ;
  cims:multiplicity cims:M:0..n ;
  rdfs:domain cim:ConformLoadGroup ;
  rdfs:range cim:ConformLoadSchedule .

cim:ConformLoadGroup.EnergyConsumers a rdf:Property ;
  rdfs:label "EnergyConsumers"@en ;
  rdfs:comment "Conform loads assigned to this ConformLoadGroup." ;
  cims:AssociationUsed "No" ;
  cims:inverseRoleName cim:ConformLoad.LoadGroup ;
  cims:multiplicity cims:M:1..n ;
  rdfs:domain cim:ConformLoadGroup ;
  rdfs:range cim:ConformLoad .

cim:ConformLoadSchedule.ConformLoadGroup a rdf:Property ;
  rdfs:label "ConformLoadGroup"@en ;
  rdfs:comment "The ConformLoadGroup where the ConformLoadSchedule belongs." ;
  cims:AssociationUsed "Yes" ;
  cims:inverseRoleName cim:ConformLoadGroup.ConformLoadSchedules ;
  cims:multiplicity cims:M:1 ;
  rdfs:domain cim:ConformLoadSchedule ;
  rdfs:range cim:ConformLoadGroup .

cim:ConnectivityNode.ConnectivityNodeContainer a rdf:Property ;
  rdfs:label "ConnectivityNodeContainer"@en ;
  rdfs:comment "Container of this connectivity node." ;
  cims:AssociationUsed "Yes" ;
  cims:inverseRoleName cim:ConnectivityNodeContainer.ConnectivityNodes ;
  cims:multiplicity cims:M:1 ;
  rdfs:domain cim:ConnectivityNode ;
  rdfs:range cim:ConnectivityNodeContainer .

cim:ConnectivityNode.Terminals a rdf:Property ;
  rdfs:label "Terminals"@en ;
  rdfs:comment "Terminals interconnected with zero impedance at a this connectivity node. " ;
  cims:AssociationUsed "No" ;
  cims:inverseRoleName cim:Terminal.ConnectivityNode ;
  cims:multiplicity cims:M:0..n ;
  rdfs:domain cim:ConnectivityNode ;
  rdfs:range cim:Terminal .

cim:ConnectivityNodeContainer.ConnectivityNodes a rdf:Property ;
  rdfs:label "ConnectivityNodes"@en ;
  rdfs:comment "Connectivity nodes which belong to this connectivity node container." ;
  cims:AssociationUsed "No" ;
  cims:inverseRoleName cim:ConnectivityNode.ConnectivityNodeContainer ;
  cims:multiplicity cims:M:0..n ;
  rdfs:domain cim:ConnectivityNodeContainer ;
  rdfs:range cim:ConnectivityNode .

cim:ControlArea.ControlAreaGeneratingUnit a rdf:Property ;
  rdfs:label "ControlAreaGeneratingUnit"@en ;
  rdfs:comment "The generating unit specifications for the control area." ;
  cims:AssociationUsed "No" ;
  cims:inverseRoleName cim:ControlAreaGeneratingUnit.ControlArea ;
  cims:multiplicity cims:M:0..n ;
  rdfs:domain cim:ControlArea ;
  rdfs:range cim:ControlAreaGeneratingUnit .

cim:ControlArea.EnergyArea a rdf:Property ;
  rdfs:label "EnergyArea"@en ;
  rdfs:comment "The energy area that is forecast from this control area specification." ;
  cims:AssociationUsed "Yes" ;
  cims:inverseRoleName cim:EnergyArea.ControlArea ;
  cims:multiplicity cims:M:1 ;
  rdfs:domain cim:ControlArea ;
  rdfs:range cim:EnergyArea .

cim:ControlArea.TieFlow a rdf:Property ;
  rdfs:label "TieFlow"@en ;
  rdfs:comment "The tie flows associated with the control area." ;
  cims:AssociationUsed "No" ;
  cims:inverseRoleName cim:TieFlow.ControlArea ;
  cims:multiplicity cims:M:0..n ;
  rdfs:domain cim:ControlArea ;
  rdfs:range cim:TieFlow .

cim:ControlArea.type a rdf:Property ;
  rdfs:label "type"@en ;
  rdfs:comment "The primary type of control area definition used to determine if this is used for automatic generation control, for planning interchange control, or other purposes.   A control area specified with primary type of automatic generation control could still be forecast and used as an interchange area in power flow analysis." ;
  cims:multiplicity cims:M:1..1 ;
  cims:stereotype <http://iec.ch/TC57/NonStandard/UML#attribute> ;
  rdfs:domain cim:ControlArea ;
  rdfs:range cim:ControlAreaTypeKind .

cim:ControlAreaGeneratingUnit.ControlArea a rdf:Property ;
  rdfs:label "ControlArea"@en ;
  rdfs:comment "The parent control area for the generating unit specifications." ;
  cims:AssociationUsed "Yes" ;
  cims:inverseRoleName cim:ControlArea.ControlAreaGeneratingUnit ;
  cims:multiplicity cims:M:1 ;
  rdfs:domain cim:ControlAreaGeneratingUnit ;
  rdfs:range cim:ControlArea .

cim:ControlAreaGeneratingUnit.GeneratingUnit a rdf:Property ;
  rdfs:label "GeneratingUnit"@en ;
  rdfs:comment "The generating unit specified for this control area.  Note that a control area should include a GeneratingUnit only once." ;
  cims:AssociationUsed "Yes" ;
  cims:inverseRoleName cim:GeneratingUnit.ControlAreaGeneratingUnit ;
  cims:multiplicity cims:M:1 ;
  rdfs:domain cim:ControlAreaGeneratingUnit ;
  rdfs:range cim:GeneratingUnit .

cim:CsConverter.maxAlpha a rdf:Property ;
  rdfs:label "maxAlpha"@en ;
  rdfs:comment "Maximum firing angle. It is converter’s configuration data used in power flow. The attribute shall be a positive value." ;
  cims:dataType cim:AngleDegrees ;
  cims:multiplicity cims:M:0..1 ;
  cims:stereotype <http://iec.ch/TC57/NonStandard/UML#attribute> ;
  rdfs:domain cim:CsConverter .

cim:CsConverter.maxGamma a rdf:Property ;
  rdfs:label "maxGamma"@en ;
  rdfs:comment "Maximum extinction angle. It is converter’s configuration data used in power flow. The attribute shall be a positive value." ;
  cims:dataType cim:AngleDegrees ;
  cims:multiplicity cims:M:0..1 ;
  cims:stereotype <http://iec.ch/TC57/NonStandard/UML#attribute> ;
  rdfs:domain cim:CsConverter .

cim:CsConverter.maxIdc a rdf:Property ;
  rdfs:label "maxIdc"@en ;
  rdfs:comment "The maximum direct current (Id) on the DC side at which the converter should operate. It is converter’s configuration data use in power flow. The attribute shall be a positive value." ;
  cims:dataType cim:CurrentFlow ;
  cims:multiplicity cims:M:0..1 ;
  cims:stereotype <http://iec.ch/TC57/NonStandard/UML#attribute> ;
  rdfs:domain cim:CsConverter .

cim:CsConverter.minAlpha a rdf:Property ;
  rdfs:label "minAlpha"@en ;
  rdfs:comment "Minimum firing angle. It is converter’s configuration data used in power flow. The attribute shall be a positive value." ;
  cims:dataType cim:AngleDegrees ;
  cims:multiplicity cims:M:0..1 ;
  cims:stereotype <http://iec.ch/TC57/NonStandard/UML#attribute> ;
  rdfs:domain cim:CsConverter .

cim:CsConverter.minGamma a rdf:Property ;
  rdfs:label "minGamma"@en ;
  rdfs:comment "Minimum extinction angle. It is converter’s configuration data used in power flow. The attribute shall be a positive value." ;
  cims:dataType cim:AngleDegrees ;
  cims:multiplicity cims:M:0..1 ;
  cims:stereotype <http://iec.ch/TC57/NonStandard/UML#attribute> ;
  rdfs:domain cim:CsConverter .

cim:CsConverter.minIdc a rdf:Property ;
  rdfs:label "minIdc"@en ;
  rdfs:comment "The minimum direct current (Id) on the DC side at which the converter should operate. It is converter’s configuration data used in power flow. The attribute shall be a positive value." ;
  cims:dataType cim:CurrentFlow ;
  cims:multiplicity cims:M:0..1 ;
  cims:stereotype <http://iec.ch/TC57/NonStandard/UML#attribute> ;
  rdfs:domain cim:CsConverter .

cim:CsConverter.ratedIdc a rdf:Property ;
  rdfs:label "ratedIdc"@en ;
  rdfs:comment "Rated converter DC current, also called IdN. The attribute shall be a positive value. It is converter’s configuration data used in power flow." ;
  cims:dataType cim:CurrentFlow ;
  cims:multiplicity cims:M:0..1 ;
  cims:stereotype <http://iec.ch/TC57/NonStandard/UML#attribute> ;
  rdfs:domain cim:CsConverter .

cim:CurrentFlow.multiplier a rdf:Property ;
  rdfs:label "multiplier"@en ;
  cims:isFixed "none" ;
  cims:multiplicity cims:M:0..1 ;
  cims:stereotype <http://iec.ch/TC57/NonStandard/UML#attribute> ;
  rdfs:domain cim:CurrentFlow ;
  rdfs:range cim:UnitMultiplier .

cim:CurrentFlow.unit a rdf:Property ;
  rdfs:label "unit"@en ;
  cims:isFixed "A" ;
  cims:multiplicity cims:M:0..1 ;
  cims:stereotype <http://iec.ch/TC57/NonStandard/UML#attribute> ;
  rdfs:domain cim:CurrentFlow ;
  rdfs:range cim:UnitSymbol .

cim:CurrentFlow.value a rdf:Property ;
  rdfs:label "value"@en ;
  cims:dataType cim:Float ;
  cims:multiplicity cims:M:0..1 ;
  cims:stereotype <http://iec.ch/TC57/NonStandard/UML#attribute> ;
  rdfs:domain cim:CurrentFlow .

cim:CurrentLimit.normalValue a rdf:Property ;
  rdfs:label "normalValue"@en ;
  rdfs:comment "The normal value for limit on current flow. The attribute shall be a positive value or zero." ;
  cims:dataType cim:CurrentFlow ;
  cims:multiplicity cims:M:1..1 ;
  cims:stereotype <http://iec.ch/TC57/NonStandard/UML#attribute> ;
  rdfs:domain cim:CurrentLimit .

cim:Curve.CurveDatas a rdf:Property ;
  rdfs:label "CurveDatas"@en ;
  rdfs:comment "The point data values that define this curve." ;
  cims:AssociationUsed "No" ;
  cims:inverseRoleName cim:CurveData.Curve ;
  cims:multiplicity cims:M:1..n ;
  rdfs:domain cim:Curve ;
  rdfs:range cim:CurveData .

cim:Curve.curveStyle a rdf:Property ;
  rdfs:label "curveStyle"@en ;
  rdfs:comment "The style or shape of the curve." ;
  cims:multiplicity cims:M:1..1 ;
  cims:stereotype <http://iec.ch/TC57/NonStandard/UML#attribute> ;
  rdfs:domain cim:Curve ;
  rdfs:range cim:CurveStyle .

cim:Curve.xUnit a rdf:Property ;
  rdfs:label "xUnit"@en ;
  rdfs:comment "The X-axis units of measure." ;
  cims:multiplicity cims:M:1..1 ;
  cims:stereotype <http://iec.ch/TC57/NonStandard/UML#attribute> ;
  rdfs:domain cim:Curve ;
  rdfs:range cim:UnitSymbol .

cim:Curve.y1Unit a rdf:Property ;
  rdfs:label "y1Unit"@en ;
  rdfs:comment "The Y1-axis units of measure." ;
  cims:multiplicity cims:M:1..1 ;
  cims:stereotype <http://iec.ch/TC57/NonStandard/UML#attribute> ;
  rdfs:domain cim:Curve ;
  rdfs:range cim:UnitSymbol .

cim:Curve.y2Unit a rdf:Property ;
  rdfs:label "y2Unit"@en ;
  rdfs:comment "The Y2-axis units of measure." ;
  cims:multiplicity cims:M:0..1 ;
  cims:stereotype <http://iec.ch/TC57/NonStandard/UML#attribute> ;
  rdfs:domain cim:Curve ;
  rdfs:range cim:UnitSymbol .

cim:CurveData.Curve a rdf:Property ;
  rdfs:label "Curve"@en ;
  rdfs:comment "The curve of  this curve data point." ;
  cims:AssociationUsed "Yes" ;
  cims:inverseRoleName cim:Curve.CurveDatas ;
  cims:multiplicity cims:M:1 ;
  rdfs:domain cim:CurveData ;
  rdfs:range cim:Curve .

cim:CurveData.xvalue a rdf:Property ;
  rdfs:label "xvalue"@en ;
  rdfs:comment "The data value of the X-axis variable,  depending on the X-axis units." ;
  cims:dataType cim:Float ;
  cims:multiplicity cims:M:1..1 ;
  cims:stereotype <http://iec.ch/TC57/NonStandard/UML#attribute> ;
  rdfs:domain cim:CurveData .

cim:CurveData.y1value a rdf:Property ;
  rdfs:label "y1value"@en ;
  rdfs:comment "The data value of the  first Y-axis variable, depending on the Y-axis units." ;
  cims:dataType cim:Float ;
  cims:multiplicity cims:M:1..1 ;
  cims:stereotype <http://iec.ch/TC57/NonStandard/UML#attribute> ;
  rdfs:domain cim:CurveData .

cim:CurveData.y2value a rdf:Property ;
  rdfs:label "y2value"@en ;
  rdfs:comment "The data value of the second Y-axis variable (if present), depending on the Y-axis units." ;
  cims:dataType cim:Float ;
  cims:multiplicity cims:M:0..1 ;
  cims:stereotype <http://iec.ch/TC57/NonStandard/UML#attribute> ;
  rdfs:domain cim:CurveData .

cim:Cut.ACLineSegment a rdf:Property ;
  rdfs:label "ACLineSegment"@en ;
  rdfs:comment "The line segment to which the cut is applied." ;
  cims:AssociationUsed "Yes" ;
  cims:inverseRoleName cim:ACLineSegment.Cut ;
  cims:multiplicity cims:M:1 ;
  rdfs:domain cim:Cut ;
  rdfs:range cim:ACLineSegment .

cim:Cut.lengthFromTerminal1 a rdf:Property ;
  rdfs:label "lengthFromTerminal1"@en ;
  rdfs:comment "The length to the place where the cut is located starting from side one of the cut line segment, i.e. the line segment Terminal with sequenceNumber equal to 1." ;
  cims:dataType cim:Length ;
  cims:multiplicity cims:M:0..1 ;
  cims:stereotype <http://iec.ch/TC57/NonStandard/UML#attribute> ;
  rdfs:domain cim:Cut .

cim:DCBaseTerminal.DCNode a rdf:Property ;
  rdfs:label "DCNode"@en ;
  rdfs:comment "The DC connectivity node to which this DC base terminal connects with zero impedance." ;
  cims:AssociationUsed "Yes" ;
  cims:inverseRoleName cim:DCNode.DCTerminals ;
  cims:multiplicity cims:M:0..1 ;
  rdfs:domain cim:DCBaseTerminal ;
  rdfs:range cim:DCNode .

cim:DCConductingEquipment.DCTerminals a rdf:Property ;
  rdfs:label "DCTerminals"@en ;
  rdfs:comment "A DC conducting equipment has DC terminals." ;
  cims:AssociationUsed "No" ;
  cims:inverseRoleName cim:DCTerminal.DCConductingEquipment ;
  cims:multiplicity cims:M:0..n ;
  rdfs:domain cim:DCConductingEquipment ;
  rdfs:range cim:DCTerminal .

cim:DCConductingEquipment.ratedUdc a rdf:Property ;
  rdfs:label "ratedUdc"@en ;
  rdfs:comment "Rated DC device voltage. The attribute shall be a positive value. It is configuration data used in power flow." ;
  cims:dataType cim:Voltage ;
  cims:multiplicity cims:M:1..1 ;
  cims:stereotype <http://iec.ch/TC57/NonStandard/UML#attribute> ;
  rdfs:domain cim:DCConductingEquipment .

cim:DCConverterUnit.Substation a rdf:Property ;
  rdfs:label "Substation"@en ;
  rdfs:comment "The containing substation of the DC converter unit." ;
  cims:AssociationUsed "Yes" ;
  cims:inverseRoleName cim:Substation.DCConverterUnit ;
  cims:multiplicity cims:M:0..1 ;
  rdfs:domain cim:DCConverterUnit ;
  rdfs:range cim:Substation .

cim:DCConverterUnit.operationMode a rdf:Property ;
  rdfs:label "operationMode"@en ;
  rdfs:comment "The operating mode of an HVDC bipole (bipolar, monopolar metallic return, etc)." ;
  cims:multiplicity cims:M:1..1 ;
  cims:stereotype <http://iec.ch/TC57/NonStandard/UML#attribute> ;
  rdfs:domain cim:DCConverterUnit ;
  rdfs:range cim:DCConverterOperatingModeKind .

cim:DCEquipmentContainer.DCNodes a rdf:Property ;
  rdfs:label "DCNodes"@en ;
  rdfs:comment "The DC nodes contained in the DC equipment container." ;
  cims:AssociationUsed "No" ;
  cims:inverseRoleName cim:DCNode.DCEquipmentContainer ;
  cims:multiplicity cims:M:0..n ;
  rdfs:domain cim:DCEquipmentContainer ;
  rdfs:range cim:DCNode .

cim:DCGround.inductance a rdf:Property ;
  rdfs:label "inductance"@en ;
  rdfs:comment "Inductance to ground." ;
  cims:dataType cim:Inductance ;
  cims:multiplicity cims:M:0..1 ;
  cims:stereotype <http://iec.ch/TC57/NonStandard/UML#attribute> ;
  rdfs:domain cim:DCGround .

cim:DCGround.r a rdf:Property ;
  rdfs:label "r"@en ;
  rdfs:comment "Resistance to ground." ;
  cims:dataType cim:Resistance ;
  cims:multiplicity cims:M:0..1 ;
  cims:stereotype <http://iec.ch/TC57/NonStandard/UML#attribute> ;
  rdfs:domain cim:DCGround .

cim:DCLine.Region a rdf:Property ;
  rdfs:label "Region"@en ;
  rdfs:comment "The SubGeographicalRegion containing the DC line." ;
  cims:AssociationUsed "Yes" ;
  cims:inverseRoleName cim:SubGeographicalRegion.DCLines ;
  cims:multiplicity cims:M:0..1 ;
  rdfs:domain cim:DCLine ;
  rdfs:range cim:SubGeographicalRegion .

cim:DCLineSegment.capacitance a rdf:Property ;
  rdfs:label "capacitance"@en ;
  rdfs:comment "Capacitance of the DC line segment. Significant for cables only." ;
  cims:dataType cim:Capacitance ;
  cims:multiplicity cims:M:1..1 ;
  cims:stereotype <http://iec.ch/TC57/NonStandard/UML#attribute> ;
  rdfs:domain cim:DCLineSegment .

cim:DCLineSegment.inductance a rdf:Property ;
  rdfs:label "inductance"@en ;
  rdfs:comment "Inductance of the DC line segment. Negligible compared with DCSeriesDevice used for smoothing." ;
  cims:dataType cim:Inductance ;
  cims:multiplicity cims:M:1..1 ;
  cims:stereotype <http://iec.ch/TC57/NonStandard/UML#attribute> ;
  rdfs:domain cim:DCLineSegment .

cim:DCLineSegment.length a rdf:Property ;
  rdfs:label "length"@en ;
  rdfs:comment "Segment length for calculating line section capabilities." ;
  cims:dataType cim:Length ;
  cims:multiplicity cims:M:0..1 ;
  cims:stereotype <http://iec.ch/TC57/NonStandard/UML#attribute> ;
  rdfs:domain cim:DCLineSegment .

cim:DCLineSegment.resistance a rdf:Property ;
  rdfs:label "resistance"@en ;
  rdfs:comment "Resistance of the DC line segment." ;
  cims:dataType cim:Resistance ;
  cims:multiplicity cims:M:1..1 ;
  cims:stereotype <http://iec.ch/TC57/NonStandard/UML#attribute> ;
  rdfs:domain cim:DCLineSegment .

cim:DCNode.DCEquipmentContainer a rdf:Property ;
  rdfs:label "DCEquipmentContainer"@en ;
  rdfs:comment "The DC container for the DC nodes." ;
  cims:AssociationUsed "Yes" ;
  cims:inverseRoleName cim:DCEquipmentContainer.DCNodes ;
  cims:multiplicity cims:M:1 ;
  rdfs:domain cim:DCNode ;
  rdfs:range cim:DCEquipmentContainer .

cim:DCNode.DCTerminals a rdf:Property ;
  rdfs:label "DCTerminals"@en ;
  rdfs:comment "DC base terminals interconnected with zero impedance at a this DC connectivity node. " ;
  cims:AssociationUsed "No" ;
  cims:inverseRoleName cim:DCBaseTerminal.DCNode ;
  cims:multiplicity cims:M:0..n ;
  rdfs:domain cim:DCNode ;
  rdfs:range cim:DCBaseTerminal .

cim:DCSeriesDevice.inductance a rdf:Property ;
  rdfs:label "inductance"@en ;
  rdfs:comment "Inductance of the device." ;
  cims:dataType cim:Inductance ;
  cims:multiplicity cims:M:1..1 ;
  cims:stereotype <http://iec.ch/TC57/NonStandard/UML#attribute> ;
  rdfs:domain cim:DCSeriesDevice .

cim:DCSeriesDevice.resistance a rdf:Property ;
  rdfs:label "resistance"@en ;
  rdfs:comment "Resistance of the DC device." ;
  cims:dataType cim:Resistance ;
  cims:multiplicity cims:M:1..1 ;
  cims:stereotype <http://iec.ch/TC57/NonStandard/UML#attribute> ;
  rdfs:domain cim:DCSeriesDevice .

cim:DCShunt.capacitance a rdf:Property ;
  rdfs:label "capacitance"@en ;
  rdfs:comment "Capacitance of the DC shunt." ;
  cims:dataType cim:Capacitance ;
  cims:multiplicity cims:M:1..1 ;
  cims:stereotype <http://iec.ch/TC57/NonStandard/UML#attribute> ;
  rdfs:domain cim:DCShunt .

cim:DCShunt.resistance a rdf:Property ;
  rdfs:label "resistance"@en ;
  rdfs:comment "Resistance of the DC device." ;
  cims:dataType cim:Resistance ;
  cims:multiplicity cims:M:1..1 ;
  cims:stereotype <http://iec.ch/TC57/NonStandard/UML#attribute> ;
  rdfs:domain cim:DCShunt .

cim:DCTerminal.DCConductingEquipment a rdf:Property ;
  rdfs:label "DCConductingEquipment"@en ;
  rdfs:comment "An DC  terminal belong to a DC conducting equipment." ;
  cims:AssociationUsed "Yes" ;
  cims:inverseRoleName cim:DCConductingEquipment.DCTerminals ;
  cims:multiplicity cims:M:1 ;
  rdfs:domain cim:DCTerminal ;
  rdfs:range cim:DCConductingEquipment .

cim:DayType.SeasonDayTypeSchedules a rdf:Property ;
  rdfs:label "SeasonDayTypeSchedules"@en ;
  rdfs:comment "Schedules that use this DayType." ;
  cims:AssociationUsed "No" ;
  cims:inverseRoleName cim:SeasonDayTypeSchedule.DayType ;
  cims:multiplicity cims:M:0..n ;
  rdfs:domain cim:DayType ;
  rdfs:range cim:SeasonDayTypeSchedule .

cim:EnergyArea.ControlArea a rdf:Property ;
  rdfs:label "ControlArea"@en ;
  rdfs:comment "The control area specification that is used for the load forecast." ;
  cims:AssociationUsed "No" ;
  cims:inverseRoleName cim:ControlArea.EnergyArea ;
  cims:multiplicity cims:M:0..1 ;
  rdfs:domain cim:EnergyArea ;
  rdfs:range cim:ControlArea .

cim:EnergyConsumer.LoadResponse a rdf:Property ;
  rdfs:label "LoadResponse"@en ;
  rdfs:comment "The load response characteristic of this load.  If missing, this load is assumed to be constant power." ;
  cims:AssociationUsed "Yes" ;
  cims:inverseRoleName cim:LoadResponseCharacteristic.EnergyConsumer ;
  cims:multiplicity cims:M:0..1 ;
  rdfs:domain cim:EnergyConsumer ;
  rdfs:range cim:LoadResponseCharacteristic .

cim:EnergyConsumer.pfixed a rdf:Property ;
  rdfs:label "pfixed"@en ;
  rdfs:comment "Active power of the load that is a fixed quantity and does not vary as load group value varies. Load sign convention is used, i.e. positive sign means flow out from a node.  " ;
  cims:dataType cim:ActivePower ;
  cims:multiplicity cims:M:0..1 ;
  cims:stereotype <http://iec.ch/TC57/NonStandard/UML#attribute> ;
  rdfs:domain cim:EnergyConsumer .

cim:EnergyConsumer.pfixedPct a rdf:Property ;
  rdfs:label "pfixedPct"@en ;
  rdfs:comment "Fixed active power as a percentage of load group fixed active power. Used to represent the time-varying components.  Load sign convention is used, i.e. positive sign means flow out from a node." ;
  cims:dataType cim:PerCent ;
  cims:multiplicity cims:M:0..1 ;
  cims:stereotype <http://iec.ch/TC57/NonStandard/UML#attribute> ;
  rdfs:domain cim:EnergyConsumer .

cim:EnergyConsumer.qfixed a rdf:Property ;
  rdfs:label "qfixed"@en ;
  rdfs:comment "Reactive power of the load that is a fixed quantity and does not vary as load group value varies. Load sign convention is used, i.e. positive sign means flow out from a node." ;
  cims:dataType cim:ReactivePower ;
  cims:multiplicity cims:M:0..1 ;
  cims:stereotype <http://iec.ch/TC57/NonStandard/UML#attribute> ;
  rdfs:domain cim:EnergyConsumer .

cim:EnergyConsumer.qfixedPct a rdf:Property ;
  rdfs:label "qfixedPct"@en ;
  rdfs:comment "Fixed reactive power as a percentage of load group fixed reactive power. Used to represent the time-varying components.  Load sign convention is used, i.e. positive sign means flow out from a node." ;
  cims:dataType cim:PerCent ;
  cims:multiplicity cims:M:0..1 ;
  cims:stereotype <http://iec.ch/TC57/NonStandard/UML#attribute> ;
  rdfs:domain cim:EnergyConsumer .

cim:EnergySchedulingType.EnergySource a rdf:Property ;
  rdfs:label "EnergySource"@en ;
  rdfs:comment "Energy Source of a particular Energy Scheduling Type." ;
  cims:AssociationUsed "No" ;
  cims:inverseRoleName cim:EnergySource.EnergySchedulingType ;
  cims:multiplicity cims:M:0..n ;
  rdfs:domain cim:EnergySchedulingType ;
  rdfs:range cim:EnergySource .

cim:EnergySource.EnergySchedulingType a rdf:Property ;
  rdfs:label "EnergySchedulingType"@en ;
  rdfs:comment "Energy Scheduling Type of an Energy Source." ;
  cims:AssociationUsed "Yes" ;
  cims:inverseRoleName cim:EnergySchedulingType.EnergySource ;
  cims:multiplicity cims:M:0..1 ;
  rdfs:domain cim:EnergySource ;
  rdfs:range cim:EnergySchedulingType .

cim:EnergySource.nominalVoltage a rdf:Property ;
  rdfs:label "nominalVoltage"@en ;
  rdfs:comment "Phase-to-phase nominal voltage." ;
  cims:dataType cim:Voltage ;
  cims:multiplicity cims:M:0..1 ;
  cims:stereotype <http://iec.ch/TC57/NonStandard/UML#attribute> ;
  rdfs:domain cim:EnergySource .

cim:EnergySource.pMax a rdf:Property ;
  rdfs:label "pMax"@en ;
  rdfs:comment "This is the maximum active power that can be produced by the source. Load sign convention is used, i.e. positive sign means flow out from a TopologicalNode (bus) into the conducting equipment." ;
  cims:dataType cim:ActivePower ;
  cims:multiplicity cims:M:0..1 ;
  cims:stereotype <http://iec.ch/TC57/NonStandard/UML#attribute> ;
  rdfs:domain cim:EnergySource .

cim:EnergySource.pMin a rdf:Property ;
  rdfs:label "pMin"@en ;
  rdfs:comment "This is the minimum active power that can be produced by the source. Load sign convention is used, i.e. positive sign means flow out from a TopologicalNode (bus) into the conducting equipment." ;
  cims:dataType cim:ActivePower ;
  cims:multiplicity cims:M:0..1 ;
  cims:stereotype <http://iec.ch/TC57/NonStandard/UML#attribute> ;
  rdfs:domain cim:EnergySource .

cim:Equipment.EquipmentContainer a rdf:Property ;
  rdfs:label "EquipmentContainer"@en ;
  rdfs:comment "Container of this equipment." ;
  cims:AssociationUsed "Yes" ;
  cims:inverseRoleName cim:EquipmentContainer.Equipments ;
  cims:multiplicity cims:M:0..1 ;
  rdfs:domain cim:Equipment ;
  rdfs:range cim:EquipmentContainer .

cim:Equipment.OperationalLimitSet a rdf:Property ;
  rdfs:label "OperationalLimitSet"@en ;
  rdfs:comment "The operational limit sets associated with this equipment." ;
  cims:AssociationUsed "No" ;
  cims:inverseRoleName cim:OperationalLimitSet.Equipment ;
  cims:multiplicity cims:M:0..n ;
  rdfs:domain cim:Equipment ;
  rdfs:range cim:OperationalLimitSet .

cim:Equipment.aggregate a rdf:Property ;
  rdfs:label "aggregate"@en ;
  rdfs:comment """The aggregate flag provides an alternative way of representing an aggregated (equivalent) element. It is applicable in cases when the dedicated classes for equivalent equipment do not have all of the attributes necessary to represent the required level of detail.  In case the flag is set to “true” the single instance of equipment represents multiple pieces of equipment that have been modelled together as an aggregate equivalent obtained by a network reduction procedure. Examples would be power transformers or synchronous machines operating in parallel modelled as a single aggregate power transformer or aggregate synchronous machine.  
The attribute is not used for EquivalentBranch, EquivalentShunt and EquivalentInjection.""" ;
  cims:dataType cim:Boolean ;
  cims:multiplicity cims:M:0..1 ;
  cims:stereotype <http://iec.ch/TC57/NonStandard/UML#attribute> ;
  rdfs:domain cim:Equipment .

cim:Equipment.normallyInService a rdf:Property ;
  rdfs:label "normallyInService"@en ;
  rdfs:comment "Specifies the availability of the equipment under normal operating conditions. True means the equipment is available for topology processing, which determines if the equipment is energized or not. False means that the equipment is treated by network applications as if it is not in the model." ;
  cims:dataType cim:Boolean ;
  cims:multiplicity cims:M:0..1 ;
  cims:stereotype <http://iec.ch/TC57/NonStandard/UML#attribute> ;
  rdfs:domain cim:Equipment .

cim:EquipmentContainer.Equipments a rdf:Property ;
  rdfs:label "Equipments"@en ;
  rdfs:comment "Contained equipment." ;
  cims:AssociationUsed "No" ;
  cims:inverseRoleName cim:Equipment.EquipmentContainer ;
  cims:multiplicity cims:M:0..n ;
  rdfs:domain cim:EquipmentContainer ;
  rdfs:range cim:Equipment .

cim:EquivalentBranch.r a rdf:Property ;
  rdfs:label "r"@en ;
  rdfs:comment "Positive sequence series resistance of the reduced branch." ;
  cims:dataType cim:Resistance ;
  cims:multiplicity cims:M:1..1 ;
  cims:stereotype <http://iec.ch/TC57/NonStandard/UML#attribute> ;
  rdfs:domain cim:EquivalentBranch .

cim:EquivalentBranch.r21 a rdf:Property ;
  rdfs:label "r21"@en ;
  rdfs:comment """Resistance from terminal sequence 2 to terminal sequence 1 .Used for steady state power flow. This attribute is optional and represent unbalanced network such as off-nominal phase shifter. If only EquivalentBranch.r is given, then EquivalentBranch.r21 is assumed equal to EquivalentBranch.r.
Usage rule : EquivalentBranch is a result of network reduction prior to the data exchange.""" ;
  cims:dataType cim:Resistance ;
  cims:multiplicity cims:M:0..1 ;
  cims:stereotype <http://iec.ch/TC57/NonStandard/UML#attribute> ;
  rdfs:domain cim:EquivalentBranch .

cim:EquivalentBranch.x a rdf:Property ;
  rdfs:label "x"@en ;
  rdfs:comment "Positive sequence series reactance of the reduced branch." ;
  cims:dataType cim:Reactance ;
  cims:multiplicity cims:M:1..1 ;
  cims:stereotype <http://iec.ch/TC57/NonStandard/UML#attribute> ;
  rdfs:domain cim:EquivalentBranch .

cim:EquivalentBranch.x21 a rdf:Property ;
  rdfs:label "x21"@en ;
  rdfs:comment """Reactance from terminal sequence 2 to terminal sequence 1. Used for steady state power flow. This attribute is optional and represents an unbalanced network such as off-nominal phase shifter. If only EquivalentBranch.x is given, then EquivalentBranch.x21 is assumed equal to EquivalentBranch.x.
Usage rule: EquivalentBranch is a result of network reduction prior to the data exchange.""" ;
  cims:dataType cim:Reactance ;
  cims:multiplicity cims:M:0..1 ;
  cims:stereotype <http://iec.ch/TC57/NonStandard/UML#attribute> ;
  rdfs:domain cim:EquivalentBranch .

cim:EquivalentEquipment.EquivalentNetwork a rdf:Property ;
  rdfs:label "EquivalentNetwork"@en ;
  rdfs:comment "The equivalent where the reduced model belongs." ;
  cims:AssociationUsed "Yes" ;
  cims:inverseRoleName cim:EquivalentNetwork.EquivalentEquipments ;
  cims:multiplicity cims:M:0..1 ;
  rdfs:domain cim:EquivalentEquipment ;
  rdfs:range cim:EquivalentNetwork .

cim:EquivalentInjection.ReactiveCapabilityCurve a rdf:Property ;
  rdfs:label "ReactiveCapabilityCurve"@en ;
  rdfs:comment "The reactive capability curve used by this equivalent injection." ;
  cims:AssociationUsed "Yes" ;
  cims:inverseRoleName cim:ReactiveCapabilityCurve.EquivalentInjection ;
  cims:multiplicity cims:M:0..1 ;
  rdfs:domain cim:EquivalentInjection ;
  rdfs:range cim:ReactiveCapabilityCurve .

cim:EquivalentInjection.maxP a rdf:Property ;
  rdfs:label "maxP"@en ;
  rdfs:comment "Maximum active power of the injection." ;
  cims:dataType cim:ActivePower ;
  cims:multiplicity cims:M:0..1 ;
  cims:stereotype <http://iec.ch/TC57/NonStandard/UML#attribute> ;
  rdfs:domain cim:EquivalentInjection .

cim:EquivalentInjection.maxQ a rdf:Property ;
  rdfs:label "maxQ"@en ;
  rdfs:comment "Maximum reactive power of the injection.  Used for modelling of infeed for load flow exchange. Not used for short circuit modelling.  If maxQ and minQ are not used ReactiveCapabilityCurve can be used.   " ;
  cims:dataType cim:ReactivePower ;
  cims:multiplicity cims:M:0..1 ;
  cims:stereotype <http://iec.ch/TC57/NonStandard/UML#attribute> ;
  rdfs:domain cim:EquivalentInjection .

cim:EquivalentInjection.minP a rdf:Property ;
  rdfs:label "minP"@en ;
  rdfs:comment "Minimum active power of the injection." ;
  cims:dataType cim:ActivePower ;
  cims:multiplicity cims:M:0..1 ;
  cims:stereotype <http://iec.ch/TC57/NonStandard/UML#attribute> ;
  rdfs:domain cim:EquivalentInjection .

cim:EquivalentInjection.minQ a rdf:Property ;
  rdfs:label "minQ"@en ;
  rdfs:comment "Minimum reactive power of the injection.  Used for modelling of infeed for load flow exchange. Not used for short circuit modelling.  If maxQ and minQ are not used ReactiveCapabilityCurve can be used." ;
  cims:dataType cim:ReactivePower ;
  cims:multiplicity cims:M:0..1 ;
  cims:stereotype <http://iec.ch/TC57/NonStandard/UML#attribute> ;
  rdfs:domain cim:EquivalentInjection .

cim:EquivalentInjection.regulationCapability a rdf:Property ;
  rdfs:label "regulationCapability"@en ;
  rdfs:comment "Specifies whether or not the EquivalentInjection has the capability to regulate the local voltage. If true the EquivalentInjection can regulate. If false the EquivalentInjection cannot regulate. ReactiveCapabilityCurve can only be associated with EquivalentInjection  if the flag is true." ;
  cims:dataType cim:Boolean ;
  cims:multiplicity cims:M:1..1 ;
  cims:stereotype <http://iec.ch/TC57/NonStandard/UML#attribute> ;
  rdfs:domain cim:EquivalentInjection .

cim:EquivalentNetwork.EquivalentEquipments a rdf:Property ;
  rdfs:label "EquivalentEquipments"@en ;
  rdfs:comment "The associated reduced equivalents." ;
  cims:AssociationUsed "No" ;
  cims:inverseRoleName cim:EquivalentEquipment.EquivalentNetwork ;
  cims:multiplicity cims:M:0..n ;
  rdfs:domain cim:EquivalentNetwork ;
  rdfs:range cim:EquivalentEquipment .

cim:EquivalentShunt.b a rdf:Property ;
  rdfs:label "b"@en ;
  rdfs:comment "Positive sequence shunt susceptance." ;
  cims:dataType cim:Susceptance ;
  cims:multiplicity cims:M:1..1 ;
  cims:stereotype <http://iec.ch/TC57/NonStandard/UML#attribute> ;
  rdfs:domain cim:EquivalentShunt .

cim:EquivalentShunt.g a rdf:Property ;
  rdfs:label "g"@en ;
  rdfs:comment "Positive sequence shunt conductance." ;
  cims:dataType cim:Conductance ;
  cims:multiplicity cims:M:1..1 ;
  cims:stereotype <http://iec.ch/TC57/NonStandard/UML#attribute> ;
  rdfs:domain cim:EquivalentShunt .

cim:ExternalNetworkInjection.governorSCD a rdf:Property ;
  rdfs:label "governorSCD"@en ;
  rdfs:comment "Power Frequency Bias. This is the change in power injection divided by the change in frequency and negated.  A positive value of the power frequency bias provides additional power injection upon a drop in frequency." ;
  cims:dataType cim:ActivePowerPerFrequency ;
  cims:multiplicity cims:M:1..1 ;
  cims:stereotype <http://iec.ch/TC57/NonStandard/UML#attribute> ;
  rdfs:domain cim:ExternalNetworkInjection .

cim:ExternalNetworkInjection.maxP a rdf:Property ;
  rdfs:label "maxP"@en ;
  rdfs:comment "Maximum active power of the injection." ;
  cims:dataType cim:ActivePower ;
  cims:multiplicity cims:M:1..1 ;
  cims:stereotype <http://iec.ch/TC57/NonStandard/UML#attribute> ;
  rdfs:domain cim:ExternalNetworkInjection .

cim:ExternalNetworkInjection.maxQ a rdf:Property ;
  rdfs:label "maxQ"@en ;
  rdfs:comment "Maximum reactive power limit. It is used for modelling of infeed for load flow exchange and not for short circuit modelling." ;
  cims:dataType cim:ReactivePower ;
  cims:multiplicity cims:M:1..1 ;
  cims:stereotype <http://iec.ch/TC57/NonStandard/UML#attribute> ;
  rdfs:domain cim:ExternalNetworkInjection .

cim:ExternalNetworkInjection.minP a rdf:Property ;
  rdfs:label "minP"@en ;
  rdfs:comment "Minimum active power of the injection." ;
  cims:dataType cim:ActivePower ;
  cims:multiplicity cims:M:1..1 ;
  cims:stereotype <http://iec.ch/TC57/NonStandard/UML#attribute> ;
  rdfs:domain cim:ExternalNetworkInjection .

cim:ExternalNetworkInjection.minQ a rdf:Property ;
  rdfs:label "minQ"@en ;
  rdfs:comment "Minimum reactive power limit. It is used for modelling of infeed for load flow exchange and not for short circuit modelling." ;
  cims:dataType cim:ReactivePower ;
  cims:multiplicity cims:M:1..1 ;
  cims:stereotype <http://iec.ch/TC57/NonStandard/UML#attribute> ;
  rdfs:domain cim:ExternalNetworkInjection .

cim:FossilFuel.ThermalGeneratingUnit a rdf:Property ;
  rdfs:label "ThermalGeneratingUnit"@en ;
  rdfs:comment "A thermal generating unit may have one or more fossil fuels." ;
  cims:AssociationUsed "Yes" ;
  cims:inverseRoleName cim:ThermalGeneratingUnit.FossilFuels ;
  cims:multiplicity cims:M:1 ;
  rdfs:domain cim:FossilFuel ;
  rdfs:range cim:ThermalGeneratingUnit .

cim:FossilFuel.fossilFuelType a rdf:Property ;
  rdfs:label "fossilFuelType"@en ;
  rdfs:comment "The type of fossil fuel, such as coal, oil, or gas." ;
  cims:multiplicity cims:M:1..1 ;
  cims:stereotype <http://iec.ch/TC57/NonStandard/UML#attribute> ;
  rdfs:domain cim:FossilFuel ;
  rdfs:range cim:FuelType .

cim:Frequency.multiplier a rdf:Property ;
  rdfs:label "multiplier"@en ;
  cims:isFixed "none" ;
  cims:multiplicity cims:M:0..1 ;
  cims:stereotype <http://iec.ch/TC57/NonStandard/UML#attribute> ;
  rdfs:domain cim:Frequency ;
  rdfs:range cim:UnitMultiplier .

cim:Frequency.unit a rdf:Property ;
  rdfs:label "unit"@en ;
  cims:isFixed "Hz" ;
  cims:multiplicity cims:M:0..1 ;
  cims:stereotype <http://iec.ch/TC57/NonStandard/UML#attribute> ;
  rdfs:domain cim:Frequency ;
  rdfs:range cim:UnitSymbol .

cim:Frequency.value a rdf:Property ;
  rdfs:label "value"@en ;
  cims:dataType cim:Float ;
  cims:multiplicity cims:M:0..1 ;
  cims:stereotype <http://iec.ch/TC57/NonStandard/UML#attribute> ;
  rdfs:domain cim:Frequency .

cim:GeneratingUnit.ControlAreaGeneratingUnit a rdf:Property ;
  rdfs:label "ControlAreaGeneratingUnit"@en ;
  rdfs:comment "ControlArea specifications for this generating unit." ;
  cims:AssociationUsed "No" ;
  cims:inverseRoleName cim:ControlAreaGeneratingUnit.GeneratingUnit ;
  cims:multiplicity cims:M:0..n ;
  rdfs:domain cim:GeneratingUnit ;
  rdfs:range cim:ControlAreaGeneratingUnit .

cim:GeneratingUnit.GrossToNetActivePowerCurves a rdf:Property ;
  rdfs:label "GrossToNetActivePowerCurves"@en ;
  rdfs:comment "A generating unit may have a gross active power to net active power curve, describing the losses and auxiliary power requirements of the unit." ;
  cims:AssociationUsed "No" ;
  cims:inverseRoleName cim:GrossToNetActivePowerCurve.GeneratingUnit ;
  cims:multiplicity cims:M:0..n ;
  cims:stereotype <http://iec.ch/TC57/NonStandard/UML#ofAggregate> ;
  rdfs:domain cim:GeneratingUnit ;
  rdfs:range cim:GrossToNetActivePowerCurve .

cim:GeneratingUnit.RotatingMachine a rdf:Property ;
  rdfs:label "RotatingMachine"@en ;
  rdfs:comment "A synchronous machine may operate as a generator and as such becomes a member of a generating unit." ;
  cims:AssociationUsed "No" ;
  cims:inverseRoleName cim:RotatingMachine.GeneratingUnit ;
  cims:multiplicity cims:M:1..n ;
  rdfs:domain cim:GeneratingUnit ;
  rdfs:range cim:RotatingMachine .

cim:GeneratingUnit.genControlSource a rdf:Property ;
  rdfs:label "genControlSource"@en ;
  rdfs:comment "The source of controls for a generating unit.  Defines the control status of the generating unit." ;
  cims:multiplicity cims:M:0..1 ;
  cims:stereotype <http://iec.ch/TC57/NonStandard/UML#attribute> ;
  rdfs:domain cim:GeneratingUnit ;
  rdfs:range cim:GeneratorControlSource .

cim:GeneratingUnit.governorSCD a rdf:Property ;
  rdfs:label "governorSCD"@en ;
  rdfs:comment "Governor Speed Changer Droop.   This is the change in generator power output divided by the change in frequency normalized by the nominal power of the generator and the nominal frequency and expressed in percent and negated. A positive value of speed change droop provides additional generator output upon a drop in frequency." ;
  cims:dataType cim:PerCent ;
  cims:multiplicity cims:M:0..1 ;
  cims:stereotype <http://iec.ch/TC57/NonStandard/UML#attribute> ;
  rdfs:domain cim:GeneratingUnit .

cim:GeneratingUnit.longPF a rdf:Property ;
  rdfs:label "longPF"@en ;
  rdfs:comment "Generating unit long term economic participation factor." ;
  cims:dataType cim:Float ;
  cims:multiplicity cims:M:0..1 ;
  cims:stereotype <http://iec.ch/TC57/NonStandard/UML#attribute> ;
  rdfs:domain cim:GeneratingUnit .

cim:GeneratingUnit.maxOperatingP a rdf:Property ;
  rdfs:label "maxOperatingP"@en ;
  rdfs:comment "This is the maximum operating active power limit the dispatcher can enter for this unit." ;
  cims:dataType cim:ActivePower ;
  cims:multiplicity cims:M:1..1 ;
  cims:stereotype <http://iec.ch/TC57/NonStandard/UML#attribute> ;
  rdfs:domain cim:GeneratingUnit .

cim:GeneratingUnit.maximumAllowableSpinningReserve a rdf:Property ;
  rdfs:label "maximumAllowableSpinningReserve"@en ;
  rdfs:comment "Maximum allowable spinning reserve. Spinning reserve will never be considered greater than this value regardless of the current operating point." ;
  cims:dataType cim:ActivePower ;
  cims:multiplicity cims:M:0..1 ;
  cims:stereotype <http://iec.ch/TC57/NonStandard/UML#attribute> ;
  rdfs:domain cim:GeneratingUnit .

cim:GeneratingUnit.minOperatingP a rdf:Property ;
  rdfs:label "minOperatingP"@en ;
  rdfs:comment "This is the minimum operating active power limit the dispatcher can enter for this unit." ;
  cims:dataType cim:ActivePower ;
  cims:multiplicity cims:M:1..1 ;
  cims:stereotype <http://iec.ch/TC57/NonStandard/UML#attribute> ;
  rdfs:domain cim:GeneratingUnit .

cim:GeneratingUnit.nominalP a rdf:Property ;
  rdfs:label "nominalP"@en ;
  rdfs:comment """The nominal power of the generating unit.  Used to give precise meaning to percentage based attributes such as the governor speed change droop (governorSCD attribute).
The attribute shall be a positive value equal to or less than RotatingMachine.ratedS.""" ;
  cims:dataType cim:ActivePower ;
  cims:multiplicity cims:M:0..1 ;
  cims:stereotype <http://iec.ch/TC57/NonStandard/UML#attribute> ;
  rdfs:domain cim:GeneratingUnit .

cim:GeneratingUnit.ratedGrossMaxP a rdf:Property ;
  rdfs:label "ratedGrossMaxP"@en ;
  rdfs:comment """The unit's gross rated maximum capacity (book value).
The attribute shall be a positive value.""" ;
  cims:dataType cim:ActivePower ;
  cims:multiplicity cims:M:0..1 ;
  cims:stereotype <http://iec.ch/TC57/NonStandard/UML#attribute> ;
  rdfs:domain cim:GeneratingUnit .

cim:GeneratingUnit.ratedGrossMinP a rdf:Property ;
  rdfs:label "ratedGrossMinP"@en ;
  rdfs:comment """The gross rated minimum generation level which the unit can safely operate at while delivering power to the transmission grid.
The attribute shall be a positive value.""" ;
  cims:dataType cim:ActivePower ;
  cims:multiplicity cims:M:0..1 ;
  cims:stereotype <http://iec.ch/TC57/NonStandard/UML#attribute> ;
  rdfs:domain cim:GeneratingUnit .

cim:GeneratingUnit.ratedNetMaxP a rdf:Property ;
  rdfs:label "ratedNetMaxP"@en ;
  rdfs:comment """The net rated maximum capacity determined by subtracting the auxiliary power used to operate the internal plant machinery from the rated gross maximum capacity.
The attribute shall be a positive value.""" ;
  cims:dataType cim:ActivePower ;
  cims:multiplicity cims:M:0..1 ;
  cims:stereotype <http://iec.ch/TC57/NonStandard/UML#attribute> ;
  rdfs:domain cim:GeneratingUnit .

cim:GeneratingUnit.shortPF a rdf:Property ;
  rdfs:label "shortPF"@en ;
  rdfs:comment "Generating unit short term economic participation factor." ;
  cims:dataType cim:Float ;
  cims:multiplicity cims:M:0..1 ;
  cims:stereotype <http://iec.ch/TC57/NonStandard/UML#attribute> ;
  rdfs:domain cim:GeneratingUnit .

cim:GeneratingUnit.startupCost a rdf:Property ;
  rdfs:label "startupCost"@en ;
  rdfs:comment "The initial startup cost incurred for each start of the GeneratingUnit." ;
  cims:dataType cim:Money ;
  cims:multiplicity cims:M:0..1 ;
  cims:stereotype <http://iec.ch/TC57/NonStandard/UML#attribute> ;
  rdfs:domain cim:GeneratingUnit .

cim:GeneratingUnit.startupTime a rdf:Property ;
  rdfs:label "startupTime"@en ;
  rdfs:comment "Time it takes to get the unit on-line, from the time that the prime mover mechanical power is applied." ;
  cims:dataType cim:Seconds ;
  cims:multiplicity cims:M:0..1 ;
  cims:stereotype <http://iec.ch/TC57/NonStandard/UML#attribute> ;
  rdfs:domain cim:GeneratingUnit .

cim:GeneratingUnit.totalEfficiency a rdf:Property ;
  rdfs:label "totalEfficiency"@en ;
  rdfs:comment "The efficiency of the unit in converting the fuel into electrical energy." ;
  cims:dataType cim:PerCent ;
  cims:multiplicity cims:M:0..1 ;
  cims:stereotype <http://iec.ch/TC57/NonStandard/UML#attribute> ;
  rdfs:domain cim:GeneratingUnit .

cim:GeneratingUnit.variableCost a rdf:Property ;
  rdfs:label "variableCost"@en ;
  rdfs:comment "The variable cost component of production per unit of ActivePower." ;
  cims:dataType cim:Money ;
  cims:multiplicity cims:M:0..1 ;
  cims:stereotype <http://iec.ch/TC57/NonStandard/UML#attribute> ;
  rdfs:domain cim:GeneratingUnit .

cim:GeographicalRegion.Regions a rdf:Property ;
  rdfs:label "Regions"@en ;
  rdfs:comment "All sub-geographical regions within this geographical region." ;
  cims:AssociationUsed "No" ;
  cims:inverseRoleName cim:SubGeographicalRegion.Region ;
  cims:multiplicity cims:M:0..n ;
  rdfs:domain cim:GeographicalRegion ;
  rdfs:range cim:SubGeographicalRegion .

cim:GrossToNetActivePowerCurve.GeneratingUnit a rdf:Property ;
  rdfs:label "GeneratingUnit"@en ;
  rdfs:comment "A generating unit may have a gross active power to net active power curve, describing the losses and auxiliary power requirements of the unit." ;
  cims:AssociationUsed "Yes" ;
  cims:inverseRoleName cim:GeneratingUnit.GrossToNetActivePowerCurves ;
  cims:multiplicity cims:M:1 ;
  rdfs:domain cim:GrossToNetActivePowerCurve ;
  rdfs:range cim:GeneratingUnit .

cim:HydroGeneratingUnit.HydroPowerPlant a rdf:Property ;
  rdfs:label "HydroPowerPlant"@en ;
  rdfs:comment "The hydro generating unit belongs to a hydro power plant." ;
  cims:AssociationUsed "Yes" ;
  cims:inverseRoleName cim:HydroPowerPlant.HydroGeneratingUnits ;
  cims:multiplicity cims:M:0..1 ;
  rdfs:domain cim:HydroGeneratingUnit ;
  rdfs:range cim:HydroPowerPlant .

cim:HydroGeneratingUnit.dropHeight a rdf:Property ;
  rdfs:label "dropHeight"@en ;
  rdfs:comment "The height water drops from the reservoir mid-point to the turbine." ;
  cims:dataType cim:Length ;
  cims:multiplicity cims:M:0..1 ;
  cims:stereotype <http://iec.ch/TC57/NonStandard/UML#attribute> ;
  rdfs:domain cim:HydroGeneratingUnit .

cim:HydroGeneratingUnit.energyConversionCapability a rdf:Property ;
  rdfs:label "energyConversionCapability"@en ;
  rdfs:comment "Energy conversion capability for generating." ;
  cims:multiplicity cims:M:0..1 ;
  cims:stereotype <http://iec.ch/TC57/NonStandard/UML#attribute> ;
  rdfs:domain cim:HydroGeneratingUnit ;
  rdfs:range cim:HydroEnergyConversionKind .

cim:HydroGeneratingUnit.turbineType a rdf:Property ;
  rdfs:label "turbineType"@en ;
  rdfs:comment "Type of turbine." ;
  cims:multiplicity cims:M:0..1 ;
  cims:stereotype <http://iec.ch/TC57/NonStandard/UML#attribute> ;
  rdfs:domain cim:HydroGeneratingUnit ;
  rdfs:range cim:HydroTurbineKind .

cim:HydroPowerPlant.HydroGeneratingUnits a rdf:Property ;
  rdfs:label "HydroGeneratingUnits"@en ;
  rdfs:comment "The hydro generating unit belongs to a hydro power plant." ;
  cims:AssociationUsed "No" ;
  cims:inverseRoleName cim:HydroGeneratingUnit.HydroPowerPlant ;
  cims:multiplicity cims:M:0..n ;
  rdfs:domain cim:HydroPowerPlant ;
  rdfs:range cim:HydroGeneratingUnit .

cim:HydroPowerPlant.HydroPumps a rdf:Property ;
  rdfs:label "HydroPumps"@en ;
  rdfs:comment "The hydro pump may be a member of a pumped storage plant or a pump for distributing water." ;
  cims:AssociationUsed "No" ;
  cims:inverseRoleName cim:HydroPump.HydroPowerPlant ;
  cims:multiplicity cims:M:0..n ;
  rdfs:domain cim:HydroPowerPlant ;
  rdfs:range cim:HydroPump .

cim:HydroPowerPlant.hydroPlantStorageType a rdf:Property ;
  rdfs:label "hydroPlantStorageType"@en ;
  rdfs:comment "The type of hydro power plant water storage." ;
  cims:multiplicity cims:M:1..1 ;
  cims:stereotype <http://iec.ch/TC57/NonStandard/UML#attribute> ;
  rdfs:domain cim:HydroPowerPlant ;
  rdfs:range cim:HydroPlantStorageKind .

cim:HydroPump.HydroPowerPlant a rdf:Property ;
  rdfs:label "HydroPowerPlant"@en ;
  rdfs:comment "The hydro pump may be a member of a pumped storage plant or a pump for distributing water." ;
  cims:AssociationUsed "Yes" ;
  cims:inverseRoleName cim:HydroPowerPlant.HydroPumps ;
  cims:multiplicity cims:M:0..1 ;
  rdfs:domain cim:HydroPump ;
  rdfs:range cim:HydroPowerPlant .

cim:HydroPump.RotatingMachine a rdf:Property ;
  rdfs:label "RotatingMachine"@en ;
  rdfs:comment "The synchronous machine drives the turbine which moves the water from a low elevation to a higher elevation. The direction of machine rotation for pumping may or may not be the same as for generating." ;
  cims:AssociationUsed "Yes" ;
  cims:inverseRoleName cim:RotatingMachine.HydroPump ;
  cims:multiplicity cims:M:1 ;
  rdfs:domain cim:HydroPump ;
  rdfs:range cim:RotatingMachine .

cim:IdentifiedObject.description a rdf:Property ;
  rdfs:label "description"@en ;
  rdfs:comment "The description is a free human readable text describing or naming the object. It may be non unique and may not correlate to a naming hierarchy." ;
  cims:dataType cim:String ;
  cims:multiplicity cims:M:0..1 ;
  cims:stereotype <http://iec.ch/TC57/NonStandard/UML#attribute> ;
  rdfs:domain cim:IdentifiedObject .

cim:IdentifiedObject.mRID a rdf:Property ;
  rdfs:label "mRID"@en ;
  rdfs:comment """Master resource identifier issued by a model authority. The mRID is unique within an exchange context. Global uniqueness is easily achieved by using a UUID, as specified in RFC 4122, for the mRID. The use of UUID is strongly recommended.
For CIMXML data files in RDF syntax conforming to IEC 61970-552, the mRID is mapped to rdf:ID or rdf:about attributes that identify CIM object elements.""" ;
  cims:dataType cim:String ;
  cims:multiplicity cims:M:1..1 ;
  cims:stereotype <http://iec.ch/TC57/NonStandard/UML#attribute> ;
  rdfs:domain cim:IdentifiedObject .

cim:IdentifiedObject.name a rdf:Property ;
  rdfs:label "name"@en ;
  rdfs:comment "The name is any free human readable and possibly non unique text naming the object." ;
  cims:dataType cim:String ;
  cims:multiplicity cims:M:1..1 ;
  cims:stereotype <http://iec.ch/TC57/NonStandard/UML#attribute> ;
  rdfs:domain cim:IdentifiedObject .

cim:Inductance.multiplier a rdf:Property ;
  rdfs:label "multiplier"@en ;
  cims:isFixed "none" ;
  cims:multiplicity cims:M:0..1 ;
  cims:stereotype <http://iec.ch/TC57/NonStandard/UML#attribute> ;
  rdfs:domain cim:Inductance ;
  rdfs:range cim:UnitMultiplier .

cim:Inductance.unit a rdf:Property ;
  rdfs:label "unit"@en ;
  cims:isFixed "H" ;
  cims:multiplicity cims:M:0..1 ;
  cims:stereotype <http://iec.ch/TC57/NonStandard/UML#attribute> ;
  rdfs:domain cim:Inductance ;
  rdfs:range cim:UnitSymbol .

cim:Inductance.value a rdf:Property ;
  rdfs:label "value"@en ;
  cims:dataType cim:Float ;
  cims:multiplicity cims:M:0..1 ;
  cims:stereotype <http://iec.ch/TC57/NonStandard/UML#attribute> ;
  rdfs:domain cim:Inductance .

cim:Length.multiplier a rdf:Property ;
  rdfs:label "multiplier"@en ;
  cims:isFixed "k" ;
  cims:multiplicity cims:M:0..1 ;
  cims:stereotype <http://iec.ch/TC57/NonStandard/UML#attribute> ;
  rdfs:domain cim:Length ;
  rdfs:range cim:UnitMultiplier .

cim:Length.unit a rdf:Property ;
  rdfs:label "unit"@en ;
  cims:isFixed "m" ;
  cims:multiplicity cims:M:0..1 ;
  cims:stereotype <http://iec.ch/TC57/NonStandard/UML#attribute> ;
  rdfs:domain cim:Length ;
  rdfs:range cim:UnitSymbol .

cim:Length.value a rdf:Property ;
  rdfs:label "value"@en ;
  cims:dataType cim:Float ;
  cims:multiplicity cims:M:0..1 ;
  cims:stereotype <http://iec.ch/TC57/NonStandard/UML#attribute> ;
  rdfs:domain cim:Length .

cim:Line.Region a rdf:Property ;
  rdfs:label "Region"@en ;
  rdfs:comment "The sub-geographical region of the line." ;
  cims:AssociationUsed "Yes" ;
  cims:inverseRoleName cim:SubGeographicalRegion.Lines ;
  cims:multiplicity cims:M:0..1 ;
  rdfs:domain cim:Line ;
  rdfs:range cim:SubGeographicalRegion .

cim:LinearShuntCompensator.bPerSection a rdf:Property ;
  rdfs:label "bPerSection"@en ;
  rdfs:comment "Positive sequence shunt (charging) susceptance per section." ;
  cims:dataType cim:Susceptance ;
  cims:multiplicity cims:M:1..1 ;
  cims:stereotype <http://iec.ch/TC57/NonStandard/UML#attribute> ;
  rdfs:domain cim:LinearShuntCompensator .

cim:LinearShuntCompensator.gPerSection a rdf:Property ;
  rdfs:label "gPerSection"@en ;
  rdfs:comment "Positive sequence shunt (charging) conductance per section." ;
  cims:dataType cim:Conductance ;
  cims:multiplicity cims:M:1..1 ;
  cims:stereotype <http://iec.ch/TC57/NonStandard/UML#attribute> ;
  rdfs:domain cim:LinearShuntCompensator .

cim:LoadArea.SubLoadAreas a rdf:Property ;
  rdfs:label "SubLoadAreas"@en ;
  rdfs:comment "The SubLoadAreas in the LoadArea." ;
  cims:AssociationUsed "No" ;
  cims:inverseRoleName cim:SubLoadArea.LoadArea ;
  cims:multiplicity cims:M:1..n ;
  rdfs:domain cim:LoadArea ;
  rdfs:range cim:SubLoadArea .

cim:LoadGroup.SubLoadArea a rdf:Property ;
  rdfs:label "SubLoadArea"@en ;
  rdfs:comment "The SubLoadArea where the Loadgroup belongs." ;
  cims:AssociationUsed "Yes" ;
  cims:inverseRoleName cim:SubLoadArea.LoadGroups ;
  cims:multiplicity cims:M:1 ;
  rdfs:domain cim:LoadGroup ;
  rdfs:range cim:SubLoadArea .

cim:LoadResponseCharacteristic.EnergyConsumer a rdf:Property ;
  rdfs:label "EnergyConsumer"@en ;
  rdfs:comment "The set of loads that have the response characteristics." ;
  cims:AssociationUsed "No" ;
  cims:inverseRoleName cim:EnergyConsumer.LoadResponse ;
  cims:multiplicity cims:M:0..n ;
  rdfs:domain cim:LoadResponseCharacteristic ;
  rdfs:range cim:EnergyConsumer .

cim:LoadResponseCharacteristic.exponentModel a rdf:Property ;
  rdfs:label "exponentModel"@en ;
  rdfs:comment """Indicates the exponential voltage dependency model is to be used. If false, the coefficient model is to be used.
The exponential voltage dependency model consist of the attributes:
- pVoltageExponent
- qVoltageExponent
- pFrequencyExponent
- qFrequencyExponent.
The coefficient model consist of the attributes:
- pConstantImpedance
- pConstantCurrent
- pConstantPower
- qConstantImpedance
- qConstantCurrent
- qConstantPower.
The sum of pConstantImpedance, pConstantCurrent and pConstantPower shall equal 1.
The sum of qConstantImpedance, qConstantCurrent and qConstantPower shall equal 1.""" ;
  cims:dataType cim:Boolean ;
  cims:multiplicity cims:M:1..1 ;
  cims:stereotype <http://iec.ch/TC57/NonStandard/UML#attribute> ;
  rdfs:domain cim:LoadResponseCharacteristic .

cim:LoadResponseCharacteristic.pConstantCurrent a rdf:Property ;
  rdfs:label "pConstantCurrent"@en ;
  rdfs:comment "Portion of active power load modelled as constant current." ;
  cims:dataType cim:Float ;
  cims:multiplicity cims:M:0..1 ;
  cims:stereotype <http://iec.ch/TC57/NonStandard/UML#attribute> ;
  rdfs:domain cim:LoadResponseCharacteristic .

cim:LoadResponseCharacteristic.pConstantImpedance a rdf:Property ;
  rdfs:label "pConstantImpedance"@en ;
  rdfs:comment "Portion of active power load modelled as constant impedance." ;
  cims:dataType cim:Float ;
  cims:multiplicity cims:M:0..1 ;
  cims:stereotype <http://iec.ch/TC57/NonStandard/UML#attribute> ;
  rdfs:domain cim:LoadResponseCharacteristic .

cim:LoadResponseCharacteristic.pConstantPower a rdf:Property ;
  rdfs:label "pConstantPower"@en ;
  rdfs:comment "Portion of active power load modelled as constant power." ;
  cims:dataType cim:Float ;
  cims:multiplicity cims:M:0..1 ;
  cims:stereotype <http://iec.ch/TC57/NonStandard/UML#attribute> ;
  rdfs:domain cim:LoadResponseCharacteristic .

cim:LoadResponseCharacteristic.pFrequencyExponent a rdf:Property ;
  rdfs:label "pFrequencyExponent"@en ;
  rdfs:comment "Exponent of per unit frequency effecting active power." ;
  cims:dataType cim:Float ;
  cims:multiplicity cims:M:0..1 ;
  cims:stereotype <http://iec.ch/TC57/NonStandard/UML#attribute> ;
  rdfs:domain cim:LoadResponseCharacteristic .

cim:LoadResponseCharacteristic.pVoltageExponent a rdf:Property ;
  rdfs:label "pVoltageExponent"@en ;
  rdfs:comment "Exponent of per unit voltage effecting real power." ;
  cims:dataType cim:Float ;
  cims:multiplicity cims:M:0..1 ;
  cims:stereotype <http://iec.ch/TC57/NonStandard/UML#attribute> ;
  rdfs:domain cim:LoadResponseCharacteristic .

cim:LoadResponseCharacteristic.qConstantCurrent a rdf:Property ;
  rdfs:label "qConstantCurrent"@en ;
  rdfs:comment "Portion of reactive power load modelled as constant current." ;
  cims:dataType cim:Float ;
  cims:multiplicity cims:M:0..1 ;
  cims:stereotype <http://iec.ch/TC57/NonStandard/UML#attribute> ;
  rdfs:domain cim:LoadResponseCharacteristic .

cim:LoadResponseCharacteristic.qConstantImpedance a rdf:Property ;
  rdfs:label "qConstantImpedance"@en ;
  rdfs:comment "Portion of reactive power load modelled as constant impedance." ;
  cims:dataType cim:Float ;
  cims:multiplicity cims:M:0..1 ;
  cims:stereotype <http://iec.ch/TC57/NonStandard/UML#attribute> ;
  rdfs:domain cim:LoadResponseCharacteristic .

cim:LoadResponseCharacteristic.qConstantPower a rdf:Property ;
  rdfs:label "qConstantPower"@en ;
  rdfs:comment "Portion of reactive power load modelled as constant power." ;
  cims:dataType cim:Float ;
  cims:multiplicity cims:M:0..1 ;
  cims:stereotype <http://iec.ch/TC57/NonStandard/UML#attribute> ;
  rdfs:domain cim:LoadResponseCharacteristic .

cim:LoadResponseCharacteristic.qFrequencyExponent a rdf:Property ;
  rdfs:label "qFrequencyExponent"@en ;
  rdfs:comment "Exponent of per unit frequency effecting reactive power." ;
  cims:dataType cim:Float ;
  cims:multiplicity cims:M:0..1 ;
  cims:stereotype <http://iec.ch/TC57/NonStandard/UML#attribute> ;
  rdfs:domain cim:LoadResponseCharacteristic .

cim:LoadResponseCharacteristic.qVoltageExponent a rdf:Property ;
  rdfs:label "qVoltageExponent"@en ;
  rdfs:comment "Exponent of per unit voltage effecting reactive power." ;
  cims:dataType cim:Float ;
  cims:multiplicity cims:M:0..1 ;
  cims:stereotype <http://iec.ch/TC57/NonStandard/UML#attribute> ;
  rdfs:domain cim:LoadResponseCharacteristic .

cim:Money.multiplier a rdf:Property ;
  rdfs:label "multiplier"@en ;
  cims:isFixed "none" ;
  cims:multiplicity cims:M:0..1 ;
  cims:stereotype <http://iec.ch/TC57/NonStandard/UML#attribute> ;
  rdfs:domain cim:Money ;
  rdfs:range cim:UnitMultiplier .

cim:Money.unit a rdf:Property ;
  rdfs:label "unit"@en ;
  cims:multiplicity cims:M:0..1 ;
  cims:stereotype <http://iec.ch/TC57/NonStandard/UML#attribute> ;
  rdfs:domain cim:Money ;
  rdfs:range cim:Currency .

cim:Money.value a rdf:Property ;
  rdfs:label "value"@en ;
  cims:dataType cim:Decimal ;
  cims:multiplicity cims:M:0..1 ;
  cims:stereotype <http://iec.ch/TC57/NonStandard/UML#attribute> ;
  rdfs:domain cim:Money .

cim:NonConformLoad.LoadGroup a rdf:Property ;
  rdfs:label "LoadGroup"@en ;
  rdfs:comment "Group of this ConformLoad." ;
  cims:AssociationUsed "Yes" ;
  cims:inverseRoleName cim:NonConformLoadGroup.EnergyConsumers ;
  cims:multiplicity cims:M:1 ;
  rdfs:domain cim:NonConformLoad ;
  rdfs:range cim:NonConformLoadGroup .

cim:NonConformLoadGroup.EnergyConsumers a rdf:Property ;
  rdfs:label "EnergyConsumers"@en ;
  rdfs:comment "Conform loads assigned to this ConformLoadGroup." ;
  cims:AssociationUsed "No" ;
  cims:inverseRoleName cim:NonConformLoad.LoadGroup ;
  cims:multiplicity cims:M:1..n ;
  rdfs:domain cim:NonConformLoadGroup ;
  rdfs:range cim:NonConformLoad .

cim:NonConformLoadGroup.NonConformLoadSchedules a rdf:Property ;
  rdfs:label "NonConformLoadSchedules"@en ;
  rdfs:comment "The NonConformLoadSchedules in the NonConformLoadGroup." ;
  cims:AssociationUsed "No" ;
  cims:inverseRoleName cim:NonConformLoadSchedule.NonConformLoadGroup ;
  cims:multiplicity cims:M:0..n ;
  rdfs:domain cim:NonConformLoadGroup ;
  rdfs:range cim:NonConformLoadSchedule .

cim:NonConformLoadSchedule.NonConformLoadGroup a rdf:Property ;
  rdfs:label "NonConformLoadGroup"@en ;
  rdfs:comment "The NonConformLoadGroup where the NonConformLoadSchedule belongs." ;
  cims:AssociationUsed "Yes" ;
  cims:inverseRoleName cim:NonConformLoadGroup.NonConformLoadSchedules ;
  cims:multiplicity cims:M:1 ;
  rdfs:domain cim:NonConformLoadSchedule ;
  rdfs:range cim:NonConformLoadGroup .

cim:NonlinearShuntCompensator.NonlinearShuntCompensatorPoints a rdf:Property ;
  rdfs:label "NonlinearShuntCompensatorPoints"@en ;
  rdfs:comment "All points of the non-linear shunt compensator." ;
  cims:AssociationUsed "No" ;
  cims:inverseRoleName cim:NonlinearShuntCompensatorPoint.NonlinearShuntCompensator ;
  cims:multiplicity cims:M:1..n ;
  rdfs:domain cim:NonlinearShuntCompensator ;
  rdfs:range cim:NonlinearShuntCompensatorPoint .

cim:NonlinearShuntCompensatorPoint.NonlinearShuntCompensator a rdf:Property ;
  rdfs:label "NonlinearShuntCompensator"@en ;
  rdfs:comment "Non-linear shunt compensator owning this point." ;
  cims:AssociationUsed "Yes" ;
  cims:inverseRoleName cim:NonlinearShuntCompensator.NonlinearShuntCompensatorPoints ;
  cims:multiplicity cims:M:1 ;
  rdfs:domain cim:NonlinearShuntCompensatorPoint ;
  rdfs:range cim:NonlinearShuntCompensator .

cim:NonlinearShuntCompensatorPoint.b a rdf:Property ;
  rdfs:label "b"@en ;
  rdfs:comment "Positive sequence shunt (charging) susceptance per section." ;
  cims:dataType cim:Susceptance ;
  cims:multiplicity cims:M:1..1 ;
  cims:stereotype <http://iec.ch/TC57/NonStandard/UML#attribute> ;
  rdfs:domain cim:NonlinearShuntCompensatorPoint .

cim:NonlinearShuntCompensatorPoint.g a rdf:Property ;
  rdfs:label "g"@en ;
  rdfs:comment "Positive sequence shunt (charging) conductance per section." ;
  cims:dataType cim:Conductance ;
  cims:multiplicity cims:M:1..1 ;
  cims:stereotype <http://iec.ch/TC57/NonStandard/UML#attribute> ;
  rdfs:domain cim:NonlinearShuntCompensatorPoint .

cim:NonlinearShuntCompensatorPoint.sectionNumber a rdf:Property ;
  rdfs:label "sectionNumber"@en ;
  rdfs:comment "The number of the section." ;
  cims:dataType cim:Integer ;
  cims:multiplicity cims:M:1..1 ;
  cims:stereotype <http://iec.ch/TC57/NonStandard/UML#attribute> ;
  rdfs:domain cim:NonlinearShuntCompensatorPoint .

cim:OperationalLimit.OperationalLimitSet a rdf:Property ;
  rdfs:label "OperationalLimitSet"@en ;
  rdfs:comment "The limit set to which the limit values belong." ;
  cims:AssociationUsed "Yes" ;
  cims:inverseRoleName cim:OperationalLimitSet.OperationalLimitValue ;
  cims:multiplicity cims:M:1 ;
  rdfs:domain cim:OperationalLimit ;
  rdfs:range cim:OperationalLimitSet .

cim:OperationalLimit.OperationalLimitType a rdf:Property ;
  rdfs:label "OperationalLimitType"@en ;
  rdfs:comment "The limit type associated with this limit." ;
  cims:AssociationUsed "Yes" ;
  cims:inverseRoleName cim:OperationalLimitType.OperationalLimit ;
  cims:multiplicity cims:M:1..1 ;
  rdfs:domain cim:OperationalLimit ;
  rdfs:range cim:OperationalLimitType .

cim:OperationalLimitSet.Equipment a rdf:Property ;
  rdfs:label "Equipment"@en ;
  rdfs:comment "The equipment to which the limit set applies." ;
  cims:AssociationUsed "Yes" ;
  cims:inverseRoleName cim:Equipment.OperationalLimitSet ;
  cims:multiplicity cims:M:0..1 ;
  rdfs:domain cim:OperationalLimitSet ;
  rdfs:range cim:Equipment .

cim:OperationalLimitSet.OperationalLimitValue a rdf:Property ;
  rdfs:label "OperationalLimitValue"@en ;
  rdfs:comment "Values of equipment limits." ;
  cims:AssociationUsed "No" ;
  cims:inverseRoleName cim:OperationalLimit.OperationalLimitSet ;
  cims:multiplicity cims:M:0..n ;
  rdfs:domain cim:OperationalLimitSet ;
  rdfs:range cim:OperationalLimit .

cim:OperationalLimitSet.Terminal a rdf:Property ;
  rdfs:label "Terminal"@en ;
  rdfs:comment "The terminal where the operational limit set apply." ;
  cims:AssociationUsed "Yes" ;
  cims:inverseRoleName cim:ACDCTerminal.OperationalLimitSet ;
  cims:multiplicity cims:M:1 ;
  rdfs:domain cim:OperationalLimitSet ;
  rdfs:range cim:ACDCTerminal .

cim:OperationalLimitType.OperationalLimit a rdf:Property ;
  rdfs:label "OperationalLimit"@en ;
  rdfs:comment "The operational limits associated with this type of limit." ;
  cims:AssociationUsed "No" ;
  cims:inverseRoleName cim:OperationalLimit.OperationalLimitType ;
  cims:multiplicity cims:M:0..n ;
  rdfs:domain cim:OperationalLimitType ;
  rdfs:range cim:OperationalLimit .

cim:OperationalLimitType.acceptableDuration a rdf:Property ;
  rdfs:label "acceptableDuration"@en ;
  rdfs:comment "The nominal acceptable duration of the limit. Limits are commonly expressed in terms of the time limit for which the limit is normally acceptable. The actual acceptable duration of a specific limit may depend on other local factors such as temperature or wind speed. The attribute has meaning only if the flag isInfiniteDuration is set to false, hence it shall not be exchanged when isInfiniteDuration is set to true." ;
  cims:dataType cim:Seconds ;
  cims:multiplicity cims:M:0..1 ;
  cims:stereotype <http://iec.ch/TC57/NonStandard/UML#attribute> ;
  rdfs:domain cim:OperationalLimitType .

cim:OperationalLimitType.direction a rdf:Property ;
  rdfs:label "direction"@en ;
  rdfs:comment "The direction of the limit." ;
  cims:multiplicity cims:M:1..1 ;
  cims:stereotype <http://iec.ch/TC57/NonStandard/UML#attribute> ;
  rdfs:domain cim:OperationalLimitType ;
  rdfs:range cim:OperationalLimitDirectionKind .

cim:OperationalLimitType.isInfiniteDuration a rdf:Property ;
  rdfs:label "isInfiniteDuration"@en ;
  rdfs:comment "Defines if the operational limit type has infinite duration. If true, the limit has infinite duration. If false, the limit has definite duration which is defined by the attribute acceptableDuration." ;
  cims:dataType cim:Boolean ;
  cims:multiplicity cims:M:1..1 ;
  cims:stereotype <http://iec.ch/TC57/NonStandard/UML#attribute> ;
  rdfs:domain cim:OperationalLimitType .

cim:PerCent.multiplier a rdf:Property ;
  rdfs:label "multiplier"@en ;
  cims:isFixed "none" ;
  cims:multiplicity cims:M:0..1 ;
  cims:stereotype <http://iec.ch/TC57/NonStandard/UML#attribute> ;
  rdfs:domain cim:PerCent ;
  rdfs:range cim:UnitMultiplier .

cim:PerCent.unit a rdf:Property ;
  rdfs:label "unit"@en ;
  cims:isFixed "none" ;
  cims:multiplicity cims:M:0..1 ;
  cims:stereotype <http://iec.ch/TC57/NonStandard/UML#attribute> ;
  rdfs:domain cim:PerCent ;
  rdfs:range cim:UnitSymbol .

cim:PerCent.value a rdf:Property ;
  rdfs:label "value"@en ;
  rdfs:comment "Normally 0 to 100 on a defined base." ;
  cims:dataType cim:Float ;
  cims:multiplicity cims:M:0..1 ;
  cims:stereotype <http://iec.ch/TC57/NonStandard/UML#attribute> ;
  rdfs:domain cim:PerCent .

cim:PhaseTapChanger.TransformerEnd a rdf:Property ;
  rdfs:label "TransformerEnd"@en ;
  rdfs:comment "Transformer end to which this phase tap changer belongs." ;
  cims:AssociationUsed "Yes" ;
  cims:inverseRoleName cim:TransformerEnd.PhaseTapChanger ;
  cims:multiplicity cims:M:1 ;
  rdfs:domain cim:PhaseTapChanger ;
  rdfs:range cim:TransformerEnd .

cim:PhaseTapChangerAsymmetrical.windingConnectionAngle a rdf:Property ;
  rdfs:label "windingConnectionAngle"@en ;
  rdfs:comment "The phase angle between the in-phase winding and the out-of -phase winding used for creating phase shift. The out-of-phase winding produces what is known as the difference voltage.  Setting this angle to 90 degrees is not the same as a symmetrical transformer. The attribute can only be multiples of 30 degrees.  The allowed range is -150 degrees to 150 degrees excluding 0." ;
  cims:dataType cim:AngleDegrees ;
  cims:multiplicity cims:M:1..1 ;
  cims:stereotype <http://iec.ch/TC57/NonStandard/UML#attribute> ;
  rdfs:domain cim:PhaseTapChangerAsymmetrical .

cim:PhaseTapChangerLinear.stepPhaseShiftIncrement a rdf:Property ;
  rdfs:label "stepPhaseShiftIncrement"@en ;
  rdfs:comment """Phase shift per step position. A positive value indicates a positive angle variation from the Terminal at the  PowerTransformerEnd,  where the TapChanger is located, into the transformer.
The actual phase shift increment might be more accurately computed from the symmetrical or asymmetrical models or a tap step table lookup if those are available.""" ;
  cims:dataType cim:AngleDegrees ;
  cims:multiplicity cims:M:1..1 ;
  cims:stereotype <http://iec.ch/TC57/NonStandard/UML#attribute> ;
  rdfs:domain cim:PhaseTapChangerLinear .

cim:PhaseTapChangerLinear.xMax a rdf:Property ;
  rdfs:label "xMax"@en ;
  rdfs:comment "The reactance depends on the tap position according to a \"u\" shaped curve. The maximum reactance (xMax) appears at the low and high tap positions. Depending on the “u” curve the attribute can be either higher or lower than PowerTransformerEnd.x." ;
  cims:dataType cim:Reactance ;
  cims:multiplicity cims:M:1..1 ;
  cims:stereotype <http://iec.ch/TC57/NonStandard/UML#attribute> ;
  rdfs:domain cim:PhaseTapChangerLinear .

cim:PhaseTapChangerLinear.xMin a rdf:Property ;
  rdfs:label "xMin"@en ;
  rdfs:comment "The reactance depends on the tap position according to a \"u\" shaped curve. The minimum reactance (xMin) appears at the mid tap position.  PowerTransformerEnd.x shall be consistent with PhaseTapChangerLinear.xMin and PhaseTapChangerNonLinear.xMin. In case of inconsistency, PowerTransformerEnd.x shall be used." ;
  cims:dataType cim:Reactance ;
  cims:multiplicity cims:M:1..1 ;
  cims:stereotype "deprecated", <http://iec.ch/TC57/NonStandard/UML#attribute> ;
  rdfs:domain cim:PhaseTapChangerLinear .

cim:PhaseTapChangerNonLinear.voltageStepIncrement a rdf:Property ;
  rdfs:label "voltageStepIncrement"@en ;
  rdfs:comment """The voltage step increment on the out of phase winding (the PowerTransformerEnd where the TapChanger is located) specified in percent of rated voltage of the PowerTransformerEnd. A positive value means a positive voltage variation from the Terminal at the PowerTransformerEnd, where the TapChanger is located, into the transformer.
When the increment is negative, the voltage decreases when the tap step increases.""" ;
  cims:dataType cim:PerCent ;
  cims:multiplicity cims:M:1..1 ;
  cims:stereotype <http://iec.ch/TC57/NonStandard/UML#attribute> ;
  rdfs:domain cim:PhaseTapChangerNonLinear .

cim:PhaseTapChangerNonLinear.xMax a rdf:Property ;
  rdfs:label "xMax"@en ;
  rdfs:comment "The reactance depends on the tap position according to a \"u\" shaped curve. The maximum reactance (xMax) appears at the low and high tap positions. Depending on the “u” curve the attribute can be either higher or lower than PowerTransformerEnd.x." ;
  cims:dataType cim:Reactance ;
  cims:multiplicity cims:M:1..1 ;
  cims:stereotype <http://iec.ch/TC57/NonStandard/UML#attribute> ;
  rdfs:domain cim:PhaseTapChangerNonLinear .

cim:PhaseTapChangerNonLinear.xMin a rdf:Property ;
  rdfs:label "xMin"@en ;
  rdfs:comment "The reactance depend on the tap position according to a \"u\" shaped curve. The minimum reactance (xMin) appear at the mid tap position.   PowerTransformerEnd.x shall be consistent with PhaseTapChangerLinear.xMin and PhaseTapChangerNonLinear.xMin. In case of inconsistency, PowerTransformerEnd.x shall be used." ;
  cims:dataType cim:Reactance ;
  cims:multiplicity cims:M:1..1 ;
  cims:stereotype "deprecated", <http://iec.ch/TC57/NonStandard/UML#attribute> ;
  rdfs:domain cim:PhaseTapChangerNonLinear .

cim:PhaseTapChangerTable.PhaseTapChangerTablePoint a rdf:Property ;
  rdfs:label "PhaseTapChangerTablePoint"@en ;
  rdfs:comment "The points of this table." ;
  cims:AssociationUsed "No" ;
  cims:inverseRoleName cim:PhaseTapChangerTablePoint.PhaseTapChangerTable ;
  cims:multiplicity cims:M:1..n ;
  rdfs:domain cim:PhaseTapChangerTable ;
  rdfs:range cim:PhaseTapChangerTablePoint .

cim:PhaseTapChangerTable.PhaseTapChangerTabular a rdf:Property ;
  rdfs:label "PhaseTapChangerTabular"@en ;
  rdfs:comment "The phase tap changers to which this phase tap table applies." ;
  cims:AssociationUsed "No" ;
  cims:inverseRoleName cim:PhaseTapChangerTabular.PhaseTapChangerTable ;
  cims:multiplicity cims:M:0..n ;
  rdfs:domain cim:PhaseTapChangerTable ;
  rdfs:range cim:PhaseTapChangerTabular .

cim:PhaseTapChangerTablePoint.PhaseTapChangerTable a rdf:Property ;
  rdfs:label "PhaseTapChangerTable"@en ;
  rdfs:comment "The table of this point." ;
  cims:AssociationUsed "Yes" ;
  cims:inverseRoleName cim:PhaseTapChangerTable.PhaseTapChangerTablePoint ;
  cims:multiplicity cims:M:1 ;
  rdfs:domain cim:PhaseTapChangerTablePoint ;
  rdfs:range cim:PhaseTapChangerTable .

cim:PhaseTapChangerTablePoint.angle a rdf:Property ;
  rdfs:label "angle"@en ;
  rdfs:comment "The angle difference in degrees. A positive value indicates a positive angle variation from the Terminal at the  PowerTransformerEnd,  where the TapChanger is located, into the transformer." ;
  cims:dataType cim:AngleDegrees ;
  cims:multiplicity cims:M:1..1 ;
  cims:stereotype <http://iec.ch/TC57/NonStandard/UML#attribute> ;
  rdfs:domain cim:PhaseTapChangerTablePoint .

cim:PhaseTapChangerTabular.PhaseTapChangerTable a rdf:Property ;
  rdfs:label "PhaseTapChangerTable"@en ;
  rdfs:comment "The phase tap changer table for this phase tap changer." ;
  cims:AssociationUsed "Yes" ;
  cims:inverseRoleName cim:PhaseTapChangerTable.PhaseTapChangerTabular ;
  cims:multiplicity cims:M:1 ;
  rdfs:domain cim:PhaseTapChangerTabular ;
  rdfs:range cim:PhaseTapChangerTable .

cim:PowerElectronicsConnection.PowerElectronicsUnit a rdf:Property ;
  rdfs:label "PowerElectronicsUnit"@en ;
  rdfs:comment "An AC network connection may have several power electronics units connecting through it." ;
  cims:AssociationUsed "Yes" ;
  cims:inverseRoleName cim:PowerElectronicsUnit.PowerElectronicsConnection ;
  cims:multiplicity cims:M:0..1 ;
  rdfs:domain cim:PowerElectronicsConnection ;
  rdfs:range cim:PowerElectronicsUnit .

cim:PowerElectronicsConnection.maxQ a rdf:Property ;
  rdfs:label "maxQ"@en ;
  rdfs:comment "Maximum reactive power limit. This is the maximum (nameplate) limit for the unit." ;
  cims:dataType cim:ReactivePower ;
  cims:multiplicity cims:M:0..1 ;
  cims:stereotype <http://iec.ch/TC57/NonStandard/UML#attribute> ;
  rdfs:domain cim:PowerElectronicsConnection .

cim:PowerElectronicsConnection.minQ a rdf:Property ;
  rdfs:label "minQ"@en ;
  rdfs:comment "Minimum reactive power limit for the unit. This is the minimum (nameplate) limit for the unit." ;
  cims:dataType cim:ReactivePower ;
  cims:multiplicity cims:M:0..1 ;
  cims:stereotype <http://iec.ch/TC57/NonStandard/UML#attribute> ;
  rdfs:domain cim:PowerElectronicsConnection .

cim:PowerElectronicsConnection.ratedS a rdf:Property ;
  rdfs:label "ratedS"@en ;
  rdfs:comment """Nameplate apparent power rating for the unit.
The attribute shall have a positive value.""" ;
  cims:dataType cim:ApparentPower ;
  cims:multiplicity cims:M:0..1 ;
  cims:stereotype <http://iec.ch/TC57/NonStandard/UML#attribute> ;
  rdfs:domain cim:PowerElectronicsConnection .

cim:PowerElectronicsConnection.ratedU a rdf:Property ;
  rdfs:label "ratedU"@en ;
  rdfs:comment """Rated voltage (nameplate data, Ur in IEC 60909-0). It is primarily used for short circuit data exchange according to IEC 60909.
The attribute shall be a positive value.""" ;
  cims:dataType cim:Voltage ;
  cims:multiplicity cims:M:0..1 ;
  cims:stereotype <http://iec.ch/TC57/NonStandard/UML#attribute> ;
  rdfs:domain cim:PowerElectronicsConnection .

cim:PowerElectronicsUnit.PowerElectronicsConnection a rdf:Property ;
  rdfs:label "PowerElectronicsConnection"@en ;
  rdfs:comment "A power electronics unit has a connection to the AC network." ;
  cims:AssociationUsed "No" ;
  cims:inverseRoleName cim:PowerElectronicsConnection.PowerElectronicsUnit ;
  cims:multiplicity cims:M:1 ;
  rdfs:domain cim:PowerElectronicsUnit ;
  rdfs:range cim:PowerElectronicsConnection .

cim:PowerElectronicsUnit.maxP a rdf:Property ;
  rdfs:label "maxP"@en ;
  rdfs:comment "Maximum active power limit. This is the maximum (nameplate) limit for the unit." ;
  cims:dataType cim:ActivePower ;
  cims:multiplicity cims:M:0..1 ;
  cims:stereotype <http://iec.ch/TC57/NonStandard/UML#attribute> ;
  rdfs:domain cim:PowerElectronicsUnit .

cim:PowerElectronicsUnit.minP a rdf:Property ;
  rdfs:label "minP"@en ;
  rdfs:comment "Minimum active power limit. This is the minimum (nameplate) limit for the unit." ;
  cims:dataType cim:ActivePower ;
  cims:multiplicity cims:M:0..1 ;
  cims:stereotype <http://iec.ch/TC57/NonStandard/UML#attribute> ;
  rdfs:domain cim:PowerElectronicsUnit .

cim:PowerTransformer.PowerTransformerEnd a rdf:Property ;
  rdfs:label "PowerTransformerEnd"@en ;
  rdfs:comment "The ends of this power transformer." ;
  cims:AssociationUsed "No" ;
  cims:inverseRoleName cim:PowerTransformerEnd.PowerTransformer ;
  cims:multiplicity cims:M:0..n ;
  rdfs:domain cim:PowerTransformer ;
  rdfs:range cim:PowerTransformerEnd .

cim:PowerTransformerEnd.PowerTransformer a rdf:Property ;
  rdfs:label "PowerTransformer"@en ;
  rdfs:comment "The power transformer of this power transformer end." ;
  cims:AssociationUsed "Yes" ;
  cims:inverseRoleName cim:PowerTransformer.PowerTransformerEnd ;
  cims:multiplicity cims:M:1..1 ;
  rdfs:domain cim:PowerTransformerEnd ;
  rdfs:range cim:PowerTransformer .

cim:PowerTransformerEnd.b a rdf:Property ;
  rdfs:label "b"@en ;
  rdfs:comment "Magnetizing branch susceptance (B mag).  The value can be positive or negative." ;
  cims:dataType cim:Susceptance ;
  cims:multiplicity cims:M:1..1 ;
  cims:stereotype <http://iec.ch/TC57/NonStandard/UML#attribute> ;
  rdfs:domain cim:PowerTransformerEnd .

cim:PowerTransformerEnd.connectionKind a rdf:Property ;
  rdfs:label "connectionKind"@en ;
  rdfs:comment "Kind of connection." ;
  cims:multiplicity cims:M:0..1 ;
  cims:stereotype <http://iec.ch/TC57/NonStandard/UML#attribute> ;
  rdfs:domain cim:PowerTransformerEnd ;
  rdfs:range cim:WindingConnection .

cim:PowerTransformerEnd.g a rdf:Property ;
  rdfs:label "g"@en ;
  rdfs:comment "Magnetizing branch conductance." ;
  cims:dataType cim:Conductance ;
  cims:multiplicity cims:M:0..1 ;
  cims:stereotype <http://iec.ch/TC57/NonStandard/UML#attribute> ;
  rdfs:domain cim:PowerTransformerEnd .

cim:PowerTransformerEnd.r a rdf:Property ;
  rdfs:label "r"@en ;
  rdfs:comment """Resistance (star-model) of the transformer end.
The attribute shall be equal to or greater than zero for non-equivalent transformers.""" ;
  cims:dataType cim:Resistance ;
  cims:multiplicity cims:M:1..1 ;
  cims:stereotype <http://iec.ch/TC57/NonStandard/UML#attribute> ;
  rdfs:domain cim:PowerTransformerEnd .

cim:PowerTransformerEnd.ratedS a rdf:Property ;
  rdfs:label "ratedS"@en ;
  rdfs:comment """Normal apparent power rating.
The attribute shall be a positive value. For a two-winding transformer the values for the high and low voltage sides shall be identical. """ ;
  cims:dataType cim:ApparentPower ;
  cims:multiplicity cims:M:0..1 ;
  cims:stereotype <http://iec.ch/TC57/NonStandard/UML#attribute> ;
  rdfs:domain cim:PowerTransformerEnd .

cim:PowerTransformerEnd.ratedU a rdf:Property ;
  rdfs:label "ratedU"@en ;
  rdfs:comment """Rated voltage: phase-phase for three-phase windings, and either phase-phase or phase-neutral for single-phase windings.
A high voltage side, as given by TransformerEnd.endNumber, shall have a ratedU that is greater than or equal to ratedU for the lower voltage sides.
The attribute shall be a positive value.""" ;
  cims:dataType cim:Voltage ;
  cims:multiplicity cims:M:1..1 ;
  cims:stereotype <http://iec.ch/TC57/NonStandard/UML#attribute> ;
  rdfs:domain cim:PowerTransformerEnd .

cim:PowerTransformerEnd.x a rdf:Property ;
  rdfs:label "x"@en ;
  rdfs:comment "Positive sequence series reactance (star-model) of the transformer end." ;
  cims:dataType cim:Reactance ;
  cims:multiplicity cims:M:1..1 ;
  cims:stereotype <http://iec.ch/TC57/NonStandard/UML#attribute> ;
  rdfs:domain cim:PowerTransformerEnd .

cim:RatioTapChanger.RatioTapChangerTable a rdf:Property ;
  rdfs:label "RatioTapChangerTable"@en ;
  rdfs:comment "The tap ratio table for this ratio  tap changer." ;
  cims:AssociationUsed "Yes" ;
  cims:inverseRoleName cim:RatioTapChangerTable.RatioTapChanger ;
  cims:multiplicity cims:M:0..1 ;
  rdfs:domain cim:RatioTapChanger ;
  rdfs:range cim:RatioTapChangerTable .

cim:RatioTapChanger.TransformerEnd a rdf:Property ;
  rdfs:label "TransformerEnd"@en ;
  rdfs:comment "Transformer end to which this ratio tap changer belongs." ;
  cims:AssociationUsed "Yes" ;
  cims:inverseRoleName cim:TransformerEnd.RatioTapChanger ;
  cims:multiplicity cims:M:1 ;
  rdfs:domain cim:RatioTapChanger ;
  rdfs:range cim:TransformerEnd .

cim:RatioTapChanger.stepVoltageIncrement a rdf:Property ;
  rdfs:label "stepVoltageIncrement"@en ;
  rdfs:comment """Tap step increment, in per cent of rated voltage of the power transformer end, per step position.
When the increment is negative, the voltage decreases when the tap step increases.""" ;
  cims:dataType cim:PerCent ;
  cims:multiplicity cims:M:1..1 ;
  cims:stereotype <http://iec.ch/TC57/NonStandard/UML#attribute> ;
  rdfs:domain cim:RatioTapChanger .

cim:RatioTapChangerTable.RatioTapChanger a rdf:Property ;
  rdfs:label "RatioTapChanger"@en ;
  rdfs:comment "The ratio tap changer of this tap ratio table." ;
  cims:AssociationUsed "No" ;
  cims:inverseRoleName cim:RatioTapChanger.RatioTapChangerTable ;
  cims:multiplicity cims:M:0..n ;
  rdfs:domain cim:RatioTapChangerTable ;
  rdfs:range cim:RatioTapChanger .

cim:RatioTapChangerTable.RatioTapChangerTablePoint a rdf:Property ;
  rdfs:label "RatioTapChangerTablePoint"@en ;
  rdfs:comment "Points of this table." ;
  cims:AssociationUsed "No" ;
  cims:inverseRoleName cim:RatioTapChangerTablePoint.RatioTapChangerTable ;
  cims:multiplicity cims:M:1..n ;
  rdfs:domain cim:RatioTapChangerTable ;
  rdfs:range cim:RatioTapChangerTablePoint .

cim:RatioTapChangerTablePoint.RatioTapChangerTable a rdf:Property ;
  rdfs:label "RatioTapChangerTable"@en ;
  rdfs:comment "Table of this point." ;
  cims:AssociationUsed "Yes" ;
  cims:inverseRoleName cim:RatioTapChangerTable.RatioTapChangerTablePoint ;
  cims:multiplicity cims:M:1 ;
  rdfs:domain cim:RatioTapChangerTablePoint ;
  rdfs:range cim:RatioTapChangerTable .

cim:Reactance.multiplier a rdf:Property ;
  rdfs:label "multiplier"@en ;
  cims:isFixed "none" ;
  cims:multiplicity cims:M:0..1 ;
  cims:stereotype <http://iec.ch/TC57/NonStandard/UML#attribute> ;
  rdfs:domain cim:Reactance ;
  rdfs:range cim:UnitMultiplier .

cim:Reactance.unit a rdf:Property ;
  rdfs:label "unit"@en ;
  cims:isFixed "ohm" ;
  cims:multiplicity cims:M:0..1 ;
  cims:stereotype <http://iec.ch/TC57/NonStandard/UML#attribute> ;
  rdfs:domain cim:Reactance ;
  rdfs:range cim:UnitSymbol .

cim:Reactance.value a rdf:Property ;
  rdfs:label "value"@en ;
  cims:dataType cim:Float ;
  cims:multiplicity cims:M:0..1 ;
  cims:stereotype <http://iec.ch/TC57/NonStandard/UML#attribute> ;
  rdfs:domain cim:Reactance .

cim:ReactiveCapabilityCurve.EquivalentInjection a rdf:Property ;
  rdfs:label "EquivalentInjection"@en ;
  rdfs:comment "The equivalent injection using this reactive capability curve." ;
  cims:AssociationUsed "No" ;
  cims:inverseRoleName cim:EquivalentInjection.ReactiveCapabilityCurve ;
  cims:multiplicity cims:M:0..n ;
  rdfs:domain cim:ReactiveCapabilityCurve ;
  rdfs:range cim:EquivalentInjection .

cim:ReactiveCapabilityCurve.InitiallyUsedBySynchronousMachines a rdf:Property ;
  rdfs:label "InitiallyUsedBySynchronousMachines"@en ;
  rdfs:comment "Synchronous machines using this curve as default." ;
  cims:AssociationUsed "No" ;
  cims:inverseRoleName cim:SynchronousMachine.InitialReactiveCapabilityCurve ;
  cims:multiplicity cims:M:1..n ;
  rdfs:domain cim:ReactiveCapabilityCurve ;
  rdfs:range cim:SynchronousMachine .

cim:ReactivePower.multiplier a rdf:Property ;
  rdfs:label "multiplier"@en ;
  cims:isFixed "M" ;
  cims:multiplicity cims:M:0..1 ;
  cims:stereotype <http://iec.ch/TC57/NonStandard/UML#attribute> ;
  rdfs:domain cim:ReactivePower ;
  rdfs:range cim:UnitMultiplier .

cim:ReactivePower.unit a rdf:Property ;
  rdfs:label "unit"@en ;
  cims:isFixed "VAr" ;
  cims:multiplicity cims:M:0..1 ;
  cims:stereotype <http://iec.ch/TC57/NonStandard/UML#attribute> ;
  rdfs:domain cim:ReactivePower ;
  rdfs:range cim:UnitSymbol .

cim:ReactivePower.value a rdf:Property ;
  rdfs:label "value"@en ;
  cims:dataType cim:Float ;
  cims:multiplicity cims:M:0..1 ;
  cims:stereotype <http://iec.ch/TC57/NonStandard/UML#attribute> ;
  rdfs:domain cim:ReactivePower .

cim:RealEnergy.multiplier a rdf:Property ;
  rdfs:label "multiplier"@en ;
  cims:isFixed "M" ;
  cims:multiplicity cims:M:0..1 ;
  cims:stereotype <http://iec.ch/TC57/NonStandard/UML#attribute> ;
  rdfs:domain cim:RealEnergy ;
  rdfs:range cim:UnitMultiplier .

cim:RealEnergy.unit a rdf:Property ;
  rdfs:label "unit"@en ;
  cims:isFixed "Wh" ;
  cims:multiplicity cims:M:0..1 ;
  cims:stereotype <http://iec.ch/TC57/NonStandard/UML#attribute> ;
  rdfs:domain cim:RealEnergy ;
  rdfs:range cim:UnitSymbol .

cim:RealEnergy.value a rdf:Property ;
  rdfs:label "value"@en ;
  cims:dataType cim:Float ;
  cims:multiplicity cims:M:0..1 ;
  cims:stereotype <http://iec.ch/TC57/NonStandard/UML#attribute> ;
  rdfs:domain cim:RealEnergy .

cim:RegularIntervalSchedule.TimePoints a rdf:Property ;
  rdfs:label "TimePoints"@en ;
  rdfs:comment "The regular interval time point data values that define this schedule." ;
  cims:AssociationUsed "No" ;
  cims:inverseRoleName cim:RegularTimePoint.IntervalSchedule ;
  cims:multiplicity cims:M:1..n ;
  rdfs:domain cim:RegularIntervalSchedule ;
  rdfs:range cim:RegularTimePoint .

cim:RegularIntervalSchedule.endTime a rdf:Property ;
  rdfs:label "endTime"@en ;
  rdfs:comment "The time for the last time point.  The value can be a time of day, not a specific date." ;
  cims:dataType cim:DateTime ;
  cims:multiplicity cims:M:1..1 ;
  cims:stereotype <http://iec.ch/TC57/NonStandard/UML#attribute> ;
  rdfs:domain cim:RegularIntervalSchedule .

cim:RegularIntervalSchedule.timeStep a rdf:Property ;
  rdfs:label "timeStep"@en ;
  rdfs:comment "The time between each pair of subsequent regular time points in sequence order." ;
  cims:dataType cim:Seconds ;
  cims:multiplicity cims:M:1..1 ;
  cims:stereotype <http://iec.ch/TC57/NonStandard/UML#attribute> ;
  rdfs:domain cim:RegularIntervalSchedule .

cim:RegularTimePoint.IntervalSchedule a rdf:Property ;
  rdfs:label "IntervalSchedule"@en ;
  rdfs:comment "Regular interval schedule containing this time point." ;
  cims:AssociationUsed "Yes" ;
  cims:inverseRoleName cim:RegularIntervalSchedule.TimePoints ;
  cims:multiplicity cims:M:1 ;
  rdfs:domain cim:RegularTimePoint ;
  rdfs:range cim:RegularIntervalSchedule .

cim:RegularTimePoint.sequenceNumber a rdf:Property ;
  rdfs:label "sequenceNumber"@en ;
  rdfs:comment "The position of the regular time point in the sequence. Note that time points don't have to be sequential, i.e. time points may be omitted. The actual time for a RegularTimePoint is computed by multiplying the associated regular interval schedule's time step with the regular time point sequence number and adding the associated schedules start time. To specify values for the start time, use sequence number 0.  The sequence number cannot be negative." ;
  cims:dataType cim:Integer ;
  cims:multiplicity cims:M:1..1 ;
  cims:stereotype <http://iec.ch/TC57/NonStandard/UML#attribute> ;
  rdfs:domain cim:RegularTimePoint .

cim:RegularTimePoint.value1 a rdf:Property ;
  rdfs:label "value1"@en ;
  rdfs:comment "The first value at the time. The meaning of the value is defined by the derived type of the associated schedule." ;
  cims:dataType cim:Float ;
  cims:multiplicity cims:M:1..1 ;
  cims:stereotype <http://iec.ch/TC57/NonStandard/UML#attribute> ;
  rdfs:domain cim:RegularTimePoint .

cim:RegularTimePoint.value2 a rdf:Property ;
  rdfs:label "value2"@en ;
  rdfs:comment "The second value at the time. The meaning of the value is defined by the derived type of the associated schedule." ;
  cims:dataType cim:Float ;
  cims:multiplicity cims:M:0..1 ;
  cims:stereotype <http://iec.ch/TC57/NonStandard/UML#attribute> ;
  rdfs:domain cim:RegularTimePoint .

cim:RegulatingCondEq.RegulatingControl a rdf:Property ;
  rdfs:label "RegulatingControl"@en ;
  rdfs:comment "The regulating control scheme in which this equipment participates." ;
  cims:AssociationUsed "Yes" ;
  cims:inverseRoleName cim:RegulatingControl.RegulatingCondEq ;
  cims:multiplicity cims:M:0..1 ;
  rdfs:domain cim:RegulatingCondEq ;
  rdfs:range cim:RegulatingControl .

cim:RegulatingControl.RegulatingCondEq a rdf:Property ;
  rdfs:label "RegulatingCondEq"@en ;
  rdfs:comment "The equipment that participates in this regulating control scheme." ;
  cims:AssociationUsed "No" ;
  cims:inverseRoleName cim:RegulatingCondEq.RegulatingControl ;
  cims:multiplicity cims:M:0..n ;
  rdfs:domain cim:RegulatingControl ;
  rdfs:range cim:RegulatingCondEq .

cim:RegulatingControl.RegulationSchedule a rdf:Property ;
  rdfs:label "RegulationSchedule"@en ;
  rdfs:comment "Schedule for this regulating control." ;
  cims:AssociationUsed "No" ;
  cims:inverseRoleName cim:RegulationSchedule.RegulatingControl ;
  cims:multiplicity cims:M:0..n ;
  rdfs:domain cim:RegulatingControl ;
  rdfs:range cim:RegulationSchedule .

cim:RegulatingControl.Terminal a rdf:Property ;
  rdfs:label "Terminal"@en ;
  rdfs:comment "The terminal associated with this regulating control.  The terminal is associated instead of a node, since the terminal could connect into either a topological node or a connectivity node.  Sometimes it is useful to model regulation at a terminal of a bus bar object. " ;
  cims:AssociationUsed "Yes" ;
  cims:inverseRoleName cim:Terminal.RegulatingControl ;
  cims:multiplicity cims:M:1..1 ;
  rdfs:domain cim:RegulatingControl ;
  rdfs:range cim:Terminal .

cim:RegulatingControl.mode a rdf:Property ;
  rdfs:label "mode"@en ;
  rdfs:comment "The regulating control mode presently available.  This specification allows for determining the kind of regulation without need for obtaining the units from a schedule." ;
  cims:multiplicity cims:M:1..1 ;
  cims:stereotype <http://iec.ch/TC57/NonStandard/UML#attribute> ;
  rdfs:domain cim:RegulatingControl ;
  rdfs:range cim:RegulatingControlModeKind .

cim:RegulationSchedule.RegulatingControl a rdf:Property ;
  rdfs:label "RegulatingControl"@en ;
  rdfs:comment "Regulating controls that have this schedule." ;
  cims:AssociationUsed "Yes" ;
  cims:inverseRoleName cim:RegulatingControl.RegulationSchedule ;
  cims:multiplicity cims:M:1 ;
  rdfs:domain cim:RegulationSchedule ;
  rdfs:range cim:RegulatingControl .

cim:ReportingGroup.BusNameMarker a rdf:Property ;
  rdfs:label "BusNameMarker"@en ;
  rdfs:comment "The bus name markers that belong to this reporting group." ;
  cims:AssociationUsed "No" ;
  cims:inverseRoleName cim:BusNameMarker.ReportingGroup ;
  cims:multiplicity cims:M:0..n ;
  rdfs:domain cim:ReportingGroup ;
  rdfs:range cim:BusNameMarker .

cim:Resistance.multiplier a rdf:Property ;
  rdfs:label "multiplier"@en ;
  cims:isFixed "none" ;
  cims:multiplicity cims:M:0..1 ;
  cims:stereotype <http://iec.ch/TC57/NonStandard/UML#attribute> ;
  rdfs:domain cim:Resistance ;
  rdfs:range cim:UnitMultiplier .

cim:Resistance.unit a rdf:Property ;
  rdfs:label "unit"@en ;
  cims:isFixed "ohm" ;
  cims:multiplicity cims:M:0..1 ;
  cims:stereotype <http://iec.ch/TC57/NonStandard/UML#attribute> ;
  rdfs:domain cim:Resistance ;
  rdfs:range cim:UnitSymbol .

cim:Resistance.value a rdf:Property ;
  rdfs:label "value"@en ;
  cims:dataType cim:Float ;
  cims:multiplicity cims:M:0..1 ;
  cims:stereotype <http://iec.ch/TC57/NonStandard/UML#attribute> ;
  rdfs:domain cim:Resistance .

cim:RotatingMachine.GeneratingUnit a rdf:Property ;
  rdfs:label "GeneratingUnit"@en ;
  rdfs:comment "A synchronous machine may operate as a generator and as such becomes a member of a generating unit." ;
  cims:AssociationUsed "Yes" ;
  cims:inverseRoleName cim:GeneratingUnit.RotatingMachine ;
  cims:multiplicity cims:M:0..1 ;
  rdfs:domain cim:RotatingMachine ;
  rdfs:range cim:GeneratingUnit .

cim:RotatingMachine.HydroPump a rdf:Property ;
  rdfs:label "HydroPump"@en ;
  rdfs:comment "The synchronous machine drives the turbine which moves the water from a low elevation to a higher elevation. The direction of machine rotation for pumping may or may not be the same as for generating." ;
  cims:AssociationUsed "No" ;
  cims:inverseRoleName cim:HydroPump.RotatingMachine ;
  cims:multiplicity cims:M:0..1 ;
  rdfs:domain cim:RotatingMachine ;
  rdfs:range cim:HydroPump .

cim:RotatingMachine.ratedPowerFactor a rdf:Property ;
  rdfs:label "ratedPowerFactor"@en ;
  rdfs:comment "Power factor (nameplate data). It is primarily used for short circuit data exchange according to IEC 60909. The attribute cannot be a negative value." ;
  cims:dataType cim:Float ;
  cims:multiplicity cims:M:0..1 ;
  cims:stereotype <http://iec.ch/TC57/NonStandard/UML#attribute> ;
  rdfs:domain cim:RotatingMachine .

cim:RotatingMachine.ratedS a rdf:Property ;
  rdfs:label "ratedS"@en ;
  rdfs:comment """Nameplate apparent power rating for the unit.
The attribute shall have a positive value.""" ;
  cims:dataType cim:ApparentPower ;
  cims:multiplicity cims:M:0..1 ;
  cims:stereotype <http://iec.ch/TC57/NonStandard/UML#attribute> ;
  rdfs:domain cim:RotatingMachine .

cim:RotatingMachine.ratedU a rdf:Property ;
  rdfs:label "ratedU"@en ;
  rdfs:comment """Rated voltage (nameplate data, Ur in IEC 60909-0). It is primarily used for short circuit data exchange according to IEC 60909.
The attribute shall be a positive value.""" ;
  cims:dataType cim:Voltage ;
  cims:multiplicity cims:M:0..1 ;
  cims:stereotype <http://iec.ch/TC57/NonStandard/UML#attribute> ;
  rdfs:domain cim:RotatingMachine .

cim:RotationSpeed.multiplier a rdf:Property ;
  rdfs:label "multiplier"@en ;
  cims:isFixed "none" ;
  cims:multiplicity cims:M:0..1 ;
  cims:stereotype <http://iec.ch/TC57/NonStandard/UML#attribute> ;
  rdfs:domain cim:RotationSpeed ;
  rdfs:range cim:UnitMultiplier .

cim:RotationSpeed.unit a rdf:Property ;
  rdfs:label "unit"@en ;
  cims:isFixed "Hz" ;
  cims:multiplicity cims:M:0..1 ;
  cims:stereotype <http://iec.ch/TC57/NonStandard/UML#attribute> ;
  rdfs:domain cim:RotationSpeed ;
  rdfs:range cim:UnitSymbol .

cim:RotationSpeed.value a rdf:Property ;
  rdfs:label "value"@en ;
  cims:dataType cim:Float ;
  cims:multiplicity cims:M:0..1 ;
  cims:stereotype <http://iec.ch/TC57/NonStandard/UML#attribute> ;
  rdfs:domain cim:RotationSpeed .

cim:Season.SeasonDayTypeSchedules a rdf:Property ;
  rdfs:label "SeasonDayTypeSchedules"@en ;
  rdfs:comment "Schedules that use this Season." ;
  cims:AssociationUsed "No" ;
  cims:inverseRoleName cim:SeasonDayTypeSchedule.Season ;
  cims:multiplicity cims:M:0..n ;
  rdfs:domain cim:Season ;
  rdfs:range cim:SeasonDayTypeSchedule .

cim:Season.endDate a rdf:Property ;
  rdfs:label "endDate"@en ;
  rdfs:comment "Date season ends." ;
  cims:dataType cim:MonthDay ;
  cims:multiplicity cims:M:1..1 ;
  cims:stereotype <http://iec.ch/TC57/NonStandard/UML#attribute> ;
  rdfs:domain cim:Season .

cim:Season.startDate a rdf:Property ;
  rdfs:label "startDate"@en ;
  rdfs:comment "Date season starts." ;
  cims:dataType cim:MonthDay ;
  cims:multiplicity cims:M:1..1 ;
  cims:stereotype <http://iec.ch/TC57/NonStandard/UML#attribute> ;
  rdfs:domain cim:Season .

cim:SeasonDayTypeSchedule.DayType a rdf:Property ;
  rdfs:label "DayType"@en ;
  rdfs:comment "DayType for the Schedule." ;
  cims:AssociationUsed "Yes" ;
  cims:inverseRoleName cim:DayType.SeasonDayTypeSchedules ;
  cims:multiplicity cims:M:1..1 ;
  rdfs:domain cim:SeasonDayTypeSchedule ;
  rdfs:range cim:DayType .

cim:SeasonDayTypeSchedule.Season a rdf:Property ;
  rdfs:label "Season"@en ;
  rdfs:comment "Season for the Schedule." ;
  cims:AssociationUsed "Yes" ;
  cims:inverseRoleName cim:Season.SeasonDayTypeSchedules ;
  cims:multiplicity cims:M:1..1 ;
  rdfs:domain cim:SeasonDayTypeSchedule ;
  rdfs:range cim:Season .

cim:Seconds.multiplier a rdf:Property ;
  rdfs:label "multiplier"@en ;
  cims:isFixed "none" ;
  cims:multiplicity cims:M:0..1 ;
  cims:stereotype <http://iec.ch/TC57/NonStandard/UML#attribute> ;
  rdfs:domain cim:Seconds ;
  rdfs:range cim:UnitMultiplier .

cim:Seconds.unit a rdf:Property ;
  rdfs:label "unit"@en ;
  cims:isFixed "s" ;
  cims:multiplicity cims:M:0..1 ;
  cims:stereotype <http://iec.ch/TC57/NonStandard/UML#attribute> ;
  rdfs:domain cim:Seconds ;
  rdfs:range cim:UnitSymbol .

cim:Seconds.value a rdf:Property ;
  rdfs:label "value"@en ;
  rdfs:comment "Time, in seconds" ;
  cims:dataType cim:Float ;
  cims:multiplicity cims:M:0..1 ;
  cims:stereotype <http://iec.ch/TC57/NonStandard/UML#attribute> ;
  rdfs:domain cim:Seconds .

cim:SeriesCompensator.r a rdf:Property ;
  rdfs:label "r"@en ;
  rdfs:comment "Positive sequence resistance." ;
  cims:dataType cim:Resistance ;
  cims:multiplicity cims:M:1..1 ;
  cims:stereotype <http://iec.ch/TC57/NonStandard/UML#attribute> ;
  rdfs:domain cim:SeriesCompensator .

cim:SeriesCompensator.x a rdf:Property ;
  rdfs:label "x"@en ;
  rdfs:comment "Positive sequence reactance." ;
  cims:dataType cim:Reactance ;
  cims:multiplicity cims:M:1..1 ;
  cims:stereotype <http://iec.ch/TC57/NonStandard/UML#attribute> ;
  rdfs:domain cim:SeriesCompensator .

cim:ShuntCompensator.aVRDelay a rdf:Property ;
  rdfs:label "aVRDelay"@en ;
  rdfs:comment "An automatic voltage regulation delay (AVRDelay) which is the time delay from a change in voltage to when the capacitor is allowed to change state. This filters out temporary changes in voltage." ;
  cims:dataType cim:Seconds ;
  cims:multiplicity cims:M:0..1 ;
  cims:stereotype <http://iec.ch/TC57/NonStandard/UML#attribute> ;
  rdfs:domain cim:ShuntCompensator .

cim:ShuntCompensator.grounded a rdf:Property ;
  rdfs:label "grounded"@en ;
  rdfs:comment "Used for Yn and Zn connections. True if the neutral is solidly grounded." ;
  cims:dataType cim:Boolean ;
  cims:multiplicity cims:M:0..1 ;
  cims:stereotype <http://iec.ch/TC57/NonStandard/UML#attribute> ;
  rdfs:domain cim:ShuntCompensator .

cim:ShuntCompensator.maximumSections a rdf:Property ;
  rdfs:label "maximumSections"@en ;
  rdfs:comment "The maximum number of sections that may be switched in. " ;
  cims:dataType cim:Integer ;
  cims:multiplicity cims:M:1..1 ;
  cims:stereotype <http://iec.ch/TC57/NonStandard/UML#attribute> ;
  rdfs:domain cim:ShuntCompensator .

cim:ShuntCompensator.nomU a rdf:Property ;
  rdfs:label "nomU"@en ;
  rdfs:comment "The voltage at which the nominal reactive power may be calculated. This should normally be within 10% of the voltage at which the capacitor is connected to the network." ;
  cims:dataType cim:Voltage ;
  cims:multiplicity cims:M:1..1 ;
  cims:stereotype <http://iec.ch/TC57/NonStandard/UML#attribute> ;
  rdfs:domain cim:ShuntCompensator .

cim:ShuntCompensator.normalSections a rdf:Property ;
  rdfs:label "normalSections"@en ;
  rdfs:comment "The normal number of sections switched in. The value shall be between zero and ShuntCompensator.maximumSections." ;
  cims:dataType cim:Integer ;
  cims:multiplicity cims:M:1..1 ;
  cims:stereotype <http://iec.ch/TC57/NonStandard/UML#attribute> ;
  rdfs:domain cim:ShuntCompensator .

cim:ShuntCompensator.voltageSensitivity a rdf:Property ;
  rdfs:label "voltageSensitivity"@en ;
  rdfs:comment "Voltage sensitivity required for the device to regulate the bus voltage, in voltage/reactive power." ;
  cims:dataType cim:VoltagePerReactivePower ;
  cims:multiplicity cims:M:0..1 ;
  cims:stereotype <http://iec.ch/TC57/NonStandard/UML#attribute> ;
  rdfs:domain cim:ShuntCompensator .

cim:StaticVarCompensator.capacitiveRating a rdf:Property ;
  rdfs:label "capacitiveRating"@en ;
  rdfs:comment "Capacitive reactance at maximum capacitive reactive power.  Shall always be positive." ;
  cims:dataType cim:Reactance ;
  cims:multiplicity cims:M:1..1 ;
  cims:stereotype <http://iec.ch/TC57/NonStandard/UML#attribute> ;
  rdfs:domain cim:StaticVarCompensator .

cim:StaticVarCompensator.inductiveRating a rdf:Property ;
  rdfs:label "inductiveRating"@en ;
  rdfs:comment "Inductive reactance at maximum inductive reactive power.  Shall always be negative.  " ;
  cims:dataType cim:Reactance ;
  cims:multiplicity cims:M:1..1 ;
  cims:stereotype <http://iec.ch/TC57/NonStandard/UML#attribute> ;
  rdfs:domain cim:StaticVarCompensator .

cim:StaticVarCompensator.sVCControlMode a rdf:Property ;
  rdfs:label "sVCControlMode"@en ;
  rdfs:comment "SVC control mode." ;
  cims:multiplicity cims:M:0..1 ;
  cims:stereotype "deprecated", <http://iec.ch/TC57/NonStandard/UML#attribute> ;
  rdfs:domain cim:StaticVarCompensator ;
  rdfs:range cim:SVCControlMode .

cim:StaticVarCompensator.slope a rdf:Property ;
  rdfs:label "slope"@en ;
  rdfs:comment """The characteristics slope of an SVC defines how the reactive power output changes in proportion to the difference between the regulated bus voltage and the voltage setpoint.
The attribute shall be a positive value or zero.""" ;
  cims:dataType cim:VoltagePerReactivePower ;
  cims:multiplicity cims:M:1..1 ;
  cims:stereotype <http://iec.ch/TC57/NonStandard/UML#attribute> ;
  rdfs:domain cim:StaticVarCompensator .

cim:StaticVarCompensator.voltageSetPoint a rdf:Property ;
  rdfs:label "voltageSetPoint"@en ;
  rdfs:comment "The reactive power output of the SVC is proportional to the difference between the voltage at the regulated bus and the voltage setpoint.  When the regulated bus voltage is equal to the voltage setpoint, the reactive power output is zero." ;
  cims:dataType cim:Voltage ;
  cims:multiplicity cims:M:0..1 ;
  cims:stereotype "deprecated", <http://iec.ch/TC57/NonStandard/UML#attribute> ;
  rdfs:domain cim:StaticVarCompensator .

cim:SubGeographicalRegion.DCLines a rdf:Property ;
  rdfs:label "DCLines"@en ;
  rdfs:comment "The DC lines in this sub-geographical region." ;
  cims:AssociationUsed "No" ;
  cims:inverseRoleName cim:DCLine.Region ;
  cims:multiplicity cims:M:0..n ;
  rdfs:domain cim:SubGeographicalRegion ;
  rdfs:range cim:DCLine .

cim:SubGeographicalRegion.Lines a rdf:Property ;
  rdfs:label "Lines"@en ;
  rdfs:comment "The lines within the sub-geographical region." ;
  cims:AssociationUsed "No" ;
  cims:inverseRoleName cim:Line.Region ;
  cims:multiplicity cims:M:0..n ;
  rdfs:domain cim:SubGeographicalRegion ;
  rdfs:range cim:Line .

cim:SubGeographicalRegion.Region a rdf:Property ;
  rdfs:label "Region"@en ;
  rdfs:comment "The geographical region which this sub-geographical region is within." ;
  cims:AssociationUsed "Yes" ;
  cims:inverseRoleName cim:GeographicalRegion.Regions ;
  cims:multiplicity cims:M:1 ;
  rdfs:domain cim:SubGeographicalRegion ;
  rdfs:range cim:GeographicalRegion .

cim:SubGeographicalRegion.Substations a rdf:Property ;
  rdfs:label "Substations"@en ;
  rdfs:comment "The substations in this sub-geographical region." ;
  cims:AssociationUsed "No" ;
  cims:inverseRoleName cim:Substation.Region ;
  cims:multiplicity cims:M:0..n ;
  rdfs:domain cim:SubGeographicalRegion ;
  rdfs:range cim:Substation .

cim:SubLoadArea.LoadArea a rdf:Property ;
  rdfs:label "LoadArea"@en ;
  rdfs:comment "The LoadArea where the SubLoadArea belongs." ;
  cims:AssociationUsed "Yes" ;
  cims:inverseRoleName cim:LoadArea.SubLoadAreas ;
  cims:multiplicity cims:M:1 ;
  rdfs:domain cim:SubLoadArea ;
  rdfs:range cim:LoadArea .

cim:SubLoadArea.LoadGroups a rdf:Property ;
  rdfs:label "LoadGroups"@en ;
  rdfs:comment "The Loadgroups in the SubLoadArea." ;
  cims:AssociationUsed "No" ;
  cims:inverseRoleName cim:LoadGroup.SubLoadArea ;
  cims:multiplicity cims:M:1..n ;
  rdfs:domain cim:SubLoadArea ;
  rdfs:range cim:LoadGroup .

cim:Substation.DCConverterUnit a rdf:Property ;
  rdfs:label "DCConverterUnit"@en ;
  rdfs:comment "The DC converter unit belonging of the substation." ;
  cims:AssociationUsed "No" ;
  cims:inverseRoleName cim:DCConverterUnit.Substation ;
  cims:multiplicity cims:M:0..n ;
  rdfs:domain cim:Substation ;
  rdfs:range cim:DCConverterUnit .

cim:Substation.Region a rdf:Property ;
  rdfs:label "Region"@en ;
  rdfs:comment "The SubGeographicalRegion containing the substation." ;
  cims:AssociationUsed "Yes" ;
  cims:inverseRoleName cim:SubGeographicalRegion.Substations ;
  cims:multiplicity cims:M:1 ;
  rdfs:domain cim:Substation ;
  rdfs:range cim:SubGeographicalRegion .

cim:Substation.VoltageLevels a rdf:Property ;
  rdfs:label "VoltageLevels"@en ;
  rdfs:comment "The voltage levels within this substation." ;
  cims:AssociationUsed "No" ;
  cims:inverseRoleName cim:VoltageLevel.Substation ;
  cims:multiplicity cims:M:0..n ;
  rdfs:domain cim:Substation ;
  rdfs:range cim:VoltageLevel .

cim:Susceptance.multiplier a rdf:Property ;
  rdfs:label "multiplier"@en ;
  cims:isFixed "none" ;
  cims:multiplicity cims:M:0..1 ;
  cims:stereotype <http://iec.ch/TC57/NonStandard/UML#attribute> ;
  rdfs:domain cim:Susceptance ;
  rdfs:range cim:UnitMultiplier .

cim:Susceptance.unit a rdf:Property ;
  rdfs:label "unit"@en ;
  cims:isFixed "S" ;
  cims:multiplicity cims:M:0..1 ;
  cims:stereotype <http://iec.ch/TC57/NonStandard/UML#attribute> ;
  rdfs:domain cim:Susceptance ;
  rdfs:range cim:UnitSymbol .

cim:Susceptance.value a rdf:Property ;
  rdfs:label "value"@en ;
  cims:dataType cim:Float ;
  cims:multiplicity cims:M:0..1 ;
  cims:stereotype <http://iec.ch/TC57/NonStandard/UML#attribute> ;
  rdfs:domain cim:Susceptance .

cim:Switch.SwitchSchedules a rdf:Property ;
  rdfs:label "SwitchSchedules"@en ;
  rdfs:comment "A Switch can be associated with SwitchSchedules." ;
  cims:AssociationUsed "No" ;
  cims:inverseRoleName cim:SwitchSchedule.Switch ;
  cims:multiplicity cims:M:0..n ;
  rdfs:domain cim:Switch ;
  rdfs:range cim:SwitchSchedule .

cim:Switch.normalOpen a rdf:Property ;
  rdfs:label "normalOpen"@en ;
  rdfs:comment "The attribute is used in cases when no Measurement for the status value is present. If the Switch has a status measurement the Discrete.normalValue is expected to match with the Switch.normalOpen." ;
  cims:dataType cim:Boolean ;
  cims:multiplicity cims:M:1..1 ;
  cims:stereotype <http://iec.ch/TC57/NonStandard/UML#attribute> ;
  rdfs:domain cim:Switch .

cim:Switch.ratedCurrent a rdf:Property ;
  rdfs:label "ratedCurrent"@en ;
  rdfs:comment """The maximum continuous current carrying capacity in amps governed by the device material and construction.
The attribute shall be a positive value.""" ;
  cims:dataType cim:CurrentFlow ;
  cims:multiplicity cims:M:0..1 ;
  cims:stereotype <http://iec.ch/TC57/NonStandard/UML#attribute> ;
  rdfs:domain cim:Switch .

cim:Switch.retained a rdf:Property ;
  rdfs:label "retained"@en ;
  rdfs:comment "Branch is retained in the topological solution.  The flow through retained switches will normally be calculated in power flow." ;
  cims:dataType cim:Boolean ;
  cims:multiplicity cims:M:1..1 ;
  cims:stereotype <http://iec.ch/TC57/NonStandard/UML#attribute> ;
  rdfs:domain cim:Switch .

cim:SwitchSchedule.Switch a rdf:Property ;
  rdfs:label "Switch"@en ;
  rdfs:comment "A SwitchSchedule is associated with a Switch." ;
  cims:AssociationUsed "Yes" ;
  cims:inverseRoleName cim:Switch.SwitchSchedules ;
  cims:multiplicity cims:M:1 ;
  rdfs:domain cim:SwitchSchedule ;
  rdfs:range cim:Switch .

cim:SynchronousMachine.InitialReactiveCapabilityCurve a rdf:Property ;
  rdfs:label "InitialReactiveCapabilityCurve"@en ;
  rdfs:comment "The default reactive capability curve for use by a synchronous machine." ;
  cims:AssociationUsed "Yes" ;
  cims:inverseRoleName cim:ReactiveCapabilityCurve.InitiallyUsedBySynchronousMachines ;
  cims:multiplicity cims:M:0..1 ;
  rdfs:domain cim:SynchronousMachine ;
  rdfs:range cim:ReactiveCapabilityCurve .

cim:SynchronousMachine.maxQ a rdf:Property ;
  rdfs:label "maxQ"@en ;
  rdfs:comment "Maximum reactive power limit. This is the maximum (nameplate) limit for the unit." ;
  cims:dataType cim:ReactivePower ;
  cims:multiplicity cims:M:0..1 ;
  cims:stereotype <http://iec.ch/TC57/NonStandard/UML#attribute> ;
  rdfs:domain cim:SynchronousMachine .

cim:SynchronousMachine.minQ a rdf:Property ;
  rdfs:label "minQ"@en ;
  rdfs:comment "Minimum reactive power limit for the unit." ;
  cims:dataType cim:ReactivePower ;
  cims:multiplicity cims:M:0..1 ;
  cims:stereotype <http://iec.ch/TC57/NonStandard/UML#attribute> ;
  rdfs:domain cim:SynchronousMachine .

cim:SynchronousMachine.qPercent a rdf:Property ;
  rdfs:label "qPercent"@en ;
  rdfs:comment "Part of the coordinated reactive control that comes from this machine. The attribute is used as a participation factor not necessarily summing up to 100% for the participating devices in the control." ;
  cims:dataType cim:PerCent ;
  cims:multiplicity cims:M:0..1 ;
  cims:stereotype <http://iec.ch/TC57/NonStandard/UML#attribute> ;
  rdfs:domain cim:SynchronousMachine .

cim:SynchronousMachine.type a rdf:Property ;
  rdfs:label "type"@en ;
  rdfs:comment "Modes that this synchronous machine can operate in." ;
  cims:multiplicity cims:M:1..1 ;
  cims:stereotype <http://iec.ch/TC57/NonStandard/UML#attribute> ;
  rdfs:domain cim:SynchronousMachine ;
  rdfs:range cim:SynchronousMachineKind .

cim:TapChanger.TapChangerControl a rdf:Property ;
  rdfs:label "TapChangerControl"@en ;
  rdfs:comment "The regulating control scheme in which this tap changer participates." ;
  cims:AssociationUsed "Yes" ;
  cims:inverseRoleName cim:TapChangerControl.TapChanger ;
  cims:multiplicity cims:M:0..1 ;
  rdfs:domain cim:TapChanger ;
  rdfs:range cim:TapChangerControl .

cim:TapChanger.TapSchedules a rdf:Property ;
  rdfs:label "TapSchedules"@en ;
  rdfs:comment "A TapChanger can have TapSchedules." ;
  cims:AssociationUsed "No" ;
  cims:inverseRoleName cim:TapSchedule.TapChanger ;
  cims:multiplicity cims:M:0..n ;
  rdfs:domain cim:TapChanger ;
  rdfs:range cim:TapSchedule .

cim:TapChanger.highStep a rdf:Property ;
  rdfs:label "highStep"@en ;
  rdfs:comment """Highest possible tap step position, advance from neutral.
The attribute shall be greater than lowStep.""" ;
  cims:dataType cim:Integer ;
  cims:multiplicity cims:M:1..1 ;
  cims:stereotype <http://iec.ch/TC57/NonStandard/UML#attribute> ;
  rdfs:domain cim:TapChanger .

cim:TapChanger.lowStep a rdf:Property ;
  rdfs:label "lowStep"@en ;
  rdfs:comment "Lowest possible tap step position, retard from neutral." ;
  cims:dataType cim:Integer ;
  cims:multiplicity cims:M:1..1 ;
  cims:stereotype <http://iec.ch/TC57/NonStandard/UML#attribute> ;
  rdfs:domain cim:TapChanger .

cim:TapChanger.ltcFlag a rdf:Property ;
  rdfs:label "ltcFlag"@en ;
  rdfs:comment "Specifies whether or not a TapChanger has load tap changing capabilities." ;
  cims:dataType cim:Boolean ;
  cims:multiplicity cims:M:1..1 ;
  cims:stereotype <http://iec.ch/TC57/NonStandard/UML#attribute> ;
  rdfs:domain cim:TapChanger .

cim:TapChanger.neutralStep a rdf:Property ;
  rdfs:label "neutralStep"@en ;
  rdfs:comment """The neutral tap step position for this winding.
The attribute shall be equal to or greater than lowStep and equal or less than highStep.
It is the step position where the voltage is neutralU when the other terminals of the transformer are at the ratedU.  If there are other tap changers on the transformer those taps are kept constant at their neutralStep.""" ;
  cims:dataType cim:Integer ;
  cims:multiplicity cims:M:1..1 ;
  cims:stereotype <http://iec.ch/TC57/NonStandard/UML#attribute> ;
  rdfs:domain cim:TapChanger .

cim:TapChanger.neutralU a rdf:Property ;
  rdfs:label "neutralU"@en ;
  rdfs:comment """Voltage at which the winding operates at the neutral tap setting. It is the voltage at the terminal of the PowerTransformerEnd associated with the tap changer when all tap changers on the transformer are at their neutralStep position.  Normally neutralU of the tap changer is the same as ratedU of the PowerTransformerEnd, but it can differ in special cases such as when the tapping mechanism is separate from the winding more common on lower voltage transformers.
This attribute is not relevant for PhaseTapChangerAsymmetrical, PhaseTapChangerSymmetrical and PhaseTapChangerLinear. """ ;
  cims:dataType cim:Voltage ;
  cims:multiplicity cims:M:1..1 ;
  cims:stereotype <http://iec.ch/TC57/NonStandard/UML#attribute> ;
  rdfs:domain cim:TapChanger .

cim:TapChanger.normalStep a rdf:Property ;
  rdfs:label "normalStep"@en ;
  rdfs:comment """The tap step position used in "normal" network operation for this winding. For a "Fixed" tap changer indicates the current physical tap setting.
The attribute shall be equal to or greater than lowStep and equal to or less than highStep.""" ;
  cims:dataType cim:Integer ;
  cims:multiplicity cims:M:1..1 ;
  cims:stereotype <http://iec.ch/TC57/NonStandard/UML#attribute> ;
  rdfs:domain cim:TapChanger .

cim:TapChangerControl.TapChanger a rdf:Property ;
  rdfs:label "TapChanger"@en ;
  rdfs:comment "The tap changers that participates in this regulating tap control scheme." ;
  cims:AssociationUsed "No" ;
  cims:inverseRoleName cim:TapChanger.TapChangerControl ;
  cims:multiplicity cims:M:1..n ;
  rdfs:domain cim:TapChangerControl ;
  rdfs:range cim:TapChanger .

cim:TapChangerTablePoint.b a rdf:Property ;
  rdfs:label "b"@en ;
  rdfs:comment """The magnetizing branch susceptance deviation as a percentage of nominal value. The actual susceptance is calculated as follows:
calculated magnetizing susceptance = b(nominal) * (1 + b(from this class)/100).   The b(nominal) is defined as the static magnetizing susceptance on the associated power transformer end or ends.  This model assumes the star impedance (pi model) form.""" ;
  cims:dataType cim:PerCent ;
  cims:multiplicity cims:M:0..1 ;
  cims:stereotype <http://iec.ch/TC57/NonStandard/UML#attribute> ;
  rdfs:domain cim:TapChangerTablePoint .

cim:TapChangerTablePoint.g a rdf:Property ;
  rdfs:label "g"@en ;
  rdfs:comment """The magnetizing branch conductance deviation as a percentage of nominal value. The actual conductance is calculated as follows:
calculated magnetizing conductance = g(nominal) * (1 + g(from this class)/100).   The g(nominal) is defined as the static magnetizing conductance on the associated power transformer end or ends.  This model assumes the star impedance (pi model) form.""" ;
  cims:dataType cim:PerCent ;
  cims:multiplicity cims:M:0..1 ;
  cims:stereotype <http://iec.ch/TC57/NonStandard/UML#attribute> ;
  rdfs:domain cim:TapChangerTablePoint .

cim:TapChangerTablePoint.r a rdf:Property ;
  rdfs:label "r"@en ;
  rdfs:comment """The resistance deviation as a percentage of nominal value. The actual reactance is calculated as follows:
calculated resistance = r(nominal) * (1 + r(from this class)/100).   The r(nominal) is defined as the static resistance on the associated power transformer end or ends.  This model assumes the star impedance (pi model) form.""" ;
  cims:dataType cim:PerCent ;
  cims:multiplicity cims:M:0..1 ;
  cims:stereotype <http://iec.ch/TC57/NonStandard/UML#attribute> ;
  rdfs:domain cim:TapChangerTablePoint .

cim:TapChangerTablePoint.ratio a rdf:Property ;
  rdfs:label "ratio"@en ;
  rdfs:comment """The voltage at the tap step divided by rated voltage of the transformer end having the tap changer. Hence this is a value close to one.
For example, if the ratio at step 1 is 1.01, and the rated voltage of the transformer end is 110kV, then the voltage obtained by setting the tap changer to step 1 to is 111.1kV.""" ;
  cims:dataType cim:Float ;
  cims:multiplicity cims:M:0..1 ;
  cims:stereotype <http://iec.ch/TC57/NonStandard/UML#attribute> ;
  rdfs:domain cim:TapChangerTablePoint .

cim:TapChangerTablePoint.step a rdf:Property ;
  rdfs:label "step"@en ;
  rdfs:comment "The tap step." ;
  cims:dataType cim:Integer ;
  cims:multiplicity cims:M:1..1 ;
  cims:stereotype <http://iec.ch/TC57/NonStandard/UML#attribute> ;
  rdfs:domain cim:TapChangerTablePoint .

cim:TapChangerTablePoint.x a rdf:Property ;
  rdfs:label "x"@en ;
  rdfs:comment """The series reactance deviation as a percentage of nominal value. The actual reactance is calculated as follows:
calculated reactance = x(nominal) * (1 + x(from this class)/100).   The x(nominal) is defined as the static series reactance on the associated power transformer end or ends.  This model assumes the star impedance (pi model) form.""" ;
  cims:dataType cim:PerCent ;
  cims:multiplicity cims:M:0..1 ;
  cims:stereotype <http://iec.ch/TC57/NonStandard/UML#attribute> ;
  rdfs:domain cim:TapChangerTablePoint .

cim:TapSchedule.TapChanger a rdf:Property ;
  rdfs:label "TapChanger"@en ;
  rdfs:comment "A TapSchedule is associated with a TapChanger." ;
  cims:AssociationUsed "Yes" ;
  cims:inverseRoleName cim:TapChanger.TapSchedules ;
  cims:multiplicity cims:M:1 ;
  rdfs:domain cim:TapSchedule ;
  rdfs:range cim:TapChanger .

cim:Terminal.AuxiliaryEquipment a rdf:Property ;
  rdfs:label "AuxiliaryEquipment"@en ;
  rdfs:comment "The auxiliary equipment connected to the terminal." ;
  cims:AssociationUsed "No" ;
  cims:inverseRoleName cim:AuxiliaryEquipment.Terminal ;
  cims:multiplicity cims:M:0..n ;
  rdfs:domain cim:Terminal ;
  rdfs:range cim:AuxiliaryEquipment .

cim:Terminal.ConductingEquipment a rdf:Property ;
  rdfs:label "ConductingEquipment"@en ;
  rdfs:comment "The conducting equipment of the terminal.  Conducting equipment have  terminals that may be connected to other conducting equipment terminals via connectivity nodes or topological nodes." ;
  cims:AssociationUsed "Yes" ;
  cims:inverseRoleName cim:ConductingEquipment.Terminals ;
  cims:multiplicity cims:M:1 ;
  rdfs:domain cim:Terminal ;
  rdfs:range cim:ConductingEquipment .

cim:Terminal.ConnectivityNode a rdf:Property ;
  rdfs:label "ConnectivityNode"@en ;
  rdfs:comment "The connectivity node to which this terminal connects with zero impedance." ;
  cims:AssociationUsed "Yes" ;
  cims:inverseRoleName cim:ConnectivityNode.Terminals ;
  cims:multiplicity cims:M:0..1 ;
  rdfs:domain cim:Terminal ;
  rdfs:range cim:ConnectivityNode .

cim:Terminal.ConverterDCSides a rdf:Property ;
  rdfs:label "ConverterDCSides"@en ;
  rdfs:comment "All converters' DC sides linked to this point of common coupling terminal." ;
  cims:AssociationUsed "No" ;
  cims:inverseRoleName cim:ACDCConverter.PccTerminal ;
  cims:multiplicity cims:M:0..n ;
  rdfs:domain cim:Terminal ;
  rdfs:range cim:ACDCConverter .

cim:Terminal.RegulatingControl a rdf:Property ;
  rdfs:label "RegulatingControl"@en ;
  rdfs:comment "The controls regulating this terminal." ;
  cims:AssociationUsed "No" ;
  cims:inverseRoleName cim:RegulatingControl.Terminal ;
  cims:multiplicity cims:M:0..n ;
  rdfs:domain cim:Terminal ;
  rdfs:range cim:RegulatingControl .

cim:Terminal.TieFlow a rdf:Property ;
  rdfs:label "TieFlow"@en ;
  rdfs:comment "The control area tie flows to which this terminal associates." ;
  cims:AssociationUsed "No" ;
  cims:inverseRoleName cim:TieFlow.Terminal ;
  cims:multiplicity cims:M:0..2 ;
  rdfs:domain cim:Terminal ;
  rdfs:range cim:TieFlow .

cim:Terminal.TransformerEnd a rdf:Property ;
  rdfs:label "TransformerEnd"@en ;
  rdfs:comment "All transformer ends connected at this terminal." ;
  cims:AssociationUsed "No" ;
  cims:inverseRoleName cim:TransformerEnd.Terminal ;
  cims:multiplicity cims:M:0..n ;
  rdfs:domain cim:Terminal ;
  rdfs:range cim:TransformerEnd .

cim:Terminal.phases a rdf:Property ;
  rdfs:label "phases"@en ;
  rdfs:comment """Represents the normal network phasing condition. If the attribute is missing, three phases (ABC) shall be assumed, except for terminals of grounding classes (specializations of EarthFaultCompensator, GroundDisconnector, and Ground) which will be assumed to be N. Therefore, phase code ABCN is explicitly declared when needed, e.g. for star point grounding equipment.
The phase code on terminals connecting same ConnectivityNode or same TopologicalNode as well as for equipment between two terminals shall be consistent.""" ;
  cims:multiplicity cims:M:0..1 ;
  cims:stereotype <http://iec.ch/TC57/NonStandard/UML#attribute> ;
  rdfs:domain cim:Terminal ;
  rdfs:range cim:PhaseCode .

cim:ThermalGeneratingUnit.CAESPlant a rdf:Property ;
  rdfs:label "CAESPlant"@en ;
  rdfs:comment "A thermal generating unit may be a member of a compressed air energy storage plant." ;
  cims:AssociationUsed "Yes" ;
  cims:inverseRoleName cim:CAESPlant.ThermalGeneratingUnit ;
  cims:multiplicity cims:M:0..1 ;
  rdfs:domain cim:ThermalGeneratingUnit ;
  rdfs:range cim:CAESPlant .

cim:ThermalGeneratingUnit.CogenerationPlant a rdf:Property ;
  rdfs:label "CogenerationPlant"@en ;
  rdfs:comment "A thermal generating unit may be a member of a cogeneration plant." ;
  cims:AssociationUsed "Yes" ;
  cims:inverseRoleName cim:CogenerationPlant.ThermalGeneratingUnits ;
  cims:multiplicity cims:M:0..1 ;
  rdfs:domain cim:ThermalGeneratingUnit ;
  rdfs:range cim:CogenerationPlant .

cim:ThermalGeneratingUnit.CombinedCyclePlant a rdf:Property ;
  rdfs:label "CombinedCyclePlant"@en ;
  rdfs:comment "A thermal generating unit may be a member of a combined cycle plant." ;
  cims:AssociationUsed "Yes" ;
  cims:inverseRoleName cim:CombinedCyclePlant.ThermalGeneratingUnits ;
  cims:multiplicity cims:M:0..1 ;
  rdfs:domain cim:ThermalGeneratingUnit ;
  rdfs:range cim:CombinedCyclePlant .

cim:ThermalGeneratingUnit.FossilFuels a rdf:Property ;
  rdfs:label "FossilFuels"@en ;
  rdfs:comment "A thermal generating unit may have one or more fossil fuels." ;
  cims:AssociationUsed "No" ;
  cims:inverseRoleName cim:FossilFuel.ThermalGeneratingUnit ;
  cims:multiplicity cims:M:0..n ;
  rdfs:domain cim:ThermalGeneratingUnit ;
  rdfs:range cim:FossilFuel .

cim:TieFlow.ControlArea a rdf:Property ;
  rdfs:label "ControlArea"@en ;
  rdfs:comment "The control area of the tie flows." ;
  cims:AssociationUsed "Yes" ;
  cims:inverseRoleName cim:ControlArea.TieFlow ;
  cims:multiplicity cims:M:1 ;
  rdfs:domain cim:TieFlow ;
  rdfs:range cim:ControlArea .

cim:TieFlow.Terminal a rdf:Property ;
  rdfs:label "Terminal"@en ;
  rdfs:comment "The terminal to which this tie flow belongs." ;
  cims:AssociationUsed "Yes" ;
  cims:inverseRoleName cim:Terminal.TieFlow ;
  cims:multiplicity cims:M:1 ;
  rdfs:domain cim:TieFlow ;
  rdfs:range cim:Terminal .

cim:TieFlow.positiveFlowIn a rdf:Property ;
  rdfs:label "positiveFlowIn"@en ;
  rdfs:comment "Specifies the sign of the tie flow associated with a control area. True if positive flow into the terminal (load convention) is also positive flow into the control area.  See the description of ControlArea for further explanation of how TieFlow.positiveFlowIn is used." ;
  cims:dataType cim:Boolean ;
  cims:multiplicity cims:M:1..1 ;
  cims:stereotype <http://iec.ch/TC57/NonStandard/UML#attribute> ;
  rdfs:domain cim:TieFlow .

cim:TransformerEnd.BaseVoltage a rdf:Property ;
  rdfs:label "BaseVoltage"@en ;
  rdfs:comment "Base voltage of the transformer end.  This is essential for PU calculation." ;
  cims:AssociationUsed "Yes" ;
  cims:inverseRoleName cim:BaseVoltage.TransformerEnds ;
  cims:multiplicity cims:M:1 ;
  rdfs:domain cim:TransformerEnd ;
  rdfs:range cim:BaseVoltage .

cim:TransformerEnd.PhaseTapChanger a rdf:Property ;
  rdfs:label "PhaseTapChanger"@en ;
  rdfs:comment "Phase tap changer associated with this transformer end." ;
  cims:AssociationUsed "No" ;
  cims:inverseRoleName cim:PhaseTapChanger.TransformerEnd ;
  cims:multiplicity cims:M:0..1 ;
  rdfs:domain cim:TransformerEnd ;
  rdfs:range cim:PhaseTapChanger .

cim:TransformerEnd.RatioTapChanger a rdf:Property ;
  rdfs:label "RatioTapChanger"@en ;
  rdfs:comment "Ratio tap changer associated with this transformer end." ;
  cims:AssociationUsed "No" ;
  cims:inverseRoleName cim:RatioTapChanger.TransformerEnd ;
  cims:multiplicity cims:M:0..1 ;
  rdfs:domain cim:TransformerEnd ;
  rdfs:range cim:RatioTapChanger .

cim:TransformerEnd.Terminal a rdf:Property ;
  rdfs:label "Terminal"@en ;
  rdfs:comment "Terminal of the power transformer to which this transformer end belongs." ;
  cims:AssociationUsed "Yes" ;
  cims:inverseRoleName cim:Terminal.TransformerEnd ;
  cims:multiplicity cims:M:1..1 ;
  rdfs:domain cim:TransformerEnd ;
  rdfs:range cim:Terminal .

cim:TransformerEnd.endNumber a rdf:Property ;
  rdfs:label "endNumber"@en ;
  rdfs:comment "Number for this transformer end, corresponding to the end's order in the power transformer vector group or phase angle clock number.  Highest voltage winding should be 1.  Each end within a power transformer should have a unique subsequent end number.   Note the transformer end number need not match the terminal sequence number." ;
  cims:dataType cim:Integer ;
  cims:multiplicity cims:M:1..1 ;
  cims:stereotype <http://iec.ch/TC57/NonStandard/UML#attribute> ;
  rdfs:domain cim:TransformerEnd .

cim:Voltage.multiplier a rdf:Property ;
  rdfs:label "multiplier"@en ;
  cims:isFixed "k" ;
  cims:multiplicity cims:M:0..1 ;
  cims:stereotype <http://iec.ch/TC57/NonStandard/UML#attribute> ;
  rdfs:domain cim:Voltage ;
  rdfs:range cim:UnitMultiplier .

cim:Voltage.unit a rdf:Property ;
  rdfs:label "unit"@en ;
  cims:isFixed "V" ;
  cims:multiplicity cims:M:0..1 ;
  cims:stereotype <http://iec.ch/TC57/NonStandard/UML#attribute> ;
  rdfs:domain cim:Voltage ;
  rdfs:range cim:UnitSymbol .

cim:Voltage.value a rdf:Property ;
  rdfs:label "value"@en ;
  cims:dataType cim:Float ;
  cims:multiplicity cims:M:0..1 ;
  cims:stereotype <http://iec.ch/TC57/NonStandard/UML#attribute> ;
  rdfs:domain cim:Voltage .

cim:VoltageLevel.BaseVoltage a rdf:Property ;
  rdfs:label "BaseVoltage"@en ;
  rdfs:comment "The base voltage used for all equipment within the voltage level." ;
  cims:AssociationUsed "Yes" ;
  cims:inverseRoleName cim:BaseVoltage.VoltageLevel ;
  cims:multiplicity cims:M:1 ;
  rdfs:domain cim:VoltageLevel ;
  rdfs:range cim:BaseVoltage .

cim:VoltageLevel.Bays a rdf:Property ;
  rdfs:label "Bays"@en ;
  rdfs:comment "The bays within this voltage level." ;
  cims:AssociationUsed "No" ;
  cims:inverseRoleName cim:Bay.VoltageLevel ;
  cims:multiplicity cims:M:0..n ;
  rdfs:domain cim:VoltageLevel ;
  rdfs:range cim:Bay .

cim:VoltageLevel.Substation a rdf:Property ;
  rdfs:label "Substation"@en ;
  rdfs:comment "The substation of the voltage level." ;
  cims:AssociationUsed "Yes" ;
  cims:inverseRoleName cim:Substation.VoltageLevels ;
  cims:multiplicity cims:M:1 ;
  rdfs:domain cim:VoltageLevel ;
  rdfs:range cim:Substation .

cim:VoltageLevel.highVoltageLimit a rdf:Property ;
  rdfs:label "highVoltageLimit"@en ;
  rdfs:comment """The bus bar's high voltage limit.
The limit applies to all equipment and nodes contained in a given VoltageLevel. It is not required that it is exchanged in pair with lowVoltageLimit. It is preferable to use operational VoltageLimit, which prevails, if present.""" ;
  cims:dataType cim:Voltage ;
  cims:multiplicity cims:M:0..1 ;
  cims:stereotype <http://iec.ch/TC57/NonStandard/UML#attribute> ;
  rdfs:domain cim:VoltageLevel .

cim:VoltageLevel.lowVoltageLimit a rdf:Property ;
  rdfs:label "lowVoltageLimit"@en ;
  rdfs:comment """The bus bar's low voltage limit.
The limit applies to all equipment and nodes contained in a given VoltageLevel. It is not required that it is exchanged in pair with highVoltageLimit. It is preferable to use operational VoltageLimit, which prevails, if present.""" ;
  cims:dataType cim:Voltage ;
  cims:multiplicity cims:M:0..1 ;
  cims:stereotype <http://iec.ch/TC57/NonStandard/UML#attribute> ;
  rdfs:domain cim:VoltageLevel .

cim:VoltageLimit.normalValue a rdf:Property ;
  rdfs:label "normalValue"@en ;
  rdfs:comment "The normal limit on voltage. High or low limit nature of the limit depends upon the properties of the operational limit type. The attribute shall be a positive value or zero." ;
  cims:dataType cim:Voltage ;
  cims:multiplicity cims:M:1..1 ;
  cims:stereotype <http://iec.ch/TC57/NonStandard/UML#attribute> ;
  rdfs:domain cim:VoltageLimit .

cim:VoltagePerReactivePower.multiplier a rdf:Property ;
  rdfs:label "multiplier"@en ;
  cims:isFixed "none" ;
  cims:multiplicity cims:M:0..1 ;
  cims:stereotype <http://iec.ch/TC57/NonStandard/UML#attribute> ;
  rdfs:domain cim:VoltagePerReactivePower ;
  rdfs:range cim:UnitMultiplier .

cim:VoltagePerReactivePower.unit a rdf:Property ;
  rdfs:label "unit"@en ;
  cims:isFixed "VPerVAr" ;
  cims:multiplicity cims:M:0..1 ;
  cims:stereotype <http://iec.ch/TC57/NonStandard/UML#attribute> ;
  rdfs:domain cim:VoltagePerReactivePower ;
  rdfs:range cim:UnitSymbol .

cim:VoltagePerReactivePower.value a rdf:Property ;
  rdfs:label "value"@en ;
  cims:dataType cim:Float ;
  cims:multiplicity cims:M:0..1 ;
  cims:stereotype <http://iec.ch/TC57/NonStandard/UML#attribute> ;
  rdfs:domain cim:VoltagePerReactivePower .

cim:VsCapabilityCurve.VsConverterDCSides a rdf:Property ;
  rdfs:label "VsConverterDCSides"@en ;
  rdfs:comment "All converters with this capability curve." ;
  cims:AssociationUsed "No" ;
  cims:inverseRoleName cim:VsConverter.CapabilityCurve ;
  cims:multiplicity cims:M:0..n ;
  rdfs:domain cim:VsCapabilityCurve ;
  rdfs:range cim:VsConverter .

cim:VsConverter.CapabilityCurve a rdf:Property ;
  rdfs:label "CapabilityCurve"@en ;
  rdfs:comment "Capability curve of this converter." ;
  cims:AssociationUsed "Yes" ;
  cims:inverseRoleName cim:VsCapabilityCurve.VsConverterDCSides ;
  cims:multiplicity cims:M:0..1 ;
  rdfs:domain cim:VsConverter ;
  rdfs:range cim:VsCapabilityCurve .

cim:VsConverter.maxModulationIndex a rdf:Property ;
  rdfs:label "maxModulationIndex"@en ;
  rdfs:comment "The maximum quotient between the AC converter voltage (Uc) and DC voltage (Ud). A factor typically less than 1. It is converter’s configuration data used in power flow." ;
  cims:dataType cim:Float ;
  cims:multiplicity cims:M:0..1 ;
  cims:stereotype <http://iec.ch/TC57/NonStandard/UML#attribute> ;
  rdfs:domain cim:VsConverter .

cim:WindGeneratingUnit.windGenUnitType a rdf:Property ;
  rdfs:label "windGenUnitType"@en ;
  rdfs:comment "The kind of wind generating unit." ;
  cims:multiplicity cims:M:1..1 ;
  cims:stereotype <http://iec.ch/TC57/NonStandard/UML#attribute> ;
  rdfs:domain cim:WindGeneratingUnit ;
  rdfs:range cim:WindGenUnitKind .

eu:BoundaryPoint.ConnectivityNode a rdf:Property ;
  rdfs:label "ConnectivityNode"@en ;
  rdfs:comment "The connectivity node that is designated as a boundary point." ;
  cims:AssociationUsed "Yes" ;
  cims:inverseRoleName eu:ConnectivityNode.BoundaryPoint ;
  cims:multiplicity cims:M:1 ;
  cims:stereotype "European" ;
  rdfs:domain eu:BoundaryPoint ;
  rdfs:range cim:ConnectivityNode .

eu:BoundaryPoint.fromEndIsoCode a rdf:Property ;
  rdfs:label "fromEndIsoCode"@en ;
  rdfs:comment """The ISO code of the region which the "From" side of the Boundary point belongs to or it is connected to.
The ISO code is a two-character country code as defined by ISO 3166 (http://www.iso.org/iso/country_codes). The length of the string is 2 characters maximum.""" ;
  cims:dataType cim:String ;
  cims:multiplicity cims:M:1..1 ;
  cims:stereotype "European", <http://iec.ch/TC57/NonStandard/UML#attribute> ;
  rdfs:domain eu:BoundaryPoint .

eu:BoundaryPoint.fromEndName a rdf:Property ;
  rdfs:label "fromEndName"@en ;
  rdfs:comment """A human readable name with length of the string 64 characters maximum. It covers the following two cases:
-if the Boundary point is placed on a tie-line, it is the name (IdentifiedObject.name) of the substation at which the "From" side of the tie-line is connected to.
-if the Boundary point is placed in a substation, it is the name (IdentifiedObject.name) of the element (e.g. PowerTransformer, ACLineSegment, Switch, etc.) at which the "From" side of the Boundary point is connected to.""" ;
  cims:dataType cim:String ;
  cims:multiplicity cims:M:1..1 ;
  cims:stereotype "European", <http://iec.ch/TC57/NonStandard/UML#attribute> ;
  rdfs:domain eu:BoundaryPoint .

eu:BoundaryPoint.fromEndNameTso a rdf:Property ;
  rdfs:label "fromEndNameTso"@en ;
  rdfs:comment "Identifies the name of the transmission system operator, distribution system operator or other entity at which the \"From\" side of the interconnection is connected to. The length of the string is 64 characters maximum." ;
  cims:dataType cim:String ;
  cims:multiplicity cims:M:1..1 ;
  cims:stereotype "European", <http://iec.ch/TC57/NonStandard/UML#attribute> ;
  rdfs:domain eu:BoundaryPoint .

eu:BoundaryPoint.isDirectCurrent a rdf:Property ;
  rdfs:label "isDirectCurrent"@en ;
  rdfs:comment "If true, this boundary point is a point of common coupling (PCC) of a direct current (DC) interconnection, otherwise the interconnection is AC (default)." ;
  cims:dataType cim:Boolean ;
  cims:multiplicity cims:M:0..1 ;
  cims:stereotype "European", <http://iec.ch/TC57/NonStandard/UML#attribute> ;
  rdfs:domain eu:BoundaryPoint .

eu:BoundaryPoint.isExcludedFromAreaInterchange a rdf:Property ;
  rdfs:label "isExcludedFromAreaInterchange"@en ;
  rdfs:comment "If true, this boundary point is on the interconnection that is excluded from control area interchange calculation and consequently has no related tie flows. Otherwise, the interconnection is included in control area interchange and a TieFlow is required at all sides of the boundary point (default)." ;
  cims:dataType cim:Boolean ;
  cims:multiplicity cims:M:0..1 ;
  cims:stereotype "European", <http://iec.ch/TC57/NonStandard/UML#attribute> ;
  rdfs:domain eu:BoundaryPoint .

eu:BoundaryPoint.toEndIsoCode a rdf:Property ;
  rdfs:label "toEndIsoCode"@en ;
  rdfs:comment """The ISO code of the region which the "To" side of the Boundary point belongs to or is connected to.
The ISO code is a two-character country code as defined by ISO 3166 (http://www.iso.org/iso/country_codes). The length of the string is 2 characters maximum.""" ;
  cims:dataType cim:String ;
  cims:multiplicity cims:M:1..1 ;
  cims:stereotype "European", <http://iec.ch/TC57/NonStandard/UML#attribute> ;
  rdfs:domain eu:BoundaryPoint .

eu:BoundaryPoint.toEndName a rdf:Property ;
  rdfs:label "toEndName"@en ;
  rdfs:comment """A human readable name with length of the string 64 characters maximum. It covers the following two cases:
-if the Boundary point is placed on a tie-line, it is the name (IdentifiedObject.name) of the substation at which the "To" side of the tie-line is connected to.
-if the Boundary point is placed in a substation, it is the name (IdentifiedObject.name) of the element (e.g. PowerTransformer, ACLineSegment, Switch, etc.) at which the "To" side of the Boundary point is connected to.""" ;
  cims:dataType cim:String ;
  cims:multiplicity cims:M:1..1 ;
  cims:stereotype "European", <http://iec.ch/TC57/NonStandard/UML#attribute> ;
  rdfs:domain eu:BoundaryPoint .

eu:BoundaryPoint.toEndNameTso a rdf:Property ;
  rdfs:label "toEndNameTso"@en ;
  rdfs:comment "Identifies the name of the transmission system operator, distribution system operator or other entity at which the \"To\" side of the interconnection is connected to. The length of the string is 64 characters maximum." ;
  cims:dataType cim:String ;
  cims:multiplicity cims:M:1..1 ;
  cims:stereotype "European", <http://iec.ch/TC57/NonStandard/UML#attribute> ;
  rdfs:domain eu:BoundaryPoint .

eu:ConnectivityNode.BoundaryPoint a rdf:Property ;
  rdfs:label "BoundaryPoint"@en ;
  rdfs:comment "The boundary point associated with the connectivity node." ;
  cims:AssociationUsed "No" ;
  cims:inverseRoleName eu:BoundaryPoint.ConnectivityNode ;
  cims:multiplicity cims:M:0..1 ;
  cims:stereotype "European" ;
  rdfs:domain cim:ConnectivityNode ;
  rdfs:range eu:BoundaryPoint .

eu:IdentifiedObject.energyIdentCodeEic a rdf:Property ;
  rdfs:label "energyIdentCodeEic"@en ;
  rdfs:comment "The attribute is used for an exchange of the EIC code (Energy identification Code). The length of the string is 16 characters as defined by the EIC code. For details on EIC scheme please refer to ENTSO-E web site." ;
  cims:dataType cim:String ;
  cims:multiplicity cims:M:0..1 ;
  cims:stereotype "European", "deprecated", <http://iec.ch/TC57/NonStandard/UML#attribute> ;
  rdfs:domain cim:IdentifiedObject .

eu:IdentifiedObject.shortName a rdf:Property ;
  rdfs:label "shortName"@en ;
  rdfs:comment "The attribute is used for an exchange of a human readable short name with length of the string 12 characters maximum." ;
  cims:dataType cim:String ;
  cims:multiplicity cims:M:0..1 ;
  cims:stereotype "European", "deprecated", <http://iec.ch/TC57/NonStandard/UML#attribute> ;
  rdfs:domain cim:IdentifiedObject .

eu:OperationalLimitType.kind a rdf:Property ;
  rdfs:label "kind"@en ;
  rdfs:comment "Types of limits defined in the ENTSO-E Operational Handbook Policy 3." ;
  cims:multiplicity cims:M:1..1 ;
  cims:stereotype "European", <http://iec.ch/TC57/NonStandard/UML#attribute> ;
  rdfs:domain cim:OperationalLimitType ;
  rdfs:range eu:LimitKind .

eu:SolarGeneratingUnit.SolarPowerPlant a rdf:Property ;
  rdfs:label "SolarPowerPlant"@en ;
  rdfs:comment "A solar power plant may have solar generating units." ;
  cims:AssociationUsed "Yes" ;
  cims:inverseRoleName eu:SolarPowerPlant.SolarGeneratingUnits ;
  cims:multiplicity cims:M:0..1 ;
  cims:stereotype "European" ;
  rdfs:domain cim:SolarGeneratingUnit ;
  rdfs:range eu:SolarPowerPlant .

eu:SolarPowerPlant.SolarGeneratingUnits a rdf:Property ;
  rdfs:label "SolarGeneratingUnits"@en ;
  rdfs:comment "A solar generating unit or units may be a member of a solar power plant." ;
  cims:AssociationUsed "No" ;
  cims:inverseRoleName eu:SolarGeneratingUnit.SolarPowerPlant ;
  cims:multiplicity cims:M:0..n ;
  cims:stereotype "European" ;
  rdfs:domain eu:SolarPowerPlant ;
  rdfs:range cim:SolarGeneratingUnit .

eu:WindGeneratingUnit.WindPowerPlant a rdf:Property ;
  rdfs:label "WindPowerPlant"@en ;
  rdfs:comment "A wind power plant may have wind generating units." ;
  cims:AssociationUsed "Yes" ;
  cims:inverseRoleName eu:WindPowerPlant.WindGeneratingUnits ;
  cims:multiplicity cims:M:0..1 ;
  cims:stereotype "European" ;
  rdfs:domain cim:WindGeneratingUnit ;
  rdfs:range eu:WindPowerPlant .

eu:WindPowerPlant.WindGeneratingUnits a rdf:Property ;
  rdfs:label "WindGeneratingUnits"@en ;
  rdfs:comment "A wind generating unit or units may be a member of a wind power plant." ;
  cims:AssociationUsed "No" ;
  cims:inverseRoleName eu:WindGeneratingUnit.WindPowerPlant ;
  cims:multiplicity cims:M:0..n ;
  cims:stereotype "European" ;
  rdfs:domain eu:WindPowerPlant ;
  rdfs:range cim:WindGeneratingUnit .

cim:ControlAreaTypeKind.AGC a cim:ControlAreaTypeKind ;
  rdfs:label "AGC"@en ;
  rdfs:comment "Used for automatic generation control." ;
  cims:stereotype "enum" .

cim:ControlAreaTypeKind.Forecast a cim:ControlAreaTypeKind ;
  rdfs:label "Forecast"@en ;
  rdfs:comment "Used for load forecast." ;
  cims:stereotype "enum" .

cim:ControlAreaTypeKind.Interchange a cim:ControlAreaTypeKind ;
  rdfs:label "Interchange"@en ;
  rdfs:comment "Used for interchange specification or control." ;
  cims:stereotype "enum" .

cim:Currency.AED a cim:Currency ;
  rdfs:label "AED"@en ;
  rdfs:comment "United Arab Emirates dirham." ;
  cims:stereotype "enum" .

cim:Currency.AFN a cim:Currency ;
  rdfs:label "AFN"@en ;
  rdfs:comment "Afghan afghani." ;
  cims:stereotype "enum" .

cim:Currency.ALL a cim:Currency ;
  rdfs:label "ALL"@en ;
  rdfs:comment "Albanian lek." ;
  cims:stereotype "enum" .

cim:Currency.AMD a cim:Currency ;
  rdfs:label "AMD"@en ;
  rdfs:comment "Armenian dram." ;
  cims:stereotype "enum" .

cim:Currency.ANG a cim:Currency ;
  rdfs:label "ANG"@en ;
  rdfs:comment "Netherlands Antillean guilder." ;
  cims:stereotype "enum" .

cim:Currency.AOA a cim:Currency ;
  rdfs:label "AOA"@en ;
  rdfs:comment "Angolan kwanza." ;
  cims:stereotype "enum" .

cim:Currency.ARS a cim:Currency ;
  rdfs:label "ARS"@en ;
  rdfs:comment "Argentine peso." ;
  cims:stereotype "enum" .

cim:Currency.AUD a cim:Currency ;
  rdfs:label "AUD"@en ;
  rdfs:comment "Australian dollar." ;
  cims:stereotype "enum" .

cim:Currency.AWG a cim:Currency ;
  rdfs:label "AWG"@en ;
  rdfs:comment "Aruban florin." ;
  cims:stereotype "enum" .

cim:Currency.AZN a cim:Currency ;
  rdfs:label "AZN"@en ;
  rdfs:comment "Azerbaijani manat." ;
  cims:stereotype "enum" .

cim:Currency.BAM a cim:Currency ;
  rdfs:label "BAM"@en ;
  rdfs:comment "Bosnia and Herzegovina convertible mark." ;
  cims:stereotype "enum" .

cim:Currency.BBD a cim:Currency ;
  rdfs:label "BBD"@en ;
  rdfs:comment "Barbados dollar." ;
  cims:stereotype "enum" .

cim:Currency.BDT a cim:Currency ;
  rdfs:label "BDT"@en ;
  rdfs:comment "Bangladeshi taka." ;
  cims:stereotype "enum" .

cim:Currency.BGN a cim:Currency ;
  rdfs:label "BGN"@en ;
  rdfs:comment "Bulgarian lev." ;
  cims:stereotype "enum" .

cim:Currency.BHD a cim:Currency ;
  rdfs:label "BHD"@en ;
  rdfs:comment "Bahraini dinar." ;
  cims:stereotype "enum" .

cim:Currency.BIF a cim:Currency ;
  rdfs:label "BIF"@en ;
  rdfs:comment "Burundian franc." ;
  cims:stereotype "enum" .

cim:Currency.BMD a cim:Currency ;
  rdfs:label "BMD"@en ;
  rdfs:comment "Bermudian dollar (customarily known as Bermuda dollar)." ;
  cims:stereotype "enum" .

cim:Currency.BND a cim:Currency ;
  rdfs:label "BND"@en ;
  rdfs:comment "Brunei dollar." ;
  cims:stereotype "enum" .

cim:Currency.BOB a cim:Currency ;
  rdfs:label "BOB"@en ;
  rdfs:comment "Boliviano." ;
  cims:stereotype "enum" .

cim:Currency.BOV a cim:Currency ;
  rdfs:label "BOV"@en ;
  rdfs:comment "Bolivian Mvdol (funds code)." ;
  cims:stereotype "enum" .

cim:Currency.BRL a cim:Currency ;
  rdfs:label "BRL"@en ;
  rdfs:comment "Brazilian real." ;
  cims:stereotype "enum" .

cim:Currency.BSD a cim:Currency ;
  rdfs:label "BSD"@en ;
  rdfs:comment "Bahamian dollar." ;
  cims:stereotype "enum" .

cim:Currency.BTN a cim:Currency ;
  rdfs:label "BTN"@en ;
  rdfs:comment "Bhutanese ngultrum." ;
  cims:stereotype "enum" .

cim:Currency.BWP a cim:Currency ;
  rdfs:label "BWP"@en ;
  rdfs:comment "Botswana pula." ;
  cims:stereotype "enum" .

cim:Currency.BYR a cim:Currency ;
  rdfs:label "BYR"@en ;
  rdfs:comment "Belarusian ruble." ;
  cims:stereotype "enum" .

cim:Currency.BZD a cim:Currency ;
  rdfs:label "BZD"@en ;
  rdfs:comment "Belize dollar." ;
  cims:stereotype "enum" .

cim:Currency.CAD a cim:Currency ;
  rdfs:label "CAD"@en ;
  rdfs:comment "Canadian dollar." ;
  cims:stereotype "enum" .

cim:Currency.CDF a cim:Currency ;
  rdfs:label "CDF"@en ;
  rdfs:comment "Congolese franc." ;
  cims:stereotype "enum" .

cim:Currency.CHF a cim:Currency ;
  rdfs:label "CHF"@en ;
  rdfs:comment "Swiss franc." ;
  cims:stereotype "enum" .

cim:Currency.CLF a cim:Currency ;
  rdfs:label "CLF"@en ;
  rdfs:comment "Unidad de Fomento (funds code), Chile." ;
  cims:stereotype "enum" .

cim:Currency.CLP a cim:Currency ;
  rdfs:label "CLP"@en ;
  rdfs:comment "Chilean peso." ;
  cims:stereotype "enum" .

cim:Currency.CNY a cim:Currency ;
  rdfs:label "CNY"@en ;
  rdfs:comment "Chinese yuan." ;
  cims:stereotype "enum" .

cim:Currency.COP a cim:Currency ;
  rdfs:label "COP"@en ;
  rdfs:comment "Colombian peso." ;
  cims:stereotype "enum" .

cim:Currency.COU a cim:Currency ;
  rdfs:label "COU"@en ;
  rdfs:comment "Unidad de Valor Real." ;
  cims:stereotype "enum" .

cim:Currency.CRC a cim:Currency ;
  rdfs:label "CRC"@en ;
  rdfs:comment "Costa Rican colon." ;
  cims:stereotype "enum" .

cim:Currency.CUC a cim:Currency ;
  rdfs:label "CUC"@en ;
  rdfs:comment "Cuban convertible peso." ;
  cims:stereotype "enum" .

cim:Currency.CUP a cim:Currency ;
  rdfs:label "CUP"@en ;
  rdfs:comment "Cuban peso." ;
  cims:stereotype "enum" .

cim:Currency.CVE a cim:Currency ;
  rdfs:label "CVE"@en ;
  rdfs:comment "Cape Verde escudo." ;
  cims:stereotype "enum" .

cim:Currency.CZK a cim:Currency ;
  rdfs:label "CZK"@en ;
  rdfs:comment "Czech koruna." ;
  cims:stereotype "enum" .

cim:Currency.DJF a cim:Currency ;
  rdfs:label "DJF"@en ;
  rdfs:comment "Djiboutian franc." ;
  cims:stereotype "enum" .

cim:Currency.DKK a cim:Currency ;
  rdfs:label "DKK"@en ;
  rdfs:comment "Danish krone." ;
  cims:stereotype "enum" .

cim:Currency.DOP a cim:Currency ;
  rdfs:label "DOP"@en ;
  rdfs:comment "Dominican peso." ;
  cims:stereotype "enum" .

cim:Currency.DZD a cim:Currency ;
  rdfs:label "DZD"@en ;
  rdfs:comment "Algerian dinar." ;
  cims:stereotype "enum" .

cim:Currency.EEK a cim:Currency ;
  rdfs:label "EEK"@en ;
  rdfs:comment "Estonian kroon." ;
  cims:stereotype "enum" .

cim:Currency.EGP a cim:Currency ;
  rdfs:label "EGP"@en ;
  rdfs:comment "Egyptian pound." ;
  cims:stereotype "enum" .

cim:Currency.ERN a cim:Currency ;
  rdfs:label "ERN"@en ;
  rdfs:comment "Eritrean nakfa." ;
  cims:stereotype "enum" .

cim:Currency.ETB a cim:Currency ;
  rdfs:label "ETB"@en ;
  rdfs:comment "Ethiopian birr." ;
  cims:stereotype "enum" .

cim:Currency.EUR a cim:Currency ;
  rdfs:label "EUR"@en ;
  rdfs:comment "Euro." ;
  cims:stereotype "enum" .

cim:Currency.FJD a cim:Currency ;
  rdfs:label "FJD"@en ;
  rdfs:comment "Fiji dollar." ;
  cims:stereotype "enum" .

cim:Currency.FKP a cim:Currency ;
  rdfs:label "FKP"@en ;
  rdfs:comment "Falkland Islands pound." ;
  cims:stereotype "enum" .

cim:Currency.GBP a cim:Currency ;
  rdfs:label "GBP"@en ;
  rdfs:comment "Pound sterling." ;
  cims:stereotype "enum" .

cim:Currency.GEL a cim:Currency ;
  rdfs:label "GEL"@en ;
  rdfs:comment "Georgian lari." ;
  cims:stereotype "enum" .

cim:Currency.GHS a cim:Currency ;
  rdfs:label "GHS"@en ;
  rdfs:comment "Ghanaian cedi." ;
  cims:stereotype "enum" .

cim:Currency.GIP a cim:Currency ;
  rdfs:label "GIP"@en ;
  rdfs:comment "Gibraltar pound." ;
  cims:stereotype "enum" .

cim:Currency.GMD a cim:Currency ;
  rdfs:label "GMD"@en ;
  rdfs:comment "Gambian dalasi." ;
  cims:stereotype "enum" .

cim:Currency.GNF a cim:Currency ;
  rdfs:label "GNF"@en ;
  rdfs:comment "Guinean franc." ;
  cims:stereotype "enum" .

cim:Currency.GTQ a cim:Currency ;
  rdfs:label "GTQ"@en ;
  rdfs:comment "Guatemalan quetzal." ;
  cims:stereotype "enum" .

cim:Currency.GYD a cim:Currency ;
  rdfs:label "GYD"@en ;
  rdfs:comment "Guyanese dollar." ;
  cims:stereotype "enum" .

cim:Currency.HKD a cim:Currency ;
  rdfs:label "HKD"@en ;
  rdfs:comment "Hong Kong dollar." ;
  cims:stereotype "enum" .

cim:Currency.HNL a cim:Currency ;
  rdfs:label "HNL"@en ;
  rdfs:comment "Honduran lempira." ;
  cims:stereotype "enum" .

cim:Currency.HRK a cim:Currency ;
  rdfs:label "HRK"@en ;
  rdfs:comment "Croatian kuna." ;
  cims:stereotype "enum" .

cim:Currency.HTG a cim:Currency ;
  rdfs:label "HTG"@en ;
  rdfs:comment "Haitian gourde." ;
  cims:stereotype "enum" .

cim:Currency.HUF a cim:Currency ;
  rdfs:label "HUF"@en ;
  rdfs:comment "Hungarian forint." ;
  cims:stereotype "enum" .

cim:Currency.IDR a cim:Currency ;
  rdfs:label "IDR"@en ;
  rdfs:comment "Indonesian rupiah." ;
  cims:stereotype "enum" .

cim:Currency.ILS a cim:Currency ;
  rdfs:label "ILS"@en ;
  rdfs:comment "Israeli new sheqel." ;
  cims:stereotype "enum" .

cim:Currency.INR a cim:Currency ;
  rdfs:label "INR"@en ;
  rdfs:comment "Indian rupee." ;
  cims:stereotype "enum" .

cim:Currency.IQD a cim:Currency ;
  rdfs:label "IQD"@en ;
  rdfs:comment "Iraqi dinar." ;
  cims:stereotype "enum" .

cim:Currency.IRR a cim:Currency ;
  rdfs:label "IRR"@en ;
  rdfs:comment "Iranian rial." ;
  cims:stereotype "enum" .

cim:Currency.ISK a cim:Currency ;
  rdfs:label "ISK"@en ;
  rdfs:comment "Icelandic króna." ;
  cims:stereotype "enum" .

cim:Currency.JMD a cim:Currency ;
  rdfs:label "JMD"@en ;
  rdfs:comment "Jamaican dollar." ;
  cims:stereotype "enum" .

cim:Currency.JOD a cim:Currency ;
  rdfs:label "JOD"@en ;
  rdfs:comment "Jordanian dinar." ;
  cims:stereotype "enum" .

cim:Currency.JPY a cim:Currency ;
  rdfs:label "JPY"@en ;
  rdfs:comment "Japanese yen." ;
  cims:stereotype "enum" .

cim:Currency.KES a cim:Currency ;
  rdfs:label "KES"@en ;
  rdfs:comment "Kenyan shilling." ;
  cims:stereotype "enum" .

cim:Currency.KGS a cim:Currency ;
  rdfs:label "KGS"@en ;
  rdfs:comment "Kyrgyzstani som." ;
  cims:stereotype "enum" .

cim:Currency.KHR a cim:Currency ;
  rdfs:label "KHR"@en ;
  rdfs:comment "Cambodian riel." ;
  cims:stereotype "enum" .

cim:Currency.KMF a cim:Currency ;
  rdfs:label "KMF"@en ;
  rdfs:comment "Comoro franc." ;
  cims:stereotype "enum" .

cim:Currency.KPW a cim:Currency ;
  rdfs:label "KPW"@en ;
  rdfs:comment "North Korean won." ;
  cims:stereotype "enum" .

cim:Currency.KRW a cim:Currency ;
  rdfs:label "KRW"@en ;
  rdfs:comment "South Korean won." ;
  cims:stereotype "enum" .

cim:Currency.KWD a cim:Currency ;
  rdfs:label "KWD"@en ;
  rdfs:comment "Kuwaiti dinar." ;
  cims:stereotype "enum" .

cim:Currency.KYD a cim:Currency ;
  rdfs:label "KYD"@en ;
  rdfs:comment "Cayman Islands dollar." ;
  cims:stereotype "enum" .

cim:Currency.KZT a cim:Currency ;
  rdfs:label "KZT"@en ;
  rdfs:comment "Kazakhstani tenge." ;
  cims:stereotype "enum" .

cim:Currency.LAK a cim:Currency ;
  rdfs:label "LAK"@en ;
  rdfs:comment "Lao kip." ;
  cims:stereotype "enum" .

cim:Currency.LBP a cim:Currency ;
  rdfs:label "LBP"@en ;
  rdfs:comment "Lebanese pound." ;
  cims:stereotype "enum" .

cim:Currency.LKR a cim:Currency ;
  rdfs:label "LKR"@en ;
  rdfs:comment "Sri Lanka rupee." ;
  cims:stereotype "enum" .

cim:Currency.LRD a cim:Currency ;
  rdfs:label "LRD"@en ;
  rdfs:comment "Liberian dollar." ;
  cims:stereotype "enum" .

cim:Currency.LSL a cim:Currency ;
  rdfs:label "LSL"@en ;
  rdfs:comment "Lesotho loti." ;
  cims:stereotype "enum" .

cim:Currency.LTL a cim:Currency ;
  rdfs:label "LTL"@en ;
  rdfs:comment "Lithuanian litas." ;
  cims:stereotype "enum" .

cim:Currency.LVL a cim:Currency ;
  rdfs:label "LVL"@en ;
  rdfs:comment "Latvian lats." ;
  cims:stereotype "enum" .

cim:Currency.LYD a cim:Currency ;
  rdfs:label "LYD"@en ;
  rdfs:comment "Libyan dinar." ;
  cims:stereotype "enum" .

cim:Currency.MAD a cim:Currency ;
  rdfs:label "MAD"@en ;
  rdfs:comment "Moroccan dirham." ;
  cims:stereotype "enum" .

cim:Currency.MDL a cim:Currency ;
  rdfs:label "MDL"@en ;
  rdfs:comment "Moldovan leu." ;
  cims:stereotype "enum" .

cim:Currency.MGA a cim:Currency ;
  rdfs:label "MGA"@en ;
  rdfs:comment "Malagasy ariary." ;
  cims:stereotype "enum" .

cim:Currency.MKD a cim:Currency ;
  rdfs:label "MKD"@en ;
  rdfs:comment "Macedonian denar." ;
  cims:stereotype "enum" .

cim:Currency.MMK a cim:Currency ;
  rdfs:label "MMK"@en ;
  rdfs:comment "Myanma kyat." ;
  cims:stereotype "enum" .

cim:Currency.MNT a cim:Currency ;
  rdfs:label "MNT"@en ;
  rdfs:comment "Mongolian tugrik." ;
  cims:stereotype "enum" .

cim:Currency.MOP a cim:Currency ;
  rdfs:label "MOP"@en ;
  rdfs:comment "Macanese pataca." ;
  cims:stereotype "enum" .

cim:Currency.MRO a cim:Currency ;
  rdfs:label "MRO"@en ;
  rdfs:comment "Mauritanian ouguiya." ;
  cims:stereotype "enum" .

cim:Currency.MUR a cim:Currency ;
  rdfs:label "MUR"@en ;
  rdfs:comment "Mauritian rupee." ;
  cims:stereotype "enum" .

cim:Currency.MVR a cim:Currency ;
  rdfs:label "MVR"@en ;
  rdfs:comment "Maldivian rufiyaa." ;
  cims:stereotype "enum" .

cim:Currency.MWK a cim:Currency ;
  rdfs:label "MWK"@en ;
  rdfs:comment "Malawian kwacha." ;
  cims:stereotype "enum" .

cim:Currency.MXN a cim:Currency ;
  rdfs:label "MXN"@en ;
  rdfs:comment "Mexican peso." ;
  cims:stereotype "enum" .

cim:Currency.MYR a cim:Currency ;
  rdfs:label "MYR"@en ;
  rdfs:comment "Malaysian ringgit." ;
  cims:stereotype "enum" .

cim:Currency.MZN a cim:Currency ;
  rdfs:label "MZN"@en ;
  rdfs:comment "Mozambican metical." ;
  cims:stereotype "enum" .

cim:Currency.NAD a cim:Currency ;
  rdfs:label "NAD"@en ;
  rdfs:comment "Namibian dollar." ;
  cims:stereotype "enum" .

cim:Currency.NGN a cim:Currency ;
  rdfs:label "NGN"@en ;
  rdfs:comment "Nigerian naira." ;
  cims:stereotype "enum" .

cim:Currency.NIO a cim:Currency ;
  rdfs:label "NIO"@en ;
  rdfs:comment "Cordoba oro." ;
  cims:stereotype "enum" .

cim:Currency.NOK a cim:Currency ;
  rdfs:label "NOK"@en ;
  rdfs:comment "Norwegian krone." ;
  cims:stereotype "enum" .

cim:Currency.NPR a cim:Currency ;
  rdfs:label "NPR"@en ;
  rdfs:comment "Nepalese rupee." ;
  cims:stereotype "enum" .

cim:Currency.NZD a cim:Currency ;
  rdfs:label "NZD"@en ;
  rdfs:comment "New Zealand dollar." ;
  cims:stereotype "enum" .

cim:Currency.OMR a cim:Currency ;
  rdfs:label "OMR"@en ;
  rdfs:comment "Omani rial." ;
  cims:stereotype "enum" .

cim:Currency.PAB a cim:Currency ;
  rdfs:label "PAB"@en ;
  rdfs:comment "Panamanian balboa." ;
  cims:stereotype "enum" .

cim:Currency.PEN a cim:Currency ;
  rdfs:label "PEN"@en ;
  rdfs:comment "Peruvian nuevo sol." ;
  cims:stereotype "enum" .

cim:Currency.PGK a cim:Currency ;
  rdfs:label "PGK"@en ;
  rdfs:comment "Papua New Guinean kina." ;
  cims:stereotype "enum" .

cim:Currency.PHP a cim:Currency ;
  rdfs:label "PHP"@en ;
  rdfs:comment "Philippine peso." ;
  cims:stereotype "enum" .

cim:Currency.PKR a cim:Currency ;
  rdfs:label "PKR"@en ;
  rdfs:comment "Pakistani rupee." ;
  cims:stereotype "enum" .

cim:Currency.PLN a cim:Currency ;
  rdfs:label "PLN"@en ;
  rdfs:comment "Polish zloty." ;
  cims:stereotype "enum" .

cim:Currency.PYG a cim:Currency ;
  rdfs:label "PYG"@en ;
  rdfs:comment "Paraguayan guaraní." ;
  cims:stereotype "enum" .

cim:Currency.QAR a cim:Currency ;
  rdfs:label "QAR"@en ;
  rdfs:comment "Qatari rial." ;
  cims:stereotype "enum" .

cim:Currency.RON a cim:Currency ;
  rdfs:label "RON"@en ;
  rdfs:comment "Romanian new leu." ;
  cims:stereotype "enum" .

cim:Currency.RSD a cim:Currency ;
  rdfs:label "RSD"@en ;
  rdfs:comment "Serbian dinar." ;
  cims:stereotype "enum" .

cim:Currency.RUB a cim:Currency ;
  rdfs:label "RUB"@en ;
  rdfs:comment "Russian rouble." ;
  cims:stereotype "enum" .

cim:Currency.RWF a cim:Currency ;
  rdfs:label "RWF"@en ;
  rdfs:comment "Rwandan franc." ;
  cims:stereotype "enum" .

cim:Currency.SAR a cim:Currency ;
  rdfs:label "SAR"@en ;
  rdfs:comment "Saudi riyal." ;
  cims:stereotype "enum" .

cim:Currency.SBD a cim:Currency ;
  rdfs:label "SBD"@en ;
  rdfs:comment "Solomon Islands dollar." ;
  cims:stereotype "enum" .

cim:Currency.SCR a cim:Currency ;
  rdfs:label "SCR"@en ;
  rdfs:comment "Seychelles rupee." ;
  cims:stereotype "enum" .

cim:Currency.SDG a cim:Currency ;
  rdfs:label "SDG"@en ;
  rdfs:comment "Sudanese pound." ;
  cims:stereotype "enum" .

cim:Currency.SEK a cim:Currency ;
  rdfs:label "SEK"@en ;
  rdfs:comment "Swedish krona/kronor." ;
  cims:stereotype "enum" .

cim:Currency.SGD a cim:Currency ;
  rdfs:label "SGD"@en ;
  rdfs:comment "Singapore dollar." ;
  cims:stereotype "enum" .

cim:Currency.SHP a cim:Currency ;
  rdfs:label "SHP"@en ;
  rdfs:comment "Saint Helena pound." ;
  cims:stereotype "enum" .

cim:Currency.SLL a cim:Currency ;
  rdfs:label "SLL"@en ;
  rdfs:comment "Sierra Leonean leone." ;
  cims:stereotype "enum" .

cim:Currency.SOS a cim:Currency ;
  rdfs:label "SOS"@en ;
  rdfs:comment "Somali shilling." ;
  cims:stereotype "enum" .

cim:Currency.SRD a cim:Currency ;
  rdfs:label "SRD"@en ;
  rdfs:comment "Surinamese dollar." ;
  cims:stereotype "enum" .

cim:Currency.STD a cim:Currency ;
  rdfs:label "STD"@en ;
  rdfs:comment "São Tomé and Príncipe dobra." ;
  cims:stereotype "enum" .

cim:Currency.SYP a cim:Currency ;
  rdfs:label "SYP"@en ;
  rdfs:comment "Syrian pound." ;
  cims:stereotype "enum" .

cim:Currency.SZL a cim:Currency ;
  rdfs:label "SZL"@en ;
  rdfs:comment "Lilangeni." ;
  cims:stereotype "enum" .

cim:Currency.THB a cim:Currency ;
  rdfs:label "THB"@en ;
  rdfs:comment "Thai baht." ;
  cims:stereotype "enum" .

cim:Currency.TJS a cim:Currency ;
  rdfs:label "TJS"@en ;
  rdfs:comment "Tajikistani somoni." ;
  cims:stereotype "enum" .

cim:Currency.TMT a cim:Currency ;
  rdfs:label "TMT"@en ;
  rdfs:comment "Turkmenistani manat." ;
  cims:stereotype "enum" .

cim:Currency.TND a cim:Currency ;
  rdfs:label "TND"@en ;
  rdfs:comment "Tunisian dinar." ;
  cims:stereotype "enum" .

cim:Currency.TOP a cim:Currency ;
  rdfs:label "TOP"@en ;
  rdfs:comment "Tongan pa'anga." ;
  cims:stereotype "enum" .

cim:Currency.TRY a cim:Currency ;
  rdfs:label "TRY"@en ;
  rdfs:comment "Turkish lira." ;
  cims:stereotype "enum" .

cim:Currency.TTD a cim:Currency ;
  rdfs:label "TTD"@en ;
  rdfs:comment "Trinidad and Tobago dollar." ;
  cims:stereotype "enum" .

cim:Currency.TWD a cim:Currency ;
  rdfs:label "TWD"@en ;
  rdfs:comment "New Taiwan dollar." ;
  cims:stereotype "enum" .

cim:Currency.TZS a cim:Currency ;
  rdfs:label "TZS"@en ;
  rdfs:comment "Tanzanian shilling." ;
  cims:stereotype "enum" .

cim:Currency.UAH a cim:Currency ;
  rdfs:label "UAH"@en ;
  rdfs:comment "Ukrainian hryvnia." ;
  cims:stereotype "enum" .

cim:Currency.UGX a cim:Currency ;
  rdfs:label "UGX"@en ;
  rdfs:comment "Ugandan shilling." ;
  cims:stereotype "enum" .

cim:Currency.USD a cim:Currency ;
  rdfs:label "USD"@en ;
  rdfs:comment "United States dollar." ;
  cims:stereotype "enum" .

cim:Currency.UYU a cim:Currency ;
  rdfs:label "UYU"@en ;
  rdfs:comment "Uruguayan peso." ;
  cims:stereotype "enum" .

cim:Currency.UZS a cim:Currency ;
  rdfs:label "UZS"@en ;
  rdfs:comment "Uzbekistan som." ;
  cims:stereotype "enum" .

cim:Currency.VEF a cim:Currency ;
  rdfs:label "VEF"@en ;
  rdfs:comment "Venezuelan bolívar fuerte." ;
  cims:stereotype "enum" .

cim:Currency.VND a cim:Currency ;
  rdfs:label "VND"@en ;
  rdfs:comment "Vietnamese Dong." ;
  cims:stereotype "enum" .

cim:Currency.VUV a cim:Currency ;
  rdfs:label "VUV"@en ;
  rdfs:comment "Vanuatu vatu." ;
  cims:stereotype "enum" .

cim:Currency.WST a cim:Currency ;
  rdfs:label "WST"@en ;
  rdfs:comment "Samoan tala." ;
  cims:stereotype "enum" .

cim:Currency.XAF a cim:Currency ;
  rdfs:label "XAF"@en ;
  rdfs:comment "CFA franc BEAC." ;
  cims:stereotype "enum" .

cim:Currency.XCD a cim:Currency ;
  rdfs:label "XCD"@en ;
  rdfs:comment "East Caribbean dollar." ;
  cims:stereotype "enum" .

cim:Currency.XOF a cim:Currency ;
  rdfs:label "XOF"@en ;
  rdfs:comment "CFA Franc BCEAO." ;
  cims:stereotype "enum" .

cim:Currency.XPF a cim:Currency ;
  rdfs:label "XPF"@en ;
  rdfs:comment "CFP franc." ;
  cims:stereotype "enum" .

cim:Currency.YER a cim:Currency ;
  rdfs:label "YER"@en ;
  rdfs:comment "Yemeni rial." ;
  cims:stereotype "enum" .

cim:Currency.ZAR a cim:Currency ;
  rdfs:label "ZAR"@en ;
  rdfs:comment "South African rand." ;
  cims:stereotype "enum" .

cim:Currency.ZMK a cim:Currency ;
  rdfs:label "ZMK"@en ;
  rdfs:comment "Zambian kwacha." ;
  cims:stereotype "enum" .

cim:Currency.ZWL a cim:Currency ;
  rdfs:label "ZWL"@en ;
  rdfs:comment "Zimbabwe dollar." ;
  cims:stereotype "enum" .

cim:CurveStyle.constantYValue a cim:CurveStyle ;
  rdfs:label "constantYValue"@en ;
  rdfs:comment "The Y-axis values are assumed constant until the next curve point and prior to the first curve point." ;
  cims:stereotype "enum" .

cim:CurveStyle.straightLineYValues a cim:CurveStyle ;
  rdfs:label "straightLineYValues"@en ;
  rdfs:comment "The Y-axis values are assumed to be a straight line between values.  Also known as linear interpolation." ;
  cims:stereotype "enum" .

cim:DCConverterOperatingModeKind.bipolar a cim:DCConverterOperatingModeKind ;
  rdfs:label "bipolar"@en ;
  rdfs:comment "Bipolar operation." ;
  cims:stereotype "enum" .

cim:DCConverterOperatingModeKind.monopolarGroundReturn a cim:DCConverterOperatingModeKind ;
  rdfs:label "monopolarGroundReturn"@en ;
  rdfs:comment "Monopolar operation with ground return." ;
  cims:stereotype "enum" .

cim:DCConverterOperatingModeKind.monopolarMetallicReturn a cim:DCConverterOperatingModeKind ;
  rdfs:label "monopolarMetallicReturn"@en ;
  rdfs:comment "Monopolar operation with metallic return." ;
  cims:stereotype "enum" .

cim:DCPolarityKind.middle a cim:DCPolarityKind ;
  rdfs:label "middle"@en ;
  rdfs:comment "Middle pole. The converter terminal is the midpoint in a bipolar or symmetric monopole configuration. The midpoint can be grounded and/or have a metallic return." ;
  cims:stereotype "enum" .

cim:DCPolarityKind.negative a cim:DCPolarityKind ;
  rdfs:label "negative"@en ;
  rdfs:comment "Negative pole. The converter terminal is intended to operate at a negative voltage relative the midpoint or positive terminal." ;
  cims:stereotype "enum" .

cim:DCPolarityKind.positive a cim:DCPolarityKind ;
  rdfs:label "positive"@en ;
  rdfs:comment "Positive pole. The converter terminal is intended to operate at a positive voltage relative the midpoint or negative terminal." ;
  cims:stereotype "enum" .

cim:FuelType.brownCoalLignite a cim:FuelType ;
  rdfs:label "brownCoalLignite"@en ;
  rdfs:comment "Brown coal lignite." ;
  cims:stereotype "enum" .

cim:FuelType.coal a cim:FuelType ;
  rdfs:label "coal"@en ;
  rdfs:comment "Generic coal, not including lignite type." ;
  cims:stereotype "enum" .

cim:FuelType.coalDerivedGas a cim:FuelType ;
  rdfs:label "coalDerivedGas"@en ;
  rdfs:comment "Coal derived gas." ;
  cims:stereotype "enum" .

cim:FuelType.gas a cim:FuelType ;
  rdfs:label "gas"@en ;
  rdfs:comment "Natural gas." ;
  cims:stereotype "enum" .

cim:FuelType.hardCoal a cim:FuelType ;
  rdfs:label "hardCoal"@en ;
  rdfs:comment "Hard coal." ;
  cims:stereotype "enum" .

cim:FuelType.lignite a cim:FuelType ;
  rdfs:label "lignite"@en ;
  rdfs:comment "The fuel is lignite coal.  Note that this is a special type of coal, so the other enum of coal is reserved for hard coal types or if the exact type of coal is not known." ;
  cims:stereotype "enum" .

cim:FuelType.oil a cim:FuelType ;
  rdfs:label "oil"@en ;
  rdfs:comment "Oil." ;
  cims:stereotype "enum" .

cim:FuelType.oilShale a cim:FuelType ;
  rdfs:label "oilShale"@en ;
  rdfs:comment "Oil Shale." ;
  cims:stereotype "enum" .

cim:FuelType.other a cim:FuelType ;
  rdfs:label "other"@en ;
  rdfs:comment "Any fuel type not included in the rest of the enumerated value." ;
  cims:stereotype "enum" .

cim:FuelType.peat a cim:FuelType ;
  rdfs:label "peat"@en ;
  rdfs:comment "Peat." ;
  cims:stereotype "enum" .

cim:GeneratorControlSource.offAGC a cim:GeneratorControlSource ;
  rdfs:label "offAGC"@en ;
  rdfs:comment "Off of automatic generation control (AGC)." ;
  cims:stereotype "enum" .

cim:GeneratorControlSource.onAGC a cim:GeneratorControlSource ;
  rdfs:label "onAGC"@en ;
  rdfs:comment "On automatic generation control (AGC)." ;
  cims:stereotype "enum" .

cim:GeneratorControlSource.plantControl a cim:GeneratorControlSource ;
  rdfs:label "plantControl"@en ;
  rdfs:comment "Plant is controlling." ;
  cims:stereotype "enum" .

cim:GeneratorControlSource.unavailable a cim:GeneratorControlSource ;
  rdfs:label "unavailable"@en ;
  rdfs:comment "Not available." ;
  cims:stereotype "enum" .

cim:HydroEnergyConversionKind.generator a cim:HydroEnergyConversionKind ;
  rdfs:label "generator"@en ;
  rdfs:comment "Able to generate power, but not able to pump water for energy storage." ;
  cims:stereotype "enum" .

cim:HydroEnergyConversionKind.pumpAndGenerator a cim:HydroEnergyConversionKind ;
  rdfs:label "pumpAndGenerator"@en ;
  rdfs:comment "Able to both generate power and pump water for energy storage." ;
  cims:stereotype "enum" .

cim:HydroPlantStorageKind.pumpedStorage a cim:HydroPlantStorageKind ;
  rdfs:label "pumpedStorage"@en ;
  rdfs:comment "Pumped storage." ;
  cims:stereotype "enum" .

cim:HydroPlantStorageKind.runOfRiver a cim:HydroPlantStorageKind ;
  rdfs:label "runOfRiver"@en ;
  rdfs:comment "Run of river." ;
  cims:stereotype "enum" .

cim:HydroPlantStorageKind.storage a cim:HydroPlantStorageKind ;
  rdfs:label "storage"@en ;
  rdfs:comment "Storage." ;
  cims:stereotype "enum" .

cim:HydroTurbineKind.francis a cim:HydroTurbineKind ;
  rdfs:label "francis"@en ;
  rdfs:comment "Francis." ;
  cims:stereotype "enum" .

cim:HydroTurbineKind.kaplan a cim:HydroTurbineKind ;
  rdfs:label "kaplan"@en ;
  rdfs:comment "Kaplan." ;
  cims:stereotype "enum" .

cim:HydroTurbineKind.pelton a cim:HydroTurbineKind ;
  rdfs:label "pelton"@en ;
  rdfs:comment "Pelton." ;
  cims:stereotype "enum" .

cim:OperationalLimitDirectionKind.absoluteValue a cim:OperationalLimitDirectionKind ;
  rdfs:label "absoluteValue"@en ;
  rdfs:comment "An absoluteValue limit means that a monitored absolute value above the limit value is a violation." ;
  cims:stereotype "enum" .

cim:OperationalLimitDirectionKind.high a cim:OperationalLimitDirectionKind ;
  rdfs:label "high"@en ;
  rdfs:comment "High means that a monitored value above the limit value is a violation.   If applied to a terminal flow, the positive direction is into the terminal." ;
  cims:stereotype "enum" .

cim:OperationalLimitDirectionKind.low a cim:OperationalLimitDirectionKind ;
  rdfs:label "low"@en ;
  rdfs:comment "Low means a monitored value below the limit is a violation.  If applied to a terminal flow, the positive direction is into the terminal." ;
  cims:stereotype "enum" .

cim:PhaseCode.A a cim:PhaseCode ;
  rdfs:label "A"@en ;
  rdfs:comment "Phase A." ;
  cims:stereotype "enum" .

cim:PhaseCode.AB a cim:PhaseCode ;
  rdfs:label "AB"@en ;
  rdfs:comment "Phases A and B." ;
  cims:stereotype "enum" .

cim:PhaseCode.ABC a cim:PhaseCode ;
  rdfs:label "ABC"@en ;
  rdfs:comment "Phases A, B, and C." ;
  cims:stereotype "enum" .

cim:PhaseCode.ABCN a cim:PhaseCode ;
  rdfs:label "ABCN"@en ;
  rdfs:comment "Phases A, B, C, and N." ;
  cims:stereotype "enum" .

cim:PhaseCode.ABN a cim:PhaseCode ;
  rdfs:label "ABN"@en ;
  rdfs:comment "Phases A, B, and neutral." ;
  cims:stereotype "enum" .

cim:PhaseCode.AC a cim:PhaseCode ;
  rdfs:label "AC"@en ;
  rdfs:comment "Phases A and C." ;
  cims:stereotype "enum" .

cim:PhaseCode.ACN a cim:PhaseCode ;
  rdfs:label "ACN"@en ;
  rdfs:comment "Phases A, C and neutral." ;
  cims:stereotype "enum" .

cim:PhaseCode.AN a cim:PhaseCode ;
  rdfs:label "AN"@en ;
  rdfs:comment "Phases A and neutral." ;
  cims:stereotype "enum" .

cim:PhaseCode.B a cim:PhaseCode ;
  rdfs:label "B"@en ;
  rdfs:comment "Phase B." ;
  cims:stereotype "enum" .

cim:PhaseCode.BC a cim:PhaseCode ;
  rdfs:label "BC"@en ;
  rdfs:comment "Phases B and C." ;
  cims:stereotype "enum" .

cim:PhaseCode.BCN a cim:PhaseCode ;
  rdfs:label "BCN"@en ;
  rdfs:comment "Phases B, C, and neutral." ;
  cims:stereotype "enum" .

cim:PhaseCode.BN a cim:PhaseCode ;
  rdfs:label "BN"@en ;
  rdfs:comment "Phases B and neutral." ;
  cims:stereotype "enum" .

cim:PhaseCode.C a cim:PhaseCode ;
  rdfs:label "C"@en ;
  rdfs:comment "Phase C." ;
  cims:stereotype "enum" .

cim:PhaseCode.CN a cim:PhaseCode ;
  rdfs:label "CN"@en ;
  rdfs:comment "Phases C and neutral." ;
  cims:stereotype "enum" .

cim:PhaseCode.N a cim:PhaseCode ;
  rdfs:label "N"@en ;
  rdfs:comment "Neutral phase." ;
  cims:stereotype "enum" .

cim:PhaseCode.X a cim:PhaseCode ;
  rdfs:label "X"@en ;
  rdfs:comment "Unknown non-neutral phase." ;
  cims:stereotype "enum" .

cim:PhaseCode.XN a cim:PhaseCode ;
  rdfs:label "XN"@en ;
  rdfs:comment "Unknown non-neutral phase plus neutral." ;
  cims:stereotype "enum" .

cim:PhaseCode.XY a cim:PhaseCode ;
  rdfs:label "XY"@en ;
  rdfs:comment "Two unknown non-neutral phases." ;
  cims:stereotype "enum" .

cim:PhaseCode.XYN a cim:PhaseCode ;
  rdfs:label "XYN"@en ;
  rdfs:comment "Two unknown non-neutral phases plus neutral." ;
  cims:stereotype "enum" .

cim:PhaseCode.none a cim:PhaseCode ;
  rdfs:label "none"@en ;
  rdfs:comment "No phases specified." ;
  cims:stereotype "enum" .

cim:PhaseCode.s1 a cim:PhaseCode ;
  rdfs:label "s1"@en ;
  rdfs:comment "Secondary phase 1." ;
  cims:stereotype "enum" .

cim:PhaseCode.s12 a cim:PhaseCode ;
  rdfs:label "s12"@en ;
  rdfs:comment "Secondary phase 1 and 2." ;
  cims:stereotype "enum" .

cim:PhaseCode.s12N a cim:PhaseCode ;
  rdfs:label "s12N"@en ;
  rdfs:comment "Secondary phases 1, 2, and neutral." ;
  cims:stereotype "enum" .

cim:PhaseCode.s1N a cim:PhaseCode ;
  rdfs:label "s1N"@en ;
  rdfs:comment "Secondary phase 1 and neutral." ;
  cims:stereotype "enum" .

cim:PhaseCode.s2 a cim:PhaseCode ;
  rdfs:label "s2"@en ;
  rdfs:comment "Secondary phase 2." ;
  cims:stereotype "enum" .

cim:PhaseCode.s2N a cim:PhaseCode ;
  rdfs:label "s2N"@en ;
  rdfs:comment "Secondary phase 2 and neutral." ;
  cims:stereotype "enum" .

cim:RegulatingControlModeKind.activePower a cim:RegulatingControlModeKind ;
  rdfs:label "activePower"@en ;
  rdfs:comment "Active power is specified." ;
  cims:stereotype "enum" .

cim:RegulatingControlModeKind.admittance a cim:RegulatingControlModeKind ;
  rdfs:label "admittance"@en ;
  rdfs:comment "Admittance is specified." ;
  cims:stereotype "enum" .

cim:RegulatingControlModeKind.currentFlow a cim:RegulatingControlModeKind ;
  rdfs:label "currentFlow"@en ;
  rdfs:comment "Current flow is specified." ;
  cims:stereotype "enum" .

cim:RegulatingControlModeKind.powerFactor a cim:RegulatingControlModeKind ;
  rdfs:label "powerFactor"@en ;
  rdfs:comment "Power factor is specified." ;
  cims:stereotype "enum" .

cim:RegulatingControlModeKind.reactivePower a cim:RegulatingControlModeKind ;
  rdfs:label "reactivePower"@en ;
  rdfs:comment "Reactive power is specified." ;
  cims:stereotype "enum" .

cim:RegulatingControlModeKind.temperature a cim:RegulatingControlModeKind ;
  rdfs:label "temperature"@en ;
  rdfs:comment "Control switches on/off based on the local temperature (i.e., a thermostat)." ;
  cims:stereotype "enum" .

cim:RegulatingControlModeKind.timeScheduled a cim:RegulatingControlModeKind ;
  rdfs:label "timeScheduled"@en ;
  rdfs:comment "Control switches on/off by time of day. The times may change on the weekend, or in different seasons." ;
  cims:stereotype "enum" .

cim:RegulatingControlModeKind.voltage a cim:RegulatingControlModeKind ;
  rdfs:label "voltage"@en ;
  rdfs:comment "Voltage is specified." ;
  cims:stereotype "enum" .

cim:SVCControlMode.reactivePower a cim:SVCControlMode ;
  rdfs:label "reactivePower"@en ;
  rdfs:comment "Reactive power control." ;
  cims:stereotype "enum" .

cim:SVCControlMode.voltage a cim:SVCControlMode ;
  rdfs:label "voltage"@en ;
  rdfs:comment "Voltage control." ;
  cims:stereotype "enum" .

cim:SynchronousMachineKind.condenser a cim:SynchronousMachineKind ;
  rdfs:label "condenser"@en ;
  rdfs:comment "Indicates the synchronous machine can operate as a condenser." ;
  cims:stereotype "enum" .

cim:SynchronousMachineKind.generator a cim:SynchronousMachineKind ;
  rdfs:label "generator"@en ;
  rdfs:comment "Indicates the synchronous machine can operate as a generator." ;
  cims:stereotype "enum" .

cim:SynchronousMachineKind.generatorOrCondenser a cim:SynchronousMachineKind ;
  rdfs:label "generatorOrCondenser"@en ;
  rdfs:comment "Indicates the synchronous machine can operate as a generator or as a condenser." ;
  cims:stereotype "enum" .

cim:SynchronousMachineKind.generatorOrCondenserOrMotor a cim:SynchronousMachineKind ;
  rdfs:label "generatorOrCondenserOrMotor"@en ;
  rdfs:comment "Indicates the synchronous machine can operate as a generator or as a condenser or as a motor." ;
  cims:stereotype "enum" .

cim:SynchronousMachineKind.generatorOrMotor a cim:SynchronousMachineKind ;
  rdfs:label "generatorOrMotor"@en ;
  rdfs:comment "Indicates the synchronous machine can operate as a generator or as a motor." ;
  cims:stereotype "enum" .

cim:SynchronousMachineKind.motor a cim:SynchronousMachineKind ;
  rdfs:label "motor"@en ;
  rdfs:comment "Indicates the synchronous machine can operate as a motor." ;
  cims:stereotype "enum" .

cim:SynchronousMachineKind.motorOrCondenser a cim:SynchronousMachineKind ;
  rdfs:label "motorOrCondenser"@en ;
  rdfs:comment "Indicates the synchronous machine can operate as a motor or as a condenser." ;
  cims:stereotype "enum" .

cim:UnitMultiplier.E a cim:UnitMultiplier ;
  rdfs:label "E"@en ;
  rdfs:comment "Exa 10**18." ;
  cims:stereotype "enum" .

cim:UnitMultiplier.G a cim:UnitMultiplier ;
  rdfs:label "G"@en ;
  rdfs:comment "Giga 10**9." ;
  cims:stereotype "enum" .

cim:UnitMultiplier.M a cim:UnitMultiplier ;
  rdfs:label "M"@en ;
  rdfs:comment "Mega 10**6." ;
  cims:stereotype "enum" .

cim:UnitMultiplier.P a cim:UnitMultiplier ;
  rdfs:label "P"@en ;
  rdfs:comment "Peta 10**15." ;
  cims:stereotype "enum" .

cim:UnitMultiplier.T a cim:UnitMultiplier ;
  rdfs:label "T"@en ;
  rdfs:comment "Tera 10**12." ;
  cims:stereotype "enum" .

cim:UnitMultiplier.Y a cim:UnitMultiplier ;
  rdfs:label "Y"@en ;
  rdfs:comment "Yotta 10**24." ;
  cims:stereotype "enum" .

cim:UnitMultiplier.Z a cim:UnitMultiplier ;
  rdfs:label "Z"@en ;
  rdfs:comment "Zetta 10**21." ;
  cims:stereotype "enum" .

cim:UnitMultiplier.a a cim:UnitMultiplier ;
  rdfs:label "a"@en ;
  rdfs:comment "Atto 10**-18." ;
  cims:stereotype "enum" .

cim:UnitMultiplier.c a cim:UnitMultiplier ;
  rdfs:label "c"@en ;
  rdfs:comment "Centi 10**-2." ;
  cims:stereotype "enum" .

cim:UnitMultiplier.d a cim:UnitMultiplier ;
  rdfs:label "d"@en ;
  rdfs:comment "Deci 10**-1." ;
  cims:stereotype "enum" .

cim:UnitMultiplier.da a cim:UnitMultiplier ;
  rdfs:label "da"@en ;
  rdfs:comment "Deca 10**1." ;
  cims:stereotype "enum" .

cim:UnitMultiplier.f a cim:UnitMultiplier ;
  rdfs:label "f"@en ;
  rdfs:comment "Femto 10**-15." ;
  cims:stereotype "enum" .

cim:UnitMultiplier.h a cim:UnitMultiplier ;
  rdfs:label "h"@en ;
  rdfs:comment "Hecto 10**2." ;
  cims:stereotype "enum" .

cim:UnitMultiplier.k a cim:UnitMultiplier ;
  rdfs:label "k"@en ;
  rdfs:comment "Kilo 10**3." ;
  cims:stereotype "enum" .

cim:UnitMultiplier.m a cim:UnitMultiplier ;
  rdfs:label "m"@en ;
  rdfs:comment "Milli 10**-3." ;
  cims:stereotype "enum" .

cim:UnitMultiplier.micro a cim:UnitMultiplier ;
  rdfs:label "micro"@en ;
  rdfs:comment "Micro 10**-6." ;
  cims:stereotype "enum" .

cim:UnitMultiplier.n a cim:UnitMultiplier ;
  rdfs:label "n"@en ;
  rdfs:comment "Nano 10**-9." ;
  cims:stereotype "enum" .

cim:UnitMultiplier.none a cim:UnitMultiplier ;
  rdfs:label "none"@en ;
  rdfs:comment "No multiplier or equivalently multiply by 1." ;
  cims:stereotype "enum" .

cim:UnitMultiplier.p a cim:UnitMultiplier ;
  rdfs:label "p"@en ;
  rdfs:comment "Pico 10**-12." ;
  cims:stereotype "enum" .

cim:UnitMultiplier.y a cim:UnitMultiplier ;
  rdfs:label "y"@en ;
  rdfs:comment "Yocto 10**-24." ;
  cims:stereotype "enum" .

cim:UnitMultiplier.z a cim:UnitMultiplier ;
  rdfs:label "z"@en ;
  rdfs:comment "Zepto 10**-21." ;
  cims:stereotype "enum" .

cim:UnitSymbol.A a cim:UnitSymbol ;
  rdfs:label "A"@en ;
  rdfs:comment "Current in amperes." ;
  cims:stereotype "enum" .

cim:UnitSymbol.A2 a cim:UnitSymbol ;
  rdfs:label "A2"@en ;
  rdfs:comment "Amperes squared (A²)." ;
  cims:stereotype "enum" .

cim:UnitSymbol.A2h a cim:UnitSymbol ;
  rdfs:label "A2h"@en ;
  rdfs:comment "Ampere-squared hour, ampere-squared hour." ;
  cims:stereotype "enum" .

cim:UnitSymbol.A2s a cim:UnitSymbol ;
  rdfs:label "A2s"@en ;
  rdfs:comment "Ampere squared time in square amperes (A²s)." ;
  cims:stereotype "enum" .

cim:UnitSymbol.APerA a cim:UnitSymbol ;
  rdfs:label "APerA"@en ;
  rdfs:comment "Current, ratio of amperages.   Note: Users may need to supply a prefix such as ‘m’ to show rates such as ‘mA/A’." ;
  cims:stereotype "enum" .

cim:UnitSymbol.APerm a cim:UnitSymbol ;
  rdfs:label "APerm"@en ;
  rdfs:comment "A/m, magnetic field strength, amperes per metre." ;
  cims:stereotype "enum" .

cim:UnitSymbol.Ah a cim:UnitSymbol ;
  rdfs:label "Ah"@en ;
  rdfs:comment "Ampere-hours, ampere-hours." ;
  cims:stereotype "enum" .

cim:UnitSymbol.As a cim:UnitSymbol ;
  rdfs:label "As"@en ;
  rdfs:comment "Ampere seconds (A·s)." ;
  cims:stereotype "enum" .

cim:UnitSymbol.Bq a cim:UnitSymbol ;
  rdfs:label "Bq"@en ;
  rdfs:comment "Radioactivity in becquerels (1/s)." ;
  cims:stereotype "enum" .

cim:UnitSymbol.Btu a cim:UnitSymbol ;
  rdfs:label "Btu"@en ;
  rdfs:comment "Energy, British Thermal Units." ;
  cims:stereotype "enum" .

cim:UnitSymbol.C a cim:UnitSymbol ;
  rdfs:label "C"@en ;
  rdfs:comment "Electric charge in coulombs (A·s)." ;
  cims:stereotype "enum" .

cim:UnitSymbol.CPerkg a cim:UnitSymbol ;
  rdfs:label "CPerkg"@en ;
  rdfs:comment "Exposure (x rays), coulombs per kilogram." ;
  cims:stereotype "enum" .

cim:UnitSymbol.CPerm2 a cim:UnitSymbol ;
  rdfs:label "CPerm2"@en ;
  rdfs:comment "Surface charge density, coulombs per square metre." ;
  cims:stereotype "enum" .

cim:UnitSymbol.CPerm3 a cim:UnitSymbol ;
  rdfs:label "CPerm3"@en ;
  rdfs:comment "Electric charge density, coulombs per cubic metre." ;
  cims:stereotype "enum" .

cim:UnitSymbol.F a cim:UnitSymbol ;
  rdfs:label "F"@en ;
  rdfs:comment "Electric capacitance in farads (C/V)." ;
  cims:stereotype "enum" .

cim:UnitSymbol.FPerm a cim:UnitSymbol ;
  rdfs:label "FPerm"@en ;
  rdfs:comment "Permittivity, farads per metre." ;
  cims:stereotype "enum" .

cim:UnitSymbol.G a cim:UnitSymbol ;
  rdfs:label "G"@en ;
  rdfs:comment "Magnetic flux density, gausses (1 G = 10-4 T)." ;
  cims:stereotype "enum" .

cim:UnitSymbol.Gy a cim:UnitSymbol ;
  rdfs:label "Gy"@en ;
  rdfs:comment "Absorbed dose in grays (J/kg)." ;
  cims:stereotype "enum" .

cim:UnitSymbol.GyPers a cim:UnitSymbol ;
  rdfs:label "GyPers"@en ;
  rdfs:comment "Absorbed dose rate, grays per second." ;
  cims:stereotype "enum" .

cim:UnitSymbol.H a cim:UnitSymbol ;
  rdfs:label "H"@en ;
  rdfs:comment "Electric inductance in henrys (Wb/A)." ;
  cims:stereotype "enum" .

cim:UnitSymbol.HPerm a cim:UnitSymbol ;
  rdfs:label "HPerm"@en ;
  rdfs:comment "Permeability, henrys per metre." ;
  cims:stereotype "enum" .

cim:UnitSymbol.Hz a cim:UnitSymbol ;
  rdfs:label "Hz"@en ;
  rdfs:comment "Frequency in hertz (1/s)." ;
  cims:stereotype "enum" .

cim:UnitSymbol.HzPerHz a cim:UnitSymbol ;
  rdfs:label "HzPerHz"@en ;
  rdfs:comment "Frequency, rate of frequency change.   Note: Users may need to supply a prefix such as ‘m’ to show rates such as ‘mHz/Hz’." ;
  cims:stereotype "enum" .

cim:UnitSymbol.HzPers a cim:UnitSymbol ;
  rdfs:label "HzPers"@en ;
  rdfs:comment "Rate of change of frequency in hertz per second." ;
  cims:stereotype "enum" .

cim:UnitSymbol.J a cim:UnitSymbol ;
  rdfs:label "J"@en ;
  rdfs:comment "Energy in joules (N·m = C·V = W·s)." ;
  cims:stereotype "enum" .

cim:UnitSymbol.JPerK a cim:UnitSymbol ;
  rdfs:label "JPerK"@en ;
  rdfs:comment "Heat capacity in joules/kelvin." ;
  cims:stereotype "enum" .

cim:UnitSymbol.JPerkg a cim:UnitSymbol ;
  rdfs:label "JPerkg"@en ;
  rdfs:comment "Specific energy, Joules / kg." ;
  cims:stereotype "enum" .

cim:UnitSymbol.JPerkgK a cim:UnitSymbol ;
  rdfs:label "JPerkgK"@en ;
  rdfs:comment "Specific heat capacity, specific entropy, joules per kilogram Kelvin." ;
  cims:stereotype "enum" .

cim:UnitSymbol.JPerm2 a cim:UnitSymbol ;
  rdfs:label "JPerm2"@en ;
  rdfs:comment "Insulation energy density, joules per square metre or watt second per square metre." ;
  cims:stereotype "enum" .

cim:UnitSymbol.JPerm3 a cim:UnitSymbol ;
  rdfs:label "JPerm3"@en ;
  rdfs:comment "Energy density, joules per cubic metre." ;
  cims:stereotype "enum" .

cim:UnitSymbol.JPermol a cim:UnitSymbol ;
  rdfs:label "JPermol"@en ;
  rdfs:comment "Molar energy, joules per mole." ;
  cims:stereotype "enum" .

cim:UnitSymbol.JPermolK a cim:UnitSymbol ;
  rdfs:label "JPermolK"@en ;
  rdfs:comment "Molar entropy, molar heat capacity, joules per mole kelvin." ;
  cims:stereotype "enum" .

cim:UnitSymbol.JPers a cim:UnitSymbol ;
  rdfs:label "JPers"@en ;
  rdfs:comment "Energy rate in joules per second (J/s)." ;
  cims:stereotype "enum" .

cim:UnitSymbol.K a cim:UnitSymbol ;
  rdfs:label "K"@en ;
  rdfs:comment "Temperature in kelvins." ;
  cims:stereotype "enum" .

cim:UnitSymbol.KPers a cim:UnitSymbol ;
  rdfs:label "KPers"@en ;
  rdfs:comment "Temperature change rate in kelvins per second." ;
  cims:stereotype "enum" .

cim:UnitSymbol.M a cim:UnitSymbol ;
  rdfs:label "M"@en ;
  rdfs:comment "Length, nautical miles (1 M = 1852 m)." ;
  cims:stereotype "enum" .

cim:UnitSymbol.Mx a cim:UnitSymbol ;
  rdfs:label "Mx"@en ;
  rdfs:comment "Magnetic flux, maxwells (1 Mx = 10-8 Wb)." ;
  cims:stereotype "enum" .

cim:UnitSymbol.N a cim:UnitSymbol ;
  rdfs:label "N"@en ;
  rdfs:comment "Force in newtons (kg·m/s²)." ;
  cims:stereotype "enum" .

cim:UnitSymbol.NPerm a cim:UnitSymbol ;
  rdfs:label "NPerm"@en ;
  rdfs:comment "Surface tension, newton per metre." ;
  cims:stereotype "enum" .

cim:UnitSymbol.Nm a cim:UnitSymbol ;
  rdfs:label "Nm"@en ;
  rdfs:comment "Moment of force, newton metres." ;
  cims:stereotype "enum" .

cim:UnitSymbol.Oe a cim:UnitSymbol ;
  rdfs:label "Oe"@en ;
  rdfs:comment "Magnetic field in oersteds, (1 Oe = (103/4p) A/m)." ;
  cims:stereotype "enum" .

cim:UnitSymbol.Pa a cim:UnitSymbol ;
  rdfs:label "Pa"@en ;
  rdfs:comment "Pressure in pascals (N/m²). Note: the absolute or relative measurement of pressure is implied with this entry. See below for more explicit forms." ;
  cims:stereotype "enum" .

cim:UnitSymbol.PaPers a cim:UnitSymbol ;
  rdfs:label "PaPers"@en ;
  rdfs:comment "Pressure change rate in pascals per second." ;
  cims:stereotype "enum" .

cim:UnitSymbol.Pas a cim:UnitSymbol ;
  rdfs:label "Pas"@en ;
  rdfs:comment "Dynamic viscosity, pascal seconds." ;
  cims:stereotype "enum" .

cim:UnitSymbol.Q a cim:UnitSymbol ;
  rdfs:label "Q"@en ;
  rdfs:comment "Quantity power, Q." ;
  cims:stereotype "enum" .

cim:UnitSymbol.Qh a cim:UnitSymbol ;
  rdfs:label "Qh"@en ;
  rdfs:comment "Quantity energy, Qh." ;
  cims:stereotype "enum" .

cim:UnitSymbol.S a cim:UnitSymbol ;
  rdfs:label "S"@en ;
  rdfs:comment "Conductance in siemens." ;
  cims:stereotype "enum" .

cim:UnitSymbol.SPerm a cim:UnitSymbol ;
  rdfs:label "SPerm"@en ;
  rdfs:comment "Conductance per length (F/m)." ;
  cims:stereotype "enum" .

cim:UnitSymbol.Sv a cim:UnitSymbol ;
  rdfs:label "Sv"@en ;
  rdfs:comment "Dose equivalent in sieverts (J/kg)." ;
  cims:stereotype "enum" .

cim:UnitSymbol.T a cim:UnitSymbol ;
  rdfs:label "T"@en ;
  rdfs:comment "Magnetic flux density in teslas (Wb/m2)." ;
  cims:stereotype "enum" .

cim:UnitSymbol.V a cim:UnitSymbol ;
  rdfs:label "V"@en ;
  rdfs:comment "Electric potential in volts (W/A)." ;
  cims:stereotype "enum" .

cim:UnitSymbol.V2 a cim:UnitSymbol ;
  rdfs:label "V2"@en ;
  rdfs:comment "Volt squared (W²/A²)." ;
  cims:stereotype "enum" .

cim:UnitSymbol.V2h a cim:UnitSymbol ;
  rdfs:label "V2h"@en ;
  rdfs:comment "Volt-squared hour, volt-squared-hours." ;
  cims:stereotype "enum" .

cim:UnitSymbol.VA a cim:UnitSymbol ;
  rdfs:label "VA"@en ;
  rdfs:comment "Apparent power in volt amperes. See also real power and reactive power." ;
  cims:stereotype "enum" .

cim:UnitSymbol.VAh a cim:UnitSymbol ;
  rdfs:label "VAh"@en ;
  rdfs:comment "Apparent energy in volt ampere hours." ;
  cims:stereotype "enum" .

cim:UnitSymbol.VAr a cim:UnitSymbol ;
  rdfs:label "VAr"@en ;
  rdfs:comment """Reactive power in volt amperes reactive. The “reactive” or “imaginary” component of electrical power (VIsin(phi)). (See also real power and apparent power).
Note: Different meter designs use different methods to arrive at their results. Some meters may compute reactive power as an arithmetic value, while others compute the value vectorially. The data consumer should determine the method in use and the suitability of the measurement for the intended purpose.""" ;
  cims:stereotype "enum" .

cim:UnitSymbol.VArh a cim:UnitSymbol ;
  rdfs:label "VArh"@en ;
  rdfs:comment "Reactive energy in volt ampere reactive hours." ;
  cims:stereotype "enum" .

cim:UnitSymbol.VPerHz a cim:UnitSymbol ;
  rdfs:label "VPerHz"@en ;
  rdfs:comment "Magnetic flux in volt per hertz." ;
  cims:stereotype "enum" .

cim:UnitSymbol.VPerV a cim:UnitSymbol ;
  rdfs:label "VPerV"@en ;
  rdfs:comment "Voltage, ratio of voltages.  Note: Users may need to supply a prefix such as ‘m’ to show rates such as ‘mV/V’." ;
  cims:stereotype "enum" .

cim:UnitSymbol.VPerVA a cim:UnitSymbol ;
  rdfs:label "VPerVA"@en ;
  rdfs:comment "Power factor, PF, the ratio of the active power to the apparent power.  Note: The sign convention used for power factor will differ between IEC meters and EEI (ANSI) meters. It is assumed that the data consumers understand the type of meter being used and agree on the sign convention in use at any given utility." ;
  cims:stereotype "enum" .

cim:UnitSymbol.VPerVAr a cim:UnitSymbol ;
  rdfs:label "VPerVAr"@en ;
  rdfs:comment "Power factor, PF, the ratio of the active power to the apparent power. Note: The sign convention used for power factor will differ between IEC meters and EEI (ANSI) meters. It is assumed that the data consumers understand the type of meter being used and agree on the sign convention in use at any given utility." ;
  cims:stereotype "enum" .

cim:UnitSymbol.VPerm a cim:UnitSymbol ;
  rdfs:label "VPerm"@en ;
  rdfs:comment "Electric field strength, volts per metre." ;
  cims:stereotype "enum" .

cim:UnitSymbol.Vh a cim:UnitSymbol ;
  rdfs:label "Vh"@en ;
  rdfs:comment "Volt-hour, Volt hours." ;
  cims:stereotype "enum" .

cim:UnitSymbol.Vs a cim:UnitSymbol ;
  rdfs:label "Vs"@en ;
  rdfs:comment "Volt seconds (Ws/A)." ;
  cims:stereotype "enum" .

cim:UnitSymbol.W a cim:UnitSymbol ;
  rdfs:label "W"@en ;
  rdfs:comment "Real power in watts (J/s). Electrical power may have real and reactive components. The real portion of electrical power (I&#178;R or VIcos(phi)), is expressed in Watts. See also apparent power and reactive power." ;
  cims:stereotype "enum" .

cim:UnitSymbol.WPerA a cim:UnitSymbol ;
  rdfs:label "WPerA"@en ;
  rdfs:comment "Active power per current flow, watts per Ampere." ;
  cims:stereotype "enum" .

cim:UnitSymbol.WPerW a cim:UnitSymbol ;
  rdfs:label "WPerW"@en ;
  rdfs:comment "Signal Strength, ratio of power.   Note: Users may need to supply a prefix such as ‘m’ to show rates such as ‘mW/W’." ;
  cims:stereotype "enum" .

cim:UnitSymbol.WPerm2 a cim:UnitSymbol ;
  rdfs:label "WPerm2"@en ;
  rdfs:comment "Heat flux density, irradiance, watts per square metre." ;
  cims:stereotype "enum" .

cim:UnitSymbol.WPerm2sr a cim:UnitSymbol ;
  rdfs:label "WPerm2sr"@en ;
  rdfs:comment "Radiance, watts per square metre steradian." ;
  cims:stereotype "enum" .

cim:UnitSymbol.WPermK a cim:UnitSymbol ;
  rdfs:label "WPermK"@en ;
  rdfs:comment "Thermal conductivity in watt/metres kelvin." ;
  cims:stereotype "enum" .

cim:UnitSymbol.WPers a cim:UnitSymbol ;
  rdfs:label "WPers"@en ;
  rdfs:comment "Ramp rate in watts per second." ;
  cims:stereotype "enum" .

cim:UnitSymbol.WPersr a cim:UnitSymbol ;
  rdfs:label "WPersr"@en ;
  rdfs:comment "Radiant intensity, watts per steradian." ;
  cims:stereotype "enum" .

cim:UnitSymbol.Wb a cim:UnitSymbol ;
  rdfs:label "Wb"@en ;
  rdfs:comment "Magnetic flux in webers (V·s)." ;
  cims:stereotype "enum" .

cim:UnitSymbol.Wh a cim:UnitSymbol ;
  rdfs:label "Wh"@en ;
  rdfs:comment "Real energy in watt hours." ;
  cims:stereotype "enum" .

cim:UnitSymbol.anglemin a cim:UnitSymbol ;
  rdfs:label "anglemin"@en ;
  rdfs:comment "Plane angle, minutes." ;
  cims:stereotype "enum" .

cim:UnitSymbol.anglesec a cim:UnitSymbol ;
  rdfs:label "anglesec"@en ;
  rdfs:comment "Plane angle, seconds." ;
  cims:stereotype "enum" .

cim:UnitSymbol.bar a cim:UnitSymbol ;
  rdfs:label "bar"@en ;
  rdfs:comment "Pressure in bars, (1 bar = 100 kPa)." ;
  cims:stereotype "enum" .

cim:UnitSymbol.cd a cim:UnitSymbol ;
  rdfs:label "cd"@en ;
  rdfs:comment "Luminous intensity in candelas." ;
  cims:stereotype "enum" .

cim:UnitSymbol.charPers a cim:UnitSymbol ;
  rdfs:label "charPers"@en ;
  rdfs:comment "Data rate (baud) in characters per second." ;
  cims:stereotype "enum" .

cim:UnitSymbol.character a cim:UnitSymbol ;
  rdfs:label "character"@en ;
  rdfs:comment "Number of characters." ;
  cims:stereotype "enum" .

cim:UnitSymbol.cosPhi a cim:UnitSymbol ;
  rdfs:label "cosPhi"@en ;
  rdfs:comment """Power factor, dimensionless.
Note 1: This definition of power factor only holds for balanced systems. See the alternative definition under code 153.
Note 2 : Beware of differing sign conventions in use between the IEC and EEI. It is assumed that the data consumer understands the type of meter in use and the sign convention in use by the utility.""" ;
  cims:stereotype "enum" .

cim:UnitSymbol.count a cim:UnitSymbol ;
  rdfs:label "count"@en ;
  rdfs:comment "Amount of substance, Counter value." ;
  cims:stereotype "enum" .

cim:UnitSymbol.d a cim:UnitSymbol ;
  rdfs:label "d"@en ;
  rdfs:comment "Time in days, day = 24 h = 86400 s." ;
  cims:stereotype "enum" .

cim:UnitSymbol.dB a cim:UnitSymbol ;
  rdfs:label "dB"@en ;
  rdfs:comment "Sound pressure level in decibels. Note:  multiplier “d” is included in this unit symbol for compatibility with IEC 61850-7-3." ;
  cims:stereotype "enum" .

cim:UnitSymbol.dBm a cim:UnitSymbol ;
  rdfs:label "dBm"@en ;
  rdfs:comment "Power level (logarithmic ratio of signal strength , Bel-mW), normalized to 1mW. Note:  multiplier “d” is included in this unit symbol for compatibility with IEC 61850-7-3." ;
  cims:stereotype "enum" .

cim:UnitSymbol.deg a cim:UnitSymbol ;
  rdfs:label "deg"@en ;
  rdfs:comment "Plane angle in degrees." ;
  cims:stereotype "enum" .

cim:UnitSymbol.degC a cim:UnitSymbol ;
  rdfs:label "degC"@en ;
  rdfs:comment """Relative temperature in degrees Celsius.
In the SI unit system the symbol is °C. Electric charge is measured in coulomb that has the unit symbol C. To distinguish degree Celsius from coulomb the symbol used in the UML is degC. The reason for not using °C is that the special character ° is difficult to manage in software.""" ;
  cims:stereotype "enum" .

cim:UnitSymbol.ft3 a cim:UnitSymbol ;
  rdfs:label "ft3"@en ;
  rdfs:comment "Volume, cubic feet." ;
  cims:stereotype "enum" .

cim:UnitSymbol.gPerg a cim:UnitSymbol ;
  rdfs:label "gPerg"@en ;
  rdfs:comment "Concentration, The ratio of the mass of a solute divided by the mass of  the solution. Note: Users may need use a prefix such a ‘µ’ to express a quantity such as ‘µg/g’." ;
  cims:stereotype "enum" .

cim:UnitSymbol.gal a cim:UnitSymbol ;
  rdfs:label "gal"@en ;
  rdfs:comment "Volume in gallons, US gallon (1 gal = 231 in3 = 128 fl ounce)." ;
  cims:stereotype "enum" .

cim:UnitSymbol.h a cim:UnitSymbol ;
  rdfs:label "h"@en ;
  rdfs:comment "Time in hours, hour = 60 min = 3600 s." ;
  cims:stereotype "enum" .

cim:UnitSymbol.ha a cim:UnitSymbol ;
  rdfs:label "ha"@en ;
  rdfs:comment "Area, hectares." ;
  cims:stereotype "enum" .

cim:UnitSymbol.kat a cim:UnitSymbol ;
  rdfs:label "kat"@en ;
  rdfs:comment "Catalytic activity, katal = mol / s." ;
  cims:stereotype "enum" .

cim:UnitSymbol.katPerm3 a cim:UnitSymbol ;
  rdfs:label "katPerm3"@en ;
  rdfs:comment "Catalytic activity concentration, katals per cubic metre." ;
  cims:stereotype "enum" .

cim:UnitSymbol.kg a cim:UnitSymbol ;
  rdfs:label "kg"@en ;
  rdfs:comment "Mass in kilograms.  Note: multiplier “k” is included in this unit symbol for compatibility with IEC 61850-7-3." ;
  cims:stereotype "enum" .

cim:UnitSymbol.kgPerJ a cim:UnitSymbol ;
  rdfs:label "kgPerJ"@en ;
  rdfs:comment "Weight per energy in kilograms per joule (kg/J). Note: multiplier “k” is included in this unit symbol for compatibility with IEC 61850-7-3." ;
  cims:stereotype "enum" .

cim:UnitSymbol.kgPerm3 a cim:UnitSymbol ;
  rdfs:label "kgPerm3"@en ;
  rdfs:comment "Density in kilogram/cubic metres (kg/m³). Note: multiplier “k” is included in this unit symbol for compatibility with IEC 61850-7-3." ;
  cims:stereotype "enum" .

cim:UnitSymbol.kgm a cim:UnitSymbol ;
  rdfs:label "kgm"@en ;
  rdfs:comment "Moment of mass in kilogram metres (kg·m) (first moment of mass). Note: multiplier “k” is included in this unit symbol for compatibility with IEC 61850-7-3." ;
  cims:stereotype "enum" .

cim:UnitSymbol.kgm2 a cim:UnitSymbol ;
  rdfs:label "kgm2"@en ;
  rdfs:comment "Moment of mass in kilogram square metres (kg·m²) (Second moment of mass, commonly called the moment of inertia). Note: multiplier “k” is included in this unit symbol for compatibility with IEC 61850-7-3." ;
  cims:stereotype "enum" .

cim:UnitSymbol.kn a cim:UnitSymbol ;
  rdfs:label "kn"@en ;
  rdfs:comment "Speed, knots (1 kn = 1852/3600) m/s." ;
  cims:stereotype "enum" .

cim:UnitSymbol.l a cim:UnitSymbol ;
  rdfs:label "l"@en ;
  rdfs:comment "Volume in litres, litre = dm3 = m3/1000." ;
  cims:stereotype "enum" .

cim:UnitSymbol.lPerh a cim:UnitSymbol ;
  rdfs:label "lPerh"@en ;
  rdfs:comment "Volumetric flow rate, litres per hour." ;
  cims:stereotype "enum" .

cim:UnitSymbol.lPerl a cim:UnitSymbol ;
  rdfs:label "lPerl"@en ;
  rdfs:comment "Concentration, The ratio of the volume of a solute divided by the volume of  the solution. Note: Users may need use a prefix such a ‘µ’ to express a quantity such as ‘µL/L’." ;
  cims:stereotype "enum" .

cim:UnitSymbol.lPers a cim:UnitSymbol ;
  rdfs:label "lPers"@en ;
  rdfs:comment "Volumetric flow rate in litres per second." ;
  cims:stereotype "enum" .

cim:UnitSymbol.lm a cim:UnitSymbol ;
  rdfs:label "lm"@en ;
  rdfs:comment "Luminous flux in lumens (cd·sr)." ;
  cims:stereotype "enum" .

cim:UnitSymbol.lx a cim:UnitSymbol ;
  rdfs:label "lx"@en ;
  rdfs:comment "Illuminance in lux (lm/m²)." ;
  cims:stereotype "enum" .

cim:UnitSymbol.m a cim:UnitSymbol ;
  rdfs:label "m"@en ;
  rdfs:comment "Length in metres." ;
  cims:stereotype "enum" .

cim:UnitSymbol.m2 a cim:UnitSymbol ;
  rdfs:label "m2"@en ;
  rdfs:comment "Area in square metres (m²)." ;
  cims:stereotype "enum" .

cim:UnitSymbol.m2Pers a cim:UnitSymbol ;
  rdfs:label "m2Pers"@en ;
  rdfs:comment "Viscosity in square metres / second (m²/s)." ;
  cims:stereotype "enum" .

cim:UnitSymbol.m3 a cim:UnitSymbol ;
  rdfs:label "m3"@en ;
  rdfs:comment "Volume in cubic metres (m³)." ;
  cims:stereotype "enum" .

cim:UnitSymbol.m3Compensated a cim:UnitSymbol ;
  rdfs:label "m3Compensated"@en ;
  rdfs:comment "Volume, cubic metres, with the value compensated for weather effects." ;
  cims:stereotype "enum" .

cim:UnitSymbol.m3Perh a cim:UnitSymbol ;
  rdfs:label "m3Perh"@en ;
  rdfs:comment "Volumetric flow rate, cubic metres per hour." ;
  cims:stereotype "enum" .

cim:UnitSymbol.m3Perkg a cim:UnitSymbol ;
  rdfs:label "m3Perkg"@en ;
  rdfs:comment "Specific volume, cubic metres per kilogram, v." ;
  cims:stereotype "enum" .

cim:UnitSymbol.m3Pers a cim:UnitSymbol ;
  rdfs:label "m3Pers"@en ;
  rdfs:comment "Volumetric flow rate in cubic metres per second (m³/s)." ;
  cims:stereotype "enum" .

cim:UnitSymbol.m3Uncompensated a cim:UnitSymbol ;
  rdfs:label "m3Uncompensated"@en ;
  rdfs:comment "Volume, cubic metres, with the value uncompensated for weather effects." ;
  cims:stereotype "enum" .

cim:UnitSymbol.mPerm3 a cim:UnitSymbol ;
  rdfs:label "mPerm3"@en ;
  rdfs:comment "Fuel efficiency in metres per cubic metres (m/m³)." ;
  cims:stereotype "enum" .

cim:UnitSymbol.mPers a cim:UnitSymbol ;
  rdfs:label "mPers"@en ;
  rdfs:comment "Velocity in metres per second (m/s)." ;
  cims:stereotype "enum" .

cim:UnitSymbol.mPers2 a cim:UnitSymbol ;
  rdfs:label "mPers2"@en ;
  rdfs:comment "Acceleration in metres per second squared (m/s²)." ;
  cims:stereotype "enum" .

cim:UnitSymbol.min a cim:UnitSymbol ;
  rdfs:label "min"@en ;
  rdfs:comment "Time in minutes, minute  = 60 s." ;
  cims:stereotype "enum" .

cim:UnitSymbol.mmHg a cim:UnitSymbol ;
  rdfs:label "mmHg"@en ;
  rdfs:comment "Pressure, millimetres of mercury (1 mmHg is approximately 133.3 Pa)." ;
  cims:stereotype "enum" .

cim:UnitSymbol.mol a cim:UnitSymbol ;
  rdfs:label "mol"@en ;
  rdfs:comment "Amount of substance in moles." ;
  cims:stereotype "enum" .

cim:UnitSymbol.molPerkg a cim:UnitSymbol ;
  rdfs:label "molPerkg"@en ;
  rdfs:comment "Concentration, Molality, the amount of solute in moles and the amount of solvent in kilograms." ;
  cims:stereotype "enum" .

cim:UnitSymbol.molPerm3 a cim:UnitSymbol ;
  rdfs:label "molPerm3"@en ;
  rdfs:comment "Concentration, The amount of substance concentration, (c), the amount of solvent in moles divided by the volume of solution in m³." ;
  cims:stereotype "enum" .

cim:UnitSymbol.molPermol a cim:UnitSymbol ;
  rdfs:label "molPermol"@en ;
  rdfs:comment "Concentration, Molar fraction, the ratio of the molar amount of a solute divided by the molar amount of the solution." ;
  cims:stereotype "enum" .

cim:UnitSymbol.none a cim:UnitSymbol ;
  rdfs:label "none"@en ;
  rdfs:comment "Dimension less quantity, e.g. count, per unit, etc." ;
  cims:stereotype "enum" .

cim:UnitSymbol.ohm a cim:UnitSymbol ;
  rdfs:label "ohm"@en ;
  rdfs:comment "Electric resistance in ohms (V/A)." ;
  cims:stereotype "enum" .

cim:UnitSymbol.ohmPerm a cim:UnitSymbol ;
  rdfs:label "ohmPerm"@en ;
  rdfs:comment "Electric resistance per length in ohms per metre ((V/A)/m)." ;
  cims:stereotype "enum" .

cim:UnitSymbol.ohmm a cim:UnitSymbol ;
  rdfs:label "ohmm"@en ;
  rdfs:comment "Resistivity, ohm metres, (rho)." ;
  cims:stereotype "enum" .

cim:UnitSymbol.onePerHz a cim:UnitSymbol ;
  rdfs:label "onePerHz"@en ;
  rdfs:comment "Reciprocal of frequency (1/Hz)." ;
  cims:stereotype "enum" .

cim:UnitSymbol.onePerm a cim:UnitSymbol ;
  rdfs:label "onePerm"@en ;
  rdfs:comment "Wavenumber, reciprocal metres,  (1/m)." ;
  cims:stereotype "enum" .

cim:UnitSymbol.ppm a cim:UnitSymbol ;
  rdfs:label "ppm"@en ;
  rdfs:comment "Concentration in parts per million." ;
  cims:stereotype "enum" .

cim:UnitSymbol.rad a cim:UnitSymbol ;
  rdfs:label "rad"@en ;
  rdfs:comment "Plane angle in radians (m/m)." ;
  cims:stereotype "enum" .

cim:UnitSymbol.radPers a cim:UnitSymbol ;
  rdfs:label "radPers"@en ;
  rdfs:comment "Angular velocity in radians per second (rad/s)." ;
  cims:stereotype "enum" .

cim:UnitSymbol.radPers2 a cim:UnitSymbol ;
  rdfs:label "radPers2"@en ;
  rdfs:comment "Angular acceleration, radians per second squared." ;
  cims:stereotype "enum" .

cim:UnitSymbol.rev a cim:UnitSymbol ;
  rdfs:label "rev"@en ;
  rdfs:comment "Amount of rotation, revolutions." ;
  cims:stereotype "enum" .

cim:UnitSymbol.rotPers a cim:UnitSymbol ;
  rdfs:label "rotPers"@en ;
  rdfs:comment "Rotations per second (1/s). See also Hz (1/s)." ;
  cims:stereotype "enum" .

cim:UnitSymbol.s a cim:UnitSymbol ;
  rdfs:label "s"@en ;
  rdfs:comment "Time in seconds." ;
  cims:stereotype "enum" .

cim:UnitSymbol.sPers a cim:UnitSymbol ;
  rdfs:label "sPers"@en ;
  rdfs:comment "Time, Ratio of time.  Note: Users may need to supply a prefix such as ‘&#181;’ to show rates such as ‘&#181;s/s’." ;
  cims:stereotype "enum" .

cim:UnitSymbol.sr a cim:UnitSymbol ;
  rdfs:label "sr"@en ;
  rdfs:comment "Solid angle in steradians (m2/m2)." ;
  cims:stereotype "enum" .

cim:UnitSymbol.therm a cim:UnitSymbol ;
  rdfs:label "therm"@en ;
  rdfs:comment "Energy, therms." ;
  cims:stereotype "enum" .

cim:UnitSymbol.tonne a cim:UnitSymbol ;
  rdfs:label "tonne"@en ;
  rdfs:comment "Mass in tons, “tonne” or “metric  ton” (1000 kg = 1 Mg)." ;
  cims:stereotype "enum" .

cim:WindGenUnitKind.offshore a cim:WindGenUnitKind ;
  rdfs:label "offshore"@en ;
  rdfs:comment "The wind generating unit is located offshore." ;
  cims:stereotype "enum" .

cim:WindGenUnitKind.onshore a cim:WindGenUnitKind ;
  rdfs:label "onshore"@en ;
  rdfs:comment "The wind generating unit is located onshore." ;
  cims:stereotype "enum" .

cim:WindingConnection.A a cim:WindingConnection ;
  rdfs:label "A"@en ;
  rdfs:comment "Autotransformer common winding." ;
  cims:stereotype "enum" .

cim:WindingConnection.D a cim:WindingConnection ;
  rdfs:label "D"@en ;
  rdfs:comment "Delta." ;
  cims:stereotype "enum" .

cim:WindingConnection.I a cim:WindingConnection ;
  rdfs:label "I"@en ;
  rdfs:comment "Independent winding, for single-phase connections." ;
  cims:stereotype "enum" .

cim:WindingConnection.Y a cim:WindingConnection ;
  rdfs:label "Y"@en ;
  rdfs:comment "Wye." ;
  cims:stereotype "enum" .

cim:WindingConnection.Yn a cim:WindingConnection ;
  rdfs:label "Yn"@en ;
  rdfs:comment "Wye, with neutral brought out for grounding." ;
  cims:stereotype "enum" .

cim:WindingConnection.Z a cim:WindingConnection ;
  rdfs:label "Z"@en ;
  rdfs:comment "ZigZag." ;
  cims:stereotype "enum" .

cim:WindingConnection.Zn a cim:WindingConnection ;
  rdfs:label "Zn"@en ;
  rdfs:comment "ZigZag, with neutral brought out for grounding." ;
  cims:stereotype "enum" .

eq:Package_CoreEquipmentProfile a cims:ClassCategory ;
  rdfs:label "CoreEquipmentProfile"@en ;
  rdfs:comment "This is the IEC 61970-452 core equipment profile." .

eu:LimitKind.alarmVoltage a eu:LimitKind ;
  rdfs:label "alarmVoltage"@en ;
  rdfs:comment "Voltage alarm." ;
  cims:stereotype "European", "enum" .

eu:LimitKind.highVoltage a eu:LimitKind ;
  rdfs:label "highVoltage"@en ;
  rdfs:comment """Referring to the rating of the equipments, a voltage too high can lead to accelerated ageing or the destruction of the equipment. 
This limit type may or may not have duration.""" ;
  cims:stereotype "European", "enum" .

eu:LimitKind.lowVoltage a eu:LimitKind ;
  rdfs:label "lowVoltage"@en ;
  rdfs:comment """A too low voltage can disturb the normal operation of some protections and transformer equipped with on-load tap changers, electronic power devices or can affect the behaviour of the auxiliaries of generation units.
This limit type may or may not have duration.""" ;
  cims:stereotype "European", "enum" .

eu:LimitKind.operationalVoltageLimit a eu:LimitKind ;
  rdfs:label "operationalVoltageLimit"@en ;
  rdfs:comment "Operational voltage limit." ;
  cims:stereotype "European", "enum" .

eu:LimitKind.patl a eu:LimitKind ;
  rdfs:label "patl"@en ;
  rdfs:comment """The Permanent Admissible Transmission Loading (PATL) is the loading in amperes, MVA or MW that can be accepted by a network branch for an unlimited duration without any risk for the material.
The OperationnalLimitType.isInfiniteDuration is set to true. There shall be only one OperationalLimitType of kind PATL per OperationalLimitSet if the PATL is ApparentPowerLimit, ActivePowerLimit, or CurrentLimit for a given Terminal or Equipment.""" ;
  cims:stereotype "European", "enum" .

eu:LimitKind.patlt a eu:LimitKind ;
  rdfs:label "patlt"@en ;
  rdfs:comment "Permanent Admissible Transmission Loading Threshold  (PATLT) is a value in engineering units defined for PATL and calculated using a percentage less than 100 % of the PATL type intended to alert operators of an arising condition. The percentage should be given in the name of the OperationalLimitSet. The aceptableDuration is another way to express the severity of the limit." ;
  cims:stereotype "European", "enum" .

eu:LimitKind.stability a eu:LimitKind ;
  rdfs:label "stability"@en ;
  rdfs:comment "Stability." ;
  cims:stereotype "European", "enum" .

eu:LimitKind.tatl a eu:LimitKind ;
  rdfs:label "tatl"@en ;
  rdfs:comment """Temporarily Admissible Transmission Loading (TATL) which is the loading in amperes, MVA or MW that can be accepted by a branch for a certain limited duration.
The TATL can be defined in different ways:
<ul>
\t<li>as a fixed percentage of the PATL for a given time (for example, 115% of the PATL that can be accepted during 15 minutes),</li>
</ul>
<ul>
\t<li>pairs of TATL type and Duration calculated for each line taking into account its particular configuration and conditions of functioning (for example, it can define a TATL acceptable during 20 minutes and another one acceptable during 10 minutes).</li>
</ul>
Such a definition of TATL can depend on the initial operating conditions of the network element (sag situation of a line).
The duration attribute can be used to define several TATL limit types. Hence multiple TATL limit values may exist having different durations.""" ;
  cims:stereotype "European", "enum" .

eu:LimitKind.tc a eu:LimitKind ;
  rdfs:label "tc"@en ;
  rdfs:comment """Tripping Current (TC) is the ultimate intensity without any delay. It is defined as the threshold the line will trip without any possible remedial actions.
The tripping of the network element is ordered by protections against short circuits or by overload protections, but in any case, the activation delay of these protections is not compatible with the reaction delay of an operator (less than one minute).
The duration is always zero if the OperationalLimitType.acceptableDuration is exchanged. Only one limit value exists for the TC type.""" ;
  cims:stereotype "European", "enum" .

eu:LimitKind.tct a eu:LimitKind ;
  rdfs:label "tct"@en ;
  rdfs:comment "Tripping Current Threshold  (TCT) is a value in engineering units defined for TC and calculated using a percentage less than 100 % of the TC type intended to alert operators of an arising condition. The percentage should be given in the name of the OperationalLimitSet. The aceptableDuration is another way to express the severity of the limit." ;
  cims:stereotype "European", "enum" .

eu:LimitKind.warningVoltage a eu:LimitKind ;
  rdfs:label "warningVoltage"@en ;
  rdfs:comment "Voltage warning." ;
  cims:stereotype "European", "enum" .


