@prefix cim    : <http://iec.ch/TC57/CIM100#> .
@prefix dy     : <http://iec.ch/TC57/ns/CIM/Dynamics-EU#> .
@prefix dcat   : <http://www.w3.org/ns/dcat#> .
@prefix dct    : <http://purl.org/dc/terms/> .
@prefix owl    : <http://www.w3.org/2002/07/owl#> .
@prefix rdf    : <http://www.w3.org/1999/02/22-rdf-syntax-ns#> .
@prefix rdfs   : <http://www.w3.org/2000/01/rdf-schema#> .
@prefix skos   : <http://www.w3.org/2004/02/skos/core#> .
@prefix xsd    : <http://www.w3.org/2001/XMLSchema#> .

dy:Ontology a owl:Ontology ;
  dct:description "This vocabulary is describing the dynamics profile from IEC 61970-600-2."@en ;
  dcat:keyword "DY" ;
  dcat:theme "vocabulary"@en ;
  dct:conformsTo "file://iec61970cim17v40_iec61968cim13v13a_iec62325cim03v17a.eap", "urn:iso:std:iec:61970-301:ed-7:amd1", "urn:iso:std:iec:61970-302:ed-1", "urn:iso:std:iec:61970-401:draft:ed-1", "urn:iso:std:iec:61970-501:draft:ed-2", "urn:iso:std:iec:61970-600-2:ed-1" ;
  dct:creator "ENTSO-E"@en ;
  dct:identifier "urn:uuid:ba96da07-eca3-4259-b96c-cf5b51baa082" ;
  dct:issued "2021-01-27T13:04:24Z"^^xsd:dateTime ;
  dct:language "en-GB" ;
  dct:modified "2020-10-12"^^xsd:date ;
  dct:publisher "ENTSO-E"@en ;
  dct:rights "Copyright"@en ;
  dct:rightsHolder "ENTSO-E"@en ;
  dct:title "Dynamics Vocabulary"@en ;
  owl:incompatibleWith <http://entsoe.eu/2009/profile1> ;
  owl:versionIRI <http://iec.ch/TC57/ns/CIM/Dynamics-EU/1.0> ;
  owl:versionInfo "1.0.0"@en .

cim:ACDCConverter a owl:Class ;
  rdfs:label "ACDCConverter"@en ;
  dy:Package "Package_DC" ;
  dy:isAbstract "True" ;
  rdfs:subClassOf cim:ConductingEquipment ;
  skos:definition "A unit with valves for three phases, together with unit control equipment, essential protective and switching devices, DC storage capacitors, phase reactors and auxiliaries, if any, used for conversion."@en .

cim:ACDCTerminal a owl:Class ;
  rdfs:label "ACDCTerminal"@en ;
  dy:Package "Package_Core" ;
  dy:isAbstract "True" ;
  rdfs:subClassOf cim:IdentifiedObject ;
  skos:definition "An electrical connection point (AC or DC) to a piece of conducting equipment. Terminals are connected at physical connection points called connectivity nodes."@en .

cim:ActivePower a owl:Class ;
  rdfs:label "ActivePower"@en ;
  dy:Package "Package_Domain" ;
  dy:isCIMDatatype "True" ;
  skos:definition "Product of RMS value of the voltage and the RMS value of the in-phase component of the current."@en .

cim:AngleDegrees a owl:Class ;
  rdfs:label "AngleDegrees"@en ;
  dy:Package "Package_Domain" ;
  dy:isCIMDatatype "True" ;
  skos:definition """
Measurement of angle in degrees.

\t"""@en .

cim:ApparentPower a owl:Class ;
  rdfs:label "ApparentPower"@en ;
  dy:Package "Package_Domain" ;
  dy:isCIMDatatype "True" ;
  skos:definition """
Product of the RMS value of the voltage and the RMS value of the current.

\t"""@en .

cim:Area a owl:Class ;
  rdfs:label "Area"@en ;
  dy:Package "Package_Domain" ;
  dy:isCIMDatatype "True" ;
  skos:definition "Area."@en .

cim:AsynchronousMachine a owl:Class ;
  rdfs:label "AsynchronousMachine"@en ;
  dy:Package "Package_Wires" ;
  dy:isAbstract "True" ;
  rdfs:subClassOf cim:RotatingMachine ;
  skos:definition "A rotating machine whose shaft rotates asynchronously with the electrical field.  Also known as an induction machine with no external connection to the rotor windings, e.g. squirrel-cage induction machine."@en .

cim:AsynchronousMachineDynamics a owl:Class ;
  rdfs:label "AsynchronousMachineDynamics"@en ;
  dy:Package "Package_AsynchronousMachineDynamics" ;
  dy:isAbstract "True" ;
  rdfs:subClassOf cim:RotatingMachineDynamics ;
  skos:definition """
Asynchronous machine whose behaviour is described by reference to a standard model expressed in either time constant reactance form or equivalent circuit form <font color="#0f0f0f">or by definition of a user-defined model.</font>
Parameter details:
<ol>
<li>Asynchronous machine parameters such as <i>Xl, Xs,</i> etc. are actually used as inductances in the model, but are commonly referred to as reactances since, at nominal frequency, the PU values are the same. However, some references use the symbol <i>L</i> instead of <i>X</i>.</li>
</ol>
\t"""@en .

cim:AsynchronousMachineEquivalentCircuit a owl:Class ;
  rdfs:label "AsynchronousMachineEquivalentCircuit"@en ;
  dy:Package "Package_AsynchronousMachineDynamics" ;
  rdfs:subClassOf cim:AsynchronousMachineDynamics ;
  skos:definition """
The electrical equations of all variations of the asynchronous model are based on the AsynchronousEquivalentCircuit diagram for the direct- and quadrature- axes, with two equivalent rotor windings in each axis.  
Equations for conversion between equivalent circuit and time constant reactance forms:
<i>Xs</i> = <i>Xm</i> + <i>Xl</i>
<i>X'</i> = <i>Xl</i> + <i>Xm</i> x <i>Xlr1 </i>/ (<i>Xm </i>+ <i>Xlr1</i>)
<i>X''</i> = <i>Xl</i> + <i>Xm</i> x <i>Xlr1</i> x <i>Xlr2</i> / (<i>Xm</i> x <i>Xlr1</i> + <i>Xm</i> x <i>Xlr2</i> + <i>Xlr1</i> x <i>Xlr2</i>)
<i>T'o</i> = (<i>Xm</i> + <i>Xlr1</i>) / (<i>omega</i><i><sub>0</sub></i> x <i>Rr1</i>)
<i>T''o</i> = (<i>Xm</i> x <i>Xlr1</i> + <i>Xm</i> x <i>Xlr2</i> + <i>Xlr1</i> x <i>Xlr2</i>) / (<i>omega</i><i><sub>0</sub></i> x <i>Rr2</i> x (<i>Xm</i> + <i>Xlr1</i>)
Same equations using CIM attributes from AsynchronousMachineTimeConstantReactance class on left of "=" and AsynchronousMachineEquivalentCircuit class on right (except as noted):
xs = xm + RotatingMachineDynamics.statorLeakageReactance
xp = RotatingMachineDynamics.statorLeakageReactance + xm x xlr1 / (xm + xlr1)
xpp = RotatingMachineDynamics.statorLeakageReactance + xm x xlr1 x xlr2 / (xm x xlr1 + xm x xlr2 + xlr1 x xlr2)
tpo = (xm + xlr1) / (2 x pi x nominal frequency x rr1)
tppo = (xm x xlr1 + xm x xlr2 + xlr1 x xlr2) / (2 x pi x nominal frequency x rr2 x (xm + xlr1).
\t"""@en .

cim:AsynchronousMachineTimeConstantReactance a owl:Class ;
  rdfs:label "AsynchronousMachineTimeConstantReactance"@en ;
  dy:Package "Package_AsynchronousMachineDynamics" ;
  rdfs:subClassOf cim:AsynchronousMachineDynamics ;
  skos:definition """
Parameter details:
<ol>
<li>If <i>X'' </i>=<i> X'</i>, a single cage (one equivalent rotor winding per axis) is modelled.</li>
<li>The “<i>p</i>” in the attribute names is a substitution for a “prime” in the usual parameter notation, e.g. <i>tpo</i> refers to <i>T'o</i>.</li>
</ol>
The parameters used for models expressed in time constant reactance form include:
- RotatingMachine.ratedS (<i>MVAbase</i>);
- RotatingMachineDynamics.damping (<i>D</i>);
- RotatingMachineDynamics.inertia (<i>H</i>);
- RotatingMachineDynamics.saturationFactor (<i>S1</i>);
- RotatingMachineDynamics.saturationFactor120 (<i>S12</i>);
- RotatingMachineDynamics.statorLeakageReactance (<i>Xl</i>);
- RotatingMachineDynamics.statorResistance (<i>Rs</i>);
- .xs (<i>Xs</i>);
- .xp (<i>X'</i>);
- .xpp (<i>X''</i>);
- .tpo (<i>T'o</i>);
- .tppo (<i>T''o</i>).
\t"""@en .

cim:AsynchronousMachineUserDefined a owl:Class ;
  rdfs:label "AsynchronousMachineUserDefined"@en ;
  dy:Package "Package_UserDefinedModels" ;
  rdfs:subClassOf cim:AsynchronousMachineDynamics ;
  skos:definition "Asynchronous machine whose dynamic behaviour is described by a user-defined model."@en .

cim:Boolean a owl:Class ;
  rdfs:label "Boolean"@en ;
  dy:Package "Package_Domain" ;
  dy:isPrimitive "True" ;
  skos:definition """
A type with the value space "true" and "false".

\t"""@en .

cim:CSCDynamics a owl:Class ;
  rdfs:label "CSCDynamics"@en ;
  dy:Package "Package_HVDCDynamics" ;
  dy:isAbstract "True" ;
  rdfs:subClassOf cim:HVDCDynamics ;
  skos:definition "CSC function block whose behaviour is described by reference to a standard model <font color=\"#0f0f0f\">or by definition of a user-defined model.</font>"@en .

cim:CSCUserDefined a owl:Class ;
  rdfs:label "CSCUserDefined"@en ;
  dy:Package "Package_UserDefinedModels" ;
  rdfs:subClassOf cim:CSCDynamics ;
  skos:definition "Current source converter (CSC) function block whose dynamic behaviour is described by <font color=\"#0f0f0f\">a user-defined model.</font>"@en .

cim:ConductingEquipment a owl:Class ;
  rdfs:label "ConductingEquipment"@en ;
  dy:Package "Package_Core" ;
  dy:isAbstract "True" ;
  rdfs:subClassOf cim:Equipment ;
  skos:definition "The parts of the AC power system that are designed to carry current or that are conductively connected through terminals."@en .

cim:CrossCompoundTurbineGovernorDynamics a owl:Class ;
  rdfs:label "CrossCompoundTurbineGovernorDynamics"@en ;
  dy:Package "Package_TurbineGovernorDynamics" ;
  dy:isAbstract "True" ;
  rdfs:subClassOf cim:DynamicsFunctionBlock ;
  skos:definition "Turbine-governor cross-compound function block whose behaviour is described by reference to a standard model <font color=\"#0f0f0f\">or by definition of a user-defined model.</font>"@en .

cim:CsConverter a owl:Class ;
  rdfs:label "CsConverter"@en ;
  dy:Package "Package_DC" ;
  dy:isAbstract "True" ;
  rdfs:subClassOf cim:ACDCConverter ;
  skos:definition """
DC side of the current source converter (CSC).
The firing angle controls the dc voltage at the converter, both for rectifier and inverter. The difference between the dc voltages of the rectifier and inverter determines the dc current. The extinction angle is used to limit the dc voltage at the inverter, if needed, and is not used in active power control. The firing angle, transformer tap position and number of connected filters are the primary means to control a current source dc line. Higher level controls are built on top, e.g. dc voltage, dc current and active power. From a steady state perspective it is sufficient to specify the wanted active power transfer (ACDCConverter.targetPpcc) and the control functions will set the dc voltage, dc current, firing angle, transformer tap position and number of connected filters to meet this. Therefore attributes targetAlpha and targetGamma are not applicable in this case.
The reactive power consumed by the converter is a function of the firing angle, transformer tap position and number of connected filter, which can be approximated with half of the active power. The losses is a function of the dc voltage and dc current.
The attributes minAlpha and maxAlpha define the range of firing angles for rectifier operation between which no discrete tap changer action takes place. The range is typically 10-18 degrees.
The attributes minGamma and maxGamma define the range of extinction angles for inverter operation between which no discrete tap changer action takes place. The range is typically 17-20 degrees.
\t"""@en .

cim:Date a owl:Class ;
  rdfs:label "Date"@en ;
  dy:Package "Package_Domain" ;
  dy:isPrimitive "True" ;
  skos:definition "Date as \"yyyy-mm-dd\", which conforms with ISO 8601. UTC time zone is specified as \"yyyy-mm-ddZ\". A local timezone relative UTC is specified as \"yyyy-mm-dd(+/-)hh:mm\"."@en .

cim:DiscExcContIEEEDEC1A a owl:Class ;
  rdfs:label "DiscExcContIEEEDEC1A"@en ;
  dy:Package "Package_DiscontinuousExcitationControlDynamics" ;
  rdfs:subClassOf cim:DiscontinuousExcitationControlDynamics ;
  skos:definition """
IEEE type DEC1A discontinuous excitation control model that boosts generator excitation to a level higher than that demanded by the voltage regulator and stabilizer immediately following a system fault.
Reference: IEEE 421.5-2005, 12.2. 
\t"""@en .

cim:DiscExcContIEEEDEC2A a owl:Class ;
  rdfs:label "DiscExcContIEEEDEC2A"@en ;
  dy:Package "Package_DiscontinuousExcitationControlDynamics" ;
  rdfs:subClassOf cim:DiscontinuousExcitationControlDynamics ;
  skos:definition """
IEEE type DEC2A model for discontinuous excitation control. This system provides transient excitation boosting via an open-loop control as initiated by a trigger signal generated remotely.
Reference: IEEE 421.5-2005 12.3. 
\t"""@en .

cim:DiscExcContIEEEDEC3A a owl:Class ;
  rdfs:label "DiscExcContIEEEDEC3A"@en ;
  dy:Package "Package_DiscontinuousExcitationControlDynamics" ;
  rdfs:subClassOf cim:DiscontinuousExcitationControlDynamics ;
  skos:definition """
IEEE type DEC3A model. In some systems, the stabilizer output is disconnected from the regulator immediately following a severe fault to prevent the stabilizer from competing with action of voltage regulator during the first swing.
Reference: IEEE 421.5-2005 12.4. 
\t"""@en .

cim:DiscontinuousExcitationControlDynamics a owl:Class ;
  rdfs:label "DiscontinuousExcitationControlDynamics"@en ;
  dy:Package "Package_DiscontinuousExcitationControlDynamics" ;
  dy:isAbstract "True" ;
  rdfs:subClassOf cim:DynamicsFunctionBlock ;
  skos:definition "Discontinuous excitation control function block whose behaviour is described by reference to a standard model <font color=\"#0f0f0f\">or by definition of a user-defined model</font>."@en .

cim:DiscontinuousExcitationControlUserDefined a owl:Class ;
  rdfs:label "DiscontinuousExcitationControlUserDefined"@en ;
  dy:Package "Package_UserDefinedModels" ;
  rdfs:subClassOf cim:DiscontinuousExcitationControlDynamics ;
  skos:definition "Discontinuous excitation control function block whose dynamic behaviour is described by <font color=\"#0f0f0f\">a user-defined model.</font>"@en .

cim:DroopSignalFeedbackKind a owl:Class ;
  rdfs:label "DroopSignalFeedbackKind"@en ;
  dy:Package "Package_Domain" ;
  owl:oneOf ( cim:DroopSignalFeedbackKind.electricalPower cim:DroopSignalFeedbackKind.none
    cim:DroopSignalFeedbackKind.fuelValveStroke cim:DroopSignalFeedbackKind.governorOutput ) ;
  rdfs:subClassOf cim:Enumeration ;
  skos:definition "Governor droop signal feedback source."@en .

cim:DynamicsFunctionBlock a owl:Class ;
  rdfs:label "DynamicsFunctionBlock"@en ;
  dy:Package "Package_StandardModels" ;
  dy:isAbstract "True" ;
  rdfs:subClassOf cim:IdentifiedObject ;
  skos:definition "Abstract parent class for all Dynamics function blocks."@en .

cim:EnergyConnection a owl:Class ;
  rdfs:label "EnergyConnection"@en ;
  dy:Package "Package_Wires" ;
  dy:isAbstract "True" ;
  rdfs:subClassOf cim:ConductingEquipment ;
  skos:definition "A connection of energy generation or consumption on the power system model."@en .

cim:EnergyConsumer a owl:Class ;
  rdfs:label "EnergyConsumer"@en ;
  dy:Package "Package_Wires" ;
  dy:isDescription "True" ;
  rdfs:subClassOf cim:EnergyConnection ;
  skos:definition """
Generic user of energy - a  point of consumption on the power system model.
EnergyConsumer.pfixed, .qfixed, .pfixedPct and .qfixedPct have meaning only if there is no LoadResponseCharacteristic associated with EnergyConsumer or if LoadResponseCharacteristic.exponentModel is set to False.
\t"""@en .

cim:Equipment a owl:Class ;
  rdfs:label "Equipment"@en ;
  dy:Package "Package_Core" ;
  dy:isAbstract "True" ;
  rdfs:subClassOf cim:PowerSystemResource ;
  skos:definition "The parts of a power system that are physical devices, electronic or mechanical."@en .

cim:ExcAC1A a owl:Class ;
  rdfs:label "ExcAC1A"@en ;
  dy:Package "Package_ExcitationSystemDynamics" ;
  rdfs:subClassOf cim:ExcitationSystemDynamics ;
  skos:definition "Modified IEEE AC1A alternator-supplied rectifier excitation system with different rate feedback source."@en .

cim:ExcAC2A a owl:Class ;
  rdfs:label "ExcAC2A"@en ;
  dy:Package "Package_ExcitationSystemDynamics" ;
  rdfs:subClassOf cim:ExcitationSystemDynamics ;
  skos:definition "Modified IEEE AC2A alternator-supplied rectifier excitation system with different field current limit."@en .

cim:ExcAC3A a owl:Class ;
  rdfs:label "ExcAC3A"@en ;
  dy:Package "Package_ExcitationSystemDynamics" ;
  rdfs:subClassOf cim:ExcitationSystemDynamics ;
  skos:definition "Modified IEEE AC3A alternator-supplied rectifier excitation system with different field current limit."@en .

cim:ExcAC4A a owl:Class ;
  rdfs:label "ExcAC4A"@en ;
  dy:Package "Package_ExcitationSystemDynamics" ;
  rdfs:subClassOf cim:ExcitationSystemDynamics ;
  skos:definition "Modified IEEE AC4A alternator-supplied rectifier excitation system with different minimum controller output."@en .

cim:ExcAC5A a owl:Class ;
  rdfs:label "ExcAC5A"@en ;
  dy:Package "Package_ExcitationSystemDynamics" ;
  rdfs:subClassOf cim:ExcitationSystemDynamics ;
  skos:definition "Modified IEEE AC5A alternator-supplied rectifier excitation system with different minimum controller output."@en .

cim:ExcAC6A a owl:Class ;
  rdfs:label "ExcAC6A"@en ;
  dy:Package "Package_ExcitationSystemDynamics" ;
  rdfs:subClassOf cim:ExcitationSystemDynamics ;
  skos:definition "Modified IEEE AC6A alternator-supplied rectifier excitation system with speed input."@en .

cim:ExcAC8B a owl:Class ;
  rdfs:label "ExcAC8B"@en ;
  dy:Package "Package_ExcitationSystemDynamics" ;
  rdfs:subClassOf cim:ExcitationSystemDynamics ;
  skos:definition "Modified IEEE AC8B alternator-supplied rectifier excitation system with speed input and input limiter."@en .

cim:ExcANS a owl:Class ;
  rdfs:label "ExcANS"@en ;
  dy:Package "Package_ExcitationSystemDynamics" ;
  rdfs:subClassOf cim:ExcitationSystemDynamics ;
  skos:definition "Italian excitation system. It represents static field voltage or excitation current feedback excitation system."@en .

cim:ExcAVR1 a owl:Class ;
  rdfs:label "ExcAVR1"@en ;
  dy:Package "Package_ExcitationSystemDynamics" ;
  rdfs:subClassOf cim:ExcitationSystemDynamics ;
  skos:definition "Italian excitation system corresponding to IEEE (1968) type 1 model. It represents an exciter dynamo and electromechanical regulator."@en .

cim:ExcAVR2 a owl:Class ;
  rdfs:label "ExcAVR2"@en ;
  dy:Package "Package_ExcitationSystemDynamics" ;
  rdfs:subClassOf cim:ExcitationSystemDynamics ;
  skos:definition "Italian excitation system corresponding to IEEE (1968) type 2 model. It represents an alternator and rotating diodes and electromechanic voltage regulators."@en .

cim:ExcAVR3 a owl:Class ;
  rdfs:label "ExcAVR3"@en ;
  dy:Package "Package_ExcitationSystemDynamics" ;
  rdfs:subClassOf cim:ExcitationSystemDynamics ;
  skos:definition "Italian excitation system. It represents an exciter dynamo and electric regulator. "@en .

cim:ExcAVR4 a owl:Class ;
  rdfs:label "ExcAVR4"@en ;
  dy:Package "Package_ExcitationSystemDynamics" ;
  rdfs:subClassOf cim:ExcitationSystemDynamics ;
  skos:definition "Italian excitation system. It represents a static exciter and electric voltage regulator."@en .

cim:ExcAVR5 a owl:Class ;
  rdfs:label "ExcAVR5"@en ;
  dy:Package "Package_ExcitationSystemDynamics" ;
  rdfs:subClassOf cim:ExcitationSystemDynamics ;
  skos:definition "Manual excitation control with field circuit resistance. This model can be used as a very simple representation of manual voltage control."@en .

cim:ExcAVR7 a owl:Class ;
  rdfs:label "ExcAVR7"@en ;
  dy:Package "Package_ExcitationSystemDynamics" ;
  rdfs:subClassOf cim:ExcitationSystemDynamics ;
  skos:definition "IVO excitation system."@en .

cim:ExcBBC a owl:Class ;
  rdfs:label "ExcBBC"@en ;
  dy:Package "Package_ExcitationSystemDynamics" ;
  rdfs:subClassOf cim:ExcitationSystemDynamics ;
  skos:definition "Transformer fed static excitation system (static with ABB regulator). This model represents a static excitation system in which a gated thyristor bridge fed by a transformer at the main generator terminals feeds the main generator directly."@en .

cim:ExcCZ a owl:Class ;
  rdfs:label "ExcCZ"@en ;
  dy:Package "Package_ExcitationSystemDynamics" ;
  rdfs:subClassOf cim:ExcitationSystemDynamics ;
  skos:definition "Czech proportion/integral exciter."@en .

cim:ExcDC1A a owl:Class ;
  rdfs:label "ExcDC1A"@en ;
  dy:Package "Package_ExcitationSystemDynamics" ;
  rdfs:subClassOf cim:ExcitationSystemDynamics ;
  skos:definition "Modified IEEE DC1A direct current commutator exciter with speed input and without underexcitation limiters (UEL) inputs."@en .

cim:ExcDC2A a owl:Class ;
  rdfs:label "ExcDC2A"@en ;
  dy:Package "Package_ExcitationSystemDynamics" ;
  rdfs:subClassOf cim:ExcitationSystemDynamics ;
  skos:definition "Modified IEEE DC2A direct current commutator exciter with speed input, one more leg block in feedback loop and without underexcitation limiters (UEL) inputs.  DC type 2 excitation system model with added speed multiplier, added lead-lag, and voltage-dependent limits."@en .

cim:ExcDC3A a owl:Class ;
  rdfs:label "ExcDC3A"@en ;
  dy:Package "Package_ExcitationSystemDynamics" ;
  rdfs:subClassOf cim:ExcitationSystemDynamics ;
  skos:definition "Modified IEEE DC3A direct current commutator exciter with speed input, and deadband.  DC old type 4."@en .

cim:ExcDC3A1 a owl:Class ;
  rdfs:label "ExcDC3A1"@en ;
  dy:Package "Package_ExcitationSystemDynamics" ;
  rdfs:subClassOf cim:ExcitationSystemDynamics ;
  skos:definition "Modified old IEEE type 3 excitation system."@en .

cim:ExcELIN1 a owl:Class ;
  rdfs:label "ExcELIN1"@en ;
  dy:Package "Package_ExcitationSystemDynamics" ;
  rdfs:subClassOf cim:ExcitationSystemDynamics ;
  skos:definition "Static PI transformer fed excitation system ELIN (VATECH) - simplified model.  This model represents an all-static excitation system. A PI voltage controller establishes a desired field current set point for a proportional current controller. The integrator of the PI controller has a follow-up input to match its signal to the present field current.  A power system stabilizer with power input is included in the model."@en .

cim:ExcELIN2 a owl:Class ;
  rdfs:label "ExcELIN2"@en ;
  dy:Package "Package_ExcitationSystemDynamics" ;
  rdfs:subClassOf cim:ExcitationSystemDynamics ;
  skos:definition "Detailed excitation system ELIN (VATECH).  This model represents an all-static excitation system. A PI voltage controller establishes a desired field current set point for a proportional current controller. The integrator of the PI controller has a follow-up input to match its signal to the present field current.  Power system stabilizer models used in conjunction with this excitation system model: PssELIN2, PssIEEE2B, Pss2B."@en .

cim:ExcHU a owl:Class ;
  rdfs:label "ExcHU"@en ;
  dy:Package "Package_ExcitationSystemDynamics" ;
  rdfs:subClassOf cim:ExcitationSystemDynamics ;
  skos:definition "Hungarian excitation system, with built-in voltage transducer."@en .

cim:ExcIEEEAC1A a owl:Class ;
  rdfs:label "ExcIEEEAC1A"@en ;
  dy:Package "Package_ExcitationSystemDynamics" ;
  rdfs:subClassOf cim:ExcitationSystemDynamics ;
  skos:definition """
IEEE 421.5-2005 type AC1A model. The model represents the field-controlled alternator-rectifier excitation systems designated type AC1A. These excitation systems consist of an alternator main exciter with non-controlled rectifiers.
Reference: IEEE 421.5-2005, 6.1.
\t"""@en .

cim:ExcIEEEAC2A a owl:Class ;
  rdfs:label "ExcIEEEAC2A"@en ;
  dy:Package "Package_ExcitationSystemDynamics" ;
  rdfs:subClassOf cim:ExcitationSystemDynamics ;
  skos:definition """
IEEE 421.5-2005 type AC2A model. The model represents a high initial response field-controlled alternator-rectifier excitation system. The alternator main exciter is used with non-controlled rectifiers. The type AC2A model is similar to that of type AC1A except for the inclusion of exciter time constant compensation and exciter field current limiting elements.
Reference: IEEE 421.5-2005, 6.2.
\t"""@en .

cim:ExcIEEEAC3A a owl:Class ;
  rdfs:label "ExcIEEEAC3A"@en ;
  dy:Package "Package_ExcitationSystemDynamics" ;
  rdfs:subClassOf cim:ExcitationSystemDynamics ;
  skos:definition """
IEEE 421.5-2005 type AC3A model. The model represents the field-controlled alternator-rectifier excitation systems designated type AC3A. These excitation systems include an alternator main exciter with non-controlled rectifiers. The exciter employs self-excitation, and the voltage regulator power is derived from the exciter output voltage.  Therefore, this system has an additional nonlinearity, simulated by the use of a multiplier whose inputs are the voltage regulator command signal, <i>Va</i>, and the exciter output voltage, <i>Efd</i>, times <i>K</i><i><sub>R</sub></i>.  This model is applicable to excitation systems employing static voltage regulators.
Reference: IEEE 421.5-2005, 6.3.
\t"""@en .

cim:ExcIEEEAC4A a owl:Class ;
  rdfs:label "ExcIEEEAC4A"@en ;
  dy:Package "Package_ExcitationSystemDynamics" ;
  rdfs:subClassOf cim:ExcitationSystemDynamics ;
  skos:definition """
IEEE 421.5-2005 type AC4A model. The model represents type AC4A alternator-supplied controlled-rectifier excitation system which is quite different from the other types of AC systems. This high initial response excitation system utilizes a full thyristor bridge in the exciter output circuit.  The voltage regulator controls the firing of the thyristor bridges. The exciter alternator uses an independent voltage regulator to control its output voltage to a constant value. These effects are not modelled; however, transient loading effects on the exciter alternator are included.
Reference: IEEE 421.5-2005, 6.4.
\t"""@en .

cim:ExcIEEEAC5A a owl:Class ;
  rdfs:label "ExcIEEEAC5A"@en ;
  dy:Package "Package_ExcitationSystemDynamics" ;
  rdfs:subClassOf cim:ExcitationSystemDynamics ;
  skos:definition """
IEEE 421.5-2005 type AC5A model. The model represents a simplified model for brushless excitation systems. The regulator is supplied from a source, such as a permanent magnet generator, which is not affected by system disturbances.  Unlike other AC models, this model uses loaded rather than open circuit exciter saturation data in the same way as it is used for the DC models.  Because the model has been widely implemented by the industry, it is sometimes used to represent other types of systems when either detailed data for them are not available or simplified models are required.
Reference: IEEE 421.5-2005, 6.5.
\t"""@en .

cim:ExcIEEEAC6A a owl:Class ;
  rdfs:label "ExcIEEEAC6A"@en ;
  dy:Package "Package_ExcitationSystemDynamics" ;
  rdfs:subClassOf cim:ExcitationSystemDynamics ;
  skos:definition """
IEEE 421.5-2005 type AC6A model. The model represents field-controlled alternator-rectifier excitation systems with system-supplied electronic voltage regulators.  The maximum output of the regulator, <i>V</i><i><sub>R</sub></i>, is a function of terminal voltage, <i>V</i><i><sub>T</sub></i>. The field current limiter included in the original model AC6A remains in the 2005 update.
Reference: IEEE 421.5-2005, 6.6. 


\t"""@en .

cim:ExcIEEEAC7B a owl:Class ;
  rdfs:label "ExcIEEEAC7B"@en ;
  dy:Package "Package_ExcitationSystemDynamics" ;
  rdfs:subClassOf cim:ExcitationSystemDynamics ;
  skos:definition """
IEEE 421.5-2005 type AC7B model. The model represents excitation systems which consist of an AC alternator with either stationary or rotating rectifiers to produce the DC field requirements. It is an upgrade to earlier AC excitation systems, which replace only the controls but retain the AC alternator and diode rectifier bridge.
Reference: IEEE 421.5-2005, 6.7. Note, however, that in IEEE 421.5-2005, the [1 / <i>sT</i><i><sub>E</sub></i>] block is shown as [1 / (1 + <i>sT</i><i><sub>E</sub></i>)], which is incorrect.
\t"""@en .

cim:ExcIEEEAC8B a owl:Class ;
  rdfs:label "ExcIEEEAC8B"@en ;
  dy:Package "Package_ExcitationSystemDynamics" ;
  rdfs:subClassOf cim:ExcitationSystemDynamics ;
  skos:definition """
IEEE 421.5-2005 type AC8B model. This model represents a PID voltage regulator with either a brushless exciter or DC exciter. The AVR in this model consists of PID control, with separate constants for the proportional (<i>K</i><i><sub>PR</sub></i>), integral (<i>K</i><i><sub>IR</sub></i>), and derivative (<i>K</i><i><sub>DR</sub></i>) gains. The representation of the brushless exciter (<i>T</i><i><sub>E</sub></i>, <i>K</i><i><sub>E</sub></i>, <i>S</i><i><sub>E</sub></i>, <i>K</i><i><sub>C</sub></i>, <i>K</i><i><sub>D</sub></i>) is similar to the model type AC2A. The type AC8B model can be used to represent static voltage regulators applied to brushless excitation systems. Digitally based voltage regulators feeding DC rotating main exciters can be represented with the AC type AC8B model with the parameters <i>K</i><i><sub>C</sub></i> and <i>K</i><i><sub>D</sub></i> set to 0.  For thyristor power stages fed from the generator terminals, the limits <i>V</i><i><sub>RMAX</sub></i> and <i>V</i><i><sub>RMIN</sub></i><i> </i>should be a function of terminal voltage: V<i><sub>T</sub></i> x <i>V</i><i><sub>RMAX</sub></i><sub> </sub>and <i>V</i><i><sub>T</sub></i> x <i>V</i><i><sub>RMIN</sub></i>.
Reference: IEEE 421.5-2005, 6.8. 
\t"""@en .

cim:ExcIEEEDC1A a owl:Class ;
  rdfs:label "ExcIEEEDC1A"@en ;
  dy:Package "Package_ExcitationSystemDynamics" ;
  rdfs:subClassOf cim:ExcitationSystemDynamics ;
  skos:definition """
IEEE 421.5-2005 type DC1A model. This model represents field-controlled DC commutator exciters with continuously acting voltage regulators (especially the direct-acting rheostatic, rotating amplifier, and magnetic amplifier types).  Because this model has been widely implemented by the industry, it is sometimes used to represent other types of systems when detailed data for them are not available or when a simplified model is required.
Reference: IEEE 421.5-2005, 5.1. 
\t"""@en .

cim:ExcIEEEDC2A a owl:Class ;
  rdfs:label "ExcIEEEDC2A"@en ;
  dy:Package "Package_ExcitationSystemDynamics" ;
  rdfs:subClassOf cim:ExcitationSystemDynamics ;
  skos:definition """
IEEE 421.5-2005 type DC2A model. This model represents field-controlled DC commutator exciters with continuously acting voltage regulators having supplies obtained from the generator or auxiliary bus.  It differs from the type DC1A model only in the voltage regulator output limits, which are now proportional to terminal voltage <i>V</i><i><sub>T</sub></i>.
It is representative of solid-state replacements for various forms of older mechanical and rotating amplifier regulating equipment connected to DC commutator exciters.
Reference: IEEE 421.5-2005, 5.2. 
\t"""@en .

cim:ExcIEEEDC3A a owl:Class ;
  rdfs:label "ExcIEEEDC3A"@en ;
  dy:Package "Package_ExcitationSystemDynamics" ;
  rdfs:subClassOf cim:ExcitationSystemDynamics ;
  skos:definition """
IEEE 421.5-2005 type DC3A model. This model represents older systems, in particular those DC commutator exciters with non-continuously acting regulators that were commonly used before the development of the continuously acting varieties.  These systems respond at basically two different rates, depending upon the magnitude of voltage error. For small errors, adjustment is made periodically with a signal to a motor-operated rheostat. Larger errors cause resistors to be quickly shorted or inserted and a strong forcing signal applied to the exciter. Continuous motion of the motor-operated rheostat occurs for these larger error signals, even though it is bypassed by contactor action.
Reference: IEEE 421.5-2005, 5.3. 
\t"""@en .

cim:ExcIEEEDC4B a owl:Class ;
  rdfs:label "ExcIEEEDC4B"@en ;
  dy:Package "Package_ExcitationSystemDynamics" ;
  rdfs:subClassOf cim:ExcitationSystemDynamics ;
  skos:definition """
IEEE 421.5-2005 type DC4B model. These excitation systems utilize a field-controlled DC commutator exciter with a continuously acting voltage regulator having supplies obtained from the generator or auxiliary bus.
Reference: IEEE 421.5-2005, 5.4. 
\t"""@en .

cim:ExcIEEEST1A a owl:Class ;
  rdfs:label "ExcIEEEST1A"@en ;
  dy:Package "Package_ExcitationSystemDynamics" ;
  rdfs:subClassOf cim:ExcitationSystemDynamics ;
  skos:definition """
IEEE 421.5-2005 type ST1A model. This model represents systems in which excitation power is supplied through a transformer from the generator terminals (or the unit’s auxiliary bus) and is regulated by a controlled rectifier.  The maximum exciter voltage available from such systems is directly related to the generator terminal voltage.
Reference: IEEE 421.5-2005, 7.1. 
\t"""@en .

cim:ExcIEEEST1AUELselectorKind a owl:Class ;
  rdfs:label "ExcIEEEST1AUELselectorKind"@en ;
  dy:Package "Package_Domain" ;
  owl:oneOf ( cim:ExcIEEEST1AUELselectorKind.ignoreUELsignal
    cim:ExcIEEEST1AUELselectorKind.inputHVgateVoltageOutput
    cim:ExcIEEEST1AUELselectorKind.inputHVgateErrorSignal
    cim:ExcIEEEST1AUELselectorKind.inputAddedToErrorSignal ) ;
  rdfs:subClassOf cim:Enumeration ;
  skos:definition "Types of connections for the UEL input used in ExcIEEEST1A."@en .

cim:ExcIEEEST2A a owl:Class ;
  rdfs:label "ExcIEEEST2A"@en ;
  dy:Package "Package_ExcitationSystemDynamics" ;
  rdfs:subClassOf cim:ExcitationSystemDynamics ;
  skos:definition """
IEEE 421.5-2005 type ST2A model. Some static systems use both current and voltage sources (generator terminal quantities) to comprise the power source.  The regulator controls the exciter output through controlled saturation of the power transformer components.  These compound-source rectifier excitation systems are designated type ST2A and are represented by ExcIEEEST2A.
Reference: IEEE 421.5-2005, 7.2. 
\t"""@en .

cim:ExcIEEEST3A a owl:Class ;
  rdfs:label "ExcIEEEST3A"@en ;
  dy:Package "Package_ExcitationSystemDynamics" ;
  rdfs:subClassOf cim:ExcitationSystemDynamics ;
  skos:definition """
IEEE 421.5-2005 type ST3A model.  Some static systems utilize a field voltage control loop to linearize the exciter control characteristic. This also makes the output independent of supply source variations until supply limitations are reached.  These systems utilize a variety of controlled-rectifier designs: full thyristor complements or hybrid bridges in either series or shunt configurations. The power source can consist of only a potential source, either fed from the machine terminals or from internal windings. Some designs can have compound power sources utilizing both machine potential and current. These power sources are represented as phasor combinations of machine terminal current and voltage and are accommodated by suitable parameters in model type ST3A which is represented by ExcIEEEST3A.
Reference: IEEE 421.5-2005, 7.3. 
\t"""@en .

cim:ExcIEEEST4B a owl:Class ;
  rdfs:label "ExcIEEEST4B"@en ;
  dy:Package "Package_ExcitationSystemDynamics" ;
  rdfs:subClassOf cim:ExcitationSystemDynamics ;
  skos:definition """
IEEE 421.5-2005 type ST4B model. This model is a variation of the type ST3A model, with a proportional plus integral (PI) regulator block replacing the lag-lead regulator characteristic that is in the ST3A model. Both potential and compound source rectifier excitation systems are modelled.  The PI regulator blocks have non-windup limits that are represented. The voltage regulator of this model is typically implemented digitally.
Reference: IEEE 421.5-2005, 7.4. 
\t"""@en .

cim:ExcIEEEST5B a owl:Class ;
  rdfs:label "ExcIEEEST5B"@en ;
  dy:Package "Package_ExcitationSystemDynamics" ;
  rdfs:subClassOf cim:ExcitationSystemDynamics ;
  skos:definition """
IEEE 421.5-2005 type ST5B model. The type ST5B excitation system is a variation of the type ST1A model, with alternative overexcitation and underexcitation inputs and additional limits.
The block diagram in the IEEE 421.5 standard has input signal <i>Vc </i>and does not indicate the summation point with <i>Vref</i>. The implementation of the ExcIEEEST5B shall consider summation point with <i>Vref</i>.
Reference: IEEE 421.5-2005, 7.5. 
\t"""@en .

cim:ExcIEEEST6B a owl:Class ;
  rdfs:label "ExcIEEEST6B"@en ;
  dy:Package "Package_ExcitationSystemDynamics" ;
  rdfs:subClassOf cim:ExcitationSystemDynamics ;
  skos:definition """
IEEE 421.5-2005 type ST6B model. This model consists of a PI voltage regulator with an inner loop field voltage regulator and pre-control. The field voltage regulator implements a proportional control. The pre-control and the delay in the feedback circuit increase the dynamic response.
Reference: IEEE 421.5-2005, 7.6. 
\t"""@en .

cim:ExcIEEEST7B a owl:Class ;
  rdfs:label "ExcIEEEST7B"@en ;
  dy:Package "Package_ExcitationSystemDynamics" ;
  rdfs:subClassOf cim:ExcitationSystemDynamics ;
  skos:definition """
IEEE 421.5-2005 type ST7B model. This model is representative of static potential-source excitation systems. In this system, the AVR consists of a PI voltage regulator. A phase lead-lag filter in series allows the introduction of a derivative function, typically used with brushless excitation systems. In that case, the regulator is of the PID type. In addition, the terminal voltage channel includes a phase lead-lag filter.  The AVR includes the appropriate inputs on its reference for overexcitation limiter (OEL1), underexcitation limiter (UEL), stator current limiter (SCL), and current compensator (DROOP). All these limitations, when they work at voltage reference level, keep the PSS (VS signal from PSS) in operation. However, the UEL limitation can also be transferred to the high value (HV) gate acting on the output signal. In addition, the output signal passes through a low value (LV) gate for a ceiling overexcitation limiter (OEL2).
Reference: IEEE 421.5-2005, 7.7. 
\t"""@en .

cim:ExcNI a owl:Class ;
  rdfs:label "ExcNI"@en ;
  dy:Package "Package_ExcitationSystemDynamics" ;
  rdfs:subClassOf cim:ExcitationSystemDynamics ;
  skos:definition "Bus or solid fed SCR (silicon-controlled rectifier) bridge excitation system model type NI (NVE)."@en .

cim:ExcOEX3T a owl:Class ;
  rdfs:label "ExcOEX3T"@en ;
  dy:Package "Package_ExcitationSystemDynamics" ;
  rdfs:subClassOf cim:ExcitationSystemDynamics ;
  skos:definition "Modified IEEE type ST1 excitation system with semi-continuous and acting terminal voltage limiter."@en .

cim:ExcPIC a owl:Class ;
  rdfs:label "ExcPIC"@en ;
  dy:Package "Package_ExcitationSystemDynamics" ;
  rdfs:subClassOf cim:ExcitationSystemDynamics ;
  skos:definition "Proportional/integral regulator excitation system.  This model can be used to represent excitation systems with a proportional-integral (PI) voltage regulator controller. "@en .

cim:ExcREXS a owl:Class ;
  rdfs:label "ExcREXS"@en ;
  dy:Package "Package_ExcitationSystemDynamics" ;
  rdfs:subClassOf cim:ExcitationSystemDynamics ;
  skos:definition "General purpose rotating excitation system.  This model can be used to represent a wide range of excitation systems whose DC power source is an AC or DC generator. It encompasses IEEE type AC1, AC2, DC1, and DC2 excitation system models. "@en .

cim:ExcREXSFeedbackSignalKind a owl:Class ;
  rdfs:label "ExcREXSFeedbackSignalKind"@en ;
  dy:Package "Package_Domain" ;
  owl:oneOf ( cim:ExcREXSFeedbackSignalKind.fieldVoltage cim:ExcREXSFeedbackSignalKind.fieldCurrent
    cim:ExcREXSFeedbackSignalKind.outputVoltage ) ;
  rdfs:subClassOf cim:Enumeration ;
  skos:definition "Types of rate feedback signals. "@en .

cim:ExcRQB a owl:Class ;
  rdfs:label "ExcRQB"@en ;
  dy:Package "Package_ExcitationSystemDynamics" ;
  rdfs:subClassOf cim:ExcitationSystemDynamics ;
  skos:definition "Excitation system type RQB (four-loop regulator, r?gulateur quatre boucles, developed in France) primarily used in nuclear or thermal generating units. This excitation system shall be always used together with power system stabilizer type PssRQB.   "@en .

cim:ExcSCRX a owl:Class ;
  rdfs:label "ExcSCRX"@en ;
  dy:Package "Package_ExcitationSystemDynamics" ;
  rdfs:subClassOf cim:ExcitationSystemDynamics ;
  skos:definition "Simple excitation system with generic characteristics typical of many excitation systems; intended for use where negative field current could be a problem."@en .

cim:ExcSEXS a owl:Class ;
  rdfs:label "ExcSEXS"@en ;
  dy:Package "Package_ExcitationSystemDynamics" ;
  rdfs:subClassOf cim:ExcitationSystemDynamics ;
  skos:definition "Simplified excitation system."@en .

cim:ExcSK a owl:Class ;
  rdfs:label "ExcSK"@en ;
  dy:Package "Package_ExcitationSystemDynamics" ;
  rdfs:subClassOf cim:ExcitationSystemDynamics ;
  skos:definition "Slovakian excitation system.  UEL and secondary voltage control are included in this model. When this model is used, there cannot be a separate underexcitation limiter or VAr controller model."@en .

cim:ExcST1A a owl:Class ;
  rdfs:label "ExcST1A"@en ;
  dy:Package "Package_ExcitationSystemDynamics" ;
  rdfs:subClassOf cim:ExcitationSystemDynamics ;
  skos:definition "Modification of an old IEEE ST1A static excitation system without overexcitation limiter (OEL) and underexcitation limiter (UEL)."@en .

cim:ExcST2A a owl:Class ;
  rdfs:label "ExcST2A"@en ;
  dy:Package "Package_ExcitationSystemDynamics" ;
  rdfs:subClassOf cim:ExcitationSystemDynamics ;
  skos:definition "Modified IEEE ST2A static excitation system with another lead-lag block added to match the model defined by WECC."@en .

cim:ExcST3A a owl:Class ;
  rdfs:label "ExcST3A"@en ;
  dy:Package "Package_ExcitationSystemDynamics" ;
  rdfs:subClassOf cim:ExcitationSystemDynamics ;
  skos:definition "Modified IEEE ST3A static excitation system with added speed multiplier."@en .

cim:ExcST4B a owl:Class ;
  rdfs:label "ExcST4B"@en ;
  dy:Package "Package_ExcitationSystemDynamics" ;
  rdfs:subClassOf cim:ExcitationSystemDynamics ;
  skos:definition "Modified IEEE ST4B static excitation system with maximum inner loop feedback gain <i>Vgmax</i>."@en .

cim:ExcST6B a owl:Class ;
  rdfs:label "ExcST6B"@en ;
  dy:Package "Package_ExcitationSystemDynamics" ;
  rdfs:subClassOf cim:ExcitationSystemDynamics ;
  skos:definition "Modified IEEE ST6B static excitation system with PID controller and optional inner feedback loop."@en .

cim:ExcST6BOELselectorKind a owl:Class ;
  rdfs:label "ExcST6BOELselectorKind"@en ;
  dy:Package "Package_Domain" ;
  owl:oneOf ( cim:ExcST6BOELselectorKind.noOELinput cim:ExcST6BOELselectorKind.beforeUEL
    cim:ExcST6BOELselectorKind.afterUEL ) ;
  rdfs:subClassOf cim:Enumeration ;
  skos:definition "Types of connections for the OEL input used for static excitation systems type 6B."@en .

cim:ExcST7B a owl:Class ;
  rdfs:label "ExcST7B"@en ;
  dy:Package "Package_ExcitationSystemDynamics" ;
  rdfs:subClassOf cim:ExcitationSystemDynamics ;
  skos:definition "Modified IEEE ST7B static excitation system without stator current limiter (SCL) and current compensator (DROOP) inputs."@en .

cim:ExcST7BOELselectorKind a owl:Class ;
  rdfs:label "ExcST7BOELselectorKind"@en ;
  dy:Package "Package_Domain" ;
  owl:oneOf ( cim:ExcST7BOELselectorKind.noOELinput cim:ExcST7BOELselectorKind.addVref
    cim:ExcST7BOELselectorKind.inputLVgate cim:ExcST7BOELselectorKind.outputLVgate ) ;
  rdfs:subClassOf cim:Enumeration ;
  skos:definition "Types of connections for the OEL input used for static excitation systems type 7B."@en .

cim:ExcST7BUELselectorKind a owl:Class ;
  rdfs:label "ExcST7BUELselectorKind"@en ;
  dy:Package "Package_Domain" ;
  owl:oneOf ( cim:ExcST7BUELselectorKind.noUELinput cim:ExcST7BUELselectorKind.addVref
    cim:ExcST7BUELselectorKind.inputHVgate cim:ExcST7BUELselectorKind.outputHVgate ) ;
  rdfs:subClassOf cim:Enumeration ;
  skos:definition "Types of connections for the UEL input used for static excitation systems type 7B."@en .

cim:ExcitationSystemDynamics a owl:Class ;
  rdfs:label "ExcitationSystemDynamics"@en ;
  dy:Package "Package_ExcitationSystemDynamics" ;
  dy:isAbstract "True" ;
  rdfs:subClassOf cim:DynamicsFunctionBlock ;
  skos:definition "Excitation system function block whose behaviour is described by reference to a standard model <font color=\"#0f0f0f\">or by definition of a user-defined model.</font>"@en .

cim:ExcitationSystemUserDefined a owl:Class ;
  rdfs:label "ExcitationSystemUserDefined"@en ;
  dy:Package "Package_UserDefinedModels" ;
  rdfs:subClassOf cim:ExcitationSystemDynamics ;
  skos:definition "Excitation system function block whose dynamic behaviour is described by <font color=\"#0f0f0f\">a user-defined model.</font>"@en .

cim:Float a owl:Class ;
  rdfs:label "Float"@en ;
  dy:Package "Package_Domain" ;
  dy:isPrimitive "True" ;
  skos:definition """
A floating point number. The range is unspecified and not limited.

\t"""@en .

cim:FrancisGovernorControlKind a owl:Class ;
  rdfs:label "FrancisGovernorControlKind"@en ;
  dy:Package "Package_Domain" ;
  owl:oneOf ( cim:FrancisGovernorControlKind.mechanicHydrolicTachoAccelerator
    cim:FrancisGovernorControlKind.mechanicHydraulicTransientFeedback
    cim:FrancisGovernorControlKind.electromechanicalElectrohydraulic ) ;
  rdfs:subClassOf cim:Enumeration ;
  skos:definition "Governor control flag for Francis hydro model."@en .

cim:Frequency a owl:Class ;
  rdfs:label "Frequency"@en ;
  dy:Package "Package_Domain" ;
  dy:isCIMDatatype "True" ;
  skos:definition "Cycles per second."@en .

cim:GenICompensationForGenJ a owl:Class ;
  rdfs:label "GenICompensationForGenJ"@en ;
  dy:Package "Package_VoltageCompensatorDynamics" ;
  rdfs:subClassOf cim:IdentifiedObject ;
  skos:definition "Resistive and reactive components of compensation for generator associated with IEEE type 2 voltage compensator for current flow out of another generator in the interconnection."@en .

cim:GenericNonLinearLoadModelKind a owl:Class ;
  rdfs:label "GenericNonLinearLoadModelKind"@en ;
  dy:Package "Package_Domain" ;
  owl:oneOf ( cim:GenericNonLinearLoadModelKind.exponentialRecovery
    cim:GenericNonLinearLoadModelKind.loadAdaptive ) ;
  rdfs:subClassOf cim:Enumeration ;
  skos:definition "Type of generic non-linear load model."@en .

cim:GovCT1 a owl:Class ;
  rdfs:label "GovCT1"@en ;
  dy:Package "Package_TurbineGovernorDynamics" ;
  rdfs:subClassOf cim:TurbineGovernorDynamics ;
  skos:definition """
General model for any prime mover with a PID governor, used primarily for combustion turbine and combined cycle units.
This model can be used to represent a variety of prime movers controlled by PID governors.  It is suitable, for example, for the representation of: 
<ul>
<li>gas turbine and single shaft combined cycle turbines</li>
</ul>
<ul>
<li>diesel engines with modern electronic or digital governors  </li>
</ul>
<ul>
<li>steam turbines where steam is supplied from a large boiler drum or a large header whose pressure is substantially constant over the period under study</li>
<li>simple hydro turbines in dam configurations where the water column length is short and water inertia effects are minimal.</li>
</ul>
Additional information on this model is available in the 2012 IEEE report, <i><u>Dynamic Models for Turbine-Governors in Power System Studies</u></i>, 3.1.2.3 pages 3-4 (GGOV1).
\t"""@en .

cim:GovCT2 a owl:Class ;
  rdfs:label "GovCT2"@en ;
  dy:Package "Package_TurbineGovernorDynamics" ;
  rdfs:subClassOf cim:TurbineGovernorDynamics ;
  skos:definition "General governor with frequency-dependent fuel flow limit.  This model is a modification of the GovCT1<b> </b>model in order to represent the frequency-dependent fuel flow limit of a specific gas turbine manufacturer."@en .

cim:GovGAST a owl:Class ;
  rdfs:label "GovGAST"@en ;
  dy:Package "Package_TurbineGovernorDynamics" ;
  rdfs:subClassOf cim:TurbineGovernorDynamics ;
  skos:definition "Single shaft gas turbine."@en .

cim:GovGAST1 a owl:Class ;
  rdfs:label "GovGAST1"@en ;
  dy:Package "Package_TurbineGovernorDynamics" ;
  rdfs:subClassOf cim:TurbineGovernorDynamics ;
  skos:definition "Modified single shaft gas turbine."@en .

cim:GovGAST2 a owl:Class ;
  rdfs:label "GovGAST2"@en ;
  dy:Package "Package_TurbineGovernorDynamics" ;
  rdfs:subClassOf cim:TurbineGovernorDynamics ;
  skos:definition "Gas turbine."@en .

cim:GovGAST3 a owl:Class ;
  rdfs:label "GovGAST3"@en ;
  dy:Package "Package_TurbineGovernorDynamics" ;
  rdfs:subClassOf cim:TurbineGovernorDynamics ;
  skos:definition "Generic turbogas with acceleration and temperature controller."@en .

cim:GovGAST4 a owl:Class ;
  rdfs:label "GovGAST4"@en ;
  dy:Package "Package_TurbineGovernorDynamics" ;
  rdfs:subClassOf cim:TurbineGovernorDynamics ;
  skos:definition "Generic turbogas."@en .

cim:GovGASTWD a owl:Class ;
  rdfs:label "GovGASTWD"@en ;
  dy:Package "Package_TurbineGovernorDynamics" ;
  rdfs:subClassOf cim:TurbineGovernorDynamics ;
  skos:definition """
Woodward™ gas turbine governor. 
[Footnote: Woodward gas turbines are an example of suitable products available commercially. This information is given for the convenience of users of this document and does not constitute an endorsement by IEC of these products.] 


\t"""@en .

cim:GovHydro1 a owl:Class ;
  rdfs:label "GovHydro1"@en ;
  dy:Package "Package_TurbineGovernorDynamics" ;
  rdfs:subClassOf cim:TurbineGovernorDynamics ;
  skos:definition "Basic hydro turbine governor."@en .

cim:GovHydro2 a owl:Class ;
  rdfs:label "GovHydro2"@en ;
  dy:Package "Package_TurbineGovernorDynamics" ;
  rdfs:subClassOf cim:TurbineGovernorDynamics ;
  skos:definition "IEEE hydro turbine governor with straightforward penstock configuration and hydraulic-dashpot governor."@en .

cim:GovHydro3 a owl:Class ;
  rdfs:label "GovHydro3"@en ;
  dy:Package "Package_TurbineGovernorDynamics" ;
  rdfs:subClassOf cim:TurbineGovernorDynamics ;
  skos:definition "Modified IEEE hydro governor-turbine. This model differs from that defined in the IEEE modelling guideline paper in that the limits on gate position and velocity do not permit \"wind up\" of the upstream signals."@en .

cim:GovHydro4 a owl:Class ;
  rdfs:label "GovHydro4"@en ;
  dy:Package "Package_TurbineGovernorDynamics" ;
  rdfs:subClassOf cim:TurbineGovernorDynamics ;
  skos:definition "Hydro turbine and governor. Represents plants with straight-forward penstock configurations and hydraulic governors of the traditional 'dashpot' type.  This model can be used to represent simple, Francis/Pelton or Kaplan turbines."@en .

cim:GovHydro4ModelKind a owl:Class ;
  rdfs:label "GovHydro4ModelKind"@en ;
  dy:Package "Package_Domain" ;
  owl:oneOf ( cim:GovHydro4ModelKind.simple cim:GovHydro4ModelKind.francisPelton
    cim:GovHydro4ModelKind.kaplan ) ;
  rdfs:subClassOf cim:Enumeration ;
  skos:definition "Possible types of GovHydro4 models."@en .

cim:GovHydroDD a owl:Class ;
  rdfs:label "GovHydroDD"@en ;
  dy:Package "Package_TurbineGovernorDynamics" ;
  rdfs:subClassOf cim:TurbineGovernorDynamics ;
  skos:definition "Double derivative hydro governor and turbine."@en .

cim:GovHydroFrancis a owl:Class ;
  rdfs:label "GovHydroFrancis"@en ;
  dy:Package "Package_TurbineGovernorDynamics" ;
  rdfs:subClassOf cim:TurbineGovernorDynamics ;
  skos:definition """
Detailed hydro unit - Francis model.  This model can be used to represent three types of governors.
A schematic of the hydraulic system of detailed hydro unit models, such as Francis and Pelton, is provided in the DetailedHydroModelHydraulicSystem diagram.
\t"""@en .

cim:GovHydroIEEE0 a owl:Class ;
  rdfs:label "GovHydroIEEE0"@en ;
  dy:Package "Package_TurbineGovernorDynamics" ;
  rdfs:subClassOf cim:TurbineGovernorDynamics ;
  skos:definition """
IEEE simplified hydro governor-turbine model.  Used for mechanical-hydraulic and electro-hydraulic turbine governors, with or without steam feedback. Typical values given are for mechanical-hydraulic turbine-governor.
Ref<font color="#0f0f0f">erence: IEEE Transactions on Power Apparatus and Systems, November/December 1973, Volume PAS-92, Number 6, <i><u>Dynamic Models for Steam and Hydro Turbines in Power System Studies</u></i>, page 1904.</font>
\t"""@en .

cim:GovHydroIEEE2 a owl:Class ;
  rdfs:label "GovHydroIEEE2"@en ;
  dy:Package "Package_TurbineGovernorDynamics" ;
  rdfs:subClassOf cim:TurbineGovernorDynamics ;
  skos:definition """
IEEE hydro turbine governor model represents plants with straightforward penstock configurations and hydraulic-dashpot governors.
Ref<font color="#0f0f0f">erence: IEEE Transactions on Power Apparatus and Systems, November/December 1973, Volume PAS-92, Number 6, <i><u>Dynamic Models for Steam and Hydro Turbines in Power System Studies</u></i>, page 1904.</font>
\t"""@en .

cim:GovHydroPID a owl:Class ;
  rdfs:label "GovHydroPID"@en ;
  dy:Package "Package_TurbineGovernorDynamics" ;
  rdfs:subClassOf cim:TurbineGovernorDynamics ;
  skos:definition "PID governor and turbine."@en .

cim:GovHydroPID2 a owl:Class ;
  rdfs:label "GovHydroPID2"@en ;
  dy:Package "Package_TurbineGovernorDynamics" ;
  rdfs:subClassOf cim:TurbineGovernorDynamics ;
  skos:definition """
Hydro turbine and governor. Represents plants with straightforward penstock configurations and "three term" electro-hydraulic governors (i.e. Woodward<sup>TM</sup> electronic).
[Footnote: Woodward electronic governors are an example of suitable products available commercially. This information is given for the convenience of users of this document and does not constitute an endorsement by IEC of these products.] 

\t"""@en .

cim:GovHydroPelton a owl:Class ;
  rdfs:label "GovHydroPelton"@en ;
  dy:Package "Package_TurbineGovernorDynamics" ;
  rdfs:subClassOf cim:TurbineGovernorDynamics ;
  skos:definition """
Detailed hydro unit - Pelton model.  This model can be used to represent the dynamic related to water tunnel and surge chamber.
The DetailedHydroModelHydraulicSystem diagram, located under the GovHydroFrancis class, provides a schematic of the hydraulic system of detailed hydro unit models, such as Francis and Pelton.
\t"""@en .

cim:GovHydroR a owl:Class ;
  rdfs:label "GovHydroR"@en ;
  dy:Package "Package_TurbineGovernorDynamics" ;
  rdfs:subClassOf cim:TurbineGovernorDynamics ;
  skos:definition "Fourth order lead-lag governor and hydro turbine. "@en .

cim:GovHydroWEH a owl:Class ;
  rdfs:label "GovHydroWEH"@en ;
  dy:Package "Package_TurbineGovernorDynamics" ;
  rdfs:subClassOf cim:TurbineGovernorDynamics ;
  skos:definition """
Woodward<sup>TM </sup>electric hydro governor. 
[Footnote: Woodward electric hydro governors are an example of suitable products available commercially. This information is given for the convenience of users of this document and does not constitute an endorsement by IEC of these products.]
\t"""@en .

cim:GovHydroWPID a owl:Class ;
  rdfs:label "GovHydroWPID"@en ;
  dy:Package "Package_TurbineGovernorDynamics" ;
  rdfs:subClassOf cim:TurbineGovernorDynamics ;
  skos:definition """
Woodward<sup>TM</sup> PID hydro governor.
[Footnote: Woodward PID hydro governors are an example of suitable products available commercially. This information is given for the convenience of users of this document and does not constitute an endorsement by IEC of these products.]
\t"""@en .

cim:GovSteam0 a owl:Class ;
  rdfs:label "GovSteam0"@en ;
  dy:Package "Package_TurbineGovernorDynamics" ;
  rdfs:subClassOf cim:TurbineGovernorDynamics ;
  skos:definition "A simplified steam turbine governor."@en .

cim:GovSteam1 a owl:Class ;
  rdfs:label "GovSteam1"@en ;
  dy:Package "Package_TurbineGovernorDynamics" ;
  rdfs:subClassOf cim:TurbineGovernorDynamics ;
  skos:definition "Steam turbine governor, based on the GovSteamIEEE1 (with optional deadband and nonlinear valve gain added). "@en .

cim:GovSteam2 a owl:Class ;
  rdfs:label "GovSteam2"@en ;
  dy:Package "Package_TurbineGovernorDynamics" ;
  rdfs:subClassOf cim:TurbineGovernorDynamics ;
  skos:definition "Simplified governor."@en .

cim:GovSteamBB a owl:Class ;
  rdfs:label "GovSteamBB"@en ;
  dy:Package "Package_TurbineGovernorDynamics" ;
  rdfs:subClassOf cim:TurbineGovernorDynamics ;
  skos:definition "European governor model."@en .

cim:GovSteamCC a owl:Class ;
  rdfs:label "GovSteamCC"@en ;
  dy:Package "Package_TurbineGovernorDynamics" ;
  rdfs:subClassOf cim:CrossCompoundTurbineGovernorDynamics ;
  skos:definition "Cross compound turbine governor.  Unlike tandem compound units, cross compound units are not on the same shaft."@en .

cim:GovSteamEU a owl:Class ;
  rdfs:label "GovSteamEU"@en ;
  dy:Package "Package_TurbineGovernorDynamics" ;
  rdfs:subClassOf cim:TurbineGovernorDynamics ;
  skos:definition "Simplified boiler and steam turbine with PID governor."@en .

cim:GovSteamFV2 a owl:Class ;
  rdfs:label "GovSteamFV2"@en ;
  dy:Package "Package_TurbineGovernorDynamics" ;
  rdfs:subClassOf cim:TurbineGovernorDynamics ;
  skos:definition "Steam turbine governor with reheat time constants and modelling of the effects of fast valve closing to reduce mechanical power."@en .

cim:GovSteamFV3 a owl:Class ;
  rdfs:label "GovSteamFV3"@en ;
  dy:Package "Package_TurbineGovernorDynamics" ;
  rdfs:subClassOf cim:TurbineGovernorDynamics ;
  skos:definition "Simplified GovSteamIEEE1 steam turbine governor with Prmax limit and fast valving."@en .

cim:GovSteamFV4 a owl:Class ;
  rdfs:label "GovSteamFV4"@en ;
  dy:Package "Package_TurbineGovernorDynamics" ;
  rdfs:subClassOf cim:TurbineGovernorDynamics ;
  skos:definition "Detailed electro-hydraulic governor for steam unit."@en .

cim:GovSteamIEEE1 a owl:Class ;
  rdfs:label "GovSteamIEEE1"@en ;
  dy:Package "Package_TurbineGovernorDynamics" ;
  rdfs:subClassOf cim:TurbineGovernorDynamics ;
  skos:definition """
IEEE steam turbine governor model.
Ref<font color="#0f0f0f">erence: IEEE Transactions on Power Apparatus and Systems, November/December 1973, Volume PAS-92, Number 6, <i><u>Dynamic Models for Steam and Hydro Turbines in Power System Studies</u></i>, page 1904.</font>
\t"""@en .

cim:GovSteamSGO a owl:Class ;
  rdfs:label "GovSteamSGO"@en ;
  dy:Package "Package_TurbineGovernorDynamics" ;
  rdfs:subClassOf cim:TurbineGovernorDynamics ;
  skos:definition "Simplified steam turbine governor."@en .

cim:HVDCDynamics a owl:Class ;
  rdfs:label "HVDCDynamics"@en ;
  dy:Package "Package_HVDCDynamics" ;
  dy:isAbstract "True" ;
  rdfs:subClassOf cim:DynamicsFunctionBlock ;
  skos:definition "HVDC whose behaviour is described by reference to a standard model <font color=\"#0f0f0f\">or by definition of a user-defined model.</font>"@en .

cim:IdentifiedObject a owl:Class ;
  rdfs:label "IdentifiedObject"@en ;
  dy:Package "Package_Core" ;
  dy:isAbstract "True" ;
  skos:definition "This is a root class to provide common identification for all classes needing identification and naming attributes."@en .

cim:IfdBaseKind a owl:Class ;
  rdfs:label "IfdBaseKind"@en ;
  dy:Package "Package_Domain" ;
  owl:oneOf ( cim:IfdBaseKind.ifag cim:IfdBaseKind.ifnl cim:IfdBaseKind.iffl ) ;
  rdfs:subClassOf cim:Enumeration ;
  skos:definition "Excitation base system mode."@en .

cim:InputSignalKind a owl:Class ;
  rdfs:label "InputSignalKind"@en ;
  dy:Package "Package_Domain" ;
  owl:oneOf ( cim:InputSignalKind.rotorSpeed cim:InputSignalKind.rotorAngularFrequencyDeviation
    cim:InputSignalKind.busFrequency cim:InputSignalKind.busFrequencyDeviation
    cim:InputSignalKind.generatorElectricalPower cim:InputSignalKind.generatorAcceleratingPower
    cim:InputSignalKind.busVoltage cim:InputSignalKind.busVoltageDerivative
    cim:InputSignalKind.branchCurrent cim:InputSignalKind.fieldCurrent
    cim:InputSignalKind.generatorMechanicalPower ) ;
  rdfs:subClassOf cim:Enumeration ;
  skos:definition "Types of input signals.  In dynamics modelling, commonly represented by the <i>j</i> parameter."@en .

cim:Integer a owl:Class ;
  rdfs:label "Integer"@en ;
  dy:Package "Package_Domain" ;
  dy:isPrimitive "True" ;
  skos:definition """
An integer number. The range is unspecified and not limited.

\t"""@en .

cim:Length a owl:Class ;
  rdfs:label "Length"@en ;
  dy:Package "Package_Domain" ;
  dy:isCIMDatatype "True" ;
  skos:definition "Unit of length. It shall be a positive value or zero."@en .

cim:LoadAggregate a owl:Class ;
  rdfs:label "LoadAggregate"@en ;
  dy:Package "Package_LoadDynamics" ;
  rdfs:subClassOf cim:LoadDynamics ;
  skos:definition """
Aggregate loads are used to represent all or part of the real and reactive load from one or more loads in the static (power flow) data. This load is usually the aggregation of many individual load devices and the load model is an approximate representation of the aggregate response of the load devices to system disturbances.
Standard aggregate load model comprised of static and/or dynamic components.  A static load model represents the sensitivity of the real and reactive power consumed by the load to the amplitude and frequency of the bus voltage. A dynamic load model can be used to represent the aggregate response of the motor components of the load.



\t"""@en .

cim:LoadComposite a owl:Class ;
  rdfs:label "LoadComposite"@en ;
  dy:Package "Package_LoadDynamics" ;
  rdfs:subClassOf cim:LoadDynamics ;
  skos:definition """
Combined static load and induction motor load effects.
The dynamics of the motor are simplified by linearizing the induction machine equations.
\t"""@en .

cim:LoadDynamics a owl:Class ;
  rdfs:label "LoadDynamics"@en ;
  dy:Package "Package_LoadDynamics" ;
  dy:isAbstract "True" ;
  rdfs:subClassOf cim:IdentifiedObject ;
  skos:definition """
Load whose behaviour is described by reference to a standard model <font color="#0f0f0f">or by definition of a user-defined model.</font>
A standard feature of dynamic load behaviour modelling is the ability to associate the same behaviour to multiple energy consumers by means of a single load definition.  The load model is always applied to individual bus loads (energy consumers).
\t"""@en .

cim:LoadGenericNonLinear a owl:Class ;
  rdfs:label "LoadGenericNonLinear"@en ;
  dy:Package "Package_LoadDynamics" ;
  rdfs:subClassOf cim:LoadDynamics ;
  skos:definition "Generic non-linear dynamic (GNLD) load. This model can be used in mid-term and long-term voltage stability simulations (i.e., to study voltage collapse), as it can replace a more detailed representation of aggregate load, including induction motors, thermostatically controlled and static loads."@en .

cim:LoadMotor a owl:Class ;
  rdfs:label "LoadMotor"@en ;
  dy:Package "Package_LoadDynamics" ;
  rdfs:subClassOf cim:IdentifiedObject ;
  skos:definition """
Aggregate induction motor load. This model is used to represent a fraction of an ordinary load as "induction motor load".  It allows a load that is treated as an ordinary constant power in power flow analysis to be represented by an induction motor in dynamic simulation. This model is intended for representation of aggregations of many motors dispersed through a load represented at a high voltage bus but where there is no information on the characteristics of individual motors.
Either a "one-cage" or "two-cage" model of the induction machine can be modelled. Magnetic saturation is not modelled.
This model treats a fraction of the constant power part of a load as a motor. During initialisation, the initial power drawn by the motor is set equal to <i>Pfrac</i> times the constant <i>P</i> part of the static load.  The remainder of the load is left as a static load.
The reactive power demand of the motor is calculated during initialisation as a function of voltage at the load bus. This reactive power demand can be less than or greater than the constant <i>Q</i> component of the load.  If the motor's reactive demand is greater than the constant <i>Q</i> component of the load, the model inserts a shunt capacitor at the terminal of the motor to bring its reactive demand down to equal the constant <i>Q</i> reactive load.  
If an induction motor load model and a static load model are both present for a load, the motor <i>Pfrac</i> is assumed to be subtracted from the power flow constant <i>P</i> load before the static load model is applied.  The remainder of the load, if any, is then represented by the static load model.
\t"""@en .

cim:LoadStatic a owl:Class ;
  rdfs:label "LoadStatic"@en ;
  dy:Package "Package_LoadDynamics" ;
  rdfs:subClassOf cim:IdentifiedObject ;
  skos:definition "General static load. This model represents the sensitivity of the real and reactive power consumed by the load to the amplitude and frequency of the bus voltage."@en .

cim:LoadUserDefined a owl:Class ;
  rdfs:label "LoadUserDefined"@en ;
  dy:Package "Package_UserDefinedModels" ;
  rdfs:subClassOf cim:LoadDynamics ;
  skos:definition "Load whose dynamic behaviour is described by a user-defined model."@en .

cim:MechLoad1 a owl:Class ;
  rdfs:label "MechLoad1"@en ;
  dy:Package "Package_MechanicalLoadDynamics" ;
  rdfs:subClassOf cim:MechanicalLoadDynamics ;
  skos:definition "Mechanical load model type 1."@en .

cim:MechanicalLoadDynamics a owl:Class ;
  rdfs:label "MechanicalLoadDynamics"@en ;
  dy:Package "Package_MechanicalLoadDynamics" ;
  dy:isAbstract "True" ;
  rdfs:subClassOf cim:DynamicsFunctionBlock ;
  skos:definition "Mechanical load function block whose behaviour is described by reference to a standard model <font color=\"#0f0f0f\">or by definition of a user-defined model.</font>"@en .

cim:MechanicalLoadUserDefined a owl:Class ;
  rdfs:label "MechanicalLoadUserDefined"@en ;
  dy:Package "Package_UserDefinedModels" ;
  rdfs:subClassOf cim:MechanicalLoadDynamics ;
  skos:definition "Mechanical load function block whose dynamic behaviour is described by <font color=\"#0f0f0f\">a user-defined model.</font>"@en .

cim:OverexcLim2 a owl:Class ;
  rdfs:label "OverexcLim2"@en ;
  dy:Package "Package_OverexcitationLimiterDynamics" ;
  rdfs:subClassOf cim:OverexcitationLimiterDynamics ;
  skos:definition """
Different from LimIEEEOEL, LimOEL2 has a fixed pickup threshold and reduces the excitation set-point by means of a non-windup integral regulator.
<i>Irated</i> is the rated machine excitation current (calculated from nameplate conditions: <i>V</i><i><sub>nom</sub></i>, <i>P</i><i><sub>nom</sub></i>, <i>CosPhi</i><i><sub>nom</sub></i>).
\t"""@en .

cim:OverexcLimIEEE a owl:Class ;
  rdfs:label "OverexcLimIEEE"@en ;
  dy:Package "Package_OverexcitationLimiterDynamics" ;
  rdfs:subClassOf cim:OverexcitationLimiterDynamics ;
  skos:definition """
The over excitation limiter model is intended to represent the significant features of OELs necessary for some large-scale system studies. It is the result of a pragmatic approach to obtain a model that can be widely applied with attainable data from generator owners. An attempt to include all variations in the functionality of OELs and duplicate how they interact with the rest of the excitation systems would likely result in a level of application insufficient for the studies for which they are intended.
Reference: IEEE OEL 421.5-2005, 9. 
\t"""@en .

cim:OverexcLimX1 a owl:Class ;
  rdfs:label "OverexcLimX1"@en ;
  dy:Package "Package_OverexcitationLimiterDynamics" ;
  rdfs:subClassOf cim:OverexcitationLimiterDynamics ;
  skos:definition "Field voltage over excitation limiter."@en .

cim:OverexcLimX2 a owl:Class ;
  rdfs:label "OverexcLimX2"@en ;
  dy:Package "Package_OverexcitationLimiterDynamics" ;
  rdfs:subClassOf cim:OverexcitationLimiterDynamics ;
  skos:definition "Field voltage or current overexcitation limiter designed to protect the generator field of an AC machine with automatic excitation control from overheating due to prolonged overexcitation."@en .

cim:OverexcitationLimiterDynamics a owl:Class ;
  rdfs:label "OverexcitationLimiterDynamics"@en ;
  dy:Package "Package_OverexcitationLimiterDynamics" ;
  dy:isAbstract "True" ;
  rdfs:subClassOf cim:DynamicsFunctionBlock ;
  skos:definition "Overexcitation limiter function block whose behaviour is described by reference to a standard model <font color=\"#0f0f0f\">or by definition of a user-defined model.</font>"@en .

cim:OverexcitationLimiterUserDefined a owl:Class ;
  rdfs:label "OverexcitationLimiterUserDefined"@en ;
  dy:Package "Package_UserDefinedModels" ;
  rdfs:subClassOf cim:OverexcitationLimiterDynamics ;
  skos:definition "Overexcitation limiter system function block whose dynamic behaviour is described by <font color=\"#0f0f0f\">a user-defined model.</font>"@en .

cim:PFVArControllerType1Dynamics a owl:Class ;
  rdfs:label "PFVArControllerType1Dynamics"@en ;
  dy:Package "Package_PFVArControllerType1Dynamics" ;
  dy:isAbstract "True" ;
  rdfs:subClassOf cim:DynamicsFunctionBlock ;
  skos:definition "Power factor or VAr controller type 1 function block whose behaviour is described by reference to a standard model <font color=\"#0f0f0f\">or by definition of a user-defined model.</font>"@en .

cim:PFVArControllerType1UserDefined a owl:Class ;
  rdfs:label "PFVArControllerType1UserDefined"@en ;
  dy:Package "Package_UserDefinedModels" ;
  rdfs:subClassOf cim:PFVArControllerType1Dynamics ;
  skos:definition "Power factor or VAr controller type 1 function block whose dynamic behaviour is described by <font color=\"#0f0f0f\">a user-defined model.</font>"@en .

cim:PFVArControllerType2Dynamics a owl:Class ;
  rdfs:label "PFVArControllerType2Dynamics"@en ;
  dy:Package "Package_PFVArControllerType2Dynamics" ;
  dy:isAbstract "True" ;
  rdfs:subClassOf cim:DynamicsFunctionBlock ;
  skos:definition "Power factor or VAr controller type 2 function block whose behaviour is described by reference to a standard model <font color=\"#0f0f0f\">or by definition of a user-defined model.</font>"@en .

cim:PFVArControllerType2UserDefined a owl:Class ;
  rdfs:label "PFVArControllerType2UserDefined"@en ;
  dy:Package "Package_UserDefinedModels" ;
  rdfs:subClassOf cim:PFVArControllerType2Dynamics ;
  skos:definition "Power factor or VAr controller type 2 function block whose dynamic behaviour is described by <font color=\"#0f0f0f\">a user-defined model.</font>"@en .

cim:PFVArType1IEEEPFController a owl:Class ;
  rdfs:label "PFVArType1IEEEPFController"@en ;
  dy:Package "Package_PFVArControllerType1Dynamics" ;
  rdfs:subClassOf cim:PFVArControllerType1Dynamics ;
  skos:definition """
IEEE PF controller type 1 which operates by moving the voltage reference directly.
Reference: IEEE 421.5-2005, 11.2. 
\t"""@en .

cim:PFVArType1IEEEVArController a owl:Class ;
  rdfs:label "PFVArType1IEEEVArController"@en ;
  dy:Package "Package_PFVArControllerType1Dynamics" ;
  rdfs:subClassOf cim:PFVArControllerType1Dynamics ;
  skos:definition """
IEEE VAR controller type 1 which operates by moving the voltage reference directly.
Reference: IEEE 421.5-2005, 11.3.
\t"""@en .

cim:PFVArType2Common1 a owl:Class ;
  rdfs:label "PFVArType2Common1"@en ;
  dy:Package "Package_PFVArControllerType2Dynamics" ;
  rdfs:subClassOf cim:PFVArControllerType2Dynamics ;
  skos:definition """
Power factor / reactive power regulator. This model represents the power factor or reactive power controller such as the Basler SCP-250. The controller measures power factor or reactive power (PU on generator rated power) and compares it with the operator's set point.
[Footnote: Basler SCP-250 is an example of a suitable product available commercially. This information is given for the convenience of users of this document and does not constitute an endorsement by IEC of this product.]
\t"""@en .

cim:PFVArType2IEEEPFController a owl:Class ;
  rdfs:label "PFVArType2IEEEPFController"@en ;
  dy:Package "Package_PFVArControllerType2Dynamics" ;
  rdfs:subClassOf cim:PFVArControllerType2Dynamics ;
  skos:definition """
IEEE PF controller type 2 which is a summing point type controller making up the outside loop of a two-loop system. This controller is implemented as a slow PI type controller. The voltage regulator forms the inner loop and is implemented as a fast controller.
Reference: IEEE 421.5-2005, 11.4. 
\t"""@en .

cim:PFVArType2IEEEVArController a owl:Class ;
  rdfs:label "PFVArType2IEEEVArController"@en ;
  dy:Package "Package_PFVArControllerType2Dynamics" ;
  rdfs:subClassOf cim:PFVArControllerType2Dynamics ;
  skos:definition """
IEEE VAR controller type 2 which is a summing point type controller. It makes up the outside loop of a two-loop system. This controller is implemented as a slow PI type controller, and the voltage regulator forms the inner loop and is implemented as a fast controller.
Reference: IEEE 421.5-2005, 11.5.
\t"""@en .

cim:PU a owl:Class ;
  rdfs:label "PU"@en ;
  dy:Package "Package_Domain" ;
  dy:isCIMDatatype "True" ;
  skos:definition """
Per Unit - a positive or negative value referred to a defined base. Values typically range from -10 to +10.

\t"""@en .

cim:PowerElectronicsConnection a owl:Class ;
  rdfs:label "PowerElectronicsConnection"@en ;
  dy:Package "Package_Wires" ;
  dy:isAbstract "True" ;
  rdfs:subClassOf cim:RegulatingCondEq ;
  skos:definition "A connection to the AC network for energy production or consumption that uses power electronics rather than rotating machines."@en .

cim:PowerSystemResource a owl:Class ;
  rdfs:label "PowerSystemResource"@en ;
  dy:Package "Package_Core" ;
  dy:isAbstract "True" ;
  rdfs:subClassOf cim:IdentifiedObject ;
  skos:definition "A power system resource (PSR) can be an item of equipment such as a switch, an equipment container containing many individual items of equipment such as a substation, or an organisational entity such as sub-control area. Power system resources can have measurements associated."@en .

cim:PowerSystemStabilizerDynamics a owl:Class ;
  rdfs:label "PowerSystemStabilizerDynamics"@en ;
  dy:Package "Package_PowerSystemStabilizerDynamics" ;
  dy:isAbstract "True" ;
  rdfs:subClassOf cim:DynamicsFunctionBlock ;
  skos:definition "Power system stabilizer function block whose behaviour is described by reference to a standard model <font color=\"#0f0f0f\">or by definition of a user-defined model.</font>"@en .

cim:PowerSystemStabilizerUserDefined a owl:Class ;
  rdfs:label "PowerSystemStabilizerUserDefined"@en ;
  dy:Package "Package_UserDefinedModels" ;
  rdfs:subClassOf cim:PowerSystemStabilizerDynamics ;
  skos:definition "<font color=\"#0f0f0f\">Power system stabilizer</font> function block whose dynamic behaviour is described by <font color=\"#0f0f0f\">a user-defined model.</font>"@en .

cim:ProprietaryParameterDynamics a owl:Class ;
  rdfs:label "ProprietaryParameterDynamics"@en ;
  dy:Package "Package_UserDefinedModels" ;
  skos:definition """
Supports definition of one or more parameters of several different datatypes for use by proprietary user-defined models.  
This class does not inherit from IdentifiedObject since it is not intended that a single instance of it be referenced by more than one proprietary user-defined model instance.
\t"""@en .

cim:Pss1 a owl:Class ;
  rdfs:label "Pss1"@en ;
  dy:Package "Package_PowerSystemStabilizerDynamics" ;
  rdfs:subClassOf cim:PowerSystemStabilizerDynamics ;
  skos:definition "Italian PSS with three inputs (speed, frequency, power)."@en .

cim:Pss1A a owl:Class ;
  rdfs:label "Pss1A"@en ;
  dy:Package "Package_PowerSystemStabilizerDynamics" ;
  rdfs:subClassOf cim:PowerSystemStabilizerDynamics ;
  skos:definition "Single input power system stabilizer. It is a modified version in order to allow representation of various vendors' implementations on PSS type 1A."@en .

cim:Pss2B a owl:Class ;
  rdfs:label "Pss2B"@en ;
  dy:Package "Package_PowerSystemStabilizerDynamics" ;
  rdfs:subClassOf cim:PowerSystemStabilizerDynamics ;
  skos:definition "Modified IEEE PSS2B.  Extra lead/lag (or rate) block added at end (up to 4 lead/lags total)."@en .

cim:Pss2ST a owl:Class ;
  rdfs:label "Pss2ST"@en ;
  dy:Package "Package_PowerSystemStabilizerDynamics" ;
  rdfs:subClassOf cim:PowerSystemStabilizerDynamics ;
  skos:definition "PTI microprocessor-based stabilizer type 1."@en .

cim:Pss5 a owl:Class ;
  rdfs:label "Pss5"@en ;
  dy:Package "Package_PowerSystemStabilizerDynamics" ;
  rdfs:subClassOf cim:PowerSystemStabilizerDynamics ;
  skos:definition "Detailed Italian PSS."@en .

cim:PssELIN2 a owl:Class ;
  rdfs:label "PssELIN2"@en ;
  dy:Package "Package_PowerSystemStabilizerDynamics" ;
  rdfs:subClassOf cim:PowerSystemStabilizerDynamics ;
  skos:definition "Power system stabilizer typically associated with ExcELIN2 (though PssIEEE2B or Pss2B can also be used)."@en .

cim:PssIEEE1A a owl:Class ;
  rdfs:label "PssIEEE1A"@en ;
  dy:Package "Package_PowerSystemStabilizerDynamics" ;
  rdfs:subClassOf cim:PowerSystemStabilizerDynamics ;
  skos:definition """
IEEE 421.5-2005 type PSS1A power system stabilizer model. PSS1A is the generalized form of a PSS with a single input signal. 
Reference: IEEE 1A 421.5-2005, 8.1. 
\t"""@en .

cim:PssIEEE2B a owl:Class ;
  rdfs:label "PssIEEE2B"@en ;
  dy:Package "Package_PowerSystemStabilizerDynamics" ;
  rdfs:subClassOf cim:PowerSystemStabilizerDynamics ;
  skos:definition """
IEEE 421.5-2005 type PSS2B power system stabilizer model. This stabilizer model is designed to represent a variety of dual-input stabilizers, which normally use combinations of power and speed or frequency to derive the stabilizing signal.
Reference: IEEE 2B 421.5-2005, 8.2.
\t"""@en .

cim:PssIEEE3B a owl:Class ;
  rdfs:label "PssIEEE3B"@en ;
  dy:Package "Package_PowerSystemStabilizerDynamics" ;
  rdfs:subClassOf cim:PowerSystemStabilizerDynamics ;
  skos:definition """
IEEE 421.5-2005 type PSS3B power system stabilizer model. The PSS model PSS3B has dual inputs of electrical power and rotor angular frequency deviation. The signals are used to derive an equivalent mechanical power signal.
This model has 2 input signals. They have the following fixed types (expressed in terms of InputSignalKind values): the first one is of rotorAngleFrequencyDeviation type and the second one is of generatorElectricalPower type.
Reference: IEEE 3B 421.5-2005, 8.3. 


\t"""@en .

cim:PssIEEE4B a owl:Class ;
  rdfs:label "PssIEEE4B"@en ;
  dy:Package "Package_PowerSystemStabilizerDynamics" ;
  rdfs:subClassOf cim:PowerSystemStabilizerDynamics ;
  skos:definition """
IEEE 421.5-2005 type PSS4B power system stabilizer. The PSS4B model represents a structure based on multiple working frequency bands. Three separate bands, respectively dedicated to the low-, intermediate- and high-frequency modes of oscillations, are used in this delta omega (speed input) PSS.
There is an error in the in IEEE 421.5-2005 PSS4B model: the <i>Pe</i> input should read –<i>Pe</i>. This implies that the input <i>Pe</i> needs to be multiplied by -1.
Reference: IEEE 4B 421.5-2005, 8.4. 
Parameter details:
This model has 2 input signals. They have the following fixed types (expressed in terms of InputSignalKind values): the first one is of rotorAngleFrequencyDeviation type and the second one is of generatorElectricalPower type.

\t"""@en .

cim:PssPTIST1 a owl:Class ;
  rdfs:label "PssPTIST1"@en ;
  dy:Package "Package_PowerSystemStabilizerDynamics" ;
  rdfs:subClassOf cim:PowerSystemStabilizerDynamics ;
  skos:definition "PTI microprocessor-based stabilizer type 1."@en .

cim:PssPTIST3 a owl:Class ;
  rdfs:label "PssPTIST3"@en ;
  dy:Package "Package_PowerSystemStabilizerDynamics" ;
  rdfs:subClassOf cim:PowerSystemStabilizerDynamics ;
  skos:definition "PTI microprocessor-based stabilizer type 3."@en .

cim:PssRQB a owl:Class ;
  rdfs:label "PssRQB"@en ;
  dy:Package "Package_PowerSystemStabilizerDynamics" ;
  rdfs:subClassOf cim:PowerSystemStabilizerDynamics ;
  skos:definition "Power system stabilizer type RQB. This power system stabilizer is intended to be used together with excitation system type ExcRQB, which is primarily used in nuclear or thermal generating units."@en .

cim:PssSB4 a owl:Class ;
  rdfs:label "PssSB4"@en ;
  dy:Package "Package_PowerSystemStabilizerDynamics" ;
  rdfs:subClassOf cim:PowerSystemStabilizerDynamics ;
  skos:definition "Power sensitive stabilizer model."@en .

cim:PssSH a owl:Class ;
  rdfs:label "PssSH"@en ;
  dy:Package "Package_PowerSystemStabilizerDynamics" ;
  rdfs:subClassOf cim:PowerSystemStabilizerDynamics ;
  skos:definition """
Siemens<sup>TM</sup> “H infinity” power system stabilizer with generator electrical power input.
[Footnote: Siemens "H infinity" power system stabilizers are an example of suitable products available commercially. This information is given for the convenience of users of this document and does not constitute an endorsement by IEC of these products.] 

\t"""@en .

cim:PssSK a owl:Class ;
  rdfs:label "PssSK"@en ;
  dy:Package "Package_PowerSystemStabilizerDynamics" ;
  rdfs:subClassOf cim:PowerSystemStabilizerDynamics ;
  skos:definition "Slovakian PSS with three inputs."@en .

cim:PssSTAB2A a owl:Class ;
  rdfs:label "PssSTAB2A"@en ;
  dy:Package "Package_PowerSystemStabilizerDynamics" ;
  rdfs:subClassOf cim:PowerSystemStabilizerDynamics ;
  skos:definition """
Power system stabilizer part of an ABB excitation system.
[Footnote: ABB excitation systems are an example of suitable products available commercially. This information is given for the convenience of users of this document and does not constitute an endorsement by IEC of these products.]

\t"""@en .

cim:PssWECC a owl:Class ;
  rdfs:label "PssWECC"@en ;
  dy:Package "Package_PowerSystemStabilizerDynamics" ;
  rdfs:subClassOf cim:PowerSystemStabilizerDynamics ;
  skos:definition "Dual input power system stabilizer, based on IEEE type 2, with modified output limiter defined by WECC (Western Electricity Coordinating Council, USA)."@en .

cim:RegulatingCondEq a owl:Class ;
  rdfs:label "RegulatingCondEq"@en ;
  dy:Package "Package_Wires" ;
  dy:isAbstract "True" ;
  rdfs:subClassOf cim:EnergyConnection ;
  skos:definition "A type of conducting equipment that can regulate a quantity (i.e. voltage or flow) at a specific point in the network. "@en .

cim:RemoteInputSignal a owl:Class ;
  rdfs:label "RemoteInputSignal"@en ;
  dy:Package "Package_StandardInterconnections" ;
  rdfs:subClassOf cim:IdentifiedObject ;
  skos:definition "Supports connection to a terminal associated with a remote bus from which an input signal of a specific type is coming."@en .

cim:RemoteSignalKind a owl:Class ;
  rdfs:label "RemoteSignalKind"@en ;
  dy:Package "Package_Domain" ;
  owl:oneOf ( cim:RemoteSignalKind.remoteBusVoltageFrequency
    cim:RemoteSignalKind.remoteBusVoltageFrequencyDeviation cim:RemoteSignalKind.remoteBusFrequency
    cim:RemoteSignalKind.remoteBusFrequencyDeviation cim:RemoteSignalKind.remoteBusVoltageAmplitude
    cim:RemoteSignalKind.remoteBusVoltage cim:RemoteSignalKind.remoteBranchCurrentAmplitude
    cim:RemoteSignalKind.remoteBusVoltageAmplitudeDerivative
    cim:RemoteSignalKind.remotePuBusVoltageDerivative ) ;
  rdfs:subClassOf cim:Enumeration ;
  skos:definition "Type of input signal coming from remote bus."@en .

cim:RotatingMachine a owl:Class ;
  rdfs:label "RotatingMachine"@en ;
  dy:Package "Package_Wires" ;
  dy:isAbstract "True" ;
  rdfs:subClassOf cim:RegulatingCondEq ;
  skos:definition "A rotating machine which may be used as a generator or motor."@en .

cim:RotatingMachineDynamics a owl:Class ;
  rdfs:label "RotatingMachineDynamics"@en ;
  dy:Package "Package_StandardModels" ;
  dy:isAbstract "True" ;
  rdfs:subClassOf cim:DynamicsFunctionBlock ;
  skos:definition "Abstract parent class for all synchronous and asynchronous machine standard models."@en .

cim:RotorKind a owl:Class ;
  rdfs:label "RotorKind"@en ;
  dy:Package "Package_Domain" ;
  owl:oneOf ( cim:RotorKind.roundRotor cim:RotorKind.salientPole ) ;
  rdfs:subClassOf cim:Enumeration ;
  skos:definition "Type of rotor on physical machine."@en .

cim:SVCUserDefined a owl:Class ;
  rdfs:label "SVCUserDefined"@en ;
  dy:Package "Package_UserDefinedModels" ;
  rdfs:subClassOf cim:StaticVarCompensatorDynamics ;
  skos:definition "Static var compensator (SVC) function block whose dynamic behaviour is described by <font color=\"#0f0f0f\">a user-defined model.</font>"@en .

cim:Seconds a owl:Class ;
  rdfs:label "Seconds"@en ;
  dy:Package "Package_Domain" ;
  dy:isCIMDatatype "True" ;
  skos:definition """
Time, in seconds.

\t"""@en .

cim:StaticLoadModelKind a owl:Class ;
  rdfs:label "StaticLoadModelKind"@en ;
  dy:Package "Package_Domain" ;
  owl:oneOf ( cim:StaticLoadModelKind.exponential cim:StaticLoadModelKind.zIP1
    cim:StaticLoadModelKind.zIP2 cim:StaticLoadModelKind.constantZ ) ;
  rdfs:subClassOf cim:Enumeration ;
  skos:definition "Type of static load model."@en .

cim:StaticVarCompensator a owl:Class ;
  rdfs:label "StaticVarCompensator"@en ;
  dy:Package "Package_Wires" ;
  dy:isAbstract "True" ;
  rdfs:subClassOf cim:RegulatingCondEq ;
  skos:definition """
A facility for providing variable and controllable shunt reactive power. The SVC typically consists of a stepdown transformer, filter, thyristor-controlled reactor, and thyristor-switched capacitor arms.

The SVC may operate in fixed MVar output mode or in voltage control mode. When in voltage control mode, the output of the SVC will be proportional to the deviation of voltage at the controlled bus from the voltage setpoint.  The SVC characteristic slope defines the proportion.  If the voltage at the controlled bus is equal to the voltage setpoint, the SVC MVar output is zero.
\t"""@en .

cim:StaticVarCompensatorDynamics a owl:Class ;
  rdfs:label "StaticVarCompensatorDynamics"@en ;
  dy:Package "Package_StaticVarCompensatorDynamics" ;
  dy:isAbstract "True" ;
  rdfs:subClassOf cim:DynamicsFunctionBlock ;
  skos:definition "Static var compensator whose behaviour is described by reference to a standard model <font color=\"#0f0f0f\">or by definition of a user-defined model.</font>"@en .

cim:String a owl:Class ;
  rdfs:label "String"@en ;
  dy:Package "Package_Domain" ;
  dy:isPrimitive "True" ;
  skos:definition "A string consisting of a sequence of characters. The character encoding is UTF-8. The string length is unspecified and unlimited."@en .

cim:SynchronousMachine a owl:Class ;
  rdfs:label "SynchronousMachine"@en ;
  dy:Package "Package_Wires" ;
  dy:isAbstract "True" ;
  rdfs:subClassOf cim:RotatingMachine ;
  skos:definition "An electromechanical device that operates with shaft rotating synchronously with the network. It is a single machine operating either as a generator or synchronous condenser or pump."@en .

cim:SynchronousMachineDetailed a owl:Class ;
  rdfs:label "SynchronousMachineDetailed"@en ;
  dy:Package "Package_SynchronousMachineDynamics" ;
  dy:isAbstract "True" ;
  rdfs:subClassOf cim:SynchronousMachineDynamics ;
  skos:definition """
All synchronous machine detailed types use a subset of the same data parameters and input/output variables.  
The several variations differ in the following ways:
- the number of  equivalent windings that are included;
- the way in which saturation is incorporated into the model;
- whether or not “subtransient saliency” (<i>X''q</i> not = <i>X''d</i>) is represented.
It is not necessary for each simulation tool to have separate models for each of the model types.  The same model can often be used for several types by alternative logic within the model.  Also, differences in saturation representation might not result in significant model performance differences so model substitutions are often acceptable. 
\t"""@en .

cim:SynchronousMachineDynamics a owl:Class ;
  rdfs:label "SynchronousMachineDynamics"@en ;
  dy:Package "Package_SynchronousMachineDynamics" ;
  dy:isAbstract "True" ;
  rdfs:subClassOf cim:RotatingMachineDynamics ;
  skos:definition """
Synchronous machine whose behaviour is described by reference to a standard model expressed in one of the following forms:
- simplified (or classical), where a group of generators or motors is not modelled in detail;
- detailed, in equivalent circuit form;
- detailed, in time constant reactance form; or
<font color="#0f0f0f">- by definition of a user-defined model.</font>
<font color="#0f0f0f">It is a common practice to represent small generators by a negative load rather than by a dynamic generator model when performing dynamics simulations. In this case, a SynchronousMachine in the static model is not represented by anything in the dynamics model, instead it is treated as an ordinary load.</font>
<font color="#0f0f0f">Parameter details:</font>
<ol>
<li><font color="#0f0f0f">Synchronous machine parameters such as <i>Xl, Xd, Xp</i> etc. are actually used as inductances in the models,</font> but are commonly referred to as reactances since, at nominal frequency, the PU values are the same. However, some references use the symbol <i>L</i> instead of <i>X</i>.</li>
</ol>
\t"""@en .

cim:SynchronousMachineEquivalentCircuit a owl:Class ;
  rdfs:label "SynchronousMachineEquivalentCircuit"@en ;
  dy:Package "Package_SynchronousMachineDynamics" ;
  rdfs:subClassOf cim:SynchronousMachineDetailed ;
  skos:definition """
The electrical equations for all variations of the synchronous models are based on the SynchronousEquivalentCircuit diagram for the direct- and quadrature- axes.
Equations for conversion between equivalent circuit and time constant reactance forms:
<i>Xd</i> = <i>Xad </i>+<i> Xl</i>
<i>X’d</i> = <i>Xl</i> + <i>Xad</i> x <i>Xfd</i> / (<i>Xad</i> + <i>Xfd</i>)
<i>X”d</i> = <i>Xl</i> + <i>Xad</i> x <i>Xfd</i> x <i>X1d</i> / (<i>Xad</i> x <i>Xfd</i> + <i>Xad</i> x <i>X1d</i> + <i>Xfd</i> x <i>X1d</i>)
<i>Xq</i> = <i>Xaq</i> + <i>Xl</i>
<i>X’q</i> = <i>Xl</i> + <i>Xaq</i> x <i>X1q</i> / (<i>Xaq</i> + <i>X1q</i>)
<i>X”q</i> = <i>Xl</i> + <i>Xaq</i> x <i>X1q</i> x <i>X2q</i> / (<i>Xaq</i> x <i>X1q</i> + <i>Xaq</i> x <i>X2q</i> + <i>X1q</i> x <i>X2q</i>)
<i>T’do</i> = (<i>Xad</i> + <i>Xfd</i>) / (<i>omega</i><i><sub>0</sub></i> x <i>Rfd</i>)
<i>T”do</i> = (<i>Xad</i> x <i>Xfd</i> + <i>Xad</i> x <i>X1d</i> + <i>Xfd</i> x <i>X1d</i>) / (<i>omega</i><i><sub>0</sub></i> x <i>R1d</i> x (<i>Xad</i> + <i>Xfd</i>)
<i>T’qo</i> = (<i>Xaq</i> + <i>X1q</i>) / (<i>omega</i><i><sub>0</sub></i> x <i>R1q</i>)
<i>T”qo</i> = (<i>Xaq</i> x <i>X1q</i> + <i>Xaq</i> x <i>X2q</i> + <i>X1q</i> x <i>X2q</i>) / (<i>omega</i><i><sub>0</sub></i> x <i>R2q</i> x (<i>Xaq</i> + <i>X1q</i>)
Same equations using CIM attributes from SynchronousMachineTimeConstantReactance class on left of "=" and SynchronousMachineEquivalentCircuit class on right (except as noted):
xDirectSync = xad + RotatingMachineDynamics.statorLeakageReactance
xDirectTrans = RotatingMachineDynamics.statorLeakageReactance + xad x xfd / (xad + xfd)
xDirectSubtrans = RotatingMachineDynamics.statorLeakageReactance + xad x xfd x x1d / (xad x xfd + xad x x1d + xfd x x1d)
xQuadSync = xaq + RotatingMachineDynamics.statorLeakageReactance
xQuadTrans = RotatingMachineDynamics.statorLeakageReactance + xaq x x1q / (xaq+ x1q)
xQuadSubtrans = RotatingMachineDynamics.statorLeakageReactance + xaq x x1q x x2q / (xaq x x1q + xaq x x2q + x1q x x2q) 
tpdo = (xad + xfd) / (2 x pi x nominal frequency x rfd)
tppdo = (xad x xfd + xad x x1d + xfd x x1d) / (2 x pi x nominal frequency x r1d x (xad + xfd)
tpqo = (xaq + x1q) / (2 x pi x nominal frequency x r1q)
tppqo = (xaq x x1q + xaq x x2q + x1q x x2q) / (2 x pi x nominal frequency x r2q x (xaq + x1q)
These are only valid for a simplified model where "Canay" reactance is zero.
\t"""@en .

cim:SynchronousMachineModelKind a owl:Class ;
  rdfs:label "SynchronousMachineModelKind"@en ;
  dy:Package "Package_Domain" ;
  owl:oneOf ( cim:SynchronousMachineModelKind.subtransient
    cim:SynchronousMachineModelKind.subtransientTypeF
    cim:SynchronousMachineModelKind.subtransientTypeJ
    cim:SynchronousMachineModelKind.subtransientSimplified
    cim:SynchronousMachineModelKind.subtransientSimplifiedDirectAxis ) ;
  rdfs:subClassOf cim:Enumeration ;
  skos:definition "Type of synchronous machine model used in dynamic simulation applications."@en .

cim:SynchronousMachineSimplified a owl:Class ;
  rdfs:label "SynchronousMachineSimplified"@en ;
  dy:Package "Package_SynchronousMachineDynamics" ;
  rdfs:subClassOf cim:SynchronousMachineDynamics ;
  skos:definition """
The simplified model represents a synchronous generator as a constant internal voltage behind an impedance<i> </i>(<i>Rs + jXp</i>) as shown in the Simplified diagram.
Since internal voltage is held constant, there is no <i>Efd</i> input and any excitation system model will be ignored.  There is also no <i>Ifd</i> output.
This model should not be used for representing a real generator except, perhaps, small generators whose response is insignificant.  
The parameters used for the simplified model include:
- RotatingMachineDynamics.damping (<i>D</i>);
- RotatingMachineDynamics.inertia (<i>H</i>);
- RotatingMachineDynamics.statorLeakageReactance (used to exchange <i>jXp </i>for SynchronousMachineSimplified);
- RotatingMachineDynamics.statorResistance (<i>Rs</i>).
\t"""@en .

cim:SynchronousMachineTimeConstantReactance a owl:Class ;
  rdfs:label "SynchronousMachineTimeConstantReactance"@en ;
  dy:Package "Package_SynchronousMachineDynamics" ;
  rdfs:subClassOf cim:SynchronousMachineDetailed ;
  skos:definition """
Synchronous machine detailed modelling types are defined by the combination of the attributes SynchronousMachineTimeConstantReactance.modelType and SynchronousMachineTimeConstantReactance.rotorType.  
Parameter details:
<ol>
<li>The “p” in the time-related attribute names is a substitution for a “prime” in the usual parameter notation, e.g. tpdo refers to <i>T'do</i>.</li>
<li>The parameters used for models expressed in time constant reactance form include:</li>
</ol>
- RotatingMachine.ratedS (<i>MVAbase</i>);
- RotatingMachineDynamics.damping (<i>D</i>);
- RotatingMachineDynamics.inertia (<i>H</i>);
- RotatingMachineDynamics.saturationFactor (<i>S1</i>);
- RotatingMachineDynamics.saturationFactor120 (<i>S12</i>);
- RotatingMachineDynamics.statorLeakageReactance (<i>Xl</i>);
- RotatingMachineDynamics.statorResistance (<i>Rs</i>);
- SynchronousMachineTimeConstantReactance.ks (<i>Ks</i>);
- SynchronousMachineDetailed.saturationFactorQAxis (<i>S1q</i>);
- SynchronousMachineDetailed.saturationFactor120QAxis (<i>S12q</i>);
- SynchronousMachineDetailed.efdBaseRatio;
- SynchronousMachineDetailed.ifdBaseType;
- .xDirectSync (<i>Xd</i>);
- .xDirectTrans (<i>X'd</i>);
- .xDirectSubtrans (<i>X''d</i>);
- .xQuadSync (<i>Xq</i>);
- .xQuadTrans (<i>X'q</i>);
- .xQuadSubtrans (<i>X''q</i>);
- .tpdo (<i>T'do</i>);
- .tppdo (<i>T''do</i>);
- .tpqo (<i>T'qo</i>);
- .tppqo (<i>T''qo</i>);
- .tc.
\t"""@en .

cim:SynchronousMachineUserDefined a owl:Class ;
  rdfs:label "SynchronousMachineUserDefined"@en ;
  dy:Package "Package_UserDefinedModels" ;
  rdfs:subClassOf cim:SynchronousMachineDynamics ;
  skos:definition "Synchronous machine whose dynamic behaviour is described by a user-defined model."@en .

cim:Temperature a owl:Class ;
  rdfs:label "Temperature"@en ;
  dy:Package "Package_Domain" ;
  dy:isCIMDatatype "True" ;
  skos:definition """
Value of temperature in degrees Celsius.

\t"""@en .

cim:Terminal a owl:Class ;
  rdfs:label "Terminal"@en ;
  dy:Package "Package_Core" ;
  dy:isAbstract "True" ;
  rdfs:subClassOf cim:ACDCTerminal ;
  skos:definition "An AC electrical connection point to a piece of conducting equipment. Terminals are connected at physical connection points called connectivity nodes."@en .

cim:TurbLCFB1 a owl:Class ;
  rdfs:label "TurbLCFB1"@en ;
  dy:Package "Package_TurbineLoadControllerDynamics" ;
  rdfs:subClassOf cim:TurbineLoadControllerDynamics ;
  skos:definition "Turbine load controller model developed by WECC.  This model represents a supervisory turbine load controller that acts to maintain turbine power at a set value by continuous adjustment of the turbine governor speed-load reference. This model is intended to represent slow reset 'outer loop' controllers managing the action of the turbine governor."@en .

cim:TurbineGovernorDynamics a owl:Class ;
  rdfs:label "TurbineGovernorDynamics"@en ;
  dy:Package "Package_TurbineGovernorDynamics" ;
  dy:isAbstract "True" ;
  rdfs:subClassOf cim:DynamicsFunctionBlock ;
  skos:definition "Turbine-governor function block whose behaviour is described by reference to a standard model <font color=\"#0f0f0f\">or by definition of a user-defined model.</font>"@en .

cim:TurbineGovernorUserDefined a owl:Class ;
  rdfs:label "TurbineGovernorUserDefined"@en ;
  dy:Package "Package_UserDefinedModels" ;
  rdfs:subClassOf cim:TurbineGovernorDynamics ;
  skos:definition "Turbine-governor function block whose dynamic behaviour is described by <font color=\"#0f0f0f\">a user-defined model.</font>"@en .

cim:TurbineLoadControllerDynamics a owl:Class ;
  rdfs:label "TurbineLoadControllerDynamics"@en ;
  dy:Package "Package_TurbineLoadControllerDynamics" ;
  dy:isAbstract "True" ;
  rdfs:subClassOf cim:DynamicsFunctionBlock ;
  skos:definition "Turbine load controller function block whose behaviour is described by reference to a standard model <font color=\"#0f0f0f\">or by definition of a user-defined model.</font>"@en .

cim:TurbineLoadControllerUserDefined a owl:Class ;
  rdfs:label "TurbineLoadControllerUserDefined"@en ;
  dy:Package "Package_UserDefinedModels" ;
  rdfs:subClassOf cim:TurbineLoadControllerDynamics ;
  skos:definition "Turbine load controller function block whose dynamic behaviour is described by <font color=\"#0f0f0f\">a user-defined model.</font>"@en .

cim:UnderexcLim2Simplified a owl:Class ;
  rdfs:label "UnderexcLim2Simplified"@en ;
  dy:Package "Package_UnderexcitationLimiterDynamics" ;
  rdfs:subClassOf cim:UnderexcitationLimiterDynamics ;
  skos:definition "Simplified type UEL2 underexcitation limiter.  This model can be derived from UnderexcLimIEEE2.  The limit characteristic (look –up table) is a single straight-line, the same as UnderexcLimIEEE2 (see Figure 10.4 (p 32), IEEE 421.5-2005 Section 10.2)."@en .

cim:UnderexcLimIEEE1 a owl:Class ;
  rdfs:label "UnderexcLimIEEE1"@en ;
  dy:Package "Package_UnderexcitationLimiterDynamics" ;
  rdfs:subClassOf cim:UnderexcitationLimiterDynamics ;
  skos:definition """
Type UEL1 model which has a circular limit boundary when plotted in terms of machine reactive power vs. real power output.
Reference: IEEE UEL1 421.5-2005, 10.1. 
\t"""@en .

cim:UnderexcLimIEEE2 a owl:Class ;
  rdfs:label "UnderexcLimIEEE2"@en ;
  dy:Package "Package_UnderexcitationLimiterDynamics" ;
  rdfs:subClassOf cim:UnderexcitationLimiterDynamics ;
  skos:definition """
Type UEL2 underexcitation limiter which has either a straight-line or multi-segment characteristic when plotted in terms of machine reactive power output vs. real power output.
Reference: IEEE UEL2 421.5-2005, 10.2  (limit characteristic lookup table shown in Figure 10.4 (p 32)).
\t"""@en .

cim:UnderexcLimX1 a owl:Class ;
  rdfs:label "UnderexcLimX1"@en ;
  dy:Package "Package_UnderexcitationLimiterDynamics" ;
  rdfs:subClassOf cim:UnderexcitationLimiterDynamics ;
  skos:definition "<font color=\"#0f0f0f\">Allis-Chalmers minimum excitation limiter.</font>"@en .

cim:UnderexcLimX2 a owl:Class ;
  rdfs:label "UnderexcLimX2"@en ;
  dy:Package "Package_UnderexcitationLimiterDynamics" ;
  rdfs:subClassOf cim:UnderexcitationLimiterDynamics ;
  skos:definition "<font color=\"#0f0f0f\">Westinghouse minimum excitation limiter.</font>"@en .

cim:UnderexcitationLimiterDynamics a owl:Class ;
  rdfs:label "UnderexcitationLimiterDynamics"@en ;
  dy:Package "Package_UnderexcitationLimiterDynamics" ;
  dy:isAbstract "True" ;
  rdfs:subClassOf cim:DynamicsFunctionBlock ;
  skos:definition "Underexcitation limiter function block whose behaviour is described by reference to a standard model <font color=\"#0f0f0f\">or by definition of a user-defined model.</font>"@en .

cim:UnderexcitationLimiterUserDefined a owl:Class ;
  rdfs:label "UnderexcitationLimiterUserDefined"@en ;
  dy:Package "Package_UserDefinedModels" ;
  rdfs:subClassOf cim:UnderexcitationLimiterDynamics ;
  skos:definition "Underexcitation limiter function block whose dynamic behaviour is described by <font color=\"#0f0f0f\">a user-defined model.</font>"@en .

cim:UnitMultiplier a owl:Class ;
  rdfs:label "UnitMultiplier"@en ;
  dy:Package "Package_Domain" ;
  owl:oneOf ( cim:UnitMultiplier.y cim:UnitMultiplier.z cim:UnitMultiplier.a cim:UnitMultiplier.f
    cim:UnitMultiplier.p cim:UnitMultiplier.n cim:UnitMultiplier.micro cim:UnitMultiplier.m
    cim:UnitMultiplier.c cim:UnitMultiplier.d cim:UnitMultiplier.none cim:UnitMultiplier.da
    cim:UnitMultiplier.h cim:UnitMultiplier.k cim:UnitMultiplier.M cim:UnitMultiplier.G
    cim:UnitMultiplier.T cim:UnitMultiplier.P cim:UnitMultiplier.E cim:UnitMultiplier.Z
    cim:UnitMultiplier.Y ) ;
  rdfs:subClassOf cim:Enumeration ;
  skos:definition """
The unit multipliers defined for the CIM.  When applied to unit symbols, the unit symbol is treated as a derived unit. Regardless of the contents of the unit symbol text, the unit symbol shall be treated as if it were a single-character unit symbol. Unit symbols should not contain multipliers, and it should be left to the multiplier to define the multiple for an entire data type. 

For example, if a unit symbol is "m2Pers" and the multiplier is "k", then the value is k(m**2/s), and the multiplier applies to the entire final value, not to any individual part of the value. This can be conceptualized by substituting a derived unit symbol for the unit type. If one imagines that the symbol "Þ" represents the derived unit "m2Pers", then applying the multiplier "k" can be conceptualized simply as "kÞ".

For example, the SI unit for mass is "kg" and not "g".  If the unit symbol is defined as "kg", then the multiplier is applied to "kg" as a whole and does not replace the "k" in front of the "g". In this case, the multiplier of "m" would be used with the unit symbol of "kg" to represent one gram.  As a text string, this violates the instructions in IEC 80000-1. However, because the unit symbol in CIM is treated as a derived unit instead of as an SI unit, it makes more sense to conceptualize the "kg" as if it were replaced by one of the proposed replacements for the SI mass symbol. If one imagines that the "kg" were replaced by a symbol "Þ", then it is easier to conceptualize the multiplier "m" as creating the proper unit "mÞ", and not the forbidden unit "mkg".
\t"""@en .

cim:UnitSymbol a owl:Class ;
  rdfs:label "UnitSymbol"@en ;
  dy:Package "Package_Domain" ;
  owl:oneOf ( cim:UnitSymbol.none cim:UnitSymbol.m cim:UnitSymbol.kg cim:UnitSymbol.s
    cim:UnitSymbol.A cim:UnitSymbol.K cim:UnitSymbol.mol cim:UnitSymbol.cd cim:UnitSymbol.deg
    cim:UnitSymbol.rad cim:UnitSymbol.sr cim:UnitSymbol.Gy cim:UnitSymbol.Bq cim:UnitSymbol.degC
    cim:UnitSymbol.Sv cim:UnitSymbol.F cim:UnitSymbol.C cim:UnitSymbol.S cim:UnitSymbol.H
    cim:UnitSymbol.V cim:UnitSymbol.ohm cim:UnitSymbol.J cim:UnitSymbol.N cim:UnitSymbol.Hz
    cim:UnitSymbol.lx cim:UnitSymbol.lm cim:UnitSymbol.Wb cim:UnitSymbol.T cim:UnitSymbol.W
    cim:UnitSymbol.Pa cim:UnitSymbol.m2 cim:UnitSymbol.m3 cim:UnitSymbol.mPers cim:UnitSymbol.mPers2
    cim:UnitSymbol.m3Pers cim:UnitSymbol.mPerm3 cim:UnitSymbol.kgm cim:UnitSymbol.kgPerm3
    cim:UnitSymbol.m2Pers cim:UnitSymbol.WPermK cim:UnitSymbol.JPerK cim:UnitSymbol.ppm
    cim:UnitSymbol.rotPers cim:UnitSymbol.radPers cim:UnitSymbol.WPerm2 cim:UnitSymbol.JPerm2
    cim:UnitSymbol.SPerm cim:UnitSymbol.KPers cim:UnitSymbol.PaPers cim:UnitSymbol.JPerkgK
    cim:UnitSymbol.VA cim:UnitSymbol.VAr cim:UnitSymbol.cosPhi cim:UnitSymbol.Vs cim:UnitSymbol.V2
    cim:UnitSymbol.As cim:UnitSymbol.A2 cim:UnitSymbol.A2s cim:UnitSymbol.VAh cim:UnitSymbol.Wh
    cim:UnitSymbol.VArh cim:UnitSymbol.VPerHz cim:UnitSymbol.HzPers cim:UnitSymbol.character
    cim:UnitSymbol.charPers cim:UnitSymbol.kgm2 cim:UnitSymbol.dB cim:UnitSymbol.WPers
    cim:UnitSymbol.lPers cim:UnitSymbol.dBm cim:UnitSymbol.h cim:UnitSymbol.min cim:UnitSymbol.Q
    cim:UnitSymbol.Qh cim:UnitSymbol.ohmm cim:UnitSymbol.APerm cim:UnitSymbol.V2h cim:UnitSymbol.A2h
    cim:UnitSymbol.Ah cim:UnitSymbol.count cim:UnitSymbol.ft3 cim:UnitSymbol.m3Perh
    cim:UnitSymbol.gal cim:UnitSymbol.Btu cim:UnitSymbol.l cim:UnitSymbol.lPerh cim:UnitSymbol.lPerl
    cim:UnitSymbol.gPerg cim:UnitSymbol.molPerm3 cim:UnitSymbol.molPermol cim:UnitSymbol.molPerkg
    cim:UnitSymbol.sPers cim:UnitSymbol.HzPerHz cim:UnitSymbol.VPerV cim:UnitSymbol.APerA
    cim:UnitSymbol.VPerVA cim:UnitSymbol.rev cim:UnitSymbol.kat cim:UnitSymbol.JPerkg
    cim:UnitSymbol.m3Uncompensated cim:UnitSymbol.m3Compensated cim:UnitSymbol.WPerW
    cim:UnitSymbol.therm cim:UnitSymbol.onePerm cim:UnitSymbol.m3Perkg cim:UnitSymbol.Pas
    cim:UnitSymbol.Nm cim:UnitSymbol.NPerm cim:UnitSymbol.radPers2 cim:UnitSymbol.JPerm3
    cim:UnitSymbol.VPerm cim:UnitSymbol.CPerm3 cim:UnitSymbol.CPerm2 cim:UnitSymbol.FPerm
    cim:UnitSymbol.HPerm cim:UnitSymbol.JPermol cim:UnitSymbol.JPermolK cim:UnitSymbol.CPerkg
    cim:UnitSymbol.GyPers cim:UnitSymbol.WPersr cim:UnitSymbol.WPerm2sr cim:UnitSymbol.katPerm3
    cim:UnitSymbol.d cim:UnitSymbol.anglemin cim:UnitSymbol.anglesec cim:UnitSymbol.ha
    cim:UnitSymbol.tonne cim:UnitSymbol.bar cim:UnitSymbol.mmHg cim:UnitSymbol.M cim:UnitSymbol.kn
    cim:UnitSymbol.Mx cim:UnitSymbol.G cim:UnitSymbol.Oe cim:UnitSymbol.Vh cim:UnitSymbol.WPerA
    cim:UnitSymbol.onePerHz cim:UnitSymbol.VPerVAr cim:UnitSymbol.ohmPerm cim:UnitSymbol.kgPerJ
    cim:UnitSymbol.JPers ) ;
  rdfs:subClassOf cim:Enumeration ;
  skos:definition """
The derived units defined for usage in the CIM. In some cases, the derived unit is equal to an SI unit. Whenever possible, the standard derived symbol is used instead of the formula for the derived unit. For example, the unit symbol Farad is defined as "F" instead of "CPerV". In cases where a standard symbol does not exist for a derived unit, the formula for the unit is used as the unit symbol. For example, density does not have a standard symbol and so it is represented as "kgPerm3". With the exception of the "kg", which is an SI unit, the unit symbols do not contain multipliers and therefore represent the base derived unit to which a multiplier can be applied as a whole. 
Every unit symbol is treated as an unparseable text as if it were a single-letter symbol. The meaning of each unit symbol is defined by the accompanying descriptive text and not by the text contents of the unit symbol.
To allow the widest possible range of serializations without requiring special character handling, several substitutions are made which deviate from the format described in IEC 80000-1. The division symbol "/" is replaced by the letters "Per". Exponents are written in plain text after the unit as "m3" instead of being formatted as "m" with a superscript of 3  or introducing a symbol as in "m^3". The degree symbol "°" is replaced with the letters "deg". Any clarification of the meaning for a substitution is included in the description for the unit symbol.
Non-SI units are included in list of unit symbols to allow sources of data to be correctly labelled with their non-SI units (for example, a GPS sensor that is reporting numbers that represent feet instead of meters). This allows software to use the unit symbol information correctly convert and scale the raw data of those sources into SI-based units. 
The integer values are used for harmonization with IEC 61850.
\t"""@en .

cim:VAdjIEEE a owl:Class ;
  rdfs:label "VAdjIEEE"@en ;
  dy:Package "Package_VoltageAdjusterDynamics" ;
  rdfs:subClassOf cim:VoltageAdjusterDynamics ;
  skos:definition """
IEEE voltage adjuster which is used to represent the voltage adjuster in either a power factor or VAr control system.
Reference: IEEE 421.5-2005, 11.1.
\t"""@en .

cim:VCompIEEEType1 a owl:Class ;
  rdfs:label "VCompIEEEType1"@en ;
  dy:Package "Package_VoltageCompensatorDynamics" ;
  rdfs:subClassOf cim:VoltageCompensatorDynamics ;
  skos:definition """
<font color="#0f0f0f">Terminal voltage transducer and load compensator as defined in IEEE 421.5-2005, 4. This model is common to all excitation system models described in the IEEE Standard. </font>
<font color="#0f0f0f">Parameter details:</font>
<ol>
<li><font color="#0f0f0f">If <i>Rc</i> and <i>Xc</i> are set to zero, the l</font>oad compensation is not employed and the behaviour is as a simple sensing circuit.</li>
</ol>
<ol>
<li>If all parameters (<i>Rc</i>, <i>Xc</i> and <i>Tr</i>) are set to zero, the standard model VCompIEEEType1 is bypassed.</li>
</ol>
Reference: IEEE 421.5-2005 4. 
\t"""@en .

cim:VCompIEEEType2 a owl:Class ;
  rdfs:label "VCompIEEEType2"@en ;
  dy:Package "Package_VoltageCompensatorDynamics" ;
  rdfs:subClassOf cim:VoltageCompensatorDynamics ;
  skos:definition """
<font color="#0f0f0f">Terminal voltage transducer and load compensator as defined in IEEE 421.5-2005, 4. This model is designed to cover the following types of compensation: </font>
<ul>
<li><font color="#0f0f0f">reactive droop;</font></li>
<li><font color="#0f0f0f">transformer-drop or line-drop compensation;</font></li>
<li><font color="#0f0f0f">reactive differential compensation known also as cross-current compensation.</font></li>
</ul>
<font color="#0f0f0f">Reference: IEEE 421.5-2005, 4.</font>
\t"""@en .

cim:VSCDynamics a owl:Class ;
  rdfs:label "VSCDynamics"@en ;
  dy:Package "Package_HVDCDynamics" ;
  dy:isAbstract "True" ;
  rdfs:subClassOf cim:HVDCDynamics ;
  skos:definition "VSC function block whose behaviour is described by reference to a standard model <font color=\"#0f0f0f\">or by definition of a user-defined model.</font>"@en .

cim:VSCUserDefined a owl:Class ;
  rdfs:label "VSCUserDefined"@en ;
  dy:Package "Package_UserDefinedModels" ;
  rdfs:subClassOf cim:VSCDynamics ;
  skos:definition "Voltage source converter (VSC) function block whose dynamic behaviour is described by <font color=\"#0f0f0f\">a user-defined model.</font>"@en .

cim:VoltageAdjusterDynamics a owl:Class ;
  rdfs:label "VoltageAdjusterDynamics"@en ;
  dy:Package "Package_VoltageAdjusterDynamics" ;
  dy:isAbstract "True" ;
  rdfs:subClassOf cim:DynamicsFunctionBlock ;
  skos:definition "Voltage adjuster function block whose behaviour is described by reference to a standard model <font color=\"#0f0f0f\">or by definition of a user-defined model.</font>"@en .

cim:VoltageAdjusterUserDefined a owl:Class ;
  rdfs:label "VoltageAdjusterUserDefined"@en ;
  dy:Package "Package_UserDefinedModels" ;
  rdfs:subClassOf cim:VoltageAdjusterDynamics ;
  skos:definition "<font color=\"#0f0f0f\">Voltage adjuster</font> function block whose dynamic behaviour is described by <font color=\"#0f0f0f\">a user-defined model.</font>"@en .

cim:VoltageCompensatorDynamics a owl:Class ;
  rdfs:label "VoltageCompensatorDynamics"@en ;
  dy:Package "Package_VoltageCompensatorDynamics" ;
  dy:isAbstract "True" ;
  rdfs:subClassOf cim:DynamicsFunctionBlock ;
  skos:definition "Voltage compensator function block whose behaviour is described by reference to a standard model <font color=\"#0f0f0f\">or by definition of a user-defined model.</font>"@en .

cim:VoltageCompensatorUserDefined a owl:Class ;
  rdfs:label "VoltageCompensatorUserDefined"@en ;
  dy:Package "Package_UserDefinedModels" ;
  rdfs:subClassOf cim:VoltageCompensatorDynamics ;
  skos:definition "Voltage compensator function block whose dynamic behaviour is described by <font color=\"#0f0f0f\">a user-defined model.</font>"@en .

cim:VolumeFlowRate a owl:Class ;
  rdfs:label "VolumeFlowRate"@en ;
  dy:Package "Package_Domain" ;
  dy:isCIMDatatype "True" ;
  skos:definition """
Volume per time.

\t"""@en .

cim:VsConverter a owl:Class ;
  rdfs:label "VsConverter"@en ;
  dy:Package "Package_DC" ;
  dy:isAbstract "True" ;
  rdfs:subClassOf cim:ACDCConverter ;
  skos:definition "DC side of the voltage source converter (VSC)."@en .

cim:WindAeroConstIEC a owl:Class ;
  rdfs:label "WindAeroConstIEC"@en ;
  dy:Package "Package_WindDynamics" ;
  rdfs:subClassOf cim:IdentifiedObject ;
  skos:definition """
Constant aerodynamic torque model which assumes that the aerodynamic torque is constant.
Reference: IEC 61400-27-1:2015, 5.6.1.1.
\t"""@en .

cim:WindAeroOneDimIEC a owl:Class ;
  rdfs:label "WindAeroOneDimIEC"@en ;
  dy:Package "Package_WindDynamics" ;
  rdfs:subClassOf cim:IdentifiedObject ;
  skos:definition """
One-dimensional aerodynamic model.  
Reference: IEC 61400-27-1:2015, 5.6.1.2.
\t"""@en .

cim:WindAeroTwoDimIEC a owl:Class ;
  rdfs:label "WindAeroTwoDimIEC"@en ;
  dy:Package "Package_WindDynamics" ;
  rdfs:subClassOf cim:IdentifiedObject ;
  skos:definition """
Two-dimensional aerodynamic model.  
Reference: IEC 61400-27-1:2015, 5.6.1.3.
\t"""@en .

cim:WindContCurrLimIEC a owl:Class ;
  rdfs:label "WindContCurrLimIEC"@en ;
  dy:Package "Package_WindDynamics" ;
  rdfs:subClassOf cim:IdentifiedObject ;
  skos:definition """
Current limitation model.  The current limitation model combines the physical limits and the control limits.
Reference: IEC 61400-27-1:2015, 5.6.5.8.
\t"""@en .

cim:WindContPType3IEC a owl:Class ;
  rdfs:label "WindContPType3IEC"@en ;
  dy:Package "Package_WindDynamics" ;
  rdfs:subClassOf cim:IdentifiedObject ;
  skos:definition """
P control model type 3.
Reference: IEC 61400-27-1:2015, 5.6.5.4.
\t"""@en .

cim:WindContPType4aIEC a owl:Class ;
  rdfs:label "WindContPType4aIEC"@en ;
  dy:Package "Package_WindDynamics" ;
  rdfs:subClassOf cim:IdentifiedObject ;
  skos:definition """
P control model type 4A.
Reference: IEC 61400-27-1:2015, 5.6.5.5.
\t"""@en .

cim:WindContPType4bIEC a owl:Class ;
  rdfs:label "WindContPType4bIEC"@en ;
  dy:Package "Package_WindDynamics" ;
  rdfs:subClassOf cim:IdentifiedObject ;
  skos:definition """
P control model type 4B.
Reference: IEC 61400-27-1:2015, 5.6.5.6.
\t"""@en .

cim:WindContPitchAngleIEC a owl:Class ;
  rdfs:label "WindContPitchAngleIEC"@en ;
  dy:Package "Package_WindDynamics" ;
  rdfs:subClassOf cim:IdentifiedObject ;
  skos:definition """
Pitch angle control model.
Reference: IEC 61400-27-1:2015, 5.6.5.2.
\t"""@en .

cim:WindContQIEC a owl:Class ;
  rdfs:label "WindContQIEC"@en ;
  dy:Package "Package_WindDynamics" ;
  rdfs:subClassOf cim:IdentifiedObject ;
  skos:definition """
Q control model.
Reference: IEC 61400-27-1:2015, 5.6.5.7.
\t"""@en .

cim:WindContQLimIEC a owl:Class ;
  rdfs:label "WindContQLimIEC"@en ;
  dy:Package "Package_WindDynamics" ;
  rdfs:subClassOf cim:IdentifiedObject ;
  skos:definition """
Constant Q limitation model.
Reference: IEC 61400-27-1:2015, 5.6.5.9.
\t"""@en .

cim:WindContQPQULimIEC a owl:Class ;
  rdfs:label "WindContQPQULimIEC"@en ;
  dy:Package "Package_WindDynamics" ;
  rdfs:subClassOf cim:IdentifiedObject ;
  skos:definition """
QP and QU limitation model.
Reference: IEC 61400-27-1:2015, 5.6.5.10.
\t"""@en .

cim:WindContRotorRIEC a owl:Class ;
  rdfs:label "WindContRotorRIEC"@en ;
  dy:Package "Package_WindDynamics" ;
  rdfs:subClassOf cim:IdentifiedObject ;
  skos:definition """
Rotor resistance control model.
Reference: IEC 61400-27-1:2015, 5.6.5.3.
\t"""@en .

cim:WindDynamicsLookupTable a owl:Class ;
  rdfs:label "WindDynamicsLookupTable"@en ;
  dy:Package "Package_WindDynamics" ;
  rdfs:subClassOf cim:IdentifiedObject ;
  skos:definition "Look up table for the purpose of wind standard models."@en .

cim:WindGenTurbineType1aIEC a owl:Class ;
  rdfs:label "WindGenTurbineType1aIEC"@en ;
  dy:Package "Package_WindDynamics" ;
  rdfs:subClassOf cim:WindTurbineType1or2IEC ;
  skos:definition """
Wind turbine IEC type 1A.
Reference: IEC 61400-27-1:2015, 5.5.2.2.
\t"""@en .

cim:WindGenTurbineType1bIEC a owl:Class ;
  rdfs:label "WindGenTurbineType1bIEC"@en ;
  dy:Package "Package_WindDynamics" ;
  rdfs:subClassOf cim:WindTurbineType1or2IEC ;
  skos:definition """
Wind turbine IEC type 1B.

Reference: IEC 61400-27-1:2015, 5.5.2.3.
\t"""@en .

cim:WindGenTurbineType2IEC a owl:Class ;
  rdfs:label "WindGenTurbineType2IEC"@en ;
  dy:Package "Package_WindDynamics" ;
  rdfs:subClassOf cim:WindTurbineType1or2IEC ;
  skos:definition """
Wind turbine IEC type 2.

Reference: IEC 61400-27-1:2015, 5.5.3.
\t"""@en .

cim:WindGenType3IEC a owl:Class ;
  rdfs:label "WindGenType3IEC"@en ;
  dy:Package "Package_WindDynamics" ;
  dy:isAbstract "True" ;
  rdfs:subClassOf cim:IdentifiedObject ;
  skos:definition "Parent class supporting relationships to IEC wind turbines type 3 generator models of IEC type 3A and 3B."@en .

cim:WindGenType3aIEC a owl:Class ;
  rdfs:label "WindGenType3aIEC"@en ;
  dy:Package "Package_WindDynamics" ;
  rdfs:subClassOf cim:WindGenType3IEC ;
  skos:definition """
IEC type 3A generator set model.
Reference: IEC 61400-27-1:2015, 5.6.3.2.
\t"""@en .

cim:WindGenType3bIEC a owl:Class ;
  rdfs:label "WindGenType3bIEC"@en ;
  dy:Package "Package_WindDynamics" ;
  rdfs:subClassOf cim:WindGenType3IEC ;
  skos:definition """
IEC type 3B generator set model.
Reference: IEC 61400-27-1:2015, 5.6.3.3.
\t"""@en .

cim:WindGenType4IEC a owl:Class ;
  rdfs:label "WindGenType4IEC"@en ;
  dy:Package "Package_WindDynamics" ;
  rdfs:subClassOf cim:IdentifiedObject ;
  skos:definition """
IEC type 4 generator set model.
Reference: IEC 61400-27-1:2015, 5.6.3.4.
\t"""@en .

cim:WindLookupTableFunctionKind a owl:Class ;
  rdfs:label "WindLookupTableFunctionKind"@en ;
  dy:Package "Package_Domain" ;
  owl:oneOf ( cim:WindLookupTableFunctionKind.prr cim:WindLookupTableFunctionKind.omegap
    cim:WindLookupTableFunctionKind.ipmax cim:WindLookupTableFunctionKind.iqmax
    cim:WindLookupTableFunctionKind.pwp cim:WindLookupTableFunctionKind.tcwdu
    cim:WindLookupTableFunctionKind.tduwt cim:WindLookupTableFunctionKind.qmaxp
    cim:WindLookupTableFunctionKind.qminp cim:WindLookupTableFunctionKind.qmaxu
    cim:WindLookupTableFunctionKind.qminu cim:WindLookupTableFunctionKind.tuover
    cim:WindLookupTableFunctionKind.tuunder cim:WindLookupTableFunctionKind.tfover
    cim:WindLookupTableFunctionKind.tfunder cim:WindLookupTableFunctionKind.qwp ) ;
  rdfs:subClassOf cim:Enumeration ;
  skos:definition "Function of the lookup table."@en .

cim:WindMechIEC a owl:Class ;
  rdfs:label "WindMechIEC"@en ;
  dy:Package "Package_WindDynamics" ;
  rdfs:subClassOf cim:IdentifiedObject ;
  skos:definition """
Two mass model.
Reference: IEC 61400-27-1:2015, 5.6.2.1.
\t"""@en .

cim:WindPitchContPowerIEC a owl:Class ;
  rdfs:label "WindPitchContPowerIEC"@en ;
  dy:Package "Package_WindDynamics" ;
  rdfs:subClassOf cim:IdentifiedObject ;
  skos:definition """
Pitch control power model.
Reference: IEC 61400-27-1:2015, 5.6.5.1.
\t"""@en .

cim:WindPlantDynamics a owl:Class ;
  rdfs:label "WindPlantDynamics"@en ;
  dy:Package "Package_WindDynamics" ;
  dy:isAbstract "True" ;
  rdfs:subClassOf cim:DynamicsFunctionBlock ;
  skos:definition "Parent class supporting relationships to wind turbines type 3 and type 4 and wind plant IEC and user-defined wind plants including their control models."@en .

cim:WindPlantFreqPcontrolIEC a owl:Class ;
  rdfs:label "WindPlantFreqPcontrolIEC"@en ;
  dy:Package "Package_WindDynamics" ;
  rdfs:subClassOf cim:IdentifiedObject ;
  skos:definition """
Frequency and active power controller model.
Reference: IEC 61400-27-1:2015, Annex D.
\t"""@en .

cim:WindPlantIEC a owl:Class ;
  rdfs:label "WindPlantIEC"@en ;
  dy:Package "Package_WindDynamics" ;
  rdfs:subClassOf cim:WindPlantDynamics ;
  skos:definition """
Simplified IEC type plant level model. 
Reference: IEC 61400-27-1:2015, Annex D.
\t"""@en .

cim:WindPlantQcontrolModeKind a owl:Class ;
  rdfs:label "WindPlantQcontrolModeKind"@en ;
  dy:Package "Package_Domain" ;
  owl:oneOf ( cim:WindPlantQcontrolModeKind.reactivePower cim:WindPlantQcontrolModeKind.powerFactor
    cim:WindPlantQcontrolModeKind.uqStatic cim:WindPlantQcontrolModeKind.voltageControl ) ;
  rdfs:subClassOf cim:Enumeration ;
  skos:definition "Reactive power/voltage controller mode."@en .

cim:WindPlantReactiveControlIEC a owl:Class ;
  rdfs:label "WindPlantReactiveControlIEC"@en ;
  dy:Package "Package_WindDynamics" ;
  rdfs:subClassOf cim:IdentifiedObject ;
  skos:definition """
Simplified plant voltage and reactive power control model for use with type 3 and type 4 wind turbine models.
Reference: IEC 61400-27-1:2015, Annex D.
\t"""@en .

cim:WindPlantUserDefined a owl:Class ;
  rdfs:label "WindPlantUserDefined"@en ;
  dy:Package "Package_UserDefinedModels" ;
  rdfs:subClassOf cim:WindPlantDynamics ;
  skos:definition "Wind plant function block whose dynamic behaviour is described by <font color=\"#0f0f0f\">a user-defined model.</font>"@en .

cim:WindProtectionIEC a owl:Class ;
  rdfs:label "WindProtectionIEC"@en ;
  dy:Package "Package_WindDynamics" ;
  rdfs:subClassOf cim:IdentifiedObject ;
  skos:definition """
The grid protection model includes protection against over- and under-voltage, and against over- and under-frequency.
Reference: IEC 61400-27-1:2015, 5.6.6.
\t"""@en .

cim:WindQcontrolModeKind a owl:Class ;
  rdfs:label "WindQcontrolModeKind"@en ;
  dy:Package "Package_Domain" ;
  owl:oneOf ( cim:WindQcontrolModeKind.voltage cim:WindQcontrolModeKind.reactivePower
    cim:WindQcontrolModeKind.openLoopReactivePower cim:WindQcontrolModeKind.powerFactor
    cim:WindQcontrolModeKind.openLooppowerFactor ) ;
  rdfs:subClassOf cim:Enumeration ;
  skos:definition "General wind turbine Q control modes <i>M</i><i><sub>qG</sub></i><i>.</i>"@en .

cim:WindRefFrameRotIEC a owl:Class ;
  rdfs:label "WindRefFrameRotIEC"@en ;
  dy:Package "Package_WindDynamics" ;
  rdfs:subClassOf cim:IdentifiedObject ;
  skos:definition """
Reference frame rotation model.
Reference: IEC 61400-27-1:2015, 5.6.3.5.
\t"""@en .

cim:WindTurbineType1or2Dynamics a owl:Class ;
  rdfs:label "WindTurbineType1or2Dynamics"@en ;
  dy:Package "Package_WindDynamics" ;
  dy:isAbstract "True" ;
  rdfs:subClassOf cim:DynamicsFunctionBlock ;
  skos:definition """
Parent class supporting relationships to wind turbines type 1 and type 2 and their control models.  Generator model for wind turbine of type 1 or type 2 is a standard asynchronous generator model.

\t"""@en .

cim:WindTurbineType1or2IEC a owl:Class ;
  rdfs:label "WindTurbineType1or2IEC"@en ;
  dy:Package "Package_WindDynamics" ;
  dy:isAbstract "True" ;
  rdfs:subClassOf cim:WindTurbineType1or2Dynamics ;
  skos:definition """
Parent class supporting relationships to IEC wind turbines type 1 and type 2 including their control models.
Generator model for wind turbine of IEC type 1 or type 2 is a standard asynchronous generator model.
Reference: IEC 61400-27-1:2015, 5.5.2 and 5.5.3.
\t"""@en .

cim:WindTurbineType3IEC a owl:Class ;
  rdfs:label "WindTurbineType3IEC"@en ;
  dy:Package "Package_WindDynamics" ;
  rdfs:subClassOf cim:WindTurbineType3or4IEC ;
  skos:definition "Parent class supporting relationships to IEC wind turbines type 3 including their control models."@en .

cim:WindTurbineType3or4Dynamics a owl:Class ;
  rdfs:label "WindTurbineType3or4Dynamics"@en ;
  dy:Package "Package_WindDynamics" ;
  dy:isAbstract "True" ;
  rdfs:subClassOf cim:DynamicsFunctionBlock ;
  skos:definition "Parent class supporting relationships to wind turbines type 3 and type 4 and wind plant including their control models."@en .

cim:WindTurbineType3or4IEC a owl:Class ;
  rdfs:label "WindTurbineType3or4IEC"@en ;
  dy:Package "Package_WindDynamics" ;
  dy:isAbstract "True" ;
  rdfs:subClassOf cim:WindTurbineType3or4Dynamics ;
  skos:definition "Parent class supporting relationships to IEC wind turbines type 3 and type 4 including their control models."@en .

cim:WindTurbineType4IEC a owl:Class ;
  rdfs:label "WindTurbineType4IEC"@en ;
  dy:Package "Package_WindDynamics" ;
  dy:isAbstract "True" ;
  rdfs:subClassOf cim:WindTurbineType3or4IEC ;
  skos:definition "Parent class supporting relationships to IEC wind turbines type 4 including their control models."@en .

cim:WindTurbineType4aIEC a owl:Class ;
  rdfs:label "WindTurbineType4aIEC"@en ;
  dy:Package "Package_WindDynamics" ;
  rdfs:subClassOf cim:WindTurbineType4IEC ;
  skos:definition """
Wind turbine IEC type 4A.
Reference: IEC 61400-27-1:2015, 5.5.5.2.
\t"""@en .

cim:WindTurbineType4bIEC a owl:Class ;
  rdfs:label "WindTurbineType4bIEC"@en ;
  dy:Package "Package_WindDynamics" ;
  rdfs:subClassOf cim:WindTurbineType4IEC ;
  skos:definition """
Wind turbine IEC type 4B.
Reference: IEC 61400-27-1:2015, 5.5.5.3.
\t"""@en .

cim:WindType1or2UserDefined a owl:Class ;
  rdfs:label "WindType1or2UserDefined"@en ;
  dy:Package "Package_UserDefinedModels" ;
  rdfs:subClassOf cim:WindTurbineType1or2Dynamics ;
  skos:definition "Wind type 1 or type 2 function block whose dynamic behaviour is described by <font color=\"#0f0f0f\">a user-defined model.</font>"@en .

cim:WindType3or4UserDefined a owl:Class ;
  rdfs:label "WindType3or4UserDefined"@en ;
  dy:Package "Package_UserDefinedModels" ;
  rdfs:subClassOf cim:WindTurbineType3or4Dynamics ;
  skos:definition "Wind type 3 or type 4 function block whose dynamic behaviour is described by <font color=\"#0f0f0f\">a user-defined model.</font>"@en .

cim:WindUVRTQcontrolModeKind a owl:Class ;
  rdfs:label "WindUVRTQcontrolModeKind"@en ;
  dy:Package "Package_Domain" ;
  owl:oneOf ( cim:WindUVRTQcontrolModeKind.mode0 cim:WindUVRTQcontrolModeKind.mode1
    cim:WindUVRTQcontrolModeKind.mode2 ) ;
  rdfs:subClassOf cim:Enumeration ;
  skos:definition "UVRT Q control modes <i>M</i><i><sub>qUVRT</sub></i><i>.</i>"@en .

dy:Enumeration a owl:Class ;
  rdfs:label " enumeration "@en ;
  rdfs:comment " An abstract superclass for all Enumerators. "@en ;
  dy:isAbstract "true" .

cim:AsynchronousMachine.AsynchronousMachineDynamics a owl:ObjectProperty, owl:FunctionalProperty ;
  rdfs:label "AsynchronousMachineDynamics"@en ;
  owl:inverseOf cim:AsynchronousMachineDynamics.AsynchronousMachine ;
  rdfs:domain cim:AsynchronousMachine ;
  rdfs:range cim:AsynchronousMachineDynamics ;
  skos:definition "Asynchronous machine dynamics model used to describe dynamic behaviour of this asynchronous machine."@en .

cim:AsynchronousMachineDynamics.AsynchronousMachine a owl:ObjectProperty ;
  rdfs:label "AsynchronousMachine"@en ;
  owl:inverseOf cim:AsynchronousMachine.AsynchronousMachineDynamics ;
  rdfs:domain cim:AsynchronousMachineDynamics ;
  rdfs:range cim:AsynchronousMachine ;
  skos:definition "Asynchronous machine to which this asynchronous machine dynamics model applies."@en .

cim:AsynchronousMachineDynamics.MechanicalLoadDynamics a owl:ObjectProperty, owl:FunctionalProperty ;
  rdfs:label "MechanicalLoadDynamics"@en ;
  owl:inverseOf cim:MechanicalLoadDynamics.AsynchronousMachineDynamics ;
  rdfs:domain cim:AsynchronousMachineDynamics ;
  rdfs:range cim:MechanicalLoadDynamics ;
  skos:definition "Mechanical load model associated with this asynchronous machine model."@en .

cim:AsynchronousMachineDynamics.TurbineGovernorDynamics a owl:ObjectProperty, owl:FunctionalProperty ;
  rdfs:label "TurbineGovernorDynamics"@en ;
  owl:inverseOf cim:TurbineGovernorDynamics.AsynchronousMachineDynamics ;
  rdfs:domain cim:AsynchronousMachineDynamics ;
  rdfs:range cim:TurbineGovernorDynamics ;
  skos:definition "Turbine-governor model associated with this asynchronous machine model."@en .

cim:AsynchronousMachineDynamics.WindTurbineType1or2Dynamics a owl:ObjectProperty, owl:FunctionalProperty ;
  rdfs:label "WindTurbineType1or2Dynamics"@en ;
  owl:inverseOf cim:WindTurbineType1or2Dynamics.AsynchronousMachineDynamics ;
  rdfs:domain cim:AsynchronousMachineDynamics ;
  rdfs:range cim:WindTurbineType1or2Dynamics ;
  skos:definition "Wind generator type 1 or type 2 model associated with this asynchronous machine model."@en .

cim:AsynchronousMachineUserDefined.ProprietaryParameterDynamics a owl:ObjectProperty ;
  rdfs:label "ProprietaryParameterDynamics"@en ;
  owl:inverseOf cim:ProprietaryParameterDynamics.AsynchronousMachineUserDefined ;
  rdfs:domain cim:AsynchronousMachineUserDefined ;
  rdfs:range cim:ProprietaryParameterDynamics ;
  skos:definition "Parameter of this proprietary user-defined model."@en .

cim:CSCDynamics.CSConverter a owl:ObjectProperty ;
  rdfs:label "CSConverter"@en ;
  owl:inverseOf cim:CsConverter.CSCDynamics ;
  rdfs:domain cim:CSCDynamics ;
  rdfs:range cim:CsConverter ;
  skos:definition "Current source converter to which current source converter dynamics model applies."@en .

cim:CSCUserDefined.ProprietaryParameterDynamics a owl:ObjectProperty ;
  rdfs:label "ProprietaryParameterDynamics"@en ;
  owl:inverseOf cim:ProprietaryParameterDynamics.CSCUserDefined ;
  rdfs:domain cim:CSCUserDefined ;
  rdfs:range cim:ProprietaryParameterDynamics ;
  skos:definition "Parameter of this proprietary user-defined model."@en .

cim:ConductingEquipment.Terminals a owl:ObjectProperty ;
  rdfs:label "Terminals"@en ;
  owl:inverseOf cim:Terminal.ConductingEquipment ;
  rdfs:domain cim:ConductingEquipment ;
  rdfs:range cim:Terminal ;
  skos:definition "Conducting equipment have terminals that may be connected to other conducting equipment terminals via connectivity nodes or topological nodes."@en .

cim:CrossCompoundTurbineGovernorDynamics.HighPressureSynchronousMachineDynamics a owl:ObjectProperty ;
  rdfs:label "HighPressureSynchronousMachineDynamics"@en ;
  owl:inverseOf cim:SynchronousMachineDynamics.CrossCompoundTurbineGovernorDyanmics ;
  rdfs:domain cim:CrossCompoundTurbineGovernorDynamics ;
  rdfs:range cim:SynchronousMachineDynamics ;
  skos:definition "High-pressure synchronous machine with which this cross-compound turbine governor is associated. "@en .

cim:CrossCompoundTurbineGovernorDynamics.LowPressureSynchronousMachineDynamics a owl:ObjectProperty ;
  rdfs:label "LowPressureSynchronousMachineDynamics"@en ;
  owl:inverseOf cim:SynchronousMachineDynamics.CrossCompoundTurbineGovernorDynamics ;
  rdfs:domain cim:CrossCompoundTurbineGovernorDynamics ;
  rdfs:range cim:SynchronousMachineDynamics ;
  skos:definition "Low-pressure synchronous machine with which this cross-compound turbine governor is associated. "@en .

cim:CsConverter.CSCDynamics a owl:ObjectProperty, owl:FunctionalProperty ;
  rdfs:label "CSCDynamics"@en ;
  owl:inverseOf cim:CSCDynamics.CSConverter ;
  rdfs:domain cim:CsConverter ;
  rdfs:range cim:CSCDynamics ;
  skos:definition "Current source converter dynamics model used to describe dynamic behaviour of this converter."@en .

cim:DiscontinuousExcitationControlDynamics.ExcitationSystemDynamics a owl:ObjectProperty ;
  rdfs:label "ExcitationSystemDynamics"@en ;
  owl:inverseOf cim:ExcitationSystemDynamics.DiscontinuousExcitationControlDynamics ;
  rdfs:domain cim:DiscontinuousExcitationControlDynamics ;
  rdfs:range cim:ExcitationSystemDynamics ;
  skos:definition "Excitation system model with which this discontinuous excitation control model is associated."@en .

cim:DiscontinuousExcitationControlDynamics.RemoteInputSignal a owl:ObjectProperty, owl:FunctionalProperty ;
  rdfs:label "RemoteInputSignal"@en ;
  owl:inverseOf cim:RemoteInputSignal.DiscontinuousExcitationControlDynamics ;
  rdfs:domain cim:DiscontinuousExcitationControlDynamics ;
  rdfs:range cim:RemoteInputSignal ;
  skos:definition "Remote input signal used by this discontinuous excitation control system model."@en .

cim:DiscontinuousExcitationControlUserDefined.ProprietaryParameterDynamics a owl:ObjectProperty ;
  rdfs:label "ProprietaryParameterDynamics"@en ;
  owl:inverseOf cim:ProprietaryParameterDynamics.DiscontinuousExcitationControlUserDefined ;
  rdfs:domain cim:DiscontinuousExcitationControlUserDefined ;
  rdfs:range cim:ProprietaryParameterDynamics ;
  skos:definition "Parameter of this proprietary user-defined model."@en .

cim:EnergyConsumer.LoadDynamics a owl:ObjectProperty, owl:FunctionalProperty ;
  rdfs:label "LoadDynamics"@en ;
  owl:inverseOf cim:LoadDynamics.EnergyConsumer ;
  rdfs:domain cim:EnergyConsumer ;
  rdfs:range cim:LoadDynamics ;
  skos:definition "Load dynamics model used to describe dynamic behaviour of this energy consumer."@en .

cim:ExcitationSystemDynamics.DiscontinuousExcitationControlDynamics a owl:ObjectProperty, owl:FunctionalProperty ;
  rdfs:label "DiscontinuousExcitationControlDynamics"@en ;
  owl:inverseOf cim:DiscontinuousExcitationControlDynamics.ExcitationSystemDynamics ;
  rdfs:domain cim:ExcitationSystemDynamics ;
  rdfs:range cim:DiscontinuousExcitationControlDynamics ;
  skos:definition "Discontinuous excitation control model associated with this excitation system model."@en .

cim:ExcitationSystemDynamics.OverexcitationLimiterDynamics a owl:ObjectProperty, owl:FunctionalProperty ;
  rdfs:label "OverexcitationLimiterDynamics"@en ;
  owl:inverseOf cim:OverexcitationLimiterDynamics.ExcitationSystemDynamics ;
  rdfs:domain cim:ExcitationSystemDynamics ;
  rdfs:range cim:OverexcitationLimiterDynamics ;
  skos:definition "Overexcitation limiter model associated with this excitation system model."@en .

cim:ExcitationSystemDynamics.PFVArControllerType1Dynamics a owl:ObjectProperty, owl:FunctionalProperty ;
  rdfs:label "PFVArControllerType1Dynamics"@en ;
  owl:inverseOf cim:PFVArControllerType1Dynamics.ExcitationSystemDynamics ;
  rdfs:domain cim:ExcitationSystemDynamics ;
  rdfs:range cim:PFVArControllerType1Dynamics ;
  skos:definition "Power factor or VAr controller type 1 model associated with this excitation system model."@en .

cim:ExcitationSystemDynamics.PFVArControllerType2Dynamics a owl:ObjectProperty, owl:FunctionalProperty ;
  rdfs:label "PFVArControllerType2Dynamics"@en ;
  owl:inverseOf cim:PFVArControllerType2Dynamics.ExcitationSystemDynamics ;
  rdfs:domain cim:ExcitationSystemDynamics ;
  rdfs:range cim:PFVArControllerType2Dynamics ;
  skos:definition "Power factor or VAr controller type 2 model associated with this excitation system model."@en .

cim:ExcitationSystemDynamics.PowerSystemStabilizerDynamics a owl:ObjectProperty, owl:FunctionalProperty ;
  rdfs:label "PowerSystemStabilizerDynamics"@en ;
  owl:inverseOf cim:PowerSystemStabilizerDynamics.ExcitationSystemDynamics ;
  rdfs:domain cim:ExcitationSystemDynamics ;
  rdfs:range cim:PowerSystemStabilizerDynamics ;
  skos:definition "Power system stabilizer model associated with this excitation system model."@en .

cim:ExcitationSystemDynamics.SynchronousMachineDynamics a owl:ObjectProperty ;
  rdfs:label "SynchronousMachineDynamics"@en ;
  owl:inverseOf cim:SynchronousMachineDynamics.ExcitationSystemDynamics ;
  rdfs:domain cim:ExcitationSystemDynamics ;
  rdfs:range cim:SynchronousMachineDynamics ;
  skos:definition "Synchronous machine model with which this excitation system model is associated."@en .

cim:ExcitationSystemDynamics.UnderexcitationLimiterDynamics a owl:ObjectProperty, owl:FunctionalProperty ;
  rdfs:label "UnderexcitationLimiterDynamics"@en ;
  owl:inverseOf cim:UnderexcitationLimiterDynamics.ExcitationSystemDynamics ;
  rdfs:domain cim:ExcitationSystemDynamics ;
  rdfs:range cim:UnderexcitationLimiterDynamics ;
  skos:definition "Undrexcitation limiter model associated with this excitation system model."@en .

cim:ExcitationSystemDynamics.VoltageCompensatorDynamics a owl:ObjectProperty ;
  rdfs:label "VoltageCompensatorDynamics"@en ;
  owl:inverseOf cim:VoltageCompensatorDynamics.ExcitationSystemDynamics ;
  rdfs:domain cim:ExcitationSystemDynamics ;
  rdfs:range cim:VoltageCompensatorDynamics ;
  skos:definition "Voltage compensator model associated with this excitation system model."@en .

cim:ExcitationSystemUserDefined.ProprietaryParameterDynamics a owl:ObjectProperty ;
  rdfs:label "ProprietaryParameterDynamics"@en ;
  owl:inverseOf cim:ProprietaryParameterDynamics.ExcitationSystemUserDefined ;
  rdfs:domain cim:ExcitationSystemUserDefined ;
  rdfs:range cim:ProprietaryParameterDynamics ;
  skos:definition "Parameter of this proprietary user-defined model."@en .

cim:GenICompensationForGenJ.SynchronousMachineDynamics a owl:ObjectProperty ;
  rdfs:label "SynchronousMachineDynamics"@en ;
  owl:inverseOf cim:SynchronousMachineDynamics.GenICompensationForGenJ ;
  rdfs:domain cim:GenICompensationForGenJ ;
  rdfs:range cim:SynchronousMachineDynamics ;
  skos:definition "Standard synchronous machine out of which current flow is being compensated for."@en .

cim:GenICompensationForGenJ.VcompIEEEType2 a owl:ObjectProperty ;
  rdfs:label "VcompIEEEType2"@en ;
  owl:inverseOf cim:VCompIEEEType2.GenICompensationForGenJ ;
  rdfs:domain cim:GenICompensationForGenJ ;
  rdfs:range cim:VCompIEEEType2 ;
  skos:definition "The standard IEEE type 2 voltage compensator of this compensation."@en .

cim:LoadAggregate.LoadMotor a owl:ObjectProperty, owl:FunctionalProperty ;
  rdfs:label "LoadMotor"@en ;
  owl:inverseOf cim:LoadMotor.LoadAggregate ;
  rdfs:domain cim:LoadAggregate ;
  rdfs:range cim:LoadMotor ;
  skos:definition "Aggregate motor (dynamic) load associated with this aggregate load."@en .

cim:LoadAggregate.LoadStatic a owl:ObjectProperty, owl:FunctionalProperty ;
  rdfs:label "LoadStatic"@en ;
  owl:inverseOf cim:LoadStatic.LoadAggregate ;
  rdfs:domain cim:LoadAggregate ;
  rdfs:range cim:LoadStatic ;
  skos:definition "Aggregate static load associated with this aggregate load."@en .

cim:LoadDynamics.EnergyConsumer a owl:ObjectProperty ;
  rdfs:label "EnergyConsumer"@en ;
  owl:inverseOf cim:EnergyConsumer.LoadDynamics ;
  rdfs:domain cim:LoadDynamics ;
  rdfs:range cim:EnergyConsumer ;
  skos:definition "Energy consumer to which this dynamics load model applies."@en .

cim:LoadMotor.LoadAggregate a owl:ObjectProperty ;
  rdfs:label "LoadAggregate"@en ;
  owl:inverseOf cim:LoadAggregate.LoadMotor ;
  rdfs:domain cim:LoadMotor ;
  rdfs:range cim:LoadAggregate ;
  skos:definition "Aggregate load to which this aggregate motor (dynamic) load belongs."@en .

cim:LoadStatic.LoadAggregate a owl:ObjectProperty ;
  rdfs:label "LoadAggregate"@en ;
  owl:inverseOf cim:LoadAggregate.LoadStatic ;
  rdfs:domain cim:LoadStatic ;
  rdfs:range cim:LoadAggregate ;
  skos:definition "Aggregate load to which this aggregate static load belongs."@en .

cim:LoadUserDefined.ProprietaryParameterDynamics a owl:ObjectProperty ;
  rdfs:label "ProprietaryParameterDynamics"@en ;
  owl:inverseOf cim:ProprietaryParameterDynamics.LoadUserDefined ;
  rdfs:domain cim:LoadUserDefined ;
  rdfs:range cim:ProprietaryParameterDynamics ;
  skos:definition "Parameter of this proprietary user-defined model."@en .

cim:MechanicalLoadDynamics.AsynchronousMachineDynamics a owl:ObjectProperty, owl:FunctionalProperty ;
  rdfs:label "AsynchronousMachineDynamics"@en ;
  owl:inverseOf cim:AsynchronousMachineDynamics.MechanicalLoadDynamics ;
  rdfs:domain cim:MechanicalLoadDynamics ;
  rdfs:range cim:AsynchronousMachineDynamics ;
  skos:definition "Asynchronous machine model with which this mechanical load model is associated. MechanicalLoadDynamics shall have either an association to SynchronousMachineDynamics or to AsynchronousMachineDynamics."@en .

cim:MechanicalLoadDynamics.SynchronousMachineDynamics a owl:ObjectProperty, owl:FunctionalProperty ;
  rdfs:label "SynchronousMachineDynamics"@en ;
  owl:inverseOf cim:SynchronousMachineDynamics.MechanicalLoadDynamics ;
  rdfs:domain cim:MechanicalLoadDynamics ;
  rdfs:range cim:SynchronousMachineDynamics ;
  skos:definition "Synchronous machine model with which this mechanical load model is associated. MechanicalLoadDynamics shall have either an association to SynchronousMachineDynamics or AsynchronousMachineDyanmics."@en .

cim:MechanicalLoadUserDefined.ProprietaryParameterDynamics a owl:ObjectProperty ;
  rdfs:label "ProprietaryParameterDynamics"@en ;
  owl:inverseOf cim:ProprietaryParameterDynamics.MechanicalLoadUserDefined ;
  rdfs:domain cim:MechanicalLoadUserDefined ;
  rdfs:range cim:ProprietaryParameterDynamics ;
  skos:definition "Parameter of this proprietary user-defined model."@en .

cim:OverexcitationLimiterDynamics.ExcitationSystemDynamics a owl:ObjectProperty ;
  rdfs:label "ExcitationSystemDynamics"@en ;
  owl:inverseOf cim:ExcitationSystemDynamics.OverexcitationLimiterDynamics ;
  rdfs:domain cim:OverexcitationLimiterDynamics ;
  rdfs:range cim:ExcitationSystemDynamics ;
  skos:definition "Excitation system model with which this overexcitation limiter model is associated."@en .

cim:OverexcitationLimiterUserDefined.ProprietaryParameterDynamics a owl:ObjectProperty ;
  rdfs:label "ProprietaryParameterDynamics"@en ;
  owl:inverseOf cim:ProprietaryParameterDynamics.OverexcitationLimiterUserDefined ;
  rdfs:domain cim:OverexcitationLimiterUserDefined ;
  rdfs:range cim:ProprietaryParameterDynamics ;
  skos:definition "Parameter of this proprietary user-defined model."@en .

cim:PFVArControllerType1Dynamics.ExcitationSystemDynamics a owl:ObjectProperty ;
  rdfs:label "ExcitationSystemDynamics"@en ;
  owl:inverseOf cim:ExcitationSystemDynamics.PFVArControllerType1Dynamics ;
  rdfs:domain cim:PFVArControllerType1Dynamics ;
  rdfs:range cim:ExcitationSystemDynamics ;
  skos:definition "Excitation system model with which this power actor or VAr controller type 1 model is associated."@en .

cim:PFVArControllerType1Dynamics.RemoteInputSignal a owl:ObjectProperty, owl:FunctionalProperty ;
  rdfs:label "RemoteInputSignal"@en ;
  owl:inverseOf cim:RemoteInputSignal.PFVArControllerType1Dynamics ;
  rdfs:domain cim:PFVArControllerType1Dynamics ;
  rdfs:range cim:RemoteInputSignal ;
  skos:definition "Remote input signal used by this power factor or VAr controller type 1 model."@en .

cim:PFVArControllerType1Dynamics.VoltageAdjusterDynamics a owl:ObjectProperty, owl:FunctionalProperty ;
  rdfs:label "VoltageAdjusterDynamics"@en ;
  owl:inverseOf cim:VoltageAdjusterDynamics.PFVArControllerType1Dynamics ;
  rdfs:domain cim:PFVArControllerType1Dynamics ;
  rdfs:range cim:VoltageAdjusterDynamics ;
  skos:definition "Voltage adjuster model associated with this power factor or VAr controller type 1 model."@en .

cim:PFVArControllerType1UserDefined.ProprietaryParameterDynamics a owl:ObjectProperty ;
  rdfs:label "ProprietaryParameterDynamics"@en ;
  owl:inverseOf cim:ProprietaryParameterDynamics.PFVArControllerType1UserDefined ;
  rdfs:domain cim:PFVArControllerType1UserDefined ;
  rdfs:range cim:ProprietaryParameterDynamics ;
  skos:definition "Parameter of this proprietary user-defined model."@en .

cim:PFVArControllerType2Dynamics.ExcitationSystemDynamics a owl:ObjectProperty ;
  rdfs:label "ExcitationSystemDynamics"@en ;
  owl:inverseOf cim:ExcitationSystemDynamics.PFVArControllerType2Dynamics ;
  rdfs:domain cim:PFVArControllerType2Dynamics ;
  rdfs:range cim:ExcitationSystemDynamics ;
  skos:definition "Excitation system model with which this power factor or VAr controller type 2 is associated."@en .

cim:PFVArControllerType2UserDefined.ProprietaryParameterDynamics a owl:ObjectProperty ;
  rdfs:label "ProprietaryParameterDynamics"@en ;
  owl:inverseOf cim:ProprietaryParameterDynamics.PFVArControllerType2UserDefined ;
  rdfs:domain cim:PFVArControllerType2UserDefined ;
  rdfs:range cim:ProprietaryParameterDynamics ;
  skos:definition "Parameter of this proprietary user-defined model."@en .

cim:PowerElectronicsConnection.WindTurbineType3or4Dynamics a owl:ObjectProperty, owl:FunctionalProperty ;
  rdfs:label "WindTurbineType3or4Dynamics"@en ;
  owl:inverseOf cim:WindTurbineType3or4Dynamics.PowerElectronicsConnection ;
  rdfs:domain cim:PowerElectronicsConnection ;
  rdfs:range cim:WindTurbineType3or4Dynamics ;
  skos:definition "The wind turbine type 3 or type 4 dynamics model associated with this power electronics connection."@en .

cim:PowerSystemStabilizerDynamics.ExcitationSystemDynamics a owl:ObjectProperty ;
  rdfs:label "ExcitationSystemDynamics"@en ;
  owl:inverseOf cim:ExcitationSystemDynamics.PowerSystemStabilizerDynamics ;
  rdfs:domain cim:PowerSystemStabilizerDynamics ;
  rdfs:range cim:ExcitationSystemDynamics ;
  skos:definition "Excitation system model with which this power system stabilizer model is associated."@en .

cim:PowerSystemStabilizerDynamics.RemoteInputSignal a owl:ObjectProperty ;
  rdfs:label "RemoteInputSignal"@en ;
  owl:inverseOf cim:RemoteInputSignal.PowerSystemStabilizerDynamics ;
  rdfs:domain cim:PowerSystemStabilizerDynamics ;
  rdfs:range cim:RemoteInputSignal ;
  skos:definition "Remote input signal used by this power system stabilizer model."@en .

cim:PowerSystemStabilizerUserDefined.ProprietaryParameterDynamics a owl:ObjectProperty ;
  rdfs:label "ProprietaryParameterDynamics"@en ;
  owl:inverseOf cim:ProprietaryParameterDynamics.PowerSystemStabilizerUserDefined ;
  rdfs:domain cim:PowerSystemStabilizerUserDefined ;
  rdfs:range cim:ProprietaryParameterDynamics ;
  skos:definition "Parameter of this proprietary user-defined model."@en .

cim:ProprietaryParameterDynamics.AsynchronousMachineUserDefined a owl:ObjectProperty, owl:FunctionalProperty ;
  rdfs:label "AsynchronousMachineUserDefined"@en ;
  owl:inverseOf cim:AsynchronousMachineUserDefined.ProprietaryParameterDynamics ;
  rdfs:domain cim:ProprietaryParameterDynamics ;
  rdfs:range cim:AsynchronousMachineUserDefined ;
  skos:definition "Proprietary user-defined model with which this parameter is associated."@en .

cim:ProprietaryParameterDynamics.CSCUserDefined a owl:ObjectProperty, owl:FunctionalProperty ;
  rdfs:label "CSCUserDefined"@en ;
  owl:inverseOf cim:CSCUserDefined.ProprietaryParameterDynamics ;
  rdfs:domain cim:ProprietaryParameterDynamics ;
  rdfs:range cim:CSCUserDefined ;
  skos:definition "Proprietary user-defined model with which this parameter is associated."@en .

cim:ProprietaryParameterDynamics.DiscontinuousExcitationControlUserDefined a owl:ObjectProperty, owl:FunctionalProperty ;
  rdfs:label "DiscontinuousExcitationControlUserDefined"@en ;
  owl:inverseOf cim:DiscontinuousExcitationControlUserDefined.ProprietaryParameterDynamics ;
  rdfs:domain cim:ProprietaryParameterDynamics ;
  rdfs:range cim:DiscontinuousExcitationControlUserDefined ;
  skos:definition "Proprietary user-defined model with which this parameter is associated."@en .

cim:ProprietaryParameterDynamics.ExcitationSystemUserDefined a owl:ObjectProperty, owl:FunctionalProperty ;
  rdfs:label "ExcitationSystemUserDefined"@en ;
  owl:inverseOf cim:ExcitationSystemUserDefined.ProprietaryParameterDynamics ;
  rdfs:domain cim:ProprietaryParameterDynamics ;
  rdfs:range cim:ExcitationSystemUserDefined ;
  skos:definition "Proprietary user-defined model with which this parameter is associated."@en .

cim:ProprietaryParameterDynamics.LoadUserDefined a owl:ObjectProperty, owl:FunctionalProperty ;
  rdfs:label "LoadUserDefined"@en ;
  owl:inverseOf cim:LoadUserDefined.ProprietaryParameterDynamics ;
  rdfs:domain cim:ProprietaryParameterDynamics ;
  rdfs:range cim:LoadUserDefined ;
  skos:definition "Proprietary user-defined model with which this parameter is associated."@en .

cim:ProprietaryParameterDynamics.MechanicalLoadUserDefined a owl:ObjectProperty, owl:FunctionalProperty ;
  rdfs:label "MechanicalLoadUserDefined"@en ;
  owl:inverseOf cim:MechanicalLoadUserDefined.ProprietaryParameterDynamics ;
  rdfs:domain cim:ProprietaryParameterDynamics ;
  rdfs:range cim:MechanicalLoadUserDefined ;
  skos:definition "Proprietary user-defined model with which this parameter is associated."@en .

cim:ProprietaryParameterDynamics.OverexcitationLimiterUserDefined a owl:ObjectProperty, owl:FunctionalProperty ;
  rdfs:label "OverexcitationLimiterUserDefined"@en ;
  owl:inverseOf cim:OverexcitationLimiterUserDefined.ProprietaryParameterDynamics ;
  rdfs:domain cim:ProprietaryParameterDynamics ;
  rdfs:range cim:OverexcitationLimiterUserDefined ;
  skos:definition "Proprietary user-defined model with which this parameter is associated."@en .

cim:ProprietaryParameterDynamics.PFVArControllerType1UserDefined a owl:ObjectProperty, owl:FunctionalProperty ;
  rdfs:label "PFVArControllerType1UserDefined"@en ;
  owl:inverseOf cim:PFVArControllerType1UserDefined.ProprietaryParameterDynamics ;
  rdfs:domain cim:ProprietaryParameterDynamics ;
  rdfs:range cim:PFVArControllerType1UserDefined ;
  skos:definition "Proprietary user-defined model with which this parameter is associated."@en .

cim:ProprietaryParameterDynamics.PFVArControllerType2UserDefined a owl:ObjectProperty, owl:FunctionalProperty ;
  rdfs:label "PFVArControllerType2UserDefined"@en ;
  owl:inverseOf cim:PFVArControllerType2UserDefined.ProprietaryParameterDynamics ;
  rdfs:domain cim:ProprietaryParameterDynamics ;
  rdfs:range cim:PFVArControllerType2UserDefined ;
  skos:definition "Proprietary user-defined model with which this parameter is associated."@en .

cim:ProprietaryParameterDynamics.PowerSystemStabilizerUserDefined a owl:ObjectProperty, owl:FunctionalProperty ;
  rdfs:label "PowerSystemStabilizerUserDefined"@en ;
  owl:inverseOf cim:PowerSystemStabilizerUserDefined.ProprietaryParameterDynamics ;
  rdfs:domain cim:ProprietaryParameterDynamics ;
  rdfs:range cim:PowerSystemStabilizerUserDefined ;
  skos:definition "Proprietary user-defined model with which this parameter is associated."@en .

cim:ProprietaryParameterDynamics.SVCUserDefined a owl:ObjectProperty, owl:FunctionalProperty ;
  rdfs:label "SVCUserDefined"@en ;
  owl:inverseOf cim:SVCUserDefined.ProprietaryParameterDynamics ;
  rdfs:domain cim:ProprietaryParameterDynamics ;
  rdfs:range cim:SVCUserDefined ;
  skos:definition "Proprietary user-defined model with which this parameter is associated."@en .

cim:ProprietaryParameterDynamics.SynchronousMachineUserDefined a owl:ObjectProperty, owl:FunctionalProperty ;
  rdfs:label "SynchronousMachineUserDefined"@en ;
  owl:inverseOf cim:SynchronousMachineUserDefined.ProprietaryParameterDynamics ;
  rdfs:domain cim:ProprietaryParameterDynamics ;
  rdfs:range cim:SynchronousMachineUserDefined ;
  skos:definition "Proprietary user-defined model with which this parameter is associated."@en .

cim:ProprietaryParameterDynamics.TurbineGovernorUserDefined a owl:ObjectProperty, owl:FunctionalProperty ;
  rdfs:label "TurbineGovernorUserDefined"@en ;
  owl:inverseOf cim:TurbineGovernorUserDefined.ProprietaryParameterDynamics ;
  rdfs:domain cim:ProprietaryParameterDynamics ;
  rdfs:range cim:TurbineGovernorUserDefined ;
  skos:definition "Proprietary user-defined model with which this parameter is associated."@en .

cim:ProprietaryParameterDynamics.TurbineLoadControllerUserDefined a owl:ObjectProperty, owl:FunctionalProperty ;
  rdfs:label "TurbineLoadControllerUserDefined"@en ;
  owl:inverseOf cim:TurbineLoadControllerUserDefined.ProprietaryParameterDynamics ;
  rdfs:domain cim:ProprietaryParameterDynamics ;
  rdfs:range cim:TurbineLoadControllerUserDefined ;
  skos:definition "Proprietary user-defined model with which this parameter is associated."@en .

cim:ProprietaryParameterDynamics.UnderexcitationLimiterUserDefined a owl:ObjectProperty, owl:FunctionalProperty ;
  rdfs:label "UnderexcitationLimiterUserDefined"@en ;
  owl:inverseOf cim:UnderexcitationLimiterUserDefined.ProprietaryParameterDynamics ;
  rdfs:domain cim:ProprietaryParameterDynamics ;
  rdfs:range cim:UnderexcitationLimiterUserDefined ;
  skos:definition "Proprietary user-defined model with which this parameter is associated."@en .

cim:ProprietaryParameterDynamics.VSCUserDefined a owl:ObjectProperty, owl:FunctionalProperty ;
  rdfs:label "VSCUserDefined"@en ;
  owl:inverseOf cim:VSCUserDefined.ProprietaryParameterDynamics ;
  rdfs:domain cim:ProprietaryParameterDynamics ;
  rdfs:range cim:VSCUserDefined ;
  skos:definition "Proprietary user-defined model with which this parameter is associated."@en .

cim:ProprietaryParameterDynamics.VoltageAdjusterUserDefined a owl:ObjectProperty, owl:FunctionalProperty ;
  rdfs:label "VoltageAdjusterUserDefined"@en ;
  owl:inverseOf cim:VoltageAdjusterUserDefined.ProprietaryParameterDynamics ;
  rdfs:domain cim:ProprietaryParameterDynamics ;
  rdfs:range cim:VoltageAdjusterUserDefined ;
  skos:definition "Proprietary user-defined model with which this parameter is associated."@en .

cim:ProprietaryParameterDynamics.VoltageCompensatorUserDefined a owl:ObjectProperty, owl:FunctionalProperty ;
  rdfs:label "VoltageCompensatorUserDefined"@en ;
  owl:inverseOf cim:VoltageCompensatorUserDefined.ProprietaryParameterDynamics ;
  rdfs:domain cim:ProprietaryParameterDynamics ;
  rdfs:range cim:VoltageCompensatorUserDefined ;
  skos:definition "Proprietary user-defined model with which this parameter is associated."@en .

cim:ProprietaryParameterDynamics.WindPlantUserDefined a owl:ObjectProperty, owl:FunctionalProperty ;
  rdfs:label "WindPlantUserDefined"@en ;
  owl:inverseOf cim:WindPlantUserDefined.ProprietaryParameterDynamics ;
  rdfs:domain cim:ProprietaryParameterDynamics ;
  rdfs:range cim:WindPlantUserDefined ;
  skos:definition "Proprietary user-defined model with which this parameter is associated."@en .

cim:ProprietaryParameterDynamics.WindType1or2UserDefined a owl:ObjectProperty, owl:FunctionalProperty ;
  rdfs:label "WindType1or2UserDefined"@en ;
  owl:inverseOf cim:WindType1or2UserDefined.ProprietaryParameterDynamics ;
  rdfs:domain cim:ProprietaryParameterDynamics ;
  rdfs:range cim:WindType1or2UserDefined ;
  skos:definition "Proprietary user-defined model with which this parameter is associated."@en .

cim:ProprietaryParameterDynamics.WindType3or4UserDefined a owl:ObjectProperty, owl:FunctionalProperty ;
  rdfs:label "WindType3or4UserDefined"@en ;
  owl:inverseOf cim:WindType3or4UserDefined.ProprietaryParameterDynamics ;
  rdfs:domain cim:ProprietaryParameterDynamics ;
  rdfs:range cim:WindType3or4UserDefined ;
  skos:definition "Proprietary user-defined model with which this parameter is associated."@en .

cim:RemoteInputSignal.DiscontinuousExcitationControlDynamics a owl:ObjectProperty, owl:FunctionalProperty ;
  rdfs:label "DiscontinuousExcitationControlDynamics"@en ;
  owl:inverseOf cim:DiscontinuousExcitationControlDynamics.RemoteInputSignal ;
  rdfs:domain cim:RemoteInputSignal ;
  rdfs:range cim:DiscontinuousExcitationControlDynamics ;
  skos:definition "Discontinuous excitation control model using this remote input signal."@en .

cim:RemoteInputSignal.PFVArControllerType1Dynamics a owl:ObjectProperty, owl:FunctionalProperty ;
  rdfs:label "PFVArControllerType1Dynamics"@en ;
  owl:inverseOf cim:PFVArControllerType1Dynamics.RemoteInputSignal ;
  rdfs:domain cim:RemoteInputSignal ;
  rdfs:range cim:PFVArControllerType1Dynamics ;
  skos:definition "Power factor or VAr controller type 1 model using this remote input signal."@en .

cim:RemoteInputSignal.PowerSystemStabilizerDynamics a owl:ObjectProperty, owl:FunctionalProperty ;
  rdfs:label "PowerSystemStabilizerDynamics"@en ;
  owl:inverseOf cim:PowerSystemStabilizerDynamics.RemoteInputSignal ;
  rdfs:domain cim:RemoteInputSignal ;
  rdfs:range cim:PowerSystemStabilizerDynamics ;
  skos:definition "Power system stabilizer model using this remote input signal."@en .

cim:RemoteInputSignal.Terminal a owl:ObjectProperty ;
  rdfs:label "Terminal"@en ;
  owl:inverseOf cim:Terminal.RemoteInputSignal ;
  rdfs:domain cim:RemoteInputSignal ;
  rdfs:range cim:Terminal ;
  skos:definition "Remote terminal with which this input signal is associated."@en .

cim:RemoteInputSignal.UnderexcitationLimiterDynamics a owl:ObjectProperty, owl:FunctionalProperty ;
  rdfs:label "UnderexcitationLimiterDynamics"@en ;
  owl:inverseOf cim:UnderexcitationLimiterDynamics.RemoteInputSignal ;
  rdfs:domain cim:RemoteInputSignal ;
  rdfs:range cim:UnderexcitationLimiterDynamics ;
  skos:definition "Underexcitation limiter model using this remote input signal."@en .

cim:RemoteInputSignal.VoltageCompensatorDynamics a owl:ObjectProperty, owl:FunctionalProperty ;
  rdfs:label "VoltageCompensatorDynamics"@en ;
  owl:inverseOf cim:VoltageCompensatorDynamics.RemoteInputSignal ;
  rdfs:domain cim:RemoteInputSignal ;
  rdfs:range cim:VoltageCompensatorDynamics ;
  skos:definition "Voltage compensator model using this remote input signal."@en .

cim:RemoteInputSignal.WindPlantDynamics a owl:ObjectProperty, owl:FunctionalProperty ;
  rdfs:label "WindPlantDynamics"@en ;
  owl:inverseOf cim:WindPlantDynamics.RemoteInputSignal ;
  rdfs:domain cim:RemoteInputSignal ;
  rdfs:range cim:WindPlantDynamics ;
  skos:definition "The wind plant using the remote signal."@en .

cim:RemoteInputSignal.WindTurbineType1or2Dynamics a owl:ObjectProperty, owl:FunctionalProperty ;
  rdfs:label "WindTurbineType1or2Dynamics"@en ;
  owl:inverseOf cim:WindTurbineType1or2Dynamics.RemoteInputSignal ;
  rdfs:domain cim:RemoteInputSignal ;
  rdfs:range cim:WindTurbineType1or2Dynamics ;
  skos:definition "Wind generator type 1 or type 2 model using this remote input signal."@en .

cim:RemoteInputSignal.WindTurbineType3or4Dynamics a owl:ObjectProperty, owl:FunctionalProperty ;
  rdfs:label "WindTurbineType3or4Dynamics"@en ;
  owl:inverseOf cim:WindTurbineType3or4Dynamics.RemoteInputSignal ;
  rdfs:domain cim:RemoteInputSignal ;
  rdfs:range cim:WindTurbineType3or4Dynamics ;
  skos:definition "Wind turbine type 3 or type 4 models using this remote input signal."@en .

cim:SVCUserDefined.ProprietaryParameterDynamics a owl:ObjectProperty ;
  rdfs:label "ProprietaryParameterDynamics"@en ;
  owl:inverseOf cim:ProprietaryParameterDynamics.SVCUserDefined ;
  rdfs:domain cim:SVCUserDefined ;
  rdfs:range cim:ProprietaryParameterDynamics ;
  skos:definition "Parameter of this proprietary user-defined model."@en .

cim:StaticVarCompensator.StaticVarCompensatorDynamics a owl:ObjectProperty, owl:FunctionalProperty ;
  rdfs:label "StaticVarCompensatorDynamics"@en ;
  owl:inverseOf cim:StaticVarCompensatorDynamics.StaticVarCompensator ;
  rdfs:domain cim:StaticVarCompensator ;
  rdfs:range cim:StaticVarCompensatorDynamics ;
  skos:definition "Static Var Compensator dynamics model used to describe dynamic behaviour of this Static Var Compensator."@en .

cim:StaticVarCompensatorDynamics.StaticVarCompensator a owl:ObjectProperty ;
  rdfs:label "StaticVarCompensator"@en ;
  owl:inverseOf cim:StaticVarCompensator.StaticVarCompensatorDynamics ;
  rdfs:domain cim:StaticVarCompensatorDynamics ;
  rdfs:range cim:StaticVarCompensator ;
  skos:definition "Static Var Compensator to which Static Var Compensator dynamics model applies."@en .

cim:SynchronousMachine.SynchronousMachineDynamics a owl:ObjectProperty, owl:FunctionalProperty ;
  rdfs:label "SynchronousMachineDynamics"@en ;
  owl:inverseOf cim:SynchronousMachineDynamics.SynchronousMachine ;
  rdfs:domain cim:SynchronousMachine ;
  rdfs:range cim:SynchronousMachineDynamics ;
  skos:definition "Synchronous machine dynamics model used to describe dynamic behaviour of this synchronous machine."@en .

cim:SynchronousMachineDynamics.CrossCompoundTurbineGovernorDyanmics a owl:ObjectProperty, owl:FunctionalProperty ;
  rdfs:label "CrossCompoundTurbineGovernorDyanmics"@en ;
  owl:inverseOf cim:CrossCompoundTurbineGovernorDynamics.HighPressureSynchronousMachineDynamics ;
  rdfs:domain cim:SynchronousMachineDynamics ;
  rdfs:range cim:CrossCompoundTurbineGovernorDynamics ;
  skos:definition "The cross-compound turbine governor with which this high-pressure synchronous machine is associated."@en .

cim:SynchronousMachineDynamics.CrossCompoundTurbineGovernorDynamics a owl:ObjectProperty, owl:FunctionalProperty ;
  rdfs:label "CrossCompoundTurbineGovernorDynamics"@en ;
  owl:inverseOf cim:CrossCompoundTurbineGovernorDynamics.LowPressureSynchronousMachineDynamics ;
  rdfs:domain cim:SynchronousMachineDynamics ;
  rdfs:range cim:CrossCompoundTurbineGovernorDynamics ;
  skos:definition "The cross-compound turbine governor with which this low-pressure synchronous machine is associated."@en .

cim:SynchronousMachineDynamics.ExcitationSystemDynamics a owl:ObjectProperty, owl:FunctionalProperty ;
  rdfs:label "ExcitationSystemDynamics"@en ;
  owl:inverseOf cim:ExcitationSystemDynamics.SynchronousMachineDynamics ;
  rdfs:domain cim:SynchronousMachineDynamics ;
  rdfs:range cim:ExcitationSystemDynamics ;
  skos:definition "Excitation system model associated with this synchronous machine model."@en .

cim:SynchronousMachineDynamics.GenICompensationForGenJ a owl:ObjectProperty ;
  rdfs:label "GenICompensationForGenJ"@en ;
  owl:inverseOf cim:GenICompensationForGenJ.SynchronousMachineDynamics ;
  rdfs:domain cim:SynchronousMachineDynamics ;
  rdfs:range cim:GenICompensationForGenJ ;
  skos:definition "Compensation of voltage compensator's generator for current flow out of this  generator."@en .

cim:SynchronousMachineDynamics.MechanicalLoadDynamics a owl:ObjectProperty, owl:FunctionalProperty ;
  rdfs:label "MechanicalLoadDynamics"@en ;
  owl:inverseOf cim:MechanicalLoadDynamics.SynchronousMachineDynamics ;
  rdfs:domain cim:SynchronousMachineDynamics ;
  rdfs:range cim:MechanicalLoadDynamics ;
  skos:definition "Mechanical load model associated with this synchronous machine model."@en .

cim:SynchronousMachineDynamics.SynchronousMachine a owl:ObjectProperty ;
  rdfs:label "SynchronousMachine"@en ;
  owl:inverseOf cim:SynchronousMachine.SynchronousMachineDynamics ;
  rdfs:domain cim:SynchronousMachineDynamics ;
  rdfs:range cim:SynchronousMachine ;
  skos:definition "Synchronous machine to which synchronous machine dynamics model applies."@en .

cim:SynchronousMachineDynamics.TurbineGovernorDynamics a owl:ObjectProperty ;
  rdfs:label "TurbineGovernorDynamics"@en ;
  owl:inverseOf cim:TurbineGovernorDynamics.SynchronousMachineDynamics ;
  rdfs:domain cim:SynchronousMachineDynamics ;
  rdfs:range cim:TurbineGovernorDynamics ;
  skos:definition "Turbine-governor model associated with this synchronous machine model. Multiplicity of greater than one is intended to support hydro units that have multiple turbines on one generator."@en .

cim:SynchronousMachineUserDefined.ProprietaryParameterDynamics a owl:ObjectProperty ;
  rdfs:label "ProprietaryParameterDynamics"@en ;
  owl:inverseOf cim:ProprietaryParameterDynamics.SynchronousMachineUserDefined ;
  rdfs:domain cim:SynchronousMachineUserDefined ;
  rdfs:range cim:ProprietaryParameterDynamics ;
  skos:definition "Parameter of this proprietary user-defined model."@en .

cim:Terminal.ConductingEquipment a owl:ObjectProperty ;
  rdfs:label "ConductingEquipment"@en ;
  owl:inverseOf cim:ConductingEquipment.Terminals ;
  rdfs:domain cim:Terminal ;
  rdfs:range cim:ConductingEquipment ;
  skos:definition "The conducting equipment of the terminal.  Conducting equipment have  terminals that may be connected to other conducting equipment terminals via connectivity nodes or topological nodes."@en .

cim:Terminal.RemoteInputSignal a owl:ObjectProperty ;
  rdfs:label "RemoteInputSignal"@en ;
  owl:inverseOf cim:RemoteInputSignal.Terminal ;
  rdfs:domain cim:Terminal ;
  rdfs:range cim:RemoteInputSignal ;
  skos:definition "Input signal coming from this terminal."@en .

cim:TurbineGovernorDynamics.AsynchronousMachineDynamics a owl:ObjectProperty, owl:FunctionalProperty ;
  rdfs:label "AsynchronousMachineDynamics"@en ;
  owl:inverseOf cim:AsynchronousMachineDynamics.TurbineGovernorDynamics ;
  rdfs:domain cim:TurbineGovernorDynamics ;
  rdfs:range cim:AsynchronousMachineDynamics ;
  skos:definition "Asynchronous machine model with which this turbine-governor model is associated. TurbineGovernorDynamics shall have either an association to SynchronousMachineDynamics or to AsynchronousMachineDynamics."@en .

cim:TurbineGovernorDynamics.SynchronousMachineDynamics a owl:ObjectProperty, owl:FunctionalProperty ;
  rdfs:label "SynchronousMachineDynamics"@en ;
  owl:inverseOf cim:SynchronousMachineDynamics.TurbineGovernorDynamics ;
  rdfs:domain cim:TurbineGovernorDynamics ;
  rdfs:range cim:SynchronousMachineDynamics ;
  skos:definition "Synchronous machine model with which this turbine-governor model is associated. TurbineGovernorDynamics shall have either an association to SynchronousMachineDynamics or to AsynchronousMachineDynamics."@en .

cim:TurbineGovernorDynamics.TurbineLoadControllerDynamics a owl:ObjectProperty, owl:FunctionalProperty ;
  rdfs:label "TurbineLoadControllerDynamics"@en ;
  owl:inverseOf cim:TurbineLoadControllerDynamics.TurbineGovernorDynamics ;
  rdfs:domain cim:TurbineGovernorDynamics ;
  rdfs:range cim:TurbineLoadControllerDynamics ;
  skos:definition "Turbine load controller providing input to this turbine-governor."@en .

cim:TurbineGovernorUserDefined.ProprietaryParameterDynamics a owl:ObjectProperty ;
  rdfs:label "ProprietaryParameterDynamics"@en ;
  owl:inverseOf cim:ProprietaryParameterDynamics.TurbineGovernorUserDefined ;
  rdfs:domain cim:TurbineGovernorUserDefined ;
  rdfs:range cim:ProprietaryParameterDynamics ;
  skos:definition "Parameter of this proprietary user-defined model."@en .

cim:TurbineLoadControllerDynamics.TurbineGovernorDynamics a owl:ObjectProperty ;
  rdfs:label "TurbineGovernorDynamics"@en ;
  owl:inverseOf cim:TurbineGovernorDynamics.TurbineLoadControllerDynamics ;
  rdfs:domain cim:TurbineLoadControllerDynamics ;
  rdfs:range cim:TurbineGovernorDynamics ;
  skos:definition "Turbine-governor controlled by this turbine load controller."@en .

cim:TurbineLoadControllerUserDefined.ProprietaryParameterDynamics a owl:ObjectProperty ;
  rdfs:label "ProprietaryParameterDynamics"@en ;
  owl:inverseOf cim:ProprietaryParameterDynamics.TurbineLoadControllerUserDefined ;
  rdfs:domain cim:TurbineLoadControllerUserDefined ;
  rdfs:range cim:ProprietaryParameterDynamics ;
  skos:definition "Parameter of this proprietary user-defined model."@en .

cim:UnderexcitationLimiterDynamics.ExcitationSystemDynamics a owl:ObjectProperty ;
  rdfs:label "ExcitationSystemDynamics"@en ;
  owl:inverseOf cim:ExcitationSystemDynamics.UnderexcitationLimiterDynamics ;
  rdfs:domain cim:UnderexcitationLimiterDynamics ;
  rdfs:range cim:ExcitationSystemDynamics ;
  skos:definition "Excitation system model with which this underexcitation limiter model is associated."@en .

cim:UnderexcitationLimiterDynamics.RemoteInputSignal a owl:ObjectProperty, owl:FunctionalProperty ;
  rdfs:label "RemoteInputSignal"@en ;
  owl:inverseOf cim:RemoteInputSignal.UnderexcitationLimiterDynamics ;
  rdfs:domain cim:UnderexcitationLimiterDynamics ;
  rdfs:range cim:RemoteInputSignal ;
  skos:definition "Remote input signal used by this underexcitation limiter model."@en .

cim:UnderexcitationLimiterUserDefined.ProprietaryParameterDynamics a owl:ObjectProperty ;
  rdfs:label "ProprietaryParameterDynamics"@en ;
  owl:inverseOf cim:ProprietaryParameterDynamics.UnderexcitationLimiterUserDefined ;
  rdfs:domain cim:UnderexcitationLimiterUserDefined ;
  rdfs:range cim:ProprietaryParameterDynamics ;
  skos:definition "Parameter of this proprietary user-defined model."@en .

cim:VCompIEEEType2.GenICompensationForGenJ a owl:ObjectProperty ;
  rdfs:label "GenICompensationForGenJ"@en ;
  owl:inverseOf cim:GenICompensationForGenJ.VcompIEEEType2 ;
  rdfs:domain cim:VCompIEEEType2 ;
  rdfs:range cim:GenICompensationForGenJ ;
  skos:definition "Compensation of this voltage compensator's generator for current flow out of another generator."@en .

cim:VSCDynamics.VsConverter a owl:ObjectProperty ;
  rdfs:label "VsConverter"@en ;
  owl:inverseOf cim:VsConverter.VSCDynamics ;
  rdfs:domain cim:VSCDynamics ;
  rdfs:range cim:VsConverter ;
  skos:definition "Voltage source converter to which voltage source converter dynamics model applies."@en .

cim:VSCUserDefined.ProprietaryParameterDynamics a owl:ObjectProperty ;
  rdfs:label "ProprietaryParameterDynamics"@en ;
  owl:inverseOf cim:ProprietaryParameterDynamics.VSCUserDefined ;
  rdfs:domain cim:VSCUserDefined ;
  rdfs:range cim:ProprietaryParameterDynamics ;
  skos:definition "Parameter of this proprietary user-defined model."@en .

cim:VoltageAdjusterDynamics.PFVArControllerType1Dynamics a owl:ObjectProperty ;
  rdfs:label "PFVArControllerType1Dynamics"@en ;
  owl:inverseOf cim:PFVArControllerType1Dynamics.VoltageAdjusterDynamics ;
  rdfs:domain cim:VoltageAdjusterDynamics ;
  rdfs:range cim:PFVArControllerType1Dynamics ;
  skos:definition "Power factor or VAr controller type 1 model with which this voltage adjuster is associated."@en .

cim:VoltageAdjusterUserDefined.ProprietaryParameterDynamics a owl:ObjectProperty ;
  rdfs:label "ProprietaryParameterDynamics"@en ;
  owl:inverseOf cim:ProprietaryParameterDynamics.VoltageAdjusterUserDefined ;
  rdfs:domain cim:VoltageAdjusterUserDefined ;
  rdfs:range cim:ProprietaryParameterDynamics ;
  skos:definition "Parameter of this proprietary user-defined model."@en .

cim:VoltageCompensatorDynamics.ExcitationSystemDynamics a owl:ObjectProperty ;
  rdfs:label "ExcitationSystemDynamics"@en ;
  owl:inverseOf cim:ExcitationSystemDynamics.VoltageCompensatorDynamics ;
  rdfs:domain cim:VoltageCompensatorDynamics ;
  rdfs:range cim:ExcitationSystemDynamics ;
  skos:definition "Excitation system model with which this voltage compensator is associated."@en .

cim:VoltageCompensatorDynamics.RemoteInputSignal a owl:ObjectProperty, owl:FunctionalProperty ;
  rdfs:label "RemoteInputSignal"@en ;
  owl:inverseOf cim:RemoteInputSignal.VoltageCompensatorDynamics ;
  rdfs:domain cim:VoltageCompensatorDynamics ;
  rdfs:range cim:RemoteInputSignal ;
  skos:definition "Remote input signal used by this voltage compensator model."@en .

cim:VoltageCompensatorUserDefined.ProprietaryParameterDynamics a owl:ObjectProperty ;
  rdfs:label "ProprietaryParameterDynamics"@en ;
  owl:inverseOf cim:ProprietaryParameterDynamics.VoltageCompensatorUserDefined ;
  rdfs:domain cim:VoltageCompensatorUserDefined ;
  rdfs:range cim:ProprietaryParameterDynamics ;
  skos:definition "Parameter of this proprietary user-defined model."@en .

cim:VsConverter.VSCDynamics a owl:ObjectProperty, owl:FunctionalProperty ;
  rdfs:label "VSCDynamics"@en ;
  owl:inverseOf cim:VSCDynamics.VsConverter ;
  rdfs:domain cim:VsConverter ;
  rdfs:range cim:VSCDynamics ;
  skos:definition "Voltage source converter dynamics model used to describe dynamic behaviour of this converter."@en .

cim:WindAeroConstIEC.WindGenTurbineType1aIEC a owl:ObjectProperty ;
  rdfs:label "WindGenTurbineType1aIEC"@en ;
  owl:inverseOf cim:WindGenTurbineType1aIEC.WindAeroConstIEC ;
  rdfs:domain cim:WindAeroConstIEC ;
  rdfs:range cim:WindGenTurbineType1aIEC ;
  skos:definition "Wind turbine type 1A model with which this wind aerodynamic model is associated."@en .

cim:WindAeroOneDimIEC.WindTurbineType3IEC a owl:ObjectProperty ;
  rdfs:label "WindTurbineType3IEC"@en ;
  owl:inverseOf cim:WindTurbineType3IEC.WindAeroOneDimIEC ;
  rdfs:domain cim:WindAeroOneDimIEC ;
  rdfs:range cim:WindTurbineType3IEC ;
  skos:definition "Wind turbine type 3 model with which this wind aerodynamic model is associated."@en .

cim:WindAeroTwoDimIEC.WindTurbineType3IEC a owl:ObjectProperty ;
  rdfs:label "WindTurbineType3IEC"@en ;
  owl:inverseOf cim:WindTurbineType3IEC.WindAeroTwoDimIEC ;
  rdfs:domain cim:WindAeroTwoDimIEC ;
  rdfs:range cim:WindTurbineType3IEC ;
  skos:definition "Wind turbine type 3 model with which this wind aerodynamic model is associated."@en .

cim:WindContCurrLimIEC.WindDynamicsLookupTable a owl:ObjectProperty ;
  rdfs:label "WindDynamicsLookupTable"@en ;
  owl:inverseOf cim:WindDynamicsLookupTable.WindContCurrLimIEC ;
  rdfs:domain cim:WindContCurrLimIEC ;
  rdfs:range cim:WindDynamicsLookupTable ;
  skos:definition "The wind dynamics lookup table associated with this current control limitation model."@en .

cim:WindContCurrLimIEC.WindTurbineType3or4IEC a owl:ObjectProperty ;
  rdfs:label "WindTurbineType3or4IEC"@en ;
  owl:inverseOf cim:WindTurbineType3or4IEC.WindContCurrLimIEC ;
  rdfs:domain cim:WindContCurrLimIEC ;
  rdfs:range cim:WindTurbineType3or4IEC ;
  skos:definition "Wind turbine type 3 or type 4 model with which this wind control current limitation model is associated."@en .

cim:WindContPType3IEC.WindDynamicsLookupTable a owl:ObjectProperty ;
  rdfs:label "WindDynamicsLookupTable"@en ;
  owl:inverseOf cim:WindDynamicsLookupTable.WindContPType3IEC ;
  rdfs:domain cim:WindContPType3IEC ;
  rdfs:range cim:WindDynamicsLookupTable ;
  skos:definition "The wind dynamics lookup table associated with this P control type 3 model."@en .

cim:WindContPType3IEC.WindTurbineType3IEC a owl:ObjectProperty ;
  rdfs:label "WindTurbineType3IEC"@en ;
  owl:inverseOf cim:WindTurbineType3IEC.WindContPType3IEC ;
  rdfs:domain cim:WindContPType3IEC ;
  rdfs:range cim:WindTurbineType3IEC ;
  skos:definition "Wind turbine type 3 model with which this wind control P type 3 model is associated."@en .

cim:WindContPType4aIEC.WindTurbineType4aIEC a owl:ObjectProperty ;
  rdfs:label "WindTurbineType4aIEC"@en ;
  owl:inverseOf cim:WindTurbineType4aIEC.WindContPType4aIEC ;
  rdfs:domain cim:WindContPType4aIEC ;
  rdfs:range cim:WindTurbineType4aIEC ;
  skos:definition " Wind turbine type 4A model with which this wind control P type 4A model is associated."@en .

cim:WindContPType4bIEC.WindTurbineType4bIEC a owl:ObjectProperty ;
  rdfs:label "WindTurbineType4bIEC"@en ;
  owl:inverseOf cim:WindTurbineType4bIEC.WindContPType4bIEC ;
  rdfs:domain cim:WindContPType4bIEC ;
  rdfs:range cim:WindTurbineType4bIEC ;
  skos:definition "Wind turbine type 4B model with which this wind control P type 4B model is associated."@en .

cim:WindContPitchAngleIEC.WindTurbineType3IEC a owl:ObjectProperty ;
  rdfs:label "WindTurbineType3IEC"@en ;
  owl:inverseOf cim:WindTurbineType3IEC.WindContPitchAngleIEC ;
  rdfs:domain cim:WindContPitchAngleIEC ;
  rdfs:range cim:WindTurbineType3IEC ;
  skos:definition "Wind turbine type 3 model with which this pitch control model is associated."@en .

cim:WindContQIEC.WindTurbineType3or4IEC a owl:ObjectProperty ;
  rdfs:label "WindTurbineType3or4IEC"@en ;
  owl:inverseOf cim:WindTurbineType3or4IEC.WIndContQIEC ;
  rdfs:domain cim:WindContQIEC ;
  rdfs:range cim:WindTurbineType3or4IEC ;
  skos:definition "Wind turbine type 3 or type 4 model with which this reactive control model is associated."@en .

cim:WindContQLimIEC.WindTurbineType3or4IEC a owl:ObjectProperty, owl:FunctionalProperty ;
  rdfs:label "WindTurbineType3or4IEC"@en ;
  owl:inverseOf cim:WindTurbineType3or4IEC.WindContQLimIEC ;
  rdfs:domain cim:WindContQLimIEC ;
  rdfs:range cim:WindTurbineType3or4IEC ;
  skos:definition "Wind generator type 3 or type 4 model with which this constant Q limitation model is associated."@en .

cim:WindContQPQULimIEC.WindDynamicsLookupTable a owl:ObjectProperty ;
  rdfs:label "WindDynamicsLookupTable"@en ;
  owl:inverseOf cim:WindDynamicsLookupTable.WindContQPQULimIEC ;
  rdfs:domain cim:WindContQPQULimIEC ;
  rdfs:range cim:WindDynamicsLookupTable ;
  skos:definition "The wind dynamics lookup table associated with this QP and QU limitation model."@en .

cim:WindContQPQULimIEC.WindTurbineType3or4IEC a owl:ObjectProperty, owl:FunctionalProperty ;
  rdfs:label "WindTurbineType3or4IEC"@en ;
  owl:inverseOf cim:WindTurbineType3or4IEC.WindContQPQULimIEC ;
  rdfs:domain cim:WindContQPQULimIEC ;
  rdfs:range cim:WindTurbineType3or4IEC ;
  skos:definition "Wind generator type 3 or type 4 model with which this QP and QU limitation model is associated."@en .

cim:WindContRotorRIEC.WindDynamicsLookupTable a owl:ObjectProperty ;
  rdfs:label "WindDynamicsLookupTable"@en ;
  owl:inverseOf cim:WindDynamicsLookupTable.WindContRotorRIEC ;
  rdfs:domain cim:WindContRotorRIEC ;
  rdfs:range cim:WindDynamicsLookupTable ;
  skos:definition "The wind dynamics lookup table associated with this rotor resistance control model."@en .

cim:WindContRotorRIEC.WindGenTurbineType2IEC a owl:ObjectProperty ;
  rdfs:label "WindGenTurbineType2IEC"@en ;
  owl:inverseOf cim:WindGenTurbineType2IEC.WindContRotorRIEC ;
  rdfs:domain cim:WindContRotorRIEC ;
  rdfs:range cim:WindGenTurbineType2IEC ;
  skos:definition "Wind turbine type 2 model with whitch this wind control rotor resistance model is associated."@en .

cim:WindDynamicsLookupTable.WindContCurrLimIEC a owl:ObjectProperty, owl:FunctionalProperty ;
  rdfs:label "WindContCurrLimIEC"@en ;
  owl:inverseOf cim:WindContCurrLimIEC.WindDynamicsLookupTable ;
  rdfs:domain cim:WindDynamicsLookupTable ;
  rdfs:range cim:WindContCurrLimIEC ;
  skos:definition "The current control limitation model with which this wind dynamics lookup table is associated."@en .

cim:WindDynamicsLookupTable.WindContPType3IEC a owl:ObjectProperty, owl:FunctionalProperty ;
  rdfs:label "WindContPType3IEC"@en ;
  owl:inverseOf cim:WindContPType3IEC.WindDynamicsLookupTable ;
  rdfs:domain cim:WindDynamicsLookupTable ;
  rdfs:range cim:WindContPType3IEC ;
  skos:definition "The P control type 3 model with which this wind dynamics lookup table is associated."@en .

cim:WindDynamicsLookupTable.WindContQPQULimIEC a owl:ObjectProperty, owl:FunctionalProperty ;
  rdfs:label "WindContQPQULimIEC"@en ;
  owl:inverseOf cim:WindContQPQULimIEC.WindDynamicsLookupTable ;
  rdfs:domain cim:WindDynamicsLookupTable ;
  rdfs:range cim:WindContQPQULimIEC ;
  skos:definition "The QP and QU limitation model with which this wind dynamics lookup table is associated."@en .

cim:WindDynamicsLookupTable.WindContRotorRIEC a owl:ObjectProperty, owl:FunctionalProperty ;
  rdfs:label "WindContRotorRIEC"@en ;
  owl:inverseOf cim:WindContRotorRIEC.WindDynamicsLookupTable ;
  rdfs:domain cim:WindDynamicsLookupTable ;
  rdfs:range cim:WindContRotorRIEC ;
  skos:definition "The rotor resistance control model with which this wind dynamics lookup table is associated."@en .

cim:WindDynamicsLookupTable.WindGenType3bIEC a owl:ObjectProperty, owl:FunctionalProperty ;
  rdfs:label "WindGenType3bIEC"@en ;
  owl:inverseOf cim:WindGenType3bIEC.WindDynamicsLookupTable ;
  rdfs:domain cim:WindDynamicsLookupTable ;
  rdfs:range cim:WindGenType3bIEC ;
  skos:definition "The generator type 3B model with which this wind dynamics lookup table is associated."@en .

cim:WindDynamicsLookupTable.WindPitchContPowerIEC a owl:ObjectProperty, owl:FunctionalProperty ;
  rdfs:label "WindPitchContPowerIEC"@en ;
  owl:inverseOf cim:WindPitchContPowerIEC.WindDynamicsLookupTable ;
  rdfs:domain cim:WindDynamicsLookupTable ;
  rdfs:range cim:WindPitchContPowerIEC ;
  skos:definition "The pitch control power model with which this wind dynamics lookup table is associated."@en .

cim:WindDynamicsLookupTable.WindPlantFreqPcontrolIEC a owl:ObjectProperty, owl:FunctionalProperty ;
  rdfs:label "WindPlantFreqPcontrolIEC"@en ;
  owl:inverseOf cim:WindPlantFreqPcontrolIEC.WindDynamicsLookupTable ;
  rdfs:domain cim:WindDynamicsLookupTable ;
  rdfs:range cim:WindPlantFreqPcontrolIEC ;
  skos:definition "The frequency and active power wind plant control model with which this wind dynamics lookup table is associated."@en .

cim:WindDynamicsLookupTable.WindPlantReactiveControlIEC a owl:ObjectProperty, owl:FunctionalProperty ;
  rdfs:label "WindPlantReactiveControlIEC"@en ;
  owl:inverseOf cim:WindPlantReactiveControlIEC.WindDynamicsLookupTable ;
  rdfs:domain cim:WindDynamicsLookupTable ;
  rdfs:range cim:WindPlantReactiveControlIEC ;
  skos:definition "The voltage and reactive power wind plant control model with which this wind dynamics lookup table is associated."@en .

cim:WindDynamicsLookupTable.WindProtectionIEC a owl:ObjectProperty, owl:FunctionalProperty ;
  rdfs:label "WindProtectionIEC"@en ;
  owl:inverseOf cim:WindProtectionIEC.WindDynamicsLookupTable ;
  rdfs:domain cim:WindDynamicsLookupTable ;
  rdfs:range cim:WindProtectionIEC ;
  skos:definition "The grid protection model with which this wind dynamics lookup table is associated."@en .

cim:WindGenTurbineType1aIEC.WindAeroConstIEC a owl:ObjectProperty ;
  rdfs:label "WindAeroConstIEC"@en ;
  owl:inverseOf cim:WindAeroConstIEC.WindGenTurbineType1aIEC ;
  rdfs:domain cim:WindGenTurbineType1aIEC ;
  rdfs:range cim:WindAeroConstIEC ;
  skos:definition "Wind aerodynamic model associated with this wind turbine type 1A model."@en .

cim:WindGenTurbineType1bIEC.WindPitchContPowerIEC a owl:ObjectProperty ;
  rdfs:label "WindPitchContPowerIEC"@en ;
  owl:inverseOf cim:WindPitchContPowerIEC.WindGenTurbineType1bIEC ;
  rdfs:domain cim:WindGenTurbineType1bIEC ;
  rdfs:range cim:WindPitchContPowerIEC ;
  skos:definition "Pitch control power model associated with this wind turbine type 1B model."@en .

cim:WindGenTurbineType2IEC.WindContRotorRIEC a owl:ObjectProperty ;
  rdfs:label "WindContRotorRIEC"@en ;
  owl:inverseOf cim:WindContRotorRIEC.WindGenTurbineType2IEC ;
  rdfs:domain cim:WindGenTurbineType2IEC ;
  rdfs:range cim:WindContRotorRIEC ;
  skos:definition "Wind control rotor resistance model associated with wind turbine type 2 model."@en .

cim:WindGenTurbineType2IEC.WindPitchContPowerIEC a owl:ObjectProperty ;
  rdfs:label "WindPitchContPowerIEC"@en ;
  owl:inverseOf cim:WindPitchContPowerIEC.WindGenTurbineType2IEC ;
  rdfs:domain cim:WindGenTurbineType2IEC ;
  rdfs:range cim:WindPitchContPowerIEC ;
  skos:definition "Pitch control power model associated with this wind turbine type 2 model."@en .

cim:WindGenType3IEC.WindTurbineType3IEC a owl:ObjectProperty, owl:FunctionalProperty ;
  rdfs:label "WindTurbineType3IEC"@en ;
  owl:inverseOf cim:WindTurbineType3IEC.WindGenType3IEC ;
  rdfs:domain cim:WindGenType3IEC ;
  rdfs:range cim:WindTurbineType3IEC ;
  skos:definition "Wind turbine type 3 model with which this wind generator type 3 is associated. "@en .

cim:WindGenType3aIEC.WindTurbineType4IEC a owl:ObjectProperty, owl:FunctionalProperty ;
  rdfs:label "WindTurbineType4IEC"@en ;
  owl:inverseOf cim:WindTurbineType4IEC.WindGenType3aIEC ;
  rdfs:domain cim:WindGenType3aIEC ;
  rdfs:range cim:WindTurbineType4IEC ;
  skos:definition "Wind turbine type 4 model with which this wind generator type 3A model is associated."@en .

cim:WindGenType3bIEC.WindDynamicsLookupTable a owl:ObjectProperty ;
  rdfs:label "WindDynamicsLookupTable"@en ;
  owl:inverseOf cim:WindDynamicsLookupTable.WindGenType3bIEC ;
  rdfs:domain cim:WindGenType3bIEC ;
  rdfs:range cim:WindDynamicsLookupTable ;
  skos:definition "The wind dynamics lookup table associated with this generator type 3B model."@en .

cim:WindGenType4IEC.WindTurbineType4aIEC a owl:ObjectProperty, owl:FunctionalProperty ;
  rdfs:label "WindTurbineType4aIEC"@en ;
  owl:inverseOf cim:WindTurbineType4aIEC.WindGenType4IEC ;
  rdfs:domain cim:WindGenType4IEC ;
  rdfs:range cim:WindTurbineType4aIEC ;
  skos:definition "Wind turbine type 4A model with which this wind generator type 4 model is associated."@en .

cim:WindGenType4IEC.WindTurbineType4bIEC a owl:ObjectProperty, owl:FunctionalProperty ;
  rdfs:label "WindTurbineType4bIEC"@en ;
  owl:inverseOf cim:WindTurbineType4bIEC.WindGenType4IEC ;
  rdfs:domain cim:WindGenType4IEC ;
  rdfs:range cim:WindTurbineType4bIEC ;
  skos:definition "Wind turbine type 4B model with which this wind generator type 4 model is associated."@en .

cim:WindMechIEC.WindTurbineType1or2IEC a owl:ObjectProperty, owl:FunctionalProperty ;
  rdfs:label "WindTurbineType1or2IEC"@en ;
  owl:inverseOf cim:WindTurbineType1or2IEC.WindMechIEC ;
  rdfs:domain cim:WindMechIEC ;
  rdfs:range cim:WindTurbineType1or2IEC ;
  skos:definition "Wind generator type 1 or type 2 model with which this wind mechanical model is associated."@en .

cim:WindMechIEC.WindTurbineType3IEC a owl:ObjectProperty, owl:FunctionalProperty ;
  rdfs:label "WindTurbineType3IEC"@en ;
  owl:inverseOf cim:WindTurbineType3IEC.WindMechIEC ;
  rdfs:domain cim:WindMechIEC ;
  rdfs:range cim:WindTurbineType3IEC ;
  skos:definition "Wind turbine type 3 model with which this wind mechanical model is associated."@en .

cim:WindMechIEC.WindTurbineType4bIEC a owl:ObjectProperty, owl:FunctionalProperty ;
  rdfs:label "WindTurbineType4bIEC"@en ;
  owl:inverseOf cim:WindTurbineType4bIEC.WindMechIEC ;
  rdfs:domain cim:WindMechIEC ;
  rdfs:range cim:WindTurbineType4bIEC ;
  skos:definition "Wind turbine type 4B model with which this wind mechanical model is associated."@en .

cim:WindPitchContPowerIEC.WindDynamicsLookupTable a owl:ObjectProperty ;
  rdfs:label "WindDynamicsLookupTable"@en ;
  owl:inverseOf cim:WindDynamicsLookupTable.WindPitchContPowerIEC ;
  rdfs:domain cim:WindPitchContPowerIEC ;
  rdfs:range cim:WindDynamicsLookupTable ;
  skos:definition "The wind dynamics lookup table associated with this pitch control power model."@en .

cim:WindPitchContPowerIEC.WindGenTurbineType1bIEC a owl:ObjectProperty, owl:FunctionalProperty ;
  rdfs:label "WindGenTurbineType1bIEC"@en ;
  owl:inverseOf cim:WindGenTurbineType1bIEC.WindPitchContPowerIEC ;
  rdfs:domain cim:WindPitchContPowerIEC ;
  rdfs:range cim:WindGenTurbineType1bIEC ;
  skos:definition "Wind turbine type 1B model with which this pitch control power model is associated."@en .

cim:WindPitchContPowerIEC.WindGenTurbineType2IEC a owl:ObjectProperty, owl:FunctionalProperty ;
  rdfs:label "WindGenTurbineType2IEC"@en ;
  owl:inverseOf cim:WindGenTurbineType2IEC.WindPitchContPowerIEC ;
  rdfs:domain cim:WindPitchContPowerIEC ;
  rdfs:range cim:WindGenTurbineType2IEC ;
  skos:definition "Wind turbine type 2 model with which this pitch control power model is associated."@en .

cim:WindPlantDynamics.RemoteInputSignal a owl:ObjectProperty, owl:FunctionalProperty ;
  rdfs:label "RemoteInputSignal"@en ;
  owl:inverseOf cim:RemoteInputSignal.WindPlantDynamics ;
  rdfs:domain cim:WindPlantDynamics ;
  rdfs:range cim:RemoteInputSignal ;
  skos:definition "The remote signal with which this power plant is associated."@en .

cim:WindPlantDynamics.WindTurbineType3or4Dynamics a owl:ObjectProperty ;
  rdfs:label "WindTurbineType3or4Dynamics"@en ;
  owl:inverseOf cim:WindTurbineType3or4Dynamics.WindPlantDynamics ;
  rdfs:domain cim:WindPlantDynamics ;
  rdfs:range cim:WindTurbineType3or4Dynamics ;
  skos:definition "The wind turbine type 3 or type 4 associated with this wind plant."@en .

cim:WindPlantFreqPcontrolIEC.WindDynamicsLookupTable a owl:ObjectProperty ;
  rdfs:label "WindDynamicsLookupTable"@en ;
  owl:inverseOf cim:WindDynamicsLookupTable.WindPlantFreqPcontrolIEC ;
  rdfs:domain cim:WindPlantFreqPcontrolIEC ;
  rdfs:range cim:WindDynamicsLookupTable ;
  skos:definition "The wind dynamics lookup table associated with this frequency and active power wind plant model."@en .

cim:WindPlantFreqPcontrolIEC.WindPlantIEC a owl:ObjectProperty ;
  rdfs:label "WindPlantIEC"@en ;
  owl:inverseOf cim:WindPlantIEC.WindPlantFreqPcontrolIEC ;
  rdfs:domain cim:WindPlantFreqPcontrolIEC ;
  rdfs:range cim:WindPlantIEC ;
  skos:definition "Wind plant model with which this wind plant frequency and active power control is associated."@en .

cim:WindPlantIEC.WindPlantFreqPcontrolIEC a owl:ObjectProperty ;
  rdfs:label "WindPlantFreqPcontrolIEC"@en ;
  owl:inverseOf cim:WindPlantFreqPcontrolIEC.WindPlantIEC ;
  rdfs:domain cim:WindPlantIEC ;
  rdfs:range cim:WindPlantFreqPcontrolIEC ;
  skos:definition "Wind plant frequency and active power control model associated with this wind plant."@en .

cim:WindPlantIEC.WindPlantReactiveControlIEC a owl:ObjectProperty ;
  rdfs:label "WindPlantReactiveControlIEC"@en ;
  owl:inverseOf cim:WindPlantReactiveControlIEC.WindPlantIEC ;
  rdfs:domain cim:WindPlantIEC ;
  rdfs:range cim:WindPlantReactiveControlIEC ;
  skos:definition "Wind plant model with which this wind reactive control is associated."@en .

cim:WindPlantReactiveControlIEC.WindDynamicsLookupTable a owl:ObjectProperty ;
  rdfs:label "WindDynamicsLookupTable"@en ;
  owl:inverseOf cim:WindDynamicsLookupTable.WindPlantReactiveControlIEC ;
  rdfs:domain cim:WindPlantReactiveControlIEC ;
  rdfs:range cim:WindDynamicsLookupTable ;
  skos:definition "The wind dynamics lookup table associated with this voltage and reactive power wind plant model."@en .

cim:WindPlantReactiveControlIEC.WindPlantIEC a owl:ObjectProperty ;
  rdfs:label "WindPlantIEC"@en ;
  owl:inverseOf cim:WindPlantIEC.WindPlantReactiveControlIEC ;
  rdfs:domain cim:WindPlantReactiveControlIEC ;
  rdfs:range cim:WindPlantIEC ;
  skos:definition "Wind plant reactive control model associated with this wind plant."@en .

cim:WindPlantUserDefined.ProprietaryParameterDynamics a owl:ObjectProperty ;
  rdfs:label "ProprietaryParameterDynamics"@en ;
  owl:inverseOf cim:ProprietaryParameterDynamics.WindPlantUserDefined ;
  rdfs:domain cim:WindPlantUserDefined ;
  rdfs:range cim:ProprietaryParameterDynamics ;
  skos:definition "Parameter of this proprietary user-defined model."@en .

cim:WindProtectionIEC.WindDynamicsLookupTable a owl:ObjectProperty ;
  rdfs:label "WindDynamicsLookupTable"@en ;
  owl:inverseOf cim:WindDynamicsLookupTable.WindProtectionIEC ;
  rdfs:domain cim:WindProtectionIEC ;
  rdfs:range cim:WindDynamicsLookupTable ;
  skos:definition "The wind dynamics lookup table associated with this grid protection model."@en .

cim:WindProtectionIEC.WindTurbineType1or2IEC a owl:ObjectProperty, owl:FunctionalProperty ;
  rdfs:label "WindTurbineType1or2IEC"@en ;
  owl:inverseOf cim:WindTurbineType1or2IEC.WindProtectionIEC ;
  rdfs:domain cim:WindProtectionIEC ;
  rdfs:range cim:WindTurbineType1or2IEC ;
  skos:definition "Wind generator type 1 or type 2 model with which this wind turbine protection model is associated."@en .

cim:WindProtectionIEC.WindTurbineType3or4IEC a owl:ObjectProperty, owl:FunctionalProperty ;
  rdfs:label "WindTurbineType3or4IEC"@en ;
  owl:inverseOf cim:WindTurbineType3or4IEC.WindProtectionIEC ;
  rdfs:domain cim:WindProtectionIEC ;
  rdfs:range cim:WindTurbineType3or4IEC ;
  skos:definition "Wind generator type 3 or type 4 model with which this wind turbine protection model is associated."@en .

cim:WindRefFrameRotIEC.WindTurbineType3or4IEC a owl:ObjectProperty ;
  rdfs:label "WindTurbineType3or4IEC"@en ;
  owl:inverseOf cim:WindTurbineType3or4IEC.WindRefFrameRotIEC ;
  rdfs:domain cim:WindRefFrameRotIEC ;
  rdfs:range cim:WindTurbineType3or4IEC ;
  skos:definition "Wind turbine type 3 or type 4 model with which this reference frame rotation model is associated."@en .

cim:WindTurbineType1or2Dynamics.AsynchronousMachineDynamics a owl:ObjectProperty ;
  rdfs:label "AsynchronousMachineDynamics"@en ;
  owl:inverseOf cim:AsynchronousMachineDynamics.WindTurbineType1or2Dynamics ;
  rdfs:domain cim:WindTurbineType1or2Dynamics ;
  rdfs:range cim:AsynchronousMachineDynamics ;
  skos:definition "Asynchronous machine model with which this wind generator type 1 or type 2 model is associated."@en .

cim:WindTurbineType1or2Dynamics.RemoteInputSignal a owl:ObjectProperty, owl:FunctionalProperty ;
  rdfs:label "RemoteInputSignal"@en ;
  owl:inverseOf cim:RemoteInputSignal.WindTurbineType1or2Dynamics ;
  rdfs:domain cim:WindTurbineType1or2Dynamics ;
  rdfs:range cim:RemoteInputSignal ;
  skos:definition "Remote input signal used by this wind generator type 1 or type 2 model."@en .

cim:WindTurbineType1or2IEC.WindMechIEC a owl:ObjectProperty ;
  rdfs:label "WindMechIEC"@en ;
  owl:inverseOf cim:WindMechIEC.WindTurbineType1or2IEC ;
  rdfs:domain cim:WindTurbineType1or2IEC ;
  rdfs:range cim:WindMechIEC ;
  skos:definition "Wind mechanical model associated with this wind generator type 1 or type 2 model."@en .

cim:WindTurbineType1or2IEC.WindProtectionIEC a owl:ObjectProperty ;
  rdfs:label "WindProtectionIEC"@en ;
  owl:inverseOf cim:WindProtectionIEC.WindTurbineType1or2IEC ;
  rdfs:domain cim:WindTurbineType1or2IEC ;
  rdfs:range cim:WindProtectionIEC ;
  skos:definition "Wind turbune protection model associated with this wind generator type 1 or type 2 model."@en .

cim:WindTurbineType3IEC.WindAeroOneDimIEC a owl:ObjectProperty, owl:FunctionalProperty ;
  rdfs:label "WindAeroOneDimIEC"@en ;
  owl:inverseOf cim:WindAeroOneDimIEC.WindTurbineType3IEC ;
  rdfs:domain cim:WindTurbineType3IEC ;
  rdfs:range cim:WindAeroOneDimIEC ;
  skos:definition "Wind aerodynamic model associated with this wind generator type 3 model."@en .

cim:WindTurbineType3IEC.WindAeroTwoDimIEC a owl:ObjectProperty, owl:FunctionalProperty ;
  rdfs:label "WindAeroTwoDimIEC"@en ;
  owl:inverseOf cim:WindAeroTwoDimIEC.WindTurbineType3IEC ;
  rdfs:domain cim:WindTurbineType3IEC ;
  rdfs:range cim:WindAeroTwoDimIEC ;
  skos:definition "Wind aerodynamic model associated with this wind turbine type 3 model."@en .

cim:WindTurbineType3IEC.WindContPType3IEC a owl:ObjectProperty ;
  rdfs:label "WindContPType3IEC"@en ;
  owl:inverseOf cim:WindContPType3IEC.WindTurbineType3IEC ;
  rdfs:domain cim:WindTurbineType3IEC ;
  rdfs:range cim:WindContPType3IEC ;
  skos:definition "Wind control P type 3 model associated with this wind turbine type 3 model."@en .

cim:WindTurbineType3IEC.WindContPitchAngleIEC a owl:ObjectProperty ;
  rdfs:label "WindContPitchAngleIEC"@en ;
  owl:inverseOf cim:WindContPitchAngleIEC.WindTurbineType3IEC ;
  rdfs:domain cim:WindTurbineType3IEC ;
  rdfs:range cim:WindContPitchAngleIEC ;
  skos:definition "Wind control pitch angle model associated with this wind turbine type 3."@en .

cim:WindTurbineType3IEC.WindGenType3IEC a owl:ObjectProperty, owl:FunctionalProperty ;
  rdfs:label "WindGenType3IEC"@en ;
  owl:inverseOf cim:WindGenType3IEC.WindTurbineType3IEC ;
  rdfs:domain cim:WindTurbineType3IEC ;
  rdfs:range cim:WindGenType3IEC ;
  skos:definition "Wind generator type 3 model associated with this wind turbine type 3 model."@en .

cim:WindTurbineType3IEC.WindMechIEC a owl:ObjectProperty ;
  rdfs:label "WindMechIEC"@en ;
  owl:inverseOf cim:WindMechIEC.WindTurbineType3IEC ;
  rdfs:domain cim:WindTurbineType3IEC ;
  rdfs:range cim:WindMechIEC ;
  skos:definition "Wind mechanical model associated with this wind turbine type 3 model."@en .

cim:WindTurbineType3or4Dynamics.PowerElectronicsConnection a owl:ObjectProperty ;
  rdfs:label "PowerElectronicsConnection"@en ;
  owl:inverseOf cim:PowerElectronicsConnection.WindTurbineType3or4Dynamics ;
  rdfs:domain cim:WindTurbineType3or4Dynamics ;
  rdfs:range cim:PowerElectronicsConnection ;
  skos:definition "The power electronics connection associated with this wind turbine type 3 or type 4 dynamics model."@en .

cim:WindTurbineType3or4Dynamics.RemoteInputSignal a owl:ObjectProperty, owl:FunctionalProperty ;
  rdfs:label "RemoteInputSignal"@en ;
  owl:inverseOf cim:RemoteInputSignal.WindTurbineType3or4Dynamics ;
  rdfs:domain cim:WindTurbineType3or4Dynamics ;
  rdfs:range cim:RemoteInputSignal ;
  skos:definition "Remote input signal used by these wind turbine type 3 or type 4 models."@en .

cim:WindTurbineType3or4Dynamics.WindPlantDynamics a owl:ObjectProperty, owl:FunctionalProperty ;
  rdfs:label "WindPlantDynamics"@en ;
  owl:inverseOf cim:WindPlantDynamics.WindTurbineType3or4Dynamics ;
  rdfs:domain cim:WindTurbineType3or4Dynamics ;
  rdfs:range cim:WindPlantDynamics ;
  skos:definition "The wind plant with which the wind turbines type 3 or type 4 are associated."@en .

cim:WindTurbineType3or4IEC.WIndContQIEC a owl:ObjectProperty ;
  rdfs:label "WIndContQIEC"@en ;
  owl:inverseOf cim:WindContQIEC.WindTurbineType3or4IEC ;
  rdfs:domain cim:WindTurbineType3or4IEC ;
  rdfs:range cim:WindContQIEC ;
  skos:definition "Wind control Q model associated with this wind turbine type 3 or type 4 model."@en .

cim:WindTurbineType3or4IEC.WindContCurrLimIEC a owl:ObjectProperty ;
  rdfs:label "WindContCurrLimIEC"@en ;
  owl:inverseOf cim:WindContCurrLimIEC.WindTurbineType3or4IEC ;
  rdfs:domain cim:WindTurbineType3or4IEC ;
  rdfs:range cim:WindContCurrLimIEC ;
  skos:definition "Wind control current limitation model associated with this wind turbine type 3 or type 4 model."@en .

cim:WindTurbineType3or4IEC.WindContQLimIEC a owl:ObjectProperty, owl:FunctionalProperty ;
  rdfs:label "WindContQLimIEC"@en ;
  owl:inverseOf cim:WindContQLimIEC.WindTurbineType3or4IEC ;
  rdfs:domain cim:WindTurbineType3or4IEC ;
  rdfs:range cim:WindContQLimIEC ;
  skos:definition "Constant Q limitation model associated with this wind generator type 3 or type 4 model."@en .

cim:WindTurbineType3or4IEC.WindContQPQULimIEC a owl:ObjectProperty, owl:FunctionalProperty ;
  rdfs:label "WindContQPQULimIEC"@en ;
  owl:inverseOf cim:WindContQPQULimIEC.WindTurbineType3or4IEC ;
  rdfs:domain cim:WindTurbineType3or4IEC ;
  rdfs:range cim:WindContQPQULimIEC ;
  skos:definition "QP and QU limitation model associated with this wind generator type 3 or type 4 model."@en .

cim:WindTurbineType3or4IEC.WindProtectionIEC a owl:ObjectProperty ;
  rdfs:label "WindProtectionIEC"@en ;
  owl:inverseOf cim:WindProtectionIEC.WindTurbineType3or4IEC ;
  rdfs:domain cim:WindTurbineType3or4IEC ;
  rdfs:range cim:WindProtectionIEC ;
  skos:definition "Wind turbune protection model associated with this wind generator type 3 or type 4 model."@en .

cim:WindTurbineType3or4IEC.WindRefFrameRotIEC a owl:ObjectProperty ;
  rdfs:label "WindRefFrameRotIEC"@en ;
  owl:inverseOf cim:WindRefFrameRotIEC.WindTurbineType3or4IEC ;
  rdfs:domain cim:WindTurbineType3or4IEC ;
  rdfs:range cim:WindRefFrameRotIEC ;
  skos:definition "Reference frame rotation model associated with this wind turbine type 3 or type 4 model."@en .

cim:WindTurbineType4IEC.WindGenType3aIEC a owl:ObjectProperty, owl:FunctionalProperty ;
  rdfs:label "WindGenType3aIEC"@en ;
  owl:inverseOf cim:WindGenType3aIEC.WindTurbineType4IEC ;
  rdfs:domain cim:WindTurbineType4IEC ;
  rdfs:range cim:WindGenType3aIEC ;
  skos:definition "Wind generator type 3A model associated with this wind turbine type 4 model."@en .

cim:WindTurbineType4aIEC.WindContPType4aIEC a owl:ObjectProperty ;
  rdfs:label "WindContPType4aIEC"@en ;
  owl:inverseOf cim:WindContPType4aIEC.WindTurbineType4aIEC ;
  rdfs:domain cim:WindTurbineType4aIEC ;
  rdfs:range cim:WindContPType4aIEC ;
  skos:definition "Wind control P type 4A model associated with this wind turbine type 4A model."@en .

cim:WindTurbineType4aIEC.WindGenType4IEC a owl:ObjectProperty, owl:FunctionalProperty ;
  rdfs:label "WindGenType4IEC"@en ;
  owl:inverseOf cim:WindGenType4IEC.WindTurbineType4aIEC ;
  rdfs:domain cim:WindTurbineType4aIEC ;
  rdfs:range cim:WindGenType4IEC ;
  skos:definition "Wind generator type 4 model associated with this wind turbine type 4A model."@en .

cim:WindTurbineType4bIEC.WindContPType4bIEC a owl:ObjectProperty ;
  rdfs:label "WindContPType4bIEC"@en ;
  owl:inverseOf cim:WindContPType4bIEC.WindTurbineType4bIEC ;
  rdfs:domain cim:WindTurbineType4bIEC ;
  rdfs:range cim:WindContPType4bIEC ;
  skos:definition "Wind control P type 4B model associated with this wind turbine type 4B model."@en .

cim:WindTurbineType4bIEC.WindGenType4IEC a owl:ObjectProperty, owl:FunctionalProperty ;
  rdfs:label "WindGenType4IEC"@en ;
  owl:inverseOf cim:WindGenType4IEC.WindTurbineType4bIEC ;
  rdfs:domain cim:WindTurbineType4bIEC ;
  rdfs:range cim:WindGenType4IEC ;
  skos:definition "Wind generator type 4 model associated with this wind turbine type 4B model."@en .

cim:WindTurbineType4bIEC.WindMechIEC a owl:ObjectProperty ;
  rdfs:label "WindMechIEC"@en ;
  owl:inverseOf cim:WindMechIEC.WindTurbineType4bIEC ;
  rdfs:domain cim:WindTurbineType4bIEC ;
  rdfs:range cim:WindMechIEC ;
  skos:definition "Wind mechanical model associated with this wind turbine type 4B model."@en .

cim:WindType1or2UserDefined.ProprietaryParameterDynamics a owl:ObjectProperty ;
  rdfs:label "ProprietaryParameterDynamics"@en ;
  owl:inverseOf cim:ProprietaryParameterDynamics.WindType1or2UserDefined ;
  rdfs:domain cim:WindType1or2UserDefined ;
  rdfs:range cim:ProprietaryParameterDynamics ;
  skos:definition "Parameter of this proprietary user-defined model."@en .

cim:WindType3or4UserDefined.ProprietaryParameterDynamics a owl:ObjectProperty ;
  rdfs:label "ProprietaryParameterDynamics"@en ;
  owl:inverseOf cim:ProprietaryParameterDynamics.WindType3or4UserDefined ;
  rdfs:domain cim:WindType3or4UserDefined ;
  rdfs:range cim:ProprietaryParameterDynamics ;
  skos:definition "Parameter of this proprietary user-defined model."@en .

cim:ActivePower.multiplier a owl:DatatypeProperty, owl:FunctionalProperty ;
  rdfs:label "multiplier"@en ;
  dy:isFixed "True " ;
  rdf:value "M" ;
  rdfs:domain cim:ActivePower ;
  rdfs:range cim:UnitMultiplier .

cim:ActivePower.unit a owl:DatatypeProperty, owl:FunctionalProperty ;
  rdfs:label "unit"@en ;
  dy:isFixed "True " ;
  rdf:value "W" ;
  rdfs:domain cim:ActivePower ;
  rdfs:range cim:UnitSymbol .

cim:ActivePower.value a owl:DatatypeProperty, owl:FunctionalProperty ;
  rdfs:label "value"@en ;
  rdfs:domain cim:ActivePower ;
  rdfs:range xsd:float .

cim:AngleDegrees.multiplier a owl:DatatypeProperty, owl:FunctionalProperty ;
  rdfs:label "multiplier"@en ;
  dy:isFixed "True " ;
  rdf:value "none" ;
  rdfs:domain cim:AngleDegrees ;
  rdfs:range cim:UnitMultiplier .

cim:AngleDegrees.unit a owl:DatatypeProperty, owl:FunctionalProperty ;
  rdfs:label "unit"@en ;
  dy:isFixed "True " ;
  rdf:value "deg" ;
  rdfs:domain cim:AngleDegrees ;
  rdfs:range cim:UnitSymbol .

cim:AngleDegrees.value a owl:DatatypeProperty, owl:FunctionalProperty ;
  rdfs:label "value"@en ;
  rdfs:domain cim:AngleDegrees ;
  rdfs:range xsd:float .

cim:ApparentPower.multiplier a owl:DatatypeProperty, owl:FunctionalProperty ;
  rdfs:label "multiplier"@en ;
  dy:isFixed "True " ;
  rdf:value "M" ;
  rdfs:domain cim:ApparentPower ;
  rdfs:range cim:UnitMultiplier .

cim:ApparentPower.unit a owl:DatatypeProperty, owl:FunctionalProperty ;
  rdfs:label "unit"@en ;
  dy:isFixed "True " ;
  rdf:value "VA" ;
  rdfs:domain cim:ApparentPower ;
  rdfs:range cim:UnitSymbol .

cim:ApparentPower.value a owl:DatatypeProperty, owl:FunctionalProperty ;
  rdfs:label "value"@en ;
  rdfs:domain cim:ApparentPower ;
  rdfs:range xsd:float .

cim:Area.multiplier a owl:DatatypeProperty, owl:FunctionalProperty ;
  rdfs:label "multiplier"@en ;
  dy:isFixed "True " ;
  rdf:value "none" ;
  rdfs:domain cim:Area ;
  rdfs:range cim:UnitMultiplier .

cim:Area.unit a owl:DatatypeProperty, owl:FunctionalProperty ;
  rdfs:label "unit"@en ;
  dy:isFixed "True " ;
  rdf:value "m2" ;
  rdfs:domain cim:Area ;
  rdfs:range cim:UnitSymbol .

cim:Area.value a owl:DatatypeProperty, owl:FunctionalProperty ;
  rdfs:label "value"@en ;
  rdfs:domain cim:Area ;
  rdfs:range xsd:float .

cim:AsynchronousMachineEquivalentCircuit.rr1 a owl:DatatypeProperty ;
  rdfs:label "rr1"@en ;
  rdfs:domain cim:AsynchronousMachineEquivalentCircuit ;
  rdfs:range cim:PU ;
  skos:definition "Damper 1 winding resistance."@en .

cim:AsynchronousMachineEquivalentCircuit.rr2 a owl:DatatypeProperty ;
  rdfs:label "rr2"@en ;
  rdfs:domain cim:AsynchronousMachineEquivalentCircuit ;
  rdfs:range cim:PU ;
  skos:definition "Damper 2 winding resistance."@en .

cim:AsynchronousMachineEquivalentCircuit.xlr1 a owl:DatatypeProperty ;
  rdfs:label "xlr1"@en ;
  rdfs:domain cim:AsynchronousMachineEquivalentCircuit ;
  rdfs:range cim:PU ;
  skos:definition "Damper 1 winding leakage reactance."@en .

cim:AsynchronousMachineEquivalentCircuit.xlr2 a owl:DatatypeProperty ;
  rdfs:label "xlr2"@en ;
  rdfs:domain cim:AsynchronousMachineEquivalentCircuit ;
  rdfs:range cim:PU ;
  skos:definition "Damper 2 winding leakage reactance."@en .

cim:AsynchronousMachineEquivalentCircuit.xm a owl:DatatypeProperty ;
  rdfs:label "xm"@en ;
  rdfs:domain cim:AsynchronousMachineEquivalentCircuit ;
  rdfs:range cim:PU ;
  skos:definition "Magnetizing reactance."@en .

cim:AsynchronousMachineTimeConstantReactance.tpo a owl:DatatypeProperty ;
  rdfs:label "tpo"@en ;
  rdfs:domain cim:AsynchronousMachineTimeConstantReactance ;
  rdfs:range cim:Seconds ;
  skos:definition "Transient rotor time constant (<i>T'o</i>) (&gt; AsynchronousMachineTimeConstantReactance.tppo).  Typical value = 5."@en .

cim:AsynchronousMachineTimeConstantReactance.tppo a owl:DatatypeProperty ;
  rdfs:label "tppo"@en ;
  rdfs:domain cim:AsynchronousMachineTimeConstantReactance ;
  rdfs:range cim:Seconds ;
  skos:definition "Subtransient rotor time constant (<i>T''o</i>) (&gt; 0).  Typical value = 0,03."@en .

cim:AsynchronousMachineTimeConstantReactance.xp a owl:DatatypeProperty ;
  rdfs:label "xp"@en ;
  rdfs:domain cim:AsynchronousMachineTimeConstantReactance ;
  rdfs:range cim:PU ;
  skos:definition "Transient reactance (unsaturated) (<i>X'</i>) (&gt;= AsynchronousMachineTimeConstantReactance.xpp).  Typical value = 0,5."@en .

cim:AsynchronousMachineTimeConstantReactance.xpp a owl:DatatypeProperty ;
  rdfs:label "xpp"@en ;
  rdfs:domain cim:AsynchronousMachineTimeConstantReactance ;
  rdfs:range cim:PU ;
  skos:definition "Subtransient reactance (unsaturated) (<i>X''</i>) (&gt; RotatingMachineDynamics.statorLeakageReactance).  Typical value = 0,2."@en .

cim:AsynchronousMachineTimeConstantReactance.xs a owl:DatatypeProperty ;
  rdfs:label "xs"@en ;
  rdfs:domain cim:AsynchronousMachineTimeConstantReactance ;
  rdfs:range cim:PU ;
  skos:definition "Synchronous reactance (<i>Xs</i>) (&gt;= AsynchronousMachineTimeConstantReactance.xp).  Typical value = 1,8."@en .

cim:AsynchronousMachineUserDefined.proprietary a owl:DatatypeProperty ;
  rdfs:label "proprietary"@en ;
  rdfs:domain cim:AsynchronousMachineUserDefined ;
  rdfs:range xsd:boolean ;
  skos:definition """
Behaviour is based on a proprietary model as opposed to a detailed model.
true = user-defined model is proprietary with behaviour mutually understood by sending and receiving applications and parameters passed as general attributes
false = user-defined model is explicitly defined in terms of control blocks and their input and output signals.
\t"""@en .

cim:CSCUserDefined.proprietary a owl:DatatypeProperty ;
  rdfs:label "proprietary"@en ;
  rdfs:domain cim:CSCUserDefined ;
  rdfs:range xsd:boolean ;
  skos:definition """
Behaviour is based on a proprietary model as opposed to a detailed model.
true = user-defined model is proprietary with behaviour mutually understood by sending and receiving applications and parameters passed as general attributes
false = user-defined model is explicitly defined in terms of control blocks and their input and output signals.
\t"""@en .

cim:DiscExcContIEEEDEC1A.esc a owl:DatatypeProperty ;
  rdfs:label "esc"@en ;
  rdfs:domain cim:DiscExcContIEEEDEC1A ;
  rdfs:range cim:PU ;
  skos:definition "Speed change reference (<i>E</i><i><sub>SC</sub></i>).  Typical value = 0,0015."@en .

cim:DiscExcContIEEEDEC1A.kan a owl:DatatypeProperty ;
  rdfs:label "kan"@en ;
  rdfs:domain cim:DiscExcContIEEEDEC1A ;
  rdfs:range cim:PU ;
  skos:definition "Discontinuous controller gain (<i>K</i><i><sub>AN</sub></i>).  Typical value = 400."@en .

cim:DiscExcContIEEEDEC1A.ketl a owl:DatatypeProperty ;
  rdfs:label "ketl"@en ;
  rdfs:domain cim:DiscExcContIEEEDEC1A ;
  rdfs:range cim:PU ;
  skos:definition "Terminal voltage limiter gain (<i>K</i><i><sub>ETL</sub></i>).  Typical value = 47."@en .

cim:DiscExcContIEEEDEC1A.tan a owl:DatatypeProperty ;
  rdfs:label "tan"@en ;
  rdfs:domain cim:DiscExcContIEEEDEC1A ;
  rdfs:range cim:Seconds ;
  skos:definition "Discontinuous controller time constant (<i>T</i><i><sub>AN</sub></i>) (&gt;= 0).  Typical value = 0,08."@en .

cim:DiscExcContIEEEDEC1A.td a owl:DatatypeProperty ;
  rdfs:label "td"@en ;
  rdfs:domain cim:DiscExcContIEEEDEC1A ;
  rdfs:range cim:Seconds ;
  skos:definition "Time constant (<i>T</i><i><sub>D</sub></i>) (&gt;= 0).  Typical value = 0,03."@en .

cim:DiscExcContIEEEDEC1A.tl1 a owl:DatatypeProperty ;
  rdfs:label "tl1"@en ;
  rdfs:domain cim:DiscExcContIEEEDEC1A ;
  rdfs:range cim:Seconds ;
  skos:definition "Time constant (<i>T</i><i><sub>L</sub></i><sub>1</sub>) (&gt;= 0).  Typical value = 0,025."@en .

cim:DiscExcContIEEEDEC1A.tl2 a owl:DatatypeProperty ;
  rdfs:label "tl2"@en ;
  rdfs:domain cim:DiscExcContIEEEDEC1A ;
  rdfs:range cim:Seconds ;
  skos:definition "Time constant (<i>T</i><i><sub>L</sub></i><sub>2</sub>) (&gt;= 0).  Typical value = 1,25."@en .

cim:DiscExcContIEEEDEC1A.tw5 a owl:DatatypeProperty ;
  rdfs:label "tw5"@en ;
  rdfs:domain cim:DiscExcContIEEEDEC1A ;
  rdfs:range cim:Seconds ;
  skos:definition "DEC washout time constant (<i>T</i><i><sub>W</sub></i><sub>5</sub>) (&gt;= 0).  Typical value = 5."@en .

cim:DiscExcContIEEEDEC1A.val a owl:DatatypeProperty ;
  rdfs:label "val"@en ;
  rdfs:domain cim:DiscExcContIEEEDEC1A ;
  rdfs:range cim:PU ;
  skos:definition "Regulator voltage reference (<i>V</i><i><sub>AL</sub></i>).  Typical value = 5,5."@en .

cim:DiscExcContIEEEDEC1A.vanmax a owl:DatatypeProperty ;
  rdfs:label "vanmax"@en ;
  rdfs:domain cim:DiscExcContIEEEDEC1A ;
  rdfs:range cim:PU ;
  skos:definition "Limiter for Van (<i>V</i><i><sub>ANMAX</sub></i>)."@en .

cim:DiscExcContIEEEDEC1A.vomax a owl:DatatypeProperty ;
  rdfs:label "vomax"@en ;
  rdfs:domain cim:DiscExcContIEEEDEC1A ;
  rdfs:range cim:PU ;
  skos:definition "Limiter (<i>V</i><i><sub>OMAX</sub></i>) (&gt; DiscExcContIEEEDEC1A.vomin).  Typical value = 0,3."@en .

cim:DiscExcContIEEEDEC1A.vomin a owl:DatatypeProperty ;
  rdfs:label "vomin"@en ;
  rdfs:domain cim:DiscExcContIEEEDEC1A ;
  rdfs:range cim:PU ;
  skos:definition "Limiter (<i>V</i><i><sub>OMIN</sub></i>) (&lt; DiscExcContIEEEDEC1A.vomax).  Typical value = 0,1."@en .

cim:DiscExcContIEEEDEC1A.vsmax a owl:DatatypeProperty ;
  rdfs:label "vsmax"@en ;
  rdfs:domain cim:DiscExcContIEEEDEC1A ;
  rdfs:range cim:PU ;
  skos:definition "Limiter (<i>V</i><i><sub>SMAX</sub></i>)(&gt; DiscExcContIEEEDEC1A.vsmin).  Typical value = 0,2."@en .

cim:DiscExcContIEEEDEC1A.vsmin a owl:DatatypeProperty ;
  rdfs:label "vsmin"@en ;
  rdfs:domain cim:DiscExcContIEEEDEC1A ;
  rdfs:range cim:PU ;
  skos:definition "Limiter (<i>V</i><i><sub>SMIN</sub></i>) (&lt; DiscExcContIEEEDEC1A.vsmax).  Typical value = -0,066."@en .

cim:DiscExcContIEEEDEC1A.vtc a owl:DatatypeProperty ;
  rdfs:label "vtc"@en ;
  rdfs:domain cim:DiscExcContIEEEDEC1A ;
  rdfs:range cim:PU ;
  skos:definition "Terminal voltage level reference (<i>V</i><i><sub>TC</sub></i>).  Typical value = 0,95."@en .

cim:DiscExcContIEEEDEC1A.vtlmt a owl:DatatypeProperty ;
  rdfs:label "vtlmt"@en ;
  rdfs:domain cim:DiscExcContIEEEDEC1A ;
  rdfs:range cim:PU ;
  skos:definition "Voltage reference (<i>V</i><i><sub>TLMT</sub></i>).  Typical value = 1,1."@en .

cim:DiscExcContIEEEDEC1A.vtm a owl:DatatypeProperty ;
  rdfs:label "vtm"@en ;
  rdfs:domain cim:DiscExcContIEEEDEC1A ;
  rdfs:range cim:PU ;
  skos:definition "Voltage limits (<i>V</i><i><sub>TM</sub></i>).  Typical value = 1,13."@en .

cim:DiscExcContIEEEDEC1A.vtn a owl:DatatypeProperty ;
  rdfs:label "vtn"@en ;
  rdfs:domain cim:DiscExcContIEEEDEC1A ;
  rdfs:range cim:PU ;
  skos:definition "Voltage limits (<i>V</i><i><sub>TN</sub></i>).  Typical value = 1,12."@en .

cim:DiscExcContIEEEDEC2A.td1 a owl:DatatypeProperty ;
  rdfs:label "td1"@en ;
  rdfs:domain cim:DiscExcContIEEEDEC2A ;
  rdfs:range cim:Seconds ;
  skos:definition "Discontinuous controller time constant (<i>T</i><i><sub>D1</sub></i>) (&gt;= 0). "@en .

cim:DiscExcContIEEEDEC2A.td2 a owl:DatatypeProperty ;
  rdfs:label "td2"@en ;
  rdfs:domain cim:DiscExcContIEEEDEC2A ;
  rdfs:range cim:Seconds ;
  skos:definition "Discontinuous controller washout time constant (<i>T</i><i><sub>D2</sub></i>) (&gt;= 0). "@en .

cim:DiscExcContIEEEDEC2A.vdmax a owl:DatatypeProperty ;
  rdfs:label "vdmax"@en ;
  rdfs:domain cim:DiscExcContIEEEDEC2A ;
  rdfs:range cim:PU ;
  skos:definition "Limiter (<i>V</i><i><sub>DMAX</sub></i>) (&gt; DiscExcContIEEEDEC2A.vdmin). "@en .

cim:DiscExcContIEEEDEC2A.vdmin a owl:DatatypeProperty ;
  rdfs:label "vdmin"@en ;
  rdfs:domain cim:DiscExcContIEEEDEC2A ;
  rdfs:range cim:PU ;
  skos:definition "Limiter (<i>V</i><i><sub>DMIN</sub></i>) (&lt; DiscExcContIEEEDEC2A.vdmax). "@en .

cim:DiscExcContIEEEDEC2A.vk a owl:DatatypeProperty ;
  rdfs:label "vk"@en ;
  rdfs:domain cim:DiscExcContIEEEDEC2A ;
  rdfs:range cim:PU ;
  skos:definition "Discontinuous controller input reference (<i>V</i><i><sub>K</sub></i>). "@en .

cim:DiscExcContIEEEDEC3A.tdr a owl:DatatypeProperty ;
  rdfs:label "tdr"@en ;
  rdfs:domain cim:DiscExcContIEEEDEC3A ;
  rdfs:range cim:Seconds ;
  skos:definition "Reset time delay (<i>T</i><i><sub>DR</sub></i>) (&gt;= 0). "@en .

cim:DiscExcContIEEEDEC3A.vtmin a owl:DatatypeProperty ;
  rdfs:label "vtmin"@en ;
  rdfs:domain cim:DiscExcContIEEEDEC3A ;
  rdfs:range cim:PU ;
  skos:definition "Terminal undervoltage comparison level (<i>V</i><i><sub>TMIN</sub></i>). "@en .

cim:DiscontinuousExcitationControlUserDefined.proprietary a owl:DatatypeProperty ;
  rdfs:label "proprietary"@en ;
  rdfs:domain cim:DiscontinuousExcitationControlUserDefined ;
  rdfs:range xsd:boolean ;
  skos:definition """
Behaviour is based on a proprietary model as opposed to a detailed model.
true = user-defined model is proprietary with behaviour mutually understood by sending and receiving applications and parameters passed as general attributes
false = user-defined model is explicitly defined in terms of control blocks and their input and output signals.
\t"""@en .

cim:DynamicsFunctionBlock.enabled a owl:DatatypeProperty ;
  rdfs:label "enabled"@en ;
  rdfs:domain cim:DynamicsFunctionBlock ;
  rdfs:range xsd:boolean ;
  skos:definition """
Function block used indicator.
true = use of function block is enabled
false = use of function block is disabled.
\t"""@en .

cim:ExcAC1A.hvlvgates a owl:DatatypeProperty ;
  rdfs:label "hvlvgates"@en ;
  rdfs:domain cim:ExcAC1A ;
  rdfs:range xsd:boolean ;
  skos:definition """
Indicates if both HV gate and LV gate are active (<i>HVLVgates</i>).
true = gates are used
false = gates are not used.
Typical value = true.
\t"""@en .

cim:ExcAC1A.ka a owl:DatatypeProperty ;
  rdfs:label "ka"@en ;
  rdfs:domain cim:ExcAC1A ;
  rdfs:range cim:PU ;
  skos:definition "Voltage regulator gain (<i>Ka</i>) (&gt; 0).  Typical value = 400."@en .

cim:ExcAC1A.kc a owl:DatatypeProperty ;
  rdfs:label "kc"@en ;
  rdfs:domain cim:ExcAC1A ;
  rdfs:range cim:PU ;
  skos:definition "Rectifier loading factor proportional to commutating reactance (<i>Kc</i>) (&gt;= 0). Typical value = 0,2."@en .

cim:ExcAC1A.kd a owl:DatatypeProperty ;
  rdfs:label "kd"@en ;
  rdfs:domain cim:ExcAC1A ;
  rdfs:range cim:PU ;
  skos:definition "Demagnetizing factor, a function of exciter alternator reactances (<i>Kd</i>) (&gt;= 0).  Typical value = 0,38."@en .

cim:ExcAC1A.ke a owl:DatatypeProperty ;
  rdfs:label "ke"@en ;
  rdfs:domain cim:ExcAC1A ;
  rdfs:range cim:PU ;
  skos:definition "Exciter constant related to self-excited field (<i>Ke</i>).  Typical value = 1."@en .

cim:ExcAC1A.kf a owl:DatatypeProperty ;
  rdfs:label "kf"@en ;
  rdfs:domain cim:ExcAC1A ;
  rdfs:range cim:PU ;
  skos:definition "Excitation control system stabilizer gains (<i>Kf</i>) (&gt;= 0).  Typical value = 0,03."@en .

cim:ExcAC1A.kf1 a owl:DatatypeProperty ;
  rdfs:label "kf1"@en ;
  rdfs:domain cim:ExcAC1A ;
  rdfs:range cim:PU ;
  skos:definition "Coefficient to allow different usage of the model (<i>Kf1</i>) (&gt;= 0).  Typical value = 0."@en .

cim:ExcAC1A.kf2 a owl:DatatypeProperty ;
  rdfs:label "kf2"@en ;
  rdfs:domain cim:ExcAC1A ;
  rdfs:range cim:PU ;
  skos:definition "Coefficient to allow different usage of the model (<i>Kf2</i>) (&gt;= 0).  Typical value = 1."@en .

cim:ExcAC1A.ks a owl:DatatypeProperty ;
  rdfs:label "ks"@en ;
  rdfs:domain cim:ExcAC1A ;
  rdfs:range cim:PU ;
  skos:definition "Coefficient to allow different usage of the model-speed coefficient (<i>Ks</i>) (&gt;= 0).  Typical value = 0."@en .

cim:ExcAC1A.seve1 a owl:DatatypeProperty ;
  rdfs:label "seve1"@en ;
  rdfs:domain cim:ExcAC1A ;
  rdfs:range xsd:float ;
  skos:definition "Exciter saturation function value at the corresponding exciter voltage, <i>Ve</i><i><sub>1</sub></i>, back of commutating reactance (<i>Se[Ve</i><i><sub>1</sub></i><i>]</i>) (&gt;= 0).  Typical value = 0,1."@en .

cim:ExcAC1A.seve2 a owl:DatatypeProperty ;
  rdfs:label "seve2"@en ;
  rdfs:domain cim:ExcAC1A ;
  rdfs:range xsd:float ;
  skos:definition "Exciter saturation function value at the corresponding exciter voltage, <i>Ve</i><i><sub>2</sub></i>, back of commutating reactance (<i>Se[Ve</i><i><sub>2</sub></i><i>]</i>) (&gt;= 0).  Typical value = 0,03."@en .

cim:ExcAC1A.ta a owl:DatatypeProperty ;
  rdfs:label "ta"@en ;
  rdfs:domain cim:ExcAC1A ;
  rdfs:range cim:Seconds ;
  skos:definition "Voltage regulator time constant (<i>Ta</i>) (&gt; 0).  Typical value = 0,02."@en .

cim:ExcAC1A.tb a owl:DatatypeProperty ;
  rdfs:label "tb"@en ;
  rdfs:domain cim:ExcAC1A ;
  rdfs:range cim:Seconds ;
  skos:definition "Voltage regulator time constant (<i>Tb</i>) (&gt;= 0).  Typical value = 0."@en .

cim:ExcAC1A.tc a owl:DatatypeProperty ;
  rdfs:label "tc"@en ;
  rdfs:domain cim:ExcAC1A ;
  rdfs:range cim:Seconds ;
  skos:definition "Voltage regulator time constant (<i>T</i><i><sub>c</sub></i>) (&gt;= 0).  Typical value = 0."@en .

cim:ExcAC1A.te a owl:DatatypeProperty ;
  rdfs:label "te"@en ;
  rdfs:domain cim:ExcAC1A ;
  rdfs:range cim:Seconds ;
  skos:definition "Exciter time constant, integration rate associated with exciter control (<i>Te</i>) (&gt; 0).  Typical value = 0,8."@en .

cim:ExcAC1A.tf a owl:DatatypeProperty ;
  rdfs:label "tf"@en ;
  rdfs:domain cim:ExcAC1A ;
  rdfs:range cim:Seconds ;
  skos:definition "Excitation control system stabilizer time constant (<i>Tf</i>) (&gt; 0).  Typical value = 1."@en .

cim:ExcAC1A.vamax a owl:DatatypeProperty ;
  rdfs:label "vamax"@en ;
  rdfs:domain cim:ExcAC1A ;
  rdfs:range cim:PU ;
  skos:definition "Maximum voltage regulator output (<i>V</i><i><sub>amax</sub></i>) (&gt; 0).  Typical value = 14,5."@en .

cim:ExcAC1A.vamin a owl:DatatypeProperty ;
  rdfs:label "vamin"@en ;
  rdfs:domain cim:ExcAC1A ;
  rdfs:range cim:PU ;
  skos:definition "Minimum voltage regulator output (<i>V</i><i><sub>amin</sub></i>) (&lt; 0).  Typical value = -14,5."@en .

cim:ExcAC1A.ve1 a owl:DatatypeProperty ;
  rdfs:label "ve1"@en ;
  rdfs:domain cim:ExcAC1A ;
  rdfs:range cim:PU ;
  skos:definition "Exciter alternator output voltages back of commutating reactance at which saturation is defined (<i>Ve1</i>) (&gt; 0).  Typical value = 4,18."@en .

cim:ExcAC1A.ve2 a owl:DatatypeProperty ;
  rdfs:label "ve2"@en ;
  rdfs:domain cim:ExcAC1A ;
  rdfs:range cim:PU ;
  skos:definition "Exciter alternator output voltages back of commutating reactance at which saturation is defined (<i>Ve2</i>) (&gt; 0).  Typical value = 3,14."@en .

cim:ExcAC1A.vrmax a owl:DatatypeProperty ;
  rdfs:label "vrmax"@en ;
  rdfs:domain cim:ExcAC1A ;
  rdfs:range cim:PU ;
  skos:definition "Maximum voltage regulator outputs (<i>Vrmax</i>) (&gt; 0).  Typical value = 6,03."@en .

cim:ExcAC1A.vrmin a owl:DatatypeProperty ;
  rdfs:label "vrmin"@en ;
  rdfs:domain cim:ExcAC1A ;
  rdfs:range cim:PU ;
  skos:definition "Minimum voltage regulator outputs (<i>Vrmin</i>) (&lt; 0).  Typical value = -5,43."@en .

cim:ExcAC2A.hvgate a owl:DatatypeProperty ;
  rdfs:label "hvgate"@en ;
  rdfs:domain cim:ExcAC2A ;
  rdfs:range xsd:boolean ;
  skos:definition """
Indicates if HV gate is active (<i>HVgate</i>).
true = gate is used
false = gate is not used.
Typical value = true.
\t"""@en .

cim:ExcAC2A.ka a owl:DatatypeProperty ;
  rdfs:label "ka"@en ;
  rdfs:domain cim:ExcAC2A ;
  rdfs:range cim:PU ;
  skos:definition "Voltage regulator gain (<i>Ka</i>) (&gt; 0).  Typical value = 400."@en .

cim:ExcAC2A.kb a owl:DatatypeProperty ;
  rdfs:label "kb"@en ;
  rdfs:domain cim:ExcAC2A ;
  rdfs:range cim:PU ;
  skos:definition "Second stage regulator gain (<i>Kb</i>) (&gt; 0).  Exciter field current controller gain.  Typical value = 25."@en .

cim:ExcAC2A.kb1 a owl:DatatypeProperty ;
  rdfs:label "kb1"@en ;
  rdfs:domain cim:ExcAC2A ;
  rdfs:range cim:PU ;
  skos:definition "Second stage regulator gain (<i>Kb1</i>). It is exciter field current controller gain used as alternative to <i>Kb</i> to represent a variant of the ExcAC2A model.  Typical value = 25."@en .

cim:ExcAC2A.kc a owl:DatatypeProperty ;
  rdfs:label "kc"@en ;
  rdfs:domain cim:ExcAC2A ;
  rdfs:range cim:PU ;
  skos:definition "Rectifier loading factor proportional to commutating reactance (<i>Kc</i>) (&gt;= 0).  Typical value = 0,28."@en .

cim:ExcAC2A.kd a owl:DatatypeProperty ;
  rdfs:label "kd"@en ;
  rdfs:domain cim:ExcAC2A ;
  rdfs:range cim:PU ;
  skos:definition "Demagnetizing factor, a function of exciter alternator reactances (<i>Kd</i>) (&gt;= 0).  Typical value = 0,35."@en .

cim:ExcAC2A.ke a owl:DatatypeProperty ;
  rdfs:label "ke"@en ;
  rdfs:domain cim:ExcAC2A ;
  rdfs:range cim:PU ;
  skos:definition "Exciter constant related to self-excited field (<i>Ke</i>).  Typical value = 1."@en .

cim:ExcAC2A.kf a owl:DatatypeProperty ;
  rdfs:label "kf"@en ;
  rdfs:domain cim:ExcAC2A ;
  rdfs:range cim:PU ;
  skos:definition "Excitation control system stabilizer gains (<i>Kf</i>) (&gt;= 0).  Typical value = 0,03."@en .

cim:ExcAC2A.kh a owl:DatatypeProperty ;
  rdfs:label "kh"@en ;
  rdfs:domain cim:ExcAC2A ;
  rdfs:range cim:PU ;
  skos:definition "Exciter field current feedback gain (<i>Kh</i>) (&gt;= 0).  Typical value = 1."@en .

cim:ExcAC2A.kl a owl:DatatypeProperty ;
  rdfs:label "kl"@en ;
  rdfs:domain cim:ExcAC2A ;
  rdfs:range cim:PU ;
  skos:definition "Exciter field current limiter gain (<i>Kl</i>).  Typical value = 10."@en .

cim:ExcAC2A.kl1 a owl:DatatypeProperty ;
  rdfs:label "kl1"@en ;
  rdfs:domain cim:ExcAC2A ;
  rdfs:range cim:PU ;
  skos:definition "Coefficient to allow different usage of the model (<i>Kl1</i>).  Typical value = 1."@en .

cim:ExcAC2A.ks a owl:DatatypeProperty ;
  rdfs:label "ks"@en ;
  rdfs:domain cim:ExcAC2A ;
  rdfs:range cim:PU ;
  skos:definition "Coefficient to allow different usage of the model-speed coefficient (<i>Ks</i>) (&gt;= 0).  Typical value = 0."@en .

cim:ExcAC2A.lvgate a owl:DatatypeProperty ;
  rdfs:label "lvgate"@en ;
  rdfs:domain cim:ExcAC2A ;
  rdfs:range xsd:boolean ;
  skos:definition """
Indicates if LV gate is active (<i>LVgate</i>).
true = gate is used
false = gate is not used.
Typical value = true.
\t"""@en .

cim:ExcAC2A.seve1 a owl:DatatypeProperty ;
  rdfs:label "seve1"@en ;
  rdfs:domain cim:ExcAC2A ;
  rdfs:range xsd:float ;
  skos:definition "Exciter saturation function value at the corresponding exciter voltage, <i>Ve</i><i><sub>1</sub></i>, back of commutating reactance (<i>Se[Ve</i><i><sub>1</sub></i><i>]</i>) (&gt;= 0).  Typical value = 0,037."@en .

cim:ExcAC2A.seve2 a owl:DatatypeProperty ;
  rdfs:label "seve2"@en ;
  rdfs:domain cim:ExcAC2A ;
  rdfs:range xsd:float ;
  skos:definition "Exciter saturation function value at the corresponding exciter voltage, <i>Ve</i><i><sub>2</sub></i>, back of commutating reactance (<i>Se[Ve</i><i><sub>2</sub></i><i>]</i>) (&gt;= 0).  Typical value = 0,012."@en .

cim:ExcAC2A.ta a owl:DatatypeProperty ;
  rdfs:label "ta"@en ;
  rdfs:domain cim:ExcAC2A ;
  rdfs:range cim:Seconds ;
  skos:definition "Voltage regulator time constant (<i>Ta</i>) (&gt; 0).  Typical value = 0,02."@en .

cim:ExcAC2A.tb a owl:DatatypeProperty ;
  rdfs:label "tb"@en ;
  rdfs:domain cim:ExcAC2A ;
  rdfs:range cim:Seconds ;
  skos:definition "Voltage regulator time constant (<i>Tb</i>) (&gt;= 0).  Typical value = 0."@en .

cim:ExcAC2A.tc a owl:DatatypeProperty ;
  rdfs:label "tc"@en ;
  rdfs:domain cim:ExcAC2A ;
  rdfs:range cim:Seconds ;
  skos:definition "Voltage regulator time constant (<i>Tc</i>) (&gt;= 0).  Typical value = 0."@en .

cim:ExcAC2A.te a owl:DatatypeProperty ;
  rdfs:label "te"@en ;
  rdfs:domain cim:ExcAC2A ;
  rdfs:range cim:Seconds ;
  skos:definition "Exciter time constant, integration rate associated with exciter control (<i>Te</i>) (&gt; 0).  Typical value = 0,6."@en .

cim:ExcAC2A.tf a owl:DatatypeProperty ;
  rdfs:label "tf"@en ;
  rdfs:domain cim:ExcAC2A ;
  rdfs:range cim:Seconds ;
  skos:definition "Excitation control system stabilizer time constant (<i>Tf</i>) (&gt; 0).  Typical value = 1."@en .

cim:ExcAC2A.vamax a owl:DatatypeProperty ;
  rdfs:label "vamax"@en ;
  rdfs:domain cim:ExcAC2A ;
  rdfs:range cim:PU ;
  skos:definition "Maximum voltage regulator output (<i>Vamax</i>) (&gt; 0).  Typical value = 8."@en .

cim:ExcAC2A.vamin a owl:DatatypeProperty ;
  rdfs:label "vamin"@en ;
  rdfs:domain cim:ExcAC2A ;
  rdfs:range cim:PU ;
  skos:definition "Minimum voltage regulator output (<i>Vamin</i>) (&lt; 0).  Typical value = -8."@en .

cim:ExcAC2A.ve1 a owl:DatatypeProperty ;
  rdfs:label "ve1"@en ;
  rdfs:domain cim:ExcAC2A ;
  rdfs:range cim:PU ;
  skos:definition "Exciter alternator output voltages back of commutating reactance at which saturation is defined (<i>Ve</i><i><sub>1</sub></i>) (&gt; 0).  Typical value = 4,4."@en .

cim:ExcAC2A.ve2 a owl:DatatypeProperty ;
  rdfs:label "ve2"@en ;
  rdfs:domain cim:ExcAC2A ;
  rdfs:range cim:PU ;
  skos:definition "Exciter alternator output voltages back of commutating reactance at which saturation is defined (<i>Ve</i><i><sub>2</sub></i>) (&gt; 0).  Typical value = 3,3."@en .

cim:ExcAC2A.vfemax a owl:DatatypeProperty ;
  rdfs:label "vfemax"@en ;
  rdfs:domain cim:ExcAC2A ;
  rdfs:range cim:PU ;
  skos:definition "Exciter field current limit reference (<i>Vfemax</i>) (&gt;= 0).  Typical value = 4,4."@en .

cim:ExcAC2A.vlr a owl:DatatypeProperty ;
  rdfs:label "vlr"@en ;
  rdfs:domain cim:ExcAC2A ;
  rdfs:range cim:PU ;
  skos:definition "Maximum exciter field current (<i>Vlr</i>) (&gt; 0).  Typical value = 4,4."@en .

cim:ExcAC2A.vrmax a owl:DatatypeProperty ;
  rdfs:label "vrmax"@en ;
  rdfs:domain cim:ExcAC2A ;
  rdfs:range cim:PU ;
  skos:definition "Maximum voltage regulator outputs (<i>Vrmax</i>) (&gt; 0).  Typical value = 105."@en .

cim:ExcAC2A.vrmin a owl:DatatypeProperty ;
  rdfs:label "vrmin"@en ;
  rdfs:domain cim:ExcAC2A ;
  rdfs:range cim:PU ;
  skos:definition "Minimum voltage regulator outputs (<i>Vrmin</i>) (&lt; 0).  Typical value = -95."@en .

cim:ExcAC3A.efdn a owl:DatatypeProperty ;
  rdfs:label "efdn"@en ;
  rdfs:domain cim:ExcAC3A ;
  rdfs:range cim:PU ;
  skos:definition "Value of <i>Efd </i>at which feedback gain changes (<i>Efdn</i>) (&gt; 0).  Typical value = 2,36."@en .

cim:ExcAC3A.ka a owl:DatatypeProperty ;
  rdfs:label "ka"@en ;
  rdfs:domain cim:ExcAC3A ;
  rdfs:range cim:Seconds ;
  skos:definition "Voltage regulator gain (<i>Ka</i>) (&gt; 0).  Typical value = 45,62."@en .

cim:ExcAC3A.kc a owl:DatatypeProperty ;
  rdfs:label "kc"@en ;
  rdfs:domain cim:ExcAC3A ;
  rdfs:range cim:PU ;
  skos:definition "Rectifier loading factor proportional to commutating reactance (<i>Kc</i>) (&gt;= 0).  Typical value = 0,104."@en .

cim:ExcAC3A.kd a owl:DatatypeProperty ;
  rdfs:label "kd"@en ;
  rdfs:domain cim:ExcAC3A ;
  rdfs:range cim:PU ;
  skos:definition "Demagnetizing factor, a function of exciter alternator reactances (<i>Kd</i>) (&gt;= 0).  Typical value = 0,499."@en .

cim:ExcAC3A.ke a owl:DatatypeProperty ;
  rdfs:label "ke"@en ;
  rdfs:domain cim:ExcAC3A ;
  rdfs:range cim:PU ;
  skos:definition "Exciter constant related to self-excited field (<i>Ke</i>).  Typical value = 1."@en .

cim:ExcAC3A.kf a owl:DatatypeProperty ;
  rdfs:label "kf"@en ;
  rdfs:domain cim:ExcAC3A ;
  rdfs:range cim:PU ;
  skos:definition "Excitation control system stabilizer gains (<i>Kf</i>) (&gt;= 0).  Typical value = 0,143."@en .

cim:ExcAC3A.kf1 a owl:DatatypeProperty ;
  rdfs:label "kf1"@en ;
  rdfs:domain cim:ExcAC3A ;
  rdfs:range cim:PU ;
  skos:definition "Coefficient to allow different usage of the model (<i>Kf1</i>).  Typical value = 1."@en .

cim:ExcAC3A.kf2 a owl:DatatypeProperty ;
  rdfs:label "kf2"@en ;
  rdfs:domain cim:ExcAC3A ;
  rdfs:range cim:PU ;
  skos:definition "Coefficient to allow different usage of the model (<i>Kf2</i>).  Typical value = 0."@en .

cim:ExcAC3A.klv a owl:DatatypeProperty ;
  rdfs:label "klv"@en ;
  rdfs:domain cim:ExcAC3A ;
  rdfs:range cim:PU ;
  skos:definition "Gain used in the minimum field voltage limiter loop (<i>Klv</i>).  Typical value = 0,194."@en .

cim:ExcAC3A.kn a owl:DatatypeProperty ;
  rdfs:label "kn"@en ;
  rdfs:domain cim:ExcAC3A ;
  rdfs:range cim:PU ;
  skos:definition "Excitation control system stabilizer gain (<i>Kn</i>) (&gt;= 0).  Typical value =0,05."@en .

cim:ExcAC3A.kr a owl:DatatypeProperty ;
  rdfs:label "kr"@en ;
  rdfs:domain cim:ExcAC3A ;
  rdfs:range cim:PU ;
  skos:definition "Constant associated with regulator and alternator field power supply (<i>Kr</i>) (&gt; 0).  Typical value =3,77."@en .

cim:ExcAC3A.ks a owl:DatatypeProperty ;
  rdfs:label "ks"@en ;
  rdfs:domain cim:ExcAC3A ;
  rdfs:range cim:PU ;
  skos:definition "Coefficient to allow different usage of the model-speed coefficient (<i>Ks</i>).  Typical value = 0."@en .

cim:ExcAC3A.seve1 a owl:DatatypeProperty ;
  rdfs:label "seve1"@en ;
  rdfs:domain cim:ExcAC3A ;
  rdfs:range xsd:float ;
  skos:definition "Exciter saturation function value at the corresponding exciter voltage, <i>Ve</i><i><sub>1</sub></i>, back of commutating reactance (<i>Se[Ve</i><i><sub>1</sub></i><i>]</i>) (&gt;= 0).  Typical value = 1,143."@en .

cim:ExcAC3A.seve2 a owl:DatatypeProperty ;
  rdfs:label "seve2"@en ;
  rdfs:domain cim:ExcAC3A ;
  rdfs:range xsd:float ;
  skos:definition "Exciter saturation function value at the corresponding exciter voltage, <i>Ve</i><i><sub>2</sub></i>, back of commutating reactance (<i>Se[Ve</i><i><sub>2</sub></i><i>]</i>) (&gt;= 0).  Typical value = 0,1."@en .

cim:ExcAC3A.ta a owl:DatatypeProperty ;
  rdfs:label "ta"@en ;
  rdfs:domain cim:ExcAC3A ;
  rdfs:range cim:PU ;
  skos:definition "Voltage regulator time constant (<i>Ta</i>) (&gt; 0).  Typical value = 0,013."@en .

cim:ExcAC3A.tb a owl:DatatypeProperty ;
  rdfs:label "tb"@en ;
  rdfs:domain cim:ExcAC3A ;
  rdfs:range cim:Seconds ;
  skos:definition "Voltage regulator time constant (<i>Tb</i>) (&gt;= 0).  Typical value = 0."@en .

cim:ExcAC3A.tc a owl:DatatypeProperty ;
  rdfs:label "tc"@en ;
  rdfs:domain cim:ExcAC3A ;
  rdfs:range cim:Seconds ;
  skos:definition "Voltage regulator time constant (<i>Tc</i>) (&gt;= 0).  Typical value = 0."@en .

cim:ExcAC3A.te a owl:DatatypeProperty ;
  rdfs:label "te"@en ;
  rdfs:domain cim:ExcAC3A ;
  rdfs:range cim:Seconds ;
  skos:definition "Exciter time constant, integration rate associated with exciter control (<i>Te</i>) (&gt; 0).  Typical value = 1,17."@en .

cim:ExcAC3A.tf a owl:DatatypeProperty ;
  rdfs:label "tf"@en ;
  rdfs:domain cim:ExcAC3A ;
  rdfs:range cim:Seconds ;
  skos:definition "Excitation control system stabilizer time constant (<i>Tf</i>) (&gt; 0).  Typical value = 1."@en .

cim:ExcAC3A.vamax a owl:DatatypeProperty ;
  rdfs:label "vamax"@en ;
  rdfs:domain cim:ExcAC3A ;
  rdfs:range cim:PU ;
  skos:definition "Maximum voltage regulator output (<i>Vamax</i>) (&gt; 0).  Typical value = 1."@en .

cim:ExcAC3A.vamin a owl:DatatypeProperty ;
  rdfs:label "vamin"@en ;
  rdfs:domain cim:ExcAC3A ;
  rdfs:range cim:PU ;
  skos:definition "Minimum voltage regulator output (<i>Vamin</i>) (&lt; 0).  Typical value = -0,95."@en .

cim:ExcAC3A.ve1 a owl:DatatypeProperty ;
  rdfs:label "ve1"@en ;
  rdfs:domain cim:ExcAC3A ;
  rdfs:range cim:PU ;
  skos:definition "Exciter alternator output voltages back of commutating reactance at which saturation is defined (<i>Ve</i><i><sub>1</sub></i>) (&gt; 0).  Typical value = 6.24."@en .

cim:ExcAC3A.ve2 a owl:DatatypeProperty ;
  rdfs:label "ve2"@en ;
  rdfs:domain cim:ExcAC3A ;
  rdfs:range cim:PU ;
  skos:definition "Exciter alternator output voltages back of commutating reactance at which saturation is defined (<i>Ve</i><i><sub>2</sub></i>) (&gt; 0).  Typical value = 4,68."@en .

cim:ExcAC3A.vemin a owl:DatatypeProperty ;
  rdfs:label "vemin"@en ;
  rdfs:domain cim:ExcAC3A ;
  rdfs:range cim:PU ;
  skos:definition "Minimum exciter voltage output (<i>Vemin</i>) (&lt;= 0).  Typical value = 0."@en .

cim:ExcAC3A.vfemax a owl:DatatypeProperty ;
  rdfs:label "vfemax"@en ;
  rdfs:domain cim:ExcAC3A ;
  rdfs:range cim:PU ;
  skos:definition "Exciter field current limit reference (<i>Vfemax</i>) (&gt;= 0).  Typical value = 16."@en .

cim:ExcAC3A.vlv a owl:DatatypeProperty ;
  rdfs:label "vlv"@en ;
  rdfs:domain cim:ExcAC3A ;
  rdfs:range cim:PU ;
  skos:definition "Field voltage used in the minimum field voltage limiter loop (<i>Vlv</i>).  Typical value = 0,79."@en .

cim:ExcAC4A.ka a owl:DatatypeProperty ;
  rdfs:label "ka"@en ;
  rdfs:domain cim:ExcAC4A ;
  rdfs:range cim:PU ;
  skos:definition "Voltage regulator gain (<i>Ka</i>) (&gt; 0).  Typical value = 200."@en .

cim:ExcAC4A.kc a owl:DatatypeProperty ;
  rdfs:label "kc"@en ;
  rdfs:domain cim:ExcAC4A ;
  rdfs:range cim:PU ;
  skos:definition "Rectifier loading factor proportional to commutating reactance (<i>Kc</i>) (&gt;= 0).  Typical value = 0."@en .

cim:ExcAC4A.ta a owl:DatatypeProperty ;
  rdfs:label "ta"@en ;
  rdfs:domain cim:ExcAC4A ;
  rdfs:range cim:Seconds ;
  skos:definition "Voltage regulator time constant (<i>Ta</i>) (&gt; 0).  Typical value = 0,015."@en .

cim:ExcAC4A.tb a owl:DatatypeProperty ;
  rdfs:label "tb"@en ;
  rdfs:domain cim:ExcAC4A ;
  rdfs:range cim:Seconds ;
  skos:definition "Voltage regulator time constant (<i>Tb</i>) (&gt;= 0).  Typical value = 10."@en .

cim:ExcAC4A.tc a owl:DatatypeProperty ;
  rdfs:label "tc"@en ;
  rdfs:domain cim:ExcAC4A ;
  rdfs:range cim:Seconds ;
  skos:definition "Voltage regulator time constant (<i>Tc</i>) (&gt;= 0).  Typical value = 1."@en .

cim:ExcAC4A.vimax a owl:DatatypeProperty ;
  rdfs:label "vimax"@en ;
  rdfs:domain cim:ExcAC4A ;
  rdfs:range cim:PU ;
  skos:definition "Maximum voltage regulator input limit (<i>Vimax</i>)  (&gt; 0).  Typical value = 10."@en .

cim:ExcAC4A.vimin a owl:DatatypeProperty ;
  rdfs:label "vimin"@en ;
  rdfs:domain cim:ExcAC4A ;
  rdfs:range cim:PU ;
  skos:definition "Minimum voltage regulator input limit (<i>Vimin</i>) (&lt; 0).  Typical value = -10."@en .

cim:ExcAC4A.vrmax a owl:DatatypeProperty ;
  rdfs:label "vrmax"@en ;
  rdfs:domain cim:ExcAC4A ;
  rdfs:range cim:PU ;
  skos:definition "Maximum voltage regulator output (<i>Vrmax</i>) (&gt; 0).  Typical value = 5,64."@en .

cim:ExcAC4A.vrmin a owl:DatatypeProperty ;
  rdfs:label "vrmin"@en ;
  rdfs:domain cim:ExcAC4A ;
  rdfs:range cim:PU ;
  skos:definition "Minimum voltage regulator output (<i>Vrmin</i>) (&lt; 0).  Typical value = -4,53."@en .

cim:ExcAC5A.a a owl:DatatypeProperty ;
  rdfs:label "a"@en ;
  rdfs:domain cim:ExcAC5A ;
  rdfs:range xsd:float ;
  skos:definition "Coefficient to allow different usage of the model (<i>a</i>).  Typical value = 1."@en .

cim:ExcAC5A.efd1 a owl:DatatypeProperty ;
  rdfs:label "efd1"@en ;
  rdfs:domain cim:ExcAC5A ;
  rdfs:range cim:PU ;
  skos:definition "Exciter voltage at which exciter saturation is defined (<i>Efd1</i>) (&gt; 0).  Typical value = 5,6."@en .

cim:ExcAC5A.efd2 a owl:DatatypeProperty ;
  rdfs:label "efd2"@en ;
  rdfs:domain cim:ExcAC5A ;
  rdfs:range cim:PU ;
  skos:definition "Exciter voltage at which exciter saturation is defined (<i>Efd2</i>) (&gt; 0).  Typical value = 4,2."@en .

cim:ExcAC5A.ka a owl:DatatypeProperty ;
  rdfs:label "ka"@en ;
  rdfs:domain cim:ExcAC5A ;
  rdfs:range cim:PU ;
  skos:definition "Voltage regulator gain (<i>Ka</i>) (&gt; 0).  Typical value = 400."@en .

cim:ExcAC5A.ke a owl:DatatypeProperty ;
  rdfs:label "ke"@en ;
  rdfs:domain cim:ExcAC5A ;
  rdfs:range cim:PU ;
  skos:definition "Exciter constant related to self-excited field (<i>Ke</i>).  Typical value = 1."@en .

cim:ExcAC5A.kf a owl:DatatypeProperty ;
  rdfs:label "kf"@en ;
  rdfs:domain cim:ExcAC5A ;
  rdfs:range cim:PU ;
  skos:definition "Excitation control system stabilizer gains (<i>Kf</i>) (&gt;= 0).  Typical value = 0,03."@en .

cim:ExcAC5A.ks a owl:DatatypeProperty ;
  rdfs:label "ks"@en ;
  rdfs:domain cim:ExcAC5A ;
  rdfs:range cim:PU ;
  skos:definition "Coefficient to allow different usage of the model-speed coefficient (<i>Ks</i>).  Typical value = 0."@en .

cim:ExcAC5A.seefd1 a owl:DatatypeProperty ;
  rdfs:label "seefd1"@en ;
  rdfs:domain cim:ExcAC5A ;
  rdfs:range xsd:float ;
  skos:definition "Exciter saturation function value at the corresponding exciter voltage, <i>Efd</i><i><sub>1</sub></i> (<i>Se[Efd</i><i><sub>1</sub></i><i>]</i>) (&gt;= 0).  Typical value = 0,86."@en .

cim:ExcAC5A.seefd2 a owl:DatatypeProperty ;
  rdfs:label "seefd2"@en ;
  rdfs:domain cim:ExcAC5A ;
  rdfs:range xsd:float ;
  skos:definition "Exciter saturation function value at the corresponding exciter voltage, <i>Efd</i><i><sub>2</sub></i> (<i>Se[Efd</i><i><sub>2</sub></i><i>]</i>) (&gt;= 0).  Typical value = 0,5."@en .

cim:ExcAC5A.ta a owl:DatatypeProperty ;
  rdfs:label "ta"@en ;
  rdfs:domain cim:ExcAC5A ;
  rdfs:range cim:Seconds ;
  skos:definition "Voltage regulator time constant (<i>Ta</i>) (&gt; 0).  Typical value = 0,02."@en .

cim:ExcAC5A.tb a owl:DatatypeProperty ;
  rdfs:label "tb"@en ;
  rdfs:domain cim:ExcAC5A ;
  rdfs:range cim:Seconds ;
  skos:definition "Voltage regulator time constant (<i>Tb</i>) (&gt;= 0).  Typical value = 0."@en .

cim:ExcAC5A.tc a owl:DatatypeProperty ;
  rdfs:label "tc"@en ;
  rdfs:domain cim:ExcAC5A ;
  rdfs:range cim:Seconds ;
  skos:definition "Voltage regulator time constant (<i>Tc</i>) (&gt;= 0).  Typical value = 0."@en .

cim:ExcAC5A.te a owl:DatatypeProperty ;
  rdfs:label "te"@en ;
  rdfs:domain cim:ExcAC5A ;
  rdfs:range cim:Seconds ;
  skos:definition "Exciter time constant, integration rate associated with exciter control (<i>Te</i>) (&gt; 0).  Typical value = 0,8."@en .

cim:ExcAC5A.tf1 a owl:DatatypeProperty ;
  rdfs:label "tf1"@en ;
  rdfs:domain cim:ExcAC5A ;
  rdfs:range cim:Seconds ;
  skos:definition "Excitation control system stabilizer time constant (<i>Tf1</i>) (&gt; 0).  Typical value  = 1."@en .

cim:ExcAC5A.tf2 a owl:DatatypeProperty ;
  rdfs:label "tf2"@en ;
  rdfs:domain cim:ExcAC5A ;
  rdfs:range cim:Seconds ;
  skos:definition "Excitation control system stabilizer time constant (<i>Tf2</i>) (&gt;= 0).  Typical value = 0,8."@en .

cim:ExcAC5A.tf3 a owl:DatatypeProperty ;
  rdfs:label "tf3"@en ;
  rdfs:domain cim:ExcAC5A ;
  rdfs:range cim:Seconds ;
  skos:definition "Excitation control system stabilizer time constant (<i>Tf3</i>) (&gt;= 0).  Typical value = 0."@en .

cim:ExcAC5A.vrmax a owl:DatatypeProperty ;
  rdfs:label "vrmax"@en ;
  rdfs:domain cim:ExcAC5A ;
  rdfs:range cim:PU ;
  skos:definition "Maximum voltage regulator output (<i>Vrmax</i>) (&gt; 0).  Typical value = 7,3."@en .

cim:ExcAC5A.vrmin a owl:DatatypeProperty ;
  rdfs:label "vrmin"@en ;
  rdfs:domain cim:ExcAC5A ;
  rdfs:range cim:PU ;
  skos:definition "Minimum voltage regulator output (<i>Vrmin</i>) (&lt; 0).  Typical value =-7,3."@en .

cim:ExcAC6A.ka a owl:DatatypeProperty ;
  rdfs:label "ka"@en ;
  rdfs:domain cim:ExcAC6A ;
  rdfs:range cim:PU ;
  skos:definition "Voltage regulator gain (<i>Ka</i>) (&gt; 0).  Typical value = 536."@en .

cim:ExcAC6A.kc a owl:DatatypeProperty ;
  rdfs:label "kc"@en ;
  rdfs:domain cim:ExcAC6A ;
  rdfs:range cim:PU ;
  skos:definition "Rectifier loading factor proportional to commutating reactance (<i>Kc</i>) (&gt;= 0).  Typical value = 0,173."@en .

cim:ExcAC6A.kd a owl:DatatypeProperty ;
  rdfs:label "kd"@en ;
  rdfs:domain cim:ExcAC6A ;
  rdfs:range cim:PU ;
  skos:definition "Demagnetizing factor, a function of exciter alternator reactances (<i>Kd</i>) (&gt;= 0).  Typical value = 1,91."@en .

cim:ExcAC6A.ke a owl:DatatypeProperty ;
  rdfs:label "ke"@en ;
  rdfs:domain cim:ExcAC6A ;
  rdfs:range cim:PU ;
  skos:definition "Exciter constant related to self-excited field (<i>Ke</i>).  Typical value = 1,6."@en .

cim:ExcAC6A.kh a owl:DatatypeProperty ;
  rdfs:label "kh"@en ;
  rdfs:domain cim:ExcAC6A ;
  rdfs:range cim:PU ;
  skos:definition "Exciter field current limiter gain (<i>Kh</i>) (&gt;= 0).  Typical value = 92."@en .

cim:ExcAC6A.ks a owl:DatatypeProperty ;
  rdfs:label "ks"@en ;
  rdfs:domain cim:ExcAC6A ;
  rdfs:range cim:PU ;
  skos:definition "Coefficient to allow different usage of the model-speed coefficient (<i>Ks</i>).  Typical value = 0."@en .

cim:ExcAC6A.seve1 a owl:DatatypeProperty ;
  rdfs:label "seve1"@en ;
  rdfs:domain cim:ExcAC6A ;
  rdfs:range xsd:float ;
  skos:definition "Exciter saturation function value at the corresponding exciter voltage, <i>Ve</i><i><sub>1</sub></i>, back of commutating reactance (<i>Se[Ve</i><i><sub>1</sub></i><i>]</i>) (&gt;= 0).  Typical value = 0,214."@en .

cim:ExcAC6A.seve2 a owl:DatatypeProperty ;
  rdfs:label "seve2"@en ;
  rdfs:domain cim:ExcAC6A ;
  rdfs:range xsd:float ;
  skos:definition "Exciter saturation function value at the corresponding exciter voltage, <i>Ve</i><i><sub>2</sub></i>, back of commutating reactance (<i>Se[Ve</i><i><sub>2</sub></i><i>]</i>) (&gt;= 0).  Typical value = 0,044."@en .

cim:ExcAC6A.ta a owl:DatatypeProperty ;
  rdfs:label "ta"@en ;
  rdfs:domain cim:ExcAC6A ;
  rdfs:range cim:Seconds ;
  skos:definition "Voltage regulator time constant (<i>Ta</i>) (&gt;= 0).  Typical value = 0,086."@en .

cim:ExcAC6A.tb a owl:DatatypeProperty ;
  rdfs:label "tb"@en ;
  rdfs:domain cim:ExcAC6A ;
  rdfs:range cim:Seconds ;
  skos:definition "Voltage regulator time constant (<i>Tb</i>) (&gt;= 0).  Typical value = 9."@en .

cim:ExcAC6A.tc a owl:DatatypeProperty ;
  rdfs:label "tc"@en ;
  rdfs:domain cim:ExcAC6A ;
  rdfs:range cim:Seconds ;
  skos:definition "Voltage regulator time constant (<i>Tc</i>) (&gt;= 0).  Typical value = 3."@en .

cim:ExcAC6A.te a owl:DatatypeProperty ;
  rdfs:label "te"@en ;
  rdfs:domain cim:ExcAC6A ;
  rdfs:range cim:Seconds ;
  skos:definition "Exciter time constant, integration rate associated with exciter control (<i>Te</i>) (&gt; 0).  Typical value = 1."@en .

cim:ExcAC6A.th a owl:DatatypeProperty ;
  rdfs:label "th"@en ;
  rdfs:domain cim:ExcAC6A ;
  rdfs:range cim:Seconds ;
  skos:definition "Exciter field current limiter time constant (<i>Th</i>) (&gt; 0).  Typical value = 0,08."@en .

cim:ExcAC6A.tj a owl:DatatypeProperty ;
  rdfs:label "tj"@en ;
  rdfs:domain cim:ExcAC6A ;
  rdfs:range cim:Seconds ;
  skos:definition "Exciter field current limiter time constant (<i>Tj</i>) (&gt;= 0).  Typical value = 0,02."@en .

cim:ExcAC6A.tk a owl:DatatypeProperty ;
  rdfs:label "tk"@en ;
  rdfs:domain cim:ExcAC6A ;
  rdfs:range cim:Seconds ;
  skos:definition "Voltage regulator time constant (<i>Tk</i>) (&gt;= 0).  Typical value = 0,18."@en .

cim:ExcAC6A.vamax a owl:DatatypeProperty ;
  rdfs:label "vamax"@en ;
  rdfs:domain cim:ExcAC6A ;
  rdfs:range cim:PU ;
  skos:definition "Maximum voltage regulator output (<i>Vamax</i>) (&gt; 0).  Typical value = 75."@en .

cim:ExcAC6A.vamin a owl:DatatypeProperty ;
  rdfs:label "vamin"@en ;
  rdfs:domain cim:ExcAC6A ;
  rdfs:range cim:PU ;
  skos:definition "Minimum voltage regulator output (<i>Vamin</i>) (&lt; 0).  Typical value = -75."@en .

cim:ExcAC6A.ve1 a owl:DatatypeProperty ;
  rdfs:label "ve1"@en ;
  rdfs:domain cim:ExcAC6A ;
  rdfs:range cim:PU ;
  skos:definition "Exciter alternator output voltages back of commutating reactance at which saturation is defined (<i>Ve</i><i><sub>1</sub></i>) (&gt; 0).  Typical value = 7,4."@en .

cim:ExcAC6A.ve2 a owl:DatatypeProperty ;
  rdfs:label "ve2"@en ;
  rdfs:domain cim:ExcAC6A ;
  rdfs:range cim:PU ;
  skos:definition "Exciter alternator output voltages back of commutating reactance at which saturation is defined (<i>Ve</i><i><sub>2</sub></i>) (&gt; 0).  Typical value = 5,55."@en .

cim:ExcAC6A.vfelim a owl:DatatypeProperty ;
  rdfs:label "vfelim"@en ;
  rdfs:domain cim:ExcAC6A ;
  rdfs:range cim:PU ;
  skos:definition "Exciter field current limit reference (<i>Vfelim</i>) (&gt; 0).  Typical value = 19."@en .

cim:ExcAC6A.vhmax a owl:DatatypeProperty ;
  rdfs:label "vhmax"@en ;
  rdfs:domain cim:ExcAC6A ;
  rdfs:range cim:PU ;
  skos:definition "Maximum field current limiter signal reference (<i>Vhmax</i>) (&gt; 0).  Typical value = 75."@en .

cim:ExcAC6A.vrmax a owl:DatatypeProperty ;
  rdfs:label "vrmax"@en ;
  rdfs:domain cim:ExcAC6A ;
  rdfs:range cim:PU ;
  skos:definition "Maximum voltage regulator output (<i>Vrmax</i>) (&gt; 0).  Typical value = 44."@en .

cim:ExcAC6A.vrmin a owl:DatatypeProperty ;
  rdfs:label "vrmin"@en ;
  rdfs:domain cim:ExcAC6A ;
  rdfs:range cim:PU ;
  skos:definition "Minimum voltage regulator output (<i>Vrmin</i>) (&lt; 0).  Typical value = -36."@en .

cim:ExcAC8B.inlim a owl:DatatypeProperty ;
  rdfs:label "inlim"@en ;
  rdfs:domain cim:ExcAC8B ;
  rdfs:range xsd:boolean ;
  skos:definition """
Input limiter indicator.
true = input limiter <i>Vimax</i> and <i>Vimin</i> is considered
false = input limiter <i>Vimax </i>and <i>Vimin</i> is not considered.
Typical value = true.
\t"""@en .

cim:ExcAC8B.ka a owl:DatatypeProperty ;
  rdfs:label "ka"@en ;
  rdfs:domain cim:ExcAC8B ;
  rdfs:range cim:PU ;
  skos:definition "Voltage regulator gain (<i>Ka</i>) (&gt; 0).  Typical value = 1."@en .

cim:ExcAC8B.kc a owl:DatatypeProperty ;
  rdfs:label "kc"@en ;
  rdfs:domain cim:ExcAC8B ;
  rdfs:range cim:PU ;
  skos:definition "Rectifier loading factor proportional to commutating reactance (<i>Kc</i>) (&gt;= 0). Typical value = 0,55."@en .

cim:ExcAC8B.kd a owl:DatatypeProperty ;
  rdfs:label "kd"@en ;
  rdfs:domain cim:ExcAC8B ;
  rdfs:range cim:PU ;
  skos:definition "Demagnetizing factor, a function of exciter alternator reactances (<i>Kd</i>) (&gt;= 0).  Typical value = 1,1."@en .

cim:ExcAC8B.kdr a owl:DatatypeProperty ;
  rdfs:label "kdr"@en ;
  rdfs:domain cim:ExcAC8B ;
  rdfs:range cim:PU ;
  skos:definition "Voltage regulator derivative gain (<i>Kdr</i>) (&gt;= 0).  Typical value = 10."@en .

cim:ExcAC8B.ke a owl:DatatypeProperty ;
  rdfs:label "ke"@en ;
  rdfs:domain cim:ExcAC8B ;
  rdfs:range cim:PU ;
  skos:definition "Exciter constant related to self-excited field (<i>Ke</i>).  Typical value = 1."@en .

cim:ExcAC8B.kir a owl:DatatypeProperty ;
  rdfs:label "kir"@en ;
  rdfs:domain cim:ExcAC8B ;
  rdfs:range cim:PU ;
  skos:definition "Voltage regulator integral gain (<i>Kir</i>) (&gt;= 0).  Typical value = 5."@en .

cim:ExcAC8B.kpr a owl:DatatypeProperty ;
  rdfs:label "kpr"@en ;
  rdfs:domain cim:ExcAC8B ;
  rdfs:range cim:PU ;
  skos:definition "Voltage regulator proportional gain (<i>Kpr</i>) (&gt; 0 if ExcAC8B.kir = 0).  Typical value = 80."@en .

cim:ExcAC8B.ks a owl:DatatypeProperty ;
  rdfs:label "ks"@en ;
  rdfs:domain cim:ExcAC8B ;
  rdfs:range cim:PU ;
  skos:definition "Coefficient to allow different usage of the model-speed coefficient (<i>Ks</i>).  Typical value = 0."@en .

cim:ExcAC8B.pidlim a owl:DatatypeProperty ;
  rdfs:label "pidlim"@en ;
  rdfs:domain cim:ExcAC8B ;
  rdfs:range xsd:boolean ;
  skos:definition """
PID limiter indicator.
true = input limiter <i>Vpidmax</i> and <i>Vpidmin</i> is considered
false = input limiter <i>Vpidmax</i> and <i>Vpidmin</i> is not considered.
Typical value = true.
\t"""@en .

cim:ExcAC8B.seve1 a owl:DatatypeProperty ;
  rdfs:label "seve1"@en ;
  rdfs:domain cim:ExcAC8B ;
  rdfs:range xsd:float ;
  skos:definition "Exciter saturation function value at the corresponding exciter voltage, <i>Ve</i><i><sub>1</sub></i>, back of commutating reactance (<i>Se[Ve</i><i><sub>1</sub></i><i>]</i>) (&gt;= 0).  Typical value = 0,3."@en .

cim:ExcAC8B.seve2 a owl:DatatypeProperty ;
  rdfs:label "seve2"@en ;
  rdfs:domain cim:ExcAC8B ;
  rdfs:range xsd:float ;
  skos:definition "Exciter saturation function value at the corresponding exciter voltage, <i>Ve</i><i><sub>2</sub></i>, back of commutating reactance (<i>Se[Ve</i><i><sub>2</sub></i><i>]</i>) (&gt;= 0).  Typical value = 3."@en .

cim:ExcAC8B.ta a owl:DatatypeProperty ;
  rdfs:label "ta"@en ;
  rdfs:domain cim:ExcAC8B ;
  rdfs:range cim:Seconds ;
  skos:definition "Voltage regulator time constant (<i>Ta</i>) (&gt;= 0).  Typical value = 0."@en .

cim:ExcAC8B.tdr a owl:DatatypeProperty ;
  rdfs:label "tdr"@en ;
  rdfs:domain cim:ExcAC8B ;
  rdfs:range cim:Seconds ;
  skos:definition "Lag time constant (<i>Tdr</i>) (&gt; 0 if ExcAC8B.kdr &gt; 0).  Typical value = 0,1."@en .

cim:ExcAC8B.te a owl:DatatypeProperty ;
  rdfs:label "te"@en ;
  rdfs:domain cim:ExcAC8B ;
  rdfs:range cim:Seconds ;
  skos:definition "Exciter time constant, integration rate associated with exciter control (<i>Te</i>) (&gt; 0).  Typical value = 1,2."@en .

cim:ExcAC8B.telim a owl:DatatypeProperty ;
  rdfs:label "telim"@en ;
  rdfs:domain cim:ExcAC8B ;
  rdfs:range xsd:boolean ;
  skos:definition """
Selector for the limiter on the block (<i>1/sTe</i>). 
See diagram for meaning of true and false.
Typical value = false.
\t"""@en .

cim:ExcAC8B.ve1 a owl:DatatypeProperty ;
  rdfs:label "ve1"@en ;
  rdfs:domain cim:ExcAC8B ;
  rdfs:range cim:PU ;
  skos:definition "Exciter alternator output voltages back of commutating reactance at which saturation is defined (<i>Ve</i><i><sub>1</sub></i>) (&gt; 0).  Typical value = 6,5."@en .

cim:ExcAC8B.ve2 a owl:DatatypeProperty ;
  rdfs:label "ve2"@en ;
  rdfs:domain cim:ExcAC8B ;
  rdfs:range cim:PU ;
  skos:definition "Exciter alternator output voltages back of commutating reactance at which saturation is defined (<i>Ve</i><i><sub>2</sub></i>) (&gt; 0).  Typical value = 9."@en .

cim:ExcAC8B.vemin a owl:DatatypeProperty ;
  rdfs:label "vemin"@en ;
  rdfs:domain cim:ExcAC8B ;
  rdfs:range cim:PU ;
  skos:definition "Minimum exciter voltage output (<i>Vemin</i>) (&lt;= 0).  Typical value = 0."@en .

cim:ExcAC8B.vfemax a owl:DatatypeProperty ;
  rdfs:label "vfemax"@en ;
  rdfs:domain cim:ExcAC8B ;
  rdfs:range cim:PU ;
  skos:definition "Exciter field current limit reference (<i>Vfemax</i>).  Typical value = 6."@en .

cim:ExcAC8B.vimax a owl:DatatypeProperty ;
  rdfs:label "vimax"@en ;
  rdfs:domain cim:ExcAC8B ;
  rdfs:range cim:PU ;
  skos:definition "Input signal maximum (<i>Vimax</i>) (&gt; ExcAC8B.vimin).  Typical value = 35."@en .

cim:ExcAC8B.vimin a owl:DatatypeProperty ;
  rdfs:label "vimin"@en ;
  rdfs:domain cim:ExcAC8B ;
  rdfs:range cim:PU ;
  skos:definition "Input signal minimum (<i>Vimin</i>) (&lt; ExcAC8B.vimax).  Typical value = -10."@en .

cim:ExcAC8B.vpidmax a owl:DatatypeProperty ;
  rdfs:label "vpidmax"@en ;
  rdfs:domain cim:ExcAC8B ;
  rdfs:range cim:PU ;
  skos:definition "PID maximum controller output (<i>Vpidmax</i>) (&gt; ExcAC8B.vpidmin).  Typical value = 35."@en .

cim:ExcAC8B.vpidmin a owl:DatatypeProperty ;
  rdfs:label "vpidmin"@en ;
  rdfs:domain cim:ExcAC8B ;
  rdfs:range cim:PU ;
  skos:definition "PID minimum controller output (<i>Vpidmin</i>) (&lt; ExcAC8B.vpidmax).  Typical value = -10."@en .

cim:ExcAC8B.vrmax a owl:DatatypeProperty ;
  rdfs:label "vrmax"@en ;
  rdfs:domain cim:ExcAC8B ;
  rdfs:range cim:PU ;
  skos:definition "Maximum voltage regulator output (<i>Vrmax</i>) (&gt; 0). Typical value = 35."@en .

cim:ExcAC8B.vrmin a owl:DatatypeProperty ;
  rdfs:label "vrmin"@en ;
  rdfs:domain cim:ExcAC8B ;
  rdfs:range cim:PU ;
  skos:definition "Minimum voltage regulator output (<i>Vrmin</i>) (&lt; 0).  Typical value = 0."@en .

cim:ExcAC8B.vtmult a owl:DatatypeProperty ;
  rdfs:label "vtmult"@en ;
  rdfs:domain cim:ExcAC8B ;
  rdfs:range xsd:boolean ;
  skos:definition """
Multiply by generator's terminal voltage indicator.
true =the limits <i>Vrmax</i> and <i>Vrmin</i> are multiplied by the generator’s terminal voltage to represent a thyristor power stage fed from the generator terminals
false = limits are not multiplied by generator's terminal voltage. 
Typical value = false.
\t"""@en .

cim:ExcANS.blint a owl:DatatypeProperty ;
  rdfs:label "blint"@en ;
  rdfs:domain cim:ExcANS ;
  rdfs:range xsd:integer ;
  skos:definition """
Governor control flag (<i>BLINT</i>). 
0 = lead-lag regulator
1 = proportional integral regulator.
Typical value = 0.
\t"""@en .

cim:ExcANS.ifmn a owl:DatatypeProperty ;
  rdfs:label "ifmn"@en ;
  rdfs:domain cim:ExcANS ;
  rdfs:range cim:PU ;
  skos:definition "Minimum exciter current (<i>I</i><i><sub>FMN</sub></i>).  Typical value = -5,2."@en .

cim:ExcANS.ifmx a owl:DatatypeProperty ;
  rdfs:label "ifmx"@en ;
  rdfs:domain cim:ExcANS ;
  rdfs:range cim:PU ;
  skos:definition "Maximum exciter current (<i>I</i><i><sub>FMX</sub></i>).  Typical value = 6,5."@en .

cim:ExcANS.k2 a owl:DatatypeProperty ;
  rdfs:label "k2"@en ;
  rdfs:domain cim:ExcANS ;
  rdfs:range xsd:float ;
  skos:definition "Exciter gain (<i>K</i><i><sub>2</sub></i>).  Typical value = 20."@en .

cim:ExcANS.k3 a owl:DatatypeProperty ;
  rdfs:label "k3"@en ;
  rdfs:domain cim:ExcANS ;
  rdfs:range xsd:float ;
  skos:definition "AVR gain (<i>K</i><i><sub>3</sub></i>).  Typical value = 1000."@en .

cim:ExcANS.kce a owl:DatatypeProperty ;
  rdfs:label "kce"@en ;
  rdfs:domain cim:ExcANS ;
  rdfs:range xsd:float ;
  skos:definition "Ceiling factor (<i>K</i><i><sub>CE</sub></i>).  Typical value = 1."@en .

cim:ExcANS.krvecc a owl:DatatypeProperty ;
  rdfs:label "krvecc"@en ;
  rdfs:domain cim:ExcANS ;
  rdfs:range xsd:integer ;
  skos:definition """
Feedback enabling (<i>K</i><i><sub>RVECC</sub></i>). 
0 = open loop control
1 = closed loop control.
Typical value = 1.
\t"""@en .

cim:ExcANS.kvfif a owl:DatatypeProperty ;
  rdfs:label "kvfif"@en ;
  rdfs:domain cim:ExcANS ;
  rdfs:range xsd:integer ;
  skos:definition """
Rate feedback signal flag (<i>K</i><i><sub>VFIF</sub></i>). 
0 = output voltage of the exciter
1 = exciter field current.
Typical value = 0.
\t"""@en .

cim:ExcANS.t1 a owl:DatatypeProperty ;
  rdfs:label "t1"@en ;
  rdfs:domain cim:ExcANS ;
  rdfs:range cim:Seconds ;
  skos:definition "Time constant (<i>T</i><i><sub>1</sub></i>) (&gt;= 0).  Typical value = 20."@en .

cim:ExcANS.t2 a owl:DatatypeProperty ;
  rdfs:label "t2"@en ;
  rdfs:domain cim:ExcANS ;
  rdfs:range cim:Seconds ;
  skos:definition "Time constant (<i>T</i><i><sub>2</sub></i>) (&gt;= 0).  Typical value = 0,05."@en .

cim:ExcANS.t3 a owl:DatatypeProperty ;
  rdfs:label "t3"@en ;
  rdfs:domain cim:ExcANS ;
  rdfs:range cim:Seconds ;
  skos:definition "Time constant (<i>T</i><i><sub>3</sub></i>) (&gt;= 0).  Typical value = 1,6."@en .

cim:ExcANS.tb a owl:DatatypeProperty ;
  rdfs:label "tb"@en ;
  rdfs:domain cim:ExcANS ;
  rdfs:range cim:Seconds ;
  skos:definition "Exciter time constant (<i>T</i><i><sub>B</sub></i>) (&gt;= 0).  Typical value = 0,04."@en .

cim:ExcANS.vrmn a owl:DatatypeProperty ;
  rdfs:label "vrmn"@en ;
  rdfs:domain cim:ExcANS ;
  rdfs:range cim:PU ;
  skos:definition "Minimum AVR output (<i>V</i><i><sub>RMN</sub></i>).  Typical value = -5,2."@en .

cim:ExcANS.vrmx a owl:DatatypeProperty ;
  rdfs:label "vrmx"@en ;
  rdfs:domain cim:ExcANS ;
  rdfs:range cim:PU ;
  skos:definition "Maximum AVR output (<i>V</i><i><sub>RMX</sub></i>).  Typical value = 6,5."@en .

cim:ExcAVR1.e1 a owl:DatatypeProperty ;
  rdfs:label "e1"@en ;
  rdfs:domain cim:ExcAVR1 ;
  rdfs:range cim:PU ;
  skos:definition "Field voltage value 1 (<i>E</i><i><sub>1</sub></i>).  Typical value = 4.18."@en .

cim:ExcAVR1.e2 a owl:DatatypeProperty ;
  rdfs:label "e2"@en ;
  rdfs:domain cim:ExcAVR1 ;
  rdfs:range cim:PU ;
  skos:definition "Field voltage value 2 (<i>E</i><i><sub>2</sub></i>).  Typical value = 3,14."@en .

cim:ExcAVR1.ka a owl:DatatypeProperty ;
  rdfs:label "ka"@en ;
  rdfs:domain cim:ExcAVR1 ;
  rdfs:range xsd:float ;
  skos:definition "AVR gain (<i>K</i><i><sub>A</sub></i>).  Typical value = 500."@en .

cim:ExcAVR1.kf a owl:DatatypeProperty ;
  rdfs:label "kf"@en ;
  rdfs:domain cim:ExcAVR1 ;
  rdfs:range xsd:float ;
  skos:definition "Rate feedback gain (<i>K</i><i><sub>F</sub></i>).  Typical value = 0,12."@en .

cim:ExcAVR1.se1 a owl:DatatypeProperty ;
  rdfs:label "se1"@en ;
  rdfs:domain cim:ExcAVR1 ;
  rdfs:range xsd:float ;
  skos:definition "Saturation factor at <i>E</i><i><sub>1</sub></i> (<i>S[E</i><i><sub>1</sub></i><i>]</i>).  Typical value = 0,1."@en .

cim:ExcAVR1.se2 a owl:DatatypeProperty ;
  rdfs:label "se2"@en ;
  rdfs:domain cim:ExcAVR1 ;
  rdfs:range xsd:float ;
  skos:definition "Saturation factor at <i>E</i><i><sub>2</sub></i> (<i>S[E</i><i><sub>2</sub></i><i>]</i>).  Typical value = 0,03."@en .

cim:ExcAVR1.ta a owl:DatatypeProperty ;
  rdfs:label "ta"@en ;
  rdfs:domain cim:ExcAVR1 ;
  rdfs:range cim:Seconds ;
  skos:definition "AVR time constant (<i>T</i><i><sub>A</sub></i>) (&gt;= 0).  Typical value = 0,2."@en .

cim:ExcAVR1.tb a owl:DatatypeProperty ;
  rdfs:label "tb"@en ;
  rdfs:domain cim:ExcAVR1 ;
  rdfs:range cim:Seconds ;
  skos:definition "AVR time constant (<i>T</i><i><sub>B</sub></i>) (&gt;= 0).  Typical value = 0."@en .

cim:ExcAVR1.te a owl:DatatypeProperty ;
  rdfs:label "te"@en ;
  rdfs:domain cim:ExcAVR1 ;
  rdfs:range cim:Seconds ;
  skos:definition "Exciter time constant (<i>T</i><i><sub>E</sub></i>) (&gt;= 0).  Typical value = 1."@en .

cim:ExcAVR1.tf a owl:DatatypeProperty ;
  rdfs:label "tf"@en ;
  rdfs:domain cim:ExcAVR1 ;
  rdfs:range cim:Seconds ;
  skos:definition "Rate feedback time constant (<i>T</i><i><sub>F</sub></i>) (&gt;= 0).  Typical value = 1."@en .

cim:ExcAVR1.vrmn a owl:DatatypeProperty ;
  rdfs:label "vrmn"@en ;
  rdfs:domain cim:ExcAVR1 ;
  rdfs:range cim:PU ;
  skos:definition "Minimum AVR output (<i>V</i><i><sub>RMN</sub></i>).  Typical value = -6."@en .

cim:ExcAVR1.vrmx a owl:DatatypeProperty ;
  rdfs:label "vrmx"@en ;
  rdfs:domain cim:ExcAVR1 ;
  rdfs:range cim:PU ;
  skos:definition "Maximum AVR output (<i>V</i><i><sub>RMX</sub></i>).  Typical value = 7."@en .

cim:ExcAVR2.e1 a owl:DatatypeProperty ;
  rdfs:label "e1"@en ;
  rdfs:domain cim:ExcAVR2 ;
  rdfs:range cim:PU ;
  skos:definition "Field voltage value 1 (<i>E</i><i><sub>1</sub></i>).  Typical value = 4,18."@en .

cim:ExcAVR2.e2 a owl:DatatypeProperty ;
  rdfs:label "e2"@en ;
  rdfs:domain cim:ExcAVR2 ;
  rdfs:range cim:PU ;
  skos:definition "Field voltage value 2 (<i>E</i><i><sub>2</sub></i>).  Typical value = 3,14."@en .

cim:ExcAVR2.ka a owl:DatatypeProperty ;
  rdfs:label "ka"@en ;
  rdfs:domain cim:ExcAVR2 ;
  rdfs:range xsd:float ;
  skos:definition "AVR gain (<i>K</i><i><sub>A</sub></i>).  Typical value = 500."@en .

cim:ExcAVR2.kf a owl:DatatypeProperty ;
  rdfs:label "kf"@en ;
  rdfs:domain cim:ExcAVR2 ;
  rdfs:range xsd:float ;
  skos:definition "Rate feedback gain (<i>K</i><i><sub>F</sub></i>).  Typical value = 0,12."@en .

cim:ExcAVR2.se1 a owl:DatatypeProperty ;
  rdfs:label "se1"@en ;
  rdfs:domain cim:ExcAVR2 ;
  rdfs:range xsd:float ;
  skos:definition "Saturation factor at <i>E</i><i><sub>1</sub></i> (<i>S[E</i><i><sub>1</sub></i><i>]</i>).  Typical value = 0.1."@en .

cim:ExcAVR2.se2 a owl:DatatypeProperty ;
  rdfs:label "se2"@en ;
  rdfs:domain cim:ExcAVR2 ;
  rdfs:range xsd:float ;
  skos:definition "Saturation factor at <i>E</i><i><sub>2</sub></i> (<i>S[E</i><i><sub>2</sub></i><i>]</i>).  Typical value = 0,03."@en .

cim:ExcAVR2.ta a owl:DatatypeProperty ;
  rdfs:label "ta"@en ;
  rdfs:domain cim:ExcAVR2 ;
  rdfs:range cim:Seconds ;
  skos:definition "AVR time constant (<i>T</i><i><sub>A</sub></i>) (&gt;= 0).  Typical value = 0,02."@en .

cim:ExcAVR2.tb a owl:DatatypeProperty ;
  rdfs:label "tb"@en ;
  rdfs:domain cim:ExcAVR2 ;
  rdfs:range cim:Seconds ;
  skos:definition "AVR time constant (<i>T</i><i><sub>B</sub></i>) (&gt;= 0).  Typical value = 0."@en .

cim:ExcAVR2.te a owl:DatatypeProperty ;
  rdfs:label "te"@en ;
  rdfs:domain cim:ExcAVR2 ;
  rdfs:range cim:Seconds ;
  skos:definition "Exciter time constant (<i>T</i><i><sub>E</sub></i>) (&gt;= 0).  Typical value = 1."@en .

cim:ExcAVR2.tf1 a owl:DatatypeProperty ;
  rdfs:label "tf1"@en ;
  rdfs:domain cim:ExcAVR2 ;
  rdfs:range cim:Seconds ;
  skos:definition "Rate feedback time constant (<i>T</i><i><sub>F1</sub></i>) (&gt;= 0).  Typical value = 1."@en .

cim:ExcAVR2.tf2 a owl:DatatypeProperty ;
  rdfs:label "tf2"@en ;
  rdfs:domain cim:ExcAVR2 ;
  rdfs:range cim:Seconds ;
  skos:definition "Rate feedback time constant (<i>T</i><i><sub>F2</sub></i>) (&gt;= 0).  Typical value = 1."@en .

cim:ExcAVR2.vrmn a owl:DatatypeProperty ;
  rdfs:label "vrmn"@en ;
  rdfs:domain cim:ExcAVR2 ;
  rdfs:range cim:PU ;
  skos:definition "Minimum AVR output (<i>V</i><i><sub>RMN</sub></i>).  Typical value = -6."@en .

cim:ExcAVR2.vrmx a owl:DatatypeProperty ;
  rdfs:label "vrmx"@en ;
  rdfs:domain cim:ExcAVR2 ;
  rdfs:range cim:PU ;
  skos:definition "Maximum AVR output (<i>V</i><i><sub>RMX</sub></i>).  Typical value = 7."@en .

cim:ExcAVR3.e1 a owl:DatatypeProperty ;
  rdfs:label "e1"@en ;
  rdfs:domain cim:ExcAVR3 ;
  rdfs:range cim:PU ;
  skos:definition "Field voltage value 1 (<i>E</i><i><sub>1</sub></i>).  Typical value = 4,18."@en .

cim:ExcAVR3.e2 a owl:DatatypeProperty ;
  rdfs:label "e2"@en ;
  rdfs:domain cim:ExcAVR3 ;
  rdfs:range cim:PU ;
  skos:definition "Field voltage value 2 (<i>E</i><i><sub>2</sub></i>).  Typical value = 3,14."@en .

cim:ExcAVR3.ka a owl:DatatypeProperty ;
  rdfs:label "ka"@en ;
  rdfs:domain cim:ExcAVR3 ;
  rdfs:range xsd:float ;
  skos:definition "AVR gain (<i>K</i><i><sub>A</sub></i>).  Typical value = 100."@en .

cim:ExcAVR3.se1 a owl:DatatypeProperty ;
  rdfs:label "se1"@en ;
  rdfs:domain cim:ExcAVR3 ;
  rdfs:range xsd:float ;
  skos:definition "Saturation factor at <i>E</i><i><sub>1</sub></i><i> </i>(<i>S[E</i><i><sub>1</sub></i><i>]</i>).  Typical value = 0,1."@en .

cim:ExcAVR3.se2 a owl:DatatypeProperty ;
  rdfs:label "se2"@en ;
  rdfs:domain cim:ExcAVR3 ;
  rdfs:range xsd:float ;
  skos:definition "Saturation factor at <i>E</i><i><sub>2</sub></i><i> </i>(<i>S[E</i><i><sub>2</sub></i><i>]</i>).  Typical value = 0,03."@en .

cim:ExcAVR3.t1 a owl:DatatypeProperty ;
  rdfs:label "t1"@en ;
  rdfs:domain cim:ExcAVR3 ;
  rdfs:range cim:Seconds ;
  skos:definition "AVR time constant (<i>T</i><i><sub>1</sub></i>) (&gt;= 0).  Typical value = 20."@en .

cim:ExcAVR3.t2 a owl:DatatypeProperty ;
  rdfs:label "t2"@en ;
  rdfs:domain cim:ExcAVR3 ;
  rdfs:range cim:Seconds ;
  skos:definition "AVR time constant (<i>T</i><i><sub>2</sub></i>) (&gt;= 0).  Typical value = 1,6."@en .

cim:ExcAVR3.t3 a owl:DatatypeProperty ;
  rdfs:label "t3"@en ;
  rdfs:domain cim:ExcAVR3 ;
  rdfs:range cim:Seconds ;
  skos:definition "AVR time constant (<i>T</i><i><sub>3</sub></i>) (&gt;= 0).  Typical value = 0,66."@en .

cim:ExcAVR3.t4 a owl:DatatypeProperty ;
  rdfs:label "t4"@en ;
  rdfs:domain cim:ExcAVR3 ;
  rdfs:range cim:Seconds ;
  skos:definition "AVR time constant (<i>T</i><i><sub>4</sub></i>) (&gt;= 0).  Typical value = 0,07."@en .

cim:ExcAVR3.te a owl:DatatypeProperty ;
  rdfs:label "te"@en ;
  rdfs:domain cim:ExcAVR3 ;
  rdfs:range cim:Seconds ;
  skos:definition "Exciter time constant (<i>T</i><i><sub>E</sub></i>) (&gt;= 0).  Typical value = 1."@en .

cim:ExcAVR3.vrmn a owl:DatatypeProperty ;
  rdfs:label "vrmn"@en ;
  rdfs:domain cim:ExcAVR3 ;
  rdfs:range cim:PU ;
  skos:definition "Minimum AVR output (<i>V</i><i><sub>RMN</sub></i>).  Typical value = -7,5."@en .

cim:ExcAVR3.vrmx a owl:DatatypeProperty ;
  rdfs:label "vrmx"@en ;
  rdfs:domain cim:ExcAVR3 ;
  rdfs:range cim:PU ;
  skos:definition "Maximum AVR output (<i>V</i><i><sub>RMX</sub></i>).  Typical value = 7,5."@en .

cim:ExcAVR4.imul a owl:DatatypeProperty ;
  rdfs:label "imul"@en ;
  rdfs:domain cim:ExcAVR4 ;
  rdfs:range xsd:boolean ;
  skos:definition """
AVR output voltage dependency selector (<i>I</i><i><sub>MUL</sub></i>).
true = selector is connected
false = selector is not connected.
Typical value = true.
\t"""@en .

cim:ExcAVR4.ka a owl:DatatypeProperty ;
  rdfs:label "ka"@en ;
  rdfs:domain cim:ExcAVR4 ;
  rdfs:range xsd:float ;
  skos:definition "AVR gain (<i>K</i><i><sub>A</sub></i>).  Typical value = 300."@en .

cim:ExcAVR4.ke a owl:DatatypeProperty ;
  rdfs:label "ke"@en ;
  rdfs:domain cim:ExcAVR4 ;
  rdfs:range xsd:float ;
  skos:definition "Exciter gain (<i>K</i><i><sub>E</sub></i><i>)</i>.  Typical value = 1."@en .

cim:ExcAVR4.kif a owl:DatatypeProperty ;
  rdfs:label "kif"@en ;
  rdfs:domain cim:ExcAVR4 ;
  rdfs:range xsd:float ;
  skos:definition "Exciter internal reactance (<i>K</i><i><sub>IF</sub></i>).  Typical value = 0."@en .

cim:ExcAVR4.t1 a owl:DatatypeProperty ;
  rdfs:label "t1"@en ;
  rdfs:domain cim:ExcAVR4 ;
  rdfs:range cim:Seconds ;
  skos:definition "AVR time constant (<i>T</i><i><sub>1</sub></i>) (&gt;= 0).  Typical value = 4,8."@en .

cim:ExcAVR4.t1if a owl:DatatypeProperty ;
  rdfs:label "t1if"@en ;
  rdfs:domain cim:ExcAVR4 ;
  rdfs:range cim:Seconds ;
  skos:definition "Exciter current feedback time constant (<i>T</i><i><sub>1IF</sub></i>) (&gt;= 0).  Typical value = 60."@en .

cim:ExcAVR4.t2 a owl:DatatypeProperty ;
  rdfs:label "t2"@en ;
  rdfs:domain cim:ExcAVR4 ;
  rdfs:range cim:Seconds ;
  skos:definition "AVR time constant (<i>T</i><i><sub>2</sub></i>) (&gt;= 0).  Typical value = 1,5."@en .

cim:ExcAVR4.t3 a owl:DatatypeProperty ;
  rdfs:label "t3"@en ;
  rdfs:domain cim:ExcAVR4 ;
  rdfs:range cim:Seconds ;
  skos:definition "AVR time constant (<i>T</i><i><sub>3</sub></i>) (&gt;= 0).  Typical value = 0."@en .

cim:ExcAVR4.t4 a owl:DatatypeProperty ;
  rdfs:label "t4"@en ;
  rdfs:domain cim:ExcAVR4 ;
  rdfs:range cim:Seconds ;
  skos:definition "AVR time constant (<i>T</i><i><sub>4</sub></i>) (&gt;= 0).  Typical value = 0."@en .

cim:ExcAVR4.tif a owl:DatatypeProperty ;
  rdfs:label "tif"@en ;
  rdfs:domain cim:ExcAVR4 ;
  rdfs:range cim:Seconds ;
  skos:definition "Exciter current feedback time constant (<i>T</i><i><sub>IF</sub></i>) (&gt;= 0).  Typical value = 0."@en .

cim:ExcAVR4.vfmn a owl:DatatypeProperty ;
  rdfs:label "vfmn"@en ;
  rdfs:domain cim:ExcAVR4 ;
  rdfs:range cim:PU ;
  skos:definition "Minimum exciter output (<i>V</i><i><sub>FMN</sub></i>).  Typical value = 0."@en .

cim:ExcAVR4.vfmx a owl:DatatypeProperty ;
  rdfs:label "vfmx"@en ;
  rdfs:domain cim:ExcAVR4 ;
  rdfs:range cim:PU ;
  skos:definition "Maximum exciter output (<i>V</i><i><sub>FMX</sub></i>).  Typical value = 5."@en .

cim:ExcAVR4.vrmn a owl:DatatypeProperty ;
  rdfs:label "vrmn"@en ;
  rdfs:domain cim:ExcAVR4 ;
  rdfs:range cim:PU ;
  skos:definition "Minimum AVR output (<i>V</i><i><sub>RMN</sub></i>).  Typical value = 0."@en .

cim:ExcAVR4.vrmx a owl:DatatypeProperty ;
  rdfs:label "vrmx"@en ;
  rdfs:domain cim:ExcAVR4 ;
  rdfs:range cim:PU ;
  skos:definition "Maximum AVR output (<i>V</i><i><sub>RMX</sub></i>).  Typical value = 5."@en .

cim:ExcAVR5.ka a owl:DatatypeProperty ;
  rdfs:label "ka"@en ;
  rdfs:domain cim:ExcAVR5 ;
  rdfs:range cim:PU ;
  skos:definition "Gain (<i>Ka</i>)."@en .

cim:ExcAVR5.rex a owl:DatatypeProperty ;
  rdfs:label "rex"@en ;
  rdfs:domain cim:ExcAVR5 ;
  rdfs:range cim:PU ;
  skos:definition "Effective output resistance (<i>Rex</i>). <i>Rex</i> represents the effective output resistance seen by the excitation system."@en .

cim:ExcAVR5.ta a owl:DatatypeProperty ;
  rdfs:label "ta"@en ;
  rdfs:domain cim:ExcAVR5 ;
  rdfs:range cim:Seconds ;
  skos:definition "Time constant (<i>Ta</i>) (&gt;= 0)."@en .

cim:ExcAVR7.a1 a owl:DatatypeProperty ;
  rdfs:label "a1"@en ;
  rdfs:domain cim:ExcAVR7 ;
  rdfs:range cim:PU ;
  skos:definition "Lead coefficient (<i>A</i><i><sub>1</sub></i>).  Typical value = 0,5."@en .

cim:ExcAVR7.a2 a owl:DatatypeProperty ;
  rdfs:label "a2"@en ;
  rdfs:domain cim:ExcAVR7 ;
  rdfs:range cim:PU ;
  skos:definition "Lag coefficient (<i>A</i><i><sub>2</sub></i>).  Typical value = 0,5."@en .

cim:ExcAVR7.a3 a owl:DatatypeProperty ;
  rdfs:label "a3"@en ;
  rdfs:domain cim:ExcAVR7 ;
  rdfs:range cim:PU ;
  skos:definition "Lead coefficient (<i>A</i><i><sub>3</sub></i>).  Typical value = 0,5."@en .

cim:ExcAVR7.a4 a owl:DatatypeProperty ;
  rdfs:label "a4"@en ;
  rdfs:domain cim:ExcAVR7 ;
  rdfs:range cim:PU ;
  skos:definition "Lag coefficient (<i>A</i><i><sub>4</sub></i>).  Typical value = 0,5."@en .

cim:ExcAVR7.a5 a owl:DatatypeProperty ;
  rdfs:label "a5"@en ;
  rdfs:domain cim:ExcAVR7 ;
  rdfs:range cim:PU ;
  skos:definition "Lead coefficient (<i>A</i><i><sub>5</sub></i>).  Typical value = 0,5."@en .

cim:ExcAVR7.a6 a owl:DatatypeProperty ;
  rdfs:label "a6"@en ;
  rdfs:domain cim:ExcAVR7 ;
  rdfs:range cim:PU ;
  skos:definition "Lag coefficient (<i>A</i><i><sub>6</sub></i>).  Typical value = 0,5."@en .

cim:ExcAVR7.k1 a owl:DatatypeProperty ;
  rdfs:label "k1"@en ;
  rdfs:domain cim:ExcAVR7 ;
  rdfs:range cim:PU ;
  skos:definition "Gain (<i>K</i><i><sub>1</sub></i>).  Typical value = 1."@en .

cim:ExcAVR7.k3 a owl:DatatypeProperty ;
  rdfs:label "k3"@en ;
  rdfs:domain cim:ExcAVR7 ;
  rdfs:range cim:PU ;
  skos:definition "Gain (<i>K</i><i><sub>3</sub></i>).  Typical value = 3."@en .

cim:ExcAVR7.k5 a owl:DatatypeProperty ;
  rdfs:label "k5"@en ;
  rdfs:domain cim:ExcAVR7 ;
  rdfs:range cim:PU ;
  skos:definition "Gain (<i>K</i><i><sub>5</sub></i>).  Typical value = 1."@en .

cim:ExcAVR7.t1 a owl:DatatypeProperty ;
  rdfs:label "t1"@en ;
  rdfs:domain cim:ExcAVR7 ;
  rdfs:range cim:Seconds ;
  skos:definition "Lead time constant (<i>T</i><i><sub>1</sub></i>) (&gt;= 0).  Typical value = 0,05."@en .

cim:ExcAVR7.t2 a owl:DatatypeProperty ;
  rdfs:label "t2"@en ;
  rdfs:domain cim:ExcAVR7 ;
  rdfs:range cim:Seconds ;
  skos:definition "Lag time constant (<i>T</i><i><sub>2</sub></i>) (&gt;= 0).  Typical value = 0,1."@en .

cim:ExcAVR7.t3 a owl:DatatypeProperty ;
  rdfs:label "t3"@en ;
  rdfs:domain cim:ExcAVR7 ;
  rdfs:range cim:Seconds ;
  skos:definition "Lead time constant (<i>T</i><i><sub>3</sub></i>) (&gt;= 0).  Typical value = 0,1."@en .

cim:ExcAVR7.t4 a owl:DatatypeProperty ;
  rdfs:label "t4"@en ;
  rdfs:domain cim:ExcAVR7 ;
  rdfs:range cim:Seconds ;
  skos:definition "Lag time constant (<i>T</i><i><sub>4</sub></i>) (&gt;= 0).  Typical value = 0,1."@en .

cim:ExcAVR7.t5 a owl:DatatypeProperty ;
  rdfs:label "t5"@en ;
  rdfs:domain cim:ExcAVR7 ;
  rdfs:range cim:Seconds ;
  skos:definition "Lead time constant (<i>T</i><i><sub>5</sub></i>) (&gt;= 0).  Typical value = 0,1."@en .

cim:ExcAVR7.t6 a owl:DatatypeProperty ;
  rdfs:label "t6"@en ;
  rdfs:domain cim:ExcAVR7 ;
  rdfs:range cim:Seconds ;
  skos:definition "Lag time constant (<i>T</i><i><sub>6</sub></i>) (&gt;= 0).  Typical value = 0,1."@en .

cim:ExcAVR7.vmax1 a owl:DatatypeProperty ;
  rdfs:label "vmax1"@en ;
  rdfs:domain cim:ExcAVR7 ;
  rdfs:range cim:PU ;
  skos:definition "Lead-lag maximum limit (<i>Vmax1</i>) (&gt; ExcAVR7.vmin1).  Typical value = 5."@en .

cim:ExcAVR7.vmax3 a owl:DatatypeProperty ;
  rdfs:label "vmax3"@en ;
  rdfs:domain cim:ExcAVR7 ;
  rdfs:range cim:PU ;
  skos:definition "Lead-lag maximum limit (<i>Vmax3</i>) (&gt; ExcAVR7.vmin3).  Typical value = 5."@en .

cim:ExcAVR7.vmax5 a owl:DatatypeProperty ;
  rdfs:label "vmax5"@en ;
  rdfs:domain cim:ExcAVR7 ;
  rdfs:range cim:PU ;
  skos:definition "Lead-lag maximum limit (<i>Vmax5</i>) (&gt; ExcAVR7.vmin5).  Typical value = 5."@en .

cim:ExcAVR7.vmin1 a owl:DatatypeProperty ;
  rdfs:label "vmin1"@en ;
  rdfs:domain cim:ExcAVR7 ;
  rdfs:range cim:PU ;
  skos:definition "Lead-lag minimum limit (<i>Vmin1</i>) (&lt; ExcAVR7.vmax1).  Typical value = -5."@en .

cim:ExcAVR7.vmin3 a owl:DatatypeProperty ;
  rdfs:label "vmin3"@en ;
  rdfs:domain cim:ExcAVR7 ;
  rdfs:range cim:PU ;
  skos:definition "Lead-lag minimum limit (<i>Vmin3</i>) (&lt; ExcAVR7.vmax3).  Typical value = -5."@en .

cim:ExcAVR7.vmin5 a owl:DatatypeProperty ;
  rdfs:label "vmin5"@en ;
  rdfs:domain cim:ExcAVR7 ;
  rdfs:range cim:PU ;
  skos:definition "Lead-lag minimum limit (<i>Vmin5</i>) (&lt; ExcAVR7.vmax5).  Typical value = -2."@en .

cim:ExcBBC.efdmax a owl:DatatypeProperty ;
  rdfs:label "efdmax"@en ;
  rdfs:domain cim:ExcBBC ;
  rdfs:range cim:PU ;
  skos:definition "Maximum open circuit exciter voltage (<i>Efdmax</i>) (&gt; ExcBBC.efdmin).  Typical value = 5."@en .

cim:ExcBBC.efdmin a owl:DatatypeProperty ;
  rdfs:label "efdmin"@en ;
  rdfs:domain cim:ExcBBC ;
  rdfs:range cim:PU ;
  skos:definition "Minimum open circuit exciter voltage (<i>Efdmin</i>) (&lt; ExcBBC.efdmax).  Typical value = -5."@en .

cim:ExcBBC.k a owl:DatatypeProperty ;
  rdfs:label "k"@en ;
  rdfs:domain cim:ExcBBC ;
  rdfs:range cim:PU ;
  skos:definition "Steady state gain (<i>K</i>) (not = 0).  Typical value = 300."@en .

cim:ExcBBC.switch a owl:DatatypeProperty ;
  rdfs:label "switch"@en ;
  rdfs:domain cim:ExcBBC ;
  rdfs:range xsd:boolean ;
  skos:definition """
Supplementary signal routing selector (<i>switch</i>).
true = <i>Vs</i> connected to 3rd summing point
false =  <i>Vs</i> connected to 1st summing point (see diagram).
Typical value = false.
\t"""@en .

cim:ExcBBC.t1 a owl:DatatypeProperty ;
  rdfs:label "t1"@en ;
  rdfs:domain cim:ExcBBC ;
  rdfs:range cim:Seconds ;
  skos:definition "Controller time constant (<i>T1</i>) (&gt;= 0).  Typical value = 6."@en .

cim:ExcBBC.t2 a owl:DatatypeProperty ;
  rdfs:label "t2"@en ;
  rdfs:domain cim:ExcBBC ;
  rdfs:range cim:Seconds ;
  skos:definition "Controller time constant (<i>T2</i>) (&gt;= 0).  Typical value = 1."@en .

cim:ExcBBC.t3 a owl:DatatypeProperty ;
  rdfs:label "t3"@en ;
  rdfs:domain cim:ExcBBC ;
  rdfs:range cim:Seconds ;
  skos:definition "Lead/lag time constant (<i>T3</i>) (&gt;= 0).  If = 0, block is bypassed.  Typical value = 0,05."@en .

cim:ExcBBC.t4 a owl:DatatypeProperty ;
  rdfs:label "t4"@en ;
  rdfs:domain cim:ExcBBC ;
  rdfs:range cim:Seconds ;
  skos:definition "Lead/lag time constant (<i>T4</i>) (&gt;= 0).  If = 0, block is bypassed.  Typical value = 0,01."@en .

cim:ExcBBC.vrmax a owl:DatatypeProperty ;
  rdfs:label "vrmax"@en ;
  rdfs:domain cim:ExcBBC ;
  rdfs:range cim:PU ;
  skos:definition "Maximum control element output (<i>Vrmax</i>) (&gt; ExcBBC.vrmin).  Typical value = 5."@en .

cim:ExcBBC.vrmin a owl:DatatypeProperty ;
  rdfs:label "vrmin"@en ;
  rdfs:domain cim:ExcBBC ;
  rdfs:range cim:PU ;
  skos:definition "Minimum control element output (<i>Vrmin</i>) (&lt; ExcBBC.vrmax).  Typical value = -5."@en .

cim:ExcBBC.xe a owl:DatatypeProperty ;
  rdfs:label "xe"@en ;
  rdfs:domain cim:ExcBBC ;
  rdfs:range cim:PU ;
  skos:definition "Effective excitation transformer reactance (<i>Xe</i>) (&gt;= 0).  <i>Xe</i> models the regulation of the transformer/rectifier unit.  Typical value = 0,05."@en .

cim:ExcCZ.efdmax a owl:DatatypeProperty ;
  rdfs:label "efdmax"@en ;
  rdfs:domain cim:ExcCZ ;
  rdfs:range cim:PU ;
  skos:definition "Exciter output maximum limit (<i>Efdmax</i>) (&gt; ExcCZ.efdmin)."@en .

cim:ExcCZ.efdmin a owl:DatatypeProperty ;
  rdfs:label "efdmin"@en ;
  rdfs:domain cim:ExcCZ ;
  rdfs:range cim:PU ;
  skos:definition "Exciter output minimum limit (<i>Efdmin</i>) (&lt; ExcCZ.efdmax). "@en .

cim:ExcCZ.ka a owl:DatatypeProperty ;
  rdfs:label "ka"@en ;
  rdfs:domain cim:ExcCZ ;
  rdfs:range cim:PU ;
  skos:definition "Regulator gain (<i>Ka</i>)."@en .

cim:ExcCZ.ke a owl:DatatypeProperty ;
  rdfs:label "ke"@en ;
  rdfs:domain cim:ExcCZ ;
  rdfs:range cim:PU ;
  skos:definition "Exciter constant related to self-excited field (<i>Ke</i>)."@en .

cim:ExcCZ.kp a owl:DatatypeProperty ;
  rdfs:label "kp"@en ;
  rdfs:domain cim:ExcCZ ;
  rdfs:range cim:PU ;
  skos:definition "Regulator proportional gain (<i>Kp</i>)."@en .

cim:ExcCZ.ta a owl:DatatypeProperty ;
  rdfs:label "ta"@en ;
  rdfs:domain cim:ExcCZ ;
  rdfs:range cim:Seconds ;
  skos:definition "Regulator time constant (<i>Ta</i>) (&gt;= 0)."@en .

cim:ExcCZ.tc a owl:DatatypeProperty ;
  rdfs:label "tc"@en ;
  rdfs:domain cim:ExcCZ ;
  rdfs:range cim:Seconds ;
  skos:definition "Regulator integral time constant (<i>Tc</i>) (&gt;= 0). "@en .

cim:ExcCZ.te a owl:DatatypeProperty ;
  rdfs:label "te"@en ;
  rdfs:domain cim:ExcCZ ;
  rdfs:range cim:Seconds ;
  skos:definition "Exciter time constant, integration rate associated with exciter control (<i>Te</i>) (&gt;= 0)."@en .

cim:ExcCZ.vrmax a owl:DatatypeProperty ;
  rdfs:label "vrmax"@en ;
  rdfs:domain cim:ExcCZ ;
  rdfs:range cim:PU ;
  skos:definition "Voltage regulator maximum limit (<i>Vrmax</i>) (&gt; ExcCZ.vrmin). "@en .

cim:ExcCZ.vrmin a owl:DatatypeProperty ;
  rdfs:label "vrmin"@en ;
  rdfs:domain cim:ExcCZ ;
  rdfs:range cim:PU ;
  skos:definition "Voltage regulator minimum limit (<i>Vrmin</i>) (&lt; ExcCZ.vrmax). "@en .

cim:ExcDC1A.efd1 a owl:DatatypeProperty ;
  rdfs:label "efd1"@en ;
  rdfs:domain cim:ExcDC1A ;
  rdfs:range cim:PU ;
  skos:definition "Exciter voltage at which exciter saturation is defined (<i>Efd</i><i><sub>1</sub></i>) (&gt; 0).  Typical value = 3,1."@en .

cim:ExcDC1A.efd2 a owl:DatatypeProperty ;
  rdfs:label "efd2"@en ;
  rdfs:domain cim:ExcDC1A ;
  rdfs:range cim:PU ;
  skos:definition "Exciter voltage at which exciter saturation is defined (<i>Efd</i><i><sub>2</sub></i>) (&gt; 0).  Typical value = 2,3."@en .

cim:ExcDC1A.efdmax a owl:DatatypeProperty ;
  rdfs:label "efdmax"@en ;
  rdfs:domain cim:ExcDC1A ;
  rdfs:range cim:PU ;
  skos:definition "Maximum voltage exciter output limiter (<i>Efdmax</i>) (&gt; ExcDC1A.efdmin).  Typical value = 99."@en .

cim:ExcDC1A.efdmin a owl:DatatypeProperty ;
  rdfs:label "efdmin"@en ;
  rdfs:domain cim:ExcDC1A ;
  rdfs:range cim:PU ;
  skos:definition "Minimum voltage exciter output limiter (<i>Efdmin</i>) (&lt; ExcDC1A.edfmax).  Typical value = -99."@en .

cim:ExcDC1A.exclim a owl:DatatypeProperty ;
  rdfs:label "exclim"@en ;
  rdfs:domain cim:ExcDC1A ;
  rdfs:range xsd:boolean ;
  skos:definition """
(<i>exclim</i>).  IEEE standard is ambiguous about lower limit on exciter output. 
true = a lower limit of zero is applied to integrator output
false = a lower limit of zero is not applied to integrator output.
Typical value = true.
\t"""@en .

cim:ExcDC1A.ka a owl:DatatypeProperty ;
  rdfs:label "ka"@en ;
  rdfs:domain cim:ExcDC1A ;
  rdfs:range cim:PU ;
  skos:definition "Voltage regulator gain (<i>Ka</i>) (&gt; 0).  Typical value = 46."@en .

cim:ExcDC1A.ke a owl:DatatypeProperty ;
  rdfs:label "ke"@en ;
  rdfs:domain cim:ExcDC1A ;
  rdfs:range cim:PU ;
  skos:definition "Exciter constant related to self-excited field (<i>Ke</i>).  Typical value = 0."@en .

cim:ExcDC1A.kf a owl:DatatypeProperty ;
  rdfs:label "kf"@en ;
  rdfs:domain cim:ExcDC1A ;
  rdfs:range cim:PU ;
  skos:definition "Excitation control system stabilizer gain (<i>Kf</i>) (&gt;= 0).  Typical value = 0,1."@en .

cim:ExcDC1A.ks a owl:DatatypeProperty ;
  rdfs:label "ks"@en ;
  rdfs:domain cim:ExcDC1A ;
  rdfs:range cim:PU ;
  skos:definition "Coefficient to allow different usage of the model-speed coefficient (<i>Ks</i>).  Typical value = 0."@en .

cim:ExcDC1A.seefd1 a owl:DatatypeProperty ;
  rdfs:label "seefd1"@en ;
  rdfs:domain cim:ExcDC1A ;
  rdfs:range xsd:float ;
  skos:definition "Exciter saturation function value at the corresponding exciter voltage, <i>Efd</i><i><sub>1</sub></i> (<i>Se[Eefd</i><i><sub>1</sub></i><i>]</i>) (&gt;= 0).  Typical value = 0,33."@en .

cim:ExcDC1A.seefd2 a owl:DatatypeProperty ;
  rdfs:label "seefd2"@en ;
  rdfs:domain cim:ExcDC1A ;
  rdfs:range xsd:float ;
  skos:definition "Exciter saturation function value at the corresponding exciter voltage, <i>Efd</i><i><sub>2</sub></i> (<i>Se[Eefd</i><i><sub>2</sub></i><i>]</i>) (&gt;= 0).  Typical value = 0,1."@en .

cim:ExcDC1A.ta a owl:DatatypeProperty ;
  rdfs:label "ta"@en ;
  rdfs:domain cim:ExcDC1A ;
  rdfs:range cim:Seconds ;
  skos:definition "Voltage regulator time constant (<i>Ta</i>) (&gt; 0).  Typical value = 0,06."@en .

cim:ExcDC1A.tb a owl:DatatypeProperty ;
  rdfs:label "tb"@en ;
  rdfs:domain cim:ExcDC1A ;
  rdfs:range cim:Seconds ;
  skos:definition "Voltage regulator time constant (<i>Tb</i>) (&gt;= 0).  Typical value = 0."@en .

cim:ExcDC1A.tc a owl:DatatypeProperty ;
  rdfs:label "tc"@en ;
  rdfs:domain cim:ExcDC1A ;
  rdfs:range cim:Seconds ;
  skos:definition "Voltage regulator time constant (<i>Tc</i>) (&gt;= 0).  Typical value = 0."@en .

cim:ExcDC1A.te a owl:DatatypeProperty ;
  rdfs:label "te"@en ;
  rdfs:domain cim:ExcDC1A ;
  rdfs:range cim:Seconds ;
  skos:definition "Exciter time constant, integration rate associated with exciter control (<i>Te</i>) (&gt; 0).  Typical value = 0,46."@en .

cim:ExcDC1A.tf a owl:DatatypeProperty ;
  rdfs:label "tf"@en ;
  rdfs:domain cim:ExcDC1A ;
  rdfs:range cim:Seconds ;
  skos:definition "Excitation control system stabilizer time constant (<i>Tf</i>) (&gt; 0).  Typical value = 1."@en .

cim:ExcDC1A.vrmax a owl:DatatypeProperty ;
  rdfs:label "vrmax"@en ;
  rdfs:domain cim:ExcDC1A ;
  rdfs:range cim:PU ;
  skos:definition "Maximum voltage regulator output (<i>Vrmax</i>) (&gt; ExcDC1A.vrmin).  Typical value = 1."@en .

cim:ExcDC1A.vrmin a owl:DatatypeProperty ;
  rdfs:label "vrmin"@en ;
  rdfs:domain cim:ExcDC1A ;
  rdfs:range cim:PU ;
  skos:definition "Minimum voltage regulator output (<i>Vrmin</i>) (&lt; 0 and &lt; ExcDC1A.vrmax).  Typical value = -0,9."@en .

cim:ExcDC2A.efd1 a owl:DatatypeProperty ;
  rdfs:label "efd1"@en ;
  rdfs:domain cim:ExcDC2A ;
  rdfs:range cim:PU ;
  skos:definition "Exciter voltage at which exciter saturation is defined (<i>Efd</i><i><sub>1</sub></i>) (&gt; 0).  Typical value = 3,05."@en .

cim:ExcDC2A.efd2 a owl:DatatypeProperty ;
  rdfs:label "efd2"@en ;
  rdfs:domain cim:ExcDC2A ;
  rdfs:range cim:PU ;
  skos:definition "Exciter voltage at which exciter saturation is defined (<i>Efd</i><i><sub>2</sub></i>) (&gt; 0).  Typical value = 2,29."@en .

cim:ExcDC2A.exclim a owl:DatatypeProperty ;
  rdfs:label "exclim"@en ;
  rdfs:domain cim:ExcDC2A ;
  rdfs:range xsd:boolean ;
  skos:definition """
(<i>exclim</i>).  IEEE standard is ambiguous about lower limit on exciter output.
true = a lower limit of zero is applied to integrator output
false = a lower limit of zero is not applied to integrator output.
Typical value = true.
\t"""@en .

cim:ExcDC2A.ka a owl:DatatypeProperty ;
  rdfs:label "ka"@en ;
  rdfs:domain cim:ExcDC2A ;
  rdfs:range cim:PU ;
  skos:definition "Voltage regulator gain (<i>Ka</i>) (&gt; 0).  Typical value = 300."@en .

cim:ExcDC2A.ke a owl:DatatypeProperty ;
  rdfs:label "ke"@en ;
  rdfs:domain cim:ExcDC2A ;
  rdfs:range cim:PU ;
  skos:definition "Exciter constant related to self-excited field (<i>Ke</i>).  If <i>Ke</i> is entered as zero, the model calculates an effective value of <i>Ke</i> such that the initial condition value of <i>Vr</i> is zero. The zero value of <i>Ke</i> is not changed.  If <i>Ke</i> is entered as non-zero, its value is used directly, without change.  Typical value = 1."@en .

cim:ExcDC2A.kf a owl:DatatypeProperty ;
  rdfs:label "kf"@en ;
  rdfs:domain cim:ExcDC2A ;
  rdfs:range cim:PU ;
  skos:definition "Excitation control system stabilizer gain (<i>Kf</i>) (&gt;= 0).  Typical value = 0,1."@en .

cim:ExcDC2A.ks a owl:DatatypeProperty ;
  rdfs:label "ks"@en ;
  rdfs:domain cim:ExcDC2A ;
  rdfs:range cim:PU ;
  skos:definition "Coefficient to allow different usage of the model-speed coefficient (<i>Ks</i>).  Typical value = 0."@en .

cim:ExcDC2A.seefd1 a owl:DatatypeProperty ;
  rdfs:label "seefd1"@en ;
  rdfs:domain cim:ExcDC2A ;
  rdfs:range xsd:float ;
  skos:definition "Exciter saturation function value at the corresponding exciter voltage, <i>Efd</i><i><sub>1</sub></i> (<i>Se[Efd</i><i><sub>1</sub></i><i>]</i>) (&gt;= 0).  Typical value = 0,279."@en .

cim:ExcDC2A.seefd2 a owl:DatatypeProperty ;
  rdfs:label "seefd2"@en ;
  rdfs:domain cim:ExcDC2A ;
  rdfs:range xsd:float ;
  skos:definition "Exciter saturation function value at the corresponding exciter voltage, <i>Efd</i><i><sub>2</sub></i> (<i>Se[Efd</i><i><sub>2</sub></i><i>]</i>) (&gt;= 0).  Typical value = 0,117."@en .

cim:ExcDC2A.ta a owl:DatatypeProperty ;
  rdfs:label "ta"@en ;
  rdfs:domain cim:ExcDC2A ;
  rdfs:range cim:Seconds ;
  skos:definition "Voltage regulator time constant (<i>Ta</i>) (&gt; 0).  Typical value = 0,01."@en .

cim:ExcDC2A.tb a owl:DatatypeProperty ;
  rdfs:label "tb"@en ;
  rdfs:domain cim:ExcDC2A ;
  rdfs:range cim:Seconds ;
  skos:definition "Voltage regulator time constant (<i>Tb</i>) (&gt;= 0).  Typical value = 0."@en .

cim:ExcDC2A.tc a owl:DatatypeProperty ;
  rdfs:label "tc"@en ;
  rdfs:domain cim:ExcDC2A ;
  rdfs:range cim:Seconds ;
  skos:definition "Voltage regulator time constant (<i>Tc</i>) (&gt;= 0).  Typical value = 0."@en .

cim:ExcDC2A.te a owl:DatatypeProperty ;
  rdfs:label "te"@en ;
  rdfs:domain cim:ExcDC2A ;
  rdfs:range cim:Seconds ;
  skos:definition "Exciter time constant, integration rate associated with exciter control (<i>Te</i>) (&gt; 0).  Typical value = 1,33."@en .

cim:ExcDC2A.tf a owl:DatatypeProperty ;
  rdfs:label "tf"@en ;
  rdfs:domain cim:ExcDC2A ;
  rdfs:range cim:Seconds ;
  skos:definition "Excitation control system stabilizer time constant (<i>Tf</i>) (&gt; 0).  Typical value = 0,675."@en .

cim:ExcDC2A.tf1 a owl:DatatypeProperty ;
  rdfs:label "tf1"@en ;
  rdfs:domain cim:ExcDC2A ;
  rdfs:range cim:Seconds ;
  skos:definition "Excitation control system stabilizer time constant (<i>Tf1</i>) (&gt;= 0).  Typical value = 0."@en .

cim:ExcDC2A.vrmax a owl:DatatypeProperty ;
  rdfs:label "vrmax"@en ;
  rdfs:domain cim:ExcDC2A ;
  rdfs:range cim:PU ;
  skos:definition "Maximum voltage regulator output (<i>Vrmax</i>) (&gt; ExcDC2A.vrmin).  Typical value = 4,95."@en .

cim:ExcDC2A.vrmin a owl:DatatypeProperty ;
  rdfs:label "vrmin"@en ;
  rdfs:domain cim:ExcDC2A ;
  rdfs:range cim:PU ;
  skos:definition "Minimum voltage regulator output (<i>Vrmin</i>) (&lt; 0 and &lt; ExcDC2A.vrmax).  Typical value = -4,9."@en .

cim:ExcDC2A.vtlim a owl:DatatypeProperty ;
  rdfs:label "vtlim"@en ;
  rdfs:domain cim:ExcDC2A ;
  rdfs:range xsd:boolean ;
  skos:definition """
(<i>Vtlim</i>).
true = limiter at the block (<i>Ka / [1 + sTa]</i>) is dependent on <i>Vt </i>
false = limiter at the block is not dependent on <i>Vt</i>.
Typical value = true.
\t"""@en .

cim:ExcDC3A.efd1 a owl:DatatypeProperty ;
  rdfs:label "efd1"@en ;
  rdfs:domain cim:ExcDC3A ;
  rdfs:range cim:PU ;
  skos:definition "Exciter voltage at which exciter saturation is defined (<i>Efd</i><i><sub>1</sub></i>) (&gt; 0).  Typical value = 2,6."@en .

cim:ExcDC3A.efd2 a owl:DatatypeProperty ;
  rdfs:label "efd2"@en ;
  rdfs:domain cim:ExcDC3A ;
  rdfs:range cim:PU ;
  skos:definition "Exciter voltage at which exciter saturation is defined (<i>Efd</i><i><sub>2</sub></i>) (&gt; 0).  Typical value = 3,45."@en .

cim:ExcDC3A.efdlim a owl:DatatypeProperty ;
  rdfs:label "efdlim"@en ;
  rdfs:domain cim:ExcDC3A ;
  rdfs:range xsd:boolean ;
  skos:definition """
(<i>Efdlim</i>).
true = exciter output limiter is active
false = exciter output limiter not active.
Typical value = true.
\t"""@en .

cim:ExcDC3A.efdmax a owl:DatatypeProperty ;
  rdfs:label "efdmax"@en ;
  rdfs:domain cim:ExcDC3A ;
  rdfs:range cim:PU ;
  skos:definition "Maximum voltage exciter output limiter (<i>Efdmax</i>) (&gt; ExcDC3A.efdmin).  Typical value = 99."@en .

cim:ExcDC3A.efdmin a owl:DatatypeProperty ;
  rdfs:label "efdmin"@en ;
  rdfs:domain cim:ExcDC3A ;
  rdfs:range cim:PU ;
  skos:definition "Minimum voltage exciter output limiter (<i>Efdmin</i>) (&lt; ExcDC3A.efdmax).  Typical value = -99."@en .

cim:ExcDC3A.exclim a owl:DatatypeProperty ;
  rdfs:label "exclim"@en ;
  rdfs:domain cim:ExcDC3A ;
  rdfs:range xsd:boolean ;
  skos:definition """
(<i>exclim</i>).  IEEE standard is ambiguous about lower limit on exciter output.
true = a lower limit of zero is applied to integrator output
false = a lower limit of zero not applied to integrator output.
Typical value = true.
\t"""@en .

cim:ExcDC3A.ke a owl:DatatypeProperty ;
  rdfs:label "ke"@en ;
  rdfs:domain cim:ExcDC3A ;
  rdfs:range cim:PU ;
  skos:definition "Exciter constant related to self-excited field (<i>Ke</i>).  Typical value = 1."@en .

cim:ExcDC3A.kr a owl:DatatypeProperty ;
  rdfs:label "kr"@en ;
  rdfs:domain cim:ExcDC3A ;
  rdfs:range cim:PU ;
  skos:definition "Deadband (<i>Kr</i>).  Typical value = 0."@en .

cim:ExcDC3A.ks a owl:DatatypeProperty ;
  rdfs:label "ks"@en ;
  rdfs:domain cim:ExcDC3A ;
  rdfs:range cim:PU ;
  skos:definition "Coefficient to allow different usage of the model-speed coefficient (<i>Ks</i>).  Typical value = 0."@en .

cim:ExcDC3A.kv a owl:DatatypeProperty ;
  rdfs:label "kv"@en ;
  rdfs:domain cim:ExcDC3A ;
  rdfs:range cim:PU ;
  skos:definition "Fast raise/lower contact setting (<i>Kv</i>) (&gt; 0).  Typical value = 0,05."@en .

cim:ExcDC3A.seefd1 a owl:DatatypeProperty ;
  rdfs:label "seefd1"@en ;
  rdfs:domain cim:ExcDC3A ;
  rdfs:range xsd:float ;
  skos:definition "Exciter saturation function value at the corresponding exciter voltage, <i>Efd</i><i><sub>1</sub></i> (<i>Se[Efd</i><i><sub>1</sub></i><i>]</i>) (&gt;= 0).  Typical value = 0,1."@en .

cim:ExcDC3A.seefd2 a owl:DatatypeProperty ;
  rdfs:label "seefd2"@en ;
  rdfs:domain cim:ExcDC3A ;
  rdfs:range xsd:float ;
  skos:definition "Exciter saturation function value at the corresponding exciter voltage, <i>Efd</i><i><sub>2</sub></i> (<i>Se[Efd</i><i><sub>2</sub></i><i>]</i>) (&gt;= 0).  Typical value = 0,35."@en .

cim:ExcDC3A.te a owl:DatatypeProperty ;
  rdfs:label "te"@en ;
  rdfs:domain cim:ExcDC3A ;
  rdfs:range cim:Seconds ;
  skos:definition "Exciter time constant, integration rate associated with exciter control (<i>Te</i>) (&gt; 0).  Typical value = 1,83."@en .

cim:ExcDC3A.trh a owl:DatatypeProperty ;
  rdfs:label "trh"@en ;
  rdfs:domain cim:ExcDC3A ;
  rdfs:range cim:Seconds ;
  skos:definition "Rheostat travel time (<i>Trh</i>) (&gt; 0).  Typical value = 20."@en .

cim:ExcDC3A.vrmax a owl:DatatypeProperty ;
  rdfs:label "vrmax"@en ;
  rdfs:domain cim:ExcDC3A ;
  rdfs:range cim:PU ;
  skos:definition "Maximum voltage regulator output (<i>Vrmax</i>) (&gt; 0).  Typical value = 5."@en .

cim:ExcDC3A.vrmin a owl:DatatypeProperty ;
  rdfs:label "vrmin"@en ;
  rdfs:domain cim:ExcDC3A ;
  rdfs:range cim:PU ;
  skos:definition "Minimum voltage regulator output (<i>Vrmin</i>) (&lt;= 0).  Typical value = 0."@en .

cim:ExcDC3A1.exclim a owl:DatatypeProperty ;
  rdfs:label "exclim"@en ;
  rdfs:domain cim:ExcDC3A1 ;
  rdfs:range xsd:boolean ;
  skos:definition """
(<i>exclim</i>).
true = lower limit of zero is applied to integrator output
false = lower limit of zero not applied to integrator output.
Typical value = true.
\t"""@en .

cim:ExcDC3A1.ka a owl:DatatypeProperty ;
  rdfs:label "ka"@en ;
  rdfs:domain cim:ExcDC3A1 ;
  rdfs:range cim:PU ;
  skos:definition "Voltage regulator gain (<i>Ka</i>) (&gt; 0).  Typical value = 300."@en .

cim:ExcDC3A1.ke a owl:DatatypeProperty ;
  rdfs:label "ke"@en ;
  rdfs:domain cim:ExcDC3A1 ;
  rdfs:range cim:PU ;
  skos:definition "Exciter constant related to self-excited field (<i>Ke</i>).  Typical value = 1."@en .

cim:ExcDC3A1.kf a owl:DatatypeProperty ;
  rdfs:label "kf"@en ;
  rdfs:domain cim:ExcDC3A1 ;
  rdfs:range cim:PU ;
  skos:definition "Excitation control system stabilizer gain (<i>Kf</i>) (&gt;= 0).  Typical value = 0,1."@en .

cim:ExcDC3A1.ki a owl:DatatypeProperty ;
  rdfs:label "ki"@en ;
  rdfs:domain cim:ExcDC3A1 ;
  rdfs:range cim:PU ;
  skos:definition "Potential circuit gain coefficient (<i>Ki</i>) (&gt;= 0).  Typical value = 4,83."@en .

cim:ExcDC3A1.kp a owl:DatatypeProperty ;
  rdfs:label "kp"@en ;
  rdfs:domain cim:ExcDC3A1 ;
  rdfs:range cim:PU ;
  skos:definition "Potential circuit gain coefficient (<i>Kp</i>) (&gt;= 0).  Typical value = 4,37."@en .

cim:ExcDC3A1.ta a owl:DatatypeProperty ;
  rdfs:label "ta"@en ;
  rdfs:domain cim:ExcDC3A1 ;
  rdfs:range cim:Seconds ;
  skos:definition "Voltage regulator time constant (<i>Ta</i>) (&gt; 0).  Typical value = 0,01."@en .

cim:ExcDC3A1.te a owl:DatatypeProperty ;
  rdfs:label "te"@en ;
  rdfs:domain cim:ExcDC3A1 ;
  rdfs:range cim:Seconds ;
  skos:definition "Exciter time constant, integration rate associated with exciter control (<i>Te</i>) (&gt; 0).  Typical value = 1,83."@en .

cim:ExcDC3A1.tf a owl:DatatypeProperty ;
  rdfs:label "tf"@en ;
  rdfs:domain cim:ExcDC3A1 ;
  rdfs:range cim:Seconds ;
  skos:definition "Excitation control system stabilizer time constant (<i>Tf</i>) (&gt;= 0).  Typical value = 0,675."@en .

cim:ExcDC3A1.vb1max a owl:DatatypeProperty ;
  rdfs:label "vb1max"@en ;
  rdfs:domain cim:ExcDC3A1 ;
  rdfs:range cim:PU ;
  skos:definition "Available exciter voltage limiter (<i>Vb1max</i>) (&gt; 0).  Typical value = 11,63."@en .

cim:ExcDC3A1.vblim a owl:DatatypeProperty ;
  rdfs:label "vblim"@en ;
  rdfs:domain cim:ExcDC3A1 ;
  rdfs:range xsd:boolean ;
  skos:definition """
Vb limiter indicator.
true = exciter <i>Vbmax</i> limiter is active
false = <i>Vb1max</i> is active. 
Typical value = true.
\t"""@en .

cim:ExcDC3A1.vbmax a owl:DatatypeProperty ;
  rdfs:label "vbmax"@en ;
  rdfs:domain cim:ExcDC3A1 ;
  rdfs:range cim:PU ;
  skos:definition "Available exciter voltage limiter (<i>Vbmax</i>) (&gt; 0).  Typical value = 11,63."@en .

cim:ExcDC3A1.vrmax a owl:DatatypeProperty ;
  rdfs:label "vrmax"@en ;
  rdfs:domain cim:ExcDC3A1 ;
  rdfs:range cim:PU ;
  skos:definition "Maximum voltage regulator output (<i>Vrmax</i>) (&gt; ExcDC3A1.vrmin).  Typical value = 5."@en .

cim:ExcDC3A1.vrmin a owl:DatatypeProperty ;
  rdfs:label "vrmin"@en ;
  rdfs:domain cim:ExcDC3A1 ;
  rdfs:range cim:PU ;
  skos:definition "Minimum voltage regulator output (<i>Vrmin</i>) (&lt; 0 and &lt; ExcDC3A1.vrmax).  Typical value = 0."@en .

cim:ExcELIN1.dpnf a owl:DatatypeProperty ;
  rdfs:label "dpnf"@en ;
  rdfs:domain cim:ExcELIN1 ;
  rdfs:range cim:PU ;
  skos:definition "Controller follow up deadband (<i>Dpnf</i>).  Typical value = 0."@en .

cim:ExcELIN1.efmax a owl:DatatypeProperty ;
  rdfs:label "efmax"@en ;
  rdfs:domain cim:ExcELIN1 ;
  rdfs:range cim:PU ;
  skos:definition "Maximum open circuit excitation voltage (<i>Efmax</i>) (&gt; ExcELIN1.efmin).  Typical value = 5."@en .

cim:ExcELIN1.efmin a owl:DatatypeProperty ;
  rdfs:label "efmin"@en ;
  rdfs:domain cim:ExcELIN1 ;
  rdfs:range cim:PU ;
  skos:definition "Minimum open circuit excitation voltage (<i>Efmin</i>) (&lt; ExcELIN1.efmax).  Typical value = -5."@en .

cim:ExcELIN1.ks1 a owl:DatatypeProperty ;
  rdfs:label "ks1"@en ;
  rdfs:domain cim:ExcELIN1 ;
  rdfs:range cim:PU ;
  skos:definition "Stabilizer gain 1 (<i>Ks1</i>).  Typical value = 0."@en .

cim:ExcELIN1.ks2 a owl:DatatypeProperty ;
  rdfs:label "ks2"@en ;
  rdfs:domain cim:ExcELIN1 ;
  rdfs:range cim:PU ;
  skos:definition "Stabilizer gain 2 (<i>Ks2</i>).  Typical value = 0."@en .

cim:ExcELIN1.smax a owl:DatatypeProperty ;
  rdfs:label "smax"@en ;
  rdfs:domain cim:ExcELIN1 ;
  rdfs:range cim:PU ;
  skos:definition "Stabilizer limit output (<i>smax</i>).  Typical value = 0,1."@en .

cim:ExcELIN1.tfi a owl:DatatypeProperty ;
  rdfs:label "tfi"@en ;
  rdfs:domain cim:ExcELIN1 ;
  rdfs:range cim:Seconds ;
  skos:definition "Current transducer time constant (<i>Tfi</i>) (&gt;= 0).  Typical value = 0."@en .

cim:ExcELIN1.tnu a owl:DatatypeProperty ;
  rdfs:label "tnu"@en ;
  rdfs:domain cim:ExcELIN1 ;
  rdfs:range cim:Seconds ;
  skos:definition "Controller reset time constant (<i>Tnu</i>) (&gt;= 0).  Typical value = 2."@en .

cim:ExcELIN1.ts1 a owl:DatatypeProperty ;
  rdfs:label "ts1"@en ;
  rdfs:domain cim:ExcELIN1 ;
  rdfs:range cim:Seconds ;
  skos:definition "Stabilizer phase lag time constant (<i>Ts1</i>) (&gt;= 0).  Typical value = 1."@en .

cim:ExcELIN1.ts2 a owl:DatatypeProperty ;
  rdfs:label "ts2"@en ;
  rdfs:domain cim:ExcELIN1 ;
  rdfs:range cim:Seconds ;
  skos:definition "Stabilizer filter time constant (<i>Ts2</i>) (&gt;= 0).  Typical value = 1."@en .

cim:ExcELIN1.tsw a owl:DatatypeProperty ;
  rdfs:label "tsw"@en ;
  rdfs:domain cim:ExcELIN1 ;
  rdfs:range cim:Seconds ;
  skos:definition "Stabilizer parameters (<i>Tsw</i>) (&gt;= 0).  Typical value = 3."@en .

cim:ExcELIN1.vpi a owl:DatatypeProperty ;
  rdfs:label "vpi"@en ;
  rdfs:domain cim:ExcELIN1 ;
  rdfs:range cim:PU ;
  skos:definition "Current controller gain (<i>Vpi</i>).  Typical value = 12,45."@en .

cim:ExcELIN1.vpnf a owl:DatatypeProperty ;
  rdfs:label "vpnf"@en ;
  rdfs:domain cim:ExcELIN1 ;
  rdfs:range cim:PU ;
  skos:definition "Controller follow up gain (<i>Vpnf</i>).  Typical value = 2."@en .

cim:ExcELIN1.vpu a owl:DatatypeProperty ;
  rdfs:label "vpu"@en ;
  rdfs:domain cim:ExcELIN1 ;
  rdfs:range cim:PU ;
  skos:definition "Voltage controller proportional gain (<i>Vpu</i>).  Typical value = 34,5."@en .

cim:ExcELIN1.xe a owl:DatatypeProperty ;
  rdfs:label "xe"@en ;
  rdfs:domain cim:ExcELIN1 ;
  rdfs:range cim:PU ;
  skos:definition "Excitation transformer effective reactance (<i>Xe</i>) (&gt;= 0).  <i>Xe</i> represents the regulation of the transformer/rectifier unit.  Typical value = 0,06."@en .

cim:ExcELIN2.efdbas a owl:DatatypeProperty ;
  rdfs:label "efdbas"@en ;
  rdfs:domain cim:ExcELIN2 ;
  rdfs:range cim:PU ;
  skos:definition "Gain (<i>Efdbas</i>).  Typical value = 0,1."@en .

cim:ExcELIN2.iefmax a owl:DatatypeProperty ;
  rdfs:label "iefmax"@en ;
  rdfs:domain cim:ExcELIN2 ;
  rdfs:range cim:PU ;
  skos:definition "Limiter (<i>I</i><i><sub>efmax</sub></i>) (&gt; ExcELIN2.iefmin).  Typical value = 1."@en .

cim:ExcELIN2.iefmax2 a owl:DatatypeProperty ;
  rdfs:label "iefmax2"@en ;
  rdfs:domain cim:ExcELIN2 ;
  rdfs:range cim:PU ;
  skos:definition "Minimum open circuit excitation voltage (<i>I</i><i><sub>efmax2</sub></i>).  Typical value = -5."@en .

cim:ExcELIN2.iefmin a owl:DatatypeProperty ;
  rdfs:label "iefmin"@en ;
  rdfs:domain cim:ExcELIN2 ;
  rdfs:range cim:PU ;
  skos:definition "Limiter (<i>I</i><i><sub>efmin</sub></i>) (&lt; ExcELIN2.iefmax).  Typical value = 1."@en .

cim:ExcELIN2.k1 a owl:DatatypeProperty ;
  rdfs:label "k1"@en ;
  rdfs:domain cim:ExcELIN2 ;
  rdfs:range cim:PU ;
  skos:definition "Voltage regulator input gain (<i>K1</i>).  Typical value = 0."@en .

cim:ExcELIN2.k1ec a owl:DatatypeProperty ;
  rdfs:label "k1ec"@en ;
  rdfs:domain cim:ExcELIN2 ;
  rdfs:range cim:PU ;
  skos:definition "Voltage regulator input limit (<i>K1ec</i>).  Typical value = 2."@en .

cim:ExcELIN2.k2 a owl:DatatypeProperty ;
  rdfs:label "k2"@en ;
  rdfs:domain cim:ExcELIN2 ;
  rdfs:range cim:PU ;
  skos:definition "Gain (<i>K2</i>).  Typical value = 5."@en .

cim:ExcELIN2.k3 a owl:DatatypeProperty ;
  rdfs:label "k3"@en ;
  rdfs:domain cim:ExcELIN2 ;
  rdfs:range cim:PU ;
  skos:definition "Gain (<i>K3</i>).  Typical value = 0,1."@en .

cim:ExcELIN2.k4 a owl:DatatypeProperty ;
  rdfs:label "k4"@en ;
  rdfs:domain cim:ExcELIN2 ;
  rdfs:range cim:PU ;
  skos:definition "Gain (<i>K4</i>).  Typical value = 0."@en .

cim:ExcELIN2.kd1 a owl:DatatypeProperty ;
  rdfs:label "kd1"@en ;
  rdfs:domain cim:ExcELIN2 ;
  rdfs:range cim:PU ;
  skos:definition "Voltage controller derivative gain (<i>Kd1</i>).  Typical value = 34,5."@en .

cim:ExcELIN2.ke2 a owl:DatatypeProperty ;
  rdfs:label "ke2"@en ;
  rdfs:domain cim:ExcELIN2 ;
  rdfs:range cim:PU ;
  skos:definition "Gain (<i>Ke2</i>).  Typical value = 0,1."@en .

cim:ExcELIN2.ketb a owl:DatatypeProperty ;
  rdfs:label "ketb"@en ;
  rdfs:domain cim:ExcELIN2 ;
  rdfs:range cim:PU ;
  skos:definition "Gain (<i>Ketb</i>).  Typical value = 0,06."@en .

cim:ExcELIN2.pid1max a owl:DatatypeProperty ;
  rdfs:label "pid1max"@en ;
  rdfs:domain cim:ExcELIN2 ;
  rdfs:range cim:PU ;
  skos:definition "Controller follow up gain (<i>PID1max</i>).  Typical value = 2."@en .

cim:ExcELIN2.seve1 a owl:DatatypeProperty ;
  rdfs:label "seve1"@en ;
  rdfs:domain cim:ExcELIN2 ;
  rdfs:range cim:PU ;
  skos:definition "Exciter saturation function value at the corresponding exciter voltage, <i>Ve</i><i><sub>1</sub></i>, back of commutating reactance (<i>Se[Ve</i><i><sub>1</sub></i><i>]</i>) (&gt;= 0).  Typical value = 0."@en .

cim:ExcELIN2.seve2 a owl:DatatypeProperty ;
  rdfs:label "seve2"@en ;
  rdfs:domain cim:ExcELIN2 ;
  rdfs:range cim:PU ;
  skos:definition "Exciter saturation function value at the corresponding exciter voltage, <i>Ve</i><i><sub>2</sub></i>, back of commutating reactance (<i>Se[Ve</i><i><sub>2</sub></i><i>]</i>) (&gt;= 0).  Typical value = 1."@en .

cim:ExcELIN2.tb1 a owl:DatatypeProperty ;
  rdfs:label "tb1"@en ;
  rdfs:domain cim:ExcELIN2 ;
  rdfs:range cim:Seconds ;
  skos:definition "Voltage controller derivative washout time constant (<i>Tb1</i>) (&gt;= 0).  Typical value = 12,45."@en .

cim:ExcELIN2.te a owl:DatatypeProperty ;
  rdfs:label "te"@en ;
  rdfs:domain cim:ExcELIN2 ;
  rdfs:range cim:Seconds ;
  skos:definition "Time constant (<i>Te</i>) (&gt;= 0).  Typical value = 0."@en .

cim:ExcELIN2.te2 a owl:DatatypeProperty ;
  rdfs:label "te2"@en ;
  rdfs:domain cim:ExcELIN2 ;
  rdfs:range cim:Seconds ;
  skos:definition "Time Constant (<i>T</i><i><sub>e2</sub></i>) (&gt;= 0).  Typical value = 1."@en .

cim:ExcELIN2.ti1 a owl:DatatypeProperty ;
  rdfs:label "ti1"@en ;
  rdfs:domain cim:ExcELIN2 ;
  rdfs:range cim:PU ;
  skos:definition "Controller follow up deadband (<i>Ti1</i>).  Typical value = 0."@en .

cim:ExcELIN2.ti3 a owl:DatatypeProperty ;
  rdfs:label "ti3"@en ;
  rdfs:domain cim:ExcELIN2 ;
  rdfs:range cim:Seconds ;
  skos:definition "Time constant (<i>T</i><i><sub>i3</sub></i>) (&gt;= 0).  Typical value = 3."@en .

cim:ExcELIN2.ti4 a owl:DatatypeProperty ;
  rdfs:label "ti4"@en ;
  rdfs:domain cim:ExcELIN2 ;
  rdfs:range cim:Seconds ;
  skos:definition "Time constant (<i>T</i><i><sub>i4</sub></i>) (&gt;= 0).  Typical value = 0."@en .

cim:ExcELIN2.tr4 a owl:DatatypeProperty ;
  rdfs:label "tr4"@en ;
  rdfs:domain cim:ExcELIN2 ;
  rdfs:range cim:Seconds ;
  skos:definition "Time constant (<i>T</i><i><sub>r4</sub></i>) (&gt;= 0).  Typical value = 1."@en .

cim:ExcELIN2.upmax a owl:DatatypeProperty ;
  rdfs:label "upmax"@en ;
  rdfs:domain cim:ExcELIN2 ;
  rdfs:range cim:PU ;
  skos:definition "Limiter (<i>Upmax</i>) (&gt; ExcELIN2.upmin).  Typical value = 3."@en .

cim:ExcELIN2.upmin a owl:DatatypeProperty ;
  rdfs:label "upmin"@en ;
  rdfs:domain cim:ExcELIN2 ;
  rdfs:range cim:PU ;
  skos:definition "Limiter (<i>Upmin</i>) (&lt; ExcELIN2.upmax).  Typical value = 0."@en .

cim:ExcELIN2.ve1 a owl:DatatypeProperty ;
  rdfs:label "ve1"@en ;
  rdfs:domain cim:ExcELIN2 ;
  rdfs:range cim:PU ;
  skos:definition "Exciter alternator output voltages back of commutating reactance at which saturation is defined (<i>Ve</i><i><sub>1</sub></i>) (&gt; 0).  Typical value = 3."@en .

cim:ExcELIN2.ve2 a owl:DatatypeProperty ;
  rdfs:label "ve2"@en ;
  rdfs:domain cim:ExcELIN2 ;
  rdfs:range cim:PU ;
  skos:definition "Exciter alternator output voltages back of commutating reactance at which saturation is defined (<i>Ve</i><i><sub>2</sub></i>) (&gt; 0).  Typical value = 0."@en .

cim:ExcELIN2.xp a owl:DatatypeProperty ;
  rdfs:label "xp"@en ;
  rdfs:domain cim:ExcELIN2 ;
  rdfs:range cim:PU ;
  skos:definition "Excitation transformer effective reactance (<i>Xp</i>).  Typical value = 1."@en .

cim:ExcHU.ae a owl:DatatypeProperty ;
  rdfs:label "ae"@en ;
  rdfs:domain cim:ExcHU ;
  rdfs:range cim:PU ;
  skos:definition "Major loop PI tag gain factor (<i>Ae</i>).  Typical value = 3."@en .

cim:ExcHU.ai a owl:DatatypeProperty ;
  rdfs:label "ai"@en ;
  rdfs:domain cim:ExcHU ;
  rdfs:range cim:PU ;
  skos:definition "Minor loop PI tag gain factor (<i>Ai</i>).  Typical value = 22."@en .

cim:ExcHU.atr a owl:DatatypeProperty ;
  rdfs:label "atr"@en ;
  rdfs:domain cim:ExcHU ;
  rdfs:range cim:PU ;
  skos:definition "AVR constant (<i>Atr</i>).  Typical value = 2,19."@en .

cim:ExcHU.emax a owl:DatatypeProperty ;
  rdfs:label "emax"@en ;
  rdfs:domain cim:ExcHU ;
  rdfs:range cim:PU ;
  skos:definition "Field voltage control signal upper limit on AVR base (<i>Emax</i>) (&gt; ExcHU.emin).  Typical value = 0,996."@en .

cim:ExcHU.emin a owl:DatatypeProperty ;
  rdfs:label "emin"@en ;
  rdfs:domain cim:ExcHU ;
  rdfs:range cim:PU ;
  skos:definition "Field voltage control signal lower limit on AVR base (<i>Emin</i>) (&lt; ExcHU.emax).  Typical value = -0,866."@en .

cim:ExcHU.imax a owl:DatatypeProperty ;
  rdfs:label "imax"@en ;
  rdfs:domain cim:ExcHU ;
  rdfs:range cim:PU ;
  skos:definition "Major loop PI tag output signal upper limit (<i>Imax</i>) (&gt; ExcHU.imin).  Typical value = 2,19."@en .

cim:ExcHU.imin a owl:DatatypeProperty ;
  rdfs:label "imin"@en ;
  rdfs:domain cim:ExcHU ;
  rdfs:range cim:PU ;
  skos:definition "Major loop PI tag output signal lower limit (<i>Imin</i>) (&lt; ExcHU.imax).  Typical value = 0,1."@en .

cim:ExcHU.ke a owl:DatatypeProperty ;
  rdfs:label "ke"@en ;
  rdfs:domain cim:ExcHU ;
  rdfs:range xsd:float ;
  skos:definition "Voltage base conversion constant (<i>Ke</i>).  Typical value = 4,666."@en .

cim:ExcHU.ki a owl:DatatypeProperty ;
  rdfs:label "ki"@en ;
  rdfs:domain cim:ExcHU ;
  rdfs:range xsd:float ;
  skos:definition "Current base conversion constant (<i>Ki</i>).  Typical value = 0,21428."@en .

cim:ExcHU.te a owl:DatatypeProperty ;
  rdfs:label "te"@en ;
  rdfs:domain cim:ExcHU ;
  rdfs:range cim:Seconds ;
  skos:definition "Major loop PI tag integration time constant (<i>Te</i>) (&gt;= 0).  Typical value = 0,154."@en .

cim:ExcHU.ti a owl:DatatypeProperty ;
  rdfs:label "ti"@en ;
  rdfs:domain cim:ExcHU ;
  rdfs:range cim:Seconds ;
  skos:definition "Minor loop PI control tag integration time constant (<i>Ti</i>) (&gt;= 0).  Typical value = 0,01333."@en .

cim:ExcHU.tr a owl:DatatypeProperty ;
  rdfs:label "tr"@en ;
  rdfs:domain cim:ExcHU ;
  rdfs:range cim:Seconds ;
  skos:definition "Filter time constant (<i>Tr</i>) (&gt;= 0). If a voltage compensator is used in conjunction with this excitation system model, <i>Tr </i>should be set to 0.  Typical value = 0,01."@en .

cim:ExcIEEEAC1A.ka a owl:DatatypeProperty ;
  rdfs:label "ka"@en ;
  rdfs:domain cim:ExcIEEEAC1A ;
  rdfs:range cim:PU ;
  skos:definition "Voltage regulator gain (<i>K</i><i><sub>A</sub></i>) (&gt; 0).  Typical value = 400."@en .

cim:ExcIEEEAC1A.kc a owl:DatatypeProperty ;
  rdfs:label "kc"@en ;
  rdfs:domain cim:ExcIEEEAC1A ;
  rdfs:range cim:PU ;
  skos:definition "Rectifier loading factor proportional to commutating reactance (<i>K</i><i><sub>C</sub></i>) (&gt;= 0).  Typical value = 0,2."@en .

cim:ExcIEEEAC1A.kd a owl:DatatypeProperty ;
  rdfs:label "kd"@en ;
  rdfs:domain cim:ExcIEEEAC1A ;
  rdfs:range cim:PU ;
  skos:definition "Demagnetizing factor, a function of exciter alternator reactances (<i>K</i><i><sub>D</sub></i>) (&gt;= 0).  Typical value = 0,38."@en .

cim:ExcIEEEAC1A.ke a owl:DatatypeProperty ;
  rdfs:label "ke"@en ;
  rdfs:domain cim:ExcIEEEAC1A ;
  rdfs:range cim:PU ;
  skos:definition "Exciter constant related to self-excited field (<i>K</i><i><sub>E</sub></i>).  Typical value = 1."@en .

cim:ExcIEEEAC1A.kf a owl:DatatypeProperty ;
  rdfs:label "kf"@en ;
  rdfs:domain cim:ExcIEEEAC1A ;
  rdfs:range cim:PU ;
  skos:definition "Excitation control system stabilizer gains (<i>K</i><i><sub>F</sub></i>) (&gt;= 0).  Typical value = 0,03."@en .

cim:ExcIEEEAC1A.seve1 a owl:DatatypeProperty ;
  rdfs:label "seve1"@en ;
  rdfs:domain cim:ExcIEEEAC1A ;
  rdfs:range xsd:float ;
  skos:definition "Exciter saturation function value at the corresponding exciter voltage, <i>V</i><i><sub>E1</sub></i>, back of commutating reactance (<i>S</i><i><sub>E</sub></i><i>[V</i><i><sub>E1</sub></i><i>]</i>) (&gt;= 0).  Typical value = 0,1."@en .

cim:ExcIEEEAC1A.seve2 a owl:DatatypeProperty ;
  rdfs:label "seve2"@en ;
  rdfs:domain cim:ExcIEEEAC1A ;
  rdfs:range xsd:float ;
  skos:definition "Exciter saturation function value at the corresponding exciter voltage, <i>V</i><i><sub>E2</sub></i>, back of commutating reactance (<i>S</i><i><sub>E</sub></i><i>[V</i><i><sub>E2</sub></i><i>]</i>) (&gt;= 0).  Typical value = 0,03."@en .

cim:ExcIEEEAC1A.ta a owl:DatatypeProperty ;
  rdfs:label "ta"@en ;
  rdfs:domain cim:ExcIEEEAC1A ;
  rdfs:range cim:Seconds ;
  skos:definition "Voltage regulator time constant (<i>T</i><i><sub>A</sub></i>) (&gt; 0).  Typical value = 0,02."@en .

cim:ExcIEEEAC1A.tb a owl:DatatypeProperty ;
  rdfs:label "tb"@en ;
  rdfs:domain cim:ExcIEEEAC1A ;
  rdfs:range cim:Seconds ;
  skos:definition "Voltage regulator time constant (<i>T</i><i><sub>B</sub></i>) (&gt;= 0).  Typical value = 0."@en .

cim:ExcIEEEAC1A.tc a owl:DatatypeProperty ;
  rdfs:label "tc"@en ;
  rdfs:domain cim:ExcIEEEAC1A ;
  rdfs:range cim:Seconds ;
  skos:definition "Voltage regulator time constant (<i>T</i><i><sub>C</sub></i>) (&gt;= 0).  Typical value = 0."@en .

cim:ExcIEEEAC1A.te a owl:DatatypeProperty ;
  rdfs:label "te"@en ;
  rdfs:domain cim:ExcIEEEAC1A ;
  rdfs:range cim:Seconds ;
  skos:definition "Exciter time constant, integration rate associated with exciter control (<i>T</i><i><sub>E</sub></i>) (&gt; 0).  Typical value = 0,8."@en .

cim:ExcIEEEAC1A.tf a owl:DatatypeProperty ;
  rdfs:label "tf"@en ;
  rdfs:domain cim:ExcIEEEAC1A ;
  rdfs:range cim:Seconds ;
  skos:definition "Excitation control system stabilizer time constant (<i>T</i><i><sub>F</sub></i>) (&gt; 0).  Typical value = 1."@en .

cim:ExcIEEEAC1A.vamax a owl:DatatypeProperty ;
  rdfs:label "vamax"@en ;
  rdfs:domain cim:ExcIEEEAC1A ;
  rdfs:range cim:PU ;
  skos:definition "Maximum voltage regulator output (<i>V</i><i><sub>AMAX</sub></i>) (&gt; 0).  Typical value = 14,5."@en .

cim:ExcIEEEAC1A.vamin a owl:DatatypeProperty ;
  rdfs:label "vamin"@en ;
  rdfs:domain cim:ExcIEEEAC1A ;
  rdfs:range cim:PU ;
  skos:definition "Minimum voltage regulator output (<i>V</i><i><sub>AMIN</sub></i>) (&lt; 0).  Typical value = -14,5."@en .

cim:ExcIEEEAC1A.ve1 a owl:DatatypeProperty ;
  rdfs:label "ve1"@en ;
  rdfs:domain cim:ExcIEEEAC1A ;
  rdfs:range cim:PU ;
  skos:definition "Exciter alternator output voltages back of commutating reactance at which saturation is defined (<i>V</i><i><sub>E1</sub></i>) (&gt; 0).  Typical value = 4,18."@en .

cim:ExcIEEEAC1A.ve2 a owl:DatatypeProperty ;
  rdfs:label "ve2"@en ;
  rdfs:domain cim:ExcIEEEAC1A ;
  rdfs:range cim:PU ;
  skos:definition "Exciter alternator output voltages back of commutating reactance at which saturation is defined (<i>V</i><i><sub>E2</sub></i>) (&gt; 0).  Typical value = 3,14."@en .

cim:ExcIEEEAC1A.vrmax a owl:DatatypeProperty ;
  rdfs:label "vrmax"@en ;
  rdfs:domain cim:ExcIEEEAC1A ;
  rdfs:range cim:PU ;
  skos:definition "Maximum voltage regulator outputs (<i>V</i><i><sub>RMAX</sub></i>) (&gt; 0).  Typical value = 6,03."@en .

cim:ExcIEEEAC1A.vrmin a owl:DatatypeProperty ;
  rdfs:label "vrmin"@en ;
  rdfs:domain cim:ExcIEEEAC1A ;
  rdfs:range cim:PU ;
  skos:definition "Minimum voltage regulator outputs (<i>V</i><i><sub>RMIN</sub></i>) (&lt; 0).  Typical value = -5,43."@en .

cim:ExcIEEEAC2A.ka a owl:DatatypeProperty ;
  rdfs:label "ka"@en ;
  rdfs:domain cim:ExcIEEEAC2A ;
  rdfs:range cim:PU ;
  skos:definition "Voltage regulator gain (<i>K</i><i><sub>A</sub></i>) (&gt; 0).  Typical value = 400."@en .

cim:ExcIEEEAC2A.kb a owl:DatatypeProperty ;
  rdfs:label "kb"@en ;
  rdfs:domain cim:ExcIEEEAC2A ;
  rdfs:range cim:PU ;
  skos:definition "Second stage regulator gain (<i>K</i><i><sub>B</sub></i>) (&gt; 0).  Typical value = 25."@en .

cim:ExcIEEEAC2A.kc a owl:DatatypeProperty ;
  rdfs:label "kc"@en ;
  rdfs:domain cim:ExcIEEEAC2A ;
  rdfs:range cim:PU ;
  skos:definition "Rectifier loading factor proportional to commutating reactance (<i>K</i><i><sub>C</sub></i>) (&gt;= 0).  Typical value = 0,28."@en .

cim:ExcIEEEAC2A.kd a owl:DatatypeProperty ;
  rdfs:label "kd"@en ;
  rdfs:domain cim:ExcIEEEAC2A ;
  rdfs:range cim:PU ;
  skos:definition "Demagnetizing factor, a function of exciter alternator reactances (<i>K</i><i><sub>D</sub></i>) (&gt;= 0).  Typical value = 0,35."@en .

cim:ExcIEEEAC2A.ke a owl:DatatypeProperty ;
  rdfs:label "ke"@en ;
  rdfs:domain cim:ExcIEEEAC2A ;
  rdfs:range cim:PU ;
  skos:definition "Exciter constant related to self-excited field (<i>K</i><i><sub>E</sub></i>) (&gt;= 0).  Typical value = 1."@en .

cim:ExcIEEEAC2A.kf a owl:DatatypeProperty ;
  rdfs:label "kf"@en ;
  rdfs:domain cim:ExcIEEEAC2A ;
  rdfs:range cim:PU ;
  skos:definition "Excitation control system stabilizer gains (<i>K</i><i><sub>F</sub></i>) (&gt;= 0).  Typical value = 0,03."@en .

cim:ExcIEEEAC2A.kh a owl:DatatypeProperty ;
  rdfs:label "kh"@en ;
  rdfs:domain cim:ExcIEEEAC2A ;
  rdfs:range cim:PU ;
  skos:definition "Exciter field current feedback gain (<i>K</i><i><sub>H</sub></i>) (&gt;= 0).  Typical value = 1."@en .

cim:ExcIEEEAC2A.seve1 a owl:DatatypeProperty ;
  rdfs:label "seve1"@en ;
  rdfs:domain cim:ExcIEEEAC2A ;
  rdfs:range xsd:float ;
  skos:definition "Exciter saturation function value at the corresponding exciter voltage, <i>V</i><i><sub>E1</sub></i>, back of commutating reactance (<i>S</i><i><sub>E</sub></i><i>[V</i><i><sub>E1</sub></i><i>]</i>) (&gt;= 0).  Typical value = 0,037."@en .

cim:ExcIEEEAC2A.seve2 a owl:DatatypeProperty ;
  rdfs:label "seve2"@en ;
  rdfs:domain cim:ExcIEEEAC2A ;
  rdfs:range xsd:float ;
  skos:definition "Exciter saturation function value at the corresponding exciter voltage, <i>V</i><i><sub>E2</sub></i>, back of commutating reactance (<i>S</i><i><sub>E</sub></i><i>[V</i><i><sub>E2</sub></i><i>]</i>) (&gt;= 0).  Typical value = 0,012."@en .

cim:ExcIEEEAC2A.ta a owl:DatatypeProperty ;
  rdfs:label "ta"@en ;
  rdfs:domain cim:ExcIEEEAC2A ;
  rdfs:range cim:Seconds ;
  skos:definition "Voltage regulator time constant (<i>T</i><i><sub>A</sub></i>) (&gt; 0).  Typical value = 0,02."@en .

cim:ExcIEEEAC2A.tb a owl:DatatypeProperty ;
  rdfs:label "tb"@en ;
  rdfs:domain cim:ExcIEEEAC2A ;
  rdfs:range cim:Seconds ;
  skos:definition "Voltage regulator time constant (<i>T</i><i><sub>B</sub></i>) (&gt;= 0).  Typical value = 0."@en .

cim:ExcIEEEAC2A.tc a owl:DatatypeProperty ;
  rdfs:label "tc"@en ;
  rdfs:domain cim:ExcIEEEAC2A ;
  rdfs:range cim:Seconds ;
  skos:definition "Voltage regulator time constant (<i>T</i><i><sub>C</sub></i>) (&gt;= 0).  Typical value = 0."@en .

cim:ExcIEEEAC2A.te a owl:DatatypeProperty ;
  rdfs:label "te"@en ;
  rdfs:domain cim:ExcIEEEAC2A ;
  rdfs:range cim:Seconds ;
  skos:definition "Exciter time constant, integration rate associated with exciter control (<i>T</i><i><sub>E</sub></i>) (&gt; 0).  Typical value = 0,6."@en .

cim:ExcIEEEAC2A.tf a owl:DatatypeProperty ;
  rdfs:label "tf"@en ;
  rdfs:domain cim:ExcIEEEAC2A ;
  rdfs:range cim:Seconds ;
  skos:definition "Excitation control system stabilizer time constant (<i>T</i><i><sub>F</sub></i>) (&gt; 0).  Typical value = 1."@en .

cim:ExcIEEEAC2A.vamax a owl:DatatypeProperty ;
  rdfs:label "vamax"@en ;
  rdfs:domain cim:ExcIEEEAC2A ;
  rdfs:range cim:PU ;
  skos:definition "Maximum voltage regulator output (<i>V</i><i><sub>AMAX</sub></i>) (&gt; 0).  Typical value = 8."@en .

cim:ExcIEEEAC2A.vamin a owl:DatatypeProperty ;
  rdfs:label "vamin"@en ;
  rdfs:domain cim:ExcIEEEAC2A ;
  rdfs:range cim:PU ;
  skos:definition "Minimum voltage regulator output (<i>V</i><i><sub>AMIN</sub></i>) (&lt; 0).  Typical value = -8."@en .

cim:ExcIEEEAC2A.ve1 a owl:DatatypeProperty ;
  rdfs:label "ve1"@en ;
  rdfs:domain cim:ExcIEEEAC2A ;
  rdfs:range cim:PU ;
  skos:definition "Exciter alternator output voltages back of commutating reactance at which saturation is defined (<i>V</i><i><sub>E1</sub></i>) (&gt; 0).  Typical value = 4,4."@en .

cim:ExcIEEEAC2A.ve2 a owl:DatatypeProperty ;
  rdfs:label "ve2"@en ;
  rdfs:domain cim:ExcIEEEAC2A ;
  rdfs:range cim:PU ;
  skos:definition "Exciter alternator output voltages back of commutating reactance at which saturation is defined (<i>V</i><i><sub>E2</sub></i>) (&gt; 0).  Typical value = 3,3."@en .

cim:ExcIEEEAC2A.vfemax a owl:DatatypeProperty ;
  rdfs:label "vfemax"@en ;
  rdfs:domain cim:ExcIEEEAC2A ;
  rdfs:range cim:PU ;
  skos:definition "Exciter field current limit reference (<i>V</i><i><sub>FEMAX</sub></i>) (&gt; 0).  Typical value = 4,4."@en .

cim:ExcIEEEAC2A.vrmax a owl:DatatypeProperty ;
  rdfs:label "vrmax"@en ;
  rdfs:domain cim:ExcIEEEAC2A ;
  rdfs:range cim:PU ;
  skos:definition "Maximum voltage regulator outputs (<i>V</i><i><sub>RMAX</sub></i>) (&gt; 0).  Typical value = 105."@en .

cim:ExcIEEEAC2A.vrmin a owl:DatatypeProperty ;
  rdfs:label "vrmin"@en ;
  rdfs:domain cim:ExcIEEEAC2A ;
  rdfs:range cim:PU ;
  skos:definition "Minimum voltage regulator outputs (<i>V</i><i><sub>RMIN</sub></i>) (&lt; 0).  Typical value = -95."@en .

cim:ExcIEEEAC3A.efdn a owl:DatatypeProperty ;
  rdfs:label "efdn"@en ;
  rdfs:domain cim:ExcIEEEAC3A ;
  rdfs:range cim:PU ;
  skos:definition "Value of <i>Efd </i>at which feedback gain changes (<i>E</i><i><sub>FDN</sub></i>) (&gt; 0).  Typical value = 2,36."@en .

cim:ExcIEEEAC3A.ka a owl:DatatypeProperty ;
  rdfs:label "ka"@en ;
  rdfs:domain cim:ExcIEEEAC3A ;
  rdfs:range cim:PU ;
  skos:definition "Voltage regulator gain (<i>K</i><i><sub>A</sub></i>) (&gt; 0).  Typical value = 45,62."@en .

cim:ExcIEEEAC3A.kc a owl:DatatypeProperty ;
  rdfs:label "kc"@en ;
  rdfs:domain cim:ExcIEEEAC3A ;
  rdfs:range cim:PU ;
  skos:definition "Rectifier loading factor proportional to commutating reactance (<i>K</i><i><sub>C</sub></i>) (&gt;= 0).  Typical value = 0,104."@en .

cim:ExcIEEEAC3A.kd a owl:DatatypeProperty ;
  rdfs:label "kd"@en ;
  rdfs:domain cim:ExcIEEEAC3A ;
  rdfs:range cim:PU ;
  skos:definition "Demagnetizing factor, a function of exciter alternator reactances (<i>K</i><i><sub>D</sub></i>) (&gt;= 0).  Typical value = 0,499."@en .

cim:ExcIEEEAC3A.ke a owl:DatatypeProperty ;
  rdfs:label "ke"@en ;
  rdfs:domain cim:ExcIEEEAC3A ;
  rdfs:range cim:PU ;
  skos:definition "Exciter constant related to self-excited field (<i>K</i><i><sub>E</sub></i>).  Typical value = 1."@en .

cim:ExcIEEEAC3A.kf a owl:DatatypeProperty ;
  rdfs:label "kf"@en ;
  rdfs:domain cim:ExcIEEEAC3A ;
  rdfs:range cim:PU ;
  skos:definition "Excitation control system stabilizer gains (<i>K</i><i><sub>F</sub></i>) (&gt;= 0).  Typical value = 0,143."@en .

cim:ExcIEEEAC3A.kn a owl:DatatypeProperty ;
  rdfs:label "kn"@en ;
  rdfs:domain cim:ExcIEEEAC3A ;
  rdfs:range cim:PU ;
  skos:definition "Excitation control system stabilizer gain (<i>K</i><i><sub>N</sub></i>) (&gt;= 0).  Typical value = 0,05."@en .

cim:ExcIEEEAC3A.kr a owl:DatatypeProperty ;
  rdfs:label "kr"@en ;
  rdfs:domain cim:ExcIEEEAC3A ;
  rdfs:range cim:PU ;
  skos:definition "Constant associated with regulator and alternator field power supply (<i>K</i><i><sub>R</sub></i>) (&gt; 0).  Typical value = 3,77."@en .

cim:ExcIEEEAC3A.seve1 a owl:DatatypeProperty ;
  rdfs:label "seve1"@en ;
  rdfs:domain cim:ExcIEEEAC3A ;
  rdfs:range xsd:float ;
  skos:definition "Exciter saturation function value at the corresponding exciter voltage, <i>V</i><i><sub>E1</sub></i>, back of commutating reactance (<i>S</i><i><sub>E</sub></i><i>[V</i><i><sub>E1</sub></i><i>]</i>) (&gt;= 0).  Typical value = 1,143."@en .

cim:ExcIEEEAC3A.seve2 a owl:DatatypeProperty ;
  rdfs:label "seve2"@en ;
  rdfs:domain cim:ExcIEEEAC3A ;
  rdfs:range xsd:float ;
  skos:definition "Exciter saturation function value at the corresponding exciter voltage, <i>V</i><i><sub>E2</sub></i>, back of commutating reactance (<i>S</i><i><sub>E</sub></i><i>[V</i><i><sub>E2</sub></i><i>]</i>) (&gt;= 0).  Typical value = 0,1."@en .

cim:ExcIEEEAC3A.ta a owl:DatatypeProperty ;
  rdfs:label "ta"@en ;
  rdfs:domain cim:ExcIEEEAC3A ;
  rdfs:range cim:Seconds ;
  skos:definition "Voltage regulator time constant (<i>T</i><i><sub>A</sub></i>) (&gt; 0).  Typical value = 0,013."@en .

cim:ExcIEEEAC3A.tb a owl:DatatypeProperty ;
  rdfs:label "tb"@en ;
  rdfs:domain cim:ExcIEEEAC3A ;
  rdfs:range cim:Seconds ;
  skos:definition "Voltage regulator time constant (<i>T</i><i><sub>B</sub></i>) (&gt;= 0).  Typical value = 0."@en .

cim:ExcIEEEAC3A.tc a owl:DatatypeProperty ;
  rdfs:label "tc"@en ;
  rdfs:domain cim:ExcIEEEAC3A ;
  rdfs:range cim:Seconds ;
  skos:definition "Voltage regulator time constant (<i>T</i><i><sub>C</sub></i>) (&gt;= 0).  Typical value = 0."@en .

cim:ExcIEEEAC3A.te a owl:DatatypeProperty ;
  rdfs:label "te"@en ;
  rdfs:domain cim:ExcIEEEAC3A ;
  rdfs:range cim:Seconds ;
  skos:definition "Exciter time constant, integration rate associated with exciter control (<i>T</i><i><sub>E</sub></i>) (&gt; 0).  Typical value = 1,17."@en .

cim:ExcIEEEAC3A.tf a owl:DatatypeProperty ;
  rdfs:label "tf"@en ;
  rdfs:domain cim:ExcIEEEAC3A ;
  rdfs:range cim:Seconds ;
  skos:definition "Excitation control system stabilizer time constant (<i>T</i><i><sub>F</sub></i>) (&gt; 0).  Typical value = 1."@en .

cim:ExcIEEEAC3A.vamax a owl:DatatypeProperty ;
  rdfs:label "vamax"@en ;
  rdfs:domain cim:ExcIEEEAC3A ;
  rdfs:range cim:PU ;
  skos:definition "Maximum voltage regulator output (<i>V</i><i><sub>AMAX</sub></i>) (&gt; 0).  Typical value = 1."@en .

cim:ExcIEEEAC3A.vamin a owl:DatatypeProperty ;
  rdfs:label "vamin"@en ;
  rdfs:domain cim:ExcIEEEAC3A ;
  rdfs:range cim:PU ;
  skos:definition "Minimum voltage regulator output (<i>V</i><i><sub>AMIN</sub></i>) (&lt; 0).  Typical value = -0,95."@en .

cim:ExcIEEEAC3A.ve1 a owl:DatatypeProperty ;
  rdfs:label "ve1"@en ;
  rdfs:domain cim:ExcIEEEAC3A ;
  rdfs:range cim:PU ;
  skos:definition "Exciter alternator output voltages back of commutating reactance at which saturation is defined (<i>V</i><i><sub>E1</sub></i>) (&gt; 0).  Typical value = 6,24."@en .

cim:ExcIEEEAC3A.ve2 a owl:DatatypeProperty ;
  rdfs:label "ve2"@en ;
  rdfs:domain cim:ExcIEEEAC3A ;
  rdfs:range cim:PU ;
  skos:definition "Exciter alternator output voltages back of commutating reactance at which saturation is defined (<i>V</i><i><sub>E2</sub></i>) (&gt; 0).  Typical value = 4,68."@en .

cim:ExcIEEEAC3A.vemin a owl:DatatypeProperty ;
  rdfs:label "vemin"@en ;
  rdfs:domain cim:ExcIEEEAC3A ;
  rdfs:range cim:PU ;
  skos:definition "Minimum exciter voltage output (<i>V</i><i><sub>EMIN</sub></i>) (&lt;= 0).  Typical value = 0."@en .

cim:ExcIEEEAC3A.vfemax a owl:DatatypeProperty ;
  rdfs:label "vfemax"@en ;
  rdfs:domain cim:ExcIEEEAC3A ;
  rdfs:range cim:PU ;
  skos:definition "Exciter field current limit reference (<i>V</i><i><sub>FEMAX</sub></i>) (&gt;= 0).  Typical value = 16."@en .

cim:ExcIEEEAC4A.ka a owl:DatatypeProperty ;
  rdfs:label "ka"@en ;
  rdfs:domain cim:ExcIEEEAC4A ;
  rdfs:range cim:PU ;
  skos:definition "Voltage regulator gain (<i>K</i><i><sub>A</sub></i>) (&gt; 0).  Typical value = 200."@en .

cim:ExcIEEEAC4A.kc a owl:DatatypeProperty ;
  rdfs:label "kc"@en ;
  rdfs:domain cim:ExcIEEEAC4A ;
  rdfs:range cim:PU ;
  skos:definition "Rectifier loading factor proportional to commutating reactance (<i>K</i><i><sub>C</sub></i>) (&gt;= 0).  Typical value = 0."@en .

cim:ExcIEEEAC4A.ta a owl:DatatypeProperty ;
  rdfs:label "ta"@en ;
  rdfs:domain cim:ExcIEEEAC4A ;
  rdfs:range cim:Seconds ;
  skos:definition "Voltage regulator time constant (<i>T</i><i><sub>A</sub></i>) (&gt; 0).  Typical value = 0,015."@en .

cim:ExcIEEEAC4A.tb a owl:DatatypeProperty ;
  rdfs:label "tb"@en ;
  rdfs:domain cim:ExcIEEEAC4A ;
  rdfs:range cim:Seconds ;
  skos:definition "Voltage regulator time constant (<i>T</i><i><sub>B</sub></i>) (&gt;= 0).  Typical value = 10."@en .

cim:ExcIEEEAC4A.tc a owl:DatatypeProperty ;
  rdfs:label "tc"@en ;
  rdfs:domain cim:ExcIEEEAC4A ;
  rdfs:range cim:Seconds ;
  skos:definition "Voltage regulator time constant (<i>T</i><i><sub>C</sub></i>) (&gt;= 0).  Typical value = 1."@en .

cim:ExcIEEEAC4A.vimax a owl:DatatypeProperty ;
  rdfs:label "vimax"@en ;
  rdfs:domain cim:ExcIEEEAC4A ;
  rdfs:range cim:PU ;
  skos:definition "Maximum voltage regulator input limit (<i>V</i><i><sub>IMAX</sub></i>) (&gt; 0).  Typical value = 10."@en .

cim:ExcIEEEAC4A.vimin a owl:DatatypeProperty ;
  rdfs:label "vimin"@en ;
  rdfs:domain cim:ExcIEEEAC4A ;
  rdfs:range cim:PU ;
  skos:definition "Minimum voltage regulator input limit (<i>V</i><i><sub>IMIN</sub></i>) (&lt; 0).  Typical value = -10."@en .

cim:ExcIEEEAC4A.vrmax a owl:DatatypeProperty ;
  rdfs:label "vrmax"@en ;
  rdfs:domain cim:ExcIEEEAC4A ;
  rdfs:range cim:PU ;
  skos:definition "Maximum voltage regulator output (<i>V</i><i><sub>RMAX</sub></i>) (&gt; 0).  Typical value = 5,64."@en .

cim:ExcIEEEAC4A.vrmin a owl:DatatypeProperty ;
  rdfs:label "vrmin"@en ;
  rdfs:domain cim:ExcIEEEAC4A ;
  rdfs:range cim:PU ;
  skos:definition "Minimum voltage regulator output (<i>V</i><i><sub>RMIN</sub></i>) (&lt; 0).  Typical value = -4,53."@en .

cim:ExcIEEEAC5A.efd1 a owl:DatatypeProperty ;
  rdfs:label "efd1"@en ;
  rdfs:domain cim:ExcIEEEAC5A ;
  rdfs:range cim:PU ;
  skos:definition "Exciter voltage at which exciter saturation is defined (<i>E</i><i><sub>FD1</sub></i>) (&gt; 0).  Typical value = 5,6."@en .

cim:ExcIEEEAC5A.efd2 a owl:DatatypeProperty ;
  rdfs:label "efd2"@en ;
  rdfs:domain cim:ExcIEEEAC5A ;
  rdfs:range cim:PU ;
  skos:definition "Exciter voltage at which exciter saturation is defined (<i>E</i><i><sub>FD2</sub></i>) (&gt; 0).  Typical value = 4,2."@en .

cim:ExcIEEEAC5A.ka a owl:DatatypeProperty ;
  rdfs:label "ka"@en ;
  rdfs:domain cim:ExcIEEEAC5A ;
  rdfs:range cim:PU ;
  skos:definition "Voltage regulator gain (<i>K</i><i><sub>A</sub></i>) (&gt; 0).  Typical value = 400."@en .

cim:ExcIEEEAC5A.ke a owl:DatatypeProperty ;
  rdfs:label "ke"@en ;
  rdfs:domain cim:ExcIEEEAC5A ;
  rdfs:range cim:PU ;
  skos:definition "Exciter constant related to self-excited field (<i>K</i><i><sub>E</sub></i>).  Typical value = 1."@en .

cim:ExcIEEEAC5A.kf a owl:DatatypeProperty ;
  rdfs:label "kf"@en ;
  rdfs:domain cim:ExcIEEEAC5A ;
  rdfs:range cim:PU ;
  skos:definition "Excitation control system stabilizer gains (<i>K</i><i><sub>F</sub></i>) (&gt;= 0).  Typical value = 0,03."@en .

cim:ExcIEEEAC5A.seefd1 a owl:DatatypeProperty ;
  rdfs:label "seefd1"@en ;
  rdfs:domain cim:ExcIEEEAC5A ;
  rdfs:range xsd:float ;
  skos:definition "Exciter saturation function value at the corresponding exciter voltage, <i>E</i><i><sub>FD1</sub></i> (<i>S</i><i><sub>E</sub></i><i>[E</i><i><sub>FD1</sub></i><i>]</i>) (&gt;= 0).  Typical value = 0,86."@en .

cim:ExcIEEEAC5A.seefd2 a owl:DatatypeProperty ;
  rdfs:label "seefd2"@en ;
  rdfs:domain cim:ExcIEEEAC5A ;
  rdfs:range xsd:float ;
  skos:definition "Exciter saturation function value at the corresponding exciter voltage, <i>E</i><i><sub>FD2</sub></i> (<i>S</i><i><sub>E</sub></i><i>[E</i><i><sub>FD2</sub></i><i>]</i>) (&gt;= 0).  Typical value = 0,5."@en .

cim:ExcIEEEAC5A.ta a owl:DatatypeProperty ;
  rdfs:label "ta"@en ;
  rdfs:domain cim:ExcIEEEAC5A ;
  rdfs:range cim:Seconds ;
  skos:definition "Voltage regulator time constant (<i>T</i><i><sub>A</sub></i>) (&gt; 0).  Typical value = 0,02."@en .

cim:ExcIEEEAC5A.te a owl:DatatypeProperty ;
  rdfs:label "te"@en ;
  rdfs:domain cim:ExcIEEEAC5A ;
  rdfs:range cim:Seconds ;
  skos:definition "Exciter time constant, integration rate associated with exciter control (<i>T</i><i><sub>E</sub></i>) (&gt; 0).  Typical value = 0,8."@en .

cim:ExcIEEEAC5A.tf1 a owl:DatatypeProperty ;
  rdfs:label "tf1"@en ;
  rdfs:domain cim:ExcIEEEAC5A ;
  rdfs:range cim:Seconds ;
  skos:definition "Excitation control system stabilizer time constant (<i>T</i><i><sub>F1</sub></i>) (&gt; 0).  Typical value = 1."@en .

cim:ExcIEEEAC5A.tf2 a owl:DatatypeProperty ;
  rdfs:label "tf2"@en ;
  rdfs:domain cim:ExcIEEEAC5A ;
  rdfs:range cim:Seconds ;
  skos:definition "Excitation control system stabilizer time constant (<i>T</i><i><sub>F2</sub></i>) (&gt;= 0).  Typical value = 1."@en .

cim:ExcIEEEAC5A.tf3 a owl:DatatypeProperty ;
  rdfs:label "tf3"@en ;
  rdfs:domain cim:ExcIEEEAC5A ;
  rdfs:range cim:Seconds ;
  skos:definition "Excitation control system stabilizer time constant (<i>T</i><i><sub>F3</sub></i>) (&gt;= 0).  Typical value = 1."@en .

cim:ExcIEEEAC5A.vrmax a owl:DatatypeProperty ;
  rdfs:label "vrmax"@en ;
  rdfs:domain cim:ExcIEEEAC5A ;
  rdfs:range cim:PU ;
  skos:definition "Maximum voltage regulator output (<i>V</i><i><sub>RMAX</sub></i>) (&gt; 0).  Typical value = 7,3."@en .

cim:ExcIEEEAC5A.vrmin a owl:DatatypeProperty ;
  rdfs:label "vrmin"@en ;
  rdfs:domain cim:ExcIEEEAC5A ;
  rdfs:range cim:PU ;
  skos:definition "Minimum voltage regulator output (<i>V</i><i><sub>RMIN</sub></i>) (&lt; 0).  Typical value = -7,3."@en .

cim:ExcIEEEAC6A.ka a owl:DatatypeProperty ;
  rdfs:label "ka"@en ;
  rdfs:domain cim:ExcIEEEAC6A ;
  rdfs:range cim:PU ;
  skos:definition "Voltage regulator gain (<i>K</i><i><sub>A</sub></i>) (&gt; 0).  Typical value = 536."@en .

cim:ExcIEEEAC6A.kc a owl:DatatypeProperty ;
  rdfs:label "kc"@en ;
  rdfs:domain cim:ExcIEEEAC6A ;
  rdfs:range cim:PU ;
  skos:definition "Rectifier loading factor proportional to commutating reactance (<i>K</i><i><sub>C</sub></i>) (&gt;= 0). Typical value = 0,173."@en .

cim:ExcIEEEAC6A.kd a owl:DatatypeProperty ;
  rdfs:label "kd"@en ;
  rdfs:domain cim:ExcIEEEAC6A ;
  rdfs:range cim:PU ;
  skos:definition "Demagnetizing factor, a function of exciter alternator reactances (<i>K</i><i><sub>D</sub></i>) (&gt;= 0).  Typical value = 1,91."@en .

cim:ExcIEEEAC6A.ke a owl:DatatypeProperty ;
  rdfs:label "ke"@en ;
  rdfs:domain cim:ExcIEEEAC6A ;
  rdfs:range cim:PU ;
  skos:definition "Exciter constant related to self-excited field (<i>K</i><i><sub>E</sub></i>).  Typical value = 1,6."@en .

cim:ExcIEEEAC6A.kh a owl:DatatypeProperty ;
  rdfs:label "kh"@en ;
  rdfs:domain cim:ExcIEEEAC6A ;
  rdfs:range cim:PU ;
  skos:definition "Exciter field current limiter gain (<i>K</i><i><sub>H</sub></i>) (&gt;= 0).  Typical value = 92."@en .

cim:ExcIEEEAC6A.seve1 a owl:DatatypeProperty ;
  rdfs:label "seve1"@en ;
  rdfs:domain cim:ExcIEEEAC6A ;
  rdfs:range xsd:float ;
  skos:definition "Exciter saturation function value at the corresponding exciter voltage, <i>V</i><i><sub>E1</sub></i>, back of commutating reactance (<i>S</i><i><sub>E</sub></i><i>[V</i><i><sub>E1</sub></i><i>])</i> (&gt;= 0).  Typical value = 0,214."@en .

cim:ExcIEEEAC6A.seve2 a owl:DatatypeProperty ;
  rdfs:label "seve2"@en ;
  rdfs:domain cim:ExcIEEEAC6A ;
  rdfs:range xsd:float ;
  skos:definition "Exciter saturation function value at the corresponding exciter voltage, <i>V</i><i><sub>E2</sub></i>, back of commutating reactance (<i>S</i><i><sub>E</sub></i><i>[V</i><i><sub>E2</sub></i><i>]</i>) (&gt;= 0).  Typical value = 0,044."@en .

cim:ExcIEEEAC6A.ta a owl:DatatypeProperty ;
  rdfs:label "ta"@en ;
  rdfs:domain cim:ExcIEEEAC6A ;
  rdfs:range cim:Seconds ;
  skos:definition "Voltage regulator time constant (<i>T</i><i><sub>A</sub></i>) (&gt;= 0).  Typical value = 0,086."@en .

cim:ExcIEEEAC6A.tb a owl:DatatypeProperty ;
  rdfs:label "tb"@en ;
  rdfs:domain cim:ExcIEEEAC6A ;
  rdfs:range cim:Seconds ;
  skos:definition "Voltage regulator time constant (<i>T</i><i><sub>B</sub></i>) (&gt;= 0).  Typical value = 9."@en .

cim:ExcIEEEAC6A.tc a owl:DatatypeProperty ;
  rdfs:label "tc"@en ;
  rdfs:domain cim:ExcIEEEAC6A ;
  rdfs:range cim:Seconds ;
  skos:definition "Voltage regulator time constant (<i>T</i><i><sub>C</sub></i>) (&gt;= 0).  Typical value = 3."@en .

cim:ExcIEEEAC6A.te a owl:DatatypeProperty ;
  rdfs:label "te"@en ;
  rdfs:domain cim:ExcIEEEAC6A ;
  rdfs:range cim:Seconds ;
  skos:definition "Exciter time constant, integration rate associated with exciter control (<i>T</i><i><sub>E</sub></i>) (&gt; 0).  Typical value = 1."@en .

cim:ExcIEEEAC6A.th a owl:DatatypeProperty ;
  rdfs:label "th"@en ;
  rdfs:domain cim:ExcIEEEAC6A ;
  rdfs:range cim:Seconds ;
  skos:definition "Exciter field current limiter time constant (<i>T</i><i><sub>H</sub></i>) (&gt; 0).  Typical value = 0,08."@en .

cim:ExcIEEEAC6A.tj a owl:DatatypeProperty ;
  rdfs:label "tj"@en ;
  rdfs:domain cim:ExcIEEEAC6A ;
  rdfs:range cim:Seconds ;
  skos:definition "Exciter field current limiter time constant (<i>T</i><i><sub>J</sub></i>) (&gt;= 0).  Typical value = 0,02."@en .

cim:ExcIEEEAC6A.tk a owl:DatatypeProperty ;
  rdfs:label "tk"@en ;
  rdfs:domain cim:ExcIEEEAC6A ;
  rdfs:range cim:Seconds ;
  skos:definition "Voltage regulator time constant (<i>T</i><i><sub>K</sub></i>) (&gt;= 0).  Typical value = 0,18."@en .

cim:ExcIEEEAC6A.vamax a owl:DatatypeProperty ;
  rdfs:label "vamax"@en ;
  rdfs:domain cim:ExcIEEEAC6A ;
  rdfs:range cim:PU ;
  skos:definition "Maximum voltage regulator output (<i>V</i><i><sub>AMAX</sub></i>) (&gt; 0).  Typical value = 75."@en .

cim:ExcIEEEAC6A.vamin a owl:DatatypeProperty ;
  rdfs:label "vamin"@en ;
  rdfs:domain cim:ExcIEEEAC6A ;
  rdfs:range cim:PU ;
  skos:definition "Minimum voltage regulator output (V<sub>AMIN</sub>) (&lt; 0).  Typical value = -75."@en .

cim:ExcIEEEAC6A.ve1 a owl:DatatypeProperty ;
  rdfs:label "ve1"@en ;
  rdfs:domain cim:ExcIEEEAC6A ;
  rdfs:range cim:PU ;
  skos:definition "Exciter alternator output voltages back of commutating reactance at which saturation is defined (<i>V</i><i><sub>E1</sub></i>) (&gt; 0).  Typical value = 7,4."@en .

cim:ExcIEEEAC6A.ve2 a owl:DatatypeProperty ;
  rdfs:label "ve2"@en ;
  rdfs:domain cim:ExcIEEEAC6A ;
  rdfs:range cim:PU ;
  skos:definition "Exciter alternator output voltages back of commutating reactance at which saturation is defined (<i>V</i><i><sub>E2</sub></i>) (&gt; 0).  Typical value = 5,55."@en .

cim:ExcIEEEAC6A.vfelim a owl:DatatypeProperty ;
  rdfs:label "vfelim"@en ;
  rdfs:domain cim:ExcIEEEAC6A ;
  rdfs:range cim:PU ;
  skos:definition "Exciter field current limit reference (<i>V</i><i><sub>FELIM</sub></i>) (&gt; 0).  Typical value = 19."@en .

cim:ExcIEEEAC6A.vhmax a owl:DatatypeProperty ;
  rdfs:label "vhmax"@en ;
  rdfs:domain cim:ExcIEEEAC6A ;
  rdfs:range cim:PU ;
  skos:definition "Maximum field current limiter signal reference (<i>V</i><i><sub>HMAX</sub></i>) (&gt; 0).  Typical value = 75."@en .

cim:ExcIEEEAC6A.vrmax a owl:DatatypeProperty ;
  rdfs:label "vrmax"@en ;
  rdfs:domain cim:ExcIEEEAC6A ;
  rdfs:range cim:PU ;
  skos:definition "Maximum voltage regulator output (<i>V</i><i><sub>RMAX</sub></i>) (&gt; 0).  Typical value = 44."@en .

cim:ExcIEEEAC6A.vrmin a owl:DatatypeProperty ;
  rdfs:label "vrmin"@en ;
  rdfs:domain cim:ExcIEEEAC6A ;
  rdfs:range cim:PU ;
  skos:definition "Minimum voltage regulator output (<i>V</i><i><sub>RMIN</sub></i>) (&lt; 0).  Typical value = -36."@en .

cim:ExcIEEEAC7B.kc a owl:DatatypeProperty ;
  rdfs:label "kc"@en ;
  rdfs:domain cim:ExcIEEEAC7B ;
  rdfs:range cim:PU ;
  skos:definition "Rectifier loading factor proportional to commutating reactance (<i>K</i><i><sub>C</sub></i>) (&gt;= 0). Typical value = 0,18."@en .

cim:ExcIEEEAC7B.kd a owl:DatatypeProperty ;
  rdfs:label "kd"@en ;
  rdfs:domain cim:ExcIEEEAC7B ;
  rdfs:range cim:PU ;
  skos:definition "Demagnetizing factor, a function of exciter alternator reactances (<i>K</i><i><sub>D</sub></i>) (&gt;= 0).  Typical value = 0,02."@en .

cim:ExcIEEEAC7B.kdr a owl:DatatypeProperty ;
  rdfs:label "kdr"@en ;
  rdfs:domain cim:ExcIEEEAC7B ;
  rdfs:range cim:PU ;
  skos:definition "Voltage regulator derivative gain (<i>K</i><i><sub>DR</sub></i>) (&gt;= 0).  Typical value = 0."@en .

cim:ExcIEEEAC7B.ke a owl:DatatypeProperty ;
  rdfs:label "ke"@en ;
  rdfs:domain cim:ExcIEEEAC7B ;
  rdfs:range cim:PU ;
  skos:definition "Exciter constant related to self-excited field (<i>K</i><i><sub>E</sub></i>).  Typical value = 1."@en .

cim:ExcIEEEAC7B.kf1 a owl:DatatypeProperty ;
  rdfs:label "kf1"@en ;
  rdfs:domain cim:ExcIEEEAC7B ;
  rdfs:range cim:PU ;
  skos:definition "Excitation control system stabilizer gain (<i>K</i><i><sub>F1</sub></i>) (&gt;= 0).  Typical value = 0,212."@en .

cim:ExcIEEEAC7B.kf2 a owl:DatatypeProperty ;
  rdfs:label "kf2"@en ;
  rdfs:domain cim:ExcIEEEAC7B ;
  rdfs:range cim:PU ;
  skos:definition "Excitation control system stabilizer gain (<i>K</i><i><sub>F2</sub></i>) (&gt;= 0).  Typical value = 0."@en .

cim:ExcIEEEAC7B.kf3 a owl:DatatypeProperty ;
  rdfs:label "kf3"@en ;
  rdfs:domain cim:ExcIEEEAC7B ;
  rdfs:range cim:PU ;
  skos:definition "Excitation control system stabilizer gain (<i>K</i><i><sub>F3</sub></i>) (&gt;= 0).  Typical value = 0."@en .

cim:ExcIEEEAC7B.kia a owl:DatatypeProperty ;
  rdfs:label "kia"@en ;
  rdfs:domain cim:ExcIEEEAC7B ;
  rdfs:range cim:PU ;
  skos:definition "Voltage regulator integral gain (<i>K</i><i><sub>IA</sub></i>) (&gt;= 0).  Typical value = 59,69."@en .

cim:ExcIEEEAC7B.kir a owl:DatatypeProperty ;
  rdfs:label "kir"@en ;
  rdfs:domain cim:ExcIEEEAC7B ;
  rdfs:range cim:PU ;
  skos:definition "Voltage regulator integral gain (<i>K</i><i><sub>IR</sub></i>) (&gt;= 0).  Typical value = 4,24."@en .

cim:ExcIEEEAC7B.kl a owl:DatatypeProperty ;
  rdfs:label "kl"@en ;
  rdfs:domain cim:ExcIEEEAC7B ;
  rdfs:range cim:PU ;
  skos:definition "Exciter field voltage lower limit parameter (<i>K</i><i><sub>L</sub></i>).  Typical value = 10."@en .

cim:ExcIEEEAC7B.kp a owl:DatatypeProperty ;
  rdfs:label "kp"@en ;
  rdfs:domain cim:ExcIEEEAC7B ;
  rdfs:range cim:PU ;
  skos:definition "Potential circuit gain coefficient (<i>K</i><i><sub>P</sub></i>) (&gt; 0).  Typical value = 4,96."@en .

cim:ExcIEEEAC7B.kpa a owl:DatatypeProperty ;
  rdfs:label "kpa"@en ;
  rdfs:domain cim:ExcIEEEAC7B ;
  rdfs:range cim:PU ;
  skos:definition "Voltage regulator proportional gain (<i>K</i><i><sub>PA</sub></i>) (&gt; 0 if ExcIEEEAC7B.kia = 0).  Typical value = 65,36."@en .

cim:ExcIEEEAC7B.kpr a owl:DatatypeProperty ;
  rdfs:label "kpr"@en ;
  rdfs:domain cim:ExcIEEEAC7B ;
  rdfs:range cim:PU ;
  skos:definition "Voltage regulator proportional gain (<i>K</i><i><sub>PR</sub></i>) (&gt; 0 if ExcIEEEAC7B.kir = 0).  Typical value = 4,24."@en .

cim:ExcIEEEAC7B.seve1 a owl:DatatypeProperty ;
  rdfs:label "seve1"@en ;
  rdfs:domain cim:ExcIEEEAC7B ;
  rdfs:range xsd:float ;
  skos:definition "Exciter saturation function value at the corresponding exciter voltage, <i>V</i><i><sub>E1</sub></i>, back of commutating reactance (<i>S</i><i><sub>E</sub></i><i>[V</i><i><sub>E1</sub></i><i>]</i>) (&gt;= 0).  Typical value = 0,44."@en .

cim:ExcIEEEAC7B.seve2 a owl:DatatypeProperty ;
  rdfs:label "seve2"@en ;
  rdfs:domain cim:ExcIEEEAC7B ;
  rdfs:range xsd:float ;
  skos:definition "Exciter saturation function value at the corresponding exciter voltage, <i>V</i><i><sub>E2</sub></i>, back of commutating reactance (<i>S</i><i><sub>E</sub></i><i>[V</i><i><sub>E2</sub></i><i>]</i>) (&gt;= 0).  Typical value = 0,075."@en .

cim:ExcIEEEAC7B.tdr a owl:DatatypeProperty ;
  rdfs:label "tdr"@en ;
  rdfs:domain cim:ExcIEEEAC7B ;
  rdfs:range cim:Seconds ;
  skos:definition "Lag time constant (<i>T</i><i><sub>DR</sub></i>) (&gt;= 0).  Typical value = 0."@en .

cim:ExcIEEEAC7B.te a owl:DatatypeProperty ;
  rdfs:label "te"@en ;
  rdfs:domain cim:ExcIEEEAC7B ;
  rdfs:range cim:Seconds ;
  skos:definition "Exciter time constant, integration rate associated with exciter control (<i>T</i><i><sub>E</sub></i>) (&gt; 0).  Typical value = 1,1."@en .

cim:ExcIEEEAC7B.tf a owl:DatatypeProperty ;
  rdfs:label "tf"@en ;
  rdfs:domain cim:ExcIEEEAC7B ;
  rdfs:range cim:Seconds ;
  skos:definition "Excitation control system stabilizer time constant (<i>T</i><i><sub>F</sub></i>) (&gt; 0).  Typical value = 1."@en .

cim:ExcIEEEAC7B.vamax a owl:DatatypeProperty ;
  rdfs:label "vamax"@en ;
  rdfs:domain cim:ExcIEEEAC7B ;
  rdfs:range cim:PU ;
  skos:definition "Maximum voltage regulator output (<i>V</i><i><sub>AMAX</sub></i>) (&gt; 0).  Typical value = 1."@en .

cim:ExcIEEEAC7B.vamin a owl:DatatypeProperty ;
  rdfs:label "vamin"@en ;
  rdfs:domain cim:ExcIEEEAC7B ;
  rdfs:range cim:PU ;
  skos:definition "Minimum voltage regulator output (<i>V</i><i><sub>AMIN</sub></i>) (&lt; 0).  Typical value = -0,95."@en .

cim:ExcIEEEAC7B.ve1 a owl:DatatypeProperty ;
  rdfs:label "ve1"@en ;
  rdfs:domain cim:ExcIEEEAC7B ;
  rdfs:range cim:PU ;
  skos:definition "Exciter alternator output voltages back of commutating reactance at which saturation is defined (<i>V</i><i><sub>E1</sub></i>) (&gt; 0).  Typical value = 6,3."@en .

cim:ExcIEEEAC7B.ve2 a owl:DatatypeProperty ;
  rdfs:label "ve2"@en ;
  rdfs:domain cim:ExcIEEEAC7B ;
  rdfs:range cim:PU ;
  skos:definition "Exciter alternator output voltages back of commutating reactance at which saturation is defined (<i>V</i><i><sub>E2</sub></i>) (&gt; 0).  Typical value = 3,02."@en .

cim:ExcIEEEAC7B.vemin a owl:DatatypeProperty ;
  rdfs:label "vemin"@en ;
  rdfs:domain cim:ExcIEEEAC7B ;
  rdfs:range cim:PU ;
  skos:definition "Minimum exciter voltage output (<i>V</i><i><sub>EMIN</sub></i>) (&lt;= 0).  Typical value = 0."@en .

cim:ExcIEEEAC7B.vfemax a owl:DatatypeProperty ;
  rdfs:label "vfemax"@en ;
  rdfs:domain cim:ExcIEEEAC7B ;
  rdfs:range cim:PU ;
  skos:definition "Exciter field current limit reference (<i>V</i><i><sub>FEMAX</sub></i>).  Typical value = 6,9."@en .

cim:ExcIEEEAC7B.vrmax a owl:DatatypeProperty ;
  rdfs:label "vrmax"@en ;
  rdfs:domain cim:ExcIEEEAC7B ;
  rdfs:range cim:PU ;
  skos:definition "Maximum voltage regulator output (<i>V</i><i><sub>RMAX</sub></i>) (&gt; 0).  Typical value = 5,79."@en .

cim:ExcIEEEAC7B.vrmin a owl:DatatypeProperty ;
  rdfs:label "vrmin"@en ;
  rdfs:domain cim:ExcIEEEAC7B ;
  rdfs:range cim:PU ;
  skos:definition "Minimum voltage regulator output (<i>V</i><i><sub>RMIN</sub></i>) (&lt; 0).  Typical value = -5,79."@en .

cim:ExcIEEEAC8B.ka a owl:DatatypeProperty ;
  rdfs:label "ka"@en ;
  rdfs:domain cim:ExcIEEEAC8B ;
  rdfs:range cim:PU ;
  skos:definition "Voltage regulator gain (<i>K</i><i><sub>A</sub></i>) (&gt; 0).  Typical value = 1."@en .

cim:ExcIEEEAC8B.kc a owl:DatatypeProperty ;
  rdfs:label "kc"@en ;
  rdfs:domain cim:ExcIEEEAC8B ;
  rdfs:range cim:PU ;
  skos:definition "Rectifier loading factor proportional to commutating reactance (<i>K</i><i><sub>C</sub></i>) (&gt;= 0). Typical value = 0,55."@en .

cim:ExcIEEEAC8B.kd a owl:DatatypeProperty ;
  rdfs:label "kd"@en ;
  rdfs:domain cim:ExcIEEEAC8B ;
  rdfs:range cim:PU ;
  skos:definition "Demagnetizing factor, a function of exciter alternator reactances (<i>K</i><i><sub>D</sub></i>) (&gt;= 0).  Typical value = 1,1."@en .

cim:ExcIEEEAC8B.kdr a owl:DatatypeProperty ;
  rdfs:label "kdr"@en ;
  rdfs:domain cim:ExcIEEEAC8B ;
  rdfs:range cim:PU ;
  skos:definition "Voltage regulator derivative gain (<i>K</i><i><sub>DR</sub></i>) (&gt;= 0).  Typical value = 10."@en .

cim:ExcIEEEAC8B.ke a owl:DatatypeProperty ;
  rdfs:label "ke"@en ;
  rdfs:domain cim:ExcIEEEAC8B ;
  rdfs:range cim:PU ;
  skos:definition "Exciter constant related to self-excited field (<i>K</i><i><sub>E</sub></i>).  Typical value = 1."@en .

cim:ExcIEEEAC8B.kir a owl:DatatypeProperty ;
  rdfs:label "kir"@en ;
  rdfs:domain cim:ExcIEEEAC8B ;
  rdfs:range cim:PU ;
  skos:definition "Voltage regulator integral gain (<i>K</i><i><sub>IR</sub></i>) (&gt;= 0).  Typical value = 5."@en .

cim:ExcIEEEAC8B.kpr a owl:DatatypeProperty ;
  rdfs:label "kpr"@en ;
  rdfs:domain cim:ExcIEEEAC8B ;
  rdfs:range cim:PU ;
  skos:definition "Voltage regulator proportional gain (<i>K</i><i><sub>PR</sub></i>) (&gt; 0 if ExcIEEEAC8B.kir = 0).  Typical value = 80."@en .

cim:ExcIEEEAC8B.seve1 a owl:DatatypeProperty ;
  rdfs:label "seve1"@en ;
  rdfs:domain cim:ExcIEEEAC8B ;
  rdfs:range xsd:float ;
  skos:definition "Exciter saturation function value at the corresponding exciter voltage, <i>V</i><i><sub>E1</sub></i>, back of commutating reactance (<i>S</i><i><sub>E</sub></i><i>[V</i><i><sub>E1</sub></i><i>]</i>) (&gt;= 0).  Typical value = 0,3."@en .

cim:ExcIEEEAC8B.seve2 a owl:DatatypeProperty ;
  rdfs:label "seve2"@en ;
  rdfs:domain cim:ExcIEEEAC8B ;
  rdfs:range xsd:float ;
  skos:definition "Exciter saturation function value at the corresponding exciter voltage, <i>V</i><i><sub>E2</sub></i>, back of commutating reactance (<i>S</i><i><sub>E</sub></i><i>[V</i><i><sub>E2</sub></i><i>]</i>) (&gt;= 0).  Typical value = 3."@en .

cim:ExcIEEEAC8B.ta a owl:DatatypeProperty ;
  rdfs:label "ta"@en ;
  rdfs:domain cim:ExcIEEEAC8B ;
  rdfs:range cim:Seconds ;
  skos:definition "Voltage regulator time constant (<i>T</i><i><sub>A</sub></i>) (&gt;= 0).  Typical value = 0."@en .

cim:ExcIEEEAC8B.tdr a owl:DatatypeProperty ;
  rdfs:label "tdr"@en ;
  rdfs:domain cim:ExcIEEEAC8B ;
  rdfs:range cim:Seconds ;
  skos:definition "Lag time constant (<i>T</i><i><sub>DR</sub></i>) (&gt; 0).  Typical value = 0,1."@en .

cim:ExcIEEEAC8B.te a owl:DatatypeProperty ;
  rdfs:label "te"@en ;
  rdfs:domain cim:ExcIEEEAC8B ;
  rdfs:range cim:Seconds ;
  skos:definition "Exciter time constant, integration rate associated with exciter control (<i>T</i><i><sub>E</sub></i>) (&gt; 0).  Typical value = 1,2."@en .

cim:ExcIEEEAC8B.ve1 a owl:DatatypeProperty ;
  rdfs:label "ve1"@en ;
  rdfs:domain cim:ExcIEEEAC8B ;
  rdfs:range cim:PU ;
  skos:definition "Exciter alternator output voltages back of commutating reactance at which saturation is defined (<i>V</i><i><sub>E1</sub></i>) (&gt; 0).  Typical value = 6,5."@en .

cim:ExcIEEEAC8B.ve2 a owl:DatatypeProperty ;
  rdfs:label "ve2"@en ;
  rdfs:domain cim:ExcIEEEAC8B ;
  rdfs:range cim:PU ;
  skos:definition "Exciter alternator output voltages back of commutating reactance at which saturation is defined (<i>V</i><i><sub>E2</sub></i>) (&gt; 0).  Typical value = 9."@en .

cim:ExcIEEEAC8B.vemin a owl:DatatypeProperty ;
  rdfs:label "vemin"@en ;
  rdfs:domain cim:ExcIEEEAC8B ;
  rdfs:range cim:PU ;
  skos:definition "Minimum exciter voltage output (<i>V</i><i><sub>EMIN</sub></i>) (&lt;= 0).  Typical value = 0."@en .

cim:ExcIEEEAC8B.vfemax a owl:DatatypeProperty ;
  rdfs:label "vfemax"@en ;
  rdfs:domain cim:ExcIEEEAC8B ;
  rdfs:range cim:PU ;
  skos:definition "Exciter field current limit reference (<i>V</i><i><sub>FEMAX</sub></i>).  Typical value = 6."@en .

cim:ExcIEEEAC8B.vrmax a owl:DatatypeProperty ;
  rdfs:label "vrmax"@en ;
  rdfs:domain cim:ExcIEEEAC8B ;
  rdfs:range cim:PU ;
  skos:definition "Maximum voltage regulator output (<i>V</i><i><sub>RMAX</sub></i>) (&gt; 0).  Typical value = 35."@en .

cim:ExcIEEEAC8B.vrmin a owl:DatatypeProperty ;
  rdfs:label "vrmin"@en ;
  rdfs:domain cim:ExcIEEEAC8B ;
  rdfs:range cim:PU ;
  skos:definition "Minimum voltage regulator output (<i>V</i><i><sub>RMIN</sub></i>) (&lt;= 0).  Typical value = 0."@en .

cim:ExcIEEEDC1A.efd1 a owl:DatatypeProperty ;
  rdfs:label "efd1"@en ;
  rdfs:domain cim:ExcIEEEDC1A ;
  rdfs:range cim:PU ;
  skos:definition "Exciter voltage at which exciter saturation is defined (<i>E</i><i><sub>FD1</sub></i>) (&gt; 0).  Typical value = 3,1."@en .

cim:ExcIEEEDC1A.efd2 a owl:DatatypeProperty ;
  rdfs:label "efd2"@en ;
  rdfs:domain cim:ExcIEEEDC1A ;
  rdfs:range cim:PU ;
  skos:definition "Exciter voltage at which exciter saturation is defined (<i>E</i><i><sub>FD2</sub></i>) (&gt; 0).  Typical value = 2,3."@en .

cim:ExcIEEEDC1A.exclim a owl:DatatypeProperty ;
  rdfs:label "exclim"@en ;
  rdfs:domain cim:ExcIEEEDC1A ;
  rdfs:range xsd:boolean ;
  skos:definition """
(<i>exclim</i>).  IEEE standard is ambiguous about lower limit on exciter output.
true = a lower limit of zero is applied to integrator output
false = a lower limit of zero is not applied to integrator output.
Typical value = true.
\t"""@en .

cim:ExcIEEEDC1A.ka a owl:DatatypeProperty ;
  rdfs:label "ka"@en ;
  rdfs:domain cim:ExcIEEEDC1A ;
  rdfs:range cim:PU ;
  skos:definition "Voltage regulator gain (<i>K</i><i><sub>A</sub></i>) (&gt; 0).  Typical value = 46."@en .

cim:ExcIEEEDC1A.ke a owl:DatatypeProperty ;
  rdfs:label "ke"@en ;
  rdfs:domain cim:ExcIEEEDC1A ;
  rdfs:range cim:PU ;
  skos:definition "Exciter constant related to self-excited field (<i>K</i><i><sub>E</sub></i>).  Typical value = 0."@en .

cim:ExcIEEEDC1A.kf a owl:DatatypeProperty ;
  rdfs:label "kf"@en ;
  rdfs:domain cim:ExcIEEEDC1A ;
  rdfs:range cim:PU ;
  skos:definition "Excitation control system stabilizer gain (<i>K</i><i><sub>F</sub></i>) (&gt;= 0).  Typical value = 0.1."@en .

cim:ExcIEEEDC1A.seefd1 a owl:DatatypeProperty ;
  rdfs:label "seefd1"@en ;
  rdfs:domain cim:ExcIEEEDC1A ;
  rdfs:range xsd:float ;
  skos:definition "Exciter saturation function value at the corresponding exciter voltage, <i>E</i><i><sub>FD1</sub></i> (<i>S</i><i><sub>E</sub></i><i>[E</i><i><sub>FD1</sub></i><i>]</i>) (&gt;= 0).  Typical value = 0.33."@en .

cim:ExcIEEEDC1A.seefd2 a owl:DatatypeProperty ;
  rdfs:label "seefd2"@en ;
  rdfs:domain cim:ExcIEEEDC1A ;
  rdfs:range xsd:float ;
  skos:definition "Exciter saturation function value at the corresponding exciter voltage, <i>E</i><i><sub>FD2</sub></i> (<i>S</i><i><sub>E</sub></i><i>[E</i><i><sub>FD2</sub></i><i>]</i>) (&gt;= 0).  Typical value = 0,1."@en .

cim:ExcIEEEDC1A.ta a owl:DatatypeProperty ;
  rdfs:label "ta"@en ;
  rdfs:domain cim:ExcIEEEDC1A ;
  rdfs:range cim:Seconds ;
  skos:definition "Voltage regulator time constant (<i>T</i><i><sub>A</sub></i>) (&gt; 0).  Typical value = 0,06."@en .

cim:ExcIEEEDC1A.tb a owl:DatatypeProperty ;
  rdfs:label "tb"@en ;
  rdfs:domain cim:ExcIEEEDC1A ;
  rdfs:range cim:Seconds ;
  skos:definition "Voltage regulator time constant (<i>T</i><i><sub>B</sub></i>) (&gt;= 0).  Typical value = 0."@en .

cim:ExcIEEEDC1A.tc a owl:DatatypeProperty ;
  rdfs:label "tc"@en ;
  rdfs:domain cim:ExcIEEEDC1A ;
  rdfs:range cim:Seconds ;
  skos:definition "Voltage regulator time constant (<i>T</i><i><sub>C</sub></i>) (&gt;= 0).  Typical value = 0."@en .

cim:ExcIEEEDC1A.te a owl:DatatypeProperty ;
  rdfs:label "te"@en ;
  rdfs:domain cim:ExcIEEEDC1A ;
  rdfs:range cim:Seconds ;
  skos:definition "Exciter time constant, integration rate associated with exciter control (<i>T</i><i><sub>E</sub></i>) (&gt; 0).  Typical value = 0,46."@en .

cim:ExcIEEEDC1A.tf a owl:DatatypeProperty ;
  rdfs:label "tf"@en ;
  rdfs:domain cim:ExcIEEEDC1A ;
  rdfs:range cim:Seconds ;
  skos:definition "Excitation control system stabilizer time constant (<i>T</i><i><sub>F</sub></i>) (&gt; 0).  Typical value = 1."@en .

cim:ExcIEEEDC1A.uelin a owl:DatatypeProperty ;
  rdfs:label "uelin"@en ;
  rdfs:domain cim:ExcIEEEDC1A ;
  rdfs:range xsd:boolean ;
  skos:definition """
UEL input (<i>uelin</i>).
true = input is connected to the HV gate
false = input connects to the error signal.
Typical value = true.
\t"""@en .

cim:ExcIEEEDC1A.vrmax a owl:DatatypeProperty ;
  rdfs:label "vrmax"@en ;
  rdfs:domain cim:ExcIEEEDC1A ;
  rdfs:range cim:PU ;
  skos:definition "Maximum voltage regulator output (<i>V</i><i><sub>RMAX</sub></i>) (&gt; ExcIEEEDC1A.vrmin).  Typical value = 1."@en .

cim:ExcIEEEDC1A.vrmin a owl:DatatypeProperty ;
  rdfs:label "vrmin"@en ;
  rdfs:domain cim:ExcIEEEDC1A ;
  rdfs:range cim:PU ;
  skos:definition "Minimum voltage regulator output (<i>V</i><i><sub>RMIN</sub></i>) (&lt; 0 and &lt; ExcIEEEDC1A.vrmax).  Typical value = -0,9."@en .

cim:ExcIEEEDC2A.efd1 a owl:DatatypeProperty ;
  rdfs:label "efd1"@en ;
  rdfs:domain cim:ExcIEEEDC2A ;
  rdfs:range cim:PU ;
  skos:definition "Exciter voltage at which exciter saturation is defined (<i>E</i><i><sub>FD1</sub></i>) (&gt; 0).  Typical value = 3,05."@en .

cim:ExcIEEEDC2A.efd2 a owl:DatatypeProperty ;
  rdfs:label "efd2"@en ;
  rdfs:domain cim:ExcIEEEDC2A ;
  rdfs:range cim:PU ;
  skos:definition "Exciter voltage at which exciter saturation is defined (<i>E</i><i><sub>FD2</sub></i>) (&gt; 0).  Typical value = 2,29."@en .

cim:ExcIEEEDC2A.exclim a owl:DatatypeProperty ;
  rdfs:label "exclim"@en ;
  rdfs:domain cim:ExcIEEEDC2A ;
  rdfs:range cim:PU ;
  skos:definition "(<i>exclim</i>).  IEEE standard is ambiguous about lower limit on exciter output. Typical value = - 999  which means that there is no limit applied."@en .

cim:ExcIEEEDC2A.ka a owl:DatatypeProperty ;
  rdfs:label "ka"@en ;
  rdfs:domain cim:ExcIEEEDC2A ;
  rdfs:range cim:PU ;
  skos:definition "Voltage regulator gain (<i>K</i><i><sub>A</sub></i>) (&gt; 0).  Typical value = 300."@en .

cim:ExcIEEEDC2A.ke a owl:DatatypeProperty ;
  rdfs:label "ke"@en ;
  rdfs:domain cim:ExcIEEEDC2A ;
  rdfs:range cim:PU ;
  skos:definition "Exciter constant related to self-excited field (<i>K</i><i><sub>E</sub></i>).  Typical value = 1."@en .

cim:ExcIEEEDC2A.kf a owl:DatatypeProperty ;
  rdfs:label "kf"@en ;
  rdfs:domain cim:ExcIEEEDC2A ;
  rdfs:range cim:PU ;
  skos:definition "Excitation control system stabilizer gain (<i>K</i><i><sub>F</sub></i>) (&gt;= 0).  Typical value = 0,1."@en .

cim:ExcIEEEDC2A.seefd1 a owl:DatatypeProperty ;
  rdfs:label "seefd1"@en ;
  rdfs:domain cim:ExcIEEEDC2A ;
  rdfs:range xsd:float ;
  skos:definition "Exciter saturation function value at the corresponding exciter voltage, <i>E</i><i><sub>FD1</sub></i> (<i>S</i><i><sub>E</sub></i><i>[E</i><i><sub>FD1</sub></i><i>]</i>) (&gt;= 0).  Typical value = 0,279."@en .

cim:ExcIEEEDC2A.seefd2 a owl:DatatypeProperty ;
  rdfs:label "seefd2"@en ;
  rdfs:domain cim:ExcIEEEDC2A ;
  rdfs:range xsd:float ;
  skos:definition "Exciter saturation function value at the corresponding exciter voltage, <i>E</i><i><sub>FD2</sub></i> (<i>S</i><i><sub>E</sub></i><i>[E</i><i><sub>FD2</sub></i><i>]</i>) (&gt;= 0).  Typical value = 0,117."@en .

cim:ExcIEEEDC2A.ta a owl:DatatypeProperty ;
  rdfs:label "ta"@en ;
  rdfs:domain cim:ExcIEEEDC2A ;
  rdfs:range cim:Seconds ;
  skos:definition "Voltage regulator time constant (<i>T</i><i><sub>A</sub></i>) (&gt; 0).  Typical value = 0,01."@en .

cim:ExcIEEEDC2A.tb a owl:DatatypeProperty ;
  rdfs:label "tb"@en ;
  rdfs:domain cim:ExcIEEEDC2A ;
  rdfs:range cim:Seconds ;
  skos:definition "Voltage regulator time constant (<i>T</i><i><sub>B</sub></i>) (&gt;= 0).  Typical value = 0."@en .

cim:ExcIEEEDC2A.tc a owl:DatatypeProperty ;
  rdfs:label "tc"@en ;
  rdfs:domain cim:ExcIEEEDC2A ;
  rdfs:range cim:Seconds ;
  skos:definition "Voltage regulator time constant (<i>T</i><i><sub>C</sub></i>) (&gt;= 0).  Typical value = 0."@en .

cim:ExcIEEEDC2A.te a owl:DatatypeProperty ;
  rdfs:label "te"@en ;
  rdfs:domain cim:ExcIEEEDC2A ;
  rdfs:range cim:Seconds ;
  skos:definition "Exciter time constant, integration rate associated with exciter control (<i>T</i><i><sub>E</sub></i>) (&gt; 0).  Typical value = 1,33."@en .

cim:ExcIEEEDC2A.tf a owl:DatatypeProperty ;
  rdfs:label "tf"@en ;
  rdfs:domain cim:ExcIEEEDC2A ;
  rdfs:range cim:Seconds ;
  skos:definition "Excitation control system stabilizer time constant (<i>T</i><i><sub>F</sub></i>) (&gt; 0).  Typical value = 0,675."@en .

cim:ExcIEEEDC2A.uelin a owl:DatatypeProperty ;
  rdfs:label "uelin"@en ;
  rdfs:domain cim:ExcIEEEDC2A ;
  rdfs:range xsd:boolean ;
  skos:definition """
UEL input (<i>uelin</i>).
true = input is connected to the HV gate
false = input connects to the error signal.
Typical value = true.
\t"""@en .

cim:ExcIEEEDC2A.vrmax a owl:DatatypeProperty ;
  rdfs:label "vrmax"@en ;
  rdfs:domain cim:ExcIEEEDC2A ;
  rdfs:range cim:PU ;
  skos:definition "Maximum voltage regulator output (<i>V</i><i><sub>RMAX</sub></i>)(&gt; ExcIEEEDC2A.vrmin).  Typical value = 4,95."@en .

cim:ExcIEEEDC2A.vrmin a owl:DatatypeProperty ;
  rdfs:label "vrmin"@en ;
  rdfs:domain cim:ExcIEEEDC2A ;
  rdfs:range cim:PU ;
  skos:definition "Minimum voltage regulator output (<i>V</i><i><sub>RMIN</sub></i>) (&lt; 0 and &lt; ExcIEEEDC2A.vrmax).  Typical value = -4,9."@en .

cim:ExcIEEEDC3A.efd1 a owl:DatatypeProperty ;
  rdfs:label "efd1"@en ;
  rdfs:domain cim:ExcIEEEDC3A ;
  rdfs:range cim:PU ;
  skos:definition "Exciter voltage at which exciter saturation is defined (<i>E</i><i><sub>FD1</sub></i>) (&gt; 0).  Typical value = 3,375."@en .

cim:ExcIEEEDC3A.efd2 a owl:DatatypeProperty ;
  rdfs:label "efd2"@en ;
  rdfs:domain cim:ExcIEEEDC3A ;
  rdfs:range cim:PU ;
  skos:definition "Exciter voltage at which exciter saturation is defined (<i>E</i><i><sub>FD2</sub></i>) (&gt; 0).  Typical value = 3,15."@en .

cim:ExcIEEEDC3A.exclim a owl:DatatypeProperty ;
  rdfs:label "exclim"@en ;
  rdfs:domain cim:ExcIEEEDC3A ;
  rdfs:range xsd:boolean ;
  skos:definition """
(<i>exclim</i>).  IEEE standard is ambiguous about lower limit on exciter output.
true = a lower limit of zero is applied to integrator output
false = a lower limit of zero is not applied to integrator output.
Typical value = true.
\t"""@en .

cim:ExcIEEEDC3A.ke a owl:DatatypeProperty ;
  rdfs:label "ke"@en ;
  rdfs:domain cim:ExcIEEEDC3A ;
  rdfs:range cim:PU ;
  skos:definition "Exciter constant related to self-excited field (<i>K</i><i><sub>E</sub></i>).  Typical value = 0,05."@en .

cim:ExcIEEEDC3A.kv a owl:DatatypeProperty ;
  rdfs:label "kv"@en ;
  rdfs:domain cim:ExcIEEEDC3A ;
  rdfs:range cim:PU ;
  skos:definition "Fast raise/lower contact setting (<i>K</i><i><sub>V</sub></i>) (&gt; 0).  Typical value = 0,05."@en .

cim:ExcIEEEDC3A.seefd1 a owl:DatatypeProperty ;
  rdfs:label "seefd1"@en ;
  rdfs:domain cim:ExcIEEEDC3A ;
  rdfs:range xsd:float ;
  skos:definition "Exciter saturation function value at the corresponding exciter voltage, <i>E</i><i><sub>FD1</sub></i> (<i>S</i><i><sub>E</sub></i><i>[E</i><i><sub>FD1</sub></i><i>]</i>) (&gt;= 0).  Typical value = 0,267."@en .

cim:ExcIEEEDC3A.seefd2 a owl:DatatypeProperty ;
  rdfs:label "seefd2"@en ;
  rdfs:domain cim:ExcIEEEDC3A ;
  rdfs:range xsd:float ;
  skos:definition "Exciter saturation function value at the corresponding exciter voltage, <i>E</i><i><sub>FD2</sub></i> (<i>S</i><i><sub>E</sub></i><i>[E</i><i><sub>FD2</sub></i><i>]</i>) (&gt;= 0).  Typical value = 0,068."@en .

cim:ExcIEEEDC3A.te a owl:DatatypeProperty ;
  rdfs:label "te"@en ;
  rdfs:domain cim:ExcIEEEDC3A ;
  rdfs:range cim:Seconds ;
  skos:definition "Exciter time constant, integration rate associated with exciter control (<i>T</i><i><sub>E</sub></i>) (&gt; 0).  Typical value = 0,5."@en .

cim:ExcIEEEDC3A.trh a owl:DatatypeProperty ;
  rdfs:label "trh"@en ;
  rdfs:domain cim:ExcIEEEDC3A ;
  rdfs:range cim:Seconds ;
  skos:definition "Rheostat travel time (<i>T</i><i><sub>RH</sub></i>) (&gt; 0).  Typical value = 20."@en .

cim:ExcIEEEDC3A.vrmax a owl:DatatypeProperty ;
  rdfs:label "vrmax"@en ;
  rdfs:domain cim:ExcIEEEDC3A ;
  rdfs:range cim:PU ;
  skos:definition "Maximum voltage regulator output (<i>V</i><i><sub>RMAX</sub></i>) (&gt; 0).  Typical value = 1."@en .

cim:ExcIEEEDC3A.vrmin a owl:DatatypeProperty ;
  rdfs:label "vrmin"@en ;
  rdfs:domain cim:ExcIEEEDC3A ;
  rdfs:range cim:PU ;
  skos:definition "Minimum voltage regulator output (<i>V</i><i><sub>RMIN</sub></i>) (&lt;= 0).  Typical value = 0."@en .

cim:ExcIEEEDC4B.efd1 a owl:DatatypeProperty ;
  rdfs:label "efd1"@en ;
  rdfs:domain cim:ExcIEEEDC4B ;
  rdfs:range cim:PU ;
  skos:definition "Exciter voltage at which exciter saturation is defined (<i>E</i><i><sub>FD1</sub></i>) (&gt; 0).  Typical value = 1,75."@en .

cim:ExcIEEEDC4B.efd2 a owl:DatatypeProperty ;
  rdfs:label "efd2"@en ;
  rdfs:domain cim:ExcIEEEDC4B ;
  rdfs:range cim:PU ;
  skos:definition "Exciter voltage at which exciter saturation is defined (<i>E</i><i><sub>FD2</sub></i>) (&gt; 0).  Typical value = 2,33."@en .

cim:ExcIEEEDC4B.ka a owl:DatatypeProperty ;
  rdfs:label "ka"@en ;
  rdfs:domain cim:ExcIEEEDC4B ;
  rdfs:range cim:PU ;
  skos:definition "Voltage regulator gain (<i>K</i><i><sub>A</sub></i>) (&gt; 0).  Typical value = 1."@en .

cim:ExcIEEEDC4B.kd a owl:DatatypeProperty ;
  rdfs:label "kd"@en ;
  rdfs:domain cim:ExcIEEEDC4B ;
  rdfs:range cim:PU ;
  skos:definition "Regulator derivative gain (<i>K</i><i><sub>D</sub></i>) (&gt;= 0).  Typical value = 20."@en .

cim:ExcIEEEDC4B.ke a owl:DatatypeProperty ;
  rdfs:label "ke"@en ;
  rdfs:domain cim:ExcIEEEDC4B ;
  rdfs:range cim:PU ;
  skos:definition "Exciter constant related to self-excited field (<i>K</i><i><sub>E</sub></i>).  Typical value = 1."@en .

cim:ExcIEEEDC4B.kf a owl:DatatypeProperty ;
  rdfs:label "kf"@en ;
  rdfs:domain cim:ExcIEEEDC4B ;
  rdfs:range cim:PU ;
  skos:definition "Excitation control system stabilizer gain (<i>K</i><i><sub>F</sub></i>) (&gt;= 0).  Typical value = 0."@en .

cim:ExcIEEEDC4B.ki a owl:DatatypeProperty ;
  rdfs:label "ki"@en ;
  rdfs:domain cim:ExcIEEEDC4B ;
  rdfs:range cim:PU ;
  skos:definition "Regulator integral gain (<i>K</i><i><sub>I</sub></i>) (&gt;= 0).  Typical value = 20."@en .

cim:ExcIEEEDC4B.kp a owl:DatatypeProperty ;
  rdfs:label "kp"@en ;
  rdfs:domain cim:ExcIEEEDC4B ;
  rdfs:range cim:PU ;
  skos:definition "Regulator proportional gain (<i>K</i><i><sub>P</sub></i>) (&gt;= 0).  Typical value = 20."@en .

cim:ExcIEEEDC4B.oelin a owl:DatatypeProperty ;
  rdfs:label "oelin"@en ;
  rdfs:domain cim:ExcIEEEDC4B ;
  rdfs:range xsd:boolean ;
  skos:definition """
OEL input (<i>OELin</i>).
true = LV gate
false = subtract from error signal.
Typical value = true.
\t"""@en .

cim:ExcIEEEDC4B.seefd1 a owl:DatatypeProperty ;
  rdfs:label "seefd1"@en ;
  rdfs:domain cim:ExcIEEEDC4B ;
  rdfs:range xsd:float ;
  skos:definition "Exciter saturation function value at the corresponding exciter voltage, <i>E</i><i><sub>FD1</sub></i> (<i>S</i><i><sub>E</sub></i><i>[E</i><i><sub>FD1</sub></i><i>]</i>) (&gt;= 0).  Typical value = 0,08."@en .

cim:ExcIEEEDC4B.seefd2 a owl:DatatypeProperty ;
  rdfs:label "seefd2"@en ;
  rdfs:domain cim:ExcIEEEDC4B ;
  rdfs:range xsd:float ;
  skos:definition "Exciter saturation function value at the corresponding exciter voltage, <i>E</i><i><sub>FD2</sub></i> (<i>S</i><i><sub>E</sub></i><i>[E</i><i><sub>FD2</sub></i><i>]</i>) (&gt;= 0).  Typical value = 0,27."@en .

cim:ExcIEEEDC4B.ta a owl:DatatypeProperty ;
  rdfs:label "ta"@en ;
  rdfs:domain cim:ExcIEEEDC4B ;
  rdfs:range cim:Seconds ;
  skos:definition "Voltage regulator time constant (<i>T</i><i><sub>A</sub></i>) (&gt; 0).  Typical value = 0,2."@en .

cim:ExcIEEEDC4B.td a owl:DatatypeProperty ;
  rdfs:label "td"@en ;
  rdfs:domain cim:ExcIEEEDC4B ;
  rdfs:range cim:Seconds ;
  skos:definition "Regulator derivative filter time constant (<i>T</i><i><sub>D</sub></i>) (&gt; 0 if ExcIEEEDC4B.kd &gt; 0).  Typical value = 0,01."@en .

cim:ExcIEEEDC4B.te a owl:DatatypeProperty ;
  rdfs:label "te"@en ;
  rdfs:domain cim:ExcIEEEDC4B ;
  rdfs:range cim:Seconds ;
  skos:definition "Exciter time constant, integration rate associated with exciter control (<i>T</i><i><sub>E</sub></i>) (&gt; 0).  Typical value = 0,8."@en .

cim:ExcIEEEDC4B.tf a owl:DatatypeProperty ;
  rdfs:label "tf"@en ;
  rdfs:domain cim:ExcIEEEDC4B ;
  rdfs:range cim:Seconds ;
  skos:definition "Excitation control system stabilizer time constant (<i>T</i><i><sub>F</sub></i>) (&gt;= 0).  Typical value = 1."@en .

cim:ExcIEEEDC4B.uelin a owl:DatatypeProperty ;
  rdfs:label "uelin"@en ;
  rdfs:domain cim:ExcIEEEDC4B ;
  rdfs:range xsd:boolean ;
  skos:definition """
UEL input (<i>UELin</i>).
true = HV gate
false = add to error signal.
Typical value = true.
\t"""@en .

cim:ExcIEEEDC4B.vemin a owl:DatatypeProperty ;
  rdfs:label "vemin"@en ;
  rdfs:domain cim:ExcIEEEDC4B ;
  rdfs:range cim:PU ;
  skos:definition "Minimum exciter voltage output (<i>V</i><i><sub>EMIN</sub></i>) (&lt;= 0).  Typical value = 0."@en .

cim:ExcIEEEDC4B.vrmax a owl:DatatypeProperty ;
  rdfs:label "vrmax"@en ;
  rdfs:domain cim:ExcIEEEDC4B ;
  rdfs:range cim:PU ;
  skos:definition "Maximum voltage regulator output (<i>V</i><i><sub>RMAX</sub></i>) (&gt; ExcIEEEDC4B.vrmin).  Typical value = 2,7."@en .

cim:ExcIEEEDC4B.vrmin a owl:DatatypeProperty ;
  rdfs:label "vrmin"@en ;
  rdfs:domain cim:ExcIEEEDC4B ;
  rdfs:range cim:PU ;
  skos:definition "Minimum voltage regulator output (<i>V</i><i><sub>RMIN</sub></i>) (&lt;= 0 and &lt; ExcIEEEDC4B.vrmax).  Typical value = -0,9."@en .

cim:ExcIEEEST1A.ilr a owl:DatatypeProperty ;
  rdfs:label "ilr"@en ;
  rdfs:domain cim:ExcIEEEST1A ;
  rdfs:range cim:PU ;
  skos:definition "Exciter output current limit reference (<i>I</i><i><sub>LR</sub></i><i>)</i>.  Typical value = 0."@en .

cim:ExcIEEEST1A.ka a owl:DatatypeProperty ;
  rdfs:label "ka"@en ;
  rdfs:domain cim:ExcIEEEST1A ;
  rdfs:range cim:PU ;
  skos:definition "Voltage regulator gain (<i>K</i><i><sub>A</sub></i>) (&gt; 0).  Typical value = 190."@en .

cim:ExcIEEEST1A.kc a owl:DatatypeProperty ;
  rdfs:label "kc"@en ;
  rdfs:domain cim:ExcIEEEST1A ;
  rdfs:range cim:PU ;
  skos:definition "Rectifier loading factor proportional to commutating reactance (<i>K</i><i><sub>C</sub></i>) (&gt;= 0). Typical value = 0,08."@en .

cim:ExcIEEEST1A.kf a owl:DatatypeProperty ;
  rdfs:label "kf"@en ;
  rdfs:domain cim:ExcIEEEST1A ;
  rdfs:range cim:PU ;
  skos:definition "Excitation control system stabilizer gains (<i>K</i><i><sub>F</sub></i>) (&gt;= 0).  Typical value = 0."@en .

cim:ExcIEEEST1A.klr a owl:DatatypeProperty ;
  rdfs:label "klr"@en ;
  rdfs:domain cim:ExcIEEEST1A ;
  rdfs:range cim:PU ;
  skos:definition "Exciter output current limiter gain (<i>K</i><i><sub>LR</sub></i>).  Typical value = 0."@en .

cim:ExcIEEEST1A.pssin a owl:DatatypeProperty ;
  rdfs:label "pssin"@en ;
  rdfs:domain cim:ExcIEEEST1A ;
  rdfs:range xsd:boolean ;
  skos:definition """
Selector of the Power System Stabilizer (PSS) input (<i>PSSin</i>).
true = PSS input (<i>Vs</i>) added to error signal
false = PSS input (<i>Vs</i>) added to voltage regulator output.
Typical value = true.
\t"""@en .

cim:ExcIEEEST1A.ta a owl:DatatypeProperty ;
  rdfs:label "ta"@en ;
  rdfs:domain cim:ExcIEEEST1A ;
  rdfs:range cim:Seconds ;
  skos:definition "Voltage regulator time constant (<i>T</i><i><sub>A</sub></i>) (&gt;= 0).  Typical value = 0."@en .

cim:ExcIEEEST1A.tb a owl:DatatypeProperty ;
  rdfs:label "tb"@en ;
  rdfs:domain cim:ExcIEEEST1A ;
  rdfs:range cim:Seconds ;
  skos:definition "Voltage regulator time constant (<i>T</i><i><sub>B</sub></i>) (&gt;= 0).  Typical value = 10."@en .

cim:ExcIEEEST1A.tb1 a owl:DatatypeProperty ;
  rdfs:label "tb1"@en ;
  rdfs:domain cim:ExcIEEEST1A ;
  rdfs:range cim:Seconds ;
  skos:definition "Voltage regulator time constant (<i>T</i><i><sub>B1</sub></i>) (&gt;= 0).  Typical value = 0."@en .

cim:ExcIEEEST1A.tc a owl:DatatypeProperty ;
  rdfs:label "tc"@en ;
  rdfs:domain cim:ExcIEEEST1A ;
  rdfs:range cim:Seconds ;
  skos:definition "Voltage regulator time constant (<i>T</i><i><sub>C</sub></i>) (&gt;= 0).  Typical value = 1."@en .

cim:ExcIEEEST1A.tc1 a owl:DatatypeProperty ;
  rdfs:label "tc1"@en ;
  rdfs:domain cim:ExcIEEEST1A ;
  rdfs:range cim:Seconds ;
  skos:definition "Voltage regulator time constant (<i>T</i><i><sub>C1</sub></i>) (&gt;= 0).  Typical value = 0."@en .

cim:ExcIEEEST1A.tf a owl:DatatypeProperty ;
  rdfs:label "tf"@en ;
  rdfs:domain cim:ExcIEEEST1A ;
  rdfs:range cim:Seconds ;
  skos:definition "Excitation control system stabilizer time constant (<i>T</i><i><sub>F</sub></i>) (&gt;= 0).  Typical value = 1."@en .

cim:ExcIEEEST1A.uelin a owl:DatatypeProperty ;
  rdfs:label "uelin"@en ;
  rdfs:domain cim:ExcIEEEST1A ;
  rdfs:range cim:ExcIEEEST1AUELselectorKind ;
  skos:definition "Selector of the connection of the UEL input (<i>UELin</i>).  Typical value = ignoreUELsignal."@en .

cim:ExcIEEEST1A.vamax a owl:DatatypeProperty ;
  rdfs:label "vamax"@en ;
  rdfs:domain cim:ExcIEEEST1A ;
  rdfs:range cim:PU ;
  skos:definition "Maximum voltage regulator output (<i>V</i><i><sub>AMAX</sub></i>) (&gt; 0).  Typical value = 14,5."@en .

cim:ExcIEEEST1A.vamin a owl:DatatypeProperty ;
  rdfs:label "vamin"@en ;
  rdfs:domain cim:ExcIEEEST1A ;
  rdfs:range cim:PU ;
  skos:definition "Minimum voltage regulator output (<i>V</i><i><sub>AMIN</sub></i>) (&lt; 0).  Typical value = -14,5."@en .

cim:ExcIEEEST1A.vimax a owl:DatatypeProperty ;
  rdfs:label "vimax"@en ;
  rdfs:domain cim:ExcIEEEST1A ;
  rdfs:range cim:PU ;
  skos:definition "Maximum voltage regulator input limit (<i>V</i><i><sub>IMAX</sub></i>) (&gt; 0).  Typical value = 999."@en .

cim:ExcIEEEST1A.vimin a owl:DatatypeProperty ;
  rdfs:label "vimin"@en ;
  rdfs:domain cim:ExcIEEEST1A ;
  rdfs:range cim:PU ;
  skos:definition "Minimum voltage regulator input limit (<i>V</i><i><sub>IMIN</sub></i>) (&lt; 0).  Typical value = -999."@en .

cim:ExcIEEEST1A.vrmax a owl:DatatypeProperty ;
  rdfs:label "vrmax"@en ;
  rdfs:domain cim:ExcIEEEST1A ;
  rdfs:range cim:PU ;
  skos:definition "Maximum voltage regulator outputs (<i>V</i><i><sub>RMAX</sub></i>) (&gt; 0).  Typical value = 7,8."@en .

cim:ExcIEEEST1A.vrmin a owl:DatatypeProperty ;
  rdfs:label "vrmin"@en ;
  rdfs:domain cim:ExcIEEEST1A ;
  rdfs:range cim:PU ;
  skos:definition "Minimum voltage regulator outputs (<i>V</i><i><sub>RMIN</sub></i>) (&lt; 0).  Typical value = -6,7."@en .

cim:ExcIEEEST2A.efdmax a owl:DatatypeProperty ;
  rdfs:label "efdmax"@en ;
  rdfs:domain cim:ExcIEEEST2A ;
  rdfs:range cim:PU ;
  skos:definition "Maximum field voltage (<i>E</i><i><sub>FDMax</sub></i>) (&gt;= 0).  Typical value = 99."@en .

cim:ExcIEEEST2A.ka a owl:DatatypeProperty ;
  rdfs:label "ka"@en ;
  rdfs:domain cim:ExcIEEEST2A ;
  rdfs:range cim:PU ;
  skos:definition "Voltage regulator gain (<i>K</i><i><sub>A</sub></i>) (&gt; 0).  Typical value = 120."@en .

cim:ExcIEEEST2A.kc a owl:DatatypeProperty ;
  rdfs:label "kc"@en ;
  rdfs:domain cim:ExcIEEEST2A ;
  rdfs:range cim:PU ;
  skos:definition "Rectifier loading factor proportional to commutating reactance (<i>K</i><i><sub>C</sub></i>) (&gt;= 0). Typical value = 1,82."@en .

cim:ExcIEEEST2A.ke a owl:DatatypeProperty ;
  rdfs:label "ke"@en ;
  rdfs:domain cim:ExcIEEEST2A ;
  rdfs:range cim:PU ;
  skos:definition "Exciter constant related to self-excited field (<i>K</i><i><sub>E</sub></i>).  Typical value = 1."@en .

cim:ExcIEEEST2A.kf a owl:DatatypeProperty ;
  rdfs:label "kf"@en ;
  rdfs:domain cim:ExcIEEEST2A ;
  rdfs:range cim:PU ;
  skos:definition "Excitation control system stabilizer gains (<i>K</i><i><sub>F</sub></i>) (&gt;= 0).  Typical value = 0,05."@en .

cim:ExcIEEEST2A.ki a owl:DatatypeProperty ;
  rdfs:label "ki"@en ;
  rdfs:domain cim:ExcIEEEST2A ;
  rdfs:range cim:PU ;
  skos:definition "Potential circuit gain coefficient (<i>K</i><i><sub>I</sub></i>) (&gt;= 0).  Typical value = 8."@en .

cim:ExcIEEEST2A.kp a owl:DatatypeProperty ;
  rdfs:label "kp"@en ;
  rdfs:domain cim:ExcIEEEST2A ;
  rdfs:range cim:PU ;
  skos:definition "Potential circuit gain coefficient (<i>K</i><i><sub>P</sub></i>) (&gt;= 0).  Typical value = 4,88."@en .

cim:ExcIEEEST2A.ta a owl:DatatypeProperty ;
  rdfs:label "ta"@en ;
  rdfs:domain cim:ExcIEEEST2A ;
  rdfs:range cim:Seconds ;
  skos:definition "Voltage regulator time constant (<i>T</i><i><sub>A</sub></i>) (&gt; 0).  Typical value = 0,15."@en .

cim:ExcIEEEST2A.te a owl:DatatypeProperty ;
  rdfs:label "te"@en ;
  rdfs:domain cim:ExcIEEEST2A ;
  rdfs:range cim:Seconds ;
  skos:definition "Exciter time constant, integration rate associated with exciter control (<i>T</i><i><sub>E</sub></i>) (&gt; 0).  Typical value = 0,5."@en .

cim:ExcIEEEST2A.tf a owl:DatatypeProperty ;
  rdfs:label "tf"@en ;
  rdfs:domain cim:ExcIEEEST2A ;
  rdfs:range cim:Seconds ;
  skos:definition "Excitation control system stabilizer time constant (<i>T</i><i><sub>F</sub></i>) (&gt;= 0).  Typical value = 1."@en .

cim:ExcIEEEST2A.uelin a owl:DatatypeProperty ;
  rdfs:label "uelin"@en ;
  rdfs:domain cim:ExcIEEEST2A ;
  rdfs:range xsd:boolean ;
  skos:definition """
UEL input (<i>UELin</i>).
true = HV gate
false = add to error signal.
Typical value = true.
\t"""@en .

cim:ExcIEEEST2A.vrmax a owl:DatatypeProperty ;
  rdfs:label "vrmax"@en ;
  rdfs:domain cim:ExcIEEEST2A ;
  rdfs:range cim:PU ;
  skos:definition "Maximum voltage regulator outputs (<i>V</i><i><sub>RMAX</sub></i>) (&gt; 0).  Typical value = 1."@en .

cim:ExcIEEEST2A.vrmin a owl:DatatypeProperty ;
  rdfs:label "vrmin"@en ;
  rdfs:domain cim:ExcIEEEST2A ;
  rdfs:range cim:PU ;
  skos:definition "Minimum voltage regulator outputs (<i>V</i><i><sub>RMIN</sub></i>) (&lt;= 0).  Typical value = 0."@en .

cim:ExcIEEEST3A.ka a owl:DatatypeProperty ;
  rdfs:label "ka"@en ;
  rdfs:domain cim:ExcIEEEST3A ;
  rdfs:range cim:PU ;
  skos:definition "Voltage regulator gain (<i>K</i><i><sub>A</sub></i>) (&gt; 0). This is parameter <i>K</i> in the IEEE standard. Typical value = 200."@en .

cim:ExcIEEEST3A.kc a owl:DatatypeProperty ;
  rdfs:label "kc"@en ;
  rdfs:domain cim:ExcIEEEST3A ;
  rdfs:range cim:PU ;
  skos:definition "Rectifier loading factor proportional to commutating reactance (<i>K</i><i><sub>C</sub></i>) (&gt;= 0). Typical value = 0,2."@en .

cim:ExcIEEEST3A.kg a owl:DatatypeProperty ;
  rdfs:label "kg"@en ;
  rdfs:domain cim:ExcIEEEST3A ;
  rdfs:range cim:PU ;
  skos:definition "Feedback gain constant of the inner loop field regulator (<i>K</i><i><sub>G</sub></i>) (&gt;= 0).  Typical value = 1."@en .

cim:ExcIEEEST3A.ki a owl:DatatypeProperty ;
  rdfs:label "ki"@en ;
  rdfs:domain cim:ExcIEEEST3A ;
  rdfs:range cim:PU ;
  skos:definition "Potential circuit gain coefficient (<i>K</i><i><sub>I</sub></i>) (&gt;= 0).  Typical value = 0."@en .

cim:ExcIEEEST3A.km a owl:DatatypeProperty ;
  rdfs:label "km"@en ;
  rdfs:domain cim:ExcIEEEST3A ;
  rdfs:range cim:PU ;
  skos:definition "Forward gain constant of the inner loop field regulator (<i>K</i><i><sub>M</sub></i>) (&gt; 0).  Typical value = 7,93."@en .

cim:ExcIEEEST3A.kp a owl:DatatypeProperty ;
  rdfs:label "kp"@en ;
  rdfs:domain cim:ExcIEEEST3A ;
  rdfs:range cim:PU ;
  skos:definition "Potential circuit gain coefficient (<i>K</i><i><sub>P</sub></i>) (&gt; 0).  Typical value = 6,15."@en .

cim:ExcIEEEST3A.ta a owl:DatatypeProperty ;
  rdfs:label "ta"@en ;
  rdfs:domain cim:ExcIEEEST3A ;
  rdfs:range cim:Seconds ;
  skos:definition "Voltage regulator time constant (<i>T</i><i><sub>A</sub></i>) (&gt;= 0).  Typical value = 0."@en .

cim:ExcIEEEST3A.tb a owl:DatatypeProperty ;
  rdfs:label "tb"@en ;
  rdfs:domain cim:ExcIEEEST3A ;
  rdfs:range cim:Seconds ;
  skos:definition "Voltage regulator time constant (<i>T</i><i><sub>B</sub></i>) (&gt;= 0).  Typical value = 10."@en .

cim:ExcIEEEST3A.tc a owl:DatatypeProperty ;
  rdfs:label "tc"@en ;
  rdfs:domain cim:ExcIEEEST3A ;
  rdfs:range cim:Seconds ;
  skos:definition "Voltage regulator time constant (<i>T</i><i><sub>C</sub></i>) (&gt;= 0).  Typical value = 1."@en .

cim:ExcIEEEST3A.thetap a owl:DatatypeProperty ;
  rdfs:label "thetap"@en ;
  rdfs:domain cim:ExcIEEEST3A ;
  rdfs:range cim:AngleDegrees ;
  skos:definition "Potential circuit phase angle (<i>thetap</i>).  Typical value = 0."@en .

cim:ExcIEEEST3A.tm a owl:DatatypeProperty ;
  rdfs:label "tm"@en ;
  rdfs:domain cim:ExcIEEEST3A ;
  rdfs:range cim:Seconds ;
  skos:definition "Forward time constant of inner loop field regulator (<i>T</i><i><sub>M</sub></i>) (&gt; 0).  Typical value = 0,4."@en .

cim:ExcIEEEST3A.vbmax a owl:DatatypeProperty ;
  rdfs:label "vbmax"@en ;
  rdfs:domain cim:ExcIEEEST3A ;
  rdfs:range cim:PU ;
  skos:definition "Maximum excitation voltage (<i>V</i><i><sub>BMax</sub></i>) (&gt; 0).  Typical value = 6,9."@en .

cim:ExcIEEEST3A.vgmax a owl:DatatypeProperty ;
  rdfs:label "vgmax"@en ;
  rdfs:domain cim:ExcIEEEST3A ;
  rdfs:range cim:PU ;
  skos:definition "Maximum inner loop feedback voltage (<i>V</i><i><sub>GMax</sub></i>) (&gt;= 0).  Typical value = 5,8."@en .

cim:ExcIEEEST3A.vimax a owl:DatatypeProperty ;
  rdfs:label "vimax"@en ;
  rdfs:domain cim:ExcIEEEST3A ;
  rdfs:range cim:PU ;
  skos:definition "Maximum voltage regulator input limit (<i>V</i><i><sub>IMAX</sub></i>) (&gt; 0).  Typical value = 0,2."@en .

cim:ExcIEEEST3A.vimin a owl:DatatypeProperty ;
  rdfs:label "vimin"@en ;
  rdfs:domain cim:ExcIEEEST3A ;
  rdfs:range cim:PU ;
  skos:definition "Minimum voltage regulator input limit (<i>V</i><i><sub>IMIN</sub></i>) (&lt; 0).  Typical value = -0,2."@en .

cim:ExcIEEEST3A.vmmax a owl:DatatypeProperty ;
  rdfs:label "vmmax"@en ;
  rdfs:domain cim:ExcIEEEST3A ;
  rdfs:range cim:PU ;
  skos:definition "Maximum inner loop output (<i>V</i><i><sub>MMax</sub></i>) (&gt; 0).  Typical value = 1."@en .

cim:ExcIEEEST3A.vmmin a owl:DatatypeProperty ;
  rdfs:label "vmmin"@en ;
  rdfs:domain cim:ExcIEEEST3A ;
  rdfs:range cim:PU ;
  skos:definition "Minimum inner loop output (<i>V</i><i><sub>MMin</sub></i>) (&lt;= 0).  Typical value = 0."@en .

cim:ExcIEEEST3A.vrmax a owl:DatatypeProperty ;
  rdfs:label "vrmax"@en ;
  rdfs:domain cim:ExcIEEEST3A ;
  rdfs:range cim:PU ;
  skos:definition "Maximum voltage regulator output (<i>V</i><i><sub>RMAX</sub></i>) (&gt; 0).  Typical value = 10."@en .

cim:ExcIEEEST3A.vrmin a owl:DatatypeProperty ;
  rdfs:label "vrmin"@en ;
  rdfs:domain cim:ExcIEEEST3A ;
  rdfs:range cim:PU ;
  skos:definition "Minimum voltage regulator output (<i>V</i><i><sub>RMIN</sub></i>) (&lt; 0).  Typical value = -10."@en .

cim:ExcIEEEST3A.xl a owl:DatatypeProperty ;
  rdfs:label "xl"@en ;
  rdfs:domain cim:ExcIEEEST3A ;
  rdfs:range cim:PU ;
  skos:definition "Reactance associated with potential source (<i>X</i><i><sub>L</sub></i>) (&gt;= 0).  Typical value = 0,081."@en .

cim:ExcIEEEST4B.kc a owl:DatatypeProperty ;
  rdfs:label "kc"@en ;
  rdfs:domain cim:ExcIEEEST4B ;
  rdfs:range cim:PU ;
  skos:definition "Rectifier loading factor proportional to commutating reactance (<i>K</i><i><sub>C</sub></i>) (&gt;= 0). Typical value = 0,113."@en .

cim:ExcIEEEST4B.kg a owl:DatatypeProperty ;
  rdfs:label "kg"@en ;
  rdfs:domain cim:ExcIEEEST4B ;
  rdfs:range cim:PU ;
  skos:definition "Feedback gain constant of the inner loop field regulator (<i>K</i><i><sub>G</sub></i>) (&gt;= 0).  Typical value = 0."@en .

cim:ExcIEEEST4B.ki a owl:DatatypeProperty ;
  rdfs:label "ki"@en ;
  rdfs:domain cim:ExcIEEEST4B ;
  rdfs:range cim:PU ;
  skos:definition "Potential circuit gain coefficient (<i>K</i><i><sub>I</sub></i>) (&gt;= 0).  Typical value = 0."@en .

cim:ExcIEEEST4B.kim a owl:DatatypeProperty ;
  rdfs:label "kim"@en ;
  rdfs:domain cim:ExcIEEEST4B ;
  rdfs:range cim:PU ;
  skos:definition "Voltage regulator integral gain output (<i>K</i><i><sub>IM</sub></i>).  Typical value = 0."@en .

cim:ExcIEEEST4B.kir a owl:DatatypeProperty ;
  rdfs:label "kir"@en ;
  rdfs:domain cim:ExcIEEEST4B ;
  rdfs:range cim:PU ;
  skos:definition "Voltage regulator integral gain (<i>K</i><i><sub>IR</sub></i>).  Typical value = 10,75."@en .

cim:ExcIEEEST4B.kp a owl:DatatypeProperty ;
  rdfs:label "kp"@en ;
  rdfs:domain cim:ExcIEEEST4B ;
  rdfs:range cim:PU ;
  skos:definition "Potential circuit gain coefficient (<i>K</i><i><sub>P</sub></i>) (&gt; 0).  Typical value = 9,3."@en .

cim:ExcIEEEST4B.kpm a owl:DatatypeProperty ;
  rdfs:label "kpm"@en ;
  rdfs:domain cim:ExcIEEEST4B ;
  rdfs:range cim:PU ;
  skos:definition "Voltage regulator proportional gain output (<i>K</i><i><sub>PM</sub></i>).  Typical value = 1."@en .

cim:ExcIEEEST4B.kpr a owl:DatatypeProperty ;
  rdfs:label "kpr"@en ;
  rdfs:domain cim:ExcIEEEST4B ;
  rdfs:range cim:PU ;
  skos:definition "Voltage regulator proportional gain (<i>K</i><i><sub>PR</sub></i>).  Typical value = 10,75."@en .

cim:ExcIEEEST4B.ta a owl:DatatypeProperty ;
  rdfs:label "ta"@en ;
  rdfs:domain cim:ExcIEEEST4B ;
  rdfs:range cim:Seconds ;
  skos:definition "Voltage regulator time constant (<i>T</i><i><sub>A</sub></i>) (&gt;= 0).  Typical value = 0,02."@en .

cim:ExcIEEEST4B.thetap a owl:DatatypeProperty ;
  rdfs:label "thetap"@en ;
  rdfs:domain cim:ExcIEEEST4B ;
  rdfs:range cim:AngleDegrees ;
  skos:definition "Potential circuit phase angle (<i>thetap</i>).  Typical value = 0."@en .

cim:ExcIEEEST4B.vbmax a owl:DatatypeProperty ;
  rdfs:label "vbmax"@en ;
  rdfs:domain cim:ExcIEEEST4B ;
  rdfs:range cim:PU ;
  skos:definition "Maximum excitation voltage (<i>V</i><i><sub>BMax</sub></i>) (&gt; 0).  Typical value = 11,63."@en .

cim:ExcIEEEST4B.vmmax a owl:DatatypeProperty ;
  rdfs:label "vmmax"@en ;
  rdfs:domain cim:ExcIEEEST4B ;
  rdfs:range cim:PU ;
  skos:definition "Maximum inner loop output (<i>V</i><i><sub>MMax</sub></i>) (&gt; ExcIEEEST4B.vmmin).  Typical value = 99."@en .

cim:ExcIEEEST4B.vmmin a owl:DatatypeProperty ;
  rdfs:label "vmmin"@en ;
  rdfs:domain cim:ExcIEEEST4B ;
  rdfs:range cim:PU ;
  skos:definition "Minimum inner loop output (<i>V</i><i><sub>MMin</sub></i>) (&lt; ExcIEEEST4B.vmmax).  Typical value = -99."@en .

cim:ExcIEEEST4B.vrmax a owl:DatatypeProperty ;
  rdfs:label "vrmax"@en ;
  rdfs:domain cim:ExcIEEEST4B ;
  rdfs:range cim:PU ;
  skos:definition "Maximum voltage regulator output (<i>V</i><i><sub>RMAX</sub></i>) (&gt; 0).  Typical value = 1."@en .

cim:ExcIEEEST4B.vrmin a owl:DatatypeProperty ;
  rdfs:label "vrmin"@en ;
  rdfs:domain cim:ExcIEEEST4B ;
  rdfs:range cim:PU ;
  skos:definition "Minimum voltage regulator output (<i>V</i><i><sub>RMIN</sub></i>) (&lt; 0).  Typical value = -0,87."@en .

cim:ExcIEEEST4B.xl a owl:DatatypeProperty ;
  rdfs:label "xl"@en ;
  rdfs:domain cim:ExcIEEEST4B ;
  rdfs:range cim:PU ;
  skos:definition "Reactance associated with potential source (<i>X</i><i><sub>L</sub></i>) (&gt;= 0).  Typical value = 0,124."@en .

cim:ExcIEEEST5B.kc a owl:DatatypeProperty ;
  rdfs:label "kc"@en ;
  rdfs:domain cim:ExcIEEEST5B ;
  rdfs:range cim:PU ;
  skos:definition "Rectifier regulation factor (<i>K</i><i><sub>C</sub></i>) (&gt;= 0).  Typical value = 0,004."@en .

cim:ExcIEEEST5B.kr a owl:DatatypeProperty ;
  rdfs:label "kr"@en ;
  rdfs:domain cim:ExcIEEEST5B ;
  rdfs:range cim:PU ;
  skos:definition "Regulator gain (<i>K</i><i><sub>R</sub></i>) (&gt; 0).  Typical value = 200."@en .

cim:ExcIEEEST5B.t1 a owl:DatatypeProperty ;
  rdfs:label "t1"@en ;
  rdfs:domain cim:ExcIEEEST5B ;
  rdfs:range cim:Seconds ;
  skos:definition "Firing circuit time constant (<i>T1</i>) (&gt;= 0).  Typical value = 0,004."@en .

cim:ExcIEEEST5B.tb1 a owl:DatatypeProperty ;
  rdfs:label "tb1"@en ;
  rdfs:domain cim:ExcIEEEST5B ;
  rdfs:range cim:Seconds ;
  skos:definition "Regulator lag time constant (<i>T</i><i><sub>B1</sub></i>) (&gt;= 0).  Typical value = 6."@en .

cim:ExcIEEEST5B.tb2 a owl:DatatypeProperty ;
  rdfs:label "tb2"@en ;
  rdfs:domain cim:ExcIEEEST5B ;
  rdfs:range cim:Seconds ;
  skos:definition "Regulator lag time constant (<i>T</i><i><sub>B2</sub></i>) (&gt;= 0).  Typical value = 0,01."@en .

cim:ExcIEEEST5B.tc1 a owl:DatatypeProperty ;
  rdfs:label "tc1"@en ;
  rdfs:domain cim:ExcIEEEST5B ;
  rdfs:range cim:Seconds ;
  skos:definition "Regulator lead time constant (<i>T</i><i><sub>C1</sub></i>) (&gt;= 0).  Typical value = 0,8."@en .

cim:ExcIEEEST5B.tc2 a owl:DatatypeProperty ;
  rdfs:label "tc2"@en ;
  rdfs:domain cim:ExcIEEEST5B ;
  rdfs:range cim:Seconds ;
  skos:definition "Regulator lead time constant (<i>T</i><i><sub>C2</sub></i>) (&gt;= 0).  Typical value = 0,08."@en .

cim:ExcIEEEST5B.tob1 a owl:DatatypeProperty ;
  rdfs:label "tob1"@en ;
  rdfs:domain cim:ExcIEEEST5B ;
  rdfs:range cim:Seconds ;
  skos:definition "OEL lag time constant (<i>T</i><i><sub>OB1</sub></i>) (&gt;= 0).  Typical value = 2."@en .

cim:ExcIEEEST5B.tob2 a owl:DatatypeProperty ;
  rdfs:label "tob2"@en ;
  rdfs:domain cim:ExcIEEEST5B ;
  rdfs:range cim:Seconds ;
  skos:definition "OEL lag time constant (<i>T</i><i><sub>OB2</sub></i>) (&gt;= 0).  Typical value = 0,08."@en .

cim:ExcIEEEST5B.toc1 a owl:DatatypeProperty ;
  rdfs:label "toc1"@en ;
  rdfs:domain cim:ExcIEEEST5B ;
  rdfs:range cim:Seconds ;
  skos:definition "OEL lead time constant (<i>T</i><i><sub>OC1</sub></i>) (&gt;= 0).  Typical value = 0,1."@en .

cim:ExcIEEEST5B.toc2 a owl:DatatypeProperty ;
  rdfs:label "toc2"@en ;
  rdfs:domain cim:ExcIEEEST5B ;
  rdfs:range cim:Seconds ;
  skos:definition "OEL lead time constant (<i>T</i><i><sub>OC2</sub></i>) (&gt;= 0).  Typical value = 0,08."@en .

cim:ExcIEEEST5B.tub1 a owl:DatatypeProperty ;
  rdfs:label "tub1"@en ;
  rdfs:domain cim:ExcIEEEST5B ;
  rdfs:range cim:Seconds ;
  skos:definition "UEL lag time constant (<i>T</i><i><sub>UB1</sub></i>) (&gt;= 0).  Typical value = 10."@en .

cim:ExcIEEEST5B.tub2 a owl:DatatypeProperty ;
  rdfs:label "tub2"@en ;
  rdfs:domain cim:ExcIEEEST5B ;
  rdfs:range cim:Seconds ;
  skos:definition "UEL lag time constant (<i>T</i><i><sub>UB2</sub></i>) (&gt;= 0).  Typical value = 0,05."@en .

cim:ExcIEEEST5B.tuc1 a owl:DatatypeProperty ;
  rdfs:label "tuc1"@en ;
  rdfs:domain cim:ExcIEEEST5B ;
  rdfs:range cim:Seconds ;
  skos:definition "UEL lead time constant (<i>T</i><i><sub>UC1</sub></i>) (&gt;= 0).  Typical value = 2."@en .

cim:ExcIEEEST5B.tuc2 a owl:DatatypeProperty ;
  rdfs:label "tuc2"@en ;
  rdfs:domain cim:ExcIEEEST5B ;
  rdfs:range cim:Seconds ;
  skos:definition "UEL lead time constant (<i>T</i><i><sub>UC2</sub></i>) (&gt;= 0).  Typical value = 0,1."@en .

cim:ExcIEEEST5B.vrmax a owl:DatatypeProperty ;
  rdfs:label "vrmax"@en ;
  rdfs:domain cim:ExcIEEEST5B ;
  rdfs:range cim:PU ;
  skos:definition "Maximum voltage regulator output (<i>V</i><i><sub>RMAX</sub></i>) (&gt; 0).  Typical value = 5."@en .

cim:ExcIEEEST5B.vrmin a owl:DatatypeProperty ;
  rdfs:label "vrmin"@en ;
  rdfs:domain cim:ExcIEEEST5B ;
  rdfs:range cim:PU ;
  skos:definition "Minimum voltage regulator output (<i>V</i><i><sub>RMIN</sub></i>) (&lt; 0).  Typical value = -4."@en .

cim:ExcIEEEST6B.ilr a owl:DatatypeProperty ;
  rdfs:label "ilr"@en ;
  rdfs:domain cim:ExcIEEEST6B ;
  rdfs:range cim:PU ;
  skos:definition "Exciter output current limit reference (<i>I</i><i><sub>LR</sub></i>) (&gt; 0).  Typical value = 4,164."@en .

cim:ExcIEEEST6B.kci a owl:DatatypeProperty ;
  rdfs:label "kci"@en ;
  rdfs:domain cim:ExcIEEEST6B ;
  rdfs:range cim:PU ;
  skos:definition "Exciter output current limit adjustment (<i>K</i><i><sub>CI</sub></i>) (&gt; 0).  Typical value = 1,0577."@en .

cim:ExcIEEEST6B.kff a owl:DatatypeProperty ;
  rdfs:label "kff"@en ;
  rdfs:domain cim:ExcIEEEST6B ;
  rdfs:range cim:PU ;
  skos:definition "Pre-control gain constant of the inner loop field regulator (<i>K</i><i><sub>FF</sub></i>). Typical value = 1."@en .

cim:ExcIEEEST6B.kg a owl:DatatypeProperty ;
  rdfs:label "kg"@en ;
  rdfs:domain cim:ExcIEEEST6B ;
  rdfs:range cim:PU ;
  skos:definition "Feedback gain constant of the inner loop field regulator (<i>K</i><i><sub>G</sub></i>) (&gt;= 0).  Typical value = 1."@en .

cim:ExcIEEEST6B.kia a owl:DatatypeProperty ;
  rdfs:label "kia"@en ;
  rdfs:domain cim:ExcIEEEST6B ;
  rdfs:range cim:PU ;
  skos:definition "Voltage regulator integral gain (<i>K</i><i><sub>IA</sub></i>) (&gt; 0).  Typical value = 45,094."@en .

cim:ExcIEEEST6B.klr a owl:DatatypeProperty ;
  rdfs:label "klr"@en ;
  rdfs:domain cim:ExcIEEEST6B ;
  rdfs:range cim:PU ;
  skos:definition "Exciter output current limiter gain (<i>K</i><i><sub>LR</sub></i>) (&gt; 0).  Typical value = 17,33."@en .

cim:ExcIEEEST6B.km a owl:DatatypeProperty ;
  rdfs:label "km"@en ;
  rdfs:domain cim:ExcIEEEST6B ;
  rdfs:range cim:PU ;
  skos:definition "Forward gain constant of the inner loop field regulator (<i>K</i><i><sub>M</sub></i>).  Typical value = 1."@en .

cim:ExcIEEEST6B.kpa a owl:DatatypeProperty ;
  rdfs:label "kpa"@en ;
  rdfs:domain cim:ExcIEEEST6B ;
  rdfs:range cim:PU ;
  skos:definition "Voltage regulator proportional gain (<u>K</u><u><sub>PA</sub></u>) (&gt; 0).  Typical value = 18,038."@en .

cim:ExcIEEEST6B.oelin a owl:DatatypeProperty ;
  rdfs:label "oelin"@en ;
  rdfs:domain cim:ExcIEEEST6B ;
  rdfs:range cim:ExcST6BOELselectorKind ;
  skos:definition "OEL input selector (<i>OELin</i>). Typical value = noOELinput."@en .

cim:ExcIEEEST6B.tg a owl:DatatypeProperty ;
  rdfs:label "tg"@en ;
  rdfs:domain cim:ExcIEEEST6B ;
  rdfs:range cim:Seconds ;
  skos:definition "Feedback time constant of inner loop field voltage regulator (<i>T</i><i><sub>G</sub></i>) (&gt;= 0). Typical value = 0,02."@en .

cim:ExcIEEEST6B.vamax a owl:DatatypeProperty ;
  rdfs:label "vamax"@en ;
  rdfs:domain cim:ExcIEEEST6B ;
  rdfs:range cim:PU ;
  skos:definition "Maximum voltage regulator output (V<i><sub>AMAX</sub></i>) (&gt; 0).  Typical value = 4,81."@en .

cim:ExcIEEEST6B.vamin a owl:DatatypeProperty ;
  rdfs:label "vamin"@en ;
  rdfs:domain cim:ExcIEEEST6B ;
  rdfs:range cim:PU ;
  skos:definition "Minimum voltage regulator output (<i>V</i><i><sub>AMIN</sub></i>) (&lt; 0).  Typical value = -3,85."@en .

cim:ExcIEEEST6B.vrmax a owl:DatatypeProperty ;
  rdfs:label "vrmax"@en ;
  rdfs:domain cim:ExcIEEEST6B ;
  rdfs:range cim:PU ;
  skos:definition "Maximum voltage regulator output (<i>V</i><i><sub>RMAX</sub></i>) (&gt; 0).  Typical value = 4,81."@en .

cim:ExcIEEEST6B.vrmin a owl:DatatypeProperty ;
  rdfs:label "vrmin"@en ;
  rdfs:domain cim:ExcIEEEST6B ;
  rdfs:range cim:PU ;
  skos:definition "Minimum voltage regulator output (<i>V</i><i><sub>RMIN</sub></i>) (&lt; 0).  Typical value = -3,85."@en .

cim:ExcIEEEST7B.kh a owl:DatatypeProperty ;
  rdfs:label "kh"@en ;
  rdfs:domain cim:ExcIEEEST7B ;
  rdfs:range cim:PU ;
  skos:definition "High-value gate feedback gain (<i>K</i><i><sub>H</sub></i>) (&gt;= 0).  Typical value = 1."@en .

cim:ExcIEEEST7B.kia a owl:DatatypeProperty ;
  rdfs:label "kia"@en ;
  rdfs:domain cim:ExcIEEEST7B ;
  rdfs:range cim:PU ;
  skos:definition "Voltage regulator integral gain (<i>K</i><i><sub>IA</sub></i>) (&gt;= 0).  Typical value = 1."@en .

cim:ExcIEEEST7B.kl a owl:DatatypeProperty ;
  rdfs:label "kl"@en ;
  rdfs:domain cim:ExcIEEEST7B ;
  rdfs:range cim:PU ;
  skos:definition "Low-value gate feedback gain (<i>K</i><i><sub>L</sub></i>) (&gt;= 0).  Typical value = 1."@en .

cim:ExcIEEEST7B.kpa a owl:DatatypeProperty ;
  rdfs:label "kpa"@en ;
  rdfs:domain cim:ExcIEEEST7B ;
  rdfs:range cim:PU ;
  skos:definition "Voltage regulator proportional gain (<i>K</i><i><sub>PA</sub></i>) (&gt; 0).  Typical value = 40."@en .

cim:ExcIEEEST7B.oelin a owl:DatatypeProperty ;
  rdfs:label "oelin"@en ;
  rdfs:domain cim:ExcIEEEST7B ;
  rdfs:range cim:ExcST7BOELselectorKind ;
  skos:definition "OEL input selector (<i>OELin</i>).  Typical value = noOELinput."@en .

cim:ExcIEEEST7B.tb a owl:DatatypeProperty ;
  rdfs:label "tb"@en ;
  rdfs:domain cim:ExcIEEEST7B ;
  rdfs:range cim:Seconds ;
  skos:definition "Regulator lag time constant (<i>T</i><i><sub>B</sub></i>) (&gt;= 0).  Typical value = 1."@en .

cim:ExcIEEEST7B.tc a owl:DatatypeProperty ;
  rdfs:label "tc"@en ;
  rdfs:domain cim:ExcIEEEST7B ;
  rdfs:range cim:Seconds ;
  skos:definition "Regulator lead time constant (<i>T</i><i><sub>C</sub></i>) (&gt;= 0).  Typical value = 1."@en .

cim:ExcIEEEST7B.tf a owl:DatatypeProperty ;
  rdfs:label "tf"@en ;
  rdfs:domain cim:ExcIEEEST7B ;
  rdfs:range cim:Seconds ;
  skos:definition "Excitation control system stabilizer time constant (<i>T</i><i><sub>F</sub></i>) (&gt;= 0).  Typical value = 1."@en .

cim:ExcIEEEST7B.tg a owl:DatatypeProperty ;
  rdfs:label "tg"@en ;
  rdfs:domain cim:ExcIEEEST7B ;
  rdfs:range cim:Seconds ;
  skos:definition "Feedback time constant of inner loop field voltage regulator (<i>T</i><i><sub>G</sub></i>) (&gt;= 0). Typical value = 1."@en .

cim:ExcIEEEST7B.tia a owl:DatatypeProperty ;
  rdfs:label "tia"@en ;
  rdfs:domain cim:ExcIEEEST7B ;
  rdfs:range cim:Seconds ;
  skos:definition "Feedback time constant (<i>T</i><i><sub>IA</sub></i>) (&gt;= 0).  Typical value = 3."@en .

cim:ExcIEEEST7B.uelin a owl:DatatypeProperty ;
  rdfs:label "uelin"@en ;
  rdfs:domain cim:ExcIEEEST7B ;
  rdfs:range cim:ExcST7BUELselectorKind ;
  skos:definition "UEL input selector (<i>UELin</i>). Typical value = noUELinput."@en .

cim:ExcIEEEST7B.vmax a owl:DatatypeProperty ;
  rdfs:label "vmax"@en ;
  rdfs:domain cim:ExcIEEEST7B ;
  rdfs:range cim:PU ;
  skos:definition "Maximum voltage reference signal (<i>V</i><i><sub>MAX</sub></i>) (&gt; 0 and &gt; ExcIEEEST7B.vmin).  Typical value = 1,1."@en .

cim:ExcIEEEST7B.vmin a owl:DatatypeProperty ;
  rdfs:label "vmin"@en ;
  rdfs:domain cim:ExcIEEEST7B ;
  rdfs:range cim:PU ;
  skos:definition "Minimum voltage reference signal (<i>V</i><i><sub>MIN</sub></i>) (&gt; 0 and &lt; ExcIEEEST7B.vmax).  Typical value = 0,9."@en .

cim:ExcIEEEST7B.vrmax a owl:DatatypeProperty ;
  rdfs:label "vrmax"@en ;
  rdfs:domain cim:ExcIEEEST7B ;
  rdfs:range cim:PU ;
  skos:definition "Maximum voltage regulator output (<i>V</i><i><sub>RMAX</sub></i>) (&gt; 0).  Typical value = 5."@en .

cim:ExcIEEEST7B.vrmin a owl:DatatypeProperty ;
  rdfs:label "vrmin"@en ;
  rdfs:domain cim:ExcIEEEST7B ;
  rdfs:range cim:PU ;
  skos:definition "Minimum voltage regulator output (<i>V</i><i><sub>RMIN</sub></i>) (&lt; 0).  Typical value = -4,5."@en .

cim:ExcNI.busFedSelector a owl:DatatypeProperty ;
  rdfs:label "busFedSelector"@en ;
  rdfs:domain cim:ExcNI ;
  rdfs:range xsd:boolean ;
  skos:definition """
Fed by selector (<i>BusFedSelector</i>). 
true = bus fed (switch is closed)
false = solid fed (switch is open).
Typical value = true.
\t"""@en .

cim:ExcNI.ka a owl:DatatypeProperty ;
  rdfs:label "ka"@en ;
  rdfs:domain cim:ExcNI ;
  rdfs:range cim:PU ;
  skos:definition "Voltage regulator gain (<i>Ka</i>) (&gt; 0).  Typical value = 210."@en .

cim:ExcNI.kf a owl:DatatypeProperty ;
  rdfs:label "kf"@en ;
  rdfs:domain cim:ExcNI ;
  rdfs:range cim:PU ;
  skos:definition "Excitation control system stabilizer gain (<i>Kf</i>) (&gt; 0).  Typical value 0,01."@en .

cim:ExcNI.r a owl:DatatypeProperty ;
  rdfs:label "r"@en ;
  rdfs:domain cim:ExcNI ;
  rdfs:range cim:PU ;
  skos:definition """
<i>rc</i> / <i>rfd</i> (<i>R</i>) (&gt;= 0). 
0 means exciter has negative current capability
&gt; 0 means exciter does not have negative current capability.  
Typical value = 5.
\t"""@en .

cim:ExcNI.ta a owl:DatatypeProperty ;
  rdfs:label "ta"@en ;
  rdfs:domain cim:ExcNI ;
  rdfs:range cim:Seconds ;
  skos:definition "Voltage regulator time constant (<i>Ta</i>) (&gt; 0).  Typical value = 0,02."@en .

cim:ExcNI.tf1 a owl:DatatypeProperty ;
  rdfs:label "tf1"@en ;
  rdfs:domain cim:ExcNI ;
  rdfs:range cim:Seconds ;
  skos:definition "Excitation control system stabilizer time constant (<i>Tf1</i>) (&gt; 0). Typical value = 1,0."@en .

cim:ExcNI.tf2 a owl:DatatypeProperty ;
  rdfs:label "tf2"@en ;
  rdfs:domain cim:ExcNI ;
  rdfs:range cim:Seconds ;
  skos:definition "Excitation control system stabilizer time constant (<i>Tf2</i>) (&gt; 0). Typical value = 0,1."@en .

cim:ExcNI.tr a owl:DatatypeProperty ;
  rdfs:label "tr"@en ;
  rdfs:domain cim:ExcNI ;
  rdfs:range cim:Seconds ;
  skos:definition "Time constant (<i>Tr</i>) (&gt;= 0). Typical value = 0,02."@en .

cim:ExcNI.vrmax a owl:DatatypeProperty ;
  rdfs:label "vrmax"@en ;
  rdfs:domain cim:ExcNI ;
  rdfs:range cim:PU ;
  skos:definition "Maximum voltage regulator ouput (<i>Vrmax</i>) (&gt; ExcNI.vrmin). Typical value = 5,0."@en .

cim:ExcNI.vrmin a owl:DatatypeProperty ;
  rdfs:label "vrmin"@en ;
  rdfs:domain cim:ExcNI ;
  rdfs:range cim:PU ;
  skos:definition "Minimum voltage regulator ouput (<i>Vrmin</i>) (&lt; ExcNI.vrmax). Typical value = -2,0."@en .

cim:ExcOEX3T.e1 a owl:DatatypeProperty ;
  rdfs:label "e1"@en ;
  rdfs:domain cim:ExcOEX3T ;
  rdfs:range cim:PU ;
  skos:definition "Saturation parameter (<i>E</i><i><sub>1</sub></i>)."@en .

cim:ExcOEX3T.e2 a owl:DatatypeProperty ;
  rdfs:label "e2"@en ;
  rdfs:domain cim:ExcOEX3T ;
  rdfs:range cim:PU ;
  skos:definition "Saturation parameter (<i>E</i><i><sub>2</sub></i>)."@en .

cim:ExcOEX3T.ka a owl:DatatypeProperty ;
  rdfs:label "ka"@en ;
  rdfs:domain cim:ExcOEX3T ;
  rdfs:range cim:PU ;
  skos:definition "Gain (<i>K</i><i><sub>A</sub></i>)."@en .

cim:ExcOEX3T.kc a owl:DatatypeProperty ;
  rdfs:label "kc"@en ;
  rdfs:domain cim:ExcOEX3T ;
  rdfs:range cim:PU ;
  skos:definition "Gain (<i>K</i><i><sub>C</sub></i>)."@en .

cim:ExcOEX3T.kd a owl:DatatypeProperty ;
  rdfs:label "kd"@en ;
  rdfs:domain cim:ExcOEX3T ;
  rdfs:range cim:PU ;
  skos:definition "Gain (<i>K</i><i><sub>D</sub></i>)."@en .

cim:ExcOEX3T.ke a owl:DatatypeProperty ;
  rdfs:label "ke"@en ;
  rdfs:domain cim:ExcOEX3T ;
  rdfs:range cim:PU ;
  skos:definition "Gain (<i>K</i><i><sub>E</sub></i>)."@en .

cim:ExcOEX3T.kf a owl:DatatypeProperty ;
  rdfs:label "kf"@en ;
  rdfs:domain cim:ExcOEX3T ;
  rdfs:range cim:PU ;
  skos:definition "Gain (<i>K</i><i><sub>F</sub></i>)."@en .

cim:ExcOEX3T.see1 a owl:DatatypeProperty ;
  rdfs:label "see1"@en ;
  rdfs:domain cim:ExcOEX3T ;
  rdfs:range cim:PU ;
  skos:definition "Saturation parameter (<i>S</i><i><sub>E</sub></i><i>[E</i><i><sub>1</sub></i><i>]</i>)."@en .

cim:ExcOEX3T.see2 a owl:DatatypeProperty ;
  rdfs:label "see2"@en ;
  rdfs:domain cim:ExcOEX3T ;
  rdfs:range cim:PU ;
  skos:definition "Saturation parameter (<i>S</i><i><sub>E</sub></i><i>[E</i><i><sub>2</sub></i><i>]</i>)."@en .

cim:ExcOEX3T.t1 a owl:DatatypeProperty ;
  rdfs:label "t1"@en ;
  rdfs:domain cim:ExcOEX3T ;
  rdfs:range cim:Seconds ;
  skos:definition "Time constant (<i>T</i><i><sub>1</sub></i>) (&gt;= 0)."@en .

cim:ExcOEX3T.t2 a owl:DatatypeProperty ;
  rdfs:label "t2"@en ;
  rdfs:domain cim:ExcOEX3T ;
  rdfs:range cim:Seconds ;
  skos:definition "Time constant (<i>T</i><i><sub>2</sub></i>) (&gt;= 0)."@en .

cim:ExcOEX3T.t3 a owl:DatatypeProperty ;
  rdfs:label "t3"@en ;
  rdfs:domain cim:ExcOEX3T ;
  rdfs:range cim:Seconds ;
  skos:definition "Time constant (<i>T</i><i><sub>3</sub></i>) (&gt;= 0)."@en .

cim:ExcOEX3T.t4 a owl:DatatypeProperty ;
  rdfs:label "t4"@en ;
  rdfs:domain cim:ExcOEX3T ;
  rdfs:range cim:Seconds ;
  skos:definition "Time constant (<i>T</i><i><sub>4</sub></i>) (&gt;= 0)."@en .

cim:ExcOEX3T.t5 a owl:DatatypeProperty ;
  rdfs:label "t5"@en ;
  rdfs:domain cim:ExcOEX3T ;
  rdfs:range cim:Seconds ;
  skos:definition "Time constant (<i>T</i><i><sub>5</sub></i>) (&gt;= 0)."@en .

cim:ExcOEX3T.t6 a owl:DatatypeProperty ;
  rdfs:label "t6"@en ;
  rdfs:domain cim:ExcOEX3T ;
  rdfs:range cim:Seconds ;
  skos:definition "Time constant (<i>T</i><i><sub>6</sub></i>) (&gt;= 0)."@en .

cim:ExcOEX3T.te a owl:DatatypeProperty ;
  rdfs:label "te"@en ;
  rdfs:domain cim:ExcOEX3T ;
  rdfs:range cim:Seconds ;
  skos:definition "Time constant (<i>T</i><i><sub>E</sub></i>) (&gt;= 0)."@en .

cim:ExcOEX3T.tf a owl:DatatypeProperty ;
  rdfs:label "tf"@en ;
  rdfs:domain cim:ExcOEX3T ;
  rdfs:range cim:Seconds ;
  skos:definition "Time constant (<i>T</i><i><sub>F</sub></i>) (&gt;= 0)."@en .

cim:ExcOEX3T.vrmax a owl:DatatypeProperty ;
  rdfs:label "vrmax"@en ;
  rdfs:domain cim:ExcOEX3T ;
  rdfs:range cim:PU ;
  skos:definition "Limiter (<i>V</i><i><sub>RMAX</sub></i>) (&gt; ExcOEX3T.vrmin)."@en .

cim:ExcOEX3T.vrmin a owl:DatatypeProperty ;
  rdfs:label "vrmin"@en ;
  rdfs:domain cim:ExcOEX3T ;
  rdfs:range cim:PU ;
  skos:definition "Limiter (<i>V</i><i><sub>RMIN</sub></i>) (&lt; ExcOEX3T.vrmax). "@en .

cim:ExcPIC.e1 a owl:DatatypeProperty ;
  rdfs:label "e1"@en ;
  rdfs:domain cim:ExcPIC ;
  rdfs:range cim:PU ;
  skos:definition "Field voltage value 1 (<i>E</i><i><sub>1</sub></i>).  Typical value = 0."@en .

cim:ExcPIC.e2 a owl:DatatypeProperty ;
  rdfs:label "e2"@en ;
  rdfs:domain cim:ExcPIC ;
  rdfs:range cim:PU ;
  skos:definition "Field voltage value 2 (<i>E</i><i><sub>2</sub></i>).  Typical value = 0."@en .

cim:ExcPIC.efdmax a owl:DatatypeProperty ;
  rdfs:label "efdmax"@en ;
  rdfs:domain cim:ExcPIC ;
  rdfs:range cim:PU ;
  skos:definition "Exciter maximum limit (<i>E</i><i><sub>fdmax</sub></i>) (&gt; ExcPIC.efdmin).  Typical value = 8."@en .

cim:ExcPIC.efdmin a owl:DatatypeProperty ;
  rdfs:label "efdmin"@en ;
  rdfs:domain cim:ExcPIC ;
  rdfs:range cim:PU ;
  skos:definition "Exciter minimum limit (<i>E</i><i><sub>fdmin</sub></i>) (&lt; ExcPIC.efdmax).  Typical value = -0,87."@en .

cim:ExcPIC.ka a owl:DatatypeProperty ;
  rdfs:label "ka"@en ;
  rdfs:domain cim:ExcPIC ;
  rdfs:range cim:PU ;
  skos:definition "PI controller gain (<i>K</i><i><sub>a</sub></i>).  Typical value = 3,15."@en .

cim:ExcPIC.kc a owl:DatatypeProperty ;
  rdfs:label "kc"@en ;
  rdfs:domain cim:ExcPIC ;
  rdfs:range cim:PU ;
  skos:definition "Exciter regulation factor (<i>K</i><i><sub>c</sub></i>).  Typical value = 0,08."@en .

cim:ExcPIC.ke a owl:DatatypeProperty ;
  rdfs:label "ke"@en ;
  rdfs:domain cim:ExcPIC ;
  rdfs:range cim:PU ;
  skos:definition "Exciter constant (<i>K</i><i><sub>e</sub></i>).  Typical value = 0."@en .

cim:ExcPIC.kf a owl:DatatypeProperty ;
  rdfs:label "kf"@en ;
  rdfs:domain cim:ExcPIC ;
  rdfs:range cim:PU ;
  skos:definition "Rate feedback gain (<i>K</i><i><sub>f</sub></i>).  Typical value = 0."@en .

cim:ExcPIC.ki a owl:DatatypeProperty ;
  rdfs:label "ki"@en ;
  rdfs:domain cim:ExcPIC ;
  rdfs:range cim:PU ;
  skos:definition "Current source gain (<i>K</i><i><sub>i</sub></i>).  Typical value = 0."@en .

cim:ExcPIC.kp a owl:DatatypeProperty ;
  rdfs:label "kp"@en ;
  rdfs:domain cim:ExcPIC ;
  rdfs:range cim:PU ;
  skos:definition "Potential source gain (<i>K</i><i><sub>p</sub></i>).  Typical value = 6,5."@en .

cim:ExcPIC.se1 a owl:DatatypeProperty ;
  rdfs:label "se1"@en ;
  rdfs:domain cim:ExcPIC ;
  rdfs:range cim:PU ;
  skos:definition "Saturation factor at <i>E</i><i><sub>1</sub></i> (<i>Se</i><i><sub>1</sub></i>).  Typical value = 0."@en .

cim:ExcPIC.se2 a owl:DatatypeProperty ;
  rdfs:label "se2"@en ;
  rdfs:domain cim:ExcPIC ;
  rdfs:range cim:PU ;
  skos:definition "Saturation factor at <i>E</i><i><sub>2</sub></i> (<i>Se</i><i><sub>2</sub></i>).  Typical value = 0."@en .

cim:ExcPIC.ta1 a owl:DatatypeProperty ;
  rdfs:label "ta1"@en ;
  rdfs:domain cim:ExcPIC ;
  rdfs:range cim:Seconds ;
  skos:definition "PI controller time constant (<i>T</i><i><sub>a1</sub></i>) (&gt;= 0).  Typical value = 1."@en .

cim:ExcPIC.ta2 a owl:DatatypeProperty ;
  rdfs:label "ta2"@en ;
  rdfs:domain cim:ExcPIC ;
  rdfs:range cim:Seconds ;
  skos:definition "Voltage regulator time constant (<i>T</i><i><sub>a2</sub></i>) (&gt;= 0).  Typical value = 0,01."@en .

cim:ExcPIC.ta3 a owl:DatatypeProperty ;
  rdfs:label "ta3"@en ;
  rdfs:domain cim:ExcPIC ;
  rdfs:range cim:Seconds ;
  skos:definition "Lead time constant (<i>T</i><i><sub>a3</sub></i>) (&gt;= 0).  Typical value = 0."@en .

cim:ExcPIC.ta4 a owl:DatatypeProperty ;
  rdfs:label "ta4"@en ;
  rdfs:domain cim:ExcPIC ;
  rdfs:range cim:Seconds ;
  skos:definition "Lag time constant (<i>T</i><i><sub>a4</sub></i>) (&gt;= 0).  Typical value = 0."@en .

cim:ExcPIC.te a owl:DatatypeProperty ;
  rdfs:label "te"@en ;
  rdfs:domain cim:ExcPIC ;
  rdfs:range cim:Seconds ;
  skos:definition "Exciter time constant (<i>T</i><i><sub>e</sub></i>) (&gt;= 0).  Typical value = 0."@en .

cim:ExcPIC.tf1 a owl:DatatypeProperty ;
  rdfs:label "tf1"@en ;
  rdfs:domain cim:ExcPIC ;
  rdfs:range cim:Seconds ;
  skos:definition "Rate feedback time constant (<i>T</i><i><sub>f1</sub></i>) (&gt;= 0).  Typical value = 0."@en .

cim:ExcPIC.tf2 a owl:DatatypeProperty ;
  rdfs:label "tf2"@en ;
  rdfs:domain cim:ExcPIC ;
  rdfs:range cim:Seconds ;
  skos:definition "Rate feedback lag time constant (<i>T</i><i><sub>f2</sub></i>) (&gt;= 0).  Typical value = 0."@en .

cim:ExcPIC.vr1 a owl:DatatypeProperty ;
  rdfs:label "vr1"@en ;
  rdfs:domain cim:ExcPIC ;
  rdfs:range cim:PU ;
  skos:definition "PI maximum limit (<i>V</i><i><sub>r1</sub></i>).  Typical value = 1."@en .

cim:ExcPIC.vr2 a owl:DatatypeProperty ;
  rdfs:label "vr2"@en ;
  rdfs:domain cim:ExcPIC ;
  rdfs:range cim:PU ;
  skos:definition "PI minimum limit (<i>V</i><i><sub>r2</sub></i>).  Typical value = -0,87."@en .

cim:ExcPIC.vrmax a owl:DatatypeProperty ;
  rdfs:label "vrmax"@en ;
  rdfs:domain cim:ExcPIC ;
  rdfs:range cim:PU ;
  skos:definition "Voltage regulator maximum limit (<i>V</i><i><sub>rmax</sub></i>) (&gt; ExcPIC.vrmin).  Typical value = 1."@en .

cim:ExcPIC.vrmin a owl:DatatypeProperty ;
  rdfs:label "vrmin"@en ;
  rdfs:domain cim:ExcPIC ;
  rdfs:range cim:PU ;
  skos:definition "Voltage regulator minimum limit (<i>V</i><i><sub>rmin</sub></i>) (&lt; ExcPIC.vrmax).  Typical value = -0,87."@en .

cim:ExcREXS.e1 a owl:DatatypeProperty ;
  rdfs:label "e1"@en ;
  rdfs:domain cim:ExcREXS ;
  rdfs:range cim:PU ;
  skos:definition "Field voltage value 1 (<i>E</i><i><sub>1</sub></i>).  Typical value = 3."@en .

cim:ExcREXS.e2 a owl:DatatypeProperty ;
  rdfs:label "e2"@en ;
  rdfs:domain cim:ExcREXS ;
  rdfs:range cim:PU ;
  skos:definition "Field voltage value 2 (<i>E</i><i><sub>2</sub></i>).  Typical value = 4."@en .

cim:ExcREXS.fbf a owl:DatatypeProperty ;
  rdfs:label "fbf"@en ;
  rdfs:domain cim:ExcREXS ;
  rdfs:range cim:ExcREXSFeedbackSignalKind ;
  skos:definition "Rate feedback signal flag (<i>fbf</i>). Typical value = fieldCurrent."@en .

cim:ExcREXS.flimf a owl:DatatypeProperty ;
  rdfs:label "flimf"@en ;
  rdfs:domain cim:ExcREXS ;
  rdfs:range cim:PU ;
  skos:definition "Limit type flag (<i>Flimf</i>).  Typical value = 0."@en .

cim:ExcREXS.kc a owl:DatatypeProperty ;
  rdfs:label "kc"@en ;
  rdfs:domain cim:ExcREXS ;
  rdfs:range cim:PU ;
  skos:definition "Rectifier regulation factor (<i>Kc</i>).  Typical value = 0,05."@en .

cim:ExcREXS.kd a owl:DatatypeProperty ;
  rdfs:label "kd"@en ;
  rdfs:domain cim:ExcREXS ;
  rdfs:range cim:PU ;
  skos:definition "Exciter regulation factor (<i>Kd</i>).  Typical value = 2."@en .

cim:ExcREXS.ke a owl:DatatypeProperty ;
  rdfs:label "ke"@en ;
  rdfs:domain cim:ExcREXS ;
  rdfs:range cim:PU ;
  skos:definition "Exciter field proportional constant (<i>Ke</i>).  Typical value = 1."@en .

cim:ExcREXS.kefd a owl:DatatypeProperty ;
  rdfs:label "kefd"@en ;
  rdfs:domain cim:ExcREXS ;
  rdfs:range cim:PU ;
  skos:definition "Field voltage feedback gain (<i>Kefd</i>).  Typical value = 0."@en .

cim:ExcREXS.kf a owl:DatatypeProperty ;
  rdfs:label "kf"@en ;
  rdfs:domain cim:ExcREXS ;
  rdfs:range cim:Seconds ;
  skos:definition "Rate feedback gain (<i>Kf</i>) (&gt;= 0).  Typical value = 0,05."@en .

cim:ExcREXS.kh a owl:DatatypeProperty ;
  rdfs:label "kh"@en ;
  rdfs:domain cim:ExcREXS ;
  rdfs:range cim:PU ;
  skos:definition "Field voltage controller feedback gain (<i>Kh</i>).  Typical value = 0."@en .

cim:ExcREXS.kii a owl:DatatypeProperty ;
  rdfs:label "kii"@en ;
  rdfs:domain cim:ExcREXS ;
  rdfs:range cim:PU ;
  skos:definition "Field current regulator integral gain (<i>Kii</i>).  Typical value = 0."@en .

cim:ExcREXS.kip a owl:DatatypeProperty ;
  rdfs:label "kip"@en ;
  rdfs:domain cim:ExcREXS ;
  rdfs:range cim:PU ;
  skos:definition "Field current regulator proportional gain (<i>Kip</i>).  Typical value = 1."@en .

cim:ExcREXS.ks a owl:DatatypeProperty ;
  rdfs:label "ks"@en ;
  rdfs:domain cim:ExcREXS ;
  rdfs:range cim:PU ;
  skos:definition "Coefficient to allow different usage of the model-speed coefficient (<i>Ks</i>).  Typical value = 0."@en .

cim:ExcREXS.kvi a owl:DatatypeProperty ;
  rdfs:label "kvi"@en ;
  rdfs:domain cim:ExcREXS ;
  rdfs:range cim:PU ;
  skos:definition "Voltage regulator integral gain (<i>Kvi</i>).  Typical value = 0."@en .

cim:ExcREXS.kvp a owl:DatatypeProperty ;
  rdfs:label "kvp"@en ;
  rdfs:domain cim:ExcREXS ;
  rdfs:range cim:PU ;
  skos:definition "Voltage regulator proportional gain (<i>Kvp</i>).  Typical value = 2800."@en .

cim:ExcREXS.kvphz a owl:DatatypeProperty ;
  rdfs:label "kvphz"@en ;
  rdfs:domain cim:ExcREXS ;
  rdfs:range cim:PU ;
  skos:definition "V/Hz limiter gain (<i>Kvphz</i>).  Typical value = 0."@en .

cim:ExcREXS.nvphz a owl:DatatypeProperty ;
  rdfs:label "nvphz"@en ;
  rdfs:domain cim:ExcREXS ;
  rdfs:range cim:PU ;
  skos:definition "Pickup speed of V/Hz limiter (<i>Nvphz</i>).  Typical value = 0."@en .

cim:ExcREXS.se1 a owl:DatatypeProperty ;
  rdfs:label "se1"@en ;
  rdfs:domain cim:ExcREXS ;
  rdfs:range cim:PU ;
  skos:definition "Saturation factor at <i>E</i><i><sub>1</sub></i><i> </i>(<i>Se</i><i><sub>1</sub></i>).  Typical value = 0,0001."@en .

cim:ExcREXS.se2 a owl:DatatypeProperty ;
  rdfs:label "se2"@en ;
  rdfs:domain cim:ExcREXS ;
  rdfs:range cim:PU ;
  skos:definition "Saturation factor at <i>E</i><i><sub>2</sub></i> (<i>Se</i><i><sub>2</sub></i>).  Typical value = 0,001."@en .

cim:ExcREXS.ta a owl:DatatypeProperty ;
  rdfs:label "ta"@en ;
  rdfs:domain cim:ExcREXS ;
  rdfs:range cim:Seconds ;
  skos:definition "Voltage regulator time constant (<i>Ta</i>) (&gt;= 0).  If = 0, block is bypassed.  Typical value = 0,01."@en .

cim:ExcREXS.tb1 a owl:DatatypeProperty ;
  rdfs:label "tb1"@en ;
  rdfs:domain cim:ExcREXS ;
  rdfs:range cim:Seconds ;
  skos:definition "Lag time constant (<i>Tb1</i>) (&gt;= 0).  If = 0, block is bypassed.  Typical value = 0."@en .

cim:ExcREXS.tb2 a owl:DatatypeProperty ;
  rdfs:label "tb2"@en ;
  rdfs:domain cim:ExcREXS ;
  rdfs:range cim:Seconds ;
  skos:definition "Lag time constant (<i>Tb2</i>) (&gt;= 0).  If = 0, block is bypassed.  Typical value = 0."@en .

cim:ExcREXS.tc1 a owl:DatatypeProperty ;
  rdfs:label "tc1"@en ;
  rdfs:domain cim:ExcREXS ;
  rdfs:range cim:Seconds ;
  skos:definition "Lead time constant (<i>Tc1</i>) (&gt;= 0).  Typical value = 0."@en .

cim:ExcREXS.tc2 a owl:DatatypeProperty ;
  rdfs:label "tc2"@en ;
  rdfs:domain cim:ExcREXS ;
  rdfs:range cim:Seconds ;
  skos:definition "Lead time constant (<i>Tc2</i>) (&gt;= 0).  Typical value = 0."@en .

cim:ExcREXS.te a owl:DatatypeProperty ;
  rdfs:label "te"@en ;
  rdfs:domain cim:ExcREXS ;
  rdfs:range cim:Seconds ;
  skos:definition "Exciter field time constant (<i>Te</i>) (&gt; 0).  Typical value = 1,2."@en .

cim:ExcREXS.tf a owl:DatatypeProperty ;
  rdfs:label "tf"@en ;
  rdfs:domain cim:ExcREXS ;
  rdfs:range cim:Seconds ;
  skos:definition "Rate feedback time constant (<i>Tf</i>) (&gt;= 0).  If = 0, the feedback path is not used.  Typical value = 1."@en .

cim:ExcREXS.tf1 a owl:DatatypeProperty ;
  rdfs:label "tf1"@en ;
  rdfs:domain cim:ExcREXS ;
  rdfs:range cim:Seconds ;
  skos:definition "Feedback lead time constant (<i>Tf1</i>) (&gt;= 0).  Typical value = 0."@en .

cim:ExcREXS.tf2 a owl:DatatypeProperty ;
  rdfs:label "tf2"@en ;
  rdfs:domain cim:ExcREXS ;
  rdfs:range cim:Seconds ;
  skos:definition "Feedback lag time constant (<i>Tf2</i>) (&gt;= 0).  If = 0, block is bypassed.  Typical value = 0."@en .

cim:ExcREXS.tp a owl:DatatypeProperty ;
  rdfs:label "tp"@en ;
  rdfs:domain cim:ExcREXS ;
  rdfs:range cim:Seconds ;
  skos:definition "Field current bridge time constant (<i>Tp</i>) (&gt;= 0).  Typical value = 0."@en .

cim:ExcREXS.vcmax a owl:DatatypeProperty ;
  rdfs:label "vcmax"@en ;
  rdfs:domain cim:ExcREXS ;
  rdfs:range cim:PU ;
  skos:definition "Maximum compounding voltage (<i>Vcmax</i>).  Typical value = 0."@en .

cim:ExcREXS.vfmax a owl:DatatypeProperty ;
  rdfs:label "vfmax"@en ;
  rdfs:domain cim:ExcREXS ;
  rdfs:range cim:PU ;
  skos:definition "Maximum exciter field current (<i>Vfmax</i>) (&gt; ExcREXS.vfmin).  Typical value = 47."@en .

cim:ExcREXS.vfmin a owl:DatatypeProperty ;
  rdfs:label "vfmin"@en ;
  rdfs:domain cim:ExcREXS ;
  rdfs:range cim:PU ;
  skos:definition "Minimum exciter field current (<i>Vfmin</i>) (&lt; ExcREXS.vfmax).  Typical value = -20."@en .

cim:ExcREXS.vimax a owl:DatatypeProperty ;
  rdfs:label "vimax"@en ;
  rdfs:domain cim:ExcREXS ;
  rdfs:range cim:PU ;
  skos:definition "Voltage regulator input limit (<i>Vimax</i>).  Typical value = 0,1."@en .

cim:ExcREXS.vrmax a owl:DatatypeProperty ;
  rdfs:label "vrmax"@en ;
  rdfs:domain cim:ExcREXS ;
  rdfs:range cim:PU ;
  skos:definition "Maximum controller output (V<i>rmax</i>) (&gt; ExcREXS.vrmin).  Typical value = 47."@en .

cim:ExcREXS.vrmin a owl:DatatypeProperty ;
  rdfs:label "vrmin"@en ;
  rdfs:domain cim:ExcREXS ;
  rdfs:range cim:PU ;
  skos:definition "Minimum controller output (<i>Vrmin</i>) (&lt; ExcREXS.vrmax).  Typical value = -20."@en .

cim:ExcREXS.xc a owl:DatatypeProperty ;
  rdfs:label "xc"@en ;
  rdfs:domain cim:ExcREXS ;
  rdfs:range cim:PU ;
  skos:definition "Exciter compounding reactance (<i>Xc</i>).  Typical value = 0."@en .

cim:ExcRQB.ki0 a owl:DatatypeProperty ;
  rdfs:label "ki0"@en ;
  rdfs:domain cim:ExcRQB ;
  rdfs:range xsd:float ;
  skos:definition "Voltage reference input gain (<i>Ki0</i>).  Typical value = 12,7."@en .

cim:ExcRQB.ki1 a owl:DatatypeProperty ;
  rdfs:label "ki1"@en ;
  rdfs:domain cim:ExcRQB ;
  rdfs:range xsd:float ;
  skos:definition "Voltage input gain (<i>Ki1</i>).  Typical value = -16,8."@en .

cim:ExcRQB.klir a owl:DatatypeProperty ;
  rdfs:label "klir"@en ;
  rdfs:domain cim:ExcRQB ;
  rdfs:range xsd:float ;
  skos:definition "OEL input gain (<i>KLIR</i>).  Typical value = 12,13."@en .

cim:ExcRQB.klus a owl:DatatypeProperty ;
  rdfs:label "klus"@en ;
  rdfs:domain cim:ExcRQB ;
  rdfs:range xsd:float ;
  skos:definition "Limiter gain (<i>KLUS</i>).  Typical value = 50."@en .

cim:ExcRQB.lsat a owl:DatatypeProperty ;
  rdfs:label "lsat"@en ;
  rdfs:domain cim:ExcRQB ;
  rdfs:range cim:PU ;
  skos:definition "Integrator limiter (<i>LSAT</i>).  Typical value = 5,73."@en .

cim:ExcRQB.lus a owl:DatatypeProperty ;
  rdfs:label "lus"@en ;
  rdfs:domain cim:ExcRQB ;
  rdfs:range cim:PU ;
  skos:definition "Setpoint (<i>LUS</i>).  Typical value = 0,12."@en .

cim:ExcRQB.mesu a owl:DatatypeProperty ;
  rdfs:label "mesu"@en ;
  rdfs:domain cim:ExcRQB ;
  rdfs:range cim:Seconds ;
  skos:definition "Voltage input time constant (<i>MESU</i>) (&gt;= 0).  Typical value = 0,02."@en .

cim:ExcRQB.t4m a owl:DatatypeProperty ;
  rdfs:label "t4m"@en ;
  rdfs:domain cim:ExcRQB ;
  rdfs:range cim:Seconds ;
  skos:definition "Input time constant (<i>T4M</i>) (&gt;= 0).  Typical value = 5."@en .

cim:ExcRQB.tc a owl:DatatypeProperty ;
  rdfs:label "tc"@en ;
  rdfs:domain cim:ExcRQB ;
  rdfs:range cim:Seconds ;
  skos:definition "Lead lag time constant (<i>TC</i>) (&gt;= 0).  Typical value = 0,02."@en .

cim:ExcRQB.te a owl:DatatypeProperty ;
  rdfs:label "te"@en ;
  rdfs:domain cim:ExcRQB ;
  rdfs:range cim:Seconds ;
  skos:definition "Lead lag time constant (<i>TE</i>) (&gt;= 0).  Typical value = 0,22."@en .

cim:ExcRQB.tf a owl:DatatypeProperty ;
  rdfs:label "tf"@en ;
  rdfs:domain cim:ExcRQB ;
  rdfs:range cim:Seconds ;
  skos:definition "Exciter time constant (<i>TF</i>) (&gt;= 0).  Typical value = 0,01."@en .

cim:ExcRQB.ucmax a owl:DatatypeProperty ;
  rdfs:label "ucmax"@en ;
  rdfs:domain cim:ExcRQB ;
  rdfs:range cim:PU ;
  skos:definition "Maximum voltage reference limit (<i>UCMAX</i>) (&gt; ExcRQB.ucmin).  Typical value = 1,1."@en .

cim:ExcRQB.ucmin a owl:DatatypeProperty ;
  rdfs:label "ucmin"@en ;
  rdfs:domain cim:ExcRQB ;
  rdfs:range cim:PU ;
  skos:definition "Minimum voltage reference limit (<i>UCMIN</i>) (&lt; ExcRQB.ucmax).  Typical value = 0,9."@en .

cim:ExcSCRX.cswitch a owl:DatatypeProperty ;
  rdfs:label "cswitch"@en ;
  rdfs:domain cim:ExcSCRX ;
  rdfs:range xsd:boolean ;
  skos:definition """
Power source switch (<i>Cswitch</i>).
true = fixed voltage of 1.0 PU
false = generator terminal voltage.
\t"""@en .

cim:ExcSCRX.emax a owl:DatatypeProperty ;
  rdfs:label "emax"@en ;
  rdfs:domain cim:ExcSCRX ;
  rdfs:range cim:PU ;
  skos:definition "Maximum field voltage output (<i>Emax</i>) (&gt; ExcSCRX.emin).  Typical value = 5."@en .

cim:ExcSCRX.emin a owl:DatatypeProperty ;
  rdfs:label "emin"@en ;
  rdfs:domain cim:ExcSCRX ;
  rdfs:range cim:PU ;
  skos:definition "Minimum field voltage output (<i>Emin</i>) (&lt; ExcSCRX.emax).  Typical value = 0."@en .

cim:ExcSCRX.k a owl:DatatypeProperty ;
  rdfs:label "k"@en ;
  rdfs:domain cim:ExcSCRX ;
  rdfs:range cim:PU ;
  skos:definition "Gain (<i>K</i>) (&gt; 0).  Typical value = 200."@en .

cim:ExcSCRX.rcrfd a owl:DatatypeProperty ;
  rdfs:label "rcrfd"@en ;
  rdfs:domain cim:ExcSCRX ;
  rdfs:range xsd:float ;
  skos:definition "Ratio of field discharge resistance to field winding resistance ([<i>rc / rfd]</i>).  Typical value = 0."@en .

cim:ExcSCRX.tatb a owl:DatatypeProperty ;
  rdfs:label "tatb"@en ;
  rdfs:domain cim:ExcSCRX ;
  rdfs:range xsd:float ;
  skos:definition "Gain reduction ratio of lag-lead element ([<i>Ta</i> / <i>Tb</i>]). The parameter <i>Ta</i> is not defined explicitly.  Typical value = 0.1."@en .

cim:ExcSCRX.tb a owl:DatatypeProperty ;
  rdfs:label "tb"@en ;
  rdfs:domain cim:ExcSCRX ;
  rdfs:range cim:Seconds ;
  skos:definition "Denominator time constant of lag-lead block (<i>Tb</i>) (&gt;= 0).  Typical value = 10."@en .

cim:ExcSCRX.te a owl:DatatypeProperty ;
  rdfs:label "te"@en ;
  rdfs:domain cim:ExcSCRX ;
  rdfs:range cim:Seconds ;
  skos:definition "Time constant of gain block (<i>Te</i>) (&gt; 0).  Typical value = 0,02."@en .

cim:ExcSEXS.efdmax a owl:DatatypeProperty ;
  rdfs:label "efdmax"@en ;
  rdfs:domain cim:ExcSEXS ;
  rdfs:range cim:PU ;
  skos:definition "Field voltage clipping maximum limit (<i>Efdmax</i>) (&gt; ExcSEXS.efdmin).  Typical value = 5."@en .

cim:ExcSEXS.efdmin a owl:DatatypeProperty ;
  rdfs:label "efdmin"@en ;
  rdfs:domain cim:ExcSEXS ;
  rdfs:range cim:PU ;
  skos:definition "Field voltage clipping minimum limit (<i>Efdmin</i>) (&lt; ExcSEXS.efdmax).  Typical value = -5."@en .

cim:ExcSEXS.emax a owl:DatatypeProperty ;
  rdfs:label "emax"@en ;
  rdfs:domain cim:ExcSEXS ;
  rdfs:range cim:PU ;
  skos:definition "Maximum field voltage output (<i>Emax</i>) (&gt; ExcSEXS.emin).  Typical value = 5."@en .

cim:ExcSEXS.emin a owl:DatatypeProperty ;
  rdfs:label "emin"@en ;
  rdfs:domain cim:ExcSEXS ;
  rdfs:range cim:PU ;
  skos:definition "Minimum field voltage output (<i>Emin</i>) (&lt; ExcSEXS.emax).  Typical value = -5."@en .

cim:ExcSEXS.k a owl:DatatypeProperty ;
  rdfs:label "k"@en ;
  rdfs:domain cim:ExcSEXS ;
  rdfs:range cim:PU ;
  skos:definition "Gain (<i>K</i>) (&gt; 0).  Typical value = 100."@en .

cim:ExcSEXS.kc a owl:DatatypeProperty ;
  rdfs:label "kc"@en ;
  rdfs:domain cim:ExcSEXS ;
  rdfs:range cim:PU ;
  skos:definition "PI controller gain (<i>Kc</i>) (&gt; 0 if ExcSEXS.tc &gt; 0).  Typical value = 0,08."@en .

cim:ExcSEXS.tatb a owl:DatatypeProperty ;
  rdfs:label "tatb"@en ;
  rdfs:domain cim:ExcSEXS ;
  rdfs:range xsd:float ;
  skos:definition "Gain reduction ratio of lag-lead element (<i>[Ta / Tb]</i>).  Typical value = 0,1."@en .

cim:ExcSEXS.tb a owl:DatatypeProperty ;
  rdfs:label "tb"@en ;
  rdfs:domain cim:ExcSEXS ;
  rdfs:range cim:Seconds ;
  skos:definition "Denominator time constant of lag-lead block (<i>Tb</i>) (&gt;= 0).  Typical value = 10."@en .

cim:ExcSEXS.tc a owl:DatatypeProperty ;
  rdfs:label "tc"@en ;
  rdfs:domain cim:ExcSEXS ;
  rdfs:range cim:Seconds ;
  skos:definition "PI controller phase lead time constant (<i>Tc</i>) (&gt;= 0).  Typical value = 0."@en .

cim:ExcSEXS.te a owl:DatatypeProperty ;
  rdfs:label "te"@en ;
  rdfs:domain cim:ExcSEXS ;
  rdfs:range cim:Seconds ;
  skos:definition "Time constant of gain block (<i>Te</i>) (&gt; 0).  Typical value = 0,05."@en .

cim:ExcSK.efdmax a owl:DatatypeProperty ;
  rdfs:label "efdmax"@en ;
  rdfs:domain cim:ExcSK ;
  rdfs:range cim:PU ;
  skos:definition "Field voltage clipping upper level limit (<i>Efdmax</i>) (&gt; ExcSK.efdmin)."@en .

cim:ExcSK.efdmin a owl:DatatypeProperty ;
  rdfs:label "efdmin"@en ;
  rdfs:domain cim:ExcSK ;
  rdfs:range cim:PU ;
  skos:definition "Field voltage clipping lower level limit (<i>Efdmin</i>) (&lt; ExcSK.efdmax)."@en .

cim:ExcSK.emax a owl:DatatypeProperty ;
  rdfs:label "emax"@en ;
  rdfs:domain cim:ExcSK ;
  rdfs:range cim:PU ;
  skos:definition "Maximum field voltage output (<i>Emax</i>) (&gt; ExcSK.emin).  Typical value = 20."@en .

cim:ExcSK.emin a owl:DatatypeProperty ;
  rdfs:label "emin"@en ;
  rdfs:domain cim:ExcSK ;
  rdfs:range cim:PU ;
  skos:definition "Minimum field voltage output (<i>Emin</i>) (&lt; ExcSK.emax).  Typical value = -20."@en .

cim:ExcSK.k a owl:DatatypeProperty ;
  rdfs:label "k"@en ;
  rdfs:domain cim:ExcSK ;
  rdfs:range cim:PU ;
  skos:definition "Gain (<i>K</i>).  Typical value = 1."@en .

cim:ExcSK.k1 a owl:DatatypeProperty ;
  rdfs:label "k1"@en ;
  rdfs:domain cim:ExcSK ;
  rdfs:range cim:PU ;
  skos:definition "Parameter of underexcitation limit (<i>K1</i>).  Typical value = 0,1364."@en .

cim:ExcSK.k2 a owl:DatatypeProperty ;
  rdfs:label "k2"@en ;
  rdfs:domain cim:ExcSK ;
  rdfs:range cim:PU ;
  skos:definition "Parameter of underexcitation limit (<i>K2</i>).  Typical value = -0,3861."@en .

cim:ExcSK.kc a owl:DatatypeProperty ;
  rdfs:label "kc"@en ;
  rdfs:domain cim:ExcSK ;
  rdfs:range cim:PU ;
  skos:definition "PI controller gain (<i>Kc</i>).  Typical value = 70."@en .

cim:ExcSK.kce a owl:DatatypeProperty ;
  rdfs:label "kce"@en ;
  rdfs:domain cim:ExcSK ;
  rdfs:range cim:PU ;
  skos:definition "Rectifier regulation factor (<i>Kce</i>).  Typical value = 0."@en .

cim:ExcSK.kd a owl:DatatypeProperty ;
  rdfs:label "kd"@en ;
  rdfs:domain cim:ExcSK ;
  rdfs:range cim:PU ;
  skos:definition "Exciter internal reactance (<i>Kd</i>).  Typical value = 0."@en .

cim:ExcSK.kgob a owl:DatatypeProperty ;
  rdfs:label "kgob"@en ;
  rdfs:domain cim:ExcSK ;
  rdfs:range cim:PU ;
  skos:definition "P controller gain (<i>Kgob</i>).  Typical value = 10."@en .

cim:ExcSK.kp a owl:DatatypeProperty ;
  rdfs:label "kp"@en ;
  rdfs:domain cim:ExcSK ;
  rdfs:range cim:PU ;
  skos:definition "PI controller gain (<i>Kp</i>).  Typical value = 1."@en .

cim:ExcSK.kqi a owl:DatatypeProperty ;
  rdfs:label "kqi"@en ;
  rdfs:domain cim:ExcSK ;
  rdfs:range cim:PU ;
  skos:definition "PI controller gain of integral component (<i>Kqi</i>).  Typical value = 0."@en .

cim:ExcSK.kqob a owl:DatatypeProperty ;
  rdfs:label "kqob"@en ;
  rdfs:domain cim:ExcSK ;
  rdfs:range cim:PU ;
  skos:definition "Rate of rise of the reactive power (<i>Kqob</i>). "@en .

cim:ExcSK.kqp a owl:DatatypeProperty ;
  rdfs:label "kqp"@en ;
  rdfs:domain cim:ExcSK ;
  rdfs:range cim:PU ;
  skos:definition "PI controller gain (<i>Kqp</i>).  Typical value = 0."@en .

cim:ExcSK.nq a owl:DatatypeProperty ;
  rdfs:label "nq"@en ;
  rdfs:domain cim:ExcSK ;
  rdfs:range cim:PU ;
  skos:definition "Deadband of reactive power (<i>nq</i>).  Determines the range of sensitivity.  Typical value = 0,001."@en .

cim:ExcSK.qconoff a owl:DatatypeProperty ;
  rdfs:label "qconoff"@en ;
  rdfs:domain cim:ExcSK ;
  rdfs:range xsd:boolean ;
  skos:definition """
Secondary voltage control state (<i>Qc_on_off</i>).
true = secondary voltage control is on
false = secondary voltage control is off.
Typical value = false.
\t"""@en .

cim:ExcSK.qz a owl:DatatypeProperty ;
  rdfs:label "qz"@en ;
  rdfs:domain cim:ExcSK ;
  rdfs:range cim:PU ;
  skos:definition "Desired value (setpoint) of reactive power, manual setting (<i>Qz</i>). "@en .

cim:ExcSK.remote a owl:DatatypeProperty ;
  rdfs:label "remote"@en ;
  rdfs:domain cim:ExcSK ;
  rdfs:range xsd:boolean ;
  skos:definition """
Selector to apply automatic calculation in secondary controller model (<i>remote</i>).
true = automatic calculation is activated
false = manual set is active; the use of desired value of reactive power (<i>Qz</i>) is required.
Typical value = true.
\t"""@en .

cim:ExcSK.sbase a owl:DatatypeProperty ;
  rdfs:label "sbase"@en ;
  rdfs:domain cim:ExcSK ;
  rdfs:range cim:ApparentPower ;
  skos:definition "Apparent power of the unit (<i>Sbase</i>) (&gt; 0).  Unit = MVA.  Typical value = 259."@en .

cim:ExcSK.tc a owl:DatatypeProperty ;
  rdfs:label "tc"@en ;
  rdfs:domain cim:ExcSK ;
  rdfs:range cim:Seconds ;
  skos:definition "PI controller phase lead time constant (<i>Tc</i>) (&gt;= 0).  Typical value = 8."@en .

cim:ExcSK.te a owl:DatatypeProperty ;
  rdfs:label "te"@en ;
  rdfs:domain cim:ExcSK ;
  rdfs:range cim:Seconds ;
  skos:definition "Time constant of gain block (<i>Te</i>) (&gt;= 0).  Typical value = 0,1."@en .

cim:ExcSK.ti a owl:DatatypeProperty ;
  rdfs:label "ti"@en ;
  rdfs:domain cim:ExcSK ;
  rdfs:range cim:Seconds ;
  skos:definition "PI controller phase lead time constant (<i>Ti</i>) (&gt;= 0).  Typical value = 2."@en .

cim:ExcSK.tp a owl:DatatypeProperty ;
  rdfs:label "tp"@en ;
  rdfs:domain cim:ExcSK ;
  rdfs:range cim:Seconds ;
  skos:definition "Time constant (<i>Tp</i>) (&gt;= 0).  Typical value = 0,1."@en .

cim:ExcSK.tr a owl:DatatypeProperty ;
  rdfs:label "tr"@en ;
  rdfs:domain cim:ExcSK ;
  rdfs:range cim:Seconds ;
  skos:definition "Voltage transducer time constant (<i>Tr</i>) (&gt;= 0).  Typical value = 0,01."@en .

cim:ExcSK.uimax a owl:DatatypeProperty ;
  rdfs:label "uimax"@en ;
  rdfs:domain cim:ExcSK ;
  rdfs:range cim:PU ;
  skos:definition "Maximum error (<i>UImax</i>) (&gt; ExcSK.uimin).  Typical value = 10."@en .

cim:ExcSK.uimin a owl:DatatypeProperty ;
  rdfs:label "uimin"@en ;
  rdfs:domain cim:ExcSK ;
  rdfs:range cim:PU ;
  skos:definition "Minimum error (<i>UImin</i>) (&lt; ExcSK.uimax).  Typical value = -10."@en .

cim:ExcSK.urmax a owl:DatatypeProperty ;
  rdfs:label "urmax"@en ;
  rdfs:domain cim:ExcSK ;
  rdfs:range cim:PU ;
  skos:definition "Maximum controller output (<i>URmax</i>) (&gt; ExcSK.urmin).  Typical value = 10."@en .

cim:ExcSK.urmin a owl:DatatypeProperty ;
  rdfs:label "urmin"@en ;
  rdfs:domain cim:ExcSK ;
  rdfs:range cim:PU ;
  skos:definition "Minimum controller output (<i>URmin</i>) (&lt; ExcSK.urmax).  Typical value = -10."@en .

cim:ExcSK.vtmax a owl:DatatypeProperty ;
  rdfs:label "vtmax"@en ;
  rdfs:domain cim:ExcSK ;
  rdfs:range cim:PU ;
  skos:definition "Maximum terminal voltage input (<i>Vtmax</i>) (&gt; ExcSK.vtmin).  Determines the range of voltage deadband.  Typical value = 1,05."@en .

cim:ExcSK.vtmin a owl:DatatypeProperty ;
  rdfs:label "vtmin"@en ;
  rdfs:domain cim:ExcSK ;
  rdfs:range cim:PU ;
  skos:definition "Minimum terminal voltage input (<i>Vtmin</i>) (&lt; ExcSK.vtmax).  Determines the range of voltage deadband.  Typical value = 0,95."@en .

cim:ExcSK.yp a owl:DatatypeProperty ;
  rdfs:label "yp"@en ;
  rdfs:domain cim:ExcSK ;
  rdfs:range cim:PU ;
  skos:definition "Maximum output (<i>Yp</i>).  Typical value = 1."@en .

cim:ExcST1A.ilr a owl:DatatypeProperty ;
  rdfs:label "ilr"@en ;
  rdfs:domain cim:ExcST1A ;
  rdfs:range cim:PU ;
  skos:definition "Exciter output current limit reference (<i>Ilr</i>).  Typical value = 0."@en .

cim:ExcST1A.ka a owl:DatatypeProperty ;
  rdfs:label "ka"@en ;
  rdfs:domain cim:ExcST1A ;
  rdfs:range cim:PU ;
  skos:definition "Voltage regulator gain (<i>Ka</i>) (&gt; 0).  Typical value = 190."@en .

cim:ExcST1A.kc a owl:DatatypeProperty ;
  rdfs:label "kc"@en ;
  rdfs:domain cim:ExcST1A ;
  rdfs:range cim:PU ;
  skos:definition "Rectifier loading factor proportional to commutating reactance (<i>Kc</i>) (&gt;= 0). Typical value = 0,05."@en .

cim:ExcST1A.kf a owl:DatatypeProperty ;
  rdfs:label "kf"@en ;
  rdfs:domain cim:ExcST1A ;
  rdfs:range cim:PU ;
  skos:definition "Excitation control system stabilizer gains (<i>Kf</i>) (&gt;= 0).  Typical value = 0."@en .

cim:ExcST1A.klr a owl:DatatypeProperty ;
  rdfs:label "klr"@en ;
  rdfs:domain cim:ExcST1A ;
  rdfs:range cim:PU ;
  skos:definition "Exciter output current limiter gain (<i>Klr</i>).  Typical value = 0."@en .

cim:ExcST1A.ta a owl:DatatypeProperty ;
  rdfs:label "ta"@en ;
  rdfs:domain cim:ExcST1A ;
  rdfs:range cim:Seconds ;
  skos:definition "Voltage regulator time constant (<i>Ta</i>) (&gt;= 0).  Typical value = 0,02."@en .

cim:ExcST1A.tb a owl:DatatypeProperty ;
  rdfs:label "tb"@en ;
  rdfs:domain cim:ExcST1A ;
  rdfs:range cim:Seconds ;
  skos:definition "Voltage regulator time constant (<i>Tb</i>) (&gt;= 0).  Typical value = 10."@en .

cim:ExcST1A.tb1 a owl:DatatypeProperty ;
  rdfs:label "tb1"@en ;
  rdfs:domain cim:ExcST1A ;
  rdfs:range cim:Seconds ;
  skos:definition "Voltage regulator time constant (<i>Tb1</i>) (&gt;= 0).  Typical value = 0."@en .

cim:ExcST1A.tc a owl:DatatypeProperty ;
  rdfs:label "tc"@en ;
  rdfs:domain cim:ExcST1A ;
  rdfs:range cim:Seconds ;
  skos:definition "Voltage regulator time constant (<i>Tc</i>) (&gt;= 0).  Typical value = 1."@en .

cim:ExcST1A.tc1 a owl:DatatypeProperty ;
  rdfs:label "tc1"@en ;
  rdfs:domain cim:ExcST1A ;
  rdfs:range cim:Seconds ;
  skos:definition "Voltage regulator time constant (<i>Tc1</i>) (&gt;= 0).  Typical value = 0."@en .

cim:ExcST1A.tf a owl:DatatypeProperty ;
  rdfs:label "tf"@en ;
  rdfs:domain cim:ExcST1A ;
  rdfs:range cim:Seconds ;
  skos:definition "Excitation control system stabilizer time constant (<i>Tf</i>) (&gt;= 0).  Typical value = 1."@en .

cim:ExcST1A.vamax a owl:DatatypeProperty ;
  rdfs:label "vamax"@en ;
  rdfs:domain cim:ExcST1A ;
  rdfs:range cim:PU ;
  skos:definition "Maximum voltage regulator output (<i>Vamax</i>) (&gt; 0).  Typical value = 999."@en .

cim:ExcST1A.vamin a owl:DatatypeProperty ;
  rdfs:label "vamin"@en ;
  rdfs:domain cim:ExcST1A ;
  rdfs:range cim:PU ;
  skos:definition "Minimum voltage regulator output (<i>Vamin</i>) (&lt; 0).  Typical value = -999."@en .

cim:ExcST1A.vimax a owl:DatatypeProperty ;
  rdfs:label "vimax"@en ;
  rdfs:domain cim:ExcST1A ;
  rdfs:range cim:PU ;
  skos:definition "Maximum voltage regulator input limit (<i>Vimax</i>) (&gt; 0).  Typical value = 999."@en .

cim:ExcST1A.vimin a owl:DatatypeProperty ;
  rdfs:label "vimin"@en ;
  rdfs:domain cim:ExcST1A ;
  rdfs:range cim:PU ;
  skos:definition "Minimum voltage regulator input limit (<i>Vimin</i>) (&lt; 0).  Typical value = -999."@en .

cim:ExcST1A.vrmax a owl:DatatypeProperty ;
  rdfs:label "vrmax"@en ;
  rdfs:domain cim:ExcST1A ;
  rdfs:range cim:PU ;
  skos:definition "Maximum voltage regulator outputs (<i>Vrmax</i>) (&gt; 0) .  Typical value = 7,8."@en .

cim:ExcST1A.vrmin a owl:DatatypeProperty ;
  rdfs:label "vrmin"@en ;
  rdfs:domain cim:ExcST1A ;
  rdfs:range cim:PU ;
  skos:definition "Minimum voltage regulator outputs (<i>Vrmin</i>) (&lt; 0).  Typical value = -6,7."@en .

cim:ExcST1A.xe a owl:DatatypeProperty ;
  rdfs:label "xe"@en ;
  rdfs:domain cim:ExcST1A ;
  rdfs:range cim:PU ;
  skos:definition "Excitation xfmr effective reactance (<i>Xe</i>).  Typical value = 0,04."@en .

cim:ExcST2A.efdmax a owl:DatatypeProperty ;
  rdfs:label "efdmax"@en ;
  rdfs:domain cim:ExcST2A ;
  rdfs:range cim:PU ;
  skos:definition "Maximum field voltage (<i>Efdmax</i>) (&gt;= 0).  Typical value = 99."@en .

cim:ExcST2A.ka a owl:DatatypeProperty ;
  rdfs:label "ka"@en ;
  rdfs:domain cim:ExcST2A ;
  rdfs:range cim:PU ;
  skos:definition "Voltage regulator gain (<i>Ka</i>) (&gt; 0).  Typical value = 120."@en .

cim:ExcST2A.kc a owl:DatatypeProperty ;
  rdfs:label "kc"@en ;
  rdfs:domain cim:ExcST2A ;
  rdfs:range cim:PU ;
  skos:definition "Rectifier loading factor proportional to commutating reactance (<i>Kc</i>) (&gt;= 0).  Typical value = 1,82."@en .

cim:ExcST2A.ke a owl:DatatypeProperty ;
  rdfs:label "ke"@en ;
  rdfs:domain cim:ExcST2A ;
  rdfs:range cim:PU ;
  skos:definition "Exciter constant related to self-excited field (<i>Ke</i>).  Typical value = 1."@en .

cim:ExcST2A.kf a owl:DatatypeProperty ;
  rdfs:label "kf"@en ;
  rdfs:domain cim:ExcST2A ;
  rdfs:range cim:PU ;
  skos:definition "Excitation control system stabilizer gains (<i>kf</i>) (&gt;= 0).  Typical value = 0,05."@en .

cim:ExcST2A.ki a owl:DatatypeProperty ;
  rdfs:label "ki"@en ;
  rdfs:domain cim:ExcST2A ;
  rdfs:range cim:PU ;
  skos:definition "Potential circuit gain coefficient (<i>K</i><i><sub>i</sub></i>) (&gt;= 0).  Typical value = 8."@en .

cim:ExcST2A.kp a owl:DatatypeProperty ;
  rdfs:label "kp"@en ;
  rdfs:domain cim:ExcST2A ;
  rdfs:range cim:PU ;
  skos:definition "Potential circuit gain coefficient (<i>K</i><i><sub>p</sub></i>) (&gt;= 0).  Typical value = 4,88."@en .

cim:ExcST2A.ta a owl:DatatypeProperty ;
  rdfs:label "ta"@en ;
  rdfs:domain cim:ExcST2A ;
  rdfs:range cim:Seconds ;
  skos:definition "Voltage regulator time constant (<i>Ta</i>) (&gt; 0).  Typical value = 0,15."@en .

cim:ExcST2A.tb a owl:DatatypeProperty ;
  rdfs:label "tb"@en ;
  rdfs:domain cim:ExcST2A ;
  rdfs:range cim:Seconds ;
  skos:definition "Voltage regulator time constant (<i>Tb</i>) (&gt;= 0).  Typical value = 0."@en .

cim:ExcST2A.tc a owl:DatatypeProperty ;
  rdfs:label "tc"@en ;
  rdfs:domain cim:ExcST2A ;
  rdfs:range cim:Seconds ;
  skos:definition "Voltage regulator time constant (<i>Tc</i>) (&gt;= 0).  Typical value = 0."@en .

cim:ExcST2A.te a owl:DatatypeProperty ;
  rdfs:label "te"@en ;
  rdfs:domain cim:ExcST2A ;
  rdfs:range cim:Seconds ;
  skos:definition "Exciter time constant, integration rate associated with exciter control (<i>Te</i>) (&gt; 0).  Typical value = 0,5."@en .

cim:ExcST2A.tf a owl:DatatypeProperty ;
  rdfs:label "tf"@en ;
  rdfs:domain cim:ExcST2A ;
  rdfs:range cim:Seconds ;
  skos:definition "Excitation control system stabilizer time constant (<i>Tf</i>) (&gt;= 0).  Typical value = 0,7."@en .

cim:ExcST2A.uelin a owl:DatatypeProperty ;
  rdfs:label "uelin"@en ;
  rdfs:domain cim:ExcST2A ;
  rdfs:range xsd:boolean ;
  skos:definition """
UEL input (<i>UELin</i>).
true = HV gate
false = add to error signal.
Typical value = false.
\t"""@en .

cim:ExcST2A.vrmax a owl:DatatypeProperty ;
  rdfs:label "vrmax"@en ;
  rdfs:domain cim:ExcST2A ;
  rdfs:range cim:PU ;
  skos:definition "Maximum voltage regulator outputs (<i>Vrmax</i>) (&gt; 0).  Typical value = 1."@en .

cim:ExcST2A.vrmin a owl:DatatypeProperty ;
  rdfs:label "vrmin"@en ;
  rdfs:domain cim:ExcST2A ;
  rdfs:range cim:PU ;
  skos:definition "Minimum voltage regulator outputs (<i>Vrmin</i>) (&lt; 0).  Typical value = -1."@en .

cim:ExcST3A.efdmax a owl:DatatypeProperty ;
  rdfs:label "efdmax"@en ;
  rdfs:domain cim:ExcST3A ;
  rdfs:range cim:PU ;
  skos:definition "Maximum AVR output (<i>Efdmax</i>) (&gt;= 0).  Typical value = 6,9."@en .

cim:ExcST3A.kc a owl:DatatypeProperty ;
  rdfs:label "kc"@en ;
  rdfs:domain cim:ExcST3A ;
  rdfs:range cim:PU ;
  skos:definition "Rectifier loading factor proportional to commutating reactance (<i>Kc</i>) (&gt;= 0). Typical value = 1,1."@en .

cim:ExcST3A.kg a owl:DatatypeProperty ;
  rdfs:label "kg"@en ;
  rdfs:domain cim:ExcST3A ;
  rdfs:range cim:PU ;
  skos:definition "Feedback gain constant of the inner loop field regulator (<i>Kg</i>) (&gt;= 0).  Typical value = 1."@en .

cim:ExcST3A.ki a owl:DatatypeProperty ;
  rdfs:label "ki"@en ;
  rdfs:domain cim:ExcST3A ;
  rdfs:range cim:PU ;
  skos:definition "Potential circuit gain coefficient (<i>K</i><i><sub>i</sub></i>) (&gt;= 0).  Typical value = 4,83."@en .

cim:ExcST3A.kj a owl:DatatypeProperty ;
  rdfs:label "kj"@en ;
  rdfs:domain cim:ExcST3A ;
  rdfs:range cim:PU ;
  skos:definition "AVR gain (<i>Kj</i>) (&gt; 0).  Typical value = 200."@en .

cim:ExcST3A.km a owl:DatatypeProperty ;
  rdfs:label "km"@en ;
  rdfs:domain cim:ExcST3A ;
  rdfs:range cim:PU ;
  skos:definition "Forward gain constant of the inner loop field regulator (<i>Km</i>) (&gt; 0).  Typical value = 7,04."@en .

cim:ExcST3A.kp a owl:DatatypeProperty ;
  rdfs:label "kp"@en ;
  rdfs:domain cim:ExcST3A ;
  rdfs:range cim:PU ;
  skos:definition "Potential source gain (<i>K</i><i><sub>p</sub></i>) (&gt; 0).  Typical value = 4,37."@en .

cim:ExcST3A.ks a owl:DatatypeProperty ;
  rdfs:label "ks"@en ;
  rdfs:domain cim:ExcST3A ;
  rdfs:range cim:PU ;
  skos:definition "Coefficient to allow different usage of the model-speed coefficient (<i>Ks</i>).  Typical value = 0."@en .

cim:ExcST3A.ks1 a owl:DatatypeProperty ;
  rdfs:label "ks1"@en ;
  rdfs:domain cim:ExcST3A ;
  rdfs:range cim:PU ;
  skos:definition "Coefficient to allow different usage of the model-speed coefficient (<i>Ks1</i>).  Typical value = 0."@en .

cim:ExcST3A.tb a owl:DatatypeProperty ;
  rdfs:label "tb"@en ;
  rdfs:domain cim:ExcST3A ;
  rdfs:range cim:Seconds ;
  skos:definition "Voltage regulator time constant (<i>Tb</i>) (&gt;= 0).  Typical value = 6,67."@en .

cim:ExcST3A.tc a owl:DatatypeProperty ;
  rdfs:label "tc"@en ;
  rdfs:domain cim:ExcST3A ;
  rdfs:range cim:Seconds ;
  skos:definition "Voltage regulator time constant (<i>Tc</i>) (&gt;= 0).  Typical value = 1."@en .

cim:ExcST3A.thetap a owl:DatatypeProperty ;
  rdfs:label "thetap"@en ;
  rdfs:domain cim:ExcST3A ;
  rdfs:range cim:AngleDegrees ;
  skos:definition "Potential circuit phase angle (<i>theta</i><i><sub>p</sub></i>).  Typical value = 20."@en .

cim:ExcST3A.tm a owl:DatatypeProperty ;
  rdfs:label "tm"@en ;
  rdfs:domain cim:ExcST3A ;
  rdfs:range cim:Seconds ;
  skos:definition "Forward time constant of inner loop field regulator (<i>Tm</i>) (&gt; 0).  Typical value = 1."@en .

cim:ExcST3A.vbmax a owl:DatatypeProperty ;
  rdfs:label "vbmax"@en ;
  rdfs:domain cim:ExcST3A ;
  rdfs:range cim:PU ;
  skos:definition "Maximum excitation voltage (<i>Vbmax</i>) (&gt; 0).  Typical value = 8,63."@en .

cim:ExcST3A.vgmax a owl:DatatypeProperty ;
  rdfs:label "vgmax"@en ;
  rdfs:domain cim:ExcST3A ;
  rdfs:range cim:PU ;
  skos:definition "Maximum inner loop feedback voltage (<i>Vgmax</i>) (&gt;= 0).  Typical value = 6,53."@en .

cim:ExcST3A.vimax a owl:DatatypeProperty ;
  rdfs:label "vimax"@en ;
  rdfs:domain cim:ExcST3A ;
  rdfs:range cim:PU ;
  skos:definition "Maximum voltage regulator input limit (<i>Vimax</i>) (&gt; 0).  Typical value = 0,2."@en .

cim:ExcST3A.vimin a owl:DatatypeProperty ;
  rdfs:label "vimin"@en ;
  rdfs:domain cim:ExcST3A ;
  rdfs:range cim:PU ;
  skos:definition "Minimum voltage regulator input limit (<i>Vimin</i>) (&lt; 0).  Typical value = -0,2."@en .

cim:ExcST3A.vrmax a owl:DatatypeProperty ;
  rdfs:label "vrmax"@en ;
  rdfs:domain cim:ExcST3A ;
  rdfs:range cim:PU ;
  skos:definition "Maximum voltage regulator output (<i>Vrmax</i>) (&gt; 0).  Typical value = 1."@en .

cim:ExcST3A.vrmin a owl:DatatypeProperty ;
  rdfs:label "vrmin"@en ;
  rdfs:domain cim:ExcST3A ;
  rdfs:range cim:PU ;
  skos:definition "Minimum voltage regulator output (<i>Vrmin</i>) (&lt; 0).  Typical value = -1."@en .

cim:ExcST3A.xl a owl:DatatypeProperty ;
  rdfs:label "xl"@en ;
  rdfs:domain cim:ExcST3A ;
  rdfs:range cim:PU ;
  skos:definition "Reactance associated with potential source (<i>Xl</i>) (&gt;= 0).  Typical value = 0,09."@en .

cim:ExcST4B.kc a owl:DatatypeProperty ;
  rdfs:label "kc"@en ;
  rdfs:domain cim:ExcST4B ;
  rdfs:range cim:PU ;
  skos:definition "Rectifier loading factor proportional to commutating reactance (<i>Kc</i>) (&gt;= 0). Typical value = 0,113."@en .

cim:ExcST4B.kg a owl:DatatypeProperty ;
  rdfs:label "kg"@en ;
  rdfs:domain cim:ExcST4B ;
  rdfs:range cim:PU ;
  skos:definition "Feedback gain constant of the inner loop field regulator (<i>Kg</i>) (&gt;= 0). Typical value = 0."@en .

cim:ExcST4B.ki a owl:DatatypeProperty ;
  rdfs:label "ki"@en ;
  rdfs:domain cim:ExcST4B ;
  rdfs:range cim:PU ;
  skos:definition "Potential circuit gain coefficient (<i>Ki</i>) (&gt;= 0).  Typical value = 0."@en .

cim:ExcST4B.kim a owl:DatatypeProperty ;
  rdfs:label "kim"@en ;
  rdfs:domain cim:ExcST4B ;
  rdfs:range cim:PU ;
  skos:definition "Voltage regulator integral gain output (<i>Kim</i>).  Typical value = 0."@en .

cim:ExcST4B.kir a owl:DatatypeProperty ;
  rdfs:label "kir"@en ;
  rdfs:domain cim:ExcST4B ;
  rdfs:range cim:PU ;
  skos:definition "Voltage regulator integral gain (<i>Kir</i>).  Typical value = 10,75."@en .

cim:ExcST4B.kp a owl:DatatypeProperty ;
  rdfs:label "kp"@en ;
  rdfs:domain cim:ExcST4B ;
  rdfs:range cim:PU ;
  skos:definition "Potential circuit gain coefficient (<i>Kp</i>) (&gt; 0).  Typical value = 9,3."@en .

cim:ExcST4B.kpm a owl:DatatypeProperty ;
  rdfs:label "kpm"@en ;
  rdfs:domain cim:ExcST4B ;
  rdfs:range cim:PU ;
  skos:definition "Voltage regulator proportional gain output (<i>Kpm</i>).  Typical value = 1."@en .

cim:ExcST4B.kpr a owl:DatatypeProperty ;
  rdfs:label "kpr"@en ;
  rdfs:domain cim:ExcST4B ;
  rdfs:range cim:PU ;
  skos:definition "Voltage regulator proportional gain (<i>Kpr</i>).  Typical value = 10,75."@en .

cim:ExcST4B.lvgate a owl:DatatypeProperty ;
  rdfs:label "lvgate"@en ;
  rdfs:domain cim:ExcST4B ;
  rdfs:range xsd:boolean ;
  skos:definition """
Selector (<i>LVGate</i>).
true = <i>LVGate</i> is part of the block diagram
false = <i>LVGate</i> is not part of the block diagram. 
Typical value = false.
\t"""@en .

cim:ExcST4B.ta a owl:DatatypeProperty ;
  rdfs:label "ta"@en ;
  rdfs:domain cim:ExcST4B ;
  rdfs:range cim:Seconds ;
  skos:definition "Voltage regulator time constant (<i>Ta</i>) (&gt;= 0).  Typical value = 0,02."@en .

cim:ExcST4B.thetap a owl:DatatypeProperty ;
  rdfs:label "thetap"@en ;
  rdfs:domain cim:ExcST4B ;
  rdfs:range cim:AngleDegrees ;
  skos:definition "Potential circuit phase angle (<i>theta</i><i><sub>p</sub></i>).  Typical value = 0."@en .

cim:ExcST4B.uel a owl:DatatypeProperty ;
  rdfs:label "uel"@en ;
  rdfs:domain cim:ExcST4B ;
  rdfs:range xsd:boolean ;
  skos:definition """
Selector (<i>UEL</i>).
true = <i>UEL</i> is part of block diagram
false = <i>UEL</i> is not part of block diagram. 
Typical value = false.
\t"""@en .

cim:ExcST4B.vbmax a owl:DatatypeProperty ;
  rdfs:label "vbmax"@en ;
  rdfs:domain cim:ExcST4B ;
  rdfs:range cim:PU ;
  skos:definition "Maximum excitation voltage (<i>Vbmax</i>) (&gt; 0).  Typical value = 11,63."@en .

cim:ExcST4B.vgmax a owl:DatatypeProperty ;
  rdfs:label "vgmax"@en ;
  rdfs:domain cim:ExcST4B ;
  rdfs:range cim:PU ;
  skos:definition "Maximum inner loop feedback voltage (<i>Vgmax</i>) (&gt;= 0).  Typical value = 5,8."@en .

cim:ExcST4B.vmmax a owl:DatatypeProperty ;
  rdfs:label "vmmax"@en ;
  rdfs:domain cim:ExcST4B ;
  rdfs:range cim:PU ;
  skos:definition "Maximum inner loop output (<i>Vmmax</i>) (&gt; ExcST4B.vmmin).  Typical value = 99."@en .

cim:ExcST4B.vmmin a owl:DatatypeProperty ;
  rdfs:label "vmmin"@en ;
  rdfs:domain cim:ExcST4B ;
  rdfs:range cim:PU ;
  skos:definition "Minimum inner loop output (<i>Vmmin</i>) (&lt; ExcST4B.vmmax).  Typical value = -99."@en .

cim:ExcST4B.vrmax a owl:DatatypeProperty ;
  rdfs:label "vrmax"@en ;
  rdfs:domain cim:ExcST4B ;
  rdfs:range cim:PU ;
  skos:definition "Maximum voltage regulator output (<i>Vrmax</i>) (&gt; 0).  Typical value = 1."@en .

cim:ExcST4B.vrmin a owl:DatatypeProperty ;
  rdfs:label "vrmin"@en ;
  rdfs:domain cim:ExcST4B ;
  rdfs:range cim:PU ;
  skos:definition "Minimum voltage regulator output (<i>Vrmin</i>) (&lt; 0).  Typical value = -0,87."@en .

cim:ExcST4B.xl a owl:DatatypeProperty ;
  rdfs:label "xl"@en ;
  rdfs:domain cim:ExcST4B ;
  rdfs:range cim:PU ;
  skos:definition "Reactance associated with potential source (<i>Xl</i>) (&gt;= 0).  Typical value = 0,124."@en .

cim:ExcST6B.ilr a owl:DatatypeProperty ;
  rdfs:label "ilr"@en ;
  rdfs:domain cim:ExcST6B ;
  rdfs:range cim:PU ;
  skos:definition "Exciter output current limit reference (<i>Ilr</i>) (&gt; 0).  Typical value = 4,164."@en .

cim:ExcST6B.k1 a owl:DatatypeProperty ;
  rdfs:label "k1"@en ;
  rdfs:domain cim:ExcST6B ;
  rdfs:range xsd:boolean ;
  skos:definition """
Selector (<i>K1</i>).
true = feedback is from <i>Ifd</i>
false = feedback is not from <i>Ifd</i>.
Typical value = true.
\t"""@en .

cim:ExcST6B.kcl a owl:DatatypeProperty ;
  rdfs:label "kcl"@en ;
  rdfs:domain cim:ExcST6B ;
  rdfs:range cim:PU ;
  skos:definition "Exciter output current limit adjustment (<i>Kcl</i>) (&gt; 0).  Typical value = 1,0577."@en .

cim:ExcST6B.kff a owl:DatatypeProperty ;
  rdfs:label "kff"@en ;
  rdfs:domain cim:ExcST6B ;
  rdfs:range cim:PU ;
  skos:definition "Pre-control gain constant of the inner loop field regulator (<i>Kff</i>).  Typical value = 1."@en .

cim:ExcST6B.kg a owl:DatatypeProperty ;
  rdfs:label "kg"@en ;
  rdfs:domain cim:ExcST6B ;
  rdfs:range cim:PU ;
  skos:definition "Feedback gain constant of the inner loop field regulator (<i>Kg</i>) (&gt;= 0).  Typical value = 1."@en .

cim:ExcST6B.kia a owl:DatatypeProperty ;
  rdfs:label "kia"@en ;
  rdfs:domain cim:ExcST6B ;
  rdfs:range cim:PU ;
  skos:definition "Voltage regulator integral gain (<i>Kia</i>) (&gt; 0).  Typical value = 45,094."@en .

cim:ExcST6B.klr a owl:DatatypeProperty ;
  rdfs:label "klr"@en ;
  rdfs:domain cim:ExcST6B ;
  rdfs:range cim:PU ;
  skos:definition "Exciter output current limit adjustment (<i>Kcl</i>) (&gt; 0).  Typical value = 17,33."@en .

cim:ExcST6B.km a owl:DatatypeProperty ;
  rdfs:label "km"@en ;
  rdfs:domain cim:ExcST6B ;
  rdfs:range cim:PU ;
  skos:definition "Forward gain constant of the inner loop field regulator (<i>Km</i>).  Typical value = 1."@en .

cim:ExcST6B.kpa a owl:DatatypeProperty ;
  rdfs:label "kpa"@en ;
  rdfs:domain cim:ExcST6B ;
  rdfs:range cim:PU ;
  skos:definition "Voltage regulator proportional gain (<i>Kpa</i>) (&gt; 0).  Typical value = 18,038."@en .

cim:ExcST6B.kvd a owl:DatatypeProperty ;
  rdfs:label "kvd"@en ;
  rdfs:domain cim:ExcST6B ;
  rdfs:range cim:PU ;
  skos:definition "Voltage regulator derivative gain (<i>Kvd</i>).  Typical value = 0."@en .

cim:ExcST6B.oelin a owl:DatatypeProperty ;
  rdfs:label "oelin"@en ;
  rdfs:domain cim:ExcST6B ;
  rdfs:range cim:ExcST6BOELselectorKind ;
  skos:definition "OEL input selector (<i>OELin</i>).  Typical value = noOELinput (corresponds to <i>OELin</i> = 0 on diagram)."@en .

cim:ExcST6B.tg a owl:DatatypeProperty ;
  rdfs:label "tg"@en ;
  rdfs:domain cim:ExcST6B ;
  rdfs:range cim:Seconds ;
  skos:definition "Feedback time constant of inner loop field voltage regulator (<i>Tg</i>) (&gt;= 0).  Typical value = 0,02."@en .

cim:ExcST6B.ts a owl:DatatypeProperty ;
  rdfs:label "ts"@en ;
  rdfs:domain cim:ExcST6B ;
  rdfs:range cim:Seconds ;
  skos:definition "Rectifier firing time constant (<i>Ts</i>) (&gt;= 0).  Typical value = 0."@en .

cim:ExcST6B.tvd a owl:DatatypeProperty ;
  rdfs:label "tvd"@en ;
  rdfs:domain cim:ExcST6B ;
  rdfs:range cim:Seconds ;
  skos:definition "Voltage regulator derivative gain (<i>Tvd</i>) (&gt;= 0).  Typical value = 0."@en .

cim:ExcST6B.vamax a owl:DatatypeProperty ;
  rdfs:label "vamax"@en ;
  rdfs:domain cim:ExcST6B ;
  rdfs:range cim:PU ;
  skos:definition "Maximum voltage regulator output (<i>Vamax</i>) (&gt; 0).  Typical value = 4,81."@en .

cim:ExcST6B.vamin a owl:DatatypeProperty ;
  rdfs:label "vamin"@en ;
  rdfs:domain cim:ExcST6B ;
  rdfs:range cim:PU ;
  skos:definition "Minimum voltage regulator output (<i>Vamin</i>) (&lt; 0).  Typical value = -3,85."@en .

cim:ExcST6B.vilim a owl:DatatypeProperty ;
  rdfs:label "vilim"@en ;
  rdfs:domain cim:ExcST6B ;
  rdfs:range xsd:boolean ;
  skos:definition """
Selector (<i>Vilim</i>).
true = <i>Vimin</i>-<i>Vimax</i> limiter is active
false = <i>Vimin</i>-<i>Vimax</i> limiter is not active.
Typical value = true.
\t"""@en .

cim:ExcST6B.vimax a owl:DatatypeProperty ;
  rdfs:label "vimax"@en ;
  rdfs:domain cim:ExcST6B ;
  rdfs:range cim:PU ;
  skos:definition "Maximum voltage regulator input limit (<i>Vimax</i>) (&gt; ExcST6B.vimin).  Typical value = 10."@en .

cim:ExcST6B.vimin a owl:DatatypeProperty ;
  rdfs:label "vimin"@en ;
  rdfs:domain cim:ExcST6B ;
  rdfs:range cim:PU ;
  skos:definition "Minimum voltage regulator input limit (<i>Vimin</i>) (&lt; ExcST6B.vimax).  Typical value = -10."@en .

cim:ExcST6B.vmult a owl:DatatypeProperty ;
  rdfs:label "vmult"@en ;
  rdfs:domain cim:ExcST6B ;
  rdfs:range xsd:boolean ;
  skos:definition """
Selector (<i>vmult</i>).
true = multiply regulator output by terminal voltage
false = do not multiply regulator output by terminal voltage. 
Typical value = true.
\t"""@en .

cim:ExcST6B.vrmax a owl:DatatypeProperty ;
  rdfs:label "vrmax"@en ;
  rdfs:domain cim:ExcST6B ;
  rdfs:range cim:PU ;
  skos:definition "Maximum voltage regulator output (<i>Vrmax</i>) (&gt; 0).  Typical value = 4,81."@en .

cim:ExcST6B.vrmin a owl:DatatypeProperty ;
  rdfs:label "vrmin"@en ;
  rdfs:domain cim:ExcST6B ;
  rdfs:range cim:PU ;
  skos:definition "Minimum voltage regulator output (<i>Vrmin</i>) (&lt; 0).  Typical value = -3,85."@en .

cim:ExcST6B.xc a owl:DatatypeProperty ;
  rdfs:label "xc"@en ;
  rdfs:domain cim:ExcST6B ;
  rdfs:range cim:PU ;
  skos:definition "Excitation source reactance (<i>Xc</i>).  Typical value = 0,05."@en .

cim:ExcST7B.kh a owl:DatatypeProperty ;
  rdfs:label "kh"@en ;
  rdfs:domain cim:ExcST7B ;
  rdfs:range cim:PU ;
  skos:definition "High-value gate feedback gain (<i>Kh</i>) (&gt;= 0).  Typical value = 1."@en .

cim:ExcST7B.kia a owl:DatatypeProperty ;
  rdfs:label "kia"@en ;
  rdfs:domain cim:ExcST7B ;
  rdfs:range cim:PU ;
  skos:definition "Voltage regulator integral gain (<i>Kia</i>) (&gt;= 0).  Typical value = 1."@en .

cim:ExcST7B.kl a owl:DatatypeProperty ;
  rdfs:label "kl"@en ;
  rdfs:domain cim:ExcST7B ;
  rdfs:range cim:PU ;
  skos:definition "Low-value gate feedback gain (<i>Kl</i>) (&gt;= 0).  Typical value = 1."@en .

cim:ExcST7B.kpa a owl:DatatypeProperty ;
  rdfs:label "kpa"@en ;
  rdfs:domain cim:ExcST7B ;
  rdfs:range cim:PU ;
  skos:definition "Voltage regulator proportional gain (<i>Kpa</i>) (&gt; 0).  Typical value = 40."@en .

cim:ExcST7B.oelin a owl:DatatypeProperty ;
  rdfs:label "oelin"@en ;
  rdfs:domain cim:ExcST7B ;
  rdfs:range cim:ExcST7BOELselectorKind ;
  skos:definition "OEL input selector (<i>OELin</i>). Typical value = noOELinput."@en .

cim:ExcST7B.tb a owl:DatatypeProperty ;
  rdfs:label "tb"@en ;
  rdfs:domain cim:ExcST7B ;
  rdfs:range cim:Seconds ;
  skos:definition "Regulator lag time constant (<i>Tb</i>) (&gt;= 0).  Typical value = 1."@en .

cim:ExcST7B.tc a owl:DatatypeProperty ;
  rdfs:label "tc"@en ;
  rdfs:domain cim:ExcST7B ;
  rdfs:range cim:Seconds ;
  skos:definition "Regulator lead time constant (<i>Tc</i>) (&gt;= 0).  Typical value = 1."@en .

cim:ExcST7B.tf a owl:DatatypeProperty ;
  rdfs:label "tf"@en ;
  rdfs:domain cim:ExcST7B ;
  rdfs:range cim:Seconds ;
  skos:definition "Excitation control system stabilizer time constant (<i>Tf</i>) (&gt;= 0).  Typical value = 1."@en .

cim:ExcST7B.tg a owl:DatatypeProperty ;
  rdfs:label "tg"@en ;
  rdfs:domain cim:ExcST7B ;
  rdfs:range cim:Seconds ;
  skos:definition "Feedback time constant of inner loop field voltage regulator (<i>Tg</i>) (&gt;= 0).  Typical value = 1."@en .

cim:ExcST7B.tia a owl:DatatypeProperty ;
  rdfs:label "tia"@en ;
  rdfs:domain cim:ExcST7B ;
  rdfs:range cim:Seconds ;
  skos:definition "Feedback time constant (<i>Tia</i>) (&gt;= 0).  Typical value = 3."@en .

cim:ExcST7B.ts a owl:DatatypeProperty ;
  rdfs:label "ts"@en ;
  rdfs:domain cim:ExcST7B ;
  rdfs:range cim:Seconds ;
  skos:definition "Rectifier firing time constant (<i>Ts</i>) (&gt;= 0).  Typical value = 0."@en .

cim:ExcST7B.uelin a owl:DatatypeProperty ;
  rdfs:label "uelin"@en ;
  rdfs:domain cim:ExcST7B ;
  rdfs:range cim:ExcST7BUELselectorKind ;
  skos:definition "UEL input selector (<i>UELin</i>). Typical value = noUELinput."@en .

cim:ExcST7B.vmax a owl:DatatypeProperty ;
  rdfs:label "vmax"@en ;
  rdfs:domain cim:ExcST7B ;
  rdfs:range cim:PU ;
  skos:definition "Maximum voltage reference signal (<i>Vmax</i>) (&gt; 0 and &gt; ExcST7B.vmin)).  Typical value = 1,1."@en .

cim:ExcST7B.vmin a owl:DatatypeProperty ;
  rdfs:label "vmin"@en ;
  rdfs:domain cim:ExcST7B ;
  rdfs:range cim:PU ;
  skos:definition "Minimum voltage reference signal (<i>Vmin</i>) (&gt; 0 and &lt; ExcST7B.vmax).  Typical value = 0,9."@en .

cim:ExcST7B.vrmax a owl:DatatypeProperty ;
  rdfs:label "vrmax"@en ;
  rdfs:domain cim:ExcST7B ;
  rdfs:range cim:PU ;
  skos:definition "Maximum voltage regulator output (<i>Vrmax</i>) (&gt; 0).  Typical value = 5."@en .

cim:ExcST7B.vrmin a owl:DatatypeProperty ;
  rdfs:label "vrmin"@en ;
  rdfs:domain cim:ExcST7B ;
  rdfs:range cim:PU ;
  skos:definition "Minimum voltage regulator output (<i>Vrmin</i>) (&lt; 0).  Typical value = -4,5."@en .

cim:ExcitationSystemUserDefined.proprietary a owl:DatatypeProperty ;
  rdfs:label "proprietary"@en ;
  rdfs:domain cim:ExcitationSystemUserDefined ;
  rdfs:range xsd:boolean ;
  skos:definition """
Behaviour is based on a proprietary model as opposed to a detailed model.
true = user-defined model is proprietary with behaviour mutually understood by sending and receiving applications and parameters passed as general attributes
false = user-defined model is explicitly defined in terms of control blocks and their input and output signals.
\t"""@en .

cim:Frequency.multiplier a owl:DatatypeProperty, owl:FunctionalProperty ;
  rdfs:label "multiplier"@en ;
  dy:isFixed "True " ;
  rdf:value "none" ;
  rdfs:domain cim:Frequency ;
  rdfs:range cim:UnitMultiplier .

cim:Frequency.unit a owl:DatatypeProperty, owl:FunctionalProperty ;
  rdfs:label "unit"@en ;
  dy:isFixed "True " ;
  rdf:value "Hz" ;
  rdfs:domain cim:Frequency ;
  rdfs:range cim:UnitSymbol .

cim:Frequency.value a owl:DatatypeProperty, owl:FunctionalProperty ;
  rdfs:label "value"@en ;
  rdfs:domain cim:Frequency ;
  rdfs:range xsd:float .

cim:GenICompensationForGenJ.rcij a owl:DatatypeProperty ;
  rdfs:label "rcij"@en ;
  rdfs:domain cim:GenICompensationForGenJ ;
  rdfs:range cim:PU ;
  skos:definition "<font color=\"#0f0f0f\">Resistive component of compensation of generator associated with this IEEE type 2 voltage compensator for current flow out of another generator (<i>Rcij</i>).</font>"@en .

cim:GenICompensationForGenJ.xcij a owl:DatatypeProperty ;
  rdfs:label "xcij"@en ;
  rdfs:domain cim:GenICompensationForGenJ ;
  rdfs:range cim:PU ;
  skos:definition "<font color=\"#0f0f0f\">Reactive component of compensation of generator associated with this IEEE type 2 voltage compensator for current flow out of another generator (<i>Xcij</i>).</font>"@en .

cim:GovCT1.aset a owl:DatatypeProperty ;
  rdfs:label "aset"@en ;
  rdfs:domain cim:GovCT1 ;
  rdfs:range xsd:float ;
  skos:definition "Acceleration limiter setpoint (<i>Aset</i>).  Unit = PU / s.  Typical value = 0,01."@en .

cim:GovCT1.db a owl:DatatypeProperty ;
  rdfs:label "db"@en ;
  rdfs:domain cim:GovCT1 ;
  rdfs:range cim:PU ;
  skos:definition "Speed governor deadband in PU speed (<i>db</i>).  In the majority of applications, it is recommended that this value be set to zero.  Typical value = 0."@en .

cim:GovCT1.dm a owl:DatatypeProperty ;
  rdfs:label "dm"@en ;
  rdfs:domain cim:GovCT1 ;
  rdfs:range cim:PU ;
  skos:definition "Speed sensitivity coefficient (<i>Dm</i>).  <i>Dm</i> can represent either the variation of the engine power with the shaft speed or the variation of maximum power capability with shaft speed.  If it is positive it describes the falling slope of the engine speed verses power characteristic as speed increases. A slightly falling characteristic is typical for reciprocating engines and some aero-derivative turbines.  If it is negative the engine power is assumed to be unaffected by the shaft speed, but the maximum permissible fuel flow is taken to fall with falling shaft speed. This is characteristic of single-shaft industrial turbines due to exhaust temperature limits.  Typical value = 0."@en .

cim:GovCT1.ka a owl:DatatypeProperty ;
  rdfs:label "ka"@en ;
  rdfs:domain cim:GovCT1 ;
  rdfs:range cim:PU ;
  skos:definition "Acceleration limiter gain (<i>Ka</i>).  Typical value = 10."@en .

cim:GovCT1.kdgov a owl:DatatypeProperty ;
  rdfs:label "kdgov"@en ;
  rdfs:domain cim:GovCT1 ;
  rdfs:range cim:PU ;
  skos:definition "Governor derivative gain (<i>Kdgov</i>).  Typical value = 0."@en .

cim:GovCT1.kigov a owl:DatatypeProperty ;
  rdfs:label "kigov"@en ;
  rdfs:domain cim:GovCT1 ;
  rdfs:range cim:PU ;
  skos:definition "Governor integral gain (<i>Kigov</i>).  Typical value = 2."@en .

cim:GovCT1.kiload a owl:DatatypeProperty ;
  rdfs:label "kiload"@en ;
  rdfs:domain cim:GovCT1 ;
  rdfs:range cim:PU ;
  skos:definition "Load limiter integral gain for PI controller (<i>Kiload</i>).  Typical value = 0,67."@en .

cim:GovCT1.kimw a owl:DatatypeProperty ;
  rdfs:label "kimw"@en ;
  rdfs:domain cim:GovCT1 ;
  rdfs:range cim:PU ;
  skos:definition "Power controller (reset) gain (<i>Kimw</i>).  The default value of 0,01 corresponds to a reset time of 100 s.  A value of 0,001 corresponds to a relatively slow-acting load controller.  Typical value = 0,01."@en .

cim:GovCT1.kpgov a owl:DatatypeProperty ;
  rdfs:label "kpgov"@en ;
  rdfs:domain cim:GovCT1 ;
  rdfs:range cim:PU ;
  skos:definition "Governor proportional gain (<i>Kpgov</i>).  Typical value = 10."@en .

cim:GovCT1.kpload a owl:DatatypeProperty ;
  rdfs:label "kpload"@en ;
  rdfs:domain cim:GovCT1 ;
  rdfs:range cim:PU ;
  skos:definition "Load limiter proportional gain for PI controller (<i>Kpload</i>).  Typical value = 2."@en .

cim:GovCT1.kturb a owl:DatatypeProperty ;
  rdfs:label "kturb"@en ;
  rdfs:domain cim:GovCT1 ;
  rdfs:range cim:PU ;
  skos:definition "Turbine gain (<i>Kturb</i>) (&gt; 0).  Typical value = 1,5."@en .

cim:GovCT1.ldref a owl:DatatypeProperty ;
  rdfs:label "ldref"@en ;
  rdfs:domain cim:GovCT1 ;
  rdfs:range cim:PU ;
  skos:definition "Load limiter reference value (<i>Ldref</i>).  Typical value = 1."@en .

cim:GovCT1.maxerr a owl:DatatypeProperty ;
  rdfs:label "maxerr"@en ;
  rdfs:domain cim:GovCT1 ;
  rdfs:range cim:PU ;
  skos:definition "Maximum value for speed error signal (<i>maxerr</i>) (&gt; GovCT1.minerr).  Typical value = 0,05."@en .

cim:GovCT1.minerr a owl:DatatypeProperty ;
  rdfs:label "minerr"@en ;
  rdfs:domain cim:GovCT1 ;
  rdfs:range cim:PU ;
  skos:definition "Minimum value for speed error signal (<i>minerr</i>) (&lt; GovCT1.maxerr).  Typical value = -0,05."@en .

cim:GovCT1.mwbase a owl:DatatypeProperty ;
  rdfs:label "mwbase"@en ;
  rdfs:domain cim:GovCT1 ;
  rdfs:range cim:ActivePower ;
  skos:definition "Base for power values (<i>MWbase</i>) (&gt; 0).  Unit = MW."@en .

cim:GovCT1.r a owl:DatatypeProperty ;
  rdfs:label "r"@en ;
  rdfs:domain cim:GovCT1 ;
  rdfs:range cim:PU ;
  skos:definition "Permanent droop (<i>R</i>).  Typical value = 0,04."@en .

cim:GovCT1.rclose a owl:DatatypeProperty ;
  rdfs:label "rclose"@en ;
  rdfs:domain cim:GovCT1 ;
  rdfs:range xsd:float ;
  skos:definition "Minimum valve closing rate (<i>Rclose</i>).  Unit = PU / s.  Typical value = -0,1."@en .

cim:GovCT1.rdown a owl:DatatypeProperty ;
  rdfs:label "rdown"@en ;
  rdfs:domain cim:GovCT1 ;
  rdfs:range cim:PU ;
  skos:definition "Maximum rate of load limit decrease (<i>Rdown</i>).  Typical value = -99."@en .

cim:GovCT1.ropen a owl:DatatypeProperty ;
  rdfs:label "ropen"@en ;
  rdfs:domain cim:GovCT1 ;
  rdfs:range xsd:float ;
  skos:definition "Maximum valve opening rate (<i>Ropen</i>).  Unit = PU / s.  Typical value = 0.10."@en .

cim:GovCT1.rselect a owl:DatatypeProperty ;
  rdfs:label "rselect"@en ;
  rdfs:domain cim:GovCT1 ;
  rdfs:range cim:DroopSignalFeedbackKind ;
  skos:definition "Feedback signal for droop (<i>Rselect</i>).  Typical value = electricalPower."@en .

cim:GovCT1.rup a owl:DatatypeProperty ;
  rdfs:label "rup"@en ;
  rdfs:domain cim:GovCT1 ;
  rdfs:range cim:PU ;
  skos:definition "Maximum rate of load limit increase (<i>Rup</i>).  Typical value = 99."@en .

cim:GovCT1.ta a owl:DatatypeProperty ;
  rdfs:label "ta"@en ;
  rdfs:domain cim:GovCT1 ;
  rdfs:range cim:Seconds ;
  skos:definition "Acceleration limiter time constant (<i>Ta</i>) (&gt; 0).  Typical value = 0,1."@en .

cim:GovCT1.tact a owl:DatatypeProperty ;
  rdfs:label "tact"@en ;
  rdfs:domain cim:GovCT1 ;
  rdfs:range cim:Seconds ;
  skos:definition "Actuator time constant (<i>Tact</i>) (&gt;= 0).  Typical value = 0,5."@en .

cim:GovCT1.tb a owl:DatatypeProperty ;
  rdfs:label "tb"@en ;
  rdfs:domain cim:GovCT1 ;
  rdfs:range cim:Seconds ;
  skos:definition "Turbine lag time constant (<i>Tb</i>) (&gt; 0).  Typical value = 0,5."@en .

cim:GovCT1.tc a owl:DatatypeProperty ;
  rdfs:label "tc"@en ;
  rdfs:domain cim:GovCT1 ;
  rdfs:range cim:Seconds ;
  skos:definition "Turbine lead time constant (<i>Tc</i>) (&gt;= 0).  Typical value = 0."@en .

cim:GovCT1.tdgov a owl:DatatypeProperty ;
  rdfs:label "tdgov"@en ;
  rdfs:domain cim:GovCT1 ;
  rdfs:range cim:Seconds ;
  skos:definition "Governor derivative controller time constant (<i>Tdgov</i>) (&gt;= 0).  Typical value = 1."@en .

cim:GovCT1.teng a owl:DatatypeProperty ;
  rdfs:label "teng"@en ;
  rdfs:domain cim:GovCT1 ;
  rdfs:range cim:Seconds ;
  skos:definition "Transport time delay for diesel engine used in representing diesel engines where there is a small but measurable transport delay between a change in fuel flow setting and the development of torque (<i>Teng</i>) (&gt;= 0).  <i>Teng</i> should be zero in all but special cases where this transport delay is of particular concern.  Typical value = 0."@en .

cim:GovCT1.tfload a owl:DatatypeProperty ;
  rdfs:label "tfload"@en ;
  rdfs:domain cim:GovCT1 ;
  rdfs:range cim:Seconds ;
  skos:definition "Load-limiter time constant (<i>Tfload</i>) (&gt; 0).  Typical value = 3."@en .

cim:GovCT1.tpelec a owl:DatatypeProperty ;
  rdfs:label "tpelec"@en ;
  rdfs:domain cim:GovCT1 ;
  rdfs:range cim:Seconds ;
  skos:definition "Electrical power transducer time constant (<i>Tpelec</i>) (&gt; 0).  Typical value = 1."@en .

cim:GovCT1.tsa a owl:DatatypeProperty ;
  rdfs:label "tsa"@en ;
  rdfs:domain cim:GovCT1 ;
  rdfs:range cim:Seconds ;
  skos:definition "Temperature detection lead time constant (<i>Tsa</i>) (&gt;= 0).  Typical value = 4."@en .

cim:GovCT1.tsb a owl:DatatypeProperty ;
  rdfs:label "tsb"@en ;
  rdfs:domain cim:GovCT1 ;
  rdfs:range cim:Seconds ;
  skos:definition "Temperature detection lag time constant (<i>Tsb</i>) (&gt;= 0).  Typical value = 5."@en .

cim:GovCT1.vmax a owl:DatatypeProperty ;
  rdfs:label "vmax"@en ;
  rdfs:domain cim:GovCT1 ;
  rdfs:range cim:PU ;
  skos:definition "Maximum valve position limit (<i>Vmax</i>) (&gt; GovCT1.vmin).  Typical value = 1."@en .

cim:GovCT1.vmin a owl:DatatypeProperty ;
  rdfs:label "vmin"@en ;
  rdfs:domain cim:GovCT1 ;
  rdfs:range cim:PU ;
  skos:definition "Minimum valve position limit (<i>Vmin</i>) (&lt; GovCT1.vmax).  Typical value = 0,15."@en .

cim:GovCT1.wfnl a owl:DatatypeProperty ;
  rdfs:label "wfnl"@en ;
  rdfs:domain cim:GovCT1 ;
  rdfs:range cim:PU ;
  skos:definition "No load fuel flow (<i>Wfnl</i>).  Typical value = 0,2."@en .

cim:GovCT1.wfspd a owl:DatatypeProperty ;
  rdfs:label "wfspd"@en ;
  rdfs:domain cim:GovCT1 ;
  rdfs:range xsd:boolean ;
  skos:definition """
Switch for fuel source characteristic to recognize that fuel flow, for a given fuel valve stroke, can be proportional to engine speed (<i>Wfspd</i>).
true = fuel flow proportional to speed (for some gas turbines and diesel engines with positive displacement fuel injectors)
false = fuel control system keeps fuel flow independent of engine speed.
Typical value = true.
\t"""@en .

cim:GovCT2.aset a owl:DatatypeProperty ;
  rdfs:label "aset"@en ;
  rdfs:domain cim:GovCT2 ;
  rdfs:range xsd:float ;
  skos:definition "Acceleration limiter setpoint (<i>Aset</i>).  Unit = PU / s.  Typical value = 10."@en .

cim:GovCT2.db a owl:DatatypeProperty ;
  rdfs:label "db"@en ;
  rdfs:domain cim:GovCT2 ;
  rdfs:range cim:PU ;
  skos:definition "Speed governor deadband in PU speed (<i>db</i>).  In the majority of applications, it is recommended that this value be set to zero.  Typical value = 0."@en .

cim:GovCT2.dm a owl:DatatypeProperty ;
  rdfs:label "dm"@en ;
  rdfs:domain cim:GovCT2 ;
  rdfs:range cim:PU ;
  skos:definition "Speed sensitivity coefficient (<i>Dm</i>).  <i>Dm</i> can represent either the variation of the engine power with the shaft speed or the variation of maximum power capability with shaft speed.  If it is positive it describes the falling slope of the engine speed verses power characteristic as speed increases. A slightly falling characteristic is typical for reciprocating engines and some aero-derivative turbines.  If it is negative the engine power is assumed to be unaffected by the shaft speed, but the maximum permissible fuel flow is taken to fall with falling shaft speed. This is characteristic of single-shaft industrial turbines due to exhaust temperature limits.  Typical value = 0."@en .

cim:GovCT2.flim1 a owl:DatatypeProperty ;
  rdfs:label "flim1"@en ;
  rdfs:domain cim:GovCT2 ;
  rdfs:range cim:Frequency ;
  skos:definition "Frequency threshold 1 (<i>Flim1</i>).  Unit = Hz.  Typical value = 59."@en .

cim:GovCT2.flim10 a owl:DatatypeProperty ;
  rdfs:label "flim10"@en ;
  rdfs:domain cim:GovCT2 ;
  rdfs:range cim:Frequency ;
  skos:definition "Frequency threshold 10 (<i>Flim10</i>).  Unit = Hz.  Typical value = 0."@en .

cim:GovCT2.flim2 a owl:DatatypeProperty ;
  rdfs:label "flim2"@en ;
  rdfs:domain cim:GovCT2 ;
  rdfs:range cim:Frequency ;
  skos:definition "Frequency threshold 2 (<i>Flim2</i>).  Unit = Hz.  Typical value = 0."@en .

cim:GovCT2.flim3 a owl:DatatypeProperty ;
  rdfs:label "flim3"@en ;
  rdfs:domain cim:GovCT2 ;
  rdfs:range cim:Frequency ;
  skos:definition "Frequency threshold 3 (<i>Flim3</i>).  Unit = Hz.  Typical value = 0."@en .

cim:GovCT2.flim4 a owl:DatatypeProperty ;
  rdfs:label "flim4"@en ;
  rdfs:domain cim:GovCT2 ;
  rdfs:range cim:Frequency ;
  skos:definition "Frequency threshold 4 (<i>Flim4</i>).  Unit = Hz.  Typical value = 0."@en .

cim:GovCT2.flim5 a owl:DatatypeProperty ;
  rdfs:label "flim5"@en ;
  rdfs:domain cim:GovCT2 ;
  rdfs:range cim:Frequency ;
  skos:definition "Frequency threshold 5 (<i>Flim5</i>).  Unit = Hz.  Typical value = 0."@en .

cim:GovCT2.flim6 a owl:DatatypeProperty ;
  rdfs:label "flim6"@en ;
  rdfs:domain cim:GovCT2 ;
  rdfs:range cim:Frequency ;
  skos:definition "Frequency threshold 6 (<i>Flim6</i>).  Unit = Hz.  Typical value = 0."@en .

cim:GovCT2.flim7 a owl:DatatypeProperty ;
  rdfs:label "flim7"@en ;
  rdfs:domain cim:GovCT2 ;
  rdfs:range cim:Frequency ;
  skos:definition "Frequency threshold 7 (<i>Flim7</i>).  Unit = Hz.  Typical value = 0."@en .

cim:GovCT2.flim8 a owl:DatatypeProperty ;
  rdfs:label "flim8"@en ;
  rdfs:domain cim:GovCT2 ;
  rdfs:range cim:Frequency ;
  skos:definition "Frequency threshold 8 (<i>Flim8</i>).  Unit = Hz.  Typical value = 0."@en .

cim:GovCT2.flim9 a owl:DatatypeProperty ;
  rdfs:label "flim9"@en ;
  rdfs:domain cim:GovCT2 ;
  rdfs:range cim:Frequency ;
  skos:definition "Frequency threshold 9 (<i>Flim9</i>).  Unit = Hz.  Typical value = 0."@en .

cim:GovCT2.ka a owl:DatatypeProperty ;
  rdfs:label "ka"@en ;
  rdfs:domain cim:GovCT2 ;
  rdfs:range cim:PU ;
  skos:definition "Acceleration limiter gain (<i>Ka</i>).  Typical value = 10."@en .

cim:GovCT2.kdgov a owl:DatatypeProperty ;
  rdfs:label "kdgov"@en ;
  rdfs:domain cim:GovCT2 ;
  rdfs:range cim:PU ;
  skos:definition "Governor derivative gain (<i>Kdgov</i>).  Typical value = 0."@en .

cim:GovCT2.kigov a owl:DatatypeProperty ;
  rdfs:label "kigov"@en ;
  rdfs:domain cim:GovCT2 ;
  rdfs:range cim:PU ;
  skos:definition "Governor integral gain (<i>Kigov</i>).  Typical value = 0,45."@en .

cim:GovCT2.kiload a owl:DatatypeProperty ;
  rdfs:label "kiload"@en ;
  rdfs:domain cim:GovCT2 ;
  rdfs:range cim:PU ;
  skos:definition "Load limiter integral gain for PI controller (<i>Kiload</i>).  Typical value = 1."@en .

cim:GovCT2.kimw a owl:DatatypeProperty ;
  rdfs:label "kimw"@en ;
  rdfs:domain cim:GovCT2 ;
  rdfs:range cim:PU ;
  skos:definition "Power controller (reset) gain (<i>Kimw</i>).  The default value of 0,01 corresponds to a reset time of 100 seconds.  A value of 0,001 corresponds to a relatively slow-acting load controller.  Typical value = 0."@en .

cim:GovCT2.kpgov a owl:DatatypeProperty ;
  rdfs:label "kpgov"@en ;
  rdfs:domain cim:GovCT2 ;
  rdfs:range cim:PU ;
  skos:definition "Governor proportional gain (<i>Kpgov</i>).  Typical value = 4."@en .

cim:GovCT2.kpload a owl:DatatypeProperty ;
  rdfs:label "kpload"@en ;
  rdfs:domain cim:GovCT2 ;
  rdfs:range cim:PU ;
  skos:definition "Load limiter proportional gain for PI controller (<i>Kpload</i>).  Typical value = 1."@en .

cim:GovCT2.kturb a owl:DatatypeProperty ;
  rdfs:label "kturb"@en ;
  rdfs:domain cim:GovCT2 ;
  rdfs:range cim:PU ;
  skos:definition "Turbine gain (<i>Kturb</i>).  Typical value = 1,9168."@en .

cim:GovCT2.ldref a owl:DatatypeProperty ;
  rdfs:label "ldref"@en ;
  rdfs:domain cim:GovCT2 ;
  rdfs:range cim:PU ;
  skos:definition "Load limiter reference value (<i>Ldref</i>).  Typical value = 1."@en .

cim:GovCT2.maxerr a owl:DatatypeProperty ;
  rdfs:label "maxerr"@en ;
  rdfs:domain cim:GovCT2 ;
  rdfs:range cim:PU ;
  skos:definition "Maximum value for speed error signal (<i>Maxerr</i>) (&gt; GovCT2.minerr).  Typical value = 1."@en .

cim:GovCT2.minerr a owl:DatatypeProperty ;
  rdfs:label "minerr"@en ;
  rdfs:domain cim:GovCT2 ;
  rdfs:range cim:PU ;
  skos:definition "Minimum value for speed error signal (<i>Minerr</i>) (&lt; GovCT2.maxerr).  Typical value = -1."@en .

cim:GovCT2.mwbase a owl:DatatypeProperty ;
  rdfs:label "mwbase"@en ;
  rdfs:domain cim:GovCT2 ;
  rdfs:range cim:ActivePower ;
  skos:definition "Base for power values (<i>MWbase</i>) (&gt; 0).  Unit = MW."@en .

cim:GovCT2.plim1 a owl:DatatypeProperty ;
  rdfs:label "plim1"@en ;
  rdfs:domain cim:GovCT2 ;
  rdfs:range cim:PU ;
  skos:definition "Power limit 1 (<i>Plim1</i>).  Typical value = 0,8325."@en .

cim:GovCT2.plim10 a owl:DatatypeProperty ;
  rdfs:label "plim10"@en ;
  rdfs:domain cim:GovCT2 ;
  rdfs:range cim:PU ;
  skos:definition "Power limit 10 (<i>Plim10</i>).  Typical value = 0."@en .

cim:GovCT2.plim2 a owl:DatatypeProperty ;
  rdfs:label "plim2"@en ;
  rdfs:domain cim:GovCT2 ;
  rdfs:range cim:PU ;
  skos:definition "Power limit 2 (Plim2).  Typical value = 0."@en .

cim:GovCT2.plim3 a owl:DatatypeProperty ;
  rdfs:label "plim3"@en ;
  rdfs:domain cim:GovCT2 ;
  rdfs:range cim:PU ;
  skos:definition "Power limit 3 (<i>Plim3</i>).  Typical value = 0."@en .

cim:GovCT2.plim4 a owl:DatatypeProperty ;
  rdfs:label "plim4"@en ;
  rdfs:domain cim:GovCT2 ;
  rdfs:range cim:PU ;
  skos:definition "Power limit 4 (<i>Plim4</i>).  Typical value = 0."@en .

cim:GovCT2.plim5 a owl:DatatypeProperty ;
  rdfs:label "plim5"@en ;
  rdfs:domain cim:GovCT2 ;
  rdfs:range cim:PU ;
  skos:definition "Power limit 5 (<i>Plim5</i>).  Typical value = 0."@en .

cim:GovCT2.plim6 a owl:DatatypeProperty ;
  rdfs:label "plim6"@en ;
  rdfs:domain cim:GovCT2 ;
  rdfs:range cim:PU ;
  skos:definition "Power limit 6 (<i>Plim6</i>).  Typical value = 0."@en .

cim:GovCT2.plim7 a owl:DatatypeProperty ;
  rdfs:label "plim7"@en ;
  rdfs:domain cim:GovCT2 ;
  rdfs:range cim:PU ;
  skos:definition "Power limit 7 (<i>Plim7</i>).  Typical value = 0."@en .

cim:GovCT2.plim8 a owl:DatatypeProperty ;
  rdfs:label "plim8"@en ;
  rdfs:domain cim:GovCT2 ;
  rdfs:range cim:PU ;
  skos:definition "Power limit 8 (<i>Plim8</i>).  Typical value = 0."@en .

cim:GovCT2.plim9 a owl:DatatypeProperty ;
  rdfs:label "plim9"@en ;
  rdfs:domain cim:GovCT2 ;
  rdfs:range cim:PU ;
  skos:definition "Power Limit 9 (<i>Plim9</i>).  Typical value = 0."@en .

cim:GovCT2.prate a owl:DatatypeProperty ;
  rdfs:label "prate"@en ;
  rdfs:domain cim:GovCT2 ;
  rdfs:range cim:PU ;
  skos:definition "Ramp rate for frequency-dependent power limit (<i>Prate</i>).  Typical value = 0,017."@en .

cim:GovCT2.r a owl:DatatypeProperty ;
  rdfs:label "r"@en ;
  rdfs:domain cim:GovCT2 ;
  rdfs:range cim:PU ;
  skos:definition "Permanent droop (<i>R</i>).  Typical value = 0,05."@en .

cim:GovCT2.rclose a owl:DatatypeProperty ;
  rdfs:label "rclose"@en ;
  rdfs:domain cim:GovCT2 ;
  rdfs:range xsd:float ;
  skos:definition "Minimum valve closing rate (<i>Rclose</i>).  Unit = PU / s.  Typical value = -99."@en .

cim:GovCT2.rdown a owl:DatatypeProperty ;
  rdfs:label "rdown"@en ;
  rdfs:domain cim:GovCT2 ;
  rdfs:range cim:PU ;
  skos:definition "Maximum rate of load limit decrease (<i>Rdown</i>).  Typical value = -99."@en .

cim:GovCT2.ropen a owl:DatatypeProperty ;
  rdfs:label "ropen"@en ;
  rdfs:domain cim:GovCT2 ;
  rdfs:range xsd:float ;
  skos:definition "Maximum valve opening rate (<i>Ropen</i>).  Unit = PU / s.  Typical value = 99."@en .

cim:GovCT2.rselect a owl:DatatypeProperty ;
  rdfs:label "rselect"@en ;
  rdfs:domain cim:GovCT2 ;
  rdfs:range cim:DroopSignalFeedbackKind ;
  skos:definition "Feedback signal for droop (<i>Rselect</i>).  Typical value = electricalPower."@en .

cim:GovCT2.rup a owl:DatatypeProperty ;
  rdfs:label "rup"@en ;
  rdfs:domain cim:GovCT2 ;
  rdfs:range cim:PU ;
  skos:definition "Maximum rate of load limit increase (<i>Rup</i>).  Typical value = 99."@en .

cim:GovCT2.ta a owl:DatatypeProperty ;
  rdfs:label "ta"@en ;
  rdfs:domain cim:GovCT2 ;
  rdfs:range cim:Seconds ;
  skos:definition "Acceleration limiter time constant (<i>Ta</i>) (&gt;= 0).  Typical value = 1."@en .

cim:GovCT2.tact a owl:DatatypeProperty ;
  rdfs:label "tact"@en ;
  rdfs:domain cim:GovCT2 ;
  rdfs:range cim:Seconds ;
  skos:definition "Actuator time constant (<i>Tact</i>) (&gt;= 0).  Typical value = 0,4."@en .

cim:GovCT2.tb a owl:DatatypeProperty ;
  rdfs:label "tb"@en ;
  rdfs:domain cim:GovCT2 ;
  rdfs:range cim:Seconds ;
  skos:definition "Turbine lag time constant (<i>Tb</i>) (&gt;= 0).  Typical value = 0,1."@en .

cim:GovCT2.tc a owl:DatatypeProperty ;
  rdfs:label "tc"@en ;
  rdfs:domain cim:GovCT2 ;
  rdfs:range cim:Seconds ;
  skos:definition "Turbine lead time constant (<i>Tc</i>) (&gt;= 0).  Typical value = 0."@en .

cim:GovCT2.tdgov a owl:DatatypeProperty ;
  rdfs:label "tdgov"@en ;
  rdfs:domain cim:GovCT2 ;
  rdfs:range cim:Seconds ;
  skos:definition "Governor derivative controller time constant (<i>Tdgov</i>) (&gt;= 0).  Typical value = 1."@en .

cim:GovCT2.teng a owl:DatatypeProperty ;
  rdfs:label "teng"@en ;
  rdfs:domain cim:GovCT2 ;
  rdfs:range cim:Seconds ;
  skos:definition "Transport time delay for diesel engine used in representing diesel engines where there is a small but measurable transport delay between a change in fuel flow setting and the development of torque (<i>Teng</i>) (&gt;= 0).  <i>Teng</i> should be zero in all but special cases where this transport delay is of particular concern.  Typical value = 0."@en .

cim:GovCT2.tfload a owl:DatatypeProperty ;
  rdfs:label "tfload"@en ;
  rdfs:domain cim:GovCT2 ;
  rdfs:range cim:Seconds ;
  skos:definition "Load limiter time constant (<i>Tfload</i>) (&gt;= 0).  Typical value = 3."@en .

cim:GovCT2.tpelec a owl:DatatypeProperty ;
  rdfs:label "tpelec"@en ;
  rdfs:domain cim:GovCT2 ;
  rdfs:range cim:Seconds ;
  skos:definition "Electrical power transducer time constant (<i>Tpelec</i>) (&gt;= 0).  Typical value = 2,5."@en .

cim:GovCT2.tsa a owl:DatatypeProperty ;
  rdfs:label "tsa"@en ;
  rdfs:domain cim:GovCT2 ;
  rdfs:range cim:Seconds ;
  skos:definition "Temperature detection lead time constant (<i>Tsa</i>) (&gt;= 0).  Typical value = 0."@en .

cim:GovCT2.tsb a owl:DatatypeProperty ;
  rdfs:label "tsb"@en ;
  rdfs:domain cim:GovCT2 ;
  rdfs:range cim:Seconds ;
  skos:definition "Temperature detection lag time constant (<i>Tsb</i>) (&gt;= 0).  Typical value = 50."@en .

cim:GovCT2.vmax a owl:DatatypeProperty ;
  rdfs:label "vmax"@en ;
  rdfs:domain cim:GovCT2 ;
  rdfs:range cim:PU ;
  skos:definition "Maximum valve position limit (<i>Vmax</i>) (&gt; GovCT2.vmin).  Typical value = 1."@en .

cim:GovCT2.vmin a owl:DatatypeProperty ;
  rdfs:label "vmin"@en ;
  rdfs:domain cim:GovCT2 ;
  rdfs:range cim:PU ;
  skos:definition "Minimum valve position limit (<i>Vmin</i>) (&lt; GovCT2.vmax).  Typical value = 0,175."@en .

cim:GovCT2.wfnl a owl:DatatypeProperty ;
  rdfs:label "wfnl"@en ;
  rdfs:domain cim:GovCT2 ;
  rdfs:range cim:PU ;
  skos:definition "No load fuel flow (<i>Wfnl</i>).  Typical value = 0,187."@en .

cim:GovCT2.wfspd a owl:DatatypeProperty ;
  rdfs:label "wfspd"@en ;
  rdfs:domain cim:GovCT2 ;
  rdfs:range xsd:boolean ;
  skos:definition """
Switch for fuel source characteristic to recognize that fuel flow, for a given fuel valve stroke, can be proportional to engine speed (<i>Wfspd</i>).
true = fuel flow proportional to speed (for some gas turbines and diesel engines with positive displacement fuel injectors)
false = fuel control system keeps fuel flow independent of engine speed.
Typical value = false.
\t"""@en .

cim:GovGAST.at a owl:DatatypeProperty ;
  rdfs:label "at"@en ;
  rdfs:domain cim:GovGAST ;
  rdfs:range cim:PU ;
  skos:definition "Ambient temperature load limit (<i>Load Limit</i>).  Typical value = 1."@en .

cim:GovGAST.dturb a owl:DatatypeProperty ;
  rdfs:label "dturb"@en ;
  rdfs:domain cim:GovGAST ;
  rdfs:range cim:PU ;
  skos:definition "Turbine damping factor (<i>Dturb</i>).  Typical value = 0,18."@en .

cim:GovGAST.kt a owl:DatatypeProperty ;
  rdfs:label "kt"@en ;
  rdfs:domain cim:GovGAST ;
  rdfs:range cim:PU ;
  skos:definition "Temperature limiter gain (<i>Kt</i>).  Typical value = 3."@en .

cim:GovGAST.mwbase a owl:DatatypeProperty ;
  rdfs:label "mwbase"@en ;
  rdfs:domain cim:GovGAST ;
  rdfs:range cim:ActivePower ;
  skos:definition "Base for power values (<i>MWbase</i>) (&gt; 0).  Unit = MW."@en .

cim:GovGAST.r a owl:DatatypeProperty ;
  rdfs:label "r"@en ;
  rdfs:domain cim:GovGAST ;
  rdfs:range cim:PU ;
  skos:definition "Permanent droop (<i>R</i>) (&gt;0). Typical value = 0,04."@en .

cim:GovGAST.t1 a owl:DatatypeProperty ;
  rdfs:label "t1"@en ;
  rdfs:domain cim:GovGAST ;
  rdfs:range cim:Seconds ;
  skos:definition "Governor mechanism time constant (<i>T1</i>) (&gt;= 0).  <i>T1</i> represents the natural valve positioning time constant of the governor for small disturbances, as seen when rate limiting is not in effect.  Typical value = 0,5."@en .

cim:GovGAST.t2 a owl:DatatypeProperty ;
  rdfs:label "t2"@en ;
  rdfs:domain cim:GovGAST ;
  rdfs:range cim:Seconds ;
  skos:definition "Turbine power time constant (<i>T2</i>) (&gt;= 0).  <i>T2</i> represents delay due to internal energy storage of the gas turbine engine. <i>T2</i> can be used to give a rough approximation to the delay associated with acceleration of the compressor spool of a multi-shaft engine, or with the compressibility of gas in the plenum of a free power turbine of an aero-derivative unit, for example.  Typical value = 0,5."@en .

cim:GovGAST.t3 a owl:DatatypeProperty ;
  rdfs:label "t3"@en ;
  rdfs:domain cim:GovGAST ;
  rdfs:range cim:Seconds ;
  skos:definition "Turbine exhaust temperature time constant (<i>T3</i>) (&gt;= 0).  Typical value = 3."@en .

cim:GovGAST.vmax a owl:DatatypeProperty ;
  rdfs:label "vmax"@en ;
  rdfs:domain cim:GovGAST ;
  rdfs:range cim:PU ;
  skos:definition "Maximum turbine power, PU of MWbase (<i>Vmax</i>) (&gt; GovGAST.vmin).  Typical value = 1."@en .

cim:GovGAST.vmin a owl:DatatypeProperty ;
  rdfs:label "vmin"@en ;
  rdfs:domain cim:GovGAST ;
  rdfs:range cim:PU ;
  skos:definition "Minimum turbine power, PU of MWbase (<i>Vmin</i>) (&lt; GovGAST.vmax).  Typical value = 0."@en .

cim:GovGAST1.a a owl:DatatypeProperty ;
  rdfs:label "a"@en ;
  rdfs:domain cim:GovGAST1 ;
  rdfs:range xsd:float ;
  skos:definition "Turbine power time constant numerator scale factor (<i>a</i>).  Typical value = 0,8."@en .

cim:GovGAST1.b a owl:DatatypeProperty ;
  rdfs:label "b"@en ;
  rdfs:domain cim:GovGAST1 ;
  rdfs:range xsd:float ;
  skos:definition "Turbine power time constant denominator scale factor (<i>b</i>) (&gt;0).  Typical value = 1."@en .

cim:GovGAST1.db1 a owl:DatatypeProperty ;
  rdfs:label "db1"@en ;
  rdfs:domain cim:GovGAST1 ;
  rdfs:range cim:Frequency ;
  skos:definition "Intentional dead-band width (<i>db1</i>).  Unit = Hz.  Typical value = 0."@en .

cim:GovGAST1.db2 a owl:DatatypeProperty ;
  rdfs:label "db2"@en ;
  rdfs:domain cim:GovGAST1 ;
  rdfs:range cim:ActivePower ;
  skos:definition "Unintentional dead-band (<i>db2</i>).  Unit = MW.  Typical value = 0."@en .

cim:GovGAST1.eps a owl:DatatypeProperty ;
  rdfs:label "eps"@en ;
  rdfs:domain cim:GovGAST1 ;
  rdfs:range cim:Frequency ;
  skos:definition "Intentional db hysteresis (<i>eps</i>).  Unit = Hz.  Typical value = 0."@en .

cim:GovGAST1.fidle a owl:DatatypeProperty ;
  rdfs:label "fidle"@en ;
  rdfs:domain cim:GovGAST1 ;
  rdfs:range cim:PU ;
  skos:definition "Fuel flow at zero power output (<i>Fidle</i>).  Typical value = 0,18."@en .

cim:GovGAST1.gv1 a owl:DatatypeProperty ;
  rdfs:label "gv1"@en ;
  rdfs:domain cim:GovGAST1 ;
  rdfs:range cim:PU ;
  skos:definition "Nonlinear gain point 1, PU gv (<i>Gv1</i>).  Typical value = 0."@en .

cim:GovGAST1.gv2 a owl:DatatypeProperty ;
  rdfs:label "gv2"@en ;
  rdfs:domain cim:GovGAST1 ;
  rdfs:range cim:PU ;
  skos:definition "Nonlinear gain point 2,PU gv (<i>Gv2</i>).  Typical value = 0."@en .

cim:GovGAST1.gv3 a owl:DatatypeProperty ;
  rdfs:label "gv3"@en ;
  rdfs:domain cim:GovGAST1 ;
  rdfs:range cim:PU ;
  skos:definition "Nonlinear gain point 3, PU gv (<i>Gv3</i>).  Typical value = 0."@en .

cim:GovGAST1.gv4 a owl:DatatypeProperty ;
  rdfs:label "gv4"@en ;
  rdfs:domain cim:GovGAST1 ;
  rdfs:range cim:PU ;
  skos:definition "Nonlinear gain point 4, PU gv (<i>Gv4</i>).  Typical value = 0."@en .

cim:GovGAST1.gv5 a owl:DatatypeProperty ;
  rdfs:label "gv5"@en ;
  rdfs:domain cim:GovGAST1 ;
  rdfs:range cim:PU ;
  skos:definition "Nonlinear gain point 5, PU gv (<i>Gv5</i>).  Typical value = 0."@en .

cim:GovGAST1.gv6 a owl:DatatypeProperty ;
  rdfs:label "gv6"@en ;
  rdfs:domain cim:GovGAST1 ;
  rdfs:range cim:PU ;
  skos:definition "Nonlinear gain point 6, PU gv (<i>Gv6</i>).  Typical value = 0."@en .

cim:GovGAST1.ka a owl:DatatypeProperty ;
  rdfs:label "ka"@en ;
  rdfs:domain cim:GovGAST1 ;
  rdfs:range cim:PU ;
  skos:definition "Governor gain (<i>Ka</i>).  Typical value = 0."@en .

cim:GovGAST1.kt a owl:DatatypeProperty ;
  rdfs:label "kt"@en ;
  rdfs:domain cim:GovGAST1 ;
  rdfs:range cim:PU ;
  skos:definition "Temperature limiter gain (<i>Kt</i>).  Typical value = 3."@en .

cim:GovGAST1.lmax a owl:DatatypeProperty ;
  rdfs:label "lmax"@en ;
  rdfs:domain cim:GovGAST1 ;
  rdfs:range cim:PU ;
  skos:definition "Ambient temperature load limit (<i>Lmax</i>).  <i>Lmax</i> is the turbine power output corresponding to the limiting exhaust gas temperature.  Typical value = 1."@en .

cim:GovGAST1.loadinc a owl:DatatypeProperty ;
  rdfs:label "loadinc"@en ;
  rdfs:domain cim:GovGAST1 ;
  rdfs:range cim:PU ;
  skos:definition "Valve position change allowed at fast rate (<i>Loadinc</i>).  Typical value = 0,05."@en .

cim:GovGAST1.ltrate a owl:DatatypeProperty ;
  rdfs:label "ltrate"@en ;
  rdfs:domain cim:GovGAST1 ;
  rdfs:range xsd:float ;
  skos:definition "Maximum long term fuel valve opening rate (<i>Ltrate</i>).  Typical value = 0,02."@en .

cim:GovGAST1.mwbase a owl:DatatypeProperty ;
  rdfs:label "mwbase"@en ;
  rdfs:domain cim:GovGAST1 ;
  rdfs:range cim:ActivePower ;
  skos:definition "Base for power values (<i>MWbase</i>) (&gt; 0).  Unit = MW."@en .

cim:GovGAST1.pgv1 a owl:DatatypeProperty ;
  rdfs:label "pgv1"@en ;
  rdfs:domain cim:GovGAST1 ;
  rdfs:range cim:PU ;
  skos:definition "Nonlinear gain point 1, PU power (<i>Pgv1</i>).  Typical value = 0."@en .

cim:GovGAST1.pgv2 a owl:DatatypeProperty ;
  rdfs:label "pgv2"@en ;
  rdfs:domain cim:GovGAST1 ;
  rdfs:range cim:PU ;
  skos:definition "Nonlinear gain point 2, PU power (<i>Pgv2</i>).  Typical value = 0."@en .

cim:GovGAST1.pgv3 a owl:DatatypeProperty ;
  rdfs:label "pgv3"@en ;
  rdfs:domain cim:GovGAST1 ;
  rdfs:range cim:PU ;
  skos:definition "Nonlinear gain point 3, PU power (<i>Pgv3</i>).  Typical value = 0."@en .

cim:GovGAST1.pgv4 a owl:DatatypeProperty ;
  rdfs:label "pgv4"@en ;
  rdfs:domain cim:GovGAST1 ;
  rdfs:range cim:PU ;
  skos:definition "Nonlinear gain point 4, PU power (<i>Pgv4</i>).  Typical value = 0."@en .

cim:GovGAST1.pgv5 a owl:DatatypeProperty ;
  rdfs:label "pgv5"@en ;
  rdfs:domain cim:GovGAST1 ;
  rdfs:range cim:PU ;
  skos:definition "Nonlinear gain point 5, PU power (<i>Pgv5</i>).  Typical value = 0."@en .

cim:GovGAST1.pgv6 a owl:DatatypeProperty ;
  rdfs:label "pgv6"@en ;
  rdfs:domain cim:GovGAST1 ;
  rdfs:range cim:PU ;
  skos:definition "Nonlinear gain point 6, PU power (<i>Pgv6</i>).  Typical value = 0."@en .

cim:GovGAST1.r a owl:DatatypeProperty ;
  rdfs:label "r"@en ;
  rdfs:domain cim:GovGAST1 ;
  rdfs:range cim:PU ;
  skos:definition "Permanent droop (<i>R</i>) (&gt;0).  Typical value = 0,04."@en .

cim:GovGAST1.rmax a owl:DatatypeProperty ;
  rdfs:label "rmax"@en ;
  rdfs:domain cim:GovGAST1 ;
  rdfs:range xsd:float ;
  skos:definition "Maximum fuel valve opening rate (<i>Rmax</i>).  Unit = PU / s.  Typical value = 1."@en .

cim:GovGAST1.t1 a owl:DatatypeProperty ;
  rdfs:label "t1"@en ;
  rdfs:domain cim:GovGAST1 ;
  rdfs:range cim:Seconds ;
  skos:definition "Governor mechanism time constant (<i>T1</i>) (&gt;= 0).  <i>T1</i> represents the natural valve positioning time constant of the governor for small disturbances, as seen when rate limiting is not in effect.  Typical value = 0,5."@en .

cim:GovGAST1.t2 a owl:DatatypeProperty ;
  rdfs:label "t2"@en ;
  rdfs:domain cim:GovGAST1 ;
  rdfs:range cim:Seconds ;
  skos:definition "Turbine power time constant (<i>T2</i>) (&gt;= 0). <i>T2</i> represents delay due to internal energy storage of the gas turbine engine. <i>T2</i> can be used to give a rough approximation to the delay associated with acceleration of the compressor spool of a multi-shaft engine, or with the compressibility of gas in the plenum of the free power turbine of an aero-derivative unit, for example.  Typical value = 0,5."@en .

cim:GovGAST1.t3 a owl:DatatypeProperty ;
  rdfs:label "t3"@en ;
  rdfs:domain cim:GovGAST1 ;
  rdfs:range cim:Seconds ;
  skos:definition "Turbine exhaust temperature time constant (<i>T3</i>) (&gt;= 0).  <i>T3</i> represents delay in the exhaust temperature and load limiting system. Typical value = 3."@en .

cim:GovGAST1.t4 a owl:DatatypeProperty ;
  rdfs:label "t4"@en ;
  rdfs:domain cim:GovGAST1 ;
  rdfs:range cim:Seconds ;
  skos:definition "Governor lead time constant (<i>T4</i>) (&gt;= 0).  Typical value = 0."@en .

cim:GovGAST1.t5 a owl:DatatypeProperty ;
  rdfs:label "t5"@en ;
  rdfs:domain cim:GovGAST1 ;
  rdfs:range cim:Seconds ;
  skos:definition "Governor lag time constant (<i>T5</i>) (&gt;= 0).  If = 0, entire gain and lead-lag block is bypassed.  Typical value = 0."@en .

cim:GovGAST1.tltr a owl:DatatypeProperty ;
  rdfs:label "tltr"@en ;
  rdfs:domain cim:GovGAST1 ;
  rdfs:range cim:Seconds ;
  skos:definition "Valve position averaging time constant (<i>Tltr</i>) (&gt;= 0).  Typical value = 10."@en .

cim:GovGAST1.vmax a owl:DatatypeProperty ;
  rdfs:label "vmax"@en ;
  rdfs:domain cim:GovGAST1 ;
  rdfs:range cim:PU ;
  skos:definition "Maximum turbine power, PU of MWbase (<i>Vmax</i>) (&gt; GovGAST1.vmin).  Typical value = 1."@en .

cim:GovGAST1.vmin a owl:DatatypeProperty ;
  rdfs:label "vmin"@en ;
  rdfs:domain cim:GovGAST1 ;
  rdfs:range cim:PU ;
  skos:definition "Minimum turbine power, PU of MWbase (<i>Vmin</i>) (&lt; GovGAST1.vmax).  Typical value = 0."@en .

cim:GovGAST2.a a owl:DatatypeProperty ;
  rdfs:label "a"@en ;
  rdfs:domain cim:GovGAST2 ;
  rdfs:range xsd:float ;
  skos:definition "Valve positioner (<i>A</i>)."@en .

cim:GovGAST2.af1 a owl:DatatypeProperty ;
  rdfs:label "af1"@en ;
  rdfs:domain cim:GovGAST2 ;
  rdfs:range cim:PU ;
  skos:definition "Exhaust temperature parameter (<i>Af1</i>).  Unit = PU temperature.  Based on temperature in degrees C."@en .

cim:GovGAST2.af2 a owl:DatatypeProperty ;
  rdfs:label "af2"@en ;
  rdfs:domain cim:GovGAST2 ;
  rdfs:range cim:PU ;
  skos:definition "Coefficient equal to 0,5(1-speed) (<i>Af2</i>)."@en .

cim:GovGAST2.b a owl:DatatypeProperty ;
  rdfs:label "b"@en ;
  rdfs:domain cim:GovGAST2 ;
  rdfs:range xsd:float ;
  skos:definition "Valve positioner (<i>B</i>). "@en .

cim:GovGAST2.bf1 a owl:DatatypeProperty ;
  rdfs:label "bf1"@en ;
  rdfs:domain cim:GovGAST2 ;
  rdfs:range cim:PU ;
  skos:definition "(<i>Bf1</i>).  <i>Bf1</i> = <i>E</i>(1 - <i>W</i>) where <i>E</i> (speed sensitivity coefficient) is 0,55 to 0,65 x <i>Tr</i>.  Unit = PU temperature.  Based on temperature in degrees C."@en .

cim:GovGAST2.bf2 a owl:DatatypeProperty ;
  rdfs:label "bf2"@en ;
  rdfs:domain cim:GovGAST2 ;
  rdfs:range cim:PU ;
  skos:definition "Turbine torque coefficient K<sub>hhv</sub> (depends on heating value of fuel stream in combustion chamber) (<i>Bf2</i>)."@en .

cim:GovGAST2.c a owl:DatatypeProperty ;
  rdfs:label "c"@en ;
  rdfs:domain cim:GovGAST2 ;
  rdfs:range xsd:float ;
  skos:definition "Valve positioner (<i>C</i>). "@en .

cim:GovGAST2.cf2 a owl:DatatypeProperty ;
  rdfs:label "cf2"@en ;
  rdfs:domain cim:GovGAST2 ;
  rdfs:range cim:PU ;
  skos:definition "Coefficient defining fuel flow where power output is 0% (<i>Cf2</i>).  Synchronous but no output.  Typically 0,23 x K<sub>hhv</sub> (23% fuel flow)."@en .

cim:GovGAST2.ecr a owl:DatatypeProperty ;
  rdfs:label "ecr"@en ;
  rdfs:domain cim:GovGAST2 ;
  rdfs:range cim:Seconds ;
  skos:definition "Combustion reaction time delay (<i>Ecr</i>) (&gt;= 0)."@en .

cim:GovGAST2.etd a owl:DatatypeProperty ;
  rdfs:label "etd"@en ;
  rdfs:domain cim:GovGAST2 ;
  rdfs:range cim:Seconds ;
  skos:definition "Turbine and exhaust delay (<i>Etd</i>) (&gt;= 0)."@en .

cim:GovGAST2.k3 a owl:DatatypeProperty ;
  rdfs:label "k3"@en ;
  rdfs:domain cim:GovGAST2 ;
  rdfs:range cim:PU ;
  skos:definition "Ratio of fuel adjustment (<i>K3</i>)."@en .

cim:GovGAST2.k4 a owl:DatatypeProperty ;
  rdfs:label "k4"@en ;
  rdfs:domain cim:GovGAST2 ;
  rdfs:range cim:PU ;
  skos:definition "Gain of radiation shield (<i>K4</i>)."@en .

cim:GovGAST2.k5 a owl:DatatypeProperty ;
  rdfs:label "k5"@en ;
  rdfs:domain cim:GovGAST2 ;
  rdfs:range cim:PU ;
  skos:definition "Gain of radiation shield (<i>K5</i>)."@en .

cim:GovGAST2.k6 a owl:DatatypeProperty ;
  rdfs:label "k6"@en ;
  rdfs:domain cim:GovGAST2 ;
  rdfs:range cim:PU ;
  skos:definition "Minimum fuel flow (<i>K6</i>). "@en .

cim:GovGAST2.kf a owl:DatatypeProperty ;
  rdfs:label "kf"@en ;
  rdfs:domain cim:GovGAST2 ;
  rdfs:range cim:PU ;
  skos:definition "Fuel system feedback (<i>Kf</i>)."@en .

cim:GovGAST2.mwbase a owl:DatatypeProperty ;
  rdfs:label "mwbase"@en ;
  rdfs:domain cim:GovGAST2 ;
  rdfs:range cim:ActivePower ;
  skos:definition "Base for power values (<i>MWbase</i>) (&gt; 0).  Unit = MW."@en .

cim:GovGAST2.t a owl:DatatypeProperty ;
  rdfs:label "t"@en ;
  rdfs:domain cim:GovGAST2 ;
  rdfs:range cim:Seconds ;
  skos:definition "Fuel control time constant (<i>T</i>) (&gt;= 0)."@en .

cim:GovGAST2.t3 a owl:DatatypeProperty ;
  rdfs:label "t3"@en ;
  rdfs:domain cim:GovGAST2 ;
  rdfs:range cim:Seconds ;
  skos:definition "Radiation shield time constant (<i>T3</i>) (&gt;= 0)."@en .

cim:GovGAST2.t4 a owl:DatatypeProperty ;
  rdfs:label "t4"@en ;
  rdfs:domain cim:GovGAST2 ;
  rdfs:range cim:Seconds ;
  skos:definition "Thermocouple time constant (<i>T4</i>) (&gt;= 0)."@en .

cim:GovGAST2.t5 a owl:DatatypeProperty ;
  rdfs:label "t5"@en ;
  rdfs:domain cim:GovGAST2 ;
  rdfs:range cim:Seconds ;
  skos:definition "Temperature control time constant (<i>T5</i>) (&gt;= 0)."@en .

cim:GovGAST2.tc a owl:DatatypeProperty ;
  rdfs:label "tc"@en ;
  rdfs:domain cim:GovGAST2 ;
  rdfs:range cim:Temperature ;
  skos:definition "Temperature control (<i>Tc</i>).  Unit = °F or °C depending on parameters <i>Af1</i> and <i>Bf1</i>. "@en .

cim:GovGAST2.tcd a owl:DatatypeProperty ;
  rdfs:label "tcd"@en ;
  rdfs:domain cim:GovGAST2 ;
  rdfs:range cim:Seconds ;
  skos:definition "Compressor discharge time constant (<i>Tcd</i>) (&gt;= 0)."@en .

cim:GovGAST2.tf a owl:DatatypeProperty ;
  rdfs:label "tf"@en ;
  rdfs:domain cim:GovGAST2 ;
  rdfs:range cim:Seconds ;
  skos:definition "Fuel system time constant (<i>Tf</i>) (&gt;= 0)."@en .

cim:GovGAST2.tmax a owl:DatatypeProperty ;
  rdfs:label "tmax"@en ;
  rdfs:domain cim:GovGAST2 ;
  rdfs:range cim:PU ;
  skos:definition "Maximum turbine limit (<i>Tmax</i>) (&gt; GovGAST2.tmin)."@en .

cim:GovGAST2.tmin a owl:DatatypeProperty ;
  rdfs:label "tmin"@en ;
  rdfs:domain cim:GovGAST2 ;
  rdfs:range cim:PU ;
  skos:definition "Minimum turbine limit (<i>Tmin</i>) (&lt; GovGAST2.tmax)."@en .

cim:GovGAST2.tr a owl:DatatypeProperty ;
  rdfs:label "tr"@en ;
  rdfs:domain cim:GovGAST2 ;
  rdfs:range cim:Temperature ;
  skos:definition "Rated temperature (<i>Tr</i>).  Unit = °C depending on parameters<i> Af1 </i>and <i>Bf1</i>."@en .

cim:GovGAST2.trate a owl:DatatypeProperty ;
  rdfs:label "trate"@en ;
  rdfs:domain cim:GovGAST2 ;
  rdfs:range cim:ActivePower ;
  skos:definition "Turbine rating (<i>Trate</i>).  Unit = MW."@en .

cim:GovGAST2.tt a owl:DatatypeProperty ;
  rdfs:label "tt"@en ;
  rdfs:domain cim:GovGAST2 ;
  rdfs:range cim:Seconds ;
  skos:definition "Temperature controller integration rate (<i>Tt</i>) (&gt;= 0)."@en .

cim:GovGAST2.w a owl:DatatypeProperty ;
  rdfs:label "w"@en ;
  rdfs:domain cim:GovGAST2 ;
  rdfs:range cim:PU ;
  skos:definition "Governor gain (1/droop) on turbine rating (<i>W</i>)."@en .

cim:GovGAST2.x a owl:DatatypeProperty ;
  rdfs:label "x"@en ;
  rdfs:domain cim:GovGAST2 ;
  rdfs:range cim:Seconds ;
  skos:definition "Governor lead time constant (<i>X</i>) (&gt;= 0)."@en .

cim:GovGAST2.y a owl:DatatypeProperty ;
  rdfs:label "y"@en ;
  rdfs:domain cim:GovGAST2 ;
  rdfs:range cim:Seconds ;
  skos:definition "Governor lag time constant (<i>Y</i>) (&gt; 0)."@en .

cim:GovGAST2.z a owl:DatatypeProperty ;
  rdfs:label "z"@en ;
  rdfs:domain cim:GovGAST2 ;
  rdfs:range xsd:integer ;
  skos:definition """
Governor mode (<i>Z</i>).
1 = droop
0 = isochronous.
\t"""@en .

cim:GovGAST3.bca a owl:DatatypeProperty ;
  rdfs:label "bca"@en ;
  rdfs:domain cim:GovGAST3 ;
  rdfs:range xsd:float ;
  skos:definition "Acceleration limit set-point (<i>Bca</i>).  Unit = 1/s.  Typical value = 0,01."@en .

cim:GovGAST3.bp a owl:DatatypeProperty ;
  rdfs:label "bp"@en ;
  rdfs:domain cim:GovGAST3 ;
  rdfs:range cim:PU ;
  skos:definition "Droop (<i>bp</i>).  Typical value = 0,05."@en .

cim:GovGAST3.dtc a owl:DatatypeProperty ;
  rdfs:label "dtc"@en ;
  rdfs:domain cim:GovGAST3 ;
  rdfs:range cim:Temperature ;
  skos:definition "Exhaust temperature variation due to fuel flow increasing from 0 to 1 PU (<i>deltaTc</i>).  Typical value = 390."@en .

cim:GovGAST3.ka a owl:DatatypeProperty ;
  rdfs:label "ka"@en ;
  rdfs:domain cim:GovGAST3 ;
  rdfs:range cim:PU ;
  skos:definition "Minimum fuel flow (<i>Ka</i>).  Typical value = 0,23."@en .

cim:GovGAST3.kac a owl:DatatypeProperty ;
  rdfs:label "kac"@en ;
  rdfs:domain cim:GovGAST3 ;
  rdfs:range xsd:float ;
  skos:definition "Fuel system feedback (<i>K</i><i><sub>AC</sub></i>).  Typical value = 0."@en .

cim:GovGAST3.kca a owl:DatatypeProperty ;
  rdfs:label "kca"@en ;
  rdfs:domain cim:GovGAST3 ;
  rdfs:range xsd:float ;
  skos:definition "Acceleration control integral gain (<i>Kca</i>). Unit = 1/s.  Typical value = 100."@en .

cim:GovGAST3.ksi a owl:DatatypeProperty ;
  rdfs:label "ksi"@en ;
  rdfs:domain cim:GovGAST3 ;
  rdfs:range xsd:float ;
  skos:definition "Gain of radiation shield (<i>Ksi</i>).  Typical value = 0,8."@en .

cim:GovGAST3.ky a owl:DatatypeProperty ;
  rdfs:label "ky"@en ;
  rdfs:domain cim:GovGAST3 ;
  rdfs:range xsd:float ;
  skos:definition "Coefficient of transfer function of fuel valve positioner (<i>Ky</i>).  Typical value = 1."@en .

cim:GovGAST3.mnef a owl:DatatypeProperty ;
  rdfs:label "mnef"@en ;
  rdfs:domain cim:GovGAST3 ;
  rdfs:range cim:PU ;
  skos:definition "Fuel flow maximum negative error value (<i>MNef</i>).  Typical value = -0,05."@en .

cim:GovGAST3.mxef a owl:DatatypeProperty ;
  rdfs:label "mxef"@en ;
  rdfs:domain cim:GovGAST3 ;
  rdfs:range cim:PU ;
  skos:definition "Fuel flow maximum positive error value (<i>MXef</i>).  Typical value = 0,05."@en .

cim:GovGAST3.rcmn a owl:DatatypeProperty ;
  rdfs:label "rcmn"@en ;
  rdfs:domain cim:GovGAST3 ;
  rdfs:range cim:PU ;
  skos:definition "Minimum fuel flow (<i>RCMN</i>).  Typical value = -0,1."@en .

cim:GovGAST3.rcmx a owl:DatatypeProperty ;
  rdfs:label "rcmx"@en ;
  rdfs:domain cim:GovGAST3 ;
  rdfs:range cim:PU ;
  skos:definition "Maximum fuel flow (<i>RCMX</i>).  Typical value = 1."@en .

cim:GovGAST3.tac a owl:DatatypeProperty ;
  rdfs:label "tac"@en ;
  rdfs:domain cim:GovGAST3 ;
  rdfs:range cim:Seconds ;
  skos:definition "Fuel control time constant (<i>Tac</i>) (&gt;= 0).  Typical value = 0,1."@en .

cim:GovGAST3.tc a owl:DatatypeProperty ;
  rdfs:label "tc"@en ;
  rdfs:domain cim:GovGAST3 ;
  rdfs:range cim:Seconds ;
  skos:definition "Compressor discharge volume time constant (<i>Tc</i>) (&gt;= 0).  Typical value = 0,2."@en .

cim:GovGAST3.td a owl:DatatypeProperty ;
  rdfs:label "td"@en ;
  rdfs:domain cim:GovGAST3 ;
  rdfs:range cim:Seconds ;
  skos:definition "Temperature controller derivative gain (<i>Td</i>) (&gt;= 0).  Typical value = 3,3."@en .

cim:GovGAST3.tfen a owl:DatatypeProperty ;
  rdfs:label "tfen"@en ;
  rdfs:domain cim:GovGAST3 ;
  rdfs:range cim:Temperature ;
  skos:definition "Turbine rated exhaust temperature correspondent to Pm=1 PU (<i>Tfen</i>).  Typical value = 540."@en .

cim:GovGAST3.tg a owl:DatatypeProperty ;
  rdfs:label "tg"@en ;
  rdfs:domain cim:GovGAST3 ;
  rdfs:range cim:Seconds ;
  skos:definition "Time constant of speed governor (<i>Tg</i>) (&gt;= 0).  Typical value = 0,05."@en .

cim:GovGAST3.tsi a owl:DatatypeProperty ;
  rdfs:label "tsi"@en ;
  rdfs:domain cim:GovGAST3 ;
  rdfs:range cim:Seconds ;
  skos:definition "Time constant of radiation shield (<i>Tsi</i>) (&gt;= 0).  Typical value = 15."@en .

cim:GovGAST3.tt a owl:DatatypeProperty ;
  rdfs:label "tt"@en ;
  rdfs:domain cim:GovGAST3 ;
  rdfs:range cim:Temperature ;
  skos:definition "Temperature controller integration rate (<i>Tt</i>).  Typical value = 250."@en .

cim:GovGAST3.ttc a owl:DatatypeProperty ;
  rdfs:label "ttc"@en ;
  rdfs:domain cim:GovGAST3 ;
  rdfs:range cim:Seconds ;
  skos:definition "Time constant of thermocouple (<i>Ttc</i>) (&gt;= 0).  Typical value = 2,5."@en .

cim:GovGAST3.ty a owl:DatatypeProperty ;
  rdfs:label "ty"@en ;
  rdfs:domain cim:GovGAST3 ;
  rdfs:range cim:Seconds ;
  skos:definition "Time constant of fuel valve positioner (<i>Ty</i>) (&gt;= 0).  Typical value = 0,2."@en .

cim:GovGAST4.bp a owl:DatatypeProperty ;
  rdfs:label "bp"@en ;
  rdfs:domain cim:GovGAST4 ;
  rdfs:range cim:PU ;
  skos:definition "Droop (<i>b</i><i><sub>p</sub></i>).  Typical value = 0,05."@en .

cim:GovGAST4.ktm a owl:DatatypeProperty ;
  rdfs:label "ktm"@en ;
  rdfs:domain cim:GovGAST4 ;
  rdfs:range cim:PU ;
  skos:definition "Compressor gain (<i>Ktm</i>).  Typical value = 0."@en .

cim:GovGAST4.mnef a owl:DatatypeProperty ;
  rdfs:label "mnef"@en ;
  rdfs:domain cim:GovGAST4 ;
  rdfs:range cim:PU ;
  skos:definition "Fuel flow maximum negative error value (<i>MNef</i>).  Typical value = -0,05."@en .

cim:GovGAST4.mxef a owl:DatatypeProperty ;
  rdfs:label "mxef"@en ;
  rdfs:domain cim:GovGAST4 ;
  rdfs:range cim:PU ;
  skos:definition "Fuel flow maximum positive error value (<i>MXef</i>).  Typical value = 0,05."@en .

cim:GovGAST4.rymn a owl:DatatypeProperty ;
  rdfs:label "rymn"@en ;
  rdfs:domain cim:GovGAST4 ;
  rdfs:range cim:PU ;
  skos:definition "Minimum valve opening (<i>RYMN</i>).  Typical value = 0."@en .

cim:GovGAST4.rymx a owl:DatatypeProperty ;
  rdfs:label "rymx"@en ;
  rdfs:domain cim:GovGAST4 ;
  rdfs:range cim:PU ;
  skos:definition "Maximum valve opening (<i>RYMX</i>).  Typical value = 1,1."@en .

cim:GovGAST4.ta a owl:DatatypeProperty ;
  rdfs:label "ta"@en ;
  rdfs:domain cim:GovGAST4 ;
  rdfs:range cim:Seconds ;
  skos:definition "Maximum gate opening velocity (<i>TA</i>) (&gt;= 0).  Typical value = 3."@en .

cim:GovGAST4.tc a owl:DatatypeProperty ;
  rdfs:label "tc"@en ;
  rdfs:domain cim:GovGAST4 ;
  rdfs:range cim:Seconds ;
  skos:definition "Maximum gate closing velocity (<i>TC</i>) (&gt;= 0).  Typical value = 0,5."@en .

cim:GovGAST4.tcm a owl:DatatypeProperty ;
  rdfs:label "tcm"@en ;
  rdfs:domain cim:GovGAST4 ;
  rdfs:range cim:Seconds ;
  skos:definition "Fuel control time constant (<i>Tcm</i>) (&gt;= 0).  Typical value = 0,1."@en .

cim:GovGAST4.tm a owl:DatatypeProperty ;
  rdfs:label "tm"@en ;
  rdfs:domain cim:GovGAST4 ;
  rdfs:range cim:Seconds ;
  skos:definition "Compressor discharge volume time constant (<i>Tm</i>) (&gt;= 0).  Typical value = 0,2."@en .

cim:GovGAST4.ty a owl:DatatypeProperty ;
  rdfs:label "ty"@en ;
  rdfs:domain cim:GovGAST4 ;
  rdfs:range cim:Seconds ;
  skos:definition "Time constant of fuel valve positioner (<i>Ty</i>) (&gt;= 0).  Typical value = 0,1."@en .

cim:GovGASTWD.a a owl:DatatypeProperty ;
  rdfs:label "a"@en ;
  rdfs:domain cim:GovGASTWD ;
  rdfs:range xsd:float ;
  skos:definition "Valve positioner (<i>A</i>)."@en .

cim:GovGASTWD.af1 a owl:DatatypeProperty ;
  rdfs:label "af1"@en ;
  rdfs:domain cim:GovGASTWD ;
  rdfs:range cim:PU ;
  skos:definition "Exhaust temperature parameter (<i>Af1</i>)."@en .

cim:GovGASTWD.af2 a owl:DatatypeProperty ;
  rdfs:label "af2"@en ;
  rdfs:domain cim:GovGASTWD ;
  rdfs:range cim:PU ;
  skos:definition "Coefficient equal to 0,5(1-speed) (<i>Af2</i>)."@en .

cim:GovGASTWD.b a owl:DatatypeProperty ;
  rdfs:label "b"@en ;
  rdfs:domain cim:GovGASTWD ;
  rdfs:range xsd:float ;
  skos:definition "Valve positioner (<i>B</i>). "@en .

cim:GovGASTWD.bf1 a owl:DatatypeProperty ;
  rdfs:label "bf1"@en ;
  rdfs:domain cim:GovGASTWD ;
  rdfs:range cim:PU ;
  skos:definition "(<i>Bf1</i>).  <i>Bf1</i> = <i>E</i>(1-<i>w</i>) where <i>E</i> (speed sensitivity coefficient) is 0,55 to 0,65 x <i>Tr</i>."@en .

cim:GovGASTWD.bf2 a owl:DatatypeProperty ;
  rdfs:label "bf2"@en ;
  rdfs:domain cim:GovGASTWD ;
  rdfs:range cim:PU ;
  skos:definition "Turbine torque coefficient K<sub>hhv</sub> (depends on heating value of fuel stream in combustion chamber) (<i>Bf2</i>)."@en .

cim:GovGASTWD.c a owl:DatatypeProperty ;
  rdfs:label "c"@en ;
  rdfs:domain cim:GovGASTWD ;
  rdfs:range xsd:float ;
  skos:definition "Valve positioner (<i>C</i>). "@en .

cim:GovGASTWD.cf2 a owl:DatatypeProperty ;
  rdfs:label "cf2"@en ;
  rdfs:domain cim:GovGASTWD ;
  rdfs:range cim:PU ;
  skos:definition "Coefficient defining fuel flow where power output is 0 % (<i>Cf2</i>).  Synchronous but no output.  Typically 0,23 x K<sub>hhv </sub>(23 % fuel flow)."@en .

cim:GovGASTWD.ecr a owl:DatatypeProperty ;
  rdfs:label "ecr"@en ;
  rdfs:domain cim:GovGASTWD ;
  rdfs:range cim:Seconds ;
  skos:definition "Combustion reaction time delay (<i>Ecr</i>) (&gt;= 0)."@en .

cim:GovGASTWD.etd a owl:DatatypeProperty ;
  rdfs:label "etd"@en ;
  rdfs:domain cim:GovGASTWD ;
  rdfs:range cim:Seconds ;
  skos:definition "Turbine and exhaust delay (<i>Etd</i>) (&gt;= 0)."@en .

cim:GovGASTWD.k3 a owl:DatatypeProperty ;
  rdfs:label "k3"@en ;
  rdfs:domain cim:GovGASTWD ;
  rdfs:range cim:PU ;
  skos:definition "Ratio of fuel adjustment (<i>K3</i>)."@en .

cim:GovGASTWD.k4 a owl:DatatypeProperty ;
  rdfs:label "k4"@en ;
  rdfs:domain cim:GovGASTWD ;
  rdfs:range cim:PU ;
  skos:definition "Gain of radiation shield (<i>K4</i>)."@en .

cim:GovGASTWD.k5 a owl:DatatypeProperty ;
  rdfs:label "k5"@en ;
  rdfs:domain cim:GovGASTWD ;
  rdfs:range cim:PU ;
  skos:definition "Gain of radiation shield (<i>K5</i>)."@en .

cim:GovGASTWD.k6 a owl:DatatypeProperty ;
  rdfs:label "k6"@en ;
  rdfs:domain cim:GovGASTWD ;
  rdfs:range cim:PU ;
  skos:definition "Minimum fuel flow (<i>K6</i>). "@en .

cim:GovGASTWD.kd a owl:DatatypeProperty ;
  rdfs:label "kd"@en ;
  rdfs:domain cim:GovGASTWD ;
  rdfs:range cim:PU ;
  skos:definition "Drop governor gain (<i>Kd</i>)."@en .

cim:GovGASTWD.kdroop a owl:DatatypeProperty ;
  rdfs:label "kdroop"@en ;
  rdfs:domain cim:GovGASTWD ;
  rdfs:range cim:PU ;
  skos:definition "(<i>Kdroop</i>) (&gt;= 0)."@en .

cim:GovGASTWD.kf a owl:DatatypeProperty ;
  rdfs:label "kf"@en ;
  rdfs:domain cim:GovGASTWD ;
  rdfs:range cim:PU ;
  skos:definition "Fuel system feedback (<i>Kf</i>)."@en .

cim:GovGASTWD.ki a owl:DatatypeProperty ;
  rdfs:label "ki"@en ;
  rdfs:domain cim:GovGASTWD ;
  rdfs:range cim:PU ;
  skos:definition "Isochronous Governor Gain (<i>Ki</i>)."@en .

cim:GovGASTWD.kp a owl:DatatypeProperty ;
  rdfs:label "kp"@en ;
  rdfs:domain cim:GovGASTWD ;
  rdfs:range cim:PU ;
  skos:definition "PID proportional gain (<i>Kp</i>)."@en .

cim:GovGASTWD.mwbase a owl:DatatypeProperty ;
  rdfs:label "mwbase"@en ;
  rdfs:domain cim:GovGASTWD ;
  rdfs:range cim:ActivePower ;
  skos:definition "Base for power values (<i>MWbase</i>) (&gt; 0).  Unit = MW."@en .

cim:GovGASTWD.t a owl:DatatypeProperty ;
  rdfs:label "t"@en ;
  rdfs:domain cim:GovGASTWD ;
  rdfs:range cim:Seconds ;
  skos:definition "Fuel control time constant (<i>T</i>) (&gt;= 0)."@en .

cim:GovGASTWD.t3 a owl:DatatypeProperty ;
  rdfs:label "t3"@en ;
  rdfs:domain cim:GovGASTWD ;
  rdfs:range cim:Seconds ;
  skos:definition "Radiation shield time constant (<i>T3</i>) (&gt;= 0)."@en .

cim:GovGASTWD.t4 a owl:DatatypeProperty ;
  rdfs:label "t4"@en ;
  rdfs:domain cim:GovGASTWD ;
  rdfs:range cim:Seconds ;
  skos:definition "Thermocouple time constant (<i>T4</i>) (&gt;= 0)."@en .

cim:GovGASTWD.t5 a owl:DatatypeProperty ;
  rdfs:label "t5"@en ;
  rdfs:domain cim:GovGASTWD ;
  rdfs:range cim:Seconds ;
  skos:definition "Temperature control time constant (<i>T5</i>) (&gt;= 0)."@en .

cim:GovGASTWD.tc a owl:DatatypeProperty ;
  rdfs:label "tc"@en ;
  rdfs:domain cim:GovGASTWD ;
  rdfs:range cim:Temperature ;
  skos:definition "Temperature control (<i>Tc</i>)."@en .

cim:GovGASTWD.tcd a owl:DatatypeProperty ;
  rdfs:label "tcd"@en ;
  rdfs:domain cim:GovGASTWD ;
  rdfs:range cim:Seconds ;
  skos:definition "Compressor discharge time constant (<i>Tcd</i>) (&gt;= 0)."@en .

cim:GovGASTWD.td a owl:DatatypeProperty ;
  rdfs:label "td"@en ;
  rdfs:domain cim:GovGASTWD ;
  rdfs:range cim:Seconds ;
  skos:definition "Power transducer time constant (<i>Td</i>) (&gt;= 0)."@en .

cim:GovGASTWD.tf a owl:DatatypeProperty ;
  rdfs:label "tf"@en ;
  rdfs:domain cim:GovGASTWD ;
  rdfs:range cim:Seconds ;
  skos:definition "Fuel system time constant (<i>Tf</i>) (&gt;= 0)."@en .

cim:GovGASTWD.tmax a owl:DatatypeProperty ;
  rdfs:label "tmax"@en ;
  rdfs:domain cim:GovGASTWD ;
  rdfs:range cim:PU ;
  skos:definition "Maximum Turbine limit (<i>Tmax</i>) (&gt; GovGASTWD.tmin)."@en .

cim:GovGASTWD.tmin a owl:DatatypeProperty ;
  rdfs:label "tmin"@en ;
  rdfs:domain cim:GovGASTWD ;
  rdfs:range cim:PU ;
  skos:definition "Minimum turbine limit (<i>Tmin</i>) (&lt; GovGASTWD.tmax)."@en .

cim:GovGASTWD.tr a owl:DatatypeProperty ;
  rdfs:label "tr"@en ;
  rdfs:domain cim:GovGASTWD ;
  rdfs:range cim:Temperature ;
  skos:definition "Rated temperature (<i>Tr</i>)."@en .

cim:GovGASTWD.trate a owl:DatatypeProperty ;
  rdfs:label "trate"@en ;
  rdfs:domain cim:GovGASTWD ;
  rdfs:range cim:ActivePower ;
  skos:definition "Turbine rating (<i>Trate</i>).  Unit = MW."@en .

cim:GovGASTWD.tt a owl:DatatypeProperty ;
  rdfs:label "tt"@en ;
  rdfs:domain cim:GovGASTWD ;
  rdfs:range cim:Seconds ;
  skos:definition "Temperature controller integration rate (<i>Tt</i>) (&gt;= 0)."@en .

cim:GovHydro1.at a owl:DatatypeProperty ;
  rdfs:label "at"@en ;
  rdfs:domain cim:GovHydro1 ;
  rdfs:range cim:PU ;
  skos:definition "Turbine gain (<i>At</i>) (&gt; 0).  Typical value = 1,2."@en .

cim:GovHydro1.dturb a owl:DatatypeProperty ;
  rdfs:label "dturb"@en ;
  rdfs:domain cim:GovHydro1 ;
  rdfs:range cim:PU ;
  skos:definition "Turbine damping factor (<i>Dturb</i>) (&gt;= 0).  Typical value = 0,5."@en .

cim:GovHydro1.gmax a owl:DatatypeProperty ;
  rdfs:label "gmax"@en ;
  rdfs:domain cim:GovHydro1 ;
  rdfs:range cim:PU ;
  skos:definition "Maximum gate opening (<i>Gmax</i>) (&gt; 0 and &gt; GovHydro.gmin).  Typical value = 1."@en .

cim:GovHydro1.gmin a owl:DatatypeProperty ;
  rdfs:label "gmin"@en ;
  rdfs:domain cim:GovHydro1 ;
  rdfs:range cim:PU ;
  skos:definition "Minimum gate opening (<i>Gmin</i>) (&gt;= 0 and &lt; GovHydro1.gmax).  Typical value = 0."@en .

cim:GovHydro1.hdam a owl:DatatypeProperty ;
  rdfs:label "hdam"@en ;
  rdfs:domain cim:GovHydro1 ;
  rdfs:range cim:PU ;
  skos:definition "Turbine nominal head (<i>hdam</i>).  Typical value = 1."@en .

cim:GovHydro1.mwbase a owl:DatatypeProperty ;
  rdfs:label "mwbase"@en ;
  rdfs:domain cim:GovHydro1 ;
  rdfs:range cim:ActivePower ;
  skos:definition "Base for power values (<i>MWbase</i>) (&gt; 0).  Unit = MW."@en .

cim:GovHydro1.qnl a owl:DatatypeProperty ;
  rdfs:label "qnl"@en ;
  rdfs:domain cim:GovHydro1 ;
  rdfs:range cim:PU ;
  skos:definition "No-load flow at nominal head (<i>qnl</i>) (&gt;= 0).  Typical value = 0,08."@en .

cim:GovHydro1.rperm a owl:DatatypeProperty ;
  rdfs:label "rperm"@en ;
  rdfs:domain cim:GovHydro1 ;
  rdfs:range cim:PU ;
  skos:definition "Permanent droop (<i>R</i>) (&gt; 0).  Typical value = 0,04."@en .

cim:GovHydro1.rtemp a owl:DatatypeProperty ;
  rdfs:label "rtemp"@en ;
  rdfs:domain cim:GovHydro1 ;
  rdfs:range cim:PU ;
  skos:definition "Temporary droop (<i>r</i>) (&gt; GovHydro1.rperm).  Typical value = 0,3."@en .

cim:GovHydro1.tf a owl:DatatypeProperty ;
  rdfs:label "tf"@en ;
  rdfs:domain cim:GovHydro1 ;
  rdfs:range cim:Seconds ;
  skos:definition "Filter time constant (<i>Tf</i>) (&gt; 0).  Typical value = 0,05."@en .

cim:GovHydro1.tg a owl:DatatypeProperty ;
  rdfs:label "tg"@en ;
  rdfs:domain cim:GovHydro1 ;
  rdfs:range cim:Seconds ;
  skos:definition "Gate servo time constant (<i>Tg</i>) (&gt; 0).  Typical value = 0,5."@en .

cim:GovHydro1.tr a owl:DatatypeProperty ;
  rdfs:label "tr"@en ;
  rdfs:domain cim:GovHydro1 ;
  rdfs:range cim:Seconds ;
  skos:definition "Washout time constant (<i>Tr</i>) (&gt; 0).  Typical value = 5."@en .

cim:GovHydro1.tw a owl:DatatypeProperty ;
  rdfs:label "tw"@en ;
  rdfs:domain cim:GovHydro1 ;
  rdfs:range cim:Seconds ;
  skos:definition "Water inertia time constant (<i>Tw</i>) (&gt; 0).  Typical value = 1."@en .

cim:GovHydro1.velm a owl:DatatypeProperty ;
  rdfs:label "velm"@en ;
  rdfs:domain cim:GovHydro1 ;
  rdfs:range xsd:float ;
  skos:definition "Maximum gate velocity (<i>Vlem</i>) (&gt; 0).  Typical value = 0,2."@en .

cim:GovHydro2.aturb a owl:DatatypeProperty ;
  rdfs:label "aturb"@en ;
  rdfs:domain cim:GovHydro2 ;
  rdfs:range cim:PU ;
  skos:definition "Turbine numerator multiplier (<i>Aturb</i>).  Typical value = -1."@en .

cim:GovHydro2.bturb a owl:DatatypeProperty ;
  rdfs:label "bturb"@en ;
  rdfs:domain cim:GovHydro2 ;
  rdfs:range cim:PU ;
  skos:definition "Turbine denominator multiplier (<i>Bturb</i>) (&gt; 0).  Typical value = 0,5."@en .

cim:GovHydro2.db1 a owl:DatatypeProperty ;
  rdfs:label "db1"@en ;
  rdfs:domain cim:GovHydro2 ;
  rdfs:range cim:Frequency ;
  skos:definition "Intentional deadband width (<i>db1</i>).  Unit = Hz.  Typical value = 0."@en .

cim:GovHydro2.db2 a owl:DatatypeProperty ;
  rdfs:label "db2"@en ;
  rdfs:domain cim:GovHydro2 ;
  rdfs:range cim:ActivePower ;
  skos:definition "Unintentional deadband (<i>db2</i>).  Unit = MW.  Typical value = 0."@en .

cim:GovHydro2.eps a owl:DatatypeProperty ;
  rdfs:label "eps"@en ;
  rdfs:domain cim:GovHydro2 ;
  rdfs:range cim:Frequency ;
  skos:definition "Intentional db hysteresis (<i>eps</i>).  Unit = Hz.  Typical value = 0."@en .

cim:GovHydro2.gv1 a owl:DatatypeProperty ;
  rdfs:label "gv1"@en ;
  rdfs:domain cim:GovHydro2 ;
  rdfs:range cim:PU ;
  skos:definition "Nonlinear gain point 1, PU gv (<i>Gv1</i>).  Typical value = 0."@en .

cim:GovHydro2.gv2 a owl:DatatypeProperty ;
  rdfs:label "gv2"@en ;
  rdfs:domain cim:GovHydro2 ;
  rdfs:range cim:PU ;
  skos:definition "Nonlinear gain point 2, PU gv (<i>Gv2</i>).  Typical value = 0."@en .

cim:GovHydro2.gv3 a owl:DatatypeProperty ;
  rdfs:label "gv3"@en ;
  rdfs:domain cim:GovHydro2 ;
  rdfs:range cim:PU ;
  skos:definition "Nonlinear gain point 3, PU gv (<i>Gv3</i>).  Typical value = 0."@en .

cim:GovHydro2.gv4 a owl:DatatypeProperty ;
  rdfs:label "gv4"@en ;
  rdfs:domain cim:GovHydro2 ;
  rdfs:range cim:PU ;
  skos:definition "Nonlinear gain point 4, PU gv (<i>Gv4</i>).  Typical value = 0."@en .

cim:GovHydro2.gv5 a owl:DatatypeProperty ;
  rdfs:label "gv5"@en ;
  rdfs:domain cim:GovHydro2 ;
  rdfs:range cim:PU ;
  skos:definition "Nonlinear gain point 5, PU gv (<i>Gv5</i>).  Typical value = 0."@en .

cim:GovHydro2.gv6 a owl:DatatypeProperty ;
  rdfs:label "gv6"@en ;
  rdfs:domain cim:GovHydro2 ;
  rdfs:range cim:PU ;
  skos:definition "Nonlinear gain point 6, PU gv (<i>Gv6</i>).  Typical value = 0."@en .

cim:GovHydro2.kturb a owl:DatatypeProperty ;
  rdfs:label "kturb"@en ;
  rdfs:domain cim:GovHydro2 ;
  rdfs:range cim:PU ;
  skos:definition "Turbine gain (<i>Kturb</i>).  Typical value = 1."@en .

cim:GovHydro2.mwbase a owl:DatatypeProperty ;
  rdfs:label "mwbase"@en ;
  rdfs:domain cim:GovHydro2 ;
  rdfs:range cim:ActivePower ;
  skos:definition "Base for power values (<i>MWbase</i>) (&gt; 0).  Unit = MW."@en .

cim:GovHydro2.pgv1 a owl:DatatypeProperty ;
  rdfs:label "pgv1"@en ;
  rdfs:domain cim:GovHydro2 ;
  rdfs:range cim:PU ;
  skos:definition "Nonlinear gain point 1, PU power (<i>Pgv1</i>).  Typical value = 0."@en .

cim:GovHydro2.pgv2 a owl:DatatypeProperty ;
  rdfs:label "pgv2"@en ;
  rdfs:domain cim:GovHydro2 ;
  rdfs:range cim:PU ;
  skos:definition "Nonlinear gain point 2, PU power (<i>Pgv2</i>).  Typical value = 0."@en .

cim:GovHydro2.pgv3 a owl:DatatypeProperty ;
  rdfs:label "pgv3"@en ;
  rdfs:domain cim:GovHydro2 ;
  rdfs:range cim:PU ;
  skos:definition "Nonlinear gain point 3, PU power (<i>Pgv3</i>).  Typical value = 0."@en .

cim:GovHydro2.pgv4 a owl:DatatypeProperty ;
  rdfs:label "pgv4"@en ;
  rdfs:domain cim:GovHydro2 ;
  rdfs:range cim:PU ;
  skos:definition "Nonlinear gain point 4, PU power (P<i>gv4</i>).  Typical value = 0."@en .

cim:GovHydro2.pgv5 a owl:DatatypeProperty ;
  rdfs:label "pgv5"@en ;
  rdfs:domain cim:GovHydro2 ;
  rdfs:range cim:PU ;
  skos:definition "Nonlinear gain point 5, PU power (<i>Pgv5</i>).  Typical value = 0."@en .

cim:GovHydro2.pgv6 a owl:DatatypeProperty ;
  rdfs:label "pgv6"@en ;
  rdfs:domain cim:GovHydro2 ;
  rdfs:range cim:PU ;
  skos:definition "Nonlinear gain point 6, PU power (<i>Pgv6</i>).  Typical value = 0."@en .

cim:GovHydro2.pmax a owl:DatatypeProperty ;
  rdfs:label "pmax"@en ;
  rdfs:domain cim:GovHydro2 ;
  rdfs:range cim:PU ;
  skos:definition "Maximum gate opening (<i>Pmax</i>) (&gt; GovHydro2.pmin).  Typical value = 1."@en .

cim:GovHydro2.pmin a owl:DatatypeProperty ;
  rdfs:label "pmin"@en ;
  rdfs:domain cim:GovHydro2 ;
  rdfs:range cim:PU ;
  skos:definition "Minimum gate opening (<i>Pmin</i>) (&lt; GovHydro2.pmax).  Typical value = 0."@en .

cim:GovHydro2.rperm a owl:DatatypeProperty ;
  rdfs:label "rperm"@en ;
  rdfs:domain cim:GovHydro2 ;
  rdfs:range cim:PU ;
  skos:definition "Permanent droop (<i>Rperm</i>).  Typical value = 0,05."@en .

cim:GovHydro2.rtemp a owl:DatatypeProperty ;
  rdfs:label "rtemp"@en ;
  rdfs:domain cim:GovHydro2 ;
  rdfs:range cim:PU ;
  skos:definition "Temporary droop (<i>Rtemp</i>).  Typical value = 0,5."@en .

cim:GovHydro2.tg a owl:DatatypeProperty ;
  rdfs:label "tg"@en ;
  rdfs:domain cim:GovHydro2 ;
  rdfs:range cim:Seconds ;
  skos:definition "Gate servo time constant (<i>Tg</i>) (&gt; 0).  Typical value = 0,5."@en .

cim:GovHydro2.tp a owl:DatatypeProperty ;
  rdfs:label "tp"@en ;
  rdfs:domain cim:GovHydro2 ;
  rdfs:range cim:Seconds ;
  skos:definition "Pilot servo valve time constant (<i>Tp</i>) (&gt;= 0).  Typical value = 0,03."@en .

cim:GovHydro2.tr a owl:DatatypeProperty ;
  rdfs:label "tr"@en ;
  rdfs:domain cim:GovHydro2 ;
  rdfs:range cim:Seconds ;
  skos:definition "Dashpot time constant (<i>Tr</i>) (&gt;= 0).  Typical value = 12."@en .

cim:GovHydro2.tw a owl:DatatypeProperty ;
  rdfs:label "tw"@en ;
  rdfs:domain cim:GovHydro2 ;
  rdfs:range cim:Seconds ;
  skos:definition "Water inertia time constant (<i>Tw</i>) (&gt;= 0).  Typical value = 2."@en .

cim:GovHydro2.uc a owl:DatatypeProperty ;
  rdfs:label "uc"@en ;
  rdfs:domain cim:GovHydro2 ;
  rdfs:range xsd:float ;
  skos:definition "Maximum gate closing velocity (<i>Uc</i>) (&lt; 0).  Unit = PU / s.   Typical value = -0,1."@en .

cim:GovHydro2.uo a owl:DatatypeProperty ;
  rdfs:label "uo"@en ;
  rdfs:domain cim:GovHydro2 ;
  rdfs:range xsd:float ;
  skos:definition "Maximum gate opening velocity (<i>Uo</i>).  Unit = PU / s.  Typical value = 0,1."@en .

cim:GovHydro3.at a owl:DatatypeProperty ;
  rdfs:label "at"@en ;
  rdfs:domain cim:GovHydro3 ;
  rdfs:range cim:PU ;
  skos:definition "Turbine gain (<i>At</i>) (&gt;0).  Typical value = 1,2."@en .

cim:GovHydro3.db1 a owl:DatatypeProperty ;
  rdfs:label "db1"@en ;
  rdfs:domain cim:GovHydro3 ;
  rdfs:range cim:Frequency ;
  skos:definition "Intentional dead-band width (<i>db1</i>).  Unit = Hz.  Typical value = 0."@en .

cim:GovHydro3.db2 a owl:DatatypeProperty ;
  rdfs:label "db2"@en ;
  rdfs:domain cim:GovHydro3 ;
  rdfs:range cim:ActivePower ;
  skos:definition "Unintentional dead-band (<i>db2</i>).  Unit = MW.  Typical value = 0."@en .

cim:GovHydro3.dturb a owl:DatatypeProperty ;
  rdfs:label "dturb"@en ;
  rdfs:domain cim:GovHydro3 ;
  rdfs:range cim:PU ;
  skos:definition "Turbine damping factor (<i>Dturb</i>).  Typical value = 0,2."@en .

cim:GovHydro3.eps a owl:DatatypeProperty ;
  rdfs:label "eps"@en ;
  rdfs:domain cim:GovHydro3 ;
  rdfs:range cim:Frequency ;
  skos:definition "Intentional db hysteresis (<i>eps</i>).  Unit = Hz.  Typical value = 0."@en .

cim:GovHydro3.governorControl a owl:DatatypeProperty ;
  rdfs:label "governorControl"@en ;
  rdfs:domain cim:GovHydro3 ;
  rdfs:range xsd:boolean ;
  skos:definition """
Governor control flag (<i>Cflag</i>).
true = PID control is active
false = double derivative control is active.
Typical value = true.
\t"""@en .

cim:GovHydro3.gv1 a owl:DatatypeProperty ;
  rdfs:label "gv1"@en ;
  rdfs:domain cim:GovHydro3 ;
  rdfs:range cim:PU ;
  skos:definition "Nonlinear gain point 1, PU gv (<i>Gv1</i>).  Typical value = 0."@en .

cim:GovHydro3.gv2 a owl:DatatypeProperty ;
  rdfs:label "gv2"@en ;
  rdfs:domain cim:GovHydro3 ;
  rdfs:range cim:PU ;
  skos:definition "Nonlinear gain point 2, PU gv (<i>Gv2</i>).  Typical value = 0."@en .

cim:GovHydro3.gv3 a owl:DatatypeProperty ;
  rdfs:label "gv3"@en ;
  rdfs:domain cim:GovHydro3 ;
  rdfs:range cim:PU ;
  skos:definition "Nonlinear gain point 3, PU gv (<i>Gv3</i>).  Typical value = 0."@en .

cim:GovHydro3.gv4 a owl:DatatypeProperty ;
  rdfs:label "gv4"@en ;
  rdfs:domain cim:GovHydro3 ;
  rdfs:range cim:PU ;
  skos:definition "Nonlinear gain point 4, PU gv (<i>Gv4</i>).  Typical value = 0."@en .

cim:GovHydro3.gv5 a owl:DatatypeProperty ;
  rdfs:label "gv5"@en ;
  rdfs:domain cim:GovHydro3 ;
  rdfs:range cim:PU ;
  skos:definition "Nonlinear gain point 5, PU gv (<i>Gv5</i>).  Typical value = 0."@en .

cim:GovHydro3.gv6 a owl:DatatypeProperty ;
  rdfs:label "gv6"@en ;
  rdfs:domain cim:GovHydro3 ;
  rdfs:range cim:PU ;
  skos:definition "Nonlinear gain point 6, PU gv (<i>Gv6</i>).  Typical value = 0."@en .

cim:GovHydro3.h0 a owl:DatatypeProperty ;
  rdfs:label "h0"@en ;
  rdfs:domain cim:GovHydro3 ;
  rdfs:range cim:PU ;
  skos:definition "Turbine nominal head (<i>H0</i>).  Typical value = 1."@en .

cim:GovHydro3.k1 a owl:DatatypeProperty ;
  rdfs:label "k1"@en ;
  rdfs:domain cim:GovHydro3 ;
  rdfs:range cim:PU ;
  skos:definition "Derivative gain (<i>K1</i>).  Typical value = 0,01."@en .

cim:GovHydro3.k2 a owl:DatatypeProperty ;
  rdfs:label "k2"@en ;
  rdfs:domain cim:GovHydro3 ;
  rdfs:range cim:PU ;
  skos:definition "Double derivative gain, if <i>Cflag</i> = -1 (<i>K2</i>).  Typical value = 2,5."@en .

cim:GovHydro3.kg a owl:DatatypeProperty ;
  rdfs:label "kg"@en ;
  rdfs:domain cim:GovHydro3 ;
  rdfs:range cim:PU ;
  skos:definition "Gate servo gain (<i>Kg</i>).  Typical value = 2."@en .

cim:GovHydro3.ki a owl:DatatypeProperty ;
  rdfs:label "ki"@en ;
  rdfs:domain cim:GovHydro3 ;
  rdfs:range cim:PU ;
  skos:definition "Integral gain (<i>Ki</i>).  Typical value = 0,5."@en .

cim:GovHydro3.mwbase a owl:DatatypeProperty ;
  rdfs:label "mwbase"@en ;
  rdfs:domain cim:GovHydro3 ;
  rdfs:range cim:ActivePower ;
  skos:definition "Base for power values (<i>MWbase</i>) (&gt; 0).  Unit = MW."@en .

cim:GovHydro3.pgv1 a owl:DatatypeProperty ;
  rdfs:label "pgv1"@en ;
  rdfs:domain cim:GovHydro3 ;
  rdfs:range cim:PU ;
  skos:definition "Nonlinear gain point 1, PU power (<i>Pgv1</i>).  Typical value = 0."@en .

cim:GovHydro3.pgv2 a owl:DatatypeProperty ;
  rdfs:label "pgv2"@en ;
  rdfs:domain cim:GovHydro3 ;
  rdfs:range cim:PU ;
  skos:definition "Nonlinear gain point 2, PU power (<i>Pgv2</i>).  Typical value = 0."@en .

cim:GovHydro3.pgv3 a owl:DatatypeProperty ;
  rdfs:label "pgv3"@en ;
  rdfs:domain cim:GovHydro3 ;
  rdfs:range cim:PU ;
  skos:definition "Nonlinear gain point 3, PU power (<i>Pgv3</i>).  Typical value = 0."@en .

cim:GovHydro3.pgv4 a owl:DatatypeProperty ;
  rdfs:label "pgv4"@en ;
  rdfs:domain cim:GovHydro3 ;
  rdfs:range cim:PU ;
  skos:definition "Nonlinear gain point 4, PU power (<i>Pgv4</i>).  Typical value = 0."@en .

cim:GovHydro3.pgv5 a owl:DatatypeProperty ;
  rdfs:label "pgv5"@en ;
  rdfs:domain cim:GovHydro3 ;
  rdfs:range cim:PU ;
  skos:definition "Nonlinear gain point 5, PU power (<i>Pgv5</i>).  Typical value = 0."@en .

cim:GovHydro3.pgv6 a owl:DatatypeProperty ;
  rdfs:label "pgv6"@en ;
  rdfs:domain cim:GovHydro3 ;
  rdfs:range cim:PU ;
  skos:definition "Nonlinear gain point 6, PU power (<i>Pgv6</i>).  Typical value = 0."@en .

cim:GovHydro3.pmax a owl:DatatypeProperty ;
  rdfs:label "pmax"@en ;
  rdfs:domain cim:GovHydro3 ;
  rdfs:range cim:PU ;
  skos:definition "Maximum gate opening, PU of MWbase (<i>Pmax</i>) (&gt; GovHydro3.pmin).  Typical value = 1."@en .

cim:GovHydro3.pmin a owl:DatatypeProperty ;
  rdfs:label "pmin"@en ;
  rdfs:domain cim:GovHydro3 ;
  rdfs:range cim:PU ;
  skos:definition "Minimum gate opening, PU of <i>MWbase</i> (<i>Pmin</i>) (&lt; GovHydro3.pmax).  Typical value = 0."@en .

cim:GovHydro3.qnl a owl:DatatypeProperty ;
  rdfs:label "qnl"@en ;
  rdfs:domain cim:GovHydro3 ;
  rdfs:range cim:PU ;
  skos:definition "No-load turbine flow at nominal head (<i>Qnl</i>).  Typical value = 0,08."@en .

cim:GovHydro3.relec a owl:DatatypeProperty ;
  rdfs:label "relec"@en ;
  rdfs:domain cim:GovHydro3 ;
  rdfs:range cim:PU ;
  skos:definition "Steady-state droop, PU, for electrical power feedback (<i>Relec</i>).  Typical value = 0,05."@en .

cim:GovHydro3.rgate a owl:DatatypeProperty ;
  rdfs:label "rgate"@en ;
  rdfs:domain cim:GovHydro3 ;
  rdfs:range cim:PU ;
  skos:definition "Steady-state droop, PU, for governor output feedback (<i>Rgate</i>).  Typical value = 0."@en .

cim:GovHydro3.td a owl:DatatypeProperty ;
  rdfs:label "td"@en ;
  rdfs:domain cim:GovHydro3 ;
  rdfs:range cim:Seconds ;
  skos:definition "Input filter time constant (<i>Td</i>) (&gt;= 0).  Typical value = 0,05."@en .

cim:GovHydro3.tf a owl:DatatypeProperty ;
  rdfs:label "tf"@en ;
  rdfs:domain cim:GovHydro3 ;
  rdfs:range cim:Seconds ;
  skos:definition "Washout time constant (<i>Tf</i>) (&gt;= 0).  Typical value = 0,1."@en .

cim:GovHydro3.tp a owl:DatatypeProperty ;
  rdfs:label "tp"@en ;
  rdfs:domain cim:GovHydro3 ;
  rdfs:range cim:Seconds ;
  skos:definition "Gate servo time constant (<i>Tp</i>) (&gt;= 0).  Typical value = 0,05."@en .

cim:GovHydro3.tt a owl:DatatypeProperty ;
  rdfs:label "tt"@en ;
  rdfs:domain cim:GovHydro3 ;
  rdfs:range cim:Seconds ;
  skos:definition "Power feedback time constant (<i>Tt</i>) (&gt;= 0).  Typical value = 0,2."@en .

cim:GovHydro3.tw a owl:DatatypeProperty ;
  rdfs:label "tw"@en ;
  rdfs:domain cim:GovHydro3 ;
  rdfs:range cim:Seconds ;
  skos:definition "Water inertia time constant (<i>Tw</i>) (&gt;= 0).  If = 0, block is bypassed.  Typical value = 1."@en .

cim:GovHydro3.velcl a owl:DatatypeProperty ;
  rdfs:label "velcl"@en ;
  rdfs:domain cim:GovHydro3 ;
  rdfs:range xsd:float ;
  skos:definition "Maximum gate closing velocity (<i>Velcl</i>).  Unit = PU / s.  Typical value = -0,2."@en .

cim:GovHydro3.velop a owl:DatatypeProperty ;
  rdfs:label "velop"@en ;
  rdfs:domain cim:GovHydro3 ;
  rdfs:range xsd:float ;
  skos:definition "Maximum gate opening velocity (<i>Velop</i>).  Unit = PU / s. Typical value = 0,2."@en .

cim:GovHydro4.at a owl:DatatypeProperty ;
  rdfs:label "at"@en ;
  rdfs:domain cim:GovHydro4 ;
  rdfs:range cim:PU ;
  skos:definition "Turbine gain (<i>At</i>).  Typical value = 1,2."@en .

cim:GovHydro4.bgv0 a owl:DatatypeProperty ;
  rdfs:label "bgv0"@en ;
  rdfs:domain cim:GovHydro4 ;
  rdfs:range cim:PU ;
  skos:definition "Kaplan blade servo point 0 (<i>Bgv0</i>) (= 0 for simple, = 0 for Francis/Pelton).  Typical value for Kaplan = 0."@en .

cim:GovHydro4.bgv1 a owl:DatatypeProperty ;
  rdfs:label "bgv1"@en ;
  rdfs:domain cim:GovHydro4 ;
  rdfs:range cim:PU ;
  skos:definition "Kaplan blade servo point 1 (<i>Bgv1</i>) (= 0 for simple, = 0 for Francis/Pelton).  Typical value for Kaplan = 0."@en .

cim:GovHydro4.bgv2 a owl:DatatypeProperty ;
  rdfs:label "bgv2"@en ;
  rdfs:domain cim:GovHydro4 ;
  rdfs:range cim:PU ;
  skos:definition "Kaplan blade servo point 2 (<i>Bgv2</i>) (= 0 for simple, = 0 for Francis/Pelton).  Typical value for Kaplan = 0,1."@en .

cim:GovHydro4.bgv3 a owl:DatatypeProperty ;
  rdfs:label "bgv3"@en ;
  rdfs:domain cim:GovHydro4 ;
  rdfs:range cim:PU ;
  skos:definition "Kaplan blade servo point 3 (<i>Bgv3</i>) (= 0 for simple, = 0 for Francis/Pelton).  Typical value for Kaplan = 0,667."@en .

cim:GovHydro4.bgv4 a owl:DatatypeProperty ;
  rdfs:label "bgv4"@en ;
  rdfs:domain cim:GovHydro4 ;
  rdfs:range cim:PU ;
  skos:definition "Kaplan blade servo point 4 (<i>Bgv4</i>) (= 0 for simple, = 0 for Francis/Pelton).  Typical value for Kaplan = 0,9."@en .

cim:GovHydro4.bgv5 a owl:DatatypeProperty ;
  rdfs:label "bgv5"@en ;
  rdfs:domain cim:GovHydro4 ;
  rdfs:range cim:PU ;
  skos:definition "Kaplan blade servo point 5 (<i>Bgv5</i>) (= 0 for simple, = 0 for Francis/Pelton).  Typical value for Kaplan = 1."@en .

cim:GovHydro4.bmax a owl:DatatypeProperty ;
  rdfs:label "bmax"@en ;
  rdfs:domain cim:GovHydro4 ;
  rdfs:range xsd:float ;
  skos:definition "Maximum blade adjustment factor (<i>Bmax</i>)  (= 0 for simple, = 0 for Francis/Pelton).  Typical value for Kaplan = 1,1276."@en .

cim:GovHydro4.db1 a owl:DatatypeProperty ;
  rdfs:label "db1"@en ;
  rdfs:domain cim:GovHydro4 ;
  rdfs:range cim:Frequency ;
  skos:definition "Intentional deadband width (<i>db1</i>).  Unit = Hz.  Typical value = 0."@en .

cim:GovHydro4.db2 a owl:DatatypeProperty ;
  rdfs:label "db2"@en ;
  rdfs:domain cim:GovHydro4 ;
  rdfs:range cim:ActivePower ;
  skos:definition "Unintentional dead-band (<i>db2</i>).  Unit = MW.  Typical value = 0."@en .

cim:GovHydro4.dturb a owl:DatatypeProperty ;
  rdfs:label "dturb"@en ;
  rdfs:domain cim:GovHydro4 ;
  rdfs:range cim:PU ;
  skos:definition "Turbine damping factor (<i>Dturb</i>).  Unit = delta P (PU of <i>MWbase</i>) / delta speed (PU).  Typical value for simple = 0,5, Francis/Pelton = 1,1, Kaplan = 1,1."@en .

cim:GovHydro4.eps a owl:DatatypeProperty ;
  rdfs:label "eps"@en ;
  rdfs:domain cim:GovHydro4 ;
  rdfs:range cim:Frequency ;
  skos:definition "Intentional db hysteresis (<i>eps</i>).  Unit = Hz.  Typical value = 0."@en .

cim:GovHydro4.gmax a owl:DatatypeProperty ;
  rdfs:label "gmax"@en ;
  rdfs:domain cim:GovHydro4 ;
  rdfs:range cim:PU ;
  skos:definition "Maximum gate opening, PU of <i>MWbase</i> (<i>Gmax</i>) (&gt; GovHydro4.gmin).  Typical value = 1."@en .

cim:GovHydro4.gmin a owl:DatatypeProperty ;
  rdfs:label "gmin"@en ;
  rdfs:domain cim:GovHydro4 ;
  rdfs:range cim:PU ;
  skos:definition "Minimum gate opening, PU of <i>MWbase</i> (<i>Gmin</i>) (&lt; GovHydro4.gmax).  Typical value = 0."@en .

cim:GovHydro4.gv0 a owl:DatatypeProperty ;
  rdfs:label "gv0"@en ;
  rdfs:domain cim:GovHydro4 ;
  rdfs:range cim:PU ;
  skos:definition "Nonlinear gain point 0, PU gv (<i>Gv0</i>) (= 0 for simple).  Typical for Francis/Pelton = 0,1, Kaplan = 0,1."@en .

cim:GovHydro4.gv1 a owl:DatatypeProperty ;
  rdfs:label "gv1"@en ;
  rdfs:domain cim:GovHydro4 ;
  rdfs:range cim:PU ;
  skos:definition "Nonlinear gain point 1, PU gv (<i>Gv1</i>) (= 0 for simple, &gt; GovHydro4.gv0 for Francis/Pelton and Kaplan). Typical value for Francis/Pelton = 0,4, Kaplan = 0,4."@en .

cim:GovHydro4.gv2 a owl:DatatypeProperty ;
  rdfs:label "gv2"@en ;
  rdfs:domain cim:GovHydro4 ;
  rdfs:range cim:PU ;
  skos:definition "Nonlinear gain point 2, PU gv (<i>Gv2</i>) (= 0 for simple, &gt; GovHydro4.gv1 for Francis/Pelton and Kaplan). Typical value for Francis/Pelton = 0,5, Kaplan = 0,5."@en .

cim:GovHydro4.gv3 a owl:DatatypeProperty ;
  rdfs:label "gv3"@en ;
  rdfs:domain cim:GovHydro4 ;
  rdfs:range cim:PU ;
  skos:definition "Nonlinear gain point 3, PU gv (<i>Gv3</i>)  (= 0 for simple, &gt; GovHydro4.gv2 for Francis/Pelton and Kaplan). Typical value for Francis/Pelton = 0,7, Kaplan = 0,7."@en .

cim:GovHydro4.gv4 a owl:DatatypeProperty ;
  rdfs:label "gv4"@en ;
  rdfs:domain cim:GovHydro4 ;
  rdfs:range cim:PU ;
  skos:definition "Nonlinear gain point 4, PU gv (<i>Gv4</i>)  (= 0 for simple, &gt; GovHydro4.gv3 for Francis/Pelton and Kaplan). Typical value for  Francis/Pelton = 0,8, Kaplan = 0,8."@en .

cim:GovHydro4.gv5 a owl:DatatypeProperty ;
  rdfs:label "gv5"@en ;
  rdfs:domain cim:GovHydro4 ;
  rdfs:range cim:PU ;
  skos:definition "Nonlinear gain point 5, PU gv (<i>Gv5</i>)  (= 0 for simple, &lt; 1 and &gt; GovHydro4.gv4 for Francis/Pelton and Kaplan). Typical value for Francis/Pelton = 0,9, Kaplan = 0,9."@en .

cim:GovHydro4.hdam a owl:DatatypeProperty ;
  rdfs:label "hdam"@en ;
  rdfs:domain cim:GovHydro4 ;
  rdfs:range cim:PU ;
  skos:definition "Head available at dam (<i>hdam</i>).  Typical value = 1."@en .

cim:GovHydro4.model a owl:DatatypeProperty ;
  rdfs:label "model"@en ;
  rdfs:domain cim:GovHydro4 ;
  rdfs:range cim:GovHydro4ModelKind ;
  skos:definition "The kind of model being represented (simple, Francis/Pelton or Kaplan)."@en .

cim:GovHydro4.mwbase a owl:DatatypeProperty ;
  rdfs:label "mwbase"@en ;
  rdfs:domain cim:GovHydro4 ;
  rdfs:range cim:ActivePower ;
  skos:definition "Base for power values (<i>MWbase</i>) (&gt; 0).  Unit = MW."@en .

cim:GovHydro4.pgv0 a owl:DatatypeProperty ;
  rdfs:label "pgv0"@en ;
  rdfs:domain cim:GovHydro4 ;
  rdfs:range cim:PU ;
  skos:definition "Nonlinear gain point 0, PU power (<i>Pgv0</i>) (= 0 for simple).  Typical value = 0."@en .

cim:GovHydro4.pgv1 a owl:DatatypeProperty ;
  rdfs:label "pgv1"@en ;
  rdfs:domain cim:GovHydro4 ;
  rdfs:range cim:PU ;
  skos:definition """
Nonlinear gain point 1, PU power (<i>Pgv1</i>) (= 0 for simple).
Typical value for Francis/Pelton = 0,42, Kaplan = 0,35.
\t"""@en .

cim:GovHydro4.pgv2 a owl:DatatypeProperty ;
  rdfs:label "pgv2"@en ;
  rdfs:domain cim:GovHydro4 ;
  rdfs:range cim:PU ;
  skos:definition """
Nonlinear gain point 2, PU power (<i>Pgv2</i>) (= 0 for simple).
Typical value for Francis/Pelton = 0,56, Kaplan = 0,468.
\t"""@en .

cim:GovHydro4.pgv3 a owl:DatatypeProperty ;
  rdfs:label "pgv3"@en ;
  rdfs:domain cim:GovHydro4 ;
  rdfs:range cim:PU ;
  skos:definition """
Nonlinear gain point 3, PU power (<i>Pgv3</i>) (= 0 for simple).
Typical value for Francis/Pelton = 0,8, Kaplan = 0,796.
\t"""@en .

cim:GovHydro4.pgv4 a owl:DatatypeProperty ;
  rdfs:label "pgv4"@en ;
  rdfs:domain cim:GovHydro4 ;
  rdfs:range cim:PU ;
  skos:definition """
Nonlinear gain point 4, PU power (<i>Pgv4</i>) (= 0 for simple).
Typical value for Francis/Pelton = 0,9, Kaplan = 0,917.
\t"""@en .

cim:GovHydro4.pgv5 a owl:DatatypeProperty ;
  rdfs:label "pgv5"@en ;
  rdfs:domain cim:GovHydro4 ;
  rdfs:range cim:PU ;
  skos:definition """
Nonlinear gain point 5, PU power (<i>Pgv5</i>) (= 0 for simple). 
Typical value for Francis/Pelton = 0,97, Kaplan = 0,99.
\t"""@en .

cim:GovHydro4.qnl a owl:DatatypeProperty ;
  rdfs:label "qnl"@en ;
  rdfs:domain cim:GovHydro4 ;
  rdfs:range cim:PU ;
  skos:definition """
No-load flow at nominal head (<i>Qnl</i>).
Typical value for simple = 0,08, Francis/Pelton = 0, Kaplan = 0.
\t"""@en .

cim:GovHydro4.rperm a owl:DatatypeProperty ;
  rdfs:label "rperm"@en ;
  rdfs:domain cim:GovHydro4 ;
  rdfs:range cim:Seconds ;
  skos:definition "Permanent droop (<i>Rperm</i>) (&gt;= 0).  Typical value = 0,05."@en .

cim:GovHydro4.rtemp a owl:DatatypeProperty ;
  rdfs:label "rtemp"@en ;
  rdfs:domain cim:GovHydro4 ;
  rdfs:range cim:Seconds ;
  skos:definition "Temporary droop (<i>Rtemp</i>) (&gt;= 0).  Typical value = 0,3."@en .

cim:GovHydro4.tblade a owl:DatatypeProperty ;
  rdfs:label "tblade"@en ;
  rdfs:domain cim:GovHydro4 ;
  rdfs:range cim:Seconds ;
  skos:definition "Blade servo time constant (<i>Tblade</i>) (&gt;= 0).  Typical value = 100."@en .

cim:GovHydro4.tg a owl:DatatypeProperty ;
  rdfs:label "tg"@en ;
  rdfs:domain cim:GovHydro4 ;
  rdfs:range cim:Seconds ;
  skos:definition "Gate servo time constant (<i>Tg</i>) (&gt; 0).  Typical value = 0,5."@en .

cim:GovHydro4.tp a owl:DatatypeProperty ;
  rdfs:label "tp"@en ;
  rdfs:domain cim:GovHydro4 ;
  rdfs:range cim:Seconds ;
  skos:definition "Pilot servo time constant (<i>Tp</i>) (&gt;= 0).  Typical value = 0,1."@en .

cim:GovHydro4.tr a owl:DatatypeProperty ;
  rdfs:label "tr"@en ;
  rdfs:domain cim:GovHydro4 ;
  rdfs:range cim:Seconds ;
  skos:definition "Dashpot time constant (<i>Tr</i>) (&gt;= 0).  Typical value = 5."@en .

cim:GovHydro4.tw a owl:DatatypeProperty ;
  rdfs:label "tw"@en ;
  rdfs:domain cim:GovHydro4 ;
  rdfs:range cim:Seconds ;
  skos:definition "Water inertia time constant (<i>Tw</i>) (&gt; 0).  Typical value = 1."@en .

cim:GovHydro4.uc a owl:DatatypeProperty ;
  rdfs:label "uc"@en ;
  rdfs:domain cim:GovHydro4 ;
  rdfs:range xsd:float ;
  skos:definition "Max gate closing velocity (<i>Uc</i>).  Typical value = 0,2."@en .

cim:GovHydro4.uo a owl:DatatypeProperty ;
  rdfs:label "uo"@en ;
  rdfs:domain cim:GovHydro4 ;
  rdfs:range xsd:float ;
  skos:definition "Max gate opening velocity (<i>Uo</i>).  Typical value = 0,2."@en .

cim:GovHydroDD.aturb a owl:DatatypeProperty ;
  rdfs:label "aturb"@en ;
  rdfs:domain cim:GovHydroDD ;
  rdfs:range cim:PU ;
  skos:definition "Turbine numerator multiplier (<i>Aturb</i>) (see parameter detail 3).  Typical value = -1."@en .

cim:GovHydroDD.bturb a owl:DatatypeProperty ;
  rdfs:label "bturb"@en ;
  rdfs:domain cim:GovHydroDD ;
  rdfs:range cim:PU ;
  skos:definition "Turbine denominator multiplier (<i>Bturb</i>) (see parameter detail 3).  Typical value = 0,5."@en .

cim:GovHydroDD.db1 a owl:DatatypeProperty ;
  rdfs:label "db1"@en ;
  rdfs:domain cim:GovHydroDD ;
  rdfs:range cim:Frequency ;
  skos:definition "Intentional dead-band width (<i>db1</i>).  Unit = Hz.  Typical value = 0."@en .

cim:GovHydroDD.db2 a owl:DatatypeProperty ;
  rdfs:label "db2"@en ;
  rdfs:domain cim:GovHydroDD ;
  rdfs:range cim:ActivePower ;
  skos:definition "Unintentional dead-band (<i>db2</i>).  Unit = MW.  Typical value = 0."@en .

cim:GovHydroDD.eps a owl:DatatypeProperty ;
  rdfs:label "eps"@en ;
  rdfs:domain cim:GovHydroDD ;
  rdfs:range cim:Frequency ;
  skos:definition "Intentional db hysteresis (<i>eps</i>).  Unit = Hz.  Typical value = 0."@en .

cim:GovHydroDD.gmax a owl:DatatypeProperty ;
  rdfs:label "gmax"@en ;
  rdfs:domain cim:GovHydroDD ;
  rdfs:range cim:PU ;
  skos:definition "Maximum gate opening (<i>Gmax</i>) (&gt; GovHydroDD.gmin).  Typical value = 0."@en .

cim:GovHydroDD.gmin a owl:DatatypeProperty ;
  rdfs:label "gmin"@en ;
  rdfs:domain cim:GovHydroDD ;
  rdfs:range cim:PU ;
  skos:definition "Minimum gate opening (<i>Gmin</i>) (&lt; GovHydroDD.gmax).  Typical value = 0."@en .

cim:GovHydroDD.gv1 a owl:DatatypeProperty ;
  rdfs:label "gv1"@en ;
  rdfs:domain cim:GovHydroDD ;
  rdfs:range cim:PU ;
  skos:definition "Nonlinear gain point 1, PU gv (<i>Gv1</i>).  Typical value = 0."@en .

cim:GovHydroDD.gv2 a owl:DatatypeProperty ;
  rdfs:label "gv2"@en ;
  rdfs:domain cim:GovHydroDD ;
  rdfs:range cim:PU ;
  skos:definition "Nonlinear gain point 2, PU gv (<i>Gv2</i>).  Typical value = 0."@en .

cim:GovHydroDD.gv3 a owl:DatatypeProperty ;
  rdfs:label "gv3"@en ;
  rdfs:domain cim:GovHydroDD ;
  rdfs:range cim:PU ;
  skos:definition "Nonlinear gain point 3, PU gv (<i>Gv3</i>).  Typical value = 0."@en .

cim:GovHydroDD.gv4 a owl:DatatypeProperty ;
  rdfs:label "gv4"@en ;
  rdfs:domain cim:GovHydroDD ;
  rdfs:range cim:PU ;
  skos:definition "Nonlinear gain point 4, PU gv (<i>Gv4</i>).  Typical value = 0."@en .

cim:GovHydroDD.gv5 a owl:DatatypeProperty ;
  rdfs:label "gv5"@en ;
  rdfs:domain cim:GovHydroDD ;
  rdfs:range cim:PU ;
  skos:definition "Nonlinear gain point 5, PU gv (<i>Gv5</i>).  Typical value = 0."@en .

cim:GovHydroDD.gv6 a owl:DatatypeProperty ;
  rdfs:label "gv6"@en ;
  rdfs:domain cim:GovHydroDD ;
  rdfs:range cim:PU ;
  skos:definition "Nonlinear gain point 6, PU gv (<i>Gv6</i>).  Typical value = 0."@en .

cim:GovHydroDD.inputSignal a owl:DatatypeProperty ;
  rdfs:label "inputSignal"@en ;
  rdfs:domain cim:GovHydroDD ;
  rdfs:range xsd:boolean ;
  skos:definition """
Input signal switch (<i>Flag</i>). 
true = <i>Pe</i> input is used
false = feedback is received from <i>CV</i>.
<i>Flag</i> is normally dependent on <i>Tt</i>.  If <i>Tt</i> is zero, <i>Flag</i> is set to false. If <i>Tt</i> is not zero, <i>Flag</i> is set to true.  
Typical value = true.
\t"""@en .

cim:GovHydroDD.k1 a owl:DatatypeProperty ;
  rdfs:label "k1"@en ;
  rdfs:domain cim:GovHydroDD ;
  rdfs:range cim:PU ;
  skos:definition "Single derivative gain (<i>K1</i>).  Typical value = 3,6."@en .

cim:GovHydroDD.k2 a owl:DatatypeProperty ;
  rdfs:label "k2"@en ;
  rdfs:domain cim:GovHydroDD ;
  rdfs:range cim:PU ;
  skos:definition "Double derivative gain (<i>K2</i>).  Typical value = 0,2."@en .

cim:GovHydroDD.kg a owl:DatatypeProperty ;
  rdfs:label "kg"@en ;
  rdfs:domain cim:GovHydroDD ;
  rdfs:range cim:PU ;
  skos:definition "Gate servo gain (<i>Kg</i>).  Typical value = 3."@en .

cim:GovHydroDD.ki a owl:DatatypeProperty ;
  rdfs:label "ki"@en ;
  rdfs:domain cim:GovHydroDD ;
  rdfs:range cim:PU ;
  skos:definition "Integral gain (<i>Ki</i>).  Typical value = 1."@en .

cim:GovHydroDD.mwbase a owl:DatatypeProperty ;
  rdfs:label "mwbase"@en ;
  rdfs:domain cim:GovHydroDD ;
  rdfs:range cim:ActivePower ;
  skos:definition "Base for power values (<i>MWbase</i>) (&gt;0).  Unit = MW."@en .

cim:GovHydroDD.pgv1 a owl:DatatypeProperty ;
  rdfs:label "pgv1"@en ;
  rdfs:domain cim:GovHydroDD ;
  rdfs:range cim:PU ;
  skos:definition "Nonlinear gain point 1, PU power (<i>Pgv1</i>).  Typical value = 0."@en .

cim:GovHydroDD.pgv2 a owl:DatatypeProperty ;
  rdfs:label "pgv2"@en ;
  rdfs:domain cim:GovHydroDD ;
  rdfs:range cim:PU ;
  skos:definition "Nonlinear gain point 2, PU power (<i>Pgv2</i>).  Typical value = 0."@en .

cim:GovHydroDD.pgv3 a owl:DatatypeProperty ;
  rdfs:label "pgv3"@en ;
  rdfs:domain cim:GovHydroDD ;
  rdfs:range cim:PU ;
  skos:definition "Nonlinear gain point 3, PU power (<i>Pgv3</i>).  Typical value = 0."@en .

cim:GovHydroDD.pgv4 a owl:DatatypeProperty ;
  rdfs:label "pgv4"@en ;
  rdfs:domain cim:GovHydroDD ;
  rdfs:range cim:PU ;
  skos:definition "Nonlinear gain point 4, PU power (<i>Pgv4</i>).  Typical value = 0."@en .

cim:GovHydroDD.pgv5 a owl:DatatypeProperty ;
  rdfs:label "pgv5"@en ;
  rdfs:domain cim:GovHydroDD ;
  rdfs:range cim:PU ;
  skos:definition "Nonlinear gain point 5, PU power (<i>Pgv5</i>).  Typical value = 0."@en .

cim:GovHydroDD.pgv6 a owl:DatatypeProperty ;
  rdfs:label "pgv6"@en ;
  rdfs:domain cim:GovHydroDD ;
  rdfs:range cim:PU ;
  skos:definition "Nonlinear gain point 6, PU power (<i>Pgv6</i>).  Typical value = 0."@en .

cim:GovHydroDD.pmax a owl:DatatypeProperty ;
  rdfs:label "pmax"@en ;
  rdfs:domain cim:GovHydroDD ;
  rdfs:range cim:PU ;
  skos:definition "Maximum gate opening, PU of <i>MWbase</i> (<i>Pmax</i>) (&gt; GovHydroDD.pmin).  Typical value = 1."@en .

cim:GovHydroDD.pmin a owl:DatatypeProperty ;
  rdfs:label "pmin"@en ;
  rdfs:domain cim:GovHydroDD ;
  rdfs:range cim:PU ;
  skos:definition "Minimum gate opening, PU of <i>MWbase</i> (<i>Pmin</i>) (&gt; GovHydroDD.pmax).  Typical value = 0."@en .

cim:GovHydroDD.r a owl:DatatypeProperty ;
  rdfs:label "r"@en ;
  rdfs:domain cim:GovHydroDD ;
  rdfs:range cim:PU ;
  skos:definition "Steady state droop (<i>R</i>).  Typical value = 0,05."@en .

cim:GovHydroDD.td a owl:DatatypeProperty ;
  rdfs:label "td"@en ;
  rdfs:domain cim:GovHydroDD ;
  rdfs:range cim:Seconds ;
  skos:definition "Input filter time constant (<i>Td</i>) (&gt;= 0).  If = 0, block is bypassed.  Typical value = 0."@en .

cim:GovHydroDD.tf a owl:DatatypeProperty ;
  rdfs:label "tf"@en ;
  rdfs:domain cim:GovHydroDD ;
  rdfs:range cim:Seconds ;
  skos:definition "Washout time constant (<i>Tf</i>) (&gt;= 0).  Typical value = 0,1."@en .

cim:GovHydroDD.tp a owl:DatatypeProperty ;
  rdfs:label "tp"@en ;
  rdfs:domain cim:GovHydroDD ;
  rdfs:range cim:Seconds ;
  skos:definition "Gate servo time constant (<i>Tp</i>) (&gt;= 0).  If = 0, block is bypassed.  Typical value = 0,35."@en .

cim:GovHydroDD.tt a owl:DatatypeProperty ;
  rdfs:label "tt"@en ;
  rdfs:domain cim:GovHydroDD ;
  rdfs:range cim:Seconds ;
  skos:definition "Power feedback time constant (<i>Tt</i>) (&gt;= 0).  If = 0, block is bypassed.  Typical value = 0,02."@en .

cim:GovHydroDD.tturb a owl:DatatypeProperty ;
  rdfs:label "tturb"@en ;
  rdfs:domain cim:GovHydroDD ;
  rdfs:range cim:Seconds ;
  skos:definition "Turbine time constant (<i>Tturb</i>)  (&gt;= 0).  See parameter detail 3.  Typical value = 0,8."@en .

cim:GovHydroDD.velcl a owl:DatatypeProperty ;
  rdfs:label "velcl"@en ;
  rdfs:domain cim:GovHydroDD ;
  rdfs:range xsd:float ;
  skos:definition "Maximum gate closing velocity (<i>Velcl</i>).  Unit = PU / s.  Typical value = -0,14."@en .

cim:GovHydroDD.velop a owl:DatatypeProperty ;
  rdfs:label "velop"@en ;
  rdfs:domain cim:GovHydroDD ;
  rdfs:range xsd:float ;
  skos:definition "Maximum gate opening velocity (<i>Velop</i>).  Unit = PU / s.  Typical value = 0,09."@en .

cim:GovHydroFrancis.am a owl:DatatypeProperty ;
  rdfs:label "am"@en ;
  rdfs:domain cim:GovHydroFrancis ;
  rdfs:range cim:PU ;
  skos:definition "Opening section <i>S</i><i><sub>EFF</sub></i> at the maximum efficiency (<i>Am</i>).  Typical value = 0,7."@en .

cim:GovHydroFrancis.av0 a owl:DatatypeProperty ;
  rdfs:label "av0"@en ;
  rdfs:domain cim:GovHydroFrancis ;
  rdfs:range cim:Area ;
  skos:definition "Area of the surge tank (<i>A</i><i><sub>V0</sub></i>). Unit = m<sup>2</sup>. Typical value = 30."@en .

cim:GovHydroFrancis.av1 a owl:DatatypeProperty ;
  rdfs:label "av1"@en ;
  rdfs:domain cim:GovHydroFrancis ;
  rdfs:range cim:Area ;
  skos:definition "Area of the compensation tank (<i>A</i><i><sub>V1</sub></i>). Unit = m<sup>2</sup>. Typical value = 700."@en .

cim:GovHydroFrancis.bp a owl:DatatypeProperty ;
  rdfs:label "bp"@en ;
  rdfs:domain cim:GovHydroFrancis ;
  rdfs:range cim:PU ;
  skos:definition "Droop (<i>Bp</i>).  Typical value = 0,05."@en .

cim:GovHydroFrancis.db1 a owl:DatatypeProperty ;
  rdfs:label "db1"@en ;
  rdfs:domain cim:GovHydroFrancis ;
  rdfs:range cim:Frequency ;
  skos:definition "Intentional dead-band width (<i>DB1</i>).  Unit = Hz.  Typical value = 0."@en .

cim:GovHydroFrancis.etamax a owl:DatatypeProperty ;
  rdfs:label "etamax"@en ;
  rdfs:domain cim:GovHydroFrancis ;
  rdfs:range cim:PU ;
  skos:definition "Maximum efficiency (<i>EtaMax</i>).  Typical value = 1,05."@en .

cim:GovHydroFrancis.governorControl a owl:DatatypeProperty ;
  rdfs:label "governorControl"@en ;
  rdfs:domain cim:GovHydroFrancis ;
  rdfs:range cim:FrancisGovernorControlKind ;
  skos:definition "Governor control flag (<i>Cflag</i>).  Typical value = mechanicHydrolicTachoAccelerator."@en .

cim:GovHydroFrancis.h1 a owl:DatatypeProperty ;
  rdfs:label "h1"@en ;
  rdfs:domain cim:GovHydroFrancis ;
  rdfs:range cim:Length ;
  skos:definition "Head of compensation chamber water level with respect to the level of penstock (<i>H</i><i><sub>1</sub></i>).  Unit = km.  Typical value = 0,004."@en .

cim:GovHydroFrancis.h2 a owl:DatatypeProperty ;
  rdfs:label "h2"@en ;
  rdfs:domain cim:GovHydroFrancis ;
  rdfs:range cim:Length ;
  skos:definition "Head of surge tank water level with respect to the level of penstock (<i>H</i><i><sub>2</sub></i>).  Unit = km.  Typical value = 0,040."@en .

cim:GovHydroFrancis.hn a owl:DatatypeProperty ;
  rdfs:label "hn"@en ;
  rdfs:domain cim:GovHydroFrancis ;
  rdfs:range cim:Length ;
  skos:definition "Rated hydraulic head (<i>H</i><i><sub>n</sub></i>).  Unit = km.  Typical value = 0,250."@en .

cim:GovHydroFrancis.kc a owl:DatatypeProperty ;
  rdfs:label "kc"@en ;
  rdfs:domain cim:GovHydroFrancis ;
  rdfs:range cim:PU ;
  skos:definition "Penstock loss coefficient (due to friction) (<i>Kc</i>).  Typical value = 0,025."@en .

cim:GovHydroFrancis.kg a owl:DatatypeProperty ;
  rdfs:label "kg"@en ;
  rdfs:domain cim:GovHydroFrancis ;
  rdfs:range cim:PU ;
  skos:definition "Water tunnel and surge chamber loss coefficient (due to friction) (<i>Kg</i>).  Typical value = 0,025."@en .

cim:GovHydroFrancis.kt a owl:DatatypeProperty ;
  rdfs:label "kt"@en ;
  rdfs:domain cim:GovHydroFrancis ;
  rdfs:range cim:PU ;
  skos:definition "Washout gain (<i>Kt</i>).  Typical value = 0,25."@en .

cim:GovHydroFrancis.qc0 a owl:DatatypeProperty ;
  rdfs:label "qc0"@en ;
  rdfs:domain cim:GovHydroFrancis ;
  rdfs:range cim:PU ;
  skos:definition "No-load turbine flow at nominal head (<i>Qc0</i>).  Typical value = 0,1."@en .

cim:GovHydroFrancis.qn a owl:DatatypeProperty ;
  rdfs:label "qn"@en ;
  rdfs:domain cim:GovHydroFrancis ;
  rdfs:range cim:VolumeFlowRate ;
  skos:definition "Rated flow (<i>Q</i><i><sub>n</sub></i>). Unit = m<sup>3</sup>/s. Typical value = 250."@en .

cim:GovHydroFrancis.ta a owl:DatatypeProperty ;
  rdfs:label "ta"@en ;
  rdfs:domain cim:GovHydroFrancis ;
  rdfs:range cim:Seconds ;
  skos:definition "Derivative gain (<i>Ta</i>) (&gt;= 0).  Typical value = 3."@en .

cim:GovHydroFrancis.td a owl:DatatypeProperty ;
  rdfs:label "td"@en ;
  rdfs:domain cim:GovHydroFrancis ;
  rdfs:range cim:Seconds ;
  skos:definition "Washout time constant (<i>Td</i>) (&gt;= 0).  Typical value = 6."@en .

cim:GovHydroFrancis.ts a owl:DatatypeProperty ;
  rdfs:label "ts"@en ;
  rdfs:domain cim:GovHydroFrancis ;
  rdfs:range cim:Seconds ;
  skos:definition "Gate servo time constant (<i>Ts</i>) (&gt;= 0).  Typical value = 0,5."@en .

cim:GovHydroFrancis.twnc a owl:DatatypeProperty ;
  rdfs:label "twnc"@en ;
  rdfs:domain cim:GovHydroFrancis ;
  rdfs:range cim:Seconds ;
  skos:definition "Water inertia time constant (<i>Twnc</i>) (&gt;= 0).  Typical value = 1."@en .

cim:GovHydroFrancis.twng a owl:DatatypeProperty ;
  rdfs:label "twng"@en ;
  rdfs:domain cim:GovHydroFrancis ;
  rdfs:range cim:Seconds ;
  skos:definition "Water tunnel and surge chamber inertia time constant (<i>Twng</i>) (&gt;= 0). Typical value = 3."@en .

cim:GovHydroFrancis.tx a owl:DatatypeProperty ;
  rdfs:label "tx"@en ;
  rdfs:domain cim:GovHydroFrancis ;
  rdfs:range cim:Seconds ;
  skos:definition "Derivative feedback gain (<i>Tx</i>) (&gt;= 0).  Typical value = 1."@en .

cim:GovHydroFrancis.va a owl:DatatypeProperty ;
  rdfs:label "va"@en ;
  rdfs:domain cim:GovHydroFrancis ;
  rdfs:range xsd:float ;
  skos:definition "Maximum gate opening velocity (<i>Va</i>).  Unit = PU / s.  Typical value = 0,06."@en .

cim:GovHydroFrancis.valvmax a owl:DatatypeProperty ;
  rdfs:label "valvmax"@en ;
  rdfs:domain cim:GovHydroFrancis ;
  rdfs:range cim:PU ;
  skos:definition "Maximum gate opening (<i>ValvMax</i>) (&gt; GovHydroFrancis.valvmin).  Typical value = 1,1."@en .

cim:GovHydroFrancis.valvmin a owl:DatatypeProperty ;
  rdfs:label "valvmin"@en ;
  rdfs:domain cim:GovHydroFrancis ;
  rdfs:range cim:PU ;
  skos:definition "Minimum gate opening (<i>ValvMin</i>) (&lt; GovHydroFrancis.valvmax).  Typical value = 0."@en .

cim:GovHydroFrancis.vc a owl:DatatypeProperty ;
  rdfs:label "vc"@en ;
  rdfs:domain cim:GovHydroFrancis ;
  rdfs:range xsd:float ;
  skos:definition "Maximum gate closing velocity (<i>Vc</i>).  Unit = PU / s.  Typical value = -0,06."@en .

cim:GovHydroFrancis.waterTunnelSurgeChamberSimulation a owl:DatatypeProperty ;
  rdfs:label "waterTunnelSurgeChamberSimulation"@en ;
  rdfs:domain cim:GovHydroFrancis ;
  rdfs:range xsd:boolean ;
  skos:definition """
Water tunnel and surge chamber simulation (<i>Tflag</i>).
true = enable of water tunnel and surge chamber simulation
false = inhibit of water tunnel and surge chamber simulation.
Typical value = false.
\t"""@en .

cim:GovHydroFrancis.zsfc a owl:DatatypeProperty ;
  rdfs:label "zsfc"@en ;
  rdfs:domain cim:GovHydroFrancis ;
  rdfs:range cim:Length ;
  skos:definition "Head of upper water level with respect to the level of penstock (<i>Zsfc</i>). Unit = km.  Typical value = 0,025."@en .

cim:GovHydroIEEE0.k a owl:DatatypeProperty ;
  rdfs:label "k"@en ;
  rdfs:domain cim:GovHydroIEEE0 ;
  rdfs:range cim:PU ;
  skos:definition "Governor gain (<i>K)</i>."@en .

cim:GovHydroIEEE0.mwbase a owl:DatatypeProperty ;
  rdfs:label "mwbase"@en ;
  rdfs:domain cim:GovHydroIEEE0 ;
  rdfs:range cim:ActivePower ;
  skos:definition "Base for power values (<i>MWbase</i>) (&gt; 0).  Unit = MW."@en .

cim:GovHydroIEEE0.pmax a owl:DatatypeProperty ;
  rdfs:label "pmax"@en ;
  rdfs:domain cim:GovHydroIEEE0 ;
  rdfs:range cim:PU ;
  skos:definition "Gate maximum (<i>Pmax</i>) (&gt; GovHydroIEEE0.pmin). "@en .

cim:GovHydroIEEE0.pmin a owl:DatatypeProperty ;
  rdfs:label "pmin"@en ;
  rdfs:domain cim:GovHydroIEEE0 ;
  rdfs:range cim:PU ;
  skos:definition "Gate minimum (<i>Pmin</i>) (&lt; GovHydroIEEE.pmax). "@en .

cim:GovHydroIEEE0.t1 a owl:DatatypeProperty ;
  rdfs:label "t1"@en ;
  rdfs:domain cim:GovHydroIEEE0 ;
  rdfs:range cim:Seconds ;
  skos:definition "Governor lag time constant (<i>T1</i>) (&gt;= 0).  Typical value = 0,25."@en .

cim:GovHydroIEEE0.t2 a owl:DatatypeProperty ;
  rdfs:label "t2"@en ;
  rdfs:domain cim:GovHydroIEEE0 ;
  rdfs:range cim:Seconds ;
  skos:definition "Governor lead time constant (<i>T2)</i> (&gt;= 0).  Typical value = 0."@en .

cim:GovHydroIEEE0.t3 a owl:DatatypeProperty ;
  rdfs:label "t3"@en ;
  rdfs:domain cim:GovHydroIEEE0 ;
  rdfs:range cim:Seconds ;
  skos:definition "Gate actuator time constant (<i>T3</i>) (&gt;= 0).  Typical value = 0,1."@en .

cim:GovHydroIEEE0.t4 a owl:DatatypeProperty ;
  rdfs:label "t4"@en ;
  rdfs:domain cim:GovHydroIEEE0 ;
  rdfs:range cim:Seconds ;
  skos:definition "Water starting time (<i>T4</i>) (&gt;= 0). "@en .

cim:GovHydroIEEE2.aturb a owl:DatatypeProperty ;
  rdfs:label "aturb"@en ;
  rdfs:domain cim:GovHydroIEEE2 ;
  rdfs:range cim:PU ;
  skos:definition "Turbine numerator multiplier (<i>Aturb</i>).  Typical value = -1."@en .

cim:GovHydroIEEE2.bturb a owl:DatatypeProperty ;
  rdfs:label "bturb"@en ;
  rdfs:domain cim:GovHydroIEEE2 ;
  rdfs:range cim:PU ;
  skos:definition "Turbine denominator multiplier (<i>Bturb</i>) (&gt; 0).  Typical value = 0,5."@en .

cim:GovHydroIEEE2.gv1 a owl:DatatypeProperty ;
  rdfs:label "gv1"@en ;
  rdfs:domain cim:GovHydroIEEE2 ;
  rdfs:range cim:PU ;
  skos:definition "Nonlinear gain point 1, PU gv (<i>Gv1</i>).  Typical value = 0."@en .

cim:GovHydroIEEE2.gv2 a owl:DatatypeProperty ;
  rdfs:label "gv2"@en ;
  rdfs:domain cim:GovHydroIEEE2 ;
  rdfs:range cim:PU ;
  skos:definition "Nonlinear gain point 2, PU gv (<i>Gv2</i>).  Typical value = 0."@en .

cim:GovHydroIEEE2.gv3 a owl:DatatypeProperty ;
  rdfs:label "gv3"@en ;
  rdfs:domain cim:GovHydroIEEE2 ;
  rdfs:range cim:PU ;
  skos:definition "Nonlinear gain point 3, PU gv (<i>Gv3</i>).  Typical value = 0."@en .

cim:GovHydroIEEE2.gv4 a owl:DatatypeProperty ;
  rdfs:label "gv4"@en ;
  rdfs:domain cim:GovHydroIEEE2 ;
  rdfs:range cim:PU ;
  skos:definition "Nonlinear gain point 4, PU gv (<i>Gv4</i>).  Typical value = 0."@en .

cim:GovHydroIEEE2.gv5 a owl:DatatypeProperty ;
  rdfs:label "gv5"@en ;
  rdfs:domain cim:GovHydroIEEE2 ;
  rdfs:range cim:PU ;
  skos:definition "Nonlinear gain point 5, PU gv (<i>Gv5</i>).  Typical value = 0."@en .

cim:GovHydroIEEE2.gv6 a owl:DatatypeProperty ;
  rdfs:label "gv6"@en ;
  rdfs:domain cim:GovHydroIEEE2 ;
  rdfs:range cim:PU ;
  skos:definition "Nonlinear gain point 6, PU gv (<i>Gv6</i>).  Typical value = 0."@en .

cim:GovHydroIEEE2.kturb a owl:DatatypeProperty ;
  rdfs:label "kturb"@en ;
  rdfs:domain cim:GovHydroIEEE2 ;
  rdfs:range cim:PU ;
  skos:definition "Turbine gain (<i>Kturb</i>).  Typical value = 1."@en .

cim:GovHydroIEEE2.mwbase a owl:DatatypeProperty ;
  rdfs:label "mwbase"@en ;
  rdfs:domain cim:GovHydroIEEE2 ;
  rdfs:range cim:ActivePower ;
  skos:definition "Base for power values (<i>MWbase</i>) (&gt; 0).  Unit = MW."@en .

cim:GovHydroIEEE2.pgv1 a owl:DatatypeProperty ;
  rdfs:label "pgv1"@en ;
  rdfs:domain cim:GovHydroIEEE2 ;
  rdfs:range cim:PU ;
  skos:definition "Nonlinear gain point 1, PU power (<i>Pgv1</i>).  Typical value = 0."@en .

cim:GovHydroIEEE2.pgv2 a owl:DatatypeProperty ;
  rdfs:label "pgv2"@en ;
  rdfs:domain cim:GovHydroIEEE2 ;
  rdfs:range cim:PU ;
  skos:definition "Nonlinear gain point 2, PU power (<i>Pgv2</i>).  Typical value = 0."@en .

cim:GovHydroIEEE2.pgv3 a owl:DatatypeProperty ;
  rdfs:label "pgv3"@en ;
  rdfs:domain cim:GovHydroIEEE2 ;
  rdfs:range cim:PU ;
  skos:definition "Nonlinear gain point 3, PU power (<i>Pgv3</i>).  Typical value = 0."@en .

cim:GovHydroIEEE2.pgv4 a owl:DatatypeProperty ;
  rdfs:label "pgv4"@en ;
  rdfs:domain cim:GovHydroIEEE2 ;
  rdfs:range cim:PU ;
  skos:definition "Nonlinear gain point 4, PU power (<i>Pgv4</i>).  Typical value = 0."@en .

cim:GovHydroIEEE2.pgv5 a owl:DatatypeProperty ;
  rdfs:label "pgv5"@en ;
  rdfs:domain cim:GovHydroIEEE2 ;
  rdfs:range cim:PU ;
  skos:definition "Nonlinear gain point 5, PU power (<i>Pgv5</i>).  Typical value = 0."@en .

cim:GovHydroIEEE2.pgv6 a owl:DatatypeProperty ;
  rdfs:label "pgv6"@en ;
  rdfs:domain cim:GovHydroIEEE2 ;
  rdfs:range cim:PU ;
  skos:definition "Nonlinear gain point 6, PU power (<i>Pgv6</i>).  Typical value = 0."@en .

cim:GovHydroIEEE2.pmax a owl:DatatypeProperty ;
  rdfs:label "pmax"@en ;
  rdfs:domain cim:GovHydroIEEE2 ;
  rdfs:range cim:PU ;
  skos:definition "Maximum gate opening (<i>Pmax</i>) (&gt; GovHydroIEEE2.pmin).  Typical value = 1."@en .

cim:GovHydroIEEE2.pmin a owl:DatatypeProperty ;
  rdfs:label "pmin"@en ;
  rdfs:domain cim:GovHydroIEEE2 ;
  rdfs:range cim:PU ;
  skos:definition "Minimum gate opening (<i>Pmin</i>) (&lt;GovHydroIEEE2.pmax).  Typical value = 0."@en .

cim:GovHydroIEEE2.rperm a owl:DatatypeProperty ;
  rdfs:label "rperm"@en ;
  rdfs:domain cim:GovHydroIEEE2 ;
  rdfs:range cim:PU ;
  skos:definition "Permanent droop (<i>Rperm</i>).  Typical value = 0,05."@en .

cim:GovHydroIEEE2.rtemp a owl:DatatypeProperty ;
  rdfs:label "rtemp"@en ;
  rdfs:domain cim:GovHydroIEEE2 ;
  rdfs:range cim:PU ;
  skos:definition "Temporary droop (<i>Rtemp</i>).  Typical value = 0,5."@en .

cim:GovHydroIEEE2.tg a owl:DatatypeProperty ;
  rdfs:label "tg"@en ;
  rdfs:domain cim:GovHydroIEEE2 ;
  rdfs:range cim:Seconds ;
  skos:definition "Gate servo time constant (<i>Tg</i>) (&gt;= 0).  Typical value = 0,5."@en .

cim:GovHydroIEEE2.tp a owl:DatatypeProperty ;
  rdfs:label "tp"@en ;
  rdfs:domain cim:GovHydroIEEE2 ;
  rdfs:range cim:Seconds ;
  skos:definition "Pilot servo valve time constant (<i>Tp</i>) (&gt;= 0).  Typical value = 0,03."@en .

cim:GovHydroIEEE2.tr a owl:DatatypeProperty ;
  rdfs:label "tr"@en ;
  rdfs:domain cim:GovHydroIEEE2 ;
  rdfs:range cim:Seconds ;
  skos:definition "Dashpot time constant (<i>Tr</i>) (&gt;= 0).  Typical value = 12."@en .

cim:GovHydroIEEE2.tw a owl:DatatypeProperty ;
  rdfs:label "tw"@en ;
  rdfs:domain cim:GovHydroIEEE2 ;
  rdfs:range cim:Seconds ;
  skos:definition "Water inertia time constant (<i>Tw</i>) (&gt;= 0).  Typical value = 2."@en .

cim:GovHydroIEEE2.uc a owl:DatatypeProperty ;
  rdfs:label "uc"@en ;
  rdfs:domain cim:GovHydroIEEE2 ;
  rdfs:range xsd:float ;
  skos:definition "Maximum gate closing velocity (<i>Uc</i>) (&lt;0).  Typical value = -0,1."@en .

cim:GovHydroIEEE2.uo a owl:DatatypeProperty ;
  rdfs:label "uo"@en ;
  rdfs:domain cim:GovHydroIEEE2 ;
  rdfs:range xsd:float ;
  skos:definition "Maximum gate opening velocity (<i>Uo</i>).  Unit = PU / s.  Typical value = 0,1."@en .

cim:GovHydroPID.aturb a owl:DatatypeProperty ;
  rdfs:label "aturb"@en ;
  rdfs:domain cim:GovHydroPID ;
  rdfs:range cim:PU ;
  skos:definition "Turbine numerator multiplier (<i>Aturb</i>) (see parameter detail 3).  Typical value -1."@en .

cim:GovHydroPID.bturb a owl:DatatypeProperty ;
  rdfs:label "bturb"@en ;
  rdfs:domain cim:GovHydroPID ;
  rdfs:range cim:PU ;
  skos:definition "Turbine denominator multiplier (<i>Bturb</i>) (see parameter detail 3).  Typical value = 0,5."@en .

cim:GovHydroPID.db1 a owl:DatatypeProperty ;
  rdfs:label "db1"@en ;
  rdfs:domain cim:GovHydroPID ;
  rdfs:range cim:Frequency ;
  skos:definition "Intentional dead-band width (<i>db1</i>).  Unit = Hz.  Typical value = 0."@en .

cim:GovHydroPID.db2 a owl:DatatypeProperty ;
  rdfs:label "db2"@en ;
  rdfs:domain cim:GovHydroPID ;
  rdfs:range cim:ActivePower ;
  skos:definition "Unintentional dead-band (<i>db2</i>).  Unit = MW.  Typical value = 0."@en .

cim:GovHydroPID.eps a owl:DatatypeProperty ;
  rdfs:label "eps"@en ;
  rdfs:domain cim:GovHydroPID ;
  rdfs:range cim:Frequency ;
  skos:definition "Intentional db hysteresis (<i>eps</i>).  Unit = Hz.  Typical value = 0."@en .

cim:GovHydroPID.gv1 a owl:DatatypeProperty ;
  rdfs:label "gv1"@en ;
  rdfs:domain cim:GovHydroPID ;
  rdfs:range cim:PU ;
  skos:definition "Nonlinear gain point 1, PU gv (<i>Gv1</i>).  Typical value = 0."@en .

cim:GovHydroPID.gv2 a owl:DatatypeProperty ;
  rdfs:label "gv2"@en ;
  rdfs:domain cim:GovHydroPID ;
  rdfs:range cim:PU ;
  skos:definition "Nonlinear gain point 2, PU gv (<i>Gv2</i>).  Typical value = 0."@en .

cim:GovHydroPID.gv3 a owl:DatatypeProperty ;
  rdfs:label "gv3"@en ;
  rdfs:domain cim:GovHydroPID ;
  rdfs:range cim:PU ;
  skos:definition "Nonlinear gain point 3, PU gv (<i>Gv3</i>).  Typical value = 0."@en .

cim:GovHydroPID.gv4 a owl:DatatypeProperty ;
  rdfs:label "gv4"@en ;
  rdfs:domain cim:GovHydroPID ;
  rdfs:range cim:PU ;
  skos:definition "Nonlinear gain point 4, PU gv (<i>Gv4</i>).  Typical value = 0."@en .

cim:GovHydroPID.gv5 a owl:DatatypeProperty ;
  rdfs:label "gv5"@en ;
  rdfs:domain cim:GovHydroPID ;
  rdfs:range cim:PU ;
  skos:definition "Nonlinear gain point 5, PU gv (<i>Gv5</i>).  Typical value = 0."@en .

cim:GovHydroPID.gv6 a owl:DatatypeProperty ;
  rdfs:label "gv6"@en ;
  rdfs:domain cim:GovHydroPID ;
  rdfs:range cim:PU ;
  skos:definition "Nonlinear gain point 6, PU gv (<i>Gv6</i>).  Typical value = 0."@en .

cim:GovHydroPID.inputSignal a owl:DatatypeProperty ;
  rdfs:label "inputSignal"@en ;
  rdfs:domain cim:GovHydroPID ;
  rdfs:range xsd:boolean ;
  skos:definition """
Input signal switch (<i>Flag</i>). 
true = <i>Pe</i> input is used
false = feedback is received from <i>CV</i>.
<i>Flag</i> is normally dependent on <i>Tt</i>.  If <i>Tt </i>is zero, <i>Flag</i> is set to false. If <i>Tt</i> is not zero, <i>Flag</i> is set to true.  
Typical value = true.
\t"""@en .

cim:GovHydroPID.kd a owl:DatatypeProperty ;
  rdfs:label "kd"@en ;
  rdfs:domain cim:GovHydroPID ;
  rdfs:range cim:PU ;
  skos:definition "Derivative gain (<i>Kd</i>).  Typical value = 1,11."@en .

cim:GovHydroPID.kg a owl:DatatypeProperty ;
  rdfs:label "kg"@en ;
  rdfs:domain cim:GovHydroPID ;
  rdfs:range cim:PU ;
  skos:definition "Gate servo gain (<i>Kg</i>).  Typical value = 2,5."@en .

cim:GovHydroPID.ki a owl:DatatypeProperty ;
  rdfs:label "ki"@en ;
  rdfs:domain cim:GovHydroPID ;
  rdfs:range cim:PU ;
  skos:definition "Integral gain (<i>Ki</i>).  Typical value = 0,36."@en .

cim:GovHydroPID.kp a owl:DatatypeProperty ;
  rdfs:label "kp"@en ;
  rdfs:domain cim:GovHydroPID ;
  rdfs:range cim:PU ;
  skos:definition "Proportional gain (<i>Kp</i>).  Typical value = 0,1."@en .

cim:GovHydroPID.mwbase a owl:DatatypeProperty ;
  rdfs:label "mwbase"@en ;
  rdfs:domain cim:GovHydroPID ;
  rdfs:range cim:ActivePower ;
  skos:definition "Base for power values (<i>MWbase</i>) (&gt; 0).  Unit = MW."@en .

cim:GovHydroPID.pgv1 a owl:DatatypeProperty ;
  rdfs:label "pgv1"@en ;
  rdfs:domain cim:GovHydroPID ;
  rdfs:range cim:PU ;
  skos:definition "Nonlinear gain point 1, PU power (<i>Pgv1</i>).  Typical value = 0."@en .

cim:GovHydroPID.pgv2 a owl:DatatypeProperty ;
  rdfs:label "pgv2"@en ;
  rdfs:domain cim:GovHydroPID ;
  rdfs:range cim:PU ;
  skos:definition "Nonlinear gain point 2, PU power (<i>Pgv2</i>).  Typical value = 0."@en .

cim:GovHydroPID.pgv3 a owl:DatatypeProperty ;
  rdfs:label "pgv3"@en ;
  rdfs:domain cim:GovHydroPID ;
  rdfs:range cim:PU ;
  skos:definition "Nonlinear gain point 3, PU power (<i>Pgv3</i>).  Typical value = 0."@en .

cim:GovHydroPID.pgv4 a owl:DatatypeProperty ;
  rdfs:label "pgv4"@en ;
  rdfs:domain cim:GovHydroPID ;
  rdfs:range cim:PU ;
  skos:definition "Nonlinear gain point 4, PU power (<i>Pgv4</i>).  Typical value = 0."@en .

cim:GovHydroPID.pgv5 a owl:DatatypeProperty ;
  rdfs:label "pgv5"@en ;
  rdfs:domain cim:GovHydroPID ;
  rdfs:range cim:PU ;
  skos:definition "Nonlinear gain point 5, PU power (<i>Pgv5</i>).  Typical value = 0."@en .

cim:GovHydroPID.pgv6 a owl:DatatypeProperty ;
  rdfs:label "pgv6"@en ;
  rdfs:domain cim:GovHydroPID ;
  rdfs:range cim:PU ;
  skos:definition "Nonlinear gain point 6, PU power (<i>Pgv6</i>).  Typical value = 0."@en .

cim:GovHydroPID.pmax a owl:DatatypeProperty ;
  rdfs:label "pmax"@en ;
  rdfs:domain cim:GovHydroPID ;
  rdfs:range cim:PU ;
  skos:definition "Maximum gate opening, PU of MWbase (<i>Pmax</i>) (&gt; GovHydroPID.pmin).  Typical value = 1."@en .

cim:GovHydroPID.pmin a owl:DatatypeProperty ;
  rdfs:label "pmin"@en ;
  rdfs:domain cim:GovHydroPID ;
  rdfs:range cim:PU ;
  skos:definition "Minimum gate opening, PU of MWbase (<i>Pmin</i>) (&lt; GovHydroPID.pmax).  Typical value = 0."@en .

cim:GovHydroPID.r a owl:DatatypeProperty ;
  rdfs:label "r"@en ;
  rdfs:domain cim:GovHydroPID ;
  rdfs:range cim:PU ;
  skos:definition "Steady state droop (<i>R</i>).  Typical value = 0,05."@en .

cim:GovHydroPID.td a owl:DatatypeProperty ;
  rdfs:label "td"@en ;
  rdfs:domain cim:GovHydroPID ;
  rdfs:range cim:Seconds ;
  skos:definition "Input filter time constant (<i>Td</i>) (&gt;= 0).  If = 0, block is bypassed.  Typical value = 0."@en .

cim:GovHydroPID.tf a owl:DatatypeProperty ;
  rdfs:label "tf"@en ;
  rdfs:domain cim:GovHydroPID ;
  rdfs:range cim:Seconds ;
  skos:definition "Washout time constant (<i>Tf</i>) (&gt;= 0).  Typical value = 0,1."@en .

cim:GovHydroPID.tp a owl:DatatypeProperty ;
  rdfs:label "tp"@en ;
  rdfs:domain cim:GovHydroPID ;
  rdfs:range cim:Seconds ;
  skos:definition "Gate servo time constant (<i>Tp</i>) (&gt;= 0).  If = 0, block is bypassed.  Typical value = 0,35."@en .

cim:GovHydroPID.tt a owl:DatatypeProperty ;
  rdfs:label "tt"@en ;
  rdfs:domain cim:GovHydroPID ;
  rdfs:range cim:Seconds ;
  skos:definition "Power feedback time constant (<i>Tt</i>) (&gt;= 0).  If = 0, block is bypassed.  Typical value = 0,02."@en .

cim:GovHydroPID.tturb a owl:DatatypeProperty ;
  rdfs:label "tturb"@en ;
  rdfs:domain cim:GovHydroPID ;
  rdfs:range cim:Seconds ;
  skos:definition "Turbine time constant (<i>Tturb</i>) (&gt;= 0). See Parameter detail 3.  Typical value = 0,8."@en .

cim:GovHydroPID.velcl a owl:DatatypeProperty ;
  rdfs:label "velcl"@en ;
  rdfs:domain cim:GovHydroPID ;
  rdfs:range xsd:float ;
  skos:definition "Maximum gate closing velocity (<i>Velcl</i>).  Unit = PU / s.  Typical value = -0,14."@en .

cim:GovHydroPID.velop a owl:DatatypeProperty ;
  rdfs:label "velop"@en ;
  rdfs:domain cim:GovHydroPID ;
  rdfs:range xsd:float ;
  skos:definition "Maximum gate opening velocity (<i>Velop</i>).  Unit = PU / s.  Typical value = 0,09."@en .

cim:GovHydroPID2.atw a owl:DatatypeProperty ;
  rdfs:label "atw"@en ;
  rdfs:domain cim:GovHydroPID2 ;
  rdfs:range cim:PU ;
  skos:definition "Factor multiplying <i>Tw</i> (<i>Atw</i>).  Typical value = 0."@en .

cim:GovHydroPID2.d a owl:DatatypeProperty ;
  rdfs:label "d"@en ;
  rdfs:domain cim:GovHydroPID2 ;
  rdfs:range cim:PU ;
  skos:definition "Turbine damping factor (<i>D</i>).  Unit = delta P / delta speed.  Typical value = 0."@en .

cim:GovHydroPID2.feedbackSignal a owl:DatatypeProperty ;
  rdfs:label "feedbackSignal"@en ;
  rdfs:domain cim:GovHydroPID2 ;
  rdfs:range xsd:boolean ;
  skos:definition """
Feedback signal type flag (<i>Flag</i>).
true = use gate position feedback signal
false = use Pe.
\t"""@en .

cim:GovHydroPID2.g0 a owl:DatatypeProperty ;
  rdfs:label "g0"@en ;
  rdfs:domain cim:GovHydroPID2 ;
  rdfs:range cim:PU ;
  skos:definition "Gate opening at speed no load (<i>G0</i>).  Typical value = 0."@en .

cim:GovHydroPID2.g1 a owl:DatatypeProperty ;
  rdfs:label "g1"@en ;
  rdfs:domain cim:GovHydroPID2 ;
  rdfs:range cim:PU ;
  skos:definition "Intermediate gate opening (<i>G1</i>).  Typical value = 0."@en .

cim:GovHydroPID2.g2 a owl:DatatypeProperty ;
  rdfs:label "g2"@en ;
  rdfs:domain cim:GovHydroPID2 ;
  rdfs:range cim:PU ;
  skos:definition "Intermediate gate opening (<i>G2</i>).  Typical value = 0."@en .

cim:GovHydroPID2.gmax a owl:DatatypeProperty ;
  rdfs:label "gmax"@en ;
  rdfs:domain cim:GovHydroPID2 ;
  rdfs:range cim:PU ;
  skos:definition "Maximum gate opening (<i>Gmax</i>) (&gt; GovHydroPID2.gmin).  Typical value = 0."@en .

cim:GovHydroPID2.gmin a owl:DatatypeProperty ;
  rdfs:label "gmin"@en ;
  rdfs:domain cim:GovHydroPID2 ;
  rdfs:range cim:PU ;
  skos:definition "Minimum gate opening (<i>Gmin</i>) (&gt; GovHydroPID2.gmax).  Typical value = 0."@en .

cim:GovHydroPID2.kd a owl:DatatypeProperty ;
  rdfs:label "kd"@en ;
  rdfs:domain cim:GovHydroPID2 ;
  rdfs:range cim:PU ;
  skos:definition "Derivative gain (<i>Kd</i>).  Typical value = 0."@en .

cim:GovHydroPID2.ki a owl:DatatypeProperty ;
  rdfs:label "ki"@en ;
  rdfs:domain cim:GovHydroPID2 ;
  rdfs:range xsd:float ;
  skos:definition "Reset gain (<i>Ki</i>).  Unit = PU/s.  Typical value = 0."@en .

cim:GovHydroPID2.kp a owl:DatatypeProperty ;
  rdfs:label "kp"@en ;
  rdfs:domain cim:GovHydroPID2 ;
  rdfs:range cim:PU ;
  skos:definition "Proportional gain (<i>Kp</i>).  Typical value = 0."@en .

cim:GovHydroPID2.mwbase a owl:DatatypeProperty ;
  rdfs:label "mwbase"@en ;
  rdfs:domain cim:GovHydroPID2 ;
  rdfs:range cim:ActivePower ;
  skos:definition "Base for power values (<i>MWbase</i>) (&gt;0).  Unit = MW."@en .

cim:GovHydroPID2.p1 a owl:DatatypeProperty ;
  rdfs:label "p1"@en ;
  rdfs:domain cim:GovHydroPID2 ;
  rdfs:range cim:PU ;
  skos:definition "Power at gate opening <i>G1</i> (<i>P1</i>).  Typical value = 0."@en .

cim:GovHydroPID2.p2 a owl:DatatypeProperty ;
  rdfs:label "p2"@en ;
  rdfs:domain cim:GovHydroPID2 ;
  rdfs:range cim:PU ;
  skos:definition "Power at gate opening G2 (<i>P2</i>).  Typical value = 0."@en .

cim:GovHydroPID2.p3 a owl:DatatypeProperty ;
  rdfs:label "p3"@en ;
  rdfs:domain cim:GovHydroPID2 ;
  rdfs:range cim:PU ;
  skos:definition "Power at full opened gate (<i>P3</i>).  Typical value = 0."@en .

cim:GovHydroPID2.rperm a owl:DatatypeProperty ;
  rdfs:label "rperm"@en ;
  rdfs:domain cim:GovHydroPID2 ;
  rdfs:range cim:PU ;
  skos:definition "Permanent drop (<i>Rperm</i>).  Typical value = 0."@en .

cim:GovHydroPID2.ta a owl:DatatypeProperty ;
  rdfs:label "ta"@en ;
  rdfs:domain cim:GovHydroPID2 ;
  rdfs:range cim:Seconds ;
  skos:definition "Controller time constant (<i>Ta</i>) (&gt;= 0).  Typical value = 0."@en .

cim:GovHydroPID2.tb a owl:DatatypeProperty ;
  rdfs:label "tb"@en ;
  rdfs:domain cim:GovHydroPID2 ;
  rdfs:range cim:Seconds ;
  skos:definition "Gate servo time constant (<i>Tb</i>) (&gt; 0). "@en .

cim:GovHydroPID2.treg a owl:DatatypeProperty ;
  rdfs:label "treg"@en ;
  rdfs:domain cim:GovHydroPID2 ;
  rdfs:range cim:Seconds ;
  skos:definition "Speed detector time constant (<i>Treg</i>) (&gt;= 0).  Typical value = 0."@en .

cim:GovHydroPID2.tw a owl:DatatypeProperty ;
  rdfs:label "tw"@en ;
  rdfs:domain cim:GovHydroPID2 ;
  rdfs:range cim:Seconds ;
  skos:definition "Water inertia time constant (<i>Tw</i>) (&gt;= 0).  Typical value = 0."@en .

cim:GovHydroPID2.velmax a owl:DatatypeProperty ;
  rdfs:label "velmax"@en ;
  rdfs:domain cim:GovHydroPID2 ;
  rdfs:range xsd:float ;
  skos:definition "Maximum gate opening velocity (<i>Velmax</i>) (&lt; GovHydroPID2.velmin).  Unit = PU / s.  Typical value = 0."@en .

cim:GovHydroPID2.velmin a owl:DatatypeProperty ;
  rdfs:label "velmin"@en ;
  rdfs:domain cim:GovHydroPID2 ;
  rdfs:range xsd:float ;
  skos:definition "Maximum gate closing velocity (<i>Velmin</i>) (&gt; GovHydroPID2.velmax).  Unit = PU / s.  Typical value = 0."@en .

cim:GovHydroPelton.av0 a owl:DatatypeProperty ;
  rdfs:label "av0"@en ;
  rdfs:domain cim:GovHydroPelton ;
  rdfs:range cim:Area ;
  skos:definition "Area of the surge tank (<i>A</i><i><sub>V0</sub></i>). Unit = m<sup>2</sup>. Typical value = 30."@en .

cim:GovHydroPelton.av1 a owl:DatatypeProperty ;
  rdfs:label "av1"@en ;
  rdfs:domain cim:GovHydroPelton ;
  rdfs:range cim:Area ;
  skos:definition "Area of the compensation tank (<i>A</i><i><sub>V1</sub></i>). Unit = m<sup>2</sup>. Typical value = 700."@en .

cim:GovHydroPelton.bp a owl:DatatypeProperty ;
  rdfs:label "bp"@en ;
  rdfs:domain cim:GovHydroPelton ;
  rdfs:range cim:PU ;
  skos:definition "Droop (<i>bp</i>).  Typical value = 0,05."@en .

cim:GovHydroPelton.db1 a owl:DatatypeProperty ;
  rdfs:label "db1"@en ;
  rdfs:domain cim:GovHydroPelton ;
  rdfs:range cim:Frequency ;
  skos:definition "Intentional dead-band width (<i>DB1</i>).  Unit = Hz.  Typical value = 0."@en .

cim:GovHydroPelton.db2 a owl:DatatypeProperty ;
  rdfs:label "db2"@en ;
  rdfs:domain cim:GovHydroPelton ;
  rdfs:range cim:Frequency ;
  skos:definition "Intentional dead-band width of valve opening error (<i>DB2</i>). Unit = Hz.  Typical value = 0,01."@en .

cim:GovHydroPelton.h1 a owl:DatatypeProperty ;
  rdfs:label "h1"@en ;
  rdfs:domain cim:GovHydroPelton ;
  rdfs:range cim:Length ;
  skos:definition "Head of compensation chamber water level with respect to the level of penstock (<i>H</i><i><sub>1</sub></i>).  Unit = km.  Typical value = 0,004."@en .

cim:GovHydroPelton.h2 a owl:DatatypeProperty ;
  rdfs:label "h2"@en ;
  rdfs:domain cim:GovHydroPelton ;
  rdfs:range cim:Length ;
  skos:definition "Head of surge tank water level with respect to the level of penstock (<i>H</i><i><sub>2</sub></i>).  Unit = km.  Typical value = 0,040."@en .

cim:GovHydroPelton.hn a owl:DatatypeProperty ;
  rdfs:label "hn"@en ;
  rdfs:domain cim:GovHydroPelton ;
  rdfs:range cim:Length ;
  skos:definition "Rated hydraulic head (<i>H</i><i><sub>n</sub></i>).  Unit = km.  Typical value = 0,250."@en .

cim:GovHydroPelton.kc a owl:DatatypeProperty ;
  rdfs:label "kc"@en ;
  rdfs:domain cim:GovHydroPelton ;
  rdfs:range cim:PU ;
  skos:definition "Penstock loss coefficient (due to friction) (<i>Kc</i>).  Typical value = 0,025."@en .

cim:GovHydroPelton.kg a owl:DatatypeProperty ;
  rdfs:label "kg"@en ;
  rdfs:domain cim:GovHydroPelton ;
  rdfs:range cim:PU ;
  skos:definition "Water tunnel and surge chamber loss coefficient (due to friction) (<i>Kg</i>).  Typical value = 0,025."@en .

cim:GovHydroPelton.qc0 a owl:DatatypeProperty ;
  rdfs:label "qc0"@en ;
  rdfs:domain cim:GovHydroPelton ;
  rdfs:range cim:PU ;
  skos:definition "No-load turbine flow at nominal head (<i>Qc0</i>).  Typical value = 0,05."@en .

cim:GovHydroPelton.qn a owl:DatatypeProperty ;
  rdfs:label "qn"@en ;
  rdfs:domain cim:GovHydroPelton ;
  rdfs:range cim:VolumeFlowRate ;
  skos:definition "Rated flow (<i>Q</i><i><sub>n</sub></i>). Unit = m<sup>3</sup>/s. Typical value = 250."@en .

cim:GovHydroPelton.simplifiedPelton a owl:DatatypeProperty ;
  rdfs:label "simplifiedPelton"@en ;
  rdfs:domain cim:GovHydroPelton ;
  rdfs:range xsd:boolean ;
  skos:definition """
Simplified Pelton model simulation (<i>Sflag</i>).
true = enable of simplified Pelton model simulation
false = enable of complete Pelton model simulation (non-linear gain).
Typical value = true.
\t"""@en .

cim:GovHydroPelton.staticCompensating a owl:DatatypeProperty ;
  rdfs:label "staticCompensating"@en ;
  rdfs:domain cim:GovHydroPelton ;
  rdfs:range xsd:boolean ;
  skos:definition """
Static compensating characteristic (<i>Cflag</i>). It should be true if simplifiedPelton = false.
true = enable of static compensating characteristic 
false = inhibit of static compensating characteristic.
Typical value = false.
\t"""@en .

cim:GovHydroPelton.ta a owl:DatatypeProperty ;
  rdfs:label "ta"@en ;
  rdfs:domain cim:GovHydroPelton ;
  rdfs:range cim:Seconds ;
  skos:definition "Derivative gain (accelerometer time constant) (<i>Ta</i>) (&gt;= 0).  Typical value = 3."@en .

cim:GovHydroPelton.ts a owl:DatatypeProperty ;
  rdfs:label "ts"@en ;
  rdfs:domain cim:GovHydroPelton ;
  rdfs:range cim:Seconds ;
  skos:definition "Gate servo time constant (<i>Ts</i>) (&gt;= 0).  Typical value = 0,15."@en .

cim:GovHydroPelton.tv a owl:DatatypeProperty ;
  rdfs:label "tv"@en ;
  rdfs:domain cim:GovHydroPelton ;
  rdfs:range cim:Seconds ;
  skos:definition "Servomotor integrator time constant (<i>Tv</i>) (&gt;= 0).  Typical value = 0,3."@en .

cim:GovHydroPelton.twnc a owl:DatatypeProperty ;
  rdfs:label "twnc"@en ;
  rdfs:domain cim:GovHydroPelton ;
  rdfs:range cim:Seconds ;
  skos:definition "Water inertia time constant (<i>Twnc</i>) (&gt;= 0).  Typical value = 1."@en .

cim:GovHydroPelton.twng a owl:DatatypeProperty ;
  rdfs:label "twng"@en ;
  rdfs:domain cim:GovHydroPelton ;
  rdfs:range cim:Seconds ;
  skos:definition "Water tunnel and surge chamber inertia time constant (<i>Twng</i>) (&gt;= 0). Typical value = 3."@en .

cim:GovHydroPelton.tx a owl:DatatypeProperty ;
  rdfs:label "tx"@en ;
  rdfs:domain cim:GovHydroPelton ;
  rdfs:range cim:Seconds ;
  skos:definition "Electronic integrator time constant (<i>Tx</i>) (&gt;= 0).  Typical value = 0,5."@en .

cim:GovHydroPelton.va a owl:DatatypeProperty ;
  rdfs:label "va"@en ;
  rdfs:domain cim:GovHydroPelton ;
  rdfs:range xsd:float ;
  skos:definition "Maximum gate opening velocity (<i>Va</i>).  Unit = PU / s.  Typical value = 0,06."@en .

cim:GovHydroPelton.valvmax a owl:DatatypeProperty ;
  rdfs:label "valvmax"@en ;
  rdfs:domain cim:GovHydroPelton ;
  rdfs:range cim:PU ;
  skos:definition "Maximum gate opening (<i>ValvMax</i>) (&gt; GovHydroPelton.valvmin).  Typical value = 1,1."@en .

cim:GovHydroPelton.valvmin a owl:DatatypeProperty ;
  rdfs:label "valvmin"@en ;
  rdfs:domain cim:GovHydroPelton ;
  rdfs:range cim:PU ;
  skos:definition "Minimum gate opening (<i>ValvMin</i>) (&lt; GovHydroPelton.valvmax).  Typical value = 0."@en .

cim:GovHydroPelton.vav a owl:DatatypeProperty ;
  rdfs:label "vav"@en ;
  rdfs:domain cim:GovHydroPelton ;
  rdfs:range cim:PU ;
  skos:definition "Maximum servomotor valve opening velocity (<i>Vav</i>).  Typical value = 0,1."@en .

cim:GovHydroPelton.vc a owl:DatatypeProperty ;
  rdfs:label "vc"@en ;
  rdfs:domain cim:GovHydroPelton ;
  rdfs:range xsd:float ;
  skos:definition "Maximum gate closing velocity (<i>Vc</i>).  Unit = PU / s.  Typical value = -0,06."@en .

cim:GovHydroPelton.vcv a owl:DatatypeProperty ;
  rdfs:label "vcv"@en ;
  rdfs:domain cim:GovHydroPelton ;
  rdfs:range cim:PU ;
  skos:definition "Maximum servomotor valve closing velocity (<i>Vcv</i>).  Typical value = -0,1."@en .

cim:GovHydroPelton.waterTunnelSurgeChamberSimulation a owl:DatatypeProperty ;
  rdfs:label "waterTunnelSurgeChamberSimulation"@en ;
  rdfs:domain cim:GovHydroPelton ;
  rdfs:range xsd:boolean ;
  skos:definition """
Water tunnel and surge chamber simulation (<i>Tflag</i>).
true = enable of water tunnel and surge chamber simulation
false = inhibit of water tunnel and surge chamber simulation.
Typical value = false.
\t"""@en .

cim:GovHydroPelton.zsfc a owl:DatatypeProperty ;
  rdfs:label "zsfc"@en ;
  rdfs:domain cim:GovHydroPelton ;
  rdfs:range cim:Length ;
  skos:definition "Head of upper water level with respect to the level of penstock (<i>Zsfc</i>).  Unit = km.  Typical value = 0,025."@en .

cim:GovHydroR.at a owl:DatatypeProperty ;
  rdfs:label "at"@en ;
  rdfs:domain cim:GovHydroR ;
  rdfs:range cim:PU ;
  skos:definition "Turbine gain (<i>At</i>).  Typical value = 1,2."@en .

cim:GovHydroR.db1 a owl:DatatypeProperty ;
  rdfs:label "db1"@en ;
  rdfs:domain cim:GovHydroR ;
  rdfs:range cim:Frequency ;
  skos:definition "Intentional dead-band width (<i>db1</i>).  Unit = Hz.  Typical value = 0."@en .

cim:GovHydroR.db2 a owl:DatatypeProperty ;
  rdfs:label "db2"@en ;
  rdfs:domain cim:GovHydroR ;
  rdfs:range cim:ActivePower ;
  skos:definition "Unintentional dead-band (<i>db2</i>).  Unit = MW.  Typical value = 0."@en .

cim:GovHydroR.dturb a owl:DatatypeProperty ;
  rdfs:label "dturb"@en ;
  rdfs:domain cim:GovHydroR ;
  rdfs:range cim:PU ;
  skos:definition "Turbine damping factor (<i>Dturb</i>).  Typical value = 0,2."@en .

cim:GovHydroR.eps a owl:DatatypeProperty ;
  rdfs:label "eps"@en ;
  rdfs:domain cim:GovHydroR ;
  rdfs:range cim:Frequency ;
  skos:definition "Intentional db hysteresis (<i>eps</i>).  Unit = Hz.  Typical value = 0."@en .

cim:GovHydroR.gmax a owl:DatatypeProperty ;
  rdfs:label "gmax"@en ;
  rdfs:domain cim:GovHydroR ;
  rdfs:range cim:PU ;
  skos:definition "Maximum governor output (<i>Gmax</i>) (&gt; GovHydroR.gmin).  Typical value = 1,05."@en .

cim:GovHydroR.gmin a owl:DatatypeProperty ;
  rdfs:label "gmin"@en ;
  rdfs:domain cim:GovHydroR ;
  rdfs:range cim:PU ;
  skos:definition "Minimum governor output (<i>Gmin</i>) (&lt; GovHydroR.gmax).  Typical value = -0,05."@en .

cim:GovHydroR.gv1 a owl:DatatypeProperty ;
  rdfs:label "gv1"@en ;
  rdfs:domain cim:GovHydroR ;
  rdfs:range cim:PU ;
  skos:definition "Nonlinear gain point 1, PU gv (<i>Gv1</i>).  Typical value = 0."@en .

cim:GovHydroR.gv2 a owl:DatatypeProperty ;
  rdfs:label "gv2"@en ;
  rdfs:domain cim:GovHydroR ;
  rdfs:range cim:PU ;
  skos:definition "Nonlinear gain point 2, PU gv (<i>Gv2</i>).  Typical value = 0."@en .

cim:GovHydroR.gv3 a owl:DatatypeProperty ;
  rdfs:label "gv3"@en ;
  rdfs:domain cim:GovHydroR ;
  rdfs:range cim:PU ;
  skos:definition "Nonlinear gain point 3, PU gv (<i>Gv3</i>).  Typical value = 0."@en .

cim:GovHydroR.gv4 a owl:DatatypeProperty ;
  rdfs:label "gv4"@en ;
  rdfs:domain cim:GovHydroR ;
  rdfs:range cim:PU ;
  skos:definition "Nonlinear gain point 4, PU gv (<i>Gv4</i>).  Typical value = 0."@en .

cim:GovHydroR.gv5 a owl:DatatypeProperty ;
  rdfs:label "gv5"@en ;
  rdfs:domain cim:GovHydroR ;
  rdfs:range cim:PU ;
  skos:definition "Nonlinear gain point 5, PU gv (<i>Gv5</i>).  Typical value = 0."@en .

cim:GovHydroR.gv6 a owl:DatatypeProperty ;
  rdfs:label "gv6"@en ;
  rdfs:domain cim:GovHydroR ;
  rdfs:range cim:PU ;
  skos:definition "Nonlinear gain point 6, PU gv (<i>Gv6</i>).  Typical value = 0."@en .

cim:GovHydroR.h0 a owl:DatatypeProperty ;
  rdfs:label "h0"@en ;
  rdfs:domain cim:GovHydroR ;
  rdfs:range cim:PU ;
  skos:definition "Turbine nominal head (<i>H0</i>).  Typical value = 1."@en .

cim:GovHydroR.inputSignal a owl:DatatypeProperty ;
  rdfs:label "inputSignal"@en ;
  rdfs:domain cim:GovHydroR ;
  rdfs:range xsd:boolean ;
  skos:definition """
Input signal switch (<i>Flag</i>).
true = <i>Pe</i> input is used
false = feedback is received from <i>CV</i>.
<i>Flag</i> is normally dependent on <i>Tt</i>.  If <i>Tt </i>is zero, <i>Flag</i> is set to false. If <i>Tt</i> is not zero, <i>Flag</i> is set to true.  
Typical value = true.
\t"""@en .

cim:GovHydroR.kg a owl:DatatypeProperty ;
  rdfs:label "kg"@en ;
  rdfs:domain cim:GovHydroR ;
  rdfs:range cim:PU ;
  skos:definition "Gate servo gain (<i>Kg</i>).  Typical value = 2."@en .

cim:GovHydroR.ki a owl:DatatypeProperty ;
  rdfs:label "ki"@en ;
  rdfs:domain cim:GovHydroR ;
  rdfs:range cim:PU ;
  skos:definition "Integral gain (<i>Ki</i>).  Typical value = 0,5."@en .

cim:GovHydroR.mwbase a owl:DatatypeProperty ;
  rdfs:label "mwbase"@en ;
  rdfs:domain cim:GovHydroR ;
  rdfs:range cim:ActivePower ;
  skos:definition "Base for power values (<i>MWbase</i>) (&gt; 0).  Unit = MW."@en .

cim:GovHydroR.pgv1 a owl:DatatypeProperty ;
  rdfs:label "pgv1"@en ;
  rdfs:domain cim:GovHydroR ;
  rdfs:range cim:PU ;
  skos:definition "Nonlinear gain point 1, PU power (<i>Pgv1</i>).  Typical value = 0."@en .

cim:GovHydroR.pgv2 a owl:DatatypeProperty ;
  rdfs:label "pgv2"@en ;
  rdfs:domain cim:GovHydroR ;
  rdfs:range cim:PU ;
  skos:definition "Nonlinear gain point 2, PU power (<i>Pgv2</i>).  Typical value = 0."@en .

cim:GovHydroR.pgv3 a owl:DatatypeProperty ;
  rdfs:label "pgv3"@en ;
  rdfs:domain cim:GovHydroR ;
  rdfs:range cim:PU ;
  skos:definition "Nonlinear gain point 3, PU power (<i>Pgv3</i>).  Typical value = 0."@en .

cim:GovHydroR.pgv4 a owl:DatatypeProperty ;
  rdfs:label "pgv4"@en ;
  rdfs:domain cim:GovHydroR ;
  rdfs:range cim:PU ;
  skos:definition "Nonlinear gain point 4, PU power (<i>Pgv4</i>).  Typical value = 0."@en .

cim:GovHydroR.pgv5 a owl:DatatypeProperty ;
  rdfs:label "pgv5"@en ;
  rdfs:domain cim:GovHydroR ;
  rdfs:range cim:PU ;
  skos:definition "Nonlinear gain point 5, PU power (<i>Pgv5</i>).  Typical value = 0."@en .

cim:GovHydroR.pgv6 a owl:DatatypeProperty ;
  rdfs:label "pgv6"@en ;
  rdfs:domain cim:GovHydroR ;
  rdfs:range cim:PU ;
  skos:definition "Nonlinear gain point 6, PU power (<i>Pgv6</i>).  Typical value = 0."@en .

cim:GovHydroR.pmax a owl:DatatypeProperty ;
  rdfs:label "pmax"@en ;
  rdfs:domain cim:GovHydroR ;
  rdfs:range cim:PU ;
  skos:definition "Maximum gate opening, PU of <i>MWbase</i> (<i>Pmax</i>) (&gt; GovHydroR.pmin).  Typical value = 1."@en .

cim:GovHydroR.pmin a owl:DatatypeProperty ;
  rdfs:label "pmin"@en ;
  rdfs:domain cim:GovHydroR ;
  rdfs:range cim:PU ;
  skos:definition "Minimum gate opening, PU of <i>MWbase</i> (<i>Pmin</i>) (&lt; GovHydroR.pmax).  Typical value = 0."@en .

cim:GovHydroR.qnl a owl:DatatypeProperty ;
  rdfs:label "qnl"@en ;
  rdfs:domain cim:GovHydroR ;
  rdfs:range cim:PU ;
  skos:definition "No-load turbine flow at nominal head (<i>Qnl</i>).  Typical value = 0,08."@en .

cim:GovHydroR.r a owl:DatatypeProperty ;
  rdfs:label "r"@en ;
  rdfs:domain cim:GovHydroR ;
  rdfs:range cim:PU ;
  skos:definition "Steady-state droop (<i>R</i>).  Typical value = 0,05."@en .

cim:GovHydroR.t1 a owl:DatatypeProperty ;
  rdfs:label "t1"@en ;
  rdfs:domain cim:GovHydroR ;
  rdfs:range cim:Seconds ;
  skos:definition "Lead time constant 1 (<i>T1</i>) (&gt;= 0).  Typical value = 1,5."@en .

cim:GovHydroR.t2 a owl:DatatypeProperty ;
  rdfs:label "t2"@en ;
  rdfs:domain cim:GovHydroR ;
  rdfs:range cim:Seconds ;
  skos:definition "Lag time constant 1 (<i>T2</i>) (&gt;= 0).  Typical value = 0,1."@en .

cim:GovHydroR.t3 a owl:DatatypeProperty ;
  rdfs:label "t3"@en ;
  rdfs:domain cim:GovHydroR ;
  rdfs:range cim:Seconds ;
  skos:definition "Lead time constant 2 (<i>T3</i>) (&gt;= 0).  Typical value = 1,5."@en .

cim:GovHydroR.t4 a owl:DatatypeProperty ;
  rdfs:label "t4"@en ;
  rdfs:domain cim:GovHydroR ;
  rdfs:range cim:Seconds ;
  skos:definition "Lag time constant 2 (<i>T4</i>) (&gt;= 0).  Typical value = 0,1."@en .

cim:GovHydroR.t5 a owl:DatatypeProperty ;
  rdfs:label "t5"@en ;
  rdfs:domain cim:GovHydroR ;
  rdfs:range cim:Seconds ;
  skos:definition "Lead time constant 3 (<i>T5</i>) (&gt;= 0).  Typical value = 0."@en .

cim:GovHydroR.t6 a owl:DatatypeProperty ;
  rdfs:label "t6"@en ;
  rdfs:domain cim:GovHydroR ;
  rdfs:range cim:Seconds ;
  skos:definition "Lag time constant 3 (<i>T6</i>) (&gt;= 0).  Typical value = 0,05."@en .

cim:GovHydroR.t7 a owl:DatatypeProperty ;
  rdfs:label "t7"@en ;
  rdfs:domain cim:GovHydroR ;
  rdfs:range cim:Seconds ;
  skos:definition "Lead time constant 4 (<i>T7</i>) (&gt;= 0).  Typical value = 0."@en .

cim:GovHydroR.t8 a owl:DatatypeProperty ;
  rdfs:label "t8"@en ;
  rdfs:domain cim:GovHydroR ;
  rdfs:range cim:Seconds ;
  skos:definition "Lag time constant 4 (<i>T8</i>) (&gt;= 0).  Typical value = 0,05."@en .

cim:GovHydroR.td a owl:DatatypeProperty ;
  rdfs:label "td"@en ;
  rdfs:domain cim:GovHydroR ;
  rdfs:range cim:Seconds ;
  skos:definition "Input filter time constant (<i>Td</i>) (&gt;= 0).  Typical value = 0,05."@en .

cim:GovHydroR.tp a owl:DatatypeProperty ;
  rdfs:label "tp"@en ;
  rdfs:domain cim:GovHydroR ;
  rdfs:range cim:Seconds ;
  skos:definition "Gate servo time constant (<i>Tp</i>) (&gt;= 0).  Typical value = 0,05."@en .

cim:GovHydroR.tt a owl:DatatypeProperty ;
  rdfs:label "tt"@en ;
  rdfs:domain cim:GovHydroR ;
  rdfs:range cim:Seconds ;
  skos:definition "Power feedback time constant (<i>Tt</i>) (&gt;= 0).  Typical value = 0."@en .

cim:GovHydroR.tw a owl:DatatypeProperty ;
  rdfs:label "tw"@en ;
  rdfs:domain cim:GovHydroR ;
  rdfs:range cim:Seconds ;
  skos:definition "Water inertia time constant (<i>Tw</i>) (&gt; 0).  Typical value = 1."@en .

cim:GovHydroR.velcl a owl:DatatypeProperty ;
  rdfs:label "velcl"@en ;
  rdfs:domain cim:GovHydroR ;
  rdfs:range xsd:float ;
  skos:definition "Maximum gate closing velocity (<i>Velcl</i>).  Unit = PU / s.  Typical value = -0,2."@en .

cim:GovHydroR.velop a owl:DatatypeProperty ;
  rdfs:label "velop"@en ;
  rdfs:domain cim:GovHydroR ;
  rdfs:range xsd:float ;
  skos:definition "Maximum gate opening velocity (<i>Velop</i>).  Unit = PU / s.  Typical value = 0,2."@en .

cim:GovHydroWEH.db a owl:DatatypeProperty ;
  rdfs:label "db"@en ;
  rdfs:domain cim:GovHydroWEH ;
  rdfs:range cim:PU ;
  skos:definition "Speed deadband (<i>db</i>)."@en .

cim:GovHydroWEH.dicn a owl:DatatypeProperty ;
  rdfs:label "dicn"@en ;
  rdfs:domain cim:GovHydroWEH ;
  rdfs:range cim:PU ;
  skos:definition "Value to allow the integral controller to advance beyond the gate limits (<i>Dicn</i>)."@en .

cim:GovHydroWEH.dpv a owl:DatatypeProperty ;
  rdfs:label "dpv"@en ;
  rdfs:domain cim:GovHydroWEH ;
  rdfs:range cim:PU ;
  skos:definition "Value to allow the pilot valve controller to advance beyond the gate limits (<i>Dpv</i>)."@en .

cim:GovHydroWEH.dturb a owl:DatatypeProperty ;
  rdfs:label "dturb"@en ;
  rdfs:domain cim:GovHydroWEH ;
  rdfs:range cim:PU ;
  skos:definition "Turbine damping factor (<i>Dturb</i>).  Unit = delta P (PU of <i>MWbase</i>) / delta speed (PU)."@en .

cim:GovHydroWEH.feedbackSignal a owl:DatatypeProperty ;
  rdfs:label "feedbackSignal"@en ;
  rdfs:domain cim:GovHydroWEH ;
  rdfs:range xsd:boolean ;
  skos:definition """
Feedback signal selection (<i>Sw</i>).
true = PID output (if <i>R-Perm-Gate </i>= droop and <i>R-Perm-Pe </i>= 0)
false = electrical power (if <i>R-Perm-Gate </i>= 0 and <i>R-Perm-Pe </i>= droop) or
false = gate position (if R<i>-Perm-Gate </i>= droop and <i>R-Perm-Pe </i>= 0).
Typical value = false.
\t"""@en .

cim:GovHydroWEH.fl1 a owl:DatatypeProperty ;
  rdfs:label "fl1"@en ;
  rdfs:domain cim:GovHydroWEH ;
  rdfs:range cim:PU ;
  skos:definition "Flowgate 1 (<i>Fl1</i>).  Flow value for gate position point 1 for lookup table representing water flow through the turbine as a function of gate position to produce steady state flow."@en .

cim:GovHydroWEH.fl2 a owl:DatatypeProperty ;
  rdfs:label "fl2"@en ;
  rdfs:domain cim:GovHydroWEH ;
  rdfs:range cim:PU ;
  skos:definition "Flowgate 2 (<i>Fl2</i>).  Flow value for gate position point 2 for lookup table representing water flow through the turbine as a function of gate position to produce steady state flow."@en .

cim:GovHydroWEH.fl3 a owl:DatatypeProperty ;
  rdfs:label "fl3"@en ;
  rdfs:domain cim:GovHydroWEH ;
  rdfs:range cim:PU ;
  skos:definition "Flowgate 3 (<i>Fl3</i>).  Flow value for gate position point 3 for lookup table representing water flow through the turbine as a function of gate position to produce steady state flow."@en .

cim:GovHydroWEH.fl4 a owl:DatatypeProperty ;
  rdfs:label "fl4"@en ;
  rdfs:domain cim:GovHydroWEH ;
  rdfs:range cim:PU ;
  skos:definition "Flowgate 4 (<i>Fl4</i>).  Flow value for gate position point 4 for lookup table representing water flow through the turbine as a function of gate position to produce steady state flow."@en .

cim:GovHydroWEH.fl5 a owl:DatatypeProperty ;
  rdfs:label "fl5"@en ;
  rdfs:domain cim:GovHydroWEH ;
  rdfs:range cim:PU ;
  skos:definition "Flowgate 5 (<i>Fl5</i>).  Flow value for gate position point 5 for lookup table representing water flow through the turbine as a function of gate position to produce steady state flow."@en .

cim:GovHydroWEH.fp1 a owl:DatatypeProperty ;
  rdfs:label "fp1"@en ;
  rdfs:domain cim:GovHydroWEH ;
  rdfs:range cim:PU ;
  skos:definition "Flow P1 (<i>Fp1</i>).  Turbine flow value for point 1 for lookup table representing PU mechanical power on machine MVA rating as a function of turbine flow."@en .

cim:GovHydroWEH.fp10 a owl:DatatypeProperty ;
  rdfs:label "fp10"@en ;
  rdfs:domain cim:GovHydroWEH ;
  rdfs:range cim:PU ;
  skos:definition "Flow P10 (<i>Fp10</i>).  Turbine flow value for point 10 for lookup table representing PU mechanical power on machine MVA rating as a function of turbine flow."@en .

cim:GovHydroWEH.fp2 a owl:DatatypeProperty ;
  rdfs:label "fp2"@en ;
  rdfs:domain cim:GovHydroWEH ;
  rdfs:range cim:PU ;
  skos:definition "Flow P2 (<i>Fp2</i>).  Turbine flow value for point 2 for lookup table representing PU mechanical power on machine MVA rating as a function of turbine flow."@en .

cim:GovHydroWEH.fp3 a owl:DatatypeProperty ;
  rdfs:label "fp3"@en ;
  rdfs:domain cim:GovHydroWEH ;
  rdfs:range cim:PU ;
  skos:definition "Flow P3 (<i>Fp3</i>).  Turbine flow value for point 3 for lookup table representing PU mechanical power on machine MVA rating as a function of turbine flow."@en .

cim:GovHydroWEH.fp4 a owl:DatatypeProperty ;
  rdfs:label "fp4"@en ;
  rdfs:domain cim:GovHydroWEH ;
  rdfs:range cim:PU ;
  skos:definition "Flow P4 (<i>Fp4</i>).  Turbine flow value for point 4 for lookup table representing PU mechanical power on machine MVA rating as a function of turbine flow."@en .

cim:GovHydroWEH.fp5 a owl:DatatypeProperty ;
  rdfs:label "fp5"@en ;
  rdfs:domain cim:GovHydroWEH ;
  rdfs:range cim:PU ;
  skos:definition "Flow P5 (<i>Fp5</i>).  Turbine flow value for point 5 for lookup table representing PU mechanical power on machine MVA rating as a function of turbine flow."@en .

cim:GovHydroWEH.fp6 a owl:DatatypeProperty ;
  rdfs:label "fp6"@en ;
  rdfs:domain cim:GovHydroWEH ;
  rdfs:range cim:PU ;
  skos:definition "Flow P6 (<i>Fp6</i>).  Turbine flow value for point 6 for lookup table representing PU mechanical power on machine MVA rating as a function of turbine flow."@en .

cim:GovHydroWEH.fp7 a owl:DatatypeProperty ;
  rdfs:label "fp7"@en ;
  rdfs:domain cim:GovHydroWEH ;
  rdfs:range cim:PU ;
  skos:definition "Flow P7 (<i>Fp7</i>).  Turbine flow value for point 7 for lookup table representing PU mechanical power on machine MVA rating as a function of turbine flow."@en .

cim:GovHydroWEH.fp8 a owl:DatatypeProperty ;
  rdfs:label "fp8"@en ;
  rdfs:domain cim:GovHydroWEH ;
  rdfs:range cim:PU ;
  skos:definition "Flow P8 (<i>Fp8</i>).  Turbine flow value for point 8 for lookup table representing PU mechanical power on machine MVA rating as a function of turbine flow."@en .

cim:GovHydroWEH.fp9 a owl:DatatypeProperty ;
  rdfs:label "fp9"@en ;
  rdfs:domain cim:GovHydroWEH ;
  rdfs:range cim:PU ;
  skos:definition "Flow P9 (<i>Fp9</i>).  Turbine flow value for point 9 for lookup table representing PU mechanical power on machine MVA rating as a function of turbine flow."@en .

cim:GovHydroWEH.gmax a owl:DatatypeProperty ;
  rdfs:label "gmax"@en ;
  rdfs:domain cim:GovHydroWEH ;
  rdfs:range cim:PU ;
  skos:definition "Maximum gate position (<i>Gmax</i>) (&gt; GovHydroWEH.gmin)."@en .

cim:GovHydroWEH.gmin a owl:DatatypeProperty ;
  rdfs:label "gmin"@en ;
  rdfs:domain cim:GovHydroWEH ;
  rdfs:range cim:PU ;
  skos:definition "Minimum gate position (<i>Gmin</i>) (&lt; GovHydroWEH.gmax)."@en .

cim:GovHydroWEH.gtmxcl a owl:DatatypeProperty ;
  rdfs:label "gtmxcl"@en ;
  rdfs:domain cim:GovHydroWEH ;
  rdfs:range cim:PU ;
  skos:definition "Maximum gate closing rate (<i>Gtmxcl</i>)."@en .

cim:GovHydroWEH.gtmxop a owl:DatatypeProperty ;
  rdfs:label "gtmxop"@en ;
  rdfs:domain cim:GovHydroWEH ;
  rdfs:range cim:PU ;
  skos:definition "Maximum gate opening rate (<i>Gtmxop</i>)."@en .

cim:GovHydroWEH.gv1 a owl:DatatypeProperty ;
  rdfs:label "gv1"@en ;
  rdfs:domain cim:GovHydroWEH ;
  rdfs:range cim:PU ;
  skos:definition "Gate 1 (<i>Gv1</i>).  Gate Position value for point 1 for lookup table representing water flow through the turbine as a function of gate position to produce steady state flow."@en .

cim:GovHydroWEH.gv2 a owl:DatatypeProperty ;
  rdfs:label "gv2"@en ;
  rdfs:domain cim:GovHydroWEH ;
  rdfs:range cim:PU ;
  skos:definition "Gate 2 (<i>Gv2</i>).  Gate Position value for point 2 for lookup table representing water flow through the turbine as a function of gate position to produce steady state flow."@en .

cim:GovHydroWEH.gv3 a owl:DatatypeProperty ;
  rdfs:label "gv3"@en ;
  rdfs:domain cim:GovHydroWEH ;
  rdfs:range cim:PU ;
  skos:definition "Gate 3 (<i>Gv3</i>).  Gate Position value for point 3 for lookup table representing water flow through the turbine as a function of gate position to produce steady state flow."@en .

cim:GovHydroWEH.gv4 a owl:DatatypeProperty ;
  rdfs:label "gv4"@en ;
  rdfs:domain cim:GovHydroWEH ;
  rdfs:range cim:PU ;
  skos:definition "Gate 4 (<i>Gv4</i>).  Gate Position value for point 4 for lookup table representing water flow through the turbine as a function of gate position to produce steady state flow."@en .

cim:GovHydroWEH.gv5 a owl:DatatypeProperty ;
  rdfs:label "gv5"@en ;
  rdfs:domain cim:GovHydroWEH ;
  rdfs:range cim:PU ;
  skos:definition "Gate 5 (<i>Gv5</i>).  Gate Position value for point 5 for lookup table representing water flow through the turbine as a function of gate position to produce steady state flow."@en .

cim:GovHydroWEH.kd a owl:DatatypeProperty ;
  rdfs:label "kd"@en ;
  rdfs:domain cim:GovHydroWEH ;
  rdfs:range cim:PU ;
  skos:definition "Derivative controller derivative gain (<i>Kd</i>)."@en .

cim:GovHydroWEH.ki a owl:DatatypeProperty ;
  rdfs:label "ki"@en ;
  rdfs:domain cim:GovHydroWEH ;
  rdfs:range cim:PU ;
  skos:definition "Derivative controller Integral gain (<i>Ki</i>)."@en .

cim:GovHydroWEH.kp a owl:DatatypeProperty ;
  rdfs:label "kp"@en ;
  rdfs:domain cim:GovHydroWEH ;
  rdfs:range cim:PU ;
  skos:definition "Derivative control gain (<i>Kp</i>)."@en .

cim:GovHydroWEH.mwbase a owl:DatatypeProperty ;
  rdfs:label "mwbase"@en ;
  rdfs:domain cim:GovHydroWEH ;
  rdfs:range cim:ActivePower ;
  skos:definition "Base for power values (<i>MWbase</i>) (&gt; 0).  Unit = MW."@en .

cim:GovHydroWEH.pmss1 a owl:DatatypeProperty ;
  rdfs:label "pmss1"@en ;
  rdfs:domain cim:GovHydroWEH ;
  rdfs:range cim:PU ;
  skos:definition "Pmss flow P1 (<i>Pmss1</i>).  Mechanical power output for turbine flow point 1 for lookup table representing PU mechanical power on machine MVA rating as a function of turbine flow."@en .

cim:GovHydroWEH.pmss10 a owl:DatatypeProperty ;
  rdfs:label "pmss10"@en ;
  rdfs:domain cim:GovHydroWEH ;
  rdfs:range cim:PU ;
  skos:definition """
Pmss flow P10 (<i>Pmss10</i>).  Mechanical power output for turbine flow point 10 for lookup table representing PU mechanical power on machine MVA rating as a function of turbine flow.

\t"""@en .

cim:GovHydroWEH.pmss2 a owl:DatatypeProperty ;
  rdfs:label "pmss2"@en ;
  rdfs:domain cim:GovHydroWEH ;
  rdfs:range cim:PU ;
  skos:definition """
Pmss flow P2 (<i>Pmss2</i>).  Mechanical power output for turbine flow point 2 for lookup table representing PU mechanical power on machine MVA rating as a function of turbine flow.

\t"""@en .

cim:GovHydroWEH.pmss3 a owl:DatatypeProperty ;
  rdfs:label "pmss3"@en ;
  rdfs:domain cim:GovHydroWEH ;
  rdfs:range cim:PU ;
  skos:definition """
Pmss flow P3 (<i>Pmss3</i>).  Mechanical power output for turbine flow point 3 for lookup table representing PU mechanical power on machine MVA rating as a function of turbine flow.

\t"""@en .

cim:GovHydroWEH.pmss4 a owl:DatatypeProperty ;
  rdfs:label "pmss4"@en ;
  rdfs:domain cim:GovHydroWEH ;
  rdfs:range cim:PU ;
  skos:definition """
Pmss flow P4 (<i>Pmss4</i>).  Mechanical power output for turbine flow point 4 for lookup table representing PU mechanical power on machine MVA rating as a function of turbine flow.

\t"""@en .

cim:GovHydroWEH.pmss5 a owl:DatatypeProperty ;
  rdfs:label "pmss5"@en ;
  rdfs:domain cim:GovHydroWEH ;
  rdfs:range cim:PU ;
  skos:definition "Pmss flow P5 (<i>Pmss5</i>).  Mechanical power output for turbine flow point 5 for lookup table representing PU mechanical power on machine MVA rating as a function of turbine flow."@en .

cim:GovHydroWEH.pmss6 a owl:DatatypeProperty ;
  rdfs:label "pmss6"@en ;
  rdfs:domain cim:GovHydroWEH ;
  rdfs:range cim:PU ;
  skos:definition "Pmss flow P6 (<i>Pmss6</i>).  Mechanical power output for turbine flow point 6 for lookup table representing PU mechanical power on machine MVA rating as a function of turbine flow."@en .

cim:GovHydroWEH.pmss7 a owl:DatatypeProperty ;
  rdfs:label "pmss7"@en ;
  rdfs:domain cim:GovHydroWEH ;
  rdfs:range cim:PU ;
  skos:definition "Pmss flow P7 (<i>Pmss7</i>).  Mechanical power output for turbine flow point 7 for lookup table representing PU mechanical power on machine MVA rating as a function of turbine flow."@en .

cim:GovHydroWEH.pmss8 a owl:DatatypeProperty ;
  rdfs:label "pmss8"@en ;
  rdfs:domain cim:GovHydroWEH ;
  rdfs:range cim:PU ;
  skos:definition "Pmss flow P8 (<i>Pmss8</i>).  Mechanical power output for turbine flow point 8 for lookup table representing PU mechanical power on machine MVA rating as a function of turbine flow."@en .

cim:GovHydroWEH.pmss9 a owl:DatatypeProperty ;
  rdfs:label "pmss9"@en ;
  rdfs:domain cim:GovHydroWEH ;
  rdfs:range cim:PU ;
  skos:definition "Pmss flow P9 (<i>Pmss9</i>).  Mechanical power output for turbine flow point 9 for lookup table representing PU mechanical power on machine MVA rating as a function of turbine flow."@en .

cim:GovHydroWEH.rpg a owl:DatatypeProperty ;
  rdfs:label "rpg"@en ;
  rdfs:domain cim:GovHydroWEH ;
  rdfs:range xsd:float ;
  skos:definition "Permanent droop for governor output feedback (<i>R-Perm-Gate</i>)."@en .

cim:GovHydroWEH.rpp a owl:DatatypeProperty ;
  rdfs:label "rpp"@en ;
  rdfs:domain cim:GovHydroWEH ;
  rdfs:range xsd:float ;
  skos:definition "Permanent droop for electrical power feedback (<i>R-Perm-Pe</i>)."@en .

cim:GovHydroWEH.td a owl:DatatypeProperty ;
  rdfs:label "td"@en ;
  rdfs:domain cim:GovHydroWEH ;
  rdfs:range cim:Seconds ;
  skos:definition "Derivative controller time constant (<i>Td</i>) (&gt;= 0).  Limits the derivative characteristic beyond a breakdown frequency to avoid amplification of high-frequency noise."@en .

cim:GovHydroWEH.tdv a owl:DatatypeProperty ;
  rdfs:label "tdv"@en ;
  rdfs:domain cim:GovHydroWEH ;
  rdfs:range cim:Seconds ;
  skos:definition "Distributive valve time lag time constant (<i>Tdv</i>) (&gt;= 0)."@en .

cim:GovHydroWEH.tg a owl:DatatypeProperty ;
  rdfs:label "tg"@en ;
  rdfs:domain cim:GovHydroWEH ;
  rdfs:range cim:Seconds ;
  skos:definition "Value to allow the distribution valve controller to advance beyond the gate movement rate limit (<i>Tg</i>) (&gt;= 0)."@en .

cim:GovHydroWEH.tp a owl:DatatypeProperty ;
  rdfs:label "tp"@en ;
  rdfs:domain cim:GovHydroWEH ;
  rdfs:range cim:Seconds ;
  skos:definition "Pilot valve time lag time constant (<i>Tp</i>) (&gt;= 0)."@en .

cim:GovHydroWEH.tpe a owl:DatatypeProperty ;
  rdfs:label "tpe"@en ;
  rdfs:domain cim:GovHydroWEH ;
  rdfs:range cim:Seconds ;
  skos:definition "Electrical power droop time constant (<i>Tpe</i>) (&gt;= 0)."@en .

cim:GovHydroWEH.tw a owl:DatatypeProperty ;
  rdfs:label "tw"@en ;
  rdfs:domain cim:GovHydroWEH ;
  rdfs:range cim:Seconds ;
  skos:definition "Water inertia time constant (<i>Tw</i>) (&gt; 0)."@en .

cim:GovHydroWPID.d a owl:DatatypeProperty ;
  rdfs:label "d"@en ;
  rdfs:domain cim:GovHydroWPID ;
  rdfs:range cim:PU ;
  skos:definition "Turbine damping factor (<i>D</i>).  Unit = delta P / delta speed."@en .

cim:GovHydroWPID.gatmax a owl:DatatypeProperty ;
  rdfs:label "gatmax"@en ;
  rdfs:domain cim:GovHydroWPID ;
  rdfs:range cim:PU ;
  skos:definition "Gate opening limit maximum (<i>Gatmax</i>) (&gt; GovHydroWPID.gatmin)."@en .

cim:GovHydroWPID.gatmin a owl:DatatypeProperty ;
  rdfs:label "gatmin"@en ;
  rdfs:domain cim:GovHydroWPID ;
  rdfs:range cim:PU ;
  skos:definition "Gate opening limit minimum (<i>Gatmin</i>) (&lt; GovHydroWPID.gatmax)."@en .

cim:GovHydroWPID.gv1 a owl:DatatypeProperty ;
  rdfs:label "gv1"@en ;
  rdfs:domain cim:GovHydroWPID ;
  rdfs:range cim:PU ;
  skos:definition "Gate position 1 (<i>Gv1</i>)."@en .

cim:GovHydroWPID.gv2 a owl:DatatypeProperty ;
  rdfs:label "gv2"@en ;
  rdfs:domain cim:GovHydroWPID ;
  rdfs:range cim:PU ;
  skos:definition "Gate position 2 (<i>Gv2</i>). "@en .

cim:GovHydroWPID.gv3 a owl:DatatypeProperty ;
  rdfs:label "gv3"@en ;
  rdfs:domain cim:GovHydroWPID ;
  rdfs:range cim:PU ;
  skos:definition "Gate position 3 (<i>Gv3</i>) (= 1,0)."@en .

cim:GovHydroWPID.kd a owl:DatatypeProperty ;
  rdfs:label "kd"@en ;
  rdfs:domain cim:GovHydroWPID ;
  rdfs:range cim:PU ;
  skos:definition "Derivative gain (<i>Kd</i>).  Typical value = 1,11."@en .

cim:GovHydroWPID.ki a owl:DatatypeProperty ;
  rdfs:label "ki"@en ;
  rdfs:domain cim:GovHydroWPID ;
  rdfs:range cim:PU ;
  skos:definition "Reset gain (<i>Ki</i>).  Typical value = 0,36."@en .

cim:GovHydroWPID.kp a owl:DatatypeProperty ;
  rdfs:label "kp"@en ;
  rdfs:domain cim:GovHydroWPID ;
  rdfs:range cim:PU ;
  skos:definition "Proportional gain (<i>Kp</i>).  Typical value = 0,1."@en .

cim:GovHydroWPID.mwbase a owl:DatatypeProperty ;
  rdfs:label "mwbase"@en ;
  rdfs:domain cim:GovHydroWPID ;
  rdfs:range cim:ActivePower ;
  skos:definition "Base for power values  (<i>MWbase</i>) (&gt; 0).  Unit = MW."@en .

cim:GovHydroWPID.pgv1 a owl:DatatypeProperty ;
  rdfs:label "pgv1"@en ;
  rdfs:domain cim:GovHydroWPID ;
  rdfs:range cim:PU ;
  skos:definition "Output at <i>Gv1</i> PU of <i>MWbase</i> (<i>Pgv1</i>)."@en .

cim:GovHydroWPID.pgv2 a owl:DatatypeProperty ;
  rdfs:label "pgv2"@en ;
  rdfs:domain cim:GovHydroWPID ;
  rdfs:range cim:PU ;
  skos:definition "Output at <i>Gv2</i> PU of <i>MWbase</i> (<i>Pgv2</i>)."@en .

cim:GovHydroWPID.pgv3 a owl:DatatypeProperty ;
  rdfs:label "pgv3"@en ;
  rdfs:domain cim:GovHydroWPID ;
  rdfs:range cim:PU ;
  skos:definition "Output at <i>Gv3</i> PU of <i>MWbase</i> (<i>Pgv3</i>). "@en .

cim:GovHydroWPID.pmax a owl:DatatypeProperty ;
  rdfs:label "pmax"@en ;
  rdfs:domain cim:GovHydroWPID ;
  rdfs:range cim:PU ;
  skos:definition "Maximum power output (<i>Pmax</i>) (&gt; GovHydroWPID.pmin)."@en .

cim:GovHydroWPID.pmin a owl:DatatypeProperty ;
  rdfs:label "pmin"@en ;
  rdfs:domain cim:GovHydroWPID ;
  rdfs:range cim:PU ;
  skos:definition "Minimum power output (<i>Pmin</i>) (&lt; GovHydroWPID.pmax)."@en .

cim:GovHydroWPID.reg a owl:DatatypeProperty ;
  rdfs:label "reg"@en ;
  rdfs:domain cim:GovHydroWPID ;
  rdfs:range cim:PU ;
  skos:definition "Permanent drop (<i>Reg</i>)."@en .

cim:GovHydroWPID.ta a owl:DatatypeProperty ;
  rdfs:label "ta"@en ;
  rdfs:domain cim:GovHydroWPID ;
  rdfs:range cim:Seconds ;
  skos:definition "Controller time constant (<i>Ta</i>) (&gt;= 0).  Typical value = 0."@en .

cim:GovHydroWPID.tb a owl:DatatypeProperty ;
  rdfs:label "tb"@en ;
  rdfs:domain cim:GovHydroWPID ;
  rdfs:range cim:Seconds ;
  skos:definition "Gate servo time constant (<i>Tb</i>) (&gt;= 0).  Typical value = 0."@en .

cim:GovHydroWPID.treg a owl:DatatypeProperty ;
  rdfs:label "treg"@en ;
  rdfs:domain cim:GovHydroWPID ;
  rdfs:range cim:Seconds ;
  skos:definition "Speed detector time constant (<i>Treg</i>) (&gt;= 0)."@en .

cim:GovHydroWPID.tw a owl:DatatypeProperty ;
  rdfs:label "tw"@en ;
  rdfs:domain cim:GovHydroWPID ;
  rdfs:range cim:Seconds ;
  skos:definition "Water inertia time constant (<i>Tw</i>) (&gt;= 0).  Typical value = 0."@en .

cim:GovHydroWPID.velmax a owl:DatatypeProperty ;
  rdfs:label "velmax"@en ;
  rdfs:domain cim:GovHydroWPID ;
  rdfs:range cim:PU ;
  skos:definition "Maximum gate opening velocity (<i>Velmax</i>) (&gt; GovHydroWPID.velmin).  Unit = PU / s.  Typical value = 0."@en .

cim:GovHydroWPID.velmin a owl:DatatypeProperty ;
  rdfs:label "velmin"@en ;
  rdfs:domain cim:GovHydroWPID ;
  rdfs:range cim:PU ;
  skos:definition "Maximum gate closing velocity (<i>Velmin</i>) (&lt; GovHydroWPID.velmax).  Unit = PU / s.  Typical value = 0."@en .

cim:GovSteam0.dt a owl:DatatypeProperty ;
  rdfs:label "dt"@en ;
  rdfs:domain cim:GovSteam0 ;
  rdfs:range cim:PU ;
  skos:definition "Turbine damping coefficient (<i>Dt</i>).  Unit = delta P / delta speed. Typical value = 0."@en .

cim:GovSteam0.mwbase a owl:DatatypeProperty ;
  rdfs:label "mwbase"@en ;
  rdfs:domain cim:GovSteam0 ;
  rdfs:range cim:ActivePower ;
  skos:definition "Base for power values (<i>MWbase</i>) (&gt; 0).  Unit = MW."@en .

cim:GovSteam0.r a owl:DatatypeProperty ;
  rdfs:label "r"@en ;
  rdfs:domain cim:GovSteam0 ;
  rdfs:range cim:PU ;
  skos:definition "Permanent droop (<i>R</i>).  Typical value = 0,05."@en .

cim:GovSteam0.t1 a owl:DatatypeProperty ;
  rdfs:label "t1"@en ;
  rdfs:domain cim:GovSteam0 ;
  rdfs:range cim:Seconds ;
  skos:definition "Steam bowl time constant (<i>T1</i>) (&gt; 0).  Typical value = 0,5."@en .

cim:GovSteam0.t2 a owl:DatatypeProperty ;
  rdfs:label "t2"@en ;
  rdfs:domain cim:GovSteam0 ;
  rdfs:range cim:Seconds ;
  skos:definition "Numerator time constant of <i>T2</i>/<i>T3</i> block (<i>T2</i>) (&gt;= 0).  Typical value = 3."@en .

cim:GovSteam0.t3 a owl:DatatypeProperty ;
  rdfs:label "t3"@en ;
  rdfs:domain cim:GovSteam0 ;
  rdfs:range cim:Seconds ;
  skos:definition "Reheater time constant (<i>T3</i>) (&gt; 0).  Typical value = 10."@en .

cim:GovSteam0.vmax a owl:DatatypeProperty ;
  rdfs:label "vmax"@en ;
  rdfs:domain cim:GovSteam0 ;
  rdfs:range cim:PU ;
  skos:definition "Maximum valve position, PU of <i>mwcap</i> (<i>Vmax</i>) (&gt; GovSteam0.vmin).  Typical value = 1."@en .

cim:GovSteam0.vmin a owl:DatatypeProperty ;
  rdfs:label "vmin"@en ;
  rdfs:domain cim:GovSteam0 ;
  rdfs:range cim:PU ;
  skos:definition "Minimum valve position, PU of <i>mwcap</i> (<i>Vmin</i>) (&lt; GovSteam0.vmax).  Typical value = 0."@en .

cim:GovSteam1.db1 a owl:DatatypeProperty ;
  rdfs:label "db1"@en ;
  rdfs:domain cim:GovSteam1 ;
  rdfs:range cim:Frequency ;
  skos:definition "Intentional deadband width (<i>db1</i>).  Unit = Hz.  Typical value = 0."@en .

cim:GovSteam1.db2 a owl:DatatypeProperty ;
  rdfs:label "db2"@en ;
  rdfs:domain cim:GovSteam1 ;
  rdfs:range cim:ActivePower ;
  skos:definition "Unintentional deadband (<i>db2</i>).  Unit = MW.  Typical value = 0."@en .

cim:GovSteam1.eps a owl:DatatypeProperty ;
  rdfs:label "eps"@en ;
  rdfs:domain cim:GovSteam1 ;
  rdfs:range cim:Frequency ;
  skos:definition "Intentional db hysteresis (<i>eps</i>).  Unit = Hz.  Typical value = 0."@en .

cim:GovSteam1.gv1 a owl:DatatypeProperty ;
  rdfs:label "gv1"@en ;
  rdfs:domain cim:GovSteam1 ;
  rdfs:range cim:PU ;
  skos:definition "Nonlinear gain valve position point 1 (<i>GV1</i>).  Typical value = 0."@en .

cim:GovSteam1.gv2 a owl:DatatypeProperty ;
  rdfs:label "gv2"@en ;
  rdfs:domain cim:GovSteam1 ;
  rdfs:range cim:PU ;
  skos:definition "Nonlinear gain valve position point 2 (<i>GV2</i>).  Typical value = 0,4."@en .

cim:GovSteam1.gv3 a owl:DatatypeProperty ;
  rdfs:label "gv3"@en ;
  rdfs:domain cim:GovSteam1 ;
  rdfs:range cim:PU ;
  skos:definition "Nonlinear gain valve position point 3 (<i>GV3</i>).  Typical value = 0,5."@en .

cim:GovSteam1.gv4 a owl:DatatypeProperty ;
  rdfs:label "gv4"@en ;
  rdfs:domain cim:GovSteam1 ;
  rdfs:range cim:PU ;
  skos:definition "Nonlinear gain valve position point 4 (<i>GV4</i>).  Typical value = 0,6."@en .

cim:GovSteam1.gv5 a owl:DatatypeProperty ;
  rdfs:label "gv5"@en ;
  rdfs:domain cim:GovSteam1 ;
  rdfs:range cim:PU ;
  skos:definition "Nonlinear gain valve position point 5 (<i>GV5</i>).  Typical value = 1."@en .

cim:GovSteam1.gv6 a owl:DatatypeProperty ;
  rdfs:label "gv6"@en ;
  rdfs:domain cim:GovSteam1 ;
  rdfs:range cim:PU ;
  skos:definition "Nonlinear gain valve position point 6 (<i>GV6</i>).  Typical value = 0."@en .

cim:GovSteam1.k a owl:DatatypeProperty ;
  rdfs:label "k"@en ;
  rdfs:domain cim:GovSteam1 ;
  rdfs:range cim:PU ;
  skos:definition "Governor gain (reciprocal of droop) (<i>K</i>) (&gt; 0).  Typical value = 25."@en .

cim:GovSteam1.k1 a owl:DatatypeProperty ;
  rdfs:label "k1"@en ;
  rdfs:domain cim:GovSteam1 ;
  rdfs:range xsd:float ;
  skos:definition "Fraction of HP shaft power after first boiler pass (<i>K1</i>).  Typical value = 0,2."@en .

cim:GovSteam1.k2 a owl:DatatypeProperty ;
  rdfs:label "k2"@en ;
  rdfs:domain cim:GovSteam1 ;
  rdfs:range xsd:float ;
  skos:definition "Fraction of LP shaft power after first boiler pass (<i>K2</i>).  Typical value = 0."@en .

cim:GovSteam1.k3 a owl:DatatypeProperty ;
  rdfs:label "k3"@en ;
  rdfs:domain cim:GovSteam1 ;
  rdfs:range xsd:float ;
  skos:definition "Fraction of HP shaft power after second boiler pass (<i>K3</i>).  Typical value = 0,3."@en .

cim:GovSteam1.k4 a owl:DatatypeProperty ;
  rdfs:label "k4"@en ;
  rdfs:domain cim:GovSteam1 ;
  rdfs:range xsd:float ;
  skos:definition "Fraction of LP shaft power after second boiler pass (<i>K4</i>).  Typical value = 0."@en .

cim:GovSteam1.k5 a owl:DatatypeProperty ;
  rdfs:label "k5"@en ;
  rdfs:domain cim:GovSteam1 ;
  rdfs:range xsd:float ;
  skos:definition "Fraction of HP shaft power after third boiler pass (<i>K5</i>).  Typical value = 0,5."@en .

cim:GovSteam1.k6 a owl:DatatypeProperty ;
  rdfs:label "k6"@en ;
  rdfs:domain cim:GovSteam1 ;
  rdfs:range xsd:float ;
  skos:definition "Fraction of LP shaft power after third boiler pass (<i>K6</i>).  Typical value = 0."@en .

cim:GovSteam1.k7 a owl:DatatypeProperty ;
  rdfs:label "k7"@en ;
  rdfs:domain cim:GovSteam1 ;
  rdfs:range xsd:float ;
  skos:definition "Fraction of HP shaft power after fourth boiler pass (<i>K7</i>).  Typical value = 0."@en .

cim:GovSteam1.k8 a owl:DatatypeProperty ;
  rdfs:label "k8"@en ;
  rdfs:domain cim:GovSteam1 ;
  rdfs:range xsd:float ;
  skos:definition "Fraction of LP shaft power after fourth boiler pass (<i>K8</i>).  Typical value = 0."@en .

cim:GovSteam1.mwbase a owl:DatatypeProperty ;
  rdfs:label "mwbase"@en ;
  rdfs:domain cim:GovSteam1 ;
  rdfs:range cim:ActivePower ;
  skos:definition "Base for power values (<i>MWbase</i>) (&gt; 0).  Unit = MW."@en .

cim:GovSteam1.pgv1 a owl:DatatypeProperty ;
  rdfs:label "pgv1"@en ;
  rdfs:domain cim:GovSteam1 ;
  rdfs:range cim:PU ;
  skos:definition "Nonlinear gain power value point 1 (<i>Pgv1</i>).  Typical value = 0."@en .

cim:GovSteam1.pgv2 a owl:DatatypeProperty ;
  rdfs:label "pgv2"@en ;
  rdfs:domain cim:GovSteam1 ;
  rdfs:range cim:PU ;
  skos:definition "Nonlinear gain power value point 2 (<i>Pgv2</i>).  Typical value = 0,75."@en .

cim:GovSteam1.pgv3 a owl:DatatypeProperty ;
  rdfs:label "pgv3"@en ;
  rdfs:domain cim:GovSteam1 ;
  rdfs:range cim:PU ;
  skos:definition "Nonlinear gain power value point 3 (<i>Pgv3</i>).  Typical value = 0,91."@en .

cim:GovSteam1.pgv4 a owl:DatatypeProperty ;
  rdfs:label "pgv4"@en ;
  rdfs:domain cim:GovSteam1 ;
  rdfs:range cim:PU ;
  skos:definition "Nonlinear gain power value point 4 (<i>Pgv4</i>).  Typical value = 0,98."@en .

cim:GovSteam1.pgv5 a owl:DatatypeProperty ;
  rdfs:label "pgv5"@en ;
  rdfs:domain cim:GovSteam1 ;
  rdfs:range cim:PU ;
  skos:definition "Nonlinear gain power value point 5 (<i>Pgv5</i>).  Typical value = 1."@en .

cim:GovSteam1.pgv6 a owl:DatatypeProperty ;
  rdfs:label "pgv6"@en ;
  rdfs:domain cim:GovSteam1 ;
  rdfs:range cim:PU ;
  skos:definition "Nonlinear gain power value point 6 (<i>Pgv6</i>).  Typical value = 0."@en .

cim:GovSteam1.pmax a owl:DatatypeProperty ;
  rdfs:label "pmax"@en ;
  rdfs:domain cim:GovSteam1 ;
  rdfs:range cim:PU ;
  skos:definition "Maximum valve opening (<i>Pmax</i>) (&gt; GovSteam1.pmin).  Typical value = 1."@en .

cim:GovSteam1.pmin a owl:DatatypeProperty ;
  rdfs:label "pmin"@en ;
  rdfs:domain cim:GovSteam1 ;
  rdfs:range cim:PU ;
  skos:definition "Minimum valve opening (<i>Pmin</i>) (&gt;= 0 and &lt; GovSteam1.pmax).  Typical value = 0."@en .

cim:GovSteam1.sdb1 a owl:DatatypeProperty ;
  rdfs:label "sdb1"@en ;
  rdfs:domain cim:GovSteam1 ;
  rdfs:range xsd:boolean ;
  skos:definition """
Intentional deadband indicator.
true = intentional deadband is applied
false = intentional deadband is not applied.
Typical value = true.
\t"""@en .

cim:GovSteam1.sdb2 a owl:DatatypeProperty ;
  rdfs:label "sdb2"@en ;
  rdfs:domain cim:GovSteam1 ;
  rdfs:range xsd:boolean ;
  skos:definition """
Unintentional deadband location.
true = intentional deadband is applied before point "A"
false = intentional deadband is applied after point "A".
Typical value = true.
\t"""@en .

cim:GovSteam1.t1 a owl:DatatypeProperty ;
  rdfs:label "t1"@en ;
  rdfs:domain cim:GovSteam1 ;
  rdfs:range cim:Seconds ;
  skos:definition "Governor lag time constant (<i>T1</i>) (&gt;= 0).  Typical value = 0."@en .

cim:GovSteam1.t2 a owl:DatatypeProperty ;
  rdfs:label "t2"@en ;
  rdfs:domain cim:GovSteam1 ;
  rdfs:range cim:Seconds ;
  skos:definition "Governor lead time constant (<i>T2</i>) (&gt;= 0).  Typical value = 0."@en .

cim:GovSteam1.t3 a owl:DatatypeProperty ;
  rdfs:label "t3"@en ;
  rdfs:domain cim:GovSteam1 ;
  rdfs:range cim:Seconds ;
  skos:definition "Valve positioner time constant (<i>T3) </i>(&gt; 0).  Typical value = 0,1."@en .

cim:GovSteam1.t4 a owl:DatatypeProperty ;
  rdfs:label "t4"@en ;
  rdfs:domain cim:GovSteam1 ;
  rdfs:range cim:Seconds ;
  skos:definition "Inlet piping/steam bowl time constant (<i>T4</i>) (&gt;= 0).  Typical value = 0,3."@en .

cim:GovSteam1.t5 a owl:DatatypeProperty ;
  rdfs:label "t5"@en ;
  rdfs:domain cim:GovSteam1 ;
  rdfs:range cim:Seconds ;
  skos:definition "Time constant of second boiler pass (<i>T5</i>) (&gt;= 0).  Typical value = 5."@en .

cim:GovSteam1.t6 a owl:DatatypeProperty ;
  rdfs:label "t6"@en ;
  rdfs:domain cim:GovSteam1 ;
  rdfs:range cim:Seconds ;
  skos:definition "Time constant of third boiler pass (<i>T6</i>) (&gt;= 0).  Typical value = 0,5."@en .

cim:GovSteam1.t7 a owl:DatatypeProperty ;
  rdfs:label "t7"@en ;
  rdfs:domain cim:GovSteam1 ;
  rdfs:range cim:Seconds ;
  skos:definition "Time constant of fourth boiler pass (<i>T7</i>) (&gt;= 0).  Typical value = 0."@en .

cim:GovSteam1.uc a owl:DatatypeProperty ;
  rdfs:label "uc"@en ;
  rdfs:domain cim:GovSteam1 ;
  rdfs:range xsd:float ;
  skos:definition "Maximum valve closing velocity (<i>Uc</i>) (&lt; 0).  Unit = PU / s.  Typical value = -10."@en .

cim:GovSteam1.uo a owl:DatatypeProperty ;
  rdfs:label "uo"@en ;
  rdfs:domain cim:GovSteam1 ;
  rdfs:range xsd:float ;
  skos:definition "Maximum valve opening velocity (<i>Uo</i>) (&gt; 0).  Unit = PU / s.  Typical value = 1."@en .

cim:GovSteam1.valve a owl:DatatypeProperty ;
  rdfs:label "valve"@en ;
  rdfs:domain cim:GovSteam1 ;
  rdfs:range xsd:boolean ;
  skos:definition """
Nonlinear valve characteristic.
true = nonlinear valve characteristic is used
false = nonlinear valve characteristic is not used.
Typical value = true.
\t"""@en .

cim:GovSteam2.dbf a owl:DatatypeProperty ;
  rdfs:label "dbf"@en ;
  rdfs:domain cim:GovSteam2 ;
  rdfs:range cim:PU ;
  skos:definition "Frequency deadband (<i>DBF</i>).  Typical value = 0."@en .

cim:GovSteam2.k a owl:DatatypeProperty ;
  rdfs:label "k"@en ;
  rdfs:domain cim:GovSteam2 ;
  rdfs:range xsd:float ;
  skos:definition "Governor gain (reciprocal of droop) (<i>K</i>).  Typical value = 20."@en .

cim:GovSteam2.mnef a owl:DatatypeProperty ;
  rdfs:label "mnef"@en ;
  rdfs:domain cim:GovSteam2 ;
  rdfs:range cim:PU ;
  skos:definition "Fuel flow maximum negative error value (<i>MN</i><i><sub>EF</sub></i>).  Typical value = -1."@en .

cim:GovSteam2.mxef a owl:DatatypeProperty ;
  rdfs:label "mxef"@en ;
  rdfs:domain cim:GovSteam2 ;
  rdfs:range cim:PU ;
  skos:definition "Fuel flow maximum positive error value (<i>MX</i><i><sub>EF</sub></i>).  Typical value = 1."@en .

cim:GovSteam2.pmax a owl:DatatypeProperty ;
  rdfs:label "pmax"@en ;
  rdfs:domain cim:GovSteam2 ;
  rdfs:range cim:PU ;
  skos:definition "Maximum fuel flow (<i>P</i><i><sub>MAX</sub></i>) (&gt; GovSteam2.pmin).  Typical value = 1."@en .

cim:GovSteam2.pmin a owl:DatatypeProperty ;
  rdfs:label "pmin"@en ;
  rdfs:domain cim:GovSteam2 ;
  rdfs:range cim:PU ;
  skos:definition "Minimum fuel flow (<i>P</i><i><sub>MIN</sub></i>) (&lt; GovSteam2.pmax).  Typical value = 0."@en .

cim:GovSteam2.t1 a owl:DatatypeProperty ;
  rdfs:label "t1"@en ;
  rdfs:domain cim:GovSteam2 ;
  rdfs:range cim:Seconds ;
  skos:definition "Governor lag time constant (<i>T</i><i><sub>1</sub></i>) (&gt; 0).  Typical value = 0,45."@en .

cim:GovSteam2.t2 a owl:DatatypeProperty ;
  rdfs:label "t2"@en ;
  rdfs:domain cim:GovSteam2 ;
  rdfs:range cim:Seconds ;
  skos:definition "Governor lead time constant (<i>T</i><i><sub>2</sub></i>) (&gt;= 0).  Typical value = 0."@en .

cim:GovSteamBB.fcut a owl:DatatypeProperty ;
  rdfs:label "fcut"@en ;
  rdfs:domain cim:GovSteamBB ;
  rdfs:range cim:PU ;
  skos:definition "Frequency deadband (<i>f</i><i><sub>cut</sub></i>) (&gt;= 0).  Typical value = 0,002."@en .

cim:GovSteamBB.k2 a owl:DatatypeProperty ;
  rdfs:label "k2"@en ;
  rdfs:domain cim:GovSteamBB ;
  rdfs:range cim:PU ;
  skos:definition "Gain (<i>K2</i>).  Typical value = 0,75."@en .

cim:GovSteamBB.k3 a owl:DatatypeProperty ;
  rdfs:label "k3"@en ;
  rdfs:domain cim:GovSteamBB ;
  rdfs:range cim:PU ;
  skos:definition "Gain (<i>K3</i>).  Typical value = 0,5."@en .

cim:GovSteamBB.kd a owl:DatatypeProperty ;
  rdfs:label "kd"@en ;
  rdfs:domain cim:GovSteamBB ;
  rdfs:range cim:PU ;
  skos:definition "Gain (<i>Kd</i>).  Typical value = 1,0."@en .

cim:GovSteamBB.kg a owl:DatatypeProperty ;
  rdfs:label "kg"@en ;
  rdfs:domain cim:GovSteamBB ;
  rdfs:range cim:PU ;
  skos:definition "Gain (<i>Kg</i>).  Typical value = 1,0."@en .

cim:GovSteamBB.kls a owl:DatatypeProperty ;
  rdfs:label "kls"@en ;
  rdfs:domain cim:GovSteamBB ;
  rdfs:range cim:PU ;
  skos:definition "Gain (<i>Kls</i>) (&gt; 0).  Typical value = 0,1."@en .

cim:GovSteamBB.kp a owl:DatatypeProperty ;
  rdfs:label "kp"@en ;
  rdfs:domain cim:GovSteamBB ;
  rdfs:range cim:PU ;
  skos:definition "Gain (<i>Kp</i>).  Typical value = 1,0."@en .

cim:GovSteamBB.ks a owl:DatatypeProperty ;
  rdfs:label "ks"@en ;
  rdfs:domain cim:GovSteamBB ;
  rdfs:range cim:PU ;
  skos:definition "Gain (<i>Ks</i>).  Typical value = 21,0."@en .

cim:GovSteamBB.peflag a owl:DatatypeProperty ;
  rdfs:label "peflag"@en ;
  rdfs:domain cim:GovSteamBB ;
  rdfs:range xsd:boolean ;
  skos:definition """
Electric power input selection (Peflag).  
true = electric power input
false = feedback signal.
Typical value = false.
\t"""@en .

cim:GovSteamBB.pmax a owl:DatatypeProperty ;
  rdfs:label "pmax"@en ;
  rdfs:domain cim:GovSteamBB ;
  rdfs:range cim:PU ;
  skos:definition "High power limit (<i>Pmax</i>) (&gt; GovSteamBB.pmin).  Typical value = 1,0."@en .

cim:GovSteamBB.pmin a owl:DatatypeProperty ;
  rdfs:label "pmin"@en ;
  rdfs:domain cim:GovSteamBB ;
  rdfs:range cim:PU ;
  skos:definition "Low power limit (<i>Pmin</i>) (&lt; GovSteamBB.pmax).  Typical value = 0."@en .

cim:GovSteamBB.t1 a owl:DatatypeProperty ;
  rdfs:label "t1"@en ;
  rdfs:domain cim:GovSteamBB ;
  rdfs:range cim:Seconds ;
  skos:definition "Time constant (<i>T1</i>).  Typical value = 0,05."@en .

cim:GovSteamBB.t4 a owl:DatatypeProperty ;
  rdfs:label "t4"@en ;
  rdfs:domain cim:GovSteamBB ;
  rdfs:range cim:Seconds ;
  skos:definition "Time constant (<i>T4</i>).  Typical value = 0,15."@en .

cim:GovSteamBB.t5 a owl:DatatypeProperty ;
  rdfs:label "t5"@en ;
  rdfs:domain cim:GovSteamBB ;
  rdfs:range cim:Seconds ;
  skos:definition "Time constant (<i>T5</i>).  Typical value = 12,0."@en .

cim:GovSteamBB.t6 a owl:DatatypeProperty ;
  rdfs:label "t6"@en ;
  rdfs:domain cim:GovSteamBB ;
  rdfs:range cim:Seconds ;
  skos:definition "Time constant (<i>T6</i>).  Typical value = 0,75."@en .

cim:GovSteamBB.td a owl:DatatypeProperty ;
  rdfs:label "td"@en ;
  rdfs:domain cim:GovSteamBB ;
  rdfs:range cim:Seconds ;
  skos:definition "Time constant (<i>Td</i>) (&gt; 0).  Typical value = 1,0."@en .

cim:GovSteamBB.tn a owl:DatatypeProperty ;
  rdfs:label "tn"@en ;
  rdfs:domain cim:GovSteamBB ;
  rdfs:range cim:Seconds ;
  skos:definition "Time constant (<i>Tn</i>) (&gt; 0).  Typical value = 1,0."@en .

cim:GovSteamCC.dhp a owl:DatatypeProperty ;
  rdfs:label "dhp"@en ;
  rdfs:domain cim:GovSteamCC ;
  rdfs:range cim:PU ;
  skos:definition "HP damping factor (<i>Dhp</i>).  Typical value = 0."@en .

cim:GovSteamCC.dlp a owl:DatatypeProperty ;
  rdfs:label "dlp"@en ;
  rdfs:domain cim:GovSteamCC ;
  rdfs:range cim:PU ;
  skos:definition "LP damping factor (<i>Dlp</i>).  Typical value = 0."@en .

cim:GovSteamCC.fhp a owl:DatatypeProperty ;
  rdfs:label "fhp"@en ;
  rdfs:domain cim:GovSteamCC ;
  rdfs:range cim:PU ;
  skos:definition "Fraction of HP power ahead of reheater (<i>Fhp</i>).  Typical value = 0,3."@en .

cim:GovSteamCC.flp a owl:DatatypeProperty ;
  rdfs:label "flp"@en ;
  rdfs:domain cim:GovSteamCC ;
  rdfs:range cim:PU ;
  skos:definition "Fraction of LP power ahead of reheater (<i>Flp</i>).  Typical value = 0,7."@en .

cim:GovSteamCC.mwbase a owl:DatatypeProperty ;
  rdfs:label "mwbase"@en ;
  rdfs:domain cim:GovSteamCC ;
  rdfs:range cim:ActivePower ;
  skos:definition "Base for power values (<i>MWbase</i>) (&gt; 0).  Unit = MW."@en .

cim:GovSteamCC.pmaxhp a owl:DatatypeProperty ;
  rdfs:label "pmaxhp"@en ;
  rdfs:domain cim:GovSteamCC ;
  rdfs:range cim:PU ;
  skos:definition "Maximum HP value position (<i>Pmaxhp</i>).  Typical value = 1."@en .

cim:GovSteamCC.pmaxlp a owl:DatatypeProperty ;
  rdfs:label "pmaxlp"@en ;
  rdfs:domain cim:GovSteamCC ;
  rdfs:range cim:PU ;
  skos:definition "Maximum LP value position (<i>Pmaxlp</i>).  Typical value = 1."@en .

cim:GovSteamCC.rhp a owl:DatatypeProperty ;
  rdfs:label "rhp"@en ;
  rdfs:domain cim:GovSteamCC ;
  rdfs:range cim:PU ;
  skos:definition "HP governor droop (<i>Rhp</i>) (&gt; 0).  Typical value = 0,05."@en .

cim:GovSteamCC.rlp a owl:DatatypeProperty ;
  rdfs:label "rlp"@en ;
  rdfs:domain cim:GovSteamCC ;
  rdfs:range cim:PU ;
  skos:definition "LP governor droop (<i>Rlp</i>) (&gt; 0).  Typical value = 0,05."@en .

cim:GovSteamCC.t1hp a owl:DatatypeProperty ;
  rdfs:label "t1hp"@en ;
  rdfs:domain cim:GovSteamCC ;
  rdfs:range cim:Seconds ;
  skos:definition "HP governor time constant (<i>T1hp</i>) (&gt;= 0).  Typical value = 0,1."@en .

cim:GovSteamCC.t1lp a owl:DatatypeProperty ;
  rdfs:label "t1lp"@en ;
  rdfs:domain cim:GovSteamCC ;
  rdfs:range cim:Seconds ;
  skos:definition "LP governor time constant (<i>T1lp</i>) (&gt;= 0).  Typical value = 0,1."@en .

cim:GovSteamCC.t3hp a owl:DatatypeProperty ;
  rdfs:label "t3hp"@en ;
  rdfs:domain cim:GovSteamCC ;
  rdfs:range cim:Seconds ;
  skos:definition "HP turbine time constant (<i>T3hp</i>) (&gt;= 0).  Typical value = 0,1."@en .

cim:GovSteamCC.t3lp a owl:DatatypeProperty ;
  rdfs:label "t3lp"@en ;
  rdfs:domain cim:GovSteamCC ;
  rdfs:range cim:Seconds ;
  skos:definition "LP turbine time constant (<i>T3lp</i>) (&gt;= 0).  Typical value = 0,1."@en .

cim:GovSteamCC.t4hp a owl:DatatypeProperty ;
  rdfs:label "t4hp"@en ;
  rdfs:domain cim:GovSteamCC ;
  rdfs:range cim:Seconds ;
  skos:definition "HP turbine time constant (<i>T4hp</i>) (&gt;= 0).  Typical value = 0,1."@en .

cim:GovSteamCC.t4lp a owl:DatatypeProperty ;
  rdfs:label "t4lp"@en ;
  rdfs:domain cim:GovSteamCC ;
  rdfs:range cim:Seconds ;
  skos:definition "LP turbine time constant (<i>T4lp</i>) (&gt;= 0).  Typical value = 0,1."@en .

cim:GovSteamCC.t5hp a owl:DatatypeProperty ;
  rdfs:label "t5hp"@en ;
  rdfs:domain cim:GovSteamCC ;
  rdfs:range cim:Seconds ;
  skos:definition "HP reheater time constant (<i>T5hp</i>) (&gt;= 0).  Typical value = 10."@en .

cim:GovSteamCC.t5lp a owl:DatatypeProperty ;
  rdfs:label "t5lp"@en ;
  rdfs:domain cim:GovSteamCC ;
  rdfs:range cim:Seconds ;
  skos:definition "LP reheater time constant (<i>T5lp</i>) (&gt;= 0).  Typical value = 10."@en .

cim:GovSteamEU.chc a owl:DatatypeProperty ;
  rdfs:label "chc"@en ;
  rdfs:domain cim:GovSteamEU ;
  rdfs:range xsd:float ;
  skos:definition "Control valves rate closing limit (<i>Chc</i>).  Unit = PU / s.  Typical value = -3,3."@en .

cim:GovSteamEU.cho a owl:DatatypeProperty ;
  rdfs:label "cho"@en ;
  rdfs:domain cim:GovSteamEU ;
  rdfs:range xsd:float ;
  skos:definition "Control valves rate opening limit (<i>Cho</i>).  Unit = PU / s.  Typical value = 0,17."@en .

cim:GovSteamEU.cic a owl:DatatypeProperty ;
  rdfs:label "cic"@en ;
  rdfs:domain cim:GovSteamEU ;
  rdfs:range cim:PU ;
  skos:definition "Intercept valves rate closing limit (<i>Cic</i>).  Typical value = -2,2."@en .

cim:GovSteamEU.cio a owl:DatatypeProperty ;
  rdfs:label "cio"@en ;
  rdfs:domain cim:GovSteamEU ;
  rdfs:range cim:PU ;
  skos:definition "Intercept valves rate opening limit (<i>Cio</i>).  Typical value = 0,123."@en .

cim:GovSteamEU.db1 a owl:DatatypeProperty ;
  rdfs:label "db1"@en ;
  rdfs:domain cim:GovSteamEU ;
  rdfs:range cim:PU ;
  skos:definition "Deadband of the frequency corrector (<i>db1</i>).  Typical value = 0."@en .

cim:GovSteamEU.db2 a owl:DatatypeProperty ;
  rdfs:label "db2"@en ;
  rdfs:domain cim:GovSteamEU ;
  rdfs:range cim:PU ;
  skos:definition "Deadband of the speed governor (<i>db2</i>).  Typical value = 0,0004."@en .

cim:GovSteamEU.hhpmax a owl:DatatypeProperty ;
  rdfs:label "hhpmax"@en ;
  rdfs:domain cim:GovSteamEU ;
  rdfs:range cim:PU ;
  skos:definition "Maximum control valve position (<i>Hhpmax</i>).  Typical value = 1."@en .

cim:GovSteamEU.ke a owl:DatatypeProperty ;
  rdfs:label "ke"@en ;
  rdfs:domain cim:GovSteamEU ;
  rdfs:range cim:PU ;
  skos:definition "Gain of the power controller (<i>Ke</i>).  Typical value = 0,65."@en .

cim:GovSteamEU.kfcor a owl:DatatypeProperty ;
  rdfs:label "kfcor"@en ;
  rdfs:domain cim:GovSteamEU ;
  rdfs:range cim:PU ;
  skos:definition "Gain of the frequency corrector (<i>Kfcor</i>).  Typical value = 20."@en .

cim:GovSteamEU.khp a owl:DatatypeProperty ;
  rdfs:label "khp"@en ;
  rdfs:domain cim:GovSteamEU ;
  rdfs:range cim:PU ;
  skos:definition "Fraction of total turbine output generated by HP part (<i>Khp</i>).  Typical value = 0,277."@en .

cim:GovSteamEU.klp a owl:DatatypeProperty ;
  rdfs:label "klp"@en ;
  rdfs:domain cim:GovSteamEU ;
  rdfs:range cim:PU ;
  skos:definition "Fraction of total turbine output generated by HP part (<i>Klp</i>).  Typical value = 0,723."@en .

cim:GovSteamEU.komegacor a owl:DatatypeProperty ;
  rdfs:label "komegacor"@en ;
  rdfs:domain cim:GovSteamEU ;
  rdfs:range cim:PU ;
  skos:definition "Gain of the speed governor (<i>Kwcor</i>).  Typical value = 20."@en .

cim:GovSteamEU.mwbase a owl:DatatypeProperty ;
  rdfs:label "mwbase"@en ;
  rdfs:domain cim:GovSteamEU ;
  rdfs:range cim:ActivePower ;
  skos:definition "Base for power values (<i>MWbase</i>) (&gt; 0).  Unit = MW."@en .

cim:GovSteamEU.pmax a owl:DatatypeProperty ;
  rdfs:label "pmax"@en ;
  rdfs:domain cim:GovSteamEU ;
  rdfs:range cim:PU ;
  skos:definition "Maximal active power of the turbine (<i>Pmax</i>).  Typical value = 1."@en .

cim:GovSteamEU.prhmax a owl:DatatypeProperty ;
  rdfs:label "prhmax"@en ;
  rdfs:domain cim:GovSteamEU ;
  rdfs:range cim:PU ;
  skos:definition "Maximum low pressure limit (<i>Prhmax</i>).  Typical value = 1,4."@en .

cim:GovSteamEU.simx a owl:DatatypeProperty ;
  rdfs:label "simx"@en ;
  rdfs:domain cim:GovSteamEU ;
  rdfs:range cim:PU ;
  skos:definition "Intercept valves transfer limit (<i>Simx</i>).  Typical value = 0,425."@en .

cim:GovSteamEU.tb a owl:DatatypeProperty ;
  rdfs:label "tb"@en ;
  rdfs:domain cim:GovSteamEU ;
  rdfs:range cim:Seconds ;
  skos:definition "Boiler time constant (<i>Tb</i>) (&gt;= 0).  Typical value = 100."@en .

cim:GovSteamEU.tdp a owl:DatatypeProperty ;
  rdfs:label "tdp"@en ;
  rdfs:domain cim:GovSteamEU ;
  rdfs:range cim:Seconds ;
  skos:definition "Derivative time constant of the power controller (<i>Tdp</i>) (&gt;= 0).  Typical value = 0."@en .

cim:GovSteamEU.ten a owl:DatatypeProperty ;
  rdfs:label "ten"@en ;
  rdfs:domain cim:GovSteamEU ;
  rdfs:range cim:Seconds ;
  skos:definition "Electro hydraulic transducer (<i>Ten</i>) (&gt;= 0).  Typical value = 0,1."@en .

cim:GovSteamEU.tf a owl:DatatypeProperty ;
  rdfs:label "tf"@en ;
  rdfs:domain cim:GovSteamEU ;
  rdfs:range cim:Seconds ;
  skos:definition "Frequency transducer time constant (<i>Tf</i>) (&gt;= 0).  Typical value = 0."@en .

cim:GovSteamEU.tfp a owl:DatatypeProperty ;
  rdfs:label "tfp"@en ;
  rdfs:domain cim:GovSteamEU ;
  rdfs:range cim:Seconds ;
  skos:definition "Time constant of the power controller (<i>Tfp</i>) (&gt;= 0).  Typical value = 0."@en .

cim:GovSteamEU.thp a owl:DatatypeProperty ;
  rdfs:label "thp"@en ;
  rdfs:domain cim:GovSteamEU ;
  rdfs:range cim:Seconds ;
  skos:definition "High pressure (HP) time constant of the turbine (<i>Thp</i>) (&gt;= 0).  Typical value = 0,31."@en .

cim:GovSteamEU.tip a owl:DatatypeProperty ;
  rdfs:label "tip"@en ;
  rdfs:domain cim:GovSteamEU ;
  rdfs:range cim:Seconds ;
  skos:definition "Integral time constant of the power controller (<i>Tip</i>) (&gt;= 0).  Typical value = 2."@en .

cim:GovSteamEU.tlp a owl:DatatypeProperty ;
  rdfs:label "tlp"@en ;
  rdfs:domain cim:GovSteamEU ;
  rdfs:range cim:Seconds ;
  skos:definition "Low pressure (LP) time constant of the turbine (<i>Tlp</i>) (&gt;= 0).  Typical value = 0,45."@en .

cim:GovSteamEU.tp a owl:DatatypeProperty ;
  rdfs:label "tp"@en ;
  rdfs:domain cim:GovSteamEU ;
  rdfs:range cim:Seconds ;
  skos:definition "Power transducer time constant (<i>Tp</i>) (&gt;= 0).  Typical value = 0,07."@en .

cim:GovSteamEU.trh a owl:DatatypeProperty ;
  rdfs:label "trh"@en ;
  rdfs:domain cim:GovSteamEU ;
  rdfs:range cim:Seconds ;
  skos:definition "Reheater  time constant of the turbine (<i>Trh</i>) (&gt;= 0).  Typical value = 8."@en .

cim:GovSteamEU.tvhp a owl:DatatypeProperty ;
  rdfs:label "tvhp"@en ;
  rdfs:domain cim:GovSteamEU ;
  rdfs:range cim:Seconds ;
  skos:definition "Control valves servo time constant (<i>Tvhp</i>) (&gt;= 0).  Typical value = 0,1."@en .

cim:GovSteamEU.tvip a owl:DatatypeProperty ;
  rdfs:label "tvip"@en ;
  rdfs:domain cim:GovSteamEU ;
  rdfs:range cim:Seconds ;
  skos:definition "Intercept valves servo time constant (<i>Tvip</i>) (&gt;= 0).  Typical value = 0,15."@en .

cim:GovSteamEU.tw a owl:DatatypeProperty ;
  rdfs:label "tw"@en ;
  rdfs:domain cim:GovSteamEU ;
  rdfs:range cim:Seconds ;
  skos:definition "Speed transducer time constant (<i>Tw</i>) (&gt;= 0).  Typical value = 0,02."@en .

cim:GovSteamEU.wfmax a owl:DatatypeProperty ;
  rdfs:label "wfmax"@en ;
  rdfs:domain cim:GovSteamEU ;
  rdfs:range cim:PU ;
  skos:definition "Upper limit for frequency correction (<i>Wfmax</i>) (&gt; GovSteamEU.wfmin).  Typical value = 0,05."@en .

cim:GovSteamEU.wfmin a owl:DatatypeProperty ;
  rdfs:label "wfmin"@en ;
  rdfs:domain cim:GovSteamEU ;
  rdfs:range cim:PU ;
  skos:definition "Lower limit for frequency correction (<i>Wfmin</i>) (&lt; GovSteamEU.wfmax).  Typical value = -0,05."@en .

cim:GovSteamEU.wmax1 a owl:DatatypeProperty ;
  rdfs:label "wmax1"@en ;
  rdfs:domain cim:GovSteamEU ;
  rdfs:range cim:PU ;
  skos:definition "Emergency speed control lower limit (<i>wmax1</i>).  Typical value = 1,025."@en .

cim:GovSteamEU.wmax2 a owl:DatatypeProperty ;
  rdfs:label "wmax2"@en ;
  rdfs:domain cim:GovSteamEU ;
  rdfs:range cim:PU ;
  skos:definition "Emergency speed control upper limit (<i>wmax2</i>).  Typical value = 1,05."@en .

cim:GovSteamEU.wwmax a owl:DatatypeProperty ;
  rdfs:label "wwmax"@en ;
  rdfs:domain cim:GovSteamEU ;
  rdfs:range cim:PU ;
  skos:definition "Upper limit for the speed governor (<i>Wwmax</i>) (&gt; GovSteamEU.wwmin).  Typical value = 0,1."@en .

cim:GovSteamEU.wwmin a owl:DatatypeProperty ;
  rdfs:label "wwmin"@en ;
  rdfs:domain cim:GovSteamEU ;
  rdfs:range cim:PU ;
  skos:definition "Lower limit for the speed governor frequency correction (<i>Wwmin</i>) (&lt; GovSteamEU.wwmax).  Typical value = -1."@en .

cim:GovSteamFV2.dt a owl:DatatypeProperty ;
  rdfs:label "dt"@en ;
  rdfs:domain cim:GovSteamFV2 ;
  rdfs:range cim:PU ;
  skos:definition "(<i>Dt</i>)."@en .

cim:GovSteamFV2.k a owl:DatatypeProperty ;
  rdfs:label "k"@en ;
  rdfs:domain cim:GovSteamFV2 ;
  rdfs:range cim:PU ;
  skos:definition "Fraction of the turbine power developed by turbine sections not involved in fast valving (<i>K</i>)."@en .

cim:GovSteamFV2.mwbase a owl:DatatypeProperty ;
  rdfs:label "mwbase"@en ;
  rdfs:domain cim:GovSteamFV2 ;
  rdfs:range cim:ActivePower ;
  skos:definition "Alternate base used instead of machine base in equipment model if necessary (<i>MWbase</i>) (&gt; 0).  Unit = MW."@en .

cim:GovSteamFV2.r a owl:DatatypeProperty ;
  rdfs:label "r"@en ;
  rdfs:domain cim:GovSteamFV2 ;
  rdfs:range cim:PU ;
  skos:definition "(<i>R</i>)."@en .

cim:GovSteamFV2.t1 a owl:DatatypeProperty ;
  rdfs:label "t1"@en ;
  rdfs:domain cim:GovSteamFV2 ;
  rdfs:range cim:Seconds ;
  skos:definition "Governor time constant (<i>T1</i>) (&gt;= 0)."@en .

cim:GovSteamFV2.t3 a owl:DatatypeProperty ;
  rdfs:label "t3"@en ;
  rdfs:domain cim:GovSteamFV2 ;
  rdfs:range cim:Seconds ;
  skos:definition "Reheater time constant (<i>T3</i>) (&gt;= 0)."@en .

cim:GovSteamFV2.ta a owl:DatatypeProperty ;
  rdfs:label "ta"@en ;
  rdfs:domain cim:GovSteamFV2 ;
  rdfs:range cim:Seconds ;
  skos:definition "Time after initial time for valve to close (<i>Ta</i>) (&gt;= 0)."@en .

cim:GovSteamFV2.tb a owl:DatatypeProperty ;
  rdfs:label "tb"@en ;
  rdfs:domain cim:GovSteamFV2 ;
  rdfs:range cim:Seconds ;
  skos:definition "Time after initial time for valve to begin opening (<i>Tb</i>) (&gt;= 0)."@en .

cim:GovSteamFV2.tc a owl:DatatypeProperty ;
  rdfs:label "tc"@en ;
  rdfs:domain cim:GovSteamFV2 ;
  rdfs:range cim:Seconds ;
  skos:definition "Time after initial time for valve to become fully open (<i>Tc</i>) (&gt;= 0)."@en .

cim:GovSteamFV2.tt a owl:DatatypeProperty ;
  rdfs:label "tt"@en ;
  rdfs:domain cim:GovSteamFV2 ;
  rdfs:range cim:Seconds ;
  skos:definition "Time constant with which power falls off after intercept valve closure (<i>Tt</i>) (&gt;= 0)."@en .

cim:GovSteamFV2.vmax a owl:DatatypeProperty ;
  rdfs:label "vmax"@en ;
  rdfs:domain cim:GovSteamFV2 ;
  rdfs:range cim:PU ;
  skos:definition "(<i>Vmax</i>) (&gt; GovSteamFV2.vmin)."@en .

cim:GovSteamFV2.vmin a owl:DatatypeProperty ;
  rdfs:label "vmin"@en ;
  rdfs:domain cim:GovSteamFV2 ;
  rdfs:range cim:PU ;
  skos:definition "(<i>Vmin</i>) (&lt; GovSteamFV2.vmax)."@en .

cim:GovSteamFV3.gv1 a owl:DatatypeProperty ;
  rdfs:label "gv1"@en ;
  rdfs:domain cim:GovSteamFV3 ;
  rdfs:range cim:PU ;
  skos:definition "Nonlinear gain valve position point 1 (<i>GV1</i>).  Typical value = 0."@en .

cim:GovSteamFV3.gv2 a owl:DatatypeProperty ;
  rdfs:label "gv2"@en ;
  rdfs:domain cim:GovSteamFV3 ;
  rdfs:range cim:PU ;
  skos:definition "Nonlinear gain valve position point 2 (<i>GV2</i>).  Typical value = 0,4."@en .

cim:GovSteamFV3.gv3 a owl:DatatypeProperty ;
  rdfs:label "gv3"@en ;
  rdfs:domain cim:GovSteamFV3 ;
  rdfs:range cim:PU ;
  skos:definition "Nonlinear gain valve position point 3 (<i>GV3</i>).  Typical value = 0,5."@en .

cim:GovSteamFV3.gv4 a owl:DatatypeProperty ;
  rdfs:label "gv4"@en ;
  rdfs:domain cim:GovSteamFV3 ;
  rdfs:range cim:PU ;
  skos:definition "Nonlinear gain valve position point 4 (<i>GV4</i>).  Typical value = 0,6."@en .

cim:GovSteamFV3.gv5 a owl:DatatypeProperty ;
  rdfs:label "gv5"@en ;
  rdfs:domain cim:GovSteamFV3 ;
  rdfs:range cim:PU ;
  skos:definition "Nonlinear gain valve position point 5 (<i>GV5</i>).  Typical value = 1."@en .

cim:GovSteamFV3.gv6 a owl:DatatypeProperty ;
  rdfs:label "gv6"@en ;
  rdfs:domain cim:GovSteamFV3 ;
  rdfs:range cim:PU ;
  skos:definition "Nonlinear gain valve position point 6 (<i>GV6</i>).  Typical value = 0."@en .

cim:GovSteamFV3.k a owl:DatatypeProperty ;
  rdfs:label "k"@en ;
  rdfs:domain cim:GovSteamFV3 ;
  rdfs:range cim:PU ;
  skos:definition "Governor gain, (reciprocal of droop) (<i>K</i>).  Typical value = 20."@en .

cim:GovSteamFV3.k1 a owl:DatatypeProperty ;
  rdfs:label "k1"@en ;
  rdfs:domain cim:GovSteamFV3 ;
  rdfs:range cim:PU ;
  skos:definition "Fraction of turbine power developed after first boiler pass (<i>K1</i>).  Typical value = 0,2."@en .

cim:GovSteamFV3.k2 a owl:DatatypeProperty ;
  rdfs:label "k2"@en ;
  rdfs:domain cim:GovSteamFV3 ;
  rdfs:range cim:PU ;
  skos:definition "Fraction of turbine power developed after second boiler pass (<i>K2</i>).  Typical value = 0,2."@en .

cim:GovSteamFV3.k3 a owl:DatatypeProperty ;
  rdfs:label "k3"@en ;
  rdfs:domain cim:GovSteamFV3 ;
  rdfs:range cim:PU ;
  skos:definition "Fraction of hp turbine power developed after crossover or third boiler pass (<i>K3</i>). Typical value = 0,6."@en .

cim:GovSteamFV3.mwbase a owl:DatatypeProperty ;
  rdfs:label "mwbase"@en ;
  rdfs:domain cim:GovSteamFV3 ;
  rdfs:range cim:ActivePower ;
  skos:definition "Base for power values (<i>MWbase</i>) (&gt; 0).  Unit = MW."@en .

cim:GovSteamFV3.pgv1 a owl:DatatypeProperty ;
  rdfs:label "pgv1"@en ;
  rdfs:domain cim:GovSteamFV3 ;
  rdfs:range cim:PU ;
  skos:definition "Nonlinear gain power value point 1 (<i>Pgv1</i>).  Typical value = 0."@en .

cim:GovSteamFV3.pgv2 a owl:DatatypeProperty ;
  rdfs:label "pgv2"@en ;
  rdfs:domain cim:GovSteamFV3 ;
  rdfs:range cim:PU ;
  skos:definition "Nonlinear gain power value point 2 (<i>Pgv2</i>).  Typical value = 0,75."@en .

cim:GovSteamFV3.pgv3 a owl:DatatypeProperty ;
  rdfs:label "pgv3"@en ;
  rdfs:domain cim:GovSteamFV3 ;
  rdfs:range cim:PU ;
  skos:definition "Nonlinear gain power value point 3 (<i>Pgv3</i>).  Typical value = 0,91."@en .

cim:GovSteamFV3.pgv4 a owl:DatatypeProperty ;
  rdfs:label "pgv4"@en ;
  rdfs:domain cim:GovSteamFV3 ;
  rdfs:range cim:PU ;
  skos:definition "Nonlinear gain power value point 4 (<i>Pgv4</i>).  Typical value = 0,98."@en .

cim:GovSteamFV3.pgv5 a owl:DatatypeProperty ;
  rdfs:label "pgv5"@en ;
  rdfs:domain cim:GovSteamFV3 ;
  rdfs:range cim:PU ;
  skos:definition "Nonlinear gain power value point 5 (<i>Pgv5</i>).  Typical value = 1."@en .

cim:GovSteamFV3.pgv6 a owl:DatatypeProperty ;
  rdfs:label "pgv6"@en ;
  rdfs:domain cim:GovSteamFV3 ;
  rdfs:range cim:PU ;
  skos:definition "Nonlinear gain power value point 6 (<i>Pgv6</i>).  Typical value = 0."@en .

cim:GovSteamFV3.pmax a owl:DatatypeProperty ;
  rdfs:label "pmax"@en ;
  rdfs:domain cim:GovSteamFV3 ;
  rdfs:range cim:PU ;
  skos:definition "Maximum valve opening, PU of <i>MWbase</i> (<i>Pmax</i>) (&gt; GovSteamFV3.pmin).  Typical value = 1."@en .

cim:GovSteamFV3.pmin a owl:DatatypeProperty ;
  rdfs:label "pmin"@en ;
  rdfs:domain cim:GovSteamFV3 ;
  rdfs:range cim:PU ;
  skos:definition "Minimum valve opening, PU of <i>MWbase</i> (<i>Pmin</i>) (&lt; GovSteamFV3.pmax).  Typical value = 0."@en .

cim:GovSteamFV3.prmax a owl:DatatypeProperty ;
  rdfs:label "prmax"@en ;
  rdfs:domain cim:GovSteamFV3 ;
  rdfs:range cim:PU ;
  skos:definition "Max. pressure in reheater (<i>Prmax</i>).  Typical value = 1."@en .

cim:GovSteamFV3.t1 a owl:DatatypeProperty ;
  rdfs:label "t1"@en ;
  rdfs:domain cim:GovSteamFV3 ;
  rdfs:range cim:Seconds ;
  skos:definition "Governor lead time constant (<i>T1</i>) (&gt;= 0).  Typical value = 0."@en .

cim:GovSteamFV3.t2 a owl:DatatypeProperty ;
  rdfs:label "t2"@en ;
  rdfs:domain cim:GovSteamFV3 ;
  rdfs:range cim:Seconds ;
  skos:definition "Governor lag time constant (<i>T2</i>) (&gt;= 0).  Typical value = 0."@en .

cim:GovSteamFV3.t3 a owl:DatatypeProperty ;
  rdfs:label "t3"@en ;
  rdfs:domain cim:GovSteamFV3 ;
  rdfs:range cim:Seconds ;
  skos:definition "Valve positioner time constant (<i>T3</i>) (&gt; 0).  Typical value = 0."@en .

cim:GovSteamFV3.t4 a owl:DatatypeProperty ;
  rdfs:label "t4"@en ;
  rdfs:domain cim:GovSteamFV3 ;
  rdfs:range cim:Seconds ;
  skos:definition "Inlet piping/steam bowl time constant (<i>T4</i>) (&gt;= 0).  Typical value = 0,2."@en .

cim:GovSteamFV3.t5 a owl:DatatypeProperty ;
  rdfs:label "t5"@en ;
  rdfs:domain cim:GovSteamFV3 ;
  rdfs:range cim:Seconds ;
  skos:definition "Time constant of second boiler pass (i.e. reheater) (<i>T5</i>) (&gt; 0 if fast valving is used, otherwise &gt;= 0).  Typical value = 0,5."@en .

cim:GovSteamFV3.t6 a owl:DatatypeProperty ;
  rdfs:label "t6"@en ;
  rdfs:domain cim:GovSteamFV3 ;
  rdfs:range cim:Seconds ;
  skos:definition "Time constant of crossover or third boiler pass (<i>T6</i>) (&gt;= 0).  Typical value = 10."@en .

cim:GovSteamFV3.ta a owl:DatatypeProperty ;
  rdfs:label "ta"@en ;
  rdfs:domain cim:GovSteamFV3 ;
  rdfs:range cim:Seconds ;
  skos:definition "Time to close intercept valve (IV) (<i>Ta</i>) (&gt;= 0).  Typical value = 0,97."@en .

cim:GovSteamFV3.tb a owl:DatatypeProperty ;
  rdfs:label "tb"@en ;
  rdfs:domain cim:GovSteamFV3 ;
  rdfs:range cim:Seconds ;
  skos:definition "Time until IV starts to reopen (<i>Tb</i>) (&gt;= 0).  Typical value = 0,98."@en .

cim:GovSteamFV3.tc a owl:DatatypeProperty ;
  rdfs:label "tc"@en ;
  rdfs:domain cim:GovSteamFV3 ;
  rdfs:range cim:Seconds ;
  skos:definition "Time until IV is fully open (<i>Tc</i>) (&gt;= 0).  Typical value = 0,99."@en .

cim:GovSteamFV3.uc a owl:DatatypeProperty ;
  rdfs:label "uc"@en ;
  rdfs:domain cim:GovSteamFV3 ;
  rdfs:range xsd:float ;
  skos:definition "Maximum valve closing velocity (<i>Uc</i>).  Unit = PU / s.  Typical value = -1."@en .

cim:GovSteamFV3.uo a owl:DatatypeProperty ;
  rdfs:label "uo"@en ;
  rdfs:domain cim:GovSteamFV3 ;
  rdfs:range xsd:float ;
  skos:definition "Maximum valve opening velocity (<i>Uo</i>).  Unit = PU / s.  Typical value = 0,1."@en .

cim:GovSteamFV4.cpsmn a owl:DatatypeProperty ;
  rdfs:label "cpsmn"@en ;
  rdfs:domain cim:GovSteamFV4 ;
  rdfs:range cim:PU ;
  skos:definition "Minimum value of pressure regulator output (<i>Cpsmn</i>).  Typical value = -1."@en .

cim:GovSteamFV4.cpsmx a owl:DatatypeProperty ;
  rdfs:label "cpsmx"@en ;
  rdfs:domain cim:GovSteamFV4 ;
  rdfs:range cim:PU ;
  skos:definition "Maximum value of pressure regulator output (<i>Cpsmx</i>).  Typical value = 1."@en .

cim:GovSteamFV4.crmn a owl:DatatypeProperty ;
  rdfs:label "crmn"@en ;
  rdfs:domain cim:GovSteamFV4 ;
  rdfs:range cim:PU ;
  skos:definition "Minimum value of regulator set-point (<i>Crmn</i>).  Typical value = 0."@en .

cim:GovSteamFV4.crmx a owl:DatatypeProperty ;
  rdfs:label "crmx"@en ;
  rdfs:domain cim:GovSteamFV4 ;
  rdfs:range cim:PU ;
  skos:definition "Maximum value of regulator set-point (<i>Crmx</i>).  Typical value = 1,2."@en .

cim:GovSteamFV4.kdc a owl:DatatypeProperty ;
  rdfs:label "kdc"@en ;
  rdfs:domain cim:GovSteamFV4 ;
  rdfs:range cim:PU ;
  skos:definition "Derivative gain of pressure regulator (<i>Kdc</i>).  Typical value = 1."@en .

cim:GovSteamFV4.kf1 a owl:DatatypeProperty ;
  rdfs:label "kf1"@en ;
  rdfs:domain cim:GovSteamFV4 ;
  rdfs:range cim:PU ;
  skos:definition "Frequency bias (reciprocal of droop) (<i>Kf1</i>).  Typical value = 20."@en .

cim:GovSteamFV4.kf3 a owl:DatatypeProperty ;
  rdfs:label "kf3"@en ;
  rdfs:domain cim:GovSteamFV4 ;
  rdfs:range cim:PU ;
  skos:definition "Frequency control (reciprocal of droop) (<i>Kf3</i>).  Typical value = 20."@en .

cim:GovSteamFV4.khp a owl:DatatypeProperty ;
  rdfs:label "khp"@en ;
  rdfs:domain cim:GovSteamFV4 ;
  rdfs:range cim:PU ;
  skos:definition "Fraction  of total turbine output generated by HP part (<i>Khp</i>).  Typical value = 0,35."@en .

cim:GovSteamFV4.kic a owl:DatatypeProperty ;
  rdfs:label "kic"@en ;
  rdfs:domain cim:GovSteamFV4 ;
  rdfs:range cim:PU ;
  skos:definition "Integral gain of pressure regulator (<i>Kic</i>).  Typical value = 0,0033."@en .

cim:GovSteamFV4.kip a owl:DatatypeProperty ;
  rdfs:label "kip"@en ;
  rdfs:domain cim:GovSteamFV4 ;
  rdfs:range cim:PU ;
  skos:definition "Integral gain of pressure feedback regulator (<i>Kip</i>).  Typical value = 0,5."@en .

cim:GovSteamFV4.kit a owl:DatatypeProperty ;
  rdfs:label "kit"@en ;
  rdfs:domain cim:GovSteamFV4 ;
  rdfs:range cim:PU ;
  skos:definition "Integral gain of electro-hydraulic regulator (<i>Kit</i>).  Typical value = 0,04."@en .

cim:GovSteamFV4.kmp1 a owl:DatatypeProperty ;
  rdfs:label "kmp1"@en ;
  rdfs:domain cim:GovSteamFV4 ;
  rdfs:range cim:PU ;
  skos:definition "First gain coefficient of  intercept valves characteristic (<i>Kmp1</i>).  Typical value = 0,5."@en .

cim:GovSteamFV4.kmp2 a owl:DatatypeProperty ;
  rdfs:label "kmp2"@en ;
  rdfs:domain cim:GovSteamFV4 ;
  rdfs:range cim:PU ;
  skos:definition "Second gain coefficient of intercept valves characteristic (<i>Kmp2</i>).  Typical value = 3,5."@en .

cim:GovSteamFV4.kpc a owl:DatatypeProperty ;
  rdfs:label "kpc"@en ;
  rdfs:domain cim:GovSteamFV4 ;
  rdfs:range cim:PU ;
  skos:definition "Proportional gain of pressure regulator (<i>Kpc</i>).  Typical value = 0,5."@en .

cim:GovSteamFV4.kpp a owl:DatatypeProperty ;
  rdfs:label "kpp"@en ;
  rdfs:domain cim:GovSteamFV4 ;
  rdfs:range cim:PU ;
  skos:definition "Proportional gain of pressure feedback regulator (<i>Kpp</i>).  Typical value = 1."@en .

cim:GovSteamFV4.kpt a owl:DatatypeProperty ;
  rdfs:label "kpt"@en ;
  rdfs:domain cim:GovSteamFV4 ;
  rdfs:range cim:PU ;
  skos:definition "Proportional gain of electro-hydraulic regulator (<i>Kpt</i>).  Typical value = 0,3."@en .

cim:GovSteamFV4.krc a owl:DatatypeProperty ;
  rdfs:label "krc"@en ;
  rdfs:domain cim:GovSteamFV4 ;
  rdfs:range cim:PU ;
  skos:definition "Maximum variation of fuel flow (<i>Krc</i>).  Typical value = 0,05."@en .

cim:GovSteamFV4.ksh a owl:DatatypeProperty ;
  rdfs:label "ksh"@en ;
  rdfs:domain cim:GovSteamFV4 ;
  rdfs:range cim:PU ;
  skos:definition "Pressure loss due to flow friction in the boiler tubes (<i>Ksh</i>).  Typical value = 0,08."@en .

cim:GovSteamFV4.lpi a owl:DatatypeProperty ;
  rdfs:label "lpi"@en ;
  rdfs:domain cim:GovSteamFV4 ;
  rdfs:range cim:PU ;
  skos:definition "Maximum negative power error (<i>Lpi</i>).  Typical value = -0,15."@en .

cim:GovSteamFV4.lps a owl:DatatypeProperty ;
  rdfs:label "lps"@en ;
  rdfs:domain cim:GovSteamFV4 ;
  rdfs:range cim:PU ;
  skos:definition "Maximum positive power error (<i>Lps</i>).  Typical value = 0,03."@en .

cim:GovSteamFV4.mnef a owl:DatatypeProperty ;
  rdfs:label "mnef"@en ;
  rdfs:domain cim:GovSteamFV4 ;
  rdfs:range cim:PU ;
  skos:definition "Lower limit for frequency correction (<i>MN</i><i><sub>EF</sub></i>).  Typical value = -0,05."@en .

cim:GovSteamFV4.mxef a owl:DatatypeProperty ;
  rdfs:label "mxef"@en ;
  rdfs:domain cim:GovSteamFV4 ;
  rdfs:range cim:PU ;
  skos:definition "Upper limit for frequency correction (<i>MX</i><i><sub>EF</sub></i>).  Typical value = 0,05."@en .

cim:GovSteamFV4.pr1 a owl:DatatypeProperty ;
  rdfs:label "pr1"@en ;
  rdfs:domain cim:GovSteamFV4 ;
  rdfs:range cim:PU ;
  skos:definition "First value of pressure set point static characteristic (<i>Pr1</i>).  Typical value = 0,2."@en .

cim:GovSteamFV4.pr2 a owl:DatatypeProperty ;
  rdfs:label "pr2"@en ;
  rdfs:domain cim:GovSteamFV4 ;
  rdfs:range cim:PU ;
  skos:definition "Second value of pressure set point static characteristic, corresponding to <i>Ps0</i> = 1,0 PU (<i>Pr2</i>).  Typical value = 0,75."@en .

cim:GovSteamFV4.psmn a owl:DatatypeProperty ;
  rdfs:label "psmn"@en ;
  rdfs:domain cim:GovSteamFV4 ;
  rdfs:range cim:PU ;
  skos:definition "Minimum value of pressure set point static characteristic (<i>Psmn</i>).  Typical value = 1."@en .

cim:GovSteamFV4.rsmimn a owl:DatatypeProperty ;
  rdfs:label "rsmimn"@en ;
  rdfs:domain cim:GovSteamFV4 ;
  rdfs:range cim:PU ;
  skos:definition "Minimum value of integral regulator (<i>Rsmimn</i>).  Typical value = 0."@en .

cim:GovSteamFV4.rsmimx a owl:DatatypeProperty ;
  rdfs:label "rsmimx"@en ;
  rdfs:domain cim:GovSteamFV4 ;
  rdfs:range cim:PU ;
  skos:definition "Maximum value of integral regulator (<i>Rsmimx</i>).  Typical value = 1,1."@en .

cim:GovSteamFV4.rvgmn a owl:DatatypeProperty ;
  rdfs:label "rvgmn"@en ;
  rdfs:domain cim:GovSteamFV4 ;
  rdfs:range cim:PU ;
  skos:definition "Minimum value of integral regulator (<i>Rvgmn</i>).  Typical value = 0."@en .

cim:GovSteamFV4.rvgmx a owl:DatatypeProperty ;
  rdfs:label "rvgmx"@en ;
  rdfs:domain cim:GovSteamFV4 ;
  rdfs:range cim:PU ;
  skos:definition "Maximum value of integral regulator (<i>Rvgmx</i>).  Typical value = 1,2."@en .

cim:GovSteamFV4.srmn a owl:DatatypeProperty ;
  rdfs:label "srmn"@en ;
  rdfs:domain cim:GovSteamFV4 ;
  rdfs:range cim:PU ;
  skos:definition "Minimum valve opening (<i>Srmn</i>).  Typical value = 0."@en .

cim:GovSteamFV4.srmx a owl:DatatypeProperty ;
  rdfs:label "srmx"@en ;
  rdfs:domain cim:GovSteamFV4 ;
  rdfs:range cim:PU ;
  skos:definition "Maximum valve opening (<i>Srmx</i>).  Typical value = 1,1."@en .

cim:GovSteamFV4.srsmp a owl:DatatypeProperty ;
  rdfs:label "srsmp"@en ;
  rdfs:domain cim:GovSteamFV4 ;
  rdfs:range cim:PU ;
  skos:definition "Intercept valves characteristic discontinuity point (<i>Srsmp</i>).  Typical value = 0,43."@en .

cim:GovSteamFV4.svmn a owl:DatatypeProperty ;
  rdfs:label "svmn"@en ;
  rdfs:domain cim:GovSteamFV4 ;
  rdfs:range xsd:float ;
  skos:definition "Maximum regulator gate closing velocity (<i>Svmn</i>).  Typical value = -0,0333."@en .

cim:GovSteamFV4.svmx a owl:DatatypeProperty ;
  rdfs:label "svmx"@en ;
  rdfs:domain cim:GovSteamFV4 ;
  rdfs:range xsd:float ;
  skos:definition "Maximum regulator gate opening velocity (<i>Svmx</i>).  Typical value = 0,0333."@en .

cim:GovSteamFV4.ta a owl:DatatypeProperty ;
  rdfs:label "ta"@en ;
  rdfs:domain cim:GovSteamFV4 ;
  rdfs:range cim:Seconds ;
  skos:definition "Control valves rate opening time (<i>Ta</i>) (&gt;= 0).  Typical value = 0,8."@en .

cim:GovSteamFV4.tam a owl:DatatypeProperty ;
  rdfs:label "tam"@en ;
  rdfs:domain cim:GovSteamFV4 ;
  rdfs:range cim:Seconds ;
  skos:definition "Intercept valves rate opening time (<i>Tam</i>) (&gt;= 0).  Typical value = 0,8."@en .

cim:GovSteamFV4.tc a owl:DatatypeProperty ;
  rdfs:label "tc"@en ;
  rdfs:domain cim:GovSteamFV4 ;
  rdfs:range cim:Seconds ;
  skos:definition "Control valves rate closing time (<i>Tc</i>) (&gt;= 0).  Typical value = 0,5."@en .

cim:GovSteamFV4.tcm a owl:DatatypeProperty ;
  rdfs:label "tcm"@en ;
  rdfs:domain cim:GovSteamFV4 ;
  rdfs:range cim:Seconds ;
  skos:definition "Intercept valves rate closing time (<i>Tcm</i>) (&gt;= 0).  Typical value = 0,5."@en .

cim:GovSteamFV4.tdc a owl:DatatypeProperty ;
  rdfs:label "tdc"@en ;
  rdfs:domain cim:GovSteamFV4 ;
  rdfs:range cim:Seconds ;
  skos:definition "Derivative time constant of pressure regulator (<i>Tdc</i>) (&gt;= 0).  Typical value = 90."@en .

cim:GovSteamFV4.tf1 a owl:DatatypeProperty ;
  rdfs:label "tf1"@en ;
  rdfs:domain cim:GovSteamFV4 ;
  rdfs:range cim:Seconds ;
  skos:definition "Time constant of fuel regulation (<i>Tf1</i>) (&gt;= 0).  Typical value = 10."@en .

cim:GovSteamFV4.tf2 a owl:DatatypeProperty ;
  rdfs:label "tf2"@en ;
  rdfs:domain cim:GovSteamFV4 ;
  rdfs:range cim:Seconds ;
  skos:definition "Time constant of steam chest (<i>Tf2</i>) (&gt;= 0).  Typical value = 10."@en .

cim:GovSteamFV4.thp a owl:DatatypeProperty ;
  rdfs:label "thp"@en ;
  rdfs:domain cim:GovSteamFV4 ;
  rdfs:range cim:Seconds ;
  skos:definition "High pressure (HP) time constant of the turbine (<i>Thp</i>) (&gt;= 0).  Typical value = 0,15."@en .

cim:GovSteamFV4.tmp a owl:DatatypeProperty ;
  rdfs:label "tmp"@en ;
  rdfs:domain cim:GovSteamFV4 ;
  rdfs:range cim:Seconds ;
  skos:definition "Low pressure (LP) time constant of the turbine (<i>Tmp</i>) (&gt;= 0).  Typical value = 0,4."@en .

cim:GovSteamFV4.trh a owl:DatatypeProperty ;
  rdfs:label "trh"@en ;
  rdfs:domain cim:GovSteamFV4 ;
  rdfs:range cim:Seconds ;
  skos:definition "Reheater  time constant of the turbine (<i>Trh</i>) (&gt;= 0).  Typical value = 10."@en .

cim:GovSteamFV4.tv a owl:DatatypeProperty ;
  rdfs:label "tv"@en ;
  rdfs:domain cim:GovSteamFV4 ;
  rdfs:range cim:Seconds ;
  skos:definition "Boiler time constant (<i>Tv</i>) (&gt;= 0).  Typical value = 60."@en .

cim:GovSteamFV4.ty a owl:DatatypeProperty ;
  rdfs:label "ty"@en ;
  rdfs:domain cim:GovSteamFV4 ;
  rdfs:range cim:Seconds ;
  skos:definition "Control valves servo time constant (<i>Ty</i>) (&gt;= 0).  Typical value = 0,1."@en .

cim:GovSteamFV4.y a owl:DatatypeProperty ;
  rdfs:label "y"@en ;
  rdfs:domain cim:GovSteamFV4 ;
  rdfs:range cim:PU ;
  skos:definition "Coefficient of linearized equations of turbine (Stodola formulation) (<i>Y</i>).  Typical value = 0,13."@en .

cim:GovSteamFV4.yhpmn a owl:DatatypeProperty ;
  rdfs:label "yhpmn"@en ;
  rdfs:domain cim:GovSteamFV4 ;
  rdfs:range cim:PU ;
  skos:definition "Minimum control valve position (<i>Yhpmn</i>).  Typical value = 0."@en .

cim:GovSteamFV4.yhpmx a owl:DatatypeProperty ;
  rdfs:label "yhpmx"@en ;
  rdfs:domain cim:GovSteamFV4 ;
  rdfs:range cim:PU ;
  skos:definition "Maximum control valve position (<i>Yhpmx</i>).  Typical value = 1,1."@en .

cim:GovSteamFV4.ympmn a owl:DatatypeProperty ;
  rdfs:label "ympmn"@en ;
  rdfs:domain cim:GovSteamFV4 ;
  rdfs:range cim:PU ;
  skos:definition "Minimum intercept valve position (<i>Ympmn</i>).  Typical value = 0."@en .

cim:GovSteamFV4.ympmx a owl:DatatypeProperty ;
  rdfs:label "ympmx"@en ;
  rdfs:domain cim:GovSteamFV4 ;
  rdfs:range cim:PU ;
  skos:definition "Maximum intercept valve position (<i>Ympmx</i>).  Typical value = 1,1."@en .

cim:GovSteamIEEE1.k a owl:DatatypeProperty ;
  rdfs:label "k"@en ;
  rdfs:domain cim:GovSteamIEEE1 ;
  rdfs:range cim:PU ;
  skos:definition "Governor gain (reciprocal of droop) (<i>K</i>) (&gt; 0).  Typical value = 25."@en .

cim:GovSteamIEEE1.k1 a owl:DatatypeProperty ;
  rdfs:label "k1"@en ;
  rdfs:domain cim:GovSteamIEEE1 ;
  rdfs:range xsd:float ;
  skos:definition "Fraction of HP shaft power after first boiler pass (<i>K1</i>).  Typical value = 0,2."@en .

cim:GovSteamIEEE1.k2 a owl:DatatypeProperty ;
  rdfs:label "k2"@en ;
  rdfs:domain cim:GovSteamIEEE1 ;
  rdfs:range xsd:float ;
  skos:definition "Fraction of LP shaft power after first boiler pass (<i>K2</i>).  Typical value = 0."@en .

cim:GovSteamIEEE1.k3 a owl:DatatypeProperty ;
  rdfs:label "k3"@en ;
  rdfs:domain cim:GovSteamIEEE1 ;
  rdfs:range xsd:float ;
  skos:definition "Fraction of HP shaft power after second boiler pass (<i>K3</i>).  Typical value = 0,3."@en .

cim:GovSteamIEEE1.k4 a owl:DatatypeProperty ;
  rdfs:label "k4"@en ;
  rdfs:domain cim:GovSteamIEEE1 ;
  rdfs:range xsd:float ;
  skos:definition "Fraction of LP shaft power after second boiler pass (<i>K4</i>).  Typical value = 0."@en .

cim:GovSteamIEEE1.k5 a owl:DatatypeProperty ;
  rdfs:label "k5"@en ;
  rdfs:domain cim:GovSteamIEEE1 ;
  rdfs:range xsd:float ;
  skos:definition "Fraction of HP shaft power after third boiler pass (<i>K5</i>).  Typical value = 0,5."@en .

cim:GovSteamIEEE1.k6 a owl:DatatypeProperty ;
  rdfs:label "k6"@en ;
  rdfs:domain cim:GovSteamIEEE1 ;
  rdfs:range xsd:float ;
  skos:definition "Fraction of LP shaft power after third boiler pass (<i>K6</i>).  Typical value = 0."@en .

cim:GovSteamIEEE1.k7 a owl:DatatypeProperty ;
  rdfs:label "k7"@en ;
  rdfs:domain cim:GovSteamIEEE1 ;
  rdfs:range xsd:float ;
  skos:definition "Fraction of HP shaft power after fourth boiler pass (<i>K7</i>).  Typical value = 0."@en .

cim:GovSteamIEEE1.k8 a owl:DatatypeProperty ;
  rdfs:label "k8"@en ;
  rdfs:domain cim:GovSteamIEEE1 ;
  rdfs:range xsd:float ;
  skos:definition "Fraction of LP shaft power after fourth boiler pass (<i>K8</i>).  Typical value = 0."@en .

cim:GovSteamIEEE1.mwbase a owl:DatatypeProperty ;
  rdfs:label "mwbase"@en ;
  rdfs:domain cim:GovSteamIEEE1 ;
  rdfs:range cim:ActivePower ;
  skos:definition "Base for power values (<i>MWbase</i>) (&gt; 0)<i>. </i>Unit = MW."@en .

cim:GovSteamIEEE1.pmax a owl:DatatypeProperty ;
  rdfs:label "pmax"@en ;
  rdfs:domain cim:GovSteamIEEE1 ;
  rdfs:range cim:PU ;
  skos:definition "Maximum valve opening (<i>Pmax</i>) (&gt; GovSteamIEEE1.pmin).  Typical value = 1."@en .

cim:GovSteamIEEE1.pmin a owl:DatatypeProperty ;
  rdfs:label "pmin"@en ;
  rdfs:domain cim:GovSteamIEEE1 ;
  rdfs:range cim:PU ;
  skos:definition "Minimum valve opening (<i>Pmin</i>) (&gt;= 0 and &lt; GovSteamIEEE1.pmax).  Typical value = 0."@en .

cim:GovSteamIEEE1.t1 a owl:DatatypeProperty ;
  rdfs:label "t1"@en ;
  rdfs:domain cim:GovSteamIEEE1 ;
  rdfs:range cim:Seconds ;
  skos:definition "Governor lag time constant (<i>T1</i>) (&gt;= 0).  Typical value = 0."@en .

cim:GovSteamIEEE1.t2 a owl:DatatypeProperty ;
  rdfs:label "t2"@en ;
  rdfs:domain cim:GovSteamIEEE1 ;
  rdfs:range cim:Seconds ;
  skos:definition "Governor lead time constant (<i>T2</i>) (&gt;= 0).  Typical value = 0."@en .

cim:GovSteamIEEE1.t3 a owl:DatatypeProperty ;
  rdfs:label "t3"@en ;
  rdfs:domain cim:GovSteamIEEE1 ;
  rdfs:range cim:Seconds ;
  skos:definition "Valve positioner time constant (<i>T3</i>) (&gt; 0).  Typical value = 0,1."@en .

cim:GovSteamIEEE1.t4 a owl:DatatypeProperty ;
  rdfs:label "t4"@en ;
  rdfs:domain cim:GovSteamIEEE1 ;
  rdfs:range cim:Seconds ;
  skos:definition "Inlet piping/steam bowl time constant (<i>T4</i>) (&gt;= 0).  Typical value = 0,3."@en .

cim:GovSteamIEEE1.t5 a owl:DatatypeProperty ;
  rdfs:label "t5"@en ;
  rdfs:domain cim:GovSteamIEEE1 ;
  rdfs:range cim:Seconds ;
  skos:definition "Time constant of second boiler pass (<i>T5</i>) (&gt;= 0).  Typical value = 5."@en .

cim:GovSteamIEEE1.t6 a owl:DatatypeProperty ;
  rdfs:label "t6"@en ;
  rdfs:domain cim:GovSteamIEEE1 ;
  rdfs:range cim:Seconds ;
  skos:definition "Time constant of third boiler pass (<i>T6</i>) (&gt;= 0).  Typical value = 0,5."@en .

cim:GovSteamIEEE1.t7 a owl:DatatypeProperty ;
  rdfs:label "t7"@en ;
  rdfs:domain cim:GovSteamIEEE1 ;
  rdfs:range cim:Seconds ;
  skos:definition "Time constant of fourth boiler pass (<i>T7</i>) (&gt;= 0).  Typical value = 0."@en .

cim:GovSteamIEEE1.uc a owl:DatatypeProperty ;
  rdfs:label "uc"@en ;
  rdfs:domain cim:GovSteamIEEE1 ;
  rdfs:range xsd:float ;
  skos:definition "Maximum valve closing velocity (<i>Uc</i>) (&lt; 0).  Unit = PU / s.  Typical value = -10."@en .

cim:GovSteamIEEE1.uo a owl:DatatypeProperty ;
  rdfs:label "uo"@en ;
  rdfs:domain cim:GovSteamIEEE1 ;
  rdfs:range xsd:float ;
  skos:definition "Maximum valve opening velocity (<i>Uo</i>) (&gt; 0).  Unit = PU / s.  Typical value = 1."@en .

cim:GovSteamSGO.k1 a owl:DatatypeProperty ;
  rdfs:label "k1"@en ;
  rdfs:domain cim:GovSteamSGO ;
  rdfs:range cim:PU ;
  skos:definition "One / PU regulation (<i>K1</i>). "@en .

cim:GovSteamSGO.k2 a owl:DatatypeProperty ;
  rdfs:label "k2"@en ;
  rdfs:domain cim:GovSteamSGO ;
  rdfs:range cim:PU ;
  skos:definition "Fraction (<i>K2</i>). "@en .

cim:GovSteamSGO.k3 a owl:DatatypeProperty ;
  rdfs:label "k3"@en ;
  rdfs:domain cim:GovSteamSGO ;
  rdfs:range cim:PU ;
  skos:definition "Fraction (<i>K3</i>)."@en .

cim:GovSteamSGO.mwbase a owl:DatatypeProperty ;
  rdfs:label "mwbase"@en ;
  rdfs:domain cim:GovSteamSGO ;
  rdfs:range cim:ActivePower ;
  skos:definition "Base for power values (<i>MWbase</i>) (&gt; 0).  Unit = MW."@en .

cim:GovSteamSGO.pmax a owl:DatatypeProperty ;
  rdfs:label "pmax"@en ;
  rdfs:domain cim:GovSteamSGO ;
  rdfs:range cim:PU ;
  skos:definition "Upper power limit (<i>Pmax</i>) (&gt; GovSteamSGO.pmin). "@en .

cim:GovSteamSGO.pmin a owl:DatatypeProperty ;
  rdfs:label "pmin"@en ;
  rdfs:domain cim:GovSteamSGO ;
  rdfs:range cim:Seconds ;
  skos:definition "Lower power limit (<i>Pmin</i>) (&gt;= 0 and &lt; GovSteamSGO.pmax)."@en .

cim:GovSteamSGO.t1 a owl:DatatypeProperty ;
  rdfs:label "t1"@en ;
  rdfs:domain cim:GovSteamSGO ;
  rdfs:range cim:Seconds ;
  skos:definition "Controller lag (<i>T1</i>) (&gt;= 0)."@en .

cim:GovSteamSGO.t2 a owl:DatatypeProperty ;
  rdfs:label "t2"@en ;
  rdfs:domain cim:GovSteamSGO ;
  rdfs:range cim:Seconds ;
  skos:definition "Controller lead compensation (<i>T2</i>) (&gt;= 0)."@en .

cim:GovSteamSGO.t3 a owl:DatatypeProperty ;
  rdfs:label "t3"@en ;
  rdfs:domain cim:GovSteamSGO ;
  rdfs:range cim:Seconds ;
  skos:definition "Governor lag (<i>T3</i>) (&gt; 0). "@en .

cim:GovSteamSGO.t4 a owl:DatatypeProperty ;
  rdfs:label "t4"@en ;
  rdfs:domain cim:GovSteamSGO ;
  rdfs:range cim:Seconds ;
  skos:definition "Delay due to steam inlet volumes associated with steam chest and inlet piping (<i>T4</i>) (&gt;= 0). "@en .

cim:GovSteamSGO.t5 a owl:DatatypeProperty ;
  rdfs:label "t5"@en ;
  rdfs:domain cim:GovSteamSGO ;
  rdfs:range cim:Seconds ;
  skos:definition "Reheater delay including hot and cold leads (<i>T5</i>) (&gt;= 0). "@en .

cim:GovSteamSGO.t6 a owl:DatatypeProperty ;
  rdfs:label "t6"@en ;
  rdfs:domain cim:GovSteamSGO ;
  rdfs:range cim:Seconds ;
  skos:definition "Delay due to IP-LP turbine, crossover pipes and LP end hoods (<i>T6</i>) (&gt;= 0). "@en .

cim:IdentifiedObject.description a owl:DatatypeProperty, owl:FunctionalProperty ;
  rdfs:label "description"@en ;
  rdfs:domain cim:IdentifiedObject ;
  rdfs:range xsd:string ;
  skos:definition "The description is a free human readable text describing or naming the object. It may be non unique and may not correlate to a naming hierarchy."@en .

cim:IdentifiedObject.mRID a owl:DatatypeProperty ;
  rdfs:label "mRID"@en ;
  rdfs:domain cim:IdentifiedObject ;
  rdfs:range xsd:string ;
  skos:definition """
Master resource identifier issued by a model authority. The mRID is unique within an exchange context. Global uniqueness is easily achieved by using a UUID, as specified in RFC 4122, for the mRID. The use of UUID is strongly recommended.
For CIMXML data files in RDF syntax conforming to IEC 61970-552, the mRID is mapped to rdf:ID or rdf:about attributes that identify CIM object elements.
\t"""@en .

cim:IdentifiedObject.name a owl:DatatypeProperty, owl:FunctionalProperty ;
  rdfs:label "name"@en ;
  rdfs:domain cim:IdentifiedObject ;
  rdfs:range xsd:string ;
  skos:definition """
The name is any free human readable and possibly non unique text naming the object.

\t"""@en .

cim:Length.multiplier a owl:DatatypeProperty, owl:FunctionalProperty ;
  rdfs:label "multiplier"@en ;
  dy:isFixed "True " ;
  rdf:value "k" ;
  rdfs:domain cim:Length ;
  rdfs:range cim:UnitMultiplier .

cim:Length.unit a owl:DatatypeProperty, owl:FunctionalProperty ;
  rdfs:label "unit"@en ;
  dy:isFixed "True " ;
  rdf:value "m" ;
  rdfs:domain cim:Length ;
  rdfs:range cim:UnitSymbol .

cim:Length.value a owl:DatatypeProperty, owl:FunctionalProperty ;
  rdfs:label "value"@en ;
  rdfs:domain cim:Length ;
  rdfs:range xsd:float .

cim:LoadComposite.epfd a owl:DatatypeProperty ;
  rdfs:label "epfd"@en ;
  rdfs:domain cim:LoadComposite ;
  rdfs:range xsd:float ;
  skos:definition "Active load-frequency dependence index (dynamic) (<i>Epfd</i>).  Typical value = 1,5."@en .

cim:LoadComposite.epfs a owl:DatatypeProperty ;
  rdfs:label "epfs"@en ;
  rdfs:domain cim:LoadComposite ;
  rdfs:range xsd:float ;
  skos:definition "Active load-frequency dependence index (static) (<i>Epfs</i>).  Typical value = 1,5."@en .

cim:LoadComposite.epvd a owl:DatatypeProperty ;
  rdfs:label "epvd"@en ;
  rdfs:domain cim:LoadComposite ;
  rdfs:range xsd:float ;
  skos:definition "Active load-voltage dependence index (dynamic) (<i>Epvd</i>).  Typical value = 0,7."@en .

cim:LoadComposite.epvs a owl:DatatypeProperty ;
  rdfs:label "epvs"@en ;
  rdfs:domain cim:LoadComposite ;
  rdfs:range xsd:float ;
  skos:definition "Active load-voltage dependence index (static) (<i>Epvs</i>).  Typical value = 0,7."@en .

cim:LoadComposite.eqfd a owl:DatatypeProperty ;
  rdfs:label "eqfd"@en ;
  rdfs:domain cim:LoadComposite ;
  rdfs:range xsd:float ;
  skos:definition "Reactive load-frequency dependence index (dynamic) (<i>Eqfd</i>).  Typical value = 0."@en .

cim:LoadComposite.eqfs a owl:DatatypeProperty ;
  rdfs:label "eqfs"@en ;
  rdfs:domain cim:LoadComposite ;
  rdfs:range xsd:float ;
  skos:definition "Reactive load-frequency dependence index (static) (<i>Eqfs</i>).  Typical value = 0."@en .

cim:LoadComposite.eqvd a owl:DatatypeProperty ;
  rdfs:label "eqvd"@en ;
  rdfs:domain cim:LoadComposite ;
  rdfs:range xsd:float ;
  skos:definition "Reactive load-voltage dependence index (dynamic) (<i>Eqvd</i>).  Typical value = 2."@en .

cim:LoadComposite.eqvs a owl:DatatypeProperty ;
  rdfs:label "eqvs"@en ;
  rdfs:domain cim:LoadComposite ;
  rdfs:range xsd:float ;
  skos:definition "Reactive load-voltage dependence index (static) (<i>Eqvs</i>).  Typical value = 2."@en .

cim:LoadComposite.h a owl:DatatypeProperty ;
  rdfs:label "h"@en ;
  rdfs:domain cim:LoadComposite ;
  rdfs:range cim:Seconds ;
  skos:definition "Inertia constant (<i>H</i>) (&gt;= 0).  Typical value = 2,5."@en .

cim:LoadComposite.lfac a owl:DatatypeProperty ;
  rdfs:label "lfac"@en ;
  rdfs:domain cim:LoadComposite ;
  rdfs:range xsd:float ;
  skos:definition "Loading factor (<i>L</i><i><sub>fac</sub></i>). The ratio of initial <i>P</i> to motor MVA base.  Typical value = 0,8."@en .

cim:LoadComposite.pfrac a owl:DatatypeProperty ;
  rdfs:label "pfrac"@en ;
  rdfs:domain cim:LoadComposite ;
  rdfs:range xsd:float ;
  skos:definition "Fraction of constant-power load to be represented by this motor model (<i>P</i><i><sub>FRAC</sub></i>) (&gt;= 0,0 and &lt;= 1,0).  Typical value = 0,5."@en .

cim:LoadGenericNonLinear.bs a owl:DatatypeProperty ;
  rdfs:label "bs"@en ;
  rdfs:domain cim:LoadGenericNonLinear ;
  rdfs:range xsd:float ;
  skos:definition "Steady state voltage index for reactive power (<i>BS</i>)."@en .

cim:LoadGenericNonLinear.bt a owl:DatatypeProperty ;
  rdfs:label "bt"@en ;
  rdfs:domain cim:LoadGenericNonLinear ;
  rdfs:range xsd:float ;
  skos:definition "Transient voltage index for reactive power (<i>BT</i>)."@en .

cim:LoadGenericNonLinear.genericNonLinearLoadModelType a owl:DatatypeProperty ;
  rdfs:label "genericNonLinearLoadModelType"@en ;
  rdfs:domain cim:LoadGenericNonLinear ;
  rdfs:range cim:GenericNonLinearLoadModelKind ;
  skos:definition "Type of generic non-linear load model."@en .

cim:LoadGenericNonLinear.ls a owl:DatatypeProperty ;
  rdfs:label "ls"@en ;
  rdfs:domain cim:LoadGenericNonLinear ;
  rdfs:range xsd:float ;
  skos:definition "Steady state voltage index for active power (<i>LS</i>)."@en .

cim:LoadGenericNonLinear.lt a owl:DatatypeProperty ;
  rdfs:label "lt"@en ;
  rdfs:domain cim:LoadGenericNonLinear ;
  rdfs:range xsd:float ;
  skos:definition "Transient voltage index for active power (<i>LT</i>)."@en .

cim:LoadGenericNonLinear.tp a owl:DatatypeProperty ;
  rdfs:label "tp"@en ;
  rdfs:domain cim:LoadGenericNonLinear ;
  rdfs:range cim:Seconds ;
  skos:definition "Time constant of lag function of active power (<i>T</i><i><sub>P</sub></i>) (&gt; 0)."@en .

cim:LoadGenericNonLinear.tq a owl:DatatypeProperty ;
  rdfs:label "tq"@en ;
  rdfs:domain cim:LoadGenericNonLinear ;
  rdfs:range cim:Seconds ;
  skos:definition "Time constant of lag function of reactive power (<i>T</i><i><sub>Q</sub></i>) (&gt; 0)."@en .

cim:LoadMotor.d a owl:DatatypeProperty ;
  rdfs:label "d"@en ;
  rdfs:domain cim:LoadMotor ;
  rdfs:range xsd:float ;
  skos:definition "Damping factor (<i>D</i>).  Unit = delta <i>P</i>/delta speed.  Typical value = 2."@en .

cim:LoadMotor.h a owl:DatatypeProperty ;
  rdfs:label "h"@en ;
  rdfs:domain cim:LoadMotor ;
  rdfs:range cim:Seconds ;
  skos:definition "Inertia constant (<i>H</i>) (&gt;= 0).  Typical value = 0,4."@en .

cim:LoadMotor.lfac a owl:DatatypeProperty ;
  rdfs:label "lfac"@en ;
  rdfs:domain cim:LoadMotor ;
  rdfs:range xsd:float ;
  skos:definition "Loading factor (<i>Lfac</i>). The ratio of initial <i>P</i> to motor MVA base.  Typical value = 0,8."@en .

cim:LoadMotor.lp a owl:DatatypeProperty ;
  rdfs:label "lp"@en ;
  rdfs:domain cim:LoadMotor ;
  rdfs:range cim:PU ;
  skos:definition "Transient reactance (<i>Lp</i>).  Typical value = 0,15."@en .

cim:LoadMotor.lpp a owl:DatatypeProperty ;
  rdfs:label "lpp"@en ;
  rdfs:domain cim:LoadMotor ;
  rdfs:range cim:PU ;
  skos:definition "Subtransient reactance (<i>Lpp</i>).  Typical value = 0,15."@en .

cim:LoadMotor.ls a owl:DatatypeProperty ;
  rdfs:label "ls"@en ;
  rdfs:domain cim:LoadMotor ;
  rdfs:range cim:PU ;
  skos:definition "Synchronous reactance (<i>Ls</i>).  Typical value = 3,2."@en .

cim:LoadMotor.pfrac a owl:DatatypeProperty ;
  rdfs:label "pfrac"@en ;
  rdfs:domain cim:LoadMotor ;
  rdfs:range xsd:float ;
  skos:definition "Fraction of constant-power load to be represented by this motor model (<i>Pfrac</i>) (&gt;= 0,0 and &lt;= 1,0).  Typical value = 0,3."@en .

cim:LoadMotor.ra a owl:DatatypeProperty ;
  rdfs:label "ra"@en ;
  rdfs:domain cim:LoadMotor ;
  rdfs:range cim:PU ;
  skos:definition "Stator resistance (<i>Ra</i>).  Typical value = 0."@en .

cim:LoadMotor.tbkr a owl:DatatypeProperty ;
  rdfs:label "tbkr"@en ;
  rdfs:domain cim:LoadMotor ;
  rdfs:range cim:Seconds ;
  skos:definition "Circuit breaker operating time (<i>Tbkr</i>) (&gt;= 0).  Typical value = 0,08."@en .

cim:LoadMotor.tpo a owl:DatatypeProperty ;
  rdfs:label "tpo"@en ;
  rdfs:domain cim:LoadMotor ;
  rdfs:range cim:Seconds ;
  skos:definition "Transient rotor time constant (<i>Tpo</i>) (&gt;= 0).  Typical value = 1."@en .

cim:LoadMotor.tppo a owl:DatatypeProperty ;
  rdfs:label "tppo"@en ;
  rdfs:domain cim:LoadMotor ;
  rdfs:range cim:Seconds ;
  skos:definition "Subtransient rotor time constant (<i>Tppo</i>) (&gt;= 0).  Typical value = 0,02."@en .

cim:LoadMotor.tv a owl:DatatypeProperty ;
  rdfs:label "tv"@en ;
  rdfs:domain cim:LoadMotor ;
  rdfs:range cim:Seconds ;
  skos:definition "Voltage trip pickup time (<i>Tv</i>) (&gt;= 0).  Typical value = 0,1."@en .

cim:LoadMotor.vt a owl:DatatypeProperty ;
  rdfs:label "vt"@en ;
  rdfs:domain cim:LoadMotor ;
  rdfs:range cim:PU ;
  skos:definition "Voltage threshold for tripping (<i>Vt</i>).  Typical value = 0,7."@en .

cim:LoadStatic.ep1 a owl:DatatypeProperty, owl:FunctionalProperty ;
  rdfs:label "ep1"@en ;
  rdfs:domain cim:LoadStatic ;
  rdfs:range xsd:float ;
  skos:definition "First term voltage exponent for active power (<i>Ep1</i>).  Used only when .staticLoadModelType = exponential."@en .

cim:LoadStatic.ep2 a owl:DatatypeProperty, owl:FunctionalProperty ;
  rdfs:label "ep2"@en ;
  rdfs:domain cim:LoadStatic ;
  rdfs:range xsd:float ;
  skos:definition "Second term voltage exponent for active power (<i>Ep2</i>).  Used only when .staticLoadModelType = exponential."@en .

cim:LoadStatic.ep3 a owl:DatatypeProperty, owl:FunctionalProperty ;
  rdfs:label "ep3"@en ;
  rdfs:domain cim:LoadStatic ;
  rdfs:range xsd:float ;
  skos:definition "Third term voltage exponent for active power (<i>Ep3</i>).  Used only when .staticLoadModelType = exponential."@en .

cim:LoadStatic.eq1 a owl:DatatypeProperty, owl:FunctionalProperty ;
  rdfs:label "eq1"@en ;
  rdfs:domain cim:LoadStatic ;
  rdfs:range xsd:float ;
  skos:definition "First term voltage exponent for reactive power (<i>Eq1</i>).  Used only when .staticLoadModelType = exponential."@en .

cim:LoadStatic.eq2 a owl:DatatypeProperty, owl:FunctionalProperty ;
  rdfs:label "eq2"@en ;
  rdfs:domain cim:LoadStatic ;
  rdfs:range xsd:float ;
  skos:definition "Second term voltage exponent for reactive power (<i>Eq2</i>).  Used only when .staticLoadModelType = exponential."@en .

cim:LoadStatic.eq3 a owl:DatatypeProperty, owl:FunctionalProperty ;
  rdfs:label "eq3"@en ;
  rdfs:domain cim:LoadStatic ;
  rdfs:range xsd:float ;
  skos:definition "Third term voltage exponent for reactive power (<i>Eq3</i>).  Used only when .staticLoadModelType = exponential."@en .

cim:LoadStatic.kp1 a owl:DatatypeProperty, owl:FunctionalProperty ;
  rdfs:label "kp1"@en ;
  rdfs:domain cim:LoadStatic ;
  rdfs:range xsd:float ;
  skos:definition "First term voltage coefficient for active power (<i>K</i><i><sub>p1</sub></i>).  Not used when .staticLoadModelType = constantZ."@en .

cim:LoadStatic.kp2 a owl:DatatypeProperty, owl:FunctionalProperty ;
  rdfs:label "kp2"@en ;
  rdfs:domain cim:LoadStatic ;
  rdfs:range xsd:float ;
  skos:definition "Second term voltage coefficient for active power (<i>K</i><i><sub>p2</sub></i>).  Not used when .staticLoadModelType = constantZ."@en .

cim:LoadStatic.kp3 a owl:DatatypeProperty, owl:FunctionalProperty ;
  rdfs:label "kp3"@en ;
  rdfs:domain cim:LoadStatic ;
  rdfs:range xsd:float ;
  skos:definition "Third term voltage coefficient for active power (<i>K</i><i><sub>p3</sub></i>).  Not used when .staticLoadModelType = constantZ."@en .

cim:LoadStatic.kp4 a owl:DatatypeProperty, owl:FunctionalProperty ;
  rdfs:label "kp4"@en ;
  rdfs:domain cim:LoadStatic ;
  rdfs:range xsd:float ;
  skos:definition "Frequency coefficient for active power (<i>K</i><i><sub>p4</sub></i>)  (not = 0 if .staticLoadModelType = zIP2).  Used only when .staticLoadModelType = zIP2."@en .

cim:LoadStatic.kpf a owl:DatatypeProperty, owl:FunctionalProperty ;
  rdfs:label "kpf"@en ;
  rdfs:domain cim:LoadStatic ;
  rdfs:range xsd:float ;
  skos:definition "Frequency deviation coefficient for active power (<i>K</i><i><sub>pf</sub></i>).  Not used when .staticLoadModelType = constantZ."@en .

cim:LoadStatic.kq1 a owl:DatatypeProperty, owl:FunctionalProperty ;
  rdfs:label "kq1"@en ;
  rdfs:domain cim:LoadStatic ;
  rdfs:range xsd:float ;
  skos:definition "First term voltage coefficient for reactive power (<i>K</i><i><sub>q1</sub></i>).  Not used when .staticLoadModelType = constantZ."@en .

cim:LoadStatic.kq2 a owl:DatatypeProperty, owl:FunctionalProperty ;
  rdfs:label "kq2"@en ;
  rdfs:domain cim:LoadStatic ;
  rdfs:range xsd:float ;
  skos:definition "Second term voltage coefficient for reactive power (<i>K</i><i><sub>q2</sub></i>).  Not used when .staticLoadModelType = constantZ."@en .

cim:LoadStatic.kq3 a owl:DatatypeProperty, owl:FunctionalProperty ;
  rdfs:label "kq3"@en ;
  rdfs:domain cim:LoadStatic ;
  rdfs:range xsd:float ;
  skos:definition "Third term voltage coefficient for reactive power (<i>K</i><i><sub>q3</sub></i>).  Not used when .staticLoadModelType = constantZ."@en .

cim:LoadStatic.kq4 a owl:DatatypeProperty, owl:FunctionalProperty ;
  rdfs:label "kq4"@en ;
  rdfs:domain cim:LoadStatic ;
  rdfs:range xsd:float ;
  skos:definition "Frequency coefficient for reactive power (<i>K</i><i><sub>q4</sub></i>)  (not = 0 when .staticLoadModelType = zIP2).  Used only when .staticLoadModelType - zIP2."@en .

cim:LoadStatic.kqf a owl:DatatypeProperty, owl:FunctionalProperty ;
  rdfs:label "kqf"@en ;
  rdfs:domain cim:LoadStatic ;
  rdfs:range xsd:float ;
  skos:definition "Frequency deviation coefficient for reactive power (<i>K</i><i><sub>qf</sub></i>).  Not used when .staticLoadModelType = constantZ."@en .

cim:LoadStatic.staticLoadModelType a owl:DatatypeProperty ;
  rdfs:label "staticLoadModelType"@en ;
  rdfs:domain cim:LoadStatic ;
  rdfs:range cim:StaticLoadModelKind ;
  skos:definition "Type of static load model.  Typical value = constantZ."@en .

cim:LoadUserDefined.proprietary a owl:DatatypeProperty ;
  rdfs:label "proprietary"@en ;
  rdfs:domain cim:LoadUserDefined ;
  rdfs:range xsd:boolean ;
  skos:definition """
Behaviour is based on a proprietary model as opposed to a detailed model.
true = user-defined model is proprietary with behaviour mutually understood by sending and receiving applications and parameters passed as general attributes
false = user-defined model is explicitly defined in terms of control blocks and their input and output signals.
\t"""@en .

cim:MechLoad1.a a owl:DatatypeProperty ;
  rdfs:label "a"@en ;
  rdfs:domain cim:MechLoad1 ;
  rdfs:range xsd:float ;
  skos:definition "Speed squared coefficient (<i>a</i>)."@en .

cim:MechLoad1.b a owl:DatatypeProperty ;
  rdfs:label "b"@en ;
  rdfs:domain cim:MechLoad1 ;
  rdfs:range xsd:float ;
  skos:definition "Speed coefficient (<i>b</i>)."@en .

cim:MechLoad1.d a owl:DatatypeProperty ;
  rdfs:label "d"@en ;
  rdfs:domain cim:MechLoad1 ;
  rdfs:range xsd:float ;
  skos:definition "Speed to the exponent coefficient (<i>d</i>)."@en .

cim:MechLoad1.e a owl:DatatypeProperty ;
  rdfs:label "e"@en ;
  rdfs:domain cim:MechLoad1 ;
  rdfs:range xsd:float ;
  skos:definition "Exponent (<i>e</i>)."@en .

cim:MechanicalLoadUserDefined.proprietary a owl:DatatypeProperty ;
  rdfs:label "proprietary"@en ;
  rdfs:domain cim:MechanicalLoadUserDefined ;
  rdfs:range xsd:boolean ;
  skos:definition """
Behaviour is based on a proprietary model as opposed to a detailed model.
true = user-defined model is proprietary with behaviour mutually understood by sending and receiving applications and parameters passed as general attributes
false = user-defined model is explicitly defined in terms of control blocks and their input and output signals.
\t"""@en .

cim:OverexcLim2.ifdlim a owl:DatatypeProperty ;
  rdfs:label "ifdlim"@en ;
  rdfs:domain cim:OverexcLim2 ;
  rdfs:range cim:PU ;
  skos:definition "Limit value of rated field current (<i>I</i><i><sub>FDLIM</sub></i>).  Typical value = 1,05."@en .

cim:OverexcLim2.koi a owl:DatatypeProperty ;
  rdfs:label "koi"@en ;
  rdfs:domain cim:OverexcLim2 ;
  rdfs:range cim:PU ;
  skos:definition "Gain Over excitation limiter (<i>K</i><i><sub>OI</sub></i>).  Typical value = 0,1."@en .

cim:OverexcLim2.voimax a owl:DatatypeProperty ;
  rdfs:label "voimax"@en ;
  rdfs:domain cim:OverexcLim2 ;
  rdfs:range cim:PU ;
  skos:definition "Maximum error signal (<i>V</i><i><sub>OIMAX</sub></i>) (&gt; OverexcLim2.voimin).  Typical value = 0."@en .

cim:OverexcLim2.voimin a owl:DatatypeProperty ;
  rdfs:label "voimin"@en ;
  rdfs:domain cim:OverexcLim2 ;
  rdfs:range cim:PU ;
  skos:definition "Minimum error signal (<i>V</i><i><sub>OIMIN</sub></i>) (&lt; OverexcLim2.voimax).  Typical value = -9999."@en .

cim:OverexcLimIEEE.hyst a owl:DatatypeProperty ;
  rdfs:label "hyst"@en ;
  rdfs:domain cim:OverexcLimIEEE ;
  rdfs:range cim:PU ;
  skos:definition "OEL pickup/drop-out hysteresis (<i>HYST</i>).  Typical value = 0,03."@en .

cim:OverexcLimIEEE.ifdlim a owl:DatatypeProperty ;
  rdfs:label "ifdlim"@en ;
  rdfs:domain cim:OverexcLimIEEE ;
  rdfs:range cim:PU ;
  skos:definition "OEL timed field current limit (<i>I</i><i><sub>FDLIM</sub></i>).  Typical value = 1,05."@en .

cim:OverexcLimIEEE.ifdmax a owl:DatatypeProperty ;
  rdfs:label "ifdmax"@en ;
  rdfs:domain cim:OverexcLimIEEE ;
  rdfs:range cim:PU ;
  skos:definition "OEL instantaneous field current limit (<i>I</i><i><sub>FDMAX</sub></i>).  Typical value = 1,5."@en .

cim:OverexcLimIEEE.itfpu a owl:DatatypeProperty ;
  rdfs:label "itfpu"@en ;
  rdfs:domain cim:OverexcLimIEEE ;
  rdfs:range cim:PU ;
  skos:definition "OEL timed field current limiter pickup level (<i>I</i><i><sub>TFPU</sub></i>).  Typical value = 1,05."@en .

cim:OverexcLimIEEE.kcd a owl:DatatypeProperty ;
  rdfs:label "kcd"@en ;
  rdfs:domain cim:OverexcLimIEEE ;
  rdfs:range cim:PU ;
  skos:definition "OEL cooldown gain (<i>K</i><i><sub>CD</sub></i>).  Typical value = 1."@en .

cim:OverexcLimIEEE.kramp a owl:DatatypeProperty ;
  rdfs:label "kramp"@en ;
  rdfs:domain cim:OverexcLimIEEE ;
  rdfs:range xsd:float ;
  skos:definition "OEL ramped limit rate (<i>K</i><i><sub>RAMP</sub></i>).  Unit = PU / s.  Typical value = 10."@en .

cim:OverexcLimX1.efd1 a owl:DatatypeProperty ;
  rdfs:label "efd1"@en ;
  rdfs:domain cim:OverexcLimX1 ;
  rdfs:range cim:PU ;
  skos:definition "Low voltage point on the inverse time characteristic (<i>EFD</i><i><sub>1</sub></i>).  Typical value = 1,1."@en .

cim:OverexcLimX1.efd2 a owl:DatatypeProperty ;
  rdfs:label "efd2"@en ;
  rdfs:domain cim:OverexcLimX1 ;
  rdfs:range cim:PU ;
  skos:definition "Mid voltage point on the inverse time characteristic (<i>EFD</i><i><sub>2</sub></i>).  Typical value = 1,2."@en .

cim:OverexcLimX1.efd3 a owl:DatatypeProperty ;
  rdfs:label "efd3"@en ;
  rdfs:domain cim:OverexcLimX1 ;
  rdfs:range cim:PU ;
  skos:definition "High voltage point on the inverse time characteristic (<i>EFD</i><i><sub>3</sub></i>).  Typical value = 1,5."@en .

cim:OverexcLimX1.efddes a owl:DatatypeProperty ;
  rdfs:label "efddes"@en ;
  rdfs:domain cim:OverexcLimX1 ;
  rdfs:range cim:PU ;
  skos:definition "Desired field voltage (<i>EFD</i><i><sub>DES</sub></i>).  Typical value = 0,9."@en .

cim:OverexcLimX1.efdrated a owl:DatatypeProperty ;
  rdfs:label "efdrated"@en ;
  rdfs:domain cim:OverexcLimX1 ;
  rdfs:range cim:PU ;
  skos:definition "Rated field voltage (<i>EFD</i><i><sub>RATED</sub></i>).  Typical value = 1,05."@en .

cim:OverexcLimX1.kmx a owl:DatatypeProperty ;
  rdfs:label "kmx"@en ;
  rdfs:domain cim:OverexcLimX1 ;
  rdfs:range cim:PU ;
  skos:definition "Gain (<i>K</i><i><sub>MX</sub></i>).  Typical value = 0,01."@en .

cim:OverexcLimX1.t1 a owl:DatatypeProperty ;
  rdfs:label "t1"@en ;
  rdfs:domain cim:OverexcLimX1 ;
  rdfs:range cim:Seconds ;
  skos:definition "Time to trip the exciter at the low voltage point on the inverse time characteristic (<i>TIME</i><i><sub>1</sub></i>) (&gt;= 0).  Typical value = 120."@en .

cim:OverexcLimX1.t2 a owl:DatatypeProperty ;
  rdfs:label "t2"@en ;
  rdfs:domain cim:OverexcLimX1 ;
  rdfs:range cim:Seconds ;
  skos:definition "Time to trip the exciter at the mid voltage point on the inverse time characteristic (<i>TIME</i><i><sub>2</sub></i>) (&gt;= 0).  Typical value = 40."@en .

cim:OverexcLimX1.t3 a owl:DatatypeProperty ;
  rdfs:label "t3"@en ;
  rdfs:domain cim:OverexcLimX1 ;
  rdfs:range cim:Seconds ;
  skos:definition "Time to trip the exciter at the high voltage point on the inverse time characteristic (<i>TIME</i><i><sub>3</sub></i>) (&gt;= 0).  Typical value = 15."@en .

cim:OverexcLimX1.vlow a owl:DatatypeProperty ;
  rdfs:label "vlow"@en ;
  rdfs:domain cim:OverexcLimX1 ;
  rdfs:range cim:PU ;
  skos:definition "Low voltage limit (<i>V</i><i><sub>LOW</sub></i>) (&gt; 0)."@en .

cim:OverexcLimX2.efd1 a owl:DatatypeProperty ;
  rdfs:label "efd1"@en ;
  rdfs:domain cim:OverexcLimX2 ;
  rdfs:range cim:PU ;
  skos:definition "Low voltage or current point on the inverse time characteristic (<i>EFD</i><i><sub>1</sub></i>).  Typical value = 1,1."@en .

cim:OverexcLimX2.efd2 a owl:DatatypeProperty ;
  rdfs:label "efd2"@en ;
  rdfs:domain cim:OverexcLimX2 ;
  rdfs:range cim:PU ;
  skos:definition "Mid voltage or current point on the inverse time characteristic (<i>EFD</i><i><sub>2</sub></i>).  Typical value = 1,2."@en .

cim:OverexcLimX2.efd3 a owl:DatatypeProperty ;
  rdfs:label "efd3"@en ;
  rdfs:domain cim:OverexcLimX2 ;
  rdfs:range cim:PU ;
  skos:definition "High voltage or current point on the inverse time characteristic (<i>EFD</i><i><sub>3</sub></i>).  Typical value = 1,5."@en .

cim:OverexcLimX2.efddes a owl:DatatypeProperty ;
  rdfs:label "efddes"@en ;
  rdfs:domain cim:OverexcLimX2 ;
  rdfs:range cim:PU ;
  skos:definition "Desired field voltage if <i>m</i> = false or desired field current if <i>m </i>= true (<i>EFD</i><i><sub>DES</sub></i>).  Typical value = 1."@en .

cim:OverexcLimX2.efdrated a owl:DatatypeProperty ;
  rdfs:label "efdrated"@en ;
  rdfs:domain cim:OverexcLimX2 ;
  rdfs:range cim:PU ;
  skos:definition "Rated field voltage if m = false or rated field current if m = true (<i>EFD</i><i><sub>RATED</sub></i>).  Typical value = 1,05."@en .

cim:OverexcLimX2.kmx a owl:DatatypeProperty ;
  rdfs:label "kmx"@en ;
  rdfs:domain cim:OverexcLimX2 ;
  rdfs:range cim:PU ;
  skos:definition "Gain (<i>K</i><i><sub>MX</sub></i>).  Typical value = 0,002."@en .

cim:OverexcLimX2.m a owl:DatatypeProperty ;
  rdfs:label "m"@en ;
  rdfs:domain cim:OverexcLimX2 ;
  rdfs:range xsd:boolean ;
  skos:definition """
(<i>m</i>).
true = IFD limiting
false = EFD limiting.
\t"""@en .

cim:OverexcLimX2.t1 a owl:DatatypeProperty ;
  rdfs:label "t1"@en ;
  rdfs:domain cim:OverexcLimX2 ;
  rdfs:range cim:Seconds ;
  skos:definition "Time to trip the exciter at the low voltage or current point on the inverse time characteristic (<i>TIME</i><i><sub>1</sub></i>) (&gt;= 0).  Typical value = 120."@en .

cim:OverexcLimX2.t2 a owl:DatatypeProperty ;
  rdfs:label "t2"@en ;
  rdfs:domain cim:OverexcLimX2 ;
  rdfs:range cim:Seconds ;
  skos:definition "Time to trip the exciter at the mid voltage or current point on the inverse time characteristic (<i>TIME</i><i><sub>2</sub></i>) (&gt;= 0).  Typical value = 40."@en .

cim:OverexcLimX2.t3 a owl:DatatypeProperty ;
  rdfs:label "t3"@en ;
  rdfs:domain cim:OverexcLimX2 ;
  rdfs:range cim:Seconds ;
  skos:definition "Time to trip the exciter at the high voltage or current point on the inverse time characteristic (<i>TIME</i><i><sub>3</sub></i>) (&gt;= 0).  Typical value = 15."@en .

cim:OverexcLimX2.vlow a owl:DatatypeProperty ;
  rdfs:label "vlow"@en ;
  rdfs:domain cim:OverexcLimX2 ;
  rdfs:range cim:PU ;
  skos:definition "Low voltage limit (<i>V</i><i><sub>LOW</sub></i>) (&gt; 0)."@en .

cim:OverexcitationLimiterUserDefined.proprietary a owl:DatatypeProperty ;
  rdfs:label "proprietary"@en ;
  rdfs:domain cim:OverexcitationLimiterUserDefined ;
  rdfs:range xsd:boolean ;
  skos:definition """
Behaviour is based on a proprietary model as opposed to a detailed model.
true = user-defined model is proprietary with behaviour mutually understood by sending and receiving applications and parameters passed as general attributes
false = user-defined model is explicitly defined in terms of control blocks and their input and output signals.
\t"""@en .

cim:PFVArControllerType1UserDefined.proprietary a owl:DatatypeProperty ;
  rdfs:label "proprietary"@en ;
  rdfs:domain cim:PFVArControllerType1UserDefined ;
  rdfs:range xsd:boolean ;
  skos:definition """
Behaviour is based on a proprietary model as opposed to a detailed model.
true = user-defined model is proprietary with behaviour mutually understood by sending and receiving applications and parameters passed as general attributes
false = user-defined model is explicitly defined in terms of control blocks and their input and output signals.
\t"""@en .

cim:PFVArControllerType2UserDefined.proprietary a owl:DatatypeProperty ;
  rdfs:label "proprietary"@en ;
  rdfs:domain cim:PFVArControllerType2UserDefined ;
  rdfs:range xsd:boolean ;
  skos:definition """
Behaviour is based on a proprietary model as opposed to a detailed model.
true = user-defined model is proprietary with behaviour mutually understood by sending and receiving applications and parameters passed as general attributes
false = user-defined model is explicitly defined in terms of control blocks and their input and output signals.
\t"""@en .

cim:PFVArType1IEEEPFController.ovex a owl:DatatypeProperty ;
  rdfs:label "ovex"@en ;
  rdfs:domain cim:PFVArType1IEEEPFController ;
  rdfs:range xsd:boolean ;
  skos:definition """
Overexcitation Flag (<i>OVEX</i>)
true = overexcited
false = underexcited.
\t"""@en .

cim:PFVArType1IEEEPFController.tpfc a owl:DatatypeProperty ;
  rdfs:label "tpfc"@en ;
  rdfs:domain cim:PFVArType1IEEEPFController ;
  rdfs:range cim:Seconds ;
  skos:definition "PF controller time delay (<i>T</i><i><sub>PFC</sub></i>) (&gt;= 0).  Typical value = 5."@en .

cim:PFVArType1IEEEPFController.vitmin a owl:DatatypeProperty ;
  rdfs:label "vitmin"@en ;
  rdfs:domain cim:PFVArType1IEEEPFController ;
  rdfs:range cim:PU ;
  skos:definition "Minimum machine terminal current needed to enable pf/var controller (<i>V</i><i><sub>ITMIN</sub></i>)."@en .

cim:PFVArType1IEEEPFController.vpf a owl:DatatypeProperty ;
  rdfs:label "vpf"@en ;
  rdfs:domain cim:PFVArType1IEEEPFController ;
  rdfs:range cim:PU ;
  skos:definition "Synchronous machine power factor (<i>V</i><i><sub>PF</sub></i>)."@en .

cim:PFVArType1IEEEPFController.vpfcbw a owl:DatatypeProperty ;
  rdfs:label "vpfcbw"@en ;
  rdfs:domain cim:PFVArType1IEEEPFController ;
  rdfs:range xsd:float ;
  skos:definition "PF controller deadband (<i>V</i><i><sub>PFC_BW</sub></i>).  Typical value = 0,05."@en .

cim:PFVArType1IEEEPFController.vpfref a owl:DatatypeProperty ;
  rdfs:label "vpfref"@en ;
  rdfs:domain cim:PFVArType1IEEEPFController ;
  rdfs:range cim:PU ;
  skos:definition "PF controller reference (<i>V</i><i><sub>PFREF</sub></i>)."@en .

cim:PFVArType1IEEEPFController.vvtmax a owl:DatatypeProperty ;
  rdfs:label "vvtmax"@en ;
  rdfs:domain cim:PFVArType1IEEEPFController ;
  rdfs:range cim:PU ;
  skos:definition "Maximum machine terminal voltage needed for pf/var controller to be enabled (<i>V</i><i><sub>VTMAX</sub></i>) (&gt; PFVArType1IEEEPFController.vvtmin)."@en .

cim:PFVArType1IEEEPFController.vvtmin a owl:DatatypeProperty ;
  rdfs:label "vvtmin"@en ;
  rdfs:domain cim:PFVArType1IEEEPFController ;
  rdfs:range cim:PU ;
  skos:definition "Minimum machine terminal voltage needed to enable pf/var controller (<i>V</i><i><sub>VTMIN</sub></i>) (&lt; PFVArType1IEEEPFController.vvtmax)."@en .

cim:PFVArType1IEEEVArController.tvarc a owl:DatatypeProperty ;
  rdfs:label "tvarc"@en ;
  rdfs:domain cim:PFVArType1IEEEVArController ;
  rdfs:range cim:Seconds ;
  skos:definition "Var controller time delay (<i>T</i><i><sub>VARC</sub></i>) (&gt;= 0).  Typical value = 5."@en .

cim:PFVArType1IEEEVArController.vvar a owl:DatatypeProperty ;
  rdfs:label "vvar"@en ;
  rdfs:domain cim:PFVArType1IEEEVArController ;
  rdfs:range cim:PU ;
  skos:definition "Synchronous machine power factor (<i>V</i><i><sub>VAR</sub></i>)."@en .

cim:PFVArType1IEEEVArController.vvarcbw a owl:DatatypeProperty ;
  rdfs:label "vvarcbw"@en ;
  rdfs:domain cim:PFVArType1IEEEVArController ;
  rdfs:range xsd:float ;
  skos:definition "Var controller deadband (<i>V</i><i><sub>VARC_BW</sub></i>).  Typical value = 0,02."@en .

cim:PFVArType1IEEEVArController.vvarref a owl:DatatypeProperty ;
  rdfs:label "vvarref"@en ;
  rdfs:domain cim:PFVArType1IEEEVArController ;
  rdfs:range cim:PU ;
  skos:definition "Var controller reference (<i>V</i><i><sub>VARREF</sub></i>)."@en .

cim:PFVArType1IEEEVArController.vvtmax a owl:DatatypeProperty ;
  rdfs:label "vvtmax"@en ;
  rdfs:domain cim:PFVArType1IEEEVArController ;
  rdfs:range cim:PU ;
  skos:definition "Maximum machine terminal voltage needed for pf/VAr controller to be enabled (<i>V</i><i><sub>VTMAX</sub></i>) (&gt; PVFArType1IEEEVArController.vvtmin)."@en .

cim:PFVArType1IEEEVArController.vvtmin a owl:DatatypeProperty ;
  rdfs:label "vvtmin"@en ;
  rdfs:domain cim:PFVArType1IEEEVArController ;
  rdfs:range cim:PU ;
  skos:definition "Minimum machine terminal voltage needed to enable pf/var controller (<i>V</i><i><sub>VTMIN</sub></i>) (&lt; PVFArType1IEEEVArController.vvtmax)."@en .

cim:PFVArType2Common1.j a owl:DatatypeProperty ;
  rdfs:label "j"@en ;
  rdfs:domain cim:PFVArType2Common1 ;
  rdfs:range xsd:boolean ;
  skos:definition """
Selector (<i>J</i>).
true = control mode for reactive power
false = control mode for power factor.
\t"""@en .

cim:PFVArType2Common1.ki a owl:DatatypeProperty ;
  rdfs:label "ki"@en ;
  rdfs:domain cim:PFVArType2Common1 ;
  rdfs:range cim:PU ;
  skos:definition "Reset gain (<i>Ki</i>)."@en .

cim:PFVArType2Common1.kp a owl:DatatypeProperty ;
  rdfs:label "kp"@en ;
  rdfs:domain cim:PFVArType2Common1 ;
  rdfs:range cim:PU ;
  skos:definition "Proportional gain (<i>Kp</i>)."@en .

cim:PFVArType2Common1.max a owl:DatatypeProperty ;
  rdfs:label "max"@en ;
  rdfs:domain cim:PFVArType2Common1 ;
  rdfs:range cim:PU ;
  skos:definition "Output limit (<i>max</i>)."@en .

cim:PFVArType2Common1.ref a owl:DatatypeProperty ;
  rdfs:label "ref"@en ;
  rdfs:domain cim:PFVArType2Common1 ;
  rdfs:range cim:PU ;
  skos:definition """
Reference value of reactive power or power factor (<i>Ref</i>).
The reference value is initialised by this model. This initialisation can override the value exchanged by this attribute to represent a plant operator's change of the reference setting.
\t"""@en .

cim:PFVArType2IEEEPFController.exlon a owl:DatatypeProperty ;
  rdfs:label "exlon"@en ;
  rdfs:domain cim:PFVArType2IEEEPFController ;
  rdfs:range xsd:boolean ;
  skos:definition """
Overexcitation or under excitation flag (<i>EXLON</i>)
true = 1 (not in the overexcitation or underexcitation state, integral action is active)
false = 0 (in the overexcitation or underexcitation state, so integral action is disabled to allow the limiter to play its role).
\t"""@en .

cim:PFVArType2IEEEPFController.ki a owl:DatatypeProperty ;
  rdfs:label "ki"@en ;
  rdfs:domain cim:PFVArType2IEEEPFController ;
  rdfs:range cim:PU ;
  skos:definition "Integral gain of the pf controller (<i>K</i><i><sub>I</sub></i>).  Typical value = 1."@en .

cim:PFVArType2IEEEPFController.kp a owl:DatatypeProperty ;
  rdfs:label "kp"@en ;
  rdfs:domain cim:PFVArType2IEEEPFController ;
  rdfs:range cim:PU ;
  skos:definition "Proportional gain of the pf controller (<i>K</i><i><sub>P</sub></i>).  Typical value = 1."@en .

cim:PFVArType2IEEEPFController.pfref a owl:DatatypeProperty ;
  rdfs:label "pfref"@en ;
  rdfs:domain cim:PFVArType2IEEEPFController ;
  rdfs:range cim:PU ;
  skos:definition "Power factor reference (<i>P</i><i><sub>FREF</sub></i>)."@en .

cim:PFVArType2IEEEPFController.vclmt a owl:DatatypeProperty ;
  rdfs:label "vclmt"@en ;
  rdfs:domain cim:PFVArType2IEEEPFController ;
  rdfs:range cim:PU ;
  skos:definition "Maximum output of the pf controller (<i>V</i><i><sub>CLMT</sub></i>).  Typical value = 0,1."@en .

cim:PFVArType2IEEEPFController.vref a owl:DatatypeProperty ;
  rdfs:label "vref"@en ;
  rdfs:domain cim:PFVArType2IEEEPFController ;
  rdfs:range cim:PU ;
  skos:definition "Voltage regulator reference (<i>V</i><i><sub>REF</sub></i>)."@en .

cim:PFVArType2IEEEPFController.vs a owl:DatatypeProperty ;
  rdfs:label "vs"@en ;
  rdfs:domain cim:PFVArType2IEEEPFController ;
  rdfs:range xsd:float ;
  skos:definition "Generator sensing voltage (<i>V</i><i><sub>S</sub></i>)."@en .

cim:PFVArType2IEEEVArController.exlon a owl:DatatypeProperty ;
  rdfs:label "exlon"@en ;
  rdfs:domain cim:PFVArType2IEEEVArController ;
  rdfs:range xsd:boolean ;
  skos:definition """
Overexcitation or under excitation flag (<i>EXLON</i>)
true = 1 (not in the overexcitation or underexcitation state, integral action is active)
false = 0 (in the overexcitation or underexcitation state, so integral action is disabled to allow the limiter to play its role).
\t"""@en .

cim:PFVArType2IEEEVArController.ki a owl:DatatypeProperty ;
  rdfs:label "ki"@en ;
  rdfs:domain cim:PFVArType2IEEEVArController ;
  rdfs:range cim:PU ;
  skos:definition "Integral gain of the pf controller (<i>K</i><i><sub>I</sub></i>)."@en .

cim:PFVArType2IEEEVArController.kp a owl:DatatypeProperty ;
  rdfs:label "kp"@en ;
  rdfs:domain cim:PFVArType2IEEEVArController ;
  rdfs:range cim:PU ;
  skos:definition "Proportional gain of the pf controller (<i>K</i><i><sub>P</sub></i>)."@en .

cim:PFVArType2IEEEVArController.qref a owl:DatatypeProperty ;
  rdfs:label "qref"@en ;
  rdfs:domain cim:PFVArType2IEEEVArController ;
  rdfs:range cim:PU ;
  skos:definition "Reactive power reference (<i>Q</i><i><sub>REF</sub></i>). "@en .

cim:PFVArType2IEEEVArController.vclmt a owl:DatatypeProperty ;
  rdfs:label "vclmt"@en ;
  rdfs:domain cim:PFVArType2IEEEVArController ;
  rdfs:range cim:PU ;
  skos:definition "Maximum output of the pf controller (<i>V</i><i><sub>CLMT</sub></i>)."@en .

cim:PFVArType2IEEEVArController.vref a owl:DatatypeProperty ;
  rdfs:label "vref"@en ;
  rdfs:domain cim:PFVArType2IEEEVArController ;
  rdfs:range cim:PU ;
  skos:definition "Voltage regulator reference (<i>V</i><i><sub>REF</sub></i>)."@en .

cim:PFVArType2IEEEVArController.vs a owl:DatatypeProperty ;
  rdfs:label "vs"@en ;
  rdfs:domain cim:PFVArType2IEEEVArController ;
  rdfs:range xsd:float ;
  skos:definition "Generator sensing voltage (<i>V</i><i><sub>S</sub></i>)."@en .

cim:PU.multiplier a owl:DatatypeProperty, owl:FunctionalProperty ;
  rdfs:label "multiplier"@en ;
  dy:isFixed "True " ;
  rdf:value "none" ;
  rdfs:domain cim:PU ;
  rdfs:range cim:UnitMultiplier .

cim:PU.unit a owl:DatatypeProperty, owl:FunctionalProperty ;
  rdfs:label "unit"@en ;
  dy:isFixed "True " ;
  rdf:value "none" ;
  rdfs:domain cim:PU ;
  rdfs:range cim:UnitSymbol .

cim:PU.value a owl:DatatypeProperty, owl:FunctionalProperty ;
  rdfs:label "value"@en ;
  rdfs:domain cim:PU ;
  rdfs:range xsd:float .

cim:PowerSystemStabilizerUserDefined.proprietary a owl:DatatypeProperty ;
  rdfs:label "proprietary"@en ;
  rdfs:domain cim:PowerSystemStabilizerUserDefined ;
  rdfs:range xsd:boolean ;
  skos:definition """
Behaviour is based on a proprietary model as opposed to a detailed model.
true = user-defined model is proprietary with behaviour mutually understood by sending and receiving applications and parameters passed as general attributes
false = user-defined model is explicitly defined in terms of control blocks and their input and output signals.
\t"""@en .

cim:ProprietaryParameterDynamics.booleanParameterValue a owl:DatatypeProperty, owl:FunctionalProperty ;
  rdfs:label "booleanParameterValue"@en ;
  rdfs:domain cim:ProprietaryParameterDynamics ;
  rdfs:range xsd:boolean ;
  skos:definition "Boolean parameter value. If this attribute is populated, integerParameterValue and floatParameterValue will not be."@en .

cim:ProprietaryParameterDynamics.floatParameterValue a owl:DatatypeProperty, owl:FunctionalProperty ;
  rdfs:label "floatParameterValue"@en ;
  rdfs:domain cim:ProprietaryParameterDynamics ;
  rdfs:range xsd:float ;
  skos:definition "Floating point parameter value.  If this attribute is populated, booleanParameterValue and integerParameterValue will not be."@en .

cim:ProprietaryParameterDynamics.integerParameterValue a owl:DatatypeProperty, owl:FunctionalProperty ;
  rdfs:label "integerParameterValue"@en ;
  rdfs:domain cim:ProprietaryParameterDynamics ;
  rdfs:range xsd:integer ;
  skos:definition "Integer parameter value.  If this attribute is populated, booleanParameterValue and floatParameterValue will not be."@en .

cim:ProprietaryParameterDynamics.parameterNumber a owl:DatatypeProperty ;
  rdfs:label "parameterNumber"@en ;
  rdfs:domain cim:ProprietaryParameterDynamics ;
  rdfs:range xsd:integer ;
  skos:definition "Sequence number of the parameter among the set of parameters associated with the related proprietary user-defined model."@en .

cim:Pss1.kf a owl:DatatypeProperty ;
  rdfs:label "kf"@en ;
  rdfs:domain cim:Pss1 ;
  rdfs:range xsd:float ;
  skos:definition "Frequency power input gain (<i>K</i><i><sub>F</sub></i>).  Typical value = 5."@en .

cim:Pss1.komega a owl:DatatypeProperty ;
  rdfs:label "komega"@en ;
  rdfs:domain cim:Pss1 ;
  rdfs:range xsd:float ;
  skos:definition "Shaft speed power input gain (<i>K</i><i><sub>omega</sub></i>).  Typical value = 0."@en .

cim:Pss1.kpe a owl:DatatypeProperty ;
  rdfs:label "kpe"@en ;
  rdfs:domain cim:Pss1 ;
  rdfs:range xsd:float ;
  skos:definition "Electric power input gain (<i>K</i><i><sub>PE</sub></i>).  Typical value = 0,3."@en .

cim:Pss1.ks a owl:DatatypeProperty ;
  rdfs:label "ks"@en ;
  rdfs:domain cim:Pss1 ;
  rdfs:range xsd:float ;
  skos:definition "PSS gain (<i>Ks</i>).  Typical value = 1."@en .

cim:Pss1.pmin a owl:DatatypeProperty ;
  rdfs:label "pmin"@en ;
  rdfs:domain cim:Pss1 ;
  rdfs:range cim:PU ;
  skos:definition "Minimum power PSS enabling (<i>Pmin</i>).  Typical value = 0,25."@en .

cim:Pss1.t10 a owl:DatatypeProperty ;
  rdfs:label "t10"@en ;
  rdfs:domain cim:Pss1 ;
  rdfs:range cim:Seconds ;
  skos:definition "Lead/lag time constant (<i>T</i><i><sub>10</sub></i>) (&gt;= 0).  Typical value = 0."@en .

cim:Pss1.t5 a owl:DatatypeProperty ;
  rdfs:label "t5"@en ;
  rdfs:domain cim:Pss1 ;
  rdfs:range cim:Seconds ;
  skos:definition "Washout (<i>T</i><i><sub>5</sub></i>) (&gt;= 0).  Typical value = 3,5."@en .

cim:Pss1.t6 a owl:DatatypeProperty ;
  rdfs:label "t6"@en ;
  rdfs:domain cim:Pss1 ;
  rdfs:range cim:Seconds ;
  skos:definition "Filter time constant (<i>T</i><i><sub>6</sub></i>) (&gt;= 0).  Typical value = 0."@en .

cim:Pss1.t7 a owl:DatatypeProperty ;
  rdfs:label "t7"@en ;
  rdfs:domain cim:Pss1 ;
  rdfs:range cim:Seconds ;
  skos:definition """
Lead/lag time constant (<i>T</i><i><sub>7</sub></i>) (&gt;= 0). If = 0, both blocks are bypassed.  Typical value = 0.

\t"""@en .

cim:Pss1.t8 a owl:DatatypeProperty ;
  rdfs:label "t8"@en ;
  rdfs:domain cim:Pss1 ;
  rdfs:range cim:Seconds ;
  skos:definition "Lead/lag time constant (<i>T</i><i><sub>8</sub></i>) (&gt;= 0).  Typical value = 0."@en .

cim:Pss1.t9 a owl:DatatypeProperty ;
  rdfs:label "t9"@en ;
  rdfs:domain cim:Pss1 ;
  rdfs:range cim:Seconds ;
  skos:definition "Lead/lag time constant (<i>T</i><i><sub>9</sub></i>) (&gt;= 0).  If = 0, both blocks are bypassed.  Typical value = 0."@en .

cim:Pss1.tpe a owl:DatatypeProperty ;
  rdfs:label "tpe"@en ;
  rdfs:domain cim:Pss1 ;
  rdfs:range cim:Seconds ;
  skos:definition "Electric power filter time constant (<i>T</i><i><sub>PE</sub></i>) (&gt;= 0).  Typical value = 0,05."@en .

cim:Pss1.vadat a owl:DatatypeProperty ;
  rdfs:label "vadat"@en ;
  rdfs:domain cim:Pss1 ;
  rdfs:range xsd:boolean ;
  skos:definition """
<font color="#0f0f0f">Signal selector (<i>V</i><i><sub>ADAT</sub></i>).</font>
<font color="#0f0f0f">true = closed (generator power is greater than <i>Pmin</i>)</font>
<font color="#0f0f0f">false = open (<i>Pe</i> is smaller than <i>Pmin</i>).</font>
<font color="#0f0f0f">Typical value = true.</font>
\t"""@en .

cim:Pss1.vsmn a owl:DatatypeProperty ;
  rdfs:label "vsmn"@en ;
  rdfs:domain cim:Pss1 ;
  rdfs:range cim:PU ;
  skos:definition "Stabilizer output maximum limit (<i>V</i><i><sub>SMN</sub></i>).  Typical value = -0,06."@en .

cim:Pss1.vsmx a owl:DatatypeProperty ;
  rdfs:label "vsmx"@en ;
  rdfs:domain cim:Pss1 ;
  rdfs:range cim:PU ;
  skos:definition "Stabilizer output minimum limit (<i>V</i><i><sub>SMX</sub></i>).  Typical value = 0,06."@en .

cim:Pss1A.a1 a owl:DatatypeProperty ;
  rdfs:label "a1"@en ;
  rdfs:domain cim:Pss1A ;
  rdfs:range cim:PU ;
  skos:definition "Notch filter parameter (<i>A</i><i><sub>1</sub></i>)."@en .

cim:Pss1A.a2 a owl:DatatypeProperty ;
  rdfs:label "a2"@en ;
  rdfs:domain cim:Pss1A ;
  rdfs:range cim:PU ;
  skos:definition "Notch filter parameter (<i>A</i><i><sub>2</sub></i>). "@en .

cim:Pss1A.a3 a owl:DatatypeProperty ;
  rdfs:label "a3"@en ;
  rdfs:domain cim:Pss1A ;
  rdfs:range cim:PU ;
  skos:definition "Notch filter parameter (<i>A</i><i><sub>3</sub></i>). "@en .

cim:Pss1A.a4 a owl:DatatypeProperty ;
  rdfs:label "a4"@en ;
  rdfs:domain cim:Pss1A ;
  rdfs:range cim:PU ;
  skos:definition "Notch filter parameter (<i>A</i><i><sub>4</sub></i>). "@en .

cim:Pss1A.a5 a owl:DatatypeProperty ;
  rdfs:label "a5"@en ;
  rdfs:domain cim:Pss1A ;
  rdfs:range cim:PU ;
  skos:definition "Notch filter parameter (<i>A</i><i><sub>5</sub></i>). "@en .

cim:Pss1A.a6 a owl:DatatypeProperty ;
  rdfs:label "a6"@en ;
  rdfs:domain cim:Pss1A ;
  rdfs:range cim:PU ;
  skos:definition "Notch filter parameter (<i>A</i><i><sub>6</sub></i>). "@en .

cim:Pss1A.a7 a owl:DatatypeProperty ;
  rdfs:label "a7"@en ;
  rdfs:domain cim:Pss1A ;
  rdfs:range cim:PU ;
  skos:definition "Notch filter parameter (<i>A</i><i><sub>7</sub></i>). "@en .

cim:Pss1A.a8 a owl:DatatypeProperty ;
  rdfs:label "a8"@en ;
  rdfs:domain cim:Pss1A ;
  rdfs:range cim:PU ;
  skos:definition "Notch filter parameter (<i>A</i><i><sub>8</sub></i>). "@en .

cim:Pss1A.inputSignalType a owl:DatatypeProperty ;
  rdfs:label "inputSignalType"@en ;
  rdfs:domain cim:Pss1A ;
  rdfs:range cim:InputSignalKind ;
  skos:definition "Type of input signal (rotorAngularFrequencyDeviation, busFrequencyDeviation, generatorElectricalPower, generatorAcceleratingPower, busVoltage, or busVoltageDerivative)."@en .

cim:Pss1A.kd a owl:DatatypeProperty ;
  rdfs:label "kd"@en ;
  rdfs:domain cim:Pss1A ;
  rdfs:range xsd:boolean ;
  skos:definition """
Selector (<i>Kd</i>). 
true = e<sup>-sTdelay</sup> used
false = e<sup>-sTdelay</sup> not used.
\t"""@en .

cim:Pss1A.ks a owl:DatatypeProperty ;
  rdfs:label "ks"@en ;
  rdfs:domain cim:Pss1A ;
  rdfs:range cim:PU ;
  skos:definition "Stabilizer gain (<i>K</i><i><sub>s</sub></i>). "@en .

cim:Pss1A.t1 a owl:DatatypeProperty ;
  rdfs:label "t1"@en ;
  rdfs:domain cim:Pss1A ;
  rdfs:range cim:Seconds ;
  skos:definition "Lead/lag time constant (<i>T</i><i><sub>1</sub></i>) (&gt;= 0). "@en .

cim:Pss1A.t2 a owl:DatatypeProperty ;
  rdfs:label "t2"@en ;
  rdfs:domain cim:Pss1A ;
  rdfs:range cim:Seconds ;
  skos:definition "Lead/lag time constant (<i>T</i><i><sub>2</sub></i>) (&gt;= 0). "@en .

cim:Pss1A.t3 a owl:DatatypeProperty ;
  rdfs:label "t3"@en ;
  rdfs:domain cim:Pss1A ;
  rdfs:range cim:Seconds ;
  skos:definition "Lead/lag time constant (<i>T</i><i><sub>3</sub></i>) (&gt;= 0). "@en .

cim:Pss1A.t4 a owl:DatatypeProperty ;
  rdfs:label "t4"@en ;
  rdfs:domain cim:Pss1A ;
  rdfs:range cim:Seconds ;
  skos:definition "Lead/lag time constant (<i>T</i><i><sub>4</sub></i>) (&gt;= 0). "@en .

cim:Pss1A.t5 a owl:DatatypeProperty ;
  rdfs:label "t5"@en ;
  rdfs:domain cim:Pss1A ;
  rdfs:range cim:Seconds ;
  skos:definition "Washout time constant (<i>T</i><i><sub>5</sub></i>) (&gt;= 0). "@en .

cim:Pss1A.t6 a owl:DatatypeProperty ;
  rdfs:label "t6"@en ;
  rdfs:domain cim:Pss1A ;
  rdfs:range cim:Seconds ;
  skos:definition "Transducer time constant (<i>T</i><i><sub>6</sub></i>) (&gt;= 0). "@en .

cim:Pss1A.tdelay a owl:DatatypeProperty ;
  rdfs:label "tdelay"@en ;
  rdfs:domain cim:Pss1A ;
  rdfs:range cim:Seconds ;
  skos:definition "Time constant (<i>Tdelay</i>) (&gt;= 0). "@en .

cim:Pss1A.vcl a owl:DatatypeProperty ;
  rdfs:label "vcl"@en ;
  rdfs:domain cim:Pss1A ;
  rdfs:range cim:PU ;
  skos:definition "Stabilizer input cutoff threshold (<i>Vcl</i>). "@en .

cim:Pss1A.vcu a owl:DatatypeProperty ;
  rdfs:label "vcu"@en ;
  rdfs:domain cim:Pss1A ;
  rdfs:range cim:PU ;
  skos:definition "Stabilizer input cutoff threshold (<i>Vcu</i>). "@en .

cim:Pss1A.vrmax a owl:DatatypeProperty ;
  rdfs:label "vrmax"@en ;
  rdfs:domain cim:Pss1A ;
  rdfs:range cim:PU ;
  skos:definition "Maximum stabilizer output (<i>Vrmax</i>) (&gt; Pss1A.vrmin). "@en .

cim:Pss1A.vrmin a owl:DatatypeProperty ;
  rdfs:label "vrmin"@en ;
  rdfs:domain cim:Pss1A ;
  rdfs:range cim:PU ;
  skos:definition "Minimum stabilizer output (<i>Vrmin</i>) (&lt; Pss1A.vrmax). "@en .

cim:Pss2B.a a owl:DatatypeProperty ;
  rdfs:label "a"@en ;
  rdfs:domain cim:Pss2B ;
  rdfs:range xsd:float ;
  skos:definition "Numerator constant (<i>a</i>).  Typical value = 1."@en .

cim:Pss2B.ks1 a owl:DatatypeProperty ;
  rdfs:label "ks1"@en ;
  rdfs:domain cim:Pss2B ;
  rdfs:range cim:PU ;
  skos:definition "Stabilizer gain (<i>Ks1</i>).  Typical value = 12."@en .

cim:Pss2B.ks2 a owl:DatatypeProperty ;
  rdfs:label "ks2"@en ;
  rdfs:domain cim:Pss2B ;
  rdfs:range cim:PU ;
  skos:definition "Gain on signal #2 (<i>Ks2</i>).  Typical value = 0,2."@en .

cim:Pss2B.ks3 a owl:DatatypeProperty ;
  rdfs:label "ks3"@en ;
  rdfs:domain cim:Pss2B ;
  rdfs:range cim:PU ;
  skos:definition "Gain on signal #2 input before ramp-tracking filter (<i>Ks3</i>).  Typical value = 1."@en .

cim:Pss2B.ks4 a owl:DatatypeProperty ;
  rdfs:label "ks4"@en ;
  rdfs:domain cim:Pss2B ;
  rdfs:range cim:PU ;
  skos:definition "Gain on signal #2 input after ramp-tracking filter (<i>Ks4</i>).  Typical value = 1."@en .

cim:Pss2B.m a owl:DatatypeProperty ;
  rdfs:label "m"@en ;
  rdfs:domain cim:Pss2B ;
  rdfs:range xsd:integer ;
  skos:definition "Denominator order of ramp tracking filter (<i>m</i>).  Typical value = 5."@en .

cim:Pss2B.n a owl:DatatypeProperty ;
  rdfs:label "n"@en ;
  rdfs:domain cim:Pss2B ;
  rdfs:range xsd:integer ;
  skos:definition "Order of ramp tracking filter (<i>n</i>).  Typical value = 1."@en .

cim:Pss2B.t1 a owl:DatatypeProperty ;
  rdfs:label "t1"@en ;
  rdfs:domain cim:Pss2B ;
  rdfs:range cim:Seconds ;
  skos:definition "Lead/lag time constant (<i>T</i><i><sub>1</sub></i>) (&gt;= 0).  Typical value = 0,12."@en .

cim:Pss2B.t10 a owl:DatatypeProperty ;
  rdfs:label "t10"@en ;
  rdfs:domain cim:Pss2B ;
  rdfs:range cim:Seconds ;
  skos:definition "Lead/lag time constant (<i>T</i><i><sub>10</sub></i>) (&gt;= 0).  Typical value = 0."@en .

cim:Pss2B.t11 a owl:DatatypeProperty ;
  rdfs:label "t11"@en ;
  rdfs:domain cim:Pss2B ;
  rdfs:range cim:Seconds ;
  skos:definition "Lead/lag time constant (<i>T</i><i><sub>11</sub></i>) (&gt;= 0).  Typical value = 0."@en .

cim:Pss2B.t2 a owl:DatatypeProperty ;
  rdfs:label "t2"@en ;
  rdfs:domain cim:Pss2B ;
  rdfs:range cim:Seconds ;
  skos:definition "Lead/lag time constant (<i>T</i><i><sub>2</sub></i>) (&gt;= 0).  Typical value = 0,02."@en .

cim:Pss2B.t3 a owl:DatatypeProperty ;
  rdfs:label "t3"@en ;
  rdfs:domain cim:Pss2B ;
  rdfs:range cim:Seconds ;
  skos:definition "Lead/lag time constant (<i>T</i><i><sub>3</sub></i>) (&gt;= 0).  Typical value = 0,3."@en .

cim:Pss2B.t4 a owl:DatatypeProperty ;
  rdfs:label "t4"@en ;
  rdfs:domain cim:Pss2B ;
  rdfs:range cim:Seconds ;
  skos:definition "Lead/lag time constant (<i>T</i><i><sub>4</sub></i>) (&gt;= 0).  Typical value = 0,02."@en .

cim:Pss2B.t6 a owl:DatatypeProperty ;
  rdfs:label "t6"@en ;
  rdfs:domain cim:Pss2B ;
  rdfs:range cim:Seconds ;
  skos:definition "Time constant on signal #1 (<i>T</i><i><sub>6</sub></i>) (&gt;= 0).  Typical value = 0."@en .

cim:Pss2B.t7 a owl:DatatypeProperty ;
  rdfs:label "t7"@en ;
  rdfs:domain cim:Pss2B ;
  rdfs:range cim:Seconds ;
  skos:definition "Time constant on signal #2 (<i>T</i><i><sub>7</sub></i>) (&gt;= 0).  Typical value = 2."@en .

cim:Pss2B.t8 a owl:DatatypeProperty ;
  rdfs:label "t8"@en ;
  rdfs:domain cim:Pss2B ;
  rdfs:range cim:Seconds ;
  skos:definition "Lead of ramp tracking filter (<i>T</i><i><sub>8</sub></i>) (&gt;= 0).  Typical value = 0,2."@en .

cim:Pss2B.t9 a owl:DatatypeProperty ;
  rdfs:label "t9"@en ;
  rdfs:domain cim:Pss2B ;
  rdfs:range cim:Seconds ;
  skos:definition "Lag of ramp tracking filter (<i>T</i><i><sub>9</sub></i>) (&gt;= 0).  Typical value = 0,1."@en .

cim:Pss2B.ta a owl:DatatypeProperty ;
  rdfs:label "ta"@en ;
  rdfs:domain cim:Pss2B ;
  rdfs:range cim:Seconds ;
  skos:definition "Lead constant (<i>T</i><i><sub>a</sub></i>) (&gt;= 0).  Typical value = 0."@en .

cim:Pss2B.tb a owl:DatatypeProperty ;
  rdfs:label "tb"@en ;
  rdfs:domain cim:Pss2B ;
  rdfs:range cim:Seconds ;
  skos:definition "Lag time constant (<i>T</i><i><sub>b</sub></i>) (&gt;= 0).  Typical value = 0."@en .

cim:Pss2B.tw1 a owl:DatatypeProperty ;
  rdfs:label "tw1"@en ;
  rdfs:domain cim:Pss2B ;
  rdfs:range cim:Seconds ;
  skos:definition "First washout on signal #1 (<i>T</i><i><sub>w1</sub></i>) (&gt;= 0).  Typical value = 2."@en .

cim:Pss2B.tw2 a owl:DatatypeProperty ;
  rdfs:label "tw2"@en ;
  rdfs:domain cim:Pss2B ;
  rdfs:range cim:Seconds ;
  skos:definition "Second washout on signal #1 (<i>T</i><i><sub>w2</sub></i>) (&gt;= 0).  Typical value = 2."@en .

cim:Pss2B.tw3 a owl:DatatypeProperty ;
  rdfs:label "tw3"@en ;
  rdfs:domain cim:Pss2B ;
  rdfs:range cim:Seconds ;
  skos:definition "First washout on signal #2 (<i>T</i><i><sub>w3</sub></i>) (&gt;= 0).  Typical value = 2."@en .

cim:Pss2B.tw4 a owl:DatatypeProperty ;
  rdfs:label "tw4"@en ;
  rdfs:domain cim:Pss2B ;
  rdfs:range cim:Seconds ;
  skos:definition "Second washout on signal #2 (<i>T</i><i><sub>w4</sub></i>) (&gt;= 0).  Typical value = 0."@en .

cim:Pss2B.vsi1max a owl:DatatypeProperty ;
  rdfs:label "vsi1max"@en ;
  rdfs:domain cim:Pss2B ;
  rdfs:range cim:PU ;
  skos:definition "Input signal #1 maximum limit (<i>Vsi1max</i>) (&gt; Pss2B.vsi1min).  Typical value = 2."@en .

cim:Pss2B.vsi1min a owl:DatatypeProperty ;
  rdfs:label "vsi1min"@en ;
  rdfs:domain cim:Pss2B ;
  rdfs:range cim:PU ;
  skos:definition "Input signal #1 minimum limit (<i>Vsi1min</i>) (&lt; Pss2B.vsi1max).  Typical value = -2."@en .

cim:Pss2B.vsi2max a owl:DatatypeProperty ;
  rdfs:label "vsi2max"@en ;
  rdfs:domain cim:Pss2B ;
  rdfs:range cim:PU ;
  skos:definition "Input signal #2 maximum limit (<i>Vsi2max</i>) (&gt; Pss2B.vsi2min).  Typical value = 2."@en .

cim:Pss2B.vsi2min a owl:DatatypeProperty ;
  rdfs:label "vsi2min"@en ;
  rdfs:domain cim:Pss2B ;
  rdfs:range cim:PU ;
  skos:definition "Input signal #2 minimum limit (<i>Vsi2min</i>) (&lt; Pss2B.vsi2max).  Typical value = -2."@en .

cim:Pss2B.vstmax a owl:DatatypeProperty ;
  rdfs:label "vstmax"@en ;
  rdfs:domain cim:Pss2B ;
  rdfs:range cim:PU ;
  skos:definition "Stabilizer output maximum limit (<i>Vstmax</i>) (&gt; Pss2B.vstmin).  Typical value = 0,1."@en .

cim:Pss2B.vstmin a owl:DatatypeProperty ;
  rdfs:label "vstmin"@en ;
  rdfs:domain cim:Pss2B ;
  rdfs:range cim:PU ;
  skos:definition "Stabilizer output minimum limit (<i>Vstmin</i>) (&lt; Pss2B.vstmax).  Typical value = -0,1."@en .

cim:Pss2ST.inputSignal1Type a owl:DatatypeProperty ;
  rdfs:label "inputSignal1Type"@en ;
  rdfs:domain cim:Pss2ST ;
  rdfs:range cim:InputSignalKind ;
  skos:definition "Type of input signal #1 (rotorAngularFrequencyDeviation, busFrequencyDeviation, generatorElectricalPower, generatorAcceleratingPower, busVoltage, or busVoltageDerivative - shall be different than Pss2ST.inputSignal2Type).  Typical value = rotorAngularFrequencyDeviation."@en .

cim:Pss2ST.inputSignal2Type a owl:DatatypeProperty ;
  rdfs:label "inputSignal2Type"@en ;
  rdfs:domain cim:Pss2ST ;
  rdfs:range cim:InputSignalKind ;
  skos:definition "Type of input signal #2 (rotorAngularFrequencyDeviation, busFrequencyDeviation, generatorElectricalPower, generatorAcceleratingPower, busVoltage, or busVoltageDerivative - shall be different than Pss2ST.inputSignal1Type).  Typical value = busVoltageDerivative."@en .

cim:Pss2ST.k1 a owl:DatatypeProperty ;
  rdfs:label "k1"@en ;
  rdfs:domain cim:Pss2ST ;
  rdfs:range cim:PU ;
  skos:definition "Gain (<i>K</i><i><sub>1</sub></i>). "@en .

cim:Pss2ST.k2 a owl:DatatypeProperty ;
  rdfs:label "k2"@en ;
  rdfs:domain cim:Pss2ST ;
  rdfs:range cim:PU ;
  skos:definition "Gain (<i>K</i><i><sub>2</sub></i>). "@en .

cim:Pss2ST.lsmax a owl:DatatypeProperty ;
  rdfs:label "lsmax"@en ;
  rdfs:domain cim:Pss2ST ;
  rdfs:range cim:PU ;
  skos:definition "Limiter (<i>L</i><i><sub>SMAX</sub></i>) (&gt; Pss2ST.lsmin). "@en .

cim:Pss2ST.lsmin a owl:DatatypeProperty ;
  rdfs:label "lsmin"@en ;
  rdfs:domain cim:Pss2ST ;
  rdfs:range cim:PU ;
  skos:definition "Limiter (<i>L</i><i><sub>SMIN</sub></i>) (&lt; Pss2ST.lsmax). "@en .

cim:Pss2ST.t1 a owl:DatatypeProperty ;
  rdfs:label "t1"@en ;
  rdfs:domain cim:Pss2ST ;
  rdfs:range cim:Seconds ;
  skos:definition "Time constant (<i>T</i><i><sub>1</sub></i>) (&gt;= 0). "@en .

cim:Pss2ST.t10 a owl:DatatypeProperty ;
  rdfs:label "t10"@en ;
  rdfs:domain cim:Pss2ST ;
  rdfs:range cim:Seconds ;
  skos:definition "Time constant (<i>T</i><i><sub>10</sub></i>) (&gt;= 0). "@en .

cim:Pss2ST.t2 a owl:DatatypeProperty ;
  rdfs:label "t2"@en ;
  rdfs:domain cim:Pss2ST ;
  rdfs:range cim:Seconds ;
  skos:definition "Time constant (<i>T</i><i><sub>2</sub></i>) (&gt;= 0)."@en .

cim:Pss2ST.t3 a owl:DatatypeProperty ;
  rdfs:label "t3"@en ;
  rdfs:domain cim:Pss2ST ;
  rdfs:range cim:Seconds ;
  skos:definition "Time constant (<i>T</i><i><sub>3</sub></i>) (&gt;= 0). "@en .

cim:Pss2ST.t4 a owl:DatatypeProperty ;
  rdfs:label "t4"@en ;
  rdfs:domain cim:Pss2ST ;
  rdfs:range cim:Seconds ;
  skos:definition "Time constant (<i>T</i><i><sub>4</sub></i>) (&gt;= 0)."@en .

cim:Pss2ST.t5 a owl:DatatypeProperty ;
  rdfs:label "t5"@en ;
  rdfs:domain cim:Pss2ST ;
  rdfs:range cim:Seconds ;
  skos:definition "Time constant (<i>T</i><i><sub>5</sub></i>) (&gt;= 0). "@en .

cim:Pss2ST.t6 a owl:DatatypeProperty ;
  rdfs:label "t6"@en ;
  rdfs:domain cim:Pss2ST ;
  rdfs:range cim:Seconds ;
  skos:definition "Time constant (<i>T</i><i><sub>6</sub></i>) (&gt;= 0). "@en .

cim:Pss2ST.t7 a owl:DatatypeProperty ;
  rdfs:label "t7"@en ;
  rdfs:domain cim:Pss2ST ;
  rdfs:range cim:Seconds ;
  skos:definition "Time constant (<i>T</i><i><sub>7</sub></i>) (&gt;= 0). "@en .

cim:Pss2ST.t8 a owl:DatatypeProperty ;
  rdfs:label "t8"@en ;
  rdfs:domain cim:Pss2ST ;
  rdfs:range cim:Seconds ;
  skos:definition "Time constant (<i>T</i><i><sub>8</sub></i>) (&gt;= 0). "@en .

cim:Pss2ST.t9 a owl:DatatypeProperty ;
  rdfs:label "t9"@en ;
  rdfs:domain cim:Pss2ST ;
  rdfs:range cim:Seconds ;
  skos:definition "Time constant (<i>T</i><i><sub>9</sub></i>) (&gt;= 0). "@en .

cim:Pss2ST.vcl a owl:DatatypeProperty ;
  rdfs:label "vcl"@en ;
  rdfs:domain cim:Pss2ST ;
  rdfs:range cim:PU ;
  skos:definition "Cutoff limiter (<i>V</i><i><sub>CL</sub></i>). "@en .

cim:Pss2ST.vcu a owl:DatatypeProperty ;
  rdfs:label "vcu"@en ;
  rdfs:domain cim:Pss2ST ;
  rdfs:range cim:PU ;
  skos:definition "Cutoff limiter (<i>V</i><i><sub>CU</sub></i>). "@en .

cim:Pss5.ctw2 a owl:DatatypeProperty ;
  rdfs:label "ctw2"@en ;
  rdfs:domain cim:Pss5 ;
  rdfs:range xsd:boolean ;
  skos:definition """
Selector for second washout enabling (<i>C</i><i><sub>TW2</sub></i>).
true = second washout filter is bypassed
false = second washout filter in use.
Typical value = true.
\t"""@en .

cim:Pss5.deadband a owl:DatatypeProperty ;
  rdfs:label "deadband"@en ;
  rdfs:domain cim:Pss5 ;
  rdfs:range cim:PU ;
  skos:definition "Stabilizer output deadband (<i>DEADBAND</i>).  Typical value = 0."@en .

cim:Pss5.isfreq a owl:DatatypeProperty ;
  rdfs:label "isfreq"@en ;
  rdfs:domain cim:Pss5 ;
  rdfs:range xsd:boolean ;
  skos:definition """
Selector for frequency/shaft speed input (<i>isFreq</i>).
true = speed (same meaning as InputSignaKind.rotorSpeed)
false = frequency (same meaning as InputSignalKind.busFrequency).
Typical value = true (same meaning as InputSignalKind.rotorSpeed).
\t"""@en .

cim:Pss5.kf a owl:DatatypeProperty ;
  rdfs:label "kf"@en ;
  rdfs:domain cim:Pss5 ;
  rdfs:range xsd:float ;
  skos:definition "Frequency/shaft speed input gain (<i>K</i><i><sub>F</sub></i>).  Typical value = 5."@en .

cim:Pss5.kpe a owl:DatatypeProperty ;
  rdfs:label "kpe"@en ;
  rdfs:domain cim:Pss5 ;
  rdfs:range xsd:float ;
  skos:definition "Electric power input gain (<i>K</i><i><sub>PE</sub></i>).  Typical value = 0,3."@en .

cim:Pss5.kpss a owl:DatatypeProperty ;
  rdfs:label "kpss"@en ;
  rdfs:domain cim:Pss5 ;
  rdfs:range xsd:float ;
  skos:definition "PSS gain (<i>K</i><i><sub>PSS</sub></i>).  Typical value = 1."@en .

cim:Pss5.pmin a owl:DatatypeProperty ;
  rdfs:label "pmin"@en ;
  rdfs:domain cim:Pss5 ;
  rdfs:range cim:PU ;
  skos:definition "Minimum power PSS enabling (<i>Pmin</i>).  Typical value = 0,25."@en .

cim:Pss5.tl1 a owl:DatatypeProperty ;
  rdfs:label "tl1"@en ;
  rdfs:domain cim:Pss5 ;
  rdfs:range cim:Seconds ;
  skos:definition "Lead/lag time constant (<i>T</i><i><sub>L1</sub></i>) (&gt;= 0).  Typical value = 0."@en .

cim:Pss5.tl2 a owl:DatatypeProperty ;
  rdfs:label "tl2"@en ;
  rdfs:domain cim:Pss5 ;
  rdfs:range cim:Seconds ;
  skos:definition """
Lead/lag time constant (<i>T</i><i><sub>L2</sub></i>) (&gt;= 0).  If = 0, both blocks are bypassed.  Typical value = 0.

\t"""@en .

cim:Pss5.tl3 a owl:DatatypeProperty ;
  rdfs:label "tl3"@en ;
  rdfs:domain cim:Pss5 ;
  rdfs:range cim:Seconds ;
  skos:definition "Lead/lag time constant (<i>T</i><i><sub>L3</sub></i>) (&gt;= 0).  Typical value = 0."@en .

cim:Pss5.tl4 a owl:DatatypeProperty ;
  rdfs:label "tl4"@en ;
  rdfs:domain cim:Pss5 ;
  rdfs:range cim:Seconds ;
  skos:definition "Lead/lag time constant (T<sub>L4</sub>) (&gt;= 0).  If = 0, both blocks are bypassed.  Typical value = 0."@en .

cim:Pss5.tpe a owl:DatatypeProperty ;
  rdfs:label "tpe"@en ;
  rdfs:domain cim:Pss5 ;
  rdfs:range cim:Seconds ;
  skos:definition "Electric power filter time constant (<i>T</i><i><sub>PE</sub></i>) (&gt;= 0).  Typical value = 0,05."@en .

cim:Pss5.tw1 a owl:DatatypeProperty ;
  rdfs:label "tw1"@en ;
  rdfs:domain cim:Pss5 ;
  rdfs:range cim:Seconds ;
  skos:definition "First washout (<i>T</i><i><sub>W1</sub></i>) (&gt;= 0).  Typical value = 3,5."@en .

cim:Pss5.tw2 a owl:DatatypeProperty ;
  rdfs:label "tw2"@en ;
  rdfs:domain cim:Pss5 ;
  rdfs:range cim:Seconds ;
  skos:definition "Second washout (<i>T</i><i><sub>W2</sub></i>) (&gt;= 0).  Typical value = 0."@en .

cim:Pss5.vadat a owl:DatatypeProperty ;
  rdfs:label "vadat"@en ;
  rdfs:domain cim:Pss5 ;
  rdfs:range xsd:boolean ;
  skos:definition """
<font color="#0f0f0f">Signal selector (<i>V</i><i><sub>adAtt</sub></i>).</font>
<font color="#0f0f0f">true = closed (generator power is greater than <i>Pmin</i>)</font>
<font color="#0f0f0f">false = open (<i>Pe</i> is smaller than <i>Pmin</i>).</font>
<font color="#0f0f0f">Typical value = true.</font>
\t"""@en .

cim:Pss5.vsmn a owl:DatatypeProperty ;
  rdfs:label "vsmn"@en ;
  rdfs:domain cim:Pss5 ;
  rdfs:range cim:PU ;
  skos:definition "Stabilizer output maximum limit (<i>V</i><i><sub>SMN</sub></i>).  Typical value = -0,1."@en .

cim:Pss5.vsmx a owl:DatatypeProperty ;
  rdfs:label "vsmx"@en ;
  rdfs:domain cim:Pss5 ;
  rdfs:range cim:PU ;
  skos:definition "Stabilizer output minimum limit (<i>V</i><i><sub>SMX</sub></i>).  Typical value = 0,1."@en .

cim:PssELIN2.apss a owl:DatatypeProperty ;
  rdfs:label "apss"@en ;
  rdfs:domain cim:PssELIN2 ;
  rdfs:range cim:PU ;
  skos:definition "Coefficient (<i>a_PSS</i>).  Typical value = 0,1."@en .

cim:PssELIN2.ks1 a owl:DatatypeProperty ;
  rdfs:label "ks1"@en ;
  rdfs:domain cim:PssELIN2 ;
  rdfs:range cim:PU ;
  skos:definition "Gain (<i>Ks1</i>).  Typical value = 1."@en .

cim:PssELIN2.ks2 a owl:DatatypeProperty ;
  rdfs:label "ks2"@en ;
  rdfs:domain cim:PssELIN2 ;
  rdfs:range cim:PU ;
  skos:definition "Gain (<i>Ks2</i>).  Typical value = 0,1."@en .

cim:PssELIN2.ppss a owl:DatatypeProperty ;
  rdfs:label "ppss"@en ;
  rdfs:domain cim:PssELIN2 ;
  rdfs:range cim:PU ;
  skos:definition "Coefficient (<i>p_PSS</i>) (&gt;= 0 and &lt;= 4).  Typical value = 0,1."@en .

cim:PssELIN2.psslim a owl:DatatypeProperty ;
  rdfs:label "psslim"@en ;
  rdfs:domain cim:PssELIN2 ;
  rdfs:range cim:PU ;
  skos:definition "PSS limiter (<i>psslim</i>).  Typical value = 0,1."@en .

cim:PssELIN2.ts1 a owl:DatatypeProperty ;
  rdfs:label "ts1"@en ;
  rdfs:domain cim:PssELIN2 ;
  rdfs:range cim:Seconds ;
  skos:definition "Time constant (<i>Ts1</i>) (&gt;= 0).  Typical value = 0."@en .

cim:PssELIN2.ts2 a owl:DatatypeProperty ;
  rdfs:label "ts2"@en ;
  rdfs:domain cim:PssELIN2 ;
  rdfs:range cim:Seconds ;
  skos:definition "Time constant (<i>Ts2</i>) (&gt;= 0).  Typical value = 1."@en .

cim:PssELIN2.ts3 a owl:DatatypeProperty ;
  rdfs:label "ts3"@en ;
  rdfs:domain cim:PssELIN2 ;
  rdfs:range cim:Seconds ;
  skos:definition "Time constant (<i>Ts3</i>) (&gt;= 0).  Typical value = 1."@en .

cim:PssELIN2.ts4 a owl:DatatypeProperty ;
  rdfs:label "ts4"@en ;
  rdfs:domain cim:PssELIN2 ;
  rdfs:range cim:Seconds ;
  skos:definition "Time constant (<i>Ts4</i>) (&gt;= 0).  Typical value = 0,1."@en .

cim:PssELIN2.ts5 a owl:DatatypeProperty ;
  rdfs:label "ts5"@en ;
  rdfs:domain cim:PssELIN2 ;
  rdfs:range cim:Seconds ;
  skos:definition "Time constant (<i>Ts5</i>) (&gt;= 0).  Typical value = 0."@en .

cim:PssELIN2.ts6 a owl:DatatypeProperty ;
  rdfs:label "ts6"@en ;
  rdfs:domain cim:PssELIN2 ;
  rdfs:range cim:Seconds ;
  skos:definition "Time constant (<i>Ts6</i>) (&gt;= 0).  Typical value = 1."@en .

cim:PssIEEE1A.a1 a owl:DatatypeProperty ;
  rdfs:label "a1"@en ;
  rdfs:domain cim:PssIEEE1A ;
  rdfs:range cim:PU ;
  skos:definition "PSS signal conditioning frequency filter constant (<i>A1</i>).  Typical value = 0,061."@en .

cim:PssIEEE1A.a2 a owl:DatatypeProperty ;
  rdfs:label "a2"@en ;
  rdfs:domain cim:PssIEEE1A ;
  rdfs:range cim:PU ;
  skos:definition "PSS signal conditioning frequency filter constant (<i>A2</i>).  Typical value = 0,0017."@en .

cim:PssIEEE1A.inputSignalType a owl:DatatypeProperty ;
  rdfs:label "inputSignalType"@en ;
  rdfs:domain cim:PssIEEE1A ;
  rdfs:range cim:InputSignalKind ;
  skos:definition "Type of input signal (rotorAngularFrequencyDeviation, generatorElectricalPower, or busFrequencyDeviation).  Typical value = rotorAngularFrequencyDeviation."@en .

cim:PssIEEE1A.ks a owl:DatatypeProperty ;
  rdfs:label "ks"@en ;
  rdfs:domain cim:PssIEEE1A ;
  rdfs:range cim:PU ;
  skos:definition "Stabilizer gain (<i>Ks</i>).  Typical value = 5."@en .

cim:PssIEEE1A.t1 a owl:DatatypeProperty ;
  rdfs:label "t1"@en ;
  rdfs:domain cim:PssIEEE1A ;
  rdfs:range cim:Seconds ;
  skos:definition "Lead/lag time constant (<i>T1</i>) (&gt;= 0).  Typical value = 0,3."@en .

cim:PssIEEE1A.t2 a owl:DatatypeProperty ;
  rdfs:label "t2"@en ;
  rdfs:domain cim:PssIEEE1A ;
  rdfs:range cim:Seconds ;
  skos:definition "Lead/lag time constant (<i>T2</i>) (&gt;= 0).  Typical value = 0,03."@en .

cim:PssIEEE1A.t3 a owl:DatatypeProperty ;
  rdfs:label "t3"@en ;
  rdfs:domain cim:PssIEEE1A ;
  rdfs:range cim:Seconds ;
  skos:definition "Lead/lag time constant (<i>T3</i>) (&gt;= 0).  Typical value = 0,3."@en .

cim:PssIEEE1A.t4 a owl:DatatypeProperty ;
  rdfs:label "t4"@en ;
  rdfs:domain cim:PssIEEE1A ;
  rdfs:range cim:Seconds ;
  skos:definition "Lead/lag time constant (<i>T4</i>) (&gt;= 0).  Typical value = 0,03."@en .

cim:PssIEEE1A.t5 a owl:DatatypeProperty ;
  rdfs:label "t5"@en ;
  rdfs:domain cim:PssIEEE1A ;
  rdfs:range cim:Seconds ;
  skos:definition "Washout time constant (<i>T5</i>) (&gt;= 0).  Typical value = 10."@en .

cim:PssIEEE1A.t6 a owl:DatatypeProperty ;
  rdfs:label "t6"@en ;
  rdfs:domain cim:PssIEEE1A ;
  rdfs:range cim:Seconds ;
  skos:definition "Transducer time constant (<i>T6</i>) (&gt;= 0).  Typical value = 0,01."@en .

cim:PssIEEE1A.vrmax a owl:DatatypeProperty ;
  rdfs:label "vrmax"@en ;
  rdfs:domain cim:PssIEEE1A ;
  rdfs:range cim:PU ;
  skos:definition "Maximum stabilizer output (<i>Vrmax</i>) (&gt; PssIEEE1A.vrmin).  Typical value = 0,05."@en .

cim:PssIEEE1A.vrmin a owl:DatatypeProperty ;
  rdfs:label "vrmin"@en ;
  rdfs:domain cim:PssIEEE1A ;
  rdfs:range cim:PU ;
  skos:definition "Minimum stabilizer output (<i>Vrmin</i>) (&lt; PssIEEE1A.vrmax).  Typical value = -0,05."@en .

cim:PssIEEE2B.inputSignal1Type a owl:DatatypeProperty ;
  rdfs:label "inputSignal1Type"@en ;
  rdfs:domain cim:PssIEEE2B ;
  rdfs:range cim:InputSignalKind ;
  skos:definition "Type of input signal #1 (rotorAngularFrequencyDeviation, busFrequencyDeviation).  Typical value = rotorAngularFrequencyDeviation."@en .

cim:PssIEEE2B.inputSignal2Type a owl:DatatypeProperty ;
  rdfs:label "inputSignal2Type"@en ;
  rdfs:domain cim:PssIEEE2B ;
  rdfs:range cim:InputSignalKind ;
  skos:definition "Type of input signal #2 (generatorElectricalPower).  Typical value = generatorElectricalPower."@en .

cim:PssIEEE2B.ks1 a owl:DatatypeProperty ;
  rdfs:label "ks1"@en ;
  rdfs:domain cim:PssIEEE2B ;
  rdfs:range cim:PU ;
  skos:definition "Stabilizer gain (<i>Ks1</i>).  Typical value = 12."@en .

cim:PssIEEE2B.ks2 a owl:DatatypeProperty ;
  rdfs:label "ks2"@en ;
  rdfs:domain cim:PssIEEE2B ;
  rdfs:range cim:PU ;
  skos:definition "Gain on signal #2 (<i>Ks2</i>).  Typical value = 0,2."@en .

cim:PssIEEE2B.ks3 a owl:DatatypeProperty ;
  rdfs:label "ks3"@en ;
  rdfs:domain cim:PssIEEE2B ;
  rdfs:range cim:PU ;
  skos:definition "Gain on signal #2 input before ramp-tracking filter (<i>Ks3</i>).  Typical value = 1."@en .

cim:PssIEEE2B.m a owl:DatatypeProperty ;
  rdfs:label "m"@en ;
  rdfs:domain cim:PssIEEE2B ;
  rdfs:range xsd:integer ;
  skos:definition "Denominator order of ramp tracking filter (<i>M</i>).  Typical value = 5."@en .

cim:PssIEEE2B.n a owl:DatatypeProperty ;
  rdfs:label "n"@en ;
  rdfs:domain cim:PssIEEE2B ;
  rdfs:range xsd:integer ;
  skos:definition "Order of ramp tracking filter (<i>N</i>).  Typical value = 1."@en .

cim:PssIEEE2B.t1 a owl:DatatypeProperty ;
  rdfs:label "t1"@en ;
  rdfs:domain cim:PssIEEE2B ;
  rdfs:range cim:Seconds ;
  skos:definition "Lead/lag time constant (<i>T1</i>) (&gt;= 0).  Typical value = 0,12."@en .

cim:PssIEEE2B.t10 a owl:DatatypeProperty ;
  rdfs:label "t10"@en ;
  rdfs:domain cim:PssIEEE2B ;
  rdfs:range cim:Seconds ;
  skos:definition "Lead/lag time constant (<i>T10</i>) (&gt;= 0).  Typical value = 0."@en .

cim:PssIEEE2B.t11 a owl:DatatypeProperty ;
  rdfs:label "t11"@en ;
  rdfs:domain cim:PssIEEE2B ;
  rdfs:range cim:Seconds ;
  skos:definition "Lead/lag time constant (<i>T11</i>) (&gt;= 0).  Typical value = 0."@en .

cim:PssIEEE2B.t2 a owl:DatatypeProperty ;
  rdfs:label "t2"@en ;
  rdfs:domain cim:PssIEEE2B ;
  rdfs:range cim:Seconds ;
  skos:definition "Lead/lag time constant (<i>T2</i>) (&gt;= 0).  Typical value = 0,02."@en .

cim:PssIEEE2B.t3 a owl:DatatypeProperty ;
  rdfs:label "t3"@en ;
  rdfs:domain cim:PssIEEE2B ;
  rdfs:range cim:Seconds ;
  skos:definition "Lead/lag time constant (<i>T3</i>) (&gt;= 0).  Typical value = 0,3."@en .

cim:PssIEEE2B.t4 a owl:DatatypeProperty ;
  rdfs:label "t4"@en ;
  rdfs:domain cim:PssIEEE2B ;
  rdfs:range cim:Seconds ;
  skos:definition "Lead/lag time constant (<i>T4</i>) (&gt;= 0).  Typical value = 0,02."@en .

cim:PssIEEE2B.t6 a owl:DatatypeProperty ;
  rdfs:label "t6"@en ;
  rdfs:domain cim:PssIEEE2B ;
  rdfs:range cim:Seconds ;
  skos:definition "Time constant on signal #1 (<i>T6</i>) (&gt;= 0).  Typical value = 0."@en .

cim:PssIEEE2B.t7 a owl:DatatypeProperty ;
  rdfs:label "t7"@en ;
  rdfs:domain cim:PssIEEE2B ;
  rdfs:range cim:Seconds ;
  skos:definition "Time constant on signal #2 (<i>T7</i>) (&gt;= 0).  Typical value = 2."@en .

cim:PssIEEE2B.t8 a owl:DatatypeProperty ;
  rdfs:label "t8"@en ;
  rdfs:domain cim:PssIEEE2B ;
  rdfs:range cim:Seconds ;
  skos:definition "Lead of ramp tracking filter (<i>T8</i>) (&gt;= 0).  Typical value = 0,2."@en .

cim:PssIEEE2B.t9 a owl:DatatypeProperty ;
  rdfs:label "t9"@en ;
  rdfs:domain cim:PssIEEE2B ;
  rdfs:range cim:Seconds ;
  skos:definition "Lag of ramp tracking filter (<i>T9</i>) (&gt;= 0).  Typical value = 0,1."@en .

cim:PssIEEE2B.tw1 a owl:DatatypeProperty ;
  rdfs:label "tw1"@en ;
  rdfs:domain cim:PssIEEE2B ;
  rdfs:range cim:Seconds ;
  skos:definition "First washout on signal #1 (<i>Tw1</i>) (&gt;= 0).  Typical value = 2."@en .

cim:PssIEEE2B.tw2 a owl:DatatypeProperty ;
  rdfs:label "tw2"@en ;
  rdfs:domain cim:PssIEEE2B ;
  rdfs:range cim:Seconds ;
  skos:definition "Second washout on signal #1 (<i>Tw2</i>) (&gt;= 0).  Typical value = 2."@en .

cim:PssIEEE2B.tw3 a owl:DatatypeProperty ;
  rdfs:label "tw3"@en ;
  rdfs:domain cim:PssIEEE2B ;
  rdfs:range cim:Seconds ;
  skos:definition "First washout on signal #2 (<i>Tw3</i>) (&gt;= 0).  Typical value = 2."@en .

cim:PssIEEE2B.tw4 a owl:DatatypeProperty ;
  rdfs:label "tw4"@en ;
  rdfs:domain cim:PssIEEE2B ;
  rdfs:range cim:Seconds ;
  skos:definition "Second washout on signal #2 (<i>Tw4</i>) (&gt;= 0).  Typical value = 0."@en .

cim:PssIEEE2B.vsi1max a owl:DatatypeProperty ;
  rdfs:label "vsi1max"@en ;
  rdfs:domain cim:PssIEEE2B ;
  rdfs:range cim:PU ;
  skos:definition "Input signal #1 maximum limit (<i>Vsi1max</i>) (&gt; PssIEEE2B.vsi1min).  Typical value = 2."@en .

cim:PssIEEE2B.vsi1min a owl:DatatypeProperty ;
  rdfs:label "vsi1min"@en ;
  rdfs:domain cim:PssIEEE2B ;
  rdfs:range cim:PU ;
  skos:definition "Input signal #1 minimum limit (<i>Vsi1min</i>) (&lt; PssIEEE2B.vsi1max).  Typical value = -2."@en .

cim:PssIEEE2B.vsi2max a owl:DatatypeProperty ;
  rdfs:label "vsi2max"@en ;
  rdfs:domain cim:PssIEEE2B ;
  rdfs:range cim:PU ;
  skos:definition "Input signal #2 maximum limit (<i>Vsi2max</i>) (&gt; PssIEEE2B.vsi2min).  Typical value = 2."@en .

cim:PssIEEE2B.vsi2min a owl:DatatypeProperty ;
  rdfs:label "vsi2min"@en ;
  rdfs:domain cim:PssIEEE2B ;
  rdfs:range cim:PU ;
  skos:definition "Input signal #2 minimum limit (<i>Vsi2min</i>) (&lt; PssIEEE2B.vsi2max).  Typical value = -2."@en .

cim:PssIEEE2B.vstmax a owl:DatatypeProperty ;
  rdfs:label "vstmax"@en ;
  rdfs:domain cim:PssIEEE2B ;
  rdfs:range cim:PU ;
  skos:definition "Stabilizer output maximum limit (<i>Vstmax</i>) (&gt; PssIEEE2B.vstmin).  Typical value = 0,1."@en .

cim:PssIEEE2B.vstmin a owl:DatatypeProperty ;
  rdfs:label "vstmin"@en ;
  rdfs:domain cim:PssIEEE2B ;
  rdfs:range cim:PU ;
  skos:definition "Stabilizer output minimum limit (<i>Vstmin</i>) (&lt; PssIEEE2B.vstmax).  Typical value = -0,1."@en .

cim:PssIEEE3B.a1 a owl:DatatypeProperty ;
  rdfs:label "a1"@en ;
  rdfs:domain cim:PssIEEE3B ;
  rdfs:range cim:PU ;
  skos:definition "Notch filter parameter (<i>A1</i>).  Typical value = 0,359."@en .

cim:PssIEEE3B.a2 a owl:DatatypeProperty ;
  rdfs:label "a2"@en ;
  rdfs:domain cim:PssIEEE3B ;
  rdfs:range cim:PU ;
  skos:definition "Notch filter parameter (<i>A2</i>).  Typical value = 0,586."@en .

cim:PssIEEE3B.a3 a owl:DatatypeProperty ;
  rdfs:label "a3"@en ;
  rdfs:domain cim:PssIEEE3B ;
  rdfs:range cim:PU ;
  skos:definition "Notch filter parameter (<i>A3</i>).  Typical value = 0,429."@en .

cim:PssIEEE3B.a4 a owl:DatatypeProperty ;
  rdfs:label "a4"@en ;
  rdfs:domain cim:PssIEEE3B ;
  rdfs:range cim:PU ;
  skos:definition "Notch filter parameter (<i>A4</i>).  Typical value = 0,564."@en .

cim:PssIEEE3B.a5 a owl:DatatypeProperty ;
  rdfs:label "a5"@en ;
  rdfs:domain cim:PssIEEE3B ;
  rdfs:range cim:PU ;
  skos:definition "Notch filter parameter (<i>A5</i>).  Typical value = 0,001."@en .

cim:PssIEEE3B.a6 a owl:DatatypeProperty ;
  rdfs:label "a6"@en ;
  rdfs:domain cim:PssIEEE3B ;
  rdfs:range cim:PU ;
  skos:definition "Notch filter parameter (<i>A6</i>).  Typical value = 0."@en .

cim:PssIEEE3B.a7 a owl:DatatypeProperty ;
  rdfs:label "a7"@en ;
  rdfs:domain cim:PssIEEE3B ;
  rdfs:range cim:PU ;
  skos:definition "Notch filter parameter (<i>A7</i>).  Typical value = 0,031."@en .

cim:PssIEEE3B.a8 a owl:DatatypeProperty ;
  rdfs:label "a8"@en ;
  rdfs:domain cim:PssIEEE3B ;
  rdfs:range cim:PU ;
  skos:definition "Notch filter parameter (<i>A8</i>).  Typical value = 0."@en .

cim:PssIEEE3B.ks1 a owl:DatatypeProperty ;
  rdfs:label "ks1"@en ;
  rdfs:domain cim:PssIEEE3B ;
  rdfs:range cim:PU ;
  skos:definition "Gain on signal # 1 (<i>Ks1</i>).  Typical value = -0,602."@en .

cim:PssIEEE3B.ks2 a owl:DatatypeProperty ;
  rdfs:label "ks2"@en ;
  rdfs:domain cim:PssIEEE3B ;
  rdfs:range cim:PU ;
  skos:definition "Gain on signal # 2 (<i>Ks2</i>).  Typical value = 30,12."@en .

cim:PssIEEE3B.t1 a owl:DatatypeProperty ;
  rdfs:label "t1"@en ;
  rdfs:domain cim:PssIEEE3B ;
  rdfs:range cim:Seconds ;
  skos:definition "Transducer time constant (<i>T1</i>) (&gt;= 0).  Typical value = 0,012."@en .

cim:PssIEEE3B.t2 a owl:DatatypeProperty ;
  rdfs:label "t2"@en ;
  rdfs:domain cim:PssIEEE3B ;
  rdfs:range cim:Seconds ;
  skos:definition "Transducer time constant (<i>T2</i>) (&gt;= 0).  Typical value = 0,012."@en .

cim:PssIEEE3B.tw1 a owl:DatatypeProperty ;
  rdfs:label "tw1"@en ;
  rdfs:domain cim:PssIEEE3B ;
  rdfs:range cim:Seconds ;
  skos:definition "Washout time constant (<i>Tw1</i>) (&gt;= 0).  Typical value = 0,3."@en .

cim:PssIEEE3B.tw2 a owl:DatatypeProperty ;
  rdfs:label "tw2"@en ;
  rdfs:domain cim:PssIEEE3B ;
  rdfs:range cim:Seconds ;
  skos:definition "Washout time constant (<i>Tw2</i>) (&gt;= 0).  Typical value = 0,3."@en .

cim:PssIEEE3B.tw3 a owl:DatatypeProperty ;
  rdfs:label "tw3"@en ;
  rdfs:domain cim:PssIEEE3B ;
  rdfs:range cim:Seconds ;
  skos:definition "Washout time constant (<i>Tw3</i>) (&gt;= 0).  Typical value = 0,6."@en .

cim:PssIEEE3B.vstmax a owl:DatatypeProperty ;
  rdfs:label "vstmax"@en ;
  rdfs:domain cim:PssIEEE3B ;
  rdfs:range cim:PU ;
  skos:definition "Stabilizer output maximum limit (<i>Vstmax</i>) (&gt; PssIEEE3B.vstmin).  Typical value = 0,1."@en .

cim:PssIEEE3B.vstmin a owl:DatatypeProperty ;
  rdfs:label "vstmin"@en ;
  rdfs:domain cim:PssIEEE3B ;
  rdfs:range cim:PU ;
  skos:definition "Stabilizer output minimum limit (<i>Vstmin</i>) (&lt; PssIEEE3B.vstmax).  Typical value = -0,1."@en .

cim:PssIEEE4B.bwh1 a owl:DatatypeProperty ;
  rdfs:label "bwh1"@en ;
  rdfs:domain cim:PssIEEE4B ;
  rdfs:range xsd:float ;
  skos:definition "Notch filter 1 (high-frequency band): three dB bandwidth (<i>B</i><i><sub>wi</sub></i>). "@en .

cim:PssIEEE4B.bwh2 a owl:DatatypeProperty ;
  rdfs:label "bwh2"@en ;
  rdfs:domain cim:PssIEEE4B ;
  rdfs:range xsd:float ;
  skos:definition "Notch filter 2 (high-frequency band): three dB bandwidth (<i>B</i><i><sub>wi</sub></i>). "@en .

cim:PssIEEE4B.bwl1 a owl:DatatypeProperty ;
  rdfs:label "bwl1"@en ;
  rdfs:domain cim:PssIEEE4B ;
  rdfs:range xsd:float ;
  skos:definition "Notch filter 1 (low-frequency band): three dB bandwidth (<i>B</i><i><sub>wi</sub></i>). "@en .

cim:PssIEEE4B.bwl2 a owl:DatatypeProperty ;
  rdfs:label "bwl2"@en ;
  rdfs:domain cim:PssIEEE4B ;
  rdfs:range xsd:float ;
  skos:definition "Notch filter 2 (low-frequency band): three dB bandwidth (<i>B</i><i><sub>wi</sub></i>). "@en .

cim:PssIEEE4B.kh a owl:DatatypeProperty ;
  rdfs:label "kh"@en ;
  rdfs:domain cim:PssIEEE4B ;
  rdfs:range cim:PU ;
  skos:definition "High band gain (<i>K</i><i><sub>H</sub></i>).  Typical value = 120."@en .

cim:PssIEEE4B.kh1 a owl:DatatypeProperty ;
  rdfs:label "kh1"@en ;
  rdfs:domain cim:PssIEEE4B ;
  rdfs:range cim:PU ;
  skos:definition "High band differential filter gain (<i>K</i><i><sub>H1</sub></i>).  Typical value = 66."@en .

cim:PssIEEE4B.kh11 a owl:DatatypeProperty ;
  rdfs:label "kh11"@en ;
  rdfs:domain cim:PssIEEE4B ;
  rdfs:range cim:PU ;
  skos:definition "High band first lead-lag blocks coefficient (<i>K</i><i><sub>H11</sub></i>).  Typical value = 1."@en .

cim:PssIEEE4B.kh17 a owl:DatatypeProperty ;
  rdfs:label "kh17"@en ;
  rdfs:domain cim:PssIEEE4B ;
  rdfs:range cim:PU ;
  skos:definition "High band first lead-lag blocks coefficient (<i>K</i><i><sub>H17</sub></i>).  Typical value = 1."@en .

cim:PssIEEE4B.kh2 a owl:DatatypeProperty ;
  rdfs:label "kh2"@en ;
  rdfs:domain cim:PssIEEE4B ;
  rdfs:range cim:PU ;
  skos:definition "High band differential filter gain (<i>K</i><i><sub>H2</sub></i>).  Typical value = 66."@en .

cim:PssIEEE4B.ki a owl:DatatypeProperty ;
  rdfs:label "ki"@en ;
  rdfs:domain cim:PssIEEE4B ;
  rdfs:range cim:PU ;
  skos:definition "Intermediate band gain (<i>K</i><i><sub>I</sub></i>).  Typical value = 30."@en .

cim:PssIEEE4B.ki1 a owl:DatatypeProperty ;
  rdfs:label "ki1"@en ;
  rdfs:domain cim:PssIEEE4B ;
  rdfs:range cim:PU ;
  skos:definition "Intermediate band differential filter gain (<i>K</i><i><sub>I1</sub></i>).  Typical value = 66."@en .

cim:PssIEEE4B.ki11 a owl:DatatypeProperty ;
  rdfs:label "ki11"@en ;
  rdfs:domain cim:PssIEEE4B ;
  rdfs:range cim:PU ;
  skos:definition "Intermediate band first lead-lag blocks coefficient (<i>K</i><i><sub>I11</sub></i>).  Typical value = 1."@en .

cim:PssIEEE4B.ki17 a owl:DatatypeProperty ;
  rdfs:label "ki17"@en ;
  rdfs:domain cim:PssIEEE4B ;
  rdfs:range cim:PU ;
  skos:definition "Intermediate band first lead-lag blocks coefficient (<i>K</i><i><sub>I17</sub></i>).  Typical value = 1."@en .

cim:PssIEEE4B.ki2 a owl:DatatypeProperty ;
  rdfs:label "ki2"@en ;
  rdfs:domain cim:PssIEEE4B ;
  rdfs:range cim:PU ;
  skos:definition "Intermediate band differential filter gain (<i>K</i><i><sub>I2</sub></i>).  Typical value = 66."@en .

cim:PssIEEE4B.kl a owl:DatatypeProperty ;
  rdfs:label "kl"@en ;
  rdfs:domain cim:PssIEEE4B ;
  rdfs:range cim:PU ;
  skos:definition "Low band gain (<i>K</i><i><sub>L</sub></i>).  Typical value = 7.5."@en .

cim:PssIEEE4B.kl1 a owl:DatatypeProperty ;
  rdfs:label "kl1"@en ;
  rdfs:domain cim:PssIEEE4B ;
  rdfs:range cim:PU ;
  skos:definition "Low band differential filter gain (<i>K</i><i><sub>L1</sub></i>).  Typical value = 66."@en .

cim:PssIEEE4B.kl11 a owl:DatatypeProperty ;
  rdfs:label "kl11"@en ;
  rdfs:domain cim:PssIEEE4B ;
  rdfs:range cim:PU ;
  skos:definition "Low band first lead-lag blocks coefficient (<i>K</i><i><sub>L11</sub></i>).  Typical value = 1."@en .

cim:PssIEEE4B.kl17 a owl:DatatypeProperty ;
  rdfs:label "kl17"@en ;
  rdfs:domain cim:PssIEEE4B ;
  rdfs:range cim:PU ;
  skos:definition "Low band first lead-lag blocks coefficient (<i>K</i><i><sub>L17</sub></i>).  Typical value = 1."@en .

cim:PssIEEE4B.kl2 a owl:DatatypeProperty ;
  rdfs:label "kl2"@en ;
  rdfs:domain cim:PssIEEE4B ;
  rdfs:range cim:PU ;
  skos:definition "Low band differential filter gain (<i>K</i><i><sub>L2</sub></i>).  Typical value = 66."@en .

cim:PssIEEE4B.omeganh1 a owl:DatatypeProperty ;
  rdfs:label "omeganh1"@en ;
  rdfs:domain cim:PssIEEE4B ;
  rdfs:range xsd:float ;
  skos:definition "Notch filter 1 (high-frequency band): filter frequency (<i>omega</i><i><sub>ni</sub></i>)."@en .

cim:PssIEEE4B.omeganh2 a owl:DatatypeProperty ;
  rdfs:label "omeganh2"@en ;
  rdfs:domain cim:PssIEEE4B ;
  rdfs:range xsd:float ;
  skos:definition "Notch filter 2 (high-frequency band): filter frequency (<i>omega</i><i><sub>ni</sub></i>)."@en .

cim:PssIEEE4B.omeganl1 a owl:DatatypeProperty ;
  rdfs:label "omeganl1"@en ;
  rdfs:domain cim:PssIEEE4B ;
  rdfs:range xsd:float ;
  skos:definition "Notch filter 1 (low-frequency band): filter frequency (<i>omega</i><i><sub>ni</sub></i>)."@en .

cim:PssIEEE4B.omeganl2 a owl:DatatypeProperty ;
  rdfs:label "omeganl2"@en ;
  rdfs:domain cim:PssIEEE4B ;
  rdfs:range xsd:float ;
  skos:definition "Notch filter 2 (low-frequency band): filter frequency (<i>omega</i><i><sub>ni</sub></i>)."@en .

cim:PssIEEE4B.th1 a owl:DatatypeProperty ;
  rdfs:label "th1"@en ;
  rdfs:domain cim:PssIEEE4B ;
  rdfs:range cim:Seconds ;
  skos:definition "High band time constant (<i>T</i><i><sub>H1</sub></i>) (&gt;= 0).  Typical value = 0,01513."@en .

cim:PssIEEE4B.th10 a owl:DatatypeProperty ;
  rdfs:label "th10"@en ;
  rdfs:domain cim:PssIEEE4B ;
  rdfs:range cim:Seconds ;
  skos:definition "High band time constant (<i>T</i><i><sub>H10</sub></i>) (&gt;= 0).  Typical value = 0."@en .

cim:PssIEEE4B.th11 a owl:DatatypeProperty ;
  rdfs:label "th11"@en ;
  rdfs:domain cim:PssIEEE4B ;
  rdfs:range cim:Seconds ;
  skos:definition "High band time constant (<i>T</i><i><sub>H11</sub></i>) (&gt;= 0).  Typical value = 0."@en .

cim:PssIEEE4B.th12 a owl:DatatypeProperty ;
  rdfs:label "th12"@en ;
  rdfs:domain cim:PssIEEE4B ;
  rdfs:range cim:Seconds ;
  skos:definition "High band time constant (<i>T</i><i><sub>H12</sub></i>) (&gt;= 0).  Typical value = 0."@en .

cim:PssIEEE4B.th2 a owl:DatatypeProperty ;
  rdfs:label "th2"@en ;
  rdfs:domain cim:PssIEEE4B ;
  rdfs:range cim:Seconds ;
  skos:definition "High band time constant (<i>T</i><i><sub>H2</sub></i>) (&gt;= 0).  Typical value = 0,01816."@en .

cim:PssIEEE4B.th3 a owl:DatatypeProperty ;
  rdfs:label "th3"@en ;
  rdfs:domain cim:PssIEEE4B ;
  rdfs:range cim:Seconds ;
  skos:definition "High band time constant (<i>T</i><i><sub>H3</sub></i>) (&gt;= 0).  Typical value = 0."@en .

cim:PssIEEE4B.th4 a owl:DatatypeProperty ;
  rdfs:label "th4"@en ;
  rdfs:domain cim:PssIEEE4B ;
  rdfs:range cim:Seconds ;
  skos:definition "High band time constant (<i>T</i><i><sub>H4</sub></i>) (&gt;= 0).  Typical value = 0."@en .

cim:PssIEEE4B.th5 a owl:DatatypeProperty ;
  rdfs:label "th5"@en ;
  rdfs:domain cim:PssIEEE4B ;
  rdfs:range cim:Seconds ;
  skos:definition "High band time constant (<i>T</i><i><sub>H5</sub></i>) (&gt;= 0).  Typical value = 0."@en .

cim:PssIEEE4B.th6 a owl:DatatypeProperty ;
  rdfs:label "th6"@en ;
  rdfs:domain cim:PssIEEE4B ;
  rdfs:range cim:Seconds ;
  skos:definition "High band time constant (<i>T</i><i><sub>H6</sub></i>) (&gt;= 0).  Typical value = 0."@en .

cim:PssIEEE4B.th7 a owl:DatatypeProperty ;
  rdfs:label "th7"@en ;
  rdfs:domain cim:PssIEEE4B ;
  rdfs:range cim:Seconds ;
  skos:definition "High band time constant (<i>T</i><i><sub>H7</sub></i>) (&gt;= 0).  Typical value = 0,01816."@en .

cim:PssIEEE4B.th8 a owl:DatatypeProperty ;
  rdfs:label "th8"@en ;
  rdfs:domain cim:PssIEEE4B ;
  rdfs:range cim:Seconds ;
  skos:definition "High band time constant (<i>T</i><i><sub>H8</sub></i>) (&gt;= 0).  Typical value = 0,02179."@en .

cim:PssIEEE4B.th9 a owl:DatatypeProperty ;
  rdfs:label "th9"@en ;
  rdfs:domain cim:PssIEEE4B ;
  rdfs:range cim:Seconds ;
  skos:definition "High band time constant (<i>T</i><i><sub>H9</sub></i>) (&gt;= 0).  Typical value = 0."@en .

cim:PssIEEE4B.ti1 a owl:DatatypeProperty ;
  rdfs:label "ti1"@en ;
  rdfs:domain cim:PssIEEE4B ;
  rdfs:range cim:Seconds ;
  skos:definition "Intermediate band time constant (<i>T</i><i><sub>I1</sub></i>) (&gt;= 0).  Typical value = 0,173."@en .

cim:PssIEEE4B.ti10 a owl:DatatypeProperty ;
  rdfs:label "ti10"@en ;
  rdfs:domain cim:PssIEEE4B ;
  rdfs:range cim:Seconds ;
  skos:definition "Intermediate band time constant (<i>T</i><i><sub>I10</sub></i>) (&gt;= 0).  Typical value = 0."@en .

cim:PssIEEE4B.ti11 a owl:DatatypeProperty ;
  rdfs:label "ti11"@en ;
  rdfs:domain cim:PssIEEE4B ;
  rdfs:range cim:Seconds ;
  skos:definition "Intermediate band time constant (<i>T</i><i><sub>I11</sub></i>) (&gt;= 0).  Typical value = 0."@en .

cim:PssIEEE4B.ti12 a owl:DatatypeProperty ;
  rdfs:label "ti12"@en ;
  rdfs:domain cim:PssIEEE4B ;
  rdfs:range cim:Seconds ;
  skos:definition "Intermediate band time constant (<i>T</i><i><sub>I12</sub></i>) (&gt;= 0).  Typical value = 0."@en .

cim:PssIEEE4B.ti2 a owl:DatatypeProperty ;
  rdfs:label "ti2"@en ;
  rdfs:domain cim:PssIEEE4B ;
  rdfs:range cim:Seconds ;
  skos:definition "Intermediate band time constant (<i>T</i><i><sub>I2</sub></i>) (&gt;= 0).  Typical value = 0,2075."@en .

cim:PssIEEE4B.ti3 a owl:DatatypeProperty ;
  rdfs:label "ti3"@en ;
  rdfs:domain cim:PssIEEE4B ;
  rdfs:range cim:Seconds ;
  skos:definition "Intermediate band time constant (<i>T</i><i><sub>I3</sub></i>) (&gt;= 0).  Typical value = 0."@en .

cim:PssIEEE4B.ti4 a owl:DatatypeProperty ;
  rdfs:label "ti4"@en ;
  rdfs:domain cim:PssIEEE4B ;
  rdfs:range cim:Seconds ;
  skos:definition "Intermediate band time constant (<i>T</i><i><sub>I4</sub></i>) (&gt;= 0).  Typical value = 0."@en .

cim:PssIEEE4B.ti5 a owl:DatatypeProperty ;
  rdfs:label "ti5"@en ;
  rdfs:domain cim:PssIEEE4B ;
  rdfs:range cim:Seconds ;
  skos:definition "Intermediate band time constant (<i>T</i><i><sub>I5</sub></i>) (&gt;= 0).  Typical value = 0."@en .

cim:PssIEEE4B.ti6 a owl:DatatypeProperty ;
  rdfs:label "ti6"@en ;
  rdfs:domain cim:PssIEEE4B ;
  rdfs:range cim:Seconds ;
  skos:definition "Intermediate band time constant (<i>T</i><i><sub>I6</sub></i>) (&gt;= 0).  Typical value = 0."@en .

cim:PssIEEE4B.ti7 a owl:DatatypeProperty ;
  rdfs:label "ti7"@en ;
  rdfs:domain cim:PssIEEE4B ;
  rdfs:range cim:Seconds ;
  skos:definition "Intermediate band time constant (<i>T</i><i><sub>I7</sub></i>) (&gt;= 0).  Typical value = 0,2075."@en .

cim:PssIEEE4B.ti8 a owl:DatatypeProperty ;
  rdfs:label "ti8"@en ;
  rdfs:domain cim:PssIEEE4B ;
  rdfs:range cim:Seconds ;
  skos:definition "Intermediate band time constant (<i>T</i><i><sub>I8</sub></i>) (&gt;= 0).  Typical value = 0,2491."@en .

cim:PssIEEE4B.ti9 a owl:DatatypeProperty ;
  rdfs:label "ti9"@en ;
  rdfs:domain cim:PssIEEE4B ;
  rdfs:range cim:Seconds ;
  skos:definition "Intermediate band time constant (<i>T</i><i><sub>I9</sub></i>) (&gt;= 0).  Typical value = 0."@en .

cim:PssIEEE4B.tl1 a owl:DatatypeProperty ;
  rdfs:label "tl1"@en ;
  rdfs:domain cim:PssIEEE4B ;
  rdfs:range cim:Seconds ;
  skos:definition "Low band time constant (<i>T</i><i><sub>L1</sub></i>) (&gt;= 0).  Typical value = 1,73."@en .

cim:PssIEEE4B.tl10 a owl:DatatypeProperty ;
  rdfs:label "tl10"@en ;
  rdfs:domain cim:PssIEEE4B ;
  rdfs:range cim:Seconds ;
  skos:definition "Low band time constant (<i>T</i><i><sub>L10</sub></i>) (&gt;= 0).  Typical value = 0."@en .

cim:PssIEEE4B.tl11 a owl:DatatypeProperty ;
  rdfs:label "tl11"@en ;
  rdfs:domain cim:PssIEEE4B ;
  rdfs:range cim:Seconds ;
  skos:definition "Low band time constant (<i>T</i><i><sub>L11</sub></i>) (&gt;= 0).  Typical value = 0."@en .

cim:PssIEEE4B.tl12 a owl:DatatypeProperty ;
  rdfs:label "tl12"@en ;
  rdfs:domain cim:PssIEEE4B ;
  rdfs:range cim:Seconds ;
  skos:definition "Low band time constant (<i>T</i><i><sub>L12</sub></i>) (&gt;= 0).  Typical value = 0."@en .

cim:PssIEEE4B.tl2 a owl:DatatypeProperty ;
  rdfs:label "tl2"@en ;
  rdfs:domain cim:PssIEEE4B ;
  rdfs:range cim:Seconds ;
  skos:definition "Low band time constant (<i>T</i><i><sub>L2</sub></i>) (&gt;= 0).  Typical value = 2,075."@en .

cim:PssIEEE4B.tl3 a owl:DatatypeProperty ;
  rdfs:label "tl3"@en ;
  rdfs:domain cim:PssIEEE4B ;
  rdfs:range cim:Seconds ;
  skos:definition "Low band time constant (<i>T</i><i><sub>L3</sub></i>) (&gt;= 0).  Typical value = 0."@en .

cim:PssIEEE4B.tl4 a owl:DatatypeProperty ;
  rdfs:label "tl4"@en ;
  rdfs:domain cim:PssIEEE4B ;
  rdfs:range cim:Seconds ;
  skos:definition "Low band time constant (<i>T</i><i><sub>L4</sub></i>) (&gt;= 0).  Typical value = 0."@en .

cim:PssIEEE4B.tl5 a owl:DatatypeProperty ;
  rdfs:label "tl5"@en ;
  rdfs:domain cim:PssIEEE4B ;
  rdfs:range cim:Seconds ;
  skos:definition "Low band time constant (<i>T</i><i><sub>L5</sub></i>) (&gt;= 0).  Typical value = 0."@en .

cim:PssIEEE4B.tl6 a owl:DatatypeProperty ;
  rdfs:label "tl6"@en ;
  rdfs:domain cim:PssIEEE4B ;
  rdfs:range cim:Seconds ;
  skos:definition "Low band time constant (<i>T</i><i><sub>L6</sub></i>) (&gt;= 0).  Typical value = 0."@en .

cim:PssIEEE4B.tl7 a owl:DatatypeProperty ;
  rdfs:label "tl7"@en ;
  rdfs:domain cim:PssIEEE4B ;
  rdfs:range cim:Seconds ;
  skos:definition "Low band time constant (<i>T</i><i><sub>L7</sub></i>) (&gt;= 0).  Typical value = 2,075."@en .

cim:PssIEEE4B.tl8 a owl:DatatypeProperty ;
  rdfs:label "tl8"@en ;
  rdfs:domain cim:PssIEEE4B ;
  rdfs:range cim:Seconds ;
  skos:definition "Low band time constant (<i>T</i><i><sub>L8</sub></i>) (&gt;= 0).  Typical value = 2,491."@en .

cim:PssIEEE4B.tl9 a owl:DatatypeProperty ;
  rdfs:label "tl9"@en ;
  rdfs:domain cim:PssIEEE4B ;
  rdfs:range cim:Seconds ;
  skos:definition "Low band time constant (<i>T</i><i><sub>L9</sub></i>) (&gt;= 0).  Typical value = 0."@en .

cim:PssIEEE4B.vhmax a owl:DatatypeProperty ;
  rdfs:label "vhmax"@en ;
  rdfs:domain cim:PssIEEE4B ;
  rdfs:range cim:PU ;
  skos:definition "High band output maximum limit (<i>V</i><i><sub>Hmax</sub></i>) (&gt; PssIEEE4B.vhmin).  Typical value = 0,6."@en .

cim:PssIEEE4B.vhmin a owl:DatatypeProperty ;
  rdfs:label "vhmin"@en ;
  rdfs:domain cim:PssIEEE4B ;
  rdfs:range cim:PU ;
  skos:definition "High band output minimum limit (<i>V</i><i><sub>Hmin</sub></i>) (&lt; PssIEEE4V.vhmax).  Typical value = -0,6."@en .

cim:PssIEEE4B.vimax a owl:DatatypeProperty ;
  rdfs:label "vimax"@en ;
  rdfs:domain cim:PssIEEE4B ;
  rdfs:range cim:PU ;
  skos:definition "Intermediate band output maximum limit (<i>V</i><i><sub>Imax</sub></i>) (&gt; PssIEEE4B.vimin).  Typical value = 0,6."@en .

cim:PssIEEE4B.vimin a owl:DatatypeProperty ;
  rdfs:label "vimin"@en ;
  rdfs:domain cim:PssIEEE4B ;
  rdfs:range cim:PU ;
  skos:definition "Intermediate band output minimum limit (<i>V</i><i><sub>Imin</sub></i>) (&lt; PssIEEE4B.vimax).  Typical value = -0,6."@en .

cim:PssIEEE4B.vlmax a owl:DatatypeProperty ;
  rdfs:label "vlmax"@en ;
  rdfs:domain cim:PssIEEE4B ;
  rdfs:range cim:PU ;
  skos:definition "Low band output maximum limit (<i>V</i><i><sub>Lmax</sub></i>) (&gt; PssIEEE4B.vlmin).  Typical value = 0,075."@en .

cim:PssIEEE4B.vlmin a owl:DatatypeProperty ;
  rdfs:label "vlmin"@en ;
  rdfs:domain cim:PssIEEE4B ;
  rdfs:range cim:PU ;
  skos:definition "Low band output minimum limit (<i>V</i><i><sub>Lmin</sub></i>) (&lt; PssIEEE4B.vlmax).  Typical value = -0,075."@en .

cim:PssIEEE4B.vstmax a owl:DatatypeProperty ;
  rdfs:label "vstmax"@en ;
  rdfs:domain cim:PssIEEE4B ;
  rdfs:range cim:PU ;
  skos:definition "PSS output maximum limit (<i>V</i><i><sub>STmax</sub></i>) (&gt; PssIEEE4B.vstmin).  Typical value = 0,15."@en .

cim:PssIEEE4B.vstmin a owl:DatatypeProperty ;
  rdfs:label "vstmin"@en ;
  rdfs:domain cim:PssIEEE4B ;
  rdfs:range cim:PU ;
  skos:definition "PSS output minimum limit (<i>V</i><i><sub>STmin</sub></i>) (&lt; PssIEEE4B.vstmax).  Typical value = -0,15."@en .

cim:PssPTIST1.dtc a owl:DatatypeProperty ;
  rdfs:label "dtc"@en ;
  rdfs:domain cim:PssPTIST1 ;
  rdfs:range cim:Seconds ;
  skos:definition "Time step related to activation of controls (<i>deltatc</i>) (&gt;= 0).  Typical value = 0,025."@en .

cim:PssPTIST1.dtf a owl:DatatypeProperty ;
  rdfs:label "dtf"@en ;
  rdfs:domain cim:PssPTIST1 ;
  rdfs:range cim:Seconds ;
  skos:definition "Time step frequency calculation (<i>deltatf</i>) (&gt;= 0).  Typical value = 0,025."@en .

cim:PssPTIST1.dtp a owl:DatatypeProperty ;
  rdfs:label "dtp"@en ;
  rdfs:domain cim:PssPTIST1 ;
  rdfs:range cim:Seconds ;
  skos:definition "Time step active power calculation (<i>deltatp</i>) (&gt;= 0).  Typical value = 0,0125."@en .

cim:PssPTIST1.k a owl:DatatypeProperty ;
  rdfs:label "k"@en ;
  rdfs:domain cim:PssPTIST1 ;
  rdfs:range cim:PU ;
  skos:definition "Gain (<i>K</i>).  Typical value = 9."@en .

cim:PssPTIST1.m a owl:DatatypeProperty ;
  rdfs:label "m"@en ;
  rdfs:domain cim:PssPTIST1 ;
  rdfs:range cim:PU ;
  skos:definition "(<i>M</i>).  <i>M </i>= 2 x <i>H</i>.  Typical value = 5."@en .

cim:PssPTIST1.t1 a owl:DatatypeProperty ;
  rdfs:label "t1"@en ;
  rdfs:domain cim:PssPTIST1 ;
  rdfs:range cim:Seconds ;
  skos:definition "Time constant (<i>T1</i>) (&gt;= 0).  Typical value = 0,3."@en .

cim:PssPTIST1.t2 a owl:DatatypeProperty ;
  rdfs:label "t2"@en ;
  rdfs:domain cim:PssPTIST1 ;
  rdfs:range cim:Seconds ;
  skos:definition "Time constant (<i>T2</i>) (&gt;= 0).  Typical value = 1."@en .

cim:PssPTIST1.t3 a owl:DatatypeProperty ;
  rdfs:label "t3"@en ;
  rdfs:domain cim:PssPTIST1 ;
  rdfs:range cim:Seconds ;
  skos:definition "Time constant (<i>T3</i>) (&gt;= 0).  Typical value = 0,2."@en .

cim:PssPTIST1.t4 a owl:DatatypeProperty ;
  rdfs:label "t4"@en ;
  rdfs:domain cim:PssPTIST1 ;
  rdfs:range cim:Seconds ;
  skos:definition "Time constant (<i>T4</i>) (&gt;= 0).  Typical value = 0,05."@en .

cim:PssPTIST1.tf a owl:DatatypeProperty ;
  rdfs:label "tf"@en ;
  rdfs:domain cim:PssPTIST1 ;
  rdfs:range cim:Seconds ;
  skos:definition "Time constant (<i>Tf</i>) (&gt;= 0).  Typical value = 0,2."@en .

cim:PssPTIST1.tp a owl:DatatypeProperty ;
  rdfs:label "tp"@en ;
  rdfs:domain cim:PssPTIST1 ;
  rdfs:range cim:Seconds ;
  skos:definition "Time constant (<i>Tp</i>) (&gt;= 0).  Typical value = 0,2."@en .

cim:PssPTIST3.a0 a owl:DatatypeProperty ;
  rdfs:label "a0"@en ;
  rdfs:domain cim:PssPTIST3 ;
  rdfs:range cim:PU ;
  skos:definition "Filter coefficient (<i>A0</i>). "@en .

cim:PssPTIST3.a1 a owl:DatatypeProperty ;
  rdfs:label "a1"@en ;
  rdfs:domain cim:PssPTIST3 ;
  rdfs:range cim:PU ;
  skos:definition "Limiter (<i>Al</i>). "@en .

cim:PssPTIST3.a2 a owl:DatatypeProperty ;
  rdfs:label "a2"@en ;
  rdfs:domain cim:PssPTIST3 ;
  rdfs:range cim:PU ;
  skos:definition "Filter coefficient (<i>A2</i>). "@en .

cim:PssPTIST3.a3 a owl:DatatypeProperty ;
  rdfs:label "a3"@en ;
  rdfs:domain cim:PssPTIST3 ;
  rdfs:range cim:PU ;
  skos:definition "Filter coefficient (<i>A3</i>). "@en .

cim:PssPTIST3.a4 a owl:DatatypeProperty ;
  rdfs:label "a4"@en ;
  rdfs:domain cim:PssPTIST3 ;
  rdfs:range cim:PU ;
  skos:definition "Filter coefficient (<i>A4</i>). "@en .

cim:PssPTIST3.a5 a owl:DatatypeProperty ;
  rdfs:label "a5"@en ;
  rdfs:domain cim:PssPTIST3 ;
  rdfs:range cim:PU ;
  skos:definition "Filter coefficient (<i>A5</i>). "@en .

cim:PssPTIST3.al a owl:DatatypeProperty ;
  rdfs:label "al"@en ;
  rdfs:domain cim:PssPTIST3 ;
  rdfs:range cim:PU ;
  skos:definition "Limiter (<i>Al</i>)."@en .

cim:PssPTIST3.athres a owl:DatatypeProperty ;
  rdfs:label "athres"@en ;
  rdfs:domain cim:PssPTIST3 ;
  rdfs:range cim:PU ;
  skos:definition "Threshold value above which output averaging will be bypassed (<i>Athres</i>).  Typical value = 0,005."@en .

cim:PssPTIST3.b0 a owl:DatatypeProperty ;
  rdfs:label "b0"@en ;
  rdfs:domain cim:PssPTIST3 ;
  rdfs:range cim:PU ;
  skos:definition "Filter coefficient (<i>B0</i>). "@en .

cim:PssPTIST3.b1 a owl:DatatypeProperty ;
  rdfs:label "b1"@en ;
  rdfs:domain cim:PssPTIST3 ;
  rdfs:range cim:PU ;
  skos:definition "Filter coefficient (<i>B1</i>). "@en .

cim:PssPTIST3.b2 a owl:DatatypeProperty ;
  rdfs:label "b2"@en ;
  rdfs:domain cim:PssPTIST3 ;
  rdfs:range cim:PU ;
  skos:definition "Filter coefficient (<i>B2</i>). "@en .

cim:PssPTIST3.b3 a owl:DatatypeProperty ;
  rdfs:label "b3"@en ;
  rdfs:domain cim:PssPTIST3 ;
  rdfs:range cim:PU ;
  skos:definition "Filter coefficient (<i>B3</i>). "@en .

cim:PssPTIST3.b4 a owl:DatatypeProperty ;
  rdfs:label "b4"@en ;
  rdfs:domain cim:PssPTIST3 ;
  rdfs:range cim:PU ;
  skos:definition "Filter coefficient (<i>B4</i>). "@en .

cim:PssPTIST3.b5 a owl:DatatypeProperty ;
  rdfs:label "b5"@en ;
  rdfs:domain cim:PssPTIST3 ;
  rdfs:range cim:PU ;
  skos:definition "Filter coefficient (<i>B5</i>). "@en .

cim:PssPTIST3.dl a owl:DatatypeProperty ;
  rdfs:label "dl"@en ;
  rdfs:domain cim:PssPTIST3 ;
  rdfs:range cim:PU ;
  skos:definition "Limiter (<i>Dl</i>). "@en .

cim:PssPTIST3.dtc a owl:DatatypeProperty ;
  rdfs:label "dtc"@en ;
  rdfs:domain cim:PssPTIST3 ;
  rdfs:range cim:Seconds ;
  skos:definition "Time step related to activation of controls (<i>deltatc</i>) (&gt;= 0).  Typical value = 0,025 (0,03 for 50 Hz)."@en .

cim:PssPTIST3.dtf a owl:DatatypeProperty ;
  rdfs:label "dtf"@en ;
  rdfs:domain cim:PssPTIST3 ;
  rdfs:range cim:Seconds ;
  skos:definition "Time step frequency calculation (<i>deltatf</i>) (&gt;= 0).  Typical value = 0,025 (0,03 for 50 Hz)."@en .

cim:PssPTIST3.dtp a owl:DatatypeProperty ;
  rdfs:label "dtp"@en ;
  rdfs:domain cim:PssPTIST3 ;
  rdfs:range cim:Seconds ;
  skos:definition "Time step active power calculation (<i>deltatp</i>) (&gt;= 0).  Typical value = 0,0125  (0,015 for 50 Hz)."@en .

cim:PssPTIST3.isw a owl:DatatypeProperty ;
  rdfs:label "isw"@en ;
  rdfs:domain cim:PssPTIST3 ;
  rdfs:range xsd:boolean ;
  skos:definition """
Digital/analogue output switch (<i>Isw</i>).
true = produce analogue output
false = convert to digital output, using tap selection table. 
\t"""@en .

cim:PssPTIST3.k a owl:DatatypeProperty ;
  rdfs:label "k"@en ;
  rdfs:domain cim:PssPTIST3 ;
  rdfs:range cim:PU ;
  skos:definition "Gain (<i>K</i>).  Typical value = 9."@en .

cim:PssPTIST3.lthres a owl:DatatypeProperty ;
  rdfs:label "lthres"@en ;
  rdfs:domain cim:PssPTIST3 ;
  rdfs:range cim:PU ;
  skos:definition "Threshold value (<i>Lthres</i>)."@en .

cim:PssPTIST3.m a owl:DatatypeProperty ;
  rdfs:label "m"@en ;
  rdfs:domain cim:PssPTIST3 ;
  rdfs:range cim:PU ;
  skos:definition "(<i>M</i>).  <i>M</i> = 2 x <i>H</i>.  Typical value = 5."@en .

cim:PssPTIST3.nav a owl:DatatypeProperty ;
  rdfs:label "nav"@en ;
  rdfs:domain cim:PssPTIST3 ;
  rdfs:range xsd:float ;
  skos:definition "Number of control outputs to average (<i>NAV</i>) (1 &lt;=  <i>NAV</i> &lt;= 16).  Typical value = 4."@en .

cim:PssPTIST3.ncl a owl:DatatypeProperty ;
  rdfs:label "ncl"@en ;
  rdfs:domain cim:PssPTIST3 ;
  rdfs:range xsd:float ;
  skos:definition "Number of counts at limit to active limit function (<i>NCL</i>) (&gt; 0). "@en .

cim:PssPTIST3.ncr a owl:DatatypeProperty ;
  rdfs:label "ncr"@en ;
  rdfs:domain cim:PssPTIST3 ;
  rdfs:range xsd:float ;
  skos:definition "Number of counts until reset after limit function is triggered (<i>NCR</i>). "@en .

cim:PssPTIST3.pmin a owl:DatatypeProperty ;
  rdfs:label "pmin"@en ;
  rdfs:domain cim:PssPTIST3 ;
  rdfs:range cim:PU ;
  skos:definition "(<i>Pmin</i>)."@en .

cim:PssPTIST3.t1 a owl:DatatypeProperty ;
  rdfs:label "t1"@en ;
  rdfs:domain cim:PssPTIST3 ;
  rdfs:range cim:Seconds ;
  skos:definition "Time constant (<i>T1</i>) (&gt;= 0).  Typical value = 0,3."@en .

cim:PssPTIST3.t2 a owl:DatatypeProperty ;
  rdfs:label "t2"@en ;
  rdfs:domain cim:PssPTIST3 ;
  rdfs:range cim:Seconds ;
  skos:definition "Time constant (<i>T2</i>) (&gt;= 0).  Typical value = 1."@en .

cim:PssPTIST3.t3 a owl:DatatypeProperty ;
  rdfs:label "t3"@en ;
  rdfs:domain cim:PssPTIST3 ;
  rdfs:range cim:Seconds ;
  skos:definition "Time constant (<i>T3</i>) (&gt;= 0).  Typical value = 0,2."@en .

cim:PssPTIST3.t4 a owl:DatatypeProperty ;
  rdfs:label "t4"@en ;
  rdfs:domain cim:PssPTIST3 ;
  rdfs:range cim:Seconds ;
  skos:definition "Time constant (<i>T4</i>) (&gt;= 0).  Typical value = 0,05."@en .

cim:PssPTIST3.t5 a owl:DatatypeProperty ;
  rdfs:label "t5"@en ;
  rdfs:domain cim:PssPTIST3 ;
  rdfs:range cim:Seconds ;
  skos:definition "Time constant (<i>T5</i>) (&gt;= 0). "@en .

cim:PssPTIST3.t6 a owl:DatatypeProperty ;
  rdfs:label "t6"@en ;
  rdfs:domain cim:PssPTIST3 ;
  rdfs:range cim:Seconds ;
  skos:definition "Time constant (<i>T6</i>) (&gt;= 0). "@en .

cim:PssPTIST3.tf a owl:DatatypeProperty ;
  rdfs:label "tf"@en ;
  rdfs:domain cim:PssPTIST3 ;
  rdfs:range cim:Seconds ;
  skos:definition "Time constant (<i>Tf</i>) (&gt;= 0).  Typical value = 0,2."@en .

cim:PssPTIST3.tp a owl:DatatypeProperty ;
  rdfs:label "tp"@en ;
  rdfs:domain cim:PssPTIST3 ;
  rdfs:range cim:Seconds ;
  skos:definition "Time constant (<i>Tp</i>) (&gt;= 0).  Typical value = 0,2."@en .

cim:PssRQB.kdpm a owl:DatatypeProperty ;
  rdfs:label "kdpm"@en ;
  rdfs:domain cim:PssRQB ;
  rdfs:range xsd:float ;
  skos:definition "Lead lag gain (<i>KDPM</i>). Typical value = 0,185."@en .

cim:PssRQB.ki2 a owl:DatatypeProperty ;
  rdfs:label "ki2"@en ;
  rdfs:domain cim:PssRQB ;
  rdfs:range xsd:float ;
  skos:definition "Speed input gain (<i>Ki2</i>). Typical value = 3,43."@en .

cim:PssRQB.ki3 a owl:DatatypeProperty ;
  rdfs:label "ki3"@en ;
  rdfs:domain cim:PssRQB ;
  rdfs:range xsd:float ;
  skos:definition "Electrical power input gain (<i>Ki3</i>). Typical value = -11,45."@en .

cim:PssRQB.ki4 a owl:DatatypeProperty ;
  rdfs:label "ki4"@en ;
  rdfs:domain cim:PssRQB ;
  rdfs:range xsd:float ;
  skos:definition "Mechanical power input gain (<i>Ki4</i>). Typical value = 11,86."@en .

cim:PssRQB.sibv a owl:DatatypeProperty ;
  rdfs:label "sibv"@en ;
  rdfs:domain cim:PssRQB ;
  rdfs:range cim:PU ;
  skos:definition "Speed deadband (<i>SIBV</i>). Typical value = 0,006."@en .

cim:PssRQB.t4f a owl:DatatypeProperty ;
  rdfs:label "t4f"@en ;
  rdfs:domain cim:PssRQB ;
  rdfs:range cim:Seconds ;
  skos:definition "Lead lag time constant (<i>T4F</i>) (&gt;= 0). Typical value = 0,045."@en .

cim:PssRQB.t4m a owl:DatatypeProperty ;
  rdfs:label "t4m"@en ;
  rdfs:domain cim:PssRQB ;
  rdfs:range cim:Seconds ;
  skos:definition "Input time constant (<i>T4M</i>) (&gt;= 0). Typical value = 5."@en .

cim:PssRQB.t4mom a owl:DatatypeProperty ;
  rdfs:label "t4mom"@en ;
  rdfs:domain cim:PssRQB ;
  rdfs:range cim:Seconds ;
  skos:definition "Speed time constant (<i>T4MOM</i>) (&gt;= 0). Typical value = 1,27."@en .

cim:PssRQB.tomd a owl:DatatypeProperty ;
  rdfs:label "tomd"@en ;
  rdfs:domain cim:PssRQB ;
  rdfs:range cim:Seconds ;
  skos:definition "Speed delay (<i>TOMD</i>) (&gt;= 0). Typical value = 0,02."@en .

cim:PssRQB.tomsl a owl:DatatypeProperty ;
  rdfs:label "tomsl"@en ;
  rdfs:domain cim:PssRQB ;
  rdfs:range cim:Seconds ;
  skos:definition "Speed time constant (<i>TOMSL</i>) (&gt;= 0). Typical value = 0,04."@en .

cim:PssSB4.kx a owl:DatatypeProperty ;
  rdfs:label "kx"@en ;
  rdfs:domain cim:PssSB4 ;
  rdfs:range cim:PU ;
  skos:definition "Gain (<i>Kx</i>).  Typical value = 2,7."@en .

cim:PssSB4.ta a owl:DatatypeProperty ;
  rdfs:label "ta"@en ;
  rdfs:domain cim:PssSB4 ;
  rdfs:range cim:Seconds ;
  skos:definition "Time constant (<i>Ta</i>) (&gt;= 0).  Typical value = 0,37."@en .

cim:PssSB4.tb a owl:DatatypeProperty ;
  rdfs:label "tb"@en ;
  rdfs:domain cim:PssSB4 ;
  rdfs:range cim:Seconds ;
  skos:definition "Time constant (<i>Tb</i>) (&gt;= 0).  Typical value = 0,37."@en .

cim:PssSB4.tc a owl:DatatypeProperty ;
  rdfs:label "tc"@en ;
  rdfs:domain cim:PssSB4 ;
  rdfs:range cim:Seconds ;
  skos:definition "Time constant (<i>Tc</i>) (&gt;= 0).  Typical value = 0,035."@en .

cim:PssSB4.td a owl:DatatypeProperty ;
  rdfs:label "td"@en ;
  rdfs:domain cim:PssSB4 ;
  rdfs:range cim:Seconds ;
  skos:definition "Time constant (<i>Td</i>) (&gt;= 0).  Typical value = 0,0."@en .

cim:PssSB4.te a owl:DatatypeProperty ;
  rdfs:label "te"@en ;
  rdfs:domain cim:PssSB4 ;
  rdfs:range cim:Seconds ;
  skos:definition "Time constant (<i>Te</i>) (&gt;= 0).  Typical value = 0,0169."@en .

cim:PssSB4.tt a owl:DatatypeProperty ;
  rdfs:label "tt"@en ;
  rdfs:domain cim:PssSB4 ;
  rdfs:range cim:Seconds ;
  skos:definition "Time constant (<i>Tt</i>) (&gt;= 0).  Typical value = 0,18."@en .

cim:PssSB4.tx1 a owl:DatatypeProperty ;
  rdfs:label "tx1"@en ;
  rdfs:domain cim:PssSB4 ;
  rdfs:range cim:Seconds ;
  skos:definition "Reset time constant (<i>Tx1</i>) (&gt;= 0).  Typical value = 0,035."@en .

cim:PssSB4.tx2 a owl:DatatypeProperty ;
  rdfs:label "tx2"@en ;
  rdfs:domain cim:PssSB4 ;
  rdfs:range cim:Seconds ;
  skos:definition "Time constant (<i>Tx2</i>) (&gt;= 0).  Typical value = 5,0."@en .

cim:PssSB4.vsmax a owl:DatatypeProperty ;
  rdfs:label "vsmax"@en ;
  rdfs:domain cim:PssSB4 ;
  rdfs:range cim:PU ;
  skos:definition "Limiter (<i>Vsmax</i>) (&gt; PssSB4.vsmin).  Typical value = 0,062."@en .

cim:PssSB4.vsmin a owl:DatatypeProperty ;
  rdfs:label "vsmin"@en ;
  rdfs:domain cim:PssSB4 ;
  rdfs:range cim:PU ;
  skos:definition "Limiter (<i>Vsmin</i>) (&lt; PssSB4.vsmax).  Typical value = -0,062."@en .

cim:PssSH.k a owl:DatatypeProperty ;
  rdfs:label "k"@en ;
  rdfs:domain cim:PssSH ;
  rdfs:range cim:PU ;
  skos:definition "Main gain (<i>K</i>).  Typical value = 1."@en .

cim:PssSH.k0 a owl:DatatypeProperty ;
  rdfs:label "k0"@en ;
  rdfs:domain cim:PssSH ;
  rdfs:range cim:PU ;
  skos:definition "Gain 0 (<i>K0</i>).  Typical value = 0,012."@en .

cim:PssSH.k1 a owl:DatatypeProperty ;
  rdfs:label "k1"@en ;
  rdfs:domain cim:PssSH ;
  rdfs:range cim:PU ;
  skos:definition "Gain 1 (<i>K1</i>).  Typical value = 0,488."@en .

cim:PssSH.k2 a owl:DatatypeProperty ;
  rdfs:label "k2"@en ;
  rdfs:domain cim:PssSH ;
  rdfs:range cim:PU ;
  skos:definition "Gain 2 (<i>K2</i>).  Typical value = 0,064."@en .

cim:PssSH.k3 a owl:DatatypeProperty ;
  rdfs:label "k3"@en ;
  rdfs:domain cim:PssSH ;
  rdfs:range cim:PU ;
  skos:definition "Gain 3 (<i>K3</i>).  Typical value = 0,224."@en .

cim:PssSH.k4 a owl:DatatypeProperty ;
  rdfs:label "k4"@en ;
  rdfs:domain cim:PssSH ;
  rdfs:range cim:PU ;
  skos:definition "Gain 4 (<i>K4</i>).  Typical value = 0,1."@en .

cim:PssSH.t1 a owl:DatatypeProperty ;
  rdfs:label "t1"@en ;
  rdfs:domain cim:PssSH ;
  rdfs:range cim:Seconds ;
  skos:definition "Time constant 1 (<i>T1</i>) (&gt; 0).  Typical value = 0,076."@en .

cim:PssSH.t2 a owl:DatatypeProperty ;
  rdfs:label "t2"@en ;
  rdfs:domain cim:PssSH ;
  rdfs:range cim:Seconds ;
  skos:definition "Time constant 2 (<i>T2</i>) (&gt; 0).  Typical value = 0,086."@en .

cim:PssSH.t3 a owl:DatatypeProperty ;
  rdfs:label "t3"@en ;
  rdfs:domain cim:PssSH ;
  rdfs:range cim:Seconds ;
  skos:definition "Time constant 3 (<i>T3</i>) (&gt; 0).   Typical value = 1,068."@en .

cim:PssSH.t4 a owl:DatatypeProperty ;
  rdfs:label "t4"@en ;
  rdfs:domain cim:PssSH ;
  rdfs:range cim:Seconds ;
  skos:definition "Time constant 4 (<i>T4</i>) (&gt; 0).  Typical value = 1,913."@en .

cim:PssSH.td a owl:DatatypeProperty ;
  rdfs:label "td"@en ;
  rdfs:domain cim:PssSH ;
  rdfs:range cim:Seconds ;
  skos:definition "Input time constant (<i>T</i><i><sub>d</sub></i>) (&gt;= 0).  Typical value = 10."@en .

cim:PssSH.vsmax a owl:DatatypeProperty ;
  rdfs:label "vsmax"@en ;
  rdfs:domain cim:PssSH ;
  rdfs:range cim:PU ;
  skos:definition "Output maximum limit (<i>Vsmax</i>) (&gt; PssSH.vsmin).  Typical value = 0,1."@en .

cim:PssSH.vsmin a owl:DatatypeProperty ;
  rdfs:label "vsmin"@en ;
  rdfs:domain cim:PssSH ;
  rdfs:range cim:PU ;
  skos:definition "Output minimum limit (<i>Vsmin</i>) (&lt; PssSH.vsmax).  Typical value = -0,1."@en .

cim:PssSK.k1 a owl:DatatypeProperty ;
  rdfs:label "k1"@en ;
  rdfs:domain cim:PssSK ;
  rdfs:range cim:PU ;
  skos:definition "Gain <i>P</i> (<i>K</i><i><sub>1</sub></i>).  Typical value = -0,3."@en .

cim:PssSK.k2 a owl:DatatypeProperty ;
  rdfs:label "k2"@en ;
  rdfs:domain cim:PssSK ;
  rdfs:range cim:PU ;
  skos:definition "Gain <i>f</i><i><sub>E</sub></i><i> </i>(<i>K</i><i><sub>2</sub></i>).  Typical value = -0,15."@en .

cim:PssSK.k3 a owl:DatatypeProperty ;
  rdfs:label "k3"@en ;
  rdfs:domain cim:PssSK ;
  rdfs:range cim:PU ;
  skos:definition "Gain <i>I</i><i><sub>f</sub></i><i> </i>(<i>K</i><i><sub>3</sub></i>).  Typical value = 10."@en .

cim:PssSK.t1 a owl:DatatypeProperty ;
  rdfs:label "t1"@en ;
  rdfs:domain cim:PssSK ;
  rdfs:range cim:Seconds ;
  skos:definition "Denominator time constant (<i>T</i><i><sub>1</sub></i>) (&gt; 0,005).  Typical value = 0,3."@en .

cim:PssSK.t2 a owl:DatatypeProperty ;
  rdfs:label "t2"@en ;
  rdfs:domain cim:PssSK ;
  rdfs:range cim:Seconds ;
  skos:definition "Filter time constant (<i>T</i><i><sub>2</sub></i>) (&gt; 0,005).  Typical value = 0,35."@en .

cim:PssSK.t3 a owl:DatatypeProperty ;
  rdfs:label "t3"@en ;
  rdfs:domain cim:PssSK ;
  rdfs:range cim:Seconds ;
  skos:definition "Denominator time constant (<i>T</i><i><sub>3</sub></i>) (&gt; 0,005).  Typical value = 0,22."@en .

cim:PssSK.t4 a owl:DatatypeProperty ;
  rdfs:label "t4"@en ;
  rdfs:domain cim:PssSK ;
  rdfs:range cim:Seconds ;
  skos:definition "Filter time constant (<i>T</i><i><sub>4</sub></i>) (&gt; 0,005).  Typical value = 0,02."@en .

cim:PssSK.t5 a owl:DatatypeProperty ;
  rdfs:label "t5"@en ;
  rdfs:domain cim:PssSK ;
  rdfs:range cim:Seconds ;
  skos:definition "Denominator time constant (<i>T</i><i><sub>5</sub></i>) (&gt; 0,005).  Typical value = 0,02."@en .

cim:PssSK.t6 a owl:DatatypeProperty ;
  rdfs:label "t6"@en ;
  rdfs:domain cim:PssSK ;
  rdfs:range cim:Seconds ;
  skos:definition "Filter time constant (<i>T</i><i><sub>6</sub></i>) (&gt; 0,005).  Typical value = 0,02."@en .

cim:PssSK.vsmax a owl:DatatypeProperty ;
  rdfs:label "vsmax"@en ;
  rdfs:domain cim:PssSK ;
  rdfs:range cim:PU ;
  skos:definition "Stabilizer output maximum limit (<i>V</i><i><sub>SMAX</sub></i>) (&gt; PssSK.vsmin).  Typical value = 0,4."@en .

cim:PssSK.vsmin a owl:DatatypeProperty ;
  rdfs:label "vsmin"@en ;
  rdfs:domain cim:PssSK ;
  rdfs:range cim:PU ;
  skos:definition "Stabilizer output minimum limit (<i>V</i><i><sub>SMIN</sub></i>) (&lt; PssSK.vsmax).  Typical value = -0.4."@en .

cim:PssSTAB2A.hlim a owl:DatatypeProperty ;
  rdfs:label "hlim"@en ;
  rdfs:domain cim:PssSTAB2A ;
  rdfs:range cim:PU ;
  skos:definition "Stabilizer output limiter (<i>H</i><i><sub>LIM</sub></i>).  Typical value = 0,5."@en .

cim:PssSTAB2A.k2 a owl:DatatypeProperty ;
  rdfs:label "k2"@en ;
  rdfs:domain cim:PssSTAB2A ;
  rdfs:range cim:PU ;
  skos:definition "Gain (<i>K2</i>).  Typical value = 1,0."@en .

cim:PssSTAB2A.k3 a owl:DatatypeProperty ;
  rdfs:label "k3"@en ;
  rdfs:domain cim:PssSTAB2A ;
  rdfs:range cim:PU ;
  skos:definition "Gain (<i>K3</i>).  Typical value = 0,25."@en .

cim:PssSTAB2A.k4 a owl:DatatypeProperty ;
  rdfs:label "k4"@en ;
  rdfs:domain cim:PssSTAB2A ;
  rdfs:range cim:PU ;
  skos:definition "Gain (<i>K4</i>).  Typical value = 0,075."@en .

cim:PssSTAB2A.k5 a owl:DatatypeProperty ;
  rdfs:label "k5"@en ;
  rdfs:domain cim:PssSTAB2A ;
  rdfs:range cim:PU ;
  skos:definition "Gain (<i>K5</i>).  Typical value = 2,5."@en .

cim:PssSTAB2A.t2 a owl:DatatypeProperty ;
  rdfs:label "t2"@en ;
  rdfs:domain cim:PssSTAB2A ;
  rdfs:range cim:Seconds ;
  skos:definition "Time constant (<i>T2</i>).  Typical value = 4,0."@en .

cim:PssSTAB2A.t3 a owl:DatatypeProperty ;
  rdfs:label "t3"@en ;
  rdfs:domain cim:PssSTAB2A ;
  rdfs:range cim:Seconds ;
  skos:definition "Time constant (<i>T3</i>).  Typical value = 2,0."@en .

cim:PssSTAB2A.t5 a owl:DatatypeProperty ;
  rdfs:label "t5"@en ;
  rdfs:domain cim:PssSTAB2A ;
  rdfs:range cim:Seconds ;
  skos:definition "Time constant (<i>T5</i>).  Typical value = 4,5."@en .

cim:PssWECC.inputSignal1Type a owl:DatatypeProperty ;
  rdfs:label "inputSignal1Type"@en ;
  rdfs:domain cim:PssWECC ;
  rdfs:range cim:InputSignalKind ;
  skos:definition "Type of input signal #1 (rotorAngularFrequencyDeviation, busFrequencyDeviation, generatorElectricalPower, generatorAcceleratingPower, busVoltage, or busVoltageDerivative - shall be different than PssWECC.inputSignal2Type).  Typical value = rotorAngularFrequencyDeviation."@en .

cim:PssWECC.inputSignal2Type a owl:DatatypeProperty ;
  rdfs:label "inputSignal2Type"@en ;
  rdfs:domain cim:PssWECC ;
  rdfs:range cim:InputSignalKind ;
  skos:definition "Type of input signal #2 (rotorAngularFrequencyDeviation, busFrequencyDeviation, generatorElectricalPower, generatorAcceleratingPower, busVoltage, busVoltageDerivative - shall be different than PssWECC.inputSignal1Type).  Typical value = busVoltageDerivative."@en .

cim:PssWECC.k1 a owl:DatatypeProperty ;
  rdfs:label "k1"@en ;
  rdfs:domain cim:PssWECC ;
  rdfs:range cim:PU ;
  skos:definition "Input signal 1 gain (<i>K</i><i><sub>1</sub></i>).  Typical value = 1,13. "@en .

cim:PssWECC.k2 a owl:DatatypeProperty ;
  rdfs:label "k2"@en ;
  rdfs:domain cim:PssWECC ;
  rdfs:range cim:PU ;
  skos:definition "Input signal 2 gain (<i>K</i><i><sub>2</sub></i>).  Typical value = 0,0."@en .

cim:PssWECC.t1 a owl:DatatypeProperty ;
  rdfs:label "t1"@en ;
  rdfs:domain cim:PssWECC ;
  rdfs:range cim:Seconds ;
  skos:definition "Input signal 1 transducer time constant (<i>T</i><i><sub>1</sub></i>) (&gt;= 0).  Typical value = 0,037."@en .

cim:PssWECC.t10 a owl:DatatypeProperty ;
  rdfs:label "t10"@en ;
  rdfs:domain cim:PssWECC ;
  rdfs:range cim:Seconds ;
  skos:definition "Lag time constant (<i>T</i><i><sub>10</sub></i>) (&gt;= 0).  Typical value = 0."@en .

cim:PssWECC.t2 a owl:DatatypeProperty ;
  rdfs:label "t2"@en ;
  rdfs:domain cim:PssWECC ;
  rdfs:range cim:Seconds ;
  skos:definition "Input signal 2 transducer time constant (<i>T</i><i><sub>2</sub></i>) (&gt;= 0).  Typical value = 0,0."@en .

cim:PssWECC.t3 a owl:DatatypeProperty ;
  rdfs:label "t3"@en ;
  rdfs:domain cim:PssWECC ;
  rdfs:range cim:Seconds ;
  skos:definition "Stabilizer washout time constant (<i>T</i><i><sub>3</sub></i>) (&gt;= 0).  Typical value = 9,5."@en .

cim:PssWECC.t4 a owl:DatatypeProperty ;
  rdfs:label "t4"@en ;
  rdfs:domain cim:PssWECC ;
  rdfs:range cim:Seconds ;
  skos:definition "Stabilizer washout time lag constant (<i>T</i><i><sub>4</sub></i>) (&gt;= 0).  Typical value = 9,5."@en .

cim:PssWECC.t5 a owl:DatatypeProperty ;
  rdfs:label "t5"@en ;
  rdfs:domain cim:PssWECC ;
  rdfs:range cim:Seconds ;
  skos:definition "Lead time constant (<i>T</i><i><sub>5</sub></i>) (&gt;= 0).  Typical value = 1,7."@en .

cim:PssWECC.t6 a owl:DatatypeProperty ;
  rdfs:label "t6"@en ;
  rdfs:domain cim:PssWECC ;
  rdfs:range cim:Seconds ;
  skos:definition "Lag time constant (<i>T</i><i><sub>6</sub></i>) (&gt;= 0).  Typical value = 1,5."@en .

cim:PssWECC.t7 a owl:DatatypeProperty ;
  rdfs:label "t7"@en ;
  rdfs:domain cim:PssWECC ;
  rdfs:range cim:Seconds ;
  skos:definition "Lead time constant (<i>T</i><i><sub>7</sub></i>) (&gt;= 0).  Typical value = 1,7."@en .

cim:PssWECC.t8 a owl:DatatypeProperty ;
  rdfs:label "t8"@en ;
  rdfs:domain cim:PssWECC ;
  rdfs:range cim:Seconds ;
  skos:definition "Lag time constant (<i>T</i><i><sub>8</sub></i>) (&gt;= 0).  Typical value = 1,5."@en .

cim:PssWECC.t9 a owl:DatatypeProperty ;
  rdfs:label "t9"@en ;
  rdfs:domain cim:PssWECC ;
  rdfs:range cim:Seconds ;
  skos:definition "Lead time constant (<i>T</i><i><sub>9</sub></i>) (&gt;= 0).  Typical value = 0."@en .

cim:PssWECC.vcl a owl:DatatypeProperty ;
  rdfs:label "vcl"@en ;
  rdfs:domain cim:PssWECC ;
  rdfs:range cim:PU ;
  skos:definition "Minimum value for voltage compensator output (<i>V</i><i><sub>CL</sub></i>). Typical value = 0."@en .

cim:PssWECC.vcu a owl:DatatypeProperty ;
  rdfs:label "vcu"@en ;
  rdfs:domain cim:PssWECC ;
  rdfs:range cim:PU ;
  skos:definition "Maximum value for voltage compensator output (<i>V</i><i><sub>CU</sub></i>). Typical value = 0."@en .

cim:PssWECC.vsmax a owl:DatatypeProperty ;
  rdfs:label "vsmax"@en ;
  rdfs:domain cim:PssWECC ;
  rdfs:range cim:PU ;
  skos:definition """
Maximum output signal (<i>Vsmax</i>) (&gt; PssWECC.vsmin). Typical value = 0,05.

\t"""@en .

cim:PssWECC.vsmin a owl:DatatypeProperty ;
  rdfs:label "vsmin"@en ;
  rdfs:domain cim:PssWECC ;
  rdfs:range cim:PU ;
  skos:definition "Minimum output signal (<i>Vsmin</i>) (&lt; PssWECC.vsmax).  Typical value = -0,05."@en .

cim:RemoteInputSignal.remoteSignalType a owl:DatatypeProperty ;
  rdfs:label "remoteSignalType"@en ;
  rdfs:domain cim:RemoteInputSignal ;
  rdfs:range cim:RemoteSignalKind ;
  skos:definition "Type of input signal."@en .

cim:RotatingMachineDynamics.damping a owl:DatatypeProperty ;
  rdfs:label "damping"@en ;
  rdfs:domain cim:RotatingMachineDynamics ;
  rdfs:range xsd:float ;
  skos:definition "Damping torque coefficient (<i>D</i>) (&gt;= 0).  A proportionality constant that, when multiplied by the angular velocity of the rotor poles with respect to the magnetic field (frequency), results in the damping torque.  This value is often zero when the sources of damping torques (generator damper windings, load damping effects, etc.) are modelled in detail.  Typical value = 0."@en .

cim:RotatingMachineDynamics.inertia a owl:DatatypeProperty ;
  rdfs:label "inertia"@en ;
  rdfs:domain cim:RotatingMachineDynamics ;
  rdfs:range cim:Seconds ;
  skos:definition "Inertia constant of generator or motor and mechanical load (<i>H</i>) (&gt; 0).  This is the specification for the stored energy in the rotating mass when operating at rated speed.  For a generator, this includes the generator plus all other elements (turbine, exciter) on the same shaft and has units of MW x s.  For a motor, it includes the motor plus its mechanical load. Conventional units are PU on the generator MVA base, usually expressed as MW x s / MVA or just s. This value is used in the accelerating power reference frame for operator training simulator solutions.  Typical value = 3."@en .

cim:RotatingMachineDynamics.saturationFactor a owl:DatatypeProperty, owl:FunctionalProperty ;
  rdfs:label "saturationFactor"@en ;
  rdfs:domain cim:RotatingMachineDynamics ;
  rdfs:range xsd:float ;
  skos:definition "Saturation factor at rated terminal voltage (<i>S1</i>) (&gt;= 0).  Not used by simplified model.  Defined by defined by <i>S</i>(<i>E1</i>) in the SynchronousMachineSaturationParameters diagram.  Typical value = 0,02."@en .

cim:RotatingMachineDynamics.saturationFactor120 a owl:DatatypeProperty, owl:FunctionalProperty ;
  rdfs:label "saturationFactor120"@en ;
  rdfs:domain cim:RotatingMachineDynamics ;
  rdfs:range xsd:float ;
  skos:definition "Saturation factor at 120% of rated terminal voltage (<i>S12</i>) (&gt;= RotatingMachineDynamics.saturationFactor). Not used by the simplified model, defined by <i>S</i>(<i>E2</i>) in the SynchronousMachineSaturationParameters diagram.  Typical value = 0,12."@en .

cim:RotatingMachineDynamics.statorLeakageReactance a owl:DatatypeProperty ;
  rdfs:label "statorLeakageReactance"@en ;
  rdfs:domain cim:RotatingMachineDynamics ;
  rdfs:range cim:PU ;
  skos:definition "Stator leakage reactance (<i>Xl</i>) (&gt;= 0). Typical value = 0,15."@en .

cim:RotatingMachineDynamics.statorResistance a owl:DatatypeProperty ;
  rdfs:label "statorResistance"@en ;
  rdfs:domain cim:RotatingMachineDynamics ;
  rdfs:range cim:PU ;
  skos:definition "Stator (armature) resistance (<i>Rs</i>) (&gt;= 0). Typical value = 0,005."@en .

cim:SVCUserDefined.proprietary a owl:DatatypeProperty ;
  rdfs:label "proprietary"@en ;
  rdfs:domain cim:SVCUserDefined ;
  rdfs:range xsd:boolean ;
  skos:definition """
Behaviour is based on a proprietary model as opposed to a detailed model.
true = user-defined model is proprietary with behaviour mutually understood by sending and receiving applications and parameters passed as general attributes
false = user-defined model is explicitly defined in terms of control blocks and their input and output signals.
\t"""@en .

cim:Seconds.multiplier a owl:DatatypeProperty, owl:FunctionalProperty ;
  rdfs:label "multiplier"@en ;
  dy:isFixed "True " ;
  rdf:value "none" ;
  rdfs:domain cim:Seconds ;
  rdfs:range cim:UnitMultiplier .

cim:Seconds.unit a owl:DatatypeProperty, owl:FunctionalProperty ;
  rdfs:label "unit"@en ;
  dy:isFixed "True " ;
  rdf:value "s" ;
  rdfs:domain cim:Seconds ;
  rdfs:range cim:UnitSymbol .

cim:Seconds.value a owl:DatatypeProperty, owl:FunctionalProperty ;
  rdfs:label "value"@en ;
  rdfs:domain cim:Seconds ;
  rdfs:range xsd:float ;
  skos:definition "Time, in seconds"@en .

cim:SynchronousMachineDetailed.efdBaseRatio a owl:DatatypeProperty ;
  rdfs:label "efdBaseRatio"@en ;
  rdfs:domain cim:SynchronousMachineDetailed ;
  rdfs:range xsd:float ;
  skos:definition "Ratio (exciter voltage/generator voltage) of <i>Efd</i> bases of exciter and generator models (&gt; 0). Typical value = 1."@en .

cim:SynchronousMachineDetailed.ifdBaseType a owl:DatatypeProperty ;
  rdfs:label "ifdBaseType"@en ;
  rdfs:domain cim:SynchronousMachineDetailed ;
  rdfs:range cim:IfdBaseKind ;
  skos:definition "Excitation base system mode. It should be equal to the value of <i>WLMDV</i> given by the user. <i>WLMDV</i> is the PU ratio between the field voltage and the excitation current: <i>Efd</i> = <i>WLMDV</i> x <i>Ifd</i>. Typical value = ifag."@en .

cim:SynchronousMachineDetailed.saturationFactor120QAxis a owl:DatatypeProperty, owl:FunctionalProperty ;
  rdfs:label "saturationFactor120QAxis"@en ;
  rdfs:domain cim:SynchronousMachineDetailed ;
  rdfs:range xsd:float ;
  skos:definition "Quadrature-axis saturation factor at 120% of rated terminal voltage (<i>S12q</i>) (&gt;= SynchonousMachineDetailed.saturationFactorQAxis).  Typical value = 0,12."@en .

cim:SynchronousMachineDetailed.saturationFactorQAxis a owl:DatatypeProperty, owl:FunctionalProperty ;
  rdfs:label "saturationFactorQAxis"@en ;
  rdfs:domain cim:SynchronousMachineDetailed ;
  rdfs:range xsd:float ;
  skos:definition "Quadrature-axis saturation factor at rated terminal voltage (<i>S1q</i>) (&gt;= 0). Typical value = 0,02."@en .

cim:SynchronousMachineEquivalentCircuit.r1d a owl:DatatypeProperty ;
  rdfs:label "r1d"@en ;
  rdfs:domain cim:SynchronousMachineEquivalentCircuit ;
  rdfs:range cim:PU ;
  skos:definition "Direct-axis damper 1 winding resistance."@en .

cim:SynchronousMachineEquivalentCircuit.r1q a owl:DatatypeProperty ;
  rdfs:label "r1q"@en ;
  rdfs:domain cim:SynchronousMachineEquivalentCircuit ;
  rdfs:range cim:PU ;
  skos:definition "Quadrature-axis damper 1 winding resistance."@en .

cim:SynchronousMachineEquivalentCircuit.r2q a owl:DatatypeProperty ;
  rdfs:label "r2q"@en ;
  rdfs:domain cim:SynchronousMachineEquivalentCircuit ;
  rdfs:range cim:PU ;
  skos:definition "Quadrature-axis damper 2 winding resistance."@en .

cim:SynchronousMachineEquivalentCircuit.rfd a owl:DatatypeProperty ;
  rdfs:label "rfd"@en ;
  rdfs:domain cim:SynchronousMachineEquivalentCircuit ;
  rdfs:range cim:PU ;
  skos:definition "Field winding resistance."@en .

cim:SynchronousMachineEquivalentCircuit.x1d a owl:DatatypeProperty ;
  rdfs:label "x1d"@en ;
  rdfs:domain cim:SynchronousMachineEquivalentCircuit ;
  rdfs:range cim:PU ;
  skos:definition "Direct-axis damper 1 winding leakage reactance."@en .

cim:SynchronousMachineEquivalentCircuit.x1q a owl:DatatypeProperty ;
  rdfs:label "x1q"@en ;
  rdfs:domain cim:SynchronousMachineEquivalentCircuit ;
  rdfs:range cim:PU ;
  skos:definition "Quadrature-axis damper 1 winding leakage reactance."@en .

cim:SynchronousMachineEquivalentCircuit.x2q a owl:DatatypeProperty ;
  rdfs:label "x2q"@en ;
  rdfs:domain cim:SynchronousMachineEquivalentCircuit ;
  rdfs:range cim:PU ;
  skos:definition "Quadrature-axis damper 2 winding leakage reactance."@en .

cim:SynchronousMachineEquivalentCircuit.xad a owl:DatatypeProperty ;
  rdfs:label "xad"@en ;
  rdfs:domain cim:SynchronousMachineEquivalentCircuit ;
  rdfs:range cim:PU ;
  skos:definition "Direct-axis mutual reactance."@en .

cim:SynchronousMachineEquivalentCircuit.xaq a owl:DatatypeProperty ;
  rdfs:label "xaq"@en ;
  rdfs:domain cim:SynchronousMachineEquivalentCircuit ;
  rdfs:range cim:PU ;
  skos:definition "Quadrature-axis mutual reactance."@en .

cim:SynchronousMachineEquivalentCircuit.xf1d a owl:DatatypeProperty ;
  rdfs:label "xf1d"@en ;
  rdfs:domain cim:SynchronousMachineEquivalentCircuit ;
  rdfs:range cim:PU ;
  skos:definition "Differential mutual (“Canay”) reactance."@en .

cim:SynchronousMachineEquivalentCircuit.xfd a owl:DatatypeProperty ;
  rdfs:label "xfd"@en ;
  rdfs:domain cim:SynchronousMachineEquivalentCircuit ;
  rdfs:range cim:PU ;
  skos:definition "Field winding leakage reactance."@en .

cim:SynchronousMachineTimeConstantReactance.ks a owl:DatatypeProperty ;
  rdfs:label "ks"@en ;
  rdfs:domain cim:SynchronousMachineTimeConstantReactance ;
  rdfs:range xsd:float ;
  skos:definition "Saturation loading correction factor (<i>Ks</i>) (&gt;= 0).  Used only by type J model.  Typical value = 0."@en .

cim:SynchronousMachineTimeConstantReactance.modelType a owl:DatatypeProperty ;
  rdfs:label "modelType"@en ;
  rdfs:domain cim:SynchronousMachineTimeConstantReactance ;
  rdfs:range cim:SynchronousMachineModelKind ;
  skos:definition "Type of synchronous machine model used in dynamic simulation applications."@en .

cim:SynchronousMachineTimeConstantReactance.rotorType a owl:DatatypeProperty, owl:FunctionalProperty ;
  rdfs:label "rotorType"@en ;
  rdfs:domain cim:SynchronousMachineTimeConstantReactance ;
  rdfs:range cim:RotorKind ;
  skos:definition "Type of rotor on physical machine."@en .

cim:SynchronousMachineTimeConstantReactance.tc a owl:DatatypeProperty ;
  rdfs:label "tc"@en ;
  rdfs:domain cim:SynchronousMachineTimeConstantReactance ;
  rdfs:range cim:Seconds ;
  skos:definition "Damping time constant for “Canay” reactance (&gt;= 0).  Typical value = 0."@en .

cim:SynchronousMachineTimeConstantReactance.tpdo a owl:DatatypeProperty ;
  rdfs:label "tpdo"@en ;
  rdfs:domain cim:SynchronousMachineTimeConstantReactance ;
  rdfs:range cim:Seconds ;
  skos:definition "Direct-axis transient rotor time constant (<i>T'do</i>) (&gt; SynchronousMachineTimeConstantReactance.tppdo).  Typical value = 5."@en .

cim:SynchronousMachineTimeConstantReactance.tppdo a owl:DatatypeProperty ;
  rdfs:label "tppdo"@en ;
  rdfs:domain cim:SynchronousMachineTimeConstantReactance ;
  rdfs:range cim:Seconds ;
  skos:definition "Direct-axis subtransient rotor time constant (<i>T''do</i>) (&gt; 0).  Typical value = 0,03."@en .

cim:SynchronousMachineTimeConstantReactance.tppqo a owl:DatatypeProperty ;
  rdfs:label "tppqo"@en ;
  rdfs:domain cim:SynchronousMachineTimeConstantReactance ;
  rdfs:range cim:Seconds ;
  skos:definition "Quadrature-axis subtransient rotor time constant (<i>T''qo</i>) (&gt; 0). Typical value = 0,03."@en .

cim:SynchronousMachineTimeConstantReactance.tpqo a owl:DatatypeProperty, owl:FunctionalProperty ;
  rdfs:label "tpqo"@en ;
  rdfs:domain cim:SynchronousMachineTimeConstantReactance ;
  rdfs:range cim:Seconds ;
  skos:definition "Quadrature-axis transient rotor time constant (<i>T'qo</i>) (&gt; SynchronousMachineTimeConstantReactance.tppqo). Typical value = 0,5."@en .

cim:SynchronousMachineTimeConstantReactance.xDirectSubtrans a owl:DatatypeProperty ;
  rdfs:label "xDirectSubtrans"@en ;
  rdfs:domain cim:SynchronousMachineTimeConstantReactance ;
  rdfs:range cim:PU ;
  skos:definition "Direct-axis subtransient reactance (unsaturated) (<i>X''d</i>) (&gt; RotatingMachineDynamics.statorLeakageReactance).  Typical value = 0,2."@en .

cim:SynchronousMachineTimeConstantReactance.xDirectSync a owl:DatatypeProperty ;
  rdfs:label "xDirectSync"@en ;
  rdfs:domain cim:SynchronousMachineTimeConstantReactance ;
  rdfs:range cim:PU ;
  skos:definition "Direct-axis synchronous reactance (<i>Xd</i>) (&gt;= SynchronousMachineTimeConstantReactance.xDirectTrans). The quotient of a sustained value of that AC component of armature voltage that is produced by the total direct-axis flux due to direct-axis armature current and the value of the AC component of this current, the machine running at rated speed.  Typical value = 1,8."@en .

cim:SynchronousMachineTimeConstantReactance.xDirectTrans a owl:DatatypeProperty ;
  rdfs:label "xDirectTrans"@en ;
  rdfs:domain cim:SynchronousMachineTimeConstantReactance ;
  rdfs:range cim:PU ;
  skos:definition "Direct-axis transient reactance (unsaturated) (<i>X'd</i>) (&gt;= SynchronousMachineTimeConstantReactance.xDirectSubtrans).  Typical value = 0,5."@en .

cim:SynchronousMachineTimeConstantReactance.xQuadSubtrans a owl:DatatypeProperty ;
  rdfs:label "xQuadSubtrans"@en ;
  rdfs:domain cim:SynchronousMachineTimeConstantReactance ;
  rdfs:range cim:PU ;
  skos:definition "Quadrature-axis subtransient reactance (<i>X''q</i>) (&gt; RotatingMachineDynamics.statorLeakageReactance).  Typical value = 0,2."@en .

cim:SynchronousMachineTimeConstantReactance.xQuadSync a owl:DatatypeProperty ;
  rdfs:label "xQuadSync"@en ;
  rdfs:domain cim:SynchronousMachineTimeConstantReactance ;
  rdfs:range cim:PU ;
  skos:definition """
Quadrature-axis synchronous reactance (<i>Xq</i>) (&gt;= SynchronousMachineTimeConstantReactance.xQuadTrans).
The ratio of the component of reactive armature voltage, due to the quadrature-axis component of armature current, to this component of current, under steady state conditions and at rated frequency.  Typical value = 1,6.
\t"""@en .

cim:SynchronousMachineTimeConstantReactance.xQuadTrans a owl:DatatypeProperty, owl:FunctionalProperty ;
  rdfs:label "xQuadTrans"@en ;
  rdfs:domain cim:SynchronousMachineTimeConstantReactance ;
  rdfs:range cim:PU ;
  skos:definition "Quadrature-axis transient reactance (<i>X'q</i>) (&gt;= SynchronousMachineTimeConstantReactance.xQuadSubtrans).  Typical value = 0,3."@en .

cim:SynchronousMachineUserDefined.proprietary a owl:DatatypeProperty ;
  rdfs:label "proprietary"@en ;
  rdfs:domain cim:SynchronousMachineUserDefined ;
  rdfs:range xsd:boolean ;
  skos:definition """
Behaviour is based on a proprietary model as opposed to a detailed model.
true = user-defined model is proprietary with behaviour mutually understood by sending and receiving applications and parameters passed as general attributes
false = user-defined model is explicitly defined in terms of control blocks and their input and output signals.
\t"""@en .

cim:Temperature.multiplier a owl:DatatypeProperty, owl:FunctionalProperty ;
  rdfs:label "multiplier"@en ;
  dy:isFixed "True " ;
  rdf:value "none" ;
  rdfs:domain cim:Temperature ;
  rdfs:range cim:UnitMultiplier .

cim:Temperature.unit a owl:DatatypeProperty, owl:FunctionalProperty ;
  rdfs:label "unit"@en ;
  dy:isFixed "True " ;
  rdf:value "degC" ;
  rdfs:domain cim:Temperature ;
  rdfs:range cim:UnitSymbol .

cim:Temperature.value a owl:DatatypeProperty, owl:FunctionalProperty ;
  rdfs:label "value"@en ;
  rdfs:domain cim:Temperature ;
  rdfs:range xsd:float .

cim:TurbLCFB1.db a owl:DatatypeProperty ;
  rdfs:label "db"@en ;
  rdfs:domain cim:TurbLCFB1 ;
  rdfs:range cim:PU ;
  skos:definition "Controller deadband (<i>db</i>).  Typical value = 0."@en .

cim:TurbLCFB1.emax a owl:DatatypeProperty ;
  rdfs:label "emax"@en ;
  rdfs:domain cim:TurbLCFB1 ;
  rdfs:range cim:PU ;
  skos:definition "Maximum control error (<i>Emax</i>) (see parameter detail 4).  Typical value = 0,02."@en .

cim:TurbLCFB1.fb a owl:DatatypeProperty ;
  rdfs:label "fb"@en ;
  rdfs:domain cim:TurbLCFB1 ;
  rdfs:range cim:PU ;
  skos:definition "Frequency bias gain (<i>Fb</i>).  Typical value = 0."@en .

cim:TurbLCFB1.fbf a owl:DatatypeProperty ;
  rdfs:label "fbf"@en ;
  rdfs:domain cim:TurbLCFB1 ;
  rdfs:range xsd:boolean ;
  skos:definition """
Frequency bias flag (<i>Fbf</i>).
true = enable frequency bias
false = disable frequency bias.
Typical value = false.
\t"""@en .

cim:TurbLCFB1.irmax a owl:DatatypeProperty ;
  rdfs:label "irmax"@en ;
  rdfs:domain cim:TurbLCFB1 ;
  rdfs:range cim:PU ;
  skos:definition "Maximum turbine speed/load reference bias (<i>Irmax</i>) (see parameter detail 3).  Typical value = 0."@en .

cim:TurbLCFB1.ki a owl:DatatypeProperty ;
  rdfs:label "ki"@en ;
  rdfs:domain cim:TurbLCFB1 ;
  rdfs:range cim:PU ;
  skos:definition "Integral gain (<i>Ki</i>).  Typical value = 0."@en .

cim:TurbLCFB1.kp a owl:DatatypeProperty ;
  rdfs:label "kp"@en ;
  rdfs:domain cim:TurbLCFB1 ;
  rdfs:range cim:PU ;
  skos:definition "Proportional gain (<i>Kp</i>).  Typical value = 0."@en .

cim:TurbLCFB1.mwbase a owl:DatatypeProperty ;
  rdfs:label "mwbase"@en ;
  rdfs:domain cim:TurbLCFB1 ;
  rdfs:range cim:ActivePower ;
  skos:definition "Base for power values (<i>MWbase</i>) (&gt; 0).  Unit = MW."@en .

cim:TurbLCFB1.pbf a owl:DatatypeProperty ;
  rdfs:label "pbf"@en ;
  rdfs:domain cim:TurbLCFB1 ;
  rdfs:range xsd:boolean ;
  skos:definition """
Power controller flag (<i>Pbf</i>).
true = enable load controller
false = disable load controller.
Typical value = false.
\t"""@en .

cim:TurbLCFB1.pmwset a owl:DatatypeProperty ;
  rdfs:label "pmwset"@en ;
  rdfs:domain cim:TurbLCFB1 ;
  rdfs:range cim:ActivePower ;
  skos:definition "Power controller setpoint (<i>Pmwset</i>) (see parameter detail 1).  Unit = MW. Typical value = 0."@en .

cim:TurbLCFB1.speedReferenceGovernor a owl:DatatypeProperty ;
  rdfs:label "speedReferenceGovernor"@en ;
  rdfs:domain cim:TurbLCFB1 ;
  rdfs:range xsd:boolean ;
  skos:definition """
Type of turbine governor reference (<i>Type</i>).
true = speed reference governor
false = load reference governor.
Typical value = true.
\t"""@en .

cim:TurbLCFB1.tpelec a owl:DatatypeProperty ;
  rdfs:label "tpelec"@en ;
  rdfs:domain cim:TurbLCFB1 ;
  rdfs:range cim:Seconds ;
  skos:definition "Power transducer time constant (<i>Tpelec</i>) (&gt;= 0).  Typical value = 0."@en .

cim:TurbineGovernorUserDefined.proprietary a owl:DatatypeProperty ;
  rdfs:label "proprietary"@en ;
  rdfs:domain cim:TurbineGovernorUserDefined ;
  rdfs:range xsd:boolean ;
  skos:definition """
Behaviour is based on a proprietary model as opposed to a detailed model.
true = user-defined model is proprietary with behaviour mutually understood by sending and receiving applications and parameters passed as general attributes
false = user-defined model is explicitly defined in terms of control blocks and their input and output signals.
\t"""@en .

cim:TurbineLoadControllerUserDefined.proprietary a owl:DatatypeProperty ;
  rdfs:label "proprietary"@en ;
  rdfs:domain cim:TurbineLoadControllerUserDefined ;
  rdfs:range xsd:boolean ;
  skos:definition """
Behaviour is based on a proprietary model as opposed to a detailed model.
true = user-defined model is proprietary with behaviour mutually understood by sending and receiving applications and parameters passed as general attributes
false = user-defined model is explicitly defined in terms of control blocks and their input and output signals.
\t"""@en .

cim:UnderexcLim2Simplified.kui a owl:DatatypeProperty ;
  rdfs:label "kui"@en ;
  rdfs:domain cim:UnderexcLim2Simplified ;
  rdfs:range cim:PU ;
  skos:definition "Gain Under excitation limiter (<i>K</i><i><sub>UI</sub></i>).  Typical value = 0,1."@en .

cim:UnderexcLim2Simplified.p0 a owl:DatatypeProperty ;
  rdfs:label "p0"@en ;
  rdfs:domain cim:UnderexcLim2Simplified ;
  rdfs:range cim:PU ;
  skos:definition "Segment P initial point (<i>P</i><i><sub>0</sub></i>).  Typical value = 0."@en .

cim:UnderexcLim2Simplified.p1 a owl:DatatypeProperty ;
  rdfs:label "p1"@en ;
  rdfs:domain cim:UnderexcLim2Simplified ;
  rdfs:range cim:PU ;
  skos:definition "Segment P end point (<i>P</i><i><sub>1</sub></i>).  Typical value = 1."@en .

cim:UnderexcLim2Simplified.q0 a owl:DatatypeProperty ;
  rdfs:label "q0"@en ;
  rdfs:domain cim:UnderexcLim2Simplified ;
  rdfs:range cim:PU ;
  skos:definition "Segment Q initial point (<i>Q</i><i><sub>0</sub></i>).  Typical value = -0,31."@en .

cim:UnderexcLim2Simplified.q1 a owl:DatatypeProperty ;
  rdfs:label "q1"@en ;
  rdfs:domain cim:UnderexcLim2Simplified ;
  rdfs:range cim:PU ;
  skos:definition "Segment Q end point (<i>Q</i><i><sub>1</sub></i>).  Typical value = -0,1."@en .

cim:UnderexcLim2Simplified.vuimax a owl:DatatypeProperty ;
  rdfs:label "vuimax"@en ;
  rdfs:domain cim:UnderexcLim2Simplified ;
  rdfs:range cim:PU ;
  skos:definition "Maximum error signal (<i>V</i><i><sub>UIMAX</sub></i>) (&gt; UnderexcLim2Simplified.vuimin).  Typical value = 1."@en .

cim:UnderexcLim2Simplified.vuimin a owl:DatatypeProperty ;
  rdfs:label "vuimin"@en ;
  rdfs:domain cim:UnderexcLim2Simplified ;
  rdfs:range cim:PU ;
  skos:definition "Minimum error signal (<i>V</i><i><sub>UIMIN</sub></i>) (&lt; UnderexcLim2Simplified.vuimax).  Typical value = 0."@en .

cim:UnderexcLimIEEE1.kuc a owl:DatatypeProperty ;
  rdfs:label "kuc"@en ;
  rdfs:domain cim:UnderexcLimIEEE1 ;
  rdfs:range cim:PU ;
  skos:definition "UEL centre setting (<i>K</i><i><sub>UC</sub></i>).  Typical value = 1,38."@en .

cim:UnderexcLimIEEE1.kuf a owl:DatatypeProperty ;
  rdfs:label "kuf"@en ;
  rdfs:domain cim:UnderexcLimIEEE1 ;
  rdfs:range cim:PU ;
  skos:definition "UEL excitation system stabilizer gain (<i>K</i><i><sub>UF</sub></i>).  Typical value = 3,3."@en .

cim:UnderexcLimIEEE1.kui a owl:DatatypeProperty ;
  rdfs:label "kui"@en ;
  rdfs:domain cim:UnderexcLimIEEE1 ;
  rdfs:range cim:PU ;
  skos:definition "UEL integral gain (<i>K</i><i><sub>UI</sub></i>).  Typical value = 0."@en .

cim:UnderexcLimIEEE1.kul a owl:DatatypeProperty ;
  rdfs:label "kul"@en ;
  rdfs:domain cim:UnderexcLimIEEE1 ;
  rdfs:range cim:PU ;
  skos:definition "UEL proportional gain (<i>K</i><i><sub>UL</sub></i>).  Typical value = 100."@en .

cim:UnderexcLimIEEE1.kur a owl:DatatypeProperty ;
  rdfs:label "kur"@en ;
  rdfs:domain cim:UnderexcLimIEEE1 ;
  rdfs:range cim:PU ;
  skos:definition "UEL radius setting (<i>K</i><i><sub>UR</sub></i>).  Typical value = 1,95."@en .

cim:UnderexcLimIEEE1.tu1 a owl:DatatypeProperty ;
  rdfs:label "tu1"@en ;
  rdfs:domain cim:UnderexcLimIEEE1 ;
  rdfs:range cim:Seconds ;
  skos:definition "UEL lead time constant (<i>T</i><i><sub>U1</sub></i>) (&gt;= 0).  Typical value = 0."@en .

cim:UnderexcLimIEEE1.tu2 a owl:DatatypeProperty ;
  rdfs:label "tu2"@en ;
  rdfs:domain cim:UnderexcLimIEEE1 ;
  rdfs:range cim:Seconds ;
  skos:definition "UEL lag time constant (<i>T</i><i><sub>U2</sub></i>) (&gt;= 0).  Typical value = 0,05."@en .

cim:UnderexcLimIEEE1.tu3 a owl:DatatypeProperty ;
  rdfs:label "tu3"@en ;
  rdfs:domain cim:UnderexcLimIEEE1 ;
  rdfs:range cim:Seconds ;
  skos:definition "UEL lead time constant (<i>T</i><i><sub>U3</sub></i>) (&gt;= 0).  Typical value = 0."@en .

cim:UnderexcLimIEEE1.tu4 a owl:DatatypeProperty ;
  rdfs:label "tu4"@en ;
  rdfs:domain cim:UnderexcLimIEEE1 ;
  rdfs:range cim:Seconds ;
  skos:definition "UEL lag time constant (<i>T</i><i><sub>U4</sub></i>) (&gt;= 0).  Typical value = 0."@en .

cim:UnderexcLimIEEE1.vucmax a owl:DatatypeProperty ;
  rdfs:label "vucmax"@en ;
  rdfs:domain cim:UnderexcLimIEEE1 ;
  rdfs:range cim:PU ;
  skos:definition "UEL maximum limit for operating point phasor magnitude (<i>V</i><i><sub>UCMAX</sub></i>).  Typical value = 5,8."@en .

cim:UnderexcLimIEEE1.vuimax a owl:DatatypeProperty ;
  rdfs:label "vuimax"@en ;
  rdfs:domain cim:UnderexcLimIEEE1 ;
  rdfs:range cim:PU ;
  skos:definition "UEL integrator output maximum limit (<i>V</i><i><sub>UIMAX</sub></i>) (&gt; UnderexcLimIEEE1.vuimin)."@en .

cim:UnderexcLimIEEE1.vuimin a owl:DatatypeProperty ;
  rdfs:label "vuimin"@en ;
  rdfs:domain cim:UnderexcLimIEEE1 ;
  rdfs:range cim:PU ;
  skos:definition "UEL integrator output minimum limit (<i>V</i><i><sub>UIMIN</sub></i>) (&lt; UnderexcLimIEEE1.vuimax)."@en .

cim:UnderexcLimIEEE1.vulmax a owl:DatatypeProperty ;
  rdfs:label "vulmax"@en ;
  rdfs:domain cim:UnderexcLimIEEE1 ;
  rdfs:range cim:PU ;
  skos:definition "UEL output maximum limit (<i>V</i><i><sub>ULMAX</sub></i>) (&gt; UnderexcLimIEEE1.vulmin).  Typical value = 18."@en .

cim:UnderexcLimIEEE1.vulmin a owl:DatatypeProperty ;
  rdfs:label "vulmin"@en ;
  rdfs:domain cim:UnderexcLimIEEE1 ;
  rdfs:range cim:PU ;
  skos:definition "UEL output minimum limit (<i>V</i><i><sub>ULMIN</sub></i>) (&lt; UnderexcLimIEEE1.vulmax).  Typical value = -18."@en .

cim:UnderexcLimIEEE1.vurmax a owl:DatatypeProperty ;
  rdfs:label "vurmax"@en ;
  rdfs:domain cim:UnderexcLimIEEE1 ;
  rdfs:range cim:PU ;
  skos:definition "UEL maximum limit for radius phasor magnitude (<i>V</i><i><sub>URMAX</sub></i>).  Typical value = 5,8."@en .

cim:UnderexcLimIEEE2.k1 a owl:DatatypeProperty ;
  rdfs:label "k1"@en ;
  rdfs:domain cim:UnderexcLimIEEE2 ;
  rdfs:range xsd:float ;
  skos:definition "UEL terminal voltage exponent applied to real power input to UEL limit look-up table (<i>k1</i>).  Typical value = 2."@en .

cim:UnderexcLimIEEE2.k2 a owl:DatatypeProperty ;
  rdfs:label "k2"@en ;
  rdfs:domain cim:UnderexcLimIEEE2 ;
  rdfs:range xsd:float ;
  skos:definition "UEL terminal voltage exponent applied to reactive power output from UEL limit look-up table (<i>k2</i>).  Typical value = 2."@en .

cim:UnderexcLimIEEE2.kfb a owl:DatatypeProperty ;
  rdfs:label "kfb"@en ;
  rdfs:domain cim:UnderexcLimIEEE2 ;
  rdfs:range cim:PU ;
  skos:definition "Gain associated with optional integrator feedback input signal to UEL (<i>K</i><i><sub>FB</sub></i>).  Typical value = 0."@en .

cim:UnderexcLimIEEE2.kuf a owl:DatatypeProperty ;
  rdfs:label "kuf"@en ;
  rdfs:domain cim:UnderexcLimIEEE2 ;
  rdfs:range cim:PU ;
  skos:definition "UEL excitation system stabilizer gain (<i>K</i><i><sub>UF</sub></i>).  Typical value = 0."@en .

cim:UnderexcLimIEEE2.kui a owl:DatatypeProperty ;
  rdfs:label "kui"@en ;
  rdfs:domain cim:UnderexcLimIEEE2 ;
  rdfs:range cim:PU ;
  skos:definition "UEL integral gain (<i>K</i><i><sub>UI</sub></i>).  Typical value = 0,5."@en .

cim:UnderexcLimIEEE2.kul a owl:DatatypeProperty ;
  rdfs:label "kul"@en ;
  rdfs:domain cim:UnderexcLimIEEE2 ;
  rdfs:range cim:PU ;
  skos:definition "UEL proportional gain (<i>K</i><i><sub>UL</sub></i>).  Typical value = 0,8."@en .

cim:UnderexcLimIEEE2.p0 a owl:DatatypeProperty ;
  rdfs:label "p0"@en ;
  rdfs:domain cim:UnderexcLimIEEE2 ;
  rdfs:range cim:PU ;
  skos:definition "Real power values for endpoints (<i>P</i><i><sub>0</sub></i>).  Typical value = 0."@en .

cim:UnderexcLimIEEE2.p1 a owl:DatatypeProperty ;
  rdfs:label "p1"@en ;
  rdfs:domain cim:UnderexcLimIEEE2 ;
  rdfs:range cim:PU ;
  skos:definition "Real power values for endpoints (<i>P</i><i><sub>1</sub></i>).  Typical value = 0,3."@en .

cim:UnderexcLimIEEE2.p10 a owl:DatatypeProperty ;
  rdfs:label "p10"@en ;
  rdfs:domain cim:UnderexcLimIEEE2 ;
  rdfs:range cim:PU ;
  skos:definition "Real power values for endpoints (<i>P</i><i><sub>10</sub></i>). "@en .

cim:UnderexcLimIEEE2.p2 a owl:DatatypeProperty ;
  rdfs:label "p2"@en ;
  rdfs:domain cim:UnderexcLimIEEE2 ;
  rdfs:range cim:PU ;
  skos:definition "Real power values for endpoints (<i>P</i><i><sub>2</sub></i>).  Typical value = 0,6."@en .

cim:UnderexcLimIEEE2.p3 a owl:DatatypeProperty ;
  rdfs:label "p3"@en ;
  rdfs:domain cim:UnderexcLimIEEE2 ;
  rdfs:range cim:PU ;
  skos:definition "Real power values for endpoints (<i>P</i><i><sub>3</sub></i>).  Typical value = 0,9."@en .

cim:UnderexcLimIEEE2.p4 a owl:DatatypeProperty ;
  rdfs:label "p4"@en ;
  rdfs:domain cim:UnderexcLimIEEE2 ;
  rdfs:range cim:PU ;
  skos:definition "Real power values for endpoints (<i>P</i><i><sub>4</sub></i>).  Typical value = 1,02."@en .

cim:UnderexcLimIEEE2.p5 a owl:DatatypeProperty ;
  rdfs:label "p5"@en ;
  rdfs:domain cim:UnderexcLimIEEE2 ;
  rdfs:range cim:PU ;
  skos:definition "Real power values for endpoints (<i>P</i><i><sub>5</sub></i>). "@en .

cim:UnderexcLimIEEE2.p6 a owl:DatatypeProperty ;
  rdfs:label "p6"@en ;
  rdfs:domain cim:UnderexcLimIEEE2 ;
  rdfs:range cim:PU ;
  skos:definition "Real power values for endpoints (<i>P</i><i><sub>6</sub></i>)."@en .

cim:UnderexcLimIEEE2.p7 a owl:DatatypeProperty ;
  rdfs:label "p7"@en ;
  rdfs:domain cim:UnderexcLimIEEE2 ;
  rdfs:range cim:PU ;
  skos:definition "Real power values for endpoints (<i>P</i><i><sub>7</sub></i>). "@en .

cim:UnderexcLimIEEE2.p8 a owl:DatatypeProperty ;
  rdfs:label "p8"@en ;
  rdfs:domain cim:UnderexcLimIEEE2 ;
  rdfs:range cim:PU ;
  skos:definition "Real power values for endpoints (<i>P</i><i><sub>8</sub></i>). "@en .

cim:UnderexcLimIEEE2.p9 a owl:DatatypeProperty ;
  rdfs:label "p9"@en ;
  rdfs:domain cim:UnderexcLimIEEE2 ;
  rdfs:range cim:PU ;
  skos:definition "Real power values for endpoints (<i>P</i><i><sub>9</sub></i>). "@en .

cim:UnderexcLimIEEE2.q0 a owl:DatatypeProperty ;
  rdfs:label "q0"@en ;
  rdfs:domain cim:UnderexcLimIEEE2 ;
  rdfs:range cim:PU ;
  skos:definition "Reactive power values for endpoints (<i>Q</i><i><sub>0</sub></i>).  Typical value = -0,31."@en .

cim:UnderexcLimIEEE2.q1 a owl:DatatypeProperty ;
  rdfs:label "q1"@en ;
  rdfs:domain cim:UnderexcLimIEEE2 ;
  rdfs:range cim:PU ;
  skos:definition "Reactive power values for endpoints (<i>Q</i><i><sub>1</sub></i>).  Typical value = -0,31."@en .

cim:UnderexcLimIEEE2.q10 a owl:DatatypeProperty ;
  rdfs:label "q10"@en ;
  rdfs:domain cim:UnderexcLimIEEE2 ;
  rdfs:range cim:PU ;
  skos:definition "Reactive power values for endpoints (<i>Q</i><i><sub>10</sub></i>). "@en .

cim:UnderexcLimIEEE2.q2 a owl:DatatypeProperty ;
  rdfs:label "q2"@en ;
  rdfs:domain cim:UnderexcLimIEEE2 ;
  rdfs:range cim:PU ;
  skos:definition "Reactive power values for endpoints (<i>Q</i><i><sub>2</sub></i>).  Typical value = -0,28."@en .

cim:UnderexcLimIEEE2.q3 a owl:DatatypeProperty ;
  rdfs:label "q3"@en ;
  rdfs:domain cim:UnderexcLimIEEE2 ;
  rdfs:range cim:PU ;
  skos:definition "Reactive power values for endpoints (<i>Q</i><i><sub>3</sub></i>).  Typical value = -0,21."@en .

cim:UnderexcLimIEEE2.q4 a owl:DatatypeProperty ;
  rdfs:label "q4"@en ;
  rdfs:domain cim:UnderexcLimIEEE2 ;
  rdfs:range cim:PU ;
  skos:definition "Reactive power values for endpoints (<i>Q</i><i><sub>4</sub></i>).  Typical value = 0."@en .

cim:UnderexcLimIEEE2.q5 a owl:DatatypeProperty ;
  rdfs:label "q5"@en ;
  rdfs:domain cim:UnderexcLimIEEE2 ;
  rdfs:range cim:PU ;
  skos:definition "Reactive power values for endpoints (<i>Q</i><i><sub>5</sub></i>). "@en .

cim:UnderexcLimIEEE2.q6 a owl:DatatypeProperty ;
  rdfs:label "q6"@en ;
  rdfs:domain cim:UnderexcLimIEEE2 ;
  rdfs:range cim:PU ;
  skos:definition "Reactive power values for endpoints (<i>Q</i><i><sub>6</sub></i>). "@en .

cim:UnderexcLimIEEE2.q7 a owl:DatatypeProperty ;
  rdfs:label "q7"@en ;
  rdfs:domain cim:UnderexcLimIEEE2 ;
  rdfs:range cim:PU ;
  skos:definition "Reactive power values for endpoints (<i>Q</i><i><sub>7</sub></i>). "@en .

cim:UnderexcLimIEEE2.q8 a owl:DatatypeProperty ;
  rdfs:label "q8"@en ;
  rdfs:domain cim:UnderexcLimIEEE2 ;
  rdfs:range cim:PU ;
  skos:definition "Reactive power values for endpoints (<i>Q</i><i><sub>8</sub></i>). "@en .

cim:UnderexcLimIEEE2.q9 a owl:DatatypeProperty ;
  rdfs:label "q9"@en ;
  rdfs:domain cim:UnderexcLimIEEE2 ;
  rdfs:range cim:PU ;
  skos:definition "Reactive power values for endpoints (<i>Q</i><i><sub>9</sub></i>). "@en .

cim:UnderexcLimIEEE2.tu1 a owl:DatatypeProperty ;
  rdfs:label "tu1"@en ;
  rdfs:domain cim:UnderexcLimIEEE2 ;
  rdfs:range cim:Seconds ;
  skos:definition "UEL lead time constant (<i>T</i><i><sub>U1</sub></i>) (&gt;= 0).  Typical value = 0."@en .

cim:UnderexcLimIEEE2.tu2 a owl:DatatypeProperty ;
  rdfs:label "tu2"@en ;
  rdfs:domain cim:UnderexcLimIEEE2 ;
  rdfs:range cim:Seconds ;
  skos:definition "UEL lag time constant (<i>T</i><i><sub>U2</sub></i>) (&gt;= 0).  Typical value = 0."@en .

cim:UnderexcLimIEEE2.tu3 a owl:DatatypeProperty ;
  rdfs:label "tu3"@en ;
  rdfs:domain cim:UnderexcLimIEEE2 ;
  rdfs:range cim:Seconds ;
  skos:definition "UEL lead time constant (<i>T</i><i><sub>U3</sub></i>) (&gt;= 0).  Typical value = 0."@en .

cim:UnderexcLimIEEE2.tu4 a owl:DatatypeProperty ;
  rdfs:label "tu4"@en ;
  rdfs:domain cim:UnderexcLimIEEE2 ;
  rdfs:range cim:Seconds ;
  skos:definition "UEL lag time constant (<i>T</i><i><sub>U4</sub></i>) (&gt;= 0).  Typical value = 0."@en .

cim:UnderexcLimIEEE2.tul a owl:DatatypeProperty ;
  rdfs:label "tul"@en ;
  rdfs:domain cim:UnderexcLimIEEE2 ;
  rdfs:range cim:Seconds ;
  skos:definition "Time constant associated with optional integrator feedback input signal to UEL (<i>T</i><i><sub>UL</sub></i>) (&gt;= 0).  Typical value = 0."@en .

cim:UnderexcLimIEEE2.tup a owl:DatatypeProperty ;
  rdfs:label "tup"@en ;
  rdfs:domain cim:UnderexcLimIEEE2 ;
  rdfs:range cim:Seconds ;
  skos:definition "Real power filter time constant (<i>T</i><i><sub>UP</sub></i>) (&gt;= 0).  Typical value = 5."@en .

cim:UnderexcLimIEEE2.tuq a owl:DatatypeProperty ;
  rdfs:label "tuq"@en ;
  rdfs:domain cim:UnderexcLimIEEE2 ;
  rdfs:range cim:Seconds ;
  skos:definition "Reactive power filter time constant (<i>T</i><i><sub>UQ</sub></i>) (&gt;= 0).  Typical value = 0."@en .

cim:UnderexcLimIEEE2.tuv a owl:DatatypeProperty ;
  rdfs:label "tuv"@en ;
  rdfs:domain cim:UnderexcLimIEEE2 ;
  rdfs:range cim:Seconds ;
  skos:definition "Voltage filter time constant (<i>T</i><i><sub>UV</sub></i>) (&gt;= 0).  Typical value = 5."@en .

cim:UnderexcLimIEEE2.vuimax a owl:DatatypeProperty ;
  rdfs:label "vuimax"@en ;
  rdfs:domain cim:UnderexcLimIEEE2 ;
  rdfs:range cim:PU ;
  skos:definition "UEL integrator output maximum limit (<i>V</i><i><sub>UIMAX</sub></i>) (&gt; UnderexcLimIEEE2.vuimin).  Typical value = 0,25."@en .

cim:UnderexcLimIEEE2.vuimin a owl:DatatypeProperty ;
  rdfs:label "vuimin"@en ;
  rdfs:domain cim:UnderexcLimIEEE2 ;
  rdfs:range cim:PU ;
  skos:definition "UEL integrator output minimum limit (<i>V</i><i><sub>UIMIN</sub></i>) (&lt; UnderexcLimIEEE2.vuimax).  Typical value = 0."@en .

cim:UnderexcLimIEEE2.vulmax a owl:DatatypeProperty ;
  rdfs:label "vulmax"@en ;
  rdfs:domain cim:UnderexcLimIEEE2 ;
  rdfs:range cim:PU ;
  skos:definition "UEL output maximum limit (<i>V</i><i><sub>ULMAX</sub></i>) (&gt; UnderexcLimIEEE2.vulmin).  Typical value = 0,25."@en .

cim:UnderexcLimIEEE2.vulmin a owl:DatatypeProperty ;
  rdfs:label "vulmin"@en ;
  rdfs:domain cim:UnderexcLimIEEE2 ;
  rdfs:range cim:PU ;
  skos:definition "UEL output minimum limit (<i>V</i><i><sub>ULMIN</sub></i>) (&lt; UnderexcLimIEEE2.vulmax).  Typical value = 0."@en .

cim:UnderexcLimX1.k a owl:DatatypeProperty ;
  rdfs:label "k"@en ;
  rdfs:domain cim:UnderexcLimX1 ;
  rdfs:range cim:PU ;
  skos:definition "Minimum excitation limit slope (<i>K</i>) (&gt; 0)."@en .

cim:UnderexcLimX1.kf2 a owl:DatatypeProperty ;
  rdfs:label "kf2"@en ;
  rdfs:domain cim:UnderexcLimX1 ;
  rdfs:range cim:PU ;
  skos:definition "Differential gain (<i>K</i><i><sub>F2</sub></i>)."@en .

cim:UnderexcLimX1.km a owl:DatatypeProperty ;
  rdfs:label "km"@en ;
  rdfs:domain cim:UnderexcLimX1 ;
  rdfs:range cim:PU ;
  skos:definition "Minimum excitation limit gain (<i>K</i><i><sub>M</sub></i>)."@en .

cim:UnderexcLimX1.melmax a owl:DatatypeProperty ;
  rdfs:label "melmax"@en ;
  rdfs:domain cim:UnderexcLimX1 ;
  rdfs:range cim:PU ;
  skos:definition "Minimum excitation limit value (<i>MELMAX</i>)."@en .

cim:UnderexcLimX1.tf2 a owl:DatatypeProperty ;
  rdfs:label "tf2"@en ;
  rdfs:domain cim:UnderexcLimX1 ;
  rdfs:range cim:Seconds ;
  skos:definition "Differential time constant (<i>T</i><i><sub>F2</sub></i>) (&gt;= 0)."@en .

cim:UnderexcLimX1.tm a owl:DatatypeProperty ;
  rdfs:label "tm"@en ;
  rdfs:domain cim:UnderexcLimX1 ;
  rdfs:range cim:Seconds ;
  skos:definition "Minimum excitation limit time constant (<i>T</i><i><sub>M</sub></i>) (&gt;= 0)."@en .

cim:UnderexcLimX2.kf2 a owl:DatatypeProperty ;
  rdfs:label "kf2"@en ;
  rdfs:domain cim:UnderexcLimX2 ;
  rdfs:range cim:PU ;
  skos:definition "Differential gain (<i>K</i><i><sub>F2</sub></i>)."@en .

cim:UnderexcLimX2.km a owl:DatatypeProperty ;
  rdfs:label "km"@en ;
  rdfs:domain cim:UnderexcLimX2 ;
  rdfs:range cim:PU ;
  skos:definition "Minimum excitation limit gain (<i>K</i><i><sub>M</sub></i>)."@en .

cim:UnderexcLimX2.melmax a owl:DatatypeProperty ;
  rdfs:label "melmax"@en ;
  rdfs:domain cim:UnderexcLimX2 ;
  rdfs:range cim:PU ;
  skos:definition "Minimum excitation limit value (<i>MELMAX</i>)."@en .

cim:UnderexcLimX2.qo a owl:DatatypeProperty ;
  rdfs:label "qo"@en ;
  rdfs:domain cim:UnderexcLimX2 ;
  rdfs:range cim:PU ;
  skos:definition "Excitation centre setting (<i>Q</i><i><sub>O</sub></i>)."@en .

cim:UnderexcLimX2.r a owl:DatatypeProperty ;
  rdfs:label "r"@en ;
  rdfs:domain cim:UnderexcLimX2 ;
  rdfs:range cim:PU ;
  skos:definition "Excitation radius (<i>R</i>)."@en .

cim:UnderexcLimX2.tf2 a owl:DatatypeProperty ;
  rdfs:label "tf2"@en ;
  rdfs:domain cim:UnderexcLimX2 ;
  rdfs:range cim:Seconds ;
  skos:definition "Differential time constant (<i>T</i><i><sub>F2</sub></i>) (&gt;= 0)."@en .

cim:UnderexcLimX2.tm a owl:DatatypeProperty ;
  rdfs:label "tm"@en ;
  rdfs:domain cim:UnderexcLimX2 ;
  rdfs:range cim:Seconds ;
  skos:definition "Minimum excitation limit time constant (<i>T</i><i><sub>M</sub></i>) (&gt;= 0)."@en .

cim:UnderexcitationLimiterUserDefined.proprietary a owl:DatatypeProperty ;
  rdfs:label "proprietary"@en ;
  rdfs:domain cim:UnderexcitationLimiterUserDefined ;
  rdfs:range xsd:boolean ;
  skos:definition """
Behaviour is based on a proprietary model as opposed to a detailed model.
true = user-defined model is proprietary with behaviour mutually understood by sending and receiving applications and parameters passed as general attributes
false = user-defined model is explicitly defined in terms of control blocks and their input and output signals.
\t"""@en .

cim:VAdjIEEE.adjslew a owl:DatatypeProperty ;
  rdfs:label "adjslew"@en ;
  rdfs:domain cim:VAdjIEEE ;
  rdfs:range xsd:float ;
  skos:definition "Rate at which output of adjuster changes (<i>ADJ_SLEW</i>).  Unit = s / PU.  Typical value = 300."@en .

cim:VAdjIEEE.taoff a owl:DatatypeProperty ;
  rdfs:label "taoff"@en ;
  rdfs:domain cim:VAdjIEEE ;
  rdfs:range cim:Seconds ;
  skos:definition "Time that adjuster pulses are off (<i>T</i><i><sub>AOFF</sub></i>) (&gt;= 0).  Typical value = 0,5."@en .

cim:VAdjIEEE.taon a owl:DatatypeProperty ;
  rdfs:label "taon"@en ;
  rdfs:domain cim:VAdjIEEE ;
  rdfs:range cim:Seconds ;
  skos:definition "Time that adjuster pulses are on (<i>T</i><i><sub>AON</sub></i>) (&gt;= 0).  Typical value = 0,1."@en .

cim:VAdjIEEE.vadjf a owl:DatatypeProperty ;
  rdfs:label "vadjf"@en ;
  rdfs:domain cim:VAdjIEEE ;
  rdfs:range xsd:float ;
  skos:definition "Set high to provide a continuous raise or lower (<i>V</i><i><sub>ADJF</sub></i>)."@en .

cim:VAdjIEEE.vadjmax a owl:DatatypeProperty ;
  rdfs:label "vadjmax"@en ;
  rdfs:domain cim:VAdjIEEE ;
  rdfs:range cim:PU ;
  skos:definition "Maximum output of the adjuster (<i>V</i><i><sub>ADJMAX</sub></i>) (&gt; VAdjIEEE.vadjmin).  Typical value = 1,1."@en .

cim:VAdjIEEE.vadjmin a owl:DatatypeProperty ;
  rdfs:label "vadjmin"@en ;
  rdfs:domain cim:VAdjIEEE ;
  rdfs:range cim:PU ;
  skos:definition "Minimum output of the adjuster (<i>V</i><i><sub>ADJMIN</sub></i>) (&lt; VAdjIEEE.vadjmax).  Typical value = 0,9."@en .

cim:VCompIEEEType1.rc a owl:DatatypeProperty ;
  rdfs:label "rc"@en ;
  rdfs:domain cim:VCompIEEEType1 ;
  rdfs:range cim:PU ;
  skos:definition "<font color=\"#0f0f0f\">Resistive component of compensation of a generator (<i>Rc</i>) (&gt;= 0).</font>"@en .

cim:VCompIEEEType1.tr a owl:DatatypeProperty ;
  rdfs:label "tr"@en ;
  rdfs:domain cim:VCompIEEEType1 ;
  rdfs:range cim:Seconds ;
  skos:definition "<font color=\"#0f0f0f\">Time constant which is used for the combined voltage sensing and compensation signal (<i>Tr</i>) (&gt;= 0).</font>"@en .

cim:VCompIEEEType1.xc a owl:DatatypeProperty ;
  rdfs:label "xc"@en ;
  rdfs:domain cim:VCompIEEEType1 ;
  rdfs:range cim:PU ;
  skos:definition "<font color=\"#0f0f0f\">Reactive component of compensation of a generator (<i>Xc</i>) (&gt;= 0).</font>"@en .

cim:VCompIEEEType2.tr a owl:DatatypeProperty ;
  rdfs:label "tr"@en ;
  rdfs:domain cim:VCompIEEEType2 ;
  rdfs:range cim:Seconds ;
  skos:definition "<font color=\"#0f0f0f\">Time constant which is used for the combined voltage sensing and compensation signal (<i>Tr</i>) (&gt;= 0).</font>"@en .

cim:VSCUserDefined.proprietary a owl:DatatypeProperty ;
  rdfs:label "proprietary"@en ;
  rdfs:domain cim:VSCUserDefined ;
  rdfs:range xsd:boolean ;
  skos:definition """
Behaviour is based on a proprietary model as opposed to a detailed model.
true = user-defined model is proprietary with behaviour mutually understood by sending and receiving applications and parameters passed as general attributes
false = user-defined model is explicitly defined in terms of control blocks and their input and output signals.
\t"""@en .

cim:VoltageAdjusterUserDefined.proprietary a owl:DatatypeProperty ;
  rdfs:label "proprietary"@en ;
  rdfs:domain cim:VoltageAdjusterUserDefined ;
  rdfs:range xsd:boolean ;
  skos:definition """
Behaviour is based on a proprietary model as opposed to a detailed model.
true = user-defined model is proprietary with behaviour mutually understood by sending and receiving applications and parameters passed as general attributes
false = user-defined model is explicitly defined in terms of control blocks and their input and output signals.
\t"""@en .

cim:VoltageCompensatorUserDefined.proprietary a owl:DatatypeProperty ;
  rdfs:label "proprietary"@en ;
  rdfs:domain cim:VoltageCompensatorUserDefined ;
  rdfs:range xsd:boolean ;
  skos:definition """
Behaviour is based on a proprietary model as opposed to a detailed model.
true = user-defined model is proprietary with behaviour mutually understood by sending and receiving applications and parameters passed as general attributes
false = user-defined model is explicitly defined in terms of control blocks and their input and output signals.
\t"""@en .

cim:VolumeFlowRate.multiplier a owl:DatatypeProperty, owl:FunctionalProperty ;
  rdfs:label "multiplier"@en ;
  dy:isFixed "True " ;
  rdf:value "none" ;
  rdfs:domain cim:VolumeFlowRate ;
  rdfs:range cim:UnitMultiplier .

cim:VolumeFlowRate.unit a owl:DatatypeProperty, owl:FunctionalProperty ;
  rdfs:label "unit"@en ;
  dy:isFixed "True " ;
  rdf:value "m3Pers" ;
  rdfs:domain cim:VolumeFlowRate ;
  rdfs:range cim:UnitSymbol .

cim:VolumeFlowRate.value a owl:DatatypeProperty, owl:FunctionalProperty ;
  rdfs:label "value"@en ;
  rdfs:domain cim:VolumeFlowRate ;
  rdfs:range xsd:float .

cim:WindAeroOneDimIEC.ka a owl:DatatypeProperty ;
  rdfs:label "ka"@en ;
  rdfs:domain cim:WindAeroOneDimIEC ;
  rdfs:range xsd:float ;
  skos:definition "Aerodynamic gain (<i>k</i><i><sub>a</sub></i>). It is a type-dependent parameter."@en .

cim:WindAeroOneDimIEC.thetaomega a owl:DatatypeProperty ;
  rdfs:label "thetaomega"@en ;
  rdfs:domain cim:WindAeroOneDimIEC ;
  rdfs:range cim:AngleDegrees ;
  skos:definition "Initial pitch angle (<i>theta</i><i><sub>omega0</sub></i>). It is a case-dependent parameter."@en .

cim:WindAeroTwoDimIEC.dpomega a owl:DatatypeProperty ;
  rdfs:label "dpomega"@en ;
  rdfs:domain cim:WindAeroTwoDimIEC ;
  rdfs:range cim:PU ;
  skos:definition "Partial derivative of aerodynamic power with respect to changes in WTR speed (<i>dp</i><i><sub>omega</sub></i>). It is a type-dependent parameter."@en .

cim:WindAeroTwoDimIEC.dptheta a owl:DatatypeProperty ;
  rdfs:label "dptheta"@en ;
  rdfs:domain cim:WindAeroTwoDimIEC ;
  rdfs:range cim:PU ;
  skos:definition "Partial derivative of aerodynamic power with respect to changes in pitch angle (<i>dp</i><i><sub>theta</sub></i>). It is a type-dependent parameter."@en .

cim:WindAeroTwoDimIEC.dpv1 a owl:DatatypeProperty ;
  rdfs:label "dpv1"@en ;
  rdfs:domain cim:WindAeroTwoDimIEC ;
  rdfs:range cim:PU ;
  skos:definition "Partial derivative (<i>dp</i><i><sub>v1</sub></i>). It is a type-dependent parameter."@en .

cim:WindAeroTwoDimIEC.omegazero a owl:DatatypeProperty ;
  rdfs:label "omegazero"@en ;
  rdfs:domain cim:WindAeroTwoDimIEC ;
  rdfs:range cim:PU ;
  skos:definition "Rotor speed if the wind turbine is not derated (<i>omega</i><i><sub>0</sub></i>). It is a type-dependent parameter."@en .

cim:WindAeroTwoDimIEC.pavail a owl:DatatypeProperty ;
  rdfs:label "pavail"@en ;
  rdfs:domain cim:WindAeroTwoDimIEC ;
  rdfs:range cim:PU ;
  skos:definition "Available aerodynamic power (<i>p</i><i><sub>avail</sub></i><i>)</i>. It is a case-dependent parameter."@en .

cim:WindAeroTwoDimIEC.thetav2 a owl:DatatypeProperty ;
  rdfs:label "thetav2"@en ;
  rdfs:domain cim:WindAeroTwoDimIEC ;
  rdfs:range cim:AngleDegrees ;
  skos:definition "Blade angle at twice rated wind speed (<i>theta</i><i><sub>v2</sub></i>). It is a type-dependent parameter."@en .

cim:WindAeroTwoDimIEC.thetazero a owl:DatatypeProperty ;
  rdfs:label "thetazero"@en ;
  rdfs:domain cim:WindAeroTwoDimIEC ;
  rdfs:range cim:AngleDegrees ;
  skos:definition "Pitch angle if the wind turbine is not derated (<i>theta</i><i><sub>0</sub></i>). It is a case-dependent parameter."@en .

cim:WindContCurrLimIEC.imax a owl:DatatypeProperty ;
  rdfs:label "imax"@en ;
  rdfs:domain cim:WindContCurrLimIEC ;
  rdfs:range cim:PU ;
  skos:definition "Maximum continuous current at the wind turbine terminals (<i>i</i><i><sub>max</sub></i>). It is a type-dependent parameter."@en .

cim:WindContCurrLimIEC.imaxdip a owl:DatatypeProperty ;
  rdfs:label "imaxdip"@en ;
  rdfs:domain cim:WindContCurrLimIEC ;
  rdfs:range cim:PU ;
  skos:definition "Maximum current during voltage dip at the wind turbine terminals (<i>i</i><i><sub>maxdip</sub></i>). It is a project-dependent parameter."@en .

cim:WindContCurrLimIEC.kpqu a owl:DatatypeProperty ;
  rdfs:label "kpqu"@en ;
  rdfs:domain cim:WindContCurrLimIEC ;
  rdfs:range cim:PU ;
  skos:definition "Partial derivative of reactive current limit (<i>K</i><i><sub>pqu</sub></i>) versus voltage. It is a type-dependent parameter."@en .

cim:WindContCurrLimIEC.mdfslim a owl:DatatypeProperty ;
  rdfs:label "mdfslim"@en ;
  rdfs:domain cim:WindContCurrLimIEC ;
  rdfs:range xsd:boolean ;
  skos:definition """
Limitation of type 3 stator current (<i>M</i><i><sub>DFSLim</sub></i>). <i>M</i><i><sub>DFSLim</sub></i><sub> </sub>= 1 for wind turbines type 4. It is a type-dependent parameter.
false= total current limitation (0 in the IEC model)
true=stator current limitation (1 in the IEC model).

\t"""@en .

cim:WindContCurrLimIEC.mqpri a owl:DatatypeProperty ;
  rdfs:label "mqpri"@en ;
  rdfs:domain cim:WindContCurrLimIEC ;
  rdfs:range xsd:boolean ;
  skos:definition """
Prioritisation of Q control during UVRT (<i>M</i><i><sub>qpri</sub></i>). It is a project-dependent parameter.
true = reactive power priority (1 in the IEC model)
false = active power priority (0 in the IEC model).
\t"""@en .

cim:WindContCurrLimIEC.tufiltcl a owl:DatatypeProperty ;
  rdfs:label "tufiltcl"@en ;
  rdfs:domain cim:WindContCurrLimIEC ;
  rdfs:range cim:Seconds ;
  skos:definition "Voltage measurement filter time constant (<i>T</i><i><sub>ufiltcl</sub></i>) (&gt;= 0). It is a type-dependent parameter."@en .

cim:WindContCurrLimIEC.upqumax a owl:DatatypeProperty ;
  rdfs:label "upqumax"@en ;
  rdfs:domain cim:WindContCurrLimIEC ;
  rdfs:range cim:PU ;
  skos:definition "Wind turbine voltage in the operation point where zero reactive current can be delivered (<i>u</i><i><sub>pqumax</sub></i>). It is a type-dependent parameter."@en .

cim:WindContPType3IEC.dpmax a owl:DatatypeProperty ;
  rdfs:label "dpmax"@en ;
  rdfs:domain cim:WindContPType3IEC ;
  rdfs:range cim:PU ;
  skos:definition "Maximum wind turbine power ramp rate (<i>dp</i><i><sub>max</sub></i>). It is a type-dependent parameter."@en .

cim:WindContPType3IEC.dprefmax a owl:DatatypeProperty ;
  rdfs:label "dprefmax"@en ;
  rdfs:domain cim:WindContPType3IEC ;
  rdfs:range cim:PU ;
  skos:definition "Maximum ramp rate of wind turbine reference power (<i>dp</i><i><sub>refmax</sub></i>). It is a project-dependent parameter."@en .

cim:WindContPType3IEC.dprefmin a owl:DatatypeProperty ;
  rdfs:label "dprefmin"@en ;
  rdfs:domain cim:WindContPType3IEC ;
  rdfs:range cim:PU ;
  skos:definition "Minimum ramp rate of wind turbine reference power (<i>dp</i><i><sub>refmin</sub></i>). It is a project-dependent parameter."@en .

cim:WindContPType3IEC.dthetamax a owl:DatatypeProperty ;
  rdfs:label "dthetamax"@en ;
  rdfs:domain cim:WindContPType3IEC ;
  rdfs:range cim:PU ;
  skos:definition "Ramp limitation of torque, required in some grid codes (<i>dt</i><i><sub>max</sub></i>). It is a project-dependent parameter."@en .

cim:WindContPType3IEC.dthetamaxuvrt a owl:DatatypeProperty ;
  rdfs:label "dthetamaxuvrt"@en ;
  rdfs:domain cim:WindContPType3IEC ;
  rdfs:range cim:PU ;
  skos:definition "Limitation of torque rise rate during UVRT (<i>dtheta</i><i><sub>maxUVRT</sub></i>). It is a project-dependent parameter."@en .

cim:WindContPType3IEC.kdtd a owl:DatatypeProperty ;
  rdfs:label "kdtd"@en ;
  rdfs:domain cim:WindContPType3IEC ;
  rdfs:range cim:PU ;
  skos:definition "Gain for active drive train damping (<i>K</i><i><sub>DTD</sub></i>). It is a type-dependent parameter."@en .

cim:WindContPType3IEC.kip a owl:DatatypeProperty ;
  rdfs:label "kip"@en ;
  rdfs:domain cim:WindContPType3IEC ;
  rdfs:range cim:PU ;
  skos:definition "PI controller integration parameter (<i>K</i><sub>Ip</sub>). It is a type-dependent parameter."@en .

cim:WindContPType3IEC.kpp a owl:DatatypeProperty ;
  rdfs:label "kpp"@en ;
  rdfs:domain cim:WindContPType3IEC ;
  rdfs:range cim:PU ;
  skos:definition "PI controller proportional gain (<i>K</i><sub>Pp</sub>). It is a type-dependent parameter."@en .

cim:WindContPType3IEC.mpuvrt a owl:DatatypeProperty ;
  rdfs:label "mpuvrt"@en ;
  rdfs:domain cim:WindContPType3IEC ;
  rdfs:range xsd:boolean ;
  skos:definition """
Enable UVRT power control mode (<i>M</i><i><sub>pUVRT</sub></i><sub>)</sub>.  It is a project-dependent parameter.
true = voltage control (1 in the IEC model)
false = reactive power control (0 in the IEC model).

\t"""@en .

cim:WindContPType3IEC.omegadtd a owl:DatatypeProperty ;
  rdfs:label "omegadtd"@en ;
  rdfs:domain cim:WindContPType3IEC ;
  rdfs:range cim:PU ;
  skos:definition "Active drive train damping frequency (<i>omega</i><i><sub>DTD</sub></i>). It can be calculated from two mass model parameters. It is a type-dependent parameter."@en .

cim:WindContPType3IEC.omegaoffset a owl:DatatypeProperty ;
  rdfs:label "omegaoffset"@en ;
  rdfs:domain cim:WindContPType3IEC ;
  rdfs:range cim:PU ;
  skos:definition "Offset to reference value that limits controller action during rotor speed changes (<i>omega</i><i><sub>offset</sub></i>). It is a case-dependent parameter."@en .

cim:WindContPType3IEC.pdtdmax a owl:DatatypeProperty ;
  rdfs:label "pdtdmax"@en ;
  rdfs:domain cim:WindContPType3IEC ;
  rdfs:range cim:PU ;
  skos:definition "Maximum active drive train damping power (<i>p</i><sub>DTDmax</sub>). It is a type-dependent parameter."@en .

cim:WindContPType3IEC.tdvs a owl:DatatypeProperty ;
  rdfs:label "tdvs"@en ;
  rdfs:domain cim:WindContPType3IEC ;
  rdfs:range cim:Seconds ;
  skos:definition "Time<sub> </sub>delay after deep voltage sags (<i>T</i><i><sub>DVS</sub></i>) (&gt;= 0). It is a project-dependent parameter."@en .

cim:WindContPType3IEC.thetaemin a owl:DatatypeProperty ;
  rdfs:label "thetaemin"@en ;
  rdfs:domain cim:WindContPType3IEC ;
  rdfs:range cim:PU ;
  skos:definition "Minimum electrical generator torque (<i>t</i><sub>emin</sub>). It is a type-dependent parameter."@en .

cim:WindContPType3IEC.thetauscale a owl:DatatypeProperty ;
  rdfs:label "thetauscale"@en ;
  rdfs:domain cim:WindContPType3IEC ;
  rdfs:range cim:PU ;
  skos:definition "Voltage scaling factor of reset-torque (<i>t</i><sub>uscale</sub>). It is a project-dependent parameter."@en .

cim:WindContPType3IEC.tomegafiltp3 a owl:DatatypeProperty ;
  rdfs:label "tomegafiltp3"@en ;
  rdfs:domain cim:WindContPType3IEC ;
  rdfs:range cim:Seconds ;
  skos:definition "Filter time constant for generator speed measurement (<i>T</i><sub>omegafiltp3</sub>) (&gt;= 0). It is a type-dependent parameter."@en .

cim:WindContPType3IEC.tomegaref a owl:DatatypeProperty ;
  rdfs:label "tomegaref"@en ;
  rdfs:domain cim:WindContPType3IEC ;
  rdfs:range cim:Seconds ;
  skos:definition "Time constant in speed reference filter (<i>T</i><sub>omega,ref</sub>) (&gt;= 0). It is a type-dependent parameter."@en .

cim:WindContPType3IEC.tpfiltp3 a owl:DatatypeProperty ;
  rdfs:label "tpfiltp3"@en ;
  rdfs:domain cim:WindContPType3IEC ;
  rdfs:range cim:Seconds ;
  skos:definition "Filter time constant for power measurement (<i>T</i><sub>pfiltp3</sub>) (&gt;= 0). It is a type-dependent parameter."@en .

cim:WindContPType3IEC.tpord a owl:DatatypeProperty ;
  rdfs:label "tpord"@en ;
  rdfs:domain cim:WindContPType3IEC ;
  rdfs:range cim:PU ;
  skos:definition "Time constant in power order lag (<i>T</i><sub>pord</sub>). It is a type-dependent parameter."@en .

cim:WindContPType3IEC.tufiltp3 a owl:DatatypeProperty ;
  rdfs:label "tufiltp3"@en ;
  rdfs:domain cim:WindContPType3IEC ;
  rdfs:range cim:Seconds ;
  skos:definition "Filter time constant for voltage measurement (<i>T</i><sub>ufiltp3</sub>) (&gt;= 0). It is a type-dependent parameter."@en .

cim:WindContPType3IEC.udvs a owl:DatatypeProperty ;
  rdfs:label "udvs"@en ;
  rdfs:domain cim:WindContPType3IEC ;
  rdfs:range cim:PU ;
  skos:definition "Voltage limit for hold UVRT status after deep voltage sags (<i>u</i><i><sub>DVS</sub></i>). It is a project-dependent parameter."@en .

cim:WindContPType3IEC.updip a owl:DatatypeProperty ;
  rdfs:label "updip"@en ;
  rdfs:domain cim:WindContPType3IEC ;
  rdfs:range cim:PU ;
  skos:definition "Voltage dip threshold for P-control (<i>u</i><sub>Pdip</sub>).  Part of turbine control, often different (e.g 0.8) from converter thresholds. It is a project-dependent parameter."@en .

cim:WindContPType3IEC.zeta a owl:DatatypeProperty ;
  rdfs:label "zeta"@en ;
  rdfs:domain cim:WindContPType3IEC ;
  rdfs:range xsd:float ;
  skos:definition "Coefficient for active drive train damping (<i>zeta</i>). It is a type-dependent parameter."@en .

cim:WindContPType4aIEC.dpmaxp4a a owl:DatatypeProperty ;
  rdfs:label "dpmaxp4a"@en ;
  rdfs:domain cim:WindContPType4aIEC ;
  rdfs:range cim:PU ;
  skos:definition "Maximum wind turbine power ramp rate (<i>dp</i><i><sub>maxp4A</sub></i>). It is a project-dependent parameter."@en .

cim:WindContPType4aIEC.tpordp4a a owl:DatatypeProperty ;
  rdfs:label "tpordp4a"@en ;
  rdfs:domain cim:WindContPType4aIEC ;
  rdfs:range cim:Seconds ;
  skos:definition "Time constant in power order lag (<i>T</i><i><sub>pordp4A</sub></i>) (&gt;= 0). It is a type-dependent parameter."@en .

cim:WindContPType4aIEC.tufiltp4a a owl:DatatypeProperty ;
  rdfs:label "tufiltp4a"@en ;
  rdfs:domain cim:WindContPType4aIEC ;
  rdfs:range cim:Seconds ;
  skos:definition "Voltage measurement filter time constant (<i>T</i><i><sub>ufiltp4A</sub></i>) (&gt;= 0). It is a type-dependent parameter."@en .

cim:WindContPType4bIEC.dpmaxp4b a owl:DatatypeProperty ;
  rdfs:label "dpmaxp4b"@en ;
  rdfs:domain cim:WindContPType4bIEC ;
  rdfs:range cim:PU ;
  skos:definition "Maximum wind turbine power ramp rate (<i>dp</i><i><sub>maxp4B</sub></i>). It is a project-dependent parameter."@en .

cim:WindContPType4bIEC.tpaero a owl:DatatypeProperty ;
  rdfs:label "tpaero"@en ;
  rdfs:domain cim:WindContPType4bIEC ;
  rdfs:range cim:Seconds ;
  skos:definition "Time constant in aerodynamic power response (<i>T</i><i><sub>paero</sub></i>) (&gt;= 0). It is a type-dependent parameter."@en .

cim:WindContPType4bIEC.tpordp4b a owl:DatatypeProperty ;
  rdfs:label "tpordp4b"@en ;
  rdfs:domain cim:WindContPType4bIEC ;
  rdfs:range cim:Seconds ;
  skos:definition "Time constant in power order lag (<i>T</i><i><sub>pordp4B</sub></i>) (&gt;= 0). It is a type-dependent parameter."@en .

cim:WindContPType4bIEC.tufiltp4b a owl:DatatypeProperty ;
  rdfs:label "tufiltp4b"@en ;
  rdfs:domain cim:WindContPType4bIEC ;
  rdfs:range cim:Seconds ;
  skos:definition "Voltage measurement filter time constant (<i>T</i><i><sub>ufiltp4B</sub></i>) (&gt;= 0). It is a type-dependent parameter."@en .

cim:WindContPitchAngleIEC.dthetamax a owl:DatatypeProperty ;
  rdfs:label "dthetamax"@en ;
  rdfs:domain cim:WindContPitchAngleIEC ;
  rdfs:range xsd:float ;
  skos:definition "Maximum pitch positive ramp rate (<i>dtheta</i><i><sub>max</sub></i>) (&gt; WindContPitchAngleIEC.dthetamin). It is a type-dependent parameter. Unit = degrees / s. "@en .

cim:WindContPitchAngleIEC.dthetamin a owl:DatatypeProperty ;
  rdfs:label "dthetamin"@en ;
  rdfs:domain cim:WindContPitchAngleIEC ;
  rdfs:range xsd:float ;
  skos:definition "Maximum pitch negative ramp rate (<i>dtheta</i><i><sub>min</sub></i><i>)</i> (&lt; WindContPitchAngleIEC.dthetamax). It is a type-dependent parameter. Unit = degrees / s. "@en .

cim:WindContPitchAngleIEC.kic a owl:DatatypeProperty ;
  rdfs:label "kic"@en ;
  rdfs:domain cim:WindContPitchAngleIEC ;
  rdfs:range cim:PU ;
  skos:definition "Power PI controller integration gain (<i>K</i><i><sub>Ic</sub></i>). It is a type-dependent parameter."@en .

cim:WindContPitchAngleIEC.kiomega a owl:DatatypeProperty ;
  rdfs:label "kiomega"@en ;
  rdfs:domain cim:WindContPitchAngleIEC ;
  rdfs:range cim:PU ;
  skos:definition "Speed PI controller integration gain (<i>K</i><i><sub>Iomega</sub></i>). It is a type-dependent parameter."@en .

cim:WindContPitchAngleIEC.kpc a owl:DatatypeProperty ;
  rdfs:label "kpc"@en ;
  rdfs:domain cim:WindContPitchAngleIEC ;
  rdfs:range cim:PU ;
  skos:definition "Power PI controller proportional gain (<i>K</i><i><sub>Pc</sub></i>). It is a type-dependent parameter."@en .

cim:WindContPitchAngleIEC.kpomega a owl:DatatypeProperty ;
  rdfs:label "kpomega"@en ;
  rdfs:domain cim:WindContPitchAngleIEC ;
  rdfs:range cim:PU ;
  skos:definition "Speed PI controller proportional gain (<i>K</i><i><sub>Pomega</sub></i>). It is a type-dependent parameter."@en .

cim:WindContPitchAngleIEC.kpx a owl:DatatypeProperty ;
  rdfs:label "kpx"@en ;
  rdfs:domain cim:WindContPitchAngleIEC ;
  rdfs:range cim:PU ;
  skos:definition "Pitch cross coupling gain (<i>K</i><i><sub>PX</sub></i>). It is a type-dependent parameter."@en .

cim:WindContPitchAngleIEC.thetamax a owl:DatatypeProperty ;
  rdfs:label "thetamax"@en ;
  rdfs:domain cim:WindContPitchAngleIEC ;
  rdfs:range cim:AngleDegrees ;
  skos:definition "Maximum pitch angle (<i>theta</i><i><sub>max</sub></i>) (&gt; WindContPitchAngleIEC.thetamin). It is a type-dependent parameter."@en .

cim:WindContPitchAngleIEC.thetamin a owl:DatatypeProperty ;
  rdfs:label "thetamin"@en ;
  rdfs:domain cim:WindContPitchAngleIEC ;
  rdfs:range cim:AngleDegrees ;
  skos:definition "Minimum pitch angle (<i>theta</i><i><sub>min</sub></i>) (&lt; WindContPitchAngleIEC.thetamax). It is a type-dependent parameter."@en .

cim:WindContPitchAngleIEC.ttheta a owl:DatatypeProperty ;
  rdfs:label "ttheta"@en ;
  rdfs:domain cim:WindContPitchAngleIEC ;
  rdfs:range cim:Seconds ;
  skos:definition "Pitch time constant (<i>ttheta</i>) (&gt;= 0). It is a type-dependent parameter."@en .

cim:WindContQIEC.iqh1 a owl:DatatypeProperty ;
  rdfs:label "iqh1"@en ;
  rdfs:domain cim:WindContQIEC ;
  rdfs:range cim:PU ;
  skos:definition "Maximum reactive current injection during dip (<i>i</i><i><sub>qh1</sub></i>). It is a type-dependent parameter."@en .

cim:WindContQIEC.iqmax a owl:DatatypeProperty ;
  rdfs:label "iqmax"@en ;
  rdfs:domain cim:WindContQIEC ;
  rdfs:range cim:PU ;
  skos:definition "Maximum reactive current injection (<i>i</i><i><sub>qmax</sub></i>) (&gt; WindContQIEC.iqmin). It is a type-dependent parameter."@en .

cim:WindContQIEC.iqmin a owl:DatatypeProperty ;
  rdfs:label "iqmin"@en ;
  rdfs:domain cim:WindContQIEC ;
  rdfs:range cim:PU ;
  skos:definition "Minimum reactive current injection (<i>i</i><i><sub>qmin</sub></i>) (&lt; WindContQIEC.iqmax). It is a type-dependent parameter."@en .

cim:WindContQIEC.iqpost a owl:DatatypeProperty ;
  rdfs:label "iqpost"@en ;
  rdfs:domain cim:WindContQIEC ;
  rdfs:range cim:PU ;
  skos:definition "Post fault reactive current injection (<i>i</i><i><sub>qpost</sub></i>). It is a project-dependent parameter."@en .

cim:WindContQIEC.kiq a owl:DatatypeProperty ;
  rdfs:label "kiq"@en ;
  rdfs:domain cim:WindContQIEC ;
  rdfs:range cim:PU ;
  skos:definition "Reactive power PI controller integration gain (<i>K</i><i><sub>I,q</sub></i>). It is a type-dependent parameter."@en .

cim:WindContQIEC.kiu a owl:DatatypeProperty ;
  rdfs:label "kiu"@en ;
  rdfs:domain cim:WindContQIEC ;
  rdfs:range cim:PU ;
  skos:definition "Voltage PI controller integration gain (<i>K</i><i><sub>I,u</sub></i>). It is a type-dependent parameter."@en .

cim:WindContQIEC.kpq a owl:DatatypeProperty ;
  rdfs:label "kpq"@en ;
  rdfs:domain cim:WindContQIEC ;
  rdfs:range cim:PU ;
  skos:definition "Reactive power PI controller proportional gain (<i>K</i><i><sub>P,q</sub></i>). It is a type-dependent parameter."@en .

cim:WindContQIEC.kpu a owl:DatatypeProperty ;
  rdfs:label "kpu"@en ;
  rdfs:domain cim:WindContQIEC ;
  rdfs:range cim:PU ;
  skos:definition "Voltage PI controller proportional gain (<i>K</i><i><sub>P,u</sub></i>). It is a type-dependent parameter."@en .

cim:WindContQIEC.kqv a owl:DatatypeProperty ;
  rdfs:label "kqv"@en ;
  rdfs:domain cim:WindContQIEC ;
  rdfs:range cim:PU ;
  skos:definition "Voltage scaling factor for UVRT current (<i>K</i><i><sub>qv</sub></i>). It is a project-dependent parameter."@en .

cim:WindContQIEC.rdroop a owl:DatatypeProperty ;
  rdfs:label "rdroop"@en ;
  rdfs:domain cim:WindContQIEC ;
  rdfs:range cim:PU ;
  skos:definition "Resistive component of voltage drop impedance (<i>r</i><i><sub>droop</sub></i>) (&gt;= 0). It is a project-dependent parameter."@en .

cim:WindContQIEC.tpfiltq a owl:DatatypeProperty ;
  rdfs:label "tpfiltq"@en ;
  rdfs:domain cim:WindContQIEC ;
  rdfs:range cim:Seconds ;
  skos:definition "Power measurement filter time constant (<i>T</i><i><sub>pfiltq</sub></i>) (&gt;= 0). It is a type-dependent parameter."@en .

cim:WindContQIEC.tpost a owl:DatatypeProperty ;
  rdfs:label "tpost"@en ;
  rdfs:domain cim:WindContQIEC ;
  rdfs:range cim:Seconds ;
  skos:definition "Length of time period where post fault reactive power is injected (<i>T</i><i><sub>post</sub></i>) (&gt;= 0). It is a project-dependent parameter."@en .

cim:WindContQIEC.tqord a owl:DatatypeProperty ;
  rdfs:label "tqord"@en ;
  rdfs:domain cim:WindContQIEC ;
  rdfs:range cim:Seconds ;
  skos:definition "Time constant in reactive power order lag (<i>T</i><i><sub>qord</sub></i>) (&gt;= 0). It is a type-dependent parameter."@en .

cim:WindContQIEC.tufiltq a owl:DatatypeProperty ;
  rdfs:label "tufiltq"@en ;
  rdfs:domain cim:WindContQIEC ;
  rdfs:range cim:Seconds ;
  skos:definition "Voltage measurement filter time constant (<i>T</i><i><sub>ufiltq</sub></i>) (&gt;= 0). It is a type-dependent parameter."@en .

cim:WindContQIEC.udb1 a owl:DatatypeProperty ;
  rdfs:label "udb1"@en ;
  rdfs:domain cim:WindContQIEC ;
  rdfs:range cim:PU ;
  skos:definition "Voltage deadband lower limit (<i>u</i><i><sub>db1</sub></i>). It is a type-dependent parameter."@en .

cim:WindContQIEC.udb2 a owl:DatatypeProperty ;
  rdfs:label "udb2"@en ;
  rdfs:domain cim:WindContQIEC ;
  rdfs:range cim:PU ;
  skos:definition "Voltage deadband upper limit (<i>u</i><i><sub>db2</sub></i>). It is a type-dependent parameter."@en .

cim:WindContQIEC.umax a owl:DatatypeProperty ;
  rdfs:label "umax"@en ;
  rdfs:domain cim:WindContQIEC ;
  rdfs:range cim:PU ;
  skos:definition "Maximum voltage in voltage PI controller integral term (<i>u</i><i><sub>max</sub></i>) (&gt; WindContQIEC.umin). It is a type-dependent parameter."@en .

cim:WindContQIEC.umin a owl:DatatypeProperty ;
  rdfs:label "umin"@en ;
  rdfs:domain cim:WindContQIEC ;
  rdfs:range cim:PU ;
  skos:definition "Minimum voltage in voltage PI controller integral term (<i>u</i><i><sub>min</sub></i>) (&lt; WindContQIEC.umax). It is a type-dependent parameter."@en .

cim:WindContQIEC.uqdip a owl:DatatypeProperty ;
  rdfs:label "uqdip"@en ;
  rdfs:domain cim:WindContQIEC ;
  rdfs:range cim:PU ;
  skos:definition "Voltage threshold for UVRT detection in Q control (<i>u</i><i><sub>qdip</sub></i>). It is a type-dependent parameter."@en .

cim:WindContQIEC.uref0 a owl:DatatypeProperty ;
  rdfs:label "uref0"@en ;
  rdfs:domain cim:WindContQIEC ;
  rdfs:range cim:PU ;
  skos:definition "User-defined bias in voltage reference (<i>u</i><i><sub>ref0</sub></i>). It is a case-dependent parameter."@en .

cim:WindContQIEC.windQcontrolModesType a owl:DatatypeProperty ;
  rdfs:label "windQcontrolModesType"@en ;
  rdfs:domain cim:WindContQIEC ;
  rdfs:range cim:WindQcontrolModeKind ;
  skos:definition "Types of general wind turbine Q control modes (<i>M</i><i><sub>qG</sub></i>).  It is a project-dependent parameter."@en .

cim:WindContQIEC.windUVRTQcontrolModesType a owl:DatatypeProperty ;
  rdfs:label "windUVRTQcontrolModesType"@en ;
  rdfs:domain cim:WindContQIEC ;
  rdfs:range cim:WindUVRTQcontrolModeKind ;
  skos:definition "Types of UVRT Q control modes (<i>M</i><i><sub>qUVRT</sub></i>). It is a project-dependent parameter."@en .

cim:WindContQIEC.xdroop a owl:DatatypeProperty ;
  rdfs:label "xdroop"@en ;
  rdfs:domain cim:WindContQIEC ;
  rdfs:range cim:PU ;
  skos:definition "Inductive component of voltage drop impedance (<i>x</i><i><sub>droop</sub></i>) (&gt;= 0). It is a project-dependent parameter."@en .

cim:WindContQLimIEC.qmax a owl:DatatypeProperty ;
  rdfs:label "qmax"@en ;
  rdfs:domain cim:WindContQLimIEC ;
  rdfs:range cim:PU ;
  skos:definition "Maximum reactive power (<i>q</i><i><sub>max</sub></i>) (&gt; WindContQLimIEC.qmin). It is a type-dependent parameter."@en .

cim:WindContQLimIEC.qmin a owl:DatatypeProperty ;
  rdfs:label "qmin"@en ;
  rdfs:domain cim:WindContQLimIEC ;
  rdfs:range cim:PU ;
  skos:definition "Minimum reactive power (<i>q</i><i><sub>min</sub></i>) (&lt; WindContQLimIEC.qmax). It is a type-dependent parameter."@en .

cim:WindContQPQULimIEC.tpfiltql a owl:DatatypeProperty ;
  rdfs:label "tpfiltql"@en ;
  rdfs:domain cim:WindContQPQULimIEC ;
  rdfs:range cim:Seconds ;
  skos:definition "Power measurement filter time constant for Q capacity (<i>T</i><i><sub>pfiltql</sub></i>) (&gt;= 0). It is a type-dependent parameter."@en .

cim:WindContQPQULimIEC.tufiltql a owl:DatatypeProperty ;
  rdfs:label "tufiltql"@en ;
  rdfs:domain cim:WindContQPQULimIEC ;
  rdfs:range cim:Seconds ;
  skos:definition "Voltage measurement filter time constant for Q capacity (<i>T</i><i><sub>ufiltql</sub></i>) (&gt;= 0). It is a type-dependent parameter."@en .

cim:WindContRotorRIEC.kirr a owl:DatatypeProperty ;
  rdfs:label "kirr"@en ;
  rdfs:domain cim:WindContRotorRIEC ;
  rdfs:range cim:PU ;
  skos:definition "Integral gain in rotor resistance PI controller (<i>K</i><i><sub>Irr</sub></i>). It is a type-dependent parameter."@en .

cim:WindContRotorRIEC.komegafilt a owl:DatatypeProperty ;
  rdfs:label "komegafilt"@en ;
  rdfs:domain cim:WindContRotorRIEC ;
  rdfs:range xsd:float ;
  skos:definition "Filter gain for generator speed measurement (<i>K</i><i><sub>omegafilt</sub></i>). It is a type-dependent parameter."@en .

cim:WindContRotorRIEC.kpfilt a owl:DatatypeProperty ;
  rdfs:label "kpfilt"@en ;
  rdfs:domain cim:WindContRotorRIEC ;
  rdfs:range xsd:float ;
  skos:definition "Filter gain for power measurement (<i>K</i><i><sub>pfilt</sub></i>). It is a type-dependent parameter."@en .

cim:WindContRotorRIEC.kprr a owl:DatatypeProperty ;
  rdfs:label "kprr"@en ;
  rdfs:domain cim:WindContRotorRIEC ;
  rdfs:range cim:PU ;
  skos:definition "Proportional gain in rotor resistance PI controller (<i>K</i><i><sub>Prr</sub></i>). It is a type-dependent parameter."@en .

cim:WindContRotorRIEC.rmax a owl:DatatypeProperty ;
  rdfs:label "rmax"@en ;
  rdfs:domain cim:WindContRotorRIEC ;
  rdfs:range cim:PU ;
  skos:definition "Maximum rotor resistance (<i>r</i><i><sub>max</sub></i>) (&gt; WindContRotorRIEC.rmin). It is a type-dependent parameter."@en .

cim:WindContRotorRIEC.rmin a owl:DatatypeProperty ;
  rdfs:label "rmin"@en ;
  rdfs:domain cim:WindContRotorRIEC ;
  rdfs:range cim:PU ;
  skos:definition "Minimum rotor resistance (<i>r</i><i><sub>min</sub></i>) (&lt; WindContRotorRIEC.rmax). It is a type-dependent parameter."@en .

cim:WindContRotorRIEC.tomegafiltrr a owl:DatatypeProperty ;
  rdfs:label "tomegafiltrr"@en ;
  rdfs:domain cim:WindContRotorRIEC ;
  rdfs:range cim:Seconds ;
  skos:definition "Filter time constant for generator speed measurement (<i>T</i><i><sub>omegafiltrr</sub></i>) (&gt;= 0). It is a type-dependent parameter."@en .

cim:WindContRotorRIEC.tpfiltrr a owl:DatatypeProperty ;
  rdfs:label "tpfiltrr"@en ;
  rdfs:domain cim:WindContRotorRIEC ;
  rdfs:range cim:Seconds ;
  skos:definition "Filter time constant for power measurement (<i>T</i><i><sub>pfiltrr</sub></i>) (&gt;= 0). It is a type-dependent parameter."@en .

cim:WindDynamicsLookupTable.input a owl:DatatypeProperty ;
  rdfs:label "input"@en ;
  rdfs:domain cim:WindDynamicsLookupTable ;
  rdfs:range xsd:float ;
  skos:definition "Input value (<i>x</i>) for the lookup table function."@en .

cim:WindDynamicsLookupTable.lookupTableFunctionType a owl:DatatypeProperty ;
  rdfs:label "lookupTableFunctionType"@en ;
  rdfs:domain cim:WindDynamicsLookupTable ;
  rdfs:range cim:WindLookupTableFunctionKind ;
  skos:definition "Type of the lookup table function."@en .

cim:WindDynamicsLookupTable.output a owl:DatatypeProperty ;
  rdfs:label "output"@en ;
  rdfs:domain cim:WindDynamicsLookupTable ;
  rdfs:range xsd:float ;
  skos:definition "Output value (<i>y</i>) for the lookup table function."@en .

cim:WindDynamicsLookupTable.sequence a owl:DatatypeProperty ;
  rdfs:label "sequence"@en ;
  rdfs:domain cim:WindDynamicsLookupTable ;
  rdfs:range xsd:integer ;
  skos:definition "Sequence numbers of the pairs of the input (<i>x</i>) and the output (<i>y</i>) of the lookup table function."@en .

cim:WindGenType3IEC.dipmax a owl:DatatypeProperty ;
  rdfs:label "dipmax"@en ;
  rdfs:domain cim:WindGenType3IEC ;
  rdfs:range cim:PU ;
  skos:definition "Maximum active current ramp rate (<i>di</i><i><sub>pmax</sub></i>). It is a project-dependent parameter."@en .

cim:WindGenType3IEC.diqmax a owl:DatatypeProperty ;
  rdfs:label "diqmax"@en ;
  rdfs:domain cim:WindGenType3IEC ;
  rdfs:range cim:PU ;
  skos:definition "Maximum reactive current ramp rate (<i>di</i><i><sub>qmax</sub></i>). It is a project-dependent parameter."@en .

cim:WindGenType3IEC.xs a owl:DatatypeProperty ;
  rdfs:label "xs"@en ;
  rdfs:domain cim:WindGenType3IEC ;
  rdfs:range cim:PU ;
  skos:definition "Electromagnetic transient reactance (<i>x</i><i><sub>S</sub></i>). It is a type-dependent parameter."@en .

cim:WindGenType3aIEC.kpc a owl:DatatypeProperty ;
  rdfs:label "kpc"@en ;
  rdfs:domain cim:WindGenType3aIEC ;
  rdfs:range xsd:float ;
  skos:definition "Current PI controller proportional gain (<i>K</i><i><sub>Pc</sub></i>). It is a type-dependent parameter."@en .

cim:WindGenType3aIEC.tic a owl:DatatypeProperty ;
  rdfs:label "tic"@en ;
  rdfs:domain cim:WindGenType3aIEC ;
  rdfs:range cim:Seconds ;
  skos:definition "Current PI controller integration time constant (<i>T</i><i><sub>Ic</sub></i>) (&gt;= 0). It is a type-dependent parameter."@en .

cim:WindGenType3bIEC.mwtcwp a owl:DatatypeProperty ;
  rdfs:label "mwtcwp"@en ;
  rdfs:domain cim:WindGenType3bIEC ;
  rdfs:range xsd:boolean ;
  skos:definition """
Crowbar control mode (<i>M</i><i><sub>WTcwp</sub></i>). It is a case-dependent parameter.
true = 1 in the IEC model
false = 0 in the IEC model.
\t"""@en .

cim:WindGenType3bIEC.tg a owl:DatatypeProperty ;
  rdfs:label "tg"@en ;
  rdfs:domain cim:WindGenType3bIEC ;
  rdfs:range cim:Seconds ;
  skos:definition "Current generation time constant (<i>T</i><i><sub>g</sub></i>) (&gt;= 0). It is a type-dependent parameter."@en .

cim:WindGenType3bIEC.two a owl:DatatypeProperty ;
  rdfs:label "two"@en ;
  rdfs:domain cim:WindGenType3bIEC ;
  rdfs:range cim:Seconds ;
  skos:definition "Time constant for crowbar washout filter (<i>T</i><i><sub>wo</sub></i>) (&gt;= 0). It is a case-dependent parameter."@en .

cim:WindGenType4IEC.dipmax a owl:DatatypeProperty ;
  rdfs:label "dipmax"@en ;
  rdfs:domain cim:WindGenType4IEC ;
  rdfs:range cim:PU ;
  skos:definition "Maximum active current ramp rate (<i>di</i><i><sub>pmax</sub></i>). It is a project-dependent parameter."@en .

cim:WindGenType4IEC.diqmax a owl:DatatypeProperty ;
  rdfs:label "diqmax"@en ;
  rdfs:domain cim:WindGenType4IEC ;
  rdfs:range cim:PU ;
  skos:definition "Maximum reactive current ramp rate (<i>di</i><i><sub>qmax</sub></i>). It is a project-dependent parameter."@en .

cim:WindGenType4IEC.diqmin a owl:DatatypeProperty ;
  rdfs:label "diqmin"@en ;
  rdfs:domain cim:WindGenType4IEC ;
  rdfs:range cim:PU ;
  skos:definition "Minimum reactive current ramp rate (<i>di</i><i><sub>qmin</sub></i>). It is a project-dependent parameter."@en .

cim:WindGenType4IEC.tg a owl:DatatypeProperty ;
  rdfs:label "tg"@en ;
  rdfs:domain cim:WindGenType4IEC ;
  rdfs:range cim:Seconds ;
  skos:definition "Time constant (<i>T</i><i><sub>g</sub></i>) (&gt;= 0). It is a type-dependent parameter."@en .

cim:WindMechIEC.cdrt a owl:DatatypeProperty ;
  rdfs:label "cdrt"@en ;
  rdfs:domain cim:WindMechIEC ;
  rdfs:range cim:PU ;
  skos:definition "Drive train damping (<i>c</i><i><sub>drt</sub></i><i>)</i>. It is a type-dependent parameter."@en .

cim:WindMechIEC.hgen a owl:DatatypeProperty ;
  rdfs:label "hgen"@en ;
  rdfs:domain cim:WindMechIEC ;
  rdfs:range cim:Seconds ;
  skos:definition "Inertia constant of generator (<i>H</i><i><sub>gen</sub></i>) (&gt;= 0). It is a type-dependent parameter."@en .

cim:WindMechIEC.hwtr a owl:DatatypeProperty ;
  rdfs:label "hwtr"@en ;
  rdfs:domain cim:WindMechIEC ;
  rdfs:range cim:Seconds ;
  skos:definition "Inertia constant of wind turbine rotor (<i>H</i><i><sub>WTR</sub></i>) (&gt;= 0). It is a type-dependent parameter."@en .

cim:WindMechIEC.kdrt a owl:DatatypeProperty ;
  rdfs:label "kdrt"@en ;
  rdfs:domain cim:WindMechIEC ;
  rdfs:range cim:PU ;
  skos:definition "Drive train stiffness (<i>k</i><i><sub>drt</sub></i>). It is a type-dependent parameter."@en .

cim:WindPitchContPowerIEC.dpmax a owl:DatatypeProperty ;
  rdfs:label "dpmax"@en ;
  rdfs:domain cim:WindPitchContPowerIEC ;
  rdfs:range cim:PU ;
  skos:definition "Rate limit for increasing power (<i>dp</i><i><sub>max</sub></i>) (&gt; WindPitchContPowerIEC.dpmin). It is a type-dependent parameter."@en .

cim:WindPitchContPowerIEC.dpmin a owl:DatatypeProperty ;
  rdfs:label "dpmin"@en ;
  rdfs:domain cim:WindPitchContPowerIEC ;
  rdfs:range cim:PU ;
  skos:definition "Rate limit for decreasing power (<i>dp</i><i><sub>min</sub></i>) (&lt; WindPitchContPowerIEC.dpmax). It is a type-dependent parameter."@en .

cim:WindPitchContPowerIEC.pmin a owl:DatatypeProperty ;
  rdfs:label "pmin"@en ;
  rdfs:domain cim:WindPitchContPowerIEC ;
  rdfs:range cim:PU ;
  skos:definition "Minimum power setting (<i>p</i><i><sub>min</sub></i>). It is a type-dependent parameter."@en .

cim:WindPitchContPowerIEC.pset a owl:DatatypeProperty ;
  rdfs:label "pset"@en ;
  rdfs:domain cim:WindPitchContPowerIEC ;
  rdfs:range cim:PU ;
  skos:definition "If <i>p</i><i><sub>init</sub></i><sub> </sub>&lt; <i>p</i><i><sub>set</sub></i><sub> </sub>then power will be ramped down to <i>p</i><i><sub>min</sub></i>. It is (<i>p</i><i><sub>set</sub></i>) in the IEC 61400-27-1:2015. It is a type-dependent parameter."@en .

cim:WindPitchContPowerIEC.t1 a owl:DatatypeProperty ;
  rdfs:label "t1"@en ;
  rdfs:domain cim:WindPitchContPowerIEC ;
  rdfs:range cim:Seconds ;
  skos:definition "Lag time constant (<i>T</i><i><sub>1</sub></i>) (&gt;= 0). It is a type-dependent parameter."@en .

cim:WindPitchContPowerIEC.tr a owl:DatatypeProperty ;
  rdfs:label "tr"@en ;
  rdfs:domain cim:WindPitchContPowerIEC ;
  rdfs:range cim:Seconds ;
  skos:definition "Voltage measurement time constant (<i>T</i><i><sub>r</sub></i>) (&gt;= 0). It is a type-dependent parameter."@en .

cim:WindPitchContPowerIEC.uuvrt a owl:DatatypeProperty ;
  rdfs:label "uuvrt"@en ;
  rdfs:domain cim:WindPitchContPowerIEC ;
  rdfs:range cim:PU ;
  skos:definition "Dip detection threshold (<i>u</i><i><sub>UVRT</sub></i>). It is a type-dependent parameter."@en .

cim:WindPlantFreqPcontrolIEC.dprefmax a owl:DatatypeProperty ;
  rdfs:label "dprefmax"@en ;
  rdfs:domain cim:WindPlantFreqPcontrolIEC ;
  rdfs:range cim:PU ;
  skos:definition "Maximum ramp rate of <i>p</i><i><sub>WTref</sub></i> request from the plant controller to the wind turbines (<i>dp</i><i><sub>refmax</sub></i>) (&gt; WindPlantFreqPcontrolIEC.dprefmin). It is a case-dependent parameter."@en .

cim:WindPlantFreqPcontrolIEC.dprefmin a owl:DatatypeProperty ;
  rdfs:label "dprefmin"@en ;
  rdfs:domain cim:WindPlantFreqPcontrolIEC ;
  rdfs:range cim:PU ;
  skos:definition "Minimum (negative) ramp rate of <i>p</i><i><sub>WTref</sub></i> request from the plant controller to the wind turbines (<i>dp</i><i><sub>refmin</sub></i>) (&lt; WindPlantFreqPcontrolIEC.dprefmax). It is a project-dependent parameter."@en .

cim:WindPlantFreqPcontrolIEC.dpwprefmax a owl:DatatypeProperty ;
  rdfs:label "dpwprefmax"@en ;
  rdfs:domain cim:WindPlantFreqPcontrolIEC ;
  rdfs:range cim:PU ;
  skos:definition "Maximum positive ramp rate for wind plant power reference (<i>dp</i><i><sub>WPrefmax</sub></i>) (&gt; WindPlantFreqPcontrolIEC.dpwprefmin). It is a project-dependent parameter."@en .

cim:WindPlantFreqPcontrolIEC.dpwprefmin a owl:DatatypeProperty ;
  rdfs:label "dpwprefmin"@en ;
  rdfs:domain cim:WindPlantFreqPcontrolIEC ;
  rdfs:range cim:PU ;
  skos:definition "Maximum negative ramp rate for wind plant power reference (<i>dp</i><i><sub>WPrefmin</sub></i>) (&lt; WindPlantFreqPcontrolIEC.dpwprefmax). It is a project-dependent parameter."@en .

cim:WindPlantFreqPcontrolIEC.kiwpp a owl:DatatypeProperty ;
  rdfs:label "kiwpp"@en ;
  rdfs:domain cim:WindPlantFreqPcontrolIEC ;
  rdfs:range xsd:float ;
  skos:definition "Plant P controller integral gain (<i>K</i><i><sub>IWPp</sub></i>). It is a project-dependent parameter."@en .

cim:WindPlantFreqPcontrolIEC.kiwppmax a owl:DatatypeProperty ;
  rdfs:label "kiwppmax"@en ;
  rdfs:domain cim:WindPlantFreqPcontrolIEC ;
  rdfs:range cim:PU ;
  skos:definition "Maximum PI integrator term (<i>K</i><i><sub>IWPpmax</sub></i>) (&gt; WindPlantFreqPcontrolIEC.kiwppmin). It is a project-dependent parameter."@en .

cim:WindPlantFreqPcontrolIEC.kiwppmin a owl:DatatypeProperty ;
  rdfs:label "kiwppmin"@en ;
  rdfs:domain cim:WindPlantFreqPcontrolIEC ;
  rdfs:range cim:PU ;
  skos:definition "Minimum PI integrator term (<i>K</i><i><sub>IWPpmin</sub></i>) (&lt; WindPlantFreqPcontrolIEC.kiwppmax). It is a project-dependent parameter."@en .

cim:WindPlantFreqPcontrolIEC.kpwpp a owl:DatatypeProperty ;
  rdfs:label "kpwpp"@en ;
  rdfs:domain cim:WindPlantFreqPcontrolIEC ;
  rdfs:range xsd:float ;
  skos:definition "Plant P controller proportional gain (<i>K</i><i><sub>PWPp</sub></i>). It is a project-dependent parameter."@en .

cim:WindPlantFreqPcontrolIEC.kwppref a owl:DatatypeProperty ;
  rdfs:label "kwppref"@en ;
  rdfs:domain cim:WindPlantFreqPcontrolIEC ;
  rdfs:range cim:PU ;
  skos:definition "Power reference gain (<i>K</i><i><sub>WPpref</sub></i>). It is a project-dependent parameter."@en .

cim:WindPlantFreqPcontrolIEC.prefmax a owl:DatatypeProperty ;
  rdfs:label "prefmax"@en ;
  rdfs:domain cim:WindPlantFreqPcontrolIEC ;
  rdfs:range cim:PU ;
  skos:definition "Maximum <i>p</i><i><sub>WTref</sub></i> request from the plant controller to the wind turbines (<i>p</i><i><sub>refmax</sub></i>) (&gt; WindPlantFreqPcontrolIEC.prefmin). It is a project-dependent parameter."@en .

cim:WindPlantFreqPcontrolIEC.prefmin a owl:DatatypeProperty ;
  rdfs:label "prefmin"@en ;
  rdfs:domain cim:WindPlantFreqPcontrolIEC ;
  rdfs:range cim:PU ;
  skos:definition "Minimum <i>p</i><i><sub>WTref</sub></i> request from the plant controller to the wind turbines (<i>p</i><i><sub>refmin</sub></i>) (&lt; WindPlantFreqPcontrolIEC.prefmax). It is a project-dependent parameter."@en .

cim:WindPlantFreqPcontrolIEC.tpft a owl:DatatypeProperty ;
  rdfs:label "tpft"@en ;
  rdfs:domain cim:WindPlantFreqPcontrolIEC ;
  rdfs:range cim:Seconds ;
  skos:definition "Lead time constant in reference value transfer function (<i>T</i><i><sub>pft</sub></i>) (&gt;= 0). It is a project-dependent parameter."@en .

cim:WindPlantFreqPcontrolIEC.tpfv a owl:DatatypeProperty ;
  rdfs:label "tpfv"@en ;
  rdfs:domain cim:WindPlantFreqPcontrolIEC ;
  rdfs:range cim:Seconds ;
  skos:definition "Lag time constant in reference value transfer function (<i>T</i><i><sub>pfv</sub></i>) (&gt;= 0). It is a project-dependent parameter."@en .

cim:WindPlantFreqPcontrolIEC.twpffiltp a owl:DatatypeProperty ;
  rdfs:label "twpffiltp"@en ;
  rdfs:domain cim:WindPlantFreqPcontrolIEC ;
  rdfs:range cim:Seconds ;
  skos:definition "Filter time constant for frequency measurement (<i>T</i><i><sub>WPffiltp</sub></i>) (&gt;= 0). It is a project-dependent parameter."@en .

cim:WindPlantFreqPcontrolIEC.twppfiltp a owl:DatatypeProperty ;
  rdfs:label "twppfiltp"@en ;
  rdfs:domain cim:WindPlantFreqPcontrolIEC ;
  rdfs:range cim:Seconds ;
  skos:definition "Filter time constant for active power measurement (<i>T</i><i><sub>WPpfiltp</sub></i>) (&gt;= 0). It is a project-dependent parameter."@en .

cim:WindPlantReactiveControlIEC.dxrefmax a owl:DatatypeProperty ;
  rdfs:label "dxrefmax"@en ;
  rdfs:domain cim:WindPlantReactiveControlIEC ;
  rdfs:range cim:PU ;
  skos:definition "Maximum positive ramp rate for wind turbine reactive power/voltage reference (<i>dx</i><i><sub>refmax</sub></i>) (&gt; WindPlantReactiveControlIEC.dxrefmin). It is a project-dependent parameter."@en .

cim:WindPlantReactiveControlIEC.dxrefmin a owl:DatatypeProperty ;
  rdfs:label "dxrefmin"@en ;
  rdfs:domain cim:WindPlantReactiveControlIEC ;
  rdfs:range cim:PU ;
  skos:definition "Maximum negative ramp rate for wind turbine reactive power/voltage reference (<i>dx</i><i><sub>refmin</sub></i>) (&lt; WindPlantReactiveControlIEC.dxrefmax). It is a project-dependent parameter."@en .

cim:WindPlantReactiveControlIEC.kiwpx a owl:DatatypeProperty ;
  rdfs:label "kiwpx"@en ;
  rdfs:domain cim:WindPlantReactiveControlIEC ;
  rdfs:range xsd:float ;
  skos:definition "Plant Q controller integral gain (<i>K</i><i><sub>IWPx</sub></i>). It is a project-dependent parameter."@en .

cim:WindPlantReactiveControlIEC.kiwpxmax a owl:DatatypeProperty ;
  rdfs:label "kiwpxmax"@en ;
  rdfs:domain cim:WindPlantReactiveControlIEC ;
  rdfs:range cim:PU ;
  skos:definition "Maximum reactive power/voltage reference from integration (<i>K</i><i><sub>IWPxmax</sub></i>) (&gt; WindPlantReactiveControlIEC.kiwpxmin). It is a project-dependent parameter."@en .

cim:WindPlantReactiveControlIEC.kiwpxmin a owl:DatatypeProperty ;
  rdfs:label "kiwpxmin"@en ;
  rdfs:domain cim:WindPlantReactiveControlIEC ;
  rdfs:range cim:PU ;
  skos:definition "Minimum reactive power/voltage reference from integration (<i>K</i><i><sub>IWPxmin</sub></i>) (&lt; WindPlantReactiveControlIEC.kiwpxmax). It is a project-dependent parameter."@en .

cim:WindPlantReactiveControlIEC.kpwpx a owl:DatatypeProperty ;
  rdfs:label "kpwpx"@en ;
  rdfs:domain cim:WindPlantReactiveControlIEC ;
  rdfs:range xsd:float ;
  skos:definition "Plant Q controller proportional gain (<i>K</i><i><sub>PWPx</sub></i>). It is a project-dependent parameter."@en .

cim:WindPlantReactiveControlIEC.kwpqref a owl:DatatypeProperty ;
  rdfs:label "kwpqref"@en ;
  rdfs:domain cim:WindPlantReactiveControlIEC ;
  rdfs:range cim:PU ;
  skos:definition "Reactive power reference gain (<i>K</i><i><sub>WPqref</sub></i>). It is a project-dependent parameter."@en .

cim:WindPlantReactiveControlIEC.kwpqu a owl:DatatypeProperty ;
  rdfs:label "kwpqu"@en ;
  rdfs:domain cim:WindPlantReactiveControlIEC ;
  rdfs:range cim:PU ;
  skos:definition "Plant voltage control droop (<i>K</i><i><sub>WPqu</sub></i>). It is a project-dependent parameter."@en .

cim:WindPlantReactiveControlIEC.tuqfilt a owl:DatatypeProperty ;
  rdfs:label "tuqfilt"@en ;
  rdfs:domain cim:WindPlantReactiveControlIEC ;
  rdfs:range cim:Seconds ;
  skos:definition "Filter time constant for voltage-dependent reactive power (<i>T</i><i><sub>uqfilt</sub></i>) (&gt;= 0). It is a project-dependent parameter."@en .

cim:WindPlantReactiveControlIEC.twppfiltq a owl:DatatypeProperty ;
  rdfs:label "twppfiltq"@en ;
  rdfs:domain cim:WindPlantReactiveControlIEC ;
  rdfs:range cim:Seconds ;
  skos:definition "Filter time constant for active power measurement (<i>T</i><i><sub>WPpfiltq</sub></i>) (&gt;= 0). It is a project-dependent parameter."@en .

cim:WindPlantReactiveControlIEC.twpqfiltq a owl:DatatypeProperty ;
  rdfs:label "twpqfiltq"@en ;
  rdfs:domain cim:WindPlantReactiveControlIEC ;
  rdfs:range cim:Seconds ;
  skos:definition "Filter time constant for reactive power measurement (<i>T</i><i><sub>WPqfiltq</sub></i>) (&gt;= 0). It is a project-dependent parameter."@en .

cim:WindPlantReactiveControlIEC.twpufiltq a owl:DatatypeProperty ;
  rdfs:label "twpufiltq"@en ;
  rdfs:domain cim:WindPlantReactiveControlIEC ;
  rdfs:range cim:Seconds ;
  skos:definition "Filter time constant for voltage measurement (<i>T</i><i><sub>WPufiltq</sub></i>) (&gt;= 0). It is a project-dependent parameter."@en .

cim:WindPlantReactiveControlIEC.txft a owl:DatatypeProperty ;
  rdfs:label "txft"@en ;
  rdfs:domain cim:WindPlantReactiveControlIEC ;
  rdfs:range cim:Seconds ;
  skos:definition "Lead time constant in reference value transfer function (<i>T</i><i><sub>xft</sub></i>) (&gt;= 0). It is a project-dependent parameter."@en .

cim:WindPlantReactiveControlIEC.txfv a owl:DatatypeProperty ;
  rdfs:label "txfv"@en ;
  rdfs:domain cim:WindPlantReactiveControlIEC ;
  rdfs:range cim:Seconds ;
  skos:definition "Lag time constant in reference value transfer function (<i>T</i><i><sub>xfv</sub></i>) (&gt;= 0). It is a project-dependent parameter."@en .

cim:WindPlantReactiveControlIEC.uwpqdip a owl:DatatypeProperty ;
  rdfs:label "uwpqdip"@en ;
  rdfs:domain cim:WindPlantReactiveControlIEC ;
  rdfs:range cim:PU ;
  skos:definition "Voltage threshold for UVRT detection in Q control (<i>u</i><i><sub>WPqdip</sub></i>). It is a project-dependent parameter."@en .

cim:WindPlantReactiveControlIEC.windPlantQcontrolModesType a owl:DatatypeProperty ;
  rdfs:label "windPlantQcontrolModesType"@en ;
  rdfs:domain cim:WindPlantReactiveControlIEC ;
  rdfs:range cim:WindPlantQcontrolModeKind ;
  skos:definition "Reactive power/voltage controller mode (<i>M</i><i><sub>WPqmode</sub></i>). It is a case-dependent parameter."@en .

cim:WindPlantReactiveControlIEC.xrefmax a owl:DatatypeProperty ;
  rdfs:label "xrefmax"@en ;
  rdfs:domain cim:WindPlantReactiveControlIEC ;
  rdfs:range cim:PU ;
  skos:definition "Maximum <i>x</i><sub>WTref</sub> (<i>q</i><i><sub>WTref</sub></i> or delta<i> u</i><i><sub>WTref</sub></i>) request from the plant controller (<i>x</i><i><sub>refmax</sub></i>) (&gt; WindPlantReactiveControlIEC.xrefmin). It is a case-dependent parameter."@en .

cim:WindPlantReactiveControlIEC.xrefmin a owl:DatatypeProperty ;
  rdfs:label "xrefmin"@en ;
  rdfs:domain cim:WindPlantReactiveControlIEC ;
  rdfs:range cim:PU ;
  skos:definition "Minimum <i>x</i><i><sub>WTref</sub></i> (<i>q</i><i><sub>WTref</sub></i> or delta <i>u</i><i><sub>WTref</sub></i>) request from the plant controller (<i>x</i><i><sub>refmin</sub></i>) (&lt; WindPlantReactiveControlIEC.xrefmax). It is a project-dependent parameter."@en .

cim:WindPlantUserDefined.proprietary a owl:DatatypeProperty ;
  rdfs:label "proprietary"@en ;
  rdfs:domain cim:WindPlantUserDefined ;
  rdfs:range xsd:boolean ;
  skos:definition """
Behaviour is based on a proprietary model as opposed to a detailed model.
true = user-defined model is proprietary with behaviour mutually understood by sending and receiving applications and parameters passed as general attributes
false = user-defined model is explicitly defined in terms of control blocks and their input and output signals.
\t"""@en .

cim:WindProtectionIEC.dfimax a owl:DatatypeProperty ;
  rdfs:label "dfimax"@en ;
  rdfs:domain cim:WindProtectionIEC ;
  rdfs:range cim:PU ;
  skos:definition "Maximum rate of change of frequency (<i>dF</i><i><sub>max</sub></i>). It is a type-dependent parameter."@en .

cim:WindProtectionIEC.fover a owl:DatatypeProperty ;
  rdfs:label "fover"@en ;
  rdfs:domain cim:WindProtectionIEC ;
  rdfs:range cim:PU ;
  skos:definition "Wind turbine over frequency protection activation threshold (<i>f</i><i><sub>over</sub></i>). It is a project-dependent parameter. "@en .

cim:WindProtectionIEC.funder a owl:DatatypeProperty ;
  rdfs:label "funder"@en ;
  rdfs:domain cim:WindProtectionIEC ;
  rdfs:range cim:PU ;
  skos:definition "Wind turbine under frequency protection activation threshold (<i>f</i><i><sub>under</sub></i>). It is a project-dependent parameter."@en .

cim:WindProtectionIEC.mzc a owl:DatatypeProperty ;
  rdfs:label "mzc"@en ;
  rdfs:domain cim:WindProtectionIEC ;
  rdfs:range xsd:boolean ;
  skos:definition """
Zero crossing measurement mode (<i>Mzc</i>).  It is a type-dependent parameter. 
true = WT protection system uses zero crossings to detect frequency (1 in the IEC model)
false = WT protection system does not use zero crossings to detect frequency (0 in the IEC model).
\t"""@en .

cim:WindProtectionIEC.tfma a owl:DatatypeProperty ;
  rdfs:label "tfma"@en ;
  rdfs:domain cim:WindProtectionIEC ;
  rdfs:range cim:Seconds ;
  skos:definition "Time interval of moving average window (<i>TfMA</i>) (&gt;= 0).  It is a type-dependent parameter."@en .

cim:WindProtectionIEC.uover a owl:DatatypeProperty ;
  rdfs:label "uover"@en ;
  rdfs:domain cim:WindProtectionIEC ;
  rdfs:range cim:PU ;
  skos:definition "Wind turbine over voltage protection activation threshold (<i>u</i><i><sub>over</sub></i>). It is a project-dependent parameter."@en .

cim:WindProtectionIEC.uunder a owl:DatatypeProperty ;
  rdfs:label "uunder"@en ;
  rdfs:domain cim:WindProtectionIEC ;
  rdfs:range cim:PU ;
  skos:definition "Wind turbine under voltage protection activation threshold (<i>u</i><i><sub>under</sub></i>). It is a project-dependent parameter."@en .

cim:WindRefFrameRotIEC.tpll a owl:DatatypeProperty ;
  rdfs:label "tpll"@en ;
  rdfs:domain cim:WindRefFrameRotIEC ;
  rdfs:range cim:Seconds ;
  skos:definition "Time constant for PLL first order filter model (<i>T</i><i><sub>PLL</sub></i>) (&gt;= 0). It is a type-dependent parameter."@en .

cim:WindRefFrameRotIEC.upll1 a owl:DatatypeProperty ;
  rdfs:label "upll1"@en ;
  rdfs:domain cim:WindRefFrameRotIEC ;
  rdfs:range cim:PU ;
  skos:definition "Voltage below which the angle of the voltage is filtered and possibly also frozen (<i>u</i><i><sub>PLL1</sub></i>). It is a type-dependent parameter."@en .

cim:WindRefFrameRotIEC.upll2 a owl:DatatypeProperty ;
  rdfs:label "upll2"@en ;
  rdfs:domain cim:WindRefFrameRotIEC ;
  rdfs:range cim:PU ;
  skos:definition "Voltage (<i>u</i><i><sub>PLL2</sub></i>) below which the angle of the voltage is frozen if <i>u</i><i><sub>PLL2</sub></i><sub> </sub>is smaller or equal to <i>u</i><i><sub>PLL1</sub></i> . It is a type-dependent parameter."@en .

cim:WindType1or2UserDefined.proprietary a owl:DatatypeProperty ;
  rdfs:label "proprietary"@en ;
  rdfs:domain cim:WindType1or2UserDefined ;
  rdfs:range xsd:boolean ;
  skos:definition """
Behaviour is based on a proprietary model as opposed to a detailed model.
true = user-defined model is proprietary with behaviour mutually understood by sending and receiving applications and parameters passed as general attributes
false = user-defined model is explicitly defined in terms of control blocks and their input and output signals.
\t"""@en .

cim:WindType3or4UserDefined.proprietary a owl:DatatypeProperty ;
  rdfs:label "proprietary"@en ;
  rdfs:domain cim:WindType3or4UserDefined ;
  rdfs:range xsd:boolean ;
  skos:definition """
Behaviour is based on a proprietary model as opposed to a detailed model.
true = user-defined model is proprietary with behaviour mutually understood by sending and receiving applications and parameters passed as general attributes
false = user-defined model is explicitly defined in terms of control blocks and their input and output signals.
\t"""@en .

dy:Package a owl:AnnotationProperty ;
  rdfs:label "MOF Package"@en ;
  rdfs:comment "Declaration that this is a MOF Package."@en ;
  rdfs:domain rdfs:Class ;
  rdfs:range xsd:string .

dy:isAbstract a owl:AnnotationProperty ;
  rdfs:label "is abstract"@en ;
  rdfs:comment "Flag indicating whether the class is permitted to have any direct instances."@en ;
  rdfs:domain rdfs:Class ;
  rdfs:range xsd:boolean .

dy:isCIMDatatype a owl:AnnotationProperty ;
  rdfs:label "isCIMDatatype\t"@en ;
  rdfs:comment "Flag indicating whether the class is a CIMDatatype."@en ;
  rdfs:domain rdfs:Class ;
  rdfs:range xsd:boolean .

dy:isConst a owl:AnnotationProperty ;
  rdfs:label "is fixed property"@en ;
  rdfs:comment " Flag indicating whether the property for a specific object can be updated."@en ;
  rdfs:domain rdfs:Property ;
  rdfs:range xsd:boolean .

dy:isDescription a owl:AnnotationProperty ;
  rdfs:label "isDescription\t"@en ;
  rdfs:comment "Flag indicating whether the class is a Description."@en ;
  rdfs:domain rdfs:Class, rdfs:Property ;
  rdfs:range xsd:boolean .

dy:isFixed a owl:AnnotationProperty ;
  rdfs:label "is fixed property"@en ;
  rdfs:comment " Flag indicating whether the property for a specific object can be updated."@en ;
  rdfs:domain rdfs:Property ;
  rdfs:range xsd:boolean .

dy:isPrimitive a owl:AnnotationProperty ;
  rdfs:label "isPrimitive\t"@en ;
  rdfs:comment "Flag indicating whether the class is a Primitive."@en ;
  rdfs:domain rdfs:Class ;
  rdfs:range xsd:boolean .

dy:isUnique a owl:AnnotationProperty ;
  rdfs:label "is unique "@en ;
  rdfs:comment " Flag indicating whether the property for a specific object can contain the same value more than once."@en ;
  rdfs:domain rdfs:Property ;
  rdfs:range xsd:boolean .

dy:isenum a owl:AnnotationProperty ;
  rdfs:label "isenum\t"@en ;
  rdfs:comment "Flag indicating whether the enumerated literal is an enum."@en ;
  rdfs:domain rdfs:Property ;
  rdfs:range xsd:boolean .

cim:DroopSignalFeedbackKind.electricalPower a owl:NamedIndividual, owl:Thing ;
  rdfs:label "electricalPower "@en ;
  dy:isenum "True" ;
  rdfs:domain cim:DroopSignalFeedbackKind ;
  skos:definition "Electrical power feedback (connection indicated as 1 in the block diagrams of models, e.g. GovCT1, GovCT2)."@en .

cim:DroopSignalFeedbackKind.fuelValveStroke a owl:NamedIndividual, owl:Thing ;
  rdfs:label "fuelValveStroke "@en ;
  dy:isenum "True" ;
  rdfs:domain cim:DroopSignalFeedbackKind ;
  skos:definition "Fuel valve stroke feedback (true stroke) (connection indicated as 2 in the block diagrams of model, e.g. GovCT1, GovCT2)."@en .

cim:DroopSignalFeedbackKind.governorOutput a owl:NamedIndividual, owl:Thing ;
  rdfs:label "governorOutput "@en ;
  dy:isenum "True" ;
  rdfs:domain cim:DroopSignalFeedbackKind ;
  skos:definition "Governor output feedback (requested stroke) (connection indicated as 3 in the block diagrams of models, e.g. GovCT1, GovCT2)."@en .

cim:DroopSignalFeedbackKind.none a owl:NamedIndividual, owl:Thing ;
  rdfs:label "none "@en ;
  dy:isenum "True" ;
  rdfs:domain cim:DroopSignalFeedbackKind ;
  skos:definition "No droop signal feedback, is isochronous governor."@en .

cim:ExcIEEEST1AUELselectorKind.ignoreUELsignal a owl:NamedIndividual, owl:Thing ;
  rdfs:label "ignoreUELsignal "@en ;
  dy:isenum "True" ;
  rdfs:domain cim:ExcIEEEST1AUELselectorKind ;
  skos:definition "Ignore UEL signal."@en .

cim:ExcIEEEST1AUELselectorKind.inputAddedToErrorSignal a owl:NamedIndividual, owl:Thing ;
  rdfs:label "inputAddedToErrorSignal "@en ;
  dy:isenum "True" ;
  rdfs:domain cim:ExcIEEEST1AUELselectorKind ;
  skos:definition "UEL input added to error signal."@en .

cim:ExcIEEEST1AUELselectorKind.inputHVgateErrorSignal a owl:NamedIndividual, owl:Thing ;
  rdfs:label "inputHVgateErrorSignal "@en ;
  dy:isenum "True" ;
  rdfs:domain cim:ExcIEEEST1AUELselectorKind ;
  skos:definition "UEL input HV gate with error signal."@en .

cim:ExcIEEEST1AUELselectorKind.inputHVgateVoltageOutput a owl:NamedIndividual, owl:Thing ;
  rdfs:label "inputHVgateVoltageOutput "@en ;
  dy:isenum "True" ;
  rdfs:domain cim:ExcIEEEST1AUELselectorKind ;
  skos:definition "UEL input HV gate with voltage regulator output."@en .

cim:ExcREXSFeedbackSignalKind.fieldCurrent a owl:NamedIndividual, owl:Thing ;
  rdfs:label "fieldCurrent "@en ;
  dy:isenum "True" ;
  rdfs:domain cim:ExcREXSFeedbackSignalKind ;
  skos:definition "The exciter field current is used."@en .

cim:ExcREXSFeedbackSignalKind.fieldVoltage a owl:NamedIndividual, owl:Thing ;
  rdfs:label "fieldVoltage "@en ;
  dy:isenum "True" ;
  rdfs:domain cim:ExcREXSFeedbackSignalKind ;
  skos:definition "The voltage regulator output voltage is used. It is the same as exciter field voltage."@en .

cim:ExcREXSFeedbackSignalKind.outputVoltage a owl:NamedIndividual, owl:Thing ;
  rdfs:label "outputVoltage "@en ;
  dy:isenum "True" ;
  rdfs:domain cim:ExcREXSFeedbackSignalKind ;
  skos:definition "The output voltage of the exciter is used."@en .

cim:ExcST6BOELselectorKind.afterUEL a owl:NamedIndividual, owl:Thing ;
  rdfs:label "afterUEL "@en ;
  dy:isenum "True" ;
  rdfs:domain cim:ExcST6BOELselectorKind ;
  skos:definition "The connection is after UEL. Corresponds to <i>OELin</i> = 2 on the ExcST6B diagram."@en .

cim:ExcST6BOELselectorKind.beforeUEL a owl:NamedIndividual, owl:Thing ;
  rdfs:label "beforeUEL "@en ;
  dy:isenum "True" ;
  rdfs:domain cim:ExcST6BOELselectorKind ;
  skos:definition "The connection is before UEL. Corresponds to <i>OELin</i> = 1 on the ExcST6B diagram."@en .

cim:ExcST6BOELselectorKind.noOELinput a owl:NamedIndividual, owl:Thing ;
  rdfs:label "noOELinput "@en ;
  dy:isenum "True" ;
  rdfs:domain cim:ExcST6BOELselectorKind ;
  skos:definition "No OEL input is used. Corresponds to <i>OELin</i> not = 1 and not = 2 on the ExcST6B diagram. Original ExcST6B model would have called this <i>OELin</i> = 0."@en .

cim:ExcST7BOELselectorKind.addVref a owl:NamedIndividual, owl:Thing ;
  rdfs:label "addVref "@en ;
  dy:isenum "True" ;
  rdfs:domain cim:ExcST7BOELselectorKind ;
  skos:definition """
The signal is added to <i>Vref</i>.  Corresponds to <i>OELin</i> = 1 on the ExcST7B diagram.

\t"""@en .

cim:ExcST7BOELselectorKind.inputLVgate a owl:NamedIndividual, owl:Thing ;
  rdfs:label "inputLVgate "@en ;
  dy:isenum "True" ;
  rdfs:domain cim:ExcST7BOELselectorKind ;
  skos:definition "The signal is connected into the input <i>LVGate</i>. Corresponds to <i>OELin</i> = 2 on the ExcST7B diagram."@en .

cim:ExcST7BOELselectorKind.noOELinput a owl:NamedIndividual, owl:Thing ;
  rdfs:label "noOELinput "@en ;
  dy:isenum "True" ;
  rdfs:domain cim:ExcST7BOELselectorKind ;
  skos:definition """
No OEL input is used. Corresponds to <i>OELin</i> not = 1 and not = 2 and not = 3 on the ExcST7B diagram. Original ExcST7B model would have called this <i>OELin</i> = 0.

\t"""@en .

cim:ExcST7BOELselectorKind.outputLVgate a owl:NamedIndividual, owl:Thing ;
  rdfs:label "outputLVgate "@en ;
  dy:isenum "True" ;
  rdfs:domain cim:ExcST7BOELselectorKind ;
  skos:definition "The signal is connected into the output <i>LVGate</i>.  Corresponds to <i>OELin</i> = 3 on the ExcST7B diagram."@en .

cim:ExcST7BUELselectorKind.addVref a owl:NamedIndividual, owl:Thing ;
  rdfs:label "addVref "@en ;
  dy:isenum "True" ;
  rdfs:domain cim:ExcST7BUELselectorKind ;
  skos:definition """
The signal is added to <i>Vref</i>. Corresponds to <i>UELin</i> = 1 on the ExcST7B diagram.

\t"""@en .

cim:ExcST7BUELselectorKind.inputHVgate a owl:NamedIndividual, owl:Thing ;
  rdfs:label "inputHVgate "@en ;
  dy:isenum "True" ;
  rdfs:domain cim:ExcST7BUELselectorKind ;
  skos:definition """
The signal is connected into the input <i>HVGate</i>.  Corresponds to <i>UELin</i> = 2 on the ExcST7B diagram.

\t"""@en .

cim:ExcST7BUELselectorKind.noUELinput a owl:NamedIndividual, owl:Thing ;
  rdfs:label "noUELinput "@en ;
  dy:isenum "True" ;
  rdfs:domain cim:ExcST7BUELselectorKind ;
  skos:definition """
No UEL input is used.  Corresponds to <i>UELin</i> not = 1 and not = 2 and not = 3 on the ExcST7B diagram. Original ExcST7B model would have called this <i>UELin</i> = 0.

\t"""@en .

cim:ExcST7BUELselectorKind.outputHVgate a owl:NamedIndividual, owl:Thing ;
  rdfs:label "outputHVgate "@en ;
  dy:isenum "True" ;
  rdfs:domain cim:ExcST7BUELselectorKind ;
  skos:definition """
The signal is connected into the output <i>HVGate</i>.  Corresponds to <i>UELin</i> = 3 on the ExcST7B diagram.

\t"""@en .

cim:FrancisGovernorControlKind.electromechanicalElectrohydraulic a owl:NamedIndividual, owl:Thing ;
  rdfs:label "electromechanicalElectrohydraulic "@en ;
  dy:isenum "True" ;
  rdfs:domain cim:FrancisGovernorControlKind ;
  skos:definition "Electromechanical and electrohydraulic regulator (Cflag=3)."@en .

cim:FrancisGovernorControlKind.mechanicHydraulicTransientFeedback a owl:NamedIndividual, owl:Thing ;
  rdfs:label "mechanicHydraulicTransientFeedback "@en ;
  dy:isenum "True" ;
  rdfs:domain cim:FrancisGovernorControlKind ;
  skos:definition "Mechanic-hydraulic regulator with transient feedback (Cflag=2)."@en .

cim:FrancisGovernorControlKind.mechanicHydrolicTachoAccelerator a owl:NamedIndividual, owl:Thing ;
  rdfs:label "mechanicHydrolicTachoAccelerator "@en ;
  dy:isenum "True" ;
  rdfs:domain cim:FrancisGovernorControlKind ;
  skos:definition "Mechanic-hydraulic regulator with tacho-accelerometer (Cflag = 1)."@en .

cim:GenericNonLinearLoadModelKind.exponentialRecovery a owl:NamedIndividual, owl:Thing ;
  rdfs:label "exponentialRecovery "@en ;
  dy:isenum "True" ;
  rdfs:domain cim:GenericNonLinearLoadModelKind ;
  skos:definition "Exponential recovery model."@en .

cim:GenericNonLinearLoadModelKind.loadAdaptive a owl:NamedIndividual, owl:Thing ;
  rdfs:label "loadAdaptive "@en ;
  dy:isenum "True" ;
  rdfs:domain cim:GenericNonLinearLoadModelKind ;
  skos:definition "Load adaptive model."@en .

cim:GovHydro4ModelKind.francisPelton a owl:NamedIndividual, owl:Thing ;
  rdfs:label "francisPelton "@en ;
  dy:isenum "True" ;
  rdfs:domain cim:GovHydro4ModelKind ;
  skos:definition "Francis or Pelton model."@en .

cim:GovHydro4ModelKind.kaplan a owl:NamedIndividual, owl:Thing ;
  rdfs:label "kaplan "@en ;
  dy:isenum "True" ;
  rdfs:domain cim:GovHydro4ModelKind ;
  skos:definition "Kaplan model."@en .

cim:GovHydro4ModelKind.simple a owl:NamedIndividual, owl:Thing ;
  rdfs:label "simple "@en ;
  dy:isenum "True" ;
  rdfs:domain cim:GovHydro4ModelKind ;
  skos:definition "Simple model."@en .

cim:IfdBaseKind.ifag a owl:NamedIndividual, owl:Thing ;
  rdfs:label "ifag "@en ;
  dy:isenum "True" ;
  rdfs:domain cim:IfdBaseKind ;
  skos:definition "Air gap line mode. "@en .

cim:IfdBaseKind.iffl a owl:NamedIndividual, owl:Thing ;
  rdfs:label "iffl "@en ;
  dy:isenum "True" ;
  rdfs:domain cim:IfdBaseKind ;
  skos:definition "Full load system mode. "@en .

cim:IfdBaseKind.ifnl a owl:NamedIndividual, owl:Thing ;
  rdfs:label "ifnl "@en ;
  dy:isenum "True" ;
  rdfs:domain cim:IfdBaseKind ;
  skos:definition "No load system with saturation mode. "@en .

cim:InputSignalKind.branchCurrent a owl:NamedIndividual, owl:Thing ;
  rdfs:label "branchCurrent "@en ;
  dy:isenum "True" ;
  rdfs:domain cim:InputSignalKind ;
  skos:definition "Input signal is amplitude of remote branch current."@en .

cim:InputSignalKind.busFrequency a owl:NamedIndividual, owl:Thing ;
  rdfs:label "busFrequency "@en ;
  dy:isenum "True" ;
  rdfs:domain cim:InputSignalKind ;
  skos:definition "Input signal is bus voltage fr<font color=\"#0f0f0f\">equency.  This could be a terminal frequency or remote frequency.</font>"@en .

cim:InputSignalKind.busFrequencyDeviation a owl:NamedIndividual, owl:Thing ;
  rdfs:label "busFrequencyDeviation "@en ;
  dy:isenum "True" ;
  rdfs:domain cim:InputSignalKind ;
  skos:definition "Input signal is deviation of bus voltage frequ<font color=\"#0f0f0f\">ency.  This could be a terminal frequency deviation or remote frequency deviation.</font>"@en .

cim:InputSignalKind.busVoltage a owl:NamedIndividual, owl:Thing ;
  rdfs:label "busVoltage "@en ;
  dy:isenum "True" ;
  rdfs:domain cim:InputSignalKind ;
  skos:definition "Input signal <font color=\"#0f0f0f\">is bus voltage.  This could be a terminal voltage or remote voltage.</font>"@en .

cim:InputSignalKind.busVoltageDerivative a owl:NamedIndividual, owl:Thing ;
  rdfs:label "busVoltageDerivative "@en ;
  dy:isenum "True" ;
  rdfs:domain cim:InputSignalKind ;
  skos:definition "Input signal is derivative of bus voltag<font color=\"#0f0f0f\">e.  This could be a terminal voltage derivative or remote voltage derivative.</font>"@en .

cim:InputSignalKind.fieldCurrent a owl:NamedIndividual, owl:Thing ;
  rdfs:label "fieldCurrent "@en ;
  dy:isenum "True" ;
  rdfs:domain cim:InputSignalKind ;
  skos:definition "Input signal is generator field current."@en .

cim:InputSignalKind.generatorAcceleratingPower a owl:NamedIndividual, owl:Thing ;
  rdfs:label "generatorAcceleratingPower "@en ;
  dy:isenum "True" ;
  rdfs:domain cim:InputSignalKind ;
  skos:definition "Input signal is generator accelerating power."@en .

cim:InputSignalKind.generatorElectricalPower a owl:NamedIndividual, owl:Thing ;
  rdfs:label "generatorElectricalPower "@en ;
  dy:isenum "True" ;
  rdfs:domain cim:InputSignalKind ;
  skos:definition "Input signal is generator electrical power on rated <i>S</i>."@en .

cim:InputSignalKind.generatorMechanicalPower a owl:NamedIndividual, owl:Thing ;
  rdfs:label "generatorMechanicalPower "@en ;
  dy:isenum "True" ;
  rdfs:domain cim:InputSignalKind ;
  skos:definition """
Input signal is generator mechanical power.

\t"""@en .

cim:InputSignalKind.rotorAngularFrequencyDeviation a owl:NamedIndividual, owl:Thing ;
  rdfs:label "rotorAngularFrequencyDeviation "@en ;
  dy:isenum "True" ;
  rdfs:domain cim:InputSignalKind ;
  skos:definition "Input signal is rotor or shaft angular frequency deviation."@en .

cim:InputSignalKind.rotorSpeed a owl:NamedIndividual, owl:Thing ;
  rdfs:label "rotorSpeed "@en ;
  dy:isenum "True" ;
  rdfs:domain cim:InputSignalKind ;
  skos:definition "Input signal is rotor or shaft speed (angular frequency)."@en .

cim:RemoteSignalKind.remoteBranchCurrentAmplitude a owl:NamedIndividual, owl:Thing ;
  rdfs:label "remoteBranchCurrentAmplitude "@en ;
  dy:isenum "True" ;
  rdfs:domain cim:RemoteSignalKind ;
  skos:definition "Input is branch current amplitude from remote terminal bus."@en .

cim:RemoteSignalKind.remoteBusFrequency a owl:NamedIndividual, owl:Thing ;
  rdfs:label "remoteBusFrequency "@en ;
  dy:isenum "True" ;
  rdfs:domain cim:RemoteSignalKind ;
  skos:definition "Input is frequency from remote terminal bus."@en .

cim:RemoteSignalKind.remoteBusFrequencyDeviation a owl:NamedIndividual, owl:Thing ;
  rdfs:label "remoteBusFrequencyDeviation "@en ;
  dy:isenum "True" ;
  rdfs:domain cim:RemoteSignalKind ;
  skos:definition "Input is frequency deviation from remote terminal bus."@en .

cim:RemoteSignalKind.remoteBusVoltage a owl:NamedIndividual, owl:Thing ;
  rdfs:label "remoteBusVoltage "@en ;
  dy:isenum "True" ;
  rdfs:domain cim:RemoteSignalKind ;
  skos:definition "Input is voltage from remote terminal bus."@en .

cim:RemoteSignalKind.remoteBusVoltageAmplitude a owl:NamedIndividual, owl:Thing ;
  rdfs:label "remoteBusVoltageAmplitude "@en ;
  dy:isenum "True" ;
  rdfs:domain cim:RemoteSignalKind ;
  skos:definition "Input is voltage amplitude from remote terminal bus."@en .

cim:RemoteSignalKind.remoteBusVoltageAmplitudeDerivative a owl:NamedIndividual, owl:Thing ;
  rdfs:label "remoteBusVoltageAmplitudeDerivative "@en ;
  dy:isenum "True" ;
  rdfs:domain cim:RemoteSignalKind ;
  skos:definition "Input is branch current amplitude derivative from remote terminal bus."@en .

cim:RemoteSignalKind.remoteBusVoltageFrequency a owl:NamedIndividual, owl:Thing ;
  rdfs:label "remoteBusVoltageFrequency "@en ;
  dy:isenum "True" ;
  rdfs:domain cim:RemoteSignalKind ;
  skos:definition "Input is voltage frequency from remote terminal bus."@en .

cim:RemoteSignalKind.remoteBusVoltageFrequencyDeviation a owl:NamedIndividual, owl:Thing ;
  rdfs:label "remoteBusVoltageFrequencyDeviation "@en ;
  dy:isenum "True" ;
  rdfs:domain cim:RemoteSignalKind ;
  skos:definition "Input is voltage frequency deviation from remote terminal bus."@en .

cim:RemoteSignalKind.remotePuBusVoltageDerivative a owl:NamedIndividual, owl:Thing ;
  rdfs:label "remotePuBusVoltageDerivative "@en ;
  dy:isenum "True" ;
  rdfs:domain cim:RemoteSignalKind ;
  skos:definition "Input is PU voltage derivative from remote terminal bus."@en .

cim:RotorKind.roundRotor a owl:NamedIndividual, owl:Thing ;
  rdfs:label "roundRotor "@en ;
  dy:isenum "True" ;
  rdfs:domain cim:RotorKind ;
  skos:definition "Round rotor type of synchronous machine."@en .

cim:RotorKind.salientPole a owl:NamedIndividual, owl:Thing ;
  rdfs:label "salientPole "@en ;
  dy:isenum "True" ;
  rdfs:domain cim:RotorKind ;
  skos:definition "Salient pole type of synchronous machine."@en .

cim:StaticLoadModelKind.constantZ a owl:NamedIndividual, owl:Thing ;
  rdfs:label "constantZ "@en ;
  dy:isenum "True" ;
  rdfs:domain cim:StaticLoadModelKind ;
  skos:definition "The load is represented as a constant impedance.  ConstantZ equations are used  for active and reactive power and no attributes are required."@en .

cim:StaticLoadModelKind.exponential a owl:NamedIndividual, owl:Thing ;
  rdfs:label "exponential "@en ;
  dy:isenum "True" ;
  rdfs:domain cim:StaticLoadModelKind ;
  skos:definition """
This model is an exponential representation of the load. Exponential equations for active and reactive power are used and the following attributes are required:
kp1, kp2, kp3, kpf, ep1, ep2, ep3
kq1, kq2, kq3, kqf, eq1, eq2, eq3.
\t"""@en .

cim:StaticLoadModelKind.zIP1 a owl:NamedIndividual, owl:Thing ;
  rdfs:label "zIP1 "@en ;
  dy:isenum "True" ;
  rdfs:domain cim:StaticLoadModelKind ;
  skos:definition """
This model integrates the frequency-dependent load (primarily motors).  ZIP1 equations for active and reactive power are used and the following attributes are required:
kp1, kp2, kp3, kpf
kq1, kq2, kq3, kqf.
\t"""@en .

cim:StaticLoadModelKind.zIP2 a owl:NamedIndividual, owl:Thing ;
  rdfs:label "zIP2 "@en ;
  dy:isenum "True" ;
  rdfs:domain cim:StaticLoadModelKind ;
  skos:definition """
This model separates the frequency-dependent load (primarily motors) from other load.  ZIP2 equations for active and reactive power are used and the following attributes are required:
kp1, kp2, kp3, kq4, kpf
kq1, kq2, kq3, kq4, kqf.
\t"""@en .

cim:SynchronousMachineModelKind.subtransient a owl:NamedIndividual, owl:Thing ;
  rdfs:label "subtransient "@en ;
  dy:isenum "True" ;
  rdfs:domain cim:SynchronousMachineModelKind ;
  skos:definition "Subtransient synchronous machine model."@en .

cim:SynchronousMachineModelKind.subtransientSimplified a owl:NamedIndividual, owl:Thing ;
  rdfs:label "subtransientSimplified "@en ;
  dy:isenum "True" ;
  rdfs:domain cim:SynchronousMachineModelKind ;
  skos:definition "Simplified version of subtransient synchronous machine model where magnetic coupling between the direct- and quadrature- axes is ignored."@en .

cim:SynchronousMachineModelKind.subtransientSimplifiedDirectAxis a owl:NamedIndividual, owl:Thing ;
  rdfs:label "subtransientSimplifiedDirectAxis "@en ;
  dy:isenum "True" ;
  rdfs:domain cim:SynchronousMachineModelKind ;
  skos:definition "Simplified version of a subtransient synchronous machine model with no damper circuit on the direct-axis. "@en .

cim:SynchronousMachineModelKind.subtransientTypeF a owl:NamedIndividual, owl:Thing ;
  rdfs:label "subtransientTypeF "@en ;
  dy:isenum "True" ;
  rdfs:domain cim:SynchronousMachineModelKind ;
  skos:definition "WECC type F variant of subtransient synchronous machine model."@en .

cim:SynchronousMachineModelKind.subtransientTypeJ a owl:NamedIndividual, owl:Thing ;
  rdfs:label "subtransientTypeJ "@en ;
  dy:isenum "True" ;
  rdfs:domain cim:SynchronousMachineModelKind ;
  skos:definition "WECC type J variant of subtransient synchronous machine model."@en .

cim:UnitMultiplier.E a owl:NamedIndividual, owl:Thing ;
  rdfs:label "E "@en ;
  dy:isenum "True" ;
  rdfs:domain cim:UnitMultiplier ;
  skos:definition "Exa 10**18."@en .

cim:UnitMultiplier.G a owl:NamedIndividual, owl:Thing ;
  rdfs:label "G "@en ;
  dy:isenum "True" ;
  rdfs:domain cim:UnitMultiplier ;
  skos:definition "Giga 10**9."@en .

cim:UnitMultiplier.M a owl:NamedIndividual, owl:Thing ;
  rdfs:label "M "@en ;
  dy:isenum "True" ;
  rdfs:domain cim:UnitMultiplier ;
  skos:definition "Mega 10**6."@en .

cim:UnitMultiplier.P a owl:NamedIndividual, owl:Thing ;
  rdfs:label "P "@en ;
  dy:isenum "True" ;
  rdfs:domain cim:UnitMultiplier ;
  skos:definition "Peta 10**15."@en .

cim:UnitMultiplier.T a owl:NamedIndividual, owl:Thing ;
  rdfs:label "T "@en ;
  dy:isenum "True" ;
  rdfs:domain cim:UnitMultiplier ;
  skos:definition "Tera 10**12."@en .

cim:UnitMultiplier.Y a owl:NamedIndividual, owl:Thing ;
  rdfs:label "Y "@en ;
  dy:isenum "True" ;
  rdfs:domain cim:UnitMultiplier ;
  skos:definition "Yotta 10**24."@en .

cim:UnitMultiplier.Z a owl:NamedIndividual, owl:Thing ;
  rdfs:label "Z "@en ;
  dy:isenum "True" ;
  rdfs:domain cim:UnitMultiplier ;
  skos:definition "Zetta 10**21."@en .

cim:UnitMultiplier.a a owl:NamedIndividual, owl:Thing ;
  rdfs:label "a "@en ;
  dy:isenum "True" ;
  rdfs:domain cim:UnitMultiplier ;
  skos:definition "Atto 10**-18."@en .

cim:UnitMultiplier.c a owl:NamedIndividual, owl:Thing ;
  rdfs:label "c "@en ;
  dy:isenum "True" ;
  rdfs:domain cim:UnitMultiplier ;
  skos:definition "Centi 10**-2."@en .

cim:UnitMultiplier.d a owl:NamedIndividual, owl:Thing ;
  rdfs:label "d "@en ;
  dy:isenum "True" ;
  rdfs:domain cim:UnitMultiplier ;
  skos:definition "Deci 10**-1."@en .

cim:UnitMultiplier.da a owl:NamedIndividual, owl:Thing ;
  rdfs:label "da "@en ;
  dy:isenum "True" ;
  rdfs:domain cim:UnitMultiplier ;
  skos:definition "Deca 10**1."@en .

cim:UnitMultiplier.f a owl:NamedIndividual, owl:Thing ;
  rdfs:label "f "@en ;
  dy:isenum "True" ;
  rdfs:domain cim:UnitMultiplier ;
  skos:definition "Femto 10**-15."@en .

cim:UnitMultiplier.h a owl:NamedIndividual, owl:Thing ;
  rdfs:label "h "@en ;
  dy:isenum "True" ;
  rdfs:domain cim:UnitMultiplier ;
  skos:definition "Hecto 10**2."@en .

cim:UnitMultiplier.k a owl:NamedIndividual, owl:Thing ;
  rdfs:label "k "@en ;
  dy:isenum "True" ;
  rdfs:domain cim:UnitMultiplier ;
  skos:definition "Kilo 10**3."@en .

cim:UnitMultiplier.m a owl:NamedIndividual, owl:Thing ;
  rdfs:label "m "@en ;
  dy:isenum "True" ;
  rdfs:domain cim:UnitMultiplier ;
  skos:definition "Milli 10**-3."@en .

cim:UnitMultiplier.micro a owl:NamedIndividual, owl:Thing ;
  rdfs:label "micro "@en ;
  dy:isenum "True" ;
  rdfs:domain cim:UnitMultiplier ;
  skos:definition "Micro 10**-6."@en .

cim:UnitMultiplier.n a owl:NamedIndividual, owl:Thing ;
  rdfs:label "n "@en ;
  dy:isenum "True" ;
  rdfs:domain cim:UnitMultiplier ;
  skos:definition "Nano 10**-9."@en .

cim:UnitMultiplier.none a owl:NamedIndividual, owl:Thing ;
  rdfs:label "none "@en ;
  dy:isenum "True" ;
  rdfs:domain cim:UnitMultiplier ;
  skos:definition "No multiplier or equivalently multiply by 1."@en .

cim:UnitMultiplier.p a owl:NamedIndividual, owl:Thing ;
  rdfs:label "p "@en ;
  dy:isenum "True" ;
  rdfs:domain cim:UnitMultiplier ;
  skos:definition "Pico 10**-12."@en .

cim:UnitMultiplier.y a owl:NamedIndividual, owl:Thing ;
  rdfs:label "y "@en ;
  dy:isenum "True" ;
  rdfs:domain cim:UnitMultiplier ;
  skos:definition "Yocto 10**-24."@en .

cim:UnitMultiplier.z a owl:NamedIndividual, owl:Thing ;
  rdfs:label "z "@en ;
  dy:isenum "True" ;
  rdfs:domain cim:UnitMultiplier ;
  skos:definition "Zepto 10**-21."@en .

cim:UnitSymbol.A a owl:NamedIndividual, owl:Thing ;
  rdfs:label "A "@en ;
  dy:isenum "True" ;
  rdfs:domain cim:UnitSymbol ;
  skos:definition "Current in amperes."@en .

cim:UnitSymbol.A2 a owl:NamedIndividual, owl:Thing ;
  rdfs:label "A2 "@en ;
  dy:isenum "True" ;
  rdfs:domain cim:UnitSymbol ;
  skos:definition "Amperes squared (A²)."@en .

cim:UnitSymbol.A2h a owl:NamedIndividual, owl:Thing ;
  rdfs:label "A2h "@en ;
  dy:isenum "True" ;
  rdfs:domain cim:UnitSymbol ;
  skos:definition "Ampere-squared hour, ampere-squared hour."@en .

cim:UnitSymbol.A2s a owl:NamedIndividual, owl:Thing ;
  rdfs:label "A2s "@en ;
  dy:isenum "True" ;
  rdfs:domain cim:UnitSymbol ;
  skos:definition "Ampere squared time in square amperes (A²s)."@en .

cim:UnitSymbol.APerA a owl:NamedIndividual, owl:Thing ;
  rdfs:label "APerA "@en ;
  dy:isenum "True" ;
  rdfs:domain cim:UnitSymbol ;
  skos:definition "Current, ratio of amperages.   Note: Users may need to supply a prefix such as ‘m’ to show rates such as ‘mA/A’."@en .

cim:UnitSymbol.APerm a owl:NamedIndividual, owl:Thing ;
  rdfs:label "APerm "@en ;
  dy:isenum "True" ;
  rdfs:domain cim:UnitSymbol ;
  skos:definition "A/m, magnetic field strength, amperes per metre."@en .

cim:UnitSymbol.Ah a owl:NamedIndividual, owl:Thing ;
  rdfs:label "Ah "@en ;
  dy:isenum "True" ;
  rdfs:domain cim:UnitSymbol ;
  skos:definition "Ampere-hours, ampere-hours."@en .

cim:UnitSymbol.As a owl:NamedIndividual, owl:Thing ;
  rdfs:label "As "@en ;
  dy:isenum "True" ;
  rdfs:domain cim:UnitSymbol ;
  skos:definition "Ampere seconds (A·s)."@en .

cim:UnitSymbol.Bq a owl:NamedIndividual, owl:Thing ;
  rdfs:label "Bq "@en ;
  dy:isenum "True" ;
  rdfs:domain cim:UnitSymbol ;
  skos:definition "Radioactivity in becquerels (1/s)."@en .

cim:UnitSymbol.Btu a owl:NamedIndividual, owl:Thing ;
  rdfs:label "Btu "@en ;
  dy:isenum "True" ;
  rdfs:domain cim:UnitSymbol ;
  skos:definition "Energy, British Thermal Units."@en .

cim:UnitSymbol.C a owl:NamedIndividual, owl:Thing ;
  rdfs:label "C "@en ;
  dy:isenum "True" ;
  rdfs:domain cim:UnitSymbol ;
  skos:definition "Electric charge in coulombs (A·s)."@en .

cim:UnitSymbol.CPerkg a owl:NamedIndividual, owl:Thing ;
  rdfs:label "CPerkg "@en ;
  dy:isenum "True" ;
  rdfs:domain cim:UnitSymbol ;
  skos:definition "Exposure (x rays), coulombs per kilogram."@en .

cim:UnitSymbol.CPerm2 a owl:NamedIndividual, owl:Thing ;
  rdfs:label "CPerm2 "@en ;
  dy:isenum "True" ;
  rdfs:domain cim:UnitSymbol ;
  skos:definition "Surface charge density, coulombs per square metre."@en .

cim:UnitSymbol.CPerm3 a owl:NamedIndividual, owl:Thing ;
  rdfs:label "CPerm3 "@en ;
  dy:isenum "True" ;
  rdfs:domain cim:UnitSymbol ;
  skos:definition "Electric charge density, coulombs per cubic metre."@en .

cim:UnitSymbol.F a owl:NamedIndividual, owl:Thing ;
  rdfs:label "F "@en ;
  dy:isenum "True" ;
  rdfs:domain cim:UnitSymbol ;
  skos:definition "Electric capacitance in farads (C/V)."@en .

cim:UnitSymbol.FPerm a owl:NamedIndividual, owl:Thing ;
  rdfs:label "FPerm "@en ;
  dy:isenum "True" ;
  rdfs:domain cim:UnitSymbol ;
  skos:definition "Permittivity, farads per metre."@en .

cim:UnitSymbol.G a owl:NamedIndividual, owl:Thing ;
  rdfs:label "G "@en ;
  dy:isenum "True" ;
  rdfs:domain cim:UnitSymbol ;
  skos:definition "Magnetic flux density, gausses (1 G = 10-4 T)."@en .

cim:UnitSymbol.Gy a owl:NamedIndividual, owl:Thing ;
  rdfs:label "Gy "@en ;
  dy:isenum "True" ;
  rdfs:domain cim:UnitSymbol ;
  skos:definition "Absorbed dose in grays (J/kg)."@en .

cim:UnitSymbol.GyPers a owl:NamedIndividual, owl:Thing ;
  rdfs:label "GyPers "@en ;
  dy:isenum "True" ;
  rdfs:domain cim:UnitSymbol ;
  skos:definition "Absorbed dose rate, grays per second."@en .

cim:UnitSymbol.H a owl:NamedIndividual, owl:Thing ;
  rdfs:label "H "@en ;
  dy:isenum "True" ;
  rdfs:domain cim:UnitSymbol ;
  skos:definition "Electric inductance in henrys (Wb/A)."@en .

cim:UnitSymbol.HPerm a owl:NamedIndividual, owl:Thing ;
  rdfs:label "HPerm "@en ;
  dy:isenum "True" ;
  rdfs:domain cim:UnitSymbol ;
  skos:definition "Permeability, henrys per metre."@en .

cim:UnitSymbol.Hz a owl:NamedIndividual, owl:Thing ;
  rdfs:label "Hz "@en ;
  dy:isenum "True" ;
  rdfs:domain cim:UnitSymbol ;
  skos:definition "Frequency in hertz (1/s)."@en .

cim:UnitSymbol.HzPerHz a owl:NamedIndividual, owl:Thing ;
  rdfs:label "HzPerHz "@en ;
  dy:isenum "True" ;
  rdfs:domain cim:UnitSymbol ;
  skos:definition "Frequency, rate of frequency change.   Note: Users may need to supply a prefix such as ‘m’ to show rates such as ‘mHz/Hz’."@en .

cim:UnitSymbol.HzPers a owl:NamedIndividual, owl:Thing ;
  rdfs:label "HzPers "@en ;
  dy:isenum "True" ;
  rdfs:domain cim:UnitSymbol ;
  skos:definition "Rate of change of frequency in hertz per second."@en .

cim:UnitSymbol.J a owl:NamedIndividual, owl:Thing ;
  rdfs:label "J "@en ;
  dy:isenum "True" ;
  rdfs:domain cim:UnitSymbol ;
  skos:definition "Energy in joules (N·m = C·V = W·s)."@en .

cim:UnitSymbol.JPerK a owl:NamedIndividual, owl:Thing ;
  rdfs:label "JPerK "@en ;
  dy:isenum "True" ;
  rdfs:domain cim:UnitSymbol ;
  skos:definition "Heat capacity in joules/kelvin."@en .

cim:UnitSymbol.JPerkg a owl:NamedIndividual, owl:Thing ;
  rdfs:label "JPerkg "@en ;
  dy:isenum "True" ;
  rdfs:domain cim:UnitSymbol ;
  skos:definition "Specific energy, Joules / kg."@en .

cim:UnitSymbol.JPerkgK a owl:NamedIndividual, owl:Thing ;
  rdfs:label "JPerkgK "@en ;
  dy:isenum "True" ;
  rdfs:domain cim:UnitSymbol ;
  skos:definition "Specific heat capacity, specific entropy, joules per kilogram Kelvin."@en .

cim:UnitSymbol.JPerm2 a owl:NamedIndividual, owl:Thing ;
  rdfs:label "JPerm2 "@en ;
  dy:isenum "True" ;
  rdfs:domain cim:UnitSymbol ;
  skos:definition "Insulation energy density, joules per square metre or watt second per square metre."@en .

cim:UnitSymbol.JPerm3 a owl:NamedIndividual, owl:Thing ;
  rdfs:label "JPerm3 "@en ;
  dy:isenum "True" ;
  rdfs:domain cim:UnitSymbol ;
  skos:definition "Energy density, joules per cubic metre."@en .

cim:UnitSymbol.JPermol a owl:NamedIndividual, owl:Thing ;
  rdfs:label "JPermol "@en ;
  dy:isenum "True" ;
  rdfs:domain cim:UnitSymbol ;
  skos:definition "Molar energy, joules per mole."@en .

cim:UnitSymbol.JPermolK a owl:NamedIndividual, owl:Thing ;
  rdfs:label "JPermolK "@en ;
  dy:isenum "True" ;
  rdfs:domain cim:UnitSymbol ;
  skos:definition "Molar entropy, molar heat capacity, joules per mole kelvin."@en .

cim:UnitSymbol.JPers a owl:NamedIndividual, owl:Thing ;
  rdfs:label "JPers "@en ;
  dy:isenum "True" ;
  rdfs:domain cim:UnitSymbol ;
  skos:definition "Energy rate in joules per second (J/s)."@en .

cim:UnitSymbol.K a owl:NamedIndividual, owl:Thing ;
  rdfs:label "K "@en ;
  dy:isenum "True" ;
  rdfs:domain cim:UnitSymbol ;
  skos:definition "Temperature in kelvins."@en .

cim:UnitSymbol.KPers a owl:NamedIndividual, owl:Thing ;
  rdfs:label "KPers "@en ;
  dy:isenum "True" ;
  rdfs:domain cim:UnitSymbol ;
  skos:definition "Temperature change rate in kelvins per second."@en .

cim:UnitSymbol.M a owl:NamedIndividual, owl:Thing ;
  rdfs:label "M "@en ;
  dy:isenum "True" ;
  rdfs:domain cim:UnitSymbol ;
  skos:definition "Length, nautical miles (1 M = 1852 m)."@en .

cim:UnitSymbol.Mx a owl:NamedIndividual, owl:Thing ;
  rdfs:label "Mx "@en ;
  dy:isenum "True" ;
  rdfs:domain cim:UnitSymbol ;
  skos:definition "Magnetic flux, maxwells (1 Mx = 10-8 Wb)."@en .

cim:UnitSymbol.N a owl:NamedIndividual, owl:Thing ;
  rdfs:label "N "@en ;
  dy:isenum "True" ;
  rdfs:domain cim:UnitSymbol ;
  skos:definition "Force in newtons (kg·m/s²)."@en .

cim:UnitSymbol.NPerm a owl:NamedIndividual, owl:Thing ;
  rdfs:label "NPerm "@en ;
  dy:isenum "True" ;
  rdfs:domain cim:UnitSymbol ;
  skos:definition "Surface tension, newton per metre."@en .

cim:UnitSymbol.Nm a owl:NamedIndividual, owl:Thing ;
  rdfs:label "Nm "@en ;
  dy:isenum "True" ;
  rdfs:domain cim:UnitSymbol ;
  skos:definition "Moment of force, newton metres."@en .

cim:UnitSymbol.Oe a owl:NamedIndividual, owl:Thing ;
  rdfs:label "Oe "@en ;
  dy:isenum "True" ;
  rdfs:domain cim:UnitSymbol ;
  skos:definition "Magnetic field in oersteds, (1 Oe = (103/4p) A/m)."@en .

cim:UnitSymbol.Pa a owl:NamedIndividual, owl:Thing ;
  rdfs:label "Pa "@en ;
  dy:isenum "True" ;
  rdfs:domain cim:UnitSymbol ;
  skos:definition "Pressure in pascals (N/m²). Note: the absolute or relative measurement of pressure is implied with this entry. See below for more explicit forms."@en .

cim:UnitSymbol.PaPers a owl:NamedIndividual, owl:Thing ;
  rdfs:label "PaPers "@en ;
  dy:isenum "True" ;
  rdfs:domain cim:UnitSymbol ;
  skos:definition "Pressure change rate in pascals per second."@en .

cim:UnitSymbol.Pas a owl:NamedIndividual, owl:Thing ;
  rdfs:label "Pas "@en ;
  dy:isenum "True" ;
  rdfs:domain cim:UnitSymbol ;
  skos:definition "Dynamic viscosity, pascal seconds."@en .

cim:UnitSymbol.Q a owl:NamedIndividual, owl:Thing ;
  rdfs:label "Q "@en ;
  dy:isenum "True" ;
  rdfs:domain cim:UnitSymbol ;
  skos:definition "Quantity power, Q."@en .

cim:UnitSymbol.Qh a owl:NamedIndividual, owl:Thing ;
  rdfs:label "Qh "@en ;
  dy:isenum "True" ;
  rdfs:domain cim:UnitSymbol ;
  skos:definition "Quantity energy, Qh."@en .

cim:UnitSymbol.S a owl:NamedIndividual, owl:Thing ;
  rdfs:label "S "@en ;
  dy:isenum "True" ;
  rdfs:domain cim:UnitSymbol ;
  skos:definition "Conductance in siemens."@en .

cim:UnitSymbol.SPerm a owl:NamedIndividual, owl:Thing ;
  rdfs:label "SPerm "@en ;
  dy:isenum "True" ;
  rdfs:domain cim:UnitSymbol ;
  skos:definition "Conductance per length (F/m)."@en .

cim:UnitSymbol.Sv a owl:NamedIndividual, owl:Thing ;
  rdfs:label "Sv "@en ;
  dy:isenum "True" ;
  rdfs:domain cim:UnitSymbol ;
  skos:definition "Dose equivalent in sieverts (J/kg)."@en .

cim:UnitSymbol.T a owl:NamedIndividual, owl:Thing ;
  rdfs:label "T "@en ;
  dy:isenum "True" ;
  rdfs:domain cim:UnitSymbol ;
  skos:definition "Magnetic flux density in teslas (Wb/m2)."@en .

cim:UnitSymbol.V a owl:NamedIndividual, owl:Thing ;
  rdfs:label "V "@en ;
  dy:isenum "True" ;
  rdfs:domain cim:UnitSymbol ;
  skos:definition "Electric potential in volts (W/A)."@en .

cim:UnitSymbol.V2 a owl:NamedIndividual, owl:Thing ;
  rdfs:label "V2 "@en ;
  dy:isenum "True" ;
  rdfs:domain cim:UnitSymbol ;
  skos:definition "Volt squared (W²/A²)."@en .

cim:UnitSymbol.V2h a owl:NamedIndividual, owl:Thing ;
  rdfs:label "V2h "@en ;
  dy:isenum "True" ;
  rdfs:domain cim:UnitSymbol ;
  skos:definition "Volt-squared hour, volt-squared-hours."@en .

cim:UnitSymbol.VA a owl:NamedIndividual, owl:Thing ;
  rdfs:label "VA "@en ;
  dy:isenum "True" ;
  rdfs:domain cim:UnitSymbol ;
  skos:definition "Apparent power in volt amperes. See also real power and reactive power."@en .

cim:UnitSymbol.VAh a owl:NamedIndividual, owl:Thing ;
  rdfs:label "VAh "@en ;
  dy:isenum "True" ;
  rdfs:domain cim:UnitSymbol ;
  skos:definition "Apparent energy in volt ampere hours."@en .

cim:UnitSymbol.VAr a owl:NamedIndividual, owl:Thing ;
  rdfs:label "VAr "@en ;
  dy:isenum "True" ;
  rdfs:domain cim:UnitSymbol ;
  skos:definition """
Reactive power in volt amperes reactive. The “reactive” or “imaginary” component of electrical power (VIsin(phi)). (See also real power and apparent power).
Note: Different meter designs use different methods to arrive at their results. Some meters may compute reactive power as an arithmetic value, while others compute the value vectorially. The data consumer should determine the method in use and the suitability of the measurement for the intended purpose.
\t"""@en .

cim:UnitSymbol.VArh a owl:NamedIndividual, owl:Thing ;
  rdfs:label "VArh "@en ;
  dy:isenum "True" ;
  rdfs:domain cim:UnitSymbol ;
  skos:definition "Reactive energy in volt ampere reactive hours."@en .

cim:UnitSymbol.VPerHz a owl:NamedIndividual, owl:Thing ;
  rdfs:label "VPerHz "@en ;
  dy:isenum "True" ;
  rdfs:domain cim:UnitSymbol ;
  skos:definition "Magnetic flux in volt per hertz."@en .

cim:UnitSymbol.VPerV a owl:NamedIndividual, owl:Thing ;
  rdfs:label "VPerV "@en ;
  dy:isenum "True" ;
  rdfs:domain cim:UnitSymbol ;
  skos:definition "Voltage, ratio of voltages.  Note: Users may need to supply a prefix such as ‘m’ to show rates such as ‘mV/V’."@en .

cim:UnitSymbol.VPerVA a owl:NamedIndividual, owl:Thing ;
  rdfs:label "VPerVA "@en ;
  dy:isenum "True" ;
  rdfs:domain cim:UnitSymbol ;
  skos:definition "Power factor, PF, the ratio of the active power to the apparent power.  Note: The sign convention used for power factor will differ between IEC meters and EEI (ANSI) meters. It is assumed that the data consumers understand the type of meter being used and agree on the sign convention in use at any given utility."@en .

cim:UnitSymbol.VPerVAr a owl:NamedIndividual, owl:Thing ;
  rdfs:label "VPerVAr "@en ;
  dy:isenum "True" ;
  rdfs:domain cim:UnitSymbol ;
  skos:definition "Power factor, PF, the ratio of the active power to the apparent power. Note: The sign convention used for power factor will differ between IEC meters and EEI (ANSI) meters. It is assumed that the data consumers understand the type of meter being used and agree on the sign convention in use at any given utility."@en .

cim:UnitSymbol.VPerm a owl:NamedIndividual, owl:Thing ;
  rdfs:label "VPerm "@en ;
  dy:isenum "True" ;
  rdfs:domain cim:UnitSymbol ;
  skos:definition "Electric field strength, volts per metre."@en .

cim:UnitSymbol.Vh a owl:NamedIndividual, owl:Thing ;
  rdfs:label "Vh "@en ;
  dy:isenum "True" ;
  rdfs:domain cim:UnitSymbol ;
  skos:definition "Volt-hour, Volt hours."@en .

cim:UnitSymbol.Vs a owl:NamedIndividual, owl:Thing ;
  rdfs:label "Vs "@en ;
  dy:isenum "True" ;
  rdfs:domain cim:UnitSymbol ;
  skos:definition "Volt seconds (Ws/A)."@en .

cim:UnitSymbol.W a owl:NamedIndividual, owl:Thing ;
  rdfs:label "W "@en ;
  dy:isenum "True" ;
  rdfs:domain cim:UnitSymbol ;
  skos:definition "Real power in watts (J/s). Electrical power may have real and reactive components. The real portion of electrical power (I&#178;R or VIcos(phi)), is expressed in Watts. See also apparent power and reactive power."@en .

cim:UnitSymbol.WPerA a owl:NamedIndividual, owl:Thing ;
  rdfs:label "WPerA "@en ;
  dy:isenum "True" ;
  rdfs:domain cim:UnitSymbol ;
  skos:definition "Active power per current flow, watts per Ampere."@en .

cim:UnitSymbol.WPerW a owl:NamedIndividual, owl:Thing ;
  rdfs:label "WPerW "@en ;
  dy:isenum "True" ;
  rdfs:domain cim:UnitSymbol ;
  skos:definition "Signal Strength, ratio of power.   Note: Users may need to supply a prefix such as ‘m’ to show rates such as ‘mW/W’."@en .

cim:UnitSymbol.WPerm2 a owl:NamedIndividual, owl:Thing ;
  rdfs:label "WPerm2 "@en ;
  dy:isenum "True" ;
  rdfs:domain cim:UnitSymbol ;
  skos:definition "Heat flux density, irradiance, watts per square metre."@en .

cim:UnitSymbol.WPerm2sr a owl:NamedIndividual, owl:Thing ;
  rdfs:label "WPerm2sr "@en ;
  dy:isenum "True" ;
  rdfs:domain cim:UnitSymbol ;
  skos:definition "Radiance, watts per square metre steradian."@en .

cim:UnitSymbol.WPermK a owl:NamedIndividual, owl:Thing ;
  rdfs:label "WPermK "@en ;
  dy:isenum "True" ;
  rdfs:domain cim:UnitSymbol ;
  skos:definition "Thermal conductivity in watt/metres kelvin."@en .

cim:UnitSymbol.WPers a owl:NamedIndividual, owl:Thing ;
  rdfs:label "WPers "@en ;
  dy:isenum "True" ;
  rdfs:domain cim:UnitSymbol ;
  skos:definition "Ramp rate in watts per second."@en .

cim:UnitSymbol.WPersr a owl:NamedIndividual, owl:Thing ;
  rdfs:label "WPersr "@en ;
  dy:isenum "True" ;
  rdfs:domain cim:UnitSymbol ;
  skos:definition "Radiant intensity, watts per steradian."@en .

cim:UnitSymbol.Wb a owl:NamedIndividual, owl:Thing ;
  rdfs:label "Wb "@en ;
  dy:isenum "True" ;
  rdfs:domain cim:UnitSymbol ;
  skos:definition "Magnetic flux in webers (V·s)."@en .

cim:UnitSymbol.Wh a owl:NamedIndividual, owl:Thing ;
  rdfs:label "Wh "@en ;
  dy:isenum "True" ;
  rdfs:domain cim:UnitSymbol ;
  skos:definition "Real energy in watt hours."@en .

cim:UnitSymbol.anglemin a owl:NamedIndividual, owl:Thing ;
  rdfs:label "anglemin "@en ;
  dy:isenum "True" ;
  rdfs:domain cim:UnitSymbol ;
  skos:definition "Plane angle, minutes."@en .

cim:UnitSymbol.anglesec a owl:NamedIndividual, owl:Thing ;
  rdfs:label "anglesec "@en ;
  dy:isenum "True" ;
  rdfs:domain cim:UnitSymbol ;
  skos:definition "Plane angle, seconds."@en .

cim:UnitSymbol.bar a owl:NamedIndividual, owl:Thing ;
  rdfs:label "bar "@en ;
  dy:isenum "True" ;
  rdfs:domain cim:UnitSymbol ;
  skos:definition "Pressure in bars, (1 bar = 100 kPa)."@en .

cim:UnitSymbol.cd a owl:NamedIndividual, owl:Thing ;
  rdfs:label "cd "@en ;
  dy:isenum "True" ;
  rdfs:domain cim:UnitSymbol ;
  skos:definition "Luminous intensity in candelas."@en .

cim:UnitSymbol.charPers a owl:NamedIndividual, owl:Thing ;
  rdfs:label "charPers "@en ;
  dy:isenum "True" ;
  rdfs:domain cim:UnitSymbol ;
  skos:definition "Data rate (baud) in characters per second."@en .

cim:UnitSymbol.character a owl:NamedIndividual, owl:Thing ;
  rdfs:label "character "@en ;
  dy:isenum "True" ;
  rdfs:domain cim:UnitSymbol ;
  skos:definition "Number of characters."@en .

cim:UnitSymbol.cosPhi a owl:NamedIndividual, owl:Thing ;
  rdfs:label "cosPhi "@en ;
  dy:isenum "True" ;
  rdfs:domain cim:UnitSymbol ;
  skos:definition """
Power factor, dimensionless.
Note 1: This definition of power factor only holds for balanced systems. See the alternative definition under code 153.
Note 2 : Beware of differing sign conventions in use between the IEC and EEI. It is assumed that the data consumer understands the type of meter in use and the sign convention in use by the utility.
\t"""@en .

cim:UnitSymbol.count a owl:NamedIndividual, owl:Thing ;
  rdfs:label "count "@en ;
  dy:isenum "True" ;
  rdfs:domain cim:UnitSymbol ;
  skos:definition "Amount of substance, Counter value."@en .

cim:UnitSymbol.d a owl:NamedIndividual, owl:Thing ;
  rdfs:label "d "@en ;
  dy:isenum "True" ;
  rdfs:domain cim:UnitSymbol ;
  skos:definition "Time in days, day = 24 h = 86400 s."@en .

cim:UnitSymbol.dB a owl:NamedIndividual, owl:Thing ;
  rdfs:label "dB "@en ;
  dy:isenum "True" ;
  rdfs:domain cim:UnitSymbol ;
  skos:definition "Sound pressure level in decibels. Note:  multiplier “d” is included in this unit symbol for compatibility with IEC 61850-7-3."@en .

cim:UnitSymbol.dBm a owl:NamedIndividual, owl:Thing ;
  rdfs:label "dBm "@en ;
  dy:isenum "True" ;
  rdfs:domain cim:UnitSymbol ;
  skos:definition "Power level (logarithmic ratio of signal strength , Bel-mW), normalized to 1mW. Note:  multiplier “d” is included in this unit symbol for compatibility with IEC 61850-7-3."@en .

cim:UnitSymbol.deg a owl:NamedIndividual, owl:Thing ;
  rdfs:label "deg "@en ;
  dy:isenum "True" ;
  rdfs:domain cim:UnitSymbol ;
  skos:definition "Plane angle in degrees."@en .

cim:UnitSymbol.degC a owl:NamedIndividual, owl:Thing ;
  rdfs:label "degC "@en ;
  dy:isenum "True" ;
  rdfs:domain cim:UnitSymbol ;
  skos:definition """
Relative temperature in degrees Celsius.
In the SI unit system the symbol is °C. Electric charge is measured in coulomb that has the unit symbol C. To distinguish degree Celsius from coulomb the symbol used in the UML is degC. The reason for not using °C is that the special character ° is difficult to manage in software.
\t"""@en .

cim:UnitSymbol.ft3 a owl:NamedIndividual, owl:Thing ;
  rdfs:label "ft3 "@en ;
  dy:isenum "True" ;
  rdfs:domain cim:UnitSymbol ;
  skos:definition "Volume, cubic feet."@en .

cim:UnitSymbol.gPerg a owl:NamedIndividual, owl:Thing ;
  rdfs:label "gPerg "@en ;
  dy:isenum "True" ;
  rdfs:domain cim:UnitSymbol ;
  skos:definition "Concentration, The ratio of the mass of a solute divided by the mass of  the solution. Note: Users may need use a prefix such a ‘µ’ to express a quantity such as ‘µg/g’."@en .

cim:UnitSymbol.gal a owl:NamedIndividual, owl:Thing ;
  rdfs:label "gal "@en ;
  dy:isenum "True" ;
  rdfs:domain cim:UnitSymbol ;
  skos:definition "Volume in gallons, US gallon (1 gal = 231 in3 = 128 fl ounce)."@en .

cim:UnitSymbol.h a owl:NamedIndividual, owl:Thing ;
  rdfs:label "h "@en ;
  dy:isenum "True" ;
  rdfs:domain cim:UnitSymbol ;
  skos:definition "Time in hours, hour = 60 min = 3600 s."@en .

cim:UnitSymbol.ha a owl:NamedIndividual, owl:Thing ;
  rdfs:label "ha "@en ;
  dy:isenum "True" ;
  rdfs:domain cim:UnitSymbol ;
  skos:definition "Area, hectares."@en .

cim:UnitSymbol.kat a owl:NamedIndividual, owl:Thing ;
  rdfs:label "kat "@en ;
  dy:isenum "True" ;
  rdfs:domain cim:UnitSymbol ;
  skos:definition "Catalytic activity, katal = mol / s."@en .

cim:UnitSymbol.katPerm3 a owl:NamedIndividual, owl:Thing ;
  rdfs:label "katPerm3 "@en ;
  dy:isenum "True" ;
  rdfs:domain cim:UnitSymbol ;
  skos:definition "Catalytic activity concentration, katals per cubic metre."@en .

cim:UnitSymbol.kg a owl:NamedIndividual, owl:Thing ;
  rdfs:label "kg "@en ;
  dy:isenum "True" ;
  rdfs:domain cim:UnitSymbol ;
  skos:definition "Mass in kilograms.  Note: multiplier “k” is included in this unit symbol for compatibility with IEC 61850-7-3."@en .

cim:UnitSymbol.kgPerJ a owl:NamedIndividual, owl:Thing ;
  rdfs:label "kgPerJ "@en ;
  dy:isenum "True" ;
  rdfs:domain cim:UnitSymbol ;
  skos:definition "Weight per energy in kilograms per joule (kg/J). Note: multiplier “k” is included in this unit symbol for compatibility with IEC 61850-7-3."@en .

cim:UnitSymbol.kgPerm3 a owl:NamedIndividual, owl:Thing ;
  rdfs:label "kgPerm3 "@en ;
  dy:isenum "True" ;
  rdfs:domain cim:UnitSymbol ;
  skos:definition "Density in kilogram/cubic metres (kg/m³). Note: multiplier “k” is included in this unit symbol for compatibility with IEC 61850-7-3."@en .

cim:UnitSymbol.kgm a owl:NamedIndividual, owl:Thing ;
  rdfs:label "kgm "@en ;
  dy:isenum "True" ;
  rdfs:domain cim:UnitSymbol ;
  skos:definition "Moment of mass in kilogram metres (kg·m) (first moment of mass). Note: multiplier “k” is included in this unit symbol for compatibility with IEC 61850-7-3."@en .

cim:UnitSymbol.kgm2 a owl:NamedIndividual, owl:Thing ;
  rdfs:label "kgm2 "@en ;
  dy:isenum "True" ;
  rdfs:domain cim:UnitSymbol ;
  skos:definition "Moment of mass in kilogram square metres (kg·m²) (Second moment of mass, commonly called the moment of inertia). Note: multiplier “k” is included in this unit symbol for compatibility with IEC 61850-7-3."@en .

cim:UnitSymbol.kn a owl:NamedIndividual, owl:Thing ;
  rdfs:label "kn "@en ;
  dy:isenum "True" ;
  rdfs:domain cim:UnitSymbol ;
  skos:definition "Speed, knots (1 kn = 1852/3600) m/s."@en .

cim:UnitSymbol.l a owl:NamedIndividual, owl:Thing ;
  rdfs:label "l "@en ;
  dy:isenum "True" ;
  rdfs:domain cim:UnitSymbol ;
  skos:definition "Volume in litres, litre = dm3 = m3/1000."@en .

cim:UnitSymbol.lPerh a owl:NamedIndividual, owl:Thing ;
  rdfs:label "lPerh "@en ;
  dy:isenum "True" ;
  rdfs:domain cim:UnitSymbol ;
  skos:definition "Volumetric flow rate, litres per hour."@en .

cim:UnitSymbol.lPerl a owl:NamedIndividual, owl:Thing ;
  rdfs:label "lPerl "@en ;
  dy:isenum "True" ;
  rdfs:domain cim:UnitSymbol ;
  skos:definition "Concentration, The ratio of the volume of a solute divided by the volume of  the solution. Note: Users may need use a prefix such a ‘µ’ to express a quantity such as ‘µL/L’."@en .

cim:UnitSymbol.lPers a owl:NamedIndividual, owl:Thing ;
  rdfs:label "lPers "@en ;
  dy:isenum "True" ;
  rdfs:domain cim:UnitSymbol ;
  skos:definition "Volumetric flow rate in litres per second."@en .

cim:UnitSymbol.lm a owl:NamedIndividual, owl:Thing ;
  rdfs:label "lm "@en ;
  dy:isenum "True" ;
  rdfs:domain cim:UnitSymbol ;
  skos:definition "Luminous flux in lumens (cd·sr)."@en .

cim:UnitSymbol.lx a owl:NamedIndividual, owl:Thing ;
  rdfs:label "lx "@en ;
  dy:isenum "True" ;
  rdfs:domain cim:UnitSymbol ;
  skos:definition "Illuminance in lux (lm/m²)."@en .

cim:UnitSymbol.m a owl:NamedIndividual, owl:Thing ;
  rdfs:label "m "@en ;
  dy:isenum "True" ;
  rdfs:domain cim:UnitSymbol ;
  skos:definition "Length in metres."@en .

cim:UnitSymbol.m2 a owl:NamedIndividual, owl:Thing ;
  rdfs:label "m2 "@en ;
  dy:isenum "True" ;
  rdfs:domain cim:UnitSymbol ;
  skos:definition "Area in square metres (m²)."@en .

cim:UnitSymbol.m2Pers a owl:NamedIndividual, owl:Thing ;
  rdfs:label "m2Pers "@en ;
  dy:isenum "True" ;
  rdfs:domain cim:UnitSymbol ;
  skos:definition "Viscosity in square metres / second (m²/s)."@en .

cim:UnitSymbol.m3 a owl:NamedIndividual, owl:Thing ;
  rdfs:label "m3 "@en ;
  dy:isenum "True" ;
  rdfs:domain cim:UnitSymbol ;
  skos:definition "Volume in cubic metres (m³)."@en .

cim:UnitSymbol.m3Compensated a owl:NamedIndividual, owl:Thing ;
  rdfs:label "m3Compensated "@en ;
  dy:isenum "True" ;
  rdfs:domain cim:UnitSymbol ;
  skos:definition "Volume, cubic metres, with the value compensated for weather effects."@en .

cim:UnitSymbol.m3Perh a owl:NamedIndividual, owl:Thing ;
  rdfs:label "m3Perh "@en ;
  dy:isenum "True" ;
  rdfs:domain cim:UnitSymbol ;
  skos:definition "Volumetric flow rate, cubic metres per hour."@en .

cim:UnitSymbol.m3Perkg a owl:NamedIndividual, owl:Thing ;
  rdfs:label "m3Perkg "@en ;
  dy:isenum "True" ;
  rdfs:domain cim:UnitSymbol ;
  skos:definition "Specific volume, cubic metres per kilogram, v."@en .

cim:UnitSymbol.m3Pers a owl:NamedIndividual, owl:Thing ;
  rdfs:label "m3Pers "@en ;
  dy:isenum "True" ;
  rdfs:domain cim:UnitSymbol ;
  skos:definition "Volumetric flow rate in cubic metres per second (m³/s)."@en .

cim:UnitSymbol.m3Uncompensated a owl:NamedIndividual, owl:Thing ;
  rdfs:label "m3Uncompensated "@en ;
  dy:isenum "True" ;
  rdfs:domain cim:UnitSymbol ;
  skos:definition "Volume, cubic metres, with the value uncompensated for weather effects."@en .

cim:UnitSymbol.mPerm3 a owl:NamedIndividual, owl:Thing ;
  rdfs:label "mPerm3 "@en ;
  dy:isenum "True" ;
  rdfs:domain cim:UnitSymbol ;
  skos:definition "Fuel efficiency in metres per cubic metres (m/m³)."@en .

cim:UnitSymbol.mPers a owl:NamedIndividual, owl:Thing ;
  rdfs:label "mPers "@en ;
  dy:isenum "True" ;
  rdfs:domain cim:UnitSymbol ;
  skos:definition "Velocity in metres per second (m/s)."@en .

cim:UnitSymbol.mPers2 a owl:NamedIndividual, owl:Thing ;
  rdfs:label "mPers2 "@en ;
  dy:isenum "True" ;
  rdfs:domain cim:UnitSymbol ;
  skos:definition "Acceleration in metres per second squared (m/s²)."@en .

cim:UnitSymbol.min a owl:NamedIndividual, owl:Thing ;
  rdfs:label "min "@en ;
  dy:isenum "True" ;
  rdfs:domain cim:UnitSymbol ;
  skos:definition "Time in minutes, minute  = 60 s."@en .

cim:UnitSymbol.mmHg a owl:NamedIndividual, owl:Thing ;
  rdfs:label "mmHg "@en ;
  dy:isenum "True" ;
  rdfs:domain cim:UnitSymbol ;
  skos:definition "Pressure, millimetres of mercury (1 mmHg is approximately 133.3 Pa)."@en .

cim:UnitSymbol.mol a owl:NamedIndividual, owl:Thing ;
  rdfs:label "mol "@en ;
  dy:isenum "True" ;
  rdfs:domain cim:UnitSymbol ;
  skos:definition "Amount of substance in moles."@en .

cim:UnitSymbol.molPerkg a owl:NamedIndividual, owl:Thing ;
  rdfs:label "molPerkg "@en ;
  dy:isenum "True" ;
  rdfs:domain cim:UnitSymbol ;
  skos:definition "Concentration, Molality, the amount of solute in moles and the amount of solvent in kilograms."@en .

cim:UnitSymbol.molPerm3 a owl:NamedIndividual, owl:Thing ;
  rdfs:label "molPerm3 "@en ;
  dy:isenum "True" ;
  rdfs:domain cim:UnitSymbol ;
  skos:definition "Concentration, The amount of substance concentration, (c), the amount of solvent in moles divided by the volume of solution in m³."@en .

cim:UnitSymbol.molPermol a owl:NamedIndividual, owl:Thing ;
  rdfs:label "molPermol "@en ;
  dy:isenum "True" ;
  rdfs:domain cim:UnitSymbol ;
  skos:definition "Concentration, Molar fraction, the ratio of the molar amount of a solute divided by the molar amount of the solution."@en .

cim:UnitSymbol.none a owl:NamedIndividual, owl:Thing ;
  rdfs:label "none "@en ;
  dy:isenum "True" ;
  rdfs:domain cim:UnitSymbol ;
  skos:definition "Dimension less quantity, e.g. count, per unit, etc."@en .

cim:UnitSymbol.ohm a owl:NamedIndividual, owl:Thing ;
  rdfs:label "ohm "@en ;
  dy:isenum "True" ;
  rdfs:domain cim:UnitSymbol ;
  skos:definition "Electric resistance in ohms (V/A)."@en .

cim:UnitSymbol.ohmPerm a owl:NamedIndividual, owl:Thing ;
  rdfs:label "ohmPerm "@en ;
  dy:isenum "True" ;
  rdfs:domain cim:UnitSymbol ;
  skos:definition "Electric resistance per length in ohms per metre ((V/A)/m)."@en .

cim:UnitSymbol.ohmm a owl:NamedIndividual, owl:Thing ;
  rdfs:label "ohmm "@en ;
  dy:isenum "True" ;
  rdfs:domain cim:UnitSymbol ;
  skos:definition "Resistivity, ohm metres, (rho)."@en .

cim:UnitSymbol.onePerHz a owl:NamedIndividual, owl:Thing ;
  rdfs:label "onePerHz "@en ;
  dy:isenum "True" ;
  rdfs:domain cim:UnitSymbol ;
  skos:definition "Reciprocal of frequency (1/Hz)."@en .

cim:UnitSymbol.onePerm a owl:NamedIndividual, owl:Thing ;
  rdfs:label "onePerm "@en ;
  dy:isenum "True" ;
  rdfs:domain cim:UnitSymbol ;
  skos:definition "Wavenumber, reciprocal metres,  (1/m)."@en .

cim:UnitSymbol.ppm a owl:NamedIndividual, owl:Thing ;
  rdfs:label "ppm "@en ;
  dy:isenum "True" ;
  rdfs:domain cim:UnitSymbol ;
  skos:definition "Concentration in parts per million."@en .

cim:UnitSymbol.rad a owl:NamedIndividual, owl:Thing ;
  rdfs:label "rad "@en ;
  dy:isenum "True" ;
  rdfs:domain cim:UnitSymbol ;
  skos:definition "Plane angle in radians (m/m)."@en .

cim:UnitSymbol.radPers a owl:NamedIndividual, owl:Thing ;
  rdfs:label "radPers "@en ;
  dy:isenum "True" ;
  rdfs:domain cim:UnitSymbol ;
  skos:definition "Angular velocity in radians per second (rad/s)."@en .

cim:UnitSymbol.radPers2 a owl:NamedIndividual, owl:Thing ;
  rdfs:label "radPers2 "@en ;
  dy:isenum "True" ;
  rdfs:domain cim:UnitSymbol ;
  skos:definition "Angular acceleration, radians per second squared."@en .

cim:UnitSymbol.rev a owl:NamedIndividual, owl:Thing ;
  rdfs:label "rev "@en ;
  dy:isenum "True" ;
  rdfs:domain cim:UnitSymbol ;
  skos:definition "Amount of rotation, revolutions."@en .

cim:UnitSymbol.rotPers a owl:NamedIndividual, owl:Thing ;
  rdfs:label "rotPers "@en ;
  dy:isenum "True" ;
  rdfs:domain cim:UnitSymbol ;
  skos:definition "Rotations per second (1/s). See also Hz (1/s)."@en .

cim:UnitSymbol.s a owl:NamedIndividual, owl:Thing ;
  rdfs:label "s "@en ;
  dy:isenum "True" ;
  rdfs:domain cim:UnitSymbol ;
  skos:definition "Time in seconds."@en .

cim:UnitSymbol.sPers a owl:NamedIndividual, owl:Thing ;
  rdfs:label "sPers "@en ;
  dy:isenum "True" ;
  rdfs:domain cim:UnitSymbol ;
  skos:definition "Time, Ratio of time.  Note: Users may need to supply a prefix such as ‘&#181;’ to show rates such as ‘&#181;s/s’."@en .

cim:UnitSymbol.sr a owl:NamedIndividual, owl:Thing ;
  rdfs:label "sr "@en ;
  dy:isenum "True" ;
  rdfs:domain cim:UnitSymbol ;
  skos:definition "Solid angle in steradians (m2/m2)."@en .

cim:UnitSymbol.therm a owl:NamedIndividual, owl:Thing ;
  rdfs:label "therm "@en ;
  dy:isenum "True" ;
  rdfs:domain cim:UnitSymbol ;
  skos:definition "Energy, therms."@en .

cim:UnitSymbol.tonne a owl:NamedIndividual, owl:Thing ;
  rdfs:label "tonne "@en ;
  dy:isenum "True" ;
  rdfs:domain cim:UnitSymbol ;
  skos:definition "Mass in tons, “tonne” or “metric  ton” (1000 kg = 1 Mg)."@en .

cim:WindLookupTableFunctionKind.ipmax a owl:NamedIndividual, owl:Thing ;
  rdfs:label "ipmax "@en ;
  dy:isenum "True" ;
  rdfs:domain cim:WindLookupTableFunctionKind ;
  skos:definition "Lookup table for voltage dependency of active current limits (i<sub>pmax</sub>(u<sub>WT</sub>)). It is used for the current limitation model, IEC 61400-27-1:2015, 5.6.5.8. "@en .

cim:WindLookupTableFunctionKind.iqmax a owl:NamedIndividual, owl:Thing ;
  rdfs:label "iqmax "@en ;
  dy:isenum "True" ;
  rdfs:domain cim:WindLookupTableFunctionKind ;
  skos:definition "Lookup table for voltage dependency of reactive current limits (i<sub>qmax</sub>(u<sub>WT</sub>)). It is used for the current limitation model, IEC 61400-27-1:2015, 5.6.5.8. "@en .

cim:WindLookupTableFunctionKind.omegap a owl:NamedIndividual, owl:Thing ;
  rdfs:label "omegap "@en ;
  dy:isenum "True" ;
  rdfs:domain cim:WindLookupTableFunctionKind ;
  skos:definition "Power vs. speed lookup table (omega(p)). It is used for the P control model type 3, IEC 61400-27-1:2015, 5.6.5.4. "@en .

cim:WindLookupTableFunctionKind.prr a owl:NamedIndividual, owl:Thing ;
  rdfs:label "prr "@en ;
  dy:isenum "True" ;
  rdfs:domain cim:WindLookupTableFunctionKind ;
  skos:definition "Power versus speed change (negative slip) lookup table (p<sub>rr</sub>(deltaomega)). It is used for the rotor resistance control model, IEC 61400-27-1:2015, 5.6.5.3. "@en .

cim:WindLookupTableFunctionKind.pwp a owl:NamedIndividual, owl:Thing ;
  rdfs:label "pwp "@en ;
  dy:isenum "True" ;
  rdfs:domain cim:WindLookupTableFunctionKind ;
  skos:definition "Power vs. frequency lookup table (p<sub>WPbias</sub>(f)). It is used for the wind power plant frequency and active power control model, IEC 61400-27-1:2015, Annex D. "@en .

cim:WindLookupTableFunctionKind.qmaxp a owl:NamedIndividual, owl:Thing ;
  rdfs:label "qmaxp "@en ;
  dy:isenum "True" ;
  rdfs:domain cim:WindLookupTableFunctionKind ;
  skos:definition "Lookup table for active power dependency of reactive power maximum limit (q<sub>maxp</sub>(p)). It is used for the QP and QU limitation model, IEC 61400-27-1:2015, 5.6.5.10. "@en .

cim:WindLookupTableFunctionKind.qmaxu a owl:NamedIndividual, owl:Thing ;
  rdfs:label "qmaxu "@en ;
  dy:isenum "True" ;
  rdfs:domain cim:WindLookupTableFunctionKind ;
  skos:definition "Lookup table for voltage dependency of reactive power maximum limit (q<sub>maxu</sub>(p)). It is used for the QP and QU limitation model, IEC 61400-27-1:2015, 5.6.5.10. "@en .

cim:WindLookupTableFunctionKind.qminp a owl:NamedIndividual, owl:Thing ;
  rdfs:label "qminp "@en ;
  dy:isenum "True" ;
  rdfs:domain cim:WindLookupTableFunctionKind ;
  skos:definition "Lookup table for active power dependency of reactive power minimum limit (q<sub>minp</sub>(p)). It is used for the QP and QU limitation model, IEC 61400-27-1:2015, 5.6.5.10. "@en .

cim:WindLookupTableFunctionKind.qminu a owl:NamedIndividual, owl:Thing ;
  rdfs:label "qminu "@en ;
  dy:isenum "True" ;
  rdfs:domain cim:WindLookupTableFunctionKind ;
  skos:definition "Lookup table for voltage dependency of reactive power minimum limit (q<sub>minu</sub>(p)). It is used for the QP and QU limitation model, IEC 61400-27-1:2015, 5.6.5.10. "@en .

cim:WindLookupTableFunctionKind.qwp a owl:NamedIndividual, owl:Thing ;
  rdfs:label "qwp "@en ;
  dy:isenum "True" ;
  rdfs:domain cim:WindLookupTableFunctionKind ;
  skos:definition "Look up table for the UQ static mode (q<sub>WP</sub>(u<sub>err</sub>)). It is used for the voltage and reactive power control model, IEC 61400-27-1:2015, Annex D. "@en .

cim:WindLookupTableFunctionKind.tcwdu a owl:NamedIndividual, owl:Thing ;
  rdfs:label "tcwdu "@en ;
  dy:isenum "True" ;
  rdfs:domain cim:WindLookupTableFunctionKind ;
  skos:definition "Crowbar duration versus voltage variation look-up table (T<sub>CW</sub>(du)). It is a case-dependent parameter. It is used for the type 3B generator set model, IEC 61400-27-1:2015, 5.6.3.3. "@en .

cim:WindLookupTableFunctionKind.tduwt a owl:NamedIndividual, owl:Thing ;
  rdfs:label "tduwt "@en ;
  dy:isenum "True" ;
  rdfs:domain cim:WindLookupTableFunctionKind ;
  skos:definition "Lookup table to determine the duration of the power reduction after a voltage dip, depending on the size of the voltage dip (T<sub>d</sub>(u<sub>WT</sub>)). It is a type-dependent parameter. It is used for the pitch control power model, IEC 61400-27-1:2015, 5.6.5.1. "@en .

cim:WindLookupTableFunctionKind.tfover a owl:NamedIndividual, owl:Thing ;
  rdfs:label "tfover "@en ;
  dy:isenum "True" ;
  rdfs:domain cim:WindLookupTableFunctionKind ;
  skos:definition "Disconnection time versus over-frequency lookup table (T<sub>fover</sub>(f<sub>WT</sub>)). It is used for the grid protection model, IEC 61400-27-1:2015, 5.6.6. "@en .

cim:WindLookupTableFunctionKind.tfunder a owl:NamedIndividual, owl:Thing ;
  rdfs:label "tfunder "@en ;
  dy:isenum "True" ;
  rdfs:domain cim:WindLookupTableFunctionKind ;
  skos:definition "Disconnection time versus under-frequency lookup table (T<sub>funder</sub>(f<sub>WT</sub>)). It is used for the grid protection model, IEC 61400-27-1:2015, 5.6.6. "@en .

cim:WindLookupTableFunctionKind.tuover a owl:NamedIndividual, owl:Thing ;
  rdfs:label "tuover "@en ;
  dy:isenum "True" ;
  rdfs:domain cim:WindLookupTableFunctionKind ;
  skos:definition "Disconnection time versus over-voltage lookup table (T<sub>uover</sub>(u<sub>WT</sub>)). It is used for the grid protection model, IEC 61400-27-1:2015, 5.6.6. "@en .

cim:WindLookupTableFunctionKind.tuunder a owl:NamedIndividual, owl:Thing ;
  rdfs:label "tuunder "@en ;
  dy:isenum "True" ;
  rdfs:domain cim:WindLookupTableFunctionKind ;
  skos:definition "Disconnection time versus under-voltage lookup table (T<sub>uunder</sub>(u<sub>WT</sub>)). It is used for the grid protection model, IEC 61400-27-1:2015, 5.6.6. "@en .

cim:WindPlantQcontrolModeKind.powerFactor a owl:NamedIndividual, owl:Thing ;
  rdfs:label "powerFactor "@en ;
  dy:isenum "True" ;
  rdfs:domain cim:WindPlantQcontrolModeKind ;
  skos:definition "Power factor reference."@en .

cim:WindPlantQcontrolModeKind.reactivePower a owl:NamedIndividual, owl:Thing ;
  rdfs:label "reactivePower "@en ;
  dy:isenum "True" ;
  rdfs:domain cim:WindPlantQcontrolModeKind ;
  skos:definition "Reactive power reference."@en .

cim:WindPlantQcontrolModeKind.uqStatic a owl:NamedIndividual, owl:Thing ;
  rdfs:label "uqStatic "@en ;
  dy:isenum "True" ;
  rdfs:domain cim:WindPlantQcontrolModeKind ;
  skos:definition "UQ static."@en .

cim:WindPlantQcontrolModeKind.voltageControl a owl:NamedIndividual, owl:Thing ;
  rdfs:label "voltageControl "@en ;
  dy:isenum "True" ;
  rdfs:domain cim:WindPlantQcontrolModeKind ;
  skos:definition "Voltage control."@en .

cim:WindQcontrolModeKind.openLoopReactivePower a owl:NamedIndividual, owl:Thing ;
  rdfs:label "openLoopReactivePower "@en ;
  dy:isenum "True" ;
  rdfs:domain cim:WindQcontrolModeKind ;
  skos:definition "Open loop reactive power control (only used with closed loop at plant level) (<i>M</i><i><sub>qG</sub></i><sub> </sub>equals 2)."@en .

cim:WindQcontrolModeKind.openLooppowerFactor a owl:NamedIndividual, owl:Thing ;
  rdfs:label "openLooppowerFactor "@en ;
  dy:isenum "True" ;
  rdfs:domain cim:WindQcontrolModeKind ;
  skos:definition "Open loop power factor control (<i>M</i><i><sub>qG</sub></i><sub> </sub>equals 4)."@en .

cim:WindQcontrolModeKind.powerFactor a owl:NamedIndividual, owl:Thing ;
  rdfs:label "powerFactor "@en ;
  dy:isenum "True" ;
  rdfs:domain cim:WindQcontrolModeKind ;
  skos:definition "Power factor control (<i>M</i><i><sub>qG</sub></i><sub> </sub>equals 3)."@en .

cim:WindQcontrolModeKind.reactivePower a owl:NamedIndividual, owl:Thing ;
  rdfs:label "reactivePower "@en ;
  dy:isenum "True" ;
  rdfs:domain cim:WindQcontrolModeKind ;
  skos:definition "Reactive power control (<i>M</i><i><sub>qG</sub></i> equals 1)."@en .

cim:WindQcontrolModeKind.voltage a owl:NamedIndividual, owl:Thing ;
  rdfs:label "voltage "@en ;
  dy:isenum "True" ;
  rdfs:domain cim:WindQcontrolModeKind ;
  skos:definition "Voltage control (<i>M</i><i><sub>qG</sub></i> equals 0)."@en .

cim:WindUVRTQcontrolModeKind.mode0 a owl:NamedIndividual, owl:Thing ;
  rdfs:label "mode0 "@en ;
  dy:isenum "True" ;
  rdfs:domain cim:WindUVRTQcontrolModeKind ;
  skos:definition "Voltage-dependent reactive current injection (<i>M</i><i><sub>qUVRT</sub></i> <sub> </sub>equals 0)."@en .

cim:WindUVRTQcontrolModeKind.mode1 a owl:NamedIndividual, owl:Thing ;
  rdfs:label "mode1 "@en ;
  dy:isenum "True" ;
  rdfs:domain cim:WindUVRTQcontrolModeKind ;
  skos:definition "Reactive current injection controlled as the pre-fault value plus an additional voltage dependent reactive current injection (<i>M</i><i><sub>qUVRT</sub></i> equals 1)."@en .

cim:WindUVRTQcontrolModeKind.mode2 a owl:NamedIndividual, owl:Thing ;
  rdfs:label "mode2 "@en ;
  dy:isenum "True" ;
  rdfs:domain cim:WindUVRTQcontrolModeKind ;
  skos:definition "Reactive current injection controlled as the pre-fault value plus an additional voltage-dependent reactive current injection during fault, and as the pre-fault value plus an additional constant reactive current injection post fault (<i>M</i><i><sub>qUVRT</sub></i><sub>  </sub>equals 2)."@en .

dy:Package_AsynchronousMachineDynamics a dy:Package ;
  rdfs:comment """
An asynchronous machine model represents a (induction) generator or motor with no external connection to the rotor windings, e.g. a squirrel-cage induction machine. 
The interconnection with the electrical network equations can differ among simulation tools.  The program only needs to know the terminal to which this asynchronous machine is connected in order to establish the correct interconnection.  The interconnection with the motor’s equipment could also differ due to input and output signals required by standard models.
The asynchronous machine model is used to model wind generators type 1 and type 2.  For these, normal practice is to include the rotor flux transients and neglect the stator flux transients.
\t"""@en .

dy:Package_Base a dy:Package ;
  rdfs:comment "Content of the base CIM published as IEC 61970-301."@en .

dy:Package_Core a dy:Package ;
  rdfs:comment "Contains the core PowerSystemResource and ConductingEquipment entities shared by all applications plus common collections of those entities. Not all applications require all the Core entities.  This package does not depend on any other package except the Domain package, but most of the other packages have associations and generalizations that depend on it."@en .

dy:Package_DC a dy:Package ;
  rdfs:comment "This package contains model for direct current equipment and controls."@en .

dy:Package_DiscontinuousExcitationControlDynamics a dy:Package ;
  rdfs:comment """
In certain system configurations, continuous excitation control with terminal voltage and power system stabilizing regulator input signals does not ensure that the potential of the excitation system for improving system stability is fully exploited. For these situations, discontinuous excitation control signals can be employed to enhance stability following large transient disturbances.
<font color="#0f0f0f">For additional information please refer to IEEE 421.5-2005, 12.</font>
\t"""@en .

dy:Package_Domain a dy:Package ;
  rdfs:comment """
The domain package defines primitive datatypes that are used by classes in other packages. Stereotypes are used to describe the datatypes. The following stereotypes are defined:
&lt;&lt;enumeration&gt;&gt; A list of permissible constant values.
&lt;&lt;Primitive&gt;&gt; The most basic data types used to compose all other data types.
&lt;&lt;CIMDatatype&gt;&gt; A datatype that contains a value attribute, an optional unit of measure and a unit multiplier. The unit and multiplier may be specified as a static variable initialized to the allowed value.
&lt;&lt;Compound&gt;&gt; A composite of Primitive, enumeration, CIMDatatype or other Compound classes, as long as the Compound classes do not recurse.
For all datatypes both positive and negative values are allowed unless stated otherwise for a particular datatype. 

\t"""@en .

dy:Package_Dynamics a dy:Package ;
  rdfs:comment """
The CIM dynamic model definitions reflect the most common IEEE or, in the case of wind models, IEC, representations of models as well as models included in some of the transient stability software widely used by utilities. 
These dynamic models are intended to ensure interoperability between different vendors’ software products currently in use by electric utility energy companies, utilities, Transmission System Operators (TSOs), Regional Transmission Organizations (RTOs), and Independent System Operators (ISOs).  It is important to note that each vendor is free to select its own internal implementation of these models.  Differences in vendor results, as long as they are within accepted engineering practice, caused by different internal representations, are acceptable.
Unless explicitly stated otherwise, the following modelling conventions are followed:
- limited integrators are of the non-windup type;
- it shall be possible to enter a time constant of zero (where it makes sense).

\t"""@en .

dy:Package_DynamicsProfile a dy:Package ;
  rdfs:comment """
This is the IEC 61970-457 profile.

\t"""@en .

dy:Package_ExcitationSystemDynamics a dy:Package ;
  rdfs:comment """
The excitation system model provides the field voltage (<i>Efd</i>) for a synchronous machine model.  It is linked to a specific generator (synchronous machine). 
The representation of all limits used by the models (not including IEEE standard models) shall comply with the representation defined in the Annex E of the IEEE 421.5-2005, unless specified differently in the documentation of the model.
The parameters are different for each excitation system model; the same parameter name can have different meaning in different models.

\t"""@en .

dy:Package_HVDCDynamics a dy:Package ;
  rdfs:comment "High voltage direct current (HVDC) models."@en .

dy:Package_LoadDynamics a dy:Package ;
  rdfs:comment """
Dynamic load models are used to represent the dynamic real and reactive load behaviour of a load from the static power flow model.  
Dynamic load models can be defined as applying either to a single load (energy consumer) or to a group of energy consumers.  
Large industrial motors or groups of similar motors can be represented by a synchronous machine model (SynchronousMachineDynamics) or an asynchronous machine model (AsynchronousMachineDynamics), which are usually represented as generators with negative active power output in the static (power flow) data.





  
\t"""@en .

dy:Package_MechanicalLoadDynamics a dy:Package ;
  rdfs:comment "A mechanical load represents the variation in a motor's shaft torque or power as a function of shaft speed."@en .

dy:Package_OverexcitationLimiterDynamics a dy:Package ;
  rdfs:comment "Overexcitation limiters (OELs) are also referred to as <i>maximum excitation limiters </i>and <i>field current limiters. </i>The possibility of voltage collapse in stressed power systems increases the importance of modelling these limiters in studies of system conditions that cause machines to operate at high levels of excitation for a sustained period, such as voltage collapse or system-islanding. Such events typically occur over a long time frame compared with transient or small-signal stability simulations."@en .

dy:Package_PFVArControllerType1Dynamics a dy:Package ;
  rdfs:comment """
<font color="#0f0f0f">Excitation systems for synchronous machines are sometimes supplied with an optional means of automatically adjusting generator output reactive power (VAr) or power factor (PF) to a user-specified value. This can be accomplished with either a reactive power or power factor controller or regulator.  A reactive power or power factor controller is defined as a PF/VAr controller in IEEE 421.1 as “a control function that acts through the reference adjuster to modify the voltage regulator set point to maintain the synchronous machine steady-state power factor or reactive power at a predetermined value.” </font>
<font color="#0f0f0f">For additional information please refer to IEEE 421.5-2005, 11.</font>
\t"""@en .

dy:Package_PFVArControllerType2Dynamics a dy:Package ;
  rdfs:comment """
<font color="#0f0f0f">A var/pf regulator is defined as “a synchronous machine regulator that functions to maintain the power factor or reactive component of power at a predetermined value.”  </font>
<font color="#0f0f0f">For additional information please refer to IEEE 421.5-2005, 11.</font>
<font color="#0f0f0f">
</font>
\t"""@en .

dy:Package_PowerSystemStabilizerDynamics a dy:Package ;
  rdfs:comment "The power system stabilizer (PSS) model provides an input (<i>Vs</i>) to the excitation system model to improve damping of system oscillations.  A variety of input signals can be used depending on the particular design."@en .

dy:Package_StandardInterconnections a dy:Package ;
  rdfs:comment """
This subclause describes the standard interconnections for various types of equipment. These interconnections are understood by the application programs and can be identified based on the presence of one of the key classes with a relationship to the static power flow model: SynchronousMachineDynamics, AsynchronousMachineDynamics, EnergyConsumerDynamics or WindTurbineType3or4Dynamics. 
The relationships between classes expressed in the interconnection diagrams are intended to support dynamic behaviour described by either standard models or user-defined models.
In the interconnection diagrams, boxes which are black in colour represent function blocks whose functionality can be provided by one of many standard models or by a user-defined model. Blue boxes represent specific standard models.  A dashed box means that the function block or specific standard model is optional.
\t"""@en .

dy:Package_StandardModels a dy:Package ;
  rdfs:comment """
This subclause contains standard dynamic model specifications grouped into packages by standard function block (type of equipment being modelled).
In the CIM, standard dynamic models are expressed by means of a class named with the standard model name and attributes reflecting each of the parameters necessary to describe the behaviour of an instance of the standard model.
\t"""@en .

dy:Package_StaticVarCompensatorDynamics a dy:Package ;
  rdfs:comment "Static var compensator (SVC) models."@en .

dy:Package_SynchronousMachineDynamics a dy:Package ;
  rdfs:comment """
For conventional power generating units (e.g., thermal, hydro, combustion turbine), a synchronous machine model represents the electrical characteristics of the generator and the mechanical characteristics of the turbine-generator rotational inertia.  Large industrial motors or groups of similar motors can be represented by individual motor models which are represented as generators with negative active power in the static (power flow) data.  
The interconnection with the electrical network equations can differ among simulation tools.  The tool only needs to know the synchronous machine to establish the correct interconnection.  The interconnection with the motor’s equipment could also differ due to input and output signals required by standard models.
\t"""@en .

dy:Package_TurbineGovernorDynamics a dy:Package ;
  rdfs:comment """
The turbine-governor model is linked to one or two synchronous generators and determines the shaft mechanical power (<i>Pm</i>) or torque (<i>Tm</i>) for the generator model.  
Unlike IEEE standard models for other function blocks, the three IEEE turbine-governor standard models (GovHydroIEEE0, GovHydroIEEE2, and GovSteamIEEE1) are documented in IEEE Transactions, not in IEEE standards. For that reason, diagrams are supplied for those models.
A 2012 IEEE report, <i><u>Dynamic Models for Turbine-Governors in Power System Studies</u></i>, provides updated information on a variety of models including IEEE, vendor and reliability authority models.  Fully incorporating the results of that report into the CIM dynamics model is a future effort.
\t"""@en .

dy:Package_TurbineLoadControllerDynamics a dy:Package ;
  rdfs:comment "A turbine load controller acts to maintain turbine power at a set value by continuous adjustment of the turbine governor speed-load reference."@en .

dy:Package_UnderexcitationLimiterDynamics a dy:Package ;
  rdfs:comment "Underexcitation limiters (UELs) act to boost excitation. The UEL typically senses either a combination of voltage and current of the synchronous machine or a combination of real and reactive power. Some UELs utilize a temperature or pressure recalibration feature, in which the UEL characteristic is shifted depending upon the generator cooling gas temperature or pressure. "@en .

dy:Package_UserDefinedModels a dy:Package ;
  rdfs:comment """
This subclause contains user-defined dynamic model classes to support the exchange of both proprietary and explicitly defined user-defined models.  
<u>Proprietary models</u> represent behaviour which, while not defined by a standard model class, is mutually understood by the sending and receiving applications based on the name passed in the .name attribute of the appropriate xxxUserDefined class.  Proprietary model parameters are passed as general attributes using as many instances of the ProprietaryParameterDynamics class as there are parameters.
<u>Explicitly defined models</u> describe dynamic behaviour in detail in terms of control blocks and their input and output signals.  Note that the classes to support explicitly defined modelling are not currently defined - it is future work intended to also be supported by the family of xxxUserDefined classes.
Both types of user-defined models use the family of xxxUserDefined classes, which allow a user-defined model to be used:
- as the model for an individual standard function block (such as a turbine-governor or power system stabilizer) in a standard interconnection model whose other function blocks could be either standard or user-defined.  For an illustration of this form of usage for a proprietary model, see the ExampleFunctionBlockProprietaryModel diagram in subclause 5.5.
- as the complete representation of a dynamic behaviour model (for an entire synchronous machine, for example) where standard function blocks and standard interconnections are not used at all. For an illustration of this form of usage for a proprietary model, see the ExampleCompleteProprietaryModel diagram in subclause 5.5.
\t"""@en .

dy:Package_VoltageAdjusterDynamics a dy:Package ;
  rdfs:comment """
<font color="#0f0f0f">A voltage adjuster is a reference adjuster that uses inputs from a reactive power or power factor controller to modify the voltage regulator set point to maintain the synchronous machine steady-state power factor or reactive power at a predetermined value. </font>
<font color="#0f0f0f">For additional information please refer to IEEE 421.5-2005, 11.</font>
\t"""@en .

dy:Package_VoltageCompensatorDynamics a dy:Package ;
  rdfs:comment """
<font color="#0f0f0f">Synchronous machine terminal voltage transducer and current compensator models</font> adjust the terminal voltage feedback to the excitation system by adding a quantity that is proportional to the terminal current of the generator.  It is linked to a specific generator (synchronous machine).
<font color="#0f0f0f">Several types of compensation are available on most excitation systems. Synchronous machine active and reactive current compensation are the most common. Either reactive droop compensation and/or line-drop compensation can be used, simulating an impedance drop and effectively regulating at some point other than the terminals of the machine. The impedance or range of adjustment and type of compensation should be specified for different types. </font>
<font color="#0f0f0f">Care shall be taken to ensure that a consistent PU system is utilized for the compensator parameters and the synchronous machine current base.</font>
<font color="#0f0f0f">For further information see IEEE 421.5-2005, 4.</font>


<font color="#0f0f0f">
</font>
\t"""@en .

dy:Package_WindDynamics a dy:Package ;
  rdfs:comment """
Wind turbines are generally divided into four types, which are currently significant in power systems.  The four types have the following characteristics:
- type 1: wind turbine with directly grid connected asynchronous generator with fixed rotor resistance (typically squirrel cage);
- type 2: wind turbine with directly grid connected asynchronous generator with variable rotor resistance;
- type 3: wind turbines with doubly-fed asynchronous generators (directly connected stator and rotor connected through power converter);
- type 4: wind turbines connected to the grid through a full size power converter.
Models included in this package are according to IEC 61400-27-1:2015.
\t"""@en .

dy:Package_Wires a dy:Package ;
  rdfs:comment "An extension to the Core and Topology package that models information on the electrical characteristics of Transmission and Distribution networks. This package is used by network applications such as State Estimation, Load Flow and Optimal Power Flow.  "@en .


