@prefix cim    : <http://iec.ch/TC57/CIM100#> .
@prefix cims   : <http://iec.ch/TC57/1999/rdf-schema-extensions-19990926#> .
@prefix eq     : <http://iec.ch/TC57/ns/CIM/CoreEquipment-EU#> .
@prefix eu     : <http://iec.ch/TC57/CIM100-European#> .
@prefix dcat   : <http://www.w3.org/ns/dcat#> .
@prefix dct    : <http://purl.org/dc/terms/> .
@prefix owl    : <http://www.w3.org/2002/07/owl#> .
@prefix rdf    : <http://www.w3.org/1999/02/22-rdf-syntax-ns#> .
@prefix rdfs   : <http://www.w3.org/2000/01/rdf-schema#> .
@prefix skos   : <http://www.w3.org/2004/02/skos/core#> .
@prefix xsd    : <http://www.w3.org/2001/XMLSchema#> .

eq:Ontology a owl:Ontology ;
  dct:description "This vocabulary is describing the core equipment profile from IEC 61970-600-2."@en ;
  dcat:keyword "EQ" ;
  dcat:theme "vocabulary"@en ;
  dct:conformsTo "file://iec61970cim17v40_iec61968cim13v13a_iec62325cim03v17a.eap", "urn:iso:std:iec:61970-301:ed-7:amd1", "urn:iso:std:iec:61970-401:draft:ed-1", "urn:iso:std:iec:61970-501:draft:ed-2", "urn:iso:std:iec:61970-600-2:ed-1" ;
  dct:creator "ENTSO-E CIM EG"@en ;
  dct:identifier "urn:uuid:9fd00587-84d4-4910-bbd4-e003ed7e0821" ;
  dct:issued "2021-01-27T12:41:26Z"^^xsd:dateTime ;
  dct:language "en-GB" ;
  dct:modified "2020-10-12"^^xsd:date ;
  dct:publisher "ENTSO-E"@en ;
  dct:rights "Copyright"@en ;
  dct:rightsHolder "ENTSO-E"@en ;
  dct:title "Core Equipment Vocabulary"@en ;
  owl:incompatibleWith <http://entsoe.eu/2009/profile1> ;
  owl:priorVersion <http://entsoe.eu/CIM/EquipmentCore/3/1> ;
  owl:versionIRI <http://iec.ch/TC57/ns/CIM/CoreEquipment-EU/3.0> ;
  owl:versionInfo "3.0.0"@en .

cim:ACDCConverter a owl:Class ;
  rdfs:label "ACDCConverter"@en ;
  eq:Package "Package_CoreEquipmentProfile" ;
  eq:isAbstract "True" ;
  rdfs:subClassOf cim:ConductingEquipment ;
  skos:definition "A unit with valves for three phases, together with unit control equipment, essential protective and switching devices, DC storage capacitors, phase reactors and auxiliaries, if any, used for conversion."@en .

cim:ACDCConverterDCTerminal a owl:Class ;
  rdfs:label "ACDCConverterDCTerminal"@en ;
  eq:Package "Package_CoreEquipmentProfile" ;
  rdfs:subClassOf cim:DCBaseTerminal ;
  skos:definition "A DC electrical connection point at the AC/DC converter. The AC/DC converter is electrically connected also to the AC side. The AC connection is inherited from the AC conducting equipment in the same way as any other AC equipment. The AC/DC converter DC terminal is separate from generic DC terminal to restrict the connection with the AC side to AC/DC converter and so that no other DC conducting equipment can be connected to the AC side."@en .

cim:ACDCTerminal a owl:Class ;
  rdfs:label "ACDCTerminal"@en ;
  eq:Package "Package_CoreEquipmentProfile" ;
  eq:isAbstract "True" ;
  rdfs:subClassOf cim:IdentifiedObject ;
  skos:definition "An electrical connection point (AC or DC) to a piece of conducting equipment. Terminals are connected at physical connection points called connectivity nodes."@en .

cim:ACLineSegment a owl:Class ;
  rdfs:label "ACLineSegment"@en ;
  eq:Package "Package_CoreEquipmentProfile" ;
  rdfs:subClassOf cim:Conductor ;
  skos:definition """
A wire or combination of wires, with consistent electrical characteristics, building a single electrical system, used to carry alternating current between points in the power system.
For symmetrical, transposed three phase lines, it is sufficient to use attributes of the line segment, which describe impedances and admittances for the entire length of the segment.  Additionally impedances can be computed by using length and associated per length impedances.
The BaseVoltage at the two ends of ACLineSegments in a Line shall have the same BaseVoltage.nominalVoltage. However, boundary lines may have slightly different BaseVoltage.nominalVoltages and variation is allowed. Larger voltage difference in general requires use of an equivalent branch.
\t"""@en .

cim:ActivePower a owl:Class ;
  rdfs:label "ActivePower"@en ;
  eq:Package "Package_CoreEquipmentProfile" ;
  eq:isCIMDatatype "True" ;
  skos:definition "Product of RMS value of the voltage and the RMS value of the in-phase component of the current."@en .

cim:ActivePowerLimit a owl:Class ;
  rdfs:label "ActivePowerLimit"@en ;
  eq:Package "Package_CoreEquipmentProfile" ;
  rdfs:subClassOf cim:OperationalLimit ;
  skos:definition "Limit on active power flow."@en .

cim:ActivePowerPerCurrentFlow a owl:Class ;
  rdfs:label "ActivePowerPerCurrentFlow"@en ;
  eq:Package "Package_CoreEquipmentProfile" ;
  eq:isCIMDatatype "True" ;
  skos:definition "Active power variation with current flow."@en .

cim:ActivePowerPerFrequency a owl:Class ;
  rdfs:label "ActivePowerPerFrequency"@en ;
  eq:Package "Package_CoreEquipmentProfile" ;
  eq:isCIMDatatype "True" ;
  skos:definition "Active power variation with frequency."@en .

cim:AngleDegrees a owl:Class ;
  rdfs:label "AngleDegrees"@en ;
  eq:Package "Package_CoreEquipmentProfile" ;
  eq:isCIMDatatype "True" ;
  skos:definition """
Measurement of angle in degrees.

\t"""@en .

cim:ApparentPower a owl:Class ;
  rdfs:label "ApparentPower"@en ;
  eq:Package "Package_CoreEquipmentProfile" ;
  eq:isCIMDatatype "True" ;
  skos:definition """
Product of the RMS value of the voltage and the RMS value of the current.

\t"""@en .

cim:ApparentPowerLimit a owl:Class ;
  rdfs:label "ApparentPowerLimit"@en ;
  eq:Package "Package_CoreEquipmentProfile" ;
  rdfs:subClassOf cim:OperationalLimit ;
  skos:definition "Apparent power limit."@en .

cim:AsynchronousMachine a owl:Class ;
  rdfs:label "AsynchronousMachine"@en ;
  eq:Package "Package_CoreEquipmentProfile" ;
  rdfs:subClassOf cim:RotatingMachine ;
  skos:definition "A rotating machine whose shaft rotates asynchronously with the electrical field.  Also known as an induction machine with no external connection to the rotor windings, e.g. squirrel-cage induction machine."@en .

cim:AuxiliaryEquipment a owl:Class ;
  rdfs:label "AuxiliaryEquipment"@en ;
  eq:Package "Package_CoreEquipmentProfile" ;
  eq:isAbstract "True" ;
  rdfs:subClassOf cim:Equipment ;
  skos:definition """
AuxiliaryEquipment describe equipment that is not performing any primary functions but support for the equipment performing the primary function.
AuxiliaryEquipment is attached to primary equipment via an association with Terminal.
\t"""@en .

cim:BaseVoltage a owl:Class ;
  rdfs:label "BaseVoltage"@en ;
  eq:Package "Package_CoreEquipmentProfile" ;
  rdfs:subClassOf cim:IdentifiedObject ;
  skos:definition "Defines a system base voltage which is referenced. "@en .

cim:BasicIntervalSchedule a owl:Class ;
  rdfs:label "BasicIntervalSchedule"@en ;
  eq:Package "Package_CoreEquipmentProfile" ;
  eq:isAbstract "True" ;
  rdfs:subClassOf cim:IdentifiedObject ;
  skos:definition "Schedule of values at points in time."@en .

cim:BatteryUnit a owl:Class ;
  rdfs:label "BatteryUnit"@en ;
  eq:Package "Package_CoreEquipmentProfile" ;
  rdfs:subClassOf cim:PowerElectronicsUnit ;
  skos:definition "An electrochemical energy storage device."@en .

cim:Bay a owl:Class ;
  rdfs:label "Bay"@en ;
  eq:Package "Package_CoreEquipmentProfile" ;
  rdfs:subClassOf cim:EquipmentContainer ;
  skos:definition """
A collection of power system resources (within a given substation) including conducting equipment, protection relays, measurements, and telemetry.  A bay typically represents a physical grouping related to modularization of equipment.

\t"""@en .

cim:Boolean a owl:Class ;
  rdfs:label "Boolean"@en ;
  eq:Package "Package_CoreEquipmentProfile" ;
  eq:isPrimitive "True" ;
  skos:definition """
A type with the value space "true" and "false".

\t"""@en .

cim:Breaker a owl:Class ;
  rdfs:label "Breaker"@en ;
  eq:Package "Package_CoreEquipmentProfile" ;
  rdfs:subClassOf cim:ProtectedSwitch ;
  skos:definition "A mechanical switching device capable of making, carrying, and breaking currents under normal circuit conditions and also making, carrying for a specified time, and breaking currents under specified abnormal circuit conditions e.g.  those of short circuit."@en .

cim:BusNameMarker a owl:Class ;
  rdfs:label "BusNameMarker"@en ;
  eq:Package "Package_CoreEquipmentProfile" ;
  rdfs:subClassOf cim:IdentifiedObject ;
  skos:definition "Used to apply user standard names to TopologicalNodes. Associated with one or more terminals that are normally connected with the bus name.    The associated terminals are normally connected by non-retained switches. For a ring bus station configuration, all BusbarSection terminals in the ring are typically associated.   For a breaker and a half scheme, both BusbarSections would normally be associated.  For a ring bus, all BusbarSections would normally be associated.  For a \"straight\" busbar configuration, normally only the main terminal at the BusbarSection would be associated.  "@en .

cim:BusbarSection a owl:Class ;
  rdfs:label "BusbarSection"@en ;
  eq:Package "Package_CoreEquipmentProfile" ;
  rdfs:subClassOf cim:Connector ;
  skos:definition """
A conductor, or group of conductors, with negligible impedance, that serve to connect other conducting equipment within a single substation. 
Voltage measurements are typically obtained from voltage transformers that are connected to busbar sections. A bus bar section may have many physical terminals but for analysis is modelled with exactly one logical terminal.
\t"""@en .

cim:CAESPlant a owl:Class ;
  rdfs:label "CAESPlant"@en ;
  eq:Package "Package_CoreEquipmentProfile" ;
  rdfs:subClassOf cim:PowerSystemResource ;
  skos:definition """
Compressed air energy storage plant.

\t"""@en .

cim:Capacitance a owl:Class ;
  rdfs:label "Capacitance"@en ;
  eq:Package "Package_CoreEquipmentProfile" ;
  eq:isCIMDatatype "True" ;
  skos:definition """
Capacitive part of reactance (imaginary part of impedance), at rated frequency.

\t"""@en .

cim:Clamp a owl:Class ;
  rdfs:label "Clamp"@en ;
  eq:Package "Package_CoreEquipmentProfile" ;
  rdfs:subClassOf cim:ConductingEquipment ;
  skos:definition """
A Clamp is a galvanic connection at a line segment where other equipment is connected. A Clamp does not cut the line segment. 
A Clamp is ConductingEquipment and has one Terminal with an associated ConnectivityNode. Any other ConductingEquipment can be connected to the Clamp ConnectivityNode.

\t"""@en .

cim:CogenerationPlant a owl:Class ;
  rdfs:label "CogenerationPlant"@en ;
  eq:Package "Package_CoreEquipmentProfile" ;
  rdfs:subClassOf cim:PowerSystemResource ;
  skos:definition """
A set of thermal generating units for the production of electrical energy and process steam (usually from the output of the steam turbines). The steam sendout is typically used for industrial purposes or for municipal heating and cooling.

\t"""@en .

cim:CombinedCyclePlant a owl:Class ;
  rdfs:label "CombinedCyclePlant"@en ;
  eq:Package "Package_CoreEquipmentProfile" ;
  rdfs:subClassOf cim:PowerSystemResource ;
  skos:definition """
A set of combustion turbines and steam turbines where the exhaust heat from the combustion turbines is recovered to make steam for the steam turbines, resulting in greater overall plant efficiency.

\t"""@en .

cim:Conductance a owl:Class ;
  rdfs:label "Conductance"@en ;
  eq:Package "Package_CoreEquipmentProfile" ;
  eq:isCIMDatatype "True" ;
  skos:definition """
Factor by which voltage must be multiplied to give corresponding power lost from a circuit. Real part of admittance.

\t"""@en .

cim:ConductingEquipment a owl:Class ;
  rdfs:label "ConductingEquipment"@en ;
  eq:Package "Package_CoreEquipmentProfile" ;
  eq:isAbstract "True" ;
  rdfs:subClassOf cim:Equipment ;
  skos:definition "The parts of the AC power system that are designed to carry current or that are conductively connected through terminals."@en .

cim:Conductor a owl:Class ;
  rdfs:label "Conductor"@en ;
  eq:Package "Package_CoreEquipmentProfile" ;
  eq:isAbstract "True" ;
  rdfs:subClassOf cim:ConductingEquipment ;
  skos:definition "Combination of conducting material with consistent electrical characteristics, building a single electrical system, used to carry current between points in the power system.  "@en .

cim:ConformLoad a owl:Class ;
  rdfs:label "ConformLoad"@en ;
  eq:Package "Package_CoreEquipmentProfile" ;
  rdfs:subClassOf cim:EnergyConsumer ;
  skos:definition "ConformLoad represent loads that follow a daily load change pattern where the pattern can be used to scale the load with a system load."@en .

cim:ConformLoadGroup a owl:Class ;
  rdfs:label "ConformLoadGroup"@en ;
  eq:Package "Package_CoreEquipmentProfile" ;
  rdfs:subClassOf cim:LoadGroup ;
  skos:definition "A group of loads conforming to an allocation pattern. "@en .

cim:ConformLoadSchedule a owl:Class ;
  rdfs:label "ConformLoadSchedule"@en ;
  eq:Package "Package_CoreEquipmentProfile" ;
  rdfs:subClassOf cim:SeasonDayTypeSchedule ;
  skos:definition "A curve of load  versus time (X-axis) showing the active power values (Y1-axis) and reactive power (Y2-axis) for each unit of the period covered. This curve represents a typical pattern of load over the time period for a given day type and season."@en .

cim:ConnectivityNode a owl:Class ;
  rdfs:label "ConnectivityNode"@en ;
  eq:Package "Package_CoreEquipmentProfile" ;
  rdfs:subClassOf cim:IdentifiedObject ;
  skos:definition "Connectivity nodes are points where terminals of AC conducting equipment are connected together with zero impedance."@en .

cim:ConnectivityNodeContainer a owl:Class ;
  rdfs:label "ConnectivityNodeContainer"@en ;
  eq:Package "Package_CoreEquipmentProfile" ;
  eq:isAbstract "True" ;
  rdfs:subClassOf cim:PowerSystemResource ;
  skos:definition """
A base class for all objects that may contain connectivity nodes or topological nodes.

\t"""@en .

cim:Connector a owl:Class ;
  rdfs:label "Connector"@en ;
  eq:Package "Package_CoreEquipmentProfile" ;
  eq:isAbstract "True" ;
  rdfs:subClassOf cim:ConductingEquipment ;
  skos:definition "A conductor, or group of conductors, with negligible impedance, that serve to connect other conducting equipment within a single substation and are modelled with a single logical terminal."@en .

cim:ControlArea a owl:Class ;
  rdfs:label "ControlArea"@en ;
  eq:Package "Package_CoreEquipmentProfile" ;
  rdfs:subClassOf cim:PowerSystemResource ;
  skos:definition """
A control area is a grouping of generating units and/or loads and a cutset of tie lines (as terminals) which may be used for a variety of purposes including automatic generation control, power flow solution area interchange control specification, and input to load forecasting. All generation and load within the area defined by the terminals on the border are considered in the area interchange control. Note that any number of overlapping control area specifications can be superimposed on the physical model. The following general principles apply to ControlArea:
1.  The control area orientation for net interchange is positive for an import, negative for an export.
2.  The control area net interchange is determined by summing flows in Terminals. The Terminals are identified by creating a set of TieFlow objects associated with a ControlArea object. Each TieFlow object identifies one Terminal.
3.  In a single network model, a tie between two control areas must be modelled in both control area specifications, such that the two representations of the tie flow sum to zero.
4.  The normal orientation of Terminal flow is positive for flow into the conducting equipment that owns the Terminal. (i.e. flow from a bus into a device is positive.) However, the orientation of each flow in the control area specification must align with the control area convention, i.e. import is positive. If the orientation of the Terminal flow referenced by a TieFlow is positive into the control area, then this is confirmed by setting TieFlow.positiveFlowIn flag TRUE. If not, the orientation must be reversed by setting the TieFlow.positiveFlowIn flag FALSE.
\t"""@en .

cim:ControlAreaGeneratingUnit a owl:Class ;
  rdfs:label "ControlAreaGeneratingUnit"@en ;
  eq:Package "Package_CoreEquipmentProfile" ;
  rdfs:subClassOf cim:IdentifiedObject ;
  skos:definition "A control area generating unit. This class is needed so that alternate control area definitions may include the same generating unit.   It should be noted that only one instance within a control area should reference a specific generating unit."@en .

cim:ControlAreaTypeKind a owl:Class ;
  rdfs:label "ControlAreaTypeKind"@en ;
  eq:Package "Package_CoreEquipmentProfile" ;
  owl:oneOf ( cim:ControlAreaTypeKind.AGC cim:ControlAreaTypeKind.Forecast
    cim:ControlAreaTypeKind.Interchange ) ;
  rdfs:subClassOf cim:Enumeration ;
  skos:definition """
The type of control area.

\t"""@en .

cim:CsConverter a owl:Class ;
  rdfs:label "CsConverter"@en ;
  eq:Package "Package_CoreEquipmentProfile" ;
  rdfs:subClassOf cim:ACDCConverter ;
  skos:definition """
DC side of the current source converter (CSC).
The firing angle controls the dc voltage at the converter, both for rectifier and inverter. The difference between the dc voltages of the rectifier and inverter determines the dc current. The extinction angle is used to limit the dc voltage at the inverter, if needed, and is not used in active power control. The firing angle, transformer tap position and number of connected filters are the primary means to control a current source dc line. Higher level controls are built on top, e.g. dc voltage, dc current and active power. From a steady state perspective it is sufficient to specify the wanted active power transfer (ACDCConverter.targetPpcc) and the control functions will set the dc voltage, dc current, firing angle, transformer tap position and number of connected filters to meet this. Therefore attributes targetAlpha and targetGamma are not applicable in this case.
The reactive power consumed by the converter is a function of the firing angle, transformer tap position and number of connected filter, which can be approximated with half of the active power. The losses is a function of the dc voltage and dc current.
The attributes minAlpha and maxAlpha define the range of firing angles for rectifier operation between which no discrete tap changer action takes place. The range is typically 10-18 degrees.
The attributes minGamma and maxGamma define the range of extinction angles for inverter operation between which no discrete tap changer action takes place. The range is typically 17-20 degrees.
\t"""@en .

cim:Currency a owl:Class ;
  rdfs:label "Currency"@en ;
  eq:Package "Package_CoreEquipmentProfile" ;
  owl:oneOf ( cim:Currency.AED cim:Currency.AFN cim:Currency.ALL cim:Currency.AMD cim:Currency.ANG
    cim:Currency.AOA cim:Currency.ARS cim:Currency.AUD cim:Currency.AWG cim:Currency.AZN
    cim:Currency.BAM cim:Currency.BBD cim:Currency.BDT cim:Currency.BGN cim:Currency.BHD
    cim:Currency.BIF cim:Currency.BMD cim:Currency.BND cim:Currency.BOB cim:Currency.BOV
    cim:Currency.BRL cim:Currency.BSD cim:Currency.BTN cim:Currency.BWP cim:Currency.BYR
    cim:Currency.BZD cim:Currency.CAD cim:Currency.CDF cim:Currency.CHF cim:Currency.CLF
    cim:Currency.CLP cim:Currency.CNY cim:Currency.COP cim:Currency.COU cim:Currency.CRC
    cim:Currency.CUC cim:Currency.CUP cim:Currency.CVE cim:Currency.CZK cim:Currency.DJF
    cim:Currency.DKK cim:Currency.DOP cim:Currency.DZD cim:Currency.EEK cim:Currency.EGP
    cim:Currency.ERN cim:Currency.ETB cim:Currency.EUR cim:Currency.FJD cim:Currency.FKP
    cim:Currency.GBP cim:Currency.GEL cim:Currency.GHS cim:Currency.GIP cim:Currency.GMD
    cim:Currency.GNF cim:Currency.GTQ cim:Currency.GYD cim:Currency.HKD cim:Currency.HNL
    cim:Currency.HRK cim:Currency.HTG cim:Currency.HUF cim:Currency.IDR cim:Currency.ILS
    cim:Currency.INR cim:Currency.IQD cim:Currency.IRR cim:Currency.ISK cim:Currency.JMD
    cim:Currency.JOD cim:Currency.JPY cim:Currency.KES cim:Currency.KGS cim:Currency.KHR
    cim:Currency.KMF cim:Currency.KPW cim:Currency.KRW cim:Currency.KWD cim:Currency.KYD
    cim:Currency.KZT cim:Currency.LAK cim:Currency.LBP cim:Currency.LKR cim:Currency.LRD
    cim:Currency.LSL cim:Currency.LTL cim:Currency.LVL cim:Currency.LYD cim:Currency.MAD
    cim:Currency.MDL cim:Currency.MGA cim:Currency.MKD cim:Currency.MMK cim:Currency.MNT
    cim:Currency.MOP cim:Currency.MRO cim:Currency.MUR cim:Currency.MVR cim:Currency.MWK
    cim:Currency.MXN cim:Currency.MYR cim:Currency.MZN cim:Currency.NAD cim:Currency.NGN
    cim:Currency.NIO cim:Currency.NOK cim:Currency.NPR cim:Currency.NZD cim:Currency.OMR
    cim:Currency.PAB cim:Currency.PEN cim:Currency.PGK cim:Currency.PHP cim:Currency.PKR
    cim:Currency.PLN cim:Currency.PYG cim:Currency.QAR cim:Currency.RON cim:Currency.RSD
    cim:Currency.RUB cim:Currency.RWF cim:Currency.SAR cim:Currency.SBD cim:Currency.SCR
    cim:Currency.SDG cim:Currency.SEK cim:Currency.SGD cim:Currency.SHP cim:Currency.SLL
    cim:Currency.SOS cim:Currency.SRD cim:Currency.STD cim:Currency.SYP cim:Currency.SZL
    cim:Currency.THB cim:Currency.TJS cim:Currency.TMT cim:Currency.TND cim:Currency.TOP
    cim:Currency.TRY cim:Currency.TTD cim:Currency.TWD cim:Currency.TZS cim:Currency.UAH
    cim:Currency.UGX cim:Currency.USD cim:Currency.UYU cim:Currency.UZS cim:Currency.VEF
    cim:Currency.VND cim:Currency.VUV cim:Currency.WST cim:Currency.XAF cim:Currency.XCD
    cim:Currency.XOF cim:Currency.XPF cim:Currency.YER cim:Currency.ZAR cim:Currency.ZMK
    cim:Currency.ZWL ) ;
  rdfs:subClassOf cim:Enumeration ;
  skos:definition "Monetary currencies.  ISO 4217 standard including 3-character currency code."@en .

cim:CurrentFlow a owl:Class ;
  rdfs:label "CurrentFlow"@en ;
  eq:Package "Package_CoreEquipmentProfile" ;
  eq:isCIMDatatype "True" ;
  skos:definition "Electrical current with sign convention: positive flow is out of the conducting equipment into the connectivity node. Can be both AC and DC."@en .

cim:CurrentLimit a owl:Class ;
  rdfs:label "CurrentLimit"@en ;
  eq:Package "Package_CoreEquipmentProfile" ;
  rdfs:subClassOf cim:OperationalLimit ;
  skos:definition "Operational limit on current. "@en .

cim:CurrentTransformer a owl:Class ;
  rdfs:label "CurrentTransformer"@en ;
  eq:Package "Package_CoreEquipmentProfile" ;
  rdfs:subClassOf cim:Sensor ;
  skos:definition "Instrument transformer used to measure electrical qualities of the circuit that is being protected and/or monitored. Typically used as current transducer for the purpose of metering or protection. A typical secondary current rating would be 5A."@en .

cim:Curve a owl:Class ;
  rdfs:label "Curve"@en ;
  eq:Package "Package_CoreEquipmentProfile" ;
  eq:isAbstract "True" ;
  rdfs:subClassOf cim:IdentifiedObject ;
  skos:definition """
A multi-purpose curve or functional relationship between an independent variable (X-axis) and dependent (Y-axis) variables. 

\t"""@en .

cim:CurveData a owl:Class ;
  rdfs:label "CurveData"@en ;
  eq:Package "Package_CoreEquipmentProfile" ;
  skos:definition "Multi-purpose data points for defining a curve.  The use of this generic class is discouraged if a more specific class can be used to specify the X and Y axis values along with their specific data types."@en .

cim:CurveStyle a owl:Class ;
  rdfs:label "CurveStyle"@en ;
  eq:Package "Package_CoreEquipmentProfile" ;
  owl:oneOf ( cim:CurveStyle.constantYValue cim:CurveStyle.straightLineYValues ) ;
  rdfs:subClassOf cim:Enumeration ;
  skos:definition "Style or shape of curve."@en .

cim:Cut a owl:Class ;
  rdfs:label "Cut"@en ;
  eq:Package "Package_CoreEquipmentProfile" ;
  rdfs:subClassOf cim:Switch ;
  skos:definition """
A cut separates a line segment into two parts. The cut appears as a switch inserted between these two parts and connects them together. As the cut is normally open there is no galvanic connection between the two line segment parts. But it is possible to close the cut to get galvanic connection.
The cut terminals are oriented towards the line segment terminals with the same sequence number. Hence the cut terminal with sequence number equal to 1 is oriented to the line segment's terminal with sequence number equal to 1.
The cut terminals also act as connection points for jumpers and other equipment, e.g. a mobile generator. To enable this, connectivity nodes are placed at the cut terminals. Once the connectivity nodes are in place any conducting equipment can be connected at them.

\t"""@en .

cim:DCBaseTerminal a owl:Class ;
  rdfs:label "DCBaseTerminal"@en ;
  eq:Package "Package_CoreEquipmentProfile" ;
  eq:isAbstract "True" ;
  rdfs:subClassOf cim:ACDCTerminal ;
  skos:definition "An electrical connection point at a piece of DC conducting equipment. DC terminals are connected at one physical DC node that may have multiple DC terminals connected. A DC node is similar to an AC connectivity node. The model requires that DC connections are distinct from AC connections. "@en .

cim:DCBreaker a owl:Class ;
  rdfs:label "DCBreaker"@en ;
  eq:Package "Package_CoreEquipmentProfile" ;
  rdfs:subClassOf cim:DCSwitch ;
  skos:definition "A breaker within a DC system. "@en .

cim:DCBusbar a owl:Class ;
  rdfs:label "DCBusbar"@en ;
  eq:Package "Package_CoreEquipmentProfile" ;
  rdfs:subClassOf cim:DCConductingEquipment ;
  skos:definition "A busbar within a DC system."@en .

cim:DCChopper a owl:Class ;
  rdfs:label "DCChopper"@en ;
  eq:Package "Package_CoreEquipmentProfile" ;
  rdfs:subClassOf cim:DCConductingEquipment ;
  skos:definition "Low resistance equipment used in the internal DC circuit to balance voltages. It has typically positive and negative pole terminals and a ground."@en .

cim:DCConductingEquipment a owl:Class ;
  rdfs:label "DCConductingEquipment"@en ;
  eq:Package "Package_CoreEquipmentProfile" ;
  eq:isAbstract "True" ;
  rdfs:subClassOf cim:Equipment ;
  skos:definition "The parts of the DC power system that are designed to carry current or that are conductively connected through DC terminals."@en .

cim:DCConverterOperatingModeKind a owl:Class ;
  rdfs:label "DCConverterOperatingModeKind"@en ;
  eq:Package "Package_CoreEquipmentProfile" ;
  owl:oneOf ( cim:DCConverterOperatingModeKind.bipolar
    cim:DCConverterOperatingModeKind.monopolarMetallicReturn
    cim:DCConverterOperatingModeKind.monopolarGroundReturn ) ;
  rdfs:subClassOf cim:Enumeration ;
  skos:definition "The operating mode of an HVDC bipole."@en .

cim:DCConverterUnit a owl:Class ;
  rdfs:label "DCConverterUnit"@en ;
  eq:Package "Package_CoreEquipmentProfile" ;
  rdfs:subClassOf cim:DCEquipmentContainer ;
  skos:definition "Indivisible operative unit comprising all equipment between the point of common coupling on the AC side and the point of common coupling – DC side, essentially one or more converters, together with one or more converter transformers, converter control equipment, essential protective and switching devices and auxiliaries, if any, used for conversion."@en .

cim:DCDisconnector a owl:Class ;
  rdfs:label "DCDisconnector"@en ;
  eq:Package "Package_CoreEquipmentProfile" ;
  rdfs:subClassOf cim:DCSwitch ;
  skos:definition "A disconnector within a DC system."@en .

cim:DCEquipmentContainer a owl:Class ;
  rdfs:label "DCEquipmentContainer"@en ;
  eq:Package "Package_CoreEquipmentProfile" ;
  eq:isAbstract "True" ;
  rdfs:subClassOf cim:EquipmentContainer ;
  skos:definition "A modelling construct to provide a root class for containment of DC as well as AC equipment. The class differ from the EquipmentContaner for AC in that it may also contain DCNode-s. Hence it can contain both AC and DC equipment."@en .

cim:DCGround a owl:Class ;
  rdfs:label "DCGround"@en ;
  eq:Package "Package_CoreEquipmentProfile" ;
  rdfs:subClassOf cim:DCConductingEquipment ;
  skos:definition "A ground within a DC system."@en .

cim:DCLine a owl:Class ;
  rdfs:label "DCLine"@en ;
  eq:Package "Package_CoreEquipmentProfile" ;
  rdfs:subClassOf cim:DCEquipmentContainer ;
  skos:definition "Overhead lines and/or cables connecting two or more HVDC substations."@en .

cim:DCLineSegment a owl:Class ;
  rdfs:label "DCLineSegment"@en ;
  eq:Package "Package_CoreEquipmentProfile" ;
  rdfs:subClassOf cim:DCConductingEquipment ;
  skos:definition "A wire or combination of wires not insulated from one another, with consistent electrical characteristics, used to carry direct current between points in the DC region of the power system."@en .

cim:DCNode a owl:Class ;
  rdfs:label "DCNode"@en ;
  eq:Package "Package_CoreEquipmentProfile" ;
  rdfs:subClassOf cim:IdentifiedObject ;
  skos:definition "DC nodes are points where terminals of DC conducting equipment are connected together with zero impedance."@en .

cim:DCPolarityKind a owl:Class ;
  rdfs:label "DCPolarityKind"@en ;
  eq:Package "Package_CoreEquipmentProfile" ;
  owl:oneOf ( cim:DCPolarityKind.positive cim:DCPolarityKind.middle cim:DCPolarityKind.negative ) ;
  rdfs:subClassOf cim:Enumeration ;
  skos:definition "Polarity for DC circuits."@en .

cim:DCSeriesDevice a owl:Class ;
  rdfs:label "DCSeriesDevice"@en ;
  eq:Package "Package_CoreEquipmentProfile" ;
  rdfs:subClassOf cim:DCConductingEquipment ;
  skos:definition "A series device within the DC system, typically a reactor used for filtering or smoothing.  Needed for transient and short circuit studies."@en .

cim:DCShunt a owl:Class ;
  rdfs:label "DCShunt"@en ;
  eq:Package "Package_CoreEquipmentProfile" ;
  rdfs:subClassOf cim:DCConductingEquipment ;
  skos:definition "A shunt device within the DC system, typically used for filtering.  Needed for transient and short circuit studies."@en .

cim:DCSwitch a owl:Class ;
  rdfs:label "DCSwitch"@en ;
  eq:Package "Package_CoreEquipmentProfile" ;
  rdfs:subClassOf cim:DCConductingEquipment ;
  skos:definition "A switch within the DC system."@en .

cim:DCTerminal a owl:Class ;
  rdfs:label "DCTerminal"@en ;
  eq:Package "Package_CoreEquipmentProfile" ;
  rdfs:subClassOf cim:DCBaseTerminal ;
  skos:definition "An electrical connection point to generic DC conducting equipment."@en .

cim:Date a owl:Class ;
  rdfs:label "Date"@en ;
  eq:Package "Package_CoreEquipmentProfile" ;
  eq:isPrimitive "True" ;
  skos:definition "Date as \"yyyy-mm-dd\", which conforms with ISO 8601. UTC time zone is specified as \"yyyy-mm-ddZ\". A local timezone relative UTC is specified as \"yyyy-mm-dd(+/-)hh:mm\"."@en .

cim:DateTime a owl:Class ;
  rdfs:label "DateTime"@en ;
  eq:Package "Package_CoreEquipmentProfile" ;
  eq:isPrimitive "True" ;
  skos:definition "Date and time as \"yyyy-mm-ddThh:mm:ss.sss\", which conforms with ISO 8601. UTC time zone is specified as \"yyyy-mm-ddThh:mm:ss.sssZ\". A local timezone relative UTC is specified as \"yyyy-mm-ddThh:mm:ss.sss-hh:mm\". The second component (shown here as \"ss.sss\") could have any number of digits in its fractional part to allow any kind of precision beyond seconds."@en .

cim:DayType a owl:Class ;
  rdfs:label "DayType"@en ;
  eq:Package "Package_CoreEquipmentProfile" ;
  rdfs:subClassOf cim:IdentifiedObject ;
  skos:definition """
Group of similar days.   For example it could be used to represent weekdays, weekend, or holidays.

\t"""@en .

cim:Decimal a owl:Class ;
  rdfs:label "Decimal"@en ;
  eq:Package "Package_CoreEquipmentProfile" ;
  eq:isPrimitive "True" ;
  skos:definition """
Decimal is the base-10 notational system for representing real numbers.


\t"""@en .

cim:DisconnectingCircuitBreaker a owl:Class ;
  rdfs:label "DisconnectingCircuitBreaker"@en ;
  eq:Package "Package_CoreEquipmentProfile" ;
  rdfs:subClassOf cim:Breaker ;
  skos:definition "A circuit breaking device including disconnecting function, eliminating the need for separate disconnectors."@en .

cim:Disconnector a owl:Class ;
  rdfs:label "Disconnector"@en ;
  eq:Package "Package_CoreEquipmentProfile" ;
  rdfs:subClassOf cim:Switch ;
  skos:definition "A manually operated or motor operated mechanical switching device used for changing the connections in a circuit, or for isolating a circuit or equipment from a source of power. It is required to open or close circuits when negligible current is broken or made. "@en .

cim:EarthFaultCompensator a owl:Class ;
  rdfs:label "EarthFaultCompensator"@en ;
  eq:Package "Package_CoreEquipmentProfile" ;
  eq:isAbstract "True" ;
  rdfs:subClassOf cim:ConductingEquipment ;
  skos:definition "A conducting equipment used to represent a connection to ground which is typically used to compensate earth faults.   An earth fault compensator device modelled with a single terminal implies a second terminal solidly connected to ground.  If two terminals are modelled, the ground is not assumed and normal connection rules apply."@en .

cim:EnergyArea a owl:Class ;
  rdfs:label "EnergyArea"@en ;
  eq:Package "Package_CoreEquipmentProfile" ;
  eq:isAbstract "True" ;
  rdfs:subClassOf cim:IdentifiedObject ;
  skos:definition "Describes an area having energy production or consumption.  Specializations are intended to support the load allocation function as typically required in energy management systems or planning studies to allocate hypothesized load levels to individual load points for power flow analysis.  Often the energy area can be linked to both measured and forecast load levels."@en .

cim:EnergyConnection a owl:Class ;
  rdfs:label "EnergyConnection"@en ;
  eq:Package "Package_CoreEquipmentProfile" ;
  eq:isAbstract "True" ;
  rdfs:subClassOf cim:ConductingEquipment ;
  skos:definition "A connection of energy generation or consumption on the power system model."@en .

cim:EnergyConsumer a owl:Class ;
  rdfs:label "EnergyConsumer"@en ;
  eq:Package "Package_CoreEquipmentProfile" ;
  rdfs:subClassOf cim:EnergyConnection ;
  skos:definition """
Generic user of energy - a  point of consumption on the power system model.
EnergyConsumer.pfixed, .qfixed, .pfixedPct and .qfixedPct have meaning only if there is no LoadResponseCharacteristic associated with EnergyConsumer or if LoadResponseCharacteristic.exponentModel is set to False.
\t"""@en .

cim:EnergySchedulingType a owl:Class ;
  rdfs:label "EnergySchedulingType"@en ;
  eq:Package "Package_CoreEquipmentProfile" ;
  rdfs:subClassOf cim:IdentifiedObject ;
  skos:definition "Used to define the type of generation for scheduling purposes."@en .

cim:EnergySource a owl:Class ;
  rdfs:label "EnergySource"@en ;
  eq:Package "Package_CoreEquipmentProfile" ;
  rdfs:subClassOf cim:EnergyConnection ;
  skos:definition "A generic equivalent for an energy supplier on a transmission or distribution voltage level."@en .

cim:Equipment a owl:Class ;
  rdfs:label "Equipment"@en ;
  eq:Package "Package_CoreEquipmentProfile" ;
  eq:isAbstract "True" ;
  rdfs:subClassOf cim:PowerSystemResource ;
  skos:definition "The parts of a power system that are physical devices, electronic or mechanical."@en .

cim:EquipmentContainer a owl:Class ;
  rdfs:label "EquipmentContainer"@en ;
  eq:Package "Package_CoreEquipmentProfile" ;
  eq:isAbstract "True" ;
  rdfs:subClassOf cim:ConnectivityNodeContainer ;
  skos:definition "A modelling construct to provide a root class for containing equipment. "@en .

cim:EquivalentBranch a owl:Class ;
  rdfs:label "EquivalentBranch"@en ;
  eq:Package "Package_CoreEquipmentProfile" ;
  rdfs:subClassOf cim:EquivalentEquipment ;
  skos:definition "The class represents equivalent branches. In cases where a transformer phase shift is modelled and the EquivalentBranch is spanning the same nodes, the impedance quantities for the EquivalentBranch shall consider the needed phase shift."@en .

cim:EquivalentEquipment a owl:Class ;
  rdfs:label "EquivalentEquipment"@en ;
  eq:Package "Package_CoreEquipmentProfile" ;
  eq:isAbstract "True" ;
  rdfs:subClassOf cim:ConductingEquipment ;
  skos:definition "The class represents equivalent objects that are the result of a network reduction. The class is the base for equivalent objects of different types."@en .

cim:EquivalentInjection a owl:Class ;
  rdfs:label "EquivalentInjection"@en ;
  eq:Package "Package_CoreEquipmentProfile" ;
  rdfs:subClassOf cim:EquivalentEquipment ;
  skos:definition "This class represents equivalent injections (generation or load).  Voltage regulation is allowed only at the point of connection."@en .

cim:EquivalentNetwork a owl:Class ;
  rdfs:label "EquivalentNetwork"@en ;
  eq:Package "Package_CoreEquipmentProfile" ;
  rdfs:subClassOf cim:ConnectivityNodeContainer ;
  skos:definition "A class that groups electrical equivalents, including internal nodes, of a network that has been reduced. The ConnectivityNodes contained in the equivalent are intended to reflect internal nodes of the equivalent. The boundary Connectivity nodes where the equivalent connects outside itself are not contained by the equivalent."@en .

cim:EquivalentShunt a owl:Class ;
  rdfs:label "EquivalentShunt"@en ;
  eq:Package "Package_CoreEquipmentProfile" ;
  rdfs:subClassOf cim:EquivalentEquipment ;
  skos:definition "The class represents equivalent shunts."@en .

cim:ExternalNetworkInjection a owl:Class ;
  rdfs:label "ExternalNetworkInjection"@en ;
  eq:Package "Package_CoreEquipmentProfile" ;
  rdfs:subClassOf cim:RegulatingCondEq ;
  skos:definition "This class represents the external network and it is used for IEC 60909 calculations."@en .

cim:FaultIndicator a owl:Class ;
  rdfs:label "FaultIndicator"@en ;
  eq:Package "Package_CoreEquipmentProfile" ;
  rdfs:subClassOf cim:AuxiliaryEquipment ;
  skos:definition "A FaultIndicator is typically only an indicator (which may or may not be remotely monitored), and not a piece of equipment that actually initiates a protection event. It is used for FLISR (Fault Location, Isolation and Restoration) purposes, assisting with the dispatch of crews to \"most likely\" part of the network (i.e. assists with determining circuit section where the fault most likely happened)."@en .

cim:Float a owl:Class ;
  rdfs:label "Float"@en ;
  eq:Package "Package_CoreEquipmentProfile" ;
  eq:isPrimitive "True" ;
  skos:definition """
A floating point number. The range is unspecified and not limited.

\t"""@en .

cim:FossilFuel a owl:Class ;
  rdfs:label "FossilFuel"@en ;
  eq:Package "Package_CoreEquipmentProfile" ;
  rdfs:subClassOf cim:IdentifiedObject ;
  skos:definition "The fossil fuel consumed by the non-nuclear thermal generating unit.   For example, coal, oil, gas, etc.   These are the specific fuels that the generating unit can consume."@en .

cim:Frequency a owl:Class ;
  rdfs:label "Frequency"@en ;
  eq:Package "Package_CoreEquipmentProfile" ;
  eq:isCIMDatatype "True" ;
  skos:definition "Cycles per second."@en .

cim:FuelType a owl:Class ;
  rdfs:label "FuelType"@en ;
  eq:Package "Package_CoreEquipmentProfile" ;
  owl:oneOf ( cim:FuelType.coal cim:FuelType.oil cim:FuelType.gas cim:FuelType.lignite
    cim:FuelType.hardCoal cim:FuelType.oilShale cim:FuelType.brownCoalLignite
    cim:FuelType.coalDerivedGas cim:FuelType.peat cim:FuelType.other ) ;
  rdfs:subClassOf cim:Enumeration ;
  skos:definition "Type of fuel."@en .

cim:Fuse a owl:Class ;
  rdfs:label "Fuse"@en ;
  eq:Package "Package_CoreEquipmentProfile" ;
  rdfs:subClassOf cim:Switch ;
  skos:definition "An overcurrent protective device with a circuit opening fusible part that is heated and severed by the passage of overcurrent through it. A fuse is considered a switching device because it breaks current."@en .

cim:GeneratingUnit a owl:Class ;
  rdfs:label "GeneratingUnit"@en ;
  eq:Package "Package_CoreEquipmentProfile" ;
  rdfs:subClassOf cim:Equipment ;
  skos:definition "A single or set of synchronous machines for converting mechanical power into alternating-current power. For example, individual machines within a set may be defined for scheduling purposes while a single control signal is derived for the set. In this case there would be a GeneratingUnit for each member of the set and an additional GeneratingUnit corresponding to the set."@en .

cim:GeneratorControlSource a owl:Class ;
  rdfs:label "GeneratorControlSource"@en ;
  eq:Package "Package_CoreEquipmentProfile" ;
  owl:oneOf ( cim:GeneratorControlSource.unavailable cim:GeneratorControlSource.offAGC
    cim:GeneratorControlSource.onAGC cim:GeneratorControlSource.plantControl ) ;
  rdfs:subClassOf cim:Enumeration ;
  skos:definition """
The source of controls for a generating unit.

\t"""@en .

cim:GeographicalRegion a owl:Class ;
  rdfs:label "GeographicalRegion"@en ;
  eq:Package "Package_CoreEquipmentProfile" ;
  rdfs:subClassOf cim:IdentifiedObject ;
  skos:definition """
A geographical region of a power system network model.

\t"""@en .

cim:GrossToNetActivePowerCurve a owl:Class ;
  rdfs:label "GrossToNetActivePowerCurve"@en ;
  eq:Package "Package_CoreEquipmentProfile" ;
  rdfs:subClassOf cim:Curve ;
  skos:definition "Relationship between the generating unit's gross active power output on the X-axis (measured at the terminals of the machine(s)) and the generating unit's net active power output on the Y-axis (based on utility-defined measurements at the power station). Station service loads, when modelled, should be treated as non-conforming bus loads. There may be more than one curve, depending on the auxiliary equipment that is in service."@en .

cim:Ground a owl:Class ;
  rdfs:label "Ground"@en ;
  eq:Package "Package_CoreEquipmentProfile" ;
  rdfs:subClassOf cim:ConductingEquipment ;
  skos:definition "A point where the system is grounded used for connecting conducting equipment to ground. The power system model can have any number of grounds."@en .

cim:GroundDisconnector a owl:Class ;
  rdfs:label "GroundDisconnector"@en ;
  eq:Package "Package_CoreEquipmentProfile" ;
  rdfs:subClassOf cim:Switch ;
  skos:definition "A manually operated or motor operated mechanical switching device used for isolating a circuit or equipment from ground."@en .

cim:GroundingImpedance a owl:Class ;
  rdfs:label "GroundingImpedance"@en ;
  eq:Package "Package_CoreEquipmentProfile" ;
  rdfs:subClassOf cim:EarthFaultCompensator ;
  skos:definition "A fixed impedance device used for grounding."@en .

cim:HydroEnergyConversionKind a owl:Class ;
  rdfs:label "HydroEnergyConversionKind"@en ;
  eq:Package "Package_CoreEquipmentProfile" ;
  owl:oneOf ( cim:HydroEnergyConversionKind.generator cim:HydroEnergyConversionKind.pumpAndGenerator ) ;
  rdfs:subClassOf cim:Enumeration ;
  skos:definition """
Specifies the capability of the hydro generating unit to convert energy as a generator or pump.

\t"""@en .

cim:HydroGeneratingUnit a owl:Class ;
  rdfs:label "HydroGeneratingUnit"@en ;
  eq:Package "Package_CoreEquipmentProfile" ;
  rdfs:subClassOf cim:GeneratingUnit ;
  skos:definition """
A generating unit whose prime mover is a hydraulic turbine (e.g., Francis, Pelton, Kaplan).

\t"""@en .

cim:HydroPlantStorageKind a owl:Class ;
  rdfs:label "HydroPlantStorageKind"@en ;
  eq:Package "Package_CoreEquipmentProfile" ;
  owl:oneOf ( cim:HydroPlantStorageKind.runOfRiver cim:HydroPlantStorageKind.pumpedStorage
    cim:HydroPlantStorageKind.storage ) ;
  rdfs:subClassOf cim:Enumeration ;
  skos:definition """
The type of hydro power plant.

\t"""@en .

cim:HydroPowerPlant a owl:Class ;
  rdfs:label "HydroPowerPlant"@en ;
  eq:Package "Package_CoreEquipmentProfile" ;
  rdfs:subClassOf cim:PowerSystemResource ;
  skos:definition "A hydro power station which can generate or pump. When generating, the generator turbines receive water from an upper reservoir. When pumping, the pumps receive their water from a lower reservoir."@en .

cim:HydroPump a owl:Class ;
  rdfs:label "HydroPump"@en ;
  eq:Package "Package_CoreEquipmentProfile" ;
  rdfs:subClassOf cim:Equipment ;
  skos:definition "A synchronous motor-driven pump, typically associated with a pumped storage plant."@en .

cim:HydroTurbineKind a owl:Class ;
  rdfs:label "HydroTurbineKind"@en ;
  eq:Package "Package_CoreEquipmentProfile" ;
  owl:oneOf ( cim:HydroTurbineKind.francis cim:HydroTurbineKind.pelton cim:HydroTurbineKind.kaplan ) ;
  rdfs:subClassOf cim:Enumeration ;
  skos:definition "Type of turbine."@en .

cim:IdentifiedObject a owl:Class ;
  rdfs:label "IdentifiedObject"@en ;
  eq:Package "Package_CoreEquipmentProfile" ;
  eq:isAbstract "True" ;
  skos:definition "This is a root class to provide common identification for all classes needing identification and naming attributes."@en .

cim:Inductance a owl:Class ;
  rdfs:label "Inductance"@en ;
  eq:Package "Package_CoreEquipmentProfile" ;
  eq:isCIMDatatype "True" ;
  skos:definition """
Inductive part of reactance (imaginary part of impedance), at rated frequency.

\t"""@en .

cim:Integer a owl:Class ;
  rdfs:label "Integer"@en ;
  eq:Package "Package_CoreEquipmentProfile" ;
  eq:isPrimitive "True" ;
  skos:definition """
An integer number. The range is unspecified and not limited.

\t"""@en .

cim:Jumper a owl:Class ;
  rdfs:label "Jumper"@en ;
  eq:Package "Package_CoreEquipmentProfile" ;
  rdfs:subClassOf cim:Switch ;
  skos:definition "A short section of conductor with negligible impedance which can be manually removed and replaced if the circuit is de-energized. Note that zero-impedance branches can potentially be modelled by other equipment types."@en .

cim:Junction a owl:Class ;
  rdfs:label "Junction"@en ;
  eq:Package "Package_CoreEquipmentProfile" ;
  rdfs:subClassOf cim:Connector ;
  skos:definition "A point where one or more conducting equipments are connected with zero resistance."@en .

cim:Length a owl:Class ;
  rdfs:label "Length"@en ;
  eq:Package "Package_CoreEquipmentProfile" ;
  eq:isCIMDatatype "True" ;
  skos:definition "Unit of length. It shall be a positive value or zero."@en .

cim:Line a owl:Class ;
  rdfs:label "Line"@en ;
  eq:Package "Package_CoreEquipmentProfile" ;
  rdfs:subClassOf cim:EquipmentContainer ;
  skos:definition "Contains equipment beyond a substation belonging to a power transmission line. "@en .

cim:LinearShuntCompensator a owl:Class ;
  rdfs:label "LinearShuntCompensator"@en ;
  eq:Package "Package_CoreEquipmentProfile" ;
  rdfs:subClassOf cim:ShuntCompensator ;
  skos:definition "A linear shunt compensator has banks or sections with equal admittance values."@en .

cim:LoadArea a owl:Class ;
  rdfs:label "LoadArea"@en ;
  eq:Package "Package_CoreEquipmentProfile" ;
  rdfs:subClassOf cim:EnergyArea ;
  skos:definition "The class is the root or first level in a hierarchical structure for grouping of loads for the purpose of load flow load scaling."@en .

cim:LoadBreakSwitch a owl:Class ;
  rdfs:label "LoadBreakSwitch"@en ;
  eq:Package "Package_CoreEquipmentProfile" ;
  rdfs:subClassOf cim:ProtectedSwitch ;
  skos:definition "A mechanical switching device capable of making, carrying, and breaking currents under normal operating conditions."@en .

cim:LoadGroup a owl:Class ;
  rdfs:label "LoadGroup"@en ;
  eq:Package "Package_CoreEquipmentProfile" ;
  eq:isAbstract "True" ;
  rdfs:subClassOf cim:IdentifiedObject ;
  skos:definition "The class is the third level in a hierarchical structure for grouping of loads for the purpose of load flow load scaling."@en .

cim:LoadResponseCharacteristic a owl:Class ;
  rdfs:label "LoadResponseCharacteristic"@en ;
  eq:Package "Package_CoreEquipmentProfile" ;
  rdfs:subClassOf cim:IdentifiedObject ;
  skos:definition """
Models the characteristic response of the load demand due to changes in system conditions such as voltage and frequency. It is not related to demand response.
If LoadResponseCharacteristic.exponentModel is True, the exponential voltage or frequency dependent models are specified and used as to calculate active and reactive power components of the load model.
The equations to calculate active and reactive power components of the load model are internal to the power flow calculation, hence they use different quantities depending on the use case of the data exchange. 
The equations for exponential voltage dependent load model injected power are: 
pInjection= Pnominal* (Voltage/cim:BaseVoltage.nominalVoltage) ** cim:LoadResponseCharacteristic.pVoltageExponent
qInjection= Qnominal* (Voltage/cim:BaseVoltage.nominalVoltage) ** cim:LoadResponseCharacteristic.qVoltageExponent
Where: 
1) * means "multiply" and ** is "raised to power of";
2) Pnominal and Qnominal represent the active power and reactive power at nominal voltage as any load described by the voltage exponential model shall be given at nominal voltage.  This means that EnergyConsumer.p and EnergyConsumer.q  are at nominal voltage.
3) After power flow is solved: 
-pInjection and qInjection correspond to SvPowerflow.p and SvPowerflow.q respectively.  
- Voltage corresponds to SvVoltage.v at the TopologicalNode where the load is connected.
\t"""@en .

cim:Money a owl:Class ;
  rdfs:label "Money"@en ;
  eq:Package "Package_CoreEquipmentProfile" ;
  eq:isCIMDatatype "True" ;
  skos:definition """
Amount of money.

\t"""@en .

cim:MonthDay a owl:Class ;
  rdfs:label "MonthDay"@en ;
  eq:Package "Package_CoreEquipmentProfile" ;
  eq:isPrimitive "True" ;
  skos:definition "MonthDay format as \"--mm-dd\", which conforms with XSD data type gMonthDay."@en .

cim:NonConformLoad a owl:Class ;
  rdfs:label "NonConformLoad"@en ;
  eq:Package "Package_CoreEquipmentProfile" ;
  rdfs:subClassOf cim:EnergyConsumer ;
  skos:definition "NonConformLoad represents loads that do not follow a daily load change pattern and whose changes are not correlated with the daily load change pattern."@en .

cim:NonConformLoadGroup a owl:Class ;
  rdfs:label "NonConformLoadGroup"@en ;
  eq:Package "Package_CoreEquipmentProfile" ;
  rdfs:subClassOf cim:LoadGroup ;
  skos:definition "Loads that do not follow a daily and seasonal load variation pattern."@en .

cim:NonConformLoadSchedule a owl:Class ;
  rdfs:label "NonConformLoadSchedule"@en ;
  eq:Package "Package_CoreEquipmentProfile" ;
  rdfs:subClassOf cim:SeasonDayTypeSchedule ;
  skos:definition "An active power (Y1-axis) and reactive power (Y2-axis) schedule (curves) versus time (X-axis) for non-conforming loads, e.g., large industrial load or power station service (where modelled)."@en .

cim:NonlinearShuntCompensator a owl:Class ;
  rdfs:label "NonlinearShuntCompensator"@en ;
  eq:Package "Package_CoreEquipmentProfile" ;
  rdfs:subClassOf cim:ShuntCompensator ;
  skos:definition "A non linear shunt compensator has bank or section admittance values that differ. The attributes g, b, g0 and b0 of the associated NonlinearShuntCompensatorPoint describe the total conductance and admittance of a NonlinearShuntCompensatorPoint at a section number specified by NonlinearShuntCompensatorPoint.sectionNumber."@en .

cim:NonlinearShuntCompensatorPoint a owl:Class ;
  rdfs:label "NonlinearShuntCompensatorPoint"@en ;
  eq:Package "Package_CoreEquipmentProfile" ;
  skos:definition "A non linear shunt compensator bank or section admittance value. The number of NonlinearShuntCompenstorPoint instances associated with a NonlinearShuntCompensator shall be equal to ShuntCompensator.maximumSections. ShuntCompensator.sections shall only be set to one of the NonlinearShuntCompenstorPoint.sectionNumber. There is no interpolation between NonlinearShuntCompenstorPoint-s."@en .

cim:NuclearGeneratingUnit a owl:Class ;
  rdfs:label "NuclearGeneratingUnit"@en ;
  eq:Package "Package_CoreEquipmentProfile" ;
  rdfs:subClassOf cim:GeneratingUnit ;
  skos:definition "A nuclear generating unit."@en .

cim:OperationalLimit a owl:Class ;
  rdfs:label "OperationalLimit"@en ;
  eq:Package "Package_CoreEquipmentProfile" ;
  eq:isAbstract "True" ;
  rdfs:subClassOf cim:IdentifiedObject ;
  skos:definition """
A value and normal value associated with a specific kind of limit. 
The sub class value and normalValue attributes vary inversely to the associated OperationalLimitType.acceptableDuration (acceptableDuration for short).  
If a particular piece of equipment has multiple operational limits of the same kind (apparent power, current, etc.), the limit with the greatest acceptableDuration shall have the smallest limit value and the limit with the smallest acceptableDuration shall have the largest limit value.  Note: A large current can only be allowed to flow through a piece of equipment for a short duration without causing damage, but a lesser current can be allowed to flow for a longer duration. 
\t"""@en .

cim:OperationalLimitDirectionKind a owl:Class ;
  rdfs:label "OperationalLimitDirectionKind"@en ;
  eq:Package "Package_CoreEquipmentProfile" ;
  owl:oneOf ( cim:OperationalLimitDirectionKind.high cim:OperationalLimitDirectionKind.low
    cim:OperationalLimitDirectionKind.absoluteValue ) ;
  rdfs:subClassOf cim:Enumeration ;
  skos:definition "The direction attribute describes the side of  a limit that is a violation."@en .

cim:OperationalLimitSet a owl:Class ;
  rdfs:label "OperationalLimitSet"@en ;
  eq:Package "Package_CoreEquipmentProfile" ;
  rdfs:subClassOf cim:IdentifiedObject ;
  skos:definition """
A set of limits associated with equipment.  Sets of limits might apply to a specific temperature, or season for example. A set of limits may contain different severities of limit levels that would apply to the same equipment. The set may contain limits of different types such as apparent power and current limits or high and low voltage limits  that are logically applied together as a set.

\t"""@en .

cim:OperationalLimitType a owl:Class ;
  rdfs:label "OperationalLimitType"@en ;
  eq:Package "Package_CoreEquipmentProfile" ;
  rdfs:subClassOf cim:IdentifiedObject ;
  skos:definition """
The operational meaning of a category of limits.

\t"""@en .

cim:PerCent a owl:Class ;
  rdfs:label "PerCent"@en ;
  eq:Package "Package_CoreEquipmentProfile" ;
  eq:isCIMDatatype "True" ;
  skos:definition """
Percentage on a defined base.   For example, specify as 100 to indicate at the defined base.

\t"""@en .

cim:PetersenCoil a owl:Class ;
  rdfs:label "PetersenCoil"@en ;
  eq:Package "Package_CoreEquipmentProfile" ;
  rdfs:subClassOf cim:EarthFaultCompensator ;
  skos:definition "A variable impedance device normally used to offset line charging during single line faults in an ungrounded section of network."@en .

cim:PhaseCode a owl:Class ;
  rdfs:label "PhaseCode"@en ;
  eq:Package "Package_CoreEquipmentProfile" ;
  owl:oneOf ( cim:PhaseCode.ABCN cim:PhaseCode.ABC cim:PhaseCode.ABN cim:PhaseCode.ACN
    cim:PhaseCode.BCN cim:PhaseCode.AB cim:PhaseCode.AC cim:PhaseCode.BC cim:PhaseCode.AN
    cim:PhaseCode.BN cim:PhaseCode.CN cim:PhaseCode.A cim:PhaseCode.B cim:PhaseCode.C
    cim:PhaseCode.N cim:PhaseCode.s1N cim:PhaseCode.s2N cim:PhaseCode.s12N cim:PhaseCode.s1
    cim:PhaseCode.s2 cim:PhaseCode.s12 cim:PhaseCode.none cim:PhaseCode.X cim:PhaseCode.XY
    cim:PhaseCode.XN cim:PhaseCode.XYN ) ;
  rdfs:subClassOf cim:Enumeration ;
  skos:definition """
An unordered enumeration of phase identifiers.  Allows designation of phases for both transmission and distribution equipment, circuits and loads.   The enumeration, by itself, does not describe how the phases are connected together or connected to ground.  Ground is not explicitly denoted as a phase.
Residential and small commercial loads are often served from single-phase, or split-phase, secondary circuits. For the example of s12N, phases 1 and 2 refer to hot wires that are 180 degrees out of phase, while N refers to the neutral wire. Through single-phase transformer connections, these secondary circuits may be served from one or two of the primary phases A, B, and C. For three-phase loads, use the A, B, C phase codes instead of s12N.
The integer values are from IEC 61968-9 to support revenue metering applications.
\t"""@en .

cim:PhaseTapChanger a owl:Class ;
  rdfs:label "PhaseTapChanger"@en ;
  eq:Package "Package_CoreEquipmentProfile" ;
  eq:isAbstract "True" ;
  rdfs:subClassOf cim:TapChanger ;
  skos:definition "A transformer phase shifting tap model that controls the phase angle difference across the power transformer and potentially the active power flow through the power transformer.  This phase tap model may also impact the voltage magnitude."@en .

cim:PhaseTapChangerAsymmetrical a owl:Class ;
  rdfs:label "PhaseTapChangerAsymmetrical"@en ;
  eq:Package "Package_CoreEquipmentProfile" ;
  rdfs:subClassOf cim:PhaseTapChangerNonLinear ;
  skos:definition "Describes the tap model for an asymmetrical phase shifting transformer in which the difference voltage vector adds to the in-phase winding. The out-of-phase winding is the transformer end where the tap changer is located.  The angle between the in-phase and out-of-phase windings is named the winding connection angle. The phase shift depends on both the difference voltage magnitude and the winding connection angle."@en .

cim:PhaseTapChangerLinear a owl:Class ;
  rdfs:label "PhaseTapChangerLinear"@en ;
  eq:Package "Package_CoreEquipmentProfile" ;
  rdfs:subClassOf cim:PhaseTapChanger ;
  skos:definition """
Describes a tap changer with a linear relation between the tap step and the phase angle difference across the transformer. This is a mathematical model that is an approximation of a real phase tap changer.
The phase angle is computed as stepPhaseShiftIncrement times the tap position.
The voltage magnitude of both sides is the same.
\t"""@en .

cim:PhaseTapChangerNonLinear a owl:Class ;
  rdfs:label "PhaseTapChangerNonLinear"@en ;
  eq:Package "Package_CoreEquipmentProfile" ;
  eq:isAbstract "True" ;
  rdfs:subClassOf cim:PhaseTapChanger ;
  skos:definition "The non-linear phase tap changer describes the non-linear behaviour of a phase tap changer. This is a base class for the symmetrical and asymmetrical phase tap changer models. The details of these models can be found in IEC 61970-301."@en .

cim:PhaseTapChangerSymmetrical a owl:Class ;
  rdfs:label "PhaseTapChangerSymmetrical"@en ;
  eq:Package "Package_CoreEquipmentProfile" ;
  rdfs:subClassOf cim:PhaseTapChangerNonLinear ;
  skos:definition "Describes a symmetrical phase shifting transformer tap model in which the voltage magnitude of both sides is the same. The difference voltage magnitude is the base in an equal-sided triangle where the sides corresponds to the primary and secondary voltages. The phase angle difference corresponds to the top angle and can be expressed as twice the arctangent of half the total difference voltage."@en .

cim:PhaseTapChangerTable a owl:Class ;
  rdfs:label "PhaseTapChangerTable"@en ;
  eq:Package "Package_CoreEquipmentProfile" ;
  rdfs:subClassOf cim:IdentifiedObject ;
  skos:definition "Describes a tabular curve for how the phase angle difference and impedance varies with the tap step."@en .

cim:PhaseTapChangerTablePoint a owl:Class ;
  rdfs:label "PhaseTapChangerTablePoint"@en ;
  eq:Package "Package_CoreEquipmentProfile" ;
  rdfs:subClassOf cim:TapChangerTablePoint ;
  skos:definition """
Describes each tap step in the phase tap changer tabular curve.

\t"""@en .

cim:PhaseTapChangerTabular a owl:Class ;
  rdfs:label "PhaseTapChangerTabular"@en ;
  eq:Package "Package_CoreEquipmentProfile" ;
  rdfs:subClassOf cim:PhaseTapChanger ;
  skos:definition "Describes a tap changer with a table defining the relation between the tap step and the phase angle difference across the transformer. "@en .

cim:PhotoVoltaicUnit a owl:Class ;
  rdfs:label "PhotoVoltaicUnit"@en ;
  eq:Package "Package_CoreEquipmentProfile" ;
  rdfs:subClassOf cim:PowerElectronicsUnit ;
  skos:definition "A photovoltaic device or an aggregation of such devices."@en .

cim:PostLineSensor a owl:Class ;
  rdfs:label "PostLineSensor"@en ;
  eq:Package "Package_CoreEquipmentProfile" ;
  rdfs:subClassOf cim:Sensor ;
  skos:definition """
 A sensor used mainly in overhead distribution networks as the source of both current and voltage measurements.

\t"""@en .

cim:PotentialTransformer a owl:Class ;
  rdfs:label "PotentialTransformer"@en ;
  eq:Package "Package_CoreEquipmentProfile" ;
  rdfs:subClassOf cim:Sensor ;
  skos:definition "Instrument transformer (also known as Voltage Transformer) used to measure electrical qualities of the circuit that is being protected and/or monitored. Typically used as voltage transducer for the purpose of metering, protection, or sometimes auxiliary substation supply. A typical secondary voltage rating would be 120V."@en .

cim:PowerElectronicsConnection a owl:Class ;
  rdfs:label "PowerElectronicsConnection"@en ;
  eq:Package "Package_CoreEquipmentProfile" ;
  rdfs:subClassOf cim:RegulatingCondEq ;
  skos:definition "A connection to the AC network for energy production or consumption that uses power electronics rather than rotating machines."@en .

cim:PowerElectronicsUnit a owl:Class ;
  rdfs:label "PowerElectronicsUnit"@en ;
  eq:Package "Package_CoreEquipmentProfile" ;
  eq:isAbstract "True" ;
  rdfs:subClassOf cim:Equipment ;
  skos:definition "A generating unit or battery or aggregation that connects to the AC network using power electronics rather than rotating machines."@en .

cim:PowerElectronicsWindUnit a owl:Class ;
  rdfs:label "PowerElectronicsWindUnit"@en ;
  eq:Package "Package_CoreEquipmentProfile" ;
  rdfs:subClassOf cim:PowerElectronicsUnit ;
  skos:definition "A wind generating unit that connects to the AC network with power electronics rather than rotating machines or an aggregation of such units."@en .

cim:PowerSystemResource a owl:Class ;
  rdfs:label "PowerSystemResource"@en ;
  eq:Package "Package_CoreEquipmentProfile" ;
  eq:isAbstract "True" ;
  rdfs:subClassOf cim:IdentifiedObject ;
  skos:definition "A power system resource (PSR) can be an item of equipment such as a switch, an equipment container containing many individual items of equipment such as a substation, or an organisational entity such as sub-control area. Power system resources can have measurements associated."@en .

cim:PowerTransformer a owl:Class ;
  rdfs:label "PowerTransformer"@en ;
  eq:Package "Package_CoreEquipmentProfile" ;
  rdfs:subClassOf cim:ConductingEquipment ;
  skos:definition """
An electrical device consisting of  two or more coupled windings, with or without a magnetic core, for introducing mutual coupling between electric circuits. Transformers can be used to control voltage and phase shift (active power flow).
A power transformer may be composed of separate transformer tanks that need not be identical.
A power transformer can be modelled with or without tanks and is intended for use in both balanced and unbalanced representations.   A power transformer typically has two terminals, but may have one (grounding), three or more terminals.
The inherited association ConductingEquipment.BaseVoltage should not be used.  The association from TransformerEnd to BaseVoltage should be used instead.
\t"""@en .

cim:PowerTransformerEnd a owl:Class ;
  rdfs:label "PowerTransformerEnd"@en ;
  eq:Package "Package_CoreEquipmentProfile" ;
  rdfs:subClassOf cim:TransformerEnd ;
  skos:definition """
A PowerTransformerEnd is associated with each Terminal of a PowerTransformer.
The impedance values r, r0, x, and x0 of a PowerTransformerEnd represents a star equivalent as follows.
1) for a two Terminal PowerTransformer the high voltage (TransformerEnd.endNumber=1) PowerTransformerEnd has non zero values on r, r0, x, and x0 while the low voltage (TransformerEnd.endNumber=2) PowerTransformerEnd has zero values for r, r0, x, and x0.  Parameters are always provided, even if the PowerTransformerEnds have the same rated voltage.  In this case, the parameters are provided at the PowerTransformerEnd which has TransformerEnd.endNumber equal to 1.
2) for a three Terminal PowerTransformer the three PowerTransformerEnds represent a star equivalent with each leg in the star represented by r, r0, x, and x0 values.
3) For a three Terminal transformer each PowerTransformerEnd shall have g, g0, b and b0 values corresponding to the no load losses distributed on the three PowerTransformerEnds. The total no load loss shunt impedances may also be placed at one of the PowerTransformerEnds, preferably the end numbered 1, having the shunt values on end 1.  This is the preferred way.
4) for a PowerTransformer with more than three Terminals the PowerTransformerEnd impedance values cannot be used. Instead use the TransformerMeshImpedance or split the transformer into multiple PowerTransformers.
Each PowerTransformerEnd must be contained by a PowerTransformer. Because a PowerTransformerEnd (or any other object) can not be contained by more than one parent, a PowerTransformerEnd can not have an association to an EquipmentContainer (Substation, VoltageLevel, etc).
\t"""@en .

cim:ProtectedSwitch a owl:Class ;
  rdfs:label "ProtectedSwitch"@en ;
  eq:Package "Package_CoreEquipmentProfile" ;
  eq:isAbstract "True" ;
  rdfs:subClassOf cim:Switch ;
  skos:definition "A ProtectedSwitch is a switching device that can be operated by ProtectionEquipment."@en .

cim:RatioTapChanger a owl:Class ;
  rdfs:label "RatioTapChanger"@en ;
  eq:Package "Package_CoreEquipmentProfile" ;
  rdfs:subClassOf cim:TapChanger ;
  skos:definition """
A tap changer that changes the voltage ratio impacting the voltage magnitude but not the phase angle across the transformer.

Angle sign convention (general): Positive value indicates a positive phase shift from the winding where the tap is located to the other winding (for a two-winding transformer).
\t"""@en .

cim:RatioTapChangerTable a owl:Class ;
  rdfs:label "RatioTapChangerTable"@en ;
  eq:Package "Package_CoreEquipmentProfile" ;
  rdfs:subClassOf cim:IdentifiedObject ;
  skos:definition "Describes a curve for how the voltage magnitude and impedance varies with the tap step. "@en .

cim:RatioTapChangerTablePoint a owl:Class ;
  rdfs:label "RatioTapChangerTablePoint"@en ;
  eq:Package "Package_CoreEquipmentProfile" ;
  rdfs:subClassOf cim:TapChangerTablePoint ;
  skos:definition """
Describes each tap step in the ratio tap changer tabular curve.

\t"""@en .

cim:Reactance a owl:Class ;
  rdfs:label "Reactance"@en ;
  eq:Package "Package_CoreEquipmentProfile" ;
  eq:isCIMDatatype "True" ;
  skos:definition """
Reactance (imaginary part of impedance), at rated frequency.

\t"""@en .

cim:ReactiveCapabilityCurve a owl:Class ;
  rdfs:label "ReactiveCapabilityCurve"@en ;
  eq:Package "Package_CoreEquipmentProfile" ;
  rdfs:subClassOf cim:Curve ;
  skos:definition "Reactive power rating envelope versus the synchronous machine's active power, in both the generating and motoring modes. For each active power value there is a corresponding high and low reactive power limit  value. Typically there will be a separate curve for each coolant condition, such as hydrogen pressure.  The Y1 axis values represent reactive minimum and the Y2 axis values represent reactive maximum."@en .

cim:ReactivePower a owl:Class ;
  rdfs:label "ReactivePower"@en ;
  eq:Package "Package_CoreEquipmentProfile" ;
  eq:isCIMDatatype "True" ;
  skos:definition """
Product of RMS value of the voltage and the RMS value of the quadrature component of the current.

\t"""@en .

cim:RealEnergy a owl:Class ;
  rdfs:label "RealEnergy"@en ;
  eq:Package "Package_CoreEquipmentProfile" ;
  eq:isCIMDatatype "True" ;
  skos:definition """
Real electrical energy.

\t"""@en .

cim:RegularIntervalSchedule a owl:Class ;
  rdfs:label "RegularIntervalSchedule"@en ;
  eq:Package "Package_CoreEquipmentProfile" ;
  eq:isAbstract "True" ;
  rdfs:subClassOf cim:BasicIntervalSchedule ;
  skos:definition """
The schedule has time points where the time between them is constant.

\t"""@en .

cim:RegularTimePoint a owl:Class ;
  rdfs:label "RegularTimePoint"@en ;
  eq:Package "Package_CoreEquipmentProfile" ;
  skos:definition """
Time point for a schedule where the time between the consecutive points is constant.

\t"""@en .

cim:RegulatingCondEq a owl:Class ;
  rdfs:label "RegulatingCondEq"@en ;
  eq:Package "Package_CoreEquipmentProfile" ;
  eq:isAbstract "True" ;
  rdfs:subClassOf cim:EnergyConnection ;
  skos:definition "A type of conducting equipment that can regulate a quantity (i.e. voltage or flow) at a specific point in the network. "@en .

cim:RegulatingControl a owl:Class ;
  rdfs:label "RegulatingControl"@en ;
  eq:Package "Package_CoreEquipmentProfile" ;
  rdfs:subClassOf cim:PowerSystemResource ;
  skos:definition """
Specifies a set of equipment that works together to control a power system quantity such as voltage or flow. 
Remote bus voltage control is possible by specifying the controlled terminal located at some place remote from the controlling equipment.
The specified terminal shall be associated with the connectivity node of the controlled point.  The most specific subtype of RegulatingControl shall be used in case such equipment participate in the control, e.g. TapChangerControl for tap changers.
For flow control, load sign convention is used, i.e. positive sign means flow out from a TopologicalNode (bus) into the conducting equipment.
The attribute minAllowedTargetValue and maxAllowedTargetValue are required in the following cases:
- For a power generating module operated in power factor control mode to specify maximum and minimum power factor values;
- Whenever it is necessary to have an off center target voltage for the tap changer regulator. For instance, due to long cables to off shore wind farms and the need to have a simpler setup at the off shore transformer platform, the voltage is controlled from the land at the connection point for the off shore wind farm. Since there usually is a voltage rise along the cable, there is typical and overvoltage of up 3-4 kV compared to the on shore station. Thus in normal operation the tap changer on the on shore station is operated with a target set point, which is in the lower parts of the dead band.
The attributes minAllowedTargetValue and maxAllowedTargetValue are not related to the attribute targetDeadband and thus they are not treated as an alternative of the targetDeadband. They are needed due to limitations in the local substation controller. The attribute targetDeadband is used to prevent the power flow from move the tap position in circles (hunting) that is to be used regardless of the attributes minAllowedTargetValue and maxAllowedTargetValue.
\t"""@en .

cim:RegulatingControlModeKind a owl:Class ;
  rdfs:label "RegulatingControlModeKind"@en ;
  eq:Package "Package_CoreEquipmentProfile" ;
  owl:oneOf ( cim:RegulatingControlModeKind.voltage cim:RegulatingControlModeKind.activePower
    cim:RegulatingControlModeKind.reactivePower cim:RegulatingControlModeKind.currentFlow
    cim:RegulatingControlModeKind.admittance cim:RegulatingControlModeKind.timeScheduled
    cim:RegulatingControlModeKind.temperature cim:RegulatingControlModeKind.powerFactor ) ;
  rdfs:subClassOf cim:Enumeration ;
  skos:definition "The kind of regulation model.   For example regulating voltage, reactive power, active power, etc."@en .

cim:RegulationSchedule a owl:Class ;
  rdfs:label "RegulationSchedule"@en ;
  eq:Package "Package_CoreEquipmentProfile" ;
  rdfs:subClassOf cim:SeasonDayTypeSchedule ;
  skos:definition "A pre-established pattern over time for a controlled variable, e.g., busbar voltage."@en .

cim:ReportingGroup a owl:Class ;
  rdfs:label "ReportingGroup"@en ;
  eq:Package "Package_CoreEquipmentProfile" ;
  rdfs:subClassOf cim:IdentifiedObject ;
  skos:definition """
A reporting group is used for various ad-hoc groupings used for reporting.

\t"""@en .

cim:Resistance a owl:Class ;
  rdfs:label "Resistance"@en ;
  eq:Package "Package_CoreEquipmentProfile" ;
  eq:isCIMDatatype "True" ;
  skos:definition """
Resistance (real part of impedance).

\t"""@en .

cim:RotatingMachine a owl:Class ;
  rdfs:label "RotatingMachine"@en ;
  eq:Package "Package_CoreEquipmentProfile" ;
  eq:isAbstract "True" ;
  rdfs:subClassOf cim:RegulatingCondEq ;
  skos:definition "A rotating machine which may be used as a generator or motor."@en .

cim:RotationSpeed a owl:Class ;
  rdfs:label "RotationSpeed"@en ;
  eq:Package "Package_CoreEquipmentProfile" ;
  eq:isCIMDatatype "True" ;
  skos:definition """
Number of revolutions per second.

\t"""@en .

cim:SVCControlMode a owl:Class ;
  rdfs:label "SVCControlMode"@en ;
  cims:stereotype "deprecated" ;
  eq:Package "Package_CoreEquipmentProfile" ;
  owl:oneOf ( cim:SVCControlMode.reactivePower cim:SVCControlMode.voltage ) ;
  rdfs:subClassOf cim:Enumeration ;
  skos:definition """
Static VAr Compensator control mode.

\t"""@en .

cim:Season a owl:Class ;
  rdfs:label "Season"@en ;
  eq:Package "Package_CoreEquipmentProfile" ;
  rdfs:subClassOf cim:IdentifiedObject ;
  skos:definition "A specified time period of the year."@en .

cim:SeasonDayTypeSchedule a owl:Class ;
  rdfs:label "SeasonDayTypeSchedule"@en ;
  eq:Package "Package_CoreEquipmentProfile" ;
  eq:isAbstract "True" ;
  rdfs:subClassOf cim:RegularIntervalSchedule ;
  skos:definition """
A time schedule covering a 24 hour period, with curve data for a specific type of season and day.

\t"""@en .

cim:Seconds a owl:Class ;
  rdfs:label "Seconds"@en ;
  eq:Package "Package_CoreEquipmentProfile" ;
  eq:isCIMDatatype "True" ;
  skos:definition """
Time, in seconds.

\t"""@en .

cim:Sensor a owl:Class ;
  rdfs:label "Sensor"@en ;
  eq:Package "Package_CoreEquipmentProfile" ;
  eq:isAbstract "True" ;
  rdfs:subClassOf cim:AuxiliaryEquipment ;
  skos:definition """
This class describe devices that transform a measured quantity into signals that can be presented at displays, used in control or be recorded.

\t"""@en .

cim:SeriesCompensator a owl:Class ;
  rdfs:label "SeriesCompensator"@en ;
  eq:Package "Package_CoreEquipmentProfile" ;
  rdfs:subClassOf cim:ConductingEquipment ;
  skos:definition """
A Series Compensator is a series capacitor or reactor or an AC transmission line without charging susceptance.  It is a two terminal device.

\t"""@en .

cim:ShuntCompensator a owl:Class ;
  rdfs:label "ShuntCompensator"@en ;
  eq:Package "Package_CoreEquipmentProfile" ;
  eq:isAbstract "True" ;
  rdfs:subClassOf cim:RegulatingCondEq ;
  skos:definition "A shunt capacitor or reactor or switchable bank of shunt capacitors or reactors. A section of a shunt compensator is an individual capacitor or reactor. A negative value for bPerSection indicates that the compensator is a reactor. ShuntCompensator is a single terminal device.  Ground is implied."@en .

cim:SolarGeneratingUnit a owl:Class ;
  rdfs:label "SolarGeneratingUnit"@en ;
  eq:Package "Package_CoreEquipmentProfile" ;
  rdfs:subClassOf cim:GeneratingUnit ;
  skos:definition "A solar thermal generating unit, connected to the grid by means of a rotating machine.  This class does not represent photovoltaic (PV) generation."@en .

cim:StaticVarCompensator a owl:Class ;
  rdfs:label "StaticVarCompensator"@en ;
  eq:Package "Package_CoreEquipmentProfile" ;
  rdfs:subClassOf cim:RegulatingCondEq ;
  skos:definition """
A facility for providing variable and controllable shunt reactive power. The SVC typically consists of a stepdown transformer, filter, thyristor-controlled reactor, and thyristor-switched capacitor arms.

The SVC may operate in fixed MVar output mode or in voltage control mode. When in voltage control mode, the output of the SVC will be proportional to the deviation of voltage at the controlled bus from the voltage setpoint.  The SVC characteristic slope defines the proportion.  If the voltage at the controlled bus is equal to the voltage setpoint, the SVC MVar output is zero.
\t"""@en .

cim:StationSupply a owl:Class ;
  rdfs:label "StationSupply"@en ;
  eq:Package "Package_CoreEquipmentProfile" ;
  rdfs:subClassOf cim:EnergyConsumer ;
  skos:definition "Station supply with load derived from the station output."@en .

cim:String a owl:Class ;
  rdfs:label "String"@en ;
  eq:Package "Package_CoreEquipmentProfile" ;
  eq:isPrimitive "True" ;
  skos:definition "A string consisting of a sequence of characters. The character encoding is UTF-8. The string length is unspecified and unlimited."@en .

cim:SubGeographicalRegion a owl:Class ;
  rdfs:label "SubGeographicalRegion"@en ;
  eq:Package "Package_CoreEquipmentProfile" ;
  rdfs:subClassOf cim:IdentifiedObject ;
  skos:definition """
A subset of a geographical region of a power system network model.

\t"""@en .

cim:SubLoadArea a owl:Class ;
  rdfs:label "SubLoadArea"@en ;
  eq:Package "Package_CoreEquipmentProfile" ;
  rdfs:subClassOf cim:EnergyArea ;
  skos:definition "The class is the second level in a hierarchical structure for grouping of loads for the purpose of load flow load scaling."@en .

cim:Substation a owl:Class ;
  rdfs:label "Substation"@en ;
  eq:Package "Package_CoreEquipmentProfile" ;
  rdfs:subClassOf cim:EquipmentContainer ;
  skos:definition """
A collection of equipment for purposes other than generation or utilization, through which electric energy in bulk is passed for the purposes of switching or modifying its characteristics. 

\t"""@en .

cim:SurgeArrester a owl:Class ;
  rdfs:label "SurgeArrester"@en ;
  eq:Package "Package_CoreEquipmentProfile" ;
  rdfs:subClassOf cim:AuxiliaryEquipment ;
  skos:definition "Shunt device, installed on the network, usually in the proximity of electrical equipment in order to protect the said equipment against transient voltage transients caused by lightning or switching activity."@en .

cim:Susceptance a owl:Class ;
  rdfs:label "Susceptance"@en ;
  eq:Package "Package_CoreEquipmentProfile" ;
  eq:isCIMDatatype "True" ;
  skos:definition "Imaginary part of admittance."@en .

cim:Switch a owl:Class ;
  rdfs:label "Switch"@en ;
  eq:Package "Package_CoreEquipmentProfile" ;
  rdfs:subClassOf cim:ConductingEquipment ;
  skos:definition "A generic device designed to close, or open, or both, one or more electric circuits.  All switches are two terminal devices including grounding switches. The ACDCTerminal.connected at the two sides of the switch shall not be considered for assessing switch connectivity, i.e. only Switch.open, .normalOpen and .locked are relevant."@en .

cim:SwitchSchedule a owl:Class ;
  rdfs:label "SwitchSchedule"@en ;
  eq:Package "Package_CoreEquipmentProfile" ;
  rdfs:subClassOf cim:SeasonDayTypeSchedule ;
  skos:definition "A schedule of switch positions.  If RegularTimePoint.value1 is 0, the switch is open.  If 1, the switch is closed.  "@en .

cim:SynchronousMachine a owl:Class ;
  rdfs:label "SynchronousMachine"@en ;
  eq:Package "Package_CoreEquipmentProfile" ;
  rdfs:subClassOf cim:RotatingMachine ;
  skos:definition "An electromechanical device that operates with shaft rotating synchronously with the network. It is a single machine operating either as a generator or synchronous condenser or pump."@en .

cim:SynchronousMachineKind a owl:Class ;
  rdfs:label "SynchronousMachineKind"@en ;
  eq:Package "Package_CoreEquipmentProfile" ;
  owl:oneOf ( cim:SynchronousMachineKind.generator cim:SynchronousMachineKind.condenser
    cim:SynchronousMachineKind.generatorOrCondenser cim:SynchronousMachineKind.motor
    cim:SynchronousMachineKind.generatorOrMotor cim:SynchronousMachineKind.motorOrCondenser
    cim:SynchronousMachineKind.generatorOrCondenserOrMotor ) ;
  rdfs:subClassOf cim:Enumeration ;
  skos:definition "Synchronous machine type."@en .

cim:TapChanger a owl:Class ;
  rdfs:label "TapChanger"@en ;
  eq:Package "Package_CoreEquipmentProfile" ;
  eq:isAbstract "True" ;
  rdfs:subClassOf cim:PowerSystemResource ;
  skos:definition "Mechanism for changing transformer winding tap positions."@en .

cim:TapChangerControl a owl:Class ;
  rdfs:label "TapChangerControl"@en ;
  eq:Package "Package_CoreEquipmentProfile" ;
  rdfs:subClassOf cim:RegulatingControl ;
  skos:definition "Describes behaviour specific to tap changers, e.g. how the voltage at the end of a line varies with the load level and compensation of the voltage drop by tap adjustment."@en .

cim:TapChangerTablePoint a owl:Class ;
  rdfs:label "TapChangerTablePoint"@en ;
  eq:Package "Package_CoreEquipmentProfile" ;
  eq:isAbstract "True" ;
  skos:definition "Describes each tap step in the tabular curve."@en .

cim:TapSchedule a owl:Class ;
  rdfs:label "TapSchedule"@en ;
  eq:Package "Package_CoreEquipmentProfile" ;
  rdfs:subClassOf cim:SeasonDayTypeSchedule ;
  skos:definition "A pre-established pattern over time for a tap step."@en .

cim:Terminal a owl:Class ;
  rdfs:label "Terminal"@en ;
  eq:Package "Package_CoreEquipmentProfile" ;
  rdfs:subClassOf cim:ACDCTerminal ;
  skos:definition "An AC electrical connection point to a piece of conducting equipment. Terminals are connected at physical connection points called connectivity nodes."@en .

cim:ThermalGeneratingUnit a owl:Class ;
  rdfs:label "ThermalGeneratingUnit"@en ;
  eq:Package "Package_CoreEquipmentProfile" ;
  rdfs:subClassOf cim:GeneratingUnit ;
  skos:definition """
A generating unit whose prime mover could be a steam turbine, combustion turbine, or diesel engine.

\t"""@en .

cim:TieFlow a owl:Class ;
  rdfs:label "TieFlow"@en ;
  eq:Package "Package_CoreEquipmentProfile" ;
  rdfs:subClassOf cim:IdentifiedObject ;
  skos:definition "Defines the structure (in terms of location and direction) of the net interchange constraint for a control area. This constraint may be used by either AGC or power flow."@en .

cim:TransformerEnd a owl:Class ;
  rdfs:label "TransformerEnd"@en ;
  eq:Package "Package_CoreEquipmentProfile" ;
  eq:isAbstract "True" ;
  rdfs:subClassOf cim:IdentifiedObject ;
  skos:definition "A conducting connection point of a power transformer. It corresponds to a physical transformer winding terminal.  In earlier CIM versions, the TransformerWinding class served a similar purpose, but this class is more flexible because it associates to terminal but is not a specialization of ConductingEquipment."@en .

cim:UnitMultiplier a owl:Class ;
  rdfs:label "UnitMultiplier"@en ;
  eq:Package "Package_CoreEquipmentProfile" ;
  owl:oneOf ( cim:UnitMultiplier.y cim:UnitMultiplier.z cim:UnitMultiplier.a cim:UnitMultiplier.f
    cim:UnitMultiplier.p cim:UnitMultiplier.n cim:UnitMultiplier.micro cim:UnitMultiplier.m
    cim:UnitMultiplier.c cim:UnitMultiplier.d cim:UnitMultiplier.none cim:UnitMultiplier.da
    cim:UnitMultiplier.h cim:UnitMultiplier.k cim:UnitMultiplier.M cim:UnitMultiplier.G
    cim:UnitMultiplier.T cim:UnitMultiplier.P cim:UnitMultiplier.E cim:UnitMultiplier.Z
    cim:UnitMultiplier.Y ) ;
  rdfs:subClassOf cim:Enumeration ;
  skos:definition """
The unit multipliers defined for the CIM.  When applied to unit symbols, the unit symbol is treated as a derived unit. Regardless of the contents of the unit symbol text, the unit symbol shall be treated as if it were a single-character unit symbol. Unit symbols should not contain multipliers, and it should be left to the multiplier to define the multiple for an entire data type. 

For example, if a unit symbol is "m2Pers" and the multiplier is "k", then the value is k(m**2/s), and the multiplier applies to the entire final value, not to any individual part of the value. This can be conceptualized by substituting a derived unit symbol for the unit type. If one imagines that the symbol "Þ" represents the derived unit "m2Pers", then applying the multiplier "k" can be conceptualized simply as "kÞ".

For example, the SI unit for mass is "kg" and not "g".  If the unit symbol is defined as "kg", then the multiplier is applied to "kg" as a whole and does not replace the "k" in front of the "g". In this case, the multiplier of "m" would be used with the unit symbol of "kg" to represent one gram.  As a text string, this violates the instructions in IEC 80000-1. However, because the unit symbol in CIM is treated as a derived unit instead of as an SI unit, it makes more sense to conceptualize the "kg" as if it were replaced by one of the proposed replacements for the SI mass symbol. If one imagines that the "kg" were replaced by a symbol "Þ", then it is easier to conceptualize the multiplier "m" as creating the proper unit "mÞ", and not the forbidden unit "mkg".
\t"""@en .

cim:UnitSymbol a owl:Class ;
  rdfs:label "UnitSymbol"@en ;
  eq:Package "Package_CoreEquipmentProfile" ;
  owl:oneOf ( cim:UnitSymbol.none cim:UnitSymbol.m cim:UnitSymbol.kg cim:UnitSymbol.s
    cim:UnitSymbol.A cim:UnitSymbol.K cim:UnitSymbol.mol cim:UnitSymbol.cd cim:UnitSymbol.deg
    cim:UnitSymbol.rad cim:UnitSymbol.sr cim:UnitSymbol.Gy cim:UnitSymbol.Bq cim:UnitSymbol.degC
    cim:UnitSymbol.Sv cim:UnitSymbol.F cim:UnitSymbol.C cim:UnitSymbol.S cim:UnitSymbol.H
    cim:UnitSymbol.V cim:UnitSymbol.ohm cim:UnitSymbol.J cim:UnitSymbol.N cim:UnitSymbol.Hz
    cim:UnitSymbol.lx cim:UnitSymbol.lm cim:UnitSymbol.Wb cim:UnitSymbol.T cim:UnitSymbol.W
    cim:UnitSymbol.Pa cim:UnitSymbol.m2 cim:UnitSymbol.m3 cim:UnitSymbol.mPers cim:UnitSymbol.mPers2
    cim:UnitSymbol.m3Pers cim:UnitSymbol.mPerm3 cim:UnitSymbol.kgm cim:UnitSymbol.kgPerm3
    cim:UnitSymbol.m2Pers cim:UnitSymbol.WPermK cim:UnitSymbol.JPerK cim:UnitSymbol.ppm
    cim:UnitSymbol.rotPers cim:UnitSymbol.radPers cim:UnitSymbol.WPerm2 cim:UnitSymbol.JPerm2
    cim:UnitSymbol.SPerm cim:UnitSymbol.KPers cim:UnitSymbol.PaPers cim:UnitSymbol.JPerkgK
    cim:UnitSymbol.VA cim:UnitSymbol.VAr cim:UnitSymbol.cosPhi cim:UnitSymbol.Vs cim:UnitSymbol.V2
    cim:UnitSymbol.As cim:UnitSymbol.A2 cim:UnitSymbol.A2s cim:UnitSymbol.VAh cim:UnitSymbol.Wh
    cim:UnitSymbol.VArh cim:UnitSymbol.VPerHz cim:UnitSymbol.HzPers cim:UnitSymbol.character
    cim:UnitSymbol.charPers cim:UnitSymbol.kgm2 cim:UnitSymbol.dB cim:UnitSymbol.WPers
    cim:UnitSymbol.lPers cim:UnitSymbol.dBm cim:UnitSymbol.h cim:UnitSymbol.min cim:UnitSymbol.Q
    cim:UnitSymbol.Qh cim:UnitSymbol.ohmm cim:UnitSymbol.APerm cim:UnitSymbol.V2h cim:UnitSymbol.A2h
    cim:UnitSymbol.Ah cim:UnitSymbol.count cim:UnitSymbol.ft3 cim:UnitSymbol.m3Perh
    cim:UnitSymbol.gal cim:UnitSymbol.Btu cim:UnitSymbol.l cim:UnitSymbol.lPerh cim:UnitSymbol.lPerl
    cim:UnitSymbol.gPerg cim:UnitSymbol.molPerm3 cim:UnitSymbol.molPermol cim:UnitSymbol.molPerkg
    cim:UnitSymbol.sPers cim:UnitSymbol.HzPerHz cim:UnitSymbol.VPerV cim:UnitSymbol.APerA
    cim:UnitSymbol.VPerVA cim:UnitSymbol.rev cim:UnitSymbol.kat cim:UnitSymbol.JPerkg
    cim:UnitSymbol.m3Uncompensated cim:UnitSymbol.m3Compensated cim:UnitSymbol.WPerW
    cim:UnitSymbol.therm cim:UnitSymbol.onePerm cim:UnitSymbol.m3Perkg cim:UnitSymbol.Pas
    cim:UnitSymbol.Nm cim:UnitSymbol.NPerm cim:UnitSymbol.radPers2 cim:UnitSymbol.JPerm3
    cim:UnitSymbol.VPerm cim:UnitSymbol.CPerm3 cim:UnitSymbol.CPerm2 cim:UnitSymbol.FPerm
    cim:UnitSymbol.HPerm cim:UnitSymbol.JPermol cim:UnitSymbol.JPermolK cim:UnitSymbol.CPerkg
    cim:UnitSymbol.GyPers cim:UnitSymbol.WPersr cim:UnitSymbol.WPerm2sr cim:UnitSymbol.katPerm3
    cim:UnitSymbol.d cim:UnitSymbol.anglemin cim:UnitSymbol.anglesec cim:UnitSymbol.ha
    cim:UnitSymbol.tonne cim:UnitSymbol.bar cim:UnitSymbol.mmHg cim:UnitSymbol.M cim:UnitSymbol.kn
    cim:UnitSymbol.Mx cim:UnitSymbol.G cim:UnitSymbol.Oe cim:UnitSymbol.Vh cim:UnitSymbol.WPerA
    cim:UnitSymbol.onePerHz cim:UnitSymbol.VPerVAr cim:UnitSymbol.ohmPerm cim:UnitSymbol.kgPerJ
    cim:UnitSymbol.JPers ) ;
  rdfs:subClassOf cim:Enumeration ;
  skos:definition """
The derived units defined for usage in the CIM. In some cases, the derived unit is equal to an SI unit. Whenever possible, the standard derived symbol is used instead of the formula for the derived unit. For example, the unit symbol Farad is defined as "F" instead of "CPerV". In cases where a standard symbol does not exist for a derived unit, the formula for the unit is used as the unit symbol. For example, density does not have a standard symbol and so it is represented as "kgPerm3". With the exception of the "kg", which is an SI unit, the unit symbols do not contain multipliers and therefore represent the base derived unit to which a multiplier can be applied as a whole. 
Every unit symbol is treated as an unparseable text as if it were a single-letter symbol. The meaning of each unit symbol is defined by the accompanying descriptive text and not by the text contents of the unit symbol.
To allow the widest possible range of serializations without requiring special character handling, several substitutions are made which deviate from the format described in IEC 80000-1. The division symbol "/" is replaced by the letters "Per". Exponents are written in plain text after the unit as "m3" instead of being formatted as "m" with a superscript of 3  or introducing a symbol as in "m^3". The degree symbol "°" is replaced with the letters "deg". Any clarification of the meaning for a substitution is included in the description for the unit symbol.
Non-SI units are included in list of unit symbols to allow sources of data to be correctly labelled with their non-SI units (for example, a GPS sensor that is reporting numbers that represent feet instead of meters). This allows software to use the unit symbol information correctly convert and scale the raw data of those sources into SI-based units. 
The integer values are used for harmonization with IEC 61850.
\t"""@en .

cim:Voltage a owl:Class ;
  rdfs:label "Voltage"@en ;
  eq:Package "Package_CoreEquipmentProfile" ;
  eq:isCIMDatatype "True" ;
  skos:definition "Electrical voltage, can be both AC and DC."@en .

cim:VoltageLevel a owl:Class ;
  rdfs:label "VoltageLevel"@en ;
  eq:Package "Package_CoreEquipmentProfile" ;
  rdfs:subClassOf cim:EquipmentContainer ;
  skos:definition "A collection of equipment at one common system voltage forming a switchgear. The equipment typically consists of breakers, busbars, instrumentation, control, regulation and protection devices as well as assemblies of all these."@en .

cim:VoltageLimit a owl:Class ;
  rdfs:label "VoltageLimit"@en ;
  eq:Package "Package_CoreEquipmentProfile" ;
  rdfs:subClassOf cim:OperationalLimit ;
  skos:definition """
Operational limit applied to voltage.
The use of operational VoltageLimit is preferred instead of limits defined at VoltageLevel. The operational VoltageLimits are used, if present.
\t"""@en .

cim:VoltagePerReactivePower a owl:Class ;
  rdfs:label "VoltagePerReactivePower"@en ;
  eq:Package "Package_CoreEquipmentProfile" ;
  eq:isCIMDatatype "True" ;
  skos:definition """
Voltage variation with reactive power.

\t"""@en .

cim:VsCapabilityCurve a owl:Class ;
  rdfs:label "VsCapabilityCurve"@en ;
  eq:Package "Package_CoreEquipmentProfile" ;
  rdfs:subClassOf cim:Curve ;
  skos:definition "The P-Q capability curve for a voltage source converter, with P on X-axis and Qmin and Qmax on Y1-axis and Y2-axis."@en .

cim:VsConverter a owl:Class ;
  rdfs:label "VsConverter"@en ;
  eq:Package "Package_CoreEquipmentProfile" ;
  rdfs:subClassOf cim:ACDCConverter ;
  skos:definition "DC side of the voltage source converter (VSC)."@en .

cim:WaveTrap a owl:Class ;
  rdfs:label "WaveTrap"@en ;
  eq:Package "Package_CoreEquipmentProfile" ;
  rdfs:subClassOf cim:AuxiliaryEquipment ;
  skos:definition "Line traps are devices that impede high frequency power line carrier signals yet present a negligible impedance at the main power frequency."@en .

cim:WindGenUnitKind a owl:Class ;
  rdfs:label "WindGenUnitKind"@en ;
  eq:Package "Package_CoreEquipmentProfile" ;
  owl:oneOf ( cim:WindGenUnitKind.offshore cim:WindGenUnitKind.onshore ) ;
  rdfs:subClassOf cim:Enumeration ;
  skos:definition "Kind of wind generating unit."@en .

cim:WindGeneratingUnit a owl:Class ;
  rdfs:label "WindGeneratingUnit"@en ;
  eq:Package "Package_CoreEquipmentProfile" ;
  rdfs:subClassOf cim:GeneratingUnit ;
  skos:definition "A wind driven generating unit, connected to the grid by means of a rotating machine.  May be used to represent a single turbine or an aggregation.    "@en .

cim:WindingConnection a owl:Class ;
  rdfs:label "WindingConnection"@en ;
  eq:Package "Package_CoreEquipmentProfile" ;
  owl:oneOf ( cim:WindingConnection.D cim:WindingConnection.Y cim:WindingConnection.Z
    cim:WindingConnection.Yn cim:WindingConnection.Zn cim:WindingConnection.A
    cim:WindingConnection.I ) ;
  rdfs:subClassOf cim:Enumeration ;
  skos:definition """
Winding connection type.

\t"""@en .

eq:Enumeration a owl:Class ;
  rdfs:label " enumeration "@en ;
  rdfs:comment " An abstract superclass for all Enumerators. "@en ;
  eq:isAbstract "true" .

eu:BoundaryPoint a owl:Class ;
  rdfs:label "BoundaryPoint"@en ;
  eq:Package "Package_CoreEquipmentProfile" ;
  eq:isEuropean "True" ;
  rdfs:subClassOf cim:PowerSystemResource ;
  skos:definition "Designates a connection point at which one or more model authority sets shall connect to. The location of the connection point as well as other properties are agreed between organisations responsible for the interconnection, hence all attributes of the class represent this agreement.  It is primarily used in a boundary model authority set which can contain one or many BoundaryPoint-s among other Equipment-s and their connections."@en .

eu:LimitKind a owl:Class ;
  rdfs:label "LimitKind"@en ;
  cims:stereotype "European" ;
  eq:Package "Package_CoreEquipmentProfile" ;
  owl:oneOf ( eu:LimitKind.patl eu:LimitKind.patlt eu:LimitKind.tatl eu:LimitKind.tc
    eu:LimitKind.tct eu:LimitKind.highVoltage eu:LimitKind.lowVoltage
    eu:LimitKind.operationalVoltageLimit eu:LimitKind.alarmVoltage eu:LimitKind.warningVoltage
    eu:LimitKind.stability ) ;
  rdfs:subClassOf cim:Enumeration ;
  skos:definition "Limit kinds."@en .

eu:SolarPowerPlant a owl:Class ;
  rdfs:label "SolarPowerPlant"@en ;
  eq:Package "Package_CoreEquipmentProfile" ;
  eq:isEuropean "True" ;
  rdfs:subClassOf cim:PowerSystemResource ;
  skos:definition "Solar power plant."@en .

eu:WindPowerPlant a owl:Class ;
  rdfs:label "WindPowerPlant"@en ;
  eq:Package "Package_CoreEquipmentProfile" ;
  eq:isEuropean "True" ;
  rdfs:subClassOf cim:PowerSystemResource ;
  skos:definition "Wind power plant."@en .

cim:ACDCConverter.DCTerminals a owl:ObjectProperty ;
  rdfs:label "DCTerminals"@en ;
  owl:inverseOf cim:ACDCConverterDCTerminal.DCConductingEquipment ;
  rdfs:domain cim:ACDCConverter ;
  rdfs:range cim:ACDCConverterDCTerminal ;
  skos:definition "A DC converter have DC converter terminals. A converter has two DC converter terminals."@en .

cim:ACDCConverter.PccTerminal a owl:ObjectProperty, owl:FunctionalProperty ;
  rdfs:label "PccTerminal"@en ;
  owl:inverseOf cim:Terminal.ConverterDCSides ;
  rdfs:domain cim:ACDCConverter ;
  rdfs:range cim:Terminal ;
  skos:definition "Point of common coupling terminal for this converter DC side. It is typically the terminal on the power transformer (or switch) closest to the AC network."@en .

cim:ACDCConverterDCTerminal.DCConductingEquipment a owl:ObjectProperty ;
  rdfs:label "DCConductingEquipment"@en ;
  owl:inverseOf cim:ACDCConverter.DCTerminals ;
  rdfs:domain cim:ACDCConverterDCTerminal ;
  rdfs:range cim:ACDCConverter ;
  skos:definition "A DC converter terminal belong to an DC converter."@en .

cim:ACDCTerminal.BusNameMarker a owl:ObjectProperty, owl:FunctionalProperty ;
  rdfs:label "BusNameMarker"@en ;
  owl:inverseOf cim:BusNameMarker.Terminal ;
  rdfs:domain cim:ACDCTerminal ;
  rdfs:range cim:BusNameMarker ;
  skos:definition "The bus name marker used to name the bus (topological node)."@en .

cim:ACDCTerminal.OperationalLimitSet a owl:ObjectProperty ;
  rdfs:label "OperationalLimitSet"@en ;
  owl:inverseOf cim:OperationalLimitSet.Terminal ;
  rdfs:domain cim:ACDCTerminal ;
  rdfs:range cim:OperationalLimitSet ;
  skos:definition "The operational limit sets at the terminal."@en .

cim:ACLineSegment.Clamp a owl:ObjectProperty ;
  rdfs:label "Clamp"@en ;
  owl:inverseOf cim:Clamp.ACLineSegment ;
  rdfs:domain cim:ACLineSegment ;
  rdfs:range cim:Clamp ;
  skos:definition "The clamps connected to the line segment."@en .

cim:ACLineSegment.Cut a owl:ObjectProperty ;
  rdfs:label "Cut"@en ;
  owl:inverseOf cim:Cut.ACLineSegment ;
  rdfs:domain cim:ACLineSegment ;
  rdfs:range cim:Cut ;
  skos:definition "Cuts applied to the line segment."@en .

cim:AuxiliaryEquipment.Terminal a owl:ObjectProperty ;
  rdfs:label "Terminal"@en ;
  owl:inverseOf cim:Terminal.AuxiliaryEquipment ;
  rdfs:domain cim:AuxiliaryEquipment ;
  rdfs:range cim:Terminal ;
  skos:definition "The Terminal at the equipment where the AuxiliaryEquipment is attached."@en .

cim:BaseVoltage.ConductingEquipment a owl:ObjectProperty ;
  rdfs:label "ConductingEquipment"@en ;
  owl:inverseOf cim:ConductingEquipment.BaseVoltage ;
  rdfs:domain cim:BaseVoltage ;
  rdfs:range cim:ConductingEquipment ;
  skos:definition "All conducting equipment with this base voltage.  Use only when there is no voltage level container used and only one base voltage applies.  For example, not used for transformers."@en .

cim:BaseVoltage.TransformerEnds a owl:ObjectProperty ;
  rdfs:label "TransformerEnds"@en ;
  owl:inverseOf cim:TransformerEnd.BaseVoltage ;
  rdfs:domain cim:BaseVoltage ;
  rdfs:range cim:TransformerEnd ;
  skos:definition "Transformer ends at the base voltage.  This is essential for PU calculation."@en .

cim:BaseVoltage.VoltageLevel a owl:ObjectProperty ;
  rdfs:label "VoltageLevel"@en ;
  owl:inverseOf cim:VoltageLevel.BaseVoltage ;
  rdfs:domain cim:BaseVoltage ;
  rdfs:range cim:VoltageLevel ;
  skos:definition "The voltage levels having this base voltage."@en .

cim:Bay.VoltageLevel a owl:ObjectProperty ;
  rdfs:label "VoltageLevel"@en ;
  owl:inverseOf cim:VoltageLevel.Bays ;
  rdfs:domain cim:Bay ;
  rdfs:range cim:VoltageLevel ;
  skos:definition "The voltage level containing this bay."@en .

cim:BusNameMarker.ReportingGroup a owl:ObjectProperty, owl:FunctionalProperty ;
  rdfs:label "ReportingGroup"@en ;
  owl:inverseOf cim:ReportingGroup.BusNameMarker ;
  rdfs:domain cim:BusNameMarker ;
  rdfs:range cim:ReportingGroup ;
  skos:definition "The reporting group to which this bus name marker belongs."@en .

cim:BusNameMarker.Terminal a owl:ObjectProperty ;
  rdfs:label "Terminal"@en ;
  owl:inverseOf cim:ACDCTerminal.BusNameMarker ;
  rdfs:domain cim:BusNameMarker ;
  rdfs:range cim:ACDCTerminal ;
  skos:definition "The terminals associated with this bus name marker."@en .

cim:CAESPlant.ThermalGeneratingUnit a owl:ObjectProperty, owl:FunctionalProperty ;
  rdfs:label "ThermalGeneratingUnit"@en ;
  owl:inverseOf cim:ThermalGeneratingUnit.CAESPlant ;
  rdfs:domain cim:CAESPlant ;
  rdfs:range cim:ThermalGeneratingUnit ;
  skos:definition "A thermal generating unit may be a member of a compressed air energy storage plant."@en .

cim:Clamp.ACLineSegment a owl:ObjectProperty ;
  rdfs:label "ACLineSegment"@en ;
  owl:inverseOf cim:ACLineSegment.Clamp ;
  rdfs:domain cim:Clamp ;
  rdfs:range cim:ACLineSegment ;
  skos:definition "The line segment to which the clamp is connected."@en .

cim:CogenerationPlant.ThermalGeneratingUnits a owl:ObjectProperty ;
  rdfs:label "ThermalGeneratingUnits"@en ;
  owl:inverseOf cim:ThermalGeneratingUnit.CogenerationPlant ;
  rdfs:domain cim:CogenerationPlant ;
  rdfs:range cim:ThermalGeneratingUnit ;
  skos:definition "A thermal generating unit may be a member of a cogeneration plant."@en .

cim:CombinedCyclePlant.ThermalGeneratingUnits a owl:ObjectProperty ;
  rdfs:label "ThermalGeneratingUnits"@en ;
  owl:inverseOf cim:ThermalGeneratingUnit.CombinedCyclePlant ;
  rdfs:domain cim:CombinedCyclePlant ;
  rdfs:range cim:ThermalGeneratingUnit ;
  skos:definition "A thermal generating unit may be a member of a combined cycle plant."@en .

cim:ConductingEquipment.BaseVoltage a owl:ObjectProperty, owl:FunctionalProperty ;
  rdfs:label "BaseVoltage"@en ;
  owl:inverseOf cim:BaseVoltage.ConductingEquipment ;
  rdfs:domain cim:ConductingEquipment ;
  rdfs:range cim:BaseVoltage ;
  skos:definition "Base voltage of this conducting equipment.  Use only when there is no voltage level container used and only one base voltage applies.  For example, not used for transformers."@en .

cim:ConductingEquipment.Terminals a owl:ObjectProperty ;
  rdfs:label "Terminals"@en ;
  owl:inverseOf cim:Terminal.ConductingEquipment ;
  rdfs:domain cim:ConductingEquipment ;
  rdfs:range cim:Terminal ;
  skos:definition "Conducting equipment have terminals that may be connected to other conducting equipment terminals via connectivity nodes or topological nodes."@en .

cim:ConformLoad.LoadGroup a owl:ObjectProperty ;
  rdfs:label "LoadGroup"@en ;
  owl:inverseOf cim:ConformLoadGroup.EnergyConsumers ;
  rdfs:domain cim:ConformLoad ;
  rdfs:range cim:ConformLoadGroup ;
  skos:definition "Group of this ConformLoad."@en .

cim:ConformLoadGroup.ConformLoadSchedules a owl:ObjectProperty ;
  rdfs:label "ConformLoadSchedules"@en ;
  owl:inverseOf cim:ConformLoadSchedule.ConformLoadGroup ;
  rdfs:domain cim:ConformLoadGroup ;
  rdfs:range cim:ConformLoadSchedule ;
  skos:definition "The ConformLoadSchedules in the ConformLoadGroup."@en .

cim:ConformLoadGroup.EnergyConsumers a owl:ObjectProperty ;
  rdfs:label "EnergyConsumers"@en ;
  owl:inverseOf cim:ConformLoad.LoadGroup ;
  rdfs:domain cim:ConformLoadGroup ;
  rdfs:range cim:ConformLoad ;
  skos:definition "Conform loads assigned to this ConformLoadGroup."@en .

cim:ConformLoadSchedule.ConformLoadGroup a owl:ObjectProperty ;
  rdfs:label "ConformLoadGroup"@en ;
  owl:inverseOf cim:ConformLoadGroup.ConformLoadSchedules ;
  rdfs:domain cim:ConformLoadSchedule ;
  rdfs:range cim:ConformLoadGroup ;
  skos:definition "The ConformLoadGroup where the ConformLoadSchedule belongs."@en .

cim:ConnectivityNode.BoundaryPoint a owl:ObjectProperty, owl:FunctionalProperty ;
  rdfs:label "BoundaryPoint"@en ;
  owl:inverseOf eu:BoundaryPoint.ConnectivityNode ;
  rdfs:domain cim:ConnectivityNode ;
  rdfs:range eu:BoundaryPoint ;
  skos:definition "The boundary point associated with the connectivity node."@en .

cim:ConnectivityNode.ConnectivityNodeContainer a owl:ObjectProperty ;
  rdfs:label "ConnectivityNodeContainer"@en ;
  owl:inverseOf cim:ConnectivityNodeContainer.ConnectivityNodes ;
  rdfs:domain cim:ConnectivityNode ;
  rdfs:range cim:ConnectivityNodeContainer ;
  skos:definition "Container of this connectivity node."@en .

cim:ConnectivityNode.Terminals a owl:ObjectProperty ;
  rdfs:label "Terminals"@en ;
  owl:inverseOf cim:Terminal.ConnectivityNode ;
  rdfs:domain cim:ConnectivityNode ;
  rdfs:range cim:Terminal ;
  skos:definition "Terminals interconnected with zero impedance at a this connectivity node. "@en .

cim:ConnectivityNodeContainer.ConnectivityNodes a owl:ObjectProperty ;
  rdfs:label "ConnectivityNodes"@en ;
  owl:inverseOf cim:ConnectivityNode.ConnectivityNodeContainer ;
  rdfs:domain cim:ConnectivityNodeContainer ;
  rdfs:range cim:ConnectivityNode ;
  skos:definition "Connectivity nodes which belong to this connectivity node container."@en .

cim:ControlArea.EnergyArea a owl:ObjectProperty ;
  rdfs:label "EnergyArea"@en ;
  owl:inverseOf cim:EnergyArea.ControlArea ;
  rdfs:domain cim:ControlArea ;
  rdfs:range cim:EnergyArea ;
  skos:definition "The energy area that is forecast from this control area specification."@en .

cim:ControlAreaGeneratingUnit.GeneratingUnit a owl:ObjectProperty ;
  rdfs:label "GeneratingUnit"@en ;
  owl:inverseOf cim:GeneratingUnit.ControlAreaGeneratingUnit ;
  rdfs:domain cim:ControlAreaGeneratingUnit ;
  rdfs:range cim:GeneratingUnit ;
  skos:definition "The generating unit specified for this control area.  Note that a control area should include a GeneratingUnit only once."@en .

cim:Curve.CurveDatas a owl:ObjectProperty ;
  rdfs:label "CurveDatas"@en ;
  owl:inverseOf cim:CurveData.Curve ;
  rdfs:domain cim:Curve ;
  rdfs:range cim:CurveData ;
  skos:definition "The point data values that define this curve."@en .

cim:CurveData.Curve a owl:ObjectProperty ;
  rdfs:label "Curve"@en ;
  owl:inverseOf cim:Curve.CurveDatas ;
  rdfs:domain cim:CurveData ;
  rdfs:range cim:Curve ;
  skos:definition "The curve of  this curve data point."@en .

cim:Cut.ACLineSegment a owl:ObjectProperty ;
  rdfs:label "ACLineSegment"@en ;
  owl:inverseOf cim:ACLineSegment.Cut ;
  rdfs:domain cim:Cut ;
  rdfs:range cim:ACLineSegment ;
  skos:definition "The line segment to which the cut is applied."@en .

cim:DCBaseTerminal.DCNode a owl:ObjectProperty, owl:FunctionalProperty ;
  rdfs:label "DCNode"@en ;
  owl:inverseOf cim:DCNode.DCTerminals ;
  rdfs:domain cim:DCBaseTerminal ;
  rdfs:range cim:DCNode ;
  skos:definition "The DC connectivity node to which this DC base terminal connects with zero impedance."@en .

cim:DCConductingEquipment.DCTerminals a owl:ObjectProperty ;
  rdfs:label "DCTerminals"@en ;
  owl:inverseOf cim:DCTerminal.DCConductingEquipment ;
  rdfs:domain cim:DCConductingEquipment ;
  rdfs:range cim:DCTerminal ;
  skos:definition "A DC conducting equipment has DC terminals."@en .

cim:DCEquipmentContainer.DCNodes a owl:ObjectProperty ;
  rdfs:label "DCNodes"@en ;
  owl:inverseOf cim:DCNode.DCEquipmentContainer ;
  rdfs:domain cim:DCEquipmentContainer ;
  rdfs:range cim:DCNode ;
  skos:definition "The DC nodes contained in the DC equipment container."@en .

cim:DCLine.Region a owl:ObjectProperty, owl:FunctionalProperty ;
  rdfs:label "Region"@en ;
  owl:inverseOf cim:SubGeographicalRegion.DCLines ;
  rdfs:domain cim:DCLine ;
  rdfs:range cim:SubGeographicalRegion ;
  skos:definition "The SubGeographicalRegion containing the DC line."@en .

cim:DCNode.DCEquipmentContainer a owl:ObjectProperty ;
  rdfs:label "DCEquipmentContainer"@en ;
  owl:inverseOf cim:DCEquipmentContainer.DCNodes ;
  rdfs:domain cim:DCNode ;
  rdfs:range cim:DCEquipmentContainer ;
  skos:definition "The DC container for the DC nodes."@en .

cim:DCNode.DCTerminals a owl:ObjectProperty ;
  rdfs:label "DCTerminals"@en ;
  owl:inverseOf cim:DCBaseTerminal.DCNode ;
  rdfs:domain cim:DCNode ;
  rdfs:range cim:DCBaseTerminal ;
  skos:definition "DC base terminals interconnected with zero impedance at a this DC connectivity node. "@en .

cim:DCTerminal.DCConductingEquipment a owl:ObjectProperty ;
  rdfs:label "DCConductingEquipment"@en ;
  owl:inverseOf cim:DCConductingEquipment.DCTerminals ;
  rdfs:domain cim:DCTerminal ;
  rdfs:range cim:DCConductingEquipment ;
  skos:definition "An DC  terminal belong to a DC conducting equipment."@en .

cim:DayType.SeasonDayTypeSchedules a owl:ObjectProperty ;
  rdfs:label "SeasonDayTypeSchedules"@en ;
  owl:inverseOf cim:SeasonDayTypeSchedule.DayType ;
  rdfs:domain cim:DayType ;
  rdfs:range cim:SeasonDayTypeSchedule ;
  skos:definition "Schedules that use this DayType."@en .

cim:EnergyArea.ControlArea a owl:ObjectProperty, owl:FunctionalProperty ;
  rdfs:label "ControlArea"@en ;
  owl:inverseOf cim:ControlArea.EnergyArea ;
  rdfs:domain cim:EnergyArea ;
  rdfs:range cim:ControlArea ;
  skos:definition "The control area specification that is used for the load forecast."@en .

cim:EnergyConsumer.LoadResponse a owl:ObjectProperty, owl:FunctionalProperty ;
  rdfs:label "LoadResponse"@en ;
  owl:inverseOf cim:LoadResponseCharacteristic.EnergyConsumer ;
  rdfs:domain cim:EnergyConsumer ;
  rdfs:range cim:LoadResponseCharacteristic ;
  skos:definition "The load response characteristic of this load.  If missing, this load is assumed to be constant power."@en .

cim:EnergySchedulingType.EnergySource a owl:ObjectProperty ;
  rdfs:label "EnergySource"@en ;
  owl:inverseOf cim:EnergySource.EnergySchedulingType ;
  rdfs:domain cim:EnergySchedulingType ;
  rdfs:range cim:EnergySource ;
  skos:definition "Energy Source of a particular Energy Scheduling Type."@en .

cim:EnergySource.EnergySchedulingType a owl:ObjectProperty, owl:FunctionalProperty ;
  rdfs:label "EnergySchedulingType"@en ;
  owl:inverseOf cim:EnergySchedulingType.EnergySource ;
  rdfs:domain cim:EnergySource ;
  rdfs:range cim:EnergySchedulingType ;
  skos:definition "Energy Scheduling Type of an Energy Source."@en .

cim:Equipment.EquipmentContainer a owl:ObjectProperty, owl:FunctionalProperty ;
  rdfs:label "EquipmentContainer"@en ;
  owl:inverseOf cim:EquipmentContainer.Equipments ;
  rdfs:domain cim:Equipment ;
  rdfs:range cim:EquipmentContainer ;
  skos:definition "Container of this equipment."@en .

cim:Equipment.OperationalLimitSet a owl:ObjectProperty ;
  rdfs:label "OperationalLimitSet"@en ;
  owl:inverseOf cim:OperationalLimitSet.Equipment ;
  rdfs:domain cim:Equipment ;
  rdfs:range cim:OperationalLimitSet ;
  skos:definition "The operational limit sets associated with this equipment."@en .

cim:EquipmentContainer.Equipments a owl:ObjectProperty ;
  rdfs:label "Equipments"@en ;
  owl:inverseOf cim:Equipment.EquipmentContainer ;
  rdfs:domain cim:EquipmentContainer ;
  rdfs:range cim:Equipment ;
  skos:definition "Contained equipment."@en .

cim:EquivalentEquipment.EquivalentNetwork a owl:ObjectProperty, owl:FunctionalProperty ;
  rdfs:label "EquivalentNetwork"@en ;
  owl:inverseOf cim:EquivalentNetwork.EquivalentEquipments ;
  rdfs:domain cim:EquivalentEquipment ;
  rdfs:range cim:EquivalentNetwork ;
  skos:definition "The equivalent where the reduced model belongs."@en .

cim:EquivalentInjection.ReactiveCapabilityCurve a owl:ObjectProperty, owl:FunctionalProperty ;
  rdfs:label "ReactiveCapabilityCurve"@en ;
  owl:inverseOf cim:ReactiveCapabilityCurve.EquivalentInjection ;
  rdfs:domain cim:EquivalentInjection ;
  rdfs:range cim:ReactiveCapabilityCurve ;
  skos:definition "The reactive capability curve used by this equivalent injection."@en .

cim:EquivalentNetwork.EquivalentEquipments a owl:ObjectProperty ;
  rdfs:label "EquivalentEquipments"@en ;
  owl:inverseOf cim:EquivalentEquipment.EquivalentNetwork ;
  rdfs:domain cim:EquivalentNetwork ;
  rdfs:range cim:EquivalentEquipment ;
  skos:definition "The associated reduced equivalents."@en .

cim:FossilFuel.ThermalGeneratingUnit a owl:ObjectProperty ;
  rdfs:label "ThermalGeneratingUnit"@en ;
  owl:inverseOf cim:ThermalGeneratingUnit.FossilFuels ;
  rdfs:domain cim:FossilFuel ;
  rdfs:range cim:ThermalGeneratingUnit ;
  skos:definition "A thermal generating unit may have one or more fossil fuels."@en .

cim:GeneratingUnit.ControlAreaGeneratingUnit a owl:ObjectProperty ;
  rdfs:label "ControlAreaGeneratingUnit"@en ;
  owl:inverseOf cim:ControlAreaGeneratingUnit.GeneratingUnit ;
  rdfs:domain cim:GeneratingUnit ;
  rdfs:range cim:ControlAreaGeneratingUnit ;
  skos:definition "ControlArea specifications for this generating unit."@en .

cim:GeneratingUnit.GrossToNetActivePowerCurves a owl:ObjectProperty ;
  rdfs:label "GrossToNetActivePowerCurves"@en ;
  owl:inverseOf cim:GrossToNetActivePowerCurve.GeneratingUnit ;
  rdfs:domain cim:GeneratingUnit ;
  rdfs:range cim:GrossToNetActivePowerCurve ;
  skos:definition "A generating unit may have a gross active power to net active power curve, describing the losses and auxiliary power requirements of the unit."@en .

cim:GeneratingUnit.RotatingMachine a owl:ObjectProperty ;
  rdfs:label "RotatingMachine"@en ;
  owl:inverseOf cim:RotatingMachine.GeneratingUnit ;
  rdfs:domain cim:GeneratingUnit ;
  rdfs:range cim:RotatingMachine ;
  skos:definition "A synchronous machine may operate as a generator and as such becomes a member of a generating unit."@en .

cim:GeographicalRegion.Regions a owl:ObjectProperty ;
  rdfs:label "Regions"@en ;
  owl:inverseOf cim:SubGeographicalRegion.Region ;
  rdfs:domain cim:GeographicalRegion ;
  rdfs:range cim:SubGeographicalRegion ;
  skos:definition "All sub-geographical regions within this geographical region."@en .

cim:GrossToNetActivePowerCurve.GeneratingUnit a owl:ObjectProperty ;
  rdfs:label "GeneratingUnit"@en ;
  owl:inverseOf cim:GeneratingUnit.GrossToNetActivePowerCurves ;
  rdfs:domain cim:GrossToNetActivePowerCurve ;
  rdfs:range cim:GeneratingUnit ;
  skos:definition "A generating unit may have a gross active power to net active power curve, describing the losses and auxiliary power requirements of the unit."@en .

cim:HydroGeneratingUnit.HydroPowerPlant a owl:ObjectProperty, owl:FunctionalProperty ;
  rdfs:label "HydroPowerPlant"@en ;
  owl:inverseOf cim:HydroPowerPlant.HydroGeneratingUnits ;
  rdfs:domain cim:HydroGeneratingUnit ;
  rdfs:range cim:HydroPowerPlant ;
  skos:definition "The hydro generating unit belongs to a hydro power plant."@en .

cim:HydroPowerPlant.HydroGeneratingUnits a owl:ObjectProperty ;
  rdfs:label "HydroGeneratingUnits"@en ;
  owl:inverseOf cim:HydroGeneratingUnit.HydroPowerPlant ;
  rdfs:domain cim:HydroPowerPlant ;
  rdfs:range cim:HydroGeneratingUnit ;
  skos:definition "The hydro generating unit belongs to a hydro power plant."@en .

cim:HydroPowerPlant.HydroPumps a owl:ObjectProperty ;
  rdfs:label "HydroPumps"@en ;
  owl:inverseOf cim:HydroPump.HydroPowerPlant ;
  rdfs:domain cim:HydroPowerPlant ;
  rdfs:range cim:HydroPump ;
  skos:definition "The hydro pump may be a member of a pumped storage plant or a pump for distributing water."@en .

cim:HydroPump.HydroPowerPlant a owl:ObjectProperty, owl:FunctionalProperty ;
  rdfs:label "HydroPowerPlant"@en ;
  owl:inverseOf cim:HydroPowerPlant.HydroPumps ;
  rdfs:domain cim:HydroPump ;
  rdfs:range cim:HydroPowerPlant ;
  skos:definition "The hydro pump may be a member of a pumped storage plant or a pump for distributing water."@en .

cim:HydroPump.RotatingMachine a owl:ObjectProperty ;
  rdfs:label "RotatingMachine"@en ;
  owl:inverseOf cim:RotatingMachine.HydroPump ;
  rdfs:domain cim:HydroPump ;
  rdfs:range cim:RotatingMachine ;
  skos:definition "The synchronous machine drives the turbine which moves the water from a low elevation to a higher elevation. The direction of machine rotation for pumping may or may not be the same as for generating."@en .

cim:Line.Region a owl:ObjectProperty, owl:FunctionalProperty ;
  rdfs:label "Region"@en ;
  owl:inverseOf cim:SubGeographicalRegion.Lines ;
  rdfs:domain cim:Line ;
  rdfs:range cim:SubGeographicalRegion ;
  skos:definition "The sub-geographical region of the line."@en .

cim:LoadArea.SubLoadAreas a owl:ObjectProperty ;
  rdfs:label "SubLoadAreas"@en ;
  owl:inverseOf cim:SubLoadArea.LoadArea ;
  rdfs:domain cim:LoadArea ;
  rdfs:range cim:SubLoadArea ;
  skos:definition "The SubLoadAreas in the LoadArea."@en .

cim:LoadGroup.SubLoadArea a owl:ObjectProperty ;
  rdfs:label "SubLoadArea"@en ;
  owl:inverseOf cim:SubLoadArea.LoadGroups ;
  rdfs:domain cim:LoadGroup ;
  rdfs:range cim:SubLoadArea ;
  skos:definition "The SubLoadArea where the Loadgroup belongs."@en .

cim:LoadResponseCharacteristic.EnergyConsumer a owl:ObjectProperty ;
  rdfs:label "EnergyConsumer"@en ;
  owl:inverseOf cim:EnergyConsumer.LoadResponse ;
  rdfs:domain cim:LoadResponseCharacteristic ;
  rdfs:range cim:EnergyConsumer ;
  skos:definition "The set of loads that have the response characteristics."@en .

cim:NonConformLoad.LoadGroup a owl:ObjectProperty ;
  rdfs:label "LoadGroup"@en ;
  owl:inverseOf cim:NonConformLoadGroup.EnergyConsumers ;
  rdfs:domain cim:NonConformLoad ;
  rdfs:range cim:NonConformLoadGroup ;
  skos:definition "Group of this ConformLoad."@en .

cim:NonConformLoadGroup.EnergyConsumers a owl:ObjectProperty ;
  rdfs:label "EnergyConsumers"@en ;
  owl:inverseOf cim:NonConformLoad.LoadGroup ;
  rdfs:domain cim:NonConformLoadGroup ;
  rdfs:range cim:NonConformLoad ;
  skos:definition "Conform loads assigned to this ConformLoadGroup."@en .

cim:NonConformLoadGroup.NonConformLoadSchedules a owl:ObjectProperty ;
  rdfs:label "NonConformLoadSchedules"@en ;
  owl:inverseOf cim:NonConformLoadSchedule.NonConformLoadGroup ;
  rdfs:domain cim:NonConformLoadGroup ;
  rdfs:range cim:NonConformLoadSchedule ;
  skos:definition "The NonConformLoadSchedules in the NonConformLoadGroup."@en .

cim:NonConformLoadSchedule.NonConformLoadGroup a owl:ObjectProperty ;
  rdfs:label "NonConformLoadGroup"@en ;
  owl:inverseOf cim:NonConformLoadGroup.NonConformLoadSchedules ;
  rdfs:domain cim:NonConformLoadSchedule ;
  rdfs:range cim:NonConformLoadGroup ;
  skos:definition "The NonConformLoadGroup where the NonConformLoadSchedule belongs."@en .

cim:OperationalLimit.OperationalLimitType a owl:ObjectProperty ;
  rdfs:label "OperationalLimitType"@en ;
  owl:inverseOf cim:OperationalLimitType.OperationalLimit ;
  rdfs:domain cim:OperationalLimit ;
  rdfs:range cim:OperationalLimitType ;
  skos:definition "The limit type associated with this limit."@en .

cim:OperationalLimitSet.Equipment a owl:ObjectProperty, owl:FunctionalProperty ;
  rdfs:label "Equipment"@en ;
  owl:inverseOf cim:Equipment.OperationalLimitSet ;
  rdfs:domain cim:OperationalLimitSet ;
  rdfs:range cim:Equipment ;
  skos:definition "The equipment to which the limit set applies."@en .

cim:OperationalLimitSet.Terminal a owl:ObjectProperty ;
  rdfs:label "Terminal"@en ;
  owl:inverseOf cim:ACDCTerminal.OperationalLimitSet ;
  rdfs:domain cim:OperationalLimitSet ;
  rdfs:range cim:ACDCTerminal ;
  skos:definition "The terminal where the operational limit set apply."@en .

cim:OperationalLimitType.OperationalLimit a owl:ObjectProperty ;
  rdfs:label "OperationalLimit"@en ;
  owl:inverseOf cim:OperationalLimit.OperationalLimitType ;
  rdfs:domain cim:OperationalLimitType ;
  rdfs:range cim:OperationalLimit ;
  skos:definition "The operational limits associated with this type of limit."@en .

cim:PhaseTapChanger.TransformerEnd a owl:ObjectProperty ;
  rdfs:label "TransformerEnd"@en ;
  owl:inverseOf cim:TransformerEnd.PhaseTapChanger ;
  rdfs:domain cim:PhaseTapChanger ;
  rdfs:range cim:TransformerEnd ;
  skos:definition "Transformer end to which this phase tap changer belongs."@en .

cim:PhaseTapChangerTable.PhaseTapChangerTablePoint a owl:ObjectProperty ;
  rdfs:label "PhaseTapChangerTablePoint"@en ;
  owl:inverseOf cim:PhaseTapChangerTablePoint.PhaseTapChangerTable ;
  rdfs:domain cim:PhaseTapChangerTable ;
  rdfs:range cim:PhaseTapChangerTablePoint ;
  skos:definition "The points of this table."@en .

cim:PhaseTapChangerTable.PhaseTapChangerTabular a owl:ObjectProperty ;
  rdfs:label "PhaseTapChangerTabular"@en ;
  owl:inverseOf cim:PhaseTapChangerTabular.PhaseTapChangerTable ;
  rdfs:domain cim:PhaseTapChangerTable ;
  rdfs:range cim:PhaseTapChangerTabular ;
  skos:definition "The phase tap changers to which this phase tap table applies."@en .

cim:PhaseTapChangerTablePoint.PhaseTapChangerTable a owl:ObjectProperty ;
  rdfs:label "PhaseTapChangerTable"@en ;
  owl:inverseOf cim:PhaseTapChangerTable.PhaseTapChangerTablePoint ;
  rdfs:domain cim:PhaseTapChangerTablePoint ;
  rdfs:range cim:PhaseTapChangerTable ;
  skos:definition "The table of this point."@en .

cim:PhaseTapChangerTabular.PhaseTapChangerTable a owl:ObjectProperty ;
  rdfs:label "PhaseTapChangerTable"@en ;
  owl:inverseOf cim:PhaseTapChangerTable.PhaseTapChangerTabular ;
  rdfs:domain cim:PhaseTapChangerTabular ;
  rdfs:range cim:PhaseTapChangerTable ;
  skos:definition "The phase tap changer table for this phase tap changer."@en .

cim:PowerElectronicsConnection.PowerElectronicsUnit a owl:ObjectProperty, owl:FunctionalProperty ;
  rdfs:label "PowerElectronicsUnit"@en ;
  owl:inverseOf cim:PowerElectronicsUnit.PowerElectronicsConnection ;
  rdfs:domain cim:PowerElectronicsConnection ;
  rdfs:range cim:PowerElectronicsUnit ;
  skos:definition "An AC network connection may have several power electronics units connecting through it."@en .

cim:PowerElectronicsUnit.PowerElectronicsConnection a owl:ObjectProperty ;
  rdfs:label "PowerElectronicsConnection"@en ;
  owl:inverseOf cim:PowerElectronicsConnection.PowerElectronicsUnit ;
  rdfs:domain cim:PowerElectronicsUnit ;
  rdfs:range cim:PowerElectronicsConnection ;
  skos:definition "A power electronics unit has a connection to the AC network."@en .

cim:PowerTransformer.PowerTransformerEnd a owl:ObjectProperty ;
  rdfs:label "PowerTransformerEnd"@en ;
  owl:inverseOf cim:PowerTransformerEnd.PowerTransformer ;
  rdfs:domain cim:PowerTransformer ;
  rdfs:range cim:PowerTransformerEnd ;
  skos:definition "The ends of this power transformer."@en .

cim:PowerTransformerEnd.PowerTransformer a owl:ObjectProperty ;
  rdfs:label "PowerTransformer"@en ;
  owl:inverseOf cim:PowerTransformer.PowerTransformerEnd ;
  rdfs:domain cim:PowerTransformerEnd ;
  rdfs:range cim:PowerTransformer ;
  skos:definition "The power transformer of this power transformer end."@en .

cim:RatioTapChanger.RatioTapChangerTable a owl:ObjectProperty, owl:FunctionalProperty ;
  rdfs:label "RatioTapChangerTable"@en ;
  owl:inverseOf cim:RatioTapChangerTable.RatioTapChanger ;
  rdfs:domain cim:RatioTapChanger ;
  rdfs:range cim:RatioTapChangerTable ;
  skos:definition "The tap ratio table for this ratio  tap changer."@en .

cim:RatioTapChanger.TransformerEnd a owl:ObjectProperty ;
  rdfs:label "TransformerEnd"@en ;
  owl:inverseOf cim:TransformerEnd.RatioTapChanger ;
  rdfs:domain cim:RatioTapChanger ;
  rdfs:range cim:TransformerEnd ;
  skos:definition "Transformer end to which this ratio tap changer belongs."@en .

cim:RatioTapChangerTable.RatioTapChanger a owl:ObjectProperty ;
  rdfs:label "RatioTapChanger"@en ;
  owl:inverseOf cim:RatioTapChanger.RatioTapChangerTable ;
  rdfs:domain cim:RatioTapChangerTable ;
  rdfs:range cim:RatioTapChanger ;
  skos:definition "The ratio tap changer of this tap ratio table."@en .

cim:RatioTapChangerTable.RatioTapChangerTablePoint a owl:ObjectProperty ;
  rdfs:label "RatioTapChangerTablePoint"@en ;
  owl:inverseOf cim:RatioTapChangerTablePoint.RatioTapChangerTable ;
  rdfs:domain cim:RatioTapChangerTable ;
  rdfs:range cim:RatioTapChangerTablePoint ;
  skos:definition "Points of this table."@en .

cim:RatioTapChangerTablePoint.RatioTapChangerTable a owl:ObjectProperty ;
  rdfs:label "RatioTapChangerTable"@en ;
  owl:inverseOf cim:RatioTapChangerTable.RatioTapChangerTablePoint ;
  rdfs:domain cim:RatioTapChangerTablePoint ;
  rdfs:range cim:RatioTapChangerTable ;
  skos:definition "Table of this point."@en .

cim:ReactiveCapabilityCurve.EquivalentInjection a owl:ObjectProperty ;
  rdfs:label "EquivalentInjection"@en ;
  owl:inverseOf cim:EquivalentInjection.ReactiveCapabilityCurve ;
  rdfs:domain cim:ReactiveCapabilityCurve ;
  rdfs:range cim:EquivalentInjection ;
  skos:definition "The equivalent injection using this reactive capability curve."@en .

cim:ReactiveCapabilityCurve.InitiallyUsedBySynchronousMachines a owl:ObjectProperty ;
  rdfs:label "InitiallyUsedBySynchronousMachines"@en ;
  owl:inverseOf cim:SynchronousMachine.InitialReactiveCapabilityCurve ;
  rdfs:domain cim:ReactiveCapabilityCurve ;
  rdfs:range cim:SynchronousMachine ;
  skos:definition "Synchronous machines using this curve as default."@en .

cim:RegularIntervalSchedule.TimePoints a owl:ObjectProperty ;
  rdfs:label "TimePoints"@en ;
  owl:inverseOf cim:RegularTimePoint.IntervalSchedule ;
  rdfs:domain cim:RegularIntervalSchedule ;
  rdfs:range cim:RegularTimePoint ;
  skos:definition "The regular interval time point data values that define this schedule."@en .

cim:RegularTimePoint.IntervalSchedule a owl:ObjectProperty ;
  rdfs:label "IntervalSchedule"@en ;
  owl:inverseOf cim:RegularIntervalSchedule.TimePoints ;
  rdfs:domain cim:RegularTimePoint ;
  rdfs:range cim:RegularIntervalSchedule ;
  skos:definition "Regular interval schedule containing this time point."@en .

cim:RegulatingCondEq.RegulatingControl a owl:ObjectProperty, owl:FunctionalProperty ;
  rdfs:label "RegulatingControl"@en ;
  owl:inverseOf cim:RegulatingControl.RegulatingCondEq ;
  rdfs:domain cim:RegulatingCondEq ;
  rdfs:range cim:RegulatingControl ;
  skos:definition "The regulating control scheme in which this equipment participates."@en .

cim:RegulatingControl.RegulatingCondEq a owl:ObjectProperty ;
  rdfs:label "RegulatingCondEq"@en ;
  owl:inverseOf cim:RegulatingCondEq.RegulatingControl ;
  rdfs:domain cim:RegulatingControl ;
  rdfs:range cim:RegulatingCondEq ;
  skos:definition "The equipment that participates in this regulating control scheme."@en .

cim:RegulatingControl.RegulationSchedule a owl:ObjectProperty ;
  rdfs:label "RegulationSchedule"@en ;
  owl:inverseOf cim:RegulationSchedule.RegulatingControl ;
  rdfs:domain cim:RegulatingControl ;
  rdfs:range cim:RegulationSchedule ;
  skos:definition "Schedule for this regulating control."@en .

cim:RegulatingControl.Terminal a owl:ObjectProperty ;
  rdfs:label "Terminal"@en ;
  owl:inverseOf cim:Terminal.RegulatingControl ;
  rdfs:domain cim:RegulatingControl ;
  rdfs:range cim:Terminal ;
  skos:definition "The terminal associated with this regulating control.  The terminal is associated instead of a node, since the terminal could connect into either a topological node or a connectivity node.  Sometimes it is useful to model regulation at a terminal of a bus bar object. "@en .

cim:RegulationSchedule.RegulatingControl a owl:ObjectProperty ;
  rdfs:label "RegulatingControl"@en ;
  owl:inverseOf cim:RegulatingControl.RegulationSchedule ;
  rdfs:domain cim:RegulationSchedule ;
  rdfs:range cim:RegulatingControl ;
  skos:definition "Regulating controls that have this schedule."@en .

cim:ReportingGroup.BusNameMarker a owl:ObjectProperty ;
  rdfs:label "BusNameMarker"@en ;
  owl:inverseOf cim:BusNameMarker.ReportingGroup ;
  rdfs:domain cim:ReportingGroup ;
  rdfs:range cim:BusNameMarker ;
  skos:definition "The bus name markers that belong to this reporting group."@en .

cim:RotatingMachine.GeneratingUnit a owl:ObjectProperty, owl:FunctionalProperty ;
  rdfs:label "GeneratingUnit"@en ;
  owl:inverseOf cim:GeneratingUnit.RotatingMachine ;
  rdfs:domain cim:RotatingMachine ;
  rdfs:range cim:GeneratingUnit ;
  skos:definition "A synchronous machine may operate as a generator and as such becomes a member of a generating unit."@en .

cim:RotatingMachine.HydroPump a owl:ObjectProperty, owl:FunctionalProperty ;
  rdfs:label "HydroPump"@en ;
  owl:inverseOf cim:HydroPump.RotatingMachine ;
  rdfs:domain cim:RotatingMachine ;
  rdfs:range cim:HydroPump ;
  skos:definition "The synchronous machine drives the turbine which moves the water from a low elevation to a higher elevation. The direction of machine rotation for pumping may or may not be the same as for generating."@en .

cim:Season.SeasonDayTypeSchedules a owl:ObjectProperty ;
  rdfs:label "SeasonDayTypeSchedules"@en ;
  owl:inverseOf cim:SeasonDayTypeSchedule.Season ;
  rdfs:domain cim:Season ;
  rdfs:range cim:SeasonDayTypeSchedule ;
  skos:definition "Schedules that use this Season."@en .

cim:SeasonDayTypeSchedule.DayType a owl:ObjectProperty ;
  rdfs:label "DayType"@en ;
  owl:inverseOf cim:DayType.SeasonDayTypeSchedules ;
  rdfs:domain cim:SeasonDayTypeSchedule ;
  rdfs:range cim:DayType ;
  skos:definition "DayType for the Schedule."@en .

cim:SeasonDayTypeSchedule.Season a owl:ObjectProperty ;
  rdfs:label "Season"@en ;
  owl:inverseOf cim:Season.SeasonDayTypeSchedules ;
  rdfs:domain cim:SeasonDayTypeSchedule ;
  rdfs:range cim:Season ;
  skos:definition "Season for the Schedule."@en .

cim:SolarGeneratingUnit.SolarPowerPlant a owl:ObjectProperty, owl:FunctionalProperty ;
  rdfs:label "SolarPowerPlant"@en ;
  owl:inverseOf eu:SolarPowerPlant.SolarGeneratingUnits ;
  rdfs:domain cim:SolarGeneratingUnit ;
  rdfs:range eu:SolarPowerPlant ;
  skos:definition "A solar power plant may have solar generating units."@en .

cim:SubGeographicalRegion.DCLines a owl:ObjectProperty ;
  rdfs:label "DCLines"@en ;
  owl:inverseOf cim:DCLine.Region ;
  rdfs:domain cim:SubGeographicalRegion ;
  rdfs:range cim:DCLine ;
  skos:definition "The DC lines in this sub-geographical region."@en .

cim:SubGeographicalRegion.Lines a owl:ObjectProperty ;
  rdfs:label "Lines"@en ;
  owl:inverseOf cim:Line.Region ;
  rdfs:domain cim:SubGeographicalRegion ;
  rdfs:range cim:Line ;
  skos:definition "The lines within the sub-geographical region."@en .

cim:SubGeographicalRegion.Region a owl:ObjectProperty ;
  rdfs:label "Region"@en ;
  owl:inverseOf cim:GeographicalRegion.Regions ;
  rdfs:domain cim:SubGeographicalRegion ;
  rdfs:range cim:GeographicalRegion ;
  skos:definition "The geographical region which this sub-geographical region is within."@en .

cim:SubGeographicalRegion.Substations a owl:ObjectProperty ;
  rdfs:label "Substations"@en ;
  owl:inverseOf cim:Substation.Region ;
  rdfs:domain cim:SubGeographicalRegion ;
  rdfs:range cim:Substation ;
  skos:definition "The substations in this sub-geographical region."@en .

cim:SubLoadArea.LoadArea a owl:ObjectProperty ;
  rdfs:label "LoadArea"@en ;
  owl:inverseOf cim:LoadArea.SubLoadAreas ;
  rdfs:domain cim:SubLoadArea ;
  rdfs:range cim:LoadArea ;
  skos:definition "The LoadArea where the SubLoadArea belongs."@en .

cim:SubLoadArea.LoadGroups a owl:ObjectProperty ;
  rdfs:label "LoadGroups"@en ;
  owl:inverseOf cim:LoadGroup.SubLoadArea ;
  rdfs:domain cim:SubLoadArea ;
  rdfs:range cim:LoadGroup ;
  skos:definition "The Loadgroups in the SubLoadArea."@en .

cim:Substation.Region a owl:ObjectProperty ;
  rdfs:label "Region"@en ;
  owl:inverseOf cim:SubGeographicalRegion.Substations ;
  rdfs:domain cim:Substation ;
  rdfs:range cim:SubGeographicalRegion ;
  skos:definition "The SubGeographicalRegion containing the substation."@en .

cim:Substation.VoltageLevels a owl:ObjectProperty ;
  rdfs:label "VoltageLevels"@en ;
  owl:inverseOf cim:VoltageLevel.Substation ;
  rdfs:domain cim:Substation ;
  rdfs:range cim:VoltageLevel ;
  skos:definition "The voltage levels within this substation."@en .

cim:Switch.SwitchSchedules a owl:ObjectProperty ;
  rdfs:label "SwitchSchedules"@en ;
  owl:inverseOf cim:SwitchSchedule.Switch ;
  rdfs:domain cim:Switch ;
  rdfs:range cim:SwitchSchedule ;
  skos:definition "A Switch can be associated with SwitchSchedules."@en .

cim:SwitchSchedule.Switch a owl:ObjectProperty ;
  rdfs:label "Switch"@en ;
  owl:inverseOf cim:Switch.SwitchSchedules ;
  rdfs:domain cim:SwitchSchedule ;
  rdfs:range cim:Switch ;
  skos:definition "A SwitchSchedule is associated with a Switch."@en .

cim:SynchronousMachine.InitialReactiveCapabilityCurve a owl:ObjectProperty, owl:FunctionalProperty ;
  rdfs:label "InitialReactiveCapabilityCurve"@en ;
  owl:inverseOf cim:ReactiveCapabilityCurve.InitiallyUsedBySynchronousMachines ;
  rdfs:domain cim:SynchronousMachine ;
  rdfs:range cim:ReactiveCapabilityCurve ;
  skos:definition "The default reactive capability curve for use by a synchronous machine."@en .

cim:TapChanger.TapChangerControl a owl:ObjectProperty, owl:FunctionalProperty ;
  rdfs:label "TapChangerControl"@en ;
  owl:inverseOf cim:TapChangerControl.TapChanger ;
  rdfs:domain cim:TapChanger ;
  rdfs:range cim:TapChangerControl ;
  skos:definition "The regulating control scheme in which this tap changer participates."@en .

cim:TapChanger.TapSchedules a owl:ObjectProperty ;
  rdfs:label "TapSchedules"@en ;
  owl:inverseOf cim:TapSchedule.TapChanger ;
  rdfs:domain cim:TapChanger ;
  rdfs:range cim:TapSchedule ;
  skos:definition "A TapChanger can have TapSchedules."@en .

cim:TapChangerControl.TapChanger a owl:ObjectProperty ;
  rdfs:label "TapChanger"@en ;
  owl:inverseOf cim:TapChanger.TapChangerControl ;
  rdfs:domain cim:TapChangerControl ;
  rdfs:range cim:TapChanger ;
  skos:definition "The tap changers that participates in this regulating tap control scheme."@en .

cim:TapSchedule.TapChanger a owl:ObjectProperty ;
  rdfs:label "TapChanger"@en ;
  owl:inverseOf cim:TapChanger.TapSchedules ;
  rdfs:domain cim:TapSchedule ;
  rdfs:range cim:TapChanger ;
  skos:definition "A TapSchedule is associated with a TapChanger."@en .

cim:Terminal.AuxiliaryEquipment a owl:ObjectProperty ;
  rdfs:label "AuxiliaryEquipment"@en ;
  owl:inverseOf cim:AuxiliaryEquipment.Terminal ;
  rdfs:domain cim:Terminal ;
  rdfs:range cim:AuxiliaryEquipment ;
  skos:definition "The auxiliary equipment connected to the terminal."@en .

cim:Terminal.ConductingEquipment a owl:ObjectProperty ;
  rdfs:label "ConductingEquipment"@en ;
  owl:inverseOf cim:ConductingEquipment.Terminals ;
  rdfs:domain cim:Terminal ;
  rdfs:range cim:ConductingEquipment ;
  skos:definition "The conducting equipment of the terminal.  Conducting equipment have  terminals that may be connected to other conducting equipment terminals via connectivity nodes or topological nodes."@en .

cim:Terminal.ConnectivityNode a owl:ObjectProperty, owl:FunctionalProperty ;
  rdfs:label "ConnectivityNode"@en ;
  owl:inverseOf cim:ConnectivityNode.Terminals ;
  rdfs:domain cim:Terminal ;
  rdfs:range cim:ConnectivityNode ;
  skos:definition "The connectivity node to which this terminal connects with zero impedance."@en .

cim:Terminal.ConverterDCSides a owl:ObjectProperty ;
  rdfs:label "ConverterDCSides"@en ;
  owl:inverseOf cim:ACDCConverter.PccTerminal ;
  rdfs:domain cim:Terminal ;
  rdfs:range cim:ACDCConverter ;
  skos:definition "All converters' DC sides linked to this point of common coupling terminal."@en .

cim:Terminal.RegulatingControl a owl:ObjectProperty ;
  rdfs:label "RegulatingControl"@en ;
  owl:inverseOf cim:RegulatingControl.Terminal ;
  rdfs:domain cim:Terminal ;
  rdfs:range cim:RegulatingControl ;
  skos:definition "The controls regulating this terminal."@en .

cim:Terminal.TieFlow a owl:ObjectProperty ;
  rdfs:label "TieFlow"@en ;
  owl:inverseOf cim:TieFlow.Terminal ;
  rdfs:domain cim:Terminal ;
  rdfs:range cim:TieFlow ;
  skos:definition "The control area tie flows to which this terminal associates."@en .

cim:Terminal.TransformerEnd a owl:ObjectProperty ;
  rdfs:label "TransformerEnd"@en ;
  owl:inverseOf cim:TransformerEnd.Terminal ;
  rdfs:domain cim:Terminal ;
  rdfs:range cim:TransformerEnd ;
  skos:definition "All transformer ends connected at this terminal."@en .

cim:ThermalGeneratingUnit.CAESPlant a owl:ObjectProperty, owl:FunctionalProperty ;
  rdfs:label "CAESPlant"@en ;
  owl:inverseOf cim:CAESPlant.ThermalGeneratingUnit ;
  rdfs:domain cim:ThermalGeneratingUnit ;
  rdfs:range cim:CAESPlant ;
  skos:definition "A thermal generating unit may be a member of a compressed air energy storage plant."@en .

cim:ThermalGeneratingUnit.CogenerationPlant a owl:ObjectProperty, owl:FunctionalProperty ;
  rdfs:label "CogenerationPlant"@en ;
  owl:inverseOf cim:CogenerationPlant.ThermalGeneratingUnits ;
  rdfs:domain cim:ThermalGeneratingUnit ;
  rdfs:range cim:CogenerationPlant ;
  skos:definition "A thermal generating unit may be a member of a cogeneration plant."@en .

cim:ThermalGeneratingUnit.CombinedCyclePlant a owl:ObjectProperty, owl:FunctionalProperty ;
  rdfs:label "CombinedCyclePlant"@en ;
  owl:inverseOf cim:CombinedCyclePlant.ThermalGeneratingUnits ;
  rdfs:domain cim:ThermalGeneratingUnit ;
  rdfs:range cim:CombinedCyclePlant ;
  skos:definition "A thermal generating unit may be a member of a combined cycle plant."@en .

cim:ThermalGeneratingUnit.FossilFuels a owl:ObjectProperty ;
  rdfs:label "FossilFuels"@en ;
  owl:inverseOf cim:FossilFuel.ThermalGeneratingUnit ;
  rdfs:domain cim:ThermalGeneratingUnit ;
  rdfs:range cim:FossilFuel ;
  skos:definition "A thermal generating unit may have one or more fossil fuels."@en .

cim:TieFlow.Terminal a owl:ObjectProperty ;
  rdfs:label "Terminal"@en ;
  owl:inverseOf cim:Terminal.TieFlow ;
  rdfs:domain cim:TieFlow ;
  rdfs:range cim:Terminal ;
  skos:definition "The terminal to which this tie flow belongs."@en .

cim:TransformerEnd.BaseVoltage a owl:ObjectProperty ;
  rdfs:label "BaseVoltage"@en ;
  owl:inverseOf cim:BaseVoltage.TransformerEnds ;
  rdfs:domain cim:TransformerEnd ;
  rdfs:range cim:BaseVoltage ;
  skos:definition "Base voltage of the transformer end.  This is essential for PU calculation."@en .

cim:TransformerEnd.PhaseTapChanger a owl:ObjectProperty, owl:FunctionalProperty ;
  rdfs:label "PhaseTapChanger"@en ;
  owl:inverseOf cim:PhaseTapChanger.TransformerEnd ;
  rdfs:domain cim:TransformerEnd ;
  rdfs:range cim:PhaseTapChanger ;
  skos:definition "Phase tap changer associated with this transformer end."@en .

cim:TransformerEnd.RatioTapChanger a owl:ObjectProperty, owl:FunctionalProperty ;
  rdfs:label "RatioTapChanger"@en ;
  owl:inverseOf cim:RatioTapChanger.TransformerEnd ;
  rdfs:domain cim:TransformerEnd ;
  rdfs:range cim:RatioTapChanger ;
  skos:definition "Ratio tap changer associated with this transformer end."@en .

cim:TransformerEnd.Terminal a owl:ObjectProperty ;
  rdfs:label "Terminal"@en ;
  owl:inverseOf cim:Terminal.TransformerEnd ;
  rdfs:domain cim:TransformerEnd ;
  rdfs:range cim:Terminal ;
  skos:definition "Terminal of the power transformer to which this transformer end belongs."@en .

cim:VoltageLevel.BaseVoltage a owl:ObjectProperty ;
  rdfs:label "BaseVoltage"@en ;
  owl:inverseOf cim:BaseVoltage.VoltageLevel ;
  rdfs:domain cim:VoltageLevel ;
  rdfs:range cim:BaseVoltage ;
  skos:definition "The base voltage used for all equipment within the voltage level."@en .

cim:VoltageLevel.Bays a owl:ObjectProperty ;
  rdfs:label "Bays"@en ;
  owl:inverseOf cim:Bay.VoltageLevel ;
  rdfs:domain cim:VoltageLevel ;
  rdfs:range cim:Bay ;
  skos:definition "The bays within this voltage level."@en .

cim:VoltageLevel.Substation a owl:ObjectProperty ;
  rdfs:label "Substation"@en ;
  owl:inverseOf cim:Substation.VoltageLevels ;
  rdfs:domain cim:VoltageLevel ;
  rdfs:range cim:Substation ;
  skos:definition "The substation of the voltage level."@en .

cim:VsCapabilityCurve.VsConverterDCSides a owl:ObjectProperty ;
  rdfs:label "VsConverterDCSides"@en ;
  owl:inverseOf cim:VsConverter.CapabilityCurve ;
  rdfs:domain cim:VsCapabilityCurve ;
  rdfs:range cim:VsConverter ;
  skos:definition "All converters with this capability curve."@en .

cim:VsConverter.CapabilityCurve a owl:ObjectProperty, owl:FunctionalProperty ;
  rdfs:label "CapabilityCurve"@en ;
  owl:inverseOf cim:VsCapabilityCurve.VsConverterDCSides ;
  rdfs:domain cim:VsConverter ;
  rdfs:range cim:VsCapabilityCurve ;
  skos:definition "Capability curve of this converter."@en .

cim:WindGeneratingUnit.WindPowerPlant a owl:ObjectProperty, owl:FunctionalProperty ;
  rdfs:label "WindPowerPlant"@en ;
  owl:inverseOf eu:WindPowerPlant.WindGeneratingUnits ;
  rdfs:domain cim:WindGeneratingUnit ;
  rdfs:range eu:WindPowerPlant ;
  skos:definition "A wind power plant may have wind generating units."@en .

eu:BoundaryPoint.ConnectivityNode a owl:ObjectProperty ;
  rdfs:label "ConnectivityNode"@en ;
  eq:isEuropean "True" ;
  owl:inverseOf cim:ConnectivityNode.BoundaryPoint ;
  rdfs:domain eu:BoundaryPoint ;
  rdfs:range cim:ConnectivityNode ;
  skos:definition "The connectivity node that is designated as a boundary point."@en .

eu:SolarPowerPlant.SolarGeneratingUnits a owl:ObjectProperty ;
  rdfs:label "SolarGeneratingUnits"@en ;
  eq:isEuropean "True" ;
  owl:inverseOf cim:SolarGeneratingUnit.SolarPowerPlant ;
  rdfs:domain eu:SolarPowerPlant ;
  rdfs:range cim:SolarGeneratingUnit ;
  skos:definition "A solar generating unit or units may be a member of a solar power plant."@en .

eu:WindPowerPlant.WindGeneratingUnits a owl:ObjectProperty ;
  rdfs:label "WindGeneratingUnits"@en ;
  eq:isEuropean "True" ;
  owl:inverseOf cim:WindGeneratingUnit.WindPowerPlant ;
  rdfs:domain eu:WindPowerPlant ;
  rdfs:range cim:WindGeneratingUnit ;
  skos:definition "A wind generating unit or units may be a member of a wind power plant."@en .

cim:ACDCConverter.baseS a owl:DatatypeProperty, owl:FunctionalProperty ;
  rdfs:label "baseS"@en ;
  rdfs:domain cim:ACDCConverter ;
  rdfs:range cim:ApparentPower ;
  skos:definition "Base apparent power of the converter pole. The attribute shall be a positive value."@en .

cim:ACDCConverter.idleLoss a owl:DatatypeProperty, owl:FunctionalProperty ;
  rdfs:label "idleLoss"@en ;
  rdfs:domain cim:ACDCConverter ;
  rdfs:range cim:ActivePower ;
  skos:definition "Active power loss in pole at no power transfer. It is converter’s configuration data used in power flow. The attribute shall be a positive value."@en .

cim:ACDCConverter.maxP a owl:DatatypeProperty, owl:FunctionalProperty ;
  rdfs:label "maxP"@en ;
  rdfs:domain cim:ACDCConverter ;
  rdfs:range cim:ActivePower ;
  skos:definition "Maximum active power limit. The value is overwritten by values of VsCapabilityCurve, if present."@en .

cim:ACDCConverter.maxUdc a owl:DatatypeProperty, owl:FunctionalProperty ;
  rdfs:label "maxUdc"@en ;
  rdfs:domain cim:ACDCConverter ;
  rdfs:range cim:Voltage ;
  skos:definition "The maximum voltage on the DC side at which the converter should operate. It is converter’s configuration data used in power flow. The attribute shall be a positive value."@en .

cim:ACDCConverter.minP a owl:DatatypeProperty, owl:FunctionalProperty ;
  rdfs:label "minP"@en ;
  rdfs:domain cim:ACDCConverter ;
  rdfs:range cim:ActivePower ;
  skos:definition "Minimum active power limit. The value is overwritten by values of VsCapabilityCurve, if present."@en .

cim:ACDCConverter.minUdc a owl:DatatypeProperty, owl:FunctionalProperty ;
  rdfs:label "minUdc"@en ;
  rdfs:domain cim:ACDCConverter ;
  rdfs:range cim:Voltage ;
  skos:definition "The minimum voltage on the DC side at which the converter should operate. It is converter’s configuration data used in power flow. The attribute shall be a positive value."@en .

cim:ACDCConverter.numberOfValves a owl:DatatypeProperty, owl:FunctionalProperty ;
  rdfs:label "numberOfValves"@en ;
  rdfs:domain cim:ACDCConverter ;
  rdfs:range xsd:integer ;
  skos:definition "Number of valves in the converter. Used in loss calculations."@en .

cim:ACDCConverter.ratedUdc a owl:DatatypeProperty, owl:FunctionalProperty ;
  rdfs:label "ratedUdc"@en ;
  rdfs:domain cim:ACDCConverter ;
  rdfs:range cim:Voltage ;
  skos:definition "Rated converter DC voltage, also called UdN. The attribute shall be a positive value. It is converter’s configuration data used in power flow. For instance a bipolar HVDC link with value  200 kV has a 400kV difference between the dc lines."@en .

cim:ACDCConverter.resistiveLoss a owl:DatatypeProperty, owl:FunctionalProperty ;
  rdfs:label "resistiveLoss"@en ;
  rdfs:domain cim:ACDCConverter ;
  rdfs:range cim:Resistance ;
  skos:definition "It is converter’s configuration data used in power flow. Refer to poleLossP. The attribute shall be a positive value."@en .

cim:ACDCConverter.switchingLoss a owl:DatatypeProperty, owl:FunctionalProperty ;
  rdfs:label "switchingLoss"@en ;
  rdfs:domain cim:ACDCConverter ;
  rdfs:range cim:ActivePowerPerCurrentFlow ;
  skos:definition "Switching losses, relative to the base apparent power 'baseS'. Refer to poleLossP. The attribute shall be a positive value."@en .

cim:ACDCConverter.valveU0 a owl:DatatypeProperty, owl:FunctionalProperty ;
  rdfs:label "valveU0"@en ;
  rdfs:domain cim:ACDCConverter ;
  rdfs:range cim:Voltage ;
  skos:definition "Valve threshold voltage, also called Uvalve. Forward voltage drop when the valve is conducting. Used in loss calculations, i.e. the switchLoss depend on numberOfValves * valveU0."@en .

cim:ACDCConverterDCTerminal.polarity a owl:DatatypeProperty ;
  rdfs:label "polarity"@en ;
  rdfs:domain cim:ACDCConverterDCTerminal ;
  rdfs:range cim:DCPolarityKind ;
  skos:definition """
Represents the normal network polarity condition. Depending on the converter configuration the value shall be set as follows:
- For a monopole with two converter terminals use DCPolarityKind “positive” and “negative”.
- For a bi-pole or symmetric monopole with three converter terminals use DCPolarityKind “positive”, “middle” and “negative”.
\t"""@en .

cim:ACDCTerminal.sequenceNumber a owl:DatatypeProperty ;
  rdfs:label "sequenceNumber"@en ;
  rdfs:domain cim:ACDCTerminal ;
  rdfs:range xsd:integer ;
  skos:definition """
The orientation of the terminal connections for a multiple terminal conducting equipment.  The sequence numbering starts with 1 and additional terminals should follow in increasing order.   The first terminal is the "starting point" for a two terminal branch.

\t"""@en .

cim:ACLineSegment.bch a owl:DatatypeProperty ;
  rdfs:label "bch"@en ;
  rdfs:domain cim:ACLineSegment ;
  rdfs:range cim:Susceptance ;
  skos:definition "Positive sequence shunt (charging) susceptance, uniformly distributed, of the entire line section.  This value represents the full charging over the full length of the line."@en .

cim:ACLineSegment.gch a owl:DatatypeProperty, owl:FunctionalProperty ;
  rdfs:label "gch"@en ;
  rdfs:domain cim:ACLineSegment ;
  rdfs:range cim:Conductance ;
  skos:definition "Positive sequence shunt (charging) conductance, uniformly distributed, of the entire line section."@en .

cim:ACLineSegment.r a owl:DatatypeProperty ;
  rdfs:label "r"@en ;
  rdfs:domain cim:ACLineSegment ;
  rdfs:range cim:Resistance ;
  skos:definition "Positive sequence series resistance of the entire line section."@en .

cim:ACLineSegment.x a owl:DatatypeProperty ;
  rdfs:label "x"@en ;
  rdfs:domain cim:ACLineSegment ;
  rdfs:range cim:Reactance ;
  skos:definition "Positive sequence series reactance of the entire line section."@en .

cim:ActivePower.multiplier a owl:DatatypeProperty, owl:FunctionalProperty ;
  rdfs:label "multiplier"@en ;
  eq:isFixed "True " ;
  rdf:value "M" ;
  rdfs:domain cim:ActivePower ;
  rdfs:range cim:UnitMultiplier .

cim:ActivePower.unit a owl:DatatypeProperty, owl:FunctionalProperty ;
  rdfs:label "unit"@en ;
  eq:isFixed "True " ;
  rdf:value "W" ;
  rdfs:domain cim:ActivePower ;
  rdfs:range cim:UnitSymbol .

cim:ActivePower.value a owl:DatatypeProperty, owl:FunctionalProperty ;
  rdfs:label "value"@en ;
  rdfs:domain cim:ActivePower ;
  rdfs:range xsd:float .

cim:ActivePowerLimit.normalValue a owl:DatatypeProperty ;
  rdfs:label "normalValue"@en ;
  rdfs:domain cim:ActivePowerLimit ;
  rdfs:range cim:ActivePower ;
  skos:definition "The normal value of active power limit. The attribute shall be a positive value or zero."@en .

cim:ActivePowerPerCurrentFlow.multiplier a owl:DatatypeProperty, owl:FunctionalProperty ;
  rdfs:label "multiplier"@en ;
  eq:isFixed "True " ;
  rdf:value "M" ;
  rdfs:domain cim:ActivePowerPerCurrentFlow ;
  rdfs:range cim:UnitMultiplier .

cim:ActivePowerPerCurrentFlow.unit a owl:DatatypeProperty, owl:FunctionalProperty ;
  rdfs:label "unit"@en ;
  eq:isFixed "True " ;
  rdf:value "WPerA" ;
  rdfs:domain cim:ActivePowerPerCurrentFlow ;
  rdfs:range cim:UnitSymbol .

cim:ActivePowerPerCurrentFlow.value a owl:DatatypeProperty, owl:FunctionalProperty ;
  rdfs:label "value"@en ;
  rdfs:domain cim:ActivePowerPerCurrentFlow ;
  rdfs:range xsd:float .

cim:ActivePowerPerFrequency.multiplier a owl:DatatypeProperty, owl:FunctionalProperty ;
  rdfs:label "multiplier"@en ;
  eq:isFixed "True " ;
  rdf:value "M" ;
  rdfs:domain cim:ActivePowerPerFrequency ;
  rdfs:range cim:UnitMultiplier .

cim:ActivePowerPerFrequency.unit a owl:DatatypeProperty, owl:FunctionalProperty ;
  rdfs:label "unit"@en ;
  eq:isFixed "True " ;
  rdf:value "WPers" ;
  rdfs:domain cim:ActivePowerPerFrequency ;
  rdfs:range cim:UnitSymbol .

cim:ActivePowerPerFrequency.value a owl:DatatypeProperty, owl:FunctionalProperty ;
  rdfs:label "value"@en ;
  rdfs:domain cim:ActivePowerPerFrequency ;
  rdfs:range xsd:float .

cim:AngleDegrees.multiplier a owl:DatatypeProperty, owl:FunctionalProperty ;
  rdfs:label "multiplier"@en ;
  eq:isFixed "True " ;
  rdf:value "none" ;
  rdfs:domain cim:AngleDegrees ;
  rdfs:range cim:UnitMultiplier .

cim:AngleDegrees.unit a owl:DatatypeProperty, owl:FunctionalProperty ;
  rdfs:label "unit"@en ;
  eq:isFixed "True " ;
  rdf:value "deg" ;
  rdfs:domain cim:AngleDegrees ;
  rdfs:range cim:UnitSymbol .

cim:AngleDegrees.value a owl:DatatypeProperty, owl:FunctionalProperty ;
  rdfs:label "value"@en ;
  rdfs:domain cim:AngleDegrees ;
  rdfs:range xsd:float .

cim:ApparentPower.multiplier a owl:DatatypeProperty, owl:FunctionalProperty ;
  rdfs:label "multiplier"@en ;
  eq:isFixed "True " ;
  rdf:value "M" ;
  rdfs:domain cim:ApparentPower ;
  rdfs:range cim:UnitMultiplier .

cim:ApparentPower.unit a owl:DatatypeProperty, owl:FunctionalProperty ;
  rdfs:label "unit"@en ;
  eq:isFixed "True " ;
  rdf:value "VA" ;
  rdfs:domain cim:ApparentPower ;
  rdfs:range cim:UnitSymbol .

cim:ApparentPower.value a owl:DatatypeProperty, owl:FunctionalProperty ;
  rdfs:label "value"@en ;
  rdfs:domain cim:ApparentPower ;
  rdfs:range xsd:float .

cim:ApparentPowerLimit.normalValue a owl:DatatypeProperty ;
  rdfs:label "normalValue"@en ;
  rdfs:domain cim:ApparentPowerLimit ;
  rdfs:range cim:ApparentPower ;
  skos:definition "The normal apparent power limit. The attribute shall be a positive value or zero."@en .

cim:AsynchronousMachine.nominalFrequency a owl:DatatypeProperty, owl:FunctionalProperty ;
  rdfs:label "nominalFrequency"@en ;
  rdfs:domain cim:AsynchronousMachine ;
  rdfs:range cim:Frequency ;
  skos:definition "Nameplate data indicates if the machine is 50 Hz or 60 Hz."@en .

cim:AsynchronousMachine.nominalSpeed a owl:DatatypeProperty, owl:FunctionalProperty ;
  rdfs:label "nominalSpeed"@en ;
  rdfs:domain cim:AsynchronousMachine ;
  rdfs:range cim:RotationSpeed ;
  skos:definition "Nameplate data.  Depends on the slip and number of pole pairs."@en .

cim:BaseVoltage.nominalVoltage a owl:DatatypeProperty ;
  rdfs:label "nominalVoltage"@en ;
  rdfs:domain cim:BaseVoltage ;
  rdfs:range cim:Voltage ;
  skos:definition "The power system resource's base voltage.  Shall be a positive value and not zero."@en .

cim:BasicIntervalSchedule.startTime a owl:DatatypeProperty ;
  rdfs:label "startTime"@en ;
  rdfs:domain cim:BasicIntervalSchedule ;
  rdfs:range xsd:dateTime ;
  skos:definition "The time for the first time point.  The value can be a time of day, not a specific date."@en .

cim:BasicIntervalSchedule.value1Unit a owl:DatatypeProperty ;
  rdfs:label "value1Unit"@en ;
  rdfs:domain cim:BasicIntervalSchedule ;
  rdfs:range cim:UnitSymbol ;
  skos:definition "Value1 units of measure."@en .

cim:BasicIntervalSchedule.value2Unit a owl:DatatypeProperty, owl:FunctionalProperty ;
  rdfs:label "value2Unit"@en ;
  rdfs:domain cim:BasicIntervalSchedule ;
  rdfs:range cim:UnitSymbol ;
  skos:definition "Value2 units of measure."@en .

cim:BatteryUnit.ratedE a owl:DatatypeProperty ;
  rdfs:label "ratedE"@en ;
  rdfs:domain cim:BatteryUnit ;
  rdfs:range cim:RealEnergy ;
  skos:definition "Full energy storage capacity of the battery. The attribute shall be a positive value."@en .

cim:BusNameMarker.priority a owl:DatatypeProperty, owl:FunctionalProperty ;
  rdfs:label "priority"@en ;
  rdfs:domain cim:BusNameMarker ;
  rdfs:range xsd:integer ;
  skos:definition "Priority of bus name marker for use as topology bus name.  Use 0 for do not care.  Use 1 for highest priority.  Use 2 as priority is less than 1 and so on."@en .

cim:Capacitance.multiplier a owl:DatatypeProperty, owl:FunctionalProperty ;
  rdfs:label "multiplier"@en ;
  eq:isFixed "True " ;
  rdf:value "none" ;
  rdfs:domain cim:Capacitance ;
  rdfs:range cim:UnitMultiplier .

cim:Capacitance.unit a owl:DatatypeProperty, owl:FunctionalProperty ;
  rdfs:label "unit"@en ;
  eq:isFixed "True " ;
  rdf:value "F" ;
  rdfs:domain cim:Capacitance ;
  rdfs:range cim:UnitSymbol .

cim:Capacitance.value a owl:DatatypeProperty, owl:FunctionalProperty ;
  rdfs:label "value"@en ;
  rdfs:domain cim:Capacitance ;
  rdfs:range xsd:float .

cim:Clamp.lengthFromTerminal1 a owl:DatatypeProperty, owl:FunctionalProperty ;
  rdfs:label "lengthFromTerminal1"@en ;
  rdfs:domain cim:Clamp ;
  rdfs:range cim:Length ;
  skos:definition """
The length to the place where the clamp is located starting from side one of the line segment, i.e. the line segment terminal with sequence number equal to 1.

\t"""@en .

cim:Conductance.multiplier a owl:DatatypeProperty, owl:FunctionalProperty ;
  rdfs:label "multiplier"@en ;
  eq:isFixed "True " ;
  rdf:value "none" ;
  rdfs:domain cim:Conductance ;
  rdfs:range cim:UnitMultiplier .

cim:Conductance.unit a owl:DatatypeProperty, owl:FunctionalProperty ;
  rdfs:label "unit"@en ;
  eq:isFixed "True " ;
  rdf:value "S" ;
  rdfs:domain cim:Conductance ;
  rdfs:range cim:UnitSymbol .

cim:Conductance.value a owl:DatatypeProperty, owl:FunctionalProperty ;
  rdfs:label "value"@en ;
  rdfs:domain cim:Conductance ;
  rdfs:range xsd:float .

cim:Conductor.length a owl:DatatypeProperty, owl:FunctionalProperty ;
  rdfs:label "length"@en ;
  rdfs:domain cim:Conductor ;
  rdfs:range cim:Length ;
  skos:definition "Segment length for calculating line section capabilities."@en .

cim:ControlArea.type a owl:DatatypeProperty ;
  rdfs:label "type"@en ;
  rdfs:domain cim:ControlArea ;
  rdfs:range cim:ControlAreaTypeKind ;
  skos:definition "The primary type of control area definition used to determine if this is used for automatic generation control, for planning interchange control, or other purposes.   A control area specified with primary type of automatic generation control could still be forecast and used as an interchange area in power flow analysis."@en .

cim:CsConverter.maxAlpha a owl:DatatypeProperty, owl:FunctionalProperty ;
  rdfs:label "maxAlpha"@en ;
  rdfs:domain cim:CsConverter ;
  rdfs:range cim:AngleDegrees ;
  skos:definition "Maximum firing angle. It is converter’s configuration data used in power flow. The attribute shall be a positive value."@en .

cim:CsConverter.maxGamma a owl:DatatypeProperty, owl:FunctionalProperty ;
  rdfs:label "maxGamma"@en ;
  rdfs:domain cim:CsConverter ;
  rdfs:range cim:AngleDegrees ;
  skos:definition "Maximum extinction angle. It is converter’s configuration data used in power flow. The attribute shall be a positive value."@en .

cim:CsConverter.maxIdc a owl:DatatypeProperty, owl:FunctionalProperty ;
  rdfs:label "maxIdc"@en ;
  rdfs:domain cim:CsConverter ;
  rdfs:range cim:CurrentFlow ;
  skos:definition "The maximum direct current (Id) on the DC side at which the converter should operate. It is converter’s configuration data use in power flow. The attribute shall be a positive value."@en .

cim:CsConverter.minAlpha a owl:DatatypeProperty, owl:FunctionalProperty ;
  rdfs:label "minAlpha"@en ;
  rdfs:domain cim:CsConverter ;
  rdfs:range cim:AngleDegrees ;
  skos:definition "Minimum firing angle. It is converter’s configuration data used in power flow. The attribute shall be a positive value."@en .

cim:CsConverter.minGamma a owl:DatatypeProperty, owl:FunctionalProperty ;
  rdfs:label "minGamma"@en ;
  rdfs:domain cim:CsConverter ;
  rdfs:range cim:AngleDegrees ;
  skos:definition "Minimum extinction angle. It is converter’s configuration data used in power flow. The attribute shall be a positive value."@en .

cim:CsConverter.minIdc a owl:DatatypeProperty, owl:FunctionalProperty ;
  rdfs:label "minIdc"@en ;
  rdfs:domain cim:CsConverter ;
  rdfs:range cim:CurrentFlow ;
  skos:definition "The minimum direct current (Id) on the DC side at which the converter should operate. It is converter’s configuration data used in power flow. The attribute shall be a positive value."@en .

cim:CsConverter.ratedIdc a owl:DatatypeProperty, owl:FunctionalProperty ;
  rdfs:label "ratedIdc"@en ;
  rdfs:domain cim:CsConverter ;
  rdfs:range cim:CurrentFlow ;
  skos:definition "Rated converter DC current, also called IdN. The attribute shall be a positive value. It is converter’s configuration data used in power flow."@en .

cim:CurrentFlow.multiplier a owl:DatatypeProperty, owl:FunctionalProperty ;
  rdfs:label "multiplier"@en ;
  eq:isFixed "True " ;
  rdf:value "none" ;
  rdfs:domain cim:CurrentFlow ;
  rdfs:range cim:UnitMultiplier .

cim:CurrentFlow.unit a owl:DatatypeProperty, owl:FunctionalProperty ;
  rdfs:label "unit"@en ;
  eq:isFixed "True " ;
  rdf:value "A" ;
  rdfs:domain cim:CurrentFlow ;
  rdfs:range cim:UnitSymbol .

cim:CurrentFlow.value a owl:DatatypeProperty, owl:FunctionalProperty ;
  rdfs:label "value"@en ;
  rdfs:domain cim:CurrentFlow ;
  rdfs:range xsd:float .

cim:CurrentLimit.normalValue a owl:DatatypeProperty ;
  rdfs:label "normalValue"@en ;
  rdfs:domain cim:CurrentLimit ;
  rdfs:range cim:CurrentFlow ;
  skos:definition "The normal value for limit on current flow. The attribute shall be a positive value or zero."@en .

cim:Curve.curveStyle a owl:DatatypeProperty ;
  rdfs:label "curveStyle"@en ;
  rdfs:domain cim:Curve ;
  rdfs:range cim:CurveStyle ;
  skos:definition "The style or shape of the curve."@en .

cim:Curve.xUnit a owl:DatatypeProperty ;
  rdfs:label "xUnit"@en ;
  rdfs:domain cim:Curve ;
  rdfs:range cim:UnitSymbol ;
  skos:definition "The X-axis units of measure."@en .

cim:Curve.y1Unit a owl:DatatypeProperty ;
  rdfs:label "y1Unit"@en ;
  rdfs:domain cim:Curve ;
  rdfs:range cim:UnitSymbol ;
  skos:definition "The Y1-axis units of measure."@en .

cim:Curve.y2Unit a owl:DatatypeProperty, owl:FunctionalProperty ;
  rdfs:label "y2Unit"@en ;
  rdfs:domain cim:Curve ;
  rdfs:range cim:UnitSymbol ;
  skos:definition "The Y2-axis units of measure."@en .

cim:CurveData.xvalue a owl:DatatypeProperty ;
  rdfs:label "xvalue"@en ;
  rdfs:domain cim:CurveData ;
  rdfs:range xsd:float ;
  skos:definition """
The data value of the X-axis variable,  depending on the X-axis units.

\t"""@en .

cim:CurveData.y1value a owl:DatatypeProperty ;
  rdfs:label "y1value"@en ;
  rdfs:domain cim:CurveData ;
  rdfs:range xsd:float ;
  skos:definition """
The data value of the  first Y-axis variable, depending on the Y-axis units.

\t"""@en .

cim:CurveData.y2value a owl:DatatypeProperty, owl:FunctionalProperty ;
  rdfs:label "y2value"@en ;
  rdfs:domain cim:CurveData ;
  rdfs:range xsd:float ;
  skos:definition """
The data value of the second Y-axis variable (if present), depending on the Y-axis units.

\t"""@en .

cim:Cut.lengthFromTerminal1 a owl:DatatypeProperty, owl:FunctionalProperty ;
  rdfs:label "lengthFromTerminal1"@en ;
  rdfs:domain cim:Cut ;
  rdfs:range cim:Length ;
  skos:definition """
The length to the place where the cut is located starting from side one of the cut line segment, i.e. the line segment Terminal with sequenceNumber equal to 1.

\t"""@en .

cim:DCConductingEquipment.ratedUdc a owl:DatatypeProperty ;
  rdfs:label "ratedUdc"@en ;
  rdfs:domain cim:DCConductingEquipment ;
  rdfs:range cim:Voltage ;
  skos:definition "Rated DC device voltage. The attribute shall be a positive value. It is configuration data used in power flow."@en .

cim:DCConverterUnit.operationMode a owl:DatatypeProperty ;
  rdfs:label "operationMode"@en ;
  rdfs:domain cim:DCConverterUnit ;
  rdfs:range cim:DCConverterOperatingModeKind ;
  skos:definition "The operating mode of an HVDC bipole (bipolar, monopolar metallic return, etc)."@en .

cim:DCGround.inductance a owl:DatatypeProperty, owl:FunctionalProperty ;
  rdfs:label "inductance"@en ;
  rdfs:domain cim:DCGround ;
  rdfs:range cim:Inductance ;
  skos:definition "Inductance to ground."@en .

cim:DCGround.r a owl:DatatypeProperty, owl:FunctionalProperty ;
  rdfs:label "r"@en ;
  rdfs:domain cim:DCGround ;
  rdfs:range cim:Resistance ;
  skos:definition "Resistance to ground."@en .

cim:DCLineSegment.capacitance a owl:DatatypeProperty ;
  rdfs:label "capacitance"@en ;
  rdfs:domain cim:DCLineSegment ;
  rdfs:range cim:Capacitance ;
  skos:definition "Capacitance of the DC line segment. Significant for cables only."@en .

cim:DCLineSegment.inductance a owl:DatatypeProperty ;
  rdfs:label "inductance"@en ;
  rdfs:domain cim:DCLineSegment ;
  rdfs:range cim:Inductance ;
  skos:definition "Inductance of the DC line segment. Negligible compared with DCSeriesDevice used for smoothing."@en .

cim:DCLineSegment.length a owl:DatatypeProperty, owl:FunctionalProperty ;
  rdfs:label "length"@en ;
  rdfs:domain cim:DCLineSegment ;
  rdfs:range cim:Length ;
  skos:definition "Segment length for calculating line section capabilities."@en .

cim:DCLineSegment.resistance a owl:DatatypeProperty ;
  rdfs:label "resistance"@en ;
  rdfs:domain cim:DCLineSegment ;
  rdfs:range cim:Resistance ;
  skos:definition "Resistance of the DC line segment."@en .

cim:DCSeriesDevice.inductance a owl:DatatypeProperty ;
  rdfs:label "inductance"@en ;
  rdfs:domain cim:DCSeriesDevice ;
  rdfs:range cim:Inductance ;
  skos:definition "Inductance of the device."@en .

cim:DCSeriesDevice.resistance a owl:DatatypeProperty ;
  rdfs:label "resistance"@en ;
  rdfs:domain cim:DCSeriesDevice ;
  rdfs:range cim:Resistance ;
  skos:definition "Resistance of the DC device."@en .

cim:DCShunt.capacitance a owl:DatatypeProperty ;
  rdfs:label "capacitance"@en ;
  rdfs:domain cim:DCShunt ;
  rdfs:range cim:Capacitance ;
  skos:definition "Capacitance of the DC shunt."@en .

cim:DCShunt.resistance a owl:DatatypeProperty ;
  rdfs:label "resistance"@en ;
  rdfs:domain cim:DCShunt ;
  rdfs:range cim:Resistance ;
  skos:definition "Resistance of the DC device."@en .

cim:EnergyConsumer.pfixed a owl:DatatypeProperty, owl:FunctionalProperty ;
  rdfs:label "pfixed"@en ;
  rdfs:domain cim:EnergyConsumer ;
  rdfs:range cim:ActivePower ;
  skos:definition "Active power of the load that is a fixed quantity and does not vary as load group value varies. Load sign convention is used, i.e. positive sign means flow out from a node.  "@en .

cim:EnergyConsumer.pfixedPct a owl:DatatypeProperty, owl:FunctionalProperty ;
  rdfs:label "pfixedPct"@en ;
  rdfs:domain cim:EnergyConsumer ;
  rdfs:range cim:PerCent ;
  skos:definition "Fixed active power as a percentage of load group fixed active power. Used to represent the time-varying components.  Load sign convention is used, i.e. positive sign means flow out from a node."@en .

cim:EnergyConsumer.qfixed a owl:DatatypeProperty, owl:FunctionalProperty ;
  rdfs:label "qfixed"@en ;
  rdfs:domain cim:EnergyConsumer ;
  rdfs:range cim:ReactivePower ;
  skos:definition """
Reactive power of the load that is a fixed quantity and does not vary as load group value varies. Load sign convention is used, i.e. positive sign means flow out from a node.

\t"""@en .

cim:EnergyConsumer.qfixedPct a owl:DatatypeProperty, owl:FunctionalProperty ;
  rdfs:label "qfixedPct"@en ;
  rdfs:domain cim:EnergyConsumer ;
  rdfs:range cim:PerCent ;
  skos:definition "Fixed reactive power as a percentage of load group fixed reactive power. Used to represent the time-varying components.  Load sign convention is used, i.e. positive sign means flow out from a node."@en .

cim:EnergySource.nominalVoltage a owl:DatatypeProperty, owl:FunctionalProperty ;
  rdfs:label "nominalVoltage"@en ;
  rdfs:domain cim:EnergySource ;
  rdfs:range cim:Voltage ;
  skos:definition "Phase-to-phase nominal voltage."@en .

cim:EnergySource.pMax a owl:DatatypeProperty, owl:FunctionalProperty ;
  rdfs:label "pMax"@en ;
  rdfs:domain cim:EnergySource ;
  rdfs:range cim:ActivePower ;
  skos:definition "This is the maximum active power that can be produced by the source. Load sign convention is used, i.e. positive sign means flow out from a TopologicalNode (bus) into the conducting equipment."@en .

cim:EnergySource.pMin a owl:DatatypeProperty, owl:FunctionalProperty ;
  rdfs:label "pMin"@en ;
  rdfs:domain cim:EnergySource ;
  rdfs:range cim:ActivePower ;
  skos:definition "This is the minimum active power that can be produced by the source. Load sign convention is used, i.e. positive sign means flow out from a TopologicalNode (bus) into the conducting equipment."@en .

cim:Equipment.aggregate a owl:DatatypeProperty, owl:FunctionalProperty ;
  rdfs:label "aggregate"@en ;
  rdfs:domain cim:Equipment ;
  rdfs:range xsd:boolean ;
  skos:definition """
The aggregate flag provides an alternative way of representing an aggregated (equivalent) element. It is applicable in cases when the dedicated classes for equivalent equipment do not have all of the attributes necessary to represent the required level of detail.  In case the flag is set to “true” the single instance of equipment represents multiple pieces of equipment that have been modelled together as an aggregate equivalent obtained by a network reduction procedure. Examples would be power transformers or synchronous machines operating in parallel modelled as a single aggregate power transformer or aggregate synchronous machine.  
The attribute is not used for EquivalentBranch, EquivalentShunt and EquivalentInjection.
\t"""@en .

cim:Equipment.normallyInService a owl:DatatypeProperty, owl:FunctionalProperty ;
  rdfs:label "normallyInService"@en ;
  rdfs:domain cim:Equipment ;
  rdfs:range xsd:boolean ;
  skos:definition "Specifies the availability of the equipment under normal operating conditions. True means the equipment is available for topology processing, which determines if the equipment is energized or not. False means that the equipment is treated by network applications as if it is not in the model."@en .

cim:EquivalentBranch.r a owl:DatatypeProperty ;
  rdfs:label "r"@en ;
  rdfs:domain cim:EquivalentBranch ;
  rdfs:range cim:Resistance ;
  skos:definition "Positive sequence series resistance of the reduced branch."@en .

cim:EquivalentBranch.r21 a owl:DatatypeProperty, owl:FunctionalProperty ;
  rdfs:label "r21"@en ;
  rdfs:domain cim:EquivalentBranch ;
  rdfs:range cim:Resistance ;
  skos:definition """
Resistance from terminal sequence 2 to terminal sequence 1 .Used for steady state power flow. This attribute is optional and represent unbalanced network such as off-nominal phase shifter. If only EquivalentBranch.r is given, then EquivalentBranch.r21 is assumed equal to EquivalentBranch.r.
Usage rule : EquivalentBranch is a result of network reduction prior to the data exchange.
\t"""@en .

cim:EquivalentBranch.x a owl:DatatypeProperty ;
  rdfs:label "x"@en ;
  rdfs:domain cim:EquivalentBranch ;
  rdfs:range cim:Reactance ;
  skos:definition "Positive sequence series reactance of the reduced branch."@en .

cim:EquivalentBranch.x21 a owl:DatatypeProperty, owl:FunctionalProperty ;
  rdfs:label "x21"@en ;
  rdfs:domain cim:EquivalentBranch ;
  rdfs:range cim:Reactance ;
  skos:definition """
Reactance from terminal sequence 2 to terminal sequence 1. Used for steady state power flow. This attribute is optional and represents an unbalanced network such as off-nominal phase shifter. If only EquivalentBranch.x is given, then EquivalentBranch.x21 is assumed equal to EquivalentBranch.x.
Usage rule: EquivalentBranch is a result of network reduction prior to the data exchange.
\t"""@en .

cim:EquivalentInjection.maxP a owl:DatatypeProperty, owl:FunctionalProperty ;
  rdfs:label "maxP"@en ;
  rdfs:domain cim:EquivalentInjection ;
  rdfs:range cim:ActivePower ;
  skos:definition "Maximum active power of the injection."@en .

cim:EquivalentInjection.maxQ a owl:DatatypeProperty, owl:FunctionalProperty ;
  rdfs:label "maxQ"@en ;
  rdfs:domain cim:EquivalentInjection ;
  rdfs:range cim:ReactivePower ;
  skos:definition "Maximum reactive power of the injection.  Used for modelling of infeed for load flow exchange. Not used for short circuit modelling.  If maxQ and minQ are not used ReactiveCapabilityCurve can be used.   "@en .

cim:EquivalentInjection.minP a owl:DatatypeProperty, owl:FunctionalProperty ;
  rdfs:label "minP"@en ;
  rdfs:domain cim:EquivalentInjection ;
  rdfs:range cim:ActivePower ;
  skos:definition "Minimum active power of the injection."@en .

cim:EquivalentInjection.minQ a owl:DatatypeProperty, owl:FunctionalProperty ;
  rdfs:label "minQ"@en ;
  rdfs:domain cim:EquivalentInjection ;
  rdfs:range cim:ReactivePower ;
  skos:definition "Minimum reactive power of the injection.  Used for modelling of infeed for load flow exchange. Not used for short circuit modelling.  If maxQ and minQ are not used ReactiveCapabilityCurve can be used."@en .

cim:EquivalentInjection.regulationCapability a owl:DatatypeProperty ;
  rdfs:label "regulationCapability"@en ;
  rdfs:domain cim:EquivalentInjection ;
  rdfs:range xsd:boolean ;
  skos:definition "Specifies whether or not the EquivalentInjection has the capability to regulate the local voltage. If true the EquivalentInjection can regulate. If false the EquivalentInjection cannot regulate. ReactiveCapabilityCurve can only be associated with EquivalentInjection  if the flag is true."@en .

cim:EquivalentShunt.b a owl:DatatypeProperty ;
  rdfs:label "b"@en ;
  rdfs:domain cim:EquivalentShunt ;
  rdfs:range cim:Susceptance ;
  skos:definition "Positive sequence shunt susceptance."@en .

cim:EquivalentShunt.g a owl:DatatypeProperty ;
  rdfs:label "g"@en ;
  rdfs:domain cim:EquivalentShunt ;
  rdfs:range cim:Conductance ;
  skos:definition "Positive sequence shunt conductance."@en .

cim:ExternalNetworkInjection.governorSCD a owl:DatatypeProperty ;
  rdfs:label "governorSCD"@en ;
  rdfs:domain cim:ExternalNetworkInjection ;
  rdfs:range cim:ActivePowerPerFrequency ;
  skos:definition "Power Frequency Bias. This is the change in power injection divided by the change in frequency and negated.  A positive value of the power frequency bias provides additional power injection upon a drop in frequency."@en .

cim:ExternalNetworkInjection.maxP a owl:DatatypeProperty ;
  rdfs:label "maxP"@en ;
  rdfs:domain cim:ExternalNetworkInjection ;
  rdfs:range cim:ActivePower ;
  skos:definition "Maximum active power of the injection."@en .

cim:ExternalNetworkInjection.maxQ a owl:DatatypeProperty ;
  rdfs:label "maxQ"@en ;
  rdfs:domain cim:ExternalNetworkInjection ;
  rdfs:range cim:ReactivePower ;
  skos:definition """
Maximum reactive power limit. It is used for modelling of infeed for load flow exchange and not for short circuit modelling.

\t"""@en .

cim:ExternalNetworkInjection.minP a owl:DatatypeProperty ;
  rdfs:label "minP"@en ;
  rdfs:domain cim:ExternalNetworkInjection ;
  rdfs:range cim:ActivePower ;
  skos:definition "Minimum active power of the injection."@en .

cim:ExternalNetworkInjection.minQ a owl:DatatypeProperty ;
  rdfs:label "minQ"@en ;
  rdfs:domain cim:ExternalNetworkInjection ;
  rdfs:range cim:ReactivePower ;
  skos:definition """
Minimum reactive power limit. It is used for modelling of infeed for load flow exchange and not for short circuit modelling.

\t"""@en .

cim:FossilFuel.fossilFuelType a owl:DatatypeProperty ;
  rdfs:label "fossilFuelType"@en ;
  rdfs:domain cim:FossilFuel ;
  rdfs:range cim:FuelType ;
  skos:definition "The type of fossil fuel, such as coal, oil, or gas."@en .

cim:Frequency.multiplier a owl:DatatypeProperty, owl:FunctionalProperty ;
  rdfs:label "multiplier"@en ;
  eq:isFixed "True " ;
  rdf:value "none" ;
  rdfs:domain cim:Frequency ;
  rdfs:range cim:UnitMultiplier .

cim:Frequency.unit a owl:DatatypeProperty, owl:FunctionalProperty ;
  rdfs:label "unit"@en ;
  eq:isFixed "True " ;
  rdf:value "Hz" ;
  rdfs:domain cim:Frequency ;
  rdfs:range cim:UnitSymbol .

cim:Frequency.value a owl:DatatypeProperty, owl:FunctionalProperty ;
  rdfs:label "value"@en ;
  rdfs:domain cim:Frequency ;
  rdfs:range xsd:float .

cim:GeneratingUnit.genControlSource a owl:DatatypeProperty, owl:FunctionalProperty ;
  rdfs:label "genControlSource"@en ;
  rdfs:domain cim:GeneratingUnit ;
  rdfs:range cim:GeneratorControlSource ;
  skos:definition "The source of controls for a generating unit.  Defines the control status of the generating unit."@en .

cim:GeneratingUnit.governorSCD a owl:DatatypeProperty, owl:FunctionalProperty ;
  rdfs:label "governorSCD"@en ;
  rdfs:domain cim:GeneratingUnit ;
  rdfs:range cim:PerCent ;
  skos:definition "Governor Speed Changer Droop.   This is the change in generator power output divided by the change in frequency normalized by the nominal power of the generator and the nominal frequency and expressed in percent and negated. A positive value of speed change droop provides additional generator output upon a drop in frequency."@en .

cim:GeneratingUnit.longPF a owl:DatatypeProperty, owl:FunctionalProperty ;
  rdfs:label "longPF"@en ;
  rdfs:domain cim:GeneratingUnit ;
  rdfs:range xsd:float ;
  skos:definition """
Generating unit long term economic participation factor.

\t"""@en .

cim:GeneratingUnit.maxOperatingP a owl:DatatypeProperty ;
  rdfs:label "maxOperatingP"@en ;
  rdfs:domain cim:GeneratingUnit ;
  rdfs:range cim:ActivePower ;
  skos:definition """
This is the maximum operating active power limit the dispatcher can enter for this unit.

\t"""@en .

cim:GeneratingUnit.maximumAllowableSpinningReserve a owl:DatatypeProperty, owl:FunctionalProperty ;
  rdfs:label "maximumAllowableSpinningReserve"@en ;
  rdfs:domain cim:GeneratingUnit ;
  rdfs:range cim:ActivePower ;
  skos:definition "Maximum allowable spinning reserve. Spinning reserve will never be considered greater than this value regardless of the current operating point."@en .

cim:GeneratingUnit.minOperatingP a owl:DatatypeProperty ;
  rdfs:label "minOperatingP"@en ;
  rdfs:domain cim:GeneratingUnit ;
  rdfs:range cim:ActivePower ;
  skos:definition "This is the minimum operating active power limit the dispatcher can enter for this unit."@en .

cim:GeneratingUnit.nominalP a owl:DatatypeProperty, owl:FunctionalProperty ;
  rdfs:label "nominalP"@en ;
  rdfs:domain cim:GeneratingUnit ;
  rdfs:range cim:ActivePower ;
  skos:definition """
The nominal power of the generating unit.  Used to give precise meaning to percentage based attributes such as the governor speed change droop (governorSCD attribute).
The attribute shall be a positive value equal to or less than RotatingMachine.ratedS.
\t"""@en .

cim:GeneratingUnit.ratedGrossMaxP a owl:DatatypeProperty, owl:FunctionalProperty ;
  rdfs:label "ratedGrossMaxP"@en ;
  rdfs:domain cim:GeneratingUnit ;
  rdfs:range cim:ActivePower ;
  skos:definition """
The unit's gross rated maximum capacity (book value).
The attribute shall be a positive value.

\t"""@en .

cim:GeneratingUnit.ratedGrossMinP a owl:DatatypeProperty, owl:FunctionalProperty ;
  rdfs:label "ratedGrossMinP"@en ;
  rdfs:domain cim:GeneratingUnit ;
  rdfs:range cim:ActivePower ;
  skos:definition """
The gross rated minimum generation level which the unit can safely operate at while delivering power to the transmission grid.
The attribute shall be a positive value.

\t"""@en .

cim:GeneratingUnit.ratedNetMaxP a owl:DatatypeProperty, owl:FunctionalProperty ;
  rdfs:label "ratedNetMaxP"@en ;
  rdfs:domain cim:GeneratingUnit ;
  rdfs:range cim:ActivePower ;
  skos:definition """
The net rated maximum capacity determined by subtracting the auxiliary power used to operate the internal plant machinery from the rated gross maximum capacity.
The attribute shall be a positive value.

\t"""@en .

cim:GeneratingUnit.shortPF a owl:DatatypeProperty, owl:FunctionalProperty ;
  rdfs:label "shortPF"@en ;
  rdfs:domain cim:GeneratingUnit ;
  rdfs:range xsd:float ;
  skos:definition """
Generating unit short term economic participation factor.

\t"""@en .

cim:GeneratingUnit.startupCost a owl:DatatypeProperty, owl:FunctionalProperty ;
  rdfs:label "startupCost"@en ;
  rdfs:domain cim:GeneratingUnit ;
  rdfs:range cim:Money ;
  skos:definition "The initial startup cost incurred for each start of the GeneratingUnit."@en .

cim:GeneratingUnit.startupTime a owl:DatatypeProperty, owl:FunctionalProperty ;
  rdfs:label "startupTime"@en ;
  rdfs:domain cim:GeneratingUnit ;
  rdfs:range cim:Seconds ;
  skos:definition """
Time it takes to get the unit on-line, from the time that the prime mover mechanical power is applied.

\t"""@en .

cim:GeneratingUnit.totalEfficiency a owl:DatatypeProperty, owl:FunctionalProperty ;
  rdfs:label "totalEfficiency"@en ;
  rdfs:domain cim:GeneratingUnit ;
  rdfs:range cim:PerCent ;
  skos:definition "The efficiency of the unit in converting the fuel into electrical energy."@en .

cim:GeneratingUnit.variableCost a owl:DatatypeProperty, owl:FunctionalProperty ;
  rdfs:label "variableCost"@en ;
  rdfs:domain cim:GeneratingUnit ;
  rdfs:range cim:Money ;
  skos:definition "The variable cost component of production per unit of ActivePower."@en .

cim:HydroGeneratingUnit.dropHeight a owl:DatatypeProperty, owl:FunctionalProperty ;
  rdfs:label "dropHeight"@en ;
  rdfs:domain cim:HydroGeneratingUnit ;
  rdfs:range cim:Length ;
  skos:definition "The height water drops from the reservoir mid-point to the turbine."@en .

cim:HydroGeneratingUnit.energyConversionCapability a owl:DatatypeProperty, owl:FunctionalProperty ;
  rdfs:label "energyConversionCapability"@en ;
  rdfs:domain cim:HydroGeneratingUnit ;
  rdfs:range cim:HydroEnergyConversionKind ;
  skos:definition "Energy conversion capability for generating."@en .

cim:HydroGeneratingUnit.turbineType a owl:DatatypeProperty, owl:FunctionalProperty ;
  rdfs:label "turbineType"@en ;
  rdfs:domain cim:HydroGeneratingUnit ;
  rdfs:range cim:HydroTurbineKind ;
  skos:definition "Type of turbine."@en .

cim:HydroPowerPlant.hydroPlantStorageType a owl:DatatypeProperty ;
  rdfs:label "hydroPlantStorageType"@en ;
  rdfs:domain cim:HydroPowerPlant ;
  rdfs:range cim:HydroPlantStorageKind ;
  skos:definition "The type of hydro power plant water storage."@en .

cim:IdentifiedObject.description a owl:DatatypeProperty, owl:FunctionalProperty ;
  rdfs:label "description"@en ;
  rdfs:domain cim:IdentifiedObject ;
  rdfs:range xsd:string ;
  skos:definition "The description is a free human readable text describing or naming the object. It may be non unique and may not correlate to a naming hierarchy."@en .

cim:IdentifiedObject.mRID a owl:DatatypeProperty ;
  rdfs:label "mRID"@en ;
  rdfs:domain cim:IdentifiedObject ;
  rdfs:range xsd:string ;
  skos:definition """
Master resource identifier issued by a model authority. The mRID is unique within an exchange context. Global uniqueness is easily achieved by using a UUID, as specified in RFC 4122, for the mRID. The use of UUID is strongly recommended.
For CIMXML data files in RDF syntax conforming to IEC 61970-552, the mRID is mapped to rdf:ID or rdf:about attributes that identify CIM object elements.
\t"""@en .

cim:IdentifiedObject.name a owl:DatatypeProperty ;
  rdfs:label "name"@en ;
  rdfs:domain cim:IdentifiedObject ;
  rdfs:range xsd:string ;
  skos:definition """
The name is any free human readable and possibly non unique text naming the object.

\t"""@en .

cim:Inductance.multiplier a owl:DatatypeProperty, owl:FunctionalProperty ;
  rdfs:label "multiplier"@en ;
  eq:isFixed "True " ;
  rdf:value "none" ;
  rdfs:domain cim:Inductance ;
  rdfs:range cim:UnitMultiplier .

cim:Inductance.unit a owl:DatatypeProperty, owl:FunctionalProperty ;
  rdfs:label "unit"@en ;
  eq:isFixed "True " ;
  rdf:value "H" ;
  rdfs:domain cim:Inductance ;
  rdfs:range cim:UnitSymbol .

cim:Inductance.value a owl:DatatypeProperty, owl:FunctionalProperty ;
  rdfs:label "value"@en ;
  rdfs:domain cim:Inductance ;
  rdfs:range xsd:float .

cim:Length.multiplier a owl:DatatypeProperty, owl:FunctionalProperty ;
  rdfs:label "multiplier"@en ;
  eq:isFixed "True " ;
  rdf:value "k" ;
  rdfs:domain cim:Length ;
  rdfs:range cim:UnitMultiplier .

cim:Length.unit a owl:DatatypeProperty, owl:FunctionalProperty ;
  rdfs:label "unit"@en ;
  eq:isFixed "True " ;
  rdf:value "m" ;
  rdfs:domain cim:Length ;
  rdfs:range cim:UnitSymbol .

cim:Length.value a owl:DatatypeProperty, owl:FunctionalProperty ;
  rdfs:label "value"@en ;
  rdfs:domain cim:Length ;
  rdfs:range xsd:float .

cim:LinearShuntCompensator.bPerSection a owl:DatatypeProperty ;
  rdfs:label "bPerSection"@en ;
  rdfs:domain cim:LinearShuntCompensator ;
  rdfs:range cim:Susceptance ;
  skos:definition "Positive sequence shunt (charging) susceptance per section."@en .

cim:LinearShuntCompensator.gPerSection a owl:DatatypeProperty ;
  rdfs:label "gPerSection"@en ;
  rdfs:domain cim:LinearShuntCompensator ;
  rdfs:range cim:Conductance ;
  skos:definition "Positive sequence shunt (charging) conductance per section."@en .

cim:LoadResponseCharacteristic.exponentModel a owl:DatatypeProperty ;
  rdfs:label "exponentModel"@en ;
  rdfs:domain cim:LoadResponseCharacteristic ;
  rdfs:range xsd:boolean ;
  skos:definition """
Indicates the exponential voltage dependency model is to be used. If false, the coefficient model is to be used.
The exponential voltage dependency model consist of the attributes:
- pVoltageExponent
- qVoltageExponent
- pFrequencyExponent
- qFrequencyExponent.
The coefficient model consist of the attributes:
- pConstantImpedance
- pConstantCurrent
- pConstantPower
- qConstantImpedance
- qConstantCurrent
- qConstantPower.
The sum of pConstantImpedance, pConstantCurrent and pConstantPower shall equal 1.
The sum of qConstantImpedance, qConstantCurrent and qConstantPower shall equal 1.
\t"""@en .

cim:LoadResponseCharacteristic.pConstantCurrent a owl:DatatypeProperty, owl:FunctionalProperty ;
  rdfs:label "pConstantCurrent"@en ;
  rdfs:domain cim:LoadResponseCharacteristic ;
  rdfs:range xsd:float ;
  skos:definition "Portion of active power load modelled as constant current."@en .

cim:LoadResponseCharacteristic.pConstantImpedance a owl:DatatypeProperty, owl:FunctionalProperty ;
  rdfs:label "pConstantImpedance"@en ;
  rdfs:domain cim:LoadResponseCharacteristic ;
  rdfs:range xsd:float ;
  skos:definition "Portion of active power load modelled as constant impedance."@en .

cim:LoadResponseCharacteristic.pConstantPower a owl:DatatypeProperty, owl:FunctionalProperty ;
  rdfs:label "pConstantPower"@en ;
  rdfs:domain cim:LoadResponseCharacteristic ;
  rdfs:range xsd:float ;
  skos:definition "Portion of active power load modelled as constant power."@en .

cim:LoadResponseCharacteristic.pFrequencyExponent a owl:DatatypeProperty, owl:FunctionalProperty ;
  rdfs:label "pFrequencyExponent"@en ;
  rdfs:domain cim:LoadResponseCharacteristic ;
  rdfs:range xsd:float ;
  skos:definition """
Exponent of per unit frequency effecting active power.

\t"""@en .

cim:LoadResponseCharacteristic.pVoltageExponent a owl:DatatypeProperty, owl:FunctionalProperty ;
  rdfs:label "pVoltageExponent"@en ;
  rdfs:domain cim:LoadResponseCharacteristic ;
  rdfs:range xsd:float ;
  skos:definition "Exponent of per unit voltage effecting real power."@en .

cim:LoadResponseCharacteristic.qConstantCurrent a owl:DatatypeProperty, owl:FunctionalProperty ;
  rdfs:label "qConstantCurrent"@en ;
  rdfs:domain cim:LoadResponseCharacteristic ;
  rdfs:range xsd:float ;
  skos:definition "Portion of reactive power load modelled as constant current."@en .

cim:LoadResponseCharacteristic.qConstantImpedance a owl:DatatypeProperty, owl:FunctionalProperty ;
  rdfs:label "qConstantImpedance"@en ;
  rdfs:domain cim:LoadResponseCharacteristic ;
  rdfs:range xsd:float ;
  skos:definition "Portion of reactive power load modelled as constant impedance."@en .

cim:LoadResponseCharacteristic.qConstantPower a owl:DatatypeProperty, owl:FunctionalProperty ;
  rdfs:label "qConstantPower"@en ;
  rdfs:domain cim:LoadResponseCharacteristic ;
  rdfs:range xsd:float ;
  skos:definition "Portion of reactive power load modelled as constant power."@en .

cim:LoadResponseCharacteristic.qFrequencyExponent a owl:DatatypeProperty, owl:FunctionalProperty ;
  rdfs:label "qFrequencyExponent"@en ;
  rdfs:domain cim:LoadResponseCharacteristic ;
  rdfs:range xsd:float ;
  skos:definition """
Exponent of per unit frequency effecting reactive power.

\t"""@en .

cim:LoadResponseCharacteristic.qVoltageExponent a owl:DatatypeProperty, owl:FunctionalProperty ;
  rdfs:label "qVoltageExponent"@en ;
  rdfs:domain cim:LoadResponseCharacteristic ;
  rdfs:range xsd:float ;
  skos:definition "Exponent of per unit voltage effecting reactive power."@en .

cim:Money.multiplier a owl:DatatypeProperty, owl:FunctionalProperty ;
  rdfs:label "multiplier"@en ;
  eq:isFixed "True " ;
  rdf:value "none" ;
  rdfs:domain cim:Money ;
  rdfs:range cim:UnitMultiplier .

cim:Money.unit a owl:DatatypeProperty, owl:FunctionalProperty ;
  rdfs:label "unit"@en ;
  rdfs:domain cim:Money ;
  rdfs:range cim:Currency .

cim:Money.value a owl:DatatypeProperty, owl:FunctionalProperty ;
  rdfs:label "value"@en ;
  rdfs:domain cim:Money ;
  rdfs:range xsd:decimal .

cim:NonlinearShuntCompensatorPoint.b a owl:DatatypeProperty ;
  rdfs:label "b"@en ;
  rdfs:domain cim:NonlinearShuntCompensatorPoint ;
  rdfs:range cim:Susceptance ;
  skos:definition "Positive sequence shunt (charging) susceptance per section."@en .

cim:NonlinearShuntCompensatorPoint.g a owl:DatatypeProperty ;
  rdfs:label "g"@en ;
  rdfs:domain cim:NonlinearShuntCompensatorPoint ;
  rdfs:range cim:Conductance ;
  skos:definition "Positive sequence shunt (charging) conductance per section."@en .

cim:NonlinearShuntCompensatorPoint.sectionNumber a owl:DatatypeProperty ;
  rdfs:label "sectionNumber"@en ;
  rdfs:domain cim:NonlinearShuntCompensatorPoint ;
  rdfs:range xsd:integer ;
  skos:definition "The number of the section."@en .

cim:OperationalLimitType.acceptableDuration a owl:DatatypeProperty, owl:FunctionalProperty ;
  rdfs:label "acceptableDuration"@en ;
  rdfs:domain cim:OperationalLimitType ;
  rdfs:range cim:Seconds ;
  skos:definition "The nominal acceptable duration of the limit. Limits are commonly expressed in terms of the time limit for which the limit is normally acceptable. The actual acceptable duration of a specific limit may depend on other local factors such as temperature or wind speed. The attribute has meaning only if the flag isInfiniteDuration is set to false, hence it shall not be exchanged when isInfiniteDuration is set to true."@en .

cim:OperationalLimitType.direction a owl:DatatypeProperty ;
  rdfs:label "direction"@en ;
  rdfs:domain cim:OperationalLimitType ;
  rdfs:range cim:OperationalLimitDirectionKind ;
  skos:definition "The direction of the limit."@en .

cim:OperationalLimitType.isInfiniteDuration a owl:DatatypeProperty ;
  rdfs:label "isInfiniteDuration"@en ;
  rdfs:domain cim:OperationalLimitType ;
  rdfs:range xsd:boolean ;
  skos:definition "Defines if the operational limit type has infinite duration. If true, the limit has infinite duration. If false, the limit has definite duration which is defined by the attribute acceptableDuration."@en .

cim:PerCent.multiplier a owl:DatatypeProperty, owl:FunctionalProperty ;
  rdfs:label "multiplier"@en ;
  eq:isFixed "True " ;
  rdf:value "none" ;
  rdfs:domain cim:PerCent ;
  rdfs:range cim:UnitMultiplier .

cim:PerCent.unit a owl:DatatypeProperty, owl:FunctionalProperty ;
  rdfs:label "unit"@en ;
  eq:isFixed "True " ;
  rdf:value "none" ;
  rdfs:domain cim:PerCent ;
  rdfs:range cim:UnitSymbol .

cim:PerCent.value a owl:DatatypeProperty, owl:FunctionalProperty ;
  rdfs:label "value"@en ;
  rdfs:domain cim:PerCent ;
  rdfs:range xsd:float ;
  skos:definition "Normally 0 to 100 on a defined base."@en .

cim:PhaseTapChangerAsymmetrical.windingConnectionAngle a owl:DatatypeProperty ;
  rdfs:label "windingConnectionAngle"@en ;
  rdfs:domain cim:PhaseTapChangerAsymmetrical ;
  rdfs:range cim:AngleDegrees ;
  skos:definition "The phase angle between the in-phase winding and the out-of -phase winding used for creating phase shift. The out-of-phase winding produces what is known as the difference voltage.  Setting this angle to 90 degrees is not the same as a symmetrical transformer. The attribute can only be multiples of 30 degrees.  The allowed range is -150 degrees to 150 degrees excluding 0."@en .

cim:PhaseTapChangerLinear.stepPhaseShiftIncrement a owl:DatatypeProperty ;
  rdfs:label "stepPhaseShiftIncrement"@en ;
  rdfs:domain cim:PhaseTapChangerLinear ;
  rdfs:range cim:AngleDegrees ;
  skos:definition """
Phase shift per step position. A positive value indicates a positive angle variation from the Terminal at the  PowerTransformerEnd,  where the TapChanger is located, into the transformer.
The actual phase shift increment might be more accurately computed from the symmetrical or asymmetrical models or a tap step table lookup if those are available.
\t"""@en .

cim:PhaseTapChangerLinear.xMax a owl:DatatypeProperty ;
  rdfs:label "xMax"@en ;
  rdfs:domain cim:PhaseTapChangerLinear ;
  rdfs:range cim:Reactance ;
  skos:definition "The reactance depends on the tap position according to a \"u\" shaped curve. The maximum reactance (xMax) appears at the low and high tap positions. Depending on the “u” curve the attribute can be either higher or lower than PowerTransformerEnd.x."@en .

cim:PhaseTapChangerLinear.xMin a owl:DatatypeProperty ;
  rdfs:label "xMin"@en ;
  eq:isdeprecated "True" ;
  rdfs:domain cim:PhaseTapChangerLinear ;
  rdfs:range cim:Reactance ;
  skos:definition "The reactance depends on the tap position according to a \"u\" shaped curve. The minimum reactance (xMin) appears at the mid tap position.  PowerTransformerEnd.x shall be consistent with PhaseTapChangerLinear.xMin and PhaseTapChangerNonLinear.xMin. In case of inconsistency, PowerTransformerEnd.x shall be used."@en .

cim:PhaseTapChangerNonLinear.voltageStepIncrement a owl:DatatypeProperty ;
  rdfs:label "voltageStepIncrement"@en ;
  rdfs:domain cim:PhaseTapChangerNonLinear ;
  rdfs:range cim:PerCent ;
  skos:definition """
The voltage step increment on the out of phase winding (the PowerTransformerEnd where the TapChanger is located) specified in percent of rated voltage of the PowerTransformerEnd. A positive value means a positive voltage variation from the Terminal at the PowerTransformerEnd, where the TapChanger is located, into the transformer.
When the increment is negative, the voltage decreases when the tap step increases.
\t"""@en .

cim:PhaseTapChangerNonLinear.xMax a owl:DatatypeProperty ;
  rdfs:label "xMax"@en ;
  rdfs:domain cim:PhaseTapChangerNonLinear ;
  rdfs:range cim:Reactance ;
  skos:definition """
The reactance depends on the tap position according to a "u" shaped curve. The maximum reactance (xMax) appears at the low and high tap positions. Depending on the “u” curve the attribute can be either higher or lower than PowerTransformerEnd.x.

\t"""@en .

cim:PhaseTapChangerNonLinear.xMin a owl:DatatypeProperty ;
  rdfs:label "xMin"@en ;
  eq:isdeprecated "True" ;
  rdfs:domain cim:PhaseTapChangerNonLinear ;
  rdfs:range cim:Reactance ;
  skos:definition """
The reactance depend on the tap position according to a "u" shaped curve. The minimum reactance (xMin) appear at the mid tap position.   PowerTransformerEnd.x shall be consistent with PhaseTapChangerLinear.xMin and PhaseTapChangerNonLinear.xMin. In case of inconsistency, PowerTransformerEnd.x shall be used.

\t"""@en .

cim:PhaseTapChangerTablePoint.angle a owl:DatatypeProperty ;
  rdfs:label "angle"@en ;
  rdfs:domain cim:PhaseTapChangerTablePoint ;
  rdfs:range cim:AngleDegrees ;
  skos:definition """
The angle difference in degrees. A positive value indicates a positive angle variation from the Terminal at the  PowerTransformerEnd,  where the TapChanger is located, into the transformer.

\t"""@en .

cim:PowerElectronicsConnection.maxQ a owl:DatatypeProperty, owl:FunctionalProperty ;
  rdfs:label "maxQ"@en ;
  rdfs:domain cim:PowerElectronicsConnection ;
  rdfs:range cim:ReactivePower ;
  skos:definition "Maximum reactive power limit. This is the maximum (nameplate) limit for the unit."@en .

cim:PowerElectronicsConnection.minQ a owl:DatatypeProperty, owl:FunctionalProperty ;
  rdfs:label "minQ"@en ;
  rdfs:domain cim:PowerElectronicsConnection ;
  rdfs:range cim:ReactivePower ;
  skos:definition "Minimum reactive power limit for the unit. This is the minimum (nameplate) limit for the unit."@en .

cim:PowerElectronicsConnection.ratedS a owl:DatatypeProperty, owl:FunctionalProperty ;
  rdfs:label "ratedS"@en ;
  rdfs:domain cim:PowerElectronicsConnection ;
  rdfs:range cim:ApparentPower ;
  skos:definition """
Nameplate apparent power rating for the unit.
The attribute shall have a positive value.
\t"""@en .

cim:PowerElectronicsConnection.ratedU a owl:DatatypeProperty, owl:FunctionalProperty ;
  rdfs:label "ratedU"@en ;
  rdfs:domain cim:PowerElectronicsConnection ;
  rdfs:range cim:Voltage ;
  skos:definition """
Rated voltage (nameplate data, Ur in IEC 60909-0). It is primarily used for short circuit data exchange according to IEC 60909.
The attribute shall be a positive value.
\t"""@en .

cim:PowerElectronicsUnit.maxP a owl:DatatypeProperty, owl:FunctionalProperty ;
  rdfs:label "maxP"@en ;
  rdfs:domain cim:PowerElectronicsUnit ;
  rdfs:range cim:ActivePower ;
  skos:definition "Maximum active power limit. This is the maximum (nameplate) limit for the unit."@en .

cim:PowerElectronicsUnit.minP a owl:DatatypeProperty, owl:FunctionalProperty ;
  rdfs:label "minP"@en ;
  rdfs:domain cim:PowerElectronicsUnit ;
  rdfs:range cim:ActivePower ;
  skos:definition "Minimum active power limit. This is the minimum (nameplate) limit for the unit."@en .

cim:PowerTransformerEnd.b a owl:DatatypeProperty ;
  rdfs:label "b"@en ;
  rdfs:domain cim:PowerTransformerEnd ;
  rdfs:range cim:Susceptance ;
  skos:definition """
Magnetizing branch susceptance (B mag).  The value can be positive or negative.

\t"""@en .

cim:PowerTransformerEnd.connectionKind a owl:DatatypeProperty, owl:FunctionalProperty ;
  rdfs:label "connectionKind"@en ;
  rdfs:domain cim:PowerTransformerEnd ;
  rdfs:range cim:WindingConnection ;
  skos:definition """
Kind of connection.

\t"""@en .

cim:PowerTransformerEnd.g a owl:DatatypeProperty, owl:FunctionalProperty ;
  rdfs:label "g"@en ;
  rdfs:domain cim:PowerTransformerEnd ;
  rdfs:range cim:Conductance ;
  skos:definition """
Magnetizing branch conductance.

\t"""@en .

cim:PowerTransformerEnd.r a owl:DatatypeProperty ;
  rdfs:label "r"@en ;
  rdfs:domain cim:PowerTransformerEnd ;
  rdfs:range cim:Resistance ;
  skos:definition """
Resistance (star-model) of the transformer end.
The attribute shall be equal to or greater than zero for non-equivalent transformers.
\t"""@en .

cim:PowerTransformerEnd.ratedS a owl:DatatypeProperty, owl:FunctionalProperty ;
  rdfs:label "ratedS"@en ;
  rdfs:domain cim:PowerTransformerEnd ;
  rdfs:range cim:ApparentPower ;
  skos:definition """
Normal apparent power rating.
The attribute shall be a positive value. For a two-winding transformer the values for the high and low voltage sides shall be identical. 
\t"""@en .

cim:PowerTransformerEnd.ratedU a owl:DatatypeProperty ;
  rdfs:label "ratedU"@en ;
  rdfs:domain cim:PowerTransformerEnd ;
  rdfs:range cim:Voltage ;
  skos:definition """
Rated voltage: phase-phase for three-phase windings, and either phase-phase or phase-neutral for single-phase windings.
A high voltage side, as given by TransformerEnd.endNumber, shall have a ratedU that is greater than or equal to ratedU for the lower voltage sides.
The attribute shall be a positive value.
\t"""@en .

cim:PowerTransformerEnd.x a owl:DatatypeProperty ;
  rdfs:label "x"@en ;
  rdfs:domain cim:PowerTransformerEnd ;
  rdfs:range cim:Reactance ;
  skos:definition """
Positive sequence series reactance (star-model) of the transformer end.

\t"""@en .

cim:RatioTapChanger.stepVoltageIncrement a owl:DatatypeProperty ;
  rdfs:label "stepVoltageIncrement"@en ;
  rdfs:domain cim:RatioTapChanger ;
  rdfs:range cim:PerCent ;
  skos:definition """
Tap step increment, in per cent of rated voltage of the power transformer end, per step position.
When the increment is negative, the voltage decreases when the tap step increases.
\t"""@en .

cim:Reactance.multiplier a owl:DatatypeProperty, owl:FunctionalProperty ;
  rdfs:label "multiplier"@en ;
  eq:isFixed "True " ;
  rdf:value "none" ;
  rdfs:domain cim:Reactance ;
  rdfs:range cim:UnitMultiplier .

cim:Reactance.unit a owl:DatatypeProperty, owl:FunctionalProperty ;
  rdfs:label "unit"@en ;
  eq:isFixed "True " ;
  rdf:value "ohm" ;
  rdfs:domain cim:Reactance ;
  rdfs:range cim:UnitSymbol .

cim:Reactance.value a owl:DatatypeProperty, owl:FunctionalProperty ;
  rdfs:label "value"@en ;
  rdfs:domain cim:Reactance ;
  rdfs:range xsd:float .

cim:ReactivePower.multiplier a owl:DatatypeProperty, owl:FunctionalProperty ;
  rdfs:label "multiplier"@en ;
  eq:isFixed "True " ;
  rdf:value "M" ;
  rdfs:domain cim:ReactivePower ;
  rdfs:range cim:UnitMultiplier .

cim:ReactivePower.unit a owl:DatatypeProperty, owl:FunctionalProperty ;
  rdfs:label "unit"@en ;
  eq:isFixed "True " ;
  rdf:value "VAr" ;
  rdfs:domain cim:ReactivePower ;
  rdfs:range cim:UnitSymbol .

cim:ReactivePower.value a owl:DatatypeProperty, owl:FunctionalProperty ;
  rdfs:label "value"@en ;
  rdfs:domain cim:ReactivePower ;
  rdfs:range xsd:float .

cim:RealEnergy.multiplier a owl:DatatypeProperty, owl:FunctionalProperty ;
  rdfs:label "multiplier"@en ;
  eq:isFixed "True " ;
  rdf:value "M" ;
  rdfs:domain cim:RealEnergy ;
  rdfs:range cim:UnitMultiplier .

cim:RealEnergy.unit a owl:DatatypeProperty, owl:FunctionalProperty ;
  rdfs:label "unit"@en ;
  eq:isFixed "True " ;
  rdf:value "Wh" ;
  rdfs:domain cim:RealEnergy ;
  rdfs:range cim:UnitSymbol .

cim:RealEnergy.value a owl:DatatypeProperty, owl:FunctionalProperty ;
  rdfs:label "value"@en ;
  rdfs:domain cim:RealEnergy ;
  rdfs:range xsd:float .

cim:RegularIntervalSchedule.endTime a owl:DatatypeProperty ;
  rdfs:label "endTime"@en ;
  rdfs:domain cim:RegularIntervalSchedule ;
  rdfs:range xsd:dateTime ;
  skos:definition "The time for the last time point.  The value can be a time of day, not a specific date."@en .

cim:RegularIntervalSchedule.timeStep a owl:DatatypeProperty ;
  rdfs:label "timeStep"@en ;
  rdfs:domain cim:RegularIntervalSchedule ;
  rdfs:range cim:Seconds ;
  skos:definition """
The time between each pair of subsequent regular time points in sequence order.

\t"""@en .

cim:RegularTimePoint.sequenceNumber a owl:DatatypeProperty ;
  rdfs:label "sequenceNumber"@en ;
  rdfs:domain cim:RegularTimePoint ;
  rdfs:range xsd:integer ;
  skos:definition """
The position of the regular time point in the sequence. Note that time points don't have to be sequential, i.e. time points may be omitted. The actual time for a RegularTimePoint is computed by multiplying the associated regular interval schedule's time step with the regular time point sequence number and adding the associated schedules start time. To specify values for the start time, use sequence number 0.  The sequence number cannot be negative.

\t"""@en .

cim:RegularTimePoint.value1 a owl:DatatypeProperty ;
  rdfs:label "value1"@en ;
  rdfs:domain cim:RegularTimePoint ;
  rdfs:range xsd:float ;
  skos:definition """
The first value at the time. The meaning of the value is defined by the derived type of the associated schedule.

\t"""@en .

cim:RegularTimePoint.value2 a owl:DatatypeProperty, owl:FunctionalProperty ;
  rdfs:label "value2"@en ;
  rdfs:domain cim:RegularTimePoint ;
  rdfs:range xsd:float ;
  skos:definition """
The second value at the time. The meaning of the value is defined by the derived type of the associated schedule.


\t"""@en .

cim:RegulatingControl.mode a owl:DatatypeProperty ;
  rdfs:label "mode"@en ;
  rdfs:domain cim:RegulatingControl ;
  rdfs:range cim:RegulatingControlModeKind ;
  skos:definition "The regulating control mode presently available.  This specification allows for determining the kind of regulation without need for obtaining the units from a schedule."@en .

cim:Resistance.multiplier a owl:DatatypeProperty, owl:FunctionalProperty ;
  rdfs:label "multiplier"@en ;
  eq:isFixed "True " ;
  rdf:value "none" ;
  rdfs:domain cim:Resistance ;
  rdfs:range cim:UnitMultiplier .

cim:Resistance.unit a owl:DatatypeProperty, owl:FunctionalProperty ;
  rdfs:label "unit"@en ;
  eq:isFixed "True " ;
  rdf:value "ohm" ;
  rdfs:domain cim:Resistance ;
  rdfs:range cim:UnitSymbol .

cim:Resistance.value a owl:DatatypeProperty, owl:FunctionalProperty ;
  rdfs:label "value"@en ;
  rdfs:domain cim:Resistance ;
  rdfs:range xsd:float .

cim:RotatingMachine.ratedPowerFactor a owl:DatatypeProperty, owl:FunctionalProperty ;
  rdfs:label "ratedPowerFactor"@en ;
  rdfs:domain cim:RotatingMachine ;
  rdfs:range xsd:float ;
  skos:definition "Power factor (nameplate data). It is primarily used for short circuit data exchange according to IEC 60909. The attribute cannot be a negative value."@en .

cim:RotatingMachine.ratedS a owl:DatatypeProperty, owl:FunctionalProperty ;
  rdfs:label "ratedS"@en ;
  rdfs:domain cim:RotatingMachine ;
  rdfs:range cim:ApparentPower ;
  skos:definition """
Nameplate apparent power rating for the unit.
The attribute shall have a positive value.
\t"""@en .

cim:RotatingMachine.ratedU a owl:DatatypeProperty, owl:FunctionalProperty ;
  rdfs:label "ratedU"@en ;
  rdfs:domain cim:RotatingMachine ;
  rdfs:range cim:Voltage ;
  skos:definition """
Rated voltage (nameplate data, Ur in IEC 60909-0). It is primarily used for short circuit data exchange according to IEC 60909.
The attribute shall be a positive value.
\t"""@en .

cim:RotationSpeed.multiplier a owl:DatatypeProperty, owl:FunctionalProperty ;
  rdfs:label "multiplier"@en ;
  eq:isFixed "True " ;
  rdf:value "none" ;
  rdfs:domain cim:RotationSpeed ;
  rdfs:range cim:UnitMultiplier .

cim:RotationSpeed.unit a owl:DatatypeProperty, owl:FunctionalProperty ;
  rdfs:label "unit"@en ;
  eq:isFixed "True " ;
  rdf:value "Hz" ;
  rdfs:domain cim:RotationSpeed ;
  rdfs:range cim:UnitSymbol .

cim:RotationSpeed.value a owl:DatatypeProperty, owl:FunctionalProperty ;
  rdfs:label "value"@en ;
  rdfs:domain cim:RotationSpeed ;
  rdfs:range xsd:float .

cim:Season.endDate a owl:DatatypeProperty ;
  rdfs:label "endDate"@en ;
  rdfs:domain cim:Season ;
  rdfs:range xsd:gMonthDay ;
  skos:definition "Date season ends."@en .

cim:Season.startDate a owl:DatatypeProperty ;
  rdfs:label "startDate"@en ;
  rdfs:domain cim:Season ;
  rdfs:range xsd:gMonthDay ;
  skos:definition "Date season starts."@en .

cim:Seconds.multiplier a owl:DatatypeProperty, owl:FunctionalProperty ;
  rdfs:label "multiplier"@en ;
  eq:isFixed "True " ;
  rdf:value "none" ;
  rdfs:domain cim:Seconds ;
  rdfs:range cim:UnitMultiplier .

cim:Seconds.unit a owl:DatatypeProperty, owl:FunctionalProperty ;
  rdfs:label "unit"@en ;
  eq:isFixed "True " ;
  rdf:value "s" ;
  rdfs:domain cim:Seconds ;
  rdfs:range cim:UnitSymbol .

cim:Seconds.value a owl:DatatypeProperty, owl:FunctionalProperty ;
  rdfs:label "value"@en ;
  rdfs:domain cim:Seconds ;
  rdfs:range xsd:float ;
  skos:definition "Time, in seconds"@en .

cim:SeriesCompensator.r a owl:DatatypeProperty ;
  rdfs:label "r"@en ;
  rdfs:domain cim:SeriesCompensator ;
  rdfs:range cim:Resistance ;
  skos:definition "Positive sequence resistance."@en .

cim:SeriesCompensator.x a owl:DatatypeProperty ;
  rdfs:label "x"@en ;
  rdfs:domain cim:SeriesCompensator ;
  rdfs:range cim:Reactance ;
  skos:definition "Positive sequence reactance."@en .

cim:ShuntCompensator.aVRDelay a owl:DatatypeProperty, owl:FunctionalProperty ;
  rdfs:label "aVRDelay"@en ;
  rdfs:domain cim:ShuntCompensator ;
  rdfs:range cim:Seconds ;
  skos:definition "An automatic voltage regulation delay (AVRDelay) which is the time delay from a change in voltage to when the capacitor is allowed to change state. This filters out temporary changes in voltage."@en .

cim:ShuntCompensator.grounded a owl:DatatypeProperty, owl:FunctionalProperty ;
  rdfs:label "grounded"@en ;
  rdfs:domain cim:ShuntCompensator ;
  rdfs:range xsd:boolean ;
  skos:definition "Used for Yn and Zn connections. True if the neutral is solidly grounded."@en .

cim:ShuntCompensator.maximumSections a owl:DatatypeProperty ;
  rdfs:label "maximumSections"@en ;
  rdfs:domain cim:ShuntCompensator ;
  rdfs:range xsd:integer ;
  skos:definition """
The maximum number of sections that may be switched in. 

\t"""@en .

cim:ShuntCompensator.nomU a owl:DatatypeProperty ;
  rdfs:label "nomU"@en ;
  rdfs:domain cim:ShuntCompensator ;
  rdfs:range cim:Voltage ;
  skos:definition """
The voltage at which the nominal reactive power may be calculated. This should normally be within 10% of the voltage at which the capacitor is connected to the network.

\t"""@en .

cim:ShuntCompensator.normalSections a owl:DatatypeProperty ;
  rdfs:label "normalSections"@en ;
  rdfs:domain cim:ShuntCompensator ;
  rdfs:range xsd:integer ;
  skos:definition """
The normal number of sections switched in. The value shall be between zero and ShuntCompensator.maximumSections.

\t"""@en .

cim:ShuntCompensator.voltageSensitivity a owl:DatatypeProperty, owl:FunctionalProperty ;
  rdfs:label "voltageSensitivity"@en ;
  rdfs:domain cim:ShuntCompensator ;
  rdfs:range cim:VoltagePerReactivePower ;
  skos:definition "Voltage sensitivity required for the device to regulate the bus voltage, in voltage/reactive power."@en .

cim:StaticVarCompensator.capacitiveRating a owl:DatatypeProperty ;
  rdfs:label "capacitiveRating"@en ;
  rdfs:domain cim:StaticVarCompensator ;
  rdfs:range cim:Reactance ;
  skos:definition "Capacitive reactance at maximum capacitive reactive power.  Shall always be positive."@en .

cim:StaticVarCompensator.inductiveRating a owl:DatatypeProperty ;
  rdfs:label "inductiveRating"@en ;
  rdfs:domain cim:StaticVarCompensator ;
  rdfs:range cim:Reactance ;
  skos:definition "Inductive reactance at maximum inductive reactive power.  Shall always be negative.  "@en .

cim:StaticVarCompensator.sVCControlMode a owl:DatatypeProperty, owl:FunctionalProperty ;
  rdfs:label "sVCControlMode"@en ;
  eq:isdeprecated "True" ;
  rdfs:domain cim:StaticVarCompensator ;
  rdfs:range cim:SVCControlMode ;
  skos:definition "SVC control mode."@en .

cim:StaticVarCompensator.slope a owl:DatatypeProperty ;
  rdfs:label "slope"@en ;
  rdfs:domain cim:StaticVarCompensator ;
  rdfs:range cim:VoltagePerReactivePower ;
  skos:definition """
The characteristics slope of an SVC defines how the reactive power output changes in proportion to the difference between the regulated bus voltage and the voltage setpoint.
The attribute shall be a positive value or zero.
\t"""@en .

cim:StaticVarCompensator.voltageSetPoint a owl:DatatypeProperty, owl:FunctionalProperty ;
  rdfs:label "voltageSetPoint"@en ;
  eq:isdeprecated "True" ;
  rdfs:domain cim:StaticVarCompensator ;
  rdfs:range cim:Voltage ;
  skos:definition "The reactive power output of the SVC is proportional to the difference between the voltage at the regulated bus and the voltage setpoint.  When the regulated bus voltage is equal to the voltage setpoint, the reactive power output is zero."@en .

cim:Susceptance.multiplier a owl:DatatypeProperty, owl:FunctionalProperty ;
  rdfs:label "multiplier"@en ;
  eq:isFixed "True " ;
  rdf:value "none" ;
  rdfs:domain cim:Susceptance ;
  rdfs:range cim:UnitMultiplier .

cim:Susceptance.unit a owl:DatatypeProperty, owl:FunctionalProperty ;
  rdfs:label "unit"@en ;
  eq:isFixed "True " ;
  rdf:value "S" ;
  rdfs:domain cim:Susceptance ;
  rdfs:range cim:UnitSymbol .

cim:Susceptance.value a owl:DatatypeProperty, owl:FunctionalProperty ;
  rdfs:label "value"@en ;
  rdfs:domain cim:Susceptance ;
  rdfs:range xsd:float .

cim:Switch.normalOpen a owl:DatatypeProperty ;
  rdfs:label "normalOpen"@en ;
  rdfs:domain cim:Switch ;
  rdfs:range xsd:boolean ;
  skos:definition "The attribute is used in cases when no Measurement for the status value is present. If the Switch has a status measurement the Discrete.normalValue is expected to match with the Switch.normalOpen."@en .

cim:Switch.ratedCurrent a owl:DatatypeProperty, owl:FunctionalProperty ;
  rdfs:label "ratedCurrent"@en ;
  rdfs:domain cim:Switch ;
  rdfs:range cim:CurrentFlow ;
  skos:definition """
The maximum continuous current carrying capacity in amps governed by the device material and construction.
The attribute shall be a positive value.


\t"""@en .

cim:Switch.retained a owl:DatatypeProperty ;
  rdfs:label "retained"@en ;
  rdfs:domain cim:Switch ;
  rdfs:range xsd:boolean ;
  skos:definition "Branch is retained in the topological solution.  The flow through retained switches will normally be calculated in power flow."@en .

cim:SynchronousMachine.maxQ a owl:DatatypeProperty, owl:FunctionalProperty ;
  rdfs:label "maxQ"@en ;
  rdfs:domain cim:SynchronousMachine ;
  rdfs:range cim:ReactivePower ;
  skos:definition "Maximum reactive power limit. This is the maximum (nameplate) limit for the unit."@en .

cim:SynchronousMachine.minQ a owl:DatatypeProperty, owl:FunctionalProperty ;
  rdfs:label "minQ"@en ;
  rdfs:domain cim:SynchronousMachine ;
  rdfs:range cim:ReactivePower ;
  skos:definition "Minimum reactive power limit for the unit."@en .

cim:SynchronousMachine.qPercent a owl:DatatypeProperty, owl:FunctionalProperty ;
  rdfs:label "qPercent"@en ;
  rdfs:domain cim:SynchronousMachine ;
  rdfs:range cim:PerCent ;
  skos:definition "Part of the coordinated reactive control that comes from this machine. The attribute is used as a participation factor not necessarily summing up to 100% for the participating devices in the control."@en .

cim:SynchronousMachine.type a owl:DatatypeProperty ;
  rdfs:label "type"@en ;
  rdfs:domain cim:SynchronousMachine ;
  rdfs:range cim:SynchronousMachineKind ;
  skos:definition "Modes that this synchronous machine can operate in."@en .

cim:TapChanger.highStep a owl:DatatypeProperty ;
  rdfs:label "highStep"@en ;
  rdfs:domain cim:TapChanger ;
  rdfs:range xsd:integer ;
  skos:definition """
Highest possible tap step position, advance from neutral.
The attribute shall be greater than lowStep.
\t"""@en .

cim:TapChanger.lowStep a owl:DatatypeProperty ;
  rdfs:label "lowStep"@en ;
  rdfs:domain cim:TapChanger ;
  rdfs:range xsd:integer ;
  skos:definition "Lowest possible tap step position, retard from neutral."@en .

cim:TapChanger.ltcFlag a owl:DatatypeProperty ;
  rdfs:label "ltcFlag"@en ;
  rdfs:domain cim:TapChanger ;
  rdfs:range xsd:boolean ;
  skos:definition "Specifies whether or not a TapChanger has load tap changing capabilities."@en .

cim:TapChanger.neutralStep a owl:DatatypeProperty ;
  rdfs:label "neutralStep"@en ;
  rdfs:domain cim:TapChanger ;
  rdfs:range xsd:integer ;
  skos:definition """
The neutral tap step position for this winding.
The attribute shall be equal to or greater than lowStep and equal or less than highStep.
It is the step position where the voltage is neutralU when the other terminals of the transformer are at the ratedU.  If there are other tap changers on the transformer those taps are kept constant at their neutralStep.
\t"""@en .

cim:TapChanger.neutralU a owl:DatatypeProperty ;
  rdfs:label "neutralU"@en ;
  rdfs:domain cim:TapChanger ;
  rdfs:range cim:Voltage ;
  skos:definition """
Voltage at which the winding operates at the neutral tap setting. It is the voltage at the terminal of the PowerTransformerEnd associated with the tap changer when all tap changers on the transformer are at their neutralStep position.  Normally neutralU of the tap changer is the same as ratedU of the PowerTransformerEnd, but it can differ in special cases such as when the tapping mechanism is separate from the winding more common on lower voltage transformers.
This attribute is not relevant for PhaseTapChangerAsymmetrical, PhaseTapChangerSymmetrical and PhaseTapChangerLinear. 
\t"""@en .

cim:TapChanger.normalStep a owl:DatatypeProperty ;
  rdfs:label "normalStep"@en ;
  rdfs:domain cim:TapChanger ;
  rdfs:range xsd:integer ;
  skos:definition """
The tap step position used in "normal" network operation for this winding. For a "Fixed" tap changer indicates the current physical tap setting.
The attribute shall be equal to or greater than lowStep and equal to or less than highStep.
\t"""@en .

cim:TapChangerTablePoint.b a owl:DatatypeProperty, owl:FunctionalProperty ;
  rdfs:label "b"@en ;
  rdfs:domain cim:TapChangerTablePoint ;
  rdfs:range cim:PerCent ;
  skos:definition """
The magnetizing branch susceptance deviation as a percentage of nominal value. The actual susceptance is calculated as follows:
calculated magnetizing susceptance = b(nominal) * (1 + b(from this class)/100).   The b(nominal) is defined as the static magnetizing susceptance on the associated power transformer end or ends.  This model assumes the star impedance (pi model) form.
\t"""@en .

cim:TapChangerTablePoint.g a owl:DatatypeProperty, owl:FunctionalProperty ;
  rdfs:label "g"@en ;
  rdfs:domain cim:TapChangerTablePoint ;
  rdfs:range cim:PerCent ;
  skos:definition """
The magnetizing branch conductance deviation as a percentage of nominal value. The actual conductance is calculated as follows:
calculated magnetizing conductance = g(nominal) * (1 + g(from this class)/100).   The g(nominal) is defined as the static magnetizing conductance on the associated power transformer end or ends.  This model assumes the star impedance (pi model) form.
\t"""@en .

cim:TapChangerTablePoint.r a owl:DatatypeProperty, owl:FunctionalProperty ;
  rdfs:label "r"@en ;
  rdfs:domain cim:TapChangerTablePoint ;
  rdfs:range cim:PerCent ;
  skos:definition """
The resistance deviation as a percentage of nominal value. The actual reactance is calculated as follows:
calculated resistance = r(nominal) * (1 + r(from this class)/100).   The r(nominal) is defined as the static resistance on the associated power transformer end or ends.  This model assumes the star impedance (pi model) form.
\t"""@en .

cim:TapChangerTablePoint.ratio a owl:DatatypeProperty, owl:FunctionalProperty ;
  rdfs:label "ratio"@en ;
  rdfs:domain cim:TapChangerTablePoint ;
  rdfs:range xsd:float ;
  skos:definition """
The voltage at the tap step divided by rated voltage of the transformer end having the tap changer. Hence this is a value close to one.
For example, if the ratio at step 1 is 1.01, and the rated voltage of the transformer end is 110kV, then the voltage obtained by setting the tap changer to step 1 to is 111.1kV.

\t"""@en .

cim:TapChangerTablePoint.step a owl:DatatypeProperty ;
  rdfs:label "step"@en ;
  rdfs:domain cim:TapChangerTablePoint ;
  rdfs:range xsd:integer ;
  skos:definition """
The tap step.

\t"""@en .

cim:TapChangerTablePoint.x a owl:DatatypeProperty, owl:FunctionalProperty ;
  rdfs:label "x"@en ;
  rdfs:domain cim:TapChangerTablePoint ;
  rdfs:range cim:PerCent ;
  skos:definition """
The series reactance deviation as a percentage of nominal value. The actual reactance is calculated as follows:
calculated reactance = x(nominal) * (1 + x(from this class)/100).   The x(nominal) is defined as the static series reactance on the associated power transformer end or ends.  This model assumes the star impedance (pi model) form.
\t"""@en .

cim:Terminal.phases a owl:DatatypeProperty, owl:FunctionalProperty ;
  rdfs:label "phases"@en ;
  rdfs:domain cim:Terminal ;
  rdfs:range cim:PhaseCode ;
  skos:definition """
Represents the normal network phasing condition. If the attribute is missing, three phases (ABC) shall be assumed, except for terminals of grounding classes (specializations of EarthFaultCompensator, GroundDisconnector, and Ground) which will be assumed to be N. Therefore, phase code ABCN is explicitly declared when needed, e.g. for star point grounding equipment.
The phase code on terminals connecting same ConnectivityNode or same TopologicalNode as well as for equipment between two terminals shall be consistent.
\t"""@en .

cim:TieFlow.positiveFlowIn a owl:DatatypeProperty ;
  rdfs:label "positiveFlowIn"@en ;
  rdfs:domain cim:TieFlow ;
  rdfs:range xsd:boolean ;
  skos:definition "Specifies the sign of the tie flow associated with a control area. True if positive flow into the terminal (load convention) is also positive flow into the control area.  See the description of ControlArea for further explanation of how TieFlow.positiveFlowIn is used."@en .

cim:TransformerEnd.endNumber a owl:DatatypeProperty ;
  rdfs:label "endNumber"@en ;
  rdfs:domain cim:TransformerEnd ;
  rdfs:range xsd:integer ;
  skos:definition """
Number for this transformer end, corresponding to the end's order in the power transformer vector group or phase angle clock number.  Highest voltage winding should be 1.  Each end within a power transformer should have a unique subsequent end number.   Note the transformer end number need not match the terminal sequence number.

\t"""@en .

cim:Voltage.multiplier a owl:DatatypeProperty, owl:FunctionalProperty ;
  rdfs:label "multiplier"@en ;
  eq:isFixed "True " ;
  rdf:value "k" ;
  rdfs:domain cim:Voltage ;
  rdfs:range cim:UnitMultiplier .

cim:Voltage.unit a owl:DatatypeProperty, owl:FunctionalProperty ;
  rdfs:label "unit"@en ;
  eq:isFixed "True " ;
  rdf:value "V" ;
  rdfs:domain cim:Voltage ;
  rdfs:range cim:UnitSymbol .

cim:Voltage.value a owl:DatatypeProperty, owl:FunctionalProperty ;
  rdfs:label "value"@en ;
  rdfs:domain cim:Voltage ;
  rdfs:range xsd:float .

cim:VoltageLevel.highVoltageLimit a owl:DatatypeProperty, owl:FunctionalProperty ;
  rdfs:label "highVoltageLimit"@en ;
  rdfs:domain cim:VoltageLevel ;
  rdfs:range cim:Voltage ;
  skos:definition """
The bus bar's high voltage limit.
The limit applies to all equipment and nodes contained in a given VoltageLevel. It is not required that it is exchanged in pair with lowVoltageLimit. It is preferable to use operational VoltageLimit, which prevails, if present.
\t"""@en .

cim:VoltageLevel.lowVoltageLimit a owl:DatatypeProperty, owl:FunctionalProperty ;
  rdfs:label "lowVoltageLimit"@en ;
  rdfs:domain cim:VoltageLevel ;
  rdfs:range cim:Voltage ;
  skos:definition """
The bus bar's low voltage limit.
The limit applies to all equipment and nodes contained in a given VoltageLevel. It is not required that it is exchanged in pair with highVoltageLimit. It is preferable to use operational VoltageLimit, which prevails, if present.
\t"""@en .

cim:VoltageLimit.normalValue a owl:DatatypeProperty ;
  rdfs:label "normalValue"@en ;
  rdfs:domain cim:VoltageLimit ;
  rdfs:range cim:Voltage ;
  skos:definition "The normal limit on voltage. High or low limit nature of the limit depends upon the properties of the operational limit type. The attribute shall be a positive value or zero."@en .

cim:VoltagePerReactivePower.multiplier a owl:DatatypeProperty, owl:FunctionalProperty ;
  rdfs:label "multiplier"@en ;
  eq:isFixed "True " ;
  rdf:value "none" ;
  rdfs:domain cim:VoltagePerReactivePower ;
  rdfs:range cim:UnitMultiplier .

cim:VoltagePerReactivePower.unit a owl:DatatypeProperty, owl:FunctionalProperty ;
  rdfs:label "unit"@en ;
  eq:isFixed "True " ;
  rdf:value "VPerVAr" ;
  rdfs:domain cim:VoltagePerReactivePower ;
  rdfs:range cim:UnitSymbol .

cim:VoltagePerReactivePower.value a owl:DatatypeProperty, owl:FunctionalProperty ;
  rdfs:label "value"@en ;
  rdfs:domain cim:VoltagePerReactivePower ;
  rdfs:range xsd:float .

cim:VsConverter.maxModulationIndex a owl:DatatypeProperty, owl:FunctionalProperty ;
  rdfs:label "maxModulationIndex"@en ;
  rdfs:domain cim:VsConverter ;
  rdfs:range xsd:float ;
  skos:definition "The maximum quotient between the AC converter voltage (Uc) and DC voltage (Ud). A factor typically less than 1. It is converter’s configuration data used in power flow."@en .

cim:WindGeneratingUnit.windGenUnitType a owl:DatatypeProperty ;
  rdfs:label "windGenUnitType"@en ;
  rdfs:domain cim:WindGeneratingUnit ;
  rdfs:range cim:WindGenUnitKind ;
  skos:definition "The kind of wind generating unit."@en .

eu:BoundaryPoint.fromEndIsoCode a owl:DatatypeProperty ;
  rdfs:label "fromEndIsoCode"@en ;
  eq:isEuropean "True" ;
  rdfs:domain eu:BoundaryPoint ;
  rdfs:range xsd:string ;
  skos:definition """
The ISO code of the region which the "From" side of the Boundary point belongs to or it is connected to.
The ISO code is a two-character country code as defined by ISO 3166 (http://www.iso.org/iso/country_codes). The length of the string is 2 characters maximum.
\t"""@en .

eu:BoundaryPoint.fromEndName a owl:DatatypeProperty ;
  rdfs:label "fromEndName"@en ;
  eq:isEuropean "True" ;
  rdfs:domain eu:BoundaryPoint ;
  rdfs:range xsd:string ;
  skos:definition """
A human readable name with length of the string 64 characters maximum. It covers the following two cases:
-if the Boundary point is placed on a tie-line, it is the name (IdentifiedObject.name) of the substation at which the "From" side of the tie-line is connected to.
-if the Boundary point is placed in a substation, it is the name (IdentifiedObject.name) of the element (e.g. PowerTransformer, ACLineSegment, Switch, etc.) at which the "From" side of the Boundary point is connected to.
\t"""@en .

eu:BoundaryPoint.fromEndNameTso a owl:DatatypeProperty ;
  rdfs:label "fromEndNameTso"@en ;
  eq:isEuropean "True" ;
  rdfs:domain eu:BoundaryPoint ;
  rdfs:range xsd:string ;
  skos:definition "Identifies the name of the transmission system operator, distribution system operator or other entity at which the \"From\" side of the interconnection is connected to. The length of the string is 64 characters maximum."@en .

eu:BoundaryPoint.isDirectCurrent a owl:DatatypeProperty, owl:FunctionalProperty ;
  rdfs:label "isDirectCurrent"@en ;
  eq:isEuropean "True" ;
  rdfs:domain eu:BoundaryPoint ;
  rdfs:range xsd:boolean ;
  skos:definition "If true, this boundary point is a point of common coupling (PCC) of a direct current (DC) interconnection, otherwise the interconnection is AC (default)."@en .

eu:BoundaryPoint.isExcludedFromAreaInterchange a owl:DatatypeProperty, owl:FunctionalProperty ;
  rdfs:label "isExcludedFromAreaInterchange"@en ;
  eq:isEuropean "True" ;
  rdfs:domain eu:BoundaryPoint ;
  rdfs:range xsd:boolean ;
  skos:definition "If true, this boundary point is on the interconnection that is excluded from control area interchange calculation and consequently has no related tie flows. Otherwise, the interconnection is included in control area interchange and a TieFlow is required at all sides of the boundary point (default)."@en .

eu:BoundaryPoint.toEndIsoCode a owl:DatatypeProperty ;
  rdfs:label "toEndIsoCode"@en ;
  eq:isEuropean "True" ;
  rdfs:domain eu:BoundaryPoint ;
  rdfs:range xsd:string ;
  skos:definition """
The ISO code of the region which the "To" side of the Boundary point belongs to or is connected to.
The ISO code is a two-character country code as defined by ISO 3166 (http://www.iso.org/iso/country_codes). The length of the string is 2 characters maximum.
\t"""@en .

eu:BoundaryPoint.toEndName a owl:DatatypeProperty ;
  rdfs:label "toEndName"@en ;
  eq:isEuropean "True" ;
  rdfs:domain eu:BoundaryPoint ;
  rdfs:range xsd:string ;
  skos:definition """
A human readable name with length of the string 64 characters maximum. It covers the following two cases:
-if the Boundary point is placed on a tie-line, it is the name (IdentifiedObject.name) of the substation at which the "To" side of the tie-line is connected to.
-if the Boundary point is placed in a substation, it is the name (IdentifiedObject.name) of the element (e.g. PowerTransformer, ACLineSegment, Switch, etc.) at which the "To" side of the Boundary point is connected to.
\t"""@en .

eu:BoundaryPoint.toEndNameTso a owl:DatatypeProperty ;
  rdfs:label "toEndNameTso"@en ;
  eq:isEuropean "True" ;
  rdfs:domain eu:BoundaryPoint ;
  rdfs:range xsd:string ;
  skos:definition "Identifies the name of the transmission system operator, distribution system operator or other entity at which the \"To\" side of the interconnection is connected to. The length of the string is 64 characters maximum."@en .

eu:IdentifiedObject.energyIdentCodeEic a owl:DatatypeProperty, owl:FunctionalProperty ;
  rdfs:label "energyIdentCodeEic"@en ;
  eq:isEuropean "True" ;
  eq:isdeprecated "True" ;
  rdfs:domain eu:IdentifiedObject ;
  rdfs:range xsd:string ;
  skos:definition "The attribute is used for an exchange of the EIC code (Energy identification Code). The length of the string is 16 characters as defined by the EIC code. For details on EIC scheme please refer to ENTSO-E web site."@en .

eu:IdentifiedObject.shortName a owl:DatatypeProperty, owl:FunctionalProperty ;
  rdfs:label "shortName"@en ;
  eq:isEuropean "True" ;
  eq:isdeprecated "True" ;
  rdfs:domain eu:IdentifiedObject ;
  rdfs:range xsd:string ;
  skos:definition "The attribute is used for an exchange of a human readable short name with length of the string 12 characters maximum."@en .

eu:OperationalLimitType.kind a owl:DatatypeProperty ;
  rdfs:label "kind"@en ;
  eq:isEuropean "True" ;
  rdfs:domain eu:OperationalLimitType ;
  rdfs:range eu:LimitKind ;
  skos:definition "Types of limits defined in the ENTSO-E Operational Handbook Policy 3."@en .

eq:Package a owl:AnnotationProperty ;
  rdfs:label "MOF Package"@en ;
  rdfs:comment "Declaration that this is a MOF Package."@en ;
  rdfs:domain rdfs:Class ;
  rdfs:range xsd:string .

eq:isAbstract a owl:AnnotationProperty ;
  rdfs:label "is abstract"@en ;
  rdfs:comment "Flag indicating whether the class is permitted to have any direct instances."@en ;
  rdfs:domain rdfs:Class ;
  rdfs:range xsd:boolean .

eq:isCIMDatatype a owl:AnnotationProperty ;
  rdfs:label "isCIMDatatype\t"@en ;
  rdfs:comment "Flag indicating whether the class is a CIMDatatype."@en ;
  rdfs:domain rdfs:Class ;
  rdfs:range xsd:boolean .

eq:isConst a owl:AnnotationProperty ;
  rdfs:label "is fixed property"@en ;
  rdfs:comment " Flag indicating whether the property for a specific object can be updated."@en ;
  rdfs:domain rdfs:Property ;
  rdfs:range xsd:boolean .

eq:isEuropean a owl:AnnotationProperty ;
  rdfs:label "isEuropean\t"@en ;
  rdfs:comment "Flag indicating whether the class is a European."@en ;
  rdfs:domain rdfs:Class, rdfs:Property ;
  rdfs:range xsd:boolean .

eq:isFixed a owl:AnnotationProperty ;
  rdfs:label "is fixed property"@en ;
  rdfs:comment " Flag indicating whether the property for a specific object can be updated."@en ;
  rdfs:domain rdfs:Property ;
  rdfs:range xsd:boolean .

eq:isPrimitive a owl:AnnotationProperty ;
  rdfs:label "isPrimitive\t"@en ;
  rdfs:comment "Flag indicating whether the class is a Primitive."@en ;
  rdfs:domain rdfs:Class ;
  rdfs:range xsd:boolean .

eq:isUnique a owl:AnnotationProperty ;
  rdfs:label "is unique "@en ;
  rdfs:comment " Flag indicating whether the property for a specific object can contain the same value more than once."@en ;
  rdfs:domain rdfs:Property ;
  rdfs:range xsd:boolean .

eq:isdeprecated a owl:AnnotationProperty ;
  rdfs:label "isdeprecated\t"@en ;
  rdfs:comment "Flag indicating whether the class is a deprecated."@en ;
  rdfs:domain rdfs:Class, rdfs:Property ;
  rdfs:range xsd:boolean .

eq:isenum a owl:AnnotationProperty ;
  rdfs:label "isenum\t"@en ;
  rdfs:comment "Flag indicating whether the enumerated literal is an enum."@en ;
  rdfs:domain rdfs:Property ;
  rdfs:range xsd:boolean .

cim:ControlAreaTypeKind.AGC a owl:NamedIndividual, owl:Thing ;
  rdfs:label "AGC "@en ;
  eq:isenum "True" ;
  rdfs:domain cim:ControlAreaTypeKind ;
  skos:definition "Used for automatic generation control."@en .

cim:ControlAreaTypeKind.Forecast a owl:NamedIndividual, owl:Thing ;
  rdfs:label "Forecast "@en ;
  eq:isenum "True" ;
  rdfs:domain cim:ControlAreaTypeKind ;
  skos:definition "Used for load forecast."@en .

cim:ControlAreaTypeKind.Interchange a owl:NamedIndividual, owl:Thing ;
  rdfs:label "Interchange "@en ;
  eq:isenum "True" ;
  rdfs:domain cim:ControlAreaTypeKind ;
  skos:definition "Used for interchange specification or control."@en .

cim:Currency.AED a owl:NamedIndividual, owl:Thing ;
  rdfs:label "AED "@en ;
  eq:isenum "True" ;
  rdfs:domain cim:Currency ;
  skos:definition "United Arab Emirates dirham."@en .

cim:Currency.AFN a owl:NamedIndividual, owl:Thing ;
  rdfs:label "AFN "@en ;
  eq:isenum "True" ;
  rdfs:domain cim:Currency ;
  skos:definition "Afghan afghani."@en .

cim:Currency.ALL a owl:NamedIndividual, owl:Thing ;
  rdfs:label "ALL "@en ;
  eq:isenum "True" ;
  rdfs:domain cim:Currency ;
  skos:definition "Albanian lek."@en .

cim:Currency.AMD a owl:NamedIndividual, owl:Thing ;
  rdfs:label "AMD "@en ;
  eq:isenum "True" ;
  rdfs:domain cim:Currency ;
  skos:definition "Armenian dram."@en .

cim:Currency.ANG a owl:NamedIndividual, owl:Thing ;
  rdfs:label "ANG "@en ;
  eq:isenum "True" ;
  rdfs:domain cim:Currency ;
  skos:definition "Netherlands Antillean guilder."@en .

cim:Currency.AOA a owl:NamedIndividual, owl:Thing ;
  rdfs:label "AOA "@en ;
  eq:isenum "True" ;
  rdfs:domain cim:Currency ;
  skos:definition "Angolan kwanza."@en .

cim:Currency.ARS a owl:NamedIndividual, owl:Thing ;
  rdfs:label "ARS "@en ;
  eq:isenum "True" ;
  rdfs:domain cim:Currency ;
  skos:definition "Argentine peso."@en .

cim:Currency.AUD a owl:NamedIndividual, owl:Thing ;
  rdfs:label "AUD "@en ;
  eq:isenum "True" ;
  rdfs:domain cim:Currency ;
  skos:definition "Australian dollar."@en .

cim:Currency.AWG a owl:NamedIndividual, owl:Thing ;
  rdfs:label "AWG "@en ;
  eq:isenum "True" ;
  rdfs:domain cim:Currency ;
  skos:definition "Aruban florin."@en .

cim:Currency.AZN a owl:NamedIndividual, owl:Thing ;
  rdfs:label "AZN "@en ;
  eq:isenum "True" ;
  rdfs:domain cim:Currency ;
  skos:definition "Azerbaijani manat."@en .

cim:Currency.BAM a owl:NamedIndividual, owl:Thing ;
  rdfs:label "BAM "@en ;
  eq:isenum "True" ;
  rdfs:domain cim:Currency ;
  skos:definition "Bosnia and Herzegovina convertible mark."@en .

cim:Currency.BBD a owl:NamedIndividual, owl:Thing ;
  rdfs:label "BBD "@en ;
  eq:isenum "True" ;
  rdfs:domain cim:Currency ;
  skos:definition "Barbados dollar."@en .

cim:Currency.BDT a owl:NamedIndividual, owl:Thing ;
  rdfs:label "BDT "@en ;
  eq:isenum "True" ;
  rdfs:domain cim:Currency ;
  skos:definition "Bangladeshi taka."@en .

cim:Currency.BGN a owl:NamedIndividual, owl:Thing ;
  rdfs:label "BGN "@en ;
  eq:isenum "True" ;
  rdfs:domain cim:Currency ;
  skos:definition "Bulgarian lev."@en .

cim:Currency.BHD a owl:NamedIndividual, owl:Thing ;
  rdfs:label "BHD "@en ;
  eq:isenum "True" ;
  rdfs:domain cim:Currency ;
  skos:definition "Bahraini dinar."@en .

cim:Currency.BIF a owl:NamedIndividual, owl:Thing ;
  rdfs:label "BIF "@en ;
  eq:isenum "True" ;
  rdfs:domain cim:Currency ;
  skos:definition "Burundian franc."@en .

cim:Currency.BMD a owl:NamedIndividual, owl:Thing ;
  rdfs:label "BMD "@en ;
  eq:isenum "True" ;
  rdfs:domain cim:Currency ;
  skos:definition "Bermudian dollar (customarily known as Bermuda dollar)."@en .

cim:Currency.BND a owl:NamedIndividual, owl:Thing ;
  rdfs:label "BND "@en ;
  eq:isenum "True" ;
  rdfs:domain cim:Currency ;
  skos:definition "Brunei dollar."@en .

cim:Currency.BOB a owl:NamedIndividual, owl:Thing ;
  rdfs:label "BOB "@en ;
  eq:isenum "True" ;
  rdfs:domain cim:Currency ;
  skos:definition "Boliviano."@en .

cim:Currency.BOV a owl:NamedIndividual, owl:Thing ;
  rdfs:label "BOV "@en ;
  eq:isenum "True" ;
  rdfs:domain cim:Currency ;
  skos:definition "Bolivian Mvdol (funds code)."@en .

cim:Currency.BRL a owl:NamedIndividual, owl:Thing ;
  rdfs:label "BRL "@en ;
  eq:isenum "True" ;
  rdfs:domain cim:Currency ;
  skos:definition "Brazilian real."@en .

cim:Currency.BSD a owl:NamedIndividual, owl:Thing ;
  rdfs:label "BSD "@en ;
  eq:isenum "True" ;
  rdfs:domain cim:Currency ;
  skos:definition "Bahamian dollar."@en .

cim:Currency.BTN a owl:NamedIndividual, owl:Thing ;
  rdfs:label "BTN "@en ;
  eq:isenum "True" ;
  rdfs:domain cim:Currency ;
  skos:definition "Bhutanese ngultrum."@en .

cim:Currency.BWP a owl:NamedIndividual, owl:Thing ;
  rdfs:label "BWP "@en ;
  eq:isenum "True" ;
  rdfs:domain cim:Currency ;
  skos:definition "Botswana pula."@en .

cim:Currency.BYR a owl:NamedIndividual, owl:Thing ;
  rdfs:label "BYR "@en ;
  eq:isenum "True" ;
  rdfs:domain cim:Currency ;
  skos:definition "Belarusian ruble."@en .

cim:Currency.BZD a owl:NamedIndividual, owl:Thing ;
  rdfs:label "BZD "@en ;
  eq:isenum "True" ;
  rdfs:domain cim:Currency ;
  skos:definition "Belize dollar."@en .

cim:Currency.CAD a owl:NamedIndividual, owl:Thing ;
  rdfs:label "CAD "@en ;
  eq:isenum "True" ;
  rdfs:domain cim:Currency ;
  skos:definition """
Canadian dollar.

\t"""@en .

cim:Currency.CDF a owl:NamedIndividual, owl:Thing ;
  rdfs:label "CDF "@en ;
  eq:isenum "True" ;
  rdfs:domain cim:Currency ;
  skos:definition "Congolese franc."@en .

cim:Currency.CHF a owl:NamedIndividual, owl:Thing ;
  rdfs:label "CHF "@en ;
  eq:isenum "True" ;
  rdfs:domain cim:Currency ;
  skos:definition "Swiss franc."@en .

cim:Currency.CLF a owl:NamedIndividual, owl:Thing ;
  rdfs:label "CLF "@en ;
  eq:isenum "True" ;
  rdfs:domain cim:Currency ;
  skos:definition "Unidad de Fomento (funds code), Chile."@en .

cim:Currency.CLP a owl:NamedIndividual, owl:Thing ;
  rdfs:label "CLP "@en ;
  eq:isenum "True" ;
  rdfs:domain cim:Currency ;
  skos:definition "Chilean peso."@en .

cim:Currency.CNY a owl:NamedIndividual, owl:Thing ;
  rdfs:label "CNY "@en ;
  eq:isenum "True" ;
  rdfs:domain cim:Currency ;
  skos:definition "Chinese yuan."@en .

cim:Currency.COP a owl:NamedIndividual, owl:Thing ;
  rdfs:label "COP "@en ;
  eq:isenum "True" ;
  rdfs:domain cim:Currency ;
  skos:definition "Colombian peso."@en .

cim:Currency.COU a owl:NamedIndividual, owl:Thing ;
  rdfs:label "COU "@en ;
  eq:isenum "True" ;
  rdfs:domain cim:Currency ;
  skos:definition "Unidad de Valor Real."@en .

cim:Currency.CRC a owl:NamedIndividual, owl:Thing ;
  rdfs:label "CRC "@en ;
  eq:isenum "True" ;
  rdfs:domain cim:Currency ;
  skos:definition "Costa Rican colon."@en .

cim:Currency.CUC a owl:NamedIndividual, owl:Thing ;
  rdfs:label "CUC "@en ;
  eq:isenum "True" ;
  rdfs:domain cim:Currency ;
  skos:definition "Cuban convertible peso."@en .

cim:Currency.CUP a owl:NamedIndividual, owl:Thing ;
  rdfs:label "CUP "@en ;
  eq:isenum "True" ;
  rdfs:domain cim:Currency ;
  skos:definition "Cuban peso."@en .

cim:Currency.CVE a owl:NamedIndividual, owl:Thing ;
  rdfs:label "CVE "@en ;
  eq:isenum "True" ;
  rdfs:domain cim:Currency ;
  skos:definition "Cape Verde escudo."@en .

cim:Currency.CZK a owl:NamedIndividual, owl:Thing ;
  rdfs:label "CZK "@en ;
  eq:isenum "True" ;
  rdfs:domain cim:Currency ;
  skos:definition "Czech koruna."@en .

cim:Currency.DJF a owl:NamedIndividual, owl:Thing ;
  rdfs:label "DJF "@en ;
  eq:isenum "True" ;
  rdfs:domain cim:Currency ;
  skos:definition "Djiboutian franc."@en .

cim:Currency.DKK a owl:NamedIndividual, owl:Thing ;
  rdfs:label "DKK "@en ;
  eq:isenum "True" ;
  rdfs:domain cim:Currency ;
  skos:definition "Danish krone."@en .

cim:Currency.DOP a owl:NamedIndividual, owl:Thing ;
  rdfs:label "DOP "@en ;
  eq:isenum "True" ;
  rdfs:domain cim:Currency ;
  skos:definition "Dominican peso."@en .

cim:Currency.DZD a owl:NamedIndividual, owl:Thing ;
  rdfs:label "DZD "@en ;
  eq:isenum "True" ;
  rdfs:domain cim:Currency ;
  skos:definition "Algerian dinar."@en .

cim:Currency.EEK a owl:NamedIndividual, owl:Thing ;
  rdfs:label "EEK "@en ;
  eq:isenum "True" ;
  rdfs:domain cim:Currency ;
  skos:definition "Estonian kroon."@en .

cim:Currency.EGP a owl:NamedIndividual, owl:Thing ;
  rdfs:label "EGP "@en ;
  eq:isenum "True" ;
  rdfs:domain cim:Currency ;
  skos:definition "Egyptian pound."@en .

cim:Currency.ERN a owl:NamedIndividual, owl:Thing ;
  rdfs:label "ERN "@en ;
  eq:isenum "True" ;
  rdfs:domain cim:Currency ;
  skos:definition "Eritrean nakfa."@en .

cim:Currency.ETB a owl:NamedIndividual, owl:Thing ;
  rdfs:label "ETB "@en ;
  eq:isenum "True" ;
  rdfs:domain cim:Currency ;
  skos:definition "Ethiopian birr."@en .

cim:Currency.EUR a owl:NamedIndividual, owl:Thing ;
  rdfs:label "EUR "@en ;
  eq:isenum "True" ;
  rdfs:domain cim:Currency ;
  skos:definition "Euro."@en .

cim:Currency.FJD a owl:NamedIndividual, owl:Thing ;
  rdfs:label "FJD "@en ;
  eq:isenum "True" ;
  rdfs:domain cim:Currency ;
  skos:definition "Fiji dollar."@en .

cim:Currency.FKP a owl:NamedIndividual, owl:Thing ;
  rdfs:label "FKP "@en ;
  eq:isenum "True" ;
  rdfs:domain cim:Currency ;
  skos:definition "Falkland Islands pound."@en .

cim:Currency.GBP a owl:NamedIndividual, owl:Thing ;
  rdfs:label "GBP "@en ;
  eq:isenum "True" ;
  rdfs:domain cim:Currency ;
  skos:definition "Pound sterling."@en .

cim:Currency.GEL a owl:NamedIndividual, owl:Thing ;
  rdfs:label "GEL "@en ;
  eq:isenum "True" ;
  rdfs:domain cim:Currency ;
  skos:definition "Georgian lari."@en .

cim:Currency.GHS a owl:NamedIndividual, owl:Thing ;
  rdfs:label "GHS "@en ;
  eq:isenum "True" ;
  rdfs:domain cim:Currency ;
  skos:definition "Ghanaian cedi."@en .

cim:Currency.GIP a owl:NamedIndividual, owl:Thing ;
  rdfs:label "GIP "@en ;
  eq:isenum "True" ;
  rdfs:domain cim:Currency ;
  skos:definition "Gibraltar pound."@en .

cim:Currency.GMD a owl:NamedIndividual, owl:Thing ;
  rdfs:label "GMD "@en ;
  eq:isenum "True" ;
  rdfs:domain cim:Currency ;
  skos:definition "Gambian dalasi."@en .

cim:Currency.GNF a owl:NamedIndividual, owl:Thing ;
  rdfs:label "GNF "@en ;
  eq:isenum "True" ;
  rdfs:domain cim:Currency ;
  skos:definition "Guinean franc."@en .

cim:Currency.GTQ a owl:NamedIndividual, owl:Thing ;
  rdfs:label "GTQ "@en ;
  eq:isenum "True" ;
  rdfs:domain cim:Currency ;
  skos:definition "Guatemalan quetzal."@en .

cim:Currency.GYD a owl:NamedIndividual, owl:Thing ;
  rdfs:label "GYD "@en ;
  eq:isenum "True" ;
  rdfs:domain cim:Currency ;
  skos:definition "Guyanese dollar."@en .

cim:Currency.HKD a owl:NamedIndividual, owl:Thing ;
  rdfs:label "HKD "@en ;
  eq:isenum "True" ;
  rdfs:domain cim:Currency ;
  skos:definition "Hong Kong dollar."@en .

cim:Currency.HNL a owl:NamedIndividual, owl:Thing ;
  rdfs:label "HNL "@en ;
  eq:isenum "True" ;
  rdfs:domain cim:Currency ;
  skos:definition "Honduran lempira."@en .

cim:Currency.HRK a owl:NamedIndividual, owl:Thing ;
  rdfs:label "HRK "@en ;
  eq:isenum "True" ;
  rdfs:domain cim:Currency ;
  skos:definition "Croatian kuna."@en .

cim:Currency.HTG a owl:NamedIndividual, owl:Thing ;
  rdfs:label "HTG "@en ;
  eq:isenum "True" ;
  rdfs:domain cim:Currency ;
  skos:definition "Haitian gourde."@en .

cim:Currency.HUF a owl:NamedIndividual, owl:Thing ;
  rdfs:label "HUF "@en ;
  eq:isenum "True" ;
  rdfs:domain cim:Currency ;
  skos:definition "Hungarian forint."@en .

cim:Currency.IDR a owl:NamedIndividual, owl:Thing ;
  rdfs:label "IDR "@en ;
  eq:isenum "True" ;
  rdfs:domain cim:Currency ;
  skos:definition "Indonesian rupiah."@en .

cim:Currency.ILS a owl:NamedIndividual, owl:Thing ;
  rdfs:label "ILS "@en ;
  eq:isenum "True" ;
  rdfs:domain cim:Currency ;
  skos:definition "Israeli new sheqel."@en .

cim:Currency.INR a owl:NamedIndividual, owl:Thing ;
  rdfs:label "INR "@en ;
  eq:isenum "True" ;
  rdfs:domain cim:Currency ;
  skos:definition "Indian rupee."@en .

cim:Currency.IQD a owl:NamedIndividual, owl:Thing ;
  rdfs:label "IQD "@en ;
  eq:isenum "True" ;
  rdfs:domain cim:Currency ;
  skos:definition "Iraqi dinar."@en .

cim:Currency.IRR a owl:NamedIndividual, owl:Thing ;
  rdfs:label "IRR "@en ;
  eq:isenum "True" ;
  rdfs:domain cim:Currency ;
  skos:definition "Iranian rial."@en .

cim:Currency.ISK a owl:NamedIndividual, owl:Thing ;
  rdfs:label "ISK "@en ;
  eq:isenum "True" ;
  rdfs:domain cim:Currency ;
  skos:definition "Icelandic króna."@en .

cim:Currency.JMD a owl:NamedIndividual, owl:Thing ;
  rdfs:label "JMD "@en ;
  eq:isenum "True" ;
  rdfs:domain cim:Currency ;
  skos:definition "Jamaican dollar."@en .

cim:Currency.JOD a owl:NamedIndividual, owl:Thing ;
  rdfs:label "JOD "@en ;
  eq:isenum "True" ;
  rdfs:domain cim:Currency ;
  skos:definition "Jordanian dinar."@en .

cim:Currency.JPY a owl:NamedIndividual, owl:Thing ;
  rdfs:label "JPY "@en ;
  eq:isenum "True" ;
  rdfs:domain cim:Currency ;
  skos:definition "Japanese yen."@en .

cim:Currency.KES a owl:NamedIndividual, owl:Thing ;
  rdfs:label "KES "@en ;
  eq:isenum "True" ;
  rdfs:domain cim:Currency ;
  skos:definition "Kenyan shilling."@en .

cim:Currency.KGS a owl:NamedIndividual, owl:Thing ;
  rdfs:label "KGS "@en ;
  eq:isenum "True" ;
  rdfs:domain cim:Currency ;
  skos:definition "Kyrgyzstani som."@en .

cim:Currency.KHR a owl:NamedIndividual, owl:Thing ;
  rdfs:label "KHR "@en ;
  eq:isenum "True" ;
  rdfs:domain cim:Currency ;
  skos:definition "Cambodian riel."@en .

cim:Currency.KMF a owl:NamedIndividual, owl:Thing ;
  rdfs:label "KMF "@en ;
  eq:isenum "True" ;
  rdfs:domain cim:Currency ;
  skos:definition "Comoro franc."@en .

cim:Currency.KPW a owl:NamedIndividual, owl:Thing ;
  rdfs:label "KPW "@en ;
  eq:isenum "True" ;
  rdfs:domain cim:Currency ;
  skos:definition "North Korean won."@en .

cim:Currency.KRW a owl:NamedIndividual, owl:Thing ;
  rdfs:label "KRW "@en ;
  eq:isenum "True" ;
  rdfs:domain cim:Currency ;
  skos:definition "South Korean won."@en .

cim:Currency.KWD a owl:NamedIndividual, owl:Thing ;
  rdfs:label "KWD "@en ;
  eq:isenum "True" ;
  rdfs:domain cim:Currency ;
  skos:definition "Kuwaiti dinar."@en .

cim:Currency.KYD a owl:NamedIndividual, owl:Thing ;
  rdfs:label "KYD "@en ;
  eq:isenum "True" ;
  rdfs:domain cim:Currency ;
  skos:definition "Cayman Islands dollar."@en .

cim:Currency.KZT a owl:NamedIndividual, owl:Thing ;
  rdfs:label "KZT "@en ;
  eq:isenum "True" ;
  rdfs:domain cim:Currency ;
  skos:definition "Kazakhstani tenge."@en .

cim:Currency.LAK a owl:NamedIndividual, owl:Thing ;
  rdfs:label "LAK "@en ;
  eq:isenum "True" ;
  rdfs:domain cim:Currency ;
  skos:definition "Lao kip."@en .

cim:Currency.LBP a owl:NamedIndividual, owl:Thing ;
  rdfs:label "LBP "@en ;
  eq:isenum "True" ;
  rdfs:domain cim:Currency ;
  skos:definition "Lebanese pound."@en .

cim:Currency.LKR a owl:NamedIndividual, owl:Thing ;
  rdfs:label "LKR "@en ;
  eq:isenum "True" ;
  rdfs:domain cim:Currency ;
  skos:definition "Sri Lanka rupee."@en .

cim:Currency.LRD a owl:NamedIndividual, owl:Thing ;
  rdfs:label "LRD "@en ;
  eq:isenum "True" ;
  rdfs:domain cim:Currency ;
  skos:definition "Liberian dollar."@en .

cim:Currency.LSL a owl:NamedIndividual, owl:Thing ;
  rdfs:label "LSL "@en ;
  eq:isenum "True" ;
  rdfs:domain cim:Currency ;
  skos:definition "Lesotho loti."@en .

cim:Currency.LTL a owl:NamedIndividual, owl:Thing ;
  rdfs:label "LTL "@en ;
  eq:isenum "True" ;
  rdfs:domain cim:Currency ;
  skos:definition "Lithuanian litas."@en .

cim:Currency.LVL a owl:NamedIndividual, owl:Thing ;
  rdfs:label "LVL "@en ;
  eq:isenum "True" ;
  rdfs:domain cim:Currency ;
  skos:definition "Latvian lats."@en .

cim:Currency.LYD a owl:NamedIndividual, owl:Thing ;
  rdfs:label "LYD "@en ;
  eq:isenum "True" ;
  rdfs:domain cim:Currency ;
  skos:definition "Libyan dinar."@en .

cim:Currency.MAD a owl:NamedIndividual, owl:Thing ;
  rdfs:label "MAD "@en ;
  eq:isenum "True" ;
  rdfs:domain cim:Currency ;
  skos:definition "Moroccan dirham."@en .

cim:Currency.MDL a owl:NamedIndividual, owl:Thing ;
  rdfs:label "MDL "@en ;
  eq:isenum "True" ;
  rdfs:domain cim:Currency ;
  skos:definition "Moldovan leu."@en .

cim:Currency.MGA a owl:NamedIndividual, owl:Thing ;
  rdfs:label "MGA "@en ;
  eq:isenum "True" ;
  rdfs:domain cim:Currency ;
  skos:definition "Malagasy ariary."@en .

cim:Currency.MKD a owl:NamedIndividual, owl:Thing ;
  rdfs:label "MKD "@en ;
  eq:isenum "True" ;
  rdfs:domain cim:Currency ;
  skos:definition "Macedonian denar."@en .

cim:Currency.MMK a owl:NamedIndividual, owl:Thing ;
  rdfs:label "MMK "@en ;
  eq:isenum "True" ;
  rdfs:domain cim:Currency ;
  skos:definition "Myanma kyat."@en .

cim:Currency.MNT a owl:NamedIndividual, owl:Thing ;
  rdfs:label "MNT "@en ;
  eq:isenum "True" ;
  rdfs:domain cim:Currency ;
  skos:definition "Mongolian tugrik."@en .

cim:Currency.MOP a owl:NamedIndividual, owl:Thing ;
  rdfs:label "MOP "@en ;
  eq:isenum "True" ;
  rdfs:domain cim:Currency ;
  skos:definition "Macanese pataca."@en .

cim:Currency.MRO a owl:NamedIndividual, owl:Thing ;
  rdfs:label "MRO "@en ;
  eq:isenum "True" ;
  rdfs:domain cim:Currency ;
  skos:definition "Mauritanian ouguiya."@en .

cim:Currency.MUR a owl:NamedIndividual, owl:Thing ;
  rdfs:label "MUR "@en ;
  eq:isenum "True" ;
  rdfs:domain cim:Currency ;
  skos:definition "Mauritian rupee."@en .

cim:Currency.MVR a owl:NamedIndividual, owl:Thing ;
  rdfs:label "MVR "@en ;
  eq:isenum "True" ;
  rdfs:domain cim:Currency ;
  skos:definition "Maldivian rufiyaa."@en .

cim:Currency.MWK a owl:NamedIndividual, owl:Thing ;
  rdfs:label "MWK "@en ;
  eq:isenum "True" ;
  rdfs:domain cim:Currency ;
  skos:definition "Malawian kwacha."@en .

cim:Currency.MXN a owl:NamedIndividual, owl:Thing ;
  rdfs:label "MXN "@en ;
  eq:isenum "True" ;
  rdfs:domain cim:Currency ;
  skos:definition "Mexican peso."@en .

cim:Currency.MYR a owl:NamedIndividual, owl:Thing ;
  rdfs:label "MYR "@en ;
  eq:isenum "True" ;
  rdfs:domain cim:Currency ;
  skos:definition "Malaysian ringgit."@en .

cim:Currency.MZN a owl:NamedIndividual, owl:Thing ;
  rdfs:label "MZN "@en ;
  eq:isenum "True" ;
  rdfs:domain cim:Currency ;
  skos:definition "Mozambican metical."@en .

cim:Currency.NAD a owl:NamedIndividual, owl:Thing ;
  rdfs:label "NAD "@en ;
  eq:isenum "True" ;
  rdfs:domain cim:Currency ;
  skos:definition "Namibian dollar."@en .

cim:Currency.NGN a owl:NamedIndividual, owl:Thing ;
  rdfs:label "NGN "@en ;
  eq:isenum "True" ;
  rdfs:domain cim:Currency ;
  skos:definition "Nigerian naira."@en .

cim:Currency.NIO a owl:NamedIndividual, owl:Thing ;
  rdfs:label "NIO "@en ;
  eq:isenum "True" ;
  rdfs:domain cim:Currency ;
  skos:definition "Cordoba oro."@en .

cim:Currency.NOK a owl:NamedIndividual, owl:Thing ;
  rdfs:label "NOK "@en ;
  eq:isenum "True" ;
  rdfs:domain cim:Currency ;
  skos:definition "Norwegian krone."@en .

cim:Currency.NPR a owl:NamedIndividual, owl:Thing ;
  rdfs:label "NPR "@en ;
  eq:isenum "True" ;
  rdfs:domain cim:Currency ;
  skos:definition "Nepalese rupee."@en .

cim:Currency.NZD a owl:NamedIndividual, owl:Thing ;
  rdfs:label "NZD "@en ;
  eq:isenum "True" ;
  rdfs:domain cim:Currency ;
  skos:definition "New Zealand dollar."@en .

cim:Currency.OMR a owl:NamedIndividual, owl:Thing ;
  rdfs:label "OMR "@en ;
  eq:isenum "True" ;
  rdfs:domain cim:Currency ;
  skos:definition "Omani rial."@en .

cim:Currency.PAB a owl:NamedIndividual, owl:Thing ;
  rdfs:label "PAB "@en ;
  eq:isenum "True" ;
  rdfs:domain cim:Currency ;
  skos:definition "Panamanian balboa."@en .

cim:Currency.PEN a owl:NamedIndividual, owl:Thing ;
  rdfs:label "PEN "@en ;
  eq:isenum "True" ;
  rdfs:domain cim:Currency ;
  skos:definition "Peruvian nuevo sol."@en .

cim:Currency.PGK a owl:NamedIndividual, owl:Thing ;
  rdfs:label "PGK "@en ;
  eq:isenum "True" ;
  rdfs:domain cim:Currency ;
  skos:definition "Papua New Guinean kina."@en .

cim:Currency.PHP a owl:NamedIndividual, owl:Thing ;
  rdfs:label "PHP "@en ;
  eq:isenum "True" ;
  rdfs:domain cim:Currency ;
  skos:definition "Philippine peso."@en .

cim:Currency.PKR a owl:NamedIndividual, owl:Thing ;
  rdfs:label "PKR "@en ;
  eq:isenum "True" ;
  rdfs:domain cim:Currency ;
  skos:definition "Pakistani rupee."@en .

cim:Currency.PLN a owl:NamedIndividual, owl:Thing ;
  rdfs:label "PLN "@en ;
  eq:isenum "True" ;
  rdfs:domain cim:Currency ;
  skos:definition "Polish zloty."@en .

cim:Currency.PYG a owl:NamedIndividual, owl:Thing ;
  rdfs:label "PYG "@en ;
  eq:isenum "True" ;
  rdfs:domain cim:Currency ;
  skos:definition "Paraguayan guaraní."@en .

cim:Currency.QAR a owl:NamedIndividual, owl:Thing ;
  rdfs:label "QAR "@en ;
  eq:isenum "True" ;
  rdfs:domain cim:Currency ;
  skos:definition "Qatari rial."@en .

cim:Currency.RON a owl:NamedIndividual, owl:Thing ;
  rdfs:label "RON "@en ;
  eq:isenum "True" ;
  rdfs:domain cim:Currency ;
  skos:definition "Romanian new leu."@en .

cim:Currency.RSD a owl:NamedIndividual, owl:Thing ;
  rdfs:label "RSD "@en ;
  eq:isenum "True" ;
  rdfs:domain cim:Currency ;
  skos:definition "Serbian dinar."@en .

cim:Currency.RUB a owl:NamedIndividual, owl:Thing ;
  rdfs:label "RUB "@en ;
  eq:isenum "True" ;
  rdfs:domain cim:Currency ;
  skos:definition "Russian rouble."@en .

cim:Currency.RWF a owl:NamedIndividual, owl:Thing ;
  rdfs:label "RWF "@en ;
  eq:isenum "True" ;
  rdfs:domain cim:Currency ;
  skos:definition "Rwandan franc."@en .

cim:Currency.SAR a owl:NamedIndividual, owl:Thing ;
  rdfs:label "SAR "@en ;
  eq:isenum "True" ;
  rdfs:domain cim:Currency ;
  skos:definition "Saudi riyal."@en .

cim:Currency.SBD a owl:NamedIndividual, owl:Thing ;
  rdfs:label "SBD "@en ;
  eq:isenum "True" ;
  rdfs:domain cim:Currency ;
  skos:definition "Solomon Islands dollar."@en .

cim:Currency.SCR a owl:NamedIndividual, owl:Thing ;
  rdfs:label "SCR "@en ;
  eq:isenum "True" ;
  rdfs:domain cim:Currency ;
  skos:definition "Seychelles rupee."@en .

cim:Currency.SDG a owl:NamedIndividual, owl:Thing ;
  rdfs:label "SDG "@en ;
  eq:isenum "True" ;
  rdfs:domain cim:Currency ;
  skos:definition "Sudanese pound."@en .

cim:Currency.SEK a owl:NamedIndividual, owl:Thing ;
  rdfs:label "SEK "@en ;
  eq:isenum "True" ;
  rdfs:domain cim:Currency ;
  skos:definition "Swedish krona/kronor."@en .

cim:Currency.SGD a owl:NamedIndividual, owl:Thing ;
  rdfs:label "SGD "@en ;
  eq:isenum "True" ;
  rdfs:domain cim:Currency ;
  skos:definition "Singapore dollar."@en .

cim:Currency.SHP a owl:NamedIndividual, owl:Thing ;
  rdfs:label "SHP "@en ;
  eq:isenum "True" ;
  rdfs:domain cim:Currency ;
  skos:definition "Saint Helena pound."@en .

cim:Currency.SLL a owl:NamedIndividual, owl:Thing ;
  rdfs:label "SLL "@en ;
  eq:isenum "True" ;
  rdfs:domain cim:Currency ;
  skos:definition "Sierra Leonean leone."@en .

cim:Currency.SOS a owl:NamedIndividual, owl:Thing ;
  rdfs:label "SOS "@en ;
  eq:isenum "True" ;
  rdfs:domain cim:Currency ;
  skos:definition "Somali shilling."@en .

cim:Currency.SRD a owl:NamedIndividual, owl:Thing ;
  rdfs:label "SRD "@en ;
  eq:isenum "True" ;
  rdfs:domain cim:Currency ;
  skos:definition "Surinamese dollar."@en .

cim:Currency.STD a owl:NamedIndividual, owl:Thing ;
  rdfs:label "STD "@en ;
  eq:isenum "True" ;
  rdfs:domain cim:Currency ;
  skos:definition "São Tomé and Príncipe dobra."@en .

cim:Currency.SYP a owl:NamedIndividual, owl:Thing ;
  rdfs:label "SYP "@en ;
  eq:isenum "True" ;
  rdfs:domain cim:Currency ;
  skos:definition "Syrian pound."@en .

cim:Currency.SZL a owl:NamedIndividual, owl:Thing ;
  rdfs:label "SZL "@en ;
  eq:isenum "True" ;
  rdfs:domain cim:Currency ;
  skos:definition "Lilangeni."@en .

cim:Currency.THB a owl:NamedIndividual, owl:Thing ;
  rdfs:label "THB "@en ;
  eq:isenum "True" ;
  rdfs:domain cim:Currency ;
  skos:definition "Thai baht."@en .

cim:Currency.TJS a owl:NamedIndividual, owl:Thing ;
  rdfs:label "TJS "@en ;
  eq:isenum "True" ;
  rdfs:domain cim:Currency ;
  skos:definition "Tajikistani somoni."@en .

cim:Currency.TMT a owl:NamedIndividual, owl:Thing ;
  rdfs:label "TMT "@en ;
  eq:isenum "True" ;
  rdfs:domain cim:Currency ;
  skos:definition "Turkmenistani manat."@en .

cim:Currency.TND a owl:NamedIndividual, owl:Thing ;
  rdfs:label "TND "@en ;
  eq:isenum "True" ;
  rdfs:domain cim:Currency ;
  skos:definition "Tunisian dinar."@en .

cim:Currency.TOP a owl:NamedIndividual, owl:Thing ;
  rdfs:label "TOP "@en ;
  eq:isenum "True" ;
  rdfs:domain cim:Currency ;
  skos:definition "Tongan pa'anga."@en .

cim:Currency.TRY a owl:NamedIndividual, owl:Thing ;
  rdfs:label "TRY "@en ;
  eq:isenum "True" ;
  rdfs:domain cim:Currency ;
  skos:definition "Turkish lira."@en .

cim:Currency.TTD a owl:NamedIndividual, owl:Thing ;
  rdfs:label "TTD "@en ;
  eq:isenum "True" ;
  rdfs:domain cim:Currency ;
  skos:definition "Trinidad and Tobago dollar."@en .

cim:Currency.TWD a owl:NamedIndividual, owl:Thing ;
  rdfs:label "TWD "@en ;
  eq:isenum "True" ;
  rdfs:domain cim:Currency ;
  skos:definition "New Taiwan dollar."@en .

cim:Currency.TZS a owl:NamedIndividual, owl:Thing ;
  rdfs:label "TZS "@en ;
  eq:isenum "True" ;
  rdfs:domain cim:Currency ;
  skos:definition "Tanzanian shilling."@en .

cim:Currency.UAH a owl:NamedIndividual, owl:Thing ;
  rdfs:label "UAH "@en ;
  eq:isenum "True" ;
  rdfs:domain cim:Currency ;
  skos:definition "Ukrainian hryvnia."@en .

cim:Currency.UGX a owl:NamedIndividual, owl:Thing ;
  rdfs:label "UGX "@en ;
  eq:isenum "True" ;
  rdfs:domain cim:Currency ;
  skos:definition "Ugandan shilling."@en .

cim:Currency.USD a owl:NamedIndividual, owl:Thing ;
  rdfs:label "USD "@en ;
  eq:isenum "True" ;
  rdfs:domain cim:Currency ;
  skos:definition "United States dollar."@en .

cim:Currency.UYU a owl:NamedIndividual, owl:Thing ;
  rdfs:label "UYU "@en ;
  eq:isenum "True" ;
  rdfs:domain cim:Currency ;
  skos:definition "Uruguayan peso."@en .

cim:Currency.UZS a owl:NamedIndividual, owl:Thing ;
  rdfs:label "UZS "@en ;
  eq:isenum "True" ;
  rdfs:domain cim:Currency ;
  skos:definition "Uzbekistan som."@en .

cim:Currency.VEF a owl:NamedIndividual, owl:Thing ;
  rdfs:label "VEF "@en ;
  eq:isenum "True" ;
  rdfs:domain cim:Currency ;
  skos:definition "Venezuelan bolívar fuerte."@en .

cim:Currency.VND a owl:NamedIndividual, owl:Thing ;
  rdfs:label "VND "@en ;
  eq:isenum "True" ;
  rdfs:domain cim:Currency ;
  skos:definition "Vietnamese Dong."@en .

cim:Currency.VUV a owl:NamedIndividual, owl:Thing ;
  rdfs:label "VUV "@en ;
  eq:isenum "True" ;
  rdfs:domain cim:Currency ;
  skos:definition "Vanuatu vatu."@en .

cim:Currency.WST a owl:NamedIndividual, owl:Thing ;
  rdfs:label "WST "@en ;
  eq:isenum "True" ;
  rdfs:domain cim:Currency ;
  skos:definition "Samoan tala."@en .

cim:Currency.XAF a owl:NamedIndividual, owl:Thing ;
  rdfs:label "XAF "@en ;
  eq:isenum "True" ;
  rdfs:domain cim:Currency ;
  skos:definition "CFA franc BEAC."@en .

cim:Currency.XCD a owl:NamedIndividual, owl:Thing ;
  rdfs:label "XCD "@en ;
  eq:isenum "True" ;
  rdfs:domain cim:Currency ;
  skos:definition "East Caribbean dollar."@en .

cim:Currency.XOF a owl:NamedIndividual, owl:Thing ;
  rdfs:label "XOF "@en ;
  eq:isenum "True" ;
  rdfs:domain cim:Currency ;
  skos:definition "CFA Franc BCEAO."@en .

cim:Currency.XPF a owl:NamedIndividual, owl:Thing ;
  rdfs:label "XPF "@en ;
  eq:isenum "True" ;
  rdfs:domain cim:Currency ;
  skos:definition "CFP franc."@en .

cim:Currency.YER a owl:NamedIndividual, owl:Thing ;
  rdfs:label "YER "@en ;
  eq:isenum "True" ;
  rdfs:domain cim:Currency ;
  skos:definition "Yemeni rial."@en .

cim:Currency.ZAR a owl:NamedIndividual, owl:Thing ;
  rdfs:label "ZAR "@en ;
  eq:isenum "True" ;
  rdfs:domain cim:Currency ;
  skos:definition "South African rand."@en .

cim:Currency.ZMK a owl:NamedIndividual, owl:Thing ;
  rdfs:label "ZMK "@en ;
  eq:isenum "True" ;
  rdfs:domain cim:Currency ;
  skos:definition "Zambian kwacha."@en .

cim:Currency.ZWL a owl:NamedIndividual, owl:Thing ;
  rdfs:label "ZWL "@en ;
  eq:isenum "True" ;
  rdfs:domain cim:Currency ;
  skos:definition "Zimbabwe dollar."@en .

cim:CurveStyle.constantYValue a owl:NamedIndividual, owl:Thing ;
  rdfs:label "constantYValue "@en ;
  eq:isenum "True" ;
  rdfs:domain cim:CurveStyle ;
  skos:definition """
The Y-axis values are assumed constant until the next curve point and prior to the first curve point.

\t"""@en .

cim:CurveStyle.straightLineYValues a owl:NamedIndividual, owl:Thing ;
  rdfs:label "straightLineYValues "@en ;
  eq:isenum "True" ;
  rdfs:domain cim:CurveStyle ;
  skos:definition """
The Y-axis values are assumed to be a straight line between values.  Also known as linear interpolation.

\t"""@en .

cim:DCConverterOperatingModeKind.bipolar a owl:NamedIndividual, owl:Thing ;
  rdfs:label "bipolar "@en ;
  eq:isenum "True" ;
  rdfs:domain cim:DCConverterOperatingModeKind ;
  skos:definition "Bipolar operation."@en .

cim:DCConverterOperatingModeKind.monopolarGroundReturn a owl:NamedIndividual, owl:Thing ;
  rdfs:label "monopolarGroundReturn "@en ;
  eq:isenum "True" ;
  rdfs:domain cim:DCConverterOperatingModeKind ;
  skos:definition "Monopolar operation with ground return."@en .

cim:DCConverterOperatingModeKind.monopolarMetallicReturn a owl:NamedIndividual, owl:Thing ;
  rdfs:label "monopolarMetallicReturn "@en ;
  eq:isenum "True" ;
  rdfs:domain cim:DCConverterOperatingModeKind ;
  skos:definition "Monopolar operation with metallic return."@en .

cim:DCPolarityKind.middle a owl:NamedIndividual, owl:Thing ;
  rdfs:label "middle "@en ;
  eq:isenum "True" ;
  rdfs:domain cim:DCPolarityKind ;
  skos:definition "Middle pole. The converter terminal is the midpoint in a bipolar or symmetric monopole configuration. The midpoint can be grounded and/or have a metallic return."@en .

cim:DCPolarityKind.negative a owl:NamedIndividual, owl:Thing ;
  rdfs:label "negative "@en ;
  eq:isenum "True" ;
  rdfs:domain cim:DCPolarityKind ;
  skos:definition "Negative pole. The converter terminal is intended to operate at a negative voltage relative the midpoint or positive terminal."@en .

cim:DCPolarityKind.positive a owl:NamedIndividual, owl:Thing ;
  rdfs:label "positive "@en ;
  eq:isenum "True" ;
  rdfs:domain cim:DCPolarityKind ;
  skos:definition "Positive pole. The converter terminal is intended to operate at a positive voltage relative the midpoint or negative terminal."@en .

cim:FuelType.brownCoalLignite a owl:NamedIndividual, owl:Thing ;
  rdfs:label "brownCoalLignite "@en ;
  eq:isenum "True" ;
  rdfs:domain cim:FuelType ;
  skos:definition "Brown coal lignite."@en .

cim:FuelType.coal a owl:NamedIndividual, owl:Thing ;
  rdfs:label "coal "@en ;
  eq:isenum "True" ;
  rdfs:domain cim:FuelType ;
  skos:definition "Generic coal, not including lignite type."@en .

cim:FuelType.coalDerivedGas a owl:NamedIndividual, owl:Thing ;
  rdfs:label "coalDerivedGas "@en ;
  eq:isenum "True" ;
  rdfs:domain cim:FuelType ;
  skos:definition "Coal derived gas."@en .

cim:FuelType.gas a owl:NamedIndividual, owl:Thing ;
  rdfs:label "gas "@en ;
  eq:isenum "True" ;
  rdfs:domain cim:FuelType ;
  skos:definition "Natural gas."@en .

cim:FuelType.hardCoal a owl:NamedIndividual, owl:Thing ;
  rdfs:label "hardCoal "@en ;
  eq:isenum "True" ;
  rdfs:domain cim:FuelType ;
  skos:definition "Hard coal."@en .

cim:FuelType.lignite a owl:NamedIndividual, owl:Thing ;
  rdfs:label "lignite "@en ;
  eq:isenum "True" ;
  rdfs:domain cim:FuelType ;
  skos:definition "The fuel is lignite coal.  Note that this is a special type of coal, so the other enum of coal is reserved for hard coal types or if the exact type of coal is not known."@en .

cim:FuelType.oil a owl:NamedIndividual, owl:Thing ;
  rdfs:label "oil "@en ;
  eq:isenum "True" ;
  rdfs:domain cim:FuelType ;
  skos:definition """
Oil.

\t"""@en .

cim:FuelType.oilShale a owl:NamedIndividual, owl:Thing ;
  rdfs:label "oilShale "@en ;
  eq:isenum "True" ;
  rdfs:domain cim:FuelType ;
  skos:definition "Oil Shale."@en .

cim:FuelType.other a owl:NamedIndividual, owl:Thing ;
  rdfs:label "other "@en ;
  eq:isenum "True" ;
  rdfs:domain cim:FuelType ;
  skos:definition "Any fuel type not included in the rest of the enumerated value."@en .

cim:FuelType.peat a owl:NamedIndividual, owl:Thing ;
  rdfs:label "peat "@en ;
  eq:isenum "True" ;
  rdfs:domain cim:FuelType ;
  skos:definition "Peat."@en .

cim:GeneratorControlSource.offAGC a owl:NamedIndividual, owl:Thing ;
  rdfs:label "offAGC "@en ;
  eq:isenum "True" ;
  rdfs:domain cim:GeneratorControlSource ;
  skos:definition """
Off of automatic generation control (AGC).

\t"""@en .

cim:GeneratorControlSource.onAGC a owl:NamedIndividual, owl:Thing ;
  rdfs:label "onAGC "@en ;
  eq:isenum "True" ;
  rdfs:domain cim:GeneratorControlSource ;
  skos:definition """
On automatic generation control (AGC).

\t"""@en .

cim:GeneratorControlSource.plantControl a owl:NamedIndividual, owl:Thing ;
  rdfs:label "plantControl "@en ;
  eq:isenum "True" ;
  rdfs:domain cim:GeneratorControlSource ;
  skos:definition """
Plant is controlling.

\t"""@en .

cim:GeneratorControlSource.unavailable a owl:NamedIndividual, owl:Thing ;
  rdfs:label "unavailable "@en ;
  eq:isenum "True" ;
  rdfs:domain cim:GeneratorControlSource ;
  skos:definition """
Not available.

\t"""@en .

cim:HydroEnergyConversionKind.generator a owl:NamedIndividual, owl:Thing ;
  rdfs:label "generator "@en ;
  eq:isenum "True" ;
  rdfs:domain cim:HydroEnergyConversionKind ;
  skos:definition "Able to generate power, but not able to pump water for energy storage."@en .

cim:HydroEnergyConversionKind.pumpAndGenerator a owl:NamedIndividual, owl:Thing ;
  rdfs:label "pumpAndGenerator "@en ;
  eq:isenum "True" ;
  rdfs:domain cim:HydroEnergyConversionKind ;
  skos:definition "Able to both generate power and pump water for energy storage."@en .

cim:HydroPlantStorageKind.pumpedStorage a owl:NamedIndividual, owl:Thing ;
  rdfs:label "pumpedStorage "@en ;
  eq:isenum "True" ;
  rdfs:domain cim:HydroPlantStorageKind ;
  skos:definition """
Pumped storage.

\t"""@en .

cim:HydroPlantStorageKind.runOfRiver a owl:NamedIndividual, owl:Thing ;
  rdfs:label "runOfRiver "@en ;
  eq:isenum "True" ;
  rdfs:domain cim:HydroPlantStorageKind ;
  skos:definition """
Run of river.

\t"""@en .

cim:HydroPlantStorageKind.storage a owl:NamedIndividual, owl:Thing ;
  rdfs:label "storage "@en ;
  eq:isenum "True" ;
  rdfs:domain cim:HydroPlantStorageKind ;
  skos:definition "Storage."@en .

cim:HydroTurbineKind.francis a owl:NamedIndividual, owl:Thing ;
  rdfs:label "francis "@en ;
  eq:isenum "True" ;
  rdfs:domain cim:HydroTurbineKind ;
  skos:definition """
Francis.

\t"""@en .

cim:HydroTurbineKind.kaplan a owl:NamedIndividual, owl:Thing ;
  rdfs:label "kaplan "@en ;
  eq:isenum "True" ;
  rdfs:domain cim:HydroTurbineKind ;
  skos:definition """
Kaplan.

\t"""@en .

cim:HydroTurbineKind.pelton a owl:NamedIndividual, owl:Thing ;
  rdfs:label "pelton "@en ;
  eq:isenum "True" ;
  rdfs:domain cim:HydroTurbineKind ;
  skos:definition """
Pelton.

\t"""@en .

cim:OperationalLimitDirectionKind.absoluteValue a owl:NamedIndividual, owl:Thing ;
  rdfs:label "absoluteValue "@en ;
  eq:isenum "True" ;
  rdfs:domain cim:OperationalLimitDirectionKind ;
  skos:definition "An absoluteValue limit means that a monitored absolute value above the limit value is a violation."@en .

cim:OperationalLimitDirectionKind.high a owl:NamedIndividual, owl:Thing ;
  rdfs:label "high "@en ;
  eq:isenum "True" ;
  rdfs:domain cim:OperationalLimitDirectionKind ;
  skos:definition "High means that a monitored value above the limit value is a violation.   If applied to a terminal flow, the positive direction is into the terminal."@en .

cim:OperationalLimitDirectionKind.low a owl:NamedIndividual, owl:Thing ;
  rdfs:label "low "@en ;
  eq:isenum "True" ;
  rdfs:domain cim:OperationalLimitDirectionKind ;
  skos:definition "Low means a monitored value below the limit is a violation.  If applied to a terminal flow, the positive direction is into the terminal."@en .

cim:PhaseCode.A a owl:NamedIndividual, owl:Thing ;
  rdfs:label "A "@en ;
  eq:isenum "True" ;
  rdfs:domain cim:PhaseCode ;
  skos:definition "Phase A."@en .

cim:PhaseCode.AB a owl:NamedIndividual, owl:Thing ;
  rdfs:label "AB "@en ;
  eq:isenum "True" ;
  rdfs:domain cim:PhaseCode ;
  skos:definition "Phases A and B."@en .

cim:PhaseCode.ABC a owl:NamedIndividual, owl:Thing ;
  rdfs:label "ABC "@en ;
  eq:isenum "True" ;
  rdfs:domain cim:PhaseCode ;
  skos:definition "Phases A, B, and C."@en .

cim:PhaseCode.ABCN a owl:NamedIndividual, owl:Thing ;
  rdfs:label "ABCN "@en ;
  eq:isenum "True" ;
  rdfs:domain cim:PhaseCode ;
  skos:definition "Phases A, B, C, and N."@en .

cim:PhaseCode.ABN a owl:NamedIndividual, owl:Thing ;
  rdfs:label "ABN "@en ;
  eq:isenum "True" ;
  rdfs:domain cim:PhaseCode ;
  skos:definition "Phases A, B, and neutral."@en .

cim:PhaseCode.AC a owl:NamedIndividual, owl:Thing ;
  rdfs:label "AC "@en ;
  eq:isenum "True" ;
  rdfs:domain cim:PhaseCode ;
  skos:definition "Phases A and C."@en .

cim:PhaseCode.ACN a owl:NamedIndividual, owl:Thing ;
  rdfs:label "ACN "@en ;
  eq:isenum "True" ;
  rdfs:domain cim:PhaseCode ;
  skos:definition "Phases A, C and neutral."@en .

cim:PhaseCode.AN a owl:NamedIndividual, owl:Thing ;
  rdfs:label "AN "@en ;
  eq:isenum "True" ;
  rdfs:domain cim:PhaseCode ;
  skos:definition "Phases A and neutral."@en .

cim:PhaseCode.B a owl:NamedIndividual, owl:Thing ;
  rdfs:label "B "@en ;
  eq:isenum "True" ;
  rdfs:domain cim:PhaseCode ;
  skos:definition "Phase B."@en .

cim:PhaseCode.BC a owl:NamedIndividual, owl:Thing ;
  rdfs:label "BC "@en ;
  eq:isenum "True" ;
  rdfs:domain cim:PhaseCode ;
  skos:definition "Phases B and C."@en .

cim:PhaseCode.BCN a owl:NamedIndividual, owl:Thing ;
  rdfs:label "BCN "@en ;
  eq:isenum "True" ;
  rdfs:domain cim:PhaseCode ;
  skos:definition "Phases B, C, and neutral."@en .

cim:PhaseCode.BN a owl:NamedIndividual, owl:Thing ;
  rdfs:label "BN "@en ;
  eq:isenum "True" ;
  rdfs:domain cim:PhaseCode ;
  skos:definition "Phases B and neutral."@en .

cim:PhaseCode.C a owl:NamedIndividual, owl:Thing ;
  rdfs:label "C "@en ;
  eq:isenum "True" ;
  rdfs:domain cim:PhaseCode ;
  skos:definition "Phase C."@en .

cim:PhaseCode.CN a owl:NamedIndividual, owl:Thing ;
  rdfs:label "CN "@en ;
  eq:isenum "True" ;
  rdfs:domain cim:PhaseCode ;
  skos:definition "Phases C and neutral."@en .

cim:PhaseCode.N a owl:NamedIndividual, owl:Thing ;
  rdfs:label "N "@en ;
  eq:isenum "True" ;
  rdfs:domain cim:PhaseCode ;
  skos:definition "Neutral phase."@en .

cim:PhaseCode.X a owl:NamedIndividual, owl:Thing ;
  rdfs:label "X "@en ;
  eq:isenum "True" ;
  rdfs:domain cim:PhaseCode ;
  skos:definition "Unknown non-neutral phase."@en .

cim:PhaseCode.XN a owl:NamedIndividual, owl:Thing ;
  rdfs:label "XN "@en ;
  eq:isenum "True" ;
  rdfs:domain cim:PhaseCode ;
  skos:definition "Unknown non-neutral phase plus neutral."@en .

cim:PhaseCode.XY a owl:NamedIndividual, owl:Thing ;
  rdfs:label "XY "@en ;
  eq:isenum "True" ;
  rdfs:domain cim:PhaseCode ;
  skos:definition "Two unknown non-neutral phases."@en .

cim:PhaseCode.XYN a owl:NamedIndividual, owl:Thing ;
  rdfs:label "XYN "@en ;
  eq:isenum "True" ;
  rdfs:domain cim:PhaseCode ;
  skos:definition "Two unknown non-neutral phases plus neutral."@en .

cim:PhaseCode.none a owl:NamedIndividual, owl:Thing ;
  rdfs:label "none "@en ;
  eq:isenum "True" ;
  rdfs:domain cim:PhaseCode ;
  skos:definition "No phases specified."@en .

cim:PhaseCode.s1 a owl:NamedIndividual, owl:Thing ;
  rdfs:label "s1 "@en ;
  eq:isenum "True" ;
  rdfs:domain cim:PhaseCode ;
  skos:definition "Secondary phase 1."@en .

cim:PhaseCode.s12 a owl:NamedIndividual, owl:Thing ;
  rdfs:label "s12 "@en ;
  eq:isenum "True" ;
  rdfs:domain cim:PhaseCode ;
  skos:definition "Secondary phase 1 and 2."@en .

cim:PhaseCode.s12N a owl:NamedIndividual, owl:Thing ;
  rdfs:label "s12N "@en ;
  eq:isenum "True" ;
  rdfs:domain cim:PhaseCode ;
  skos:definition "Secondary phases 1, 2, and neutral."@en .

cim:PhaseCode.s1N a owl:NamedIndividual, owl:Thing ;
  rdfs:label "s1N "@en ;
  eq:isenum "True" ;
  rdfs:domain cim:PhaseCode ;
  skos:definition "Secondary phase 1 and neutral."@en .

cim:PhaseCode.s2 a owl:NamedIndividual, owl:Thing ;
  rdfs:label "s2 "@en ;
  eq:isenum "True" ;
  rdfs:domain cim:PhaseCode ;
  skos:definition "Secondary phase 2."@en .

cim:PhaseCode.s2N a owl:NamedIndividual, owl:Thing ;
  rdfs:label "s2N "@en ;
  eq:isenum "True" ;
  rdfs:domain cim:PhaseCode ;
  skos:definition "Secondary phase 2 and neutral."@en .

cim:RegulatingControlModeKind.activePower a owl:NamedIndividual, owl:Thing ;
  rdfs:label "activePower "@en ;
  eq:isenum "True" ;
  rdfs:domain cim:RegulatingControlModeKind ;
  skos:definition "Active power is specified."@en .

cim:RegulatingControlModeKind.admittance a owl:NamedIndividual, owl:Thing ;
  rdfs:label "admittance "@en ;
  eq:isenum "True" ;
  rdfs:domain cim:RegulatingControlModeKind ;
  skos:definition """
Admittance is specified.

\t"""@en .

cim:RegulatingControlModeKind.currentFlow a owl:NamedIndividual, owl:Thing ;
  rdfs:label "currentFlow "@en ;
  eq:isenum "True" ;
  rdfs:domain cim:RegulatingControlModeKind ;
  skos:definition "Current flow is specified."@en .

cim:RegulatingControlModeKind.powerFactor a owl:NamedIndividual, owl:Thing ;
  rdfs:label "powerFactor "@en ;
  eq:isenum "True" ;
  rdfs:domain cim:RegulatingControlModeKind ;
  skos:definition """
Power factor is specified.

\t"""@en .

cim:RegulatingControlModeKind.reactivePower a owl:NamedIndividual, owl:Thing ;
  rdfs:label "reactivePower "@en ;
  eq:isenum "True" ;
  rdfs:domain cim:RegulatingControlModeKind ;
  skos:definition "Reactive power is specified."@en .

cim:RegulatingControlModeKind.temperature a owl:NamedIndividual, owl:Thing ;
  rdfs:label "temperature "@en ;
  eq:isenum "True" ;
  rdfs:domain cim:RegulatingControlModeKind ;
  skos:definition "Control switches on/off based on the local temperature (i.e., a thermostat)."@en .

cim:RegulatingControlModeKind.timeScheduled a owl:NamedIndividual, owl:Thing ;
  rdfs:label "timeScheduled "@en ;
  eq:isenum "True" ;
  rdfs:domain cim:RegulatingControlModeKind ;
  skos:definition "Control switches on/off by time of day. The times may change on the weekend, or in different seasons."@en .

cim:RegulatingControlModeKind.voltage a owl:NamedIndividual, owl:Thing ;
  rdfs:label "voltage "@en ;
  eq:isenum "True" ;
  rdfs:domain cim:RegulatingControlModeKind ;
  skos:definition "Voltage is specified."@en .

cim:SVCControlMode.reactivePower a owl:NamedIndividual, owl:Thing ;
  rdfs:label "reactivePower "@en ;
  eq:isenum "True" ;
  rdfs:domain cim:SVCControlMode ;
  skos:definition "Reactive power control."@en .

cim:SVCControlMode.voltage a owl:NamedIndividual, owl:Thing ;
  rdfs:label "voltage "@en ;
  eq:isenum "True" ;
  rdfs:domain cim:SVCControlMode ;
  skos:definition "Voltage control."@en .

cim:SynchronousMachineKind.condenser a owl:NamedIndividual, owl:Thing ;
  rdfs:label "condenser "@en ;
  eq:isenum "True" ;
  rdfs:domain cim:SynchronousMachineKind ;
  skos:definition "Indicates the synchronous machine can operate as a condenser."@en .

cim:SynchronousMachineKind.generator a owl:NamedIndividual, owl:Thing ;
  rdfs:label "generator "@en ;
  eq:isenum "True" ;
  rdfs:domain cim:SynchronousMachineKind ;
  skos:definition "Indicates the synchronous machine can operate as a generator."@en .

cim:SynchronousMachineKind.generatorOrCondenser a owl:NamedIndividual, owl:Thing ;
  rdfs:label "generatorOrCondenser "@en ;
  eq:isenum "True" ;
  rdfs:domain cim:SynchronousMachineKind ;
  skos:definition "Indicates the synchronous machine can operate as a generator or as a condenser."@en .

cim:SynchronousMachineKind.generatorOrCondenserOrMotor a owl:NamedIndividual, owl:Thing ;
  rdfs:label "generatorOrCondenserOrMotor "@en ;
  eq:isenum "True" ;
  rdfs:domain cim:SynchronousMachineKind ;
  skos:definition "Indicates the synchronous machine can operate as a generator or as a condenser or as a motor."@en .

cim:SynchronousMachineKind.generatorOrMotor a owl:NamedIndividual, owl:Thing ;
  rdfs:label "generatorOrMotor "@en ;
  eq:isenum "True" ;
  rdfs:domain cim:SynchronousMachineKind ;
  skos:definition "Indicates the synchronous machine can operate as a generator or as a motor."@en .

cim:SynchronousMachineKind.motor a owl:NamedIndividual, owl:Thing ;
  rdfs:label "motor "@en ;
  eq:isenum "True" ;
  rdfs:domain cim:SynchronousMachineKind ;
  skos:definition "Indicates the synchronous machine can operate as a motor."@en .

cim:SynchronousMachineKind.motorOrCondenser a owl:NamedIndividual, owl:Thing ;
  rdfs:label "motorOrCondenser "@en ;
  eq:isenum "True" ;
  rdfs:domain cim:SynchronousMachineKind ;
  skos:definition "Indicates the synchronous machine can operate as a motor or as a condenser."@en .

cim:UnitMultiplier.E a owl:NamedIndividual, owl:Thing ;
  rdfs:label "E "@en ;
  eq:isenum "True" ;
  rdfs:domain cim:UnitMultiplier ;
  skos:definition "Exa 10**18."@en .

cim:UnitMultiplier.G a owl:NamedIndividual, owl:Thing ;
  rdfs:label "G "@en ;
  eq:isenum "True" ;
  rdfs:domain cim:UnitMultiplier ;
  skos:definition "Giga 10**9."@en .

cim:UnitMultiplier.M a owl:NamedIndividual, owl:Thing ;
  rdfs:label "M "@en ;
  eq:isenum "True" ;
  rdfs:domain cim:UnitMultiplier ;
  skos:definition "Mega 10**6."@en .

cim:UnitMultiplier.P a owl:NamedIndividual, owl:Thing ;
  rdfs:label "P "@en ;
  eq:isenum "True" ;
  rdfs:domain cim:UnitMultiplier ;
  skos:definition "Peta 10**15."@en .

cim:UnitMultiplier.T a owl:NamedIndividual, owl:Thing ;
  rdfs:label "T "@en ;
  eq:isenum "True" ;
  rdfs:domain cim:UnitMultiplier ;
  skos:definition "Tera 10**12."@en .

cim:UnitMultiplier.Y a owl:NamedIndividual, owl:Thing ;
  rdfs:label "Y "@en ;
  eq:isenum "True" ;
  rdfs:domain cim:UnitMultiplier ;
  skos:definition "Yotta 10**24."@en .

cim:UnitMultiplier.Z a owl:NamedIndividual, owl:Thing ;
  rdfs:label "Z "@en ;
  eq:isenum "True" ;
  rdfs:domain cim:UnitMultiplier ;
  skos:definition "Zetta 10**21."@en .

cim:UnitMultiplier.a a owl:NamedIndividual, owl:Thing ;
  rdfs:label "a "@en ;
  eq:isenum "True" ;
  rdfs:domain cim:UnitMultiplier ;
  skos:definition "Atto 10**-18."@en .

cim:UnitMultiplier.c a owl:NamedIndividual, owl:Thing ;
  rdfs:label "c "@en ;
  eq:isenum "True" ;
  rdfs:domain cim:UnitMultiplier ;
  skos:definition "Centi 10**-2."@en .

cim:UnitMultiplier.d a owl:NamedIndividual, owl:Thing ;
  rdfs:label "d "@en ;
  eq:isenum "True" ;
  rdfs:domain cim:UnitMultiplier ;
  skos:definition "Deci 10**-1."@en .

cim:UnitMultiplier.da a owl:NamedIndividual, owl:Thing ;
  rdfs:label "da "@en ;
  eq:isenum "True" ;
  rdfs:domain cim:UnitMultiplier ;
  skos:definition "Deca 10**1."@en .

cim:UnitMultiplier.f a owl:NamedIndividual, owl:Thing ;
  rdfs:label "f "@en ;
  eq:isenum "True" ;
  rdfs:domain cim:UnitMultiplier ;
  skos:definition "Femto 10**-15."@en .

cim:UnitMultiplier.h a owl:NamedIndividual, owl:Thing ;
  rdfs:label "h "@en ;
  eq:isenum "True" ;
  rdfs:domain cim:UnitMultiplier ;
  skos:definition "Hecto 10**2."@en .

cim:UnitMultiplier.k a owl:NamedIndividual, owl:Thing ;
  rdfs:label "k "@en ;
  eq:isenum "True" ;
  rdfs:domain cim:UnitMultiplier ;
  skos:definition "Kilo 10**3."@en .

cim:UnitMultiplier.m a owl:NamedIndividual, owl:Thing ;
  rdfs:label "m "@en ;
  eq:isenum "True" ;
  rdfs:domain cim:UnitMultiplier ;
  skos:definition "Milli 10**-3."@en .

cim:UnitMultiplier.micro a owl:NamedIndividual, owl:Thing ;
  rdfs:label "micro "@en ;
  eq:isenum "True" ;
  rdfs:domain cim:UnitMultiplier ;
  skos:definition "Micro 10**-6."@en .

cim:UnitMultiplier.n a owl:NamedIndividual, owl:Thing ;
  rdfs:label "n "@en ;
  eq:isenum "True" ;
  rdfs:domain cim:UnitMultiplier ;
  skos:definition "Nano 10**-9."@en .

cim:UnitMultiplier.none a owl:NamedIndividual, owl:Thing ;
  rdfs:label "none "@en ;
  eq:isenum "True" ;
  rdfs:domain cim:UnitMultiplier ;
  skos:definition "No multiplier or equivalently multiply by 1."@en .

cim:UnitMultiplier.p a owl:NamedIndividual, owl:Thing ;
  rdfs:label "p "@en ;
  eq:isenum "True" ;
  rdfs:domain cim:UnitMultiplier ;
  skos:definition "Pico 10**-12."@en .

cim:UnitMultiplier.y a owl:NamedIndividual, owl:Thing ;
  rdfs:label "y "@en ;
  eq:isenum "True" ;
  rdfs:domain cim:UnitMultiplier ;
  skos:definition "Yocto 10**-24."@en .

cim:UnitMultiplier.z a owl:NamedIndividual, owl:Thing ;
  rdfs:label "z "@en ;
  eq:isenum "True" ;
  rdfs:domain cim:UnitMultiplier ;
  skos:definition "Zepto 10**-21."@en .

cim:UnitSymbol.A a owl:NamedIndividual, owl:Thing ;
  rdfs:label "A "@en ;
  eq:isenum "True" ;
  rdfs:domain cim:UnitSymbol ;
  skos:definition "Current in amperes."@en .

cim:UnitSymbol.A2 a owl:NamedIndividual, owl:Thing ;
  rdfs:label "A2 "@en ;
  eq:isenum "True" ;
  rdfs:domain cim:UnitSymbol ;
  skos:definition "Amperes squared (A²)."@en .

cim:UnitSymbol.A2h a owl:NamedIndividual, owl:Thing ;
  rdfs:label "A2h "@en ;
  eq:isenum "True" ;
  rdfs:domain cim:UnitSymbol ;
  skos:definition "Ampere-squared hour, ampere-squared hour."@en .

cim:UnitSymbol.A2s a owl:NamedIndividual, owl:Thing ;
  rdfs:label "A2s "@en ;
  eq:isenum "True" ;
  rdfs:domain cim:UnitSymbol ;
  skos:definition "Ampere squared time in square amperes (A²s)."@en .

cim:UnitSymbol.APerA a owl:NamedIndividual, owl:Thing ;
  rdfs:label "APerA "@en ;
  eq:isenum "True" ;
  rdfs:domain cim:UnitSymbol ;
  skos:definition "Current, ratio of amperages.   Note: Users may need to supply a prefix such as ‘m’ to show rates such as ‘mA/A’."@en .

cim:UnitSymbol.APerm a owl:NamedIndividual, owl:Thing ;
  rdfs:label "APerm "@en ;
  eq:isenum "True" ;
  rdfs:domain cim:UnitSymbol ;
  skos:definition "A/m, magnetic field strength, amperes per metre."@en .

cim:UnitSymbol.Ah a owl:NamedIndividual, owl:Thing ;
  rdfs:label "Ah "@en ;
  eq:isenum "True" ;
  rdfs:domain cim:UnitSymbol ;
  skos:definition "Ampere-hours, ampere-hours."@en .

cim:UnitSymbol.As a owl:NamedIndividual, owl:Thing ;
  rdfs:label "As "@en ;
  eq:isenum "True" ;
  rdfs:domain cim:UnitSymbol ;
  skos:definition "Ampere seconds (A·s)."@en .

cim:UnitSymbol.Bq a owl:NamedIndividual, owl:Thing ;
  rdfs:label "Bq "@en ;
  eq:isenum "True" ;
  rdfs:domain cim:UnitSymbol ;
  skos:definition "Radioactivity in becquerels (1/s)."@en .

cim:UnitSymbol.Btu a owl:NamedIndividual, owl:Thing ;
  rdfs:label "Btu "@en ;
  eq:isenum "True" ;
  rdfs:domain cim:UnitSymbol ;
  skos:definition "Energy, British Thermal Units."@en .

cim:UnitSymbol.C a owl:NamedIndividual, owl:Thing ;
  rdfs:label "C "@en ;
  eq:isenum "True" ;
  rdfs:domain cim:UnitSymbol ;
  skos:definition "Electric charge in coulombs (A·s)."@en .

cim:UnitSymbol.CPerkg a owl:NamedIndividual, owl:Thing ;
  rdfs:label "CPerkg "@en ;
  eq:isenum "True" ;
  rdfs:domain cim:UnitSymbol ;
  skos:definition "Exposure (x rays), coulombs per kilogram."@en .

cim:UnitSymbol.CPerm2 a owl:NamedIndividual, owl:Thing ;
  rdfs:label "CPerm2 "@en ;
  eq:isenum "True" ;
  rdfs:domain cim:UnitSymbol ;
  skos:definition "Surface charge density, coulombs per square metre."@en .

cim:UnitSymbol.CPerm3 a owl:NamedIndividual, owl:Thing ;
  rdfs:label "CPerm3 "@en ;
  eq:isenum "True" ;
  rdfs:domain cim:UnitSymbol ;
  skos:definition "Electric charge density, coulombs per cubic metre."@en .

cim:UnitSymbol.F a owl:NamedIndividual, owl:Thing ;
  rdfs:label "F "@en ;
  eq:isenum "True" ;
  rdfs:domain cim:UnitSymbol ;
  skos:definition "Electric capacitance in farads (C/V)."@en .

cim:UnitSymbol.FPerm a owl:NamedIndividual, owl:Thing ;
  rdfs:label "FPerm "@en ;
  eq:isenum "True" ;
  rdfs:domain cim:UnitSymbol ;
  skos:definition "Permittivity, farads per metre."@en .

cim:UnitSymbol.G a owl:NamedIndividual, owl:Thing ;
  rdfs:label "G "@en ;
  eq:isenum "True" ;
  rdfs:domain cim:UnitSymbol ;
  skos:definition "Magnetic flux density, gausses (1 G = 10-4 T)."@en .

cim:UnitSymbol.Gy a owl:NamedIndividual, owl:Thing ;
  rdfs:label "Gy "@en ;
  eq:isenum "True" ;
  rdfs:domain cim:UnitSymbol ;
  skos:definition "Absorbed dose in grays (J/kg)."@en .

cim:UnitSymbol.GyPers a owl:NamedIndividual, owl:Thing ;
  rdfs:label "GyPers "@en ;
  eq:isenum "True" ;
  rdfs:domain cim:UnitSymbol ;
  skos:definition "Absorbed dose rate, grays per second."@en .

cim:UnitSymbol.H a owl:NamedIndividual, owl:Thing ;
  rdfs:label "H "@en ;
  eq:isenum "True" ;
  rdfs:domain cim:UnitSymbol ;
  skos:definition "Electric inductance in henrys (Wb/A)."@en .

cim:UnitSymbol.HPerm a owl:NamedIndividual, owl:Thing ;
  rdfs:label "HPerm "@en ;
  eq:isenum "True" ;
  rdfs:domain cim:UnitSymbol ;
  skos:definition "Permeability, henrys per metre."@en .

cim:UnitSymbol.Hz a owl:NamedIndividual, owl:Thing ;
  rdfs:label "Hz "@en ;
  eq:isenum "True" ;
  rdfs:domain cim:UnitSymbol ;
  skos:definition "Frequency in hertz (1/s)."@en .

cim:UnitSymbol.HzPerHz a owl:NamedIndividual, owl:Thing ;
  rdfs:label "HzPerHz "@en ;
  eq:isenum "True" ;
  rdfs:domain cim:UnitSymbol ;
  skos:definition "Frequency, rate of frequency change.   Note: Users may need to supply a prefix such as ‘m’ to show rates such as ‘mHz/Hz’."@en .

cim:UnitSymbol.HzPers a owl:NamedIndividual, owl:Thing ;
  rdfs:label "HzPers "@en ;
  eq:isenum "True" ;
  rdfs:domain cim:UnitSymbol ;
  skos:definition "Rate of change of frequency in hertz per second."@en .

cim:UnitSymbol.J a owl:NamedIndividual, owl:Thing ;
  rdfs:label "J "@en ;
  eq:isenum "True" ;
  rdfs:domain cim:UnitSymbol ;
  skos:definition "Energy in joules (N·m = C·V = W·s)."@en .

cim:UnitSymbol.JPerK a owl:NamedIndividual, owl:Thing ;
  rdfs:label "JPerK "@en ;
  eq:isenum "True" ;
  rdfs:domain cim:UnitSymbol ;
  skos:definition "Heat capacity in joules/kelvin."@en .

cim:UnitSymbol.JPerkg a owl:NamedIndividual, owl:Thing ;
  rdfs:label "JPerkg "@en ;
  eq:isenum "True" ;
  rdfs:domain cim:UnitSymbol ;
  skos:definition "Specific energy, Joules / kg."@en .

cim:UnitSymbol.JPerkgK a owl:NamedIndividual, owl:Thing ;
  rdfs:label "JPerkgK "@en ;
  eq:isenum "True" ;
  rdfs:domain cim:UnitSymbol ;
  skos:definition "Specific heat capacity, specific entropy, joules per kilogram Kelvin."@en .

cim:UnitSymbol.JPerm2 a owl:NamedIndividual, owl:Thing ;
  rdfs:label "JPerm2 "@en ;
  eq:isenum "True" ;
  rdfs:domain cim:UnitSymbol ;
  skos:definition "Insulation energy density, joules per square metre or watt second per square metre."@en .

cim:UnitSymbol.JPerm3 a owl:NamedIndividual, owl:Thing ;
  rdfs:label "JPerm3 "@en ;
  eq:isenum "True" ;
  rdfs:domain cim:UnitSymbol ;
  skos:definition "Energy density, joules per cubic metre."@en .

cim:UnitSymbol.JPermol a owl:NamedIndividual, owl:Thing ;
  rdfs:label "JPermol "@en ;
  eq:isenum "True" ;
  rdfs:domain cim:UnitSymbol ;
  skos:definition "Molar energy, joules per mole."@en .

cim:UnitSymbol.JPermolK a owl:NamedIndividual, owl:Thing ;
  rdfs:label "JPermolK "@en ;
  eq:isenum "True" ;
  rdfs:domain cim:UnitSymbol ;
  skos:definition "Molar entropy, molar heat capacity, joules per mole kelvin."@en .

cim:UnitSymbol.JPers a owl:NamedIndividual, owl:Thing ;
  rdfs:label "JPers "@en ;
  eq:isenum "True" ;
  rdfs:domain cim:UnitSymbol ;
  skos:definition "Energy rate in joules per second (J/s)."@en .

cim:UnitSymbol.K a owl:NamedIndividual, owl:Thing ;
  rdfs:label "K "@en ;
  eq:isenum "True" ;
  rdfs:domain cim:UnitSymbol ;
  skos:definition "Temperature in kelvins."@en .

cim:UnitSymbol.KPers a owl:NamedIndividual, owl:Thing ;
  rdfs:label "KPers "@en ;
  eq:isenum "True" ;
  rdfs:domain cim:UnitSymbol ;
  skos:definition "Temperature change rate in kelvins per second."@en .

cim:UnitSymbol.M a owl:NamedIndividual, owl:Thing ;
  rdfs:label "M "@en ;
  eq:isenum "True" ;
  rdfs:domain cim:UnitSymbol ;
  skos:definition "Length, nautical miles (1 M = 1852 m)."@en .

cim:UnitSymbol.Mx a owl:NamedIndividual, owl:Thing ;
  rdfs:label "Mx "@en ;
  eq:isenum "True" ;
  rdfs:domain cim:UnitSymbol ;
  skos:definition "Magnetic flux, maxwells (1 Mx = 10-8 Wb)."@en .

cim:UnitSymbol.N a owl:NamedIndividual, owl:Thing ;
  rdfs:label "N "@en ;
  eq:isenum "True" ;
  rdfs:domain cim:UnitSymbol ;
  skos:definition "Force in newtons (kg·m/s²)."@en .

cim:UnitSymbol.NPerm a owl:NamedIndividual, owl:Thing ;
  rdfs:label "NPerm "@en ;
  eq:isenum "True" ;
  rdfs:domain cim:UnitSymbol ;
  skos:definition "Surface tension, newton per metre."@en .

cim:UnitSymbol.Nm a owl:NamedIndividual, owl:Thing ;
  rdfs:label "Nm "@en ;
  eq:isenum "True" ;
  rdfs:domain cim:UnitSymbol ;
  skos:definition "Moment of force, newton metres."@en .

cim:UnitSymbol.Oe a owl:NamedIndividual, owl:Thing ;
  rdfs:label "Oe "@en ;
  eq:isenum "True" ;
  rdfs:domain cim:UnitSymbol ;
  skos:definition "Magnetic field in oersteds, (1 Oe = (103/4p) A/m)."@en .

cim:UnitSymbol.Pa a owl:NamedIndividual, owl:Thing ;
  rdfs:label "Pa "@en ;
  eq:isenum "True" ;
  rdfs:domain cim:UnitSymbol ;
  skos:definition "Pressure in pascals (N/m²). Note: the absolute or relative measurement of pressure is implied with this entry. See below for more explicit forms."@en .

cim:UnitSymbol.PaPers a owl:NamedIndividual, owl:Thing ;
  rdfs:label "PaPers "@en ;
  eq:isenum "True" ;
  rdfs:domain cim:UnitSymbol ;
  skos:definition "Pressure change rate in pascals per second."@en .

cim:UnitSymbol.Pas a owl:NamedIndividual, owl:Thing ;
  rdfs:label "Pas "@en ;
  eq:isenum "True" ;
  rdfs:domain cim:UnitSymbol ;
  skos:definition "Dynamic viscosity, pascal seconds."@en .

cim:UnitSymbol.Q a owl:NamedIndividual, owl:Thing ;
  rdfs:label "Q "@en ;
  eq:isenum "True" ;
  rdfs:domain cim:UnitSymbol ;
  skos:definition "Quantity power, Q."@en .

cim:UnitSymbol.Qh a owl:NamedIndividual, owl:Thing ;
  rdfs:label "Qh "@en ;
  eq:isenum "True" ;
  rdfs:domain cim:UnitSymbol ;
  skos:definition "Quantity energy, Qh."@en .

cim:UnitSymbol.S a owl:NamedIndividual, owl:Thing ;
  rdfs:label "S "@en ;
  eq:isenum "True" ;
  rdfs:domain cim:UnitSymbol ;
  skos:definition "Conductance in siemens."@en .

cim:UnitSymbol.SPerm a owl:NamedIndividual, owl:Thing ;
  rdfs:label "SPerm "@en ;
  eq:isenum "True" ;
  rdfs:domain cim:UnitSymbol ;
  skos:definition "Conductance per length (F/m)."@en .

cim:UnitSymbol.Sv a owl:NamedIndividual, owl:Thing ;
  rdfs:label "Sv "@en ;
  eq:isenum "True" ;
  rdfs:domain cim:UnitSymbol ;
  skos:definition "Dose equivalent in sieverts (J/kg)."@en .

cim:UnitSymbol.T a owl:NamedIndividual, owl:Thing ;
  rdfs:label "T "@en ;
  eq:isenum "True" ;
  rdfs:domain cim:UnitSymbol ;
  skos:definition "Magnetic flux density in teslas (Wb/m2)."@en .

cim:UnitSymbol.V a owl:NamedIndividual, owl:Thing ;
  rdfs:label "V "@en ;
  eq:isenum "True" ;
  rdfs:domain cim:UnitSymbol ;
  skos:definition "Electric potential in volts (W/A)."@en .

cim:UnitSymbol.V2 a owl:NamedIndividual, owl:Thing ;
  rdfs:label "V2 "@en ;
  eq:isenum "True" ;
  rdfs:domain cim:UnitSymbol ;
  skos:definition "Volt squared (W²/A²)."@en .

cim:UnitSymbol.V2h a owl:NamedIndividual, owl:Thing ;
  rdfs:label "V2h "@en ;
  eq:isenum "True" ;
  rdfs:domain cim:UnitSymbol ;
  skos:definition "Volt-squared hour, volt-squared-hours."@en .

cim:UnitSymbol.VA a owl:NamedIndividual, owl:Thing ;
  rdfs:label "VA "@en ;
  eq:isenum "True" ;
  rdfs:domain cim:UnitSymbol ;
  skos:definition "Apparent power in volt amperes. See also real power and reactive power."@en .

cim:UnitSymbol.VAh a owl:NamedIndividual, owl:Thing ;
  rdfs:label "VAh "@en ;
  eq:isenum "True" ;
  rdfs:domain cim:UnitSymbol ;
  skos:definition "Apparent energy in volt ampere hours."@en .

cim:UnitSymbol.VAr a owl:NamedIndividual, owl:Thing ;
  rdfs:label "VAr "@en ;
  eq:isenum "True" ;
  rdfs:domain cim:UnitSymbol ;
  skos:definition """
Reactive power in volt amperes reactive. The “reactive” or “imaginary” component of electrical power (VIsin(phi)). (See also real power and apparent power).
Note: Different meter designs use different methods to arrive at their results. Some meters may compute reactive power as an arithmetic value, while others compute the value vectorially. The data consumer should determine the method in use and the suitability of the measurement for the intended purpose.
\t"""@en .

cim:UnitSymbol.VArh a owl:NamedIndividual, owl:Thing ;
  rdfs:label "VArh "@en ;
  eq:isenum "True" ;
  rdfs:domain cim:UnitSymbol ;
  skos:definition "Reactive energy in volt ampere reactive hours."@en .

cim:UnitSymbol.VPerHz a owl:NamedIndividual, owl:Thing ;
  rdfs:label "VPerHz "@en ;
  eq:isenum "True" ;
  rdfs:domain cim:UnitSymbol ;
  skos:definition "Magnetic flux in volt per hertz."@en .

cim:UnitSymbol.VPerV a owl:NamedIndividual, owl:Thing ;
  rdfs:label "VPerV "@en ;
  eq:isenum "True" ;
  rdfs:domain cim:UnitSymbol ;
  skos:definition "Voltage, ratio of voltages.  Note: Users may need to supply a prefix such as ‘m’ to show rates such as ‘mV/V’."@en .

cim:UnitSymbol.VPerVA a owl:NamedIndividual, owl:Thing ;
  rdfs:label "VPerVA "@en ;
  eq:isenum "True" ;
  rdfs:domain cim:UnitSymbol ;
  skos:definition "Power factor, PF, the ratio of the active power to the apparent power.  Note: The sign convention used for power factor will differ between IEC meters and EEI (ANSI) meters. It is assumed that the data consumers understand the type of meter being used and agree on the sign convention in use at any given utility."@en .

cim:UnitSymbol.VPerVAr a owl:NamedIndividual, owl:Thing ;
  rdfs:label "VPerVAr "@en ;
  eq:isenum "True" ;
  rdfs:domain cim:UnitSymbol ;
  skos:definition "Power factor, PF, the ratio of the active power to the apparent power. Note: The sign convention used for power factor will differ between IEC meters and EEI (ANSI) meters. It is assumed that the data consumers understand the type of meter being used and agree on the sign convention in use at any given utility."@en .

cim:UnitSymbol.VPerm a owl:NamedIndividual, owl:Thing ;
  rdfs:label "VPerm "@en ;
  eq:isenum "True" ;
  rdfs:domain cim:UnitSymbol ;
  skos:definition "Electric field strength, volts per metre."@en .

cim:UnitSymbol.Vh a owl:NamedIndividual, owl:Thing ;
  rdfs:label "Vh "@en ;
  eq:isenum "True" ;
  rdfs:domain cim:UnitSymbol ;
  skos:definition "Volt-hour, Volt hours."@en .

cim:UnitSymbol.Vs a owl:NamedIndividual, owl:Thing ;
  rdfs:label "Vs "@en ;
  eq:isenum "True" ;
  rdfs:domain cim:UnitSymbol ;
  skos:definition "Volt seconds (Ws/A)."@en .

cim:UnitSymbol.W a owl:NamedIndividual, owl:Thing ;
  rdfs:label "W "@en ;
  eq:isenum "True" ;
  rdfs:domain cim:UnitSymbol ;
  skos:definition "Real power in watts (J/s). Electrical power may have real and reactive components. The real portion of electrical power (I&#178;R or VIcos(phi)), is expressed in Watts. See also apparent power and reactive power."@en .

cim:UnitSymbol.WPerA a owl:NamedIndividual, owl:Thing ;
  rdfs:label "WPerA "@en ;
  eq:isenum "True" ;
  rdfs:domain cim:UnitSymbol ;
  skos:definition "Active power per current flow, watts per Ampere."@en .

cim:UnitSymbol.WPerW a owl:NamedIndividual, owl:Thing ;
  rdfs:label "WPerW "@en ;
  eq:isenum "True" ;
  rdfs:domain cim:UnitSymbol ;
  skos:definition "Signal Strength, ratio of power.   Note: Users may need to supply a prefix such as ‘m’ to show rates such as ‘mW/W’."@en .

cim:UnitSymbol.WPerm2 a owl:NamedIndividual, owl:Thing ;
  rdfs:label "WPerm2 "@en ;
  eq:isenum "True" ;
  rdfs:domain cim:UnitSymbol ;
  skos:definition "Heat flux density, irradiance, watts per square metre."@en .

cim:UnitSymbol.WPerm2sr a owl:NamedIndividual, owl:Thing ;
  rdfs:label "WPerm2sr "@en ;
  eq:isenum "True" ;
  rdfs:domain cim:UnitSymbol ;
  skos:definition "Radiance, watts per square metre steradian."@en .

cim:UnitSymbol.WPermK a owl:NamedIndividual, owl:Thing ;
  rdfs:label "WPermK "@en ;
  eq:isenum "True" ;
  rdfs:domain cim:UnitSymbol ;
  skos:definition "Thermal conductivity in watt/metres kelvin."@en .

cim:UnitSymbol.WPers a owl:NamedIndividual, owl:Thing ;
  rdfs:label "WPers "@en ;
  eq:isenum "True" ;
  rdfs:domain cim:UnitSymbol ;
  skos:definition "Ramp rate in watts per second."@en .

cim:UnitSymbol.WPersr a owl:NamedIndividual, owl:Thing ;
  rdfs:label "WPersr "@en ;
  eq:isenum "True" ;
  rdfs:domain cim:UnitSymbol ;
  skos:definition "Radiant intensity, watts per steradian."@en .

cim:UnitSymbol.Wb a owl:NamedIndividual, owl:Thing ;
  rdfs:label "Wb "@en ;
  eq:isenum "True" ;
  rdfs:domain cim:UnitSymbol ;
  skos:definition "Magnetic flux in webers (V·s)."@en .

cim:UnitSymbol.Wh a owl:NamedIndividual, owl:Thing ;
  rdfs:label "Wh "@en ;
  eq:isenum "True" ;
  rdfs:domain cim:UnitSymbol ;
  skos:definition "Real energy in watt hours."@en .

cim:UnitSymbol.anglemin a owl:NamedIndividual, owl:Thing ;
  rdfs:label "anglemin "@en ;
  eq:isenum "True" ;
  rdfs:domain cim:UnitSymbol ;
  skos:definition "Plane angle, minutes."@en .

cim:UnitSymbol.anglesec a owl:NamedIndividual, owl:Thing ;
  rdfs:label "anglesec "@en ;
  eq:isenum "True" ;
  rdfs:domain cim:UnitSymbol ;
  skos:definition "Plane angle, seconds."@en .

cim:UnitSymbol.bar a owl:NamedIndividual, owl:Thing ;
  rdfs:label "bar "@en ;
  eq:isenum "True" ;
  rdfs:domain cim:UnitSymbol ;
  skos:definition "Pressure in bars, (1 bar = 100 kPa)."@en .

cim:UnitSymbol.cd a owl:NamedIndividual, owl:Thing ;
  rdfs:label "cd "@en ;
  eq:isenum "True" ;
  rdfs:domain cim:UnitSymbol ;
  skos:definition "Luminous intensity in candelas."@en .

cim:UnitSymbol.charPers a owl:NamedIndividual, owl:Thing ;
  rdfs:label "charPers "@en ;
  eq:isenum "True" ;
  rdfs:domain cim:UnitSymbol ;
  skos:definition "Data rate (baud) in characters per second."@en .

cim:UnitSymbol.character a owl:NamedIndividual, owl:Thing ;
  rdfs:label "character "@en ;
  eq:isenum "True" ;
  rdfs:domain cim:UnitSymbol ;
  skos:definition "Number of characters."@en .

cim:UnitSymbol.cosPhi a owl:NamedIndividual, owl:Thing ;
  rdfs:label "cosPhi "@en ;
  eq:isenum "True" ;
  rdfs:domain cim:UnitSymbol ;
  skos:definition """
Power factor, dimensionless.
Note 1: This definition of power factor only holds for balanced systems. See the alternative definition under code 153.
Note 2 : Beware of differing sign conventions in use between the IEC and EEI. It is assumed that the data consumer understands the type of meter in use and the sign convention in use by the utility.
\t"""@en .

cim:UnitSymbol.count a owl:NamedIndividual, owl:Thing ;
  rdfs:label "count "@en ;
  eq:isenum "True" ;
  rdfs:domain cim:UnitSymbol ;
  skos:definition "Amount of substance, Counter value."@en .

cim:UnitSymbol.d a owl:NamedIndividual, owl:Thing ;
  rdfs:label "d "@en ;
  eq:isenum "True" ;
  rdfs:domain cim:UnitSymbol ;
  skos:definition "Time in days, day = 24 h = 86400 s."@en .

cim:UnitSymbol.dB a owl:NamedIndividual, owl:Thing ;
  rdfs:label "dB "@en ;
  eq:isenum "True" ;
  rdfs:domain cim:UnitSymbol ;
  skos:definition "Sound pressure level in decibels. Note:  multiplier “d” is included in this unit symbol for compatibility with IEC 61850-7-3."@en .

cim:UnitSymbol.dBm a owl:NamedIndividual, owl:Thing ;
  rdfs:label "dBm "@en ;
  eq:isenum "True" ;
  rdfs:domain cim:UnitSymbol ;
  skos:definition "Power level (logarithmic ratio of signal strength , Bel-mW), normalized to 1mW. Note:  multiplier “d” is included in this unit symbol for compatibility with IEC 61850-7-3."@en .

cim:UnitSymbol.deg a owl:NamedIndividual, owl:Thing ;
  rdfs:label "deg "@en ;
  eq:isenum "True" ;
  rdfs:domain cim:UnitSymbol ;
  skos:definition "Plane angle in degrees."@en .

cim:UnitSymbol.degC a owl:NamedIndividual, owl:Thing ;
  rdfs:label "degC "@en ;
  eq:isenum "True" ;
  rdfs:domain cim:UnitSymbol ;
  skos:definition """
Relative temperature in degrees Celsius.
In the SI unit system the symbol is °C. Electric charge is measured in coulomb that has the unit symbol C. To distinguish degree Celsius from coulomb the symbol used in the UML is degC. The reason for not using °C is that the special character ° is difficult to manage in software.
\t"""@en .

cim:UnitSymbol.ft3 a owl:NamedIndividual, owl:Thing ;
  rdfs:label "ft3 "@en ;
  eq:isenum "True" ;
  rdfs:domain cim:UnitSymbol ;
  skos:definition "Volume, cubic feet."@en .

cim:UnitSymbol.gPerg a owl:NamedIndividual, owl:Thing ;
  rdfs:label "gPerg "@en ;
  eq:isenum "True" ;
  rdfs:domain cim:UnitSymbol ;
  skos:definition "Concentration, The ratio of the mass of a solute divided by the mass of  the solution. Note: Users may need use a prefix such a ‘µ’ to express a quantity such as ‘µg/g’."@en .

cim:UnitSymbol.gal a owl:NamedIndividual, owl:Thing ;
  rdfs:label "gal "@en ;
  eq:isenum "True" ;
  rdfs:domain cim:UnitSymbol ;
  skos:definition "Volume in gallons, US gallon (1 gal = 231 in3 = 128 fl ounce)."@en .

cim:UnitSymbol.h a owl:NamedIndividual, owl:Thing ;
  rdfs:label "h "@en ;
  eq:isenum "True" ;
  rdfs:domain cim:UnitSymbol ;
  skos:definition "Time in hours, hour = 60 min = 3600 s."@en .

cim:UnitSymbol.ha a owl:NamedIndividual, owl:Thing ;
  rdfs:label "ha "@en ;
  eq:isenum "True" ;
  rdfs:domain cim:UnitSymbol ;
  skos:definition "Area, hectares."@en .

cim:UnitSymbol.kat a owl:NamedIndividual, owl:Thing ;
  rdfs:label "kat "@en ;
  eq:isenum "True" ;
  rdfs:domain cim:UnitSymbol ;
  skos:definition "Catalytic activity, katal = mol / s."@en .

cim:UnitSymbol.katPerm3 a owl:NamedIndividual, owl:Thing ;
  rdfs:label "katPerm3 "@en ;
  eq:isenum "True" ;
  rdfs:domain cim:UnitSymbol ;
  skos:definition "Catalytic activity concentration, katals per cubic metre."@en .

cim:UnitSymbol.kg a owl:NamedIndividual, owl:Thing ;
  rdfs:label "kg "@en ;
  eq:isenum "True" ;
  rdfs:domain cim:UnitSymbol ;
  skos:definition "Mass in kilograms.  Note: multiplier “k” is included in this unit symbol for compatibility with IEC 61850-7-3."@en .

cim:UnitSymbol.kgPerJ a owl:NamedIndividual, owl:Thing ;
  rdfs:label "kgPerJ "@en ;
  eq:isenum "True" ;
  rdfs:domain cim:UnitSymbol ;
  skos:definition "Weight per energy in kilograms per joule (kg/J). Note: multiplier “k” is included in this unit symbol for compatibility with IEC 61850-7-3."@en .

cim:UnitSymbol.kgPerm3 a owl:NamedIndividual, owl:Thing ;
  rdfs:label "kgPerm3 "@en ;
  eq:isenum "True" ;
  rdfs:domain cim:UnitSymbol ;
  skos:definition "Density in kilogram/cubic metres (kg/m³). Note: multiplier “k” is included in this unit symbol for compatibility with IEC 61850-7-3."@en .

cim:UnitSymbol.kgm a owl:NamedIndividual, owl:Thing ;
  rdfs:label "kgm "@en ;
  eq:isenum "True" ;
  rdfs:domain cim:UnitSymbol ;
  skos:definition "Moment of mass in kilogram metres (kg·m) (first moment of mass). Note: multiplier “k” is included in this unit symbol for compatibility with IEC 61850-7-3."@en .

cim:UnitSymbol.kgm2 a owl:NamedIndividual, owl:Thing ;
  rdfs:label "kgm2 "@en ;
  eq:isenum "True" ;
  rdfs:domain cim:UnitSymbol ;
  skos:definition "Moment of mass in kilogram square metres (kg·m²) (Second moment of mass, commonly called the moment of inertia). Note: multiplier “k” is included in this unit symbol for compatibility with IEC 61850-7-3."@en .

cim:UnitSymbol.kn a owl:NamedIndividual, owl:Thing ;
  rdfs:label "kn "@en ;
  eq:isenum "True" ;
  rdfs:domain cim:UnitSymbol ;
  skos:definition "Speed, knots (1 kn = 1852/3600) m/s."@en .

cim:UnitSymbol.l a owl:NamedIndividual, owl:Thing ;
  rdfs:label "l "@en ;
  eq:isenum "True" ;
  rdfs:domain cim:UnitSymbol ;
  skos:definition "Volume in litres, litre = dm3 = m3/1000."@en .

cim:UnitSymbol.lPerh a owl:NamedIndividual, owl:Thing ;
  rdfs:label "lPerh "@en ;
  eq:isenum "True" ;
  rdfs:domain cim:UnitSymbol ;
  skos:definition "Volumetric flow rate, litres per hour."@en .

cim:UnitSymbol.lPerl a owl:NamedIndividual, owl:Thing ;
  rdfs:label "lPerl "@en ;
  eq:isenum "True" ;
  rdfs:domain cim:UnitSymbol ;
  skos:definition "Concentration, The ratio of the volume of a solute divided by the volume of  the solution. Note: Users may need use a prefix such a ‘µ’ to express a quantity such as ‘µL/L’."@en .

cim:UnitSymbol.lPers a owl:NamedIndividual, owl:Thing ;
  rdfs:label "lPers "@en ;
  eq:isenum "True" ;
  rdfs:domain cim:UnitSymbol ;
  skos:definition "Volumetric flow rate in litres per second."@en .

cim:UnitSymbol.lm a owl:NamedIndividual, owl:Thing ;
  rdfs:label "lm "@en ;
  eq:isenum "True" ;
  rdfs:domain cim:UnitSymbol ;
  skos:definition "Luminous flux in lumens (cd·sr)."@en .

cim:UnitSymbol.lx a owl:NamedIndividual, owl:Thing ;
  rdfs:label "lx "@en ;
  eq:isenum "True" ;
  rdfs:domain cim:UnitSymbol ;
  skos:definition "Illuminance in lux (lm/m²)."@en .

cim:UnitSymbol.m a owl:NamedIndividual, owl:Thing ;
  rdfs:label "m "@en ;
  eq:isenum "True" ;
  rdfs:domain cim:UnitSymbol ;
  skos:definition "Length in metres."@en .

cim:UnitSymbol.m2 a owl:NamedIndividual, owl:Thing ;
  rdfs:label "m2 "@en ;
  eq:isenum "True" ;
  rdfs:domain cim:UnitSymbol ;
  skos:definition "Area in square metres (m²)."@en .

cim:UnitSymbol.m2Pers a owl:NamedIndividual, owl:Thing ;
  rdfs:label "m2Pers "@en ;
  eq:isenum "True" ;
  rdfs:domain cim:UnitSymbol ;
  skos:definition "Viscosity in square metres / second (m²/s)."@en .

cim:UnitSymbol.m3 a owl:NamedIndividual, owl:Thing ;
  rdfs:label "m3 "@en ;
  eq:isenum "True" ;
  rdfs:domain cim:UnitSymbol ;
  skos:definition "Volume in cubic metres (m³)."@en .

cim:UnitSymbol.m3Compensated a owl:NamedIndividual, owl:Thing ;
  rdfs:label "m3Compensated "@en ;
  eq:isenum "True" ;
  rdfs:domain cim:UnitSymbol ;
  skos:definition "Volume, cubic metres, with the value compensated for weather effects."@en .

cim:UnitSymbol.m3Perh a owl:NamedIndividual, owl:Thing ;
  rdfs:label "m3Perh "@en ;
  eq:isenum "True" ;
  rdfs:domain cim:UnitSymbol ;
  skos:definition "Volumetric flow rate, cubic metres per hour."@en .

cim:UnitSymbol.m3Perkg a owl:NamedIndividual, owl:Thing ;
  rdfs:label "m3Perkg "@en ;
  eq:isenum "True" ;
  rdfs:domain cim:UnitSymbol ;
  skos:definition "Specific volume, cubic metres per kilogram, v."@en .

cim:UnitSymbol.m3Pers a owl:NamedIndividual, owl:Thing ;
  rdfs:label "m3Pers "@en ;
  eq:isenum "True" ;
  rdfs:domain cim:UnitSymbol ;
  skos:definition "Volumetric flow rate in cubic metres per second (m³/s)."@en .

cim:UnitSymbol.m3Uncompensated a owl:NamedIndividual, owl:Thing ;
  rdfs:label "m3Uncompensated "@en ;
  eq:isenum "True" ;
  rdfs:domain cim:UnitSymbol ;
  skos:definition "Volume, cubic metres, with the value uncompensated for weather effects."@en .

cim:UnitSymbol.mPerm3 a owl:NamedIndividual, owl:Thing ;
  rdfs:label "mPerm3 "@en ;
  eq:isenum "True" ;
  rdfs:domain cim:UnitSymbol ;
  skos:definition "Fuel efficiency in metres per cubic metres (m/m³)."@en .

cim:UnitSymbol.mPers a owl:NamedIndividual, owl:Thing ;
  rdfs:label "mPers "@en ;
  eq:isenum "True" ;
  rdfs:domain cim:UnitSymbol ;
  skos:definition "Velocity in metres per second (m/s)."@en .

cim:UnitSymbol.mPers2 a owl:NamedIndividual, owl:Thing ;
  rdfs:label "mPers2 "@en ;
  eq:isenum "True" ;
  rdfs:domain cim:UnitSymbol ;
  skos:definition "Acceleration in metres per second squared (m/s²)."@en .

cim:UnitSymbol.min a owl:NamedIndividual, owl:Thing ;
  rdfs:label "min "@en ;
  eq:isenum "True" ;
  rdfs:domain cim:UnitSymbol ;
  skos:definition "Time in minutes, minute  = 60 s."@en .

cim:UnitSymbol.mmHg a owl:NamedIndividual, owl:Thing ;
  rdfs:label "mmHg "@en ;
  eq:isenum "True" ;
  rdfs:domain cim:UnitSymbol ;
  skos:definition "Pressure, millimetres of mercury (1 mmHg is approximately 133.3 Pa)."@en .

cim:UnitSymbol.mol a owl:NamedIndividual, owl:Thing ;
  rdfs:label "mol "@en ;
  eq:isenum "True" ;
  rdfs:domain cim:UnitSymbol ;
  skos:definition "Amount of substance in moles."@en .

cim:UnitSymbol.molPerkg a owl:NamedIndividual, owl:Thing ;
  rdfs:label "molPerkg "@en ;
  eq:isenum "True" ;
  rdfs:domain cim:UnitSymbol ;
  skos:definition "Concentration, Molality, the amount of solute in moles and the amount of solvent in kilograms."@en .

cim:UnitSymbol.molPerm3 a owl:NamedIndividual, owl:Thing ;
  rdfs:label "molPerm3 "@en ;
  eq:isenum "True" ;
  rdfs:domain cim:UnitSymbol ;
  skos:definition "Concentration, The amount of substance concentration, (c), the amount of solvent in moles divided by the volume of solution in m³."@en .

cim:UnitSymbol.molPermol a owl:NamedIndividual, owl:Thing ;
  rdfs:label "molPermol "@en ;
  eq:isenum "True" ;
  rdfs:domain cim:UnitSymbol ;
  skos:definition "Concentration, Molar fraction, the ratio of the molar amount of a solute divided by the molar amount of the solution."@en .

cim:UnitSymbol.none a owl:NamedIndividual, owl:Thing ;
  rdfs:label "none "@en ;
  eq:isenum "True" ;
  rdfs:domain cim:UnitSymbol ;
  skos:definition "Dimension less quantity, e.g. count, per unit, etc."@en .

cim:UnitSymbol.ohm a owl:NamedIndividual, owl:Thing ;
  rdfs:label "ohm "@en ;
  eq:isenum "True" ;
  rdfs:domain cim:UnitSymbol ;
  skos:definition "Electric resistance in ohms (V/A)."@en .

cim:UnitSymbol.ohmPerm a owl:NamedIndividual, owl:Thing ;
  rdfs:label "ohmPerm "@en ;
  eq:isenum "True" ;
  rdfs:domain cim:UnitSymbol ;
  skos:definition "Electric resistance per length in ohms per metre ((V/A)/m)."@en .

cim:UnitSymbol.ohmm a owl:NamedIndividual, owl:Thing ;
  rdfs:label "ohmm "@en ;
  eq:isenum "True" ;
  rdfs:domain cim:UnitSymbol ;
  skos:definition "Resistivity, ohm metres, (rho)."@en .

cim:UnitSymbol.onePerHz a owl:NamedIndividual, owl:Thing ;
  rdfs:label "onePerHz "@en ;
  eq:isenum "True" ;
  rdfs:domain cim:UnitSymbol ;
  skos:definition "Reciprocal of frequency (1/Hz)."@en .

cim:UnitSymbol.onePerm a owl:NamedIndividual, owl:Thing ;
  rdfs:label "onePerm "@en ;
  eq:isenum "True" ;
  rdfs:domain cim:UnitSymbol ;
  skos:definition "Wavenumber, reciprocal metres,  (1/m)."@en .

cim:UnitSymbol.ppm a owl:NamedIndividual, owl:Thing ;
  rdfs:label "ppm "@en ;
  eq:isenum "True" ;
  rdfs:domain cim:UnitSymbol ;
  skos:definition "Concentration in parts per million."@en .

cim:UnitSymbol.rad a owl:NamedIndividual, owl:Thing ;
  rdfs:label "rad "@en ;
  eq:isenum "True" ;
  rdfs:domain cim:UnitSymbol ;
  skos:definition "Plane angle in radians (m/m)."@en .

cim:UnitSymbol.radPers a owl:NamedIndividual, owl:Thing ;
  rdfs:label "radPers "@en ;
  eq:isenum "True" ;
  rdfs:domain cim:UnitSymbol ;
  skos:definition "Angular velocity in radians per second (rad/s)."@en .

cim:UnitSymbol.radPers2 a owl:NamedIndividual, owl:Thing ;
  rdfs:label "radPers2 "@en ;
  eq:isenum "True" ;
  rdfs:domain cim:UnitSymbol ;
  skos:definition "Angular acceleration, radians per second squared."@en .

cim:UnitSymbol.rev a owl:NamedIndividual, owl:Thing ;
  rdfs:label "rev "@en ;
  eq:isenum "True" ;
  rdfs:domain cim:UnitSymbol ;
  skos:definition "Amount of rotation, revolutions."@en .

cim:UnitSymbol.rotPers a owl:NamedIndividual, owl:Thing ;
  rdfs:label "rotPers "@en ;
  eq:isenum "True" ;
  rdfs:domain cim:UnitSymbol ;
  skos:definition "Rotations per second (1/s). See also Hz (1/s)."@en .

cim:UnitSymbol.s a owl:NamedIndividual, owl:Thing ;
  rdfs:label "s "@en ;
  eq:isenum "True" ;
  rdfs:domain cim:UnitSymbol ;
  skos:definition "Time in seconds."@en .

cim:UnitSymbol.sPers a owl:NamedIndividual, owl:Thing ;
  rdfs:label "sPers "@en ;
  eq:isenum "True" ;
  rdfs:domain cim:UnitSymbol ;
  skos:definition "Time, Ratio of time.  Note: Users may need to supply a prefix such as ‘&#181;’ to show rates such as ‘&#181;s/s’."@en .

cim:UnitSymbol.sr a owl:NamedIndividual, owl:Thing ;
  rdfs:label "sr "@en ;
  eq:isenum "True" ;
  rdfs:domain cim:UnitSymbol ;
  skos:definition "Solid angle in steradians (m2/m2)."@en .

cim:UnitSymbol.therm a owl:NamedIndividual, owl:Thing ;
  rdfs:label "therm "@en ;
  eq:isenum "True" ;
  rdfs:domain cim:UnitSymbol ;
  skos:definition "Energy, therms."@en .

cim:UnitSymbol.tonne a owl:NamedIndividual, owl:Thing ;
  rdfs:label "tonne "@en ;
  eq:isenum "True" ;
  rdfs:domain cim:UnitSymbol ;
  skos:definition "Mass in tons, “tonne” or “metric  ton” (1000 kg = 1 Mg)."@en .

cim:WindGenUnitKind.offshore a owl:NamedIndividual, owl:Thing ;
  rdfs:label "offshore "@en ;
  eq:isenum "True" ;
  rdfs:domain cim:WindGenUnitKind ;
  skos:definition "The wind generating unit is located offshore."@en .

cim:WindGenUnitKind.onshore a owl:NamedIndividual, owl:Thing ;
  rdfs:label "onshore "@en ;
  eq:isenum "True" ;
  rdfs:domain cim:WindGenUnitKind ;
  skos:definition "The wind generating unit is located onshore."@en .

cim:WindingConnection.A a owl:NamedIndividual, owl:Thing ;
  rdfs:label "A "@en ;
  eq:isenum "True" ;
  rdfs:domain cim:WindingConnection ;
  skos:definition "Autotransformer common winding."@en .

cim:WindingConnection.D a owl:NamedIndividual, owl:Thing ;
  rdfs:label "D "@en ;
  eq:isenum "True" ;
  rdfs:domain cim:WindingConnection ;
  skos:definition "Delta."@en .

cim:WindingConnection.I a owl:NamedIndividual, owl:Thing ;
  rdfs:label "I "@en ;
  eq:isenum "True" ;
  rdfs:domain cim:WindingConnection ;
  skos:definition "Independent winding, for single-phase connections."@en .

cim:WindingConnection.Y a owl:NamedIndividual, owl:Thing ;
  rdfs:label "Y "@en ;
  eq:isenum "True" ;
  rdfs:domain cim:WindingConnection ;
  skos:definition "Wye."@en .

cim:WindingConnection.Yn a owl:NamedIndividual, owl:Thing ;
  rdfs:label "Yn "@en ;
  eq:isenum "True" ;
  rdfs:domain cim:WindingConnection ;
  skos:definition "Wye, with neutral brought out for grounding."@en .

cim:WindingConnection.Z a owl:NamedIndividual, owl:Thing ;
  rdfs:label "Z "@en ;
  eq:isenum "True" ;
  rdfs:domain cim:WindingConnection ;
  skos:definition "ZigZag."@en .

cim:WindingConnection.Zn a owl:NamedIndividual, owl:Thing ;
  rdfs:label "Zn "@en ;
  eq:isenum "True" ;
  rdfs:domain cim:WindingConnection ;
  skos:definition "ZigZag, with neutral brought out for grounding."@en .

eu:LimitKind.alarmVoltage a owl:NamedIndividual, owl:Thing ;
  rdfs:label "alarmVoltage "@en ;
  eq:isEuropean "True" ;
  eq:isenum "True" ;
  rdfs:domain eu:LimitKind ;
  skos:definition "Voltage alarm."@en .

eu:LimitKind.highVoltage a owl:NamedIndividual, owl:Thing ;
  rdfs:label "highVoltage "@en ;
  eq:isEuropean "True" ;
  eq:isenum "True" ;
  rdfs:domain eu:LimitKind ;
  skos:definition """
Referring to the rating of the equipments, a voltage too high can lead to accelerated ageing or the destruction of the equipment. 
This limit type may or may not have duration.
\t"""@en .

eu:LimitKind.lowVoltage a owl:NamedIndividual, owl:Thing ;
  rdfs:label "lowVoltage "@en ;
  eq:isEuropean "True" ;
  eq:isenum "True" ;
  rdfs:domain eu:LimitKind ;
  skos:definition """
A too low voltage can disturb the normal operation of some protections and transformer equipped with on-load tap changers, electronic power devices or can affect the behaviour of the auxiliaries of generation units.
This limit type may or may not have duration.
\t"""@en .

eu:LimitKind.operationalVoltageLimit a owl:NamedIndividual, owl:Thing ;
  rdfs:label "operationalVoltageLimit "@en ;
  eq:isEuropean "True" ;
  eq:isenum "True" ;
  rdfs:domain eu:LimitKind ;
  skos:definition "Operational voltage limit."@en .

eu:LimitKind.patl a owl:NamedIndividual, owl:Thing ;
  rdfs:label "patl "@en ;
  eq:isEuropean "True" ;
  eq:isenum "True" ;
  rdfs:domain eu:LimitKind ;
  skos:definition """
The Permanent Admissible Transmission Loading (PATL) is the loading in amperes, MVA or MW that can be accepted by a network branch for an unlimited duration without any risk for the material.
The OperationnalLimitType.isInfiniteDuration is set to true. There shall be only one OperationalLimitType of kind PATL per OperationalLimitSet if the PATL is ApparentPowerLimit, ActivePowerLimit, or CurrentLimit for a given Terminal or Equipment.
\t"""@en .

eu:LimitKind.patlt a owl:NamedIndividual, owl:Thing ;
  rdfs:label "patlt "@en ;
  eq:isEuropean "True" ;
  eq:isenum "True" ;
  rdfs:domain eu:LimitKind ;
  skos:definition "Permanent Admissible Transmission Loading Threshold  (PATLT) is a value in engineering units defined for PATL and calculated using a percentage less than 100 % of the PATL type intended to alert operators of an arising condition. The percentage should be given in the name of the OperationalLimitSet. The aceptableDuration is another way to express the severity of the limit."@en .

eu:LimitKind.stability a owl:NamedIndividual, owl:Thing ;
  rdfs:label "stability "@en ;
  eq:isEuropean "True" ;
  eq:isenum "True" ;
  rdfs:domain eu:LimitKind ;
  skos:definition "Stability."@en .

eu:LimitKind.tatl a owl:NamedIndividual, owl:Thing ;
  rdfs:label "tatl "@en ;
  eq:isEuropean "True" ;
  eq:isenum "True" ;
  rdfs:domain eu:LimitKind ;
  skos:definition """
Temporarily Admissible Transmission Loading (TATL) which is the loading in amperes, MVA or MW that can be accepted by a branch for a certain limited duration.
The TATL can be defined in different ways:
<ul>
<li>as a fixed percentage of the PATL for a given time (for example, 115% of the PATL that can be accepted during 15 minutes),</li>
</ul>
<ul>
<li>pairs of TATL type and Duration calculated for each line taking into account its particular configuration and conditions of functioning (for example, it can define a TATL acceptable during 20 minutes and another one acceptable during 10 minutes).</li>
</ul>
Such a definition of TATL can depend on the initial operating conditions of the network element (sag situation of a line).
The duration attribute can be used to define several TATL limit types. Hence multiple TATL limit values may exist having different durations.
\t"""@en .

eu:LimitKind.tc a owl:NamedIndividual, owl:Thing ;
  rdfs:label "tc "@en ;
  eq:isEuropean "True" ;
  eq:isenum "True" ;
  rdfs:domain eu:LimitKind ;
  skos:definition """
Tripping Current (TC) is the ultimate intensity without any delay. It is defined as the threshold the line will trip without any possible remedial actions.
The tripping of the network element is ordered by protections against short circuits or by overload protections, but in any case, the activation delay of these protections is not compatible with the reaction delay of an operator (less than one minute).
The duration is always zero if the OperationalLimitType.acceptableDuration is exchanged. Only one limit value exists for the TC type.
\t"""@en .

eu:LimitKind.tct a owl:NamedIndividual, owl:Thing ;
  rdfs:label "tct "@en ;
  eq:isEuropean "True" ;
  eq:isenum "True" ;
  rdfs:domain eu:LimitKind ;
  skos:definition "Tripping Current Threshold  (TCT) is a value in engineering units defined for TC and calculated using a percentage less than 100 % of the TC type intended to alert operators of an arising condition. The percentage should be given in the name of the OperationalLimitSet. The aceptableDuration is another way to express the severity of the limit."@en .

eu:LimitKind.warningVoltage a owl:NamedIndividual, owl:Thing ;
  rdfs:label "warningVoltage "@en ;
  eq:isEuropean "True" ;
  eq:isenum "True" ;
  rdfs:domain eu:LimitKind ;
  skos:definition "Voltage warning."@en .

eq:Package_CoreEquipmentProfile a eq:Package ;
  rdfs:comment """
This is the IEC 61970-452 core equipment profile.

\t"""@en .


