<?xml version="1.0" encoding="UTF-8"?>
<rdf:RDF
xmlns:cim="http://iec.ch/TC57/CIM100#"
xmlns:cims="http://iec.ch/TC57/1999/rdf-schema-extensions-19990926#"
xmlns:dc="http://purl.org/dc/elements/1.1/"
xmlns:dcat="http://www.w3.org/ns/dcat#"
xmlns:dct="http://purl.org/dc/terms/"
xmlns:eu="http://iec.ch/TC57/CIM100-European#"
xmlns:owl="http://www.w3.org/2002/07/owl#"
xmlns:prof="http://iec.ch/TC57/ns/CIM/prof-cim#"
xmlns:profcim="http://iec.ch/TC57/ns/CIM/prof-cim#"
xmlns:rdf="http://www.w3.org/1999/02/22-rdf-syntax-ns#"
xmlns:rdfs="http://www.w3.org/2000/01/rdf-schema#"
xmlns:sh="http://www.w3.org/ns/shacl#"
xmlns:skos="http://www.w3.org/2004/02/skos/core#"
xmlns:xsd="http://www.w3.org/2001/XMLSchema#"
xmlns:gl="http://iec.ch/TC57/ns/CIM/GeographicalLocation-EU#"
xml:base ="http://iec.ch/TC57/CIM100"
>
<!--  ********** Header **************** -->
<!-- RDFS header -->
<rdf:Description rdf:about = "http://iec.ch/TC57/ns/CIM/GeographicalLocation-EU#Ontology">
	<dcat:keyword>GL</dcat:keyword>
	<owl:incompatibleWith rdf:resource="http://entsoe.eu/2009/profile1"/>
	<owl:priorVersion rdf:resource="http://entsoe.eu/CIM/GeographicalLocation/2/1"/>
	<dcat:theme xml:lang ="en">vocabulary</dcat:theme>
	<owl:versionIRI rdf:resource="http://iec.ch/TC57/ns/CIM/GeographicalLocation-EU/3.0"/>
	<dct:conformsTo>urn:iso:std:iec:61970-600-2:ed-1</dct:conformsTo>
	<dct:conformsTo>urn:iso:std:iec:61970-301:ed-7:amd1</dct:conformsTo>
	<dct:conformsTo>file://iec61970cim17v40_iec61968cim13v13a_iec62325cim03v17a.eap</dct:conformsTo>
	<dct:conformsTo>urn:iso:std:iec:61970-401:draft:ed-1</dct:conformsTo>
	<dct:conformsTo>urn:iso:std:iec:61970-501:draft:ed-2</dct:conformsTo>
	<owl:versionInfo xml:lang ="en">3.0.0</owl:versionInfo>
	<dct:creator xml:lang ="en">ENTSO-E CIM EG</dct:creator>
	<dct:description xml:lang ="en">This vocabulary is describing the geographical location profile from IEC 61970-600-2.</dct:description>
	<dct:identifier>urn:uuid:862c1230-be19-4a01-bd6f-1a6c03d213ff</dct:identifier>
	<dct:issued rdf:datatype="http://www.w3.org/2001/XMLSchema#dateTime">2021-01-27T15:33:28Z</dct:issued>
	<dct:language>en-GB</dct:language>
	<dct:modified rdf:datatype="http://www.w3.org/2001/XMLSchema#date">2020-10-12</dct:modified>
	<dct:publisher xml:lang ="en">ENTSO-E</dct:publisher>
	<dct:rights xml:lang ="en">Copyright</dct:rights>
	<dct:rightsHolder xml:lang ="en">ENTSO-E</dct:rightsHolder>
	<dct:title xml:lang ="en">Geographical Location Vocabulary</dct:title>
<rdf:type rdf:resource="http://www.w3.org/2002/07/owl#Ontology"/>
</rdf:Description >
<!-- ******************************** -->
<rdf:Description rdf:about="http://iec.ch/TC57/ns/CIM/GeographicalLocation-EU#Package" >
	<rdf:type rdf:resource="http://www.w3.org/2002/07/owl#AnnotationProperty" />
	<rdfs:label xml:lang="en">MOF Package</rdfs:label>
	<rdfs:comment xml:lang="en">Declaration that this is a MOF Package.</rdfs:comment>
	<rdfs:domain rdf:resource="http://www.w3.org/2000/01/rdf-schema#Class" />
	<rdfs:range rdf:resource="http://www.w3.org/2001/XMLSchema#string" />
</rdf:Description>
<rdf:Description rdf:about = "http://iec.ch/TC57/ns/CIM/GeographicalLocation-EU#Enumeration" >
	<rdfs:comment xml:lang = "en" > An abstract superclass for all Enumerators. </rdfs:comment>
	<rdfs:label xml:lang= "en"> enumeration </rdfs:label>
	<rdf:type rdf:resource="http://www.w3.org/2002/07/owl#Class" />
	<gl:isAbstract>true</gl:isAbstract>
</rdf:Description>
<rdf:Description rdf:about="http://iec.ch/TC57/ns/CIM/GeographicalLocation-EU#isAbstract">
	<rdf:type rdf:resource="http://www.w3.org/2002/07/owl#AnnotationProperty"/>
	<rdfs:label xml:lang="en">is abstract</rdfs:label>
	<rdfs:comment xml:lang="en">Flag indicating whether the class is permitted to have any direct instances.</rdfs:comment>
	<rdfs:domain rdf:resource="http://www.w3.org/2000/01/rdf-schema#Class" />
	<rdfs:range rdf:resource="http://www.w3.org/2001/XMLSchema#boolean" />
</rdf:Description > 
<rdf:Description rdf:about="http://iec.ch/TC57/ns/CIM/GeographicalLocation-EU#isenum">
	<rdf:type rdf:resource="http://www.w3.org/2002/07/owl#AnnotationProperty"/>
	<rdfs:label xml:lang="en">isenum	</rdfs:label>
	<rdfs:comment xml:lang="en">Flag indicating whether the enumerated literal is an enum.</rdfs:comment>
	<rdfs:domain rdf:resource="http://www.w3.org/2000/01/rdf-schema#Property" />
	<rdfs:range rdf:resource="http://www.w3.org/2001/XMLSchema#boolean" />
</rdf:Description>
<rdf:Description rdf:about= "http://iec.ch/TC57/ns/CIM/GeographicalLocation-EU#isUnique" >
	<rdf:type rdf:resource="http://www.w3.org/2002/07/owl#AnnotationProperty" />
	<rdfs:label xml:lang="en">is unique </rdfs:label>
	<rdfs:comment xml:lang="en"> Flag indicating whether the property for a specific object can contain the same value more than once.</rdfs:comment>
	<rdfs:domain rdf:resource="http://www.w3.org/2000/01/rdf-schema#Property" />
	<rdfs:range rdf:resource="http://www.w3.org/2001/XMLSchema#boolean" />
</rdf:Description > 
<rdf:Description rdf:about= "http://iec.ch/TC57/ns/CIM/GeographicalLocation-EU#isFixed" >
	<rdf:type rdf:resource="http://www.w3.org/2002/07/owl#AnnotationProperty" />
	<rdfs:label xml:lang="en">is fixed property</rdfs:label>
	<rdfs:comment xml:lang="en"> Flag indicating whether the property for a specific object can be updated.</rdfs:comment>
	<rdfs:domain rdf:resource="http://www.w3.org/2000/01/rdf-schema#Property" />
	<rdfs:range rdf:resource="http://www.w3.org/2001/XMLSchema#boolean" />
</rdf:Description> 
<rdf:Description rdf:about= "http://iec.ch/TC57/ns/CIM/GeographicalLocation-EU#isConst" >
	<rdf:type rdf:resource="http://www.w3.org/2002/07/owl#AnnotationProperty" />
	<rdfs:label xml:lang="en">is fixed property</rdfs:label>
	<rdfs:comment xml:lang="en"> Flag indicating whether the property for a specific object can be updated.</rdfs:comment>
	<rdfs:domain rdf:resource="http://www.w3.org/2000/01/rdf-schema#Property" />
	<rdfs:range rdf:resource="http://www.w3.org/2001/XMLSchema#boolean" />
</rdf:Description > 
<rdf:Description rdf:about="http://iec.ch/TC57/ns/CIM/GeographicalLocation-EU#Package_GeographicalLocationProfile">
	<rdf:type rdf:resource="http://iec.ch/TC57/ns/CIM/GeographicalLocation-EU#Package"/>
	<rdfs:comment  xml:lang="en">This is the  geographical location profile as in 61968-13.</rdfs:comment>
</rdf:Description>
<rdf:Description rdf:about="#IdentifiedObject">
	<rdfs:label xml:lang="en">IdentifiedObject</rdfs:label>
	<rdf:type rdf:resource="http://www.w3.org/2002/07/owl#Class"/>
	<skos:definition  xml:lang="en">This is a root class to provide common identification for all classes needing identification and naming attributes.</skos:definition>
	<gl:Package>Package_GeographicalLocationProfile</gl:Package>
	<gl:isAbstract>True</gl:isAbstract>
</rdf:Description>
<rdf:Description rdf:about="#IdentifiedObject.mRID">
	<rdf:type rdf:resource = "http://www.w3.org/2002/07/owl#DatatypeProperty" />
	<rdfs:label xml:lang="en">mRID</rdfs:label>
	<rdfs:domain rdf:resource="#IdentifiedObject"/>
	<rdfs:range rdf:resource = "http://www.w3.org/2001/XMLSchema#string" />
	<skos:definition  xml:lang="en">
Master resource identifier issued by a model authority. The mRID is unique within an exchange context. Global uniqueness is easily achieved by using a UUID, as specified in RFC 4122, for the mRID. The use of UUID is strongly recommended.
For CIMXML data files in RDF syntax conforming to IEC 61970-552, the mRID is mapped to rdf:ID or rdf:about attributes that identify CIM object elements.
	</skos:definition>
</rdf:Description>
<rdf:Description rdf:about="#String">
	<rdfs:label xml:lang="en">String</rdfs:label>
	<rdf:type rdf:resource="http://www.w3.org/2002/07/owl#Class"/>
	<skos:definition  xml:lang="en">A string consisting of a sequence of characters. The character encoding is UTF-8. The string length is unspecified and unlimited.</skos:definition>
	<gl:isPrimitive>True</gl:isPrimitive>
	<gl:Package>Package_GeographicalLocationProfile</gl:Package>
</rdf:Description>
<rdf:Description rdf:about="#IdentifiedObject.name">
	<rdf:type rdf:resource = "http://www.w3.org/2002/07/owl#DatatypeProperty" />
	<rdfs:label xml:lang="en">name</rdfs:label>
	<rdfs:domain rdf:resource="#IdentifiedObject"/>
	<rdfs:range rdf:resource = "http://www.w3.org/2001/XMLSchema#string" />
	<rdf:type rdf:resource = "http://www.w3.org/2002/07/owl#FunctionalProperty" />
	<skos:definition  xml:lang="en">
The name is any free human readable and possibly non unique text naming the object.

	</skos:definition>
</rdf:Description>
<rdf:Description rdf:about="#ServiceLocation">
	<rdfs:label xml:lang="en">ServiceLocation</rdfs:label>
	<rdf:type rdf:resource="http://www.w3.org/2002/07/owl#Class"/>
	<rdfs:subClassOf rdf:resource="#WorkLocation"/>
	<skos:definition  xml:lang="en">A real estate location, commonly referred to as premises.</skos:definition>
	<gl:Package>Package_GeographicalLocationProfile</gl:Package>
</rdf:Description>
<rdf:Description rdf:about="#WorkLocation">
	<rdfs:label xml:lang="en">WorkLocation</rdfs:label>
	<rdf:type rdf:resource="http://www.w3.org/2002/07/owl#Class"/>
	<rdfs:subClassOf rdf:resource="#Location"/>
	<skos:definition  xml:lang="en">Information about a particular location for various forms of work.</skos:definition>
	<gl:Package>Package_GeographicalLocationProfile</gl:Package>
	<gl:isAbstract>True</gl:isAbstract>
</rdf:Description>
<rdf:Description rdf:about="#CoordinateSystem">
	<rdfs:label xml:lang="en">CoordinateSystem</rdfs:label>
	<rdf:type rdf:resource="http://www.w3.org/2002/07/owl#Class"/>
	<rdfs:subClassOf rdf:resource="#IdentifiedObject"/>
	<skos:definition  xml:lang="en">
Coordinate reference system.

	</skos:definition>
	<gl:Package>Package_GeographicalLocationProfile</gl:Package>
</rdf:Description>
<rdf:Description rdf:about="#CoordinateSystem.crsUrn">
	<rdf:type rdf:resource = "http://www.w3.org/2002/07/owl#DatatypeProperty" />
	<rdfs:label xml:lang="en">crsUrn</rdfs:label>
	<rdfs:domain rdf:resource="#CoordinateSystem"/>
	<rdfs:range rdf:resource = "http://www.w3.org/2001/XMLSchema#string" />
	<skos:definition  xml:lang="en">
A Uniform Resource Name (URN) for the coordinate reference system (crs) used to define &apos;Location.PositionPoints&apos;.
An example would be the European Petroleum Survey Group (EPSG) code for a coordinate reference system, defined in URN under the Open Geospatial Consortium (OGC) namespace as: urn:ogc:def:crs:EPSG::XXXX, where XXXX is an EPSG code (a full list of codes can be found at the EPSG Registry web site http://www.epsg-registry.org/). To define the coordinate system as being WGS84 (latitude, longitude) using an EPSG OGC, this attribute would be urn:ogc:def:crs:EPSG::4236.
A profile should limit this code to a set of allowed URNs agreed to by all sending and receiving parties.
	</skos:definition>
</rdf:Description>
<rdf:Description rdf:about = "#Location.CoordinateSystem" >
	<rdf:type rdf:resource = "http://www.w3.org/2002/07/owl#ObjectProperty" />
	<rdfs:label xml:lang="en">CoordinateSystem</rdfs:label>
	<skos:definition  xml:lang="en">Coordinate system used to describe position points of this location.</skos:definition>
	<rdfs:domain rdf:resource="#Location"/>
	<rdfs:range rdf:resource="#CoordinateSystem"/>
	<owl:inverseOf rdf:resource="#CoordinateSystem.Locations"/>
</rdf:Description >
<rdf:Description rdf:about = "#CoordinateSystem.Locations" >
	<rdf:type rdf:resource = "http://www.w3.org/2002/07/owl#ObjectProperty" />
	<rdfs:label xml:lang="en">Locations</rdfs:label>
	<skos:definition  xml:lang="en">All locations described with position points in this coordinate system.</skos:definition>
	<rdfs:domain rdf:resource="#CoordinateSystem"/>
	<rdfs:range rdf:resource="#Location"/>
	<owl:inverseOf rdf:resource="#Location.CoordinateSystem"/>
</rdf:Description >
<rdf:Description rdf:about="#Location">
	<rdfs:label xml:lang="en">Location</rdfs:label>
	<rdf:type rdf:resource="http://www.w3.org/2002/07/owl#Class"/>
	<rdfs:subClassOf rdf:resource="#IdentifiedObject"/>
	<skos:definition  xml:lang="en">
The place, scene, or point of something where someone or something has been, is, and/or will be at a given moment in time. It can be defined with one or more position points (coordinates) in a given coordinate system.

	</skos:definition>
	<gl:Package>Package_GeographicalLocationProfile</gl:Package>
</rdf:Description>
<rdf:Description rdf:about="#Location.mainAddress">
	<rdf:type rdf:resource = "http://www.w3.org/2002/07/owl#DatatypeProperty" />
	<rdfs:label xml:lang="en">mainAddress</rdfs:label>
	<rdfs:domain rdf:resource="#Location"/>
	<rdfs:range rdf:resource = "#StreetAddress" />
	<rdf:type rdf:resource = "http://www.w3.org/2002/07/owl#FunctionalProperty" />
	<skos:definition  xml:lang="en">Main address of the location.</skos:definition>
</rdf:Description>
<rdf:Description rdf:about="#StreetAddress">
	<rdfs:label xml:lang="en">StreetAddress</rdfs:label>
	<rdf:type rdf:resource="http://www.w3.org/2002/07/owl#Class"/>
	<skos:definition  xml:lang="en">General purpose street and postal address information.</skos:definition>
	<gl:isCompound>True</gl:isCompound>
	<gl:Package>Package_GeographicalLocationProfile</gl:Package>
</rdf:Description>
<rdf:Description rdf:about="#StreetAddress.streetDetail">
	<rdf:type rdf:resource = "http://www.w3.org/2002/07/owl#DatatypeProperty" />
	<rdfs:label xml:lang="en">streetDetail</rdfs:label>
	<rdfs:domain rdf:resource="#StreetAddress"/>
	<rdfs:range rdf:resource = "#StreetDetail" />
	<rdf:type rdf:resource = "http://www.w3.org/2002/07/owl#FunctionalProperty" />
	<skos:definition  xml:lang="en">Street detail.</skos:definition>
</rdf:Description>
<rdf:Description rdf:about="#StreetDetail">
	<rdfs:label xml:lang="en">StreetDetail</rdfs:label>
	<rdf:type rdf:resource="http://www.w3.org/2002/07/owl#Class"/>
	<skos:definition  xml:lang="en">
Street details, in the context of address.

	</skos:definition>
	<gl:isCompound>True</gl:isCompound>
	<gl:Package>Package_GeographicalLocationProfile</gl:Package>
</rdf:Description>
<rdf:Description rdf:about="#StreetDetail.number">
	<rdf:type rdf:resource = "http://www.w3.org/2002/07/owl#DatatypeProperty" />
	<rdfs:label xml:lang="en">number</rdfs:label>
	<rdfs:domain rdf:resource="#StreetDetail"/>
	<rdfs:range rdf:resource = "http://www.w3.org/2001/XMLSchema#string" />
	<rdf:type rdf:resource = "http://www.w3.org/2002/07/owl#FunctionalProperty" />
	<skos:definition  xml:lang="en">Designator of the specific location on the street.</skos:definition>
</rdf:Description>
<rdf:Description rdf:about="#StreetDetail.name">
	<rdf:type rdf:resource = "http://www.w3.org/2002/07/owl#DatatypeProperty" />
	<rdfs:label xml:lang="en">name</rdfs:label>
	<rdfs:domain rdf:resource="#StreetDetail"/>
	<rdfs:range rdf:resource = "http://www.w3.org/2001/XMLSchema#string" />
	<rdf:type rdf:resource = "http://www.w3.org/2002/07/owl#FunctionalProperty" />
	<skos:definition  xml:lang="en">Name of the street.</skos:definition>
</rdf:Description>
<rdf:Description rdf:about="#StreetDetail.suffix">
	<rdf:type rdf:resource = "http://www.w3.org/2002/07/owl#DatatypeProperty" />
	<rdfs:label xml:lang="en">suffix</rdfs:label>
	<rdfs:domain rdf:resource="#StreetDetail"/>
	<rdfs:range rdf:resource = "http://www.w3.org/2001/XMLSchema#string" />
	<rdf:type rdf:resource = "http://www.w3.org/2002/07/owl#FunctionalProperty" />
	<skos:definition  xml:lang="en">Suffix to the street name. For example: North, South, East, West.</skos:definition>
</rdf:Description>
<rdf:Description rdf:about="#StreetDetail.prefix">
	<rdf:type rdf:resource = "http://www.w3.org/2002/07/owl#DatatypeProperty" />
	<rdfs:label xml:lang="en">prefix</rdfs:label>
	<rdfs:domain rdf:resource="#StreetDetail"/>
	<rdfs:range rdf:resource = "http://www.w3.org/2001/XMLSchema#string" />
	<rdf:type rdf:resource = "http://www.w3.org/2002/07/owl#FunctionalProperty" />
	<skos:definition  xml:lang="en">Prefix to the street name. For example: North, South, East, West.</skos:definition>
</rdf:Description>
<rdf:Description rdf:about="#StreetDetail.type">
	<rdf:type rdf:resource = "http://www.w3.org/2002/07/owl#DatatypeProperty" />
	<rdfs:label xml:lang="en">type</rdfs:label>
	<rdfs:domain rdf:resource="#StreetDetail"/>
	<rdfs:range rdf:resource = "http://www.w3.org/2001/XMLSchema#string" />
	<rdf:type rdf:resource = "http://www.w3.org/2002/07/owl#FunctionalProperty" />
	<skos:definition  xml:lang="en">Type of street. Examples include: street, circle, boulevard, avenue, road, drive, etc.</skos:definition>
</rdf:Description>
<rdf:Description rdf:about="#StreetDetail.code">
	<rdf:type rdf:resource = "http://www.w3.org/2002/07/owl#DatatypeProperty" />
	<rdfs:label xml:lang="en">code</rdfs:label>
	<rdfs:domain rdf:resource="#StreetDetail"/>
	<rdfs:range rdf:resource = "http://www.w3.org/2001/XMLSchema#string" />
	<rdf:type rdf:resource = "http://www.w3.org/2002/07/owl#FunctionalProperty" />
	<skos:definition  xml:lang="en">(if applicable) Utilities often make use of external reference systems, such as those of the town-planner&apos;s department or surveyor general&apos;s mapping system, that allocate global reference codes to streets.</skos:definition>
</rdf:Description>
<rdf:Description rdf:about="#StreetDetail.buildingName">
	<rdf:type rdf:resource = "http://www.w3.org/2002/07/owl#DatatypeProperty" />
	<rdfs:label xml:lang="en">buildingName</rdfs:label>
	<rdfs:domain rdf:resource="#StreetDetail"/>
	<rdfs:range rdf:resource = "http://www.w3.org/2001/XMLSchema#string" />
	<rdf:type rdf:resource = "http://www.w3.org/2002/07/owl#FunctionalProperty" />
	<skos:definition  xml:lang="en">(if applicable) In certain cases the physical location of the place of interest does not have a direct point of entry from the street, but may be located inside a larger structure such as a building, complex, office block, apartment, etc.</skos:definition>
</rdf:Description>
<rdf:Description rdf:about="#StreetDetail.suiteNumber">
	<rdf:type rdf:resource = "http://www.w3.org/2002/07/owl#DatatypeProperty" />
	<rdfs:label xml:lang="en">suiteNumber</rdfs:label>
	<rdfs:domain rdf:resource="#StreetDetail"/>
	<rdfs:range rdf:resource = "http://www.w3.org/2001/XMLSchema#string" />
	<rdf:type rdf:resource = "http://www.w3.org/2002/07/owl#FunctionalProperty" />
	<skos:definition  xml:lang="en">Number of the apartment or suite.</skos:definition>
</rdf:Description>
<rdf:Description rdf:about="#StreetDetail.addressGeneral">
	<rdf:type rdf:resource = "http://www.w3.org/2002/07/owl#DatatypeProperty" />
	<rdfs:label xml:lang="en">addressGeneral</rdfs:label>
	<rdfs:domain rdf:resource="#StreetDetail"/>
	<rdfs:range rdf:resource = "http://www.w3.org/2001/XMLSchema#string" />
	<rdf:type rdf:resource = "http://www.w3.org/2002/07/owl#FunctionalProperty" />
	<skos:definition  xml:lang="en">First line of a free form address or some additional address information (for example a mail stop).</skos:definition>
</rdf:Description>
<rdf:Description rdf:about="#StreetDetail.addressGeneral2">
	<rdf:type rdf:resource = "http://www.w3.org/2002/07/owl#DatatypeProperty" />
	<rdfs:label xml:lang="en">addressGeneral2</rdfs:label>
	<rdfs:domain rdf:resource="#StreetDetail"/>
	<rdfs:range rdf:resource = "http://www.w3.org/2001/XMLSchema#string" />
	<rdf:type rdf:resource = "http://www.w3.org/2002/07/owl#FunctionalProperty" />
	<skos:definition  xml:lang="en">(if applicable) Second line of a free form address.</skos:definition>
</rdf:Description>
<rdf:Description rdf:about="#StreetDetail.addressGeneral3">
	<rdf:type rdf:resource = "http://www.w3.org/2002/07/owl#DatatypeProperty" />
	<rdfs:label xml:lang="en">addressGeneral3</rdfs:label>
	<rdfs:domain rdf:resource="#StreetDetail"/>
	<rdfs:range rdf:resource = "http://www.w3.org/2001/XMLSchema#string" />
	<rdf:type rdf:resource = "http://www.w3.org/2002/07/owl#FunctionalProperty" />
	<skos:definition  xml:lang="en">(if applicable) Third line of a free form address.</skos:definition>
</rdf:Description>
<rdf:Description rdf:about="#StreetDetail.withinTownLimits">
	<rdf:type rdf:resource = "http://www.w3.org/2002/07/owl#DatatypeProperty" />
	<rdfs:label xml:lang="en">withinTownLimits</rdfs:label>
	<rdfs:domain rdf:resource="#StreetDetail"/>
	<rdfs:range rdf:resource = "http://www.w3.org/2001/XMLSchema#boolean" />
	<rdf:type rdf:resource = "http://www.w3.org/2002/07/owl#FunctionalProperty" />
	<skos:definition  xml:lang="en">True if this street is within the legal geographical boundaries of the specified town (default).</skos:definition>
</rdf:Description>
<rdf:Description rdf:about="#Boolean">
	<rdfs:label xml:lang="en">Boolean</rdfs:label>
	<rdf:type rdf:resource="http://www.w3.org/2002/07/owl#Class"/>
	<skos:definition  xml:lang="en">
A type with the value space &quot;true&quot; and &quot;false&quot;.

	</skos:definition>
	<gl:isPrimitive>True</gl:isPrimitive>
	<gl:Package>Package_GeographicalLocationProfile</gl:Package>
</rdf:Description>
<rdf:Description rdf:about="#StreetDetail.floorIdentification">
	<rdf:type rdf:resource = "http://www.w3.org/2002/07/owl#DatatypeProperty" />
	<rdfs:label xml:lang="en">floorIdentification</rdfs:label>
	<rdfs:domain rdf:resource="#StreetDetail"/>
	<rdfs:range rdf:resource = "http://www.w3.org/2001/XMLSchema#string" />
	<rdf:type rdf:resource = "http://www.w3.org/2002/07/owl#FunctionalProperty" />
	<skos:definition  xml:lang="en">The identification by name or number, expressed as text, of the floor in the building as part of this address.</skos:definition>
</rdf:Description>
<rdf:Description rdf:about="#StreetAddress.townDetail">
	<rdf:type rdf:resource = "http://www.w3.org/2002/07/owl#DatatypeProperty" />
	<rdfs:label xml:lang="en">townDetail</rdfs:label>
	<rdfs:domain rdf:resource="#StreetAddress"/>
	<rdfs:range rdf:resource = "#TownDetail" />
	<rdf:type rdf:resource = "http://www.w3.org/2002/07/owl#FunctionalProperty" />
	<skos:definition  xml:lang="en">Town detail.</skos:definition>
</rdf:Description>
<rdf:Description rdf:about="#TownDetail">
	<rdfs:label xml:lang="en">TownDetail</rdfs:label>
	<rdf:type rdf:resource="http://www.w3.org/2002/07/owl#Class"/>
	<skos:definition  xml:lang="en">
Town details, in the context of address.

	</skos:definition>
	<gl:isCompound>True</gl:isCompound>
	<gl:Package>Package_GeographicalLocationProfile</gl:Package>
</rdf:Description>
<rdf:Description rdf:about="#TownDetail.code">
	<rdf:type rdf:resource = "http://www.w3.org/2002/07/owl#DatatypeProperty" />
	<rdfs:label xml:lang="en">code</rdfs:label>
	<rdfs:domain rdf:resource="#TownDetail"/>
	<rdfs:range rdf:resource = "http://www.w3.org/2001/XMLSchema#string" />
	<rdf:type rdf:resource = "http://www.w3.org/2002/07/owl#FunctionalProperty" />
	<skos:definition  xml:lang="en">Town code.</skos:definition>
</rdf:Description>
<rdf:Description rdf:about="#TownDetail.section">
	<rdf:type rdf:resource = "http://www.w3.org/2002/07/owl#DatatypeProperty" />
	<rdfs:label xml:lang="en">section</rdfs:label>
	<rdfs:domain rdf:resource="#TownDetail"/>
	<rdfs:range rdf:resource = "http://www.w3.org/2001/XMLSchema#string" />
	<rdf:type rdf:resource = "http://www.w3.org/2002/07/owl#FunctionalProperty" />
	<skos:definition  xml:lang="en">Town section. For example, it is common for there to be 36 sections per township.</skos:definition>
</rdf:Description>
<rdf:Description rdf:about="#TownDetail.name">
	<rdf:type rdf:resource = "http://www.w3.org/2002/07/owl#DatatypeProperty" />
	<rdfs:label xml:lang="en">name</rdfs:label>
	<rdfs:domain rdf:resource="#TownDetail"/>
	<rdfs:range rdf:resource = "http://www.w3.org/2001/XMLSchema#string" />
	<rdf:type rdf:resource = "http://www.w3.org/2002/07/owl#FunctionalProperty" />
	<skos:definition  xml:lang="en">Town name.</skos:definition>
</rdf:Description>
<rdf:Description rdf:about="#TownDetail.stateOrProvince">
	<rdf:type rdf:resource = "http://www.w3.org/2002/07/owl#DatatypeProperty" />
	<rdfs:label xml:lang="en">stateOrProvince</rdfs:label>
	<rdfs:domain rdf:resource="#TownDetail"/>
	<rdfs:range rdf:resource = "http://www.w3.org/2001/XMLSchema#string" />
	<rdf:type rdf:resource = "http://www.w3.org/2002/07/owl#FunctionalProperty" />
	<skos:definition  xml:lang="en">Name of the state or province.</skos:definition>
</rdf:Description>
<rdf:Description rdf:about="#TownDetail.country">
	<rdf:type rdf:resource = "http://www.w3.org/2002/07/owl#DatatypeProperty" />
	<rdfs:label xml:lang="en">country</rdfs:label>
	<rdfs:domain rdf:resource="#TownDetail"/>
	<rdfs:range rdf:resource = "http://www.w3.org/2001/XMLSchema#string" />
	<rdf:type rdf:resource = "http://www.w3.org/2002/07/owl#FunctionalProperty" />
	<skos:definition  xml:lang="en">Name of the country.</skos:definition>
</rdf:Description>
<rdf:Description rdf:about="#StreetAddress.status">
	<rdf:type rdf:resource = "http://www.w3.org/2002/07/owl#DatatypeProperty" />
	<rdfs:label xml:lang="en">status</rdfs:label>
	<rdfs:domain rdf:resource="#StreetAddress"/>
	<rdfs:range rdf:resource = "#Status" />
	<rdf:type rdf:resource = "http://www.w3.org/2002/07/owl#FunctionalProperty" />
	<skos:definition  xml:lang="en">Status of this address.</skos:definition>
</rdf:Description>
<rdf:Description rdf:about="#Status">
	<rdfs:label xml:lang="en">Status</rdfs:label>
	<rdf:type rdf:resource="http://www.w3.org/2002/07/owl#Class"/>
	<skos:definition  xml:lang="en">
Current status information relevant to an entity.

	</skos:definition>
	<gl:isCompound>True</gl:isCompound>
	<gl:Package>Package_GeographicalLocationProfile</gl:Package>
</rdf:Description>
<rdf:Description rdf:about="#Status.value">
	<rdf:type rdf:resource = "http://www.w3.org/2002/07/owl#DatatypeProperty" />
	<rdfs:label xml:lang="en">value</rdfs:label>
	<rdfs:domain rdf:resource="#Status"/>
	<rdfs:range rdf:resource = "http://www.w3.org/2001/XMLSchema#string" />
	<rdf:type rdf:resource = "http://www.w3.org/2002/07/owl#FunctionalProperty" />
	<skos:definition  xml:lang="en">
Status value at &apos;dateTime&apos;; prior status changes may have been kept in instances of activity records associated with the object to which this status applies.

	</skos:definition>
</rdf:Description>
<rdf:Description rdf:about="#Status.dateTime">
	<rdf:type rdf:resource = "http://www.w3.org/2002/07/owl#DatatypeProperty" />
	<rdfs:label xml:lang="en">dateTime</rdfs:label>
	<rdfs:domain rdf:resource="#Status"/>
	<rdfs:range rdf:resource = "http://www.w3.org/2001/XMLSchema#dateTime" />
	<rdf:type rdf:resource = "http://www.w3.org/2002/07/owl#FunctionalProperty" />
	<skos:definition  xml:lang="en">
Date and time for which status &apos;value&apos; applies.

	</skos:definition>
</rdf:Description>
<rdf:Description rdf:about="#DateTime">
	<rdfs:label xml:lang="en">DateTime</rdfs:label>
	<rdf:type rdf:resource="http://www.w3.org/2002/07/owl#Class"/>
	<skos:definition  xml:lang="en">Date and time as &quot;yyyy-mm-ddThh:mm:ss.sss&quot;, which conforms with ISO 8601. UTC time zone is specified as &quot;yyyy-mm-ddThh:mm:ss.sssZ&quot;. A local timezone relative UTC is specified as &quot;yyyy-mm-ddThh:mm:ss.sss-hh:mm&quot;. The second component (shown here as &quot;ss.sss&quot;) could have any number of digits in its fractional part to allow any kind of precision beyond seconds.</skos:definition>
	<gl:isPrimitive>True</gl:isPrimitive>
	<gl:Package>Package_GeographicalLocationProfile</gl:Package>
</rdf:Description>
<rdf:Description rdf:about="#Status.remark">
	<rdf:type rdf:resource = "http://www.w3.org/2002/07/owl#DatatypeProperty" />
	<rdfs:label xml:lang="en">remark</rdfs:label>
	<rdfs:domain rdf:resource="#Status"/>
	<rdfs:range rdf:resource = "http://www.w3.org/2001/XMLSchema#string" />
	<rdf:type rdf:resource = "http://www.w3.org/2002/07/owl#FunctionalProperty" />
	<skos:definition  xml:lang="en">Pertinent information regarding the current &apos;value&apos;, as free form text.</skos:definition>
</rdf:Description>
<rdf:Description rdf:about="#Status.reason">
	<rdf:type rdf:resource = "http://www.w3.org/2002/07/owl#DatatypeProperty" />
	<rdfs:label xml:lang="en">reason</rdfs:label>
	<rdfs:domain rdf:resource="#Status"/>
	<rdfs:range rdf:resource = "http://www.w3.org/2001/XMLSchema#string" />
	<rdf:type rdf:resource = "http://www.w3.org/2002/07/owl#FunctionalProperty" />
	<skos:definition  xml:lang="en">Reason code or explanation for why an object went to the current status &apos;value&apos;.</skos:definition>
</rdf:Description>
<rdf:Description rdf:about="#StreetAddress.postalCode">
	<rdf:type rdf:resource = "http://www.w3.org/2002/07/owl#DatatypeProperty" />
	<rdfs:label xml:lang="en">postalCode</rdfs:label>
	<rdfs:domain rdf:resource="#StreetAddress"/>
	<rdfs:range rdf:resource = "http://www.w3.org/2001/XMLSchema#string" />
	<rdf:type rdf:resource = "http://www.w3.org/2002/07/owl#FunctionalProperty" />
	<skos:definition  xml:lang="en">Postal code for the address.</skos:definition>
</rdf:Description>
<rdf:Description rdf:about="#StreetAddress.poBox">
	<rdf:type rdf:resource = "http://www.w3.org/2002/07/owl#DatatypeProperty" />
	<rdfs:label xml:lang="en">poBox</rdfs:label>
	<rdfs:domain rdf:resource="#StreetAddress"/>
	<rdfs:range rdf:resource = "http://www.w3.org/2001/XMLSchema#string" />
	<rdf:type rdf:resource = "http://www.w3.org/2002/07/owl#FunctionalProperty" />
	<skos:definition  xml:lang="en">Post office box.</skos:definition>
</rdf:Description>
<rdf:Description rdf:about="#StreetAddress.language">
	<rdf:type rdf:resource = "http://www.w3.org/2002/07/owl#DatatypeProperty" />
	<rdfs:label xml:lang="en">language</rdfs:label>
	<rdfs:domain rdf:resource="#StreetAddress"/>
	<rdfs:range rdf:resource = "http://www.w3.org/2001/XMLSchema#string" />
	<rdf:type rdf:resource = "http://www.w3.org/2002/07/owl#FunctionalProperty" />
	<skos:definition  xml:lang="en">The language in which the address is specified, using ISO 639-1 two digit language code.</skos:definition>
</rdf:Description>
<rdf:Description rdf:about = "#Location.PowerSystemResources" >
	<rdf:type rdf:resource = "http://www.w3.org/2002/07/owl#ObjectProperty" />
	<rdfs:label xml:lang="en">PowerSystemResources</rdfs:label>
	<skos:definition  xml:lang="en">All power system resources at this location.</skos:definition>
	<rdfs:domain rdf:resource="#Location"/>
	<rdfs:range rdf:resource="#PowerSystemResource"/>
	<owl:inverseOf rdf:resource="#PowerSystemResource.Location"/>
</rdf:Description >
<rdf:Description rdf:about = "#PowerSystemResource.Location" >
	<rdf:type rdf:resource = "http://www.w3.org/2002/07/owl#ObjectProperty" />
	<rdfs:label xml:lang="en">Location</rdfs:label>
	<skos:definition  xml:lang="en">Location of this power system resource.</skos:definition>
	<rdfs:domain rdf:resource="#PowerSystemResource"/>
	<rdfs:range rdf:resource="#Location"/>
	<owl:inverseOf rdf:resource="#Location.PowerSystemResources"/>
<rdf:type rdf:resource = "http://www.w3.org/2002/07/owl#FunctionalProperty"/>
</rdf:Description >
<rdf:Description rdf:about = "#Location.PositionPoints" >
	<rdf:type rdf:resource = "http://www.w3.org/2002/07/owl#ObjectProperty" />
	<rdfs:label xml:lang="en">PositionPoints</rdfs:label>
	<skos:definition  xml:lang="en">Sequence of position points describing this location, expressed in coordinate system &apos;Location.CoordinateSystem&apos;.</skos:definition>
	<rdfs:domain rdf:resource="#Location"/>
	<rdfs:range rdf:resource="#PositionPoint"/>
	<owl:inverseOf rdf:resource="#PositionPoint.Location"/>
</rdf:Description >
<rdf:Description rdf:about = "#PositionPoint.Location" >
	<rdf:type rdf:resource = "http://www.w3.org/2002/07/owl#ObjectProperty" />
	<rdfs:label xml:lang="en">Location</rdfs:label>
	<skos:definition  xml:lang="en">Location described by this position point.</skos:definition>
	<rdfs:domain rdf:resource="#PositionPoint"/>
	<rdfs:range rdf:resource="#Location"/>
	<owl:inverseOf rdf:resource="#Location.PositionPoints"/>
</rdf:Description >
<rdf:Description rdf:about="#PositionPoint">
	<rdfs:label xml:lang="en">PositionPoint</rdfs:label>
	<rdf:type rdf:resource="http://www.w3.org/2002/07/owl#Class"/>
	<skos:definition  xml:lang="en">Set of spatial coordinates that determine a point, defined in the coordinate system specified in &apos;Location.CoordinateSystem&apos;. Use a single position point instance to describe a point-oriented location. Use a sequence of position points to describe a line-oriented object (physical location of non-point oriented objects like cables or lines), or area of an object (like a substation or a geographical zone - in this case, have first and last position point with the same values).</skos:definition>
	<gl:Package>Package_GeographicalLocationProfile</gl:Package>
</rdf:Description>
<rdf:Description rdf:about="#PositionPoint.sequenceNumber">
	<rdf:type rdf:resource = "http://www.w3.org/2002/07/owl#DatatypeProperty" />
	<rdfs:label xml:lang="en">sequenceNumber</rdfs:label>
	<rdfs:domain rdf:resource="#PositionPoint"/>
	<rdfs:range rdf:resource = "http://www.w3.org/2001/XMLSchema#integer" />
	<rdf:type rdf:resource = "http://www.w3.org/2002/07/owl#FunctionalProperty" />
	<skos:definition  xml:lang="en">Zero-relative sequence number of this point within a series of points.</skos:definition>
</rdf:Description>
<rdf:Description rdf:about="#Integer">
	<rdfs:label xml:lang="en">Integer</rdfs:label>
	<rdf:type rdf:resource="http://www.w3.org/2002/07/owl#Class"/>
	<skos:definition  xml:lang="en">
An integer number. The range is unspecified and not limited.

	</skos:definition>
	<gl:isPrimitive>True</gl:isPrimitive>
	<gl:Package>Package_GeographicalLocationProfile</gl:Package>
</rdf:Description>
<rdf:Description rdf:about="#PositionPoint.xPosition">
	<rdf:type rdf:resource = "http://www.w3.org/2002/07/owl#DatatypeProperty" />
	<rdfs:label xml:lang="en">xPosition</rdfs:label>
	<rdfs:domain rdf:resource="#PositionPoint"/>
	<rdfs:range rdf:resource = "http://www.w3.org/2001/XMLSchema#string" />
	<skos:definition  xml:lang="en">X axis position.</skos:definition>
</rdf:Description>
<rdf:Description rdf:about="#PositionPoint.yPosition">
	<rdf:type rdf:resource = "http://www.w3.org/2002/07/owl#DatatypeProperty" />
	<rdfs:label xml:lang="en">yPosition</rdfs:label>
	<rdfs:domain rdf:resource="#PositionPoint"/>
	<rdfs:range rdf:resource = "http://www.w3.org/2001/XMLSchema#string" />
	<skos:definition  xml:lang="en">Y axis position.</skos:definition>
</rdf:Description>
<rdf:Description rdf:about="#PositionPoint.zPosition">
	<rdf:type rdf:resource = "http://www.w3.org/2002/07/owl#DatatypeProperty" />
	<rdfs:label xml:lang="en">zPosition</rdfs:label>
	<rdfs:domain rdf:resource="#PositionPoint"/>
	<rdfs:range rdf:resource = "http://www.w3.org/2001/XMLSchema#string" />
	<rdf:type rdf:resource = "http://www.w3.org/2002/07/owl#FunctionalProperty" />
	<skos:definition  xml:lang="en">(if applicable) Z axis position.</skos:definition>
</rdf:Description>
<rdf:Description rdf:about="#PowerSystemResource">
	<rdfs:label xml:lang="en">PowerSystemResource</rdfs:label>
	<rdf:type rdf:resource="http://www.w3.org/2002/07/owl#Class"/>
	<rdfs:subClassOf rdf:resource="#IdentifiedObject"/>
	<skos:definition  xml:lang="en">A power system resource (PSR) can be an item of equipment such as a switch, an equipment container containing many individual items of equipment such as a substation, or an organisational entity such as sub-control area. Power system resources can have measurements associated.</skos:definition>
	<gl:Package>Package_GeographicalLocationProfile</gl:Package>
	<gl:isAbstract>True</gl:isAbstract>
</rdf:Description>
<rdf:Description rdf:about="#Date">
	<rdfs:label xml:lang="en">Date</rdfs:label>
	<rdf:type rdf:resource="http://www.w3.org/2002/07/owl#Class"/>
	<skos:definition  xml:lang="en">Date as &quot;yyyy-mm-dd&quot;, which conforms with ISO 8601. UTC time zone is specified as &quot;yyyy-mm-ddZ&quot;. A local timezone relative UTC is specified as &quot;yyyy-mm-dd(+/-)hh:mm&quot;.</skos:definition>
	<gl:isPrimitive>True</gl:isPrimitive>
	<gl:Package>Package_GeographicalLocationProfile</gl:Package>
</rdf:Description>
<rdf:Description rdf:about="http://iec.ch/TC57/ns/CIM/GeographicalLocation-EU#isPrimitive">
	<rdf:type rdf:resource="http://www.w3.org/2002/07/owl#AnnotationProperty"/>
	<rdfs:label xml:lang="en">isPrimitive	</rdfs:label>
	<rdfs:comment xml:lang="en">Flag indicating whether the class is a Primitive.</rdfs:comment>
	<rdfs:domain rdf:resource="http://www.w3.org/2000/01/rdf-schema#Class" />
	<rdfs:range rdf:resource="http://www.w3.org/2001/XMLSchema#boolean" />
</rdf:Description>
<rdf:Description rdf:about="http://iec.ch/TC57/ns/CIM/GeographicalLocation-EU#isCompound">
	<rdf:type rdf:resource="http://www.w3.org/2002/07/owl#AnnotationProperty"/>
	<rdfs:label xml:lang="en">isCompound	</rdfs:label>
	<rdfs:comment xml:lang="en">Flag indicating whether the class is a Compound.</rdfs:comment>
	<rdfs:domain rdf:resource="http://www.w3.org/2000/01/rdf-schema#Class" />
	<rdfs:range rdf:resource="http://www.w3.org/2001/XMLSchema#boolean" />
</rdf:Description>
</rdf:RDF>
